<?xml version="1.0" encoding="UTF-8"?>
<rdf:RDF xmlns:rdf="http://www.w3.org/1999/02/22-rdf-syntax-ns#"
         xmlns:skos="http://www.w3.org/2004/02/skos/core#"
         xmlns:owl="http://www.w3.org/2002/07/owl#"
         xmlns:dcterms="http://purl.org/dc/terms/"
>
   <rdf:Description rdf:about="http://rdf-vocabulary.ddialliance.org/cv/TypeOfAddress/1.1.0/">
      <rdf:type rdf:resource="http://www.w3.org/2004/02/skos/core#ConceptScheme"/>
      <dcterms:isVersionOf rdf:resource="http://rdf-vocabulary.ddialliance.org/cv/TypeOfAddress/"/>
      <skos:notation xml:lang="en">TypeOfAddress</skos:notation>
      <dcterms:title xml:lang="en">Type of Address</dcterms:title>
      <dcterms:description xml:lang="en">Identifies the type of address entered as contact information for an individual or an organization.
</dcterms:description>
      <skos:prefLabel xml:lang="en">Type of Address</skos:prefLabel>
      <owl:versionInfo>1.1.0</owl:versionInfo>
      <dcterms:license rdf:resource="http://creativecommons.org/licenses/by/4.0/"/>
      <dcterms:rights>Copyright &#xa9;DDI Alliance 2020</dcterms:rights>
      <skos:hasTopConcept rdf:resource="http://rdf-vocabulary.ddialliance.org/cv/TypeOfAddress/1.1.0/c8896d7"/>
      <skos:hasTopConcept rdf:resource="http://rdf-vocabulary.ddialliance.org/cv/TypeOfAddress/1.1.0/a9a6096"/>
      <skos:hasTopConcept rdf:resource="http://rdf-vocabulary.ddialliance.org/cv/TypeOfAddress/1.1.0/6311ae1"/>
   </rdf:Description>
   <rdf:Description rdf:about="http://rdf-vocabulary.ddialliance.org/cv/TypeOfAddress/1.1.0/c8896d7">
      <rdf:type rdf:resource="http://www.w3.org/2004/02/skos/core#Concept"/>
      <skos:inScheme rdf:resource="http://rdf-vocabulary.ddialliance.org/cv/TypeOfAddress/1.1.0/"/>
      <skos:notation xml:lang="en">Mailing</skos:notation>
      <skos:prefLabel xml:lang="en">Mailing address</skos:prefLabel>
      <skos:definition xml:lang="en">Includes both &quot;street&quot;, and P.O. Box addresses used for sending and receiving physical/conventional mail through the postal system.</skos:definition>
      <skos:narrower rdf:resource="http://rdf-vocabulary.ddialliance.org/cv/TypeOfAddress/1.1.0/8ef080c"/>
      <skos:narrower rdf:resource="http://rdf-vocabulary.ddialliance.org/cv/TypeOfAddress/1.1.0/c1ddd21"/>
   </rdf:Description>
   <rdf:Description rdf:about="http://rdf-vocabulary.ddialliance.org/cv/TypeOfAddress/1.1.0/8ef080c">
      <rdf:type rdf:resource="http://www.w3.org/2004/02/skos/core#Concept"/>
      <skos:inScheme rdf:resource="http://rdf-vocabulary.ddialliance.org/cv/TypeOfAddress/1.1.0/"/>
      <skos:notation xml:lang="en">Mailing.Residential</skos:notation>
      <skos:prefLabel xml:lang="en">Mailing address: Residential</skos:prefLabel>
      <skos:definition xml:lang="en">Address for directing physical/conventional mail to a person&apos;s residence, including institutional residence.</skos:definition>
   </rdf:Description>
   <rdf:Description rdf:about="http://rdf-vocabulary.ddialliance.org/cv/TypeOfAddress/1.1.0/c1ddd21">
      <rdf:type rdf:resource="http://www.w3.org/2004/02/skos/core#Concept"/>
      <skos:inScheme rdf:resource="http://rdf-vocabulary.ddialliance.org/cv/TypeOfAddress/1.1.0/"/>
      <skos:notation xml:lang="en">Mailing.Nonresidential</skos:notation>
      <skos:prefLabel xml:lang="en">Mailing address: Nonresidential</skos:prefLabel>
      <skos:definition xml:lang="en">Address for directing physical/conventional mail to a business, organization, or other type of association.</skos:definition>
   </rdf:Description>
   <rdf:Description rdf:about="http://rdf-vocabulary.ddialliance.org/cv/TypeOfAddress/1.1.0/a9a6096">
      <rdf:type rdf:resource="http://www.w3.org/2004/02/skos/core#Concept"/>
      <skos:inScheme rdf:resource="http://rdf-vocabulary.ddialliance.org/cv/TypeOfAddress/1.1.0/"/>
      <skos:notation xml:lang="en">Visiting</skos:notation>
      <skos:prefLabel xml:lang="en">Visiting address</skos:prefLabel>
      <skos:definition xml:lang="en">Address used to identify a physical location (typically a building or a unit in a building) that may be accessed in person.</skos:definition>
      <skos:narrower rdf:resource="http://rdf-vocabulary.ddialliance.org/cv/TypeOfAddress/1.1.0/d7892ee"/>
      <skos:narrower rdf:resource="http://rdf-vocabulary.ddialliance.org/cv/TypeOfAddress/1.1.0/af04d20"/>
   </rdf:Description>
   <rdf:Description rdf:about="http://rdf-vocabulary.ddialliance.org/cv/TypeOfAddress/1.1.0/d7892ee">
      <rdf:type rdf:resource="http://www.w3.org/2004/02/skos/core#Concept"/>
      <skos:inScheme rdf:resource="http://rdf-vocabulary.ddialliance.org/cv/TypeOfAddress/1.1.0/"/>
      <skos:notation xml:lang="en">Visiting.Residential</skos:notation>
      <skos:prefLabel xml:lang="en">Visiting address: Residential</skos:prefLabel>
      <skos:definition xml:lang="en">Visiting address for a person&apos;s residence, including institutional residence.</skos:definition>
   </rdf:Description>
   <rdf:Description rdf:about="http://rdf-vocabulary.ddialliance.org/cv/TypeOfAddress/1.1.0/af04d20">
      <rdf:type rdf:resource="http://www.w3.org/2004/02/skos/core#Concept"/>
      <skos:inScheme rdf:resource="http://rdf-vocabulary.ddialliance.org/cv/TypeOfAddress/1.1.0/"/>
      <skos:notation xml:lang="en">Visiting.Nonresidential</skos:notation>
      <skos:prefLabel xml:lang="en">Visiting address: Nonresidential</skos:prefLabel>
      <skos:definition xml:lang="en">Visiting address for a business, organization, or other type of association.</skos:definition>
   </rdf:Description>
   <rdf:Description rdf:about="http://rdf-vocabulary.ddialliance.org/cv/TypeOfAddress/1.1.0/6311ae1">
      <rdf:type rdf:resource="http://www.w3.org/2004/02/skos/core#Concept"/>
      <skos:inScheme rdf:resource="http://rdf-vocabulary.ddialliance.org/cv/TypeOfAddress/1.1.0/"/>
      <skos:notation xml:lang="en">Other</skos:notation>
      <skos:prefLabel xml:lang="en">Other</skos:prefLabel>
      <skos:definition xml:lang="en">Use if type of address is known, but not found in the list.</skos:definition>
   </rdf:Description>
</rdf:RDF>
