<?xml version="1.0" encoding="UTF-8"?>
<rdf:RDF xmlns:rdf="http://www.w3.org/1999/02/22-rdf-syntax-ns#"
         xmlns:skos="http://www.w3.org/2004/02/skos/core#"
         xmlns:owl="http://www.w3.org/2002/07/owl#"
         xmlns:dcterms="http://purl.org/dc/terms/"
>
   <rdf:Description rdf:about="http://rdf-vocabulary.ddialliance.org/cv/AnalysisUnit/1.0/">
      <rdf:type rdf:resource="http://www.w3.org/2004/02/skos/core#ConceptScheme"/>
      <dcterms:isVersionOf rdf:resource="http://rdf-vocabulary.ddialliance.org/cv/AnalysisUnit/"/>
      <skos:notation xml:lang="en">AnalysisUnit</skos:notation>
      <dcterms:title xml:lang="en">Analysis Unit</dcterms:title>
      <dcterms:description xml:lang="en">Describes the entity being analyzed in the study or in the variable.</dcterms:description>
      <skos:prefLabel xml:lang="en">Analysis Unit</skos:prefLabel>
      <dcterms:title xml:lang="da">Analysenhed</dcterms:title>
      <dcterms:description xml:lang="da">Beskriver den enhed som analyseres i studiet eller i variablen.</dcterms:description>
      <skos:prefLabel xml:lang="da">Analysenhed</skos:prefLabel>
      <dcterms:title xml:lang="de">Analyseeinheit</dcterms:title>
      <dcterms:description xml:lang="de">Beschreibt die Entit&#xe4;t, die in der Studie oder in der Variable analysiert wird.</dcterms:description>
      <skos:prefLabel xml:lang="de">Analyseeinheit</skos:prefLabel>
      <dcterms:title xml:lang="fi">Havainto/aineistoyksikk&#xf6;tyyppi</dcterms:title>
      <dcterms:description xml:lang="fi">Yksikk&#xf6;, jonka edustajana vastataan/esiinnyt&#xe4;&#xe4;n ja/tai jota havainnoidaan.</dcterms:description>
      <skos:prefLabel xml:lang="fi">Havainto/aineistoyksikk&#xf6;tyyppi</skos:prefLabel>
      <dcterms:title xml:lang="no">Analyseenhet</dcterms:title>
      <dcterms:description xml:lang="no">Beskrivelse av enhet som blir analysert i studien eller i variablene.</dcterms:description>
      <skos:prefLabel xml:lang="no">Analyseenhet</skos:prefLabel>
      <dcterms:title xml:lang="sv">Analysenhet</dcterms:title>
      <dcterms:description xml:lang="sv">Beskriver den enhet som analyseras i studien eller i variabeln.</dcterms:description>
      <skos:prefLabel xml:lang="sv">Analysenhet</skos:prefLabel>
      <owl:versionInfo>1.0.0</owl:versionInfo>
      <dcterms:license rdf:resource="http://creativecommons.org/licenses/by/4.0/"/>
      <dcterms:rights>Copyright &#xa9;DDI Alliance 2020</dcterms:rights>
      <skos:hasTopConcept rdf:resource="http://rdf-vocabulary.ddialliance.org/cv/AnalysisUnit/1.0/2dd4472"/>
      <skos:hasTopConcept rdf:resource="http://rdf-vocabulary.ddialliance.org/cv/AnalysisUnit/1.0/d6b2587"/>
      <skos:hasTopConcept rdf:resource="http://rdf-vocabulary.ddialliance.org/cv/AnalysisUnit/1.0/cefc4f7"/>
      <skos:hasTopConcept rdf:resource="http://rdf-vocabulary.ddialliance.org/cv/AnalysisUnit/1.0/ea4be67"/>
      <skos:hasTopConcept rdf:resource="http://rdf-vocabulary.ddialliance.org/cv/AnalysisUnit/1.0/4358d21"/>
      <skos:hasTopConcept rdf:resource="http://rdf-vocabulary.ddialliance.org/cv/AnalysisUnit/1.0/44604e9"/>
      <skos:hasTopConcept rdf:resource="http://rdf-vocabulary.ddialliance.org/cv/AnalysisUnit/1.0/435eb71"/>
      <skos:hasTopConcept rdf:resource="http://rdf-vocabulary.ddialliance.org/cv/AnalysisUnit/1.0/8b62b80"/>
      <skos:hasTopConcept rdf:resource="http://rdf-vocabulary.ddialliance.org/cv/AnalysisUnit/1.0/89b8575"/>
      <skos:hasTopConcept rdf:resource="http://rdf-vocabulary.ddialliance.org/cv/AnalysisUnit/1.0/0393713"/>
      <skos:hasTopConcept rdf:resource="http://rdf-vocabulary.ddialliance.org/cv/AnalysisUnit/1.0/4970317"/>
      <skos:hasTopConcept rdf:resource="http://rdf-vocabulary.ddialliance.org/cv/AnalysisUnit/1.0/6311ae1"/>
   </rdf:Description>
   <rdf:Description rdf:about="http://rdf-vocabulary.ddialliance.org/cv/AnalysisUnit/1.0/2dd4472">
      <rdf:type rdf:resource="http://www.w3.org/2004/02/skos/core#Concept"/>
      <skos:inScheme rdf:resource="http://rdf-vocabulary.ddialliance.org/cv/AnalysisUnit/1.0/"/>
      <skos:notation xml:lang="en">Individual</skos:notation>
      <skos:prefLabel xml:lang="en">Individual</skos:prefLabel>
      <skos:definition xml:lang="en">Any individual person, irrespective of demographic characteristics, professional, social or legal status, or affiliation.</skos:definition>
      <skos:prefLabel xml:lang="da">Individ</skos:prefLabel>
      <skos:definition xml:lang="da">Enhver individuel person, uafh&#xe6;ngig af demografiske karakteristik, erhvervs-, social- eller juridisk status eller tilh&#xf8;rsforhold.</skos:definition>
      <skos:prefLabel xml:lang="de">Individuum</skos:prefLabel>
      <skos:definition xml:lang="de">Jede einzelne Person, unabh&#xe4;ngig von demographischen Merkmalen, dem Beruf, dem sozialen Status, Rechtsstatus oder sozialer Status, Zugeh&#xf6;rigkeit.</skos:definition>
      <skos:prefLabel xml:lang="fi">Henkil&#xf6;</skos:prefLabel>
      <skos:definition xml:lang="fi">Tutkimuksen tarkastelukohteena ovat yksitt&#xe4;iset henkil&#xf6;t.</skos:definition>
      <skos:prefLabel xml:lang="no">Individ</skos:prefLabel>
      <skos:definition xml:lang="no">En individuell person, uavhengig av demografiske kjennetegn, yrkesmessig, sosial eller juridisk status, eller tilh&#xf8;righet.</skos:definition>
      <skos:prefLabel xml:lang="sv">Individ</skos:prefLabel>
      <skos:definition xml:lang="sv">En enskild person, oavsett dennas demografiska s&#xe4;rdrag, yrkesm&#xe4;ssiga, sociala eller juridiska status, eller tillh&#xf6;righet.</skos:definition>
   </rdf:Description>
   <rdf:Description rdf:about="http://rdf-vocabulary.ddialliance.org/cv/AnalysisUnit/1.0/d6b2587">
      <rdf:type rdf:resource="http://www.w3.org/2004/02/skos/core#Concept"/>
      <skos:inScheme rdf:resource="http://rdf-vocabulary.ddialliance.org/cv/AnalysisUnit/1.0/"/>
      <skos:notation xml:lang="en">Organization</skos:notation>
      <skos:prefLabel xml:lang="en">Organization</skos:prefLabel>
      <skos:definition xml:lang="en">Any kind of formal administrative and functional structure - includes associations, institutions, agencies, businesses, political parties, schools, etc.</skos:definition>
      <skos:prefLabel xml:lang="da">Organisation</skos:prefLabel>
      <skos:definition xml:lang="da">Enhver form for formel administrativ eller funktionel struktur. Omfatter foreninger, institutioner, agenturer, virksomheder, politiske partier, skoler mm.</skos:definition>
      <skos:prefLabel xml:lang="de">Organisation</skos:prefLabel>
      <skos:definition xml:lang="de">Jede Art von formaler Verwaltungsstruktur und funktionaler Struktur - schlie&#xdf;t Verb&#xe4;nde, Institutionen, Agenturen, Unternehmen, politische Parteien, Schulen usw. ein.</skos:definition>
      <skos:prefLabel xml:lang="fi">Organisaatio</skos:prefLabel>
      <skos:definition xml:lang="fi">Mik&#xe4; tahansa hallinnollinen tai toiminnallinen struktuuri, esimerkiksi koulu, yhdistys, j&#xe4;rjest&#xf6;, instituutio, toimisto, yritys, poliittinen puolue, jne. Kysymykset kohdistuvat itse organisaatioon ja vastaaja esiintyy p&#xe4;&#xe4;asiassa organisaation, ei itsens&#xe4; edustajana. Esimerkiksi miten korkeakoulut toteuttivat tutkinnonuudistuksen tai miten yritykset ottavat ymp&#xe4;rist&#xf6;seikat huomioon toiminnassaan.</skos:definition>
      <skos:prefLabel xml:lang="no">Organisasjon</skos:prefLabel>
      <skos:definition xml:lang="no">Former for formelle administrative og funksjonelle strukturerer - inkluderer foreninger, institusjoner, foretak, bedrifter, politiske partier, skoler etc.</skos:definition>
      <skos:prefLabel xml:lang="sv">Organisation</skos:prefLabel>
      <skos:definition xml:lang="sv">N&#xe5;gon typ av formell administrativ och funktionell struktur. Inkluderar f&#xf6;reningar, institutioner, f&#xf6;retag, myndigheter, politiska partier, skolor, m.m.</skos:definition>
   </rdf:Description>
   <rdf:Description rdf:about="http://rdf-vocabulary.ddialliance.org/cv/AnalysisUnit/1.0/cefc4f7">
      <rdf:type rdf:resource="http://www.w3.org/2004/02/skos/core#Concept"/>
      <skos:inScheme rdf:resource="http://rdf-vocabulary.ddialliance.org/cv/AnalysisUnit/1.0/"/>
      <skos:notation xml:lang="en">Family</skos:notation>
      <skos:prefLabel xml:lang="en">Family</skos:prefLabel>
      <skos:definition xml:lang="en">Two or more people related by blood, marriage (including step-relations), adoption or fostering and who may or may not live together (National Community Services Data Dictionary, Vers 3, AIHW, 2004). For example, used when researching the extent to which people provide support and assistance for their relatives.</skos:definition>
      <skos:prefLabel xml:lang="da">Familie</skos:prefLabel>
      <skos:definition xml:lang="da">To eller flere mennesker, der er&#xa0;besl&#xe6;gtede ved blod, &#xe6;gteskab (inklusiv stedfamilie), adoption eller pleje (plejefor&#xe6;ldre og plejeb&#xf8;rn mm.), der enten bor sammen eller ikke bor sammen. Anvendes fx til unders&#xf8;gelser af i hvor h&#xf8;j grad mennesker st&#xf8;tter og hj&#xe6;lper sl&#xe6;gtninge.</skos:definition>
      <skos:prefLabel xml:lang="de">Familie</skos:prefLabel>
      <skos:definition xml:lang="de">Zwei oder mehr Menschen, die miteinander blutsverwandt sind, oder durch Heirat (einschlie&#xdf;lich der Verwandschaft des Ehepartners), Adoption oder Pflege (Pflegeeltern, Pflegekinder etc.) anverwandt sind - unabh&#xe4;ngig davon, ob sie zusammenleben oder nicht. Wird zum Beispiel genutzt bei der Erforschung des Ausma&#xdf;es, in dem die Menschen ihre Verwandten unterst&#xfc;tzen.</skos:definition>
      <skos:prefLabel xml:lang="fi">Perhe</skos:prefLabel>
      <skos:definition xml:lang="fi">Kaksi tai useampi henkil&#xf6;, jotka liittyv&#xe4;t toisiinsa sukulaisuuden, avo- tai avioliiton (laskien mukaan esim. sisar- ja velipuolet), rekister&#xf6;idyn parisuhteen, adoption tai sijaisvanhemmuuden kautta, riippumatta siit&#xe4;, asuvatko he yhdess&#xe4; vai eiv&#xe4;t. Esimerkiksi tutkittaessa perheenj&#xe4;senten v&#xe4;lisi&#xe4; kontakteja ja auttamistapoja.</skos:definition>
      <skos:prefLabel xml:lang="no">Familie</skos:prefLabel>
      <skos:definition xml:lang="no">To eller flere personer som er i slekt gjennom blodsb&#xe5;nd, ekteskap (inkludert ste-relasjoner), adopsjon eller fosterfamilie, som bor eller ikke bor sammen. Brukes for eksempel n&#xe5;r man forsker p&#xe5; i hvilken grad folk bist&#xe5;r med st&#xf8;tte og hjelp til slektninger.</skos:definition>
      <skos:prefLabel xml:lang="sv">Familj</skos:prefLabel>
      <skos:definition xml:lang="sv">Tv&#xe5; eller fler personer som &#xe4;r sl&#xe4;kt genom blodsband, &#xe4;ktenskap (inklusive styvsyskon, -f&#xf6;r&#xe4;ldrar, -barn m.m.), adoption eller fosterfamiljeskap, men som inte n&#xf6;dv&#xe4;ndigtvis bor tillsammans (National Community Services Data Dictionary, Vers 3, AIHW, 2004). Anv&#xe4;nds t.ex. vid forskning om i vilken omfattning m&#xe4;nniskor erbjuder hj&#xe4;lp och st&#xf6;d f&#xf6;r sina sl&#xe4;ktingar.</skos:definition>
      <skos:narrower rdf:resource="http://rdf-vocabulary.ddialliance.org/cv/AnalysisUnit/1.0/4a75b73"/>
   </rdf:Description>
   <rdf:Description rdf:about="http://rdf-vocabulary.ddialliance.org/cv/AnalysisUnit/1.0/4a75b73">
      <rdf:type rdf:resource="http://www.w3.org/2004/02/skos/core#Concept"/>
      <skos:inScheme rdf:resource="http://rdf-vocabulary.ddialliance.org/cv/AnalysisUnit/1.0/"/>
      <skos:notation xml:lang="en">Family.HouseholdFamily</skos:notation>
      <skos:prefLabel xml:lang="en">Family: Household family</skos:prefLabel>
      <skos:definition xml:lang="en">A more specific term, refers only to related people who live in the same household at a point in time. If not known whether the analysis unit is &apos;Family&apos; or &apos;Household family&apos;, use &apos;Family&apos;.</skos:definition>
      <skos:prefLabel xml:lang="da">Familie: Husstands familie</skos:prefLabel>
      <skos:definition xml:lang="da">Et mere specifkt begreb, der refererer til mennesker, der er besl&#xe6;gtede og bor i samme husstand p&#xe5; et givent tidspunkt. Hvis det er usikkert, hvorvidt&#xa0;analyseenheden er &apos;Familie&apos; eller &apos;Familie: Hustandsfamilie&apos; brug da &apos;Familie&apos;.</skos:definition>
      <skos:prefLabel xml:lang="de">Familie: Familienhaushalt</skos:prefLabel>
      <skos:definition xml:lang="de">Ein spezifischerer Begriff, bezieht sich nur auf verwandte Personen, die zu einem bestimmten Zeitpunkt im selben Haushalt leben. Wenn nicht bekannt ist, ob die Analyseeinheit &apos;Familie&apos; oder &apos;Haushalt Familie&apos; ist, verwenden Sie &apos;Familie&apos;.</skos:definition>
      <skos:prefLabel xml:lang="fi">Perhe: perhekotitalous</skos:prefLabel>
      <skos:definition xml:lang="fi">Spesifimpi termi, joka viittaa vain tietyll&#xe4; hetkell&#xe4; samassa kotitaloudessa asuviin perheenj&#xe4;seniin. Jos ei tiedossa, onko kyseess&#xe4; &apos;Perhe&apos; vai &apos;Perhekotitalous&apos;, k&#xe4;yt&#xe4; &apos;Perhe&apos;.</skos:definition>
      <skos:prefLabel xml:lang="no">Familie: familiehusholdning</skos:prefLabel>
      <skos:definition xml:lang="no">Et mer spesifikt begrep som kun referer til personer som bor i samme husholdning p&#xe5; et gitt tidspunkt. Om det ikke er kjent om analyseenheten er &apos;Familie&apos; eller &apos;Familiehusholdning&apos; skal begrepet &apos;Familie&apos; benyttes.</skos:definition>
      <skos:prefLabel xml:lang="sv">Familj: Familjehush&#xe5;ll</skos:prefLabel>
      <skos:definition xml:lang="sv">En mer specifik term &#xe4;n &apos;Familj&apos;. Betecknar endast m&#xe4;nniskor som bor tillsammans i samma hush&#xe5;ll vid en given tidpunkt. Om det inte &#xe4;r k&#xe4;nt huruvida analysenheten &#xe4;r &apos;Familj&apos; eller &apos;Familjehush&#xe5;ll&apos; ska &apos;Familj&apos; anv&#xe4;ndas.</skos:definition>
   </rdf:Description>
   <rdf:Description rdf:about="http://rdf-vocabulary.ddialliance.org/cv/AnalysisUnit/1.0/ea4be67">
      <rdf:type rdf:resource="http://www.w3.org/2004/02/skos/core#Concept"/>
      <skos:inScheme rdf:resource="http://rdf-vocabulary.ddialliance.org/cv/AnalysisUnit/1.0/"/>
      <skos:notation xml:lang="en">Household</skos:notation>
      <skos:prefLabel xml:lang="en">Household</skos:prefLabel>
      <skos:definition xml:lang="en">A person or a group of persons who share the same dwelling unit and common living arrangements. These common living arrangements may include pooling some, or all, of their income and wealth, and consuming certain types of goods and services collectively, mainly housing and food (Eurostat).</skos:definition>
      <skos:prefLabel xml:lang="da">Husstand</skos:prefLabel>
      <skos:definition xml:lang="da">En person eller gruppe af personer der deler den samme bop&#xe6;l og deler almindelig livsindretning. Disse former for livsindretning kan omfatte deling eller delvis deling af indkomst og finanser og forbrug af nogle typer af varer og service ydelser kollektivt, prim&#xe6;rt mad og bop&#xe6;l.</skos:definition>
      <skos:prefLabel xml:lang="de">Haushalt</skos:prefLabel>
      <skos:definition xml:lang="de">Eine Person oder eine Gruppe von Personen, die die gleiche Wohneinheit und gemeinsame Wohnverh&#xe4;ltnisse teilen. Diese gemeinsamen Wohnverh&#xe4;ltnisse k&#xf6;nnen das Zusammenbringen einiger oder aller ihrer Einkommen und ihres Verm&#xf6;gens beinhalten und bestimmte Arten von Waren und Dienstleistungen zusammenf&#xfc;hren, vor allem Wohnraum und Lebensmittel.</skos:definition>
      <skos:prefLabel xml:lang="fi">Kotitalous</skos:prefLabel>
      <skos:definition xml:lang="fi">Henkil&#xf6;t, jotka asuvat yhdess&#xe4; ja joilla on kokonaan tai osittain yhteinen ruokatalous tai jotka muuten k&#xe4;ytt&#xe4;v&#xe4;t tulojaan yhdess&#xe4;.</skos:definition>
      <skos:prefLabel xml:lang="no">Husholdning</skos:prefLabel>
      <skos:definition xml:lang="no">En person eller en gruppe av personer som har samme boligenhet og leveforhold. Disse felles leveforholdene kan inkludere at deler av, eller alt av inntekt og eiendom er felles, og at visse type varer og tjenester konsumeres i fellesskap, hovedsakelig bosted og mat (Eurostat).</skos:definition>
      <skos:prefLabel xml:lang="sv">Hush&#xe5;ll</skos:prefLabel>
      <skos:definition xml:lang="sv">En person eller grupp som har gemensam bostadsenhet och levnadsf&#xf6;rh&#xe5;llanden. Dessa delade levnadsf&#xf6;rh&#xe5;llanden kan inkludera att viss eller all inkomst och egendom &#xe4;r gemensam, och att vissa sorters varor och tj&#xe4;nster konsumeras gemensamt, f&#xf6;retr&#xe4;delsevis bostad och mat (Eurostat).</skos:definition>
   </rdf:Description>
   <rdf:Description rdf:about="http://rdf-vocabulary.ddialliance.org/cv/AnalysisUnit/1.0/4358d21">
      <rdf:type rdf:resource="http://www.w3.org/2004/02/skos/core#Concept"/>
      <skos:inScheme rdf:resource="http://rdf-vocabulary.ddialliance.org/cv/AnalysisUnit/1.0/"/>
      <skos:notation xml:lang="en">HousingUnit</skos:notation>
      <skos:prefLabel xml:lang="en">Housing Unit</skos:prefLabel>
      <skos:definition xml:lang="en">U.S. Census: A housing unit is a house, an apartment, a mobile home, a group of rooms, or a single room that is occupied (or if vacant, is intended for occupancy) as separate living quarters. Separate living quarters are those in which the occupants live and eat separately from any other persons in the building and which have direct access from the outside of the building or through a common hall.</skos:definition>
      <skos:prefLabel xml:lang="da">Boligenhed</skos:prefLabel>
      <skos:definition xml:lang="da">En boligenhed er en lejlighed, beboelsesvogne, en gruppe af v&#xe6;relser eller et enkelt v&#xe6;relse der er beboet (eller ikke beboet, men tilt&#xe6;nkt beboelse) som en separat bolig. Separate boliger er boliger, hvor beboerne lever og spiser hver for sig, men har adgang til omr&#xe5;det uden for bygningen gennem en f&#xe6;lles indgang.</skos:definition>
      <skos:prefLabel xml:lang="de">Wohneinheit</skos:prefLabel>
      <skos:definition xml:lang="de">Eine Wohneinheit ist ein Haus, eine Wohnung, ein Wohnmobil, eine Gruppe von R&#xe4;umen oder ein Einzelzimmer, sie wird bewohnt (oder wenn sie leer ist, aber f&#xfc;r das Wohnen bestimmt ist) als eine geschlossene Wohneinheit.Geschlossene Wohneinheiten sind diejenigen, in denen die Bewohner getrennt von allen anderen Personen im Geb&#xe4;ude leben und essen und die einen direkten Zugang vonau&#xdf;endes Geb&#xe4;udes oder durch einen gemeinsamen Flur haben.</skos:definition>
      <skos:prefLabel xml:lang="fi">Asuntokunta</skos:prefLabel>
      <skos:definition xml:lang="fi">Henkil&#xf6; tai henkil&#xf6;t, joilla on oma ruokatalous ja asuintilat. Asuintila voi olla talo, huoneisto, asuntovaunu, tietyt huoneet asunnosta.jne. Asuintiloihin on erillinen p&#xe4;&#xe4;sy joko suoraan ulkoa tai yhteisen aulan kautta. 
Lis&#xe4;ohje kansainv&#xe4;liseen m&#xe4;&#xe4;ritelm&#xe4;&#xe4;n: Esimerkiksi soluasunnoissa asuvilla opiskelijoilla voi olla kullakin oma ruokakunta. Termi k&#xe4;yt&#xf6;ss&#xe4; varsinkin Yhdysvalloissa.</skos:definition>
      <skos:prefLabel xml:lang="no">Bruksenhet</skos:prefLabel>
      <skos:definition xml:lang="no">En bruksenhet er et hus, en leilighet, et mobilt hjem (campingvogn), eller ett eller flere rom som er bebodd (eventuelt ledig, men som er ment &#xe5; v&#xe6;re bebodd), som adskilte enheter. Med adskilt menes det at personer bor og spiser uavhengig av andre personer i samme bruksenhet, og som har direkte tilgang til enheten utenfra, eller gjennom en felles inngang.</skos:definition>
      <skos:prefLabel xml:lang="sv">Bostadsenhet</skos:prefLabel>
      <skos:definition xml:lang="sv">En bostadsenhet &#xe4;r ett hus, en l&#xe4;genhet, en husvagn, eller ett eller flera rum som bebos (eller, om den &#xe4;r tom, &#xe4;r avsett att bebos) som avskild inkvartering. Med avskild inkvartering menas att de som &#xe4;r inkvarterade d&#xe4;r bor och &#xe4;ter avskiljt fr&#xe5;n andra personer i byggnaden och kan komma in direkt utifr&#xe5;n eller via en gemensam entr&#xe9; (U.S. Census).</skos:definition>
   </rdf:Description>
   <rdf:Description rdf:about="http://rdf-vocabulary.ddialliance.org/cv/AnalysisUnit/1.0/44604e9">
      <rdf:type rdf:resource="http://www.w3.org/2004/02/skos/core#Concept"/>
      <skos:inScheme rdf:resource="http://rdf-vocabulary.ddialliance.org/cv/AnalysisUnit/1.0/"/>
      <skos:notation xml:lang="en">EventOrProcess</skos:notation>
      <skos:prefLabel xml:lang="en">Event/Process</skos:prefLabel>
      <skos:definition xml:lang="en">Any type of incident, occurrence, or activity. Events are usually one-time, individual occurrences, with a limited, or short duration. Examples: criminal offenses, riots, meetings, elections, sports competitions, terrorist attacks, natural disasters like floods, etc. Processes typically take place over time, and may include multiple &apos;events&apos; or gradual changes that ultimately lead, or are projected to lead, to a particular result. Examples: court trials, criminal investigations, political campaigns, medical treatments, education, athletes&apos; training, etc.</skos:definition>
      <skos:prefLabel xml:lang="da">Event/Proces</skos:prefLabel>
      <skos:definition xml:lang="da">Enhver form for h&#xe6;ndelse, begivenhed eller aktivitet. Episoderne sker normalt kun &#xe9;n gang med en begr&#xe6;nset eller kort varighed. For eksempel kriminelle handlinger, opr&#xf8;r, m&#xf8;der, valg, sportsbegivenheder, terrorangreb, naturkatastrofer s&#xe5;som oversv&#xf8;mmelser mm. Disse processer sker typisk over tid og kan omfatte flere h&#xe6;ndelser eller gradvise &#xe6;ndringer, der i sidste ende og/eller muligvis leder til et bestemt resultat. Fx retssager, efterforskning af kriminelle handlinger, politiske kampagner, medicinsk behandling, uddannelse, en atlets tr&#xe6;ning mm.</skos:definition>
      <skos:prefLabel xml:lang="de">Ereignis/ Prozess</skos:prefLabel>
      <skos:definition xml:lang="de">Jede Art von Ereignis, Vorfall oder Aktivit&#xe4;t. Ereignisse sind in der Regel einmalige, einzelne Vorkommnisse, mit einer begrenzten oder kurzen Dauer. Beispiele sind: Straftaten, Tumulte, Treffen, Wahlen, Sportwettk&#xe4;mpfe, Terroranschl&#xe4;ge, Naturkatastrophen wie &#xdc;berschwemmungen usw. Prozesse finden typischerweise im Verlauf der Zeit statt und k&#xf6;nnen mehrere &apos;Ereignisse&apos; oder allm&#xe4;hliche Ver&#xe4;nderungen beinhalten, die letztendlich oder voraussichtlich zu einem bestimmten Ergebnis f&#xfc;hren. Beispiele: Gerichtsverfahren, strafrechtliche Ermittlungen, politische Kampagnen, medizinische Behandlungen, Bildung, Athletenausbildung usw.</skos:definition>
      <skos:prefLabel xml:lang="fi">Tapahtuma/prosessi/toiminta</skos:prefLabel>
      <skos:definition xml:lang="fi">Tapahtuma, tapahtumasarja, toiminta tai prosessi. Voivat olla lyhytaikaisia ja kertaluonteisia tai pidempikestoisia, usein muutoksiin johtavia. Esimerkiksi yksitt&#xe4;iset rikokset, s&#xe4;&#xe4;ilmi&#xf6;t, oikeusjutut, kuntoutushoidot. Havaintoyksikk&#xf6;n&#xe4; silloin, kun kysymyksiss&#xe4; keskityt&#xe4;&#xe4;n kyseisen tapahtuman/prosessin selvitt&#xe4;miseen, ei henkil&#xf6;ihin sin&#xe4;ns&#xe4;. Esimerkiksi ty&#xf6;ehtosopimusneuvotteluj&#xe4;rjestelm&#xe4;n vaikutus sukupuolten palkkaeroihin tai avoterapian vaikutus mielenterveyspotilaisiin.</skos:definition>
      <skos:prefLabel xml:lang="no">Hendelse/prosess</skos:prefLabel>
      <skos:definition xml:lang="no">Typer av hendelse, begivenhet eller aktivitet. Hendelser er som oftest enkeltst&#xe5;ende med begrenset eller kort varighet. For eksempel: kriminell handling, oppt&#xf8;yer, m&#xf8;ter, valg, idrettsbegivenheter, terroraksjoner, naturkatastrofer osv. Prosesser finner som regel sted over tid, og kan inkludere flere &apos;hendelser&apos; eller gradvise endringer som etterhvert f&#xf8;rer til, eller er ansl&#xe5;tt &#xe5; f&#xf8;re til, et bestemt resultat. For eksempel: rettsaker, kriminaletterforskning, politiske kampanjer, medisinsk behandling, utdanning, idrettsut&#xf8;veres treninger etc.</skos:definition>
      <skos:prefLabel xml:lang="sv">H&#xe4;ndelse/process</skos:prefLabel>
      <skos:definition xml:lang="sv">N&#xe5;gon typ av f&#xf6;reteelse, tilldragelse eller aktivitet. H&#xe4;ndelser &#xe4;r vanligtvis enstaka f&#xf6;reteelser med begr&#xe4;nsad eller kort varaktighet. Exempel: brott, upplopp, m&#xf6;ten, val, idrottst&#xe4;vlingar, terroristangrepp, naturkatastrofer som &#xf6;versv&#xe4;mningar o.dyl. Processer utspelar sig vanligtvis &#xf6;ver tid och kan omfatta flera &apos;h&#xe4;ndelser&apos; eller gradvisa f&#xf6;r&#xe4;ndringar som slutligen resulterar i, eller kan t&#xe4;nkas resultera i, en visst utg&#xe5;ng. Exempel: r&#xe4;tteg&#xe5;ngar, brottsutredningar, politiska kampanjer, medicinska behandlingar, utbildning, en idrottsut&#xf6;vares tr&#xe4;ning, m.m.</skos:definition>
   </rdf:Description>
   <rdf:Description rdf:about="http://rdf-vocabulary.ddialliance.org/cv/AnalysisUnit/1.0/435eb71">
      <rdf:type rdf:resource="http://www.w3.org/2004/02/skos/core#Concept"/>
      <skos:inScheme rdf:resource="http://rdf-vocabulary.ddialliance.org/cv/AnalysisUnit/1.0/"/>
      <skos:notation xml:lang="en">GeographicUnit</skos:notation>
      <skos:prefLabel xml:lang="en">Geographic Unit</skos:prefLabel>
      <skos:definition xml:lang="en">Any entity that can be spatially defined as a geographic area, with either natural (physical) or administrative boundaries.</skos:definition>
      <skos:prefLabel xml:lang="da">Geografisk enhed</skos:prefLabel>
      <skos:definition xml:lang="da">Enhver enhed der rummeligt kan defineres som et geografisk omr&#xe5;de med enten naturlige (fysiske) eller administrative gr&#xe6;nser.</skos:definition>
      <skos:prefLabel xml:lang="de">Geographische Einheit</skos:prefLabel>
      <skos:definition xml:lang="de">Jede Einheit, die r&#xe4;umlich als geographisches Gebiet definiert werden kann, mit einer entweder nat&#xfc;rlichen (physischen) oder administrativen Grenze.</skos:definition>
      <skos:prefLabel xml:lang="fi">Maantieteellinen alue</skos:prefLabel>
      <skos:definition xml:lang="fi">Mik&#xe4; tahansa maantieteellisesti m&#xe4;&#xe4;ritelt&#xe4;viss&#xe4; oleva alue. Lis&#xe4;ohje kansainv&#xe4;liseen m&#xe4;&#xe4;ritelm&#xe4;&#xe4;n: Tyypillisesti kunta tai valtio. Esimerkiksi tutkimukset, joissa kuntien edustajilta kysyt&#xe4;&#xe4;n kunnan palvelutuotannosta. Huom! Mik&#xe4;li kysyt&#xe4;&#xe4;n asukkaiden mielipiteit&#xe4; kunnan palveluista, havaintoyksikk&#xf6;kategoria on yleens&#xe4; Henkil&#xf6; tai kategoriana k&#xe4;ytet&#xe4;&#xe4;n molempia.</skos:definition>
      <skos:prefLabel xml:lang="no">Geografisk enhet</skos:prefLabel>
      <skos:definition xml:lang="no">Enhet som kan bli defineres romlig som et geografisk omr&#xe5;de, med enten naturlige (fysiske) eller administrative grenser.</skos:definition>
      <skos:prefLabel xml:lang="sv">Geografisk enhet</skos:prefLabel>
      <skos:definition xml:lang="sv">En enhet som kan definieras spatiellt som ett geografiskt omr&#xe5;de med antingen naturliga (fysiska) eller administrativa gr&#xe4;nser.</skos:definition>
   </rdf:Description>
   <rdf:Description rdf:about="http://rdf-vocabulary.ddialliance.org/cv/AnalysisUnit/1.0/8b62b80">
      <rdf:type rdf:resource="http://www.w3.org/2004/02/skos/core#Concept"/>
      <skos:inScheme rdf:resource="http://rdf-vocabulary.ddialliance.org/cv/AnalysisUnit/1.0/"/>
      <skos:notation xml:lang="en">TimeUnit</skos:notation>
      <skos:prefLabel xml:lang="en">Time Unit</skos:prefLabel>
      <skos:definition xml:lang="en">Any period of time: year, week, month, day, or bimonthly or quarterly periods, etc.</skos:definition>
      <skos:prefLabel xml:lang="da">Tidsenhed</skos:prefLabel>
      <skos:definition xml:lang="da">Enhver periode af tid: &#xc5;r, uge, m&#xe5;ned, dag, hver anden m&#xe5;ned, kvartaler mm.</skos:definition>
      <skos:prefLabel xml:lang="de">Zeiteinheit</skos:prefLabel>
      <skos:definition xml:lang="de">Jegliche Art von Zeitspanne: Jahr, Woche, Monat, Tag oder zweimonatliche oder viertelj&#xe4;hrliche Zeitspannen,etc.</skos:definition>
      <skos:prefLabel xml:lang="fi">Aikajakso</skos:prefLabel>
      <skos:definition xml:lang="fi">Mink&#xe4; mittainen aikajakso tahansa: sekunti, tunti, vuorokausi, viikko, kuukausi, vuosi yms.</skos:definition>
      <skos:prefLabel xml:lang="no">Tidsenhet</skos:prefLabel>
      <skos:definition xml:lang="no">Tidsperiode: &#xe5;r, uke, m&#xe5;ned, dag, annenhver m&#xe5;ned eller kvartal etc.</skos:definition>
      <skos:prefLabel xml:lang="sv">Tidsenhet</skos:prefLabel>
      <skos:definition xml:lang="sv">En tidsperiod: &#xe5;r, m&#xe5;nad, vecka, dag, kvartal, tv&#xe5;m&#xe5;naders period, e.dyl.</skos:definition>
   </rdf:Description>
   <rdf:Description rdf:about="http://rdf-vocabulary.ddialliance.org/cv/AnalysisUnit/1.0/89b8575">
      <rdf:type rdf:resource="http://www.w3.org/2004/02/skos/core#Concept"/>
      <skos:inScheme rdf:resource="http://rdf-vocabulary.ddialliance.org/cv/AnalysisUnit/1.0/"/>
      <skos:notation xml:lang="en">TextUnit</skos:notation>
      <skos:prefLabel xml:lang="en">Text Unit</skos:prefLabel>
      <skos:definition xml:lang="en">Books, articles, any written piece/entity.</skos:definition>
      <skos:prefLabel xml:lang="da">Tekstenhed</skos:prefLabel>
      <skos:definition xml:lang="da">B&#xf8;ger, artikler eller anden skreven tekst.</skos:definition>
      <skos:prefLabel xml:lang="de">Texteinheit</skos:prefLabel>
      <skos:definition xml:lang="de">B&#xfc;cher, Artikel, jegliche schriftliche St&#xfc;cke.</skos:definition>
      <skos:prefLabel xml:lang="fi">Teksti</skos:prefLabel>
      <skos:definition xml:lang="fi">Kirja, artikkeli tai mik&#xe4; tahansa muu tekstiyksikk&#xf6;. Lis&#xe4;ohje kansainv&#xe4;liseen m&#xe4;&#xe4;ritelm&#xe4;&#xe4;n: Esimerkiksi sanomalehtiartikkelit autismista tai kirjoituskilpailuissa ker&#xe4;tyt el&#xe4;m&#xe4;nkerrat.</skos:definition>
      <skos:prefLabel xml:lang="no">Tekstenhet</skos:prefLabel>
      <skos:definition xml:lang="no">B&#xf8;ker, artikler, eller annen skreven tekst.</skos:definition>
      <skos:prefLabel xml:lang="sv">Textenhet</skos:prefLabel>
      <skos:definition xml:lang="sv">B&#xf6;cker, artiklar, eller annan skriven text.</skos:definition>
   </rdf:Description>
   <rdf:Description rdf:about="http://rdf-vocabulary.ddialliance.org/cv/AnalysisUnit/1.0/0393713">
      <rdf:type rdf:resource="http://www.w3.org/2004/02/skos/core#Concept"/>
      <skos:inScheme rdf:resource="http://rdf-vocabulary.ddialliance.org/cv/AnalysisUnit/1.0/"/>
      <skos:notation xml:lang="en">Group</skos:notation>
      <skos:prefLabel xml:lang="en">Group</skos:prefLabel>
      <skos:definition xml:lang="en">Two or more individuals assembled together or having some unifying relationship.</skos:definition>
      <skos:prefLabel xml:lang="da">Gruppe</skos:prefLabel>
      <skos:definition xml:lang="da">To eller flere individer, der er samlet eller som har forenende forhold.</skos:definition>
      <skos:prefLabel xml:lang="de">Gruppe</skos:prefLabel>
      <skos:definition xml:lang="de">Zwei oder mehrere Einzelpersonen, die sich versammeln oder eine vereinende Beziehung miteinander haben.</skos:definition>
      <skos:prefLabel xml:lang="fi">Ryhm&#xe4;</skos:prefLabel>
      <skos:definition xml:lang="fi">Kaksi tai useampia henkil&#xf6;it&#xe4;, jotka ovat joko kokoontuneet yhteen tai joita yhdist&#xe4;&#xe4; jokin muu tekij&#xe4;. Lis&#xe4;ohje kansainv&#xe4;liseen m&#xe4;&#xe4;ritelm&#xe4;&#xe4;n: Mik&#xe4;li kyselytutkimus, vastaaja esiintyy joko ryhm&#xe4;n edustajana tai analysoijana. Kysymykset koskevat p&#xe4;&#xe4;asiallisesti ryhm&#xe4;&#xe4; ja ryhm&#xe4;n mielipiteit&#xe4;, ei henkil&#xf6;&#xe4; itse&#xe4;&#xe4;n. Mik&#xe4;li kysymykset koskevat sek&#xe4; ryhm&#xe4;&#xe4; ett&#xe4; henkil&#xf6;&#xe4;, k&#xe4;yt&#xe4; havaintoyksikk&#xf6;n&#xe4; molempia.</skos:definition>
      <skos:prefLabel xml:lang="no">Gruppe</skos:prefLabel>
      <skos:definition xml:lang="no">To eller flere personer som samles eller som har et forhold som forener dem.</skos:definition>
      <skos:prefLabel xml:lang="sv">Grupp</skos:prefLabel>
      <skos:definition xml:lang="sv">Tv&#xe5; eller flera personer som samlats eller som har n&#xe5;gon sorts relation som f&#xf6;renar dem.</skos:definition>
   </rdf:Description>
   <rdf:Description rdf:about="http://rdf-vocabulary.ddialliance.org/cv/AnalysisUnit/1.0/4970317">
      <rdf:type rdf:resource="http://www.w3.org/2004/02/skos/core#Concept"/>
      <skos:inScheme rdf:resource="http://rdf-vocabulary.ddialliance.org/cv/AnalysisUnit/1.0/"/>
      <skos:notation xml:lang="en">Object</skos:notation>
      <skos:prefLabel xml:lang="en">Object</skos:prefLabel>
      <skos:definition xml:lang="en">Anything material, but inanimate, that has an independent existence and may be perceived by the senses. Examples: objects of art (paintings, sculptures, etc.) or weapons, or vehicles, etc.</skos:definition>
      <skos:prefLabel xml:lang="da">Objekt</skos:prefLabel>
      <skos:definition xml:lang="da">Et hvert d&#xf8;dt materiale, der har en uafh&#xe6;ngig eksistens og som kan opfattes af sanserne. For eksempel kunstobjekter (skulpturer, malerier mm.) eller v&#xe5;ben eller k&#xf8;ret&#xf8;jer mm.</skos:definition>
      <skos:prefLabel xml:lang="de">Objekt</skos:prefLabel>
      <skos:definition xml:lang="de">Alle nicht lebenden Stoffe, die eine unabh&#xe4;ngige Existenz haben und durch Sinne wahrgenommen werden k&#xf6;nnen. Beispiele: Kunstobjekte (Gem&#xe4;lde, Skulpturen, etc.) oder Waffen oder Fahrzeuge usw.</skos:definition>
      <skos:prefLabel xml:lang="fi">Eloton objekti/esine</skos:prefLabel>
      <skos:definition xml:lang="fi">Mik&#xe4; tahansa konkreettinen, eloton esine/kohde, joka voidaan aistein havaita. Esimerkiksi taideteokset (veistokset, maalaukset, valokuvat), graffitit, aseet, ajoneuvot jne.</skos:definition>
      <skos:prefLabel xml:lang="no">Objekt</skos:prefLabel>
      <skos:definition xml:lang="no">Noe fysisk, men ikke levende som eksisterer som en uavhengig enhet og som kan oppfattes av sansene. For eksempel: kunst (malerier, skulpturer osv.), v&#xe5;pen, kj&#xf8;ret&#xf8;y etc.</skos:definition>
      <skos:prefLabel xml:lang="sv">F&#xf6;rem&#xe5;l</skos:prefLabel>
      <skos:definition xml:lang="sv">N&#xe5;got fysiskt men icke levande som existerar som en oberoende enhet och kan uppfattas av sinnena. Exempel: konstf&#xf6;rem&#xe5;l (tavlor, skulpturer, o.dyl.), vapen, fordon, m.m.</skos:definition>
   </rdf:Description>
   <rdf:Description rdf:about="http://rdf-vocabulary.ddialliance.org/cv/AnalysisUnit/1.0/6311ae1">
      <rdf:type rdf:resource="http://www.w3.org/2004/02/skos/core#Concept"/>
      <skos:inScheme rdf:resource="http://rdf-vocabulary.ddialliance.org/cv/AnalysisUnit/1.0/"/>
      <skos:notation xml:lang="en">Other</skos:notation>
      <skos:prefLabel xml:lang="en">Other</skos:prefLabel>
      <skos:definition xml:lang="en">Use if the unit of analysis is known, but not found in the list.</skos:definition>
      <skos:prefLabel xml:lang="da">Andre</skos:prefLabel>
      <skos:definition xml:lang="da">Brug denne analyseenheden er kendt, men ikke fremg&#xe5;r af listen.</skos:definition>
      <skos:prefLabel xml:lang="de">Sonstiges</skos:prefLabel>
      <skos:definition xml:lang="de">Verwenden Sie diese Kategorie, wenn die Analyseeinheit bekannt, aber nicht in der Liste vertreten ist.</skos:definition>
      <skos:prefLabel xml:lang="fi">Muu havaintoyksikk&#xf6;/aineistoyksikk&#xf6;tyyppi</skos:prefLabel>
      <skos:definition xml:lang="fi">K&#xe4;yt&#xe4; mik&#xe4;li havaintoyksikk&#xf6; on tiedossa, mutta ei l&#xf6;ydy sanastosta.</skos:definition>
      <skos:prefLabel xml:lang="no">Annet</skos:prefLabel>
      <skos:definition xml:lang="no">Benytt hvis analyseenheten er kjent, men ikke finnes i listen.</skos:definition>
      <skos:prefLabel xml:lang="sv">&#xd6;vrigt</skos:prefLabel>
      <skos:definition xml:lang="sv">Anv&#xe4;nd om analysenheten &#xe4;r k&#xe4;nd men saknas i listan.</skos:definition>
   </rdf:Description>
</rdf:RDF>
