<?xml version="1.0" encoding="UTF-8"?>
<rdf:RDF xmlns:dcterms="http://purl.org/dc/terms/"
          xmlns:owl="http://www.w3.org/2002/07/owl#"
          xmlns:rdf="http://www.w3.org/1999/02/22-rdf-syntax-ns#"
          xmlns:rdfs="http://www.w3.org/2000/01/rdf-schema#"
          xmlns:skos="http://www.w3.org/2004/02/skos/core#">
   <rdf:Description rdf:about="http://rdf-vocabulary.ddialliance.org/cv/DataSourceType/1.0/">
      <rdf:type rdf:resource="http://www.w3.org/2004/02/skos/core#ConceptScheme"/>
      <dcterms:isVersionOf rdf:resource="http://rdf-vocabulary.ddialliance.org/cv/DataSourceType"/>
      <skos:notation>DataSourceType</skos:notation>
      <skos:prefLabel xml:lang="en">Data Source Type</skos:prefLabel>
      <skos:prefLabel xml:lang="da">Type af datakilde</skos:prefLabel>
      <skos:prefLabel xml:lang="fi">Aineiston alkuperä</skos:prefLabel>
      <skos:prefLabel xml:lang="it">Tipo di fonte dei dati</skos:prefLabel>
      <skos:prefLabel xml:lang="lt">Duomenų šaltinio tipas</skos:prefLabel>
      <skos:prefLabel xml:lang="nl">Type databron</skos:prefLabel>
      <skos:prefLabel xml:lang="no">Type av datakilde</skos:prefLabel>
      <skos:prefLabel xml:lang="pt">Tipo de fonte de dados</skos:prefLabel>
      <skos:prefLabel xml:lang="sl">Vrste podatkovnih virov</skos:prefLabel>
      <skos:prefLabel xml:lang="sr">Vrste izvora podataka</skos:prefLabel>
      <skos:prefLabel xml:lang="sv">Typ av datakälla</skos:prefLabel>
      <skos:definition xml:lang="en">Includes a typology of data sources.</skos:definition>
      <skos:definition xml:lang="da">Indeholder en typologi af datakilder.</skos:definition>
      <skos:definition xml:lang="fi">Aineiston alkuperän tyyppi.</skos:definition>
      <skos:definition xml:lang="it">Include una tipologia delle fonti dei dati.</skos:definition>
      <skos:definition xml:lang="lt">Apima duomenų šaltinių tipologiją.</skos:definition>
      <skos:definition xml:lang="nl">Bevat een indeling van databronnen. </skos:definition>
      <skos:definition xml:lang="no">Inneholder en typologi av datakilder.</skos:definition>
      <skos:definition xml:lang="pt">Inclui uma tipologia de fontes de dados.</skos:definition>
      <skos:definition xml:lang="sl">Vključuje razvrstitev podatkovnih virov.</skos:definition>
      <skos:definition xml:lang="sr">Sadrži tipove izvora podataka.</skos:definition>
      <skos:definition xml:lang="sv">Innehåller en typologi av datakällor.</skos:definition>
      <owl:versionInfo>1.0</owl:versionInfo>
      <dcterms:license rdf:resource="Creative Commons Attribution 4.0 International"/>
      <dcterms:rights>Copyright ©DDI Alliance 2019</dcterms:rights>
      <skos:hasTopConcept rdf:resource="http://rdf-vocabulary.ddialliance.org/cv/DataSourceType/1.0/d53e110"/>
      <skos:hasTopConcept rdf:resource="http://rdf-vocabulary.ddialliance.org/cv/DataSourceType/1.0/d53e830"/>
      <skos:hasTopConcept rdf:resource="http://rdf-vocabulary.ddialliance.org/cv/DataSourceType/1.0/d53e909"/>
      <skos:hasTopConcept rdf:resource="http://rdf-vocabulary.ddialliance.org/cv/DataSourceType/1.0/d53e1067"/>
      <skos:hasTopConcept rdf:resource="http://rdf-vocabulary.ddialliance.org/cv/DataSourceType/1.0/d53e1305"/>
      <skos:hasTopConcept rdf:resource="http://rdf-vocabulary.ddialliance.org/cv/DataSourceType/1.0/d53e1544"/>
      <skos:hasTopConcept rdf:resource="http://rdf-vocabulary.ddialliance.org/cv/DataSourceType/1.0/d53e1622"/>
      <skos:hasTopConcept rdf:resource="http://rdf-vocabulary.ddialliance.org/cv/DataSourceType/1.0/d53e1700"/>
      <skos:hasTopConcept rdf:resource="http://rdf-vocabulary.ddialliance.org/cv/DataSourceType/1.0/d53e1778"/>
      <skos:hasTopConcept rdf:resource="http://rdf-vocabulary.ddialliance.org/cv/DataSourceType/1.0/d53e1857"/>
   </rdf:Description>
   <rdf:Description rdf:about="http://rdf-vocabulary.ddialliance.org/cv/DataSourceType/1.0/d53e110">
      <rdf:type rdf:resource="http://www.w3.org/2004/02/skos/core#Concept"/>
      <skos:inScheme rdf:resource="http://rdf-vocabulary.ddialliance.org/cv/DataSourceType/1.0/"/>
      <skos:notation>RegistersRecordsAccounts</skos:notation>
      <skos:prefLabel xml:lang="en">Registers/Records/Accounts</skos:prefLabel>
      <skos:definition xml:lang="en">Official, formal, or semi-formal documents listing for example items, names, occurrences, actions, or results, and preserved in writing or some other permanent form for later reference.</skos:definition>
      <skos:prefLabel xml:lang="da">Registre/Optegnelser/Opgørelser</skos:prefLabel>
      <skos:definition xml:lang="da">Officielle, formelle eller semi-formelle dokumenter, der for eksempel angiver elementer, navne, begivenheder, handlinger eller resultater og bevares på skrift eller i anden permanent form til senere henvisning.</skos:definition>
      <skos:prefLabel xml:lang="fi">Rekisterit/asiakirjat</skos:prefLabel>
      <skos:definition xml:lang="fi">Viralliset ja puoliviralliset asiakirjat, joissa luetellaan esimerkiksi asioita, nimiä, tapahtumia, toimintoja tai tuloksia ja jotka on säilytetty kirjoitetussa tai muussa pysyvässä muodossa myöhempää käyttöä varten.</skos:definition>
      <skos:prefLabel xml:lang="it">Registri/Documenti/Resoconti</skos:prefLabel>
      <skos:definition xml:lang="it">Documenti ufficiali, formali o semi-formali, che elencano per esempio articoli, nomi, occorrenze, azioni o risultati, e che sono conservati in forma scritta o in qualche altra forma permanente per possibili riferimenti futuri.</skos:definition>
      <skos:prefLabel xml:lang="lt">Registrai, įrašai ar ataskaitos</skos:prefLabel>
      <skos:definition xml:lang="lt">Tarnybiniai, oficialūs ar pusiau oficialūs dokumentai, kuriuose išvardijami, pavyzdžiui, vienetai, vardai, įvykiai, veiksmai ar rezultatai, ir išsaugomi vėlesniam naudojimui rašytinėje ar kitoje ilgalaikio saugojimo formoje.</skos:definition>
      <skos:prefLabel xml:lang="nl">Register</skos:prefLabel>
      <skos:definition xml:lang="nl"/>
      <skos:prefLabel xml:lang="no">Register/Registreringer/Oppføringer</skos:prefLabel>
      <skos:definition xml:lang="no">Offisielle, formelle eller semi-formelle dokumentoppføringer av for eksempel gjenstander, navn, hendelser, handlinger eller resultater, og som er bevart skriftlig eller i en annen permanent form for senere referanse.</skos:definition>
      <skos:prefLabel xml:lang="pt">Registos/Documentos/Relatórios</skos:prefLabel>
      <skos:definition xml:lang="pt">Documentos oficiais, formais ou semi-formais, que listem, por exemplo, itens, nomes, ocorrências, ações ou resultados, e preservados sob a forma escrita ou por outro meio permanente para referência posterior.</skos:definition>
      <skos:prefLabel xml:lang="sl">Registri/ Zapisi/ Računi</skos:prefLabel>
      <skos:definition xml:lang="sl">Uradni, formalni ali pol formalni seznami dokumentov, na primer enot, imen, dogodkov, dejanj ali rezultatov, ki so ohranjeni v pisni ali kakšni drugi trajni obliki za poznejšo uporabo.</skos:definition>
      <skos:prefLabel xml:lang="sr">Registri/Zapisi/Nalozi</skos:prefLabel>
      <skos:definition xml:lang="sr">Službeni, formalni ili polu-formalni dokumenti koji navode, na primer, predmete imena, pojave, radnje ili rezultate, a čuvaju se u pisanom obliku ili nekom drugom trajnom obliku koji omogućuje kasniju upotrebu.</skos:definition>
      <skos:prefLabel xml:lang="sv">Register/handlingar/förteckningar</skos:prefLabel>
      <skos:definition xml:lang="sv">Officiella, formella eller semi-formella dokument som listar till exempel namn, händelser, handlingar eller resultat och som är bevarade i skrift eller någon annan permanent form för senare användning.</skos:definition>
      <skos:narrower rdf:resource="http://rdf-vocabulary.ddialliance.org/cv/DataSourceType/1.0/d53e205"/>
      <skos:narrower rdf:resource="http://rdf-vocabulary.ddialliance.org/cv/DataSourceType/1.0/d53e283"/>
      <skos:narrower rdf:resource="http://rdf-vocabulary.ddialliance.org/cv/DataSourceType/1.0/d53e361"/>
      <skos:narrower rdf:resource="http://rdf-vocabulary.ddialliance.org/cv/DataSourceType/1.0/d53e440"/>
      <skos:narrower rdf:resource="http://rdf-vocabulary.ddialliance.org/cv/DataSourceType/1.0/d53e518"/>
      <skos:narrower rdf:resource="http://rdf-vocabulary.ddialliance.org/cv/DataSourceType/1.0/d53e596"/>
      <skos:narrower rdf:resource="http://rdf-vocabulary.ddialliance.org/cv/DataSourceType/1.0/d53e674"/>
      <skos:narrower rdf:resource="http://rdf-vocabulary.ddialliance.org/cv/DataSourceType/1.0/d53e752"/>
   </rdf:Description>
   <rdf:Description rdf:about="http://rdf-vocabulary.ddialliance.org/cv/DataSourceType/1.0/d53e205">
      <rdf:type rdf:resource="http://www.w3.org/2004/02/skos/core#Concept"/>
      <skos:inScheme rdf:resource="http://rdf-vocabulary.ddialliance.org/cv/DataSourceType/1.0/"/>
      <skos:notation>RegistersRecordsAccounts.Administrative</skos:notation>
      <skos:prefLabel xml:lang="en">Registers/Records/Accounts: Administrative</skos:prefLabel>
      <skos:definition xml:lang="en">Information collected on individuals or groups as part of the routine administrative procedures of an agency, business, or institution. Such data are not usually collected with research purposes in mind, may be voluminous, and may require preparation such as coding in order to be usable by researchers. Examples: income tax forms, population registers, naturalization records, birth/death certificates, patent applications, etc.</skos:definition>
      <skos:prefLabel xml:lang="da">Registre/Optegnelser/Opgørelser: Administrativ</skos:prefLabel>
      <skos:definition xml:lang="da">Oplysninger indsamlet om individer eller grupper som en del af de rutinemæssige, administrative procedurer hos et agentur, virksomhed eller institution. Sådanne data er ikke normalt indsamlet til forskningsbrug, kan være omfattende og kan kræve forberedelse i form af kodning for at være brugbart for forskere. Eksempler: Formularer til indkomstskat, folkeregistre, opgørelser over naturalisering, fødsels-/dødsattester, patentansøgninger mm.</skos:definition>
      <skos:prefLabel xml:lang="fi">Rekisterit/asiakirjat: hallinnolliset</skos:prefLabel>
      <skos:definition xml:lang="fi">Viraston, yrityksen tai muun organisaation esimerkiksi henkilöistä tai ryhmistä keräämää tietoa osana sen normaalia hallinnollista toimintaa. Tällaista tietoa ei yleensä kerätä ensisijaisesti tutkimustarkoituksiin ja se saattaa olla hyvin laajaa ja vaatia käsittelyä, kuten esimerkiksi koodausta, ollakseen tutkijoiden käytettävissä. Esimerkiksi tuloverotukseen liittyvät lomakkeet, väestötietorekisterit, syntymä/kuolintodistukset, patenttihakemukset.</skos:definition>
      <skos:prefLabel xml:lang="it">Registri/Documenti/Resoconti: amministrativi</skos:prefLabel>
      <skos:definition xml:lang="it">Informazioni raccolte su individui o gruppi come risultato delle procedure amministrative di routine di un'agenzia, azienda o istituzione. Tali dati non vengono solitamente raccolti per scopi di ricerca, possono essere voluminosi e possono richiedere una trasformazione - come, ad esempio, la codifica - prima di poter essere utilizzati dai ricercatori. Esempi: dichiarazione dei redditi, registri demografici, documenti di naturalizzazione, certificati di nascita/morte, domande di brevetto, ecc.</skos:definition>
      <skos:prefLabel xml:lang="lt">Registrai, įrašai ar ataskaitos: administraciniai</skos:prefLabel>
      <skos:definition xml:lang="lt">Informacija apie asmenis ar grupes, renkama vykdant agentūrų, verslo ar kitokių įstaigų įprastas administracines veiklas. Tokie duomenys paprastai nėra renkami tyrimų tikslais. Jie gali būti labai didelės apimties ir gali reikalauti specialaus paruošimo, pavyzdžiui, kodavimo, kad juos galėtų naudoti tyrėjai. Pavyzdžiai: pajamų mokesčių formos, gyventojų registrai, natūralizacijos įrašai, gimimo ar mirties liudijimai, patentų paraiškos ir kt.</skos:definition>
      <skos:prefLabel xml:lang="nl">Register: Administratief</skos:prefLabel>
      <skos:definition xml:lang="nl"/>
      <skos:prefLabel xml:lang="no">Register/Registreringer/Oppføringer: Administrativt</skos:prefLabel>
      <skos:definition xml:lang="no">Innsamlet informasjon om individer eller grupper som en del av rutinemessige administrative prosedyrer for et byrå, en virksomhet eller institusjon. Slike data er vanligvis ikke innhentet for forskningsformål, kan være omfattende og kan kreve forberedelser slik som koding for å kunne bli benyttet av forskere. For eksempel: Skjema for inntektsskatt, befolkningsregistre, naturaliseringsrate, fødsels-/dødsattester, patentsøknader etc.</skos:definition>
      <skos:prefLabel xml:lang="pt">Registos/Documentos/Relatórios: Administrativos</skos:prefLabel>
      <skos:definition xml:lang="pt">Informações recolhidas sobre indivíduos ou grupos como parte dos procedimentos administrativos de rotina de uma organização, empresa ou instituição. Estes dados não são normalmente recolhidos tendo em vista a investigação, podem ser volumosos e podem requerer preparação (como a codificação) antes de serem usados pelos pesquisadores. Exemplos: declaração de imposto sobre rendimentos, registos populacionais, registos de aquisição de nacionalidade por naturalização, certidões de nascimento/óbito, pedidos de patentes, etc.</skos:definition>
      <skos:prefLabel xml:lang="sl">Registri/ Zapisi/ Računi: administrativni</skos:prefLabel>
      <skos:definition xml:lang="sl">Informacije o posameznikih ali skupinah, zbrane v okviru vsakodnevnih upravnih postopkov agencij, podjetij ali institucij. Takšni podatki običajno prvotno niso zbrani za raziskovalne namene, lahko so obsežni in lahko zahtevajo določeno pripravo, kot je kodiranje, da jih lahko nato uporabijo raziskovalci. Primeri: obrazci za davek na dohodek, registri prebivalstva, evidence o naturalizaciji, potrdila o rojstvu/smrti, patentne prijave itd.</skos:definition>
      <skos:prefLabel xml:lang="sr">Registri/Zapisi/Nalozi: Administrativni</skos:prefLabel>
      <skos:definition xml:lang="sr">Informacije prikupljene o pojedincima ili grupama kao deo rutinskih administrativnih procedura organizacija, preduzeća ili institucija. Takvi podaci se obično ne prikupljaju u svrhu istraživanja. Mogu biti obimni i mogu zahtevati pripremu, kao što je kodiranje, kako bi istraživači mogli da ih koriste. Primeri: obrasci poreza na dohodak, registri stanovništva, evidencije o naturalizaciji, potvrde o rođenju/smrti, prijave patenta, itd.</skos:definition>
      <skos:prefLabel xml:lang="sv">Register/handlingar/förteckningar: Administrativa</skos:prefLabel>
      <skos:definition xml:lang="sv">Information som samlats in om individer eller grupper som en del av rutinmässiga administrativa förfaranden för en myndighet, företag eller institution. Sådana data samlas vanligtvis inte in med forskningsändamål i åtanke, kan vara omfattande och kräva förberedelser som kodning för att kunna användas av forskare. Exempel: inkomstskatteformulär, befolkningsregister, naturaliseringsregister, födelse-/dödsattester, patentansökningar osv.</skos:definition>
      <skos:broader rdf:resource="http://rdf-vocabulary.ddialliance.org/cv/DataSourceType/1.0/d53e110"/>
   </rdf:Description>
   <rdf:Description rdf:about="http://rdf-vocabulary.ddialliance.org/cv/DataSourceType/1.0/d53e283">
      <rdf:type rdf:resource="http://www.w3.org/2004/02/skos/core#Concept"/>
      <skos:inScheme rdf:resource="http://rdf-vocabulary.ddialliance.org/cv/DataSourceType/1.0/"/>
      <skos:notation>RegistersRecordsAccounts.Historical</skos:notation>
      <skos:prefLabel xml:lang="en">Registers/Records/Accounts: Historical</skos:prefLabel>
      <skos:definition xml:lang="en">Historical records preserve information and constitute evidence about past events. They may be produced by individuals, groups, or organizations. Administrative records become historical when they are no longer retained, or actively used by the issuing agency for their original purpose. Examples include parish registers, estate records, wills, chronicles, etc.</skos:definition>
      <skos:prefLabel xml:lang="da">Registre/Optegnelser/Opgørelser: Historisk</skos:prefLabel>
      <skos:definition xml:lang="da">Historiske opgørelser bevarer oplysninger og udgør beviser om tidligere begivenheder. De kan være produceret af individer, grupper eller organisationer. Administrative optegnelser bliver historiske, når de ikke længere beholdes eller anvendes aktivt af det udstedende agentur til deres oprindelige formål. Eksempler inkluderer sogneregistre, tingbøger, testamenter, krøniker mm.</skos:definition>
      <skos:prefLabel xml:lang="fi">Rekisterit/asiakirjat: historialliset</skos:prefLabel>
      <skos:definition xml:lang="fi">Historialliset asiakirjat säilyttävät tietoa ja toimivat todisteina menneistä tapahtumista. Ne voivat olla yksilöiden, ryhmien tai järjestöjen tuottamia. Hallinnollisista asiakirjoista tulee historiallisia, kun ne tuottanut organisaatio ei enää säilytä tai käytä niitä aktiivisesti alkuperäistä tarkoitusta varten. Esimerkiksi kirkonkirjat, kiinteistöasiakirjat, testamentit, kronikat.</skos:definition>
      <skos:prefLabel xml:lang="it">Registri/Documenti/Resoconti: storici</skos:prefLabel>
      <skos:definition xml:lang="it">I documenti storici conservano informazioni e costituiscono evidenze di eventi passati. Possono essere prodotti da individui, gruppi o organizzazioni. I documenti amministrativi diventano storici quando non vengono più conservati dall'istituzione che li ha prodotti oppure non sono più utilizzati attivamente per il loro scopo originale. Gli esempi includono registri parrocchiali, registri immobiliari, testamenti, diari, ecc.</skos:definition>
      <skos:prefLabel xml:lang="lt">Registrai, įrašai ar ataskaitos: istoriniai</skos:prefLabel>
      <skos:definition xml:lang="lt">Istoriniuose įrašuose saugoma informacija ir įrodymai apie praeities įvykius. Jų kūrėjais gali būti asmenys, grupės ar organizacijos. Administraciniai įrašai tampa istoriniais, kai jie daugiau nebėra reikalingi arba juos išdavusi agentūra jų aktyviai nebenaudoja pagal pirminį tikslą. Pavyzdžiui, parapijų, dvarų turto registrai, testamentai, kronikos ir kt.</skos:definition>
      <skos:prefLabel xml:lang="nl">Register: Historisch</skos:prefLabel>
      <skos:definition xml:lang="nl"/>
      <skos:prefLabel xml:lang="no">Register/Registreringer/Oppføringer: Historiske</skos:prefLabel>
      <skos:definition xml:lang="no">Historiske registreringer bevarer informasjon og konstituerer bevis om tidligere hendelser. De kan være produsert av individer, grupper eller organisasjoner. Administrative registre blir historiske når de ikke lenger bevares eller er i aktiv bruk for sitt originale formål. Eksempler inkluderer kirkebøker, eiendomsregistre, tesatmenter, krøniker etc.</skos:definition>
      <skos:prefLabel xml:lang="pt">Registos/Documentos/Relatórios: Históricos</skos:prefLabel>
      <skos:definition xml:lang="pt">Registos históricos preservam informações e constituem evidências/provas sobre eventos passados. Eles podem ser produzidos por indivíduos, grupos ou organizações. Os registos administrativos tornam-se históricos quando não são mais mantidos/conservados ou usados ativamente pela agência emissora com a finalidade para a qual foram originalmente criados. Exemplos: registos paroquiais, registos imobiliários, testamentos, crónicas, etc.</skos:definition>
      <skos:prefLabel xml:lang="sl">Registri/ Zapisi/ Računi: zgodovinski</skos:prefLabel>
      <skos:definition xml:lang="sl">Zgodovinski zapisi ohranjajo informacije in predstavljajo dokaze o preteklih dogodkih. Lahko jih pripravijo posamezniki, skupine ali organizacije. Upravni dokumenti postanejo zgodovinski, ko jih ustanova, ki jih je izdala, ne hrani več oziroma ne služijo več prvotnemu namenu uporabe. Primeri vključujejo župnijske knjige, zemljiške katastre, oporoke, kronike itd.</skos:definition>
      <skos:prefLabel xml:lang="sr">Registri/Zapisi/Nalozi: Istorijski</skos:prefLabel>
      <skos:definition xml:lang="sr">Istorijski zapisi čuvaju informacije i predstavljaju dokaze o prošlim događajima. Mogu ih kreirati pojedinci, grupe ili organizacije. Administrativni spisi postaju istorijski kada se više ne čuvaju ili ih aktivno ne koristi organizacija koja ih je kreirala za prvobitnu svrhu. Primeri uključuju matične knjige, evidencije o nekretninama, oporuke, dnevnike, itd.</skos:definition>
      <skos:prefLabel xml:lang="sv">Register/handlingar/förteckningar: Historiska</skos:prefLabel>
      <skos:definition xml:lang="sv">Historiska handlingar bevarar information och belägger tidigare händelser. De kan skapas av individer, grupper eller organisationer. Administrativa register blir historiska när de inte längre behålls eller används aktivt av den utfärdande verksamheten för sitt ursprungliga syfte. Exempel är kyrkoböcker, bouppteckningar, testamenten, krönikor osv.</skos:definition>
      <skos:broader rdf:resource="http://rdf-vocabulary.ddialliance.org/cv/DataSourceType/1.0/d53e110"/>
   </rdf:Description>
   <rdf:Description rdf:about="http://rdf-vocabulary.ddialliance.org/cv/DataSourceType/1.0/d53e361">
      <rdf:type rdf:resource="http://www.w3.org/2004/02/skos/core#Concept"/>
      <skos:inScheme rdf:resource="http://rdf-vocabulary.ddialliance.org/cv/DataSourceType/1.0/"/>
      <skos:notation>RegistersRecordsAccounts.Legal</skos:notation>
      <skos:prefLabel xml:lang="en">Registers/Records/Accounts: Legal</skos:prefLabel>
      <skos:definition xml:lang="en">Records pertaining to law and its administration, for example records related to cases that have been brought to court or to a tribunal.</skos:definition>
      <skos:prefLabel xml:lang="da">Registre/Optegnelser/Opgørelser: Retslige</skos:prefLabel>
      <skos:definition xml:lang="da">Optegnelser angående lovgivning og dens administration, for eksempel optegnelser relateret til sager, der har været bragt for en domstol eller et nævn.</skos:definition>
      <skos:prefLabel xml:lang="fi">Rekisterit/asiakirjat: juridiset</skos:prefLabel>
      <skos:definition xml:lang="fi">Juridiset ja juridishallinnolliset asiakirjat, kuten oikeuskäsittelyihin, oikeudenkäynteihin ja tuomioistuinten toimintaan liittyvät asiakirjat.</skos:definition>
      <skos:prefLabel xml:lang="it">Registri/Documenti/Resoconti: legali</skos:prefLabel>
      <skos:definition xml:lang="it">Documenti relativi alla legge e alla sua amministrazione, ad esempio record relativi a casi giudiziari portati in tribunale.</skos:definition>
      <skos:prefLabel xml:lang="lt">Registrai, įrašai ar ataskaitos: teisiniai</skos:prefLabel>
      <skos:definition xml:lang="lt">Įrašai susiję su įstatymais ir jų vykdymu, pavyzdžiui, įrašai, susiję su bylomis, kurios buvo perduotos teismui ar tribunolui.</skos:definition>
      <skos:prefLabel xml:lang="nl">Register: Juridisch</skos:prefLabel>
      <skos:definition xml:lang="nl"/>
      <skos:prefLabel xml:lang="no">Register/Registreringer/Oppføringer: Juridiske</skos:prefLabel>
      <skos:definition xml:lang="no">Registreringer knyttet til lovgivning og administrasjon, for eksempel knyttet til saker som har vært ført for en rett eller en domstol.</skos:definition>
      <skos:prefLabel xml:lang="pt">Registos/Documentos/Relatórios: Legais</skos:prefLabel>
      <skos:definition xml:lang="pt">Registos relativos à lei e à sua administração, por exemplo, registos relacionados com casos que foram levados a tribunal.</skos:definition>
      <skos:prefLabel xml:lang="sl">Registri/ Zapisi/ Računi: pravni</skos:prefLabel>
      <skos:definition xml:lang="sl">Zapisi, ki se na našajo na zakonodajo in njeno izvajanje, na primer evidenca primerov, ki so bili vloženi na sodišču.</skos:definition>
      <skos:prefLabel xml:lang="sr">Registri/Zapisi/Nalozi: Pravni</skos:prefLabel>
      <skos:definition xml:lang="sr">Zapisi koji se odnose na zakone i njihovu primenu. To, na primer, mogu biti zapisi koji se odnose na predmete koji su pred sudom.</skos:definition>
      <skos:prefLabel xml:lang="sv">Register/handlingar/förteckningar: Juridiska</skos:prefLabel>
      <skos:definition xml:lang="sv">Handlingar rörande lagstiftning och rättsskipning, till exempel handlingar i samband med ärenden som har väckts vid domstol eller nämnd.</skos:definition>
      <skos:broader rdf:resource="http://rdf-vocabulary.ddialliance.org/cv/DataSourceType/1.0/d53e110"/>
   </rdf:Description>
   <rdf:Description rdf:about="http://rdf-vocabulary.ddialliance.org/cv/DataSourceType/1.0/d53e440">
      <rdf:type rdf:resource="http://www.w3.org/2004/02/skos/core#Concept"/>
      <skos:inScheme rdf:resource="http://rdf-vocabulary.ddialliance.org/cv/DataSourceType/1.0/"/>
      <skos:notation>RegistersRecordsAccounts.MedicalClinical</skos:notation>
      <skos:prefLabel xml:lang="en">Registers/Records/Accounts: Medical/Clinical</skos:prefLabel>
      <skos:definition xml:lang="en">Health-related data created or collected by health care professionals about a patient. Usually include the results of medical tests or measurements, findings from consultations or clinical trial programs, etc.</skos:definition>
      <skos:prefLabel xml:lang="da">Registre/Optegnelser/Opgørelser: Medicinsk/Klinisk</skos:prefLabel>
      <skos:definition xml:lang="da">Sundhedsrelaterede data skabt eller indsamlet af sundhedspersonale om en patient. Indeholder som regel resultaterne af medicinske tests eller målinger, resultater fra konsultationer eller kliniske forsøgsprogrammer mm.</skos:definition>
      <skos:prefLabel xml:lang="fi">Rekisterit/asiakirjat: lääketieteelliset/kliiniset</skos:prefLabel>
      <skos:definition xml:lang="fi">Terveydenhuollon ammattilaisten potilaistaan keräämää tai tuottamaa, terveydentilaan liittyvää tietoa. Esimerkiksi lääketieteellisten kokeiden, testien ja mittausten tulokset, lääkärin tekemän tutkimuksen ja kliinisten tutkimusohjelmien löydökset.</skos:definition>
      <skos:prefLabel xml:lang="it">Registri/Documenti/Resoconti: medici/clinici</skos:prefLabel>
      <skos:definition xml:lang="it">Dati relativi alla salute creati o raccolti da operatori sanitari relativi a un paziente. Di solito includono risultati di esami o misurazioni mediche, risultati di consultazioni o programmi di sperimentazione clinica, ecc.</skos:definition>
      <skos:prefLabel xml:lang="lt">Registrai, įrašai ar ataskaitos: medicininiai ar klinikiniai</skos:prefLabel>
      <skos:definition xml:lang="lt">Sveikatos priežiūros specialistų sukurti ar surinkti su sveikata susiję duomenys apie pacientus. Paprastai apima medicininių tyrimų ar matavimų rezultatus, konsultacijų ar klinikinių tyrimų programų išvadas ir kt.</skos:definition>
      <skos:prefLabel xml:lang="nl">Register: Medisch/klinisch</skos:prefLabel>
      <skos:definition xml:lang="nl"/>
      <skos:prefLabel xml:lang="no">Register/Registreringer/Oppføringer: Medisinsk/Klinisk</skos:prefLabel>
      <skos:definition xml:lang="no">Helserelaterte data produsert eller innsamlet av helsepersonell om en pasient. Inneholder vanligvis resultater av medisinske tester eller målinger, funn fra konsultasjoner eller kliniske prøver etc.</skos:definition>
      <skos:prefLabel xml:lang="pt">Registos/Documentos/Relatórios: Médicos/Clínicos</skos:prefLabel>
      <skos:definition xml:lang="pt">Dados relativos à saúde criados ou recolhidos por profissionais de saúde sobre um paciente. Geralmente incluem os resultados de exames médicos ou medições, resultados de consultas ou testes de análises clínicas/ensaios clínicos, etc.</skos:definition>
      <skos:prefLabel xml:lang="sl">Registri/ Zapisi/ Računi: zdravstveni/ klinični</skos:prefLabel>
      <skos:definition xml:lang="sl">Zdravstveni podatki, ki jih ustvarijo ali zbirajo zdravstveni delavci o pacientu. Običajno vključujejo rezultate medicinskih preiskav ali meritev, ugotovitve posvetovanj ali programov kliničnega preizkušanja itd.</skos:definition>
      <skos:prefLabel xml:lang="sr">Registri/Zapisi/Nalozi: Medicinski/Klinički</skos:prefLabel>
      <skos:definition xml:lang="sr">Podaci o zdravlju pacijenata kreirani ili sakupljeni od strane zdravstvenih radnika. Obično uključuju rezultate medicinskih testova ili merenja, nalaze konsultacija ili programa kliničkih ispitivanja, itd.</skos:definition>
      <skos:prefLabel xml:lang="sv">Register/handlingar/förteckningar: Medicinska/kliniska</skos:prefLabel>
      <skos:definition xml:lang="sv">Hälsorelaterade data skapade eller insamlade av vårdpersonal om en patient. Vanligtvis ingår resultaten från konsultationer, medicinska tester eller kliniska prövningar osv.</skos:definition>
      <skos:broader rdf:resource="http://rdf-vocabulary.ddialliance.org/cv/DataSourceType/1.0/d53e110"/>
   </rdf:Description>
   <rdf:Description rdf:about="http://rdf-vocabulary.ddialliance.org/cv/DataSourceType/1.0/d53e518">
      <rdf:type rdf:resource="http://www.w3.org/2004/02/skos/core#Concept"/>
      <skos:inScheme rdf:resource="http://rdf-vocabulary.ddialliance.org/cv/DataSourceType/1.0/"/>
      <skos:notation>RegistersRecordsAccounts.AcademicAptitude</skos:notation>
      <skos:prefLabel xml:lang="en">Registers/Records/Accounts: Academic/Aptitude</skos:prefLabel>
      <skos:definition xml:lang="en">Information gathered during an evaluation process and presented as results. Examples include educational tests, IQ tests, verbal or logical reasoning tests, competence tests for professional occupations, etc.</skos:definition>
      <skos:prefLabel xml:lang="da">Registre/Optegnelser/Opgørelser: Akademisk/Egnethed</skos:prefLabel>
      <skos:definition xml:lang="da">Oplysninger indsamlet under en evalueringsproces og præsenteret som resultater. Eksempler inkluderer uddannelsesprøver, IQ-tests, tests af verbal eller logisk ræsonnement, tests af kompetencer til professionel beskæftigelse mm.</skos:definition>
      <skos:prefLabel xml:lang="fi">Rekisterit/asiakirjat: oppimis-,  soveltuvuus- ja kykytestit</skos:prefLabel>
      <skos:definition xml:lang="fi">Tietoa, joka on kerätty osana arviointiprosessia ja esitetään tuloksina. Esimerkiksi oppimiseen ja opiskeluun liittyvät kokeet ja testit, älykkyystestit, ammattien soveltuvuustestit.</skos:definition>
      <skos:prefLabel xml:lang="it">Registri/Documenti/Resoconti: accademici/attitudinali</skos:prefLabel>
      <skos:definition xml:lang="it">Informazioni raccolte durante un processo di valutazione e presentate come risultati. Esempi includono test educativi, test QI, test di ragionamento verbale o logico, test di competenza per attività professionali, ecc.</skos:definition>
      <skos:prefLabel xml:lang="lt">Registrai, įrašai ar ataskaitos: akademiniai ar gebėjimų</skos:prefLabel>
      <skos:definition xml:lang="lt">Vertinimo proceso metu surinkta informacija, pateikiama kaip rezultatas. Pavyzdžiai apima švietimo testus, IQ testus, žodinio ar loginio samprotavimo testus, profesinių gebėjimų testus ir kt.</skos:definition>
      <skos:prefLabel xml:lang="nl">Register: Onderwijs/bekwaamheid</skos:prefLabel>
      <skos:definition xml:lang="nl"/>
      <skos:prefLabel xml:lang="no">Register/Registreringer/Oppføringer: Kunnskap/Ferdighet</skos:prefLabel>
      <skos:definition xml:lang="no">Informasjon innhentet i en evalueringsprosess og som blir presentert som resultater. Eksempler inkluderer læringstester, IQ-tester, tester av verbale eller logiske resonnementer, kompetansetester for stillinger etc.</skos:definition>
      <skos:prefLabel xml:lang="pt">Registos/Documentos/Relatórios: Académicos (ou de aptidão)</skos:prefLabel>
      <skos:definition xml:lang="pt">Informações recolhidas durante um processo de avaliação e apresentadas como resultados. Exemplos incluem testes educacionais, testes de QI, testes de raciocínio verbal ou lógico, testes de competência para ocupações profissionais, etc.</skos:definition>
      <skos:prefLabel xml:lang="sl">Registri/ Zapisi/ Računi: študijski/ sposobnosti</skos:prefLabel>
      <skos:definition xml:lang="sl">Informacije, zbrane tekom izvajanja ocenjevanja in predstavljene kot rezultati. Primeri vključujejo preizkuse znanja, teste inteligentnosti, teste verbalnih in logičnih sposobnosti, preizkuse poklicnih kompetenc in usposobljenosti itd.</skos:definition>
      <skos:prefLabel xml:lang="sr">Registri/Zapisi/Nalozi: Akademski/Sposobnosti</skos:prefLabel>
      <skos:definition xml:lang="sr">Informacije prikupljene tokom procesa evaluacije i predstavljene kao rezultati. Primeri uključuju obrazovne testove, IQ testove, testove verbalnog ili logičkog rezonovanja, testove kompetencije za profesionalna zanimanja, itd.</skos:definition>
      <skos:prefLabel xml:lang="sv">Register/handlingar/förteckningar: Kunskaper/förmågor</skos:prefLabel>
      <skos:definition xml:lang="sv">Information insamlad under en utvärderingsprocess och framställd som resultat. Exempel är tentamina, IQ-tester, tester av verbal eller logisk förmåga, utvärderingar av yrkeskompetens osv.</skos:definition>
      <skos:broader rdf:resource="http://rdf-vocabulary.ddialliance.org/cv/DataSourceType/1.0/d53e110"/>
   </rdf:Description>
   <rdf:Description rdf:about="http://rdf-vocabulary.ddialliance.org/cv/DataSourceType/1.0/d53e596">
      <rdf:type rdf:resource="http://www.w3.org/2004/02/skos/core#Concept"/>
      <skos:inScheme rdf:resource="http://rdf-vocabulary.ddialliance.org/cv/DataSourceType/1.0/"/>
      <skos:notation>RegistersRecordsAccounts.EconomicFinancial</skos:notation>
      <skos:prefLabel xml:lang="en">Registers/Records/Accounts: Economic/Financial</skos:prefLabel>
      <skos:definition xml:lang="en">Records of the financial activities of a business, person, state institution or other organizations or entities. Examples are statements of retained earnings, cash flow, income statements, a company's balance sheet and tax return.</skos:definition>
      <skos:prefLabel xml:lang="da">Registre/Optegnelser/Opgørelser: Økonomisk/Finansiel</skos:prefLabel>
      <skos:definition xml:lang="da">Optegnelser af de finansielle aktiviteter hos en virksomhed, person, statslig institution eller andre organisationer eller enheder. Eksempler er redegørelser om bevaret indtjening, pengestrøm, resultatopgørelser, en virksomheds balance og selvangivelse.</skos:definition>
      <skos:prefLabel xml:lang="fi">Rekisterit/asiakirjat: taloudelliset</skos:prefLabel>
      <skos:definition xml:lang="fi">Yrityksen, henkilön, valtion viraston tai muun organisaation tai tahon taloudelliseen toimintaan liittyvät asiakirjat. Esimerkiksi rahoitus- ja tuloslaskelmat, yrityksen taseet ja veroilmoitukset.</skos:definition>
      <skos:prefLabel xml:lang="it">Registri/Documenti/Resoconti: economici/finanziari</skos:prefLabel>
      <skos:definition xml:lang="it">Registri delle attività finanziarie di un'azienda, persona, istituzione statale o di altre organizzazioni. Esempi sono le dichiarazioni di utili non distribuiti, il flusso di cassa, i conti economici, il bilancio di una società o le dichiarazioni fiscali.</skos:definition>
      <skos:prefLabel xml:lang="lt">Registrai, įrašai ar ataskaitos: ekonominiai ar finansiniai </skos:prefLabel>
      <skos:definition xml:lang="lt">Verslo, asmenų, valstybės institucijų ar kitokių organizacijų bei subjektų finansinės veiklos įrašai. Pavyzdžiui, nepaskirstyto pelno, pinigų srautų, pajamų ataskaitos, įmonių balansai ar mokesčių deklaracijos.</skos:definition>
      <skos:prefLabel xml:lang="nl">Register: Economisch/financieel</skos:prefLabel>
      <skos:definition xml:lang="nl"/>
      <skos:prefLabel xml:lang="no">Register/Registreringer/Oppføringer: Økonomisk/Finansielle</skos:prefLabel>
      <skos:definition xml:lang="no">Registreringer av finansielle aktiviteter til en virksomhet, person, statlig institusjon eller andre organisasjoner eller enheter. Eksempler inkluderer kunngjøringer om beholdt inntjening, kontantflyt, resultatregnskap, et selskaps balanseregnskap og skattemeldinger.</skos:definition>
      <skos:prefLabel xml:lang="pt">Registos/Documentos/Relatórios: Económicos/Financeiros</skos:prefLabel>
      <skos:definition xml:lang="pt">Registos das atividades financeiras de uma empresa, pessoa, instituição pública, ou outras organizações ou entidades. Exemplos são declarações de lucros acumulados, fluxo de caixa, declarações de rendimento, balanços de uma empresa e reembolso de impostos.</skos:definition>
      <skos:prefLabel xml:lang="sl">Registri/ Zapisi/ Računi: ekonomski/ finančni</skos:prefLabel>
      <skos:definition xml:lang="sl">Dokumenti o finančnih dejavnostih podjetij, posameznikov, državnih ustanov ali drugih organizacij oziroma entitet. Primeri so izkazi zadržanega dobička, denarni tok, izkazi poslovnega izida, bilanca stanja družbe in davčna napoved.</skos:definition>
      <skos:prefLabel xml:lang="sr">Registri/Zapisi/Nalozi: Ekonomski/Finansijski</skos:prefLabel>
      <skos:definition xml:lang="sr">Evidencija o finansijskim aktivnostima preduzeća, osobe, državne institucije ili drugih organizacija ili subjekata. Primeri su izveštaji o zadržanom dohotku, novčanim tokovima, izveštaji o dobiti, bilans stanja preduzeća i poreska prijava.</skos:definition>
      <skos:prefLabel xml:lang="sv">Register/handlingar/förteckningar: Ekonomiska/finansiella</skos:prefLabel>
      <skos:definition xml:lang="sv">Handlingar relaterade till den finansiella verksamheten hos en individ, ett företag, en statlig myndighet eller någon annan organisation eller enhet. Exempel är redovisning av kvarhållen vinst, kassaflöden, resultaträkningar, ett bolags bokföring eller skattedeklarationer.</skos:definition>
      <skos:broader rdf:resource="http://rdf-vocabulary.ddialliance.org/cv/DataSourceType/1.0/d53e110"/>
   </rdf:Description>
   <rdf:Description rdf:about="http://rdf-vocabulary.ddialliance.org/cv/DataSourceType/1.0/d53e674">
      <rdf:type rdf:resource="http://www.w3.org/2004/02/skos/core#Concept"/>
      <skos:inScheme rdf:resource="http://rdf-vocabulary.ddialliance.org/cv/DataSourceType/1.0/"/>
      <skos:notation>RegistersRecordsAccounts.Personal</skos:notation>
      <skos:prefLabel xml:lang="en">Registers/Records/Accounts: Personal</skos:prefLabel>
      <skos:definition xml:lang="en">Records or accounts created unofficially by individuals or families for other purposes than research. Examples may include private diaries or memoirs, family record books or Bibles, collections of personal documents, photographs, etc.</skos:definition>
      <skos:prefLabel xml:lang="da">Registre/Optegnelser/Opgørelser: Personlig</skos:prefLabel>
      <skos:definition xml:lang="da">Optegnelser eller opgørelser skabt uofficielt af individer eller familier til andre formål end forskning. Eksempler kan inkludere private dagbøger eller erindringer, familieoptegnelser eller bibler, samlinger af personlige dokumenter, fotografier mm.</skos:definition>
      <skos:prefLabel xml:lang="fi">Rekisterit/asiakirjat: henkilökohtaiset</skos:prefLabel>
      <skos:definition xml:lang="fi">Henkilöiden tai perheiden muuhun kuin tutkimustarkoituksiin epävirallisesti tuottamat asiakirjat ja dokumentit. Esimerkiksi henkilökohtaiset päiväkirjat tai muistelmat, sukukirjat tai perheraamatut, henkilökohtaisten dokumenttien kokoelmat, valokuvat.</skos:definition>
      <skos:prefLabel xml:lang="it">Registri/Documenti/Resoconti: personali</skos:prefLabel>
      <skos:definition xml:lang="it">Documenti creati in modo non ufficiale da individui o famiglie per scopi diversi dalla ricerca. Tali documenti possono riguardare diari privati o memorie, libri di famiglia, raccolte di documenti personali, fotografie, ecc.</skos:definition>
      <skos:prefLabel xml:lang="lt">Registrai, įrašai ar ataskaitos: asmeniniai</skos:prefLabel>
      <skos:definition xml:lang="lt">Įrašai ar ataskaitos, kurias neoficialiai sukūrė asmenys ar šeimos kitais nei mokslinių tyrimų tikslais. Pavyzdžiui, privatūs dienoraščiai ar atsiminimai, šeimos istorijos ar kitokių įrašų knygos, asmeninių dokumentų kolekcijos, nuotraukos ir kt.</skos:definition>
      <skos:prefLabel xml:lang="nl">Register: Persoonlijk</skos:prefLabel>
      <skos:definition xml:lang="nl"/>
      <skos:prefLabel xml:lang="no">Register/Registreringer/Oppføringer: Personlig</skos:prefLabel>
      <skos:definition xml:lang="no">Uoffisielle registreringer eller oppføringer laget av individer eller familier for andre formål enn forskning. Eksempler kan inkludere private dagbøker eller memorarer, familiebøker eller bibler, samling av private dokumenter, bilder etc.</skos:definition>
      <skos:prefLabel xml:lang="pt">Registos/Documentos/Relatórios: Pessoais</skos:prefLabel>
      <skos:definition xml:lang="pt">Registos ou cadastros criados não oficialmente por indivíduos ou famílias para outros fins que não a investigação. Exemplos podem incluir diários ou memórias privadas, livros de registos familiares, coleções de documentos pessoais, fotografias, etc.</skos:definition>
      <skos:prefLabel xml:lang="sl">Registri/ Zapisi/ Računi: osebni</skos:prefLabel>
      <skos:definition xml:lang="sl">Dokumenti oziroma poročila, ki so jih neuradno ustvarili posamezniki ali družine za prvotno neraziskovalne namene. Primeri lahko vključujejo zasebne dnevnike ali spomine, družinske knjige ali Biblije, zbirke osebnih dokumentov, fotografije itd.</skos:definition>
      <skos:prefLabel xml:lang="sr">Registri/Zapisi/Nalozi: Lični</skos:prefLabel>
      <skos:definition xml:lang="sr">Zapisi koje su nezvanično kreirali pojedinci ili porodice u druge svrhe, osim istraživanja. Primeri mogu uključivati privatne dnevnike ili memoare, porodične knjige ili Biblije, zbirke ličnih dokumenata, fotografija, itd.</skos:definition>
      <skos:prefLabel xml:lang="sv">Register/handlingar/förteckningar: Personliga</skos:prefLabel>
      <skos:definition xml:lang="sv">Handlingar eller förteckningar skapade inofficiellt av individer eller familjer för andra ändamål än forskning. Exempel kan inkludera privata dagböcker eller memoarer, nedteckningar av familjehistoria, familjebiblar, samlingar av personliga dokument, fotografier osv.</skos:definition>
      <skos:broader rdf:resource="http://rdf-vocabulary.ddialliance.org/cv/DataSourceType/1.0/d53e110"/>
   </rdf:Description>
   <rdf:Description rdf:about="http://rdf-vocabulary.ddialliance.org/cv/DataSourceType/1.0/d53e752">
      <rdf:type rdf:resource="http://www.w3.org/2004/02/skos/core#Concept"/>
      <skos:inScheme rdf:resource="http://rdf-vocabulary.ddialliance.org/cv/DataSourceType/1.0/"/>
      <skos:notation>RegistersRecordsAccounts.VotingResults</skos:notation>
      <skos:prefLabel xml:lang="en">Registers/Records/Accounts: Voting results</skos:prefLabel>
      <skos:definition xml:lang="en">Details of votes cast for candidates in an election (also known as 'election returns/results'), parliamentary or organizational votes on policies, motions or proposals, public referendums, etc.</skos:definition>
      <skos:prefLabel xml:lang="da">Registre/Optegnelser/Opgørelser: Valgresultater</skos:prefLabel>
      <skos:definition xml:lang="da">Detaljer om stemmeafgivelser på kandidater ved et valg (også kendt som 'valgresultater'), parlamentariske eller organisatoriske stemmeafgivninger om politikker, beslutningsforslag, udspil, folkeafstemninger mm.</skos:definition>
      <skos:prefLabel xml:lang="fi">Rekisterit/asiakirjat: äänestystulokset</skos:prefLabel>
      <skos:definition xml:lang="fi">Tiedot vaaleissa ehdokkaille annetuista äänistä (vaalitulokset), eduskunnan tai organisaatioiden äänestysten tulokset, kansanäänestykset jne.</skos:definition>
      <skos:prefLabel xml:lang="it">Registri/Documenti/Resoconti: risultati di voto</skos:prefLabel>
      <skos:definition xml:lang="it">Dettaglio dei voti espressi per i candidati alle elezioni (detti anche "risultati elettorali"), voti parlamentari o organizzativi espressi su politiche, mozioni o proposte, referendum pubblici, ecc.</skos:definition>
      <skos:prefLabel xml:lang="lt">Registrai, įrašai ar ataskaitos: balsavimo rezultatai </skos:prefLabel>
      <skos:definition xml:lang="lt">Informacija apie balsus, atiduotus per rinkimus (dar vadinama „rinkimų rezultatais“), per visuotinius referendumus, balsavimus parlamente ar kitose organizacijose dėl politinių pasiūlymų, įstatymų projektų, pataisų ir kt.</skos:definition>
      <skos:prefLabel xml:lang="nl">Register: Verkiezingsuitslag</skos:prefLabel>
      <skos:definition xml:lang="nl"/>
      <skos:prefLabel xml:lang="no">Register/Registreringer/Oppføringer: Valgresultat</skos:prefLabel>
      <skos:definition xml:lang="no">Detaljer om stemmegivning for kandidater i et valg (også kjent som 'valgresultat'), parlamentariske eller organisatoriske stemmegivninger om politiske saker, begjæringer eller forslag, folkeavstemninger etc.</skos:definition>
      <skos:prefLabel xml:lang="pt">Registos/Documentos/Relatórios: Resultados eleitorais</skos:prefLabel>
      <skos:definition xml:lang="pt">Detalhes dos votos expressos numa eleição (também conhecidos como 'resultados eleitorais'), votos parlamentares ou organizacionais sobre políticas, moções ou propostas, referendos públicos, etc.</skos:definition>
      <skos:prefLabel xml:lang="sl">Registri/ Zapisi/ Računi: volilni rezultati</skos:prefLabel>
      <skos:definition xml:lang="sl">Podrobnosti o oddanih glasovih za kandidate na volitvah (tudi "volilni izidi/rezultati"), parlamentarnih ali organizacijskih glasovanjih o politikah, pobudah in predlogih, javnih referendumih itd.</skos:definition>
      <skos:prefLabel xml:lang="sr">Registri/Zapisi/Nalozi: Rezultati glasanja</skos:prefLabel>
      <skos:definition xml:lang="sr">Pojedinosti glasanja za kandidate na izborima (poznate i kao „rezultati izbora“), bez obzira da li se radi o parlamentarnim ili glasanju o politikama na nivou organizacije, predlozima ili praćenju toka glasanja, javnim referendumima, itd.</skos:definition>
      <skos:prefLabel xml:lang="sv">Register/handlingar/förteckningar: Röstresultat</skos:prefLabel>
      <skos:definition xml:lang="sv">Uppgifter om avgivna röster för kandidater i ett val (även kallat "valresultat"), folkomröstningsresultat, organisationers eller parlamentledamöters röster på motioner, propositioner eller förslag osv.</skos:definition>
      <skos:broader rdf:resource="http://rdf-vocabulary.ddialliance.org/cv/DataSourceType/1.0/d53e110"/>
   </rdf:Description>
   <rdf:Description rdf:about="http://rdf-vocabulary.ddialliance.org/cv/DataSourceType/1.0/d53e830">
      <rdf:type rdf:resource="http://www.w3.org/2004/02/skos/core#Concept"/>
      <skos:inScheme rdf:resource="http://rdf-vocabulary.ddialliance.org/cv/DataSourceType/1.0/"/>
      <skos:notation>EventsInteractions</skos:notation>
      <skos:prefLabel xml:lang="en">Events/Interactions</skos:prefLabel>
      <skos:definition xml:lang="en">Events are usually one-time, individual occurrences, with a limited or short duration. An event may be listed as data source when it is directly observed or recorded for research. Interactions are events in which two or more people, groups, objects or systems act upon one another having reciprocal influence, or effect. Examples: types of gatherings (ceremonies, competitions, festivals, meetings), riots, terrorist attacks, computing events (i.e., actions or occurrences detected by computer programs), etc.</skos:definition>
      <skos:prefLabel xml:lang="da">Begivenheder/Interaktioner</skos:prefLabel>
      <skos:definition xml:lang="da">Begivenheder er som regel enkeltstående, individuelle hændelser med en begrænset eller kort varighed. En begivenhed kan være listet som en datakilde, når den observeres direkte eller optages til forskning. Interaktioner er begivenheder, hvor to eller flere personer, grupper, objekter eller systemer agerer i forhold til hinanden med gensidig indvirkning eller effekt. Eksempler: Typer af sammenkomster (ceremonier, konkurrencer, festivaler, møder), optøjer, terrorangreb, datalogiske begivenheder (dvs. handlinger eller hændelser opdaget ved hjælp af computerprogrammer) mm.</skos:definition>
      <skos:prefLabel xml:lang="fi">Tapahtumat/vuorovaikutustilanteet</skos:prefLabel>
      <skos:definition xml:lang="fi">Tapahtumat ovat yleensä yksittäisiä tapauksia, joiden kesto on lyhyt tai rajattu. Tapahtuma on aineistolähde silloin, kun sitä on suoraan havainnoitu tai taltioitu tutkimustarkoituksiin. Vuorovaikutustilanteet ovat tapahtumia, joissa kaksi tai useampi ihminen, ryhmä, esine tai järjestelmä vaikuttaa toisiinsa vastavuoroisesti. Esimerkiksi erilaiset tapaamiset (juhlat, kilpailut, festivaalit, kokoukset), mellakat, terroristihyökkäykset, tietokoneen toiminta (eli tietokoneohjelmien havaitsemat toiminnot tai tapahtumat).</skos:definition>
      <skos:prefLabel xml:lang="it">Eventi/Interazioni</skos:prefLabel>
      <skos:definition xml:lang="it">Gli eventi generalmente sono unici, accadono una sola volta, con una durata limitata o breve. Un evento può essere indicato come fonte di dati quando viene direttamente osservato o registrato per la ricerca. Le interazioni sono eventi in cui due o più persone, gruppi, oggetti o sistemi agiscono l'uno con l'altro influenzandosi reciprocamente. Esempi: raduni di vario tipo (cerimonie, concorsi, festival, riunioni), rivolte, attacchi terroristici, eventi informatici (cioè azioni o occorrenze rilevate da programmi per computer), ecc.</skos:definition>
      <skos:prefLabel xml:lang="lt">Įvykiai ar sąveikos</skos:prefLabel>
      <skos:definition xml:lang="lt">Įvykiai paprastai būna vienkartiniai, atskiri, ribotos arba trumpos trukmės. Įvykis gali būti nurodomas kaip duomenų šaltinis, kai jis tiesiogiai stebimas arba aprašomas atliekant tyrimą. Sąveikos – tai įvykiai, kurių metu veikia du ar daugiau žmonės, grupės, objektai ar sistemos, vienas kitam darydami įtaką ar poveikį. Pavyzdžiai: susibūrimai (ceremonijos, rungtynės, festivaliai, susitikimai), riaušės, teroristiniai išpuoliai, kompiuteriniai įvykiai (t. y. kompiuterių programų aptikti veiksmai ar įvykiai) ir kt.</skos:definition>
      <skos:prefLabel xml:lang="nl">Gebeurtenissen/Interactie</skos:prefLabel>
      <skos:definition xml:lang="nl"/>
      <skos:prefLabel xml:lang="no">Hendelser/Interaksjon</skos:prefLabel>
      <skos:definition xml:lang="no">Hendelser er vanligvis enkeltstående, individuelle forekomster med begrenset eller kort varighet. En hendelse kan bli oppført som en datakilde når den er direkte observert eller nedtegnet for forskningformål. Interaksjoner er hendelser hvor to eller flere personer, grupper, objekter eller systemer interagerer, og har gjensidig innflytelse eller effekt på hverandre. Eksempler: typer sammenkomster (seremonier, konkurranser, festivaler, møter), opprør, terrorangrep, cyberhendelser (som handlinger eller hendelser oppdaget av dataprogram) etc.</skos:definition>
      <skos:prefLabel xml:lang="pt">Eventos/Interações</skos:prefLabel>
      <skos:definition xml:lang="pt">Os eventos são geralmente ocorrências únicas, individuais, com uma duração curta ou limitada. Um evento pode ser catalogado como fonte de dados quando é diretamente observado ou registado para pesquisa/investigação. Interações são eventos em que duas ou mais pessoas, grupos, objetos ou sistemas, atuam uns sobre os outros, tendo uma influência ou efeito recíproco. Exemplos: alguns tipos de reuniões (cerimónias, competições, festivais, encontros), tumultos/motins, ataques terroristas, eventos de computação (i.e., ações ou ocorrências detetadas por programas de computador), etc.</skos:definition>
      <skos:prefLabel xml:lang="sl">Dogodki/ Interakcije</skos:prefLabel>
      <skos:definition xml:lang="sl">Dogodki so običajno enkratni, posamezni pojavi z omejenim ali kratkim trajanjem. Dogodek je lahko naveden kot vir podatkov, ko je neposredno opazovan ali zabeležen v okviru raziskave. Interakcije so dogodki v katerih dva ali več ljudi, skupin, objektov ali sistemov deluje hkrati drug z drugim, pri čemer imajo vzajemen vpliv ali učinek. Primeri: različne vrste zbiranj (slovesnosti, tekmovanja, festivali, srečanja), nemiri, teroristični napadi, računalniški dogodki (to so dejanja ali pojavi, ki jih odkrijejo računalniški programi) itd.</skos:definition>
      <skos:prefLabel xml:lang="sr">Događaji/Interakcije</skos:prefLabel>
      <skos:definition xml:lang="sr">Događaji su obično jednokratna, pojedinačna zbivanja, sa ograničenim ili kratkim trajanjem. Događaj se može navesti kao izvor podataka kada se direktno posmatra ili snima za istraživanje. Interakcije su događaji u kojima dve ili više ljudi, grupa, objekata ili sistema deluju jedni na druge i ostvaruju recipročni uticaj ili efekat. Primeri: različita okupljanja (ceremonije, takmičenja, festivali, sastanci), neredi, teroristički napadi, računarski događaji (tj. akcije ili događaji koje su otkrili računarski programi), itd.</skos:definition>
      <skos:prefLabel xml:lang="sv">Händelser/interaktioner</skos:prefLabel>
      <skos:definition xml:lang="sv">Händelser är vanligtvis enstaka, enskilda händelser, med begränsad eller kort varaktighet. En händelse kan anges som datakälla när den observeras direkt eller registreras för forskning. Interaktioner är händelser där två eller flera personer, grupper, föremål eller system har ömsesidig påverkan eller effekt på varandra. Exempel: typer av sammankomster (ceremonier, tävlingar, festivaler, möten), upplopp, terrorattacker, datorhändelser (dvs handlingar eller händelser som upptäcks av datorprogram) osv.</skos:definition>
   </rdf:Description>
   <rdf:Description rdf:about="http://rdf-vocabulary.ddialliance.org/cv/DataSourceType/1.0/d53e909">
      <rdf:type rdf:resource="http://www.w3.org/2004/02/skos/core#Concept"/>
      <skos:inScheme rdf:resource="http://rdf-vocabulary.ddialliance.org/cv/DataSourceType/1.0/"/>
      <skos:notation>Processes</skos:notation>
      <skos:prefLabel xml:lang="en">Processes</skos:prefLabel>
      <skos:definition xml:lang="en">Processes are sequences of occurrences, events, activities, actions or operations that take place over time and bring about changes or transformations in organisms, objects, ideas or social phenomena. For example, a business process may include receiving orders, invoicing, shipping the products, or setting a marketing budget.</skos:definition>
      <skos:prefLabel xml:lang="da">Processer</skos:prefLabel>
      <skos:definition xml:lang="da">Processer er sekvenser af hændelser, begivenheder, aktiviteter, handlinger eller operationer, der finder sted over tid og medfører forandringer eller transformationer i organismer, objekter, idéer eller sociale fænomener. For eksempel, en proces hos en virksomhed kan inkludere modtagelse af ordrer, fakturering, spedition eller fastlæggelse af et marketingsbudget.</skos:definition>
      <skos:prefLabel xml:lang="fi">Prosessit</skos:prefLabel>
      <skos:definition xml:lang="fi">Prosessit ovat tapahtumien, toimenpiteiden ja toimien sarjoja, jotka tapahtuvat tietyllä ajanjaksolla ja saavat aikaan muutoksia elollisissa olennoissa, asioissa, ideoissa tai yhteiskunnallisissa ilmiöissä. Esimerkiksi liiketoiminnan prosessi voi olla tilausten vastaanotto, laskutus, tuotteiden toimitus tai markkinointibudjetin laatiminen.</skos:definition>
      <skos:prefLabel xml:lang="it">Processi</skos:prefLabel>
      <skos:definition xml:lang="it">I processi sono sequenze di eventi, attività, azioni o operazioni che si verificano nel tempo e portano cambiamenti o trasformazioni in organismi, oggetti, idee o fenomeni sociali. Ad esempio, un processo aziendale può includere la ricezione di ordini, la fatturazione, la spedizione dei prodotti o l'impostazione di un budget di marketing.</skos:definition>
      <skos:prefLabel xml:lang="lt">Procesai </skos:prefLabel>
      <skos:definition xml:lang="lt">Procesai yra atvejų, įvykių, veiklų, veiksmų ar operacijų sekos, sukeliančios organizmų, objektų, idėjų ar socialinių reiškinių pokyčius ar transformacijas. Pavyzdžiui, verslo procesas gali apimti užsakymų gavimą, sąskaitų faktūrų išrašymą, produktų pristatymą arba rinkodaros biudžeto sudarymą.</skos:definition>
      <skos:prefLabel xml:lang="nl">Proces</skos:prefLabel>
      <skos:definition xml:lang="nl"/>
      <skos:prefLabel xml:lang="no">Prosesser</skos:prefLabel>
      <skos:definition xml:lang="no">Prosesser er sekvenser av forekomster, hendelser, aktiviteter, handlinger eller operasjoner som foregår over tid og bringer endringer eller transformasjoner i organismer, objekter, ideer eller sosiale fenomen. For eksempel kan en forretningsprosess inneholde ordrebestillinger, fakturering, leveranse, eller å sette markedsføringsbudsjett.</skos:definition>
      <skos:prefLabel xml:lang="pt">Processos</skos:prefLabel>
      <skos:definition xml:lang="pt">Processos são sequências de ocorrências, eventos, atividades, ações ou operações que ocorrem ao longo do tempo e provocam mudanças ou transformações em organismos, objetos, ideias ou fenómenos sociais. Por exemplo, um processo de negócios pode incluir receção de pedidos, faturação, remessa de produtos ou a definição de um orçamento de marketing.</skos:definition>
      <skos:prefLabel xml:lang="sl">Procesi</skos:prefLabel>
      <skos:definition xml:lang="sl">Procesi so zaporedja pojavov, dogodkov, aktivnosti, dejanj ali operacij, ki potekajo skozi čas in prinašajo spremembe ali preobrazbe v organizmih, predmetih, idejah ali družbenih pojavih. Na primer, poslovni proces lahko vključuje prejemanje naročil, izdajanje računov, pošiljanje izdelkov ali določanje proračuna za trženje.</skos:definition>
      <skos:prefLabel xml:lang="sr">Procesi</skos:prefLabel>
      <skos:definition xml:lang="sr">Procesi su nizovi pojava, događaja, aktivnosti, radnji ili operacija koji se dešavaju tokom vremena i dovode do promena ili transformacija u organizmima, predmetima, idejama ili društvenim pojavama. Na primer, poslovni proces može da uključuje primanje naloga, fakturisanje, otpremanje proizvoda ili utvrđivanje budžeta za marketing.</skos:definition>
      <skos:prefLabel xml:lang="sv">Processer</skos:prefLabel>
      <skos:definition xml:lang="sv">Processer är sekvenser av händelser, aktiviteter, handlingar eller operationer som sker över tid och leder till förändringar eller omvandlingar av organismer, föremål, idéer eller sociala fenomen. Exempelvis kan en affärsprocess omfatta mottagande av beställningar, fakturering, leverans av produkter eller beslut om marknadsföringsbudget.</skos:definition>
      <skos:narrower rdf:resource="http://rdf-vocabulary.ddialliance.org/cv/DataSourceType/1.0/d53e989"/>
   </rdf:Description>
   <rdf:Description rdf:about="http://rdf-vocabulary.ddialliance.org/cv/DataSourceType/1.0/d53e989">
      <rdf:type rdf:resource="http://www.w3.org/2004/02/skos/core#Concept"/>
      <skos:inScheme rdf:resource="http://rdf-vocabulary.ddialliance.org/cv/DataSourceType/1.0/"/>
      <skos:notation>Processes.Workflows</skos:notation>
      <skos:prefLabel xml:lang="en">Processes: Workflow(s)</skos:prefLabel>
      <skos:definition xml:lang="en">Sequence of steps and processes through which a piece of work passes from initiation to completion (adapted from the Oxford dictionary online: http://www.oxforddictionaries.com/us/definition/american_english/workflow). Examples from data life cycle: data collection, data processing, data analysis, data archiving, etc.</skos:definition>
      <skos:prefLabel xml:lang="da">Processer: Arbejdsgang(e)</skos:prefLabel>
      <skos:definition xml:lang="da">Sekvens af trin eller processer, hvor et stykke arbejde går fra at være igangsætning til afslutning (tilpasset fra the Oxford dictionary online: http://www.oxforddictionaries.com/us/definition/american_english/workflow). Eksempler fra datas livscyklus: dataindsamling, databehandling, dataanalyse, dataarkivering mm.</skos:definition>
      <skos:prefLabel xml:lang="fi">Prosessit: työnkulku</skos:prefLabel>
      <skos:definition xml:lang="fi">Sarja vaiheita ja prosesseja, joiden myötä teos tai kappale siirtyy alullepanosta valmistumiseen.</skos:definition>
      <skos:prefLabel xml:lang="it">Processi: flusso di lavoro</skos:prefLabel>
      <skos:definition xml:lang="it">Sequenza di passaggi e processi attraverso i quali una parte di lavoro passa dallo stato iniziale al suo completamento. Esempi tratti dal "ciclo di vita dei dati" sono: raccolta dei dati, elaborazione dei dati, analisi dei dati, archiviazione dei dati, ecc.</skos:definition>
      <skos:prefLabel xml:lang="lt">Procesai: darbų seka</skos:prefLabel>
      <skos:definition xml:lang="lt">Žingsnių ir procesų seka, kuriais pradedamas, vykdomas ir užbaigiamas tam tikras darbas (adaptuota pagal internetinį Oksfordo žodyną: http://www.oxforddictionaries.com/us/definition/american_english/workflow). Pavyzdžiai iš duomenų gyvavimo ciklo: duomenų rinkimas, duomenų apdorojimas, duomenų analizė, duomenų archyvavimas ir kt.</skos:definition>
      <skos:prefLabel xml:lang="nl">Proces: Workflow(s)</skos:prefLabel>
      <skos:definition xml:lang="nl"/>
      <skos:prefLabel xml:lang="no">Prosesser: Arbeidsflyt</skos:prefLabel>
      <skos:definition xml:lang="no">Sekvenser av trinn og prosesser et stykke arbeid går gjennom fra innledning til ferdigstillelse (tilpasset fra Oxford dictionary online: http://www.oxforddictionaries.com/us/definition/american_english/workflow). Eksempler fra data livssyklus: datainnsamling, databehandling, dataanalyse, dataarkivering etc.</skos:definition>
      <skos:prefLabel xml:lang="pt">Processos: Workflow(s)/Fluxo de trabalho</skos:prefLabel>
      <skos:definition xml:lang="pt">Sequência de fases e processos através dos quais um trabalho passa do início ao fim/conclusão (adaptado do dicionário Oxford online: http://www.oxforddictionaries.com/us/definition/american_english/workflow). Exemplos do ciclo de vida dos dados: recolha dos dados, processamento dos dados, análise dos dados, arquivo dos dados, etc.</skos:definition>
      <skos:prefLabel xml:lang="sl">Procesi: potek(i) dela</skos:prefLabel>
      <skos:definition xml:lang="sl">Zaporedje korakov in procesov, po katerih določeno delo poteka od začetka do zaključka (povzeto po Oxfordovem spletnem slovarju: http: // www .oxforddictionaries.com / us / definition / american_english / workflow). Primeri iz življenjskega cikla podatkov: zbiranje podatkov, obdelava podatkov, analiza podatkov, arhiviranje podatkov itd.</skos:definition>
      <skos:prefLabel xml:lang="sr">Procesi: Radni tok(ovi)</skos:prefLabel>
      <skos:definition xml:lang="sr">Redosled koraka i procesa kroz koji predmet rada prelazi od inicijacije do završetka (prilagođen onlajn iz Oksfordovog rečnika: http://www.oxforddictionaries.com/us/definition/american_english/workflow). Primeri iz životnog ciklusa podataka su: prikupljanje podataka, obrada podataka, analiza podataka, arhiviranje podataka, itd.</skos:definition>
      <skos:prefLabel xml:lang="sv">Processer: Arbetsflöde(n)</skos:prefLabel>
      <skos:definition xml:lang="sv">Sekvens av steg och processer som innebär att ett arbete går från att påbörjas till att det slutförs. Exempel från datalivscykeln: datainsamling, databehandling, dataanalys, datalagring osv.</skos:definition>
      <skos:broader rdf:resource="http://rdf-vocabulary.ddialliance.org/cv/DataSourceType/1.0/d53e909"/>
   </rdf:Description>
   <rdf:Description rdf:about="http://rdf-vocabulary.ddialliance.org/cv/DataSourceType/1.0/d53e1067">
      <rdf:type rdf:resource="http://www.w3.org/2004/02/skos/core#Concept"/>
      <skos:inScheme rdf:resource="http://rdf-vocabulary.ddialliance.org/cv/DataSourceType/1.0/"/>
      <skos:notation>Communications</skos:notation>
      <skos:prefLabel xml:lang="en">Communications</skos:prefLabel>
      <skos:definition xml:lang="en">Messages resulting from the act or process of using words, sounds, signs, or behaviors to convey or exchange information, ideas, thoughts, feelings, etc. (adapted from www.merriam-webster.com).</skos:definition>
      <skos:prefLabel xml:lang="da">Kommunikation</skos:prefLabel>
      <skos:definition xml:lang="da">Meddelelser som følge af handlingen eller processen ved at bruge ord, lyd, tegn eller adfærd til at formidle eller udveksle informationer, idéer, tanker, følelser mm. (tilpasset fra www.merriam-webster.com).</skos:definition>
      <skos:prefLabel xml:lang="fi">Viestintä</skos:prefLabel>
      <skos:definition xml:lang="fi">Esimerkiksi sanoin, äänin, merkein, ilmein tai elein tuotettavat viestit, joilla välitetään tai vaihdetaan tietoa, ideoita, ajatuksia, tunteita ym.</skos:definition>
      <skos:prefLabel xml:lang="it">Comunicazioni</skos:prefLabel>
      <skos:definition xml:lang="it">Messaggi derivanti dall'utilizzo di parole, suoni, segni o comportamenti per trasmettere o scambiare informazioni, idee, pensieri, sentimenti, ecc.</skos:definition>
      <skos:prefLabel xml:lang="lt">Komunikacija</skos:prefLabel>
      <skos:definition xml:lang="lt">Pranešimai, atsirandantys kai žodžiai, garsai, ženklai ar elgesys naudojami siekiant perduoti ar keistis informacija, idėjomis, mintimis, jausmais ir kt. (adaptuota pagal www.merriam-webster.com).</skos:definition>
      <skos:prefLabel xml:lang="nl">Communicatie</skos:prefLabel>
      <skos:definition xml:lang="nl"/>
      <skos:prefLabel xml:lang="no">Kommunikasjon</skos:prefLabel>
      <skos:definition xml:lang="no">Beskjeder som resulterer fra handlingen eller prosessen ved å bruke ord, lyder, tegn eller atferd for å formidle eller utveksle informasjon, ideer, tanker, følelser etc. (tilpasset fra www.merriam-webster.com).</skos:definition>
      <skos:prefLabel xml:lang="pt">Comunicações</skos:prefLabel>
      <skos:definition xml:lang="pt">Mensagens resultantes do ato ou processo de usar palavras, sons, sinais ou comportamentos para transmitir ou trocar informações, ideias, pensamentos, sentimentos, etc. (do inglês adaptado de www.merriam-webster.com).</skos:definition>
      <skos:prefLabel xml:lang="sl">Komunikacije</skos:prefLabel>
      <skos:definition xml:lang="sl">Sporočila, ki izhajajo iz dejanja ali procesa uporabe besed, zvokov, znakov ali vedenj za prenos ali izmenjavo informacij, idej, misli, čustev itd. (povzeto po www.merriam-webster.com).</skos:definition>
      <skos:prefLabel xml:lang="sr">Komunikacija</skos:prefLabel>
      <skos:definition xml:lang="sr">Poruke proistekle iz postupka ili procesa upotrebe reči, zvukova, znakova ili ponašanja za prenošenje ili razmenu informacija, ideja, misli, oseć́anja, itd. (Prilagođeno sa www.merriam-webster.com).</skos:definition>
      <skos:prefLabel xml:lang="sv">Kommunikation</skos:prefLabel>
      <skos:definition xml:lang="sv">Meddelanden som härrör från aktiviteten eller processen att använda ord, ljud, tecken eller beteenden för att förmedla eller utbyta information, idéer, tankar, känslor osv.</skos:definition>
      <skos:narrower rdf:resource="http://rdf-vocabulary.ddialliance.org/cv/DataSourceType/1.0/d53e1149"/>
      <skos:narrower rdf:resource="http://rdf-vocabulary.ddialliance.org/cv/DataSourceType/1.0/d53e1227"/>
   </rdf:Description>
   <rdf:Description rdf:about="http://rdf-vocabulary.ddialliance.org/cv/DataSourceType/1.0/d53e1149">
      <rdf:type rdf:resource="http://www.w3.org/2004/02/skos/core#Concept"/>
      <skos:inScheme rdf:resource="http://rdf-vocabulary.ddialliance.org/cv/DataSourceType/1.0/"/>
      <skos:notation>Communications.Public</skos:notation>
      <skos:prefLabel xml:lang="en">Communications: Public</skos:prefLabel>
      <skos:definition xml:lang="en">Communications addressed directly to a public audience, for example, in person (public gatherings, political rallies, etc.), by means of broadcast, print or Internet mass media (radio, television, print or online newspapers/journals), by means of billboards, banners or other signage placed in public view, or social media (public postings on Facebook, Twitter, and others).</skos:definition>
      <skos:prefLabel xml:lang="da">Kommunikation: Offentlig</skos:prefLabel>
      <skos:definition xml:lang="da">Kommunikation rettet direkte til et offentligt publikum, for eksempel, personligt (offentlige forsamlinger, politiske møder mm.) ved hjælp af TV-udsendelser, trykte massemedier eller massemedier på internettet (radio, fjernsyn trykte eller online netaviser/tidsskrifter), ved hjælp af reklametavler, bannere eller anden skiltning placeret i det offentlige rum, eller sociale medier (offentlige indlæg på Facebook, Twitter, og andre).</skos:definition>
      <skos:prefLabel xml:lang="fi">Viestintä: julkinen</skos:prefLabel>
      <skos:definition xml:lang="fi">Suoraan julkiselle yleisölle osoitetut viestit. Viestit voidaan välittää esimerkiksi kasvokkain (julkiset kokoontumiset, poliittiset tapahtumat), massaviestimillä (radio, televisio, painettu media, verkkolehdet/julkaisut), ulkomainoksilla ja muilla julkisissa tiloissa sijaitsevilla ilmoituksilla tai sosiaalisessa mediassa (julkiset kommentit ja julkaisut Facebookissa, Twitterissä ym.)</skos:definition>
      <skos:prefLabel xml:lang="it">Comunicazioni: pubbliche</skos:prefLabel>
      <skos:definition xml:lang="it">Comunicazioni indirizzate direttamente a un pubblico che può essere presente (raduni pubblici, manifestazioni politiche, ecc.), oppure ricevere la comunicazione tramite mezzi di trasmissione, stampa o mass media (radio, televisione, stampa o giornali/riviste online), mediante cartelloni pubblicitari, striscioni o altri tipi di segnaletica collocati in modo visibile, oppure tramite social media (messaggi pubblici su Facebook, Twitter e altri).</skos:definition>
      <skos:prefLabel xml:lang="lt">Komunikacija: viešoji</skos:prefLabel>
      <skos:definition xml:lang="lt">Pranešimai tiesiogiai skirti viešai auditorijai, pavyzdžiui, kai dalyvaujama asmeniškai (viešuose susibūrimuose, politiniuose mitinguose ir pan.), kai transliuojama ar naudojama spausdintinė ar internetinė žiniasklaida (per radiją, televiziją, spausdintuose ar internetiniuose laikraščiuose ar  žurnaluose), kai naudojami reklaminiai stendai, reklaminės juostos ar kitos priemonės, talpinamos viešai arba socialinėse medijose (vieši įrašai „Facebook“, „Twitter“ ir kt.).</skos:definition>
      <skos:prefLabel xml:lang="nl">Massacommunicatie</skos:prefLabel>
      <skos:definition xml:lang="nl"/>
      <skos:prefLabel xml:lang="no">Kommunikasjon: Offentlig</skos:prefLabel>
      <skos:definition xml:lang="no">Kommunikasjon adressert direkte til et offentlig publikum, for eksempel personlig (offentlige sammenkomster, politiske samlinger etc.), ved hjelp av kringkasting, trykket massemedia eller massemedia på internett (radio, fjernsyn, trykte aviser eller nettaviser/tidsskrift), ved hjelp av reklametavler, bannere eller annen skilting i det offentlige, eller sosiale medier (offentlige innlegg på Facebook, Twitter og annet).</skos:definition>
      <skos:prefLabel xml:lang="pt">Comunicações: Públicas</skos:prefLabel>
      <skos:definition xml:lang="pt">Comunicações dirigidas diretamente a uma audiência pública, por exemplo, presencialmente (reuniões públicas, comícios políticos, etc.), por meios de difusão impressos, comunicação social ou Internet (rádio, televisão, jornais impressos ou online), por meio de painéis (outdoors), banners/cartazes ou outras sinalizações colocadas na via pública, ou nos media sociais (por exemplo, publicações públicas no Facebook, Twitter, entre outros).</skos:definition>
      <skos:prefLabel xml:lang="sl">Komunikacije: javne</skos:prefLabel>
      <skos:definition xml:lang="sl">Sporočanje, namenjeno neposredno javnosti. Na primer, osebno (javna zbiranja, politična zborovanja itd.), s pomočjo oddajnih, tiskanih ali spletnih medijev (radio, televizija, tiskani ali spletni časopisi/revije), s pomočjo oglasnih desk in panojev, pasic ali drugih označb, objavljenih javno ali na družbenih omrežjih (javne objave na Facebooku, Twitterju in drugih).</skos:definition>
      <skos:prefLabel xml:lang="sr">Komunikacija: Javna</skos:prefLabel>
      <skos:definition xml:lang="sr">Komunikacija direktno upućena javnoj publici, na primer, lično obraćanje (javna okupljanja, politički skupovi itd.), putem emitovanja, štampe ili internet masovnih medija (radija, televizije, štampe ili internet novina/časopisa), putem bilborda, transparenata ili drugih natpisa postavljenih u javnosti ili na društvenim mrežama (javne objave na Facebooku, Twitteru i dr.).</skos:definition>
      <skos:prefLabel xml:lang="sv">Kommunikation: Offentlig</skos:prefLabel>
      <skos:definition xml:lang="sv">Kommunikation riktad direkt till en allmän publik, till exempel personligen (offentliga sammankomster, politiska sammankomster osv.), genom etermedia, tryckta medier eller massmedia på Internet (radio-, tv-, eller dagstidningar/tidskrifter i tryckt eller elektroniskt format), med hjälp av skyltar, banderoller eller annan skyltning i det offentliga rummet, eller sociala medier (offentliga inlägg på Facebook, Twitter och andra).</skos:definition>
      <skos:broader rdf:resource="http://rdf-vocabulary.ddialliance.org/cv/DataSourceType/1.0/d53e1067"/>
   </rdf:Description>
   <rdf:Description rdf:about="http://rdf-vocabulary.ddialliance.org/cv/DataSourceType/1.0/d53e1227">
      <rdf:type rdf:resource="http://www.w3.org/2004/02/skos/core#Concept"/>
      <skos:inScheme rdf:resource="http://rdf-vocabulary.ddialliance.org/cv/DataSourceType/1.0/"/>
      <skos:notation>Communications.Interpersonal</skos:notation>
      <skos:prefLabel xml:lang="en">Communications: Interpersonal</skos:prefLabel>
      <skos:definition xml:lang="en">Communications made by an individual to another individual or a private group of persons, for purposes other than research. For example emails, letters, telephone conversations, social media postings with limited access.</skos:definition>
      <skos:prefLabel xml:lang="da">Kommunikation: Interpersonel</skos:prefLabel>
      <skos:definition xml:lang="da">Kommunikation foretaget af et individ til et andet individ eller en privat grupper af personer, til andre formål end forskning. For eksempel e-mails, breve, telefonsamtaler, indlæg på sociale medier med begrænset adgang.</skos:definition>
      <skos:prefLabel xml:lang="fi">Viestintä: henkilöiden välinen</skos:prefLabel>
      <skos:definition xml:lang="fi">Henkilön toiselle henkilölle tai ryhmälle osoittamat viestit muissa kuin tutkimustarkoituksissa. Esimerkiksi sähköpostit, kirjeet, puhelinkeskustelut tai tietylle ryhmälle rajatut sosiaalisen median viestit.</skos:definition>
      <skos:prefLabel xml:lang="it">Comunicazioni: interpersonali</skos:prefLabel>
      <skos:definition xml:lang="it">Comunicazioni fatte da un individuo a un altro individuo oppure a un gruppo privato di persone, per scopi diversi dalla ricerca. Ad esempio e-mail, lettere, conversazioni telefoniche, post sui social media con accesso limitato.</skos:definition>
      <skos:prefLabel xml:lang="lt">Komunikacija: tarpasmeninė</skos:prefLabel>
      <skos:definition xml:lang="lt">Vieno asmens komunikacija kitam asmeniui ar privačiai asmenų grupei kitais nei tyrimų tikslais. Pavyzdžiui, el. laiškai, laiškai, telefoniniai pokalbiai, nevieši socialinių medijų įrašai.</skos:definition>
      <skos:prefLabel xml:lang="nl">Communicatie: Persoonlijk</skos:prefLabel>
      <skos:definition xml:lang="nl"/>
      <skos:prefLabel xml:lang="no">Kommunikasjon: Mellommenneskelig</skos:prefLabel>
      <skos:definition xml:lang="no">Kommunikasjon fra et individ til et annet individ, eller private grupper med personer, for andre formål enn forskning. For eksempel e-poster, brev, telefonsamtaler, innlegg på sosiale medier med begrenset tilgang.</skos:definition>
      <skos:prefLabel xml:lang="pt">Comunicações: Interpessoais</skos:prefLabel>
      <skos:definition xml:lang="pt">Comunicações feitas por um indivíduo dirigidas a outro indivíduo ou a um grupo privado de pessoas, com outros fins que não a investigação. Por exemplo, emails, cartas, conversas telefónicas, publicações nos media sociais com acesso restrito.</skos:definition>
      <skos:prefLabel xml:lang="sl">Komunikacije: medosebne</skos:prefLabel>
      <skos:definition xml:lang="sl">Sporočila, ki jih posameznik posreduje drugemu posamezniku ali zasebni skupini oseb, z nameni, ki niso raziskovalni. Na primer e-poštna sporočila, pisma, telefonski pogovori, objave na družbenih omrežjih z omejenim dostopom.</skos:definition>
      <skos:prefLabel xml:lang="sr">Komunikacija: Između ljudi/Privatna</skos:prefLabel>
      <skos:definition xml:lang="sr">Komunikacija koju pojedinac uspostavlja sa drugim pojedincem ili sa&amp;nbsp; grupom osoba, privatno, odnosno u druge svrhe osim istraživanja. Na primer, elektronska pošta, pisma, telefonski razgovori, objave na društvenim mrežama sa ograničenim pristupom.</skos:definition>
      <skos:prefLabel xml:lang="sv">Kommunikation: Mellanmänsklig</skos:prefLabel>
      <skos:definition xml:lang="sv">Kommunikation från en person till en annan person eller till en privat grupp av personer, för andra ändamål än forskning. Exempel: e-post, brev, telefonsamtal, inlägg på sociala medier med begränsad åtkomst.</skos:definition>
      <skos:broader rdf:resource="http://rdf-vocabulary.ddialliance.org/cv/DataSourceType/1.0/d53e1067"/>
   </rdf:Description>
   <rdf:Description rdf:about="http://rdf-vocabulary.ddialliance.org/cv/DataSourceType/1.0/d53e1305">
      <rdf:type rdf:resource="http://www.w3.org/2004/02/skos/core#Concept"/>
      <skos:inScheme rdf:resource="http://rdf-vocabulary.ddialliance.org/cv/DataSourceType/1.0/"/>
      <skos:notation>ResearchData</skos:notation>
      <skos:prefLabel xml:lang="en">Research data</skos:prefLabel>
      <skos:definition xml:lang="en">Pre-existing data; data that have already been collected and/or used for a different research project.</skos:definition>
      <skos:prefLabel xml:lang="da">Forskningsdata</skos:prefLabel>
      <skos:definition xml:lang="da">Allerede-eksisterende data; data, der allerede er indsamlet og/eller anvendt til et andet forskningsprojekt.</skos:definition>
      <skos:prefLabel xml:lang="fi">Tutkimusaineisto</skos:prefLabel>
      <skos:definition xml:lang="fi">Olemassa oleva aineisto, joka on jo kerätty aiemmin tai jota on käytetty eri tutkimusta varten. Esimerkiksi metatutkimus.</skos:definition>
      <skos:prefLabel xml:lang="it">Dati di ricerca</skos:prefLabel>
      <skos:definition xml:lang="it">Dati preesistenti; dati che sono già stati raccolti e/o utilizzati per un diverso progetto di ricerca.</skos:definition>
      <skos:prefLabel xml:lang="lt">Tyrimų duomenys</skos:prefLabel>
      <skos:definition xml:lang="lt">Egzistuojantys duomenys; duomenys, kurie buvo surinkti ir (arba) panaudoti kitam tyrimų projektui.</skos:definition>
      <skos:prefLabel xml:lang="nl">Onderzoeksdata</skos:prefLabel>
      <skos:definition xml:lang="nl"/>
      <skos:prefLabel xml:lang="no">Forskningsdata</skos:prefLabel>
      <skos:definition xml:lang="no">Eksisterende data; data som allerede er innsamlet og/eller brukt i forbindelse med et annet forkningsprosjekt.</skos:definition>
      <skos:prefLabel xml:lang="pt">Dados de investigação</skos:prefLabel>
      <skos:definition xml:lang="pt">Dados preexistentes; dados que foram já recolhidos e/ou usados para um projeto de pesquisa anterior.</skos:definition>
      <skos:prefLabel xml:lang="sl">Raziskovalni podatki</skos:prefLabel>
      <skos:definition xml:lang="sl">Že obstoječi podatki; podatki, ki so že bili zbrani in/ali uporabljeni za drug raziskovalni projekt.</skos:definition>
      <skos:prefLabel xml:lang="sr">Istraživački podaci</skos:prefLabel>
      <skos:definition xml:lang="sr">Postojeći podaci; podaci koji su već prikupljeni i/ili korišćeni za drugi istraživački projekat.</skos:definition>
      <skos:prefLabel xml:lang="sv">Forskningsdata</skos:prefLabel>
      <skos:definition xml:lang="sv">Redan existerande data; data som redan har samlats in och/eller använts för ett annat forskningsprojekt.</skos:definition>
      <skos:narrower rdf:resource="http://rdf-vocabulary.ddialliance.org/cv/DataSourceType/1.0/d53e1388"/>
      <skos:narrower rdf:resource="http://rdf-vocabulary.ddialliance.org/cv/DataSourceType/1.0/d53e1466"/>
   </rdf:Description>
   <rdf:Description rdf:about="http://rdf-vocabulary.ddialliance.org/cv/DataSourceType/1.0/d53e1388">
      <rdf:type rdf:resource="http://www.w3.org/2004/02/skos/core#Concept"/>
      <skos:inScheme rdf:resource="http://rdf-vocabulary.ddialliance.org/cv/DataSourceType/1.0/"/>
      <skos:notation>ResearchData.Published</skos:notation>
      <skos:prefLabel xml:lang="en">Research data: Published</skos:prefLabel>
      <skos:definition xml:lang="en">Pre-existing data that have been made available to the general public, or sections thereof.</skos:definition>
      <skos:prefLabel xml:lang="da">Forskningsdata: Publiceret</skos:prefLabel>
      <skos:definition xml:lang="da">Allerede-eksisterende data, der er gjort tilgængelige for den generelle offentlighed, eller dele heraf.</skos:definition>
      <skos:prefLabel xml:lang="fi">Tutkimusaineisto: julkaistu</skos:prefLabel>
      <skos:definition xml:lang="fi">Olemassa oleva aineisto, joka on julkisesti saatavilla.</skos:definition>
      <skos:prefLabel xml:lang="it">Dati di ricerca: pubblicati</skos:prefLabel>
      <skos:definition xml:lang="it">Dati preesistenti che sono stati resi disponibili al pubblico (anche solo in parte).</skos:definition>
      <skos:prefLabel xml:lang="lt">Tyrimų duomenys: publikuoti</skos:prefLabel>
      <skos:definition xml:lang="lt">Egzistuojantys duomenys arba jų dalys, kurie yra viešai prieinami plačiajai visuomenei.</skos:definition>
      <skos:prefLabel xml:lang="nl">Onderzoeksdata: Gepubliceerd</skos:prefLabel>
      <skos:definition xml:lang="nl"/>
      <skos:prefLabel xml:lang="no">Forskningsdata: Publisert</skos:prefLabel>
      <skos:definition xml:lang="no">Eksisterende data som er tilgjengeliggjort for offentligheten, eller deler av den.</skos:definition>
      <skos:prefLabel xml:lang="pt">Dados de investigação: Publicados</skos:prefLabel>
      <skos:definition xml:lang="pt">Dados preexistentes que foram disponibilizados ao público em geral, ou a determinados segmentos.</skos:definition>
      <skos:prefLabel xml:lang="sl">Raziskovalni podatki: objavljeni</skos:prefLabel>
      <skos:definition xml:lang="sl">Že obstoječi podatki, ki so že bili na voljo širši javnosti oziroma delu javnosti.</skos:definition>
      <skos:prefLabel xml:lang="sr">Istraživački podaci: Objavljeni</skos:prefLabel>
      <skos:definition xml:lang="sr">Postojeći podaci koji su dostupni javnosti u celini ili u delovima.</skos:definition>
      <skos:prefLabel xml:lang="sv">Forskningsdata: Publicerade</skos:prefLabel>
      <skos:definition xml:lang="sv">Redan existerande data som har gjorts tillgängliga för allmänheten eller delar av den.</skos:definition>
      <skos:broader rdf:resource="http://rdf-vocabulary.ddialliance.org/cv/DataSourceType/1.0/d53e1305"/>
   </rdf:Description>
   <rdf:Description rdf:about="http://rdf-vocabulary.ddialliance.org/cv/DataSourceType/1.0/d53e1466">
      <rdf:type rdf:resource="http://www.w3.org/2004/02/skos/core#Concept"/>
      <skos:inScheme rdf:resource="http://rdf-vocabulary.ddialliance.org/cv/DataSourceType/1.0/"/>
      <skos:notation>ResearchData.Unpublished</skos:notation>
      <skos:prefLabel xml:lang="en">Research data: Unpublished</skos:prefLabel>
      <skos:definition xml:lang="en">Pre-existing data that have not been made available to the general public, or sections thereof.</skos:definition>
      <skos:prefLabel xml:lang="da">Forskningsdata: Upubliceret</skos:prefLabel>
      <skos:definition xml:lang="da">Allerede-eksisterende data, der ikke er gjort tilgængelige for den generelle offentlighed, eller dele heraf.</skos:definition>
      <skos:prefLabel xml:lang="fi">Tutkimusaineisto: julkaisematon</skos:prefLabel>
      <skos:definition xml:lang="fi">Olemassa oleva aineisto, joka ei ole julkisesti saatavilla.</skos:definition>
      <skos:prefLabel xml:lang="it">Dati di ricerca: non pubblicati</skos:prefLabel>
      <skos:definition xml:lang="it">Dati preesistenti che non sono stati resi disponibili, interamente o in parte, al pubblico.</skos:definition>
      <skos:prefLabel xml:lang="lt">Tyrimų duomenys: nepublikuoti</skos:prefLabel>
      <skos:definition xml:lang="lt">Egzistuojantys duomenys arba jų dalys, kurie nėra viešai prieinami plačiajai visuomenei.</skos:definition>
      <skos:prefLabel xml:lang="nl">Onderzoeksdata: Ongepubliceerd</skos:prefLabel>
      <skos:definition xml:lang="nl"/>
      <skos:prefLabel xml:lang="no">Forskningsdata: Upublisert</skos:prefLabel>
      <skos:definition xml:lang="no">Eksisterende data som ikke er tilgjengeliggjort for offentligheten, eller deler av den.</skos:definition>
      <skos:prefLabel xml:lang="pt">Dados de investigação: Não publicados</skos:prefLabel>
      <skos:definition xml:lang="pt">Dados preexistentes que não foram disponibilizados ao público em geral, ou a determinados segmentos.</skos:definition>
      <skos:prefLabel xml:lang="sl">Raziskovalni podatki: neobjavljeni</skos:prefLabel>
      <skos:definition xml:lang="sl">Že obstoječi podatki, ki še niso bili na voljo širši javnosti oziroma delu javnosti.</skos:definition>
      <skos:prefLabel xml:lang="sr">Istraživački podaci: Neobjavljeni</skos:prefLabel>
      <skos:definition xml:lang="sr">Postojeći podaci koji nisu dostupni javnosti ni u celini, ni u delovima.</skos:definition>
      <skos:prefLabel xml:lang="sv">Forskningsdata: Opublicerade</skos:prefLabel>
      <skos:definition xml:lang="sv">Redan existerande data som inte har gjorts tillgängliga för allmänheten eller delar av den.</skos:definition>
      <skos:broader rdf:resource="http://rdf-vocabulary.ddialliance.org/cv/DataSourceType/1.0/d53e1305"/>
   </rdf:Description>
   <rdf:Description rdf:about="http://rdf-vocabulary.ddialliance.org/cv/DataSourceType/1.0/d53e1544">
      <rdf:type rdf:resource="http://www.w3.org/2004/02/skos/core#Concept"/>
      <skos:inScheme rdf:resource="http://rdf-vocabulary.ddialliance.org/cv/DataSourceType/1.0/"/>
      <skos:notation>PopulationGroup</skos:notation>
      <skos:prefLabel xml:lang="en">Population group</skos:prefLabel>
      <skos:definition xml:lang="en">Group of individuals that can be defined by one or several common characteristics: ethnicity, race, gender, age range, geographic location or distribution, level of education, income level or economic status, professional status, state of health or medical conditions, or belonging to specific communities (e.g., special interest groups, or social media), or networks, etc.</skos:definition>
      <skos:prefLabel xml:lang="da">Populationsgruppe</skos:prefLabel>
      <skos:definition xml:lang="da">Gruppe af individer, der kan defineres af en eller flere fælles karakteristika: etnicitet, race, køn, aldersspænd, geografisk placering eller fordeling, uddannelsesniveau, indkomstniveau eller økonomisk status, professionel status, helbredstilstand eller medicinske forhold, tilhørsforhold til specifikke fællesskaber (f.eks. særlige interessegrupper eller sociale medier), eller netværk, mm.</skos:definition>
      <skos:prefLabel xml:lang="fi">Väestöryhmä</skos:prefLabel>
      <skos:definition xml:lang="fi">Ryhmä henkilöitä, joka on rajattavissa yhden tai useamman yhteisen piirteen mukaan: etnisyys, rotu, sukupuoli, ikäryhmä, maantieteellinen sijainti, koulutustaso, tulotaso tai taloudellinen asema, ammatillinen asema, terveydentila, tiettyihin yhteisöihin tai verkostoihin kuuluminen (esim. eturyhmät, sosiaalisen median käyttäjät) jne.</skos:definition>
      <skos:prefLabel xml:lang="it">Gruppi di popolazione</skos:prefLabel>
      <skos:definition xml:lang="it">Gruppo di individui che possono essere definiti da una o più caratteristiche comuni: etnia, razza, genere, fascia d'età, localizzazione o distribuzione geografica, livello di istruzione, livello di reddito o status economico, status professionale, stato di salute o condizioni mediche, oppure che appartengono a comunità specifiche (ad esempio gruppi di interesse o gruppi sui social media) o a reti di persone, ecc.</skos:definition>
      <skos:prefLabel xml:lang="lt">Gyventojų grupė</skos:prefLabel>
      <skos:definition xml:lang="lt">Asmenų grupė, kurią galima apibūdinti pagal vieną ar keletą bendrų savybių: tautybę, rasę, lytį, amžių, geografinę vietą ar pasiskirstymą, išsilavinimo lygį, pajamų lygį ar ekonominį statusą, profesinį statusą, sveikatos būklę ar medicininę būklę arba pagal priklausymą konkrečioms bendruomenėms (pavyzdžiui, specifinių interesų grupėms ar socialinėms medijoms), tinklams ir kt.</skos:definition>
      <skos:prefLabel xml:lang="nl">Bevolkingsgroep</skos:prefLabel>
      <skos:definition xml:lang="nl"/>
      <skos:prefLabel xml:lang="no">Populasjonsgruppe</skos:prefLabel>
      <skos:definition xml:lang="no">Gruppe av individer som kan bli definert av en eller flere sammenfallende egenskaper: etnisitet, rase, kjønn, aldersgruppe, geografisk lokasjon eller distribusjon, utdanningsnivå, inntektsnivå eller økonomisk status, yrkesstatus, helsetilstand eller medisinsk tilstand, eller tilhørighet til spesifikke grupper (f.eks.: spesielle interessegrupper eller sosiale medier), eller nettverk etc.</skos:definition>
      <skos:prefLabel xml:lang="pt">Grupos populacionais</skos:prefLabel>
      <skos:definition xml:lang="pt">Grupo de indivíduos que pode ser definido por uma ou várias características comuns: etnia, 'raça', género, faixa etária, localização ou distribuição geográfica, nível de escolaridade, nível de rendimento ou condição económica, estatuto profissional, estado de saúde ou condições médicas, ou a pertença a comunidades específicas (por exemplo, grupos de interesse especiais ou media sociais), ou redes, etc.</skos:definition>
      <skos:prefLabel xml:lang="sl">Populacijska skupina</skos:prefLabel>
      <skos:definition xml:lang="sl">Skupina posameznikov, ki jo je mogoče opredeliti z eno ali več skupnimi značilnostmi: etnična pripadnost, rasa, spol, starostni razred, geografska lokacija ali razdelitev, stopnja izobrazbe, raven dohodka ali ekonomski status, poklicni status, zdravstveno stanje ali zdravstvene težave, pripadnost posebnim skupnostim (npr. posebne interesne skupine ali družbena omrežja) ali mreže itd.</skos:definition>
      <skos:prefLabel xml:lang="sr">Populacija</skos:prefLabel>
      <skos:definition xml:lang="sr">Grupa pojedinaca koja se može definisati po jednoj ili više zajedničkih karakteristika: etnička pripadnost, rasa, pol, starosna dob, geografski položaj ili rasprostranjenost, nivo obrazovanja, nivo prihoda ili ekonomski status, profesionalni status, zdravstveno stanje ili pripadnost određenim zajednicama (npr. posebne interesne grupe ili društveni mediji) ili mreže, itd.</skos:definition>
      <skos:prefLabel xml:lang="sv">Befolkningsgrupp</skos:prefLabel>
      <skos:definition xml:lang="sv">Grupp av individer som kan definieras av en eller flera gemensamma egenskaper: t.ex. etnicitet, ras, kön, åldersintervall, geografisk plats eller distribution, utbildningsnivå, inkomstnivå eller ekonomisk status, yrkesstatus, hälsotillstånd eller medicinska tillstånd eller som tillhör en definierbar gemenskap (t.ex. speciella intressegrupper eller sociala medier) eller nätverk.</skos:definition>
   </rdf:Description>
   <rdf:Description rdf:about="http://rdf-vocabulary.ddialliance.org/cv/DataSourceType/1.0/d53e1622">
      <rdf:type rdf:resource="http://www.w3.org/2004/02/skos/core#Concept"/>
      <skos:inScheme rdf:resource="http://rdf-vocabulary.ddialliance.org/cv/DataSourceType/1.0/"/>
      <skos:notation>GeographicArea</skos:notation>
      <skos:prefLabel xml:lang="en">Geographic area</skos:prefLabel>
      <skos:definition xml:lang="en">An area of the Earth, demarcated for the purposes of administration, politics, environment, etc. The demarcation is identifiable via coordinates or other systems used to identify position precisely.</skos:definition>
      <skos:prefLabel xml:lang="da">Geografisk område</skos:prefLabel>
      <skos:definition xml:lang="da">Et område på jorden, afgrænset med henblik på administration, politik, miljø mm. Afgrænsningen kan identificeres ved hjælp af koordinater eller andre systemer, der anvendes til at identificere position præcist.</skos:definition>
      <skos:prefLabel xml:lang="fi">Maantieteellinen alue</skos:prefLabel>
      <skos:definition xml:lang="fi">Alue, joka on rajattu poliittisten, hallinnollisten, ympäristöllisten ym. syiden vuoksi. Rajat ovat määriteltävissä ja tunnistettavissa koordinaatein tai muita tarkkoja paikannusjärjestelmiä käyttäen.</skos:definition>
      <skos:prefLabel xml:lang="it">Area geografica</skos:prefLabel>
      <skos:definition xml:lang="it">Un'area territoriale delimitata per scopi amministrativi, politici, ambientali, ecc. La delimitazione è identificabile tramite coordinate o altri sistemi utilizzati per identificare con precisione la posizione.</skos:definition>
      <skos:prefLabel xml:lang="lt">Geografinė teritorija</skos:prefLabel>
      <skos:definition xml:lang="lt">Žemės teritorija apibrėžta administraciniais, politiniais, aplinkos tvarkymo ar kt. tikslais. Ribos identifikuojamos naudojant koordinačių ar kitas tikslios vietos nustatymo sistemas.</skos:definition>
      <skos:prefLabel xml:lang="nl">Geografisch gebied</skos:prefLabel>
      <skos:definition xml:lang="nl"/>
      <skos:prefLabel xml:lang="no">Geografisk område</skos:prefLabel>
      <skos:definition xml:lang="no">Et område på jordkloden, avgrenset for administrasjons-, politiske- og/eller miljøhensyn etc. Avgrensingen er identifiserbar via koordinater eller andre systemer for å presist identifisere posisjon.</skos:definition>
      <skos:prefLabel xml:lang="pt">Área geográfica</skos:prefLabel>
      <skos:definition xml:lang="pt">Uma área da Terra, demarcada para fins de administração, política, ambiente, etc. A demarcação é identificável por meio de coordenadas ou outros sistemas usados para identificar a posição com precisão.</skos:definition>
      <skos:prefLabel xml:lang="sl">Geografsko območje</skos:prefLabel>
      <skos:definition xml:lang="sl">Ozemlje na Zemlji, razmejeno za namene uprave, politike, okolja itd. Razmejitev je mogoče prepoznati po koordinatah ali drugih sistemih, ki natančno opredeljujejo položaj.</skos:definition>
      <skos:prefLabel xml:lang="sr">Geografska oblast</skos:prefLabel>
      <skos:definition xml:lang="sr">Područje planete Zemlje, razgraničeno za administratvine, polititičke potrebe, potrebe životne sredine, i sl. Razgraničenje je moguć́e prepoznati koordinatama ili drugim sistemima koji se nedvosmisleno identifikuju.</skos:definition>
      <skos:prefLabel xml:lang="sv">Geografiskt område</skos:prefLabel>
      <skos:definition xml:lang="sv">Ett område på jorden, avgränsat administrativt, politiskt, miljömässigt m.m. Avgränsningen är identifierbar via koordinater eller andra system som används för att precist identifiera positionen.</skos:definition>
   </rdf:Description>
   <rdf:Description rdf:about="http://rdf-vocabulary.ddialliance.org/cv/DataSourceType/1.0/d53e1700">
      <rdf:type rdf:resource="http://www.w3.org/2004/02/skos/core#Concept"/>
      <skos:inScheme rdf:resource="http://rdf-vocabulary.ddialliance.org/cv/DataSourceType/1.0/"/>
      <skos:notation>PhysicalObjects</skos:notation>
      <skos:prefLabel xml:lang="en">Physical objects</skos:prefLabel>
      <skos:definition xml:lang="en">Natural or man-made entities with spatial locations. For instance, works of art, constructions, rock samples, machines, etc. These are considered data sources if the data describe the physical characteristics of the given object rather than any information encoded in it.</skos:definition>
      <skos:prefLabel xml:lang="da">Fysiske objekter</skos:prefLabel>
      <skos:definition xml:lang="da">Naturlige eller menneskeskabte enheder med rumlige lokationer. For eksempel, kunstværker, konstruktioner, stenprøver, maskiner mm. Disse betragtes som datakilder, hvis dataene beskriver de fysiske karakteristika af det givne objekt frem for enhver information indkodet i det.</skos:definition>
      <skos:prefLabel xml:lang="fi">Fyysiset objektit</skos:prefLabel>
      <skos:definition xml:lang="fi">Luonnolliset tai ihmisen tekemät paikannettavissa olevat esineet, objektit ja kokonaisuudet. Esimerkiksi taideteokset, rakennelmat, kivinäytteet, koneet jne. Nämä ovat aineistolähteitä silloin, kun aineistossa kuvaillaan esineen/objektin fyysisiä ominaisuuksia eikä sen sisältämää muuta tietoa.</skos:definition>
      <skos:prefLabel xml:lang="it">Oggetti fisici</skos:prefLabel>
      <skos:definition xml:lang="it">Entità naturali o create dall'uomo con una posizione spaziale determinata. Per esempio, opere d'arte, costruzioni, campioni di roccia, macchine, ecc. Sono considerati come fonti di dati se i dati descrivono le caratteristiche fisiche dell'oggetto anziché riportare informazioni codificate in esso.</skos:definition>
      <skos:prefLabel xml:lang="lt">Fiziniai objektai</skos:prefLabel>
      <skos:definition xml:lang="lt">Natūralūs ar žmogaus sukurti objektai, turintys vietą erdvėje. Pavyzdžiui, meno kūriniai, statiniai, uolienų pavyzdžiai, mašinos ir kt. Šie objektai laikomi duomenų šaltiniais, jei duomenys apibūdina pačio objekto fizines savybes, o ne kokią nors jame užkoduotą informaciją.</skos:definition>
      <skos:prefLabel xml:lang="nl">Fysiek object</skos:prefLabel>
      <skos:definition xml:lang="nl"/>
      <skos:prefLabel xml:lang="no">Fysiske objekter</skos:prefLabel>
      <skos:definition xml:lang="no">Naturlige eller menneskeskapte enheter med romlige lokaliseringer. For eksempel kunstverk, konstruksjoner, steinprøver, maskiner etc. Disse er betraktet som datakilder dersom data beskriver den fysiske karakteristikken av det gitte objektet framfor hvilken informasjon kodet i den.</skos:definition>
      <skos:prefLabel xml:lang="pt">Objetos físicos</skos:prefLabel>
      <skos:definition xml:lang="pt">Entidades naturais ou artificiais com localizações espaciais. Por exemplo, obras de arte, construções, amostras de rochas, máquinas, etc. Estas serão consideradas fontes de dados se os dados descreverem as características físicas do objeto em questão e não qualquer outra informação codificada no mesmo.</skos:definition>
      <skos:prefLabel xml:lang="sl">Fizični predmeti</skos:prefLabel>
      <skos:definition xml:lang="sl">Naravni ali umetno ustvarjeni predmeti, ki se fizično nahajajo v prostoru. Na primer, umetniška dela, konstrukcije, vzorci kamnin, stroji itd. Za podatkovne vire se upoštevajo, če podatki opisujejo fizične značilnosti danega predmeta in ne drugih informacij, ki sestavljajo predmet.</skos:definition>
      <skos:prefLabel xml:lang="sr">Fizički objekat</skos:prefLabel>
      <skos:definition xml:lang="sr">Prirodni ili veštački objekti sa prostornim lokacijama. Na primer, umetnička dela, građevine, uzorci stena, mašine, i sl. Oni se smatraju izvorima podataka ukoliko podaci opisuju fizičke karakteristike datog objekta, ali ne i bilo koje informacije kodirane unutar njih.</skos:definition>
      <skos:prefLabel xml:lang="sv">Fysiska föremål</skos:prefLabel>
      <skos:definition xml:lang="sv">Naturliga eller konstgjorda saker med rumslig plats. Till exempel konstverk, byggnader, stenprover, maskiner osv. Dessa betraktas som datakällor om data beskriver de fysiska egenskaperna hos det angivna föremålet snarare än någon information som kodas i det.</skos:definition>
   </rdf:Description>
   <rdf:Description rdf:about="http://rdf-vocabulary.ddialliance.org/cv/DataSourceType/1.0/d53e1778">
      <rdf:type rdf:resource="http://www.w3.org/2004/02/skos/core#Concept"/>
      <skos:inScheme rdf:resource="http://rdf-vocabulary.ddialliance.org/cv/DataSourceType/1.0/"/>
      <skos:notation>BiologicalSamples</skos:notation>
      <skos:prefLabel xml:lang="en">Biological samples</skos:prefLabel>
      <skos:definition xml:lang="en">Biological materials collected from living organisms, including, for example, biological specimens of human or animal organs, cells or tissues such as hair, muscle or tumor tissue, bodily fluids such as blood, urine, saliva, extracted material such as DNA and RNA, microorganisms, plant matter, etc. The source of the data are the samples themselves, not measurements and/or other tests applied to them.</skos:definition>
      <skos:prefLabel xml:lang="da">Biologiske prøver</skos:prefLabel>
      <skos:definition xml:lang="da">Biologiske materialer indsamlet fra levende organismer, inkluderende, for eksempel, biologiske prøver af menneske- eller dyreorganer, celler eller væv såsom hår, muskel- eller tumorvæv, kropsvæsker såsom blod, urin, spyt, ekstraheret materiale såsom DNA og RNA, mikroorganismer, plantematerie, mm. Datakilden er prøverne i sig selv, ikke målinger og/eller andre test tillagt dem.</skos:definition>
      <skos:prefLabel xml:lang="fi">Biologiset näytteet</skos:prefLabel>
      <skos:definition xml:lang="fi">Elollisilta olennoilta kerätty biologinen materiaali, esimerkiksi ihmisten tai eläinten elin-, solu- tai kudosnäytteet, kuten karvat, lihas- tai kasvainkudos; eritteet, kuten veri, virtsa tai sylki; eristetty materiaali, kuten DNA ja RNA; mikro-organismit; kasviaines jne. Käytä, kun näytteet itsessään toimivat aineistolähteenä eivätkä niihin kohdistetut mittaukset ja/tai muut testit.</skos:definition>
      <skos:prefLabel xml:lang="it">Campioni biologici</skos:prefLabel>
      <skos:definition xml:lang="it">Materiali biologici raccolti da organismi viventi inclusi, ad esempio, campioni biologici di organi umani o animali, cellule o tessuti come capelli, tessuto muscolare o tumorale, fluidi corporei come sangue, urina, saliva, materiale estratto come DNA e RNA, microrganismi, materiale vegetale, ecc. La fonte dei dati sono i campioni stessi, non le misurazioni e/o altri test applicati ad essi.</skos:definition>
      <skos:prefLabel xml:lang="lt">Biologiniai mėginiai</skos:prefLabel>
      <skos:definition xml:lang="lt">Iš gyvų organizmų surinktos biologinės medžiagos įskaitant, pavyzdžiui, biologinius žmogaus ar gyvūnų organų, ląstelių ar audinių (pavyzdžiui, plaukų, raumenų ar navikų) mėginius, kūno skysčius (pavyzdžiui, kraujas, šlapimas, seilės), išgautas medžiagas (pavyzdžiui, DNR ir RNR); taip pat mikroorganizmus, augalines medžiagas ir kt. Duomenų šaltinis yra patys mėginiai, o ne ankstesni matavimai ir (arba) kiti jiems taikyti tyrimai.</skos:definition>
      <skos:prefLabel xml:lang="nl">Biologische monsters</skos:prefLabel>
      <skos:definition xml:lang="nl"/>
      <skos:prefLabel xml:lang="no">Biologiske prøver</skos:prefLabel>
      <skos:definition xml:lang="no">Biologisk materiale innsamlet fra levende organismer, inkludert for eksempel biologiske prøver av menneske- eller dyreorganer, celler eller vev slik som hår-, muskel- eller svulstvev, kroppsvæsker som blod, urin, spytt, utvunnet DNA og RNA, mikroorganismer, plantematerie etc. Datakilden er prøvene i seg selv, ikke målinger og/eller utførte tester på dem.</skos:definition>
      <skos:prefLabel xml:lang="pt">Amostras biológicas</skos:prefLabel>
      <skos:definition xml:lang="pt">Materiais biológicos recolhidos de organismos vivos, incluindo, por exemplo, espécimes biológicos de órgãos humanos ou animais, células ou tecidos como cabelo, músculo ou tecido tumoral, fluidos corporais como sangue, urina, saliva, material extraído como ADN e ARN, microorganismos, matéria vegetal, etc. A fonte dos dados são as próprias amostras, não as medições e/ou outros testes nelas realizados.</skos:definition>
      <skos:prefLabel xml:lang="sl">Biološki vzorci</skos:prefLabel>
      <skos:definition xml:lang="sl">Biološka gradiva, zbrana iz živih organizmov, vključno z biološkimi vzorci človeških ali živalskih organov, celic ali tkiv, kot so lasje, mišice ali tumorsko tkivo, telesne tekočine, kot so kri, urin, slina, iz živih bitij pridobljena gradiva, kot sta DNA in RNA, mikroorganizmi, rastlinski deli itd. Vir podatkov so vzorci sami, ne meritve in/ali drugi preizkusi, v katerih so ti vzorci uporabljeni.</skos:definition>
      <skos:prefLabel xml:lang="sr">Biološki uzorak</skos:prefLabel>
      <skos:definition xml:lang="sr">Biološki materijali prikupljeni od živih organizama, uključujući, na primer, biološke primerke ljudskih ili životinjskih organa, ćelija ili tkiva poput dlake, mišićnog ili tumorskog tkiva, telesnih tečnosti kao što su krv, urin, slina, ekstrahovani materijal kao što su DNK i RNA, mikroorganizmi, biljna materija, itd. Izvor podataka su sami uzorci, a ne merenja i/ili drugi testovi koji su na njih primenjeni.</skos:definition>
      <skos:prefLabel xml:lang="sv">Biologiska prover</skos:prefLabel>
      <skos:definition xml:lang="sv">Biologiska material som samlats in från levande organismer, till exempel biologiska prover av mänskliga eller animaliska organ, celler eller vävnader (som t.ex. hår, muskel- eller tumörvävnad), kroppsvätskor (som t.ex. blod, urin, saliv), extraherat material (som t.ex. DNA och RNA), mikroorganismer, växtämnen osv. Datakällan är själva proverna, inte mätningar och/eller andra tester som utförts på dem.</skos:definition>
   </rdf:Description>
   <rdf:Description rdf:about="http://rdf-vocabulary.ddialliance.org/cv/DataSourceType/1.0/d53e1857">
      <rdf:type rdf:resource="http://www.w3.org/2004/02/skos/core#Concept"/>
      <skos:inScheme rdf:resource="http://rdf-vocabulary.ddialliance.org/cv/DataSourceType/1.0/"/>
      <skos:notation>Other</skos:notation>
      <skos:prefLabel xml:lang="en">Other</skos:prefLabel>
      <skos:definition xml:lang="en">Use when the data source is known, but not found in the list.</skos:definition>
      <skos:prefLabel xml:lang="da">Andet</skos:prefLabel>
      <skos:definition xml:lang="da">Anvend, når datakilden er kendt, men ikke findes i listen.</skos:definition>
      <skos:prefLabel xml:lang="fi">Muu alkuperä</skos:prefLabel>
      <skos:definition xml:lang="fi">Käytä mikäli aineiston alkuperä on tiedossa, mutta ei listassa.</skos:definition>
      <skos:prefLabel xml:lang="it">Altro</skos:prefLabel>
      <skos:definition xml:lang="it">Utilizzare quando l'origine dei dati è conosciuta, ma non è presente nell'elenco.</skos:definition>
      <skos:prefLabel xml:lang="lt">Kita</skos:prefLabel>
      <skos:definition xml:lang="lt">Naudoti, jei duomenų šaltinis yra žinomas, bet jo nėra sąraše.</skos:definition>
      <skos:prefLabel xml:lang="nl">Anders</skos:prefLabel>
      <skos:definition xml:lang="nl"/>
      <skos:prefLabel xml:lang="no">Annet</skos:prefLabel>
      <skos:definition xml:lang="no">Bruk når datakilden er kjent, men ikke funnet i listen.</skos:definition>
      <skos:prefLabel xml:lang="pt">Outro</skos:prefLabel>
      <skos:definition xml:lang="pt">Usar se a fonte de dados for conhecida, mas não se encontrar na lista.</skos:definition>
      <skos:prefLabel xml:lang="sl">Drugo</skos:prefLabel>
      <skos:definition xml:lang="sl">Uporabite, če je vir podatkov znan, a ga ne najdete na seznamu.</skos:definition>
      <skos:prefLabel xml:lang="sr">Ostalo</skos:prefLabel>
      <skos:definition xml:lang="sr">Koristite ako je izvor podataka poznat, ali nije na listi.</skos:definition>
      <skos:prefLabel xml:lang="sv">Övrigt</skos:prefLabel>
      <skos:definition xml:lang="sv">Används när datakällan är känd men saknas i listan.</skos:definition>
   </rdf:Description>
</rdf:RDF>
