<?xml version="1.0" encoding="UTF-8"?>
<rdf:RDF xmlns:rdf="http://www.w3.org/1999/02/22-rdf-syntax-ns#"
         xmlns:skos="http://www.w3.org/2004/02/skos/core#"
         xmlns:owl="http://www.w3.org/2002/07/owl#"
         xmlns:dcterms="http://purl.org/dc/terms/"
>
   <rdf:Description rdf:about="http://rdf-vocabulary.ddialliance.org/cv/LanguageProficiency/1.0.0/">
      <rdf:type rdf:resource="http://www.w3.org/2004/02/skos/core#ConceptScheme"/>
      <dcterms:isVersionOf rdf:resource="http://rdf-vocabulary.ddialliance.org/cv/LanguageProficiency/"/>
      <skos:notation xml:lang="en">LanguageProficiency</skos:notation>
      <dcterms:title xml:lang="en">Language Proficiency</dcterms:title>
      <dcterms:description xml:lang="en">Describes the level of proficiency of an individual in a natural language.</dcterms:description>
      <skos:prefLabel xml:lang="en">Language Proficiency</skos:prefLabel>
      <dcterms:title xml:lang="no">Spr&#xe5;kferdigheter</dcterms:title>
      <dcterms:description xml:lang="no">Beskriver ferdighetene et individ har i et naturlig spr&#xe5;k.</dcterms:description>
      <skos:prefLabel xml:lang="no">Spr&#xe5;kferdigheter</skos:prefLabel>
      <owl:versionInfo>1.0.0</owl:versionInfo>
      <dcterms:license rdf:resource="http://creativecommons.org/licenses/by/4.0/"/>
      <dcterms:rights>Copyright &#xa9;DDI Alliance 2020</dcterms:rights>
      <skos:hasTopConcept rdf:resource="http://rdf-vocabulary.ddialliance.org/cv/LanguageProficiency/1.0.0/925641e"/>
      <skos:hasTopConcept rdf:resource="http://rdf-vocabulary.ddialliance.org/cv/LanguageProficiency/1.0.0/223dee0"/>
      <skos:hasTopConcept rdf:resource="http://rdf-vocabulary.ddialliance.org/cv/LanguageProficiency/1.0.0/6279308"/>
      <skos:hasTopConcept rdf:resource="http://rdf-vocabulary.ddialliance.org/cv/LanguageProficiency/1.0.0/6311ae1"/>
   </rdf:Description>
   <rdf:Description rdf:about="http://rdf-vocabulary.ddialliance.org/cv/LanguageProficiency/1.0.0/925641e">
      <rdf:type rdf:resource="http://www.w3.org/2004/02/skos/core#Concept"/>
      <skos:inScheme rdf:resource="http://rdf-vocabulary.ddialliance.org/cv/LanguageProficiency/1.0.0/"/>
      <skos:notation xml:lang="en">Native</skos:notation>
      <skos:prefLabel xml:lang="en">Native</skos:prefLabel>
      <skos:definition xml:lang="en">The individual is a native user of the language whose level of proficiency is unknown/unspecified.</skos:definition>
      <skos:prefLabel xml:lang="no">Morsm&#xe5;l</skos:prefLabel>
      <skos:definition xml:lang="no">Individet har spr&#xe5;ket som morsm&#xe5;l, men ferdighetene i spr&#xe5;ken er ukjent eller uspesifisert.</skos:definition>
      <skos:narrower rdf:resource="http://rdf-vocabulary.ddialliance.org/cv/LanguageProficiency/1.0.0/28b7b7d"/>
      <skos:narrower rdf:resource="http://rdf-vocabulary.ddialliance.org/cv/LanguageProficiency/1.0.0/823f0d0"/>
      <skos:narrower rdf:resource="http://rdf-vocabulary.ddialliance.org/cv/LanguageProficiency/1.0.0/4d30d3a"/>
   </rdf:Description>
   <rdf:Description rdf:about="http://rdf-vocabulary.ddialliance.org/cv/LanguageProficiency/1.0.0/28b7b7d">
      <rdf:type rdf:resource="http://www.w3.org/2004/02/skos/core#Concept"/>
      <skos:inScheme rdf:resource="http://rdf-vocabulary.ddialliance.org/cv/LanguageProficiency/1.0.0/"/>
      <skos:notation xml:lang="en">Native.Fluent</skos:notation>
      <skos:prefLabel xml:lang="en">Native: Fluent</skos:prefLabel>
      <skos:definition xml:lang="en">The individual is a native user with excellent mastery of the language, including breadth of vocabulary and idiom, and confident command of the grammar.</skos:definition>
      <skos:prefLabel xml:lang="no">Morsm&#xe5;l: Flytende</skos:prefLabel>
      <skos:definition xml:lang="no">Individet har spr&#xe5;ket som morsm&#xe5;l og har en utmerket mestring av det, inkludert inng&#xe5;ende kjennskap til uttrykk, et bredt ordforr&#xe5;d og trygg kontroll over grammatikken.</skos:definition>
   </rdf:Description>
   <rdf:Description rdf:about="http://rdf-vocabulary.ddialliance.org/cv/LanguageProficiency/1.0.0/823f0d0">
      <rdf:type rdf:resource="http://www.w3.org/2004/02/skos/core#Concept"/>
      <skos:inScheme rdf:resource="http://rdf-vocabulary.ddialliance.org/cv/LanguageProficiency/1.0.0/"/>
      <skos:notation xml:lang="en">Native.Good</skos:notation>
      <skos:prefLabel xml:lang="en">Native: Good</skos:prefLabel>
      <skos:definition xml:lang="en">The individual is a native user of the language with good structural accuracy, vocabulary and comprehension.</skos:definition>
      <skos:prefLabel xml:lang="no">Morsm&#xe5;l: Bra</skos:prefLabel>
      <skos:definition xml:lang="no">Individet har spr&#xe5;ket som morsm&#xe5;l og behersker det med god strukturell n&#xf8;yaktighet, godt ordforr&#xe5;d og forst&#xe5;else.</skos:definition>
   </rdf:Description>
   <rdf:Description rdf:about="http://rdf-vocabulary.ddialliance.org/cv/LanguageProficiency/1.0.0/4d30d3a">
      <rdf:type rdf:resource="http://www.w3.org/2004/02/skos/core#Concept"/>
      <skos:inScheme rdf:resource="http://rdf-vocabulary.ddialliance.org/cv/LanguageProficiency/1.0.0/"/>
      <skos:notation xml:lang="en">Native.Basic</skos:notation>
      <skos:prefLabel xml:lang="en">Native: Basic</skos:prefLabel>
      <skos:definition xml:lang="en">The individual is a native user of the language with limited vocabulary, use of grammar and comprehension.</skos:definition>
      <skos:prefLabel xml:lang="no">Morsm&#xe5;l: Grunnleggende</skos:prefLabel>
      <skos:definition xml:lang="no">Individet har spr&#xe5;ket som morsm&#xe5;l, men er begrenset i ordforr&#xe5;det, grammatikk og forst&#xe5;else.</skos:definition>
   </rdf:Description>
   <rdf:Description rdf:about="http://rdf-vocabulary.ddialliance.org/cv/LanguageProficiency/1.0.0/223dee0">
      <rdf:type rdf:resource="http://www.w3.org/2004/02/skos/core#Concept"/>
      <skos:inScheme rdf:resource="http://rdf-vocabulary.ddialliance.org/cv/LanguageProficiency/1.0.0/"/>
      <skos:notation xml:lang="en">NonNative</skos:notation>
      <skos:prefLabel xml:lang="en">Non-native</skos:prefLabel>
      <skos:definition xml:lang="en">The individual is a non-native user of the language whose level of proficiency is unknown/unspecified.</skos:definition>
      <skos:prefLabel xml:lang="no">Andrespr&#xe5;k</skos:prefLabel>
      <skos:definition xml:lang="no">Individet har spr&#xe5;ket som andrespr&#xe5;k, men ferdighetene i spr&#xe5;ket er ukjent eller uspesifisert.</skos:definition>
      <skos:narrower rdf:resource="http://rdf-vocabulary.ddialliance.org/cv/LanguageProficiency/1.0.0/bdbc6ed"/>
      <skos:narrower rdf:resource="http://rdf-vocabulary.ddialliance.org/cv/LanguageProficiency/1.0.0/cf189a2"/>
      <skos:narrower rdf:resource="http://rdf-vocabulary.ddialliance.org/cv/LanguageProficiency/1.0.0/19770b6"/>
   </rdf:Description>
   <rdf:Description rdf:about="http://rdf-vocabulary.ddialliance.org/cv/LanguageProficiency/1.0.0/bdbc6ed">
      <rdf:type rdf:resource="http://www.w3.org/2004/02/skos/core#Concept"/>
      <skos:inScheme rdf:resource="http://rdf-vocabulary.ddialliance.org/cv/LanguageProficiency/1.0.0/"/>
      <skos:notation xml:lang="en">NonNative.Fluent</skos:notation>
      <skos:prefLabel xml:lang="en">Non-native: Fluent</skos:prefLabel>
      <skos:definition xml:lang="en">The individual is a non-native user with excellent mastery of the language, including breadth of vocabulary and idiom, and confident command of the grammar.</skos:definition>
      <skos:prefLabel xml:lang="no">Andre spr&#xe5;k: Flytende</skos:prefLabel>
      <skos:definition xml:lang="no">Individet har spr&#xe5;ket som andrespr&#xe5;k og har en utmerket mestring av det, inkludert inng&#xe5;ende kjennskap til uttrykk, et bredt ordforr&#xe5;d og trygg kontroll over grammatikken.</skos:definition>
   </rdf:Description>
   <rdf:Description rdf:about="http://rdf-vocabulary.ddialliance.org/cv/LanguageProficiency/1.0.0/cf189a2">
      <rdf:type rdf:resource="http://www.w3.org/2004/02/skos/core#Concept"/>
      <skos:inScheme rdf:resource="http://rdf-vocabulary.ddialliance.org/cv/LanguageProficiency/1.0.0/"/>
      <skos:notation xml:lang="en">NonNative.Good</skos:notation>
      <skos:prefLabel xml:lang="en">Non-native: Good</skos:prefLabel>
      <skos:definition xml:lang="en">The individual is a non-native user of the language with good structural accuracy, vocabulary and comprehension.</skos:definition>
      <skos:prefLabel xml:lang="no">Andrespr&#xe5;k: Bra</skos:prefLabel>
      <skos:definition xml:lang="no">Individet har spr&#xe5;ket som andrespr&#xe5;k og behersker det med god strukturell n&#xf8;yaktighet, godt ordforr&#xe5;d og forst&#xe5;else.</skos:definition>
   </rdf:Description>
   <rdf:Description rdf:about="http://rdf-vocabulary.ddialliance.org/cv/LanguageProficiency/1.0.0/19770b6">
      <rdf:type rdf:resource="http://www.w3.org/2004/02/skos/core#Concept"/>
      <skos:inScheme rdf:resource="http://rdf-vocabulary.ddialliance.org/cv/LanguageProficiency/1.0.0/"/>
      <skos:notation xml:lang="en">NonNative.Basic</skos:notation>
      <skos:prefLabel xml:lang="en">Non-native: Basic</skos:prefLabel>
      <skos:definition xml:lang="en">The individual is a non-native user of the language with limited vocabulary, use of grammar and comprehension.</skos:definition>
      <skos:prefLabel xml:lang="no">Andrespr&#xe5;k: Grunnleggende</skos:prefLabel>
      <skos:definition xml:lang="no">Individet har spr&#xe5;ket som andrespr&#xe5;k, men er begrenset i ordforr&#xe5;det, grammatikk og forst&#xe5;else.</skos:definition>
   </rdf:Description>
   <rdf:Description rdf:about="http://rdf-vocabulary.ddialliance.org/cv/LanguageProficiency/1.0.0/6279308">
      <rdf:type rdf:resource="http://www.w3.org/2004/02/skos/core#Concept"/>
      <skos:inScheme rdf:resource="http://rdf-vocabulary.ddialliance.org/cv/LanguageProficiency/1.0.0/"/>
      <skos:notation xml:lang="en">NativeStatusUnspecified</skos:notation>
      <skos:prefLabel xml:lang="en">Unspecified native status</skos:prefLabel>
      <skos:definition xml:lang="en">The individual&apos;s native status and her/his level of proficiency are both unknown, or not specified.</skos:definition>
      <skos:prefLabel xml:lang="no">Uspesifisert spr&#xe5;ktilh&#xf8;righet</skos:prefLabel>
      <skos:definition xml:lang="no">Individets spr&#xe5;ktilh&#xf8;righet og hen sine ferdigheter er begge ukjent, eller ikke spesifisert.</skos:definition>
      <skos:narrower rdf:resource="http://rdf-vocabulary.ddialliance.org/cv/LanguageProficiency/1.0.0/6b5f366"/>
      <skos:narrower rdf:resource="http://rdf-vocabulary.ddialliance.org/cv/LanguageProficiency/1.0.0/022e3d5"/>
      <skos:narrower rdf:resource="http://rdf-vocabulary.ddialliance.org/cv/LanguageProficiency/1.0.0/5c65d4e"/>
   </rdf:Description>
   <rdf:Description rdf:about="http://rdf-vocabulary.ddialliance.org/cv/LanguageProficiency/1.0.0/6b5f366">
      <rdf:type rdf:resource="http://www.w3.org/2004/02/skos/core#Concept"/>
      <skos:inScheme rdf:resource="http://rdf-vocabulary.ddialliance.org/cv/LanguageProficiency/1.0.0/"/>
      <skos:notation xml:lang="en">NativeStatusUnspecified.Fluent</skos:notation>
      <skos:prefLabel xml:lang="en">Unspecified native status: Fluent</skos:prefLabel>
      <skos:definition xml:lang="en">The individual&apos;s native status is unknown/unspecified; s/he has excellent mastery of the language, including breadth of vocabulary and idiom, and confident command of the grammar.</skos:definition>
      <skos:prefLabel xml:lang="no">Uspesifisert spr&#xe5;ktilh&#xf8;righet: Flytende</skos:prefLabel>
      <skos:definition xml:lang="no">Individets spr&#xe5;ktilh&#xf8;righet er ukjent/uspesifisert; hen har utmerket mestring av spr&#xe5;ket, inkludert inng&#xe5;ende kjennskap til uttrykk, et bredt ordforr&#xe5;d og trygg kontroll over grammatikken.</skos:definition>
   </rdf:Description>
   <rdf:Description rdf:about="http://rdf-vocabulary.ddialliance.org/cv/LanguageProficiency/1.0.0/022e3d5">
      <rdf:type rdf:resource="http://www.w3.org/2004/02/skos/core#Concept"/>
      <skos:inScheme rdf:resource="http://rdf-vocabulary.ddialliance.org/cv/LanguageProficiency/1.0.0/"/>
      <skos:notation xml:lang="en">NativeStatusUnspecified.Good</skos:notation>
      <skos:prefLabel xml:lang="en">Unspecified native status: Good</skos:prefLabel>
      <skos:definition xml:lang="en">The individual&apos;s native status is unknown/unspecified; s/he has good structural accuracy, vocabulary and comprehension.</skos:definition>
      <skos:prefLabel xml:lang="no">Uspesifisert spr&#xe5;ktilh&#xf8;righet: Bra</skos:prefLabel>
      <skos:definition xml:lang="no">Individets spr&#xe5;ktilh&#xf8;righet er ukjent/uspesifisert; hen har god strukturell n&#xf8;yaktighet, godt ordforr&#xe5;d og forst&#xe5;else.</skos:definition>
   </rdf:Description>
   <rdf:Description rdf:about="http://rdf-vocabulary.ddialliance.org/cv/LanguageProficiency/1.0.0/5c65d4e">
      <rdf:type rdf:resource="http://www.w3.org/2004/02/skos/core#Concept"/>
      <skos:inScheme rdf:resource="http://rdf-vocabulary.ddialliance.org/cv/LanguageProficiency/1.0.0/"/>
      <skos:notation xml:lang="en">NativeStatusUnspecified.Basic</skos:notation>
      <skos:prefLabel xml:lang="en">Unspecified native status: Basic</skos:prefLabel>
      <skos:definition xml:lang="en">The individual&apos;s native status is unknown/unspecified; s/he has limited vocabulary, use of grammar, and comprehension.</skos:definition>
      <skos:prefLabel xml:lang="no">Uspesifisert spr&#xe5;ktilh&#xf8;righet: Grunnleggende</skos:prefLabel>
      <skos:definition xml:lang="no">Individets spr&#xe5;ktilh&#xf8;righet er ukjent/uspesifisert; hen har begrensninger i ordforr&#xe5;d, grammatikk og forst&#xe5;else.</skos:definition>
   </rdf:Description>
   <rdf:Description rdf:about="http://rdf-vocabulary.ddialliance.org/cv/LanguageProficiency/1.0.0/6311ae1">
      <rdf:type rdf:resource="http://www.w3.org/2004/02/skos/core#Concept"/>
      <skos:inScheme rdf:resource="http://rdf-vocabulary.ddialliance.org/cv/LanguageProficiency/1.0.0/"/>
      <skos:notation xml:lang="en">Other</skos:notation>
      <skos:prefLabel xml:lang="en">Other</skos:prefLabel>
      <skos:definition xml:lang="en">Use if level of proficiency is known, but not found in the list. It is recommended that any new entry combine information about the individual&apos;s native/non-native status and his/her level of proficiency, following the format [native status].[proficiency level] as shown in the entries above.</skos:definition>
      <skos:prefLabel xml:lang="no">Annet</skos:prefLabel>
      <skos:definition xml:lang="no">Bruk hvis spr&#xe5;kferdigheter er kjent, men ikke er &#xe5; finne p&#xe5; listen. Det er anbefalt at enhver ny oppf&#xf8;ring kombinerer informasjon om individets morsm&#xe5;l/andrespr&#xe5;k status og hen sitt ferdighetsniv&#xe5; i formatet [morsm&#xe5;l/andrespr&#xe5;k/annet]. [ferdighetsniv&#xe5;] som vist ovenfor.</skos:definition>
   </rdf:Description>
</rdf:RDF>
