<?xml version="1.0" encoding="UTF-8"?>
<rdf:RDF xmlns:rdf="http://www.w3.org/1999/02/22-rdf-syntax-ns#"
         xmlns:skos="http://www.w3.org/2004/02/skos/core#"
         xmlns:owl="http://www.w3.org/2002/07/owl#"
         xmlns:dcterms="http://purl.org/dc/terms/"
>
   <rdf:Description rdf:about="http://rdf-vocabulary.ddialliance.org/cv/SamplingProcedure/2.0.1/">
      <rdf:type rdf:resource="http://www.w3.org/2004/02/skos/core#ConceptScheme"/>
      <dcterms:isVersionOf rdf:resource="http://rdf-vocabulary.ddialliance.org/cv/SamplingProcedure/"/>
      <skos:notation xml:lang="en">SamplingProcedure</skos:notation>
      <dcterms:title xml:lang="sl">Postopek vzor&#x10d;enja</dcterms:title>
      <dcterms:description xml:lang="sl">Vklju&#x10d;uje razvrstitev metod vzor&#x10d;enja.</dcterms:description>
      <skos:prefLabel xml:lang="sl">Postopek vzor&#x10d;enja</skos:prefLabel>
      <dcterms:title xml:lang="lt">Atrankos proced&#x16b;ra</dcterms:title>
      <dcterms:description xml:lang="lt">Atrankos metod&#x173; tipologija.</dcterms:description>
      <skos:prefLabel xml:lang="lt">Atrankos proced&#x16b;ra</skos:prefLabel>
      <dcterms:title xml:lang="sv">Urvalsmetod</dcterms:title>
      <dcterms:description xml:lang="sv">Inneh&#xe5;ller en typologi av olika urvalsmetoder.</dcterms:description>
      <skos:prefLabel xml:lang="sv">Urvalsmetod</skos:prefLabel>
      <dcterms:title xml:lang="it">Procedura di campionamento</dcterms:title>
      <dcterms:description xml:lang="it">Tipologia dei metodi di campionamento.</dcterms:description>
      <skos:prefLabel xml:lang="it">Procedura di campionamento</skos:prefLabel>
      <dcterms:title xml:lang="en">Sampling Procedure</dcterms:title>
      <dcterms:description xml:lang="en">A typology of sampling methods.</dcterms:description>
      <skos:prefLabel xml:lang="en">Sampling Procedure</skos:prefLabel>
      <dcterms:title xml:lang="de">Auswahlverfahren</dcterms:title>
      <dcterms:description xml:lang="de">Enth&#xe4;lt eine Typologie von Stichprobenverfahren.</dcterms:description>
      <skos:prefLabel xml:lang="de">Auswahlverfahren</skos:prefLabel>
      <dcterms:title xml:lang="fr">Proc&#xe9;dure d&apos;&#xe9;chantillonnage</dcterms:title>
      <dcterms:description xml:lang="fr">Une typologie des m&#xe9;thodes d&apos;&#xe9;chantillonnage</dcterms:description>
      <skos:prefLabel xml:lang="fr">Proc&#xe9;dure d&apos;&#xe9;chantillonnage</skos:prefLabel>
      <dcterms:title xml:lang="nl">Steekproefmethode</dcterms:title>
      <dcterms:description xml:lang="nl">Een indeling van steekproefmethodes.</dcterms:description>
      <skos:prefLabel xml:lang="nl">Steekproefmethode</skos:prefLabel>
      <dcterms:title xml:lang="no">Utvalgsmetode</dcterms:title>
      <dcterms:description xml:lang="no">Inneholder en typologi av ulike utvalgsmetoder.</dcterms:description>
      <skos:prefLabel xml:lang="no">Utvalgsmetode</skos:prefLabel>
      <owl:versionInfo>2.0.1</owl:versionInfo>
      <dcterms:license rdf:resource="http://creativecommons.org/licenses/by/4.0/"/>
      <dcterms:rights>Copyright &#xa9;DDI Alliance 2025</dcterms:rights>
      <skos:hasTopConcept rdf:resource="http://rdf-vocabulary.ddialliance.org/cv/SamplingProcedure/2.0.1/885b553"/>
      <skos:hasTopConcept rdf:resource="http://rdf-vocabulary.ddialliance.org/cv/SamplingProcedure/2.0.1/0d2765b"/>
      <skos:hasTopConcept rdf:resource="http://rdf-vocabulary.ddialliance.org/cv/SamplingProcedure/2.0.1/540b3b2"/>
      <skos:hasTopConcept rdf:resource="http://rdf-vocabulary.ddialliance.org/cv/SamplingProcedure/2.0.1/4d8364f"/>
      <skos:hasTopConcept rdf:resource="http://rdf-vocabulary.ddialliance.org/cv/SamplingProcedure/2.0.1/e890a15"/>
      <skos:hasTopConcept rdf:resource="http://rdf-vocabulary.ddialliance.org/cv/SamplingProcedure/2.0.1/6311ae1"/>
   </rdf:Description>
   <rdf:Description rdf:about="http://rdf-vocabulary.ddialliance.org/cv/SamplingProcedure/2.0.1/885b553">
      <rdf:type rdf:resource="http://www.w3.org/2004/02/skos/core#Concept"/>
      <skos:inScheme rdf:resource="http://rdf-vocabulary.ddialliance.org/cv/SamplingProcedure/2.0.1/"/>
      <skos:notation xml:lang="en">TotalUniverseCompleteEnumeration</skos:notation>
      <skos:prefLabel xml:lang="sl">Zajeta celotna populacija</skos:prefLabel>
      <skos:definition xml:lang="sl">Vse enote (posamezniki, gospodinjstva, organizacije itd.) ciljne populacije so vklju&#x10d;ene v zbiranje podatkov. Na primer, &#x10d;e je ciljna populacija opredeljena kot &#x10d;lani sindikata, so vsi &#x10d;lani sindikata vabljeni k sodelovanju v raziskavi. Imenujemo tudi &quot;popis&quot;, &#x10d;e je vklju&#x10d;eno celotno prebivalstvo dolo&#x10d;ene regionalne enote (npr. dr&#x17e;ave).</skos:definition>
      <skos:prefLabel xml:lang="lt">Tiriamoji visuma arba visas s&#x105;ra&#x161;as</skos:prefLabel>
      <skos:definition xml:lang="lt">Renkant duomenis &#x12f;traukiami visi tikslin&#x117;s populiacijos vienetai (individai, nam&#x173; &#x16b;kiai, organizacijos ir kt.). Pavyzd&#x17e;iui, jei tikslin&#x117; populiacija yra apibr&#x117;&#x17e;ta, kaip profesin&#x117;s s&#x105;jungos nariai, visi profs&#x105;jungos nariai yra kvie&#x10d;iami dalyvauti tyrime. Taip pat vadinamas &#x201e;visuotiniu sura&#x161;ymu&#x201c;, jei pasirenkami visi teritorinio vieneto (pavyzd&#x17e;iui, &#x161;alies) gyventojai.</skos:definition>
      <skos:prefLabel xml:lang="sv">Hela populationen/total r&#xe4;kning</skos:prefLabel>
      <skos:definition xml:lang="sv">Alla element (individer, hush&#xe5;ll, organisationer m.m.) i m&#xe5;lpopulationen inkluderas i datainsamlingen. Exempel: om m&#xe5;lpopulationen definieras som medlemmarna i ett fackf&#xf6;rbund s&#xe5; bjuds samtliga medlemmar in till att delta i studien. Kallas &#xe4;ven &quot;folkr&#xe4;kning&quot;, om det r&#xf6;r sig om den totala populationen i en regional enhet (t.ex. ett land).</skos:definition>
      <skos:prefLabel xml:lang="it">Intero universo</skos:prefLabel>
      <skos:definition xml:lang="it">Tutte le unit&#xe0; (individui, famiglie, organizzazioni, ecc.) della popolazione di riferimento sono incluse nella raccolta dei dati. Ad esempio, se la popolazione di riferimento &#xe8; definita come l&apos;insieme dei membri di un sindacato, tutti i membri del sindacato sono invitati a partecipare allo studio. &#xc8; anche chiamato &quot;censimento&quot; se viene selezionata l&apos;intera popolazione di un&apos;unit&#xe0; regionale (ad esempio un paese).</skos:definition>
      <skos:prefLabel xml:lang="en">Total universe/Complete enumeration</skos:prefLabel>
      <skos:definition xml:lang="en">All units (individuals, households, organizations, etc.) of a target population are included in the data collection. For example, if the target population is defined as the members of a trade union, all union members are invited to participate in the study. Also called &quot;census&quot; if the entire population of a regional unit (e.g. a country) is selected.</skos:definition>
      <skos:prefLabel xml:lang="de">Vollerhebung</skos:prefLabel>
      <skos:definition xml:lang="de">Alle Einheiten (Individuen, Haushalte, Organisationen, usw.) der Grundgesamtheit sind Teil der Erhebung. Wenn beispielsweise die Grundgesamtheit als Mitglieder einer Gewerkschaft definiert ist, werden alle Gewerkschaftsmitglieder eingeladen, an der Studie teilzunehmen. Wenn die gesamte Bev&#xf6;lkerung einer regionalen Einheit (z. B. eines Landes) Teil des Erhebungsverfahrens ist, wird dies auch als &apos;Zensus&apos; bezeichnet.</skos:definition>
      <skos:prefLabel xml:lang="fr">Univers complet / d&#xe9;nombrement complet</skos:prefLabel>
      <skos:definition xml:lang="fr">Toutes les unit&#xe9;s (individus, m&#xe9;nages, organisations, etc.) de la population cible sont incluses dans la collecte des donn&#xe9;es. Par exemple, si la population cible est d&#xe9;finie comme les membres d&apos;une organisation syndicale, tous les membres syndicaux sont invit&#xe9;s &#xe0; participer &#xe0; l&apos;&#xe9;tude. Aussi appel&#xe9; &quot;recensement&quot; si la population compl&#xe8;te d&apos;une unit&#xe9; r&#xe9;gionale (e.g. un pays) est s&#xe9;lectionn&#xe9;e.</skos:definition>
      <skos:prefLabel xml:lang="nl">Doelpopulatie</skos:prefLabel>
      <skos:definition xml:lang="nl"></skos:definition>
      <skos:prefLabel xml:lang="no">Hele populasjonen/total oppregning</skos:prefLabel>
      <skos:definition xml:lang="no">Alle enheter (individer, husholdninger, organisasjoner etc.) i m&#xe5;lpopulasjonen er inkludert i datainnsamlingen. For eksempel: dersom m&#xe5;lpopulasjonen er definert som medlemmer av en fagforening blir alle medlemmene invitert til &#xe5; delta i studien. Ogs&#xe5; kalt &apos;sensus&apos; dersom hele populasjonen av en regional enhet (f.eks et land) er valgt.</skos:definition>
   </rdf:Description>
   <rdf:Description rdf:about="http://rdf-vocabulary.ddialliance.org/cv/SamplingProcedure/2.0.1/0d2765b">
      <rdf:type rdf:resource="http://www.w3.org/2004/02/skos/core#Concept"/>
      <skos:inScheme rdf:resource="http://rdf-vocabulary.ddialliance.org/cv/SamplingProcedure/2.0.1/"/>
      <skos:notation xml:lang="en">Probability</skos:notation>
      <skos:prefLabel xml:lang="sl">Verjetnostno</skos:prefLabel>
      <skos:definition xml:lang="sl">Vse enote (posamezniki, gospodinjstva, organizacije itd.) ciljne populacije imajo dolo&#x10d;eno verjetnost (razli&#x10d;no od ni&#x10d;), da se vklju&#x10d;ijo v vzorec. To verjetnost je mogo&#x10d;e natan&#x10d;no dolo&#x10d;iti. Uporabite ta &#x161;ir&#x161;i izraz, &#x10d;e bolj dolo&#x10d;ena vrsta verjetnostnega vzor&#x10d;enja ni znana oziroma jo je te&#x17e;ko prepoznati.</skos:definition>
      <skos:prefLabel xml:lang="lt">Tikimybin&#x117;</skos:prefLabel>
      <skos:definition xml:lang="lt">Visi tikslin&#x117;s populiacijos vienetai (individai, nam&#x173; &#x16b;kiai, organizacijos ir kt.) turi ne nulin&#x119; tikimyb&#x119; patekti &#x12f; imt&#x12f; ir &#x161;i&#x105; tikimyb&#x119; galima tiksliai apskai&#x10d;iuoti. Naudoti &#x161;&#x12f; platesn&#x12f; termin&#x105;, jei ne&#x17e;inomas konkretesnis tikimybin&#x117;s atrankos tipas arba j&#x12f; sunku nustatyti.</skos:definition>
      <skos:prefLabel xml:lang="sv">Sannolikhetsurval</skos:prefLabel>
      <skos:definition xml:lang="sv">Alla element (individer, hush&#xe5;ll, organisationer m.m.) i m&#xe5;lpopulationen har en sannolikhet st&#xf6;rre &#xe4;n noll att inkluderas i urvalet och det g&#xe5;r att exakt ber&#xe4;kna sannolikheten. Anv&#xe4;nd den h&#xe4;r bredare termen om det &#xe4;r ok&#xe4;nt vilken mer specifik typ av sannolikhetsurval det r&#xf6;r sig om eller om typen &#xe4;r sv&#xe5;r att identifiera.</skos:definition>
      <skos:prefLabel xml:lang="it">Probabilistisco</skos:prefLabel>
      <skos:definition xml:lang="it">Tutte le unit&#xe0; (individui, famiglie, organizzazioni, ecc.) della popolazione di riferimento hanno una probabilit&#xe0; diversa da zero di essere incluse nel campione e tale probabilit&#xe0; pu&#xf2; essere determinata con precisione. Utilizzare questo termine pi&#xf9; ampio se non &#xe8; conosciuto oppure &#xe8; difficile identificare un tipo pi&#xf9; specifico di campionamento probabilistico.</skos:definition>
      <skos:prefLabel xml:lang="en">Probability</skos:prefLabel>
      <skos:definition xml:lang="en">All units (individuals, households, organizations, etc.) of a target population have a non-zero probability of being included in the sample and this probability can be accurately determined. Use this broader term if a more specific type of probability sampling is not known or is difficult to identify.</skos:definition>
      <skos:prefLabel xml:lang="de">Wahrscheinlichkeitsauswahl</skos:prefLabel>
      <skos:definition xml:lang="de">Alle Einheiten (Individuen, Haushalte, Organisationen, usw.) der Grundgesamtheit haben eine genau bestimmbare, von Null verschiedene Wahrscheinlichkeit, in die Stichprobe zu gelangen. Verwenden Sie diese Kategorie, wenn die genaue Art der Wahrscheinlichkeitsauswahl unbekannt oder schwierig zu bestimmen ist.</skos:definition>
      <skos:prefLabel xml:lang="fr">Probabiliste</skos:prefLabel>
      <skos:definition xml:lang="fr">Toutes les unit&#xe9;s (individus, m&#xe9;nages, organisations, etc.) de la population cible ont une probabilit&#xe9; non nulle d&apos;&#xea;tre incluses dans l&apos;&#xe9;chantillon et cette probabilit&#xe9; peut &#xea;tre fid&#xe8;lement d&#xe9;termin&#xe9;e. Utilisez ce terme si un terme plus sp&#xe9;cifique d&apos;&#xe9;chantillonnage probabiliste n&apos;est pas connu ou est difficile &#xe0; identifier.</skos:definition>
      <skos:prefLabel xml:lang="nl">Kanssteekproef</skos:prefLabel>
      <skos:definition xml:lang="nl"></skos:definition>
      <skos:prefLabel xml:lang="no">Sannsynlighetsutvalg</skos:prefLabel>
      <skos:definition xml:lang="no">Alle enheter (individer, husholdninger, organisasjoner etc.) i m&#xe5;lpopulasjonen har en sannsynlighet st&#xf8;rre enn null for &#xe5; bli inkludert i utvalget og denne sannsynligheten kan utregnes. Bruksmerknad: Bruk dette bredere begrepet dersom en mer spesifikk type sannsynlighetsutvalg ikke er kjent eller dersom det er vanskelig &#xe5; definere.</skos:definition>
      <skos:narrower rdf:resource="http://rdf-vocabulary.ddialliance.org/cv/SamplingProcedure/2.0.1/38e8e88"/>
      <skos:narrower rdf:resource="http://rdf-vocabulary.ddialliance.org/cv/SamplingProcedure/2.0.1/f189f62"/>
      <skos:narrower rdf:resource="http://rdf-vocabulary.ddialliance.org/cv/SamplingProcedure/2.0.1/55d038d"/>
      <skos:narrower rdf:resource="http://rdf-vocabulary.ddialliance.org/cv/SamplingProcedure/2.0.1/1f6e5f3"/>
      <skos:narrower rdf:resource="http://rdf-vocabulary.ddialliance.org/cv/SamplingProcedure/2.0.1/f91d8ca"/>
   </rdf:Description>
   <rdf:Description rdf:about="http://rdf-vocabulary.ddialliance.org/cv/SamplingProcedure/2.0.1/38e8e88">
      <rdf:type rdf:resource="http://www.w3.org/2004/02/skos/core#Concept"/>
      <skos:inScheme rdf:resource="http://rdf-vocabulary.ddialliance.org/cv/SamplingProcedure/2.0.1/"/>
      <skos:notation xml:lang="en">Probability.SimpleRandom</skos:notation>
      <skos:prefLabel xml:lang="sl">Verjetnostno: enostavno slu&#x10d;ajno</skos:prefLabel>
      <skos:definition xml:lang="sl">Vse enote ciljne populacije imajo enako verjetnost, da so vklju&#x10d;ene v vzorec. Obi&#x10d;ajno je celotna populacija navedena v &quot;vzor&#x10d;nem okviru&quot;, nato pa se enote izberejo iz tega okvira z uporabo metode slu&#x10d;ajnega izbora.</skos:definition>
      <skos:prefLabel xml:lang="lt">Tikimybin&#x117;: paprastoji atsitiktin&#x117; </skos:prefLabel>
      <skos:definition xml:lang="lt">Visi tikslin&#x117;s populiacijos vienetai turi vienod&#x105; tikimyb&#x119; patekti &#x12f; imt&#x12f;. Paprastai naudojamas visos populiacijos s&#x105;ra&#x161;as, i&#x161; kurio atsitiktinio parinkimo metodu atrenkami imties vienetai.</skos:definition>
      <skos:prefLabel xml:lang="sv">Sannolikhetsurval: obundet slumpm&#xe4;ssigt urval</skos:prefLabel>
      <skos:definition xml:lang="sv">Alla element i m&#xe5;lpopulationen har samma sannolikhet att inkluderas i urvalet. Vanligtvis listas hela populationen i en &quot;urvalsram&quot; och elementen v&#xe4;ljs fr&#xe5;n den ramen med en slumpvalsmetod.</skos:definition>
      <skos:prefLabel xml:lang="it">Probabilistisco: casuale semplice</skos:prefLabel>
      <skos:definition xml:lang="it">Tutte le unit&#xe0; della popolazione di riferimento hanno uguale probabilit&#xe0; di essere incluse nel campione. In genere, l&apos;intera popolazione &#xe8; inclusa in una &quot;lista di campionamento&quot; e le singole unit&#xe0; vengono quindi scelte da questa lista usando un metodo di selezione casuale.</skos:definition>
      <skos:prefLabel xml:lang="en">Probability: Simple random</skos:prefLabel>
      <skos:definition xml:lang="en">All units of a target population have an equal probability of being included in the sample. Typically, the entire population is listed in a &quot;sample frame&quot;, and units are then chosen from this frame using a random selection method.</skos:definition>
      <skos:prefLabel xml:lang="de">Wahrscheinlichkeitsauswahl: Einfache Zufallsauswahl</skos:prefLabel>
      <skos:definition xml:lang="de">Alle Einheiten (Individuen, Haushalte, Organisationen, usw.) der Grundgesamtheit haben die gleiche Wahrscheinlichkeit, in die Stichprobe zu gelangen. In der Regel werden die Einheiten der Grundgesamtheit zuf&#xe4;llig aus einer Auswahlgrundlage (z. B. eine Liste mit allen Einheiten der Grundgesamtheit) gezogen.</skos:definition>
      <skos:prefLabel xml:lang="fr">Probabiliste : al&#xe9;atoire simple</skos:prefLabel>
      <skos:definition xml:lang="fr">Toutes les unit&#xe9;s de la population cible ont une probabilit&#xe9; identique d&apos;&#xea;tre incluses dans l&apos;&#xe9;chantillon. Typiquement, la population enti&#xe8;re est list&#xe9;e dans une &quot;base de sondage&quot;, et des unit&#xe9;s sont alors choisies &#xe0; partir de cette base en utilisant une m&#xe9;thode de s&#xe9;lection al&#xe9;atoire.</skos:definition>
      <skos:prefLabel xml:lang="nl">Aselecte kansssteekproef</skos:prefLabel>
      <skos:definition xml:lang="nl"></skos:definition>
      <skos:prefLabel xml:lang="no">Sannsynlighetsutvalg: Enkelt tilfeldig</skos:prefLabel>
      <skos:definition xml:lang="no">Alle enheter i m&#xe5;lpopulasjonen har en lik sjanse for &#xe5; bli inkludert i utvalget. Vanligvis listes hele populasjonen i en &apos;utvalgsramme&apos; og enhetene blir valgt ut fra denne ved en tilfeldig utvalgsmetode.</skos:definition>
   </rdf:Description>
   <rdf:Description rdf:about="http://rdf-vocabulary.ddialliance.org/cv/SamplingProcedure/2.0.1/f189f62">
      <rdf:type rdf:resource="http://www.w3.org/2004/02/skos/core#Concept"/>
      <skos:inScheme rdf:resource="http://rdf-vocabulary.ddialliance.org/cv/SamplingProcedure/2.0.1/"/>
      <skos:notation xml:lang="en">Probability.SystematicRandom</skos:notation>
      <skos:prefLabel xml:lang="sl">Verjetnostno: sistemati&#x10d;no slu&#x10d;ajno</skos:prefLabel>
      <skos:definition xml:lang="sl">Dolo&#x10d;en interval izbiranja dobimo, ko velikost populacije delimo z &#x17e;eleno velikostjo vzorca. Izhodi&#x161;&#x10d;na to&#x10d;ka se naklju&#x10d;no vzame iz vzor&#x10d;nega okvira, ki obi&#x10d;ajno pokriva celotno ciljno populacijo. Od izhodi&#x161;&#x10d;a se nato enote v vzorec izberejo glede na interval izbiranja. Postopek poznamo tudi kot intervalno vzor&#x10d;enje. Na primer, podjetje izvaja anketo in &#x17e;eli vzorec 1.000 zaposlenih od skupno 10.000. Postopek za&#x10d;ne z naklju&#x10d;no za&#x10d;etno &#x161;tevilko, nato pa bo vsak deseti s seznama zaposlenih v podjetju povabljen k sodelovanju v raziskavi.</skos:definition>
      <skos:prefLabel xml:lang="lt">Tikimybin&#x117;: sistemingoji atsitiktin&#x117; </skos:prefLabel>
      <skos:definition xml:lang="lt">Fiksuotas atrankos &#x17e;ingsnis nustatomas populiacijos dyd&#x12f; padalijant i&#x161; norimo imties dyd&#x17e;io. Po to, vis&#x105; tikslin&#x119; populiacij&#x105; apiman&#x10d;iame s&#x105;ra&#x161;e atsitiktinai parenkamas pradinis ta&#x161;kas. Tuomet pasirinktu atrankos &#x17e;ingsniu, pradedant nuo pradinio ta&#x161;ko, parenkami visi lik&#x119; imties vienetai. Taip pat vadinama intervaline atranka. Pavyzd&#x17e;iui, &#x12f;mon&#x117;s apklausai siekiama sudaryti 1000-io darbuotoj&#x173; imt&#x12f; i&#x161; 10000-i&#x173; darbuotoj&#x173; s&#x105;ra&#x161;o. Pradedant nuo atsitiktinai parinkto pradinio skai&#x10d;iaus, dalyvauti tyrime bus pakviestas kas de&#x161;imtas darbuotojas i&#x161; s&#x105;ra&#x161;o.</skos:definition>
      <skos:prefLabel xml:lang="sv">Sannolikhetsurval: systematiskt slumpm&#xe4;ssigt urval</skos:prefLabel>
      <skos:definition xml:lang="sv">Ett fast urvalsintervall skapas genom att dela populationsstorleken med den &#xf6;nskade urvalsstorleken. En startpunkt v&#xe4;ljs d&#xe4;refter slumpm&#xe4;ssigt fr&#xe5;n urvalsramen, som vanligtvis omfattar hela m&#xe5;lpopulationen. Fr&#xe5;n denna startpunkt v&#xe4;ljs sedan element till urvalet ut med hj&#xe4;lp av det fasta urvalsintervallet. Metoden kallas &#xe4;ven f&#xf6;r intervallurval.
Exempel: ett f&#xf6;retag vill genomf&#xf6;ra en enk&#xe4;t bland 1.000 av sina 10.000 anst&#xe4;llda. Med utg&#xe5;ngspunkt fr&#xe5;n en slumpm&#xe4;ssigt vald startpunkt bjuds vart tionde namn i listan &#xf6;ver medarbetare in att delta i unders&#xf6;kningen.</skos:definition>
      <skos:prefLabel xml:lang="it">Probabilistisco: sistematico</skos:prefLabel>
      <skos:definition xml:lang="it">Si determina un intervallo fisso dividendo la dimensione della popolazione per la dimensione del campione desiderata. Successivamente viene estratto in modo casuale il punto di partenza dalla lista di campionamento che, generalmente, copre l&apos;intera popolazione di riferimento. Dal punto di partenza verranno poi estratte le unit&#xe0; in base all&apos;intervallo determinato. &#xc8; conosciuto anche come &quot;campionamento a intervalli&quot;. Ad esempio, un sondaggio aziendale cerca un campione di 1.000 dipendenti sulla popolazione totale di 10.000. A partire da un numero di partenza casuale, sar&#xe0; invitato a partecipare allo studio ogni decimo nome selezionato dall&apos;elenco dei dipendenti dell&apos;azienda.</skos:definition>
      <skos:prefLabel xml:lang="en">Probability: Systematic random</skos:prefLabel>
      <skos:definition xml:lang="en">A fixed selection interval is determined by dividing the population size by the desired sample size. A starting point is then randomly drawn from the sample frame, which normally covers the entire target population. From this starting point, units for the sample are chosen based on the selection interval. Also known as interval sampling. For example, a company survey seeks a sample of 1,000 employees out of 10,000 total. Beginning with a random starting number, every 10th name from the employee list of the company will be invited to participate in the study.</skos:definition>
      <skos:prefLabel xml:lang="de">Wahrscheinlichkeitsauswahl: Systematische Zufallsauswahl</skos:prefLabel>
      <skos:definition xml:lang="de">Aus dem Verh&#xe4;ltnis der Grundgesamtheit und der gew&#xfc;nschten Stichprobengr&#xf6;&#xdf;e ergibt sich ein Intervall f&#xfc;r die Stichprobenziehung. In der Auswahlgrundlage (z. B. eine Liste mit allen Einheiten der Grundgesamtheit) wird ein Startpunkt zuf&#xe4;llig ermittelt. Von diesem Startpunkt aus werden alle weiteren Einheiten nach dem festgelegten Intervall ausgew&#xe4;hlt. Auch bekannt als Intervall-Stichprobe. Beispielsweise sollen 1.000 Angestellte von insgesamt 10.000 Angestellten eines Unternehmens befragt werden: Zuf&#xe4;llig wird ein/e Angestellte/r aus einer Liste mit allen Angestellten ausgew&#xe4;hlt. Ausgehend von dieser Person wird dann jede/r 10. eingeladen, an der Studie teilzunehmen.</skos:definition>
      <skos:prefLabel xml:lang="fr">Probabiliste : al&#xe9;atoire syst&#xe9;matique</skos:prefLabel>
      <skos:definition xml:lang="fr">Un intervalle de s&#xe9;lection fixe est d&#xe9;termin&#xe9; en divisant la taille de la population par la taille d&#xe9;sir&#xe9;e de l&apos;&#xe9;chantillon. Le point de d&#xe9;part est alors un tirage au sort &#xe0; partir de la base de sondage, laquelle couvre normalement la population cible totale. &#xc0; partir de ce point de d&#xe9;part, des unit&#xe9;s pour l&apos;&#xe9;chantillonnage sont choisies en fonction de l&apos;intervalle de s&#xe9;lection. Aussi connu comme l&apos;&#xe9;chantillonnage par intervalle. Par exemple, une enqu&#xea;te dans une entreprise porte sur un &#xe9;chantillon de 1 000 employ&#xe9;s sur un total de 10 000. En commen&#xe7;ant par un nombre de d&#xe9;part al&#xe9;atoire, tous les 10 noms de la liste des employ&#xe9;s de l&apos;entreprise seront invit&#xe9;s &#xe0; participer &#xe0; l&apos;&#xe9;tude.</skos:definition>
      <skos:prefLabel xml:lang="nl">Systematische steekproef</skos:prefLabel>
      <skos:definition xml:lang="nl"></skos:definition>
      <skos:prefLabel xml:lang="no">Sannsynlighetsutvalg: Systematisk tilfeldig</skos:prefLabel>
      <skos:definition xml:lang="no">Et fast seleksjonsintervall er bestemt ved &#xe5; dele populasjonsst&#xf8;rrelsen p&#xe5; den &#xf8;nskede utvalgsst&#xf8;rrelsen. Et startpunkt er deretter trukket tilfeldig fra utvalgsrammen, som normalt dekker hele m&#xe5;lpopulasjonen. Fra startpunktet blir enheter for utvalget trukket basert p&#xe5; seleksjonsintervallet. Ogs&#xe5; kjent som utvalgsintervall. For eksempel, en bedriftsunders&#xf8;kelse &#xf8;nsker et utvalg p&#xe5; 1000 ansatte av 10.000 totalt. Ut fra et tilfeldig startnummer blir hvert tiende navn fra ansattlisten til bedriften invitert til &#xe5; delta i studien.</skos:definition>
   </rdf:Description>
   <rdf:Description rdf:about="http://rdf-vocabulary.ddialliance.org/cv/SamplingProcedure/2.0.1/55d038d">
      <rdf:type rdf:resource="http://www.w3.org/2004/02/skos/core#Concept"/>
      <skos:inScheme rdf:resource="http://rdf-vocabulary.ddialliance.org/cv/SamplingProcedure/2.0.1/"/>
      <skos:notation xml:lang="en">Probability.Stratified</skos:notation>
      <skos:prefLabel xml:lang="sl">Verjetnostno: stratificirano</skos:prefLabel>
      <skos:definition xml:lang="sl">Ciljna populacija je razdeljena na lo&#x10d;ene in medsebojno izklju&#x10d;ujo&#x10d;e se odseke (stratume/sloje), ki pokrivajo celotno populacijo. Iz vsakega odseka se nato vzamejo neodvisni slu&#x10d;ajni vzorci. Na primer, v nacionalni raziskavi javnega mnenja je celotno prebivalstvo razdeljeno na dva regionalna odseka: vzhodni in zahodni. Vzor&#x10d;ene enote se nato vzamejo iz vsake regije z enostavnim ali sistemati&#x10d;nim slu&#x10d;ajnim vzor&#x10d;enjem. Uporabite ta &#x161;ir&#x161;i izraz, &#x10d;e dolo&#x10d;ena vrsta stratificiranega vzor&#x10d;enja ni znana ali je te&#x17e;ko prepoznavna.</skos:definition>
      <skos:prefLabel xml:lang="lt">Tikimybin&#x117;: sluoksnin&#x117;</skos:prefLabel>
      <skos:definition xml:lang="lt">Tikslin&#x117; populiacija yra padalinama &#x12f; atskirus ir nepersidengian&#x10d;ius segmentus (sluoksnius), apiman&#x10d;ius vis&#x105; populiacij&#x105;. Tada kiekviename sluoksnyje atskirai sudaromos atsitiktin&#x117;s imtys. Pavyzd&#x17e;iui, atliekant nacionalin&#x119; vie&#x161;osios nuomon&#x117;s apklaus&#x105;, visi gyventojai suskirstomi &#x12f; du teritorinius sluoksnius: ryt&#x173; ir vakar&#x173;. Po to, naudojant paprast&#x105;j&#x105; arba sisteming&#x105;j&#x105; atsitiktin&#x119; atrank&#x105;, i&#x161; kiekvieno sluoksnio atrenkami imties vienetai. Naudoti &#x161;&#x12f; platesn&#x12f; termin&#x105;, kai ne&#x17e;inomas konkretus sluoksnin&#x117;s imties tipas arba j&#x12f; sunku nustatyti.</skos:definition>
      <skos:prefLabel xml:lang="sv">Sannolikhetsurval: stratifierat urval</skos:prefLabel>
      <skos:definition xml:lang="sv">M&#xe5;lpopulationen delas in i flera delar (strata) som utesluter varandra och t&#xe4;cker hela populationen. Oberoende slumpm&#xe4;ssiga urval g&#xf6;rs sedan fr&#xe5;n varje stratum. Exempel: i en nationell opinionsunders&#xf6;kning &#xe4;r hela populationen uppdelad i tv&#xe5; regionala strata, &#xd6;st och V&#xe4;st. D&#xe4;refter v&#xe4;ljs element slumpm&#xe4;ssigt fr&#xe5;n respektive region med obundet eller systematiskt slumpm&#xe4;ssigt urval. Anv&#xe4;nd den h&#xe4;r bredare termen om det &#xe4;r ok&#xe4;nt vilken mer specifik typ av stratifierat urval det r&#xf6;r sig om eller om typen &#xe4;r sv&#xe5;r att identifiera.</skos:definition>
      <skos:prefLabel xml:lang="it">Probabilistisco: stratificato</skos:prefLabel>
      <skos:definition xml:lang="it">La popolazione di riferimento &#xe8; suddivisa in segmenti separati e mutuamente esclusivi (strati) che coprono l&apos;intera popolazione. Da ciascun segmento vengono estratti, in modo casuale, campioni casuali indipendenti. Ad esempio, in un sondaggio nazionale sull&apos;opinione pubblica l&apos;intera popolazione &#xe8; divisa in due strati regionali: est e ovest. Le unit&#xe0; di campionamento vengono quindi estratte da ognuna dei due strati regionali utilizzando campionamenti casuali semplici o sistematici. Utilizzare questo termine pi&#xf9; ampio se non &#xe8; conosciuto oppure &#xe8; difficile identificare il tipo specifico di campionamento stratificato.</skos:definition>
      <skos:prefLabel xml:lang="en">Probability: Stratified</skos:prefLabel>
      <skos:definition xml:lang="en">The target population is subdivided into separate and mutually exclusive segments (strata) that cover the entire population. Independent random samples are then drawn from each segment. For example, in a national public opinion survey the entire population is divided into two regional strata: East and West. After this, sampling units are drawn from within each region using simple or systematic random sampling. Use this broader term if the specific type of stratified sampling is not known or difficult to identify.</skos:definition>
      <skos:prefLabel xml:lang="de">Wahrscheinlichkeitsauswahl: Geschichtete Zufallsauswahl</skos:prefLabel>
      <skos:definition xml:lang="de">Die Grundgesamtheit wird in sich gegenseitig ausschlie&#xdf;ende und insgesamt ersch&#xf6;pfende Schichten unterteilt. Aus jeder Schicht werden voneinander unabh&#xe4;ngige, einfache Zufallsstichproben gezogen. Beispielsweise wird ein Land bei einer allgemeinen Bev&#xf6;lkerungsumfrage in zwei regionale Kategorien unterteilt: Ost und West. In beiden Regionen werden jeweils getrennte Stichproben gezogen. W&#xe4;hlen Sie diese Kategorie, wenn die genaue Art der geschichteten Wahrscheinlichkeitsauswahl unbekannt oder schwierig zu bestimmen ist.</skos:definition>
      <skos:prefLabel xml:lang="fr">Probabiliste : stratifi&#xe9;</skos:prefLabel>
      <skos:definition xml:lang="fr">La population cible est subdivis&#xe9;e dans des segments (strates) s&#xe9;par&#xe9;es et mutuellement exclusifs qui couvrent la population enti&#xe8;re. Des &#xe9;chantillons al&#xe9;atoires ind&#xe9;pendants sont alors tir&#xe9;s de chaque segment. Par exemple, dans une enqu&#xea;te nationale d&apos;opinion publique la population enti&#xe8;re est divis&#xe9;e en deux strates r&#xe9;gionales : Est et Ouest. Apr&#xe8;s cela, les unit&#xe9;s d&apos;&#xe9;chantillonnage sont tir&#xe9;es &#xe0; partir de chaque r&#xe9;gion utilisant un &#xe9;chantillonnage al&#xe9;atoire simple ou syst&#xe9;matique. Utilisez ce terme si le type sp&#xe9;cifique de l&apos;&#xe9;chantillonnage stratifi&#xe9; n&apos;est pas connu ou est difficile &#xe0; identifier.</skos:definition>
      <skos:prefLabel xml:lang="nl">Gestratificeerde kanssteekproef</skos:prefLabel>
      <skos:definition xml:lang="nl"></skos:definition>
      <skos:prefLabel xml:lang="no">Sannsynlighetsutvalg: Stratifisert</skos:prefLabel>
      <skos:definition xml:lang="no">M&#xe5;lpopulasjonen er delt i ulike og gjensidig utelukkende strata som dekker hele populasjonen. Uavhengige tilfeldige utvalg blir deretter trukket innenfor hvert stratum. For eksempel i nasjonale befolkningsunders&#xf8;kelser blir hele populasjonen delt i to regionale strata: &#xf8;st og vest. Deretter blir utvalgsenheter trukket fra hver region ved bruk av tilfeldig eller systematisk utvalg. Bruk dette bredere begrepet dersom den spesifikke typen stratifisert utvalg ikke er kjent eller er vanskelig &#xe5; identifisere.</skos:definition>
      <skos:narrower rdf:resource="http://rdf-vocabulary.ddialliance.org/cv/SamplingProcedure/2.0.1/7653f19"/>
      <skos:narrower rdf:resource="http://rdf-vocabulary.ddialliance.org/cv/SamplingProcedure/2.0.1/2059a2b"/>
   </rdf:Description>
   <rdf:Description rdf:about="http://rdf-vocabulary.ddialliance.org/cv/SamplingProcedure/2.0.1/7653f19">
      <rdf:type rdf:resource="http://www.w3.org/2004/02/skos/core#Concept"/>
      <skos:inScheme rdf:resource="http://rdf-vocabulary.ddialliance.org/cv/SamplingProcedure/2.0.1/"/>
      <skos:notation xml:lang="en">Probability.Stratified.Proportional</skos:notation>
      <skos:prefLabel xml:lang="sl">Verjetnostno: stratificiano: proporcionalno</skos:prefLabel>
      <skos:definition xml:lang="sl">Ciljna populacija je razdeljena na lo&#x10d;ene in medsebojno izklju&#x10d;ujo&#x10d;e se odseke (stratume/sloje), ki pokrivajo celotno populacijo. Pri proporcionalnem stratificiranem vzor&#x10d;enju je &#x161;tevilo elementov, izbranih iz vsakega sloja, sorazmerno z velikostjo populacije v sloju glede na celotno populacijo. Na primer, dr&#x17e;ava je razdeljena na dva regionalna odseka, ki obsegata 80 odstotkov (zahod) in 20 odstotkov (vzhod) celotnega prebivalstva. Za vzorec 1.000 prebivalcev bi iz zahodnega odseka vzeli 800 (tj. 80 odstotkov) udele&#x17e;encev in iz vzhodnega odseka 200 (tj. 20 odstotkov), kar bi natan&#x10d;no predstavljalo njihov dele&#x17e; v celotni populaciji.</skos:definition>
      <skos:prefLabel xml:lang="lt">Tikimybin&#x117;: sluoksnin&#x117;: proporcingoji</skos:prefLabel>
      <skos:definition xml:lang="lt">Tikslin&#x117; populiacija yra padalinama &#x12f; atskirus ir nepersidengian&#x10d;ius segmentus (sluoksnius), apiman&#x10d;ius vis&#x105; populiacij&#x105;. Proporcin&#x117;je sluoksnin&#x117;je atrankoje i&#x161; kiekvieno sluoksnio atrinkt&#x173; element&#x173; skai&#x10d;ius yra proporcingas sluoksnio populiacijos santykiniam didumui. Pavyzd&#x17e;iui, &#x161;alis yra padalinama &#x12f; du teritorinius sluoksnius, kurie apima 80 proc. (vakaruose) ir 20 proc. (rytuose) vis&#x173; gyventoj&#x173;. Sudarant 1000-io &#x17e;moni&#x173; imt&#x12f;, 800-ai (t. y., 80 proc.) tur&#x117;t&#x173; b&#x16b;ti atrinkti i&#x161; vakar&#x173; ir 200-ai (t. y., 20 proc.) i&#x161; ryt&#x173;, tam, kad imties proporcijos atitikt&#x173; visos populiacijos proporcijas.</skos:definition>
      <skos:prefLabel xml:lang="sv">Sannolikhetsurval: stratifierat: proportionerligt urval</skos:prefLabel>
      <skos:definition xml:lang="sv">M&#xe5;lpopulationen delas in i flera delar (strata) som utesluter varandra och t&#xe4;cker hela populationen. F&#xf6;r ett proportionerligt stratifierat urval st&#xe5;r antalet element som v&#xe4;ljs fr&#xe5;n varje stratum i proportion till storleken p&#xe5; stratumet i f&#xf6;rh&#xe5;llande till hela populationen. Exempel: ett land &#xe4;r uppdelat i tv&#xe5; regionala strata som motsvarar 80 procent (V&#xe4;st) respektive 20 procent (&#xd6;st) av hela populationen. F&#xf6;r ett urval p&#xe5; 1.000 personer skulle 800 (dvs. 80 %) v&#xe4;ljas fr&#xe5;n V&#xe4;st och 200 (dvs. 20 %) fr&#xe5;n &#xd6;st f&#xf6;r att ge en korrekt representation av deras andel av hela populationen.</skos:definition>
      <skos:prefLabel xml:lang="it">Probabilistisco: stratificato proporzionale</skos:prefLabel>
      <skos:definition xml:lang="it">La popolazione di riferimento &#xe8; suddivisa in segmenti separati e mutuamente esclusivi (strati) che coprono l&apos;intera popolazione. Nel campionamento stratificato proporzionale il numero di elementi scelti da ogni strato &#xe8; proporzionale alla dimensione della popolazione dello strato, in rapporto all&apos;intera popolazione. Ad esempio, un paese &#xe8; diviso in due strati regionali che comprendono l&apos;80% (ovest) e il 20% (est) della popolazione totale. Per un campione di 1.000 persone, 800 (cio&#xe8; l&apos;80%) saranno estratte dalla regione Ovest e 200 (ossia il 20%) dalla regione Est, mantenendo adeguatamente la relativa proporzione rispetto alla popolazione totale.</skos:definition>
      <skos:prefLabel xml:lang="en">Probability: Stratified: Proportional</skos:prefLabel>
      <skos:definition xml:lang="en">The target population is subdivided into separate and mutually exclusive segments (strata) that cover the entire population. In proportional stratified sampling the number of elements chosen from each stratum is proportional to the population size of the stratum when viewed against the entire population. For example, a country is divided into two regional strata that comprise 80 percent (West) and 20 percent (East) of the total population. For a sample of 1,000 people, 800 (i.e., 80 percent) would be drawn from the West and 200 (i.e., 20 percent) from the East to accurately represent their proportion in the total population.</skos:definition>
      <skos:prefLabel xml:lang="de">Wahrscheinlichkeitsauswahl: Proportional geschichtete Zufallsauswahl</skos:prefLabel>
      <skos:definition xml:lang="de">Die Grundgesamtheit wird in sich gegenseitig ausschlie&#xdf;ende und insgesamt ersch&#xf6;pfende Schichten unterteilt. Bei der proportional geschichteten Zufallsauswahl ist die Anzahl der gezogenen Einheiten proportional zur Anzahl der Einheiten der jeweiligen Schicht in der Grundgesamtheit. Beispielsweise wird ein Land in zwei regionale Schichten unterteilt, wobei erstere 80 Prozent (West) und letztere 20 Prozent (Ost) der gesamten Bev&#xf6;lkerung umfassen. F&#xfc;r eine Stichprobe von 1.000 Personen w&#xfc;rden dann 800 Personen im Osten und 200 Personen im Westen befragt.</skos:definition>
      <skos:prefLabel xml:lang="fr">Probabiliste : stratifi&#xe9; : proportionnel</skos:prefLabel>
      <skos:definition xml:lang="fr">La population cible est subdivis&#xe9;e dans des segments (strates) s&#xe9;par&#xe9;es et mutuellement exclusives qui couvrent la population enti&#xe8;re. Dans un &#xe9;chantillon stratifi&#xe9; proportionnel le nombre d&apos;&#xe9;l&#xe9;ments choisis dans chaque strate est proportionnel &#xe0; la taille de la population de la strate par rapport &#xe0; la population enti&#xe8;re. Par exemple, un pays est divis&#xe9; en deux strates r&#xe9;gionales qui comprend 80 pour cent (Ouest) et 20 pour cent (Est) de la population totale. Pour un &#xe9;chantillon de 1 000 personnes, 800 (i. e., 80 pour cent) devraient &#xea;tre tir&#xe9;es &#xe0; partir de l&apos;Ouest et 200 (i. e., 20 pour cent) &#xe0; partir de l&apos;Est pour repr&#xe9;senter fid&#xe8;lement leur proportion dans la population totale.</skos:definition>
      <skos:prefLabel xml:lang="nl">Proportioneel gestratificeerde kanssteekproef</skos:prefLabel>
      <skos:definition xml:lang="nl"></skos:definition>
      <skos:prefLabel xml:lang="no">Sannsynlighetsutvalg: Stratifisert: Proporsjonalt</skos:prefLabel>
      <skos:definition xml:lang="no">M&#xe5;lpopulasjonen er delt i flere strata som er gjensidig utelukkende og dekker hele populasjonen. I proporsjonalt stratifisert utvalg er antallet elementer som velges fra hvert strata proporsjonalt til populasjonsst&#xf8;rrelsen til stratumet sett i forhold til hele populasjonen. For eksempel: Et land er delt i to regionale strata som tilsier 80 prosent (vest) og 20 prosent (&#xf8;st) av hele populasjonen. For et utvalg p&#xe5; 1000 personer ville 800 (dvs 80%) bli trukket fra vest og 200 (dvs 20%) fra &#xf8;st for &#xe5; gi en riktig representasjon av deres andel av den totale populasjonen.</skos:definition>
   </rdf:Description>
   <rdf:Description rdf:about="http://rdf-vocabulary.ddialliance.org/cv/SamplingProcedure/2.0.1/2059a2b">
      <rdf:type rdf:resource="http://www.w3.org/2004/02/skos/core#Concept"/>
      <skos:inScheme rdf:resource="http://rdf-vocabulary.ddialliance.org/cv/SamplingProcedure/2.0.1/"/>
      <skos:notation xml:lang="en">Probability.Stratified.Disproportional</skos:notation>
      <skos:prefLabel xml:lang="sl">Verjetnostno: startificirano: disproporcionalno</skos:prefLabel>
      <skos:definition xml:lang="sl">Ciljna populacija je razdeljena na lo&#x10d;ene in medsebojno izklju&#x10d;ujo&#x10d;e se odseke (stratume/sloje), ki pokrivajo celotno populacijo. &#x160;tevilo enot, izbranih iz vsakega odseka, pri disproporcionalnem vzor&#x10d;enju ni sorazmerno z velikostjo populacije odseka glede na celotno populacijo. &#x160;tevilo vzor&#x10d;enih enot iz vsakega odseka je lahko enako, optimalno oziroma lahko odra&#x17e;a namen raziskave, kot je nadvzor&#x10d;enje razli&#x10d;nih podskupin prebivalstva. Na primer, dr&#x17e;ava je razdeljena na dva regionalna odseka, ki obsegata 80 odstotkov (zahod) in 20 odstotkov (vzhod) prebivalstva dr&#x17e;ave. &#x10c;e je v raziskavi potrebna enakopravna zastopanost obeh regij, se v vzorec lahko vzame polovica udele&#x17e;encev iz zahoda in polovica iz vzhoda, tako da vsaka regija predstavlja 50 odstotkov vzorca. &#x10c;e je potrebna podrobnej&#x161;a analiza prebivalstva z vzhoda, lahko vzamemo 40 odstotkov enot iz zahoda in 60 odstotkov iz vzhoda, tako da je vzhod prekomerno zastopan.</skos:definition>
      <skos:prefLabel xml:lang="lt">Tikimybin&#x117;: sluoksnin&#x117;: neproporcingoji</skos:prefLabel>
      <skos:definition xml:lang="lt">Tikslin&#x117; populiacija yra padalinama &#x12f; atskirus ir nepersidengian&#x10d;ius segmentus (sluoksnius), apiman&#x10d;ius vis&#x105; populiacij&#x105;. Neproporcingoje sluoksnin&#x117;je atrankoje i&#x161; kiekvieno sluoksnio atrinkt&#x173; element&#x173; skai&#x10d;ius yra specialiai neproporcingas sluoksnio populiacijos santykiniam didumui. Kiekviename sluoksnyje atrinkt&#x173; vienet&#x173; skai&#x10d;ius gali b&#x16b;ti vienodas, optimalus arba atspind&#x117;ti kok&#x12f; nors tyrimo tiksl&#x105;, pavyzd&#x17e;iui, kai reikia gausesnio atskir&#x173; populiacijos pogrupi&#x173; atstovavimo. Pavyzd&#x17e;iui, &#x161;alis yra padalinama &#x12f; du teritorinius sluoksnius, kurie apima 80 proc. (vakaruose) ir 20 proc. (rytuose) vis&#x173; gyventoj&#x173;. Jei atliekant tyrim&#x105; reikia po lygiai reprezentuoti abu teritorinius sluoksnius, pus&#x119; imties galima atrinkti i&#x161; vakar&#x173;, pus&#x119; &#x2013; i&#x161; ryt&#x173;, taip, kad kiekvien&#x105; teritorin&#x12f; sluoksn&#x12f; atstovaut&#x173; 50 proc. imties. Jei reikia i&#x161;samesn&#x117;s ryt&#x173; gyventoj&#x173; analiz&#x117;s, 40 proc. vienet&#x173; gali b&#x16b;ti atrinkta i&#x161; vakar&#x173;, o 60 proc.&#x2013; i&#x161; ryt&#x173;, kad rytai b&#x16b;t&#x173; atstovaujami gausiau.</skos:definition>
      <skos:prefLabel xml:lang="sv">Sannolikhetsurval: stratifierat: oproportionerligt urval</skos:prefLabel>
      <skos:definition xml:lang="sv">M&#xe5;lpopulationen delas in i flera delar (strata) som utesluter varandra och t&#xe4;cker hela populationen. F&#xf6;r ett oproportionerligt urval s&#xe5; st&#xe5;r antalet element som v&#xe4;ljs fr&#xe5;n varje stratum inte i proportion till stratumets populationsstorlek i f&#xf6;rh&#xe5;llande till hela populationen. Sampelstorleken kan vara lika stor, optimal eller kan avspegla studiens syfte genom ett avsiktligt st&#xf6;rre urval fr&#xe5;n olika undergrupper i populationen. Exempel: ett land &#xe4;r uppdelat i tv&#xe5; regionala strata som motsvarar 80 procent (V&#xe4;st) respektive 20 procent (&#xd6;st) av hela populationen. Om lika representation av b&#xe5;da regionerna beh&#xf6;vs i studien kan halva samplet dras fr&#xe5;n &#xd6;st och andra halvan fr&#xe5;n V&#xe4;st s&#xe5; att varje region representeras av 50 % av samplet. Om det beh&#xf6;vs en mer detaljerad analys av population i &#xd6;st kan 40 % av elementen dras fr&#xe5;n V&#xe4;st och 60 % fr&#xe5;n &#xd6;st s&#xe5; att &#xd6;st &#xe4;r &#xf6;verrepresenterat.</skos:definition>
      <skos:prefLabel xml:lang="it">Probabilistisco: stratificato non proporzionale</skos:prefLabel>
      <skos:definition xml:lang="it">La popolazione di riferimento &#xe8; suddivisa in segmenti separati e mutuamente esclusivi (strati) che coprono l&apos;intera popolazione. Nel campionamento non proporzionale il numero di unit&#xe0; scelte da ogni strato non &#xe8; proporzionale alla dimensione della popolazione dello strato in rapporto all&apos;intera popolazione. Il numero di unit&#xe0; campionarie provenienti da ogni strato pu&#xf2; essere uguale oppure riflettere lo scopo dello studio, come nel caso di sovracampionamento di diversi sottogruppi della popolazione. Ad esempio, un paese &#xe8; diviso in due strati regionali che comprendono l&apos;80% (ovest) e il 20% (est) della popolazione totale. Se in uno studio &#xe8; necessaria una uguale rappresentazione delle due regioni, met&#xe0; del campione sar&#xe0; estratto dalla regione Est, in modo che ciascuna regione sia rappresentata dal 50% del campione. Se invece &#xe8; necessaria un&apos;analisi pi&#xf9; dettagliata della popolazione proveniente dalla regione Est, potr&#xe0; essere estratto il 40% delle unit&#xe0; dalla regione Ovest e il restante 60% dalla regione Est, in modo che quest&apos;ultima sia sovrarappresentata.</skos:definition>
      <skos:prefLabel xml:lang="en">Probability: Stratified: Disproportional</skos:prefLabel>
      <skos:definition xml:lang="en">The target population is subdivided into separate and mutually exclusive segments (strata) that cover the entire population. In disproportional sampling the number of units chosen from each stratum is not proportional to the population size of the stratum when viewed against the entire population. The number of sampled units from each stratum can be equal, optimal, or can reflect the purpose of the study, like oversampling of different subgroups of the population. For example, a country is divided into two regional strata that comprise 80 percent (West) and 20 precent (East) of the country&apos;s population. If equal representation of the two regions is needed in a study, half the sample may be drawn from the West and half from the East, so that each region is represented by 50 percent of the sample. If a more detailed analysis of the population from the East is needed, 40 percent of the units may be drawn from the West and 60 percent from the East, so that the East is over-represented.</skos:definition>
      <skos:prefLabel xml:lang="de">Wahrscheinlichkeitsauswahl: Disproportional geschichtete Zufallsauswahl</skos:prefLabel>
      <skos:definition xml:lang="de">Die Grundgesamtheit wird in sich gegenseitig ausschlie&#xdf;ende und insgesamt ersch&#xf6;pfende Schichten unterteilt, die die gesamte Bev&#xf6;lkerung abdecken. Bei der disproportionalen Zufallsauswahl ist die Anzahl der aus jeder Schicht gezogenen Einheiten nicht proportional zum Anteil der Schichten an der Grundgesamtheit. Sie k&#xf6;nnen &#xfc;ber die Schichten gleich verteilt sein oder sich an der Forschungsabsicht orientieren. Beispielsweise durch das so genannte Oversampling von in der Grundgesamtheit unterrepr&#xe4;sentierten Gruppen. Beispielsweise wird ein Land in zwei regionale Schichten unterteilt, wobei erstere 80 Prozent (West) und letztere 20 Prozent (Ost) der gesamten Bev&#xf6;lkerung umfassen. Sollen beide Regionen gleich repr&#xe4;sentiert werden, w&#xfc;rden in beiden Teilen jeweils 50 Prozent der ben&#xf6;tigten Stichprobe gezogen werden. Bei einem Oversampling der Region Ost w&#xfc;rden beispielsweise 60 Prozent der Stichproben im Osten und 40 Prozent im Westen gezogen werden.</skos:definition>
      <skos:prefLabel xml:lang="fr">Probabiliste : stratifi&#xe9; : disproportionn&#xe9;</skos:prefLabel>
      <skos:definition xml:lang="fr">La population cible est subdivis&#xe9;e dans des segments (strates) s&#xe9;par&#xe9;es et mutuellement exclusives qui couvrent la population enti&#xe8;re. Dans un &#xe9;chantillon disproportionnel le nombre des unit&#xe9;s choisies &#xe0; partir de chaque strate n&apos;est pas proportionnel &#xe0; la taille de population de la strate par rapport &#xe0; la population enti&#xe8;re. Le nombre d&apos;unit&#xe9;s &#xe9;chantillonn&#xe9;es &#xe0; partir de chaque strate peut &#xea;tre &#xe9;gal, optimal, ou peut refl&#xe9;ter la raison de l&apos;enqu&#xea;te, comme le sur-&#xe9;chantillonnage de diff&#xe9;rents sous-groupes de la population. Par exemple, un pays est divis&#xe9; en deux strates qui comprend 80 pour cent (Ouest) et 20 pour cent (Est) de la population du pays. Si une repr&#xe9;sentation &#xe9;gale des deux r&#xe9;gions est n&#xe9;cessaire dans une &#xe9;tude, la moiti&#xe9; de l&apos;&#xe9;chantillon peut &#xea;tre tir&#xe9;e &#xe0; partir de l&apos;Ouest et la moiti&#xe9; de l&apos;Est, tel que chaque r&#xe9;gion est repr&#xe9;sent&#xe9;e par 50 pour cent de l&apos;&#xe9;chantillon. Si une analyse plus d&#xe9;taill&#xe9;e de la population de l&apos;Est est n&#xe9;cessaire, 40 pour cent des unit&#xe9;s peuvent &#xea;tre tir&#xe9;es &#xe0; partir de l&apos;Ouest et 60 pour cent &#xe0; partir de l&apos;Est, tel que l&apos;Est est surrepr&#xe9;sent&#xe9;.</skos:definition>
      <skos:prefLabel xml:lang="nl">Disproportioneel gestratificeerde  kanssteekproef</skos:prefLabel>
      <skos:definition xml:lang="nl"></skos:definition>
      <skos:prefLabel xml:lang="no">Sannsynlighetsutvalg: Stratifisert: Disproporsjonalt</skos:prefLabel>
      <skos:definition xml:lang="no">M&#xe5;lpopulasjonen er delt i flere strata som er gjensidig utelukkende og dekker hele populasjonen. For et uproporsjonalt utvalg st&#xe5;r antallet elementer som velges fra hvert strata ikke proporsjonalt til st&#xf8;rrelsen p&#xe5; stratumet i forhold til hele populasjonen. Utvalgsst&#xf8;rrelsen fra hvert stratum kan v&#xe6;re lik, optimal, eller kan avspeile hensikten med studien, som er &#xe5; oversample enkelte undergrupper av populasjonen. For eksempel: Et land er delt i to regionale strata som tilsier 80 prosent (vest) og 20 prosent (&#xf8;st) av hele populasjonen. Dersom det er behov for lik representasjon av begge regionene i studien kan halve utvalget bli trukket fra &#xf8;st og andre halvdelen fra vest slik at hver region representerer 50% av utvalget. Om det er behov for en mer detaljert analyse av populasjonen i &#xf8;st kan 40% av enhetene bli trukket fra vest og 60% fra &#xf8;st, slik at &#xf8;st er overrepresentert.</skos:definition>
   </rdf:Description>
   <rdf:Description rdf:about="http://rdf-vocabulary.ddialliance.org/cv/SamplingProcedure/2.0.1/1f6e5f3">
      <rdf:type rdf:resource="http://www.w3.org/2004/02/skos/core#Concept"/>
      <skos:inScheme rdf:resource="http://rdf-vocabulary.ddialliance.org/cv/SamplingProcedure/2.0.1/"/>
      <skos:notation xml:lang="en">Probability.Cluster</skos:notation>
      <skos:prefLabel xml:lang="sl">Verjetnostno: po skupinah</skos:prefLabel>
      <skos:definition xml:lang="sl">Ciljna populacija je razdeljena na skupine, ki obstajajo same po sebi in izbran je verjetnostni vzorec skupin. Podatki se nato zbirajo na vseh enotah znotraj vsake izbrane skupine. Vzor&#x10d;ene skupine so pogosto dolo&#x10d;ene glede na geografsko obmo&#x10d;je ali &#x10d;asovno obdobje. Uporabite ta &#x161;ir&#x161;i izraz, &#x10d;e bolj dolo&#x10d;ena vrsta vzor&#x10d;enja skupin ni znana ali jo je te&#x17e;ko prepoznati.</skos:definition>
      <skos:prefLabel xml:lang="lt">Tikimybin&#x117;: lizdin&#x117;</skos:prefLabel>
      <skos:definition xml:lang="lt">Tikslin&#x117; populiacija yra padalinama &#x12f; nat&#x16b;ralius segmentus (lizdus) ir sudaroma tikimybin&#x117; j&#x173; imtis. Tada duomenys renkami apie visus atrinkt&#x173; lizd&#x173; vienetus. Lizdai da&#x17e;nai i&#x161;skiriami teritoriniu arba laiko pagrindu. Naudoti &#x161;&#x12f; platesn&#x12f; termin&#x105;, kai ne&#x17e;inomas konkretesnis lizdin&#x117;s atrankos tipas arba j&#x12f; sunku nustatyti.</skos:definition>
      <skos:prefLabel xml:lang="sv">Sannolikhetsurval: klusterurval</skos:prefLabel>
      <skos:definition xml:lang="sv">M&#xe5;lpopulationen delas in i naturligt f&#xf6;rekommande segment (kluster) och ett sannolikhetsurval g&#xf6;rs av dessa kluster. Data samlas sedan in fr&#xe5;n alla element i varje utvalt kluster. Urvalet baseras ofta p&#xe5; geografiska omr&#xe5;den eller tidsperioder. 
Anv&#xe4;nd den h&#xe4;r bredare termen om det &#xe4;r ok&#xe4;nt vilken mer specifik typ av klusterurval det r&#xf6;r sig om eller om typen &#xe4;r sv&#xe5;r att identifiera.</skos:definition>
      <skos:prefLabel xml:lang="it">Probabilistico: a grappoli</skos:prefLabel>
      <skos:definition xml:lang="it">La popolazione di riferimento &#xe8; divisa in modo naturale in gruppi (cluster) e viene selezionato un campione probabilistico dei cluster. I dati vengono quindi raccolti da tutte le unit&#xe0; individuate all&apos;interno di ciascun cluster selezionato. Il campionamento &#xe8; spesso raggruppato su base geografica o temporale. Utilizzare questo termine pi&#xf9; ampio se non &#xe8; conosciuto oppure &#xe8; difficile identificare un tipo pi&#xf9; specifico di campionamento a grappoli.</skos:definition>
      <skos:prefLabel xml:lang="en">Probability: Cluster</skos:prefLabel>
      <skos:definition xml:lang="en">The target population is divided into naturally occurring segments (clusters) and a probability sample of the clusters is selected. Data are then collected from all units within each selected cluster. Sampling is often clustered by geography, or time period. Use this broader term if a more specific type of cluster sampling is not known or is difficult to identify.</skos:definition>
      <skos:prefLabel xml:lang="de">Wahrscheinlichkeitsauswahl: Klumpenauswahl</skos:prefLabel>
      <skos:definition xml:lang="de">Die Grundgesamtheit wird in nat&#xfc;rlich auftretende Gruppen (Cluster) unterteilt. Aus diesen Gruppen wird eine Zufallsstichprobe gezogen. Innerhalb der gezogenen Gruppen werden dann Daten &#xfc;ber alle Einheiten erhoben. Die Gruppierungen ergeben sich oft durch die geografische Lage oder Zeitabschnitte. W&#xe4;hlen Sie diese Kategorie, wenn die genaue Art der Klumpenauswahl unbekannt oder schwierig zu bestimmen ist.</skos:definition>
      <skos:prefLabel xml:lang="fr">Probabiliste : grappe</skos:prefLabel>
      <skos:definition xml:lang="fr">La population cible est divis&#xe9;e dans des segments existants naturellement (grappes) et un &#xe9;chantillon probabiliste de groupes est s&#xe9;lectionn&#xe9;. Des donn&#xe9;es sont alors collect&#xe9;es &#xe0; partir de tous les unit&#xe9;s dans chaque groupe s&#xe9;lectionn&#xe9;. L&apos;&#xe9;chantillonnage est souvent regroup&#xe9; selon la g&#xe9;ographie, ou la p&#xe9;riode de temps. Utilisez ce terme si un terme plus sp&#xe9;cifique d&apos;&#xe9;chantillonnage en grappes n&apos;est pas connu ou est difficile &#xe0; identifier.</skos:definition>
      <skos:prefLabel xml:lang="nl">Clusterkanssteekproef</skos:prefLabel>
      <skos:definition xml:lang="nl"></skos:definition>
      <skos:prefLabel xml:lang="no">Sannsynlighetsutvalg: Klynge</skos:prefLabel>
      <skos:definition xml:lang="no">M&#xe5;lpopulasjonen er delt i naturlige grupper (klustere) og et sannsynlighetsutvalg av klusterne blir valgt. Data blir deretter samlet inn fra alle enhetene innen hver utvalgte kluster. Utvelgelsen er ofte gruppert ut fra geografi eller tidsperiode. Bruksmerknad: Bruk dette bredere begrepet dersom den mer spesifikke typen klusterutvalg er ukjent eller dersom typen er vanskelig &#xe5; identifisere.</skos:definition>
      <skos:narrower rdf:resource="http://rdf-vocabulary.ddialliance.org/cv/SamplingProcedure/2.0.1/8e08217"/>
      <skos:narrower rdf:resource="http://rdf-vocabulary.ddialliance.org/cv/SamplingProcedure/2.0.1/49f4571"/>
   </rdf:Description>
   <rdf:Description rdf:about="http://rdf-vocabulary.ddialliance.org/cv/SamplingProcedure/2.0.1/8e08217">
      <rdf:type rdf:resource="http://www.w3.org/2004/02/skos/core#Concept"/>
      <skos:inScheme rdf:resource="http://rdf-vocabulary.ddialliance.org/cv/SamplingProcedure/2.0.1/"/>
      <skos:notation xml:lang="en">Probability.Cluster.SimpleRandom</skos:notation>
      <skos:prefLabel xml:lang="sl">Verjetnostno: po skupinah: enostavno slu&#x10d;ajno</skos:prefLabel>
      <skos:definition xml:lang="sl">Ciljna populacija je razdeljena na skupine, ki obstajajo same po sebi in izbran je enostavni slu&#x10d;ajni vzorec skupin. Podatki se nato zbirajo na vseh enotah znotraj vsake izbrane skupine. Na primer, za vzorec u&#x10d;encev v mestu izberemo ve&#x10d; &#x161;ol z metodo slu&#x10d;ajnega izbora, nato pa vklju&#x10d;imo vse u&#x10d;ence iz vsake izbrane &#x161;ole.</skos:definition>
      <skos:prefLabel xml:lang="lt">Tikimybin&#x117;: lizdin&#x117;: paprastoji atsitiktin&#x117;</skos:prefLabel>
      <skos:definition xml:lang="lt">Tikslin&#x117; populiacija yra padalinama &#x12f; nat&#x16b;ralius segmentus (lizdus) ir sudaroma paprastoji atsitiktin&#x117; j&#x173; imtis. Tada duomenys renkami apie visus atrinkt&#x173; lizd&#x173; vienetus. Pavyzd&#x17e;iui, miesto moksleivi&#x173; im&#x10d;iai sudaryti, atsitiktin&#x117;s atrankos b&#x16b;du parenkamas tam tikras skai&#x10d;ius mokykl&#x173;, ir tada &#x12f;traukiami visi atrinkt&#x173; mokykl&#x173; mokiniai.</skos:definition>
      <skos:prefLabel xml:lang="sv">Sannolikhetsurval: klusterurval: obundet slumpm&#xe4;ssigt urval</skos:prefLabel>
      <skos:definition xml:lang="sv">M&#xe5;lpopulationen delas in i naturligt f&#xf6;rekommande segment (kluster) och det g&#xf6;rs ett obundet slumpm&#xe4;ssigt urval av dessa kluster. Data samlas sedan in fr&#xe5;n alla element i varje utvalt kluster. Exempel: f&#xf6;r att ta fram ett urval av elever i en stad skulle ett antal skolor v&#xe4;ljas med en slumpm&#xe4;ssig urvalsmetod och d&#xe4;refter skulle alla elever p&#xe5; de valda skolorna inkluderas i urvalet.</skos:definition>
      <skos:prefLabel xml:lang="it">Probabilistico: a grappoli casuale semplice</skos:prefLabel>
      <skos:definition xml:lang="it">La popolazione di riferimento &#xe8; divisa in modo naturale in gruppi (cluster) e viene selezionato un campione probabilistico dei cluster. I dati vengono quindi raccolti da tutte le unit&#xe0; individuate all&apos;interno di ciascun cluster selezionato. Ad esempio, per selezionare un campione di studenti in una citt&#xe0;, viene scelto casualmente un determinato numero di scuole e, successivamente, saranno inclusi tutti gli studenti di ogni scuola selezionata.</skos:definition>
      <skos:prefLabel xml:lang="en">Probability: Cluster: Simple random</skos:prefLabel>
      <skos:definition xml:lang="en">The target population is divided into naturally occurring segments (clusters) and a simple random sample of the clusters is selected. Data are then collected from all units within each selected cluster. For example, for a sample of students in a city, a number of schools would be chosen using the random selection method, and then all of the students from every sampled school would be included.</skos:definition>
      <skos:prefLabel xml:lang="de">Wahrscheinlichkeitsauswahl: Einfache Klumpenauswahl</skos:prefLabel>
      <skos:definition xml:lang="de">Die Grundgesamtheit wird in nat&#xfc;rlich auftretende Gruppen (Cluster) unterteilt. Aus diesen Gruppen wird eine Zufallsstichprobe gezogen. Innerhalb der gezogenen Gruppen werden dann Daten &#xfc;ber alle Einheiten erhoben. Beispielsweise wird eine bestimmte Anzahl von Schulen in einer Stadt zuf&#xe4;llig ausgew&#xe4;hlt, um dann alle Sch&#xfc;ler an den jeweiligen Schulen in die Stichprobe aufzunehmen.</skos:definition>
      <skos:prefLabel xml:lang="fr">Probabiliste : grappe : al&#xe9;atoire simple</skos:prefLabel>
      <skos:definition xml:lang="fr">La population cible est divis&#xe9;e dans des segments existants naturellement (grappes) et un &#xe9;chantillon probabiliste de groupes est s&#xe9;lectionn&#xe9;. Des donn&#xe9;es sont alors collect&#xe9;s &#xe0; partir de tous les unit&#xe9;s dans chaque groupe s&#xe9;lectionn&#xe9;. Par exemple, pour un &#xe9;chantillon d&apos;&#xe9;l&#xe8;ves d&apos;une ville, un nombre d&apos;&#xe9;coles devrait &#xea;tre choisi en utilisant une m&#xe9;thode de s&#xe9;lection al&#xe9;atoire, et puis tous les &#xe9;l&#xe8;ves de chaque &#xe9;cole &#xe9;chantillonn&#xe9;e seraient inclus.</skos:definition>
      <skos:prefLabel xml:lang="nl">Aselecte clusterkanssteekproef</skos:prefLabel>
      <skos:definition xml:lang="nl"></skos:definition>
      <skos:prefLabel xml:lang="no">Sannsynlighetsutvalg: Klynge: Enkelt tilfeldig</skos:prefLabel>
      <skos:definition xml:lang="no">M&#xe5;lpopulasjonen er delt i naturlige grupper (kluster) og et enkelt tilfeldig utvalg av klusterne blir valgt. Data blir deretter samlet inn fra alle enhetene innen hvert utvalgte kluster. For eksempel, for et utvalg av studenter i en by ville f&#xf8;rst et antall skoler bli valgt tilfeldig, og deretter ville alle studentene fra hver utvalgte skole bli inkludert.</skos:definition>
   </rdf:Description>
   <rdf:Description rdf:about="http://rdf-vocabulary.ddialliance.org/cv/SamplingProcedure/2.0.1/49f4571">
      <rdf:type rdf:resource="http://www.w3.org/2004/02/skos/core#Concept"/>
      <skos:inScheme rdf:resource="http://rdf-vocabulary.ddialliance.org/cv/SamplingProcedure/2.0.1/"/>
      <skos:notation xml:lang="en">Probability.Cluster.StratifiedRandom</skos:notation>
      <skos:prefLabel xml:lang="sl">Verjetnostno: po skupinah: stratificirano slu&#x10d;ajno</skos:prefLabel>
      <skos:definition xml:lang="sl">Ciljna populacija je razdeljena na skupine, ki obstajajo same po sebi; te so nato razdeljene na medsebojno izklju&#x10d;ujo&#x10d;e se sloje in naklju&#x10d;ni vzorec skupin je izbran iz vsakega sloja. Podatki se zbirajo na vseh enotah znotraj vsake izbrane skupine. Na primer, za vzorec u&#x10d;encev v mestu bi &#x161;ole razdelili na dva sloja glede na vrsto &#x161;ole (zasebne in javne); &#x161;ole bodo nato slu&#x10d;ajno izbrane iz vsakega sloja in vklju&#x10d;eni bodo vsi u&#x10d;enci iz vsake izbrane &#x161;ole.</skos:definition>
      <skos:prefLabel xml:lang="lt">Tikimybin&#x117;: lizdin&#x117;: sluoksnin&#x117; atsitiktin&#x117;</skos:prefLabel>
      <skos:definition xml:lang="lt">Tikslin&#x117; populiacija yra padalinama &#x12f; nat&#x16b;ralius segmentus (lizdus); tada lizdai yra suskirstomi &#x12f; atskirus ir nepersidengian&#x10d;ius sluoksnius ir atliekama atsitiktin&#x117; j&#x173; atranka kiekviename sluoksnyje. Tada duomenys renkami apie visus atrinkt&#x173; lizd&#x173; vienetus. Pavyzd&#x17e;iui, miesto moksleivi&#x173; im&#x10d;iai sudaryti mokyklos b&#x16b;t&#x173; suskirstytos &#x12f; sluoksnius pagal mokyklos tip&#x105; (privati ar valstybin&#x117;); mokyklos b&#x16b;t&#x173; atsitiktinai atrinktos i&#x161; kiekvieno sluoksnio, o tada &#x12f;traukiami visi atrinkt&#x173; mokykl&#x173; mokiniai.</skos:definition>
      <skos:prefLabel xml:lang="sv">Sannolikhetsurval: klusterurval: stratifierat slumpm&#xe4;ssigt urval</skos:prefLabel>
      <skos:definition xml:lang="sv">M&#xe5;lpopulationen delas in i naturligt f&#xf6;rekommande segment (kluster). Dessa delas sedan upp i &#xf6;msesidigt uteslutande strata och det g&#xf6;rs ett slumpm&#xe4;ssigt urval av kluster inom varje stratum. Data samlas d&#xe4;refter in fr&#xe5;n alla element inom varje utvalt kluster. Exempel: f&#xf6;r att ta fram ett urval av elever i en stad delas skolorna in i tv&#xe5; strata efter typ av skola (kommunala skolor och friskolor). Skolor v&#xe4;ljs sedan slumpm&#xe4;ssigt fr&#xe5;n varje stratum och alla elever i de utvalda skolorna ing&#xe5;r i urvalet.</skos:definition>
      <skos:prefLabel xml:lang="it">Probabilistico: a grappoli stratificato</skos:prefLabel>
      <skos:definition xml:lang="it">La popolazione di riferimento &#xe8; divisa in modo naturale in gruppi (cluster); successivamente, i cluster sono divisi in strati mutualmente esclusivi e, per ogni strato, viene selezionato in modo casuale un campione di cluster. I dati vengono quindi raccolti da tutte le unit&#xe0; individuate all&apos;interno di ciascun cluster. Ad esempio, per selezionare un campione di studenti in una citt&#xe0;, si suddividono le scuole in due strati a seconda del tipo di scuola (privato vs pubblico); le scuole saranno quindi selezionate in modo casuale per ogni strato, e saranno successivamente inclusi tutti gli studenti di ogni scuola selezionata.</skos:definition>
      <skos:prefLabel xml:lang="en">Probability: Cluster: Stratified random</skos:prefLabel>
      <skos:definition xml:lang="en">The target population is divided into naturally occurring segments (clusters); next, these are divided into mutually exclusive strata and a random sample of clusters is selected from each stratum. Data are then collected from all units within each selected cluster. For example, for a sample of students in a city, schools would be divided into two strata by school type (private vs. public); schools would be then randomly selected from each stratum, and all of the students from every sampled school would be included.</skos:definition>
      <skos:prefLabel xml:lang="de">Wahrscheinlichkeitsauswahl: Geschichtete Klumpenauswahl</skos:prefLabel>
      <skos:definition xml:lang="de">Die Grundgesamtheit wird in nat&#xfc;rlich auftretende Gruppen (Cluster) unterteilt. Diese Gruppen werden in sich gegenseitig ausschlie&#xdf;ende und insgesamt ersch&#xf6;pfende Schichten unterteilt. Aus diesen wird dann eine bestimmte Anzahl an Gruppen zuf&#xe4;llig ausgew&#xe4;hlt. Beispielsweise werden Schulen nach privaten und &#xf6;ffentlichen unterschieden, um dann aus diesen beiden Gruppen per Zufall Schulen auszuw&#xe4;hlen und alle Sch&#xfc;ler der ausgew&#xe4;hlten Schulen in die Stichprobe aufzunehmen.</skos:definition>
      <skos:prefLabel xml:lang="fr">Probabiliste : grappe : al&#xe9;atoire stratifi&#xe9;</skos:prefLabel>
      <skos:definition xml:lang="fr">La population cible est divis&#xe9;e dans des segments existants naturellement (grappes) ; Ensuite, ceux-ci sont divis&#xe9;s dans des strates mutuellement exclusives et un &#xe9;chantillon al&#xe9;atoire des groupes est s&#xe9;lectionn&#xe9; depuis chaque strate. Les donn&#xe9;es sont alors collect&#xe9;es depuis toutes les unit&#xe9;s au sein de chaque groupe. Par exemple, pour un &#xe9;chantillon d&apos;&#xe9;l&#xe8;ves d&apos;une ville, les &#xe9;coles seraient divis&#xe9;es en deux strates par type d&apos;&#xe9;cole (priv&#xe9;e vs. public) ; Les &#xe9;coles seraient alors s&#xe9;lectionn&#xe9;es al&#xe9;atoirement depuis chaque strate, et tous les &#xe9;l&#xe8;ves de chaque &#xe9;cole &#xe9;chantillonn&#xe9;e seraient inclus.</skos:definition>
      <skos:prefLabel xml:lang="nl">Gestratificeerde clusterkanssteekproef</skos:prefLabel>
      <skos:definition xml:lang="nl"></skos:definition>
      <skos:prefLabel xml:lang="no">Sannsynlighetsutvalg: Klynge: Stratifisert tilfeldig</skos:prefLabel>
      <skos:definition xml:lang="no">M&#xe5;lpopulasjonen er delt i naturlige grupper (kluster). Disse blir igjen delt i gjensidig utelukkende i strata og et tilfeldig utvalg av klustre blir valgt fra hvert stratum. Data blir deretter samlet inn fra alle enhetene i hvert utvalgte kluster. For eksempel for et utvalg av studenter i en by ville skolene bli delt i to strata ut fra type skole (privat vs.offentlig). Skoler blir deretter tilfeldig trukket fra hver stratum og alle studentene fra hver utvalgte skole ville bli inkluidert i utvalget.</skos:definition>
   </rdf:Description>
   <rdf:Description rdf:about="http://rdf-vocabulary.ddialliance.org/cv/SamplingProcedure/2.0.1/f91d8ca">
      <rdf:type rdf:resource="http://www.w3.org/2004/02/skos/core#Concept"/>
      <skos:inScheme rdf:resource="http://rdf-vocabulary.ddialliance.org/cv/SamplingProcedure/2.0.1/"/>
      <skos:notation xml:lang="en">Probability.Multistage</skos:notation>
      <skos:prefLabel xml:lang="sl">Verjetnostno: ve&#x10d;stopenjsko</skos:prefLabel>
      <skos:definition xml:lang="sl">Vzor&#x10d;enje se izvaja stopenjsko z vklju&#x10d;itvijo vedno manj&#x161;ega &#x161;tevila enot na vsaki stopnji, vse stopnje vklju&#x10d;ujejo verjetnostno izbiro. Vrsta postopka verjetnostnega vzor&#x10d;enja je lahko razli&#x10d;na na vsaki stopnji. Na primer, za vzorec u&#x10d;encev v mestu najprej na prvi stopnji slu&#x10d;ajno izberemo &#x161;ole. Na drugi stopnji poteka izbor slu&#x10d;ajnega vzorca razredov v vsaki izmed izbranih &#x161;ol. Na tretji stopnji nato slu&#x10d;ajno izberemo u&#x10d;ence iz vsakega od izbranih razredov.</skos:definition>
      <skos:prefLabel xml:lang="lt">Tikimybin&#x117;: daugiapakop&#x117;</skos:prefLabel>
      <skos:definition xml:lang="lt">Imtis sudaroma etapais kiekviename etape naudojant vis ma&#x17e;esnius vienetus, ir visuose etapuose taikoma tikimybin&#x117; atranka. Tikimybin&#x117;s atrankos proced&#x16b;ra kiekviename etape gali b&#x16b;ti skirtinga. Pavyzd&#x17e;iui, miesto moksleivi&#x173; imties sudarymo pirmajame etape, mokyklos atrenkamos atsitiktinai. Antrajame etape atliekama paprastoji atsitiktin&#x117; klasi&#x173; atranka i&#x161; kiekvienos parinktos mokyklos. Tuomet tre&#x10d;iajame etape i&#x161; kiekvienos atrinktos klas&#x117;s atsitiktinai parenkami mokiniai.</skos:definition>
      <skos:prefLabel xml:lang="sv">Sannolikhetsurval: flerstegsurval</skos:prefLabel>
      <skos:definition xml:lang="sv">Urvalet sker stegvis med allt mindre enheter f&#xf6;r varje steg, och varje steg omfattar ett sannolikhetsurval. Urvalsmetoden kan skilja sig fr&#xe5;n steg till steg. Exempel: f&#xf6;r att ta fram ett urval av elever i en stad v&#xe4;ljs skolor slumpm&#xe4;ssigt i f&#xf6;rsta steget. I ett andra steg g&#xf6;rs ett slumpm&#xe4;ssigt urval av klasser i varje vald skola. Elever v&#xe4;ljs sedan slumpm&#xe4;ssigt fr&#xe5;n dessa klasser i ett tredje steg.</skos:definition>
      <skos:prefLabel xml:lang="it">Probabilistico: multistadio</skos:prefLabel>
      <skos:definition xml:lang="it">Il campionamento viene eseguito in differenti stadi, utilizzando unit&#xe0; sempre pi&#xf9; piccole in ogni stadio. Tutti gli stadi implicano un campionamento probabilistico che pu&#xf2; essere diverso in ogni stadio. Ad esempio, per selezionare un campione di studenti in una citt&#xe0;, nel primo stadio si selezionano in modo casuale le scuole. Nel secondo stadio si effettua un campione casuale di classi all&apos;interno di ciascuna scuola selezionata. Nel terzo stadio, infine, vengono selezionati in modo casuale gli studenti da ciascuna delle classi identificate.</skos:definition>
      <skos:prefLabel xml:lang="en">Probability: Multistage</skos:prefLabel>
      <skos:definition xml:lang="en">Sampling is carried out in stages using smaller and smaller units at each stage, and all stages involve a probability selection. The type of probability sampling procedure may be different at each stage. For example, for a sample of students in a city, schools are randomly selected in the first stage. A random sample of classes within each selected school is drawn in the second stage. Students are then randomly selected from each of these classes in the third stage.</skos:definition>
      <skos:prefLabel xml:lang="de">Wahrscheinlichkeitsauswahl: Mehrstufige Zufallsauswahl</skos:prefLabel>
      <skos:definition xml:lang="de">Bei der mehrstufigen Zufallsauswahl wird eine Zufallsauswahl bestimmter Einheiten getroffen, aus denen dann jeweils zuf&#xe4;llig die n&#xe4;chstkleinere Einheit gezogen wird. Die Art der Zufallsauswahl kann dabei zwischen den Stufen variieren. F&#xfc;r eine Stichprobe von Sch&#xfc;lern werden beispielsweise zuf&#xe4;llig Schulen in einer Stadt ausgew&#xe4;hlt. Aus den Schulen werden im n&#xe4;chsten Schritt jeweils mehrere Klassen gezogen, um dann eine bestimmte Anzahl von Sch&#xfc;lern aus diesen Klassen zuf&#xe4;llig auszuw&#xe4;hlen, die zur Teilnahme an der Studie eingeladen werden.</skos:definition>
      <skos:prefLabel xml:lang="fr">Probabiliste : multi-&#xe9;tapes</skos:prefLabel>
      <skos:definition xml:lang="fr">L&apos;&#xe9;chantillonnage est effectu&#xe9; par &#xe9;tapes en utilisant des unit&#xe9;s plus en plus petites &#xe0; chaque &#xe9;tape, et toutes les &#xe9;tapes impliquent une s&#xe9;lection al&#xe9;atoire. Le type de proc&#xe9;dure d&apos;&#xe9;chantillonnage al&#xe9;atoire peut &#xea;tre diff&#xe9;rent &#xe0; chaque &#xe9;tape. Par exemple, pour un &#xe9;chantillon d&apos;&#xe9;l&#xe8;ves d&apos;une ville, les &#xe9;coles sont s&#xe9;lectionn&#xe9;es al&#xe9;atoirement dans une premi&#xe8;re &#xe9;tape. Un &#xe9;chantillon al&#xe9;atoire de classes des &#xe9;coles s&#xe9;lectionn&#xe9;es est tir&#xe9; dans une deuxi&#xe8;me &#xe9;tape. Les &#xe9;l&#xe8;ves sont alors s&#xe9;lectionn&#xe9;s al&#xe9;atoirement depuis chacune de ces classes dans une troisi&#xe8;me &#xe9;tape.</skos:definition>
      <skos:prefLabel xml:lang="nl">Meertraps steekproef</skos:prefLabel>
      <skos:definition xml:lang="nl"></skos:definition>
      <skos:prefLabel xml:lang="no">Sannsynlighetsutvalg: Flertrinns</skos:prefLabel>
      <skos:definition xml:lang="no">Utvelgelsen skjer trinnvis ved bruk av mindre og mindre enheter for hvert trinn, og hvert trinn omfatter et sannsynlighetsutvalg. Typen sannsynlighetsutvalg kan variere p&#xe5; hvert trinn. For eksempel for &#xe5; f&#xe5; et utvalg studenter i en by blir skolene trukket tilfeldig i f&#xf8;rste steg. Et tilfeldig utvalg av klasser innen hver utvalgte skole blir trukket i neste steg. Studentene blir deretter tilfeldig trukket fra hver av disse klassene p&#xe5; tredje trinn.</skos:definition>
   </rdf:Description>
   <rdf:Description rdf:about="http://rdf-vocabulary.ddialliance.org/cv/SamplingProcedure/2.0.1/540b3b2">
      <rdf:type rdf:resource="http://www.w3.org/2004/02/skos/core#Concept"/>
      <skos:inScheme rdf:resource="http://rdf-vocabulary.ddialliance.org/cv/SamplingProcedure/2.0.1/"/>
      <skos:notation xml:lang="en">TheoreticalSampling</skos:notation>
      <skos:prefLabel xml:lang="sl">Teoreti&#x10d;no vzor&#x10d;enje</skos:prefLabel>
      <skos:definition xml:lang="sl">Teoreti&#x10d;no vzor&#x10d;enje je iterativna tehnika vzor&#x10d;enja, povezana s pristopom utemeljene teorije (grounded theory), ki temelji na analiti&#x10d;ni indukciji. Od drugih metod vzor&#x10d;enja se razlikuje po tem, da je njen namen ustvarjanje in razvijanje teorij, ne pa preverjanje hipotez ali zagotavljanje reprezentativnosti dolo&#x10d;ene populacije. Pri teoreti&#x10d;nem vzor&#x10d;enju potekajo zbiranje podatkov, kodiranje in analiza hkrati in ponavljajo&#x10d;e &#x2013; ne kot lo&#x10d;eni, zaporedni koraki. Ni vnaprej dolo&#x10d;enega na&#x10d;rta, koga vklju&#x10d;iti v raziskavo, niti vnaprej dolo&#x10d;enih skupin, ki bi jih primerjali. Namesto tega se udele&#x17e;enci raziskave po za&#x10d;etnem zbiranju in analizi podatkov izbirajo glede na njihov potencial, da prispevajo k razvoju nastajajo&#x10d;ih konceptov in tem. Tak pristop raziskovalcem omogo&#x10d;a, da raziskovalno vpra&#x161;anje in teorijo sproti prilagajajo glede na zbrane podatke, namesto da bi sku&#x161;ali podatke prilagoditi vnaprej oblikovani ideji.</skos:definition>
      <skos:prefLabel xml:lang="lt">Teorin&#x117; atranka</skos:prefLabel>
      <skos:definition xml:lang="lt">Teorin&#x117; atranka &#x2013; tai iteracinis atrankos metodas, susij&#x119;s su pagr&#x12f;stosios teorijos prieiga, grind&#x17e;iama analitine indukcija. Nuo kit&#x173; atrankos metod&#x173; ji skiriasi tuo, kad ja siekiama kurti ir pl&#x117;toti teorijas, o ne tikrinti hipotezes ir (arba) reprezentuoti tam tikr&#x105; populiacij&#x105;. Teorin&#x117;s atrankos metu duomen&#x173; rinkimo, kodavimo ir analiz&#x117;s procesai vyksta tuo pa&#x10d;iu metu ir rekursyviai, o ne kaip atskiri, nuosekl&#x16b;s &#x17e;ingsniai. N&#x117;ra i&#x161; anksto nustatyt&#x173; kriterij&#x173;, k&#x105; &#x12f;traukti &#x12f; atrank&#x105;, ar i&#x161; anksto apibr&#x117;&#x17e;to &#x17e;moni&#x173; grupi&#x173; lyginimo. Vietoj to po pirminio duomen&#x173; rinkimo ir analiz&#x117;s etapo tyrimo dalyviai atrenkami atsi&#x17e;velgiant &#x12f; j&#x173; potencial&#x105; prisid&#x117;ti prie besiformuojan&#x10d;i&#x173; s&#x105;vok&#x173; ir tem&#x173; pl&#x117;tojimo. Tokia prieiga leid&#x17e;ia tyr&#x117;jams tikslinti savo tyrimo klausim&#x105; ir teorij&#x105;, remiantis surinktais duomenimis, o ne pritaikyti duomenis i&#x161; anksto suformuluotai id&#x117;jai.</skos:definition>
      <skos:prefLabel xml:lang="sv">Teoretiskt urval</skos:prefLabel>
      <skos:definition xml:lang="sv">Teoretiskt urval &#xe4;r en iterativ urvalsmetod som &#xe4;r besl&#xe4;ktad med forskningsstrategin grundad teori och bygger p&#xe5; analytisk induktion. Den skiljer sig fr&#xe5;n andra urvalsmetoder genom att den handlar om att generera och utveckla teorier, snarare &#xe4;n att testa hypoteser och/eller representera en viss population. Vid teoretiskt urval sker datainsamling, kodning och analys samtidigt och rekursivt, inte som separata steg som f&#xf6;ljer p&#xe5; varandra. Det finns ingen f&#xf6;rutbest&#xe4;md uppfattning om vilka personer som ska rekryteras eller n&#xe5;gra i f&#xf6;rv&#xe4;g definierade grupper som ska j&#xe4;mf&#xf6;ras. Ist&#xe4;llet v&#xe4;ljs deltagare efter en inledande datainsamling och analys utifr&#xe5;n deras potential at bidra till att vidareutveckla framv&#xe4;xande koncept och teman.
Den h&#xe4;r metoden g&#xf6;r det m&#xf6;jligt f&#xf6;r forskare att f&#xf6;rfina sina forskningsfr&#xe5;gor och teorier baserat p&#xe5; insamlade data, ist&#xe4;llet f&#xf6;r att anpassa data efter en f&#xf6;rutbest&#xe4;md id&#xe9;.</skos:definition>
      <skos:prefLabel xml:lang="it">Campionamento teorico</skos:prefLabel>
      <skos:definition xml:lang="it">Il campionamento teorico &#xe8; una tecnica di campionamento iterativa associata all&apos;approccio della grounded theory, basato sull&apos;induzione analitica. Si differenzia dagli altri metodi di campionamento in quanto mira a generare e sviluppare teorie piuttosto che a verificare ipotesi e/o essere rappresentativo di una determinata popolazione. Nel campionamento teorico, il processo di raccolta, codifica e analisi dei dati avviene in modo simultaneo e ricorsivo, e non come fasi discrete che si susseguono l&apos;una dopo l&apos;altra. Non esiste un&apos;idea prestabilita di chi reclutare, n&#xe9; gruppi predeterminati di persone da confrontare. Al contrario, dopo una prima fase di raccolta e analisi dei dati, i partecipanti allo studio vengono selezionati in base al loro potenziale contributo allo sviluppo dei concetti e dei temi emergenti. Questo approccio consente ai ricercatori di affinare la loro domanda di ricerca e la loro teoria sulla base dei dati raccolti, piuttosto che forzare i dati per adattarli a un&apos;idea preconcetta.</skos:definition>
      <skos:prefLabel xml:lang="en">Theoretical Sampling</skos:prefLabel>
      <skos:definition xml:lang="en">Theoretical sampling is an iterative sampling technique associated with the grounded theory approach based on analytic induction. It differs from other sampling methods by being aimed at generating and developing theories rather than testing hypotheses and/or being representative of a certain population.
In theoretical sampling, the process of collecting data, coding, and analyzing it, happens simultaneously and recursively, and not as discrete steps that lead to one another. There is no pre-set notion of who to recruit, or any predetermined groups of people to compare. Instead, after an initial round of data collection and analysis, study participants are selected based on their potential to contribute to developing the emerging concepts and themes. This approach allows researchers to refine their research question and theory based on the data they collect rather than forcing their data to fit a preconceived idea.</skos:definition>
      <skos:prefLabel xml:lang="de">Theoretische Stichprobenziehung</skos:prefLabel>
      <skos:definition xml:lang="de">Theoretische Stichprobenziehung ist eine iterative Stichprobentechnik, die mit dem qualitativen Ansatz der Grounded Theory verbunden ist. Das Verfahren unterscheidet sich von anderen Stichprobenverfahren dadurch, dass es eher auf die Entwicklung von Theorien als auf die Pr&#xfc;fung von Hypothesen und/oder die Repr&#xe4;sentativit&#xe4;t f&#xfc;r eine bestimmte Population abzielt. Bei der theoretischen Stichprobenziehung erfolgt der Prozess der Datenerhebung, der Kodierung und der Analyse der Daten gleichzeitig und rekursiv und nicht als abgegrenzte Schritte, die zueinander f&#xfc;hren. Es gibt keine im Voraus festgelegte Vorstellung davon, wer rekrutiert werden soll, und es gibt auch keine vorher festgelegten Gruppen von Personen, die verglichen werden sollen. Stattdessen werden die Studienteilnehmer*innen nach einer ersten Runde der Datenerfassung und -analyse auf der Grundlage ihres Potenzials ausgew&#xe4;hlt, zur Entwicklung der entstehenden Konzepte und Themen beizutragen. Dieser Ansatz soll es Forschenden erm&#xf6;glichen, ihre Forschungsfrage und ihre Theorie auf der Grundlage der gesammelten Daten zu verfeinern.</skos:definition>
      <skos:prefLabel xml:lang="fr">&#xc9;chantillonnage th&#xe9;orique</skos:prefLabel>
      <skos:definition xml:lang="fr">L&apos;&#xe9;chantillonnage th&#xe9;orique est une technique it&#xe9;rative d&apos;&#xe9;chantillonnage associ&#xe9;e &#xe0; la th&#xe9;orie ancr&#xe9;e et bas&#xe9;e sur l&apos;induction analytique. Il diff&#xe8;re des autres m&#xe9;thodes d&apos;&#xe9;chantillonnage en ce qu&apos;il vise &#xe0; g&#xe9;n&#xe9;rer et &#xe0; d&#xe9;velopper des th&#xe9;ories plut&#xf4;t qu&apos;&#xe0; tester des hypoth&#xe8;ses et/ou &#xe0; &#xea;tre repr&#xe9;sentatif d&apos;une certaine population. Dans l&apos;&#xe9;chantillonnage th&#xe9;orique, les processus de collecte, de codage et d&apos;analyse des donn&#xe9;es se d&#xe9;roulent de mani&#xe8;re simultan&#xe9;e et r&#xe9;cursive, et non pas comme des &#xe9;tapes distinctes qui se succ&#xe8;dent. Il n&apos;y a pas de notion pr&#xe9;&#xe9;tablie quant aux personnes &#xe0; recruter, ni de groupes pr&#xe9;d&#xe9;termin&#xe9;s &#xe0; comparer. Au contraire, apr&#xe8;s une premi&#xe8;re phase de collecte et d&apos;analyse des donn&#xe9;es, les participants &#xe0; l&apos;&#xe9;tude sont s&#xe9;lectionn&#xe9;s en fonction de leur potentiel &#xe0; contribuer au d&#xe9;veloppement des concepts et th&#xe8;mes &#xe9;mergents. Cette approche permet aux chercheurs et chercheuses d&apos;affiner leur question de recherche et leur th&#xe9;orie en fonction des donn&#xe9;es qu&apos;ils collectent, plut&#xf4;t que de forcer leurs donn&#xe9;es &#xe0; s&apos;adapter &#xe0; une id&#xe9;e pr&#xe9;con&#xe7;ue.</skos:definition>
      <skos:prefLabel xml:lang="nl">Theoretische steekproef</skos:prefLabel>
      <skos:definition xml:lang="nl"></skos:definition>
      <skos:prefLabel xml:lang="no">Teoretisk utvalg</skos:prefLabel>
      <skos:definition xml:lang="no">Teoretisk utvalg er en iterativ utvalgsmetode knyttet til grounded theory-tiln&#xe6;rmingen basert p&#xe5; analytisk induksjon. Den skiller seg fra andre utvalgsmetoder ved &#xe5; v&#xe6;re rettet mot &#xe5; generere og utvikle teorier snarere enn &#xe5; teste hypoteser og/eller v&#xe6;re representativ for en bestemt befolkning. I teoretisk utvalg skjer prosessen med &#xe5; samle inn data, koding og analyse samtidig og gjentakende, og ikke som separate trinn som leder til hverandre. Det er ingen forh&#xe5;ndsbestemt id&#xe9; om hvem som skal rekrutteres, eller noen forh&#xe5;ndsbestemte grupper av mennesker &#xe5; sammenligne. I stedet, etter en innledende runde med datainnsamling og analyse, velges studiedeltakere basert p&#xe5; deres potensial til &#xe5; bidra til utviklingen av de fremvoksende konseptene og temaene. Denne tiln&#xe6;rmingen gj&#xf8;r det mulig for forskere &#xe5; finjustere sitt forskningssp&#xf8;rsm&#xe5;l og teori basert p&#xe5; dataene de samler inn, i stedet for &#xe5; tvinge dataene til &#xe5; passe inn i en forh&#xe5;ndsbestemt id&#xe9;.</skos:definition>
   </rdf:Description>
   <rdf:Description rdf:about="http://rdf-vocabulary.ddialliance.org/cv/SamplingProcedure/2.0.1/4d8364f">
      <rdf:type rdf:resource="http://www.w3.org/2004/02/skos/core#Concept"/>
      <skos:inScheme rdf:resource="http://rdf-vocabulary.ddialliance.org/cv/SamplingProcedure/2.0.1/"/>
      <skos:notation xml:lang="en">Nonprobability</skos:notation>
      <skos:prefLabel xml:lang="sl">Neverjetnostno</skos:prefLabel>
      <skos:definition xml:lang="sl">Izbor enot (posameznikov, gospodinjstev, organizacij itd.) iz ciljne populacije ne temelji na slu&#x10d;ajnem izboru. Verjetnosti, da bo posamezni element vklju&#x10d;en v vzorec, ni mogo&#x10d;e dolo&#x10d;iti. Uporabite ta &#x161;ir&#x161;i izraz, &#x10d;e dolo&#x10d;ena vrsta neverjetnostnega vzor&#x10d;enja ni znana, jo je te&#x17e;ko dolo&#x10d;iti ali &#x10d;e uporabljate ve&#x10d; metod neverjetnostnega vzor&#x10d;enja.</skos:definition>
      <skos:prefLabel xml:lang="lt">Netikimybin&#x117;</skos:prefLabel>
      <skos:definition xml:lang="lt">Imties vienet&#x173; (individ&#x173;, nam&#x173; &#x16b;ki&#x173;, organizacij&#x173; ir kt.) atrinkimas i&#x161; tikslin&#x117;s populiacijos n&#x117;ra grind&#x17e;iamas atsitiktine atranka. Ne&#x12f;manoma nustatyti kiekvieno elemento tikimyb&#x117;s patekti &#x12f; imt&#x12f;. Naudoti &#x161;&#x12f; platesn&#x12f; termin&#x105;, kai ne&#x17e;inomas konkretesnis netikimybin&#x117;s atrankos tipas arba j&#x12f; sunku nustatyti, ar jei naudojami keli netikimybiniai metodai.</skos:definition>
      <skos:prefLabel xml:lang="sv">Icke-sannolikhetsurval</skos:prefLabel>
      <skos:definition xml:lang="sv">Urvalet av element (individer, hush&#xe5;ll, organisationer m.m.) fr&#xe5;n m&#xe5;lpopulationen g&#xf6;rs inte slumpm&#xe4;ssigt. Det g&#xe5;r inte att fastst&#xe4;lla sannolikheten f&#xf6;r att varje element ska tas med i urvalet. Anv&#xe4;nd den h&#xe4;r bredare termen om det &#xe4;r ok&#xe4;nt vilken mer specifik typ av icke-sannolikhetsurval det r&#xf6;r sig om, om typen &#xe4;r sv&#xe5;r att identifiera, eller om flera metoder f&#xf6;r icke-sannolikhetsurval anv&#xe4;nds.</skos:definition>
      <skos:prefLabel xml:lang="it">Non probabilistico</skos:prefLabel>
      <skos:definition xml:lang="it">La selezione delle unit&#xe0; (individui, famiglie, organizzazioni, ecc.) della popolazione di riferimento non &#xe8; basata su un campionamento casuale. Non &#xe8; quindi possibile determinare la probabilit&#xe0; di ciascun elemento di essere incluso nel campione. Utilizzare questo termine pi&#xf9; ampio se non &#xe8; conosciuto oppure &#xe8; difficile identificare il tipo specifico di campionamento non probabilistico, oppure se si utilizzano pi&#xf9; metodi non probabilistici.</skos:definition>
      <skos:prefLabel xml:lang="en">Non-probability</skos:prefLabel>
      <skos:definition xml:lang="en">The selection of units (individuals, households, organizations, etc.) from the target population is not based on random selection. It is not possible to determine the probability of each element to be sampled. Use this broader term if the specific type of non-probability is not known, difficult to identify, or if multiple non-probability methods are being employed.</skos:definition>
      <skos:prefLabel xml:lang="de">Nicht-Wahrscheinlichkeitsauswahl</skos:prefLabel>
      <skos:definition xml:lang="de">Die Auswahl von Einheiten (z. B. Individuen, Haushalte, Organisationen, usw.) aus der Grundgesamtheit erfolgt nicht nach dem Zufallsprinzip. Die Auswahlwahrscheinlichkeit der einzelnen Einheiten kann daher nicht ermittelt werden. W&#xe4;hlen Sie diese Kategorie, wenn die genaue Art der Nicht-Wahrscheinlichkeitsauswahl unbekannt, schwierig zu bestimmen ist oder mehrere Arten der Nicht-Wahrscheinlichkeitsauswahl angewendet werden.</skos:definition>
      <skos:prefLabel xml:lang="fr">Non probabiliste</skos:prefLabel>
      <skos:definition xml:lang="fr">La s&#xe9;lection des unit&#xe9;s (individus, m&#xe9;nages, organisations, etc.) depuis la population cible n&apos;est pas bas&#xe9; sur une s&#xe9;lection al&#xe9;atoire. Il n&apos;est pas possible de d&#xe9;terminer la probabilit&#xe9; de chaque &#xe9;l&#xe9;ment d&apos;&#xea;tre &#xe9;chantillonn&#xe9;. Utilisez ce terme si le type sp&#xe9;cifique d&apos;&#xe9;chantillonnage non probabiliste n&apos;est pas connu, difficile &#xe0; identifier, ou si de multiples m&#xe9;thodes non probabilistes ont &#xe9;t&#xe9; employ&#xe9;es.</skos:definition>
      <skos:prefLabel xml:lang="nl">Niet-kanssteekproef</skos:prefLabel>
      <skos:definition xml:lang="nl"></skos:definition>
      <skos:prefLabel xml:lang="no">Ikke-sannsynlighet</skos:prefLabel>
      <skos:definition xml:lang="no">Valget av enheter (individer, husholdninger, organisasjoner etc.) fra m&#xe5;lpopulasjonen blir ikke trukket basert p&#xe5; tilfeldig utvalg. Det er ikke mulig &#xe5; bestemme sannsynligheten for at hver enhet blir inkludert i utvalget. Bruksmerknad: Dette bredere begrepet benyttes dersom det er ukjent hvilken mer spesifikk type ikke-sannsynlighetsutvalg det omhandler, dersom typen er vanskelig &#xe5; identifisere, eller om flere metoder for ikke-sannsynlighetsutvalg benyttes.</skos:definition>
      <skos:narrower rdf:resource="http://rdf-vocabulary.ddialliance.org/cv/SamplingProcedure/2.0.1/90cbfe9"/>
      <skos:narrower rdf:resource="http://rdf-vocabulary.ddialliance.org/cv/SamplingProcedure/2.0.1/45d8ec9"/>
      <skos:narrower rdf:resource="http://rdf-vocabulary.ddialliance.org/cv/SamplingProcedure/2.0.1/f620230"/>
      <skos:narrower rdf:resource="http://rdf-vocabulary.ddialliance.org/cv/SamplingProcedure/2.0.1/086e080"/>
   </rdf:Description>
   <rdf:Description rdf:about="http://rdf-vocabulary.ddialliance.org/cv/SamplingProcedure/2.0.1/90cbfe9">
      <rdf:type rdf:resource="http://www.w3.org/2004/02/skos/core#Concept"/>
      <skos:inScheme rdf:resource="http://rdf-vocabulary.ddialliance.org/cv/SamplingProcedure/2.0.1/"/>
      <skos:notation xml:lang="en">Nonprobability.Availability</skos:notation>
      <skos:prefLabel xml:lang="sl">Neverjetnostno: prilo&#x17e;nostno</skos:prefLabel>
      <skos:definition xml:lang="sl">Izbira vzorca temelji na dostopnosti enot/relativni enostavnosti dostopa. Morda so enote dostopnej&#x161;e oziroma se same odlo&#x10d;ijo za sodelovanje v raziskavi (samoizbira). Raziskovalci imajo lahko v mislih dolo&#x10d;ene ciljne skupine, vendar ne nadzirajo mehanizmov izbire v vzorec. Na primer, pristopimo do &#x161;tudentov, ki zapustijo dolo&#x10d;eno stavbo v &#x161;tudentskem naselju; prosamezniki se prostovoljno odlo&#x10d;ijo za sodelovanje kot odgovor na vabilo, ki ni bilo naslovljeno posebej nanje, temve&#x10d; na &#x161;ir&#x161;o skupino, ki ji morda pripadajo. Imenujemo ga lahko tudi &quot;prilo&#x17e;nostno&quot; vzor&#x10d;enje.</skos:definition>
      <skos:prefLabel xml:lang="lt">Netikimybin&#x117;: patogioji</skos:prefLabel>
      <skos:definition xml:lang="lt">Imties vienet&#x173; atranka grind&#x17e;iama j&#x173; prieinamumu arba tuo, kad jie santykinai lengvai pasiekiami. Jie gali b&#x16b;ti lengvai prieinami arba patys pasirenka dalyvauti tyrime (patys save atrenka). Tyr&#x117;jai gali b&#x16b;ti numat&#x119; tam tikras tikslines grupes, ta&#x10d;iau jie nekontroliuoja atrankos mechanizmo. Pavyzd&#x17e;iui, gali b&#x16b;ti kreipiamasi &#x12f; studentus, i&#x161;einan&#x10d;ius i&#x161; tam tikro pastato universiteto miestelyje; arba asmenys &#x12f; imt&#x12f; gali &#x12f;sitraukti savanori&#x161;kai, gav&#x119; kvietim&#x105;, kuris yra adresuotas didesnei grupei, o ne jiems konkre&#x10d;iai. Taip pat &#x161;i atranka vadinama &#x201e;progine&#x201c; atranka.</skos:definition>
      <skos:prefLabel xml:lang="sv">Icke-sannolikhetsurval: tillg&#xe4;nglighetsurval</skos:prefLabel>
      <skos:definition xml:lang="sv">Urvalet baseras p&#xe5; hur (relativt) l&#xe4;ttillg&#xe4;ngliga elementen &#xe4;r. Det kan handla om att de &#xe4;r enkla att komma i kontakt med eller kan sj&#xe4;lva ha valt att delta i studien (sj&#xe4;lvurval eller sj&#xe4;lvselektion). Forskare kan ha vissa m&#xe5;lgrupper i &#xe5;tanke men har inte kontroll &#xf6;ver sj&#xe4;lva urvalsmekanismen. Exempel: studenter som g&#xe5;r ut fr&#xe5;n en viss byggnad p&#xe5; universitetsomr&#xe5;det blir tillfr&#xe5;gade, eller personer anm&#xe4;ler sig sj&#xe4;lvmant efter att ha tagit del av en inbjudan som inte riktat sig specifikt till dem, utan till en st&#xf6;rre grupp som de kanske tillh&#xf6;r. Kallas &#xe4;ven f&#xf6;r &quot;bekv&#xe4;mlighetsurval&quot; eller &quot;m&#xf6;jlighetsurval&quot;.</skos:definition>
      <skos:prefLabel xml:lang="it">Non probabilistico: di disponibilit&#xe0;</skos:prefLabel>
      <skos:definition xml:lang="it">La selezione del campione si basa sull&apos;accessibilit&#xe0; o relativa facilit&#xe0; di accesso delle unit&#xe0;. Le unit&#xe0; possono essere facilmente contattabili oppure possono scegliere autonomamente di partecipare allo studio (auto-selezione). I ricercatori possono aver immaginato determinati gruppi target, ma non controllano il meccanismo di selezione del campione. Ad esempio, il campione pu&#xf2; essere composto da studenti contattati all&apos;uscita di un determinato edificio del campus universitario oppure da individui che si offrono volontariamente di partecipare allo studio in risposta ad inviti non rivolti specificamente a loro, ma ad un gruppo pi&#xf9; ampio a cui possono appartenere. Questo campionamento &#xe8; anche denominato &quot;di convenienza&quot; o &quot;di opportunit&#xe0;&quot;.</skos:definition>
      <skos:prefLabel xml:lang="en">Non-probability: Availability</skos:prefLabel>
      <skos:definition xml:lang="en">The sample selection is based on the units&apos; accessibility/relative ease of access. They may be easy to approach, or may themselves choose to participate in the study (self-selection). Researchers may have particular target groups in mind but they do not control the sample selection mechanism. For example, students leaving a particular building on campus may be approached, or individuals may volunteer to participate in response to invitations that do not target them specifically, but a larger group to which they may belong. Also called &quot;convenience&quot; or &quot;opportunity&quot; sampling.</skos:definition>
      <skos:prefLabel xml:lang="de">Nicht-Wahrscheinlichkeitsauswahl: Willk&#xfc;rliche Auswahl</skos:prefLabel>
      <skos:definition xml:lang="de">Die Auswahl der Einheiten h&#xe4;ngt von deren relativer Verf&#xfc;gbarkeit ab. Das hei&#xdf;t, es werden Einheiten gew&#xe4;hlt, die einfach erreichbar sind oder aufgrund bestimmter Merkmale oder Verhaltensweisen eher auf die Studie aufmerksam werden (Selbstselektion). Der Forscher kann eine bestimmte Zielgruppe anstreben, die Auswahlmechanismen einer Stichprobe aber nicht kontrollieren. Beispielsweise werden Studierende, die ein bestimmtes Geb&#xe4;ude der Universit&#xe4;t verlassen, angesprochen und eingeladen, an der Studie teilzunehmen. Oder es werden allgemeine Einladungen, die sich an gr&#xf6;&#xdf;ere Gruppen richten, ausgesprochen und jede Person, die sich daraufhin meldet, ist Teil der Auswahl. Man nennt diese willk&#xfc;rliche Auswahl auch Convenience Sample oder Gelegenheitsstichprobe.</skos:definition>
      <skos:prefLabel xml:lang="fr">Non probabiliste : disponibilit&#xe9;</skos:prefLabel>
      <skos:definition xml:lang="fr">La s&#xe9;lection de l&apos;&#xe9;chantillon est bas&#xe9;e sur la disponibilit&#xe9;, l&apos;acc&#xe8;s relativement facile des unit&#xe9;s. Elles peuvent &#xea;tre facile &#xe0; approcher, ou peuvent elles-m&#xea;mes choisir de participer &#xe0; l&apos;&#xe9;tude (auto-s&#xe9;lection). Les chercheurs peuvent avoir un groupe particulier &#xe0; l&apos;esprit mais ils ne peuvent pas contr&#xf4;ler les m&#xe9;canismes de s&#xe9;lection de l&apos;&#xe9;chantillon. Par exemple, des &#xe9;tudiants vivant dans un b&#xe2;timent particulier du campus peuvent &#xea;tre approch&#xe9;s, ou des individus peuvent volontairement participer en r&#xe9;pondant &#xe0; des invitations qui ne les ciblent pas sp&#xe9;cifiquement, mais un groupe plus large auquel ils peuvent appartenir. Aussi appel&#xe9; &#xe9;chantillonnage de &quot;convenance&quot; ou d&apos;&quot;opportunit&#xe9;&quot;.</skos:definition>
      <skos:prefLabel xml:lang="nl">Gemakssteekproef</skos:prefLabel>
      <skos:definition xml:lang="nl"></skos:definition>
      <skos:prefLabel xml:lang="no">Ikke-sannsynlighet: Tilgjengelighetsutvalg</skos:prefLabel>
      <skos:definition xml:lang="no">Utvalget blir trukket basert p&#xe5; enhetenes tilgjengelighet. Enhetene kan v&#xe6;re lette &#xe5; f&#xe5; tak i, eller kan ha meldt seg selv til &#xe5; delta i studien (selvutvelgelse). Forskere kan ha tanker om &#xe5; inkludere visse m&#xe5;lgrupper, men de kan ikke kontrollere utvalgsmekanismene. For eksempel studenter som g&#xe5;r ut fra en viss bygning p&#xe5; universitetsomr&#xe5;det kan bli kontaktet, eller individer kan frivillig melde seg til &#xe5; delta som svar p&#xe5; en invitasjon som ikke spesifikt var rettet mot dem, men en st&#xf8;rre gruppe som de tilh&#xf8;rer. Blir ogs&#xe5; kalt &apos;bekvemmelighetsutvalg&apos; eller &apos;mulighetsutvalg&apos;.</skos:definition>
   </rdf:Description>
   <rdf:Description rdf:about="http://rdf-vocabulary.ddialliance.org/cv/SamplingProcedure/2.0.1/45d8ec9">
      <rdf:type rdf:resource="http://www.w3.org/2004/02/skos/core#Concept"/>
      <skos:inScheme rdf:resource="http://rdf-vocabulary.ddialliance.org/cv/SamplingProcedure/2.0.1/"/>
      <skos:notation xml:lang="en">Nonprobability.Purposive</skos:notation>
      <skos:prefLabel xml:lang="sl">Neverjetnostno: namensko</skos:prefLabel>
      <skos:definition xml:lang="sl">Vzor&#x10d;ene enote posebej opredelimo, izberemo in stopimo v stik z njimi z namenom pridobivanja informacij o raziskovalni temi. Izbor temelji na razli&#x10d;nih zna&#x10d;ilnostih neodvisnih in/ali odvisnih spremenljivk, ki jih preu&#x10d;ujemo, pri &#x10d;emer se opiramo na presojo raziskovalcev. Avtorji raziskave oziroma poobla&#x161;&#x10d;ene osebe imajo nadzor nad mehanizmom izbore v vzorec, ciljna populacija pa je opredeljena z merili za izbor. Imenujemo ga tudi vzor&#x10d;enje &quot;s presojo&quot;. Na primer, raziskovalec na podro&#x10d;ju zdravstva lahko namerno izbere posameznike, ki so si v ve&#x10d;ini pogledov podobni, z izjemo rezultatov pri raziskovalni temi, ki je lahko dolo&#x10d;ena bolezen. Nekatere vrste namenskega vzor&#x10d;enja so tipi&#x10d;ni/atipi&#x10d;ni primeri, homogena/najve&#x10d;ja varianca, izvedensko ali kriti&#x10d;no vzor&#x10d;enje primerov.</skos:definition>
      <skos:prefLabel xml:lang="lt">Netikimybin&#x117;: tikslin&#x117;</skos:prefLabel>
      <skos:definition xml:lang="lt">Imties vienetai yra specialiai apibr&#x117;&#x17e;iami, parenkami ir su jais susisiekiama, nes jie gali pateikti informacijos tiriama tema. Atranka grind&#x17e;iama tyr&#x117;j&#x173; po&#x17e;i&#x16b;riu svarbiomis tiriam&#x173; nepriklausom&#x173; ir (arba) priklausom&#x173; kintam&#x173;j&#x173; charakteristikomis. Tyrimo autoriai arba j&#x173; &#x12f;galioti asmenys kontroliuoja imties sudarymo mechanizm&#x105;, o tiriamoji visuma yra apibr&#x117;&#x17e;ta pagal atrankos kriterijus. Pavyzd&#x17e;iui, medicinos tyr&#x117;jas gali s&#x105;moningai parinkti asmenis, kurie daugeliu at&#x17e;vilgi&#x173; yra pana&#x161;&#x16b;s, ta&#x10d;iau skiriasi tiriamos temos at&#x17e;vilgiu (pavyzd&#x17e;iui, i&#x161;gijo arba nei&#x161;gijo po specifin&#x117;s ligos). Tarp tikslin&#x117;s atrankos r&#x16b;&#x161;i&#x173; yra tipini&#x173; arba deviantini&#x173; atvej&#x173; atrankos, homogeni&#x161;k&#x173; arba maksimaliai skirting&#x173; atvej&#x173; atrankos, ekspertin&#x117; atranka ar ypating&#x173; atvej&#x173; atranka.</skos:definition>
      <skos:prefLabel xml:lang="sv">Icke-sannolikhetsurval: syftesurval</skos:prefLabel>
      <skos:definition xml:lang="sv">Urvalselement identifieras, v&#xe4;ljs ut och kontaktas specifikt f&#xf6;r den information de kan bidra med kring det aktuella forsknings&#xe4;mnet. Urvalet baseras p&#xe5; olika egenskaper hos de oberoende och/eller beroende variablerna som studeras och bygger p&#xe5; forskarnas bed&#xf6;mning. Studiens upphovspersoner, eller personer med deras godk&#xe4;nnande, har kontroll &#xf6;ver urvalsmekanismen och m&#xe5;lpopulationen definieras utifr&#xe5;n urvalskriterierna. Kallas &#xe4;ven f&#xf6;r &quot;&#xe4;ndam&#xe5;lsenligt urval&quot; eller &quot;bed&#xf6;mningsurval&quot;. 
Exempel: en medicinsk forskare kan medvetet v&#xe4;lja individer som &#xe4;r lika i de flesta avseenden, med undantag f&#xf6;r utfallet i studien, till exempel en viss sjukdom. Exempel p&#xe5; syftesurval inkluderar typfall/avvikande fall, homogen/maximal variation, experturval eller kritiska fall.</skos:definition>
      <skos:prefLabel xml:lang="it">Non probabilistico: mirato</skos:prefLabel>
      <skos:definition xml:lang="it">Le unit&#xe0; campionarie vengono identificate, selezionate e contattate sulla base delle informazioni che possono fornire rispetto al tema di ricerca. La selezione si basa su diverse caratteristiche delle variabili indipendenti e/o dipendenti dello studio, e si fonda sul giudizio dei ricercatori. Gli autori dello studio, o le persone da loro autorizzate, hanno il controllo sul meccanismo di selezione del campione e l&apos;universo &#xe8; definito in relazione ai criteri di selezione. Chiamato anche &quot;campionamento di giudizio&quot;. Ad esempio, un ricercatore in ambito medico pu&#xf2; selezionare intenzionalmente individui che sono simili sotto molti aspetti, tranne che rispetto all&apos;esito relativo al tema di ricerca (ad esempio una malattia specifica). Alcuni tipi di campionamento mirato sono rappresentati dai casi tipici/devianti, variazioni omogenee/variazioni massime, campione esperto oppure casi critici.</skos:definition>
      <skos:prefLabel xml:lang="en">Non-probability: Purposive</skos:prefLabel>
      <skos:definition xml:lang="en">Sample units are specifically identified, selected and contacted for the information they can provide on the researched topic. Selection is based on different characteristics of the independent and/or dependent variables under study, and relies on the researchers&apos; judgement. The study authors, or persons authorized by them have control over the sample selection mechanism and the universe is defined in terms of the selection criteria. Also called &quot;judgement&quot; sampling. For example, a medical researcher may intentionally select individuals who are similar in most respects, except on the outcome of the research topic, which can be a specific disease. Some types of purposive sampling are typical/deviant case, homogeneous/maximum variation, expert, or critical case sampling.</skos:definition>
      <skos:prefLabel xml:lang="de">Nicht-Wahrscheinlichkeitsauswahl: Bewusste Auswahl</skos:prefLabel>
      <skos:definition xml:lang="de">Alle Einheiten der Stichprobe sind bewusst, wegen ihres potenziellen Beitrags zum Untersuchungsgegenstand, ausgew&#xe4;hlt. Die Grundgesamtheit und die Auswahlkriterien richten sich dabei nach den Auspr&#xe4;gungen der unabh&#xe4;ngigen und/oder abh&#xe4;ngigen Variablen der Untersuchung und werden von dem/der Forscher*in festgelegt. Er/Sie oder die f&#xfc;r die Stichprobenziehung autorisierte Person kontrolliert die Auswahl. Beispielsweise werden f&#xfc;r eine medizinische Studie bewusst Personen ausgew&#xe4;hlt, die eine bestimmte Krankheit aufweisen, um diese mit einer Kontrollgruppe zu vergleichen. Verschiedene Varianten sind die Auswahl typischer/abweichender F&#xe4;lle, homogener/heterogener F&#xe4;lle oder kritischer F&#xe4;lle.</skos:definition>
      <skos:prefLabel xml:lang="fr">Non probabiliste : raisonn&#xe9;</skos:prefLabel>
      <skos:definition xml:lang="fr">Les unit&#xe9;s &#xe9;chantillonn&#xe9;es sont sp&#xe9;cifiquement identifi&#xe9;es, s&#xe9;lectionn&#xe9;es et contact&#xe9;es pour les informations qu&apos;elles peuvent fournir sur le th&#xe8;me recherch&#xe9;. La s&#xe9;lection est bas&#xe9;e sur diff&#xe9;rentes caract&#xe9;ristiques de variables ind&#xe9;pendantes et / ou d&#xe9;pendantes &#xe0; l&apos;&#xe9;tude, et repose sur le jugement des chercheurs. Les auteurs de l&apos;&#xe9;tude, ou les personnes autoris&#xe9;es par eux ont le contr&#xf4;le au-del&#xe0; des m&#xe9;canismes de s&#xe9;lection de l&apos;&#xe9;chantillon et l&apos;univers est d&#xe9;fini en termes de crit&#xe8;res de s&#xe9;lection. Aussi appel&#xe9; &#xe9;chantillonnage par &quot;jugement&quot;. Par exemple, un chercheur en m&#xe9;decine peut intentionnellement s&#xe9;lectionner des individus qui sont similaires &#xe0; la plupart des &#xe9;gards, except&#xe9; en ce qui concerne le r&#xe9;sultat du sujet de recherche, qui peut &#xea;tre une maladie sp&#xe9;cifique. Certains types d&apos;&#xe9;chantillonnages raisonn&#xe9;s sont des &#xe9;chantillonnage de cas typiques / d&#xe9;viants, de variation homog&#xe8;ne / maximale, d&apos;experts ou de cas critiques.</skos:definition>
      <skos:prefLabel xml:lang="nl">Doelgerichte steekproef</skos:prefLabel>
      <skos:definition xml:lang="nl"></skos:definition>
      <skos:prefLabel xml:lang="no">Ikke-sannsynlighet: M&#xe5;lrettet utvalg</skos:prefLabel>
      <skos:definition xml:lang="no">Enhetene i utvalget identifiseres spesifikt, velges ut og kontaktes p&#xe5; grunn av informasjonen de kan gi om forskningsemnet som studeres. Utvelgelsen er basert p&#xe5; ulike karakteristikker ved de uavhengige og/eller avhengige variablene som skal studeres, og avhenger av forskerens vurdering. Studiens forfattere, eller andre personer som er gitt tillatelse, kontrollerer utvalgsmekanismene og det definerte universet med hensyn til utvalgskriteriene. Blir ogs&#xe5; kalt &apos;bed&#xf8;mmelsesutvalg&apos;. For eksempel kan en forsker innen medisin med hensikt velge individer som ligner hverandre, med unntak av visse utfall, som en spesifikk sykdom. Noen typer m&#xe5;lrettet utvalg er typiske/avvikende tilfeller, homogene/maksimal variasjon, eksperter, og utvalg av kritiske tilfeller.</skos:definition>
   </rdf:Description>
   <rdf:Description rdf:about="http://rdf-vocabulary.ddialliance.org/cv/SamplingProcedure/2.0.1/f620230">
      <rdf:type rdf:resource="http://www.w3.org/2004/02/skos/core#Concept"/>
      <skos:inScheme rdf:resource="http://rdf-vocabulary.ddialliance.org/cv/SamplingProcedure/2.0.1/"/>
      <skos:notation xml:lang="en">Nonprobability.Quota</skos:notation>
      <skos:prefLabel xml:lang="sl">Neverjetnostno: kvotno</skos:prefLabel>
      <skos:definition xml:lang="sl">Ciljna populacija je razdeljena na lo&#x10d;ene in medsebojno izklju&#x10d;ujo&#x10d;e se odseke v skladu z nekaterimi vnaprej dolo&#x10d;enimi merili za izra&#x10d;une. Porazdelitev meril za izra&#x10d;une (razmerje med spoloma/starostjo/etni&#x10d;no pripadnostjo ali drugimi zna&#x10d;ilnostmi, kot so vera, izobra&#x17e;evanje itd.) naj bi odra&#x17e;ala resni&#x10d;no strukturo ciljne populacije ali strukturo &#x17e;elene preu&#x10d;evane populacije. Iz vsakega odseka se nato vzamejo neverjetnostni vzorci, dokler ni dose&#x17e;eno dolo&#x10d;eno &#x161;tevilo enot. Na primer, &#x10d;e ciljno populacijo sestavlja 45 odstotkov &#x17e;ensk in 55 odstotkov mo&#x161;kih, bo v proporcionalni kvotni vzorec vklju&#x10d;en enak odstotek udele&#x17e;encev glede na spol, medtem ko so v neproporcionalni kvotni vzorec vklju&#x10d;eni razli&#x10d;ni odstotki, ki izhajajo iz razmislekov v povezavi z raziskavo (na primer, nadvzor&#x10d;enje nekaterih manj zastopanih delov populacije).</skos:definition>
      <skos:prefLabel xml:lang="lt">Netikimybin&#x117;: kvotin&#x117;</skos:prefLabel>
      <skos:definition xml:lang="lt">Pagal tam tikrus i&#x161; anksto nustatytus kriterijus (kvotas) tikslin&#x117; populiacija yra padalinama &#x12f; atskirus ir nepersidengian&#x10d;ius segmentus. Paskirstymas pagal kvotas (lyties, am&#x17e;iaus, etnin&#x117;s priklausomyb&#x117;s proporcijas ar kitas savybes, tokias kaip religija, i&#x161;silavinimas ir kt.) turi atspind&#x117;ti reali&#x105; tikslin&#x117;s populiacijos strukt&#x16b;r&#x105; arba norimos tiriamosios populiacijos strukt&#x16b;r&#x105;. Tada kiekviename segmente netikimybin&#x117;s atrankos b&#x16b;du renkami vienetai, kol bus pasiektas pagal kvot&#x105; reikiamas vienet&#x173; skai&#x10d;ius. Pavyzd&#x17e;iui, jei tikslin&#x119; populiacij&#x105; sudaro 45 proc. moter&#x173; ir 55 proc. vyr&#x173;, proporcingoje kvotin&#x117;je imtyje bus toks pats ly&#x10d;i&#x173; procentas, o neproporcingoje kvotin&#x117;je imtyje procentai skirsis priklausomai nuo tyrimo tiksl&#x173; (pavyzd&#x17e;iui, gali b&#x16b;ti siekiama gausesnio tam tikr&#x173; menkai atstovaujam&#x173; gyventoj&#x173; segment&#x173; dalyvavimo).</skos:definition>
      <skos:prefLabel xml:lang="sv">Icke-sannolikhetsurval: kvoturval</skos:prefLabel>
      <skos:definition xml:lang="sv">M&#xe5;lpopulationen delas in i separata och &#xf6;msesidigt uteslutande segment utifr&#xe5;n f&#xf6;rdefinierade kvotkriterier. F&#xf6;rdelningen av dessa kriterier (till exempel kvot efter k&#xf6;n/&#xe5;lder/etnicitet eller andra egenskaper, som religion, utbildning m.m.) &#xe4;r t&#xe4;nkt att spegla strukturen i m&#xe5;lpopulationen eller i den &#xf6;nskade studiepopulationen. Icke-sannolikhetsurval g&#xf6;rs sedan inom varje segment tills ett f&#xf6;rutbest&#xe4;mt antal enheter har n&#xe5;tts. 
Exempel: om m&#xe5;lpopulationen best&#xe5;r av 45 % kvinnor och 55 % m&#xe4;n s&#xe5; kommer ett proportionerligt kvoturval ha samma k&#xf6;nsf&#xf6;rdelning. Ett icke-proportionerligt kvoturval kan d&#xe4;remot ha en annan procentf&#xf6;rdelning, baserat p&#xe5; n&#xe5;gon f&#xf6;r studien relevant faktor (t.ex. behovet att &#xf6;verinkludera vissa underrepresenterade segment av populationen).</skos:definition>
      <skos:prefLabel xml:lang="it">Non probabilistico: per quota</skos:prefLabel>
      <skos:definition xml:lang="it">La popolazione di riferimento &#xe8; suddivisa in segmenti separati e mutuamente esclusivi secondo qualche criterio per quote predefinito. La distribuzione dei criteri di quotazione (genere/et&#xe0;/etnia o altre caratteristiche, come religione, istruzione, ecc.) riflette la reale struttura della popolazione di riferimento o la struttura della popolazione che si intende studiare. I campioni non probabilistici vengono quindi estratti da ciascun segmento fino a raggiungere un numero specifico di unit&#xe0;. Ad esempio, se la popolazione di riferimento &#xe8; composta per il 45% da femmine e per il 55% da maschi, un campione per quota proporzionale avr&#xe0; le stesse percentuali di genere, mentre in un campione per quota non proporzionale le percentuali saranno diverse, sulla base di specifiche considerazioni legate allo studio (ad esempio, la necessit&#xe0; di sovracampionare alcuni segmenti sottorappresentati della popolazione).</skos:definition>
      <skos:prefLabel xml:lang="en">Non-probability: Quota</skos:prefLabel>
      <skos:definition xml:lang="en">The target population is subdivided into separate and mutually exclusive segments according to some predefined quotation criteria. The distribution of the quotation criteria (gender/age/ethnicity ratio, or other characteristics, like religion, education, etc.) is intended to reflect the real structure of the target population or the structure of the desired study population. Non-probability samples are then drawn from each segment until a specific number of units has been reached. For example, if the target population consists of 45 percent females and 55 percent males, a proportional quota sample will have the same gender percentages, while in a non-proportional quota sample the percentages will be different, based on some study-related consideration (for instance, the need to oversample for certain under-represented segments of the population).</skos:definition>
      <skos:prefLabel xml:lang="de">Nicht-Wahrscheinlichkeitsauswahl: Quotenstichprobe</skos:prefLabel>
      <skos:definition xml:lang="de">Die Grundgesamtheit wird nach bestimmten Kriterien in sich gegenseitig ausschlie&#xdf;ende und insgesamt ersch&#xf6;pfende Segmente unterteilt. Die Verteilung der Quotenmerkmale (z. B. Geschlecht, Alter, Ethnizit&#xe4;t, Religion, Bildungsstand, etc.) soll die diesbez&#xfc;gliche Verteilung der Grundgesamtheit widerspiegeln. Aus jedem Segment werden dann Einheiten durch Nicht-Wahrscheinlichkeitsauswahl ausgew&#xe4;hlt, bis die gew&#xfc;nschte Anzahl der Einheiten pro Quotenmerkmal erreicht ist. Wenn die Grundgesamtheit beispielsweise einen Frauenanteil von 45 Prozent und einen M&#xe4;nneranteil von 55 Prozent aufweist, ist der Anteil der Frauen und M&#xe4;nner in der Stichprobe ebenso hoch, wenn es sich um eine proportionale Quotenstichprobe handelt. In einer nicht proportionalen Quotenstichprobe k&#xf6;nnen die Geschlechterverh&#xe4;ltnisse abweichen, beispielsweise durch ein bewusstes Oversampling von Frauen.</skos:definition>
      <skos:prefLabel xml:lang="fr">Non probabiliste : quota</skos:prefLabel>
      <skos:definition xml:lang="fr">La population cible est subdivis&#xe9;e dans des segments s&#xe9;par&#xe9;s et mutuellement exclusifs d&apos;apr&#xe8;s certains crit&#xe8;res de quotas pr&#xe9;d&#xe9;finis. La distribution des crit&#xe8;res de quotas (genre / &#xe2;ge / ratio d&apos;ethnicit&#xe9;, ou des autres caract&#xe9;ristiques, comme la religion, l&apos;&#xe9;ducation, etc.) est destin&#xe9;e &#xe0; refl&#xe9;ter la structure r&#xe9;elle de la population cible ou la structure d&#xe9;sir&#xe9;e de la population &#xe9;tudi&#xe9;e. Des &#xe9;chantillons non probabilistes sont alors tir&#xe9;s &#xe0; partir de chaque segment jusqu&apos;&#xe0; ce qu&apos;un nombre sp&#xe9;cifique d&apos;unit&#xe9;s soit atteint. Par exemple, si la population cible compte 45 pour cent de femmes et 55 pour cent d&apos;hommes, un &#xe9;chantillon par quotas proportionnel devra avoir les m&#xea;mes pourcentages par genre, alors que dans un &#xe9;chantillon par quotas non proportionnel le pourcentage sera diff&#xe9;rent, bas&#xe9; sur certaines consid&#xe9;rations li&#xe9;es &#xe0; l&apos;&#xe9;tude (par exemple, le besoin de sur-&#xe9;chantillon pour certains segments sous-repr&#xe9;sent&#xe9;s de la population).</skos:definition>
      <skos:prefLabel xml:lang="nl">Quota steekproef</skos:prefLabel>
      <skos:definition xml:lang="nl"></skos:definition>
      <skos:prefLabel xml:lang="no">Ikke-sannsynlighet: Kvote</skos:prefLabel>
      <skos:definition xml:lang="no">M&#xe5;lpopulasjonen er delt i flere ulike og gjensidig utelukkende segment i henhold til noen forh&#xe5;ndsdefinerte kvoteringskriterier. Fordelingen av kvoteringskriteriene (kj&#xf8;nn/alder/etnisitet, eller andre karakteristikker, som religion, utdanning etc.) skal reflektere den virkelige strukturen i m&#xe5;lpopulasjonen eller strukturen i den &#xf8;nskede studiepopulasjonen. Ikke-sannsynlighetsutvalg blir da trukket fra hvert segment inntil et spesifikt antall enheter er n&#xe5;dd. For eksempel dersom m&#xe5;lpopulasjonen best&#xe5;r av 45% kvinner og 55% menn, vil et proporsjonalt kvoteutvalg ha samme kj&#xf8;nnsfordeling, mens fordelingen vil v&#xe6;re annerledes i et ikke-proporsjonalt kvoteutvalg, basert p&#xe5; en studierelatert faktor (f. eks behovet for &#xe5; overinkludere visse underrepresenterte deler av populasjonen).</skos:definition>
   </rdf:Description>
   <rdf:Description rdf:about="http://rdf-vocabulary.ddialliance.org/cv/SamplingProcedure/2.0.1/086e080">
      <rdf:type rdf:resource="http://www.w3.org/2004/02/skos/core#Concept"/>
      <skos:inScheme rdf:resource="http://rdf-vocabulary.ddialliance.org/cv/SamplingProcedure/2.0.1/"/>
      <skos:notation xml:lang="en">Nonprobability.RespondentAssisted</skos:notation>
      <skos:prefLabel xml:lang="sl">Neverjetnostno: s pomo&#x10d;jo respondentov</skos:prefLabel>
      <skos:definition xml:lang="sl">Vzor&#x10d;ene enote so identificirane iz ciljne populacije s pomo&#x10d;jo &#x17e;e izbranih enot (prirejeno po &quot;Public Health Research Methods&quot;, ur. Greg Guest, Emily E. Namey, 2014). Tipi&#x10d;en primer je vzor&#x10d;enje po metodi sne&#x17e;ne kepe, v katerem raziskovalec identificira skupino enot, ki ustreza dolo&#x10d;enemu merilu upravi&#x10d;enosti za izbor. Te enote nato zaprosi za pomo&#x10d; pri pridobivanju drugih &#x10d;lanov iste populacije, ki izpolnjujejo enako merilo upravi&#x10d;enosti (vzor&#x10d;enje dolo&#x10d;enih populacij, kot so migranti itd.).</skos:definition>
      <skos:prefLabel xml:lang="lt">Netikimybin&#x117;: respondent&#x173; formuojama</skos:prefLabel>
      <skos:definition xml:lang="lt">Jau atrinkti imties vienetai padeda identifikuoti kitus tikslin&#x117;s populiacijos vienetus (adaptuota pagal &quot;Public Health Research Methods&quot;, ed. Greg Guest, Emily E. Namey, 2014). Tipi&#x161;kas tokios atrankos pavyzdys yra sniego gni&#x16b;&#x17e;t&#x117;s atranka, kai tyr&#x117;jas sudaro pirmin&#x119;, tyrime numatyt&#x105; tinkamumo kriterij&#x173; atitinkan&#x10d;i&#x105;, imties vienet&#x173; grup&#x119;. Tuomet jos atstov&#x173; yra pra&#x161;oma identifikuoti kitus tos pa&#x10d;ios populiacijos narius, atitinkan&#x10d;ius t&#x105; pat&#x12f; tinkamumo kriterij&#x173; (taikoma atrankoms specifin&#x117;se populiacijose, pavyzd&#x17e;iui, migrant&#x173; ir kt.).</skos:definition>
      <skos:prefLabel xml:lang="sv">Icke-sannolikhetsurval: respondent-assisterat urval</skos:prefLabel>
      <skos:definition xml:lang="sv">Ytterligare element i urvalet identifieras inom m&#xe5;lpopulationen med hj&#xe4;lp av redan valda element (bearbetat fr&#xe5;n &quot;Public Health Research Methods&quot;, red. Greg Guest, Emily E. Namey, 2014). En vanlig variant &#xe4;r sn&#xf6;bollsurval, d&#xe4;r forskaren f&#xf6;rst identifierar en grupp element som uppfyller vissa urvalskriterier. Dessa personer ombeds att rekrytera andra medlemmar i samma population som uppfyller samma urvalskriterier. Det kan exempelvis g&#xe4;lla urval av s&#xe4;rskilda eller sv&#xe5;r&#xe5;tkomliga populationer som till exempel migranter.</skos:definition>
      <skos:prefLabel xml:lang="it">Non probabilistico: guidato dal rispondente</skos:prefLabel>
      <skos:definition xml:lang="it">Le unit&#xe0; campionarie sono identificate all&apos;interno della popolazione di riferimento attraverso il ricorso a unit&#xe0; gi&#xe0; selezionate. Un caso tipico &#xe8; il &quot;campionamento a palla di neve&quot;, in cui il ricercatore identifica un gruppo di unit&#xe0; che soddisfa un particolare criterio di ammissibilit&#xe0;. Queste unit&#xe0; sono invitate a reclutare altri membri della stessa popolazione che soddisfano lo stesso criterio di ammissibilit&#xe0; (campionamento di popolazioni specifiche come migranti, ecc.).</skos:definition>
      <skos:prefLabel xml:lang="en">Non-probability: Respondent-assisted 	</skos:prefLabel>
      <skos:definition xml:lang="en">Sample units are identified from a target population with the assistance of units already selected (adapted from &quot;Public Health Research Methods&quot;, ed. Greg Guest, Emily E. Namey, 2014). A typical case is snowball sampling, in which the researcher identifies a group of units that matches a particular criterion of eligibility. The latter are asked to recruit other members of the same population that fulfil the same criterion of eligibility (sampling of specific populations like migrants, etc.).</skos:definition>
      <skos:prefLabel xml:lang="de">Nicht-Zufallsstichprobe: Respondenten gesteuerte Auswahl</skos:prefLabel>
      <skos:definition xml:lang="de">Die Einheiten werden aus der Grundgesamtheit mit Hilfe von Einheiten ausgew&#xe4;hlt, die bereits in der Stichprobe sind. Ein typisches Beispiel daf&#xfc;r ist das Schneeballverfahren. Hier w&#xe4;hlt der Forscher nach festgelegten Kriterien eine Gruppe von Einheiten aus. Diese werden dann gebeten, ihnen &#xe4;hnliche, f&#xfc;r die Studie geeignete Personen zu rekrutieren (z. B. Stichproben bestimmter Gruppen, wie Migranten o.&#xe4;.).</skos:definition>
      <skos:prefLabel xml:lang="fr">Non probabiliste : participation volontaire</skos:prefLabel>
      <skos:definition xml:lang="fr">Les unit&#xe9;s de l&apos;&#xe9;chantillon sont identifi&#xe9;es &#xe0; partir d&apos;une population cible avec l&apos;assistance d&apos;unit&#xe9;s d&#xe9;j&#xe0; s&#xe9;lectionn&#xe9;es (adapt&#xe9; de &quot;Public Health Research Methods&quot;, ed. Greg Guest, Emily E. Namey, 2014). Un cas typique est l&apos;&#xe9;chantillonnage boule de neige, dans lequel le chercheur identifie un groupe d&apos;unit&#xe9;s qui correspond &#xe0; un crit&#xe8;re particulier d&apos;&#xe9;ligibilit&#xe9;. Ces derni&#xe8;res sont invit&#xe9;es &#xe0; recruter d&apos;autres membres de la m&#xea;me population qui remplissent le m&#xea;me crit&#xe8;re d&apos;&#xe9;ligibilit&#xe9; (&#xe9;chantillonnage de populations sp&#xe9;cifiques comme des migrants, etc.)</skos:definition>
      <skos:prefLabel xml:lang="nl">Respondentgestuurde steekproef</skos:prefLabel>
      <skos:definition xml:lang="nl"></skos:definition>
      <skos:prefLabel xml:lang="no">Ikke-sannsynlighet: Respondent-assistert</skos:prefLabel>
      <skos:definition xml:lang="no">Enhetene i utvalget identifiseres i m&#xe5;lpopulasjonen ved hjelp av enheter som allerede er valgt (fra &apos;Public Health Research Methods&apos;, red. Greg Guest, Emily E. Namey, 2014). En typisk variant er sn&#xf8;ballutvelgelse, der forskeren identifiserer en gruppe enheter som stemmer overens med spesifikke utvalgskriterier. Disse blir spurt om &#xe5; rekruttere andre deltakere i samme populasjon som oppfyller samme utvalgskriterier (utvelgelse av s&#xe6;rskilte populasjoner som migranter, etc.).</skos:definition>
   </rdf:Description>
   <rdf:Description rdf:about="http://rdf-vocabulary.ddialliance.org/cv/SamplingProcedure/2.0.1/e890a15">
      <rdf:type rdf:resource="http://www.w3.org/2004/02/skos/core#Concept"/>
      <skos:inScheme rdf:resource="http://rdf-vocabulary.ddialliance.org/cv/SamplingProcedure/2.0.1/"/>
      <skos:notation xml:lang="en">MixedProbabilityNonprobability</skos:notation>
      <skos:prefLabel xml:lang="sl">Me&#x161;ano verjetnostno in neverjetnostno</skos:prefLabel>
      <skos:definition xml:lang="sl">Na&#x10d;rt vzor&#x10d;enja, ki zdru&#x17e;uje verjetnostno in neverjetnostno vzor&#x10d;enje v istem postopku vzor&#x10d;enja. Na razli&#x10d;nih stopnjah izdelave vzorca se lahko uporabljajo razli&#x10d;ne vrste vzor&#x10d;enja. Na primer, za vzorec u&#x10d;encev iz manj&#x161;in v mestu se najprej v prvem koraku naklju&#x10d;no izberejo &#x161;ole. Nato je v drugem koraku v vsaki &#x161;oli izbran kvotni vzorec u&#x10d;encev. &#x10c;e iz iste ciljne populacije vzamemo lo&#x10d;ene vzorce z uporabo razli&#x10d;nih metod vzor&#x10d;enja, je potrebno vrste postopkov vzor&#x10d;enja, ki smo jih uporabili pri posameznih vzorcih, razvrstiti lo&#x10d;eno.</skos:definition>
      <skos:prefLabel xml:lang="lt">Mi&#x161;ri tikimybin&#x117; ir netikimybin&#x117;</skos:prefLabel>
      <skos:definition xml:lang="lt">Imties dizainas, kuris integruoja tikimybin&#x119; ir netikimybin&#x119; atrankas tame pa&#x10d;iame atrankos sudarymo procese. Skirtinguose imties sudarymo etapuose gali b&#x16b;ti naudojami skirtingi atrankos tipai. Pavyzd&#x17e;iui, miesto ma&#x17e;um&#x173; moksleivi&#x173; im&#x10d;iai sudaryti, pirmajame etape atsitiktinai atrenkamos mokyklos. Tada antrame etape kiekvienoje mokykloje sudaroma mokini&#x173; kvotin&#x117; imtis. Jei i&#x161; tos pa&#x10d;ios tikslin&#x117;s populiacijos skirtingais atrankos metodais sudaromos atskiros imtys, tai kiekvienos imties sudarymo proced&#x16b;ra tur&#x117;t&#x173; b&#x16b;ti koduojama atskirai.</skos:definition>
      <skos:prefLabel xml:lang="sv">Blandat sannolikhets- och icke-sannolikhetsurval</skos:prefLabel>
      <skos:definition xml:lang="sv">Urvalsdesign som kombinerar sannolikhets- och icke-sannolikhetsurval inom samma urvalsprocess. Olika urvalsmetoder kan anv&#xe4;ndas i olika steg n&#xe4;r urvalet skapas. 
Exempel: f&#xf6;r ett urval av minoritetselever i en stad v&#xe4;ljs skolor slumpm&#xe4;ssigt i det f&#xf6;rsta steget. I det andra steget anv&#xe4;nds kvoturval f&#xf6;r att v&#xe4;lja elever inom varje skola. Om det g&#xf6;rs separata urval fr&#xe5;n samma m&#xe5;lpopulation med olika urvalsmetoder b&#xf6;r typ av urvalsprocess specificeras separat f&#xf6;r varje urval.</skos:definition>
      <skos:prefLabel xml:lang="it">Misto</skos:prefLabel>
      <skos:definition xml:lang="it">Disegno di campionamento che combina, all&apos;intero dello stesso processo, campionamento di tipo probabilistico e non probabilistico. Diversi tipi di campionamento possono essere utilizzati nelle diverse fasi della creazione del campione. Ad esempio, per costruire un campione di studenti appartenenti a una minoranza in una determinata citt&#xe0;, nella prima fase vengono selezionate in modo casuale le scuole. Quindi, nella seconda fase, viene selezionato un campione per quote di studenti all&apos;interno di ciascuna scuola. Se vengono estratti campioni separati dalla stessa popolazione di riferimento utilizzando diversi metodi di campionamento, il tipo di procedura di campionamento utilizzato per ciascun campione deve essere classificato separatamente.</skos:definition>
      <skos:prefLabel xml:lang="en">Mixed probability and non-probability</skos:prefLabel>
      <skos:definition xml:lang="en">Sample design that combines probability and non-probability sampling within the same sampling process. Different types of sampling may be used at different stages of creating the sample. For example, for a sample of minority students in a city, schools are randomly selected in the first stage. Then, a quota sample of students is selected within each school in the second stage. If separate samples are drawn from the same target population using different sampling methods, the type of sampling procedure used for each sample should be classified separately.</skos:definition>
      <skos:prefLabel xml:lang="de">Kombination aus Zufallsstichprobe und Nicht-Zufallsstichprobe</skos:prefLabel>
      <skos:definition xml:lang="de">Ein Verfahren, das f&#xfc;r dieselbe Grundgesamtheit Wahrscheinlichkeits- und Nicht-Wahrscheinlichkeitsauswahl miteinander kombiniert. Die verwendeten Methoden k&#xf6;nnen innerhalb oder zwischen den Stufen der Stichprobenziehung kombiniert werden. Beispielsweise kann zur Untersuchung einer religi&#xf6;sen Minderheit eine proportional geschichtete Zufallsauswahl mit einer Respondenten-gesteuerten Auswahl kombiniert werden. Alternativ w&#xe4;re f&#xfc;r dieses Beispiel auch eine Kombination von mehrstufiger Zufallsauswahl und einer Quotenstichprobe bei der letzten Ziehung m&#xf6;glich.</skos:definition>
      <skos:prefLabel xml:lang="fr">Mixte probabiliste et non probabiliste</skos:prefLabel>
      <skos:definition xml:lang="fr">Le plan d&apos;&#xe9;chantillonnage qui combine &#xe9;chantillonnage probabiliste et non probabiliste au sein d&apos;un m&#xea;me processus d&apos;&#xe9;chantillonnage. Diff&#xe9;rents type d&apos;&#xe9;chantillonnage peuvent &#xea;tre utilis&#xe9;s &#xe0; diff&#xe9;rentes &#xe9;tapes de cr&#xe9;ation de l&apos;&#xe9;chantillon. Par exemple, pour un &#xe9;chantillon d&apos;&#xe9;l&#xe8;ves issus de l&apos;immigration dans une ville, les &#xe9;coles sont s&#xe9;lectionn&#xe9;es al&#xe9;atoirement dans une premi&#xe8;re &#xe9;tape. Alors, un &#xe9;chantillon par quotas des &#xe9;l&#xe8;ves est s&#xe9;lectionn&#xe9; au sein de chaque &#xe9;cole dans une seconde &#xe9;tape. Si des &#xe9;chantillons distincts sont tir&#xe9;s &#xe0; partir de la m&#xea;me population cible &#xe0; l&apos;aide de diff&#xe9;rentes m&#xe9;thodes d&apos;&#xe9;chantillonnage, le type de proc&#xe9;dure d&apos;&#xe9;chantillonnage utilis&#xe9; pour chaque &#xe9;chantillon devra &#xea;tre class&#xe9; s&#xe9;par&#xe9;ment.</skos:definition>
      <skos:prefLabel xml:lang="nl">Gemengde kans- en niet-kanssteekproef</skos:prefLabel>
      <skos:definition xml:lang="nl"></skos:definition>
      <skos:prefLabel xml:lang="no">Blandet sannsynlighets- og ikke-sannsynlighetsutvalg</skos:prefLabel>
      <skos:definition xml:lang="no">Utvalgsdesign som kombinerer sannsynlighets- og ikke-sannsynlighetsutvalg i samme utvalgsprosess. Forskjellige utvalgsmetoder kan bli brukt p&#xe5; ulike steg i utvalgsprosessen. For eksempel for en studie av minoritetsstudenter i en by blir skoler trukket tilfeldig i f&#xf8;rste stadie. Deretter trekkes et kvoteutvalg av studenter fra hver skole i andre steg. Dersom separate utvalg er trukket fra samme m&#xe5;lpopulasjon ved bruk av ulike utvalgsmetoder, b&#xf8;r typen utvalgsprosedyre som blir brukt for hvert utvalg klassifiseres separat.</skos:definition>
   </rdf:Description>
   <rdf:Description rdf:about="http://rdf-vocabulary.ddialliance.org/cv/SamplingProcedure/2.0.1/6311ae1">
      <rdf:type rdf:resource="http://www.w3.org/2004/02/skos/core#Concept"/>
      <skos:inScheme rdf:resource="http://rdf-vocabulary.ddialliance.org/cv/SamplingProcedure/2.0.1/"/>
      <skos:notation xml:lang="en">Other</skos:notation>
      <skos:prefLabel xml:lang="sl">Drugo</skos:prefLabel>
      <skos:definition xml:lang="sl">Uporabite, &#x10d;e je postopek vzor&#x10d;enja znan, a ga ne najdete na seznamu.</skos:definition>
      <skos:prefLabel xml:lang="lt">Kita</skos:prefLabel>
      <skos:definition xml:lang="lt">Naudoti, kai atrankos proced&#x16b;ra yra &#x17e;inoma, bet jos s&#x105;ra&#x161;e n&#x117;ra.</skos:definition>
      <skos:prefLabel xml:lang="sv">&#xd6;vrigt</skos:prefLabel>
      <skos:definition xml:lang="sv">Anv&#xe4;nd om urvalsmetoden &#xe4;r k&#xe4;nd men saknas i listan.</skos:definition>
      <skos:prefLabel xml:lang="it">Altro</skos:prefLabel>
      <skos:definition xml:lang="it">Utilizzare se la procedura di campionamento &#xe8; conosciuta, ma non &#xe8; presente nell&apos;elenco.</skos:definition>
      <skos:prefLabel xml:lang="en">Other</skos:prefLabel>
      <skos:definition xml:lang="en">Use if the sampling procedure is known, but not found in the list.</skos:definition>
      <skos:prefLabel xml:lang="de">Andere</skos:prefLabel>
      <skos:definition xml:lang="de">Verwenden Sie diese Kategorie, wenn das Auswahlverfahren bekannt ist, aber nicht in der Liste vertreten ist.</skos:definition>
      <skos:prefLabel xml:lang="fr">Autre</skos:prefLabel>
      <skos:definition xml:lang="fr">Utilisez si la proc&#xe9;dure d&apos;&#xe9;chantillonnage est connue, mais pas pr&#xe9;sente dans la liste.</skos:definition>
      <skos:prefLabel xml:lang="nl">Overig</skos:prefLabel>
      <skos:definition xml:lang="nl"></skos:definition>
      <skos:prefLabel xml:lang="no">Annet</skos:prefLabel>
      <skos:definition xml:lang="no">Bruk dersom utvalgsmetoden er kjent, men ikke funnet i listen.</skos:definition>
   </rdf:Description>
</rdf:RDF>
