<?xml version="1.0" encoding="UTF-8"?>
<rdf:RDF xmlns:dcterms="http://purl.org/dc/terms/"
          xmlns:owl="http://www.w3.org/2002/07/owl#"
          xmlns:rdf="http://www.w3.org/1999/02/22-rdf-syntax-ns#"
          xmlns:rdfs="http://www.w3.org/2000/01/rdf-schema#"
          xmlns:skos="http://www.w3.org/2004/02/skos/core#">
   <rdf:Description rdf:about="http://rdf-vocabulary.ddialliance.org/cv/TypeOfTelephone/1.0.1/">
      <rdf:type rdf:resource="http://www.w3.org/2004/02/skos/core#ConceptScheme"/>
      <dcterms:isVersionOf rdf:resource="http://rdf-vocabulary.ddialliance.org/cv/TypeOfTelephone"/>
      <skos:notation>TypeOfTelephone</skos:notation>
      <skos:prefLabel xml:lang="en">Type of Telephone</skos:prefLabel>
      <skos:prefLabel xml:lang="en">Type of Telephone</skos:prefLabel>
      <skos:definition xml:lang="en">Identifies the type of telephone entered as contact information for an individual or an organization.</skos:definition>
      <skos:definition xml:lang="en">Identifies the type of telephone entered as contact information for an individual or an organization.</skos:definition>
      <owl:versionInfo>1.0.0</owl:versionInfo>
      <dcterms:license rdf:resource="Creative Commons Attribution 4.0 International"/>
      <dcterms:rights>Copyright Â©DDI Alliance 2020</dcterms:rights>
      <skos:hasTopConcept rdf:resource="http://rdf-vocabulary.ddialliance.org/cv/TypeOfTelephone/1.0.1/d201e40"/>
      <skos:hasTopConcept rdf:resource="http://rdf-vocabulary.ddialliance.org/cv/TypeOfTelephone/1.0.1/d201e110"/>
      <skos:hasTopConcept rdf:resource="http://rdf-vocabulary.ddialliance.org/cv/TypeOfTelephone/1.0.1/d201e181"/>
      <skos:hasTopConcept rdf:resource="http://rdf-vocabulary.ddialliance.org/cv/TypeOfTelephone/1.0.1/d201e251"/>
   </rdf:Description>
   <rdf:Description rdf:about="http://rdf-vocabulary.ddialliance.org/cv/TypeOfTelephone/1.0.1/d201e40">
      <rdf:type rdf:resource="http://www.w3.org/2004/02/skos/core#Concept"/>
      <skos:inScheme rdf:resource="http://rdf-vocabulary.ddialliance.org/cv/TypeOfTelephone/1.0.1/"/>
      <skos:notation>Fixed</skos:notation>
      <skos:prefLabel xml:lang="en">Fixed telephone</skos:prefLabel>
      <skos:definition xml:lang="en">A telephone that transmits signals converted from audio data through physical media, such as wire or fiber optic cable; also known as landline.</skos:definition>
      <skos:prefLabel xml:lang="en">Fixed telephone</skos:prefLabel>
      <skos:definition xml:lang="en">A telephone that transmits signals converted from audio data through physical media, such as wire or fiber optic cable; also known as landline.</skos:definition>
      <skos:narrower rdf:resource="http://rdf-vocabulary.ddialliance.org/cv/TypeOfTelephone/1.0.1/d201e66"/>
      <skos:narrower rdf:resource="http://rdf-vocabulary.ddialliance.org/cv/TypeOfTelephone/1.0.1/d201e88"/>
   </rdf:Description>
   <rdf:Description rdf:about="http://rdf-vocabulary.ddialliance.org/cv/TypeOfTelephone/1.0.1/d201e66">
      <rdf:type rdf:resource="http://www.w3.org/2004/02/skos/core#Concept"/>
      <skos:inScheme rdf:resource="http://rdf-vocabulary.ddialliance.org/cv/TypeOfTelephone/1.0.1/"/>
      <skos:notation>Fixed.PersonalPrivate</skos:notation>
      <skos:prefLabel xml:lang="en">Fixed telephone: Personal/Private</skos:prefLabel>
      <skos:definition xml:lang="en">A fixed telephone belonging to a private person, usually located in a home or a private dwelling unit.</skos:definition>
      <skos:prefLabel xml:lang="en">Fixed telephone: Personal/Private</skos:prefLabel>
      <skos:definition xml:lang="en">A fixed telephone belonging to a private person, usually located in a home or a private dwelling unit.</skos:definition>
      <skos:broader rdf:resource="http://rdf-vocabulary.ddialliance.org/cv/TypeOfTelephone/1.0.1/d201e40"/>
   </rdf:Description>
   <rdf:Description rdf:about="http://rdf-vocabulary.ddialliance.org/cv/TypeOfTelephone/1.0.1/d201e88">
      <rdf:type rdf:resource="http://www.w3.org/2004/02/skos/core#Concept"/>
      <skos:inScheme rdf:resource="http://rdf-vocabulary.ddialliance.org/cv/TypeOfTelephone/1.0.1/"/>
      <skos:notation>Fixed.OrganizationBusiness</skos:notation>
      <skos:prefLabel xml:lang="en">Fixed telephone: Organization/Business</skos:prefLabel>
      <skos:definition xml:lang="en">A fixed telephone of an organization, institution or business, or the work telephone of a person employed by the organization.</skos:definition>
      <skos:prefLabel xml:lang="en">Fixed telephone: Organization/Business</skos:prefLabel>
      <skos:definition xml:lang="en">A fixed telephone of an organization, institution or business, or the work telephone of a person employed by the organization.</skos:definition>
      <skos:broader rdf:resource="http://rdf-vocabulary.ddialliance.org/cv/TypeOfTelephone/1.0.1/d201e40"/>
   </rdf:Description>
   <rdf:Description rdf:about="http://rdf-vocabulary.ddialliance.org/cv/TypeOfTelephone/1.0.1/d201e110">
      <rdf:type rdf:resource="http://www.w3.org/2004/02/skos/core#Concept"/>
      <skos:inScheme rdf:resource="http://rdf-vocabulary.ddialliance.org/cv/TypeOfTelephone/1.0.1/"/>
      <skos:notation>Mobile</skos:notation>
      <skos:prefLabel xml:lang="en">Mobile telephone</skos:prefLabel>
      <skos:definition xml:lang="en">A portable telephone connected to a wireless communications network through radio waves or satellite transmissions; includes phones known as cellular (or cell) phones, hand phones, as well as satellite phones.</skos:definition>
      <skos:prefLabel xml:lang="en">Mobile telephone</skos:prefLabel>
      <skos:definition xml:lang="en">A portable telephone connected to a wireless communications network through radio waves or satellite transmissions; includes phones known as cellular (or cell) phones, hand phones, as well as satellite phones.</skos:definition>
      <skos:narrower rdf:resource="http://rdf-vocabulary.ddialliance.org/cv/TypeOfTelephone/1.0.1/d201e137"/>
      <skos:narrower rdf:resource="http://rdf-vocabulary.ddialliance.org/cv/TypeOfTelephone/1.0.1/d201e159"/>
   </rdf:Description>
   <rdf:Description rdf:about="http://rdf-vocabulary.ddialliance.org/cv/TypeOfTelephone/1.0.1/d201e137">
      <rdf:type rdf:resource="http://www.w3.org/2004/02/skos/core#Concept"/>
      <skos:inScheme rdf:resource="http://rdf-vocabulary.ddialliance.org/cv/TypeOfTelephone/1.0.1/"/>
      <skos:notation>Mobile.PersonalPrivate</skos:notation>
      <skos:prefLabel xml:lang="en">Mobile telephone: Personal/Private</skos:prefLabel>
      <skos:definition xml:lang="en">A mobile telephone belonging to a private person.</skos:definition>
      <skos:prefLabel xml:lang="en">Mobile telephone: Personal/Private</skos:prefLabel>
      <skos:definition xml:lang="en">A mobile telephone belonging to a private person.</skos:definition>
      <skos:broader rdf:resource="http://rdf-vocabulary.ddialliance.org/cv/TypeOfTelephone/1.0.1/d201e110"/>
   </rdf:Description>
   <rdf:Description rdf:about="http://rdf-vocabulary.ddialliance.org/cv/TypeOfTelephone/1.0.1/d201e159">
      <rdf:type rdf:resource="http://www.w3.org/2004/02/skos/core#Concept"/>
      <skos:inScheme rdf:resource="http://rdf-vocabulary.ddialliance.org/cv/TypeOfTelephone/1.0.1/"/>
      <skos:notation>Mobile.OrganizationBusiness</skos:notation>
      <skos:prefLabel xml:lang="en">Mobile telephone: Organization/Business</skos:prefLabel>
      <skos:definition xml:lang="en">A mobile telephone of an organization, institution or business, or the mobile work telephone of a person employed by the organization.</skos:definition>
      <skos:prefLabel xml:lang="en">Mobile telephone: Organization/Business</skos:prefLabel>
      <skos:definition xml:lang="en">A mobile telephone of an organization, institution or business, or the mobile work telephone of a person employed by the organization.</skos:definition>
      <skos:broader rdf:resource="http://rdf-vocabulary.ddialliance.org/cv/TypeOfTelephone/1.0.1/d201e110"/>
   </rdf:Description>
   <rdf:Description rdf:about="http://rdf-vocabulary.ddialliance.org/cv/TypeOfTelephone/1.0.1/d201e181">
      <rdf:type rdf:resource="http://www.w3.org/2004/02/skos/core#Concept"/>
      <skos:inScheme rdf:resource="http://rdf-vocabulary.ddialliance.org/cv/TypeOfTelephone/1.0.1/"/>
      <skos:notation>Fax</skos:notation>
      <skos:prefLabel xml:lang="en">Fax</skos:prefLabel>
      <skos:definition xml:lang="en">A fax (short for facsimile) is a device used for the telephonic transmission of scanned-in printed material (text or images), usually to a telephone number associated with a printer or other output device; also known as telecopying.</skos:definition>
      <skos:prefLabel xml:lang="en">Fax</skos:prefLabel>
      <skos:definition xml:lang="en">A fax (short for facsimile) is a device used for the telephonic transmission of scanned-in printed material (text or images), usually to a telephone number associated with a printer or other output device; also known as telecopying.</skos:definition>
      <skos:narrower rdf:resource="http://rdf-vocabulary.ddialliance.org/cv/TypeOfTelephone/1.0.1/d201e207"/>
      <skos:narrower rdf:resource="http://rdf-vocabulary.ddialliance.org/cv/TypeOfTelephone/1.0.1/d201e229"/>
   </rdf:Description>
   <rdf:Description rdf:about="http://rdf-vocabulary.ddialliance.org/cv/TypeOfTelephone/1.0.1/d201e207">
      <rdf:type rdf:resource="http://www.w3.org/2004/02/skos/core#Concept"/>
      <skos:inScheme rdf:resource="http://rdf-vocabulary.ddialliance.org/cv/TypeOfTelephone/1.0.1/"/>
      <skos:notation>Fax.PersonalPrivate</skos:notation>
      <skos:prefLabel xml:lang="en">Fax: Personal/Private</skos:prefLabel>
      <skos:definition xml:lang="en">A fax belonging to a private person.</skos:definition>
      <skos:prefLabel xml:lang="en">Fax: Personal/Private</skos:prefLabel>
      <skos:definition xml:lang="en">A fax belonging to a private person.</skos:definition>
      <skos:broader rdf:resource="http://rdf-vocabulary.ddialliance.org/cv/TypeOfTelephone/1.0.1/d201e181"/>
   </rdf:Description>
   <rdf:Description rdf:about="http://rdf-vocabulary.ddialliance.org/cv/TypeOfTelephone/1.0.1/d201e229">
      <rdf:type rdf:resource="http://www.w3.org/2004/02/skos/core#Concept"/>
      <skos:inScheme rdf:resource="http://rdf-vocabulary.ddialliance.org/cv/TypeOfTelephone/1.0.1/"/>
      <skos:notation>Fax.OrganizationBusiness</skos:notation>
      <skos:prefLabel xml:lang="en">Fax: Organization/Business</skos:prefLabel>
      <skos:definition xml:lang="en">The fax of an organization, institution or business, or the work fax of a person employed by the organization.</skos:definition>
      <skos:prefLabel xml:lang="en">Fax: Organization/Business</skos:prefLabel>
      <skos:definition xml:lang="en">The fax of an organization, institution or business, or the work fax of a person employed by the organization.</skos:definition>
      <skos:broader rdf:resource="http://rdf-vocabulary.ddialliance.org/cv/TypeOfTelephone/1.0.1/d201e181"/>
   </rdf:Description>
   <rdf:Description rdf:about="http://rdf-vocabulary.ddialliance.org/cv/TypeOfTelephone/1.0.1/d201e251">
      <rdf:type rdf:resource="http://www.w3.org/2004/02/skos/core#Concept"/>
      <skos:inScheme rdf:resource="http://rdf-vocabulary.ddialliance.org/cv/TypeOfTelephone/1.0.1/"/>
      <skos:notation>Other</skos:notation>
      <skos:prefLabel xml:lang="en">Other</skos:prefLabel>
      <skos:definition xml:lang="en">Use when the type of telephone is known, but not found in the list.</skos:definition>
      <skos:prefLabel xml:lang="en">Other</skos:prefLabel>
      <skos:definition xml:lang="en">Use when the type of telephone is known, but not found in the list.</skos:definition>
   </rdf:Description>
</rdf:RDF>
