<?xml version="1.0" encoding="UTF-8"?>
<rdf:RDF xmlns:dcterms="http://purl.org/dc/terms/"
          xmlns:owl="http://www.w3.org/2002/07/owl#"
          xmlns:rdf="http://www.w3.org/1999/02/22-rdf-syntax-ns#"
          xmlns:rdfs="http://www.w3.org/2000/01/rdf-schema#"
          xmlns:skos="http://www.w3.org/2004/02/skos/core#">
   <rdf:Description rdf:about="http://rdf-vocabulary.ddialliance.org/cv/AnalysisUnit/2.1.3/">
      <rdf:type rdf:resource="http://www.w3.org/2004/02/skos/core#ConceptScheme"/>
      <dcterms:isVersionOf rdf:resource="http://rdf-vocabulary.ddialliance.org/cv/AnalysisUnit"/>
      <skos:notation>AnalysisUnit</skos:notation>
      <skos:prefLabel xml:lang="en">Analysis Unit</skos:prefLabel>
      <skos:prefLabel xml:lang="en">Analysis Unit</skos:prefLabel>
      <skos:prefLabel xml:lang="de">Analyseeinheit</skos:prefLabel>
      <skos:prefLabel xml:lang="de">Analyseeinheit</skos:prefLabel>
      <skos:prefLabel xml:lang="fi">Havainto/aineistoyksikkötyyppi</skos:prefLabel>
      <skos:prefLabel xml:lang="fi">Havainto/aineistoyksikkötyyppi</skos:prefLabel>
      <skos:prefLabel xml:lang="it">Unità di analisi</skos:prefLabel>
      <skos:prefLabel xml:lang="it">Unità di analisi</skos:prefLabel>
      <skos:prefLabel xml:lang="lt">Analizės vienetas</skos:prefLabel>
      <skos:prefLabel xml:lang="lt">Analizės vienetas</skos:prefLabel>
      <skos:prefLabel xml:lang="nl">Analyse Eenheid</skos:prefLabel>
      <skos:prefLabel xml:lang="nl">Analyse Eenheid</skos:prefLabel>
      <skos:prefLabel xml:lang="no">Analyseenhet</skos:prefLabel>
      <skos:prefLabel xml:lang="no">Analyseenhet</skos:prefLabel>
      <skos:prefLabel xml:lang="pt">Unidade de Análise</skos:prefLabel>
      <skos:prefLabel xml:lang="pt">Unidade de Análise</skos:prefLabel>
      <skos:prefLabel xml:lang="sl">Enota analize</skos:prefLabel>
      <skos:prefLabel xml:lang="sl">Enota analize</skos:prefLabel>
      <skos:prefLabel xml:lang="sv">Analysenhet</skos:prefLabel>
      <skos:prefLabel xml:lang="sv">Analysenhet</skos:prefLabel>
      <skos:prefLabel xml:lang="sv">Analysenhet</skos:prefLabel>
      <skos:definition xml:lang="en">Describes the entity being analyzed in the study or variable. This vocabulary can also be used to describe the unit of observation, which is the unit being observed, or from which data are collected. The unit of observation can be the same as, or different from the unit of analysis. </skos:definition>
      <skos:definition xml:lang="en">Describes the entity being analyzed in the study or variable. This vocabulary can also be used to describe the unit of observation, which is the unit being observed, or from which data are collected. The unit of observation can be the same as, or different from the unit of analysis. </skos:definition>
      <skos:definition xml:lang="de">Beschreibt die Entität, die in der Studie oder in der Variable analysiert wird. Dieses Vokabular kann auch verwendet werden, um die Beobachtungseinheit zu beschreiben, d. h. die Einheit, die beobachtet wird oder von der Daten gesammelt werden. Die Beobachtungseinheit kann mit der Analyseeinheit identisch sein oder sich von ihr unterscheiden.</skos:definition>
      <skos:definition xml:lang="de">Beschreibt die Entität, die in der Studie oder in der Variable analysiert wird. Dieses Vokabular kann auch verwendet werden, um die Beobachtungseinheit zu beschreiben, d. h. die Einheit, die beobachtet wird oder von der Daten gesammelt werden. Die Beobachtungseinheit kann mit der Analyseeinheit identisch sein oder sich von ihr unterscheiden.</skos:definition>
      <skos:definition xml:lang="fi">Määrittelee yksikön, jota tutkimuksessa/muuttujassa analysoidaan. Sanastoa voidaan käyttää myös määrittelemään havaintoyksikkö, jota tutkimuksessa havannoidaan tai josta aineistoa kerätään. Havaintoyksikkö voi olla sama tai eri kuin analyysiyksikkö.
</skos:definition>
      <skos:definition xml:lang="fi">Määrittelee yksikön, jota tutkimuksessa/muuttujassa analysoidaan. Sanastoa voidaan käyttää myös määrittelemään havaintoyksikkö, jota tutkimuksessa havannoidaan tai josta aineistoa kerätään. Havaintoyksikkö voi olla sama tai eri kuin analyysiyksikkö.
</skos:definition>
      <skos:definition xml:lang="it">Descrive l'entità analizzata nello studio o nella variabile. Questo vocabolario può essere usato anche per descrivere l'unità di raccolta, che è l'unità che viene osservata, o sulla base della quale vengono raccolti i dati. L'unità di raccolta può coincidere con l'unità di analisi oppure può essere differente.</skos:definition>
      <skos:definition xml:lang="it">Descrive l'entità analizzata nello studio o nella variabile. Questo vocabolario può essere usato anche per descrivere l'unità di raccolta, che è l'unità che viene osservata, o sulla base della quale vengono raccolti i dati. L'unità di raccolta può coincidere con l'unità di analisi oppure può essere differente.</skos:definition>
      <skos:definition xml:lang="lt">Apibūdina tyrime ar kintamajame stebimą ar analizuojamą objektą. Šis žodynas taip pat gali būti naudojamas apibūdinant stebėjimo vienetus, kurie patys gali būti stebėjimo objektais, arba iš kurių gali būti renkami duomenys. Stebėjimo vienetas gali sutapti arba skirtis nuo analizės vieneto.</skos:definition>
      <skos:definition xml:lang="lt">Apibūdina tyrime ar kintamajame stebimą ar analizuojamą objektą. Šis žodynas taip pat gali būti naudojamas apibūdinant stebėjimo vienetus, kurie patys gali būti stebėjimo objektais, arba iš kurių gali būti renkami duomenys. Stebėjimo vienetas gali sutapti arba skirtis nuo analizės vieneto.</skos:definition>
      <skos:definition xml:lang="nl">Beschrijft de eenheid die geanalyseerd wordt in een bepaalde studie of variabele. De termen kunnen ook gebruikt worden om de waargenomen eenheid te beschrijven - dit is de eenheid die geobserveerd wordt of waarvan data wordt verzameld. De waargenomen eenheid kan hetzelfde zijn als de analyse eenheid, of ze kunnen van elkaar verschillen.</skos:definition>
      <skos:definition xml:lang="nl">Beschrijft de eenheid die geanalyseerd wordt in een bepaalde studie of variabele. De termen kunnen ook gebruikt worden om de waargenomen eenheid te beschrijven - dit is de eenheid die geobserveerd wordt of waarvan data wordt verzameld. De waargenomen eenheid kan hetzelfde zijn als de analyse eenheid, of ze kunnen van elkaar verschillen.</skos:definition>
      <skos:definition xml:lang="no">Beskrivelse av enhet som blir analysert i studien eller i variablene. Dette vokabularet kan også bli brukt for å beskrive observasjonsenheten, som er enheten som blir observert, eller enheten data er samlet inn fra. Observasjonsenhten kan være det samme eller forskjellig fra analyseenheten.</skos:definition>
      <skos:definition xml:lang="no">Beskrivelse av enhet som blir analysert i studien eller i variablene. Dette vokabularet kan også bli brukt for å beskrive observasjonsenheten, som er enheten som blir observert, eller enheten data er samlet inn fra. Observasjonsenhten kan være det samme eller forskjellig fra analyseenheten.</skos:definition>
      <skos:definition xml:lang="pt">Descreve a entidade que está a ser observada ou analisada no estudo ou na variável.</skos:definition>
      <skos:definition xml:lang="pt">Descreve a entidade que está a ser observada ou analisada no estudo ou na variável.</skos:definition>
      <skos:definition xml:lang="sl">Opisuje enoto, ki jo analiziramo v raziskavi ali v spremenljivki.</skos:definition>
      <skos:definition xml:lang="sl">Opisuje enoto, ki jo analiziramo v raziskavi ali v spremenljivki.</skos:definition>
      <skos:definition xml:lang="sv">Beskriver den enhet som analyseras i studien eller i variabeln. Den här vokabulären kan även användas för att beskriva undersökningsenhet, som är den enhet som undersöks eller observeras, eller som data samlas in från. Undersökningsenheten kan vara densamma som eller åtskild från analysenheten.</skos:definition>
      <skos:definition xml:lang="sv">Beskriver den enhet som analyseras i studien eller i variabeln. Den här vokabulären kan även användas för att beskriva undersökningsenhet, som är den enhet som undersöks eller observeras, eller som data samlas in från. Undersökningsenheten kan vara densamma som eller åtskild från analysenheten.</skos:definition>
      <skos:definition xml:lang="sv">Beskriver den enhet som analyseras i studien eller i variabeln. Den här vokabulären kan även användas för att beskriva undersökningsenhet, som är den enhet som undersöks eller observeras, eller som data samlas in från. Undersökningsenheten kan vara densamma som eller åtskild från analysenheten. </skos:definition>
      <owl:versionInfo>2.1.0</owl:versionInfo>
      <dcterms:license rdf:resource="Creative Commons Attribution 4.0 International"/>
      <dcterms:rights>Copyright ©DDI Alliance 2020</dcterms:rights>
      <skos:hasTopConcept rdf:resource="http://rdf-vocabulary.ddialliance.org/cv/AnalysisUnit/2.1.3/d151e116"/>
      <skos:hasTopConcept rdf:resource="http://rdf-vocabulary.ddialliance.org/cv/AnalysisUnit/2.1.3/d151e195"/>
      <skos:hasTopConcept rdf:resource="http://rdf-vocabulary.ddialliance.org/cv/AnalysisUnit/2.1.3/d151e274"/>
      <skos:hasTopConcept rdf:resource="http://rdf-vocabulary.ddialliance.org/cv/AnalysisUnit/2.1.3/d151e435"/>
      <skos:hasTopConcept rdf:resource="http://rdf-vocabulary.ddialliance.org/cv/AnalysisUnit/2.1.3/d151e514"/>
      <skos:hasTopConcept rdf:resource="http://rdf-vocabulary.ddialliance.org/cv/AnalysisUnit/2.1.3/d151e593"/>
      <skos:hasTopConcept rdf:resource="http://rdf-vocabulary.ddialliance.org/cv/AnalysisUnit/2.1.3/d151e672"/>
      <skos:hasTopConcept rdf:resource="http://rdf-vocabulary.ddialliance.org/cv/AnalysisUnit/2.1.3/d151e751"/>
      <skos:hasTopConcept rdf:resource="http://rdf-vocabulary.ddialliance.org/cv/AnalysisUnit/2.1.3/d151e830"/>
      <skos:hasTopConcept rdf:resource="http://rdf-vocabulary.ddialliance.org/cv/AnalysisUnit/2.1.3/d151e910"/>
      <skos:hasTopConcept rdf:resource="http://rdf-vocabulary.ddialliance.org/cv/AnalysisUnit/2.1.3/d151e1313"/>
      <skos:hasTopConcept rdf:resource="http://rdf-vocabulary.ddialliance.org/cv/AnalysisUnit/2.1.3/d151e1393"/>
      <skos:hasTopConcept rdf:resource="http://rdf-vocabulary.ddialliance.org/cv/AnalysisUnit/2.1.3/d151e1472"/>
   </rdf:Description>
   <rdf:Description rdf:about="http://rdf-vocabulary.ddialliance.org/cv/AnalysisUnit/2.1.3/d151e116">
      <rdf:type rdf:resource="http://www.w3.org/2004/02/skos/core#Concept"/>
      <skos:inScheme rdf:resource="http://rdf-vocabulary.ddialliance.org/cv/AnalysisUnit/2.1.3/"/>
      <skos:notation>Individual</skos:notation>
      <skos:prefLabel xml:lang="en">Individual</skos:prefLabel>
      <skos:definition xml:lang="en">Any individual person.</skos:definition>
      <skos:prefLabel xml:lang="en">Individual</skos:prefLabel>
      <skos:definition xml:lang="en">Any individual person.</skos:definition>
      <skos:prefLabel xml:lang="de">Individuum</skos:prefLabel>
      <skos:definition xml:lang="de">Jede einzelne Person, unabhängig von demographischen Merkmalen, dem Beruf, dem sozialen Status oder Rechtsstatus.</skos:definition>
      <skos:prefLabel xml:lang="de">Individuum</skos:prefLabel>
      <skos:definition xml:lang="de">Jede einzelne Person, unabhängig von demographischen Merkmalen, dem Beruf, dem sozialen Status oder Rechtsstatus.</skos:definition>
      <skos:prefLabel xml:lang="fi">Henkilö</skos:prefLabel>
      <skos:definition xml:lang="fi">Tutkimuksen tarkastelukohteena ovat yksittäiset henkilöt</skos:definition>
      <skos:prefLabel xml:lang="fi">Henkilö</skos:prefLabel>
      <skos:definition xml:lang="fi">Tutkimuksen tarkastelukohteena ovat yksittäiset henkilöt</skos:definition>
      <skos:prefLabel xml:lang="it">Individuo</skos:prefLabel>
      <skos:definition xml:lang="it">Qualsiasi persona.</skos:definition>
      <skos:prefLabel xml:lang="it">Individuo</skos:prefLabel>
      <skos:definition xml:lang="it">Qualsiasi persona.</skos:definition>
      <skos:prefLabel xml:lang="lt">Asmuo</skos:prefLabel>
      <skos:definition xml:lang="lt">Bet kuris atskiras asmuo.</skos:definition>
      <skos:prefLabel xml:lang="lt">Asmuo</skos:prefLabel>
      <skos:definition xml:lang="lt">Bet kuris atskiras asmuo.</skos:definition>
      <skos:prefLabel xml:lang="nl">Individueel</skos:prefLabel>
      <skos:definition xml:lang="nl"/>
      <skos:prefLabel xml:lang="nl">Individueel</skos:prefLabel>
      <skos:definition xml:lang="nl"/>
      <skos:prefLabel xml:lang="no">Individ</skos:prefLabel>
      <skos:definition xml:lang="no">Enhver individuell person.</skos:definition>
      <skos:prefLabel xml:lang="no">Individ</skos:prefLabel>
      <skos:definition xml:lang="no">Enhver individuell person.</skos:definition>
      <skos:prefLabel xml:lang="pt">Indivíduo</skos:prefLabel>
      <skos:definition xml:lang="pt">Qualquer sujeito individual.</skos:definition>
      <skos:prefLabel xml:lang="pt">Indivíduo</skos:prefLabel>
      <skos:definition xml:lang="pt">Qualquer sujeito individual.</skos:definition>
      <skos:prefLabel xml:lang="sl">Posameznik</skos:prefLabel>
      <skos:definition xml:lang="sl">Katerikoli posameznik.</skos:definition>
      <skos:prefLabel xml:lang="sl">Posameznik</skos:prefLabel>
      <skos:definition xml:lang="sl">Katerikoli posameznik.</skos:definition>
      <skos:prefLabel xml:lang="sv">Individ</skos:prefLabel>
      <skos:definition xml:lang="sv">En enskild person.</skos:definition>
      <skos:prefLabel xml:lang="sv">Individ</skos:prefLabel>
      <skos:definition xml:lang="sv">En enskild person.</skos:definition>
      <skos:prefLabel xml:lang="sv">Individ</skos:prefLabel>
      <skos:definition xml:lang="sv">En enskild person.</skos:definition>
   </rdf:Description>
   <rdf:Description rdf:about="http://rdf-vocabulary.ddialliance.org/cv/AnalysisUnit/2.1.3/d151e195">
      <rdf:type rdf:resource="http://www.w3.org/2004/02/skos/core#Concept"/>
      <skos:inScheme rdf:resource="http://rdf-vocabulary.ddialliance.org/cv/AnalysisUnit/2.1.3/"/>
      <skos:notation>OrganizationOrInstitution</skos:notation>
      <skos:prefLabel xml:lang="en">Organization/Institution</skos:prefLabel>
      <skos:definition xml:lang="en">Any kind of formal administrative and functional structure - includes associations, institutions, agencies, businesses, political parties, schools, etc. The data are collected about the organizations or institutions, even if the questions are answered by individuals. For example, data on the environmental policies of businesses, data on enrollment or graduation rates at national universities, etc.</skos:definition>
      <skos:prefLabel xml:lang="en">Organization/Institution</skos:prefLabel>
      <skos:definition xml:lang="en">Any kind of formal administrative and functional structure - includes associations, institutions, agencies, businesses, political parties, schools, etc. The data are collected about the organizations or institutions, even if the questions are answered by individuals. For example, data on the environmental policies of businesses, data on enrollment or graduation rates at national universities, etc.</skos:definition>
      <skos:prefLabel xml:lang="de">Organisation/Institution</skos:prefLabel>
      <skos:definition xml:lang="de">Jede Art von formaler Verwaltungsstruktur und funktionaler Struktur - schließt Verbände, Institutionen, Agenturen, Unternehmen, politische Parteien, Schulen usw. ein. Die Daten werden über die Organisationen oder Institutionen erhoben, auch wenn die Fragen von Individuen beantwortet werden. Zum Beispiel Daten zur Umweltpolitik von Unternehmen, Daten zu Immatrikulations- oder Absolventenquoten an Universitäten usw.</skos:definition>
      <skos:prefLabel xml:lang="de">Organisation/Institution</skos:prefLabel>
      <skos:definition xml:lang="de">Jede Art von formaler Verwaltungsstruktur und funktionaler Struktur - schließt Verbände, Institutionen, Agenturen, Unternehmen, politische Parteien, Schulen usw. ein. Die Daten werden über die Organisationen oder Institutionen erhoben, auch wenn die Fragen von Individuen beantwortet werden. Zum Beispiel Daten zur Umweltpolitik von Unternehmen, Daten zu Immatrikulations- oder Absolventenquoten an Universitäten usw.</skos:definition>
      <skos:prefLabel xml:lang="fi">Organisaatio</skos:prefLabel>
      <skos:definition xml:lang="fi">Mikä tahansa hallinnollinen tai toiminnallinen organisaatio, esimerkiksi järjestö, koulu, instituutti, toimisto, yritys, poliittinen puolue, jne. Kysymykset kohdistuvat itse organisaatioon vaikka vastaajina ovatkin yksittäiset henkilöt. Esimerkiksi tutkittaessa yritysten ympäristöpolitiikkaa tai korkeakouluista valmistuneiden määriä suhteessa opiskelijoihin jne.</skos:definition>
      <skos:prefLabel xml:lang="fi">Organisaatio</skos:prefLabel>
      <skos:definition xml:lang="fi">Mikä tahansa hallinnollinen tai toiminnallinen organisaatio, esimerkiksi järjestö, koulu, instituutti, toimisto, yritys, poliittinen puolue, jne. Kysymykset kohdistuvat itse organisaatioon vaikka vastaajina ovatkin yksittäiset henkilöt. Esimerkiksi tutkittaessa yritysten ympäristöpolitiikkaa tai korkeakouluista valmistuneiden määriä suhteessa opiskelijoihin jne.</skos:definition>
      <skos:prefLabel xml:lang="it">Organizzazione/Istituzione</skos:prefLabel>
      <skos:definition xml:lang="it">Qualsiasi tipo di struttura amministrativa e funzionale formale - incluse associazioni, istituzioni, agenzie, imprese, partiti politici, scuole, ecc. I dati raccolti si riferiscono alle organizzazioni o alle istituzioni, anche se le risposte alle domande sono fornite da singoli individui. Ad esempio, dati sulle politiche ambientali delle imprese, dati sui tassi di iscrizione o di laurea presso le università nazionali, ecc.</skos:definition>
      <skos:prefLabel xml:lang="it">Organizzazione/Istituzione</skos:prefLabel>
      <skos:definition xml:lang="it">Qualsiasi tipo di struttura amministrativa e funzionale formale - incluse associazioni, istituzioni, agenzie, imprese, partiti politici, scuole, ecc. I dati raccolti si riferiscono alle organizzazioni o alle istituzioni, anche se le risposte alle domande sono fornite da singoli individui. Ad esempio, dati sulle politiche ambientali delle imprese, dati sui tassi di iscrizione o di laurea presso le università nazionali, ecc.</skos:definition>
      <skos:prefLabel xml:lang="lt">Organizacija ar institucija</skos:prefLabel>
      <skos:definition xml:lang="lt">Bet kokia formali administracinė ir funkcinė struktūra – apima asociacijas, institucijas, agentūras, įmones, politines partijas, mokyklas ir kt. Duomenys renkami apie organizacijas ar institucijas, net jei į klausimus atsako individualūs asmenys. Pavyzdžiui, duomenys apie verslo aplinkosauginę politiką, duomenys apie stojančiųjų ar absolventų skaičių nacionaliniuose universitetuose ir kt.</skos:definition>
      <skos:prefLabel xml:lang="lt">Organizacija ar institucija</skos:prefLabel>
      <skos:definition xml:lang="lt">Bet kokia formali administracinė ir funkcinė struktūra – apima asociacijas, institucijas, agentūras, įmones, politines partijas, mokyklas ir kt. Duomenys renkami apie organizacijas ar institucijas, net jei į klausimus atsako individualūs asmenys. Pavyzdžiui, duomenys apie verslo aplinkosauginę politiką, duomenys apie stojančiųjų ar absolventų skaičių nacionaliniuose universitetuose ir kt.</skos:definition>
      <skos:prefLabel xml:lang="nl">Organisatie/Instituut</skos:prefLabel>
      <skos:definition xml:lang="nl"/>
      <skos:prefLabel xml:lang="nl">Organisatie/Instituut</skos:prefLabel>
      <skos:definition xml:lang="nl"/>
      <skos:prefLabel xml:lang="no">Organisasjon/Institusjon</skos:prefLabel>
      <skos:definition xml:lang="no">Former for formelle administrative og funksjonelle strukturerer - inkluderer foreninger, institusjoner, foretak, bedrifter, politiske partier, skoler etc. Data er samlet om organisasjoner eller institusjoner selv om spørsmålene er besvart av individer. For eksempel data om virksomheters miljøpolitikk, data om opptak eller avgangsgrader ved nasjonale universitet, etc.</skos:definition>
      <skos:prefLabel xml:lang="no">Organisasjon/Institusjon</skos:prefLabel>
      <skos:definition xml:lang="no">Former for formelle administrative og funksjonelle strukturerer - inkluderer foreninger, institusjoner, foretak, bedrifter, politiske partier, skoler etc. Data er samlet om organisasjoner eller institusjoner selv om spørsmålene er besvart av individer. For eksempel data om virksomheters miljøpolitikk, data om opptak eller avgangsgrader ved nasjonale universitet, etc.</skos:definition>
      <skos:prefLabel xml:lang="pt">Organização/Instituição</skos:prefLabel>
      <skos:definition xml:lang="pt">Qualquer tipo de estrutura funcional e administrativa formal. Inclui associações, instituições, agências, empresas, partidos políticos, escolas, etc. Os dados são recolhidos sobre as organizações e as instituições, mesmo que as questões sejam respondidas por indivíduos. Por exemplo, dados sobre políticas ambientais nas empresas, dados sobre taxas de sucesso nas universidades nacionais, etc.</skos:definition>
      <skos:prefLabel xml:lang="pt">Organização/Instituição</skos:prefLabel>
      <skos:definition xml:lang="pt">Qualquer tipo de estrutura funcional e administrativa formal. Inclui associações, instituições, agências, empresas, partidos políticos, escolas, etc. Os dados são recolhidos sobre as organizações e as instituições, mesmo que as questões sejam respondidas por indivíduos. Por exemplo, dados sobre políticas ambientais nas empresas, dados sobre taxas de sucesso nas universidades nacionais, etc.</skos:definition>
      <skos:prefLabel xml:lang="sl">Organizacija/Institucija</skos:prefLabel>
      <skos:definition xml:lang="sl">Katerakoli formalna upravna in funkcionalna oblika ali vrsta organizacije - vključuje združenja, institucije, agencije, podjetja, politične stranke, šole itd. Podatki se zbirajo o organizacijah ali ustanovah, tudi če na vprašanja odgovarjajo posamezniki. Na primer podatki o okoljski politiki podjetij, podatki o stopnjah vpisa ali diplome na nacionalnih univerzah itd.</skos:definition>
      <skos:prefLabel xml:lang="sl">Organizacija/Institucija</skos:prefLabel>
      <skos:definition xml:lang="sl">Katerakoli formalna upravna in funkcionalna oblika ali vrsta organizacije - vključuje združenja, institucije, agencije, podjetja, politične stranke, šole itd. Podatki se zbirajo o organizacijah ali ustanovah, tudi če na vprašanja odgovarjajo posamezniki. Na primer podatki o okoljski politiki podjetij, podatki o stopnjah vpisa ali diplome na nacionalnih univerzah itd.</skos:definition>
      <skos:prefLabel xml:lang="sv">Organisation/institution</skos:prefLabel>
      <skos:definition xml:lang="sv">En formell administrativ och funktionell struktur. Detta inkluderar föreningar, institutioner, myndigheter, företag, politiska partier, skolor m.m. Data om organisationerna eller institutionerna samlas in även om frågorna besvaras av enskilda personer. Det gäller till exempel data om företags miljöpolicyer, data om antagningar eller examensfrekvens vid nationella universitet m.m.</skos:definition>
      <skos:prefLabel xml:lang="sv">Organisation/institution</skos:prefLabel>
      <skos:definition xml:lang="sv">En formell administrativ och funktionell struktur. Detta inkluderar föreningar, institutioner, myndigheter, företag, politiska partier, skolor m.m. Data om organisationerna eller institutionerna samlas in även om frågorna besvaras av enskilda personer. Det gäller till exempel data om företags miljöpolicyer, data om antagningar eller examensfrekvens vid nationella universitet m.m.</skos:definition>
      <skos:prefLabel xml:lang="sv">Organisation/institution</skos:prefLabel>
      <skos:definition xml:lang="sv">En formell administrativ och funktionell struktur. Detta inkluderar föreningar, institutioner, myndigheter, företag, politiska partier, skolor m.m. Data om organisationerna eller institutionerna samlas in även om frågorna besvaras av enskilda personer. Det gäller till exempel data om företags miljöpolicyer, data om antagningar eller examensfrekvens vid nationella universitet m.m.</skos:definition>
   </rdf:Description>
   <rdf:Description rdf:about="http://rdf-vocabulary.ddialliance.org/cv/AnalysisUnit/2.1.3/d151e274">
      <rdf:type rdf:resource="http://www.w3.org/2004/02/skos/core#Concept"/>
      <skos:inScheme rdf:resource="http://rdf-vocabulary.ddialliance.org/cv/AnalysisUnit/2.1.3/"/>
      <skos:notation>Family</skos:notation>
      <skos:prefLabel xml:lang="en">Family</skos:prefLabel>
      <skos:definition xml:lang="en">Two or more people related by blood, marriage (including step-relations), co-habitation or registered partnership, adoption or fostering, and who may or may not live together. For example, data on what kind of public services the family uses or would require; or how often family members are in contact with each other.</skos:definition>
      <skos:prefLabel xml:lang="en">Family</skos:prefLabel>
      <skos:definition xml:lang="en">Two or more people related by blood, marriage (including step-relations), co-habitation or registered partnership, adoption or fostering, and who may or may not live together. For example, data on what kind of public services the family uses or would require; or how often family members are in contact with each other.</skos:definition>
      <skos:prefLabel xml:lang="de">Familie</skos:prefLabel>
      <skos:definition xml:lang="de">Zwei oder mehr Menschen, die miteinander blutsverwandt sind, oder durch Heirat (einschließlich der Verwandtschaft des Ehepartners), Adoption oder Pflege (Pflegeeltern, Pflegekinder etc.) anverwandt sind - unabhängig davon, ob sie zusammenleben oder nicht. Zum Beispiel Daten darüber, welche Art von öffentlichen Dienstleistungen die Familie nutzt oder benötigen würde; oder wie oft die Familienmitglieder miteinander in Kontakt stehen.</skos:definition>
      <skos:prefLabel xml:lang="de">Familie</skos:prefLabel>
      <skos:definition xml:lang="de">Zwei oder mehr Menschen, die miteinander blutsverwandt sind, oder durch Heirat (einschließlich der Verwandtschaft des Ehepartners), Adoption oder Pflege (Pflegeeltern, Pflegekinder etc.) anverwandt sind - unabhängig davon, ob sie zusammenleben oder nicht. Zum Beispiel Daten darüber, welche Art von öffentlichen Dienstleistungen die Familie nutzt oder benötigen würde; oder wie oft die Familienmitglieder miteinander in Kontakt stehen.</skos:definition>
      <skos:prefLabel xml:lang="fi">Perhe</skos:prefLabel>
      <skos:definition xml:lang="fi">Kaksi tai useampia henkilöitä, jotka liittyvät toisiinsa sukulaisuuden, avo- tai avioliiton (laskien mukaan esim. sisar- ja velipuolet), rekisteröidyn parisuhteen, adoption tai sijaisvanhemmuuden kautta, riippumatta siitä, asuvatko he yhdessä vai eivät. Esimerkiksi tutkittaessa mitä julkisia palveluja perhe käyttää; tai kuinka usein perheenjäsenet ovat yhteydessä toisiinsa.</skos:definition>
      <skos:prefLabel xml:lang="fi">Perhe</skos:prefLabel>
      <skos:definition xml:lang="fi">Kaksi tai useampia henkilöitä, jotka liittyvät toisiinsa sukulaisuuden, avo- tai avioliiton (laskien mukaan esim. sisar- ja velipuolet), rekisteröidyn parisuhteen, adoption tai sijaisvanhemmuuden kautta, riippumatta siitä, asuvatko he yhdessä vai eivät. Esimerkiksi tutkittaessa mitä julkisia palveluja perhe käyttää; tai kuinka usein perheenjäsenet ovat yhteydessä toisiinsa.</skos:definition>
      <skos:prefLabel xml:lang="it">Famiglia</skos:prefLabel>
      <skos:definition xml:lang="it">Due o più persone legate da vincolo di sangue, matrimonio (compresi i rapporti allargati), coabitazione o convivenza di fatto, adozione o affidamento che possono o meno vivere insieme. Ad esempio, dati sul tipo di servizi pubblici di cui la famiglia usufruisce o di cui avrebbe bisogno; oppure dati sulla frequenza con cui i membri della famiglia sono in contatto tra loro.</skos:definition>
      <skos:prefLabel xml:lang="it">Famiglia</skos:prefLabel>
      <skos:definition xml:lang="it">Due o più persone legate da vincolo di sangue, matrimonio (compresi i rapporti allargati), coabitazione o convivenza di fatto, adozione o affidamento che possono o meno vivere insieme. Ad esempio, dati sul tipo di servizi pubblici di cui la famiglia usufruisce o di cui avrebbe bisogno; oppure dati sulla frequenza con cui i membri della famiglia sono in contatto tra loro.</skos:definition>
      <skos:prefLabel xml:lang="lt">Šeima</skos:prefLabel>
      <skos:definition xml:lang="lt">Kartu gyvenantys ar negyvenantys du ar daugiau žmonių, kuriuos sieja kraujo ryšys, santuoka (įskaitant patėvius, podukras, posūnius), bendro gyvenimo sutartis ar registruota partnerystė, įvaikinimas ar globa. Pavyzdžiui, duomenys apie tai, kokias viešąsias paslaugas šeima naudoja ar norėtų naudoti; arba kaip dažnai šeimos nariai bendrauja tarpusavyje.</skos:definition>
      <skos:prefLabel xml:lang="lt">Šeima</skos:prefLabel>
      <skos:definition xml:lang="lt">Kartu gyvenantys ar negyvenantys du ar daugiau žmonių, kuriuos sieja kraujo ryšys, santuoka (įskaitant patėvius, podukras, posūnius), bendro gyvenimo sutartis ar registruota partnerystė, įvaikinimas ar globa. Pavyzdžiui, duomenys apie tai, kokias viešąsias paslaugas šeima naudoja ar norėtų naudoti; arba kaip dažnai šeimos nariai bendrauja tarpusavyje.</skos:definition>
      <skos:prefLabel xml:lang="nl">Familie</skos:prefLabel>
      <skos:definition xml:lang="nl"/>
      <skos:prefLabel xml:lang="nl">Familie</skos:prefLabel>
      <skos:definition xml:lang="nl"/>
      <skos:prefLabel xml:lang="no">Familie</skos:prefLabel>
      <skos:definition xml:lang="no">To eller flere mennesker som er i slekt med blod, ekteskap (inkludert ste-relasjoner), samboerskap eller registrerte partnere, adopsjon eller fosterbarn som enten lever eller ikke lever sammen. For eksempel, data om hvilke typer offentlige tjenster familien bruker eller har behov for; eller hvor ofte familiemedlemmene er i kontakt med hverandre.</skos:definition>
      <skos:prefLabel xml:lang="no">Familie</skos:prefLabel>
      <skos:definition xml:lang="no">To eller flere mennesker som er i slekt med blod, ekteskap (inkludert ste-relasjoner), samboerskap eller registrerte partnere, adopsjon eller fosterbarn som enten lever eller ikke lever sammen. For eksempel, data om hvilke typer offentlige tjenster familien bruker eller har behov for; eller hvor ofte familiemedlemmene er i kontakt med hverandre.</skos:definition>
      <skos:prefLabel xml:lang="pt">Família</skos:prefLabel>
      <skos:definition xml:lang="pt">Duas ou mais pessoas relacionadas por sangue, casamento (incluindo relações de famílias recompostas), coabitação ou parentalidade registada, adopção ou guarda de crianças, e que podem ou não viver juntas. Por exemplo, dados sobre que tipo de serviços públicos as famílias usam ou poderiam requerer; ou sobre quão frequentemente os membros duma família estão em contacto uns com os outros.</skos:definition>
      <skos:prefLabel xml:lang="pt">Família</skos:prefLabel>
      <skos:definition xml:lang="pt">Duas ou mais pessoas relacionadas por sangue, casamento (incluindo relações de famílias recompostas), coabitação ou parentalidade registada, adopção ou guarda de crianças, e que podem ou não viver juntas. Por exemplo, dados sobre que tipo de serviços públicos as famílias usam ou poderiam requerer; ou sobre quão frequentemente os membros duma família estão em contacto uns com os outros.</skos:definition>
      <skos:prefLabel xml:lang="sl">Družina</skos:prefLabel>
      <skos:definition xml:lang="sl">Dva ali več posameznikov, ki so medseboj sorodstveno povezani, ali z zakonsko oz. zunanjzakonsko partnersko zvezo (vključuje tudi vzpostavljeno družino), ali s posvojitvijo ali z rejništvom. Ti posamezniki lahko živijo skupaj ali pa ne (National Community Services Data Dictionary, Vers 3, AIHW, 2004). Na primer podatki o tem, kakšne javne storitve družina uporablja ali bi jih potrebovala; ali kako pogosto so družinski člani v medsebojnem stiku.</skos:definition>
      <skos:prefLabel xml:lang="sl">Družina</skos:prefLabel>
      <skos:definition xml:lang="sl">Dva ali več posameznikov, ki so medseboj sorodstveno povezani, ali z zakonsko oz. zunanjzakonsko partnersko zvezo (vključuje tudi vzpostavljeno družino), ali s posvojitvijo ali z rejništvom. Ti posamezniki lahko živijo skupaj ali pa ne (National Community Services Data Dictionary, Vers 3, AIHW, 2004). Na primer podatki o tem, kakšne javne storitve družina uporablja ali bi jih potrebovala; ali kako pogosto so družinski člani v medsebojnem stiku.</skos:definition>
      <skos:prefLabel xml:lang="sv">Familj</skos:prefLabel>
      <skos:definition xml:lang="sv">Två eller fler personer som är släkt genom blodsband, äktenskap (inklusive styvsyskon, -föräldrar, -barn m.m.), samboskap eller registrerat partnerskap, adoption eller fosterfamiljeskap, men som inte nödvändigtvis bor tillsammans. Till exempel data om vilka offentliga tjänster familjen använder eller skulle vara i behov av, eller hur ofta familjemedlemmar har kontakt med varandra.</skos:definition>
      <skos:prefLabel xml:lang="sv">Familj</skos:prefLabel>
      <skos:definition xml:lang="sv">Två eller fler personer som är släkt genom blodsband, äktenskap (inklusive styvsyskon, -föräldrar, -barn m.m.), samboskap eller registrerat partnerskap, adoption eller fosterfamiljeskap, men som inte nödvändigtvis bor tillsammans. Till exempel data om vilka offentliga tjänster familjen använder eller skulle vara i behov av, eller hur ofta familjemedlemmar har kontakt med varandra.</skos:definition>
      <skos:prefLabel xml:lang="sv">Familj</skos:prefLabel>
      <skos:definition xml:lang="sv">Två eller fler personer som är släkt genom blodsband, äktenskap (inklusive styvsyskon, -föräldrar, -barn m.m.), samboskap eller registrerat partnerskap, adoption eller fosterfamiljeskap, men som inte nödvändigtvis bor tillsammans. Till exempel data om vilka offentliga tjänster familjen använder eller skulle vara i behov av, eller hur ofta familjemedlemmar har kontakt med varandra.</skos:definition>
      <skos:narrower rdf:resource="http://rdf-vocabulary.ddialliance.org/cv/AnalysisUnit/2.1.3/d151e355"/>
   </rdf:Description>
   <rdf:Description rdf:about="http://rdf-vocabulary.ddialliance.org/cv/AnalysisUnit/2.1.3/d151e355">
      <rdf:type rdf:resource="http://www.w3.org/2004/02/skos/core#Concept"/>
      <skos:inScheme rdf:resource="http://rdf-vocabulary.ddialliance.org/cv/AnalysisUnit/2.1.3/"/>
      <skos:notation>Family.HouseholdFamily</skos:notation>
      <skos:prefLabel xml:lang="en">Family: Household family</skos:prefLabel>
      <skos:definition xml:lang="en">A more specific term that refers only to people who are related through family ties (see definition for 'Family') and live in the same household at a point in time. If not known whether the analysis unit is 'Family' or 'Household family', use 'Family'.</skos:definition>
      <skos:prefLabel xml:lang="en">Family: Household family</skos:prefLabel>
      <skos:definition xml:lang="en">A more specific term that refers only to people who are related through family ties (see definition for 'Family') and live in the same household at a point in time. If not known whether the analysis unit is 'Family' or 'Household family', use 'Family'.</skos:definition>
      <skos:prefLabel xml:lang="de">Familie: Familienhaushalt</skos:prefLabel>
      <skos:definition xml:lang="de">Ein spezifischerer Begriff, der sich nur auf Personen bezieht, die durch familiäre Bindungen miteinander verbunden sind (siehe Definition für "Familie") und zu einem bestimmten Zeitpunkt im selben Haushalt leben. Wenn nicht bekannt ist, ob die Analyseeinheit "Familie" oder "Familienhaushalt" ist, verwenden Sie "Familie".</skos:definition>
      <skos:prefLabel xml:lang="de">Familie: Familienhaushalt</skos:prefLabel>
      <skos:definition xml:lang="de">Ein spezifischerer Begriff, der sich nur auf Personen bezieht, die durch familiäre Bindungen miteinander verbunden sind (siehe Definition für "Familie") und zu einem bestimmten Zeitpunkt im selben Haushalt leben. Wenn nicht bekannt ist, ob die Analyseeinheit "Familie" oder "Familienhaushalt" ist, verwenden Sie "Familie".</skos:definition>
      <skos:prefLabel xml:lang="fi">Perhe: perhekotitalous</skos:prefLabel>
      <skos:definition xml:lang="fi">Spesifimpi termi, joka viittaa kotitalouteen, jossa tietyllä hetkellä yhdessä asuvat henkilöt myös kuuluvat perheeseen (katso määritelmä termille 'Perhe'). Jos ei tiedossa, onko kyseessä 'Perhe' vai 'Perhekotitalous', käytä 'Perhe'.</skos:definition>
      <skos:prefLabel xml:lang="fi">Perhe: perhekotitalous</skos:prefLabel>
      <skos:definition xml:lang="fi">Spesifimpi termi, joka viittaa kotitalouteen, jossa tietyllä hetkellä yhdessä asuvat henkilöt myös kuuluvat perheeseen (katso määritelmä termille 'Perhe'). Jos ei tiedossa, onko kyseessä 'Perhe' vai 'Perhekotitalous', käytä 'Perhe'.</skos:definition>
      <skos:prefLabel xml:lang="it">Famiglia: Famiglia convivente</skos:prefLabel>
      <skos:definition xml:lang="it">Un termine più specifico che si riferisce solo a persone che sono legate da vincoli familiari (si veda la definizione di "Famiglia") e che vivono nella stessa abitazione in un determinato momento. Se non è possibile distinguere tra "Famiglia" e "Famiglia convivente" come unità di analisi, utilizzare "Famiglia"</skos:definition>
      <skos:prefLabel xml:lang="it">Famiglia: Famiglia convivente</skos:prefLabel>
      <skos:definition xml:lang="it">Un termine più specifico che si riferisce solo a persone che sono legate da vincoli familiari (si veda la definizione di "Famiglia") e che vivono nella stessa abitazione in un determinato momento. Se non è possibile distinguere tra "Famiglia" e "Famiglia convivente" come unità di analisi, utilizzare "Famiglia"</skos:definition>
      <skos:prefLabel xml:lang="lt">Šeima: šeiminis namų ūkis</skos:prefLabel>
      <skos:definition xml:lang="lt">Konkretesnis terminas, nurodantis tik žmones, kurie yra susiję šeimos ryšiais (žr. apibrėžimą „Šeima“) ir tuo pačiu metu gyvena tame pačiame namų ūkyje. Jei nežinoma, ar analizės vienetas yra „Šeima“, ar „Šeimos namų ūkis“, naudoti „Šeima“.</skos:definition>
      <skos:prefLabel xml:lang="lt">Šeima: šeiminis namų ūkis</skos:prefLabel>
      <skos:definition xml:lang="lt">Konkretesnis terminas, nurodantis tik žmones, kurie yra susiję šeimos ryšiais (žr. apibrėžimą „Šeima“) ir tuo pačiu metu gyvena tame pačiame namų ūkyje. Jei nežinoma, ar analizės vienetas yra „Šeima“, ar „Šeimos namų ūkis“, naudoti „Šeima“.</skos:definition>
      <skos:prefLabel xml:lang="nl">Gezin</skos:prefLabel>
      <skos:definition xml:lang="nl"/>
      <skos:prefLabel xml:lang="nl">Gezin</skos:prefLabel>
      <skos:definition xml:lang="nl"/>
      <skos:prefLabel xml:lang="no">Familie: familiehusholdning</skos:prefLabel>
      <skos:definition xml:lang="no">Et mer spesifikt begrep som kun referer til personer som er beslektet gjennom familierelasjoner (se definisjonen for 'Familie') og som bor i den samme husholdningen på et gitt tidspunkt. Om det ikke er kjent om analyseenheten er 'Familie' eller 'Familiehusholdning' skal begrepet 'Familie' benyttes.</skos:definition>
      <skos:prefLabel xml:lang="no">Familie: familiehusholdning</skos:prefLabel>
      <skos:definition xml:lang="no">Et mer spesifikt begrep som kun referer til personer som er beslektet gjennom familierelasjoner (se definisjonen for 'Familie') og som bor i den samme husholdningen på et gitt tidspunkt. Om det ikke er kjent om analyseenheten er 'Familie' eller 'Familiehusholdning' skal begrepet 'Familie' benyttes.</skos:definition>
      <skos:prefLabel xml:lang="pt">Família: Agregado familiar</skos:prefLabel>
      <skos:definition xml:lang="pt">Termo mais específico que se refere apenas a pessoas que estão relacionadas através de ligações familiares (ver definição de 'Família') e que moram no mesmo domicílio em determinado momento. Se não souber se a unidade de análise é 'Família' ou 'Agregado familiar', usar 'Família'.</skos:definition>
      <skos:prefLabel xml:lang="pt">Família: Agregado familiar</skos:prefLabel>
      <skos:definition xml:lang="pt">Termo mais específico que se refere apenas a pessoas que estão relacionadas através de ligações familiares (ver definição de 'Família') e que moram no mesmo domicílio em determinado momento. Se não souber se a unidade de análise é 'Família' ou 'Agregado familiar', usar 'Família'.</skos:definition>
      <skos:prefLabel xml:lang="sl">Družina: družina znotraj gospodinjstva</skos:prefLabel>
      <skos:definition xml:lang="sl">Bolj določen izraz, nanaša se le na sorodnike (glej definicijo "Družina"), ki v določenem trenutku živijo v istem gospodinjstvu. Če ni znano, ali je enota analize "Družina" ali "Družina znotraj gospodinjstva", uporabite izraz "Družina".</skos:definition>
      <skos:prefLabel xml:lang="sl">Družina: družina znotraj gospodinjstva</skos:prefLabel>
      <skos:definition xml:lang="sl">Bolj določen izraz, nanaša se le na sorodnike (glej definicijo "Družina"), ki v določenem trenutku živijo v istem gospodinjstvu. Če ni znano, ali je enota analize "Družina" ali "Družina znotraj gospodinjstva", uporabite izraz "Družina".</skos:definition>
      <skos:prefLabel xml:lang="sv">Familj: Familjehushåll</skos:prefLabel>
      <skos:definition xml:lang="sv">En mer specifik term än "Familj". Betecknar endast människor som är släkt genom familjeband (se definitionen för "Familj") och som bor tillsammans i samma hushåll vid en given tidpunkt. Om det inte är känt huruvida analysenheten är "Familj" eller "Familjehushåll" ska "Familj" användas.</skos:definition>
      <skos:prefLabel xml:lang="sv">Familj: Familjehushåll</skos:prefLabel>
      <skos:definition xml:lang="sv">En mer specifik term än "Familj". Betecknar endast människor som är släkt genom familjeband (se definitionen för "Familj") och som bor tillsammans i samma hushåll vid en given tidpunkt. Om det inte är känt huruvida analysenheten är "Familj" eller "Familjehushåll" ska "Familj" användas.</skos:definition>
      <skos:prefLabel xml:lang="sv">Familj: Familjehushåll</skos:prefLabel>
      <skos:definition xml:lang="sv">En mer specifik term än "Familj". Betecknar endast människor som är släkt genom familjeband (se definitionen för "Familj") och som bor tillsammans i samma hushåll vid en given tidpunkt. Om det inte är känt huruvida analysenheten är "Familj" eller "Familjehushåll" ska "Familj" användas.</skos:definition>
      <skos:broader rdf:resource="http://rdf-vocabulary.ddialliance.org/cv/AnalysisUnit/2.1.3/d151e274"/>
   </rdf:Description>
   <rdf:Description rdf:about="http://rdf-vocabulary.ddialliance.org/cv/AnalysisUnit/2.1.3/d151e435">
      <rdf:type rdf:resource="http://www.w3.org/2004/02/skos/core#Concept"/>
      <skos:inScheme rdf:resource="http://rdf-vocabulary.ddialliance.org/cv/AnalysisUnit/2.1.3/"/>
      <skos:notation>Household</skos:notation>
      <skos:prefLabel xml:lang="en">Household</skos:prefLabel>
      <skos:definition xml:lang="en">A person or a group of persons who share the same dwelling unit and common living arrangements. These common living arrangements may include pooling some, or all, of their income and wealth, and consuming certain types of goods and services collectively, mainly housing and food (Eurostat).</skos:definition>
      <skos:prefLabel xml:lang="en">Household</skos:prefLabel>
      <skos:definition xml:lang="en">A person or a group of persons who share the same dwelling unit and common living arrangements. These common living arrangements may include pooling some, or all, of their income and wealth, and consuming certain types of goods and services collectively, mainly housing and food (Eurostat).</skos:definition>
      <skos:prefLabel xml:lang="de">Haushalt</skos:prefLabel>
      <skos:definition xml:lang="de">Eine Person oder eine Gruppe von Personen, die dieselbe Wohneinheit und gemeinsame Wohnverhältnisse teilen. Zu diesen gemeinsamen Wohnverhältnissen kann es gehören, dass sie einen Teil oder ihr gesamtes Einkommen und Vermögen zusammenlegen und bestimmte Arten von Waren und Dienstleistungen gemeinsam konsumieren, vor allem Wohnraum und Lebensmittel (Eurostat).</skos:definition>
      <skos:prefLabel xml:lang="de">Haushalt</skos:prefLabel>
      <skos:definition xml:lang="de">Eine Person oder eine Gruppe von Personen, die dieselbe Wohneinheit und gemeinsame Wohnverhältnisse teilen. Zu diesen gemeinsamen Wohnverhältnissen kann es gehören, dass sie einen Teil oder ihr gesamtes Einkommen und Vermögen zusammenlegen und bestimmte Arten von Waren und Dienstleistungen gemeinsam konsumieren, vor allem Wohnraum und Lebensmittel (Eurostat).</skos:definition>
      <skos:prefLabel xml:lang="fi">Kotitalous</skos:prefLabel>
      <skos:definition xml:lang="fi">Kotitalouden muodostaa yksi henkilö tai ryhmä henkilöitä, jotka asuvat yhdessä ja joilla on kokonaan tai osittain yhteinen ruokatalous tai jotka muuten käyttävät tulojaan ja varallisuuttaan ainakin osittain yhdessä.</skos:definition>
      <skos:prefLabel xml:lang="fi">Kotitalous</skos:prefLabel>
      <skos:definition xml:lang="fi">Kotitalouden muodostaa yksi henkilö tai ryhmä henkilöitä, jotka asuvat yhdessä ja joilla on kokonaan tai osittain yhteinen ruokatalous tai jotka muuten käyttävät tulojaan ja varallisuuttaan ainakin osittain yhdessä.</skos:definition>
      <skos:prefLabel xml:lang="it">Conviventi</skos:prefLabel>
      <skos:definition xml:lang="it">Una persona o un gruppo di persone che condividono la stessa unità abitativa e le stesse modalità di vita comuni. Queste modalità di vita comuni possono includere la condivisione di alcuni oppure di tutti i redditi e ricchezze, e il consumo collettivo di determinati tipi di beni e servizi, principalmente alloggi e cibo (Eurostat)</skos:definition>
      <skos:prefLabel xml:lang="it">Conviventi</skos:prefLabel>
      <skos:definition xml:lang="it">Una persona o un gruppo di persone che condividono la stessa unità abitativa e le stesse modalità di vita comuni. Queste modalità di vita comuni possono includere la condivisione di alcuni oppure di tutti i redditi e ricchezze, e il consumo collettivo di determinati tipi di beni e servizi, principalmente alloggi e cibo (Eurostat)</skos:definition>
      <skos:prefLabel xml:lang="lt">Namų ūkis</skos:prefLabel>
      <skos:definition xml:lang="lt">Asmuo ar asmenų grupė, kuri dalinasi tuo pačiu būsto vienetu ir bendra gyvenimo tvarka. Ši bendro gyvenimo tvarka gali apimti kai kurių arba visų pajamų ir turto bendrą kaupimą, tam tikrų tipų prekių ir paslaugų vartojimą, dažniausiai susijusį su būstu ir maistu (pagal Eurostatą).</skos:definition>
      <skos:prefLabel xml:lang="lt">Namų ūkis</skos:prefLabel>
      <skos:definition xml:lang="lt">Asmuo ar asmenų grupė, kuri dalinasi tuo pačiu būsto vienetu ir bendra gyvenimo tvarka. Ši bendro gyvenimo tvarka gali apimti kai kurių arba visų pajamų ir turto bendrą kaupimą, tam tikrų tipų prekių ir paslaugų vartojimą, dažniausiai susijusį su būstu ir maistu (pagal Eurostatą).</skos:definition>
      <skos:prefLabel xml:lang="nl">Huishouden</skos:prefLabel>
      <skos:definition xml:lang="nl"/>
      <skos:prefLabel xml:lang="nl">Huishouden</skos:prefLabel>
      <skos:definition xml:lang="nl"/>
      <skos:prefLabel xml:lang="no">Husholdning</skos:prefLabel>
      <skos:definition xml:lang="no">En person eller en gruppe av personer som har samme boligenhet og leveforhold. Disse felles leveforholdene kan inkludere at deler av, eller alt av inntekt og eiendom er felles, og at visse type varer og tjenester konsumeres i fellesskap, hovedsakelig bosted og mat (Eurostat).</skos:definition>
      <skos:prefLabel xml:lang="no">Husholdning</skos:prefLabel>
      <skos:definition xml:lang="no">En person eller en gruppe av personer som har samme boligenhet og leveforhold. Disse felles leveforholdene kan inkludere at deler av, eller alt av inntekt og eiendom er felles, og at visse type varer og tjenester konsumeres i fellesskap, hovedsakelig bosted og mat (Eurostat).</skos:definition>
      <skos:prefLabel xml:lang="pt">Agregado doméstico</skos:prefLabel>
      <skos:definition xml:lang="pt">Uma pessoa ou um grupo de pessoas que compartilham a mesma unidade de habitação e vida em comum. Esta última pode incluir a agregação de alguns ou de todos os rendimentos e riqueza e o consumo colectivo de certos tipos de bens e serviços, principalmente alojamento e alimentação (Eurostat).</skos:definition>
      <skos:prefLabel xml:lang="pt">Agregado doméstico</skos:prefLabel>
      <skos:definition xml:lang="pt">Uma pessoa ou um grupo de pessoas que compartilham a mesma unidade de habitação e vida em comum. Esta última pode incluir a agregação de alguns ou de todos os rendimentos e riqueza e o consumo colectivo de certos tipos de bens e serviços, principalmente alojamento e alimentação (Eurostat).</skos:definition>
      <skos:prefLabel xml:lang="sl">Gospodinjstvo</skos:prefLabel>
      <skos:definition xml:lang="sl">Oseba ali skupina oseb, ki si delijo isto stanovanjsko enoto in ureditev skupnega življenja. Te ureditve skupnega življenja lahko vključujejo združevanje nekaterih ali vseh prihodkov in premoženja ter skupno (u)porabo določenih vrst blaga in storitev, predvsem stanovanja in hrane (Eurostat).</skos:definition>
      <skos:prefLabel xml:lang="sl">Gospodinjstvo</skos:prefLabel>
      <skos:definition xml:lang="sl">Oseba ali skupina oseb, ki si delijo isto stanovanjsko enoto in ureditev skupnega življenja. Te ureditve skupnega življenja lahko vključujejo združevanje nekaterih ali vseh prihodkov in premoženja ter skupno (u)porabo določenih vrst blaga in storitev, predvsem stanovanja in hrane (Eurostat).</skos:definition>
      <skos:prefLabel xml:lang="sv">Hushåll</skos:prefLabel>
      <skos:definition xml:lang="sv">En person eller grupp av personer som delar bostad och levnadsförhållanden. Dessa gemensamma levnadsförhållanden kan inkludera att viss eller all inkomst och egendom är gemensam och att vissa sorters varor och tjänster konsumeras gemensamt, företrädelsevis bostad och mat (Eurostat).</skos:definition>
      <skos:prefLabel xml:lang="sv">Hushåll</skos:prefLabel>
      <skos:definition xml:lang="sv">En person eller grupp av personer som delar bostad och levnadsförhållanden. Dessa gemensamma levnadsförhållanden kan inkludera att viss eller all inkomst och egendom är gemensam och att vissa sorters varor och tjänster konsumeras gemensamt, företrädelsevis bostad och mat (Eurostat).</skos:definition>
      <skos:prefLabel xml:lang="sv">Hushåll</skos:prefLabel>
      <skos:definition xml:lang="sv">En person eller grupp av personer som delar bostad och levnadsförhållanden. Dessa gemensamma levnadsförhållanden kan inkludera att viss eller all inkomst och egendom är gemensam och att vissa sorters varor och tjänster konsumeras gemensamt, företrädelsevis bostad och mat (Eurostat).</skos:definition>
   </rdf:Description>
   <rdf:Description rdf:about="http://rdf-vocabulary.ddialliance.org/cv/AnalysisUnit/2.1.3/d151e514">
      <rdf:type rdf:resource="http://www.w3.org/2004/02/skos/core#Concept"/>
      <skos:inScheme rdf:resource="http://rdf-vocabulary.ddialliance.org/cv/AnalysisUnit/2.1.3/"/>
      <skos:notation>HousingUnit</skos:notation>
      <skos:prefLabel xml:lang="en">Housing unit</skos:prefLabel>
      <skos:definition xml:lang="en">U.S. Census: A housing unit is a house, an apartment, a mobile home, a group of rooms, or a single room that is occupied (or if vacant, is intended for occupancy) as separate living quarters. Separate living quarters are those in which the occupants live and eat separately from any other persons in the building and which have direct access from the outside of the building or through a common hall.</skos:definition>
      <skos:prefLabel xml:lang="en">Housing unit</skos:prefLabel>
      <skos:definition xml:lang="en">U.S. Census: A housing unit is a house, an apartment, a mobile home, a group of rooms, or a single room that is occupied (or if vacant, is intended for occupancy) as separate living quarters. Separate living quarters are those in which the occupants live and eat separately from any other persons in the building and which have direct access from the outside of the building or through a common hall.</skos:definition>
      <skos:prefLabel xml:lang="de">Wohneinheit</skos:prefLabel>
      <skos:definition xml:lang="de">Eine Wohneinheit ist ein Haus, eine Wohnung, ein Wohnmobil, eine Gruppe von Räumen oder ein einzelner Raum, der als separater Wohnbereich genutzt wird (oder, wenn er leer steht, zur Nutzung vorgesehen ist). Geschlossene Wohneinheiten sind solche, in denen die Bewohner getrennt von allen anderen Personen im Gebäude leben und essen und die einen direkten Zugang von der Außenseite des Gebäudes oder durch einen gemeinsamen Flur haben.</skos:definition>
      <skos:prefLabel xml:lang="de">Wohneinheit</skos:prefLabel>
      <skos:definition xml:lang="de">Eine Wohneinheit ist ein Haus, eine Wohnung, ein Wohnmobil, eine Gruppe von Räumen oder ein einzelner Raum, der als separater Wohnbereich genutzt wird (oder, wenn er leer steht, zur Nutzung vorgesehen ist). Geschlossene Wohneinheiten sind solche, in denen die Bewohner getrennt von allen anderen Personen im Gebäude leben und essen und die einen direkten Zugang von der Außenseite des Gebäudes oder durch einen gemeinsamen Flur haben.</skos:definition>
      <skos:prefLabel xml:lang="fi">Asuntokunta</skos:prefLabel>
      <skos:definition xml:lang="fi">Asuntokunta voi sijaita talossa, huoneistossa, asuntovaunussa, tai asunnon tietyssä huoneessa tai huoneissa. Asuntokunnnan asuintilassa elävillä henkilöillä on oma erillinen ruokataloutensa ja järjestelynsä. Yhdessä asunnossa voi olla useampia asuntokuntia. Esimerkiksi soluasunnoissa asuvilla opiskelijoilla voi kullakin olla oma ruoka- ja asuntokuntansa. Termi käytössä etenkin Yhdysvalloissa.</skos:definition>
      <skos:prefLabel xml:lang="fi">Asuntokunta</skos:prefLabel>
      <skos:definition xml:lang="fi">Asuntokunta voi sijaita talossa, huoneistossa, asuntovaunussa, tai asunnon tietyssä huoneessa tai huoneissa. Asuntokunnnan asuintilassa elävillä henkilöillä on oma erillinen ruokataloutensa ja järjestelynsä. Yhdessä asunnossa voi olla useampia asuntokuntia. Esimerkiksi soluasunnoissa asuvilla opiskelijoilla voi kullakin olla oma ruoka- ja asuntokuntansa. Termi käytössä etenkin Yhdysvalloissa.</skos:definition>
      <skos:prefLabel xml:lang="it">Unità abitativa</skos:prefLabel>
      <skos:definition xml:lang="it">Un'unità abitativa è una casa, un appartamento, una casa mobile, un gruppo di stanze o una stanza singola occupata (oppure, se non occupata, destinata ad ospitare) come abitazione separata. Le abitazioni separate sono quelli in cui gli occupanti vivono e mangiano separatamente da qualsiasi altra persona presente nell'edificio, e che hanno un accesso diretto dall'esterno dell'edificio oppure attraverso un ingresso comune.</skos:definition>
      <skos:prefLabel xml:lang="it">Unità abitativa</skos:prefLabel>
      <skos:definition xml:lang="it">Un'unità abitativa è una casa, un appartamento, una casa mobile, un gruppo di stanze o una stanza singola occupata (oppure, se non occupata, destinata ad ospitare) come abitazione separata. Le abitazioni separate sono quelli in cui gli occupanti vivono e mangiano separatamente da qualsiasi altra persona presente nell'edificio, e che hanno un accesso diretto dall'esterno dell'edificio oppure attraverso un ingresso comune.</skos:definition>
      <skos:prefLabel xml:lang="lt">Būsto vienetas</skos:prefLabel>
      <skos:definition xml:lang="lt">JAV visuotinis gyventojų surašymas: būsto vienetas – namas, butas, mobilus namelis, kambarių grupė arba atskiras kambarys, kuris yra užimtas (arba jei laisvas, tai skirtas apgyvendinimui), kaip atskira gyvenamoji patalpa. Atskiros gyvenamosios patalpos yra tokios, kuriose gyventojai gyvena bei valgo atskirai nuo kitų pastate esančių asmenų, ir į kurias galima tiesiogiai patekti iš pastato išorės arba per bendrą koridorių.</skos:definition>
      <skos:prefLabel xml:lang="lt">Būsto vienetas</skos:prefLabel>
      <skos:definition xml:lang="lt">JAV visuotinis gyventojų surašymas: būsto vienetas – namas, butas, mobilus namelis, kambarių grupė arba atskiras kambarys, kuris yra užimtas (arba jei laisvas, tai skirtas apgyvendinimui), kaip atskira gyvenamoji patalpa. Atskiros gyvenamosios patalpos yra tokios, kuriose gyventojai gyvena bei valgo atskirai nuo kitų pastate esančių asmenų, ir į kurias galima tiesiogiai patekti iš pastato išorės arba per bendrą koridorių.</skos:definition>
      <skos:prefLabel xml:lang="nl">Wooneenheid</skos:prefLabel>
      <skos:definition xml:lang="nl"/>
      <skos:prefLabel xml:lang="nl">Wooneenheid</skos:prefLabel>
      <skos:definition xml:lang="nl"/>
      <skos:prefLabel xml:lang="no">Boenhet</skos:prefLabel>
      <skos:definition xml:lang="no">USAs folketelling: En boenhet er et hus, en leilighet, et mobilt hjem (campingvogn), eller ett eller flere rom som er bebodd (eventuelt ledig, men som er ment å være bebodd), som adskilte enheter. Med adskilte enheter menes det at personer bor og spiser uavhengig av andre personer i samme boenhet, og som har direkte tilgang til enheten utenfra, eller gjennom en felles inngang.</skos:definition>
      <skos:prefLabel xml:lang="no">Boenhet</skos:prefLabel>
      <skos:definition xml:lang="no">USAs folketelling: En boenhet er et hus, en leilighet, et mobilt hjem (campingvogn), eller ett eller flere rom som er bebodd (eventuelt ledig, men som er ment å være bebodd), som adskilte enheter. Med adskilte enheter menes det at personer bor og spiser uavhengig av andre personer i samme boenhet, og som har direkte tilgang til enheten utenfra, eller gjennom en felles inngang.</skos:definition>
      <skos:prefLabel xml:lang="pt">Unidade residencial</skos:prefLabel>
      <skos:definition xml:lang="pt">Censo dos EUA: Uma unidade residencial é uma casa, um apartamento, uma casa móvel, um grupo de quartos ou um quarto individual que é ocupado (ou, se for vago, destinado a ocupação) enquanto alojamentos/aposentos separados. Alojamentos separados são aqueles em que os ocupantes vivem e comem separadamente de quaisquer outras pessoas no edifício e que têm acesso direto a partir do exterior do edifício ou através de um hall comum.</skos:definition>
      <skos:prefLabel xml:lang="pt">Unidade residencial</skos:prefLabel>
      <skos:definition xml:lang="pt">Censo dos EUA: Uma unidade residencial é uma casa, um apartamento, uma casa móvel, um grupo de quartos ou um quarto individual que é ocupado (ou, se for vago, destinado a ocupação) enquanto alojamentos/aposentos separados. Alojamentos separados são aqueles em que os ocupantes vivem e comem separadamente de quaisquer outras pessoas no edifício e que têm acesso direto a partir do exterior do edifício ou através de um hall comum.</skos:definition>
      <skos:prefLabel xml:lang="sl">Bivalna enota</skos:prefLabel>
      <skos:definition xml:lang="sl">Popis ZDA: Bivalna enota je hiša, stanovanje, mobilna hišica, skupina sob ali enoposteljna soba, ki se uporablja kot ločen bivalni prostor (oziroma je v primeru, da je prazna, namenjena bivanju). Ločeni bivalni prostori so tisti, v katerih stanovalci živijo in se prehranjujejo ločeno od drugih oseb v stavbi in imajo neposreden dostop do prostora pred stavbo ali do skupnega hodnika.</skos:definition>
      <skos:prefLabel xml:lang="sl">Bivalna enota</skos:prefLabel>
      <skos:definition xml:lang="sl">Popis ZDA: Bivalna enota je hiša, stanovanje, mobilna hišica, skupina sob ali enoposteljna soba, ki se uporablja kot ločen bivalni prostor (oziroma je v primeru, da je prazna, namenjena bivanju). Ločeni bivalni prostori so tisti, v katerih stanovalci živijo in se prehranjujejo ločeno od drugih oseb v stavbi in imajo neposreden dostop do prostora pred stavbo ali do skupnega hodnika.</skos:definition>
      <skos:prefLabel xml:lang="sv">Bostadsenhet</skos:prefLabel>
      <skos:definition xml:lang="sv">En bostadsenhet är ett hus, en lägenhet, en husvagn, eller ett eller flera rum som bebos (eller, om den är tom, är avsedd att bebos) som avskild inkvartering. Med avskild inkvartering menas att de som är inkvarterade där bor och äter avskilda från andra personer i byggnaden och kan komma in direkt utifrån eller via en gemensam entré (U.S. Census).</skos:definition>
      <skos:prefLabel xml:lang="sv">Bostadsenhet</skos:prefLabel>
      <skos:definition xml:lang="sv">En bostadsenhet är ett hus, en lägenhet, en husvagn, eller ett eller flera rum som bebos (eller, om den är tom, är avsedd att bebos) som avskild inkvartering. Med avskild inkvartering menas att de som är inkvarterade där bor och äter avskilda från andra personer i byggnaden och kan komma in direkt utifrån eller via en gemensam entré (U.S. Census).</skos:definition>
      <skos:prefLabel xml:lang="sv">Bostadsenhet</skos:prefLabel>
      <skos:definition xml:lang="sv">En bostadsenhet är ett hus, en lägenhet, en husvagn, eller ett eller flera rum som bebos (eller, om den är tom, är avsedd att bebos) som avskild inkvartering. Med avskild inkvartering menas att de som är inkvarterade där bor och äter avskilda från andra personer i byggnaden och kan komma in direkt utifrån eller via en gemensam entré (U.S. Census).</skos:definition>
   </rdf:Description>
   <rdf:Description rdf:about="http://rdf-vocabulary.ddialliance.org/cv/AnalysisUnit/2.1.3/d151e593">
      <rdf:type rdf:resource="http://www.w3.org/2004/02/skos/core#Concept"/>
      <skos:inScheme rdf:resource="http://rdf-vocabulary.ddialliance.org/cv/AnalysisUnit/2.1.3/"/>
      <skos:notation>EventOrProcessOrActivity</skos:notation>
      <skos:prefLabel xml:lang="en">Event/Process/Activity</skos:prefLabel>
      <skos:definition xml:lang="en">Any type of incident, occurrence, or activity. Events are usually one-time, individual occurrences, with a limited or short duration. Examples: criminal offenses, riots, meetings, elections, sports competitions, terrorist attacks, natural disasters like floods, etc. Processes typically take place over time, and may include multiple 'events' or gradual changes that ultimately lead, or are projected to lead, to a particular result. Examples: court trials, criminal investigations, political campaigns, medical treatments, education, athletes' training, etc. Use when the main focus is more on the event, process or activity itself. For example, a field observation study on slot machine gambling; or data collected on child abuse cases, such as the type and duration of abuse, the role of the persons involved, etc.</skos:definition>
      <skos:prefLabel xml:lang="en">Event/Process/Activity</skos:prefLabel>
      <skos:definition xml:lang="en">Any type of incident, occurrence, or activity. Events are usually one-time, individual occurrences, with a limited or short duration. Examples: criminal offenses, riots, meetings, elections, sports competitions, terrorist attacks, natural disasters like floods, etc. Processes typically take place over time, and may include multiple 'events' or gradual changes that ultimately lead, or are projected to lead, to a particular result. Examples: court trials, criminal investigations, political campaigns, medical treatments, education, athletes' training, etc. Use when the main focus is more on the event, process or activity itself. For example, a field observation study on slot machine gambling; or data collected on child abuse cases, such as the type and duration of abuse, the role of the persons involved, etc.</skos:definition>
      <skos:prefLabel xml:lang="de">Ereignis/Prozess/Aktivität</skos:prefLabel>
      <skos:definition xml:lang="de">Jede Art von Vorfall, Vorkommnis oder Aktivität. Ereignisse sind in der Regel einmalige, individuelle Vorkommnisse, mit einer begrenzten oder kurzen Dauer. Beispiele: Straftaten, Unruhen, Versammlungen, Wahlen, Sportwettkämpfe, Terroranschläge, Naturkatastrophen wie Überschwemmungen usw. Prozesse finden typischerweise im Laufe der Zeit statt und können mehrere "Ereignisse" oder allmähliche Veränderungen umfassen, die letztendlich zu einem bestimmten Ergebnis führen oder führen sollen. Beispiele: Gerichtsverhandlungen, strafrechtliche Ermittlungen, politische Kampagnen, medizinische Behandlungen, Bildung, Training von Sportlern usw. Der Begriff wird verwendet, wenn das Hauptaugenmerk eher auf dem Ereignis, dem Prozess oder der Aktivität selbst liegt. Beispiele: eine Feldbeobachtungsstudie zum Glücksspiel an Spielautomaten.</skos:definition>
      <skos:prefLabel xml:lang="de">Ereignis/Prozess/Aktivität</skos:prefLabel>
      <skos:definition xml:lang="de">Jede Art von Vorfall, Vorkommnis oder Aktivität. Ereignisse sind in der Regel einmalige, individuelle Vorkommnisse, mit einer begrenzten oder kurzen Dauer. Beispiele: Straftaten, Unruhen, Versammlungen, Wahlen, Sportwettkämpfe, Terroranschläge, Naturkatastrophen wie Überschwemmungen usw. Prozesse finden typischerweise im Laufe der Zeit statt und können mehrere "Ereignisse" oder allmähliche Veränderungen umfassen, die letztendlich zu einem bestimmten Ergebnis führen oder führen sollen. Beispiele: Gerichtsverhandlungen, strafrechtliche Ermittlungen, politische Kampagnen, medizinische Behandlungen, Bildung, Training von Sportlern usw. Der Begriff wird verwendet, wenn das Hauptaugenmerk eher auf dem Ereignis, dem Prozess oder der Aktivität selbst liegt. Beispiele: eine Feldbeobachtungsstudie zum Glücksspiel an Spielautomaten.</skos:definition>
      <skos:prefLabel xml:lang="fi">Tapahtuma/prosessi/toiminta</skos:prefLabel>
      <skos:definition xml:lang="fi">Tapahtuma, tapahtumasarja, toiminta tai prosessi. Tapahtumat ovat usein lyhytaikaisia ja kertaluonteisia, esimerkiksi mellakat, kokoukset, urheilukilpailut, terroristihyökkäykset ja luonnonkatastrofit. Prosessit ovat tyypillisesti pidempikestoisia, voivat sisältää useampia tapahtumia tai vähittäisiä muutoksia, jotka lopuksi johtavat tiettyyn tulokseen. Esimerkiksi oikeusjutut, rikostutkimukset, poliittiset kampanjat, kuntoutushoidot, koulutus. Tapahtuma/prosessi/toiminta -termiä käytetään silloin, kun tutkimuksessa keskitytään kyseiseen tapahtumaan, prosessiin tai toimintaan, ei henkilöihin sinänsä. Esimerkiksi havainnointitutkimus peliautomaattipelaamisesta; tutkimus lasten pahoinpitelytapauksista, niiden tyypistä ja kestosta, osallistuvien henkilöiden roolista niissä.</skos:definition>
      <skos:prefLabel xml:lang="fi">Tapahtuma/prosessi/toiminta</skos:prefLabel>
      <skos:definition xml:lang="fi">Tapahtuma, tapahtumasarja, toiminta tai prosessi. Tapahtumat ovat usein lyhytaikaisia ja kertaluonteisia, esimerkiksi mellakat, kokoukset, urheilukilpailut, terroristihyökkäykset ja luonnonkatastrofit. Prosessit ovat tyypillisesti pidempikestoisia, voivat sisältää useampia tapahtumia tai vähittäisiä muutoksia, jotka lopuksi johtavat tiettyyn tulokseen. Esimerkiksi oikeusjutut, rikostutkimukset, poliittiset kampanjat, kuntoutushoidot, koulutus. Tapahtuma/prosessi/toiminta -termiä käytetään silloin, kun tutkimuksessa keskitytään kyseiseen tapahtumaan, prosessiin tai toimintaan, ei henkilöihin sinänsä. Esimerkiksi havainnointitutkimus peliautomaattipelaamisesta; tutkimus lasten pahoinpitelytapauksista, niiden tyypistä ja kestosta, osallistuvien henkilöiden roolista niissä.</skos:definition>
      <skos:prefLabel xml:lang="it">Evento/Processo/Attività</skos:prefLabel>
      <skos:definition xml:lang="it">Qualsiasi tipo di episodio, evento o attività. Gli eventi sono generalmente occorrenze singole, con una durata limitata oppure breve. Esempi: reati, rivolte, riunioni, elezioni, competizioni sportive, attacchi terroristici, calamità naturali come inondazioni, ecc. I processi generalmente durano nel tempo, e possono includere "eventi" multipli o cambiamenti graduali che alla fine conducono, oppure tendono a condurre, a un risultato particolare. Esempi: processi giudiziari, indagini penali, campagne politiche, trattamenti sanitari, istruzione, allenamenti sportivi, ecc. Utilizzare quando l'attenzione è riposta principalmente sull'evento, sul processo o sull'attività stessa. Ad esempio, uno studio che prevede un'osservazione sul campo relativa al gioco d'azzardo attraverso slot machine; oppure dati raccolti su casi di abuso su minori, come il tipo e la durata dell'abuso, il ruolo delle persone coinvolte, ecc.</skos:definition>
      <skos:prefLabel xml:lang="it">Evento/Processo/Attività</skos:prefLabel>
      <skos:definition xml:lang="it">Qualsiasi tipo di episodio, evento o attività. Gli eventi sono generalmente occorrenze singole, con una durata limitata oppure breve. Esempi: reati, rivolte, riunioni, elezioni, competizioni sportive, attacchi terroristici, calamità naturali come inondazioni, ecc. I processi generalmente durano nel tempo, e possono includere "eventi" multipli o cambiamenti graduali che alla fine conducono, oppure tendono a condurre, a un risultato particolare. Esempi: processi giudiziari, indagini penali, campagne politiche, trattamenti sanitari, istruzione, allenamenti sportivi, ecc. Utilizzare quando l'attenzione è riposta principalmente sull'evento, sul processo o sull'attività stessa. Ad esempio, uno studio che prevede un'osservazione sul campo relativa al gioco d'azzardo attraverso slot machine; oppure dati raccolti su casi di abuso su minori, come il tipo e la durata dell'abuso, il ruolo delle persone coinvolte, ecc.</skos:definition>
      <skos:prefLabel xml:lang="lt">Įvykis, procesas ar veikla</skos:prefLabel>
      <skos:definition xml:lang="lt">Bet kokio tipo atsitikimas, atvejis ar veikla. Įvykiai paprastai būna vienkartiniai, atskiri, ribotos arba trumpos trukmės. Pavyzdžiai: nusikalstamos veikos, riaušės, susitikimai, rinkimai, sporto varžybos, teroristiniai išpuoliai, stichinės nelaimės (pvz.  potvyniai) ir kt. Procesai paprastai vyksta tam tikrą laiką ir gali apimti kelis „įvykius“ ar laipsniškus pokyčius, kurie galų gale lemia arba, kaip tikimasi, veda prie konkretaus rezultato. Pavyzdžiai: teismo procesai, kriminaliniai tyrimai, politinės kampanijos, medicininis gydymas, ugdymas, sportininkų rengimas ir kt. Naudoti, kai pagrindinis dėmesys skiriamas labiau pačiam įvykiui, procesui ar veiklai. Pavyzdžiui, lauko stebėjimo tyrimas apie lošimą žaidimų automatais; arba duomenų rinkimas apie vaikų išnaudojimo atvejus, pvz. išnaudojimo rūšis ir trukmę, dalyvaujančių asmenų vaidmenis ir kt.</skos:definition>
      <skos:prefLabel xml:lang="lt">Įvykis, procesas ar veikla</skos:prefLabel>
      <skos:definition xml:lang="lt">Bet kokio tipo atsitikimas, atvejis ar veikla. Įvykiai paprastai būna vienkartiniai, atskiri, ribotos arba trumpos trukmės. Pavyzdžiai: nusikalstamos veikos, riaušės, susitikimai, rinkimai, sporto varžybos, teroristiniai išpuoliai, stichinės nelaimės (pvz.  potvyniai) ir kt. Procesai paprastai vyksta tam tikrą laiką ir gali apimti kelis „įvykius“ ar laipsniškus pokyčius, kurie galų gale lemia arba, kaip tikimasi, veda prie konkretaus rezultato. Pavyzdžiai: teismo procesai, kriminaliniai tyrimai, politinės kampanijos, medicininis gydymas, ugdymas, sportininkų rengimas ir kt. Naudoti, kai pagrindinis dėmesys skiriamas labiau pačiam įvykiui, procesui ar veiklai. Pavyzdžiui, lauko stebėjimo tyrimas apie lošimą žaidimų automatais; arba duomenų rinkimas apie vaikų išnaudojimo atvejus, pvz. išnaudojimo rūšis ir trukmę, dalyvaujančių asmenų vaidmenis ir kt.</skos:definition>
      <skos:prefLabel xml:lang="nl">Event/Proces/Activteit</skos:prefLabel>
      <skos:definition xml:lang="nl"/>
      <skos:prefLabel xml:lang="nl">Event/Proces/Activteit</skos:prefLabel>
      <skos:definition xml:lang="nl"/>
      <skos:prefLabel xml:lang="no">Hendelse/prosess/aktivitet</skos:prefLabel>
      <skos:definition xml:lang="no">Enhver form for hendelse, begivenhet eller aktivitet. Hendelser er som oftest enkeltstående med begrenset eller kort varighet. For eksempel: kriminell handling, opptøyer, møter, valg, idrettsbegivenheter, terroristangrep, naturkatastrofer osv. Prosesser finner som regel sted over tid, og kan inkludere flere 'hendelser' eller gradvise endringer som etterhvert fører til, eller er anslått å føre til, et bestemt resultat. For eksempel: rettsaker, kriminaletterforskning, politiske kampanjer, medisinsk behandling, utdanning, idrettsutøveres treninger etc. Bruk når selve fokuset er mer på hendelsen, prosessen eller aktiviteten. For eksempel: feltobservasjonsstudie på spillemaskiner; eller data samlet inn om barnemishandlingssaker, med hensyn til type og varigheten til mishandlingen og rollen personer involvert har etc.</skos:definition>
      <skos:prefLabel xml:lang="no">Hendelse/prosess/aktivitet</skos:prefLabel>
      <skos:definition xml:lang="no">Enhver form for hendelse, begivenhet eller aktivitet. Hendelser er som oftest enkeltstående med begrenset eller kort varighet. For eksempel: kriminell handling, opptøyer, møter, valg, idrettsbegivenheter, terroristangrep, naturkatastrofer osv. Prosesser finner som regel sted over tid, og kan inkludere flere 'hendelser' eller gradvise endringer som etterhvert fører til, eller er anslått å føre til, et bestemt resultat. For eksempel: rettsaker, kriminaletterforskning, politiske kampanjer, medisinsk behandling, utdanning, idrettsutøveres treninger etc. Bruk når selve fokuset er mer på hendelsen, prosessen eller aktiviteten. For eksempel: feltobservasjonsstudie på spillemaskiner; eller data samlet inn om barnemishandlingssaker, med hensyn til type og varigheten til mishandlingen og rollen personer involvert har etc.</skos:definition>
      <skos:prefLabel xml:lang="pt">Evento/Processo/Atividade</skos:prefLabel>
      <skos:definition xml:lang="pt">Qualquer tipo de incidente, ocorrência ou atividade. Os eventos são geralmente ocorrências únicas e isoladas, com duração limitada ou curta. Exemplos: infrações criminais, tumultos, reuniões, eleições, competições desportivas, ataques terroristas, desastres naturais como inundações, etc. Os processos geralmente ocorrem ao longo do tempo e podem incluir múltiplos 'eventos' ou mudanças graduais que conduzem ou podem conduzir a um resultado particular. Exemplos: julgamentos em tribunal, investigações criminais, campanhas políticas, tratamentos médicos, educação, formação de atletas, etc. Usar quando o principal foco é mais no evento, processo ou atividade. Por exemplo, um estudo de observação no terreno sobre máquinas automáticas de jogos; ou dados recolhidos sobre casos de abuso de crianças, como o tipo e a duração do abuso, o papel das pessoas envolvidas, etc.</skos:definition>
      <skos:prefLabel xml:lang="pt">Evento/Processo/Atividade</skos:prefLabel>
      <skos:definition xml:lang="pt">Qualquer tipo de incidente, ocorrência ou atividade. Os eventos são geralmente ocorrências únicas e isoladas, com duração limitada ou curta. Exemplos: infrações criminais, tumultos, reuniões, eleições, competições desportivas, ataques terroristas, desastres naturais como inundações, etc. Os processos geralmente ocorrem ao longo do tempo e podem incluir múltiplos 'eventos' ou mudanças graduais que conduzem ou podem conduzir a um resultado particular. Exemplos: julgamentos em tribunal, investigações criminais, campanhas políticas, tratamentos médicos, educação, formação de atletas, etc. Usar quando o principal foco é mais no evento, processo ou atividade. Por exemplo, um estudo de observação no terreno sobre máquinas automáticas de jogos; ou dados recolhidos sobre casos de abuso de crianças, como o tipo e a duração do abuso, o papel das pessoas envolvidas, etc.</skos:definition>
      <skos:prefLabel xml:lang="sl">Dogodek/proces/dejavnost</skos:prefLabel>
      <skos:definition xml:lang="sl">Katerakoli vrsta dogodka, pojava ali dejavnosti. Dogodki so običajno enkratni, posamezni pojavi, omejenega ali kratkega trajanja. Primeri: kazniva dejanja, neredi, sestanki, volitve, športna tekmovanja, teroristični napadi, naravne nesreče, kot so poplave ipd. Procesi običajno potekajo dalj časa in lahko vključujejo več "dogodkov" ali postopnih sprememb, ki na koncu vodijo ali bodo predvidoma vodili do določenega rezultata. Primeri: sodni postopki, kazenske preiskave, politične kampanje, zdravljenje, izobraževanje, športni trening itd. Uporabite, kadar je glavni poudarek bolj na dogodku, postopku ali sami dejavnosti. Na primer terenska raziskava z opazovanjem igranja na srečo na igralnih avtomatih; ali zbrani podatki o primerih zlorabe otrok, kot so vrsta in trajanje zlorabe, vloga vpletenih oseb itd.</skos:definition>
      <skos:prefLabel xml:lang="sl">Dogodek/proces/dejavnost</skos:prefLabel>
      <skos:definition xml:lang="sl">Katerakoli vrsta dogodka, pojava ali dejavnosti. Dogodki so običajno enkratni, posamezni pojavi, omejenega ali kratkega trajanja. Primeri: kazniva dejanja, neredi, sestanki, volitve, športna tekmovanja, teroristični napadi, naravne nesreče, kot so poplave ipd. Procesi običajno potekajo dalj časa in lahko vključujejo več "dogodkov" ali postopnih sprememb, ki na koncu vodijo ali bodo predvidoma vodili do določenega rezultata. Primeri: sodni postopki, kazenske preiskave, politične kampanje, zdravljenje, izobraževanje, športni trening itd. Uporabite, kadar je glavni poudarek bolj na dogodku, postopku ali sami dejavnosti. Na primer terenska raziskava z opazovanjem igranja na srečo na igralnih avtomatih; ali zbrani podatki o primerih zlorabe otrok, kot so vrsta in trajanje zlorabe, vloga vpletenih oseb itd.</skos:definition>
      <skos:prefLabel xml:lang="sv">Händelse/process/aktivitet</skos:prefLabel>
      <skos:definition xml:lang="sv">En företeelse, tilldragelse eller aktivitet. Händelser är vanligtvis enstaka företeelser med begränsad eller kort varaktighet. Exempel: brott, upplopp, möten, val, idrottstävlingar, terroristangrepp, naturkatastrofer som översvämningar o.dyl. Processer utspelar sig vanligtvis över tid och kan omfatta flera "händelser" eller gradvisa förändringar som slutligen resulterar i, eller kan tänkas resultera i, en viss utgång. Exempel: rättegångar, brottsutredningar, politiska kampanjer, medicinska behandlingar, utbildning, en idrottsutövares träning, m.m. Använd detta begrepp när fokus ligger på själva händelsen, processen eller aktiviteten. Till exempel en fältobservationsstudie om spel på spelautomater; eller data om fall av övergrepp på barn, som typ av och varaktighet för övergreppet, de inblandade personernas roller osv.</skos:definition>
      <skos:prefLabel xml:lang="sv">Händelse/process/aktivitet</skos:prefLabel>
      <skos:definition xml:lang="sv">En företeelse, tilldragelse eller aktivitet. Händelser är vanligtvis enstaka företeelser med begränsad eller kort varaktighet. Exempel: brott, upplopp, möten, val, idrottstävlingar, terroristangrepp, naturkatastrofer som översvämningar o.dyl. Processer utspelar sig vanligtvis över tid och kan omfatta flera "händelser" eller gradvisa förändringar som slutligen resulterar i, eller kan tänkas resultera i, en viss utgång. Exempel: rättegångar, brottsutredningar, politiska kampanjer, medicinska behandlingar, utbildning, en idrottsutövares träning, m.m. Använd detta begrepp när fokus ligger på själva händelsen, processen eller aktiviteten. Till exempel en fältobservationsstudie om spel på spelautomater; eller data om fall av övergrepp på barn, som typ av och varaktighet för övergreppet, de inblandade personernas roller osv.</skos:definition>
      <skos:prefLabel xml:lang="sv">Händelse/process/aktivitet</skos:prefLabel>
      <skos:definition xml:lang="sv">En företeelse, tilldragelse eller aktivitet. Händelser är vanligtvis enstaka företeelser med begränsad eller kort varaktighet. Exempel: brott, upplopp, möten, val, idrottstävlingar, terroristangrepp, naturkatastrofer som översvämningar o.dyl. Processer utspelar sig vanligtvis över tid och kan omfatta flera "händelser" eller gradvisa förändringar som slutligen resulterar i, eller kan tänkas resultera i, en viss utgång. Exempel: rättegångar, brottsutredningar, politiska kampanjer, medicinska behandlingar, utbildning, en idrottsutövares träning, m.m. Använd detta begrepp när fokus ligger på själva händelsen, processen eller aktiviteten. Till exempel en fältobservationsstudie om spel på spelautomater; eller data om fall av övergrepp på barn, som typ av och varaktighet för övergreppet, de inblandade personernas roller osv.</skos:definition>
   </rdf:Description>
   <rdf:Description rdf:about="http://rdf-vocabulary.ddialliance.org/cv/AnalysisUnit/2.1.3/d151e672">
      <rdf:type rdf:resource="http://www.w3.org/2004/02/skos/core#Concept"/>
      <skos:inScheme rdf:resource="http://rdf-vocabulary.ddialliance.org/cv/AnalysisUnit/2.1.3/"/>
      <skos:notation>GeographicUnit</skos:notation>
      <skos:prefLabel xml:lang="en">Geographic unit</skos:prefLabel>
      <skos:definition xml:lang="en">Any entity that can be spatially defined as a geographic area, with either natural (physical) or administrative boundaries. For example, data on home sales, landscaping changes, new constructions, or changes in the demographic composition of certain regions or districts.</skos:definition>
      <skos:prefLabel xml:lang="en">Geographic unit</skos:prefLabel>
      <skos:definition xml:lang="en">Any entity that can be spatially defined as a geographic area, with either natural (physical) or administrative boundaries. For example, data on home sales, landscaping changes, new constructions, or changes in the demographic composition of certain regions or districts.</skos:definition>
      <skos:prefLabel xml:lang="de">Geographische Einheit</skos:prefLabel>
      <skos:definition xml:lang="de">Jede Einheit, die räumlich als ein geographisches Gebiet definiert werden kann, entweder mit natürlichen (physischen) oder administrativen Grenzen. Zum Beispiel Daten über Hausverkäufe, Landschaftsveränderungen, Neubauten oder Veränderungen in der demographischen Zusammensetzung bestimmter Regionen oder Bezirke.</skos:definition>
      <skos:prefLabel xml:lang="de">Geographische Einheit</skos:prefLabel>
      <skos:definition xml:lang="de">Jede Einheit, die räumlich als ein geographisches Gebiet definiert werden kann, entweder mit natürlichen (physischen) oder administrativen Grenzen. Zum Beispiel Daten über Hausverkäufe, Landschaftsveränderungen, Neubauten oder Veränderungen in der demographischen Zusammensetzung bestimmter Regionen oder Bezirke.</skos:definition>
      <skos:prefLabel xml:lang="fi">Maantieteellinen yksikkö</skos:prefLabel>
      <skos:definition xml:lang="fi">Mikä tahansa maantieteellisesti määriteltävissä oleva alue, jolla on joko luontaiset fyysiset rajat tai hallinnolliset rajat. Esimerkiksi muutokset tiettyjen alueiden väestössä tai asuntojen myyntiluvut tai rakennusluvat tietyllä alueella.</skos:definition>
      <skos:prefLabel xml:lang="fi">Maantieteellinen yksikkö</skos:prefLabel>
      <skos:definition xml:lang="fi">Mikä tahansa maantieteellisesti määriteltävissä oleva alue, jolla on joko luontaiset fyysiset rajat tai hallinnolliset rajat. Esimerkiksi muutokset tiettyjen alueiden väestössä tai asuntojen myyntiluvut tai rakennusluvat tietyllä alueella.</skos:definition>
      <skos:prefLabel xml:lang="it">Unità geografica</skos:prefLabel>
      <skos:definition xml:lang="it">Qualsiasi entità che possa essere definita nello spazio, come un'area geografica, con confini naturali (fisici) o amministrativi. Ad esempio, i dati sulle vendite di case, sui mutamenti del paesaggio, sulle nuove costruzioni o sui cambiamenti nella composizione demografica di alcune regioni o distretti territoriali.</skos:definition>
      <skos:prefLabel xml:lang="it">Unità geografica</skos:prefLabel>
      <skos:definition xml:lang="it">Qualsiasi entità che possa essere definita nello spazio, come un'area geografica, con confini naturali (fisici) o amministrativi. Ad esempio, i dati sulle vendite di case, sui mutamenti del paesaggio, sulle nuove costruzioni o sui cambiamenti nella composizione demografica di alcune regioni o distretti territoriali.</skos:definition>
      <skos:prefLabel xml:lang="lt">Geografinis vienetas</skos:prefLabel>
      <skos:definition xml:lang="lt">Bet kuris objektas, kuris gali būti apibrėžtas geografine teritorija, turinčia natūralias (fizines) arba administracines ribas. Pavyzdžiui, duomenys apie namų pardavimus, kraštovaizdžio pokyčius, naujus statinius ar demografinės sudėties pokyčius tam tikruose regionuose ar rajonuose.</skos:definition>
      <skos:prefLabel xml:lang="lt">Geografinis vienetas</skos:prefLabel>
      <skos:definition xml:lang="lt">Bet kuris objektas, kuris gali būti apibrėžtas geografine teritorija, turinčia natūralias (fizines) arba administracines ribas. Pavyzdžiui, duomenys apie namų pardavimus, kraštovaizdžio pokyčius, naujus statinius ar demografinės sudėties pokyčius tam tikruose regionuose ar rajonuose.</skos:definition>
      <skos:prefLabel xml:lang="nl">Geografische eenheid</skos:prefLabel>
      <skos:definition xml:lang="nl"/>
      <skos:prefLabel xml:lang="nl">Geografische eenheid</skos:prefLabel>
      <skos:definition xml:lang="nl"/>
      <skos:prefLabel xml:lang="no">Geografisk enhet</skos:prefLabel>
      <skos:definition xml:lang="no">Enhver enhet som romlig kan defineres som et geografisk område, med enten naturlige (fysiske) eller administrative grenser. For eksempel: data om boligsalg, landskapsforandringer, nye konstruksjoner eller endringer i den demografiske sammensetningen i bestemte regioner eller distrikter.</skos:definition>
      <skos:prefLabel xml:lang="no">Geografisk enhet</skos:prefLabel>
      <skos:definition xml:lang="no">Enhver enhet som romlig kan defineres som et geografisk område, med enten naturlige (fysiske) eller administrative grenser. For eksempel: data om boligsalg, landskapsforandringer, nye konstruksjoner eller endringer i den demografiske sammensetningen i bestemte regioner eller distrikter.</skos:definition>
      <skos:prefLabel xml:lang="pt">Unidade geográfica</skos:prefLabel>
      <skos:definition xml:lang="pt">Qualquer entidade que possa ser definida espacialmente como uma área geográfica, com limites naturais (físicos) ou administrativos. Por exemplo, dados sobre venda de casas, mudanças paisagísticas, novas construções, ou mudanças na composição demográfica de certas regiões ou distritos.</skos:definition>
      <skos:prefLabel xml:lang="pt">Unidade geográfica</skos:prefLabel>
      <skos:definition xml:lang="pt">Qualquer entidade que possa ser definida espacialmente como uma área geográfica, com limites naturais (físicos) ou administrativos. Por exemplo, dados sobre venda de casas, mudanças paisagísticas, novas construções, ou mudanças na composição demográfica de certas regiões ou distritos.</skos:definition>
      <skos:prefLabel xml:lang="sl">Geografska enota</skos:prefLabel>
      <skos:definition xml:lang="sl">Vsaka enota, ki je prostorsko opredeljena kot geografsko območje z naravnimi (fizičnimi) ali administrativnimi mejami. Na primer podatki o prodaji nepremičnin, spremembah krajine, novogradnjah ali demografski sestavi nekaterih regij ali okrožij.</skos:definition>
      <skos:prefLabel xml:lang="sl">Geografska enota</skos:prefLabel>
      <skos:definition xml:lang="sl">Vsaka enota, ki je prostorsko opredeljena kot geografsko območje z naravnimi (fizičnimi) ali administrativnimi mejami. Na primer podatki o prodaji nepremičnin, spremembah krajine, novogradnjah ali demografski sestavi nekaterih regij ali okrožij.</skos:definition>
      <skos:prefLabel xml:lang="sv">Geografisk enhet</skos:prefLabel>
      <skos:definition xml:lang="sv">En enhet som kan definieras spatialt som ett geografiskt område med antingen naturliga (fysiska) eller administrativa gränser. Till exempel data om husförsäljning, landskapsförändringar, nybyggen eller förändringar av den demografiska sammansättningen i vissa regioner eller distrikt.</skos:definition>
      <skos:prefLabel xml:lang="sv">Geografisk enhet</skos:prefLabel>
      <skos:definition xml:lang="sv">En enhet som kan definieras spatialt som ett geografiskt område med antingen naturliga (fysiska) eller administrativa gränser. Till exempel data om husförsäljning, landskapsförändringar, nybyggen eller förändringar av den demografiska sammansättningen i vissa regioner eller distrikt.</skos:definition>
      <skos:prefLabel xml:lang="sv">Geografisk enhet</skos:prefLabel>
      <skos:definition xml:lang="sv">En enhet som kan definieras spatialt som ett geografiskt område med antingen naturliga (fysiska) eller administrativa gränser. Till exempel data om husförsäljning, landskapsförändringar, nybyggen eller förändringar av den demografiska sammansättningen i vissa regioner eller distrikt.</skos:definition>
   </rdf:Description>
   <rdf:Description rdf:about="http://rdf-vocabulary.ddialliance.org/cv/AnalysisUnit/2.1.3/d151e751">
      <rdf:type rdf:resource="http://www.w3.org/2004/02/skos/core#Concept"/>
      <skos:inScheme rdf:resource="http://rdf-vocabulary.ddialliance.org/cv/AnalysisUnit/2.1.3/"/>
      <skos:notation>PoliticalAdministrativeArea</skos:notation>
      <skos:prefLabel xml:lang="en">Political-administrative area</skos:prefLabel>
      <skos:definition xml:lang="en">A geographical area governed by a sovereign authority that has the power to take administrative or policy decisions for that area. This includes areas at the supranational (e.g., unions of states like the European Union),  national (e.g., individual states or countries), sub-national (e.g., administrative subdivisions like federal states, provinces, etc.), and local (e.g., municipalities) levels.</skos:definition>
      <skos:prefLabel xml:lang="en">Political-administrative area</skos:prefLabel>
      <skos:definition xml:lang="en">A geographical area governed by a sovereign authority that has the power to take administrative or policy decisions for that area. This includes areas at the supranational (e.g., unions of states like the European Union),  national (e.g., individual states or countries), sub-national (e.g., administrative subdivisions like federal states, provinces, etc.), and local (e.g., municipalities) levels.</skos:definition>
      <skos:prefLabel xml:lang="de">Politisch-administratives Gebiet</skos:prefLabel>
      <skos:definition xml:lang="de">Ein geographisches Gebiet, das von einer souveränen Staatsgewalt regiert wird, die die Befugnis hat, administrative oder politische Entscheidungen für dieses Gebiet zu treffen. Dazu gehören Gebiete auf supranationaler (z. B. Staatenbünde wie die Europäische Union), nationaler (z. B. einzelne Staaten oder Länder), subnationaler (z. B. Verwaltungsgliederungen wie Bundesländer, Provinzen usw.) und lokaler (z. B. Gemeinden) Ebene.</skos:definition>
      <skos:prefLabel xml:lang="de">Politisch-administratives Gebiet</skos:prefLabel>
      <skos:definition xml:lang="de">Ein geographisches Gebiet, das von einer souveränen Staatsgewalt regiert wird, die die Befugnis hat, administrative oder politische Entscheidungen für dieses Gebiet zu treffen. Dazu gehören Gebiete auf supranationaler (z. B. Staatenbünde wie die Europäische Union), nationaler (z. B. einzelne Staaten oder Länder), subnationaler (z. B. Verwaltungsgliederungen wie Bundesländer, Provinzen usw.) und lokaler (z. B. Gemeinden) Ebene.</skos:definition>
      <skos:prefLabel xml:lang="fi">Poliittis-hallinnollinen alue</skos:prefLabel>
      <skos:definition xml:lang="fi">Maantieteellinen alue, jota hallinnoivilla viranomaisilla tai päätäntäelimillä on oikeus tehdä aluetta koskevia hallinnollisia tai poliittisia päätöksiä. Sisältää ylikansalliset (esim. Euroopan unioni), kansalliset (esim. valtiot), maansisäiset (esim. maakunnat) ja paikalliset (esim. kunnat) alueet.</skos:definition>
      <skos:prefLabel xml:lang="fi">Poliittis-hallinnollinen alue</skos:prefLabel>
      <skos:definition xml:lang="fi">Maantieteellinen alue, jota hallinnoivilla viranomaisilla tai päätäntäelimillä on oikeus tehdä aluetta koskevia hallinnollisia tai poliittisia päätöksiä. Sisältää ylikansalliset (esim. Euroopan unioni), kansalliset (esim. valtiot), maansisäiset (esim. maakunnat) ja paikalliset (esim. kunnat) alueet.</skos:definition>
      <skos:prefLabel xml:lang="it">Area politico-amministrativa</skos:prefLabel>
      <skos:definition xml:lang="it">Un'area geografica governata da un'autorità che ha il potere di prendere decisioni amministrative o politiche relative a quell'area. Comprende aree a livello sovranazionale (ad esempio unioni di stati come l'Unione Europea), nazionale (ad esempio singoli stati o paesi), subnazionale (ad esempio suddivisioni amministrative come stati federali, province, ecc.), e locale (ad esempio comuni).</skos:definition>
      <skos:prefLabel xml:lang="it">Area politico-amministrativa</skos:prefLabel>
      <skos:definition xml:lang="it">Un'area geografica governata da un'autorità che ha il potere di prendere decisioni amministrative o politiche relative a quell'area. Comprende aree a livello sovranazionale (ad esempio unioni di stati come l'Unione Europea), nazionale (ad esempio singoli stati o paesi), subnazionale (ad esempio suddivisioni amministrative come stati federali, province, ecc.), e locale (ad esempio comuni).</skos:definition>
      <skos:prefLabel xml:lang="lt">Politinė administracinė teritorija</skos:prefLabel>
      <skos:definition xml:lang="lt">Geografinė teritorija valdoma suverenios valdžios, kuri turi galią joje priimti administracinius ar politinius sprendimus. Tai apima viršnacionalinį (pavyzdžiui, valstybių sąjungos, kaip Europos Sąjunga), nacionalinį (pavyzdžiui, atskiros valstybės ar šalys), regioninį (pavyzdžiui, administraciniai vienetai, kaip federalinės žemės, provincijos, apskritys ir kt.) ir vietos (pavyzdžiui, savivaldybių) lygmenis.</skos:definition>
      <skos:prefLabel xml:lang="lt">Politinė administracinė teritorija</skos:prefLabel>
      <skos:definition xml:lang="lt">Geografinė teritorija valdoma suverenios valdžios, kuri turi galią joje priimti administracinius ar politinius sprendimus. Tai apima viršnacionalinį (pavyzdžiui, valstybių sąjungos, kaip Europos Sąjunga), nacionalinį (pavyzdžiui, atskiros valstybės ar šalys), regioninį (pavyzdžiui, administraciniai vienetai, kaip federalinės žemės, provincijos, apskritys ir kt.) ir vietos (pavyzdžiui, savivaldybių) lygmenis.</skos:definition>
      <skos:prefLabel xml:lang="nl">Poltiek administratief gebied</skos:prefLabel>
      <skos:definition xml:lang="nl"/>
      <skos:prefLabel xml:lang="nl">Poltiek administratief gebied</skos:prefLabel>
      <skos:definition xml:lang="nl"/>
      <skos:prefLabel xml:lang="no">Politisk administrativt område</skos:prefLabel>
      <skos:definition xml:lang="no">Et geografisk område styrt av en suveren myndighet som har makten til beslutte administrative eller politiske avgjørelser for det området. Dette inkluderer områder på overstatlig (f.eks sammenslutninger av stater som Den Europeiske Union), nasjonalt (f.eks individuelle stater eller land), subnasjonalt (f.eks administrative oppdelinger som føderale stater, provinser etc.) og lokalt (f.eks kommuner) nivå.</skos:definition>
      <skos:prefLabel xml:lang="no">Politisk administrativt område</skos:prefLabel>
      <skos:definition xml:lang="no">Et geografisk område styrt av en suveren myndighet som har makten til beslutte administrative eller politiske avgjørelser for det området. Dette inkluderer områder på overstatlig (f.eks sammenslutninger av stater som Den Europeiske Union), nasjonalt (f.eks individuelle stater eller land), subnasjonalt (f.eks administrative oppdelinger som føderale stater, provinser etc.) og lokalt (f.eks kommuner) nivå.</skos:definition>
      <skos:prefLabel xml:lang="pt">Área político-administrativa</skos:prefLabel>
      <skos:definition xml:lang="pt">Uma área geográfica governada por autoridade soberana que tem o poder de tomar decisões políticas ou administrativas para aquela área. Isto inclui áreas ao nível supranacional (por exemplo, uniões de vários estados como a União Europeia), nacional (por exemplo, estados individuais ou países), subnacional (por exemplo, subdivisões administrativas como estados federais, províncias, etc.), e local (por exemplo, municípios).</skos:definition>
      <skos:prefLabel xml:lang="pt">Área político-administrativa</skos:prefLabel>
      <skos:definition xml:lang="pt">Uma área geográfica governada por autoridade soberana que tem o poder de tomar decisões políticas ou administrativas para aquela área. Isto inclui áreas ao nível supranacional (por exemplo, uniões de vários estados como a União Europeia), nacional (por exemplo, estados individuais ou países), subnacional (por exemplo, subdivisões administrativas como estados federais, províncias, etc.), e local (por exemplo, municípios).</skos:definition>
      <skos:prefLabel xml:lang="sl">Politično-upravno območje</skos:prefLabel>
      <skos:definition xml:lang="sl">Geografsko območje, ki ga vodi suverena oblast, ki ima lastno pristojnost za sprejemanje upravnih ali političnih odločitev za to območje. To vključuje nadnacionalna območja (npr. zveze držav, kot je Evropska unija), nacionalna (npr. posamezne državne uprave ali države), podnacionalna (npr. upravna podobmočja, kot so zvezne države, province itd.) In lokalna (npr. občine).</skos:definition>
      <skos:prefLabel xml:lang="sl">Politično-upravno območje</skos:prefLabel>
      <skos:definition xml:lang="sl">Geografsko območje, ki ga vodi suverena oblast, ki ima lastno pristojnost za sprejemanje upravnih ali političnih odločitev za to območje. To vključuje nadnacionalna območja (npr. zveze držav, kot je Evropska unija), nacionalna (npr. posamezne državne uprave ali države), podnacionalna (npr. upravna podobmočja, kot so zvezne države, province itd.) In lokalna (npr. občine).</skos:definition>
      <skos:prefLabel xml:lang="sv">Politiskt förvaltningsområde</skos:prefLabel>
      <skos:definition xml:lang="sv">Ett geografiskt område som styrs av en bestämmande myndighet med makt att fatta administrativa eller politiska beslut för området. Detta inkluderar områden på överstatlig (t.ex. unioner av stater som EU), statlig (t.ex. delstater eller länder), subnationell/regional (t.ex. förvaltningsområden som federala delstater, provinser osv.) och lokal (t.ex. kommuner) nivå.</skos:definition>
      <skos:prefLabel xml:lang="sv">Politiskt förvaltningsområde</skos:prefLabel>
      <skos:definition xml:lang="sv">Ett geografiskt område som styrs av en bestämmande myndighet med makt att fatta administrativa eller politiska beslut för området. Detta inkluderar områden på överstatlig (t.ex. unioner av stater som EU), statlig (t.ex. delstater eller länder), subnationell/regional (t.ex. förvaltningsområden som federala delstater, provinser osv.) och lokal (t.ex. kommuner) nivå.</skos:definition>
      <skos:prefLabel xml:lang="sv">Politiskt förvaltningsområde</skos:prefLabel>
      <skos:definition xml:lang="sv">Ett geografiskt område som styrs av en bestämmande myndighet med makt att fatta administrativa eller politiska beslut för området. Detta inkluderar områden på överstatlig (t.ex. unioner av stater som EU), statlig (t.ex. delstater eller länder), subnationell/regional (t.ex. förvaltningsområden som federala delstater, provinser osv.) och lokal (t.ex. kommuner) nivå.</skos:definition>
   </rdf:Description>
   <rdf:Description rdf:about="http://rdf-vocabulary.ddialliance.org/cv/AnalysisUnit/2.1.3/d151e830">
      <rdf:type rdf:resource="http://www.w3.org/2004/02/skos/core#Concept"/>
      <skos:inScheme rdf:resource="http://rdf-vocabulary.ddialliance.org/cv/AnalysisUnit/2.1.3/"/>
      <skos:notation>TimeUnit</skos:notation>
      <skos:prefLabel xml:lang="en">Time unit</skos:prefLabel>
      <skos:definition xml:lang="en">Any period of time: year, week, month, day, or bimonthly or quarterly periods, etc.</skos:definition>
      <skos:prefLabel xml:lang="en">Time unit</skos:prefLabel>
      <skos:definition xml:lang="en">Any period of time: year, week, month, day, or bimonthly or quarterly periods, etc.</skos:definition>
      <skos:prefLabel xml:lang="de">Zeiteinheit</skos:prefLabel>
      <skos:definition xml:lang="de">Beliebiger Zeitraum: Jahr, Woche, Monat, Tag, oder zweimonatliche oder vierteljährliche Zeiträume, usw.</skos:definition>
      <skos:prefLabel xml:lang="de">Zeiteinheit</skos:prefLabel>
      <skos:definition xml:lang="de">Beliebiger Zeitraum: Jahr, Woche, Monat, Tag, oder zweimonatliche oder vierteljährliche Zeiträume, usw.</skos:definition>
      <skos:prefLabel xml:lang="fi">Aikajakso</skos:prefLabel>
      <skos:definition xml:lang="fi">Minkä mittainen aikajakso tahansa: sekunti, tunti, vuorokausi, viikko, kuukausi, vuosi yms.</skos:definition>
      <skos:prefLabel xml:lang="fi">Aikajakso</skos:prefLabel>
      <skos:definition xml:lang="fi">Minkä mittainen aikajakso tahansa: sekunti, tunti, vuorokausi, viikko, kuukausi, vuosi yms.</skos:definition>
      <skos:prefLabel xml:lang="it">Unità temporale</skos:prefLabel>
      <skos:definition xml:lang="it">Qualsiasi periodo di tempo: anno, settimana, mese, giorno, bimestre, trimestre, ecc.</skos:definition>
      <skos:prefLabel xml:lang="it">Unità temporale</skos:prefLabel>
      <skos:definition xml:lang="it">Qualsiasi periodo di tempo: anno, settimana, mese, giorno, bimestre, trimestre, ecc.</skos:definition>
      <skos:prefLabel xml:lang="lt">Laiko vienetas</skos:prefLabel>
      <skos:definition xml:lang="lt">Bet koks laikotarpis: metai, savaitė, mėnuo, diena, du mėnesiai, ketvirtis ir kt.</skos:definition>
      <skos:prefLabel xml:lang="lt">Laiko vienetas</skos:prefLabel>
      <skos:definition xml:lang="lt">Bet koks laikotarpis: metai, savaitė, mėnuo, diena, du mėnesiai, ketvirtis ir kt.</skos:definition>
      <skos:prefLabel xml:lang="nl">Tijdseenheid</skos:prefLabel>
      <skos:definition xml:lang="nl"/>
      <skos:prefLabel xml:lang="nl">Tijdseenheid</skos:prefLabel>
      <skos:definition xml:lang="nl"/>
      <skos:prefLabel xml:lang="no">Tidsenhet</skos:prefLabel>
      <skos:definition xml:lang="no">Tidsperiode: år, uke, måned, dag, annenhver måned eller kvartal etc.</skos:definition>
      <skos:prefLabel xml:lang="no">Tidsenhet</skos:prefLabel>
      <skos:definition xml:lang="no">Tidsperiode: år, uke, måned, dag, annenhver måned eller kvartal etc.</skos:definition>
      <skos:prefLabel xml:lang="pt">Unidade de tempo</skos:prefLabel>
      <skos:definition xml:lang="pt">Qualquer período de tempo: ano, semana, mês, dia, ou períodos bimestrais ou trimestrais, etc.</skos:definition>
      <skos:prefLabel xml:lang="pt">Unidade de tempo</skos:prefLabel>
      <skos:definition xml:lang="pt">Qualquer período de tempo: ano, semana, mês, dia, ou períodos bimestrais ou trimestrais, etc.</skos:definition>
      <skos:prefLabel xml:lang="sl">Časovna enota</skos:prefLabel>
      <skos:definition xml:lang="sl">Katerokoli časovno obdobje: leto, teden, mesec, dan, dvomesečno ali četrtletno obdobje itd.</skos:definition>
      <skos:prefLabel xml:lang="sl">Časovna enota</skos:prefLabel>
      <skos:definition xml:lang="sl">Katerokoli časovno obdobje: leto, teden, mesec, dan, dvomesečno ali četrtletno obdobje itd.</skos:definition>
      <skos:prefLabel xml:lang="sv">Tidsenhet</skos:prefLabel>
      <skos:definition xml:lang="sv">En tidsperiod: år, månad, vecka, dag, kvartal, tvåmånadersperiod osv.</skos:definition>
      <skos:prefLabel xml:lang="sv">Tidsenhet</skos:prefLabel>
      <skos:definition xml:lang="sv">En tidsperiod: år, månad, vecka, dag, kvartal, tvåmånadersperiod osv.</skos:definition>
      <skos:prefLabel xml:lang="sv">Tidsenhet</skos:prefLabel>
      <skos:definition xml:lang="sv">En tidsperiod: år, månad, vecka, dag, kvartal, tvåmånadersperiod osv.</skos:definition>
   </rdf:Description>
   <rdf:Description rdf:about="http://rdf-vocabulary.ddialliance.org/cv/AnalysisUnit/2.1.3/d151e910">
      <rdf:type rdf:resource="http://www.w3.org/2004/02/skos/core#Concept"/>
      <skos:inScheme rdf:resource="http://rdf-vocabulary.ddialliance.org/cv/AnalysisUnit/2.1.3/"/>
      <skos:notation>MediaUnit</skos:notation>
      <skos:prefLabel xml:lang="en">Media unit</skos:prefLabel>
      <skos:definition xml:lang="en">Includes text, still image, video and sound.</skos:definition>
      <skos:prefLabel xml:lang="en">Media unit</skos:prefLabel>
      <skos:definition xml:lang="en">Includes text, still image, video and sound.</skos:definition>
      <skos:prefLabel xml:lang="de">Medieneinheit</skos:prefLabel>
      <skos:definition xml:lang="de">Beinhaltet Text, Standbild, Video und Ton.</skos:definition>
      <skos:prefLabel xml:lang="de">Medieneinheit</skos:prefLabel>
      <skos:definition xml:lang="de">Beinhaltet Text, Standbild, Video und Ton.</skos:definition>
      <skos:prefLabel xml:lang="fi">Mediatyyppi (teksti, ääni, still-kuva, liikkuva kuva)</skos:prefLabel>
      <skos:definition xml:lang="fi">Sisältää teksti-, kuva- ja äänimuodossa olevan viestinnän.</skos:definition>
      <skos:prefLabel xml:lang="fi">Mediatyyppi (teksti, ääni, still-kuva, liikkuva kuva)</skos:prefLabel>
      <skos:definition xml:lang="fi">Sisältää teksti-, kuva- ja äänimuodossa olevan viestinnän.</skos:definition>
      <skos:prefLabel xml:lang="it">Unità di supporto</skos:prefLabel>
      <skos:definition xml:lang="it">Include testi, immagini, video e suoni.</skos:definition>
      <skos:prefLabel xml:lang="it">Unità di supporto</skos:prefLabel>
      <skos:definition xml:lang="it">Include testi, immagini, video e suoni.</skos:definition>
      <skos:prefLabel xml:lang="lt">Medijos vienetas</skos:prefLabel>
      <skos:definition xml:lang="lt">Apima tekstus, statinius vaizdus, vaizdo ir garso įrašus.</skos:definition>
      <skos:prefLabel xml:lang="lt">Medijos vienetas</skos:prefLabel>
      <skos:definition xml:lang="lt">Apima tekstus, statinius vaizdus, vaizdo ir garso įrašus.</skos:definition>
      <skos:prefLabel xml:lang="nl">Media-eenheid</skos:prefLabel>
      <skos:definition xml:lang="nl"/>
      <skos:prefLabel xml:lang="nl">Media-eenheid</skos:prefLabel>
      <skos:definition xml:lang="nl"/>
      <skos:prefLabel xml:lang="no">Medieenhet</skos:prefLabel>
      <skos:definition xml:lang="no">Inkluderer tekst, stillbilder, video og lyd.</skos:definition>
      <skos:prefLabel xml:lang="no">Medieenhet</skos:prefLabel>
      <skos:definition xml:lang="no">Inkluderer tekst, stillbilder, video og lyd.</skos:definition>
      <skos:prefLabel xml:lang="pt">Unidade de Media</skos:prefLabel>
      <skos:definition xml:lang="pt">Inclui texto, imagem, vídeo e som.</skos:definition>
      <skos:prefLabel xml:lang="pt">Unidade de Media</skos:prefLabel>
      <skos:definition xml:lang="pt">Inclui texto, imagem, vídeo e som.</skos:definition>
      <skos:prefLabel xml:lang="sl">Medijska enota</skos:prefLabel>
      <skos:definition xml:lang="sl">Enota, ki vsebuje določeno multimedijsko vsebino: besedilo, mirujočo sliko, posnetek in zvok.</skos:definition>
      <skos:prefLabel xml:lang="sl">Medijska enota</skos:prefLabel>
      <skos:definition xml:lang="sl">Enota, ki vsebuje določeno multimedijsko vsebino: besedilo, mirujočo sliko, posnetek in zvok.</skos:definition>
      <skos:prefLabel xml:lang="sv">Mediaenhet</skos:prefLabel>
      <skos:definition xml:lang="sv">Inkluderar text, stillbilder, video och ljud.</skos:definition>
      <skos:prefLabel xml:lang="sv">Mediaenhet</skos:prefLabel>
      <skos:definition xml:lang="sv">Inkluderar text, stillbilder, video och ljud.</skos:definition>
      <skos:prefLabel xml:lang="sv">Mediaenhet</skos:prefLabel>
      <skos:definition xml:lang="sv">Inkluderar text, stillbilder, video och ljud.</skos:definition>
      <skos:narrower rdf:resource="http://rdf-vocabulary.ddialliance.org/cv/AnalysisUnit/2.1.3/d151e997"/>
      <skos:narrower rdf:resource="http://rdf-vocabulary.ddialliance.org/cv/AnalysisUnit/2.1.3/d151e1076"/>
      <skos:narrower rdf:resource="http://rdf-vocabulary.ddialliance.org/cv/AnalysisUnit/2.1.3/d151e1155"/>
      <skos:narrower rdf:resource="http://rdf-vocabulary.ddialliance.org/cv/AnalysisUnit/2.1.3/d151e1234"/>
   </rdf:Description>
   <rdf:Description rdf:about="http://rdf-vocabulary.ddialliance.org/cv/AnalysisUnit/2.1.3/d151e997">
      <rdf:type rdf:resource="http://www.w3.org/2004/02/skos/core#Concept"/>
      <skos:inScheme rdf:resource="http://rdf-vocabulary.ddialliance.org/cv/AnalysisUnit/2.1.3/"/>
      <skos:notation>MediaUnit.Sound</skos:notation>
      <skos:prefLabel xml:lang="en">Media unit: Sound</skos:prefLabel>
      <skos:definition xml:lang="en">Recorded sound, including voice, music, etc.</skos:definition>
      <skos:prefLabel xml:lang="en">Media unit: Sound</skos:prefLabel>
      <skos:definition xml:lang="en">Recorded sound, including voice, music, etc.</skos:definition>
      <skos:prefLabel xml:lang="de">Medieneinheit: Ton</skos:prefLabel>
      <skos:definition xml:lang="de">Aufgenommener Ton, einschließlich Sprache, Musik usw.</skos:definition>
      <skos:prefLabel xml:lang="de">Medieneinheit: Ton</skos:prefLabel>
      <skos:definition xml:lang="de">Aufgenommener Ton, einschließlich Sprache, Musik usw.</skos:definition>
      <skos:prefLabel xml:lang="fi">Mediatyyppi: ääni</skos:prefLabel>
      <skos:definition xml:lang="fi">Taltioitu ääni, esimerkiksi puhe, musiikki jne.</skos:definition>
      <skos:prefLabel xml:lang="fi">Mediatyyppi: ääni</skos:prefLabel>
      <skos:definition xml:lang="fi">Taltioitu ääni, esimerkiksi puhe, musiikki jne.</skos:definition>
      <skos:prefLabel xml:lang="it">Unità di supporto: suono</skos:prefLabel>
      <skos:definition xml:lang="it">Suoni registrati, inclusa la voce, la musica, ecc.</skos:definition>
      <skos:prefLabel xml:lang="it">Unità di supporto: suono</skos:prefLabel>
      <skos:definition xml:lang="it">Suoni registrati, inclusa la voce, la musica, ecc.</skos:definition>
      <skos:prefLabel xml:lang="lt">Medijos vienetas: garso įrašas</skos:prefLabel>
      <skos:definition xml:lang="lt">Įrašytas garsas, įskaitant balsą, muziką ir kt.</skos:definition>
      <skos:prefLabel xml:lang="lt">Medijos vienetas: garso įrašas</skos:prefLabel>
      <skos:definition xml:lang="lt">Įrašytas garsas, įskaitant balsą, muziką ir kt.</skos:definition>
      <skos:prefLabel xml:lang="nl">Media-eenheid: Geluid</skos:prefLabel>
      <skos:definition xml:lang="nl"/>
      <skos:prefLabel xml:lang="nl">Media-eenheid: Geluid</skos:prefLabel>
      <skos:definition xml:lang="nl"/>
      <skos:prefLabel xml:lang="no">Medieenhet: Lyd</skos:prefLabel>
      <skos:definition xml:lang="no">Lydopptak, inkludert stemme, musikk, etc.</skos:definition>
      <skos:prefLabel xml:lang="no">Medieenhet: Lyd</skos:prefLabel>
      <skos:definition xml:lang="no">Lydopptak, inkludert stemme, musikk, etc.</skos:definition>
      <skos:prefLabel xml:lang="pt">Unidade de Media: Som</skos:prefLabel>
      <skos:definition xml:lang="pt">Som gravado, incluindo voz, música, etc.</skos:definition>
      <skos:prefLabel xml:lang="pt">Unidade de Media: Som</skos:prefLabel>
      <skos:definition xml:lang="pt">Som gravado, incluindo voz, música, etc.</skos:definition>
      <skos:prefLabel xml:lang="sl">Medijska enota: zvok</skos:prefLabel>
      <skos:definition xml:lang="sl">Posneti zvok, vključno z glasom, glasbo itd.</skos:definition>
      <skos:prefLabel xml:lang="sl">Medijska enota: zvok</skos:prefLabel>
      <skos:definition xml:lang="sl">Posneti zvok, vključno z glasom, glasbo itd.</skos:definition>
      <skos:prefLabel xml:lang="sv">Mediaenhet: Ljud</skos:prefLabel>
      <skos:definition xml:lang="sv">Inspelat ljud, som röst, musik m.m.</skos:definition>
      <skos:prefLabel xml:lang="sv">Mediaenhet: Ljud</skos:prefLabel>
      <skos:definition xml:lang="sv">Inspelat ljud, som röst, musik m.m.</skos:definition>
      <skos:prefLabel xml:lang="sv">Mediaenhet: Ljud</skos:prefLabel>
      <skos:definition xml:lang="sv">Inspelat ljud, som röst, musik m.m.</skos:definition>
      <skos:broader rdf:resource="http://rdf-vocabulary.ddialliance.org/cv/AnalysisUnit/2.1.3/d151e910"/>
   </rdf:Description>
   <rdf:Description rdf:about="http://rdf-vocabulary.ddialliance.org/cv/AnalysisUnit/2.1.3/d151e1076">
      <rdf:type rdf:resource="http://www.w3.org/2004/02/skos/core#Concept"/>
      <skos:inScheme rdf:resource="http://rdf-vocabulary.ddialliance.org/cv/AnalysisUnit/2.1.3/"/>
      <skos:notation>MediaUnit.StillImage</skos:notation>
      <skos:prefLabel xml:lang="en">Media unit: Still image</skos:prefLabel>
      <skos:definition xml:lang="en">Static images, such as graphs, drawings, photographs, diagnostic/medical images like X-rays and other types of imaging tests, etc.</skos:definition>
      <skos:prefLabel xml:lang="en">Media unit: Still image</skos:prefLabel>
      <skos:definition xml:lang="en">Static images, such as graphs, drawings, photographs, diagnostic/medical images like X-rays and other types of imaging tests, etc.</skos:definition>
      <skos:prefLabel xml:lang="de">Medieneinheit: Unbewegtes Bild</skos:prefLabel>
      <skos:definition xml:lang="de">Statische Bilder, wie z. B. Diagramme, Zeichnungen, Fotos, diagnostische/medizinische Bilder wie Röntgenbilder und andere Arten von bildgebenden Tests usw.</skos:definition>
      <skos:prefLabel xml:lang="de">Medieneinheit: Unbewegtes Bild</skos:prefLabel>
      <skos:definition xml:lang="de">Statische Bilder, wie z. B. Diagramme, Zeichnungen, Fotos, diagnostische/medizinische Bilder wie Röntgenbilder und andere Arten von bildgebenden Tests usw.</skos:definition>
      <skos:prefLabel xml:lang="fi">Mediatyyppi: still-kuva</skos:prefLabel>
      <skos:definition xml:lang="fi">Still-kuvat kuten esimerkiksi graafit, piirrokset, valokuvat, röntgenkuvat tai muut lääketieteelliset still-kuvat.</skos:definition>
      <skos:prefLabel xml:lang="fi">Mediatyyppi: still-kuva</skos:prefLabel>
      <skos:definition xml:lang="fi">Still-kuvat kuten esimerkiksi graafit, piirrokset, valokuvat, röntgenkuvat tai muut lääketieteelliset still-kuvat.</skos:definition>
      <skos:prefLabel xml:lang="it">Unità di supporto: immagine</skos:prefLabel>
      <skos:definition xml:lang="it">Immagini statiche, come grafici, disegni, fotografie, immagini diagnostiche/mediche come radiografie e altri tipi di esami per immagini, ecc.</skos:definition>
      <skos:prefLabel xml:lang="it">Unità di supporto: immagine</skos:prefLabel>
      <skos:definition xml:lang="it">Immagini statiche, come grafici, disegni, fotografie, immagini diagnostiche/mediche come radiografie e altri tipi di esami per immagini, ecc.</skos:definition>
      <skos:prefLabel xml:lang="lt">Medijos vienetas: statinis vaizdas</skos:prefLabel>
      <skos:definition xml:lang="lt">Statiniai vaizdai, tokie kaip grafikai, brėžiniai, nuotraukos, diagnostiniai ar medicininiai vaizdai (rentgeno nuotraukos ir kitokio tipo vaizdo tyrimai) ir kt.</skos:definition>
      <skos:prefLabel xml:lang="lt">Medijos vienetas: statinis vaizdas</skos:prefLabel>
      <skos:definition xml:lang="lt">Statiniai vaizdai, tokie kaip grafikai, brėžiniai, nuotraukos, diagnostiniai ar medicininiai vaizdai (rentgeno nuotraukos ir kitokio tipo vaizdo tyrimai) ir kt.</skos:definition>
      <skos:prefLabel xml:lang="nl">Media-eenheid: Beeld</skos:prefLabel>
      <skos:definition xml:lang="nl"/>
      <skos:prefLabel xml:lang="nl">Media-eenheid: Beeld</skos:prefLabel>
      <skos:definition xml:lang="nl"/>
      <skos:prefLabel xml:lang="no">Medieenhet: Stillbilde</skos:prefLabel>
      <skos:definition xml:lang="no">Statiske bilder som grafer, tegninger, fotografier, diagnostiske/medisinske bilder som røntgen og andre bildetester, etc.</skos:definition>
      <skos:prefLabel xml:lang="no">Medieenhet: Stillbilde</skos:prefLabel>
      <skos:definition xml:lang="no">Statiske bilder som grafer, tegninger, fotografier, diagnostiske/medisinske bilder som røntgen og andre bildetester, etc.</skos:definition>
      <skos:prefLabel xml:lang="pt">Unidade de Media: Imagem</skos:prefLabel>
      <skos:definition xml:lang="pt">Imagens estáticas, como gráficos, desenhos, fotografias, imagens médicas/de diagnóstico como raio-x e outros tipos de testes de imagem, etc.</skos:definition>
      <skos:prefLabel xml:lang="pt">Unidade de Media: Imagem</skos:prefLabel>
      <skos:definition xml:lang="pt">Imagens estáticas, como gráficos, desenhos, fotografias, imagens médicas/de diagnóstico como raio-x e outros tipos de testes de imagem, etc.</skos:definition>
      <skos:prefLabel xml:lang="sl">Medijska enota: mirujoča slika</skos:prefLabel>
      <skos:definition xml:lang="sl">Statične slike, kot so grafi, risbe, fotografije, diagnostične/medicinske slike, kot so rentgenske slike in druge vrste slikovnih testov itd.</skos:definition>
      <skos:prefLabel xml:lang="sl">Medijska enota: mirujoča slika</skos:prefLabel>
      <skos:definition xml:lang="sl">Statične slike, kot so grafi, risbe, fotografije, diagnostične/medicinske slike, kot so rentgenske slike in druge vrste slikovnih testov itd.</skos:definition>
      <skos:prefLabel xml:lang="sv">Mediaenhet: Stillbild</skos:prefLabel>
      <skos:definition xml:lang="sv">Statiska bilder, som diagram, ritningar, fotografier, diagnostiska/medicinska bilder som röntgenbilder eller andra typer av bilddiagnostiska undersökningar&amp;nbsp;osv.</skos:definition>
      <skos:prefLabel xml:lang="sv">Mediaenhet: Stillbild</skos:prefLabel>
      <skos:definition xml:lang="sv">Statiska bilder, som diagram, ritningar, fotografier, diagnostiska/medicinska bilder som röntgenbilder eller andra typer av bilddiagnostiska undersökningar&amp;nbsp;osv.</skos:definition>
      <skos:prefLabel xml:lang="sv">Mediaenhet: Stillbild</skos:prefLabel>
      <skos:definition xml:lang="sv">Statiska bilder, som diagram, ritningar, fotografier, diagnostiska/medicinska bilder som röntgenbilder eller andra typer av bilddiagnostiska undersökningar&amp;nbsp;osv.</skos:definition>
      <skos:broader rdf:resource="http://rdf-vocabulary.ddialliance.org/cv/AnalysisUnit/2.1.3/d151e910"/>
   </rdf:Description>
   <rdf:Description rdf:about="http://rdf-vocabulary.ddialliance.org/cv/AnalysisUnit/2.1.3/d151e1155">
      <rdf:type rdf:resource="http://www.w3.org/2004/02/skos/core#Concept"/>
      <skos:inScheme rdf:resource="http://rdf-vocabulary.ddialliance.org/cv/AnalysisUnit/2.1.3/"/>
      <skos:notation>MediaUnit.Text</skos:notation>
      <skos:prefLabel xml:lang="en">Media unit: Text</skos:prefLabel>
      <skos:definition xml:lang="en">Any written piece/entity, such as books, articles, tweets, blogs, etc. For example, a study on hate speech in tweets, or a study of the way newspapers present certain political/social issues over time, like women's or minorities' rights, etc.</skos:definition>
      <skos:prefLabel xml:lang="en">Media unit: Text</skos:prefLabel>
      <skos:definition xml:lang="en">Any written piece/entity, such as books, articles, tweets, blogs, etc. For example, a study on hate speech in tweets, or a study of the way newspapers present certain political/social issues over time, like women's or minorities' rights, etc.</skos:definition>
      <skos:prefLabel xml:lang="de">Medieneinheit: Text</skos:prefLabel>
      <skos:definition xml:lang="de">Jede schriftliche Arbeit/Einheit, wie Bücher, Artikel, Tweets, Blogbeiträge usw. Zum Beispiel eine Studie über Hassreden in Tweets oder eine Studie über die Art und Weise, wie Zeitungen bestimmte politische/soziale Themen im Laufe der Zeit darstellen, wie z. B. die Rechte von Frauen oder Minderheiten, usw.</skos:definition>
      <skos:prefLabel xml:lang="de">Medieneinheit: Text</skos:prefLabel>
      <skos:definition xml:lang="de">Jede schriftliche Arbeit/Einheit, wie Bücher, Artikel, Tweets, Blogbeiträge usw. Zum Beispiel eine Studie über Hassreden in Tweets oder eine Studie über die Art und Weise, wie Zeitungen bestimmte politische/soziale Themen im Laufe der Zeit darstellen, wie z. B. die Rechte von Frauen oder Minderheiten, usw.</skos:definition>
      <skos:prefLabel xml:lang="fi">Mediatyyppi: teksti</skos:prefLabel>
      <skos:definition xml:lang="fi">Kirja, artikkeli, tweet, blogikirjoitus tai mikä tahansa muu tekstiyksikkö. Esimerkiksi tutkittaessa miten sanomalehdet ovat käsitelleet tiettyä aihetta ajan saatossa tai tutkittaessa vihapuhetta blogikirjoituksissa.</skos:definition>
      <skos:prefLabel xml:lang="fi">Mediatyyppi: teksti</skos:prefLabel>
      <skos:definition xml:lang="fi">Kirja, artikkeli, tweet, blogikirjoitus tai mikä tahansa muu tekstiyksikkö. Esimerkiksi tutkittaessa miten sanomalehdet ovat käsitelleet tiettyä aihetta ajan saatossa tai tutkittaessa vihapuhetta blogikirjoituksissa.</skos:definition>
      <skos:prefLabel xml:lang="it">Unità di supporto: testo</skos:prefLabel>
      <skos:definition xml:lang="it">Qualsiasi entità scritta, come libri, articoli, tweet, blog, ecc. Ad esempio, uno studio sugli hate speech nei tweet, oppure uno studio sul modo in cui i giornali presentano nel tempo alcuni temi politici/sociali, come i diritti delle donne o delle minoranze, ecc.</skos:definition>
      <skos:prefLabel xml:lang="it">Unità di supporto: testo</skos:prefLabel>
      <skos:definition xml:lang="it">Qualsiasi entità scritta, come libri, articoli, tweet, blog, ecc. Ad esempio, uno studio sugli hate speech nei tweet, oppure uno studio sul modo in cui i giornali presentano nel tempo alcuni temi politici/sociali, come i diritti delle donne o delle minoranze, ecc.</skos:definition>
      <skos:prefLabel xml:lang="lt">Medijos vienetas: tekstas</skos:prefLabel>
      <skos:definition xml:lang="lt">Bet koks parašytas kūrinys ar objektas, pavyzdžiui, knygos, straipsniai, socialinių medijų žinutės, tinklaraščiai ir kt. Pavyzdžiui, tyrimas apie neapykantos kalbą socialinių medijų žinutėse arba tyrimas apie tai, kaip laikraščiai pateikia tam tikras politines ar socialines problemas, pavyzdžiui, moterų ar mažumų teises ir kt.</skos:definition>
      <skos:prefLabel xml:lang="lt">Medijos vienetas: tekstas</skos:prefLabel>
      <skos:definition xml:lang="lt">Bet koks parašytas kūrinys ar objektas, pavyzdžiui, knygos, straipsniai, socialinių medijų žinutės, tinklaraščiai ir kt. Pavyzdžiui, tyrimas apie neapykantos kalbą socialinių medijų žinutėse arba tyrimas apie tai, kaip laikraščiai pateikia tam tikras politines ar socialines problemas, pavyzdžiui, moterų ar mažumų teises ir kt.</skos:definition>
      <skos:prefLabel xml:lang="nl">Media-eenheid: Tekst</skos:prefLabel>
      <skos:definition xml:lang="nl"/>
      <skos:prefLabel xml:lang="nl">Media-eenheid: Tekst</skos:prefLabel>
      <skos:definition xml:lang="nl"/>
      <skos:prefLabel xml:lang="no">Medieenhet: Tekst</skos:prefLabel>
      <skos:definition xml:lang="no">Alle skrevne tekster/enheter som bøker, artikler, tweets, blogger, etc. For eksempel: en studie om hatefulle ytringer i tweets, en studie om måten nyhetsaviser fremstiller enkelte politiske/sosiale problemer over tid, som kvinners eller minoriteters rettigheter.</skos:definition>
      <skos:prefLabel xml:lang="no">Medieenhet: Tekst</skos:prefLabel>
      <skos:definition xml:lang="no">Alle skrevne tekster/enheter som bøker, artikler, tweets, blogger, etc. For eksempel: en studie om hatefulle ytringer i tweets, en studie om måten nyhetsaviser fremstiller enkelte politiske/sosiale problemer over tid, som kvinners eller minoriteters rettigheter.</skos:definition>
      <skos:prefLabel xml:lang="pt">Unidade de Media: Texto</skos:prefLabel>
      <skos:definition xml:lang="pt">Qualquer entidade/peça escrita, como livros, artigos, tweets, blogues, etc. Por exemplo, um estudo sobre discurso de ódio nos tweets, ou um estudo sobre a forma como os jornais apresentam certos fenómenos políticos/sociais ao longo do tempo, como os direitos das mulheres ou de outras minorias, etc.</skos:definition>
      <skos:prefLabel xml:lang="pt">Unidade de Media: Texto</skos:prefLabel>
      <skos:definition xml:lang="pt">Qualquer entidade/peça escrita, como livros, artigos, tweets, blogues, etc. Por exemplo, um estudo sobre discurso de ódio nos tweets, ou um estudo sobre a forma como os jornais apresentam certos fenómenos políticos/sociais ao longo do tempo, como os direitos das mulheres ou de outras minorias, etc.</skos:definition>
      <skos:prefLabel xml:lang="sl">Medijska enota: besedilo</skos:prefLabel>
      <skos:definition xml:lang="sl">Vsak pisni izdelek/entiteta, na primer knjige, članki, tviti, blogi itd. Na primer študija o sovražnem govoru v tvitih ali študija o tem, kako časopisi predstavljajo določena politična/družbena vprašanja v času, na primer pravice žensk ali manjšin itd.</skos:definition>
      <skos:prefLabel xml:lang="sl">Medijska enota: besedilo</skos:prefLabel>
      <skos:definition xml:lang="sl">Vsak pisni izdelek/entiteta, na primer knjige, članki, tviti, blogi itd. Na primer študija o sovražnem govoru v tvitih ali študija o tem, kako časopisi predstavljajo določena politična/družbena vprašanja v času, na primer pravice žensk ali manjšin itd.</skos:definition>
      <skos:prefLabel xml:lang="sv">Mediaenhet: Text</skos:prefLabel>
      <skos:definition xml:lang="sv">Skrivna texter, som böcker, artiklar, tweets, bloggar m.m. Till exempel en studie om hets mot folkgrupp i tweets, eller en studie om hur tidningar beskriver olika politiska/sociala ämnen över tid, som kvinnors eller minoriteters rättigheter osv.</skos:definition>
      <skos:prefLabel xml:lang="sv">Mediaenhet: Text</skos:prefLabel>
      <skos:definition xml:lang="sv">Skrivna texter, som böcker, artiklar, tweets, bloggar m.m. Till exempel en studie om hets mot folkgrupp i tweets, eller en studie om hur tidningar beskriver olika politiska/sociala ämnen över tid, som kvinnors eller minoriteters rättigheter osv.</skos:definition>
      <skos:prefLabel xml:lang="sv">Mediaenhet: Text</skos:prefLabel>
      <skos:definition xml:lang="sv">Skrivna texter, som böcker, artiklar, tweets, bloggar m.m. Till exempel en studie om hets mot folkgrupp i tweets, eller en studie om hur tidningar beskriver olika politiska/sociala ämnen över tid, som kvinnors eller minoriteters rättigheter osv.</skos:definition>
      <skos:broader rdf:resource="http://rdf-vocabulary.ddialliance.org/cv/AnalysisUnit/2.1.3/d151e910"/>
   </rdf:Description>
   <rdf:Description rdf:about="http://rdf-vocabulary.ddialliance.org/cv/AnalysisUnit/2.1.3/d151e1234">
      <rdf:type rdf:resource="http://www.w3.org/2004/02/skos/core#Concept"/>
      <skos:inScheme rdf:resource="http://rdf-vocabulary.ddialliance.org/cv/AnalysisUnit/2.1.3/"/>
      <skos:notation>MediaUnit.Video</skos:notation>
      <skos:prefLabel xml:lang="en">Media unit: Video</skos:prefLabel>
      <skos:definition xml:lang="en">Moving images. May include films, animation, digital recordings, visual output from simulations, recorded television programs, diagnostic/medical videos like ultrasound scans, etc. May be mute or may include synchronized sound.</skos:definition>
      <skos:prefLabel xml:lang="en">Media unit: Video</skos:prefLabel>
      <skos:definition xml:lang="en">Moving images. May include films, animation, digital recordings, visual output from simulations, recorded television programs, diagnostic/medical videos like ultrasound scans, etc. May be mute or may include synchronized sound.</skos:definition>
      <skos:prefLabel xml:lang="de">Medieneinheit: Video</skos:prefLabel>
      <skos:definition xml:lang="de">Bewegte Bilder. Das kann Filme, Animationen, digitale Aufnahmen, visuelle Ausgaben von Simulationen, aufgezeichnete Fernsehsendungen, diagnostische/medizinische Videos wie Ultraschalluntersuchungen usw. beinhalten. Das kann stummgeschalteten oder synchronisierten Ton beinhalten.</skos:definition>
      <skos:prefLabel xml:lang="de">Medieneinheit: Video</skos:prefLabel>
      <skos:definition xml:lang="de">Bewegte Bilder. Das kann Filme, Animationen, digitale Aufnahmen, visuelle Ausgaben von Simulationen, aufgezeichnete Fernsehsendungen, diagnostische/medizinische Videos wie Ultraschalluntersuchungen usw. beinhalten. Das kann stummgeschalteten oder synchronisierten Ton beinhalten.</skos:definition>
      <skos:prefLabel xml:lang="fi">Mediatyyppi: liikkuva kuva</skos:prefLabel>
      <skos:definition xml:lang="fi">Liikkuva kuva äänellä tai ilman. Esimerkiksi elokuvat, animaatiot, digitaaliset taltiot, simulaatioiden liikkuvat kuvat, taltioidut televisio-ohjelmat ja ultraäänikuvat.</skos:definition>
      <skos:prefLabel xml:lang="fi">Mediatyyppi: liikkuva kuva</skos:prefLabel>
      <skos:definition xml:lang="fi">Liikkuva kuva äänellä tai ilman. Esimerkiksi elokuvat, animaatiot, digitaaliset taltiot, simulaatioiden liikkuvat kuvat, taltioidut televisio-ohjelmat ja ultraäänikuvat.</skos:definition>
      <skos:prefLabel xml:lang="it">Unità di supporto: video</skos:prefLabel>
      <skos:definition xml:lang="it">Immagini in movimento. Può includere film, animazioni, registrazioni digitali, output visivi prodotti da simulazioni, programmi televisivi registrati, video medico/diagnostici come ecografie, ecc. Può essere muto o può includere il suono sincronizzato.</skos:definition>
      <skos:prefLabel xml:lang="it">Unità di supporto: video</skos:prefLabel>
      <skos:definition xml:lang="it">Immagini in movimento. Può includere film, animazioni, registrazioni digitali, output visivi prodotti da simulazioni, programmi televisivi registrati, video medico/diagnostici come ecografie, ecc. Può essere muto o può includere il suono sincronizzato.</skos:definition>
      <skos:prefLabel xml:lang="lt">Medijos vienetas: vaizdo įrašas</skos:prefLabel>
      <skos:definition xml:lang="lt">Judantys vaizdai. Gali apimti filmus, animaciją, skaitmeninius įrašus, simuliacijų vaizdinius produktus, įrašytas televizijos programas, diagnostinius ar medicininius vaizdo įrašus, tokius kaip ultragarso tyrimai ir kt. Gali būti be garso ar turėti garso sinchronizaciją.</skos:definition>
      <skos:prefLabel xml:lang="lt">Medijos vienetas: vaizdo įrašas</skos:prefLabel>
      <skos:definition xml:lang="lt">Judantys vaizdai. Gali apimti filmus, animaciją, skaitmeninius įrašus, simuliacijų vaizdinius produktus, įrašytas televizijos programas, diagnostinius ar medicininius vaizdo įrašus, tokius kaip ultragarso tyrimai ir kt. Gali būti be garso ar turėti garso sinchronizaciją.</skos:definition>
      <skos:prefLabel xml:lang="nl">Media-eenheid: Video</skos:prefLabel>
      <skos:definition xml:lang="nl"/>
      <skos:prefLabel xml:lang="nl">Media-eenheid: Video</skos:prefLabel>
      <skos:definition xml:lang="nl"/>
      <skos:prefLabel xml:lang="no">Medieenhet: video</skos:prefLabel>
      <skos:definition xml:lang="no">Bevegelige bilder. Kan inkludere filmer, animasjoner, digitale opptak, visuell produksjon fra simuleringer, innspilte fjernsynsprogram, diagnostiske/medisinske videor som ultralyd skanninger, etc. Kan være uten lyd eller med synkronisert lyd.</skos:definition>
      <skos:prefLabel xml:lang="no">Medieenhet: video</skos:prefLabel>
      <skos:definition xml:lang="no">Bevegelige bilder. Kan inkludere filmer, animasjoner, digitale opptak, visuell produksjon fra simuleringer, innspilte fjernsynsprogram, diagnostiske/medisinske videor som ultralyd skanninger, etc. Kan være uten lyd eller med synkronisert lyd.</skos:definition>
      <skos:prefLabel xml:lang="pt">Unidade de Media: Vídeo</skos:prefLabel>
      <skos:definition xml:lang="pt">Imagens em movimento. Pode incluir filmes, animação, gravações digitais, output visual de simulações, programas televisivos gravados, vídeos médicos/de diagnóstico como ultrasons, etc. Podem ser silenciosos ou podem incluir som sincronizado.</skos:definition>
      <skos:prefLabel xml:lang="pt">Unidade de Media: Vídeo</skos:prefLabel>
      <skos:definition xml:lang="pt">Imagens em movimento. Pode incluir filmes, animação, gravações digitais, output visual de simulações, programas televisivos gravados, vídeos médicos/de diagnóstico como ultrasons, etc. Podem ser silenciosos ou podem incluir som sincronizado.</skos:definition>
      <skos:prefLabel xml:lang="sl">Medijska enota: video</skos:prefLabel>
      <skos:definition xml:lang="sl">Premične slike. Vključujejo lahko filme, animacije, digitalne posnetke, vizualne rezultate simulacij, posnete televizijske programe, diagnostične/medicinske video posnetke, kot so ultrazvočni pregledi itd.</skos:definition>
      <skos:prefLabel xml:lang="sl">Medijska enota: video</skos:prefLabel>
      <skos:definition xml:lang="sl">Premične slike. Vključujejo lahko filme, animacije, digitalne posnetke, vizualne rezultate simulacij, posnete televizijske programe, diagnostične/medicinske video posnetke, kot so ultrazvočni pregledi itd.</skos:definition>
      <skos:prefLabel xml:lang="sv">Mediaenhet: Video</skos:prefLabel>
      <skos:definition xml:lang="sv">Rörliga bilder. Det kan inkludera filmer, animationer, digitala inspelningar, visuella utdata från simuleringar, inspelade tv-program, diagnostiska/medicinska videor som ultraljudsundersökningar osv. De kan vara utan ljud eller med synkroniserat ljud.</skos:definition>
      <skos:prefLabel xml:lang="sv">Mediaenhet: Video</skos:prefLabel>
      <skos:definition xml:lang="sv">Rörliga bilder. Det kan inkludera filmer, animationer, digitala inspelningar, visuella utdata från simuleringar, inspelade tv-program, diagnostiska/medicinska videor som ultraljudsundersökningar osv. De kan vara utan ljud eller med synkroniserat ljud.</skos:definition>
      <skos:prefLabel xml:lang="sv">Mediaenhet: Video</skos:prefLabel>
      <skos:definition xml:lang="sv">Rörliga bilder. Det kan inkludera filmer, animationer, digitala inspelningar, visuella utdata från simuleringar, inspelade tv-program, diagnostiska/medicinska videor som ultraljudsundersökningar osv. De kan vara utan ljud eller med synkroniserat ljud.</skos:definition>
      <skos:broader rdf:resource="http://rdf-vocabulary.ddialliance.org/cv/AnalysisUnit/2.1.3/d151e910"/>
   </rdf:Description>
   <rdf:Description rdf:about="http://rdf-vocabulary.ddialliance.org/cv/AnalysisUnit/2.1.3/d151e1313">
      <rdf:type rdf:resource="http://www.w3.org/2004/02/skos/core#Concept"/>
      <skos:inScheme rdf:resource="http://rdf-vocabulary.ddialliance.org/cv/AnalysisUnit/2.1.3/"/>
      <skos:notation>Group</skos:notation>
      <skos:prefLabel xml:lang="en">Group</skos:prefLabel>
      <skos:definition xml:lang="en">Two or more individuals assembled together or having some unifying relationship or characteristic. In surveys, the questions are mainly focused on the group and the attitudes/experiences of the group, rather than on those of the individual respondents. If questions cover both the group and the individual, use  both as analysis units.</skos:definition>
      <skos:prefLabel xml:lang="en">Group</skos:prefLabel>
      <skos:definition xml:lang="en">Two or more individuals assembled together or having some unifying relationship or characteristic. In surveys, the questions are mainly focused on the group and the attitudes/experiences of the group, rather than on those of the individual respondents. If questions cover both the group and the individual, use  both as analysis units.</skos:definition>
      <skos:prefLabel xml:lang="de">Gruppe</skos:prefLabel>
      <skos:definition xml:lang="de">Zwei oder mehr Individuen, die zusammen versammelt sind oder eine verbindende Beziehung oder Eigenschaft haben. In Umfragen konzentrieren sich die Fragen hauptsächlich auf die Gruppe und die Einstellungen/Erfahrungen der Gruppe und nicht auf die der einzelnen Befragten. Wenn sich die Fragen sowohl auf die Gruppe als auch auf das Individuum beziehen, können beide Analyseeinheiten verwendet werden.</skos:definition>
      <skos:prefLabel xml:lang="de">Gruppe</skos:prefLabel>
      <skos:definition xml:lang="de">Zwei oder mehr Individuen, die zusammen versammelt sind oder eine verbindende Beziehung oder Eigenschaft haben. In Umfragen konzentrieren sich die Fragen hauptsächlich auf die Gruppe und die Einstellungen/Erfahrungen der Gruppe und nicht auf die der einzelnen Befragten. Wenn sich die Fragen sowohl auf die Gruppe als auch auf das Individuum beziehen, können beide Analyseeinheiten verwendet werden.</skos:definition>
      <skos:prefLabel xml:lang="fi">Ryhmä</skos:prefLabel>
      <skos:definition xml:lang="fi">Kaksi tai useampia henkilöitä, jotka ovat joko kokoontuneet yhteen tai joita yhdistää jokin muu tekijä. Mikäli kyselytutkimus, kysymykset koskevat pääasiassa itse ryhmää, ryhmän kokemuksia ja asenteita ryhmää kohtaan, ei henkilöä itseään. Mikäli kysymykset koskevat sekä ryhmää että henkilöä, käytä havaintoyksikkönä molempia.</skos:definition>
      <skos:prefLabel xml:lang="fi">Ryhmä</skos:prefLabel>
      <skos:definition xml:lang="fi">Kaksi tai useampia henkilöitä, jotka ovat joko kokoontuneet yhteen tai joita yhdistää jokin muu tekijä. Mikäli kyselytutkimus, kysymykset koskevat pääasiassa itse ryhmää, ryhmän kokemuksia ja asenteita ryhmää kohtaan, ei henkilöä itseään. Mikäli kysymykset koskevat sekä ryhmää että henkilöä, käytä havaintoyksikkönä molempia.</skos:definition>
      <skos:prefLabel xml:lang="it">Gruppo</skos:prefLabel>
      <skos:definition xml:lang="it">Due o più individui riuniti oppure che possiedono una qualsiasi relazione o caratteristica unificante. Nelle indagini le domande si concentrano principalmente sul gruppo e sugli atteggiamenti/esperienze del gruppo, piuttosto che su quelle dei singoli intervistati. Se le domande riguardano sia il gruppo che l'individuo, utilizzare entrambi come unità di analisi.</skos:definition>
      <skos:prefLabel xml:lang="it">Gruppo</skos:prefLabel>
      <skos:definition xml:lang="it">Due o più individui riuniti oppure che possiedono una qualsiasi relazione o caratteristica unificante. Nelle indagini le domande si concentrano principalmente sul gruppo e sugli atteggiamenti/esperienze del gruppo, piuttosto che su quelle dei singoli intervistati. Se le domande riguardano sia il gruppo che l'individuo, utilizzare entrambi come unità di analisi.</skos:definition>
      <skos:prefLabel xml:lang="lt">Grupė </skos:prefLabel>
      <skos:definition xml:lang="lt">Du ar daugiau asmenų, susibūrusių kartu arba turinčių tam tikrų vienijančių ryšių ar savybių. Atliekant apklausas klausimai gali būti nukreipti į grupę ir grupės, o ne atskirų respondentų, požiūrius ar patirtis. Jei klausimai apima tiek grupę, tiek asmenį, naudoti abu kaip analizės vienetus.</skos:definition>
      <skos:prefLabel xml:lang="lt">Grupė </skos:prefLabel>
      <skos:definition xml:lang="lt">Du ar daugiau asmenų, susibūrusių kartu arba turinčių tam tikrų vienijančių ryšių ar savybių. Atliekant apklausas klausimai gali būti nukreipti į grupę ir grupės, o ne atskirų respondentų, požiūrius ar patirtis. Jei klausimai apima tiek grupę, tiek asmenį, naudoti abu kaip analizės vienetus.</skos:definition>
      <skos:prefLabel xml:lang="nl">Groep</skos:prefLabel>
      <skos:definition xml:lang="nl"/>
      <skos:prefLabel xml:lang="nl">Groep</skos:prefLabel>
      <skos:definition xml:lang="nl"/>
      <skos:prefLabel xml:lang="no">Gruppe</skos:prefLabel>
      <skos:definition xml:lang="no">To eller flere personer som samles eller som har et forhold som forener dem. I spørreundersøkelser er spørsmålene hovedsaklig rettet mot gruppen og holdningen/opplevelsene til gruppen i steden for de individuelle respondentene. Hvis spørsmål angår både gruppen og individene, bruk begge som analyseenhet.</skos:definition>
      <skos:prefLabel xml:lang="no">Gruppe</skos:prefLabel>
      <skos:definition xml:lang="no">To eller flere personer som samles eller som har et forhold som forener dem. I spørreundersøkelser er spørsmålene hovedsaklig rettet mot gruppen og holdningen/opplevelsene til gruppen i steden for de individuelle respondentene. Hvis spørsmål angår både gruppen og individene, bruk begge som analyseenhet.</skos:definition>
      <skos:prefLabel xml:lang="pt">Grupo</skos:prefLabel>
      <skos:definition xml:lang="pt">Dois ou mais indivíduos que se assemelham ou que têm uma relação ou característica unificadora. Nos inquéritos, as questões são principalmente focadas no grupo e nas atitudes e experiências do grupo, e não tanto nos indivíduos entrevistados. Se as questões abrangem o indivíduo e o grupo, usar ambos como unidades de análise.</skos:definition>
      <skos:prefLabel xml:lang="pt">Grupo</skos:prefLabel>
      <skos:definition xml:lang="pt">Dois ou mais indivíduos que se assemelham ou que têm uma relação ou característica unificadora. Nos inquéritos, as questões são principalmente focadas no grupo e nas atitudes e experiências do grupo, e não tanto nos indivíduos entrevistados. Se as questões abrangem o indivíduo e o grupo, usar ambos como unidades de análise.</skos:definition>
      <skos:prefLabel xml:lang="sl">Skupina</skos:prefLabel>
      <skos:definition xml:lang="sl">Dva ali več posameznikov, zbranih skupaj oziroma vključenih v medsebojen odnos. V anketnih raziskavah so vprašanja osredotočena predvsem na skupino in stališča / izkušnje skupine, ne pa na stališča posameznih anketirancev. Če se vprašanja nanašajo skupino in posameznika, uporabite oba kot enoti za analizo.</skos:definition>
      <skos:prefLabel xml:lang="sl">Skupina</skos:prefLabel>
      <skos:definition xml:lang="sl">Dva ali več posameznikov, zbranih skupaj oziroma vključenih v medsebojen odnos. V anketnih raziskavah so vprašanja osredotočena predvsem na skupino in stališča / izkušnje skupine, ne pa na stališča posameznih anketirancev. Če se vprašanja nanašajo skupino in posameznika, uporabite oba kot enoti za analizo.</skos:definition>
      <skos:prefLabel xml:lang="sv">Grupp</skos:prefLabel>
      <skos:definition xml:lang="sv">Två eller fler personer som samlats eller som har någon form av relation eller egenskap som förenar dem. I surveyundersökningar fokuserar frågorna framför allt på gruppen och gruppens attityder/erfarenheter, snarare än på de enskilda respondenterna. Om frågorna gäller både gruppen och individen, använd båda som analysenheter.</skos:definition>
      <skos:prefLabel xml:lang="sv">Grupp</skos:prefLabel>
      <skos:definition xml:lang="sv">Två eller fler personer som samlats eller som har någon form av relation eller egenskap som förenar dem. I surveyundersökningar fokuserar frågorna framför allt på gruppen och gruppens attityder/erfarenheter, snarare än på de enskilda respondenterna. Om frågorna gäller både gruppen och individen, använd båda som analysenheter.</skos:definition>
      <skos:prefLabel xml:lang="sv">Grupp</skos:prefLabel>
      <skos:definition xml:lang="sv">Två eller fler personer som samlats eller som har någon form av relation eller egenskap som förenar dem. I surveyundersökningar fokuserar frågorna framför allt på gruppen och gruppens attityder/erfarenheter, snarare än på de enskilda respondenterna. Om frågorna gäller både gruppen och individen, använd båda som analysenheter.</skos:definition>
   </rdf:Description>
   <rdf:Description rdf:about="http://rdf-vocabulary.ddialliance.org/cv/AnalysisUnit/2.1.3/d151e1393">
      <rdf:type rdf:resource="http://www.w3.org/2004/02/skos/core#Concept"/>
      <skos:inScheme rdf:resource="http://rdf-vocabulary.ddialliance.org/cv/AnalysisUnit/2.1.3/"/>
      <skos:notation>Object</skos:notation>
      <skos:prefLabel xml:lang="en">Object</skos:prefLabel>
      <skos:definition xml:lang="en">Anything material, but inanimate, that has an independent existence and may be perceived by the senses. Examples: objects of art (paintings, sculptures, etc.) or weapons, or vehicles, etc.</skos:definition>
      <skos:prefLabel xml:lang="en">Object</skos:prefLabel>
      <skos:definition xml:lang="en">Anything material, but inanimate, that has an independent existence and may be perceived by the senses. Examples: objects of art (paintings, sculptures, etc.) or weapons, or vehicles, etc.</skos:definition>
      <skos:prefLabel xml:lang="de">Objekt</skos:prefLabel>
      <skos:definition xml:lang="de">Alle nicht lebenden Stoffe, die eine unabhängige Existenz haben und mit den Sinnen wahrgenommen werden können. Beispiele: Kunstobjekte (Gemälde, Skulpturen, etc.) oder Waffen oder Fahrzeuge usw.</skos:definition>
      <skos:prefLabel xml:lang="de">Objekt</skos:prefLabel>
      <skos:definition xml:lang="de">Alle nicht lebenden Stoffe, die eine unabhängige Existenz haben und mit den Sinnen wahrgenommen werden können. Beispiele: Kunstobjekte (Gemälde, Skulpturen, etc.) oder Waffen oder Fahrzeuge usw.</skos:definition>
      <skos:prefLabel xml:lang="fi">Eloton objekti/esine</skos:prefLabel>
      <skos:definition xml:lang="fi">Mikä tahansa konkreettinen, eloton esine/kohde, joka voidaan aistein havaita. Esimerkiksi taideteokset (veistokset, maalaukset), aseet, ajoneuvot jne.</skos:definition>
      <skos:prefLabel xml:lang="fi">Eloton objekti/esine</skos:prefLabel>
      <skos:definition xml:lang="fi">Mikä tahansa konkreettinen, eloton esine/kohde, joka voidaan aistein havaita. Esimerkiksi taideteokset (veistokset, maalaukset), aseet, ajoneuvot jne.</skos:definition>
      <skos:prefLabel xml:lang="it">Oggetto</skos:prefLabel>
      <skos:definition xml:lang="it">Tutto ciò che è materiale, inanimato, che ha un'esistenza indipendente e che può essere percepito attraverso i sensi. Esempi: oggetti d'arte (dipinti, sculture, ecc.), armi, veicoli, ecc.</skos:definition>
      <skos:prefLabel xml:lang="it">Oggetto</skos:prefLabel>
      <skos:definition xml:lang="it">Tutto ciò che è materiale, inanimato, che ha un'esistenza indipendente e che può essere percepito attraverso i sensi. Esempi: oggetti d'arte (dipinti, sculture, ecc.), armi, veicoli, ecc.</skos:definition>
      <skos:prefLabel xml:lang="lt">Objektas</skos:prefLabel>
      <skos:definition xml:lang="lt">Visa, kas materialu, bet negyva, egzistuoja savarankiškai ir gali būti juntama juslėmis. Pavyzdžiai: meno kūriniai (paveikslai, skulptūros ir kt.), ginklai ar transporto priemonės ir kt.</skos:definition>
      <skos:prefLabel xml:lang="lt">Objektas</skos:prefLabel>
      <skos:definition xml:lang="lt">Visa, kas materialu, bet negyva, egzistuoja savarankiškai ir gali būti juntama juslėmis. Pavyzdžiai: meno kūriniai (paveikslai, skulptūros ir kt.), ginklai ar transporto priemonės ir kt.</skos:definition>
      <skos:prefLabel xml:lang="nl">Voorwerp</skos:prefLabel>
      <skos:definition xml:lang="nl"/>
      <skos:prefLabel xml:lang="nl">Voorwerp</skos:prefLabel>
      <skos:definition xml:lang="nl"/>
      <skos:prefLabel xml:lang="no">Objekt</skos:prefLabel>
      <skos:definition xml:lang="no">Noe fysisk, men ikke levende som eksisterer som en uavhengig enhet og som kan oppfattes av sansene. For eksempel: kunst (malerier, skulpturer osv.), våpen, kjøretøy etc.</skos:definition>
      <skos:prefLabel xml:lang="no">Objekt</skos:prefLabel>
      <skos:definition xml:lang="no">Noe fysisk, men ikke levende som eksisterer som en uavhengig enhet og som kan oppfattes av sansene. For eksempel: kunst (malerier, skulpturer osv.), våpen, kjøretøy etc.</skos:definition>
      <skos:prefLabel xml:lang="pt">Objeto</skos:prefLabel>
      <skos:definition xml:lang="pt">Qualquer coisa material, mas inanimada, que tenha uma existência independente e possa ser percebida pelos sentidos. Exemplos: objetos de arte (pinturas, esculturas, etc.) ou armas, ou veículos, etc.</skos:definition>
      <skos:prefLabel xml:lang="pt">Objeto</skos:prefLabel>
      <skos:definition xml:lang="pt">Qualquer coisa material, mas inanimada, que tenha uma existência independente e possa ser percebida pelos sentidos. Exemplos: objetos de arte (pinturas, esculturas, etc.) ou armas, ou veículos, etc.</skos:definition>
      <skos:prefLabel xml:lang="sl">Predmet</skos:prefLabel>
      <skos:definition xml:lang="sl">Karkoli materialnega, toda neživega, kar ima neodvisen obstoj in ga lahko zaznamo s čutili. Primeri: umetniški predmeti (slike, skulpture itd.), orožje, vozila itd.</skos:definition>
      <skos:prefLabel xml:lang="sl">Predmet</skos:prefLabel>
      <skos:definition xml:lang="sl">Karkoli materialnega, toda neživega, kar ima neodvisen obstoj in ga lahko zaznamo s čutili. Primeri: umetniški predmeti (slike, skulpture itd.), orožje, vozila itd.</skos:definition>
      <skos:prefLabel xml:lang="sv">Föremål</skos:prefLabel>
      <skos:definition xml:lang="sv">Något fysiskt men icke levande som existerar som en oberoende enhet och kan uppfattas av sinnena. Exempel: konstföremål (tavlor, skulpturer, o.dyl.), vapen, fordon m.m.</skos:definition>
      <skos:prefLabel xml:lang="sv">Föremål</skos:prefLabel>
      <skos:definition xml:lang="sv">Något fysiskt men icke levande som existerar som en oberoende enhet och kan uppfattas av sinnena. Exempel: konstföremål (tavlor, skulpturer, o.dyl.), vapen, fordon m.m.</skos:definition>
      <skos:prefLabel xml:lang="sv">Föremål</skos:prefLabel>
      <skos:definition xml:lang="sv">Något fysiskt men icke levande som existerar som en oberoende enhet och kan uppfattas av sinnena. Exempel: konstföremål (tavlor, skulpturer, o.dyl.), vapen, fordon m.m.</skos:definition>
   </rdf:Description>
   <rdf:Description rdf:about="http://rdf-vocabulary.ddialliance.org/cv/AnalysisUnit/2.1.3/d151e1472">
      <rdf:type rdf:resource="http://www.w3.org/2004/02/skos/core#Concept"/>
      <skos:inScheme rdf:resource="http://rdf-vocabulary.ddialliance.org/cv/AnalysisUnit/2.1.3/"/>
      <skos:notation>Other</skos:notation>
      <skos:prefLabel xml:lang="en">Other</skos:prefLabel>
      <skos:definition xml:lang="en">Use if the unit of analysis is known, but not found in the list.</skos:definition>
      <skos:prefLabel xml:lang="en">Other</skos:prefLabel>
      <skos:definition xml:lang="en">Use if the unit of analysis is known, but not found in the list.</skos:definition>
      <skos:prefLabel xml:lang="de">Sonstiges</skos:prefLabel>
      <skos:definition xml:lang="de">Wird verwendet, wenn die Analyseeinheit bekannt ist, aber nicht in der Liste vertreten ist.</skos:definition>
      <skos:prefLabel xml:lang="de">Sonstiges</skos:prefLabel>
      <skos:definition xml:lang="de">Wird verwendet, wenn die Analyseeinheit bekannt ist, aber nicht in der Liste vertreten ist.</skos:definition>
      <skos:prefLabel xml:lang="fi">Muu havainto/aineistoyksikkötyyppi</skos:prefLabel>
      <skos:definition xml:lang="fi">Käytä mikäli havaintoyksikkö on tiedossa, mutta ei löydy sanastosta.</skos:definition>
      <skos:prefLabel xml:lang="fi">Muu havainto/aineistoyksikkötyyppi</skos:prefLabel>
      <skos:definition xml:lang="fi">Käytä mikäli havaintoyksikkö on tiedossa, mutta ei löydy sanastosta.</skos:definition>
      <skos:prefLabel xml:lang="it">Altro</skos:prefLabel>
      <skos:definition xml:lang="it">Utilizzare se l'unità di analisi è nota, ma non riconducibile a nessun termine presente nell'elenco.</skos:definition>
      <skos:prefLabel xml:lang="it">Altro</skos:prefLabel>
      <skos:definition xml:lang="it">Utilizzare se l'unità di analisi è nota, ma non riconducibile a nessun termine presente nell'elenco.</skos:definition>
      <skos:prefLabel xml:lang="lt">Kita</skos:prefLabel>
      <skos:definition xml:lang="lt">Naudoti, kai analizės vienetas yra žinomas, bet sąraše jo nėra.</skos:definition>
      <skos:prefLabel xml:lang="lt">Kita</skos:prefLabel>
      <skos:definition xml:lang="lt">Naudoti, kai analizės vienetas yra žinomas, bet sąraše jo nėra.</skos:definition>
      <skos:prefLabel xml:lang="nl">Anders</skos:prefLabel>
      <skos:definition xml:lang="nl"/>
      <skos:prefLabel xml:lang="nl">Anders</skos:prefLabel>
      <skos:definition xml:lang="nl"/>
      <skos:prefLabel xml:lang="no">Annet</skos:prefLabel>
      <skos:definition xml:lang="no">Benytt hvis analyseenheten er kjent, men ikke finnes i listen.</skos:definition>
      <skos:prefLabel xml:lang="no">Annet</skos:prefLabel>
      <skos:definition xml:lang="no">Benytt hvis analyseenheten er kjent, men ikke finnes i listen.</skos:definition>
      <skos:prefLabel xml:lang="pt">Outro </skos:prefLabel>
      <skos:definition xml:lang="pt">Usar se a unidade de análise for conhecida, mas não se encontrar na lista.</skos:definition>
      <skos:prefLabel xml:lang="pt">Outro </skos:prefLabel>
      <skos:definition xml:lang="pt">Usar se a unidade de análise for conhecida, mas não se encontrar na lista.</skos:definition>
      <skos:prefLabel xml:lang="sl">Drugo</skos:prefLabel>
      <skos:definition xml:lang="sl">Uporabite, če je enota analize poznana, a je ne najdete na seznamu.</skos:definition>
      <skos:prefLabel xml:lang="sl">Drugo</skos:prefLabel>
      <skos:definition xml:lang="sl">Uporabite, če je enota analize poznana, a je ne najdete na seznamu.</skos:definition>
      <skos:prefLabel xml:lang="sv">Övrigt</skos:prefLabel>
      <skos:definition xml:lang="sv">Använd om analysenheten är känd men saknas i listan.</skos:definition>
      <skos:prefLabel xml:lang="sv">Övrigt</skos:prefLabel>
      <skos:definition xml:lang="sv">Använd om analysenheten är känd men saknas i listan.</skos:definition>
      <skos:prefLabel xml:lang="sv">Övrigt</skos:prefLabel>
      <skos:definition xml:lang="sv">Använd om analysenheten är känd men saknas i listan.</skos:definition>
   </rdf:Description>
</rdf:RDF>
