<?xml version="1.0" encoding="UTF-8"?>
<rdf:RDF xmlns:rdf="http://www.w3.org/1999/02/22-rdf-syntax-ns#"
         xmlns:skos="http://www.w3.org/2004/02/skos/core#"
         xmlns:owl="http://www.w3.org/2002/07/owl#"
         xmlns:dcterms="http://purl.org/dc/terms/"
>
   <rdf:Description rdf:about="http://rdf-vocabulary.ddialliance.org/cv/ModeOfCollection/3.0.0/">
      <rdf:type rdf:resource="http://www.w3.org/2004/02/skos/core#ConceptScheme"/>
      <dcterms:isVersionOf rdf:resource="http://rdf-vocabulary.ddialliance.org/cv/ModeOfCollection/"/>
      <skos:notation xml:lang="en">ModeOfCollection</skos:notation>
      <dcterms:title xml:lang="en">Mode Of Collection</dcterms:title>
      <dcterms:description xml:lang="en">The procedure, technique, or mode of inquiry used to attain the data.</dcterms:description>
      <skos:prefLabel xml:lang="en">Mode Of Collection</skos:prefLabel>
      <dcterms:title xml:lang="da">Indsamlingsmetode</dcterms:title>
      <dcterms:description xml:lang="da">Fremgangsm&#xe5;den, teknikken eller unders&#xf8;gelsesmetoden, der er anvendt til at opn&#xe5; dataene.</dcterms:description>
      <skos:prefLabel xml:lang="da">Indsamlingsmetode</skos:prefLabel>
      <dcterms:title xml:lang="fi">Keruumenetelm&#xe4;</dcterms:title>
      <dcterms:description xml:lang="fi">Kuvailtavan aineiston ensisijainen keruumenetelm&#xe4;.</dcterms:description>
      <skos:prefLabel xml:lang="fi">Keruumenetelm&#xe4;</skos:prefLabel>
      <dcterms:title xml:lang="fr">Mode de collecte</dcterms:title>
      <dcterms:description xml:lang="fr">La proc&#xe9;dure, la technique ou le mode d&apos;enqu&#xea;te utilis&#xe9; pour obtenir les donn&#xe9;es.</dcterms:description>
      <skos:prefLabel xml:lang="fr">Mode de collecte</skos:prefLabel>
      <dcterms:title xml:lang="it">Metodo di raccolta dei dati</dcterms:title>
      <dcterms:description xml:lang="it">La procedura, la tecnica o la modalit&#xe0; di indagine utilizzata per ottenere i dati.</dcterms:description>
      <skos:prefLabel xml:lang="it">Metodo di raccolta dei dati</skos:prefLabel>
      <dcterms:title xml:lang="no">Innsamlingsmetode</dcterms:title>
      <dcterms:description xml:lang="no">Framgangsm&#xe5;ten, teknikken, eller metoden som er anvendt for &#xe5; samle inn data.</dcterms:description>
      <skos:prefLabel xml:lang="no">Innsamlingsmetode</skos:prefLabel>
      <dcterms:title xml:lang="pt">M&#xe9;todo de recolha de dados</dcterms:title>
      <dcterms:description xml:lang="pt">Procedimentos, t&#xe9;cnicas ou m&#xe9;todos de recolha de dados.</dcterms:description>
      <skos:prefLabel xml:lang="pt">M&#xe9;todo de recolha de dados</skos:prefLabel>
      <dcterms:title xml:lang="sl">Na&#x10d;in zbiranja podatkov</dcterms:title>
      <dcterms:description xml:lang="sl">Postopki, tehnike ali na&#x10d;ini raziskovanja, uporabljeni za pridobivanje podatkov.</dcterms:description>
      <skos:prefLabel xml:lang="sl">Na&#x10d;in zbiranja podatkov</skos:prefLabel>
      <dcterms:title xml:lang="sr">Na&#x10d;in prikupljanja</dcterms:title>
      <dcterms:description xml:lang="sr">Postupak, tehnika ili na&#x10d;in ispitivanja koji se koristi za dobijanje podataka.</dcterms:description>
      <skos:prefLabel xml:lang="sr">Na&#x10d;in prikupljanja</skos:prefLabel>
      <dcterms:title xml:lang="sv">Insamlingsmetod</dcterms:title>
      <dcterms:description xml:lang="sv">Den process, metod eller teknik som anv&#xe4;ndes f&#xf6;r att samla in data.</dcterms:description>
      <skos:prefLabel xml:lang="sv">Insamlingsmetod</skos:prefLabel>
      <owl:versionInfo>3.0.0</owl:versionInfo>
      <dcterms:license rdf:resource="http://creativecommons.org/licenses/by/4.0/"/>
      <dcterms:rights>Copyright &#xa9;DDI Alliance 2020</dcterms:rights>
      <skos:hasTopConcept rdf:resource="http://rdf-vocabulary.ddialliance.org/cv/ModeOfCollection/3.0.0/cb20d17"/>
      <skos:hasTopConcept rdf:resource="http://rdf-vocabulary.ddialliance.org/cv/ModeOfCollection/3.0.0/35e4248"/>
      <skos:hasTopConcept rdf:resource="http://rdf-vocabulary.ddialliance.org/cv/ModeOfCollection/3.0.0/9ec957d"/>
      <skos:hasTopConcept rdf:resource="http://rdf-vocabulary.ddialliance.org/cv/ModeOfCollection/3.0.0/08e658a"/>
      <skos:hasTopConcept rdf:resource="http://rdf-vocabulary.ddialliance.org/cv/ModeOfCollection/3.0.0/c680d43"/>
      <skos:hasTopConcept rdf:resource="http://rdf-vocabulary.ddialliance.org/cv/ModeOfCollection/3.0.0/05aeba4"/>
      <skos:hasTopConcept rdf:resource="http://rdf-vocabulary.ddialliance.org/cv/ModeOfCollection/3.0.0/c5564d2"/>
      <skos:hasTopConcept rdf:resource="http://rdf-vocabulary.ddialliance.org/cv/ModeOfCollection/3.0.0/4848ed5"/>
      <skos:hasTopConcept rdf:resource="http://rdf-vocabulary.ddialliance.org/cv/ModeOfCollection/3.0.0/df9aac3"/>
      <skos:hasTopConcept rdf:resource="http://rdf-vocabulary.ddialliance.org/cv/ModeOfCollection/3.0.0/6decc77"/>
      <skos:hasTopConcept rdf:resource="http://rdf-vocabulary.ddialliance.org/cv/ModeOfCollection/3.0.0/2906121"/>
      <skos:hasTopConcept rdf:resource="http://rdf-vocabulary.ddialliance.org/cv/ModeOfCollection/3.0.0/d9ceca6"/>
      <skos:hasTopConcept rdf:resource="http://rdf-vocabulary.ddialliance.org/cv/ModeOfCollection/3.0.0/4f502b5"/>
      <skos:hasTopConcept rdf:resource="http://rdf-vocabulary.ddialliance.org/cv/ModeOfCollection/3.0.0/38ceaa4"/>
      <skos:hasTopConcept rdf:resource="http://rdf-vocabulary.ddialliance.org/cv/ModeOfCollection/3.0.0/6311ae1"/>
   </rdf:Description>
   <rdf:Description rdf:about="http://rdf-vocabulary.ddialliance.org/cv/ModeOfCollection/3.0.0/cb20d17">
      <rdf:type rdf:resource="http://www.w3.org/2004/02/skos/core#Concept"/>
      <skos:inScheme rdf:resource="http://rdf-vocabulary.ddialliance.org/cv/ModeOfCollection/3.0.0/"/>
      <skos:notation xml:lang="en">Interview</skos:notation>
      <skos:prefLabel xml:lang="en">Interview</skos:prefLabel>
      <skos:definition xml:lang="en">A pre-planned communication between two (or more) people - the interviewer(s) and the interviewee(s) - in which information is obtained by the interviewer(s) from the interviewee(s). If group interaction is part of the method, use &quot;Focus group&quot;.</skos:definition>
      <skos:prefLabel xml:lang="da">Interview</skos:prefLabel>
      <skos:definition xml:lang="da">En forudplanlagt kommunikation mellem to (eller flere) personer &#x2013; interviewere(n) og de(n) interviewede - hvor intervieweren(ne)&#xa0;f&#xe5;r information&#xa0;fra de(n) interviewede. Hvis gruppeinteraktion er en del af metoden, anvend &#x201d;Fokusgruppe&#x201d;.</skos:definition>
      <skos:prefLabel xml:lang="fi">Haastattelu</skos:prefLabel>
      <skos:definition xml:lang="fi">Ennalta suunniteltu, haastattelijan ja yhden tai useamman haastateltavan v&#xe4;linen keskustelu, jossa haastattelija saa tietoa tutkimustarkoituksiin. K&#xe4;yt&#xe4; tarkempaa haastattelutermi&#xe4;, mik&#xe4;li mahdollista. Jos haastateltavia on enemm&#xe4;n kuin yksi ja ryhm&#xe4;n keskin&#xe4;inen vuorovaikutus on t&#xe4;rke&#xe4;&#xe4;, k&#xe4;ytet&#xe4;&#xe4;n termi&#xe4; &apos;Kohderyhm&#xe4;keskustelu&apos;.</skos:definition>
      <skos:prefLabel xml:lang="fr">Entretien</skos:prefLabel>
      <skos:definition xml:lang="fr">Un &#xe9;change pr&#xe9;vu entre deux (ou plusieurs) personnes - l(es) enqu&#xea;teur(s) et l(es) enqu&#xea;t&#xe9;(s) - dans lequel des informations sont obtenus par l(es) enqu&#xea;teur(s) d(es) enqu&#xea;t&#xe9;(s). Si l&apos;interaction de groupe fait partie de la m&#xe9;thode, utilisez &quot;Focus group&quot;</skos:definition>
      <skos:prefLabel xml:lang="it">Intervista</skos:prefLabel>
      <skos:definition xml:lang="it">Una comunicazione pianificata tra due (o pi&#xf9;) persone - l&apos;intervistatore/i e l&apos;intervistato/i - in cui le informazioni ottenute dall&apos;intervistatore sono state rilasciate dagli intervistati. Se l&apos;interazione di gruppo &#xe8; parte della tecnica, utilizzare &quot;Focus group&quot;.</skos:definition>
      <skos:prefLabel xml:lang="no">Intervju</skos:prefLabel>
      <skos:definition xml:lang="no">En forh&#xe5;ndsbestemt kommunikasjon mellom to (eller flere) personer &#x2013; intervjueren(e) og intervjuobjekt(et/ene) &#x2013; hvor intervjueren(e) henter informasjon fra intervjuobjekt(et/ene). Dersom gruppeinteraksjoner er del av metoden, bruk &apos;Fokusgruppe&apos;.</skos:definition>
      <skos:prefLabel xml:lang="pt">Entrevista</skos:prefLabel>
      <skos:definition xml:lang="pt">Uma comunica&#xe7;&#xe3;o pr&#xe9;-planeada entre duas (ou mais) pessoas - o(s) entrevistador(es) e o(s) entrevistado(s) - em que a informa&#xe7;&#xe3;o &#xe9; obtida pelo(s) entrevistador(es) do(s) entrevistado(s). Se a intera&#xe7;&#xe3;o no grupo fizer parte do m&#xe9;todo, usar &quot;Focus group&quot;.</skos:definition>
      <skos:prefLabel xml:lang="sl">Intervju</skos:prefLabel>
      <skos:definition xml:lang="sl">Vnaprej na&#x10d;rtovana komunikacija med dvema (ali ve&#x10d;) osebami - spra&#x161;evalcem(-ci) in spra&#x161;evancem(-ci) -, kjer spra&#x161;evalec(-ci) pridobi(jo) informacije s strani spra&#x161;evanca(-cev). &#x10c;e je v metodo vklju&#x10d;ena skupinska interakcija, uporabite izraz &quot;fokusna skupina&quot;.</skos:definition>
      <skos:prefLabel xml:lang="sr">Intervju</skos:prefLabel>
      <skos:definition xml:lang="sr">Unapred planirana komunikacija izme&#x111;u dve (ili vi&#x161;e) osoba - anketara i sagovornika (anketiranog), u kojoj informacije dobija anketar od anketiranog. Ukoliko je grupna interakcija deo ove metode, koristite termin &#x201e;Fokus grupa&#x201c;.</skos:definition>
      <skos:prefLabel xml:lang="sv">Intervju</skos:prefLabel>
      <skos:definition xml:lang="sv">Planerad kommunikation mellan tv&#xe5; (eller flera) personer &#x2013; intervjuaren/-na och intervjuobjektet/-en &#x2013; d&#xe4;r intervjuaren/-na f&#xe5;r information fr&#xe5;n intervjuobjektet/-en. Om gruppinteraktion &#xe4;r del av metoden, anv&#xe4;nd &quot;Fokusgrupp&quot;.</skos:definition>
      <skos:narrower rdf:resource="http://rdf-vocabulary.ddialliance.org/cv/ModeOfCollection/3.0.0/9f669a4"/>
      <skos:narrower rdf:resource="http://rdf-vocabulary.ddialliance.org/cv/ModeOfCollection/3.0.0/ae68e25"/>
      <skos:narrower rdf:resource="http://rdf-vocabulary.ddialliance.org/cv/ModeOfCollection/3.0.0/b0b2868"/>
      <skos:narrower rdf:resource="http://rdf-vocabulary.ddialliance.org/cv/ModeOfCollection/3.0.0/1af2bfa"/>
   </rdf:Description>
   <rdf:Description rdf:about="http://rdf-vocabulary.ddialliance.org/cv/ModeOfCollection/3.0.0/9f669a4">
      <rdf:type rdf:resource="http://www.w3.org/2004/02/skos/core#Concept"/>
      <skos:inScheme rdf:resource="http://rdf-vocabulary.ddialliance.org/cv/ModeOfCollection/3.0.0/"/>
      <skos:notation xml:lang="en">Interview.FaceToFace</skos:notation>
      <skos:prefLabel xml:lang="en">Face-to-face interview</skos:prefLabel>
      <skos:definition xml:lang="en">Data collection method in which a live interviewer conducts a personal interview, presenting questions and entering the responses. Use this broader term if not CAPI or PAPI, or if not known whether CAPI/PAPI or not.</skos:definition>
      <skos:prefLabel xml:lang="da">Personligt interview</skos:prefLabel>
      <skos:definition xml:lang="da">Dataindsamlingsmetode, hvor en tilstedev&#xe6;rende interviewer&#xa0;foretager et personligt interview, stiller sp&#xf8;rgsm&#xe5;l og noterer svar.&#xa0;Brug dette bredere begreb, hvis det ikke er CAPI eller PAPI, eller hvis det ikke vides, om det er CAPI eller PAPI.</skos:definition>
      <skos:prefLabel xml:lang="fi">Kasvokkainen haastattelu</skos:prefLabel>
      <skos:definition xml:lang="fi">Kasvokkain tehty yksil&#xf6;- tai ryhm&#xe4;haastattelu, jossa haastattelija esitt&#xe4;&#xe4; kysymykset ja taltioi vastaukset. K&#xe4;ytet&#xe4;&#xe4;n silloin, kun haastattelija tallentaa saamansa tiedot haastattelumuistiinpanoilla, tai haastattelu &#xe4;&#xe4;nitet&#xe4;&#xe4;n tai videoidaan (eli ei mene mihink&#xe4;&#xe4;n kasvokkaisen haastattelun alaluokkaan).</skos:definition>
      <skos:prefLabel xml:lang="fr">Entretien en face-&#xe0;-face</skos:prefLabel>
      <skos:definition xml:lang="fr">M&#xe9;thode de recueil de donn&#xe9;es dans laquelle un enqu&#xea;teur conduit un entretien personnel, posant des questions et &#xe9;crivant les r&#xe9;ponses. Utilisez ce terme si pas CAPI ou PAPI, ou si vous ne savez pas si CAPI/PAPI ou pas.</skos:definition>
      <skos:prefLabel xml:lang="it">Intervista faccia a faccia</skos:prefLabel>
      <skos:definition xml:lang="it">Tecnica di raccolta dei dati in cui un intervistatore conduce un colloquio personale in presenza, facendo domande e registrando le risposte. Utilizzare questo termine pi&#xf9; ampio se l&apos;intervista non &#xe8; CAPI o PAPI, o se non si &#xe8; in grado di stabilire se sia CAPI o PAPI.</skos:definition>
      <skos:prefLabel xml:lang="no">Personlig intervju</skos:prefLabel>
      <skos:definition xml:lang="no">Datainnsamlingsmetode hvor en tilstedev&#xe6;rende intervjuer gjennomf&#xf8;rer et personlig intervju, presenterer sp&#xf8;rsm&#xe5;l og registrerer svarene. Bruk dette bredere begrepet dersom det ikke er CATI eller PAPI, eller dersom det er uvisst om det er CATI/PAPI.</skos:definition>
      <skos:prefLabel xml:lang="pt">Entrevista presencial</skos:prefLabel>
      <skos:definition xml:lang="pt">M&#xe9;todo de recolha de dados em que um entrevistador presencial realiza uma entrevista pessoal, colocando as perguntas e inserindo as respostas. Usar este termo mais amplo se n&#xe3;o for CAPI ou PAPI, ou se n&#xe3;o souber se &#xe9; CAPI/PAPI.</skos:definition>
      <skos:prefLabel xml:lang="sl">Osebni intervju</skos:prefLabel>
      <skos:definition xml:lang="sl">Metoda zbiranja podatkov, kjer spra&#x161;evalec izvede osebni intervju, postavlja vpra&#x161;anja in vnese odgovore. Uporabite ta &#x161;ir&#x161;i izraz, &#x10d;e ne morete uporabiti CAPI ali PAPI ozioma ni znano, ali gre za CAPI/PAPI.</skos:definition>
      <skos:prefLabel xml:lang="sr">Intervju licem u lice</skos:prefLabel>
      <skos:definition xml:lang="sr">Na&#x10d;in prikupljanja podataka u kojem anketar u&#x17e;ivo vodi usmeni razgovor, postavljajuc&#x301;i pitanja i unosec&#x301;i odgovore. Koristite ovaj &#x161;iri pojam ukoliko nije ta&#x10d;no navedno da se radi o CAPI (Intervju licem u lice: podr&#x17e;an ra&#x10d;unarom) ili PAPI (Intervju licem u lice: bele&#x17e;i se na papiru) ili ukoliko vama nije poznato da li je u pitanju CAPI ili PAPI.</skos:definition>
      <skos:prefLabel xml:lang="sv">Personlig intervju</skos:prefLabel>
      <skos:definition xml:lang="sv">En n&#xe4;rvarande intervjuare genomf&#xf6;r en personlig intervju genom att st&#xe4;lla fr&#xe5;gor och notera svaren. Anv&#xe4;nd denna bredare term om det inte r&#xf6;r sig om CAPI eller PAPI, eller om det inte &#xe4;r k&#xe4;nt huruvida det r&#xf6;r sig om CAPI/PAPI eller inte.</skos:definition>
      <skos:narrower rdf:resource="http://rdf-vocabulary.ddialliance.org/cv/ModeOfCollection/3.0.0/89e4fb4"/>
      <skos:narrower rdf:resource="http://rdf-vocabulary.ddialliance.org/cv/ModeOfCollection/3.0.0/e477963"/>
   </rdf:Description>
   <rdf:Description rdf:about="http://rdf-vocabulary.ddialliance.org/cv/ModeOfCollection/3.0.0/89e4fb4">
      <rdf:type rdf:resource="http://www.w3.org/2004/02/skos/core#Concept"/>
      <skos:inScheme rdf:resource="http://rdf-vocabulary.ddialliance.org/cv/ModeOfCollection/3.0.0/"/>
      <skos:notation xml:lang="en">Interview.FaceToFace.CAPIorCAMI</skos:notation>
      <skos:prefLabel xml:lang="en">Face-to-face interview: Computer-assisted (CAPI/CAMI)</skos:prefLabel>
      <skos:definition xml:lang="en">Computer-assisted personal interviewing (CAPI), or computer-assisted mobile interviewing (CAMI). Data collection method in which the interviewer reads questions to the respondents from the screen of a computer, laptop, or a mobile device like tablet or smartphone, and enters the answers in the same device. The administration of the interview is managed by a specifically designed program/application.</skos:definition>
      <skos:prefLabel xml:lang="da">Personligt interview: Computerassisteret (CAPI/CAMI)</skos:prefLabel>
      <skos:definition xml:lang="da">Computer-assisted personal interviewing (CAPI) eller computer-assisted mobile interviewing (CAMI). Dataindsamlingsmetode, hvor intervieweren l&#xe6;ser sp&#xf8;rgsm&#xe5;l op til respondenterne fra sk&#xe6;rmen p&#xe5; en computer, b&#xe6;rbar eller en mobil enhed s&#xe5;som tablet eller smartphone og indtaster svarene p&#xe5; den samme enhed. Administrationen af interviewet styres af et specifikt designet program/applikation.</skos:definition>
      <skos:prefLabel xml:lang="fi">Kasvokkainen haastattelu: tietokoneavusteinen (CAPI tai CAMI)</skos:prefLabel>
      <skos:definition xml:lang="fi">Computer-assisted personal interviewing (CAPI) tai Computer-assisted mobile interviewing (CAMI). Haastattelija lukee kysymykset kannettavalta tietokoneelta, k&#xe4;mmentietokoneelta, tabletista tai &#xe4;lypuhelimesta ja tallentaa haastateltavan vastaukset suoraan laitteeseen.</skos:definition>
      <skos:prefLabel xml:lang="fr">Entretien en face-&#xe0;-face : assist&#xe9; par ordinateur (CAPI / CAMI)</skos:prefLabel>
      <skos:definition xml:lang="fr">Entretien assist&#xe9; par ordinateur (CAPI), ou entretien assist&#xe9; par un appareil mobile (CAMI). M&#xe9;thode de collecte des donn&#xe9;es dans laquelle l&apos;enqu&#xea;teur lit les questions aux r&#xe9;pondants depuis l&apos;&#xe9;cran d&apos;un ordinateur, d&apos;un ordinateur portable ou d&apos;un appareil mobile tel qu&apos;une tablette ou un smartphone, et entre les r&#xe9;ponses sur le m&#xea;me appareil. L&apos;administration de l&apos;entretien est g&#xe9;r&#xe9; par un programme / application sp&#xe9;cialement con&#xe7;ue.</skos:definition>
      <skos:prefLabel xml:lang="it">Intervista faccia a faccia: computer-assistita (CAPI/CAMI)</skos:prefLabel>
      <skos:definition xml:lang="it">Interviste personali assistite da computer (CAPI) o da cellulare (CAMI). Metodo di raccolta dei dati in cui l&apos;intervistatore legge le domande ai rispondenti dallo schermo di un computer, laptop o dispositivo mobile come un tablet o uno smartphone e inserisce le risposte nello stesso dispositivo. L&apos;intervista &#xe8; gestita da un programma/applicazione appositamente progettata.</skos:definition>
      <skos:prefLabel xml:lang="no">Personlig intervju: CAPI/CAMI</skos:prefLabel>
      <skos:definition xml:lang="no">Dataassistert personlig intervjuing (CAPI). Datainnsamlingsmetode hvor intervjueren leser opp sp&#xf8;rsm&#xe5;l for respondenten fra skjermen til en datamaskin, b&#xe6;rbar datamaskin, smarttelefon eller nettbrett, og registrerer svarene p&#xe5; det samme apparatet. Administreringen av intervjuet er styrt av et spesialdesignet program eller en applikasjon.</skos:definition>
      <skos:prefLabel xml:lang="pt">Entrevista presencial: Assistida por computador (CAPI/CAMI)</skos:prefLabel>
      <skos:definition xml:lang="pt">Entrevista pessoal assistida por computador (Computer Assisted Personal Interviewing - CAPI) ou entrevista m&#xf3;vel assistida por computador (Computer Assisted Mobile Interviewing - CAMI). Modo de recolha de dados em que o entrevistador l&#xea; perguntas aos entrevistados na tela de um computador, laptop ou dispositivo m&#xf3;vel, como tablet ou smartphone, e insere as respostas no mesmo dispositivo. A administra&#xe7;&#xe3;o da entrevista &#xe9; gerida por um programa especialmente elaborado para o efeito.</skos:definition>
      <skos:prefLabel xml:lang="sl">Osebni intervju: CAPI/CAMI</skos:prefLabel>
      <skos:definition xml:lang="sl">Ra&#x10d;unalni&#x161;ko podprto osebno intervjuvanje (CAPI). Metoda zbiranja podatkov, kjer spra&#x161;evalec prebere vpra&#x161;anja spra&#x161;evancu z zaslona na ra&#x10d;unalniku, prenosnem ra&#x10d;unalniku ali mobilni napravi, kot na primer na tablici ali pametnemu telefonu, in vnese odgovore v isto napravo. Intervju izvedemo s pomo&#x10d;jo posebej zasnovanega programa/ aplikacije.</skos:definition>
      <skos:prefLabel xml:lang="sr">Intervju licem u lice: Podr&#x17e;an ra&#x10d;unarom (CAPI/CAMI)</skos:prefLabel>
      <skos:definition xml:lang="sr">Ra&#x10d;unarsko li&#x10d;no intervjuisanje (CAPI) ili ra&#x10d;unarsko potpomognuto mobilno intervjuisanje (CAMI). Na&#x10d;in prikupljanja podataka u kojem anketar &#x10d;ita pitanja anketiranima sa ekrana ra&#x10d;unara, laptopa ili mobilnog ure&#x111;aja poput tableta ili pametnog telefona i unosi odgovore u isti ure&#x111;aj. Administriranjem intervjua upravlja se posebno dizajniranim programom / aplikacijom.</skos:definition>
      <skos:prefLabel xml:lang="sv">Personlig intervju: CAPI/CAMI</skos:prefLabel>
      <skos:definition xml:lang="sv">Datorst&#xf6;dd personlig intervju. Intervjuaren l&#xe4;ser fr&#xe5;gor f&#xf6;r respondenterna fr&#xe5;n en datorsk&#xe4;rm eller mobil enhet (t.ex. surfplatta eller mobiltelefon) och skriver in svaren direkt i datorn. Intervjun hanteras med ett program som utvecklats f&#xf6;r detta syfte.</skos:definition>
   </rdf:Description>
   <rdf:Description rdf:about="http://rdf-vocabulary.ddialliance.org/cv/ModeOfCollection/3.0.0/e477963">
      <rdf:type rdf:resource="http://www.w3.org/2004/02/skos/core#Concept"/>
      <skos:inScheme rdf:resource="http://rdf-vocabulary.ddialliance.org/cv/ModeOfCollection/3.0.0/"/>
      <skos:notation xml:lang="en">Interview.FaceToFace.PAPI</skos:notation>
      <skos:prefLabel xml:lang="en">Face-to-face interview: Paper-and-pencil (PAPI)</skos:prefLabel>
      <skos:definition xml:lang="en">Paper-and-pencil interviewing (PAPI). The interviewer uses a traditional paper questionnaire to read the questions and enter the answers.</skos:definition>
      <skos:prefLabel xml:lang="da">Personligt interview: Papir og pen (PAPI)</skos:prefLabel>
      <skos:definition xml:lang="da">Paper-and-pencil interviewing (PAPI). Intervieweren anvender et traditionelt sp&#xf8;rgeskema p&#xe5; papir til at&#xa0;opl&#xe6;se sp&#xf8;rgsm&#xe5;lene og registrere svarene.</skos:definition>
      <skos:prefLabel xml:lang="fi">Kasvokkainen haastattelu: paperikyselylomake (PAPI)</skos:prefLabel>
      <skos:definition xml:lang="fi">Paper-and-pencil interviewing (PAPI). Paperilomaketta k&#xe4;ytt&#xe4;en tehty henkil&#xf6;kohtainen haastattelu. Haastattelija lukee kysymykset paperilomakkeelta ja kirjoittaa haastateltavan vastaukset lomakkeelle.</skos:definition>
      <skos:prefLabel xml:lang="fr">Entretien en face-&#xe0;-face : papier et crayon (PAPI)</skos:prefLabel>
      <skos:definition xml:lang="fr">Entretien avec papier et crayon (PAPI). L&apos;enqu&#xea;teur utilise un questionnaire papier traditionnel pour lire les questions et &#xe9;crire les r&#xe9;ponses.</skos:definition>
      <skos:prefLabel xml:lang="it">Intervista faccia a faccia: carta e penna (PAPI)</skos:prefLabel>
      <skos:definition xml:lang="it">Interviste con carta e penna (PAPI). L&apos;intervistatore utilizza un tradizionale questionario cartaceo per leggere le domande e inserire le risposte.</skos:definition>
      <skos:prefLabel xml:lang="no">Personlig intervju: PAPI</skos:prefLabel>
      <skos:definition xml:lang="no">Penn og papir intervju. Intervjueren bruker et tradisjonelt papirsp&#xf8;rreskjema for &#xe5; lese opp sp&#xf8;rsm&#xe5;lene og til &#xe5; registrere svarene.</skos:definition>
      <skos:prefLabel xml:lang="pt">Entrevista presencial: Papel e l&#xe1;pis (PAPI)</skos:prefLabel>
      <skos:definition xml:lang="pt">Entrevista de papel e l&#xe1;pis (PAPI - Paper-and-pencil interviewing). O entrevistador usa um question&#xe1;rio tradicional em papel para ler as perguntas e inserir as respostas.</skos:definition>
      <skos:prefLabel xml:lang="sl">Osebni intervju: PAPI</skos:prefLabel>
      <skos:definition xml:lang="sl">&quot;Intervjuvanje s papirjem in svin&#x10d;nikom&quot;. Spra&#x161;evalec uporabi tradicionalni papirnati vpra&#x161;alnik, s katerega prebere vpra&#x161;anja in vnese odgovore.</skos:definition>
      <skos:prefLabel xml:lang="sr">Intervju licem u lice: bele&#x17e;i se na papiru (PAPI)</skos:prefLabel>
      <skos:definition xml:lang="sr">Intervju sa papirom i olovkom (PAPI). Anketar koristi tradicionalni papirni upitnik za &#x10d;itanje pitanja i unos odgovora.</skos:definition>
      <skos:prefLabel xml:lang="sv">Personlig intervju: PAPI</skos:prefLabel>
      <skos:definition xml:lang="sv">Papper-och-penna-intervju. Intervjuaren anv&#xe4;nder ett traditionellt fr&#xe5;geformul&#xe4;r p&#xe5; papper f&#xf6;r att l&#xe4;sa fr&#xe5;gorna och skriva ned svaren.</skos:definition>
   </rdf:Description>
   <rdf:Description rdf:about="http://rdf-vocabulary.ddialliance.org/cv/ModeOfCollection/3.0.0/ae68e25">
      <rdf:type rdf:resource="http://www.w3.org/2004/02/skos/core#Concept"/>
      <skos:inScheme rdf:resource="http://rdf-vocabulary.ddialliance.org/cv/ModeOfCollection/3.0.0/"/>
      <skos:notation xml:lang="en">Interview.Telephone</skos:notation>
      <skos:prefLabel xml:lang="en">Telephone interview</skos:prefLabel>
      <skos:definition xml:lang="en">Interview administered on the telephone. Use this broader term if not CATI, or if not known whether CATI or not.</skos:definition>
      <skos:prefLabel xml:lang="da">Telefoninterview</skos:prefLabel>
      <skos:definition xml:lang="da">Interview gennemf&#xf8;rt over telefon. Brug dette bredere begreb, hvis det ikke er CATI, eller hvis det ikke vides, om det er CATI.</skos:definition>
      <skos:prefLabel xml:lang="fi">Puhelinhaastattelu</skos:prefLabel>
      <skos:definition xml:lang="fi">Puhelimitse tehty haastattelu. Termi&#xe4; voi k&#xe4;ytt&#xe4;&#xe4; sek&#xe4; kvalitatiivisesta ett&#xe4; kvantitatiivisesta haastattelusta.</skos:definition>
      <skos:prefLabel xml:lang="fr">Entretien t&#xe9;l&#xe9;phonique</skos:prefLabel>
      <skos:definition xml:lang="fr">Entretien administr&#xe9; par t&#xe9;l&#xe9;phone. Utilisez ce terme si pas CATI, ou si vous ne savez pas si CATI ou pas.</skos:definition>
      <skos:prefLabel xml:lang="it">Intervista telefonica</skos:prefLabel>
      <skos:definition xml:lang="it">Intervista somministrata via telefono. Utilizzare questo termine pi&#xf9; generale se non &#xe8; CATI, o se non si &#xe8; in grado di stabilire se lo sia.</skos:definition>
      <skos:prefLabel xml:lang="no">Telefonintervju</skos:prefLabel>
      <skos:definition xml:lang="no">Intervju som gjennomf&#xf8;res over telefon. Bruk dette bredere begrepet dersom det ikke er CATI, eller dersom det er uvisst om det er CATI.</skos:definition>
      <skos:prefLabel xml:lang="pt">Entrevista telef&#xf3;nica</skos:prefLabel>
      <skos:definition xml:lang="pt">Entrevista realizada pelo telefone. Usar este termo mais amplo se n&#xe3;o for CATI, ou se n&#xe3;o souber se &#xe9; CATI ou n&#xe3;o.</skos:definition>
      <skos:prefLabel xml:lang="sl">Telefonski intervju</skos:prefLabel>
      <skos:definition xml:lang="sl">Intervju, izveden preko telefona. Uporabite ta &#x161;ir&#x161;i izraz, &#x10d;e ni CATI, oziroma ne veste, ali je CATI ali ne.</skos:definition>
      <skos:prefLabel xml:lang="sr">Telefonski upitnik</skos:prefLabel>
      <skos:definition xml:lang="sr">Intervju administriran telefonom. Koristite ovaj &#x161;iri pojam ukoliko nije spcifikovano da je u pitanu telefonski upitnik podr&#x17e;an ra&#x10d;unarom (CATI) ili ako vam nije poznato koji tip telefonskog upitnika je kori&#x161;&#x107;en.</skos:definition>
      <skos:prefLabel xml:lang="sv">Telefonintervju</skos:prefLabel>
      <skos:definition xml:lang="sv">Intervju som genomf&#xf6;rs &#xf6;ver telefon. Anv&#xe4;nd denna bredare term om det inte r&#xf6;r sig om CATI, eller om det inte &#xe4;r k&#xe4;nt huruvida det r&#xf6;r sig om CATI.</skos:definition>
      <skos:narrower rdf:resource="http://rdf-vocabulary.ddialliance.org/cv/ModeOfCollection/3.0.0/1498dd4"/>
   </rdf:Description>
   <rdf:Description rdf:about="http://rdf-vocabulary.ddialliance.org/cv/ModeOfCollection/3.0.0/1498dd4">
      <rdf:type rdf:resource="http://www.w3.org/2004/02/skos/core#Concept"/>
      <skos:inScheme rdf:resource="http://rdf-vocabulary.ddialliance.org/cv/ModeOfCollection/3.0.0/"/>
      <skos:notation xml:lang="en">Interview.Telephone.CATI</skos:notation>
      <skos:prefLabel xml:lang="en">Telephone interview: Computer-assisted (CATI)</skos:prefLabel>
      <skos:definition xml:lang="en">Computer-assisted telephone interviewing (CATI). The interviewer asks questions as directed by a computer, responses are keyed directly into the computer and the administration of the interview is managed by a specifically designed program.</skos:definition>
      <skos:prefLabel xml:lang="da">Telefoninterview: Computerassisteret (CATI)</skos:prefLabel>
      <skos:definition xml:lang="da">Computer-assisted telephone interviewing (CATI). Intervieweren stiller sp&#xf8;rgsm&#xe5;l ved hj&#xe6;lp af en computer, svarene indtastes direkte i computeren, og administrationen af interviewet styres af et specifikt designet program.</skos:definition>
      <skos:prefLabel xml:lang="fi">Puhelinhaastattelu: tietokoneavusteinen (CATI)</skos:prefLabel>
      <skos:definition xml:lang="fi">Computer-assisted telephone interviewing (CATI). Haastattelija lukee kysymykset tietokoneelta puhelimessa ja tallentaa haastateltavan vastaukset suoraan tietokoneelle.</skos:definition>
      <skos:prefLabel xml:lang="fr">Entretien t&#xe9;l&#xe9;phonique : assist&#xe9; par ordinateur (CATI)</skos:prefLabel>
      <skos:definition xml:lang="fr">Entretien t&#xe9;l&#xe9;phonique assist&#xe9; par ordinateur (CATI). L&apos;enqu&#xea;teur pose des questions selon les directives de l&apos;ordinateur, des r&#xe9;ponses sont saisies directement dans l&apos;ordinateur et l&apos;administration de l&apos;entretien est g&#xe9;r&#xe9; pas un programme sp&#xe9;cialement con&#xe7;u.</skos:definition>
      <skos:prefLabel xml:lang="it">Intervista telefonica: assistita da computer (CATI)</skos:prefLabel>
      <skos:definition xml:lang="it">Intervista telefonica assistita da computer (CATI). L&apos;intervistatore pone le domande indicate dal computer, le risposte sono immesse direttamente nel computer e l&apos;intervista &#xe8; gestita da un programma appositamente progettato.</skos:definition>
      <skos:prefLabel xml:lang="no">Telefonintervju: CATI</skos:prefLabel>
      <skos:definition xml:lang="no">Dataassistert telefonintervju. Intervjueren stiller sp&#xf8;rsm&#xe5;l if&#xf8;lge instrukser fra en datamaskin, registrerer svarene direkte p&#xe5; datamaskinen og administreringen av intervjuet er styrt av et spesialdesignet dataprogram.</skos:definition>
      <skos:prefLabel xml:lang="pt">Entrevista telef&#xf3;nica: Assistida por computador  (CATI)</skos:prefLabel>
      <skos:definition xml:lang="pt">Entrevista telef&#xf3;nica assistida por computador (Computer Assisted Telephone Interviewing - CATI). O entrevistador faz perguntas orientado por um computador, as respostas s&#xe3;o inseridas diretamente no computador e a realiza&#xe7;&#xe3;o da entrevista &#xe9; gerida por um programa especialmente elaborado para o efeito.</skos:definition>
      <skos:prefLabel xml:lang="sl">Telefonski intervju: CATI</skos:prefLabel>
      <skos:definition xml:lang="sl">Ra&#x10d;unalni&#x161;ko podprto telefonsko intervjuvanje. Spra&#x161;evanec postavlja vpra&#x161;anja, ki jih ponuja ra&#x10d;unalnik, odgovori se vna&#x161;ajo neposredno v ra&#x10d;unalnik in intervju upravlja posebej za to zasnovan program.</skos:definition>
      <skos:prefLabel xml:lang="sr">Telefonski intervju: Podr&#x17e;an ra&#x10d;unarom (CATI)</skos:prefLabel>
      <skos:definition xml:lang="sr">Telefonski intervju (CATI) podr&#x17e;an ra&#x10d;unarom je onaj u kome anketar postavlja pitanja u skladu sa uputstvom ra&#x10d;unara, odgovori se unose direktno u ra&#x10d;unar, a administracijom intervjua upravlja posebno dizajniran program.</skos:definition>
      <skos:prefLabel xml:lang="sv">Telefonintervju: CATI</skos:prefLabel>
      <skos:definition xml:lang="sv">Datorst&#xf6;dd telefonintervju. Intervjuaren l&#xe4;ser fr&#xe5;gor f&#xf6;r respondenterna fr&#xe5;n en datorsk&#xe4;rm och skriver in svaren direkt i datorn. Intervjun hanteras genom ett program som utvecklats f&#xf6;r detta syfte.</skos:definition>
   </rdf:Description>
   <rdf:Description rdf:about="http://rdf-vocabulary.ddialliance.org/cv/ModeOfCollection/3.0.0/b0b2868">
      <rdf:type rdf:resource="http://www.w3.org/2004/02/skos/core#Concept"/>
      <skos:inScheme rdf:resource="http://rdf-vocabulary.ddialliance.org/cv/ModeOfCollection/3.0.0/"/>
      <skos:notation xml:lang="en">Interview.Email</skos:notation>
      <skos:prefLabel xml:lang="en">E-mail interview</skos:prefLabel>
      <skos:definition xml:lang="en">Interviews conducted via e-mail, usually consisting of several e-mail messages that allow the discussion to continue beyond the first set of questions and answers, or the first e-mail exchange.</skos:definition>
      <skos:prefLabel xml:lang="da">E-mail-interview</skos:prefLabel>
      <skos:definition xml:lang="da">Interviews gennemf&#xf8;rt via e-mail, som regel best&#xe5;ende af&#xa0;flere e-mail-beskeder, der tillader diskussionen at forts&#xe6;tte&#xa0;efter det f&#xf8;rste s&#xe6;t af sp&#xf8;rgsm&#xe5;l og svar eller den f&#xf8;rste udveksling af e-mails.</skos:definition>
      <skos:prefLabel xml:lang="fi">S&#xe4;hk&#xf6;postihaastattelu</skos:prefLabel>
      <skos:definition xml:lang="fi">Haastattelu tehd&#xe4;&#xe4;n s&#xe4;hk&#xf6;postin v&#xe4;lityksell&#xe4;. Usein sis&#xe4;lt&#xe4;&#xe4; useita s&#xe4;hk&#xf6;postiviestej&#xe4;, jotka mahdollistavat keskustelun jatkumisen alussa esitettyjen kysymysten ja niihin saatujen vastausten j&#xe4;lkeen.</skos:definition>
      <skos:prefLabel xml:lang="fr">Entretien par e-mail</skos:prefLabel>
      <skos:definition xml:lang="fr">Entretiens conduits via e-mail, habituellement consistant en plusieurs courriels qui permettent la discussion qui continue au-del&#xe0; d&apos;une premi&#xe8;re s&#xe9;rie de questions et de r&#xe9;ponses, ou d&apos;un premier &#xe9;change de courriels.</skos:definition>
      <skos:prefLabel xml:lang="it">Intervista e-mail</skos:prefLabel>
      <skos:definition xml:lang="it">Interviste condotte via e-mail, di solito costituite da diversi messaggi di posta elettronica che consentono alla discussione di continuare oltre la prima serie di domande e risposte, oppure dopo il primo scambio di e-mail.</skos:definition>
      <skos:prefLabel xml:lang="no">E-post intervju</skos:prefLabel>
      <skos:definition xml:lang="no">Intervjuer gjennomf&#xf8;rt over e-post, vanligvis best&#xe5;ende av en rekke e-poster som gj&#xf8;r at diskusjonen kan fortsette utover de f&#xf8;rste settene med sp&#xf8;rsm&#xe5;l og svar, eller den f&#xf8;rste e-postutvekslingen.</skos:definition>
      <skos:prefLabel xml:lang="pt">Entrevista por email/correio eletr&#xf3;nico</skos:prefLabel>
      <skos:definition xml:lang="pt">Entrevistas realizadas via email, consistindo geralmente em v&#xe1;rias mensagens de email que permitem que a discuss&#xe3;o continue al&#xe9;m do primeiro conjunto de perguntas e respostas, ou da primeira troca de emails.</skos:definition>
      <skos:prefLabel xml:lang="sl">Intervju preko elektronske po&#x161;te</skos:prefLabel>
      <skos:definition xml:lang="sl">Intervju, izveden preko elektronske po&#x161;te. Obi&#x10d;ajno ga sestavlja ve&#x10d; elektronskih sporo&#x10d;il, ki omogo&#x10d;ajo, da se pogovor nadaljuje tudi po prvem nizu vpra&#x161;anj in odgovorov, ali po prvi izmenjavi elektronskih sporo&#x10d;il.</skos:definition>
      <skos:prefLabel xml:lang="sr">Upitnik putem elektronske po&#x161;te</skos:prefLabel>
      <skos:definition xml:lang="sr">Intervju koji se vodi putem elektronske po&#x161;te, koji se obi&#x10d;no sastoji od nekoliko poruka e-po&#x161;te koje omoguc&#x301;avaju da se diskusija nastavi izvan prvog skupa pitanja i odgovora ili prve razmene e-po&#x161;te.</skos:definition>
      <skos:prefLabel xml:lang="sv">E-postintervju</skos:prefLabel>
      <skos:definition xml:lang="sv">Intervju som genomf&#xf6;rs via e-post, vanligtvis &#xf6;ver flera meddelanden som m&#xf6;jligg&#xf6;r att diskussionen forts&#xe4;tter fr&#xe5;n den f&#xf6;rsta upps&#xe4;ttningen av fr&#xe5;gor och svar eller det f&#xf6;rsta utbytet av e-brev.</skos:definition>
   </rdf:Description>
   <rdf:Description rdf:about="http://rdf-vocabulary.ddialliance.org/cv/ModeOfCollection/3.0.0/1af2bfa">
      <rdf:type rdf:resource="http://www.w3.org/2004/02/skos/core#Concept"/>
      <skos:inScheme rdf:resource="http://rdf-vocabulary.ddialliance.org/cv/ModeOfCollection/3.0.0/"/>
      <skos:notation xml:lang="en">Interview.WebBased</skos:notation>
      <skos:prefLabel xml:lang="en">Web-based interview</skos:prefLabel>
      <skos:definition xml:lang="en">An interview conducted via the Internet. For example, interviews conducted within online forums or using web-based audio-visual technology that enables the interviewer(s) and interviewee(s) to communicate in real time.</skos:definition>
      <skos:prefLabel xml:lang="da">Webbaseret interview</skos:prefLabel>
      <skos:definition xml:lang="da">Et interview gennemf&#xf8;rt via internettet. For eksempel interviews&#xa0;gennemf&#xf8;rt p&#xe5; online fora eller ved brug af webbaseret audiovisuel teknologi, der&#xa0;g&#xf8;r det muligt for&#xa0;interviewere(n) og de(n) interviewede&#xa0;at kommunikere i realtid.</skos:definition>
      <skos:prefLabel xml:lang="fi">Verkkohaastattelu</skos:prefLabel>
      <skos:definition xml:lang="fi">Verkon v&#xe4;lityksell&#xe4; tehty haastattelu, esimerkiksi verkkokeskustelufoorumilla tai k&#xe4;ytt&#xe4;en teknologiaa, jonka avulla haastattelija ja haastateltava(t) voivat keskustella samanaikaisesti (chat, skype, videokonferenssit).</skos:definition>
      <skos:prefLabel xml:lang="fr">Entretien par Internet</skos:prefLabel>
      <skos:definition xml:lang="fr">Un entretien conduit via l&apos;Internet. Par exemple, des entretiens conduits &#xe0; l&apos;int&#xe9;rieur de forums en ligne ou en utilisant des technologies web audio-vid&#xe9;o qui permettent au(x) enqu&#xea;teur(s) et au(x) r&#xe9;pondant(s) de communiquer en temps r&#xe9;el.</skos:definition>
      <skos:prefLabel xml:lang="it">Intervista web</skos:prefLabel>
      <skos:definition xml:lang="it">Un&apos;intervista condotta via Internet. Ad esempio, interviste condotte all&apos;interno di forum online o utilizzando la tecnologia audiovisiva basata sul web che consente all&apos;intervistatore e agli intervistati di comunicare in tempo reale.</skos:definition>
      <skos:prefLabel xml:lang="no">Webbasert intervju</skos:prefLabel>
      <skos:definition xml:lang="no">Intervju gjennomf&#xf8;rt over internett. For eksempel, intervjuer gjennomf&#xf8;rt p&#xe5; internettforum eller ved bruk av internettbasert audiovisuell teknologi som muliggj&#xf8;r fortl&#xf8;pende kommunikasjon mellom intervjuer(e) og Intervjuobjekt(er).</skos:definition>
      <skos:prefLabel xml:lang="pt">Entrevista via web (online)</skos:prefLabel>
      <skos:definition xml:lang="pt">Entrevistas realizadas via Internet. Por exemplo, entrevistas conduzidas em f&#xf3;runs online ou utilizando tecnologia audiovisual baseada na web que permite ao(s) entrevistador(es) e entrevistado(s) comunicar em tempo real.</skos:definition>
      <skos:prefLabel xml:lang="sl">Spletni intervju</skos:prefLabel>
      <skos:definition xml:lang="sl">Intervju preko spleta. Na primer, intervjuji izvedeni znotraj spletnih forumov ali z uporabo spletno osnovanih avdio-vizualnih tehnologij, ki omogo&#x10d;ajo komunikacijo spra&#x161;evalca(-cev) in spra&#x161;evanca(-cev) v realnem &#x10d;asu.</skos:definition>
      <skos:prefLabel xml:lang="sr">Veb upitnik</skos:prefLabel>
      <skos:definition xml:lang="sr">Intervju koji se sprovodi putem interneta. Na primer, intervjui vo&#x111;eni na internet forumima ili kori&#x161;c&#x301;enjem internet audio-vizuelne tehnologije koja omoguc&#x301;ava anketarima i anketiranim licima da komuniciraju u realnom vremenu.</skos:definition>
      <skos:prefLabel xml:lang="sv">Webbaserad intervju</skos:prefLabel>
      <skos:definition xml:lang="sv">Intervju som genomf&#xf6;rs &#xf6;ver Internet. Exempel inkluderar intervjuer genomf&#xf6;rda p&#xe5; onlineforum eller med hj&#xe4;lp av webbaserad audiovisuell teknik som till&#xe5;ter att intervjuare och intervjuobjekt kan kommunicera i realtid.</skos:definition>
   </rdf:Description>
   <rdf:Description rdf:about="http://rdf-vocabulary.ddialliance.org/cv/ModeOfCollection/3.0.0/35e4248">
      <rdf:type rdf:resource="http://www.w3.org/2004/02/skos/core#Concept"/>
      <skos:inScheme rdf:resource="http://rdf-vocabulary.ddialliance.org/cv/ModeOfCollection/3.0.0/"/>
      <skos:notation xml:lang="en">SelfAdministeredQuestionnaire</skos:notation>
      <skos:prefLabel xml:lang="en">Self-administered questionnaire</skos:prefLabel>
      <skos:definition xml:lang="en">Data collection method in which the respondent reads or listens to the questions, and enters the responses by him/herself; no live interviewer is present, or participates in the questionnaire administration. If possible, use a narrower term. Use this broader term if the method is not described by any of the narrower terms - for example, for PDF and diskette questionnaires.</skos:definition>
      <skos:prefLabel xml:lang="da">Selvadministreret sp&#xf8;rgeskema</skos:prefLabel>
      <skos:definition xml:lang="da">Dataindsamlingsmetode, hvor respondenten l&#xe6;ser eller h&#xf8;rer sp&#xf8;rgsm&#xe5;lene og selv indtaster svarene; ingen interviewer er til stede eller deltager i administrationen af sp&#xf8;rgeskemaet. Hvis det er muligt, brug da et smallere begreb. Brug dette begreb, hvis metoden ikke er beskrevet af nogle af de smallere begreber - for eksempel til PDF- eller diskettesp&#xf8;rgeskemaer.</skos:definition>
      <skos:prefLabel xml:lang="fi">Itset&#xe4;ytett&#xe4;v&#xe4; lomake</skos:prefLabel>
      <skos:definition xml:lang="fi">Tutkimuksen osanottaja t&#xe4;ytt&#xe4;&#xe4; kysely- tai ilmoituslomakkeen itsen&#xe4;isesti. P&#xe4;&#xe4;luokkaa k&#xe4;ytet&#xe4;&#xe4;n, jos ei tiedet&#xe4; miss&#xe4; muodossa lomake on saatu ja palautettu tai jos ei puhtaasti mik&#xe4;&#xe4;n suppeampi termi.</skos:definition>
      <skos:prefLabel xml:lang="fr">Questionnaire auto-administr&#xe9;</skos:prefLabel>
      <skos:definition xml:lang="fr">M&#xe9;thode de collecte de donn&#xe9;es dans laquelle l&apos;enqu&#xea;t&#xe9; lit ou &#xe9;coute les questions et saisit les r&#xe9;ponses par lui-m&#xea;me ; aucun enqu&#xea;teur n&apos;est pr&#xe9;sent, ou participe &#xe0; l&apos;administration du questionnaire. Si possible, utilisez un terme plus pr&#xe9;cis. Utilisez ce terme si la m&#xe9;thode n&apos;est pas d&#xe9;crite par aucun des termes plus pr&#xe9;cis - par exemple, pour les questionnaires PDF ou sur disquette.</skos:definition>
      <skos:prefLabel xml:lang="it">Questionario auto-compilato</skos:prefLabel>
      <skos:definition xml:lang="it">Tecnica di raccolta dei dati in cui il rispondente legge o ascolta le domande e inserisce autonomamente le risposte; nessun intervistatore &#xe8; presente o partecipa alla somministrazione del questionario. Se possibile, utilizzare un termine pi&#xf9; specifico. Utilizzare questo termine pi&#xf9; ampio se il metodo non &#xe8; descritto da nessuno dei termini pi&#xf9; specifici, ad esempio per i questionari PDF o trasmessi via floppy disk.</skos:definition>
      <skos:prefLabel xml:lang="no">Selvadministrerende sp&#xf8;rreskjema</skos:prefLabel>
      <skos:definition xml:lang="no">Datainnsamlingsmetode hvor respondenten leser eller lytter til sp&#xf8;rsm&#xe5;lene, og registrerer svarene p&#xe5; egenh&#xe5;nd; ingen intervjuer er til stede, eller deltar i administreringen av sp&#xf8;rreskjemaet. Bruk et smalere begrep dersom det er mulig. Bruk dette bredere begrepet dersom ingen av de smalere begrepene passer.</skos:definition>
      <skos:prefLabel xml:lang="pt">Question&#xe1;rio de autopreenchimento</skos:prefLabel>
      <skos:definition xml:lang="pt">M&#xe9;todo de recolha de dados em que o respondente l&#xea; ou ouve as perguntas e ele mesmo insere as respostas; nenhum entrevistador est&#xe1; presente, ou participa da administra&#xe7;&#xe3;o do question&#xe1;rio. Se poss&#xed;vel, usar um termo mais restrito. Usar este termo mais amplo se o m&#xe9;todo n&#xe3;o for descrito por nenhum dos termos mais restritos - por exemplo, question&#xe1;rios em pdf ou em disquete.</skos:definition>
      <skos:prefLabel xml:lang="sl">Vpra&#x161;alnik za samoizpolnjevanje</skos:prefLabel>
      <skos:definition xml:lang="sl">Metoda zbiranja podatkov, pri kateri spra&#x161;evanec bere ali poslu&#x161;a vpra&#x161;anja in sam vna&#x161;a odgovore; spra&#x161;evalec ni prisoten niti ne sodeluje pri upravljanju vpra&#x161;alnika. &#x10c;e je mo&#x17e;no, uporabite o&#x17e;ji izraz. Ta &#x161;ir&#x161;i izraz uporabite le, &#x10d;e metoda ni opisana z nobenem od o&#x17e;jih izrazov, npr. za PDF ali vpra&#x161;alnike na disketi.</skos:definition>
      <skos:prefLabel xml:lang="sr">Samostalni upitnik</skos:prefLabel>
      <skos:definition xml:lang="sr">Metoda prikupljanja podataka u kojoj ispitanik &#x10d;ita ili slu&#x161;a pitanja i unosi odgovore; nema &#x17e;ivog anketara ili on ne u&#x10d;estvuje u administraciji upitnika. Ako je moguc&#x301;e, koristite u&#x17e;i termin. Upotrebite ovaj &#x161;iri pojam ako metod nije opisan nijednim u&#x17e;im terminom.</skos:definition>
      <skos:prefLabel xml:lang="sv">Sj&#xe4;lvadministrerat fr&#xe5;geformul&#xe4;r</skos:prefLabel>
      <skos:definition xml:lang="sv">Respondenten l&#xe4;ser eller lyssnar p&#xe5; fr&#xe5;gorna och noterar sj&#xe4;lv svaren; ingen intervjuare &#xe4;r n&#xe4;rvarande eller deltar i administrerandet av fr&#xe5;geformul&#xe4;ret. Anv&#xe4;nd om m&#xf6;jligt en smalare term. Anv&#xe4;nd denna bredare term om metoden inte beskrivits av n&#xe5;gon av de mer precisa termerna.</skos:definition>
      <skos:narrower rdf:resource="http://rdf-vocabulary.ddialliance.org/cv/ModeOfCollection/3.0.0/69a46ca"/>
      <skos:narrower rdf:resource="http://rdf-vocabulary.ddialliance.org/cv/ModeOfCollection/3.0.0/6255fce"/>
      <skos:narrower rdf:resource="http://rdf-vocabulary.ddialliance.org/cv/ModeOfCollection/3.0.0/ddaefe8"/>
      <skos:narrower rdf:resource="http://rdf-vocabulary.ddialliance.org/cv/ModeOfCollection/3.0.0/557586d"/>
      <skos:narrower rdf:resource="http://rdf-vocabulary.ddialliance.org/cv/ModeOfCollection/3.0.0/e48ace5"/>
   </rdf:Description>
   <rdf:Description rdf:about="http://rdf-vocabulary.ddialliance.org/cv/ModeOfCollection/3.0.0/69a46ca">
      <rdf:type rdf:resource="http://www.w3.org/2004/02/skos/core#Concept"/>
      <skos:inScheme rdf:resource="http://rdf-vocabulary.ddialliance.org/cv/ModeOfCollection/3.0.0/"/>
      <skos:notation xml:lang="en">SelfAdministeredQuestionnaire.Email</skos:notation>
      <skos:prefLabel xml:lang="en">Self-administered questionnaire: E-mail</skos:prefLabel>
      <skos:definition xml:lang="en">Self-administered survey in which questions are presented to the respondent in the text body of an e-mail or as an attachment to an e-mail, but not as a link to a web-based questionnaire. Responses are also sent back via e-mail, in the e-mail body or as an attachment.</skos:definition>
      <skos:prefLabel xml:lang="da">Selvadministreret sp&#xf8;rgeskema: E-mail</skos:prefLabel>
      <skos:definition xml:lang="da">Selvadministreret&#xa0;sp&#xf8;rgeskema, hvor sp&#xf8;rgsm&#xe5;lene stilles til respondenten i en e-mails tekstfelt eller som en vedh&#xe6;ftning i en e-mail, men ikke som et link til et webbaseret sp&#xf8;rgeskema. Svarene er ogs&#xe5; sendt tilbage via e-mail, enten som tekst eller som vedh&#xe6;ftet fil.</skos:definition>
      <skos:prefLabel xml:lang="fi">Itset&#xe4;ytett&#xe4;v&#xe4; lomake: s&#xe4;hk&#xf6;postilomake</skos:prefLabel>
      <skos:definition xml:lang="fi">Osanottaja t&#xe4;ytt&#xe4;&#xe4; s&#xe4;hk&#xf6;postin tekstiosiossa tai s&#xe4;hk&#xf6;postin liitetiedostona tulleen kyselylomakkeen ja palauttaa sen s&#xe4;hk&#xf6;postilla. Jos s&#xe4;hk&#xf6;postissa on vain linkki verkkokyselylomakkeeseen, k&#xe4;yt&#xe4; termi&#xe4; &apos;Itset&#xe4;ytett&#xe4;v&#xe4; lomake: verkkolomake&apos;.</skos:definition>
      <skos:prefLabel xml:lang="fr">Questionnaire auto-administr&#xe9; : e-mail</skos:prefLabel>
      <skos:definition xml:lang="fr">Enqu&#xea;te auto-administr&#xe9;e dans laquelle les questions sont pr&#xe9;sent&#xe9;es au r&#xe9;pondant dans le corps d&apos;un e-mail ou dans une pi&#xe8;ce jointe, mais pas comme un lien vers une enqu&#xea;te par Internet. Les r&#xe9;ponses sont alors renvoy&#xe9;es via e-mail, dans le corps du message ou comme une pi&#xe8;ce jointe.</skos:definition>
      <skos:prefLabel xml:lang="it">Questionario auto-compilato: e-mail</skos:prefLabel>
      <skos:definition xml:lang="it">Questionario auto-compilato in cui le domande vengono presentate all&apos;intervistato nel corpo del testo di un&apos;e-mail o come allegato a un&apos;e-mail, ma non come un collegamento a un questionario somministrato via web. Anche le risposte vengono rispedite via e-mail, nel corpo dell&apos;e-mail o come allegato.</skos:definition>
      <skos:prefLabel xml:lang="no">Selvadministrerende sp&#xf8;rreskjema: E-post</skos:prefLabel>
      <skos:definition xml:lang="no">Unders&#xf8;kelse hvor sp&#xf8;rsm&#xe5;l blir presentert til respondenten som tekst i en e-post eller som et vedlegg i en e-post, men ikke som lenke til et web-basert sp&#xf8;rreskjema. Svarene sendes ogs&#xe5; tilbake med e-post, enten som tekst i e-posten eller som et vedlegg.</skos:definition>
      <skos:prefLabel xml:lang="pt">Question&#xe1;rio de autopreenchimento: Email/correio eletr&#xf3;nico</skos:prefLabel>
      <skos:definition xml:lang="pt">Question&#xe1;rio de autopreenchimento em que as perguntas s&#xe3;o apresentadas ao respondente no corpo do texto de um email ou num anexo de um email, mas n&#xe3;o como um link para um question&#xe1;rio baseado na web. As respostas s&#xe3;o tamb&#xe9;m devolvidas via email, no corpo do email ou como anexo.</skos:definition>
      <skos:prefLabel xml:lang="sl">Vpra&#x161;alnik za samoizpolnjevanje: elektronska po&#x161;ta</skos:prefLabel>
      <skos:definition xml:lang="sl">Vpra&#x161;alnik za samoizpolnjevanje, kjer so spra&#x161;evancu vpra&#x161;anja prikazana bodisi kot besedilo v telesu elektronskega sporo&#x10d;ila bodisi v priponki, vendar ne kot povezava do spletnega vpra&#x161;alnika. Prav tako so tudi odgovori poslani preko elektronskega sporo&#x10d;ila, bodisi v telesu elektronskega sporo&#x10d;ila, bodisi kot priponka.</skos:definition>
      <skos:prefLabel xml:lang="sr">Samostalno anketiranje: Elektronskom po&#x161;tom</skos:prefLabel>
      <skos:definition xml:lang="sr">Samostalno anketiranje u kome se ispitanicima postavljaju pitanja u tekstu e-po&#x161;te ili kao prilog e-po&#x161;ti, ali ne kao hiperlink do veb-upitnika. Odgovori se tako&#x111;e &#x161;alju nazad e-po&#x161;tom, u poruci e-po&#x161;te ili kao prilog.</skos:definition>
      <skos:prefLabel xml:lang="sv">Sj&#xe4;lvadministrerat fr&#xe5;geformul&#xe4;r: e-post</skos:prefLabel>
      <skos:definition xml:lang="sv">Fr&#xe5;gor skickas till respondenten i br&#xf6;dtexten p&#xe5;, eller som en bilaga till, ett e-brev, inte som en l&#xe4;nk till ett fr&#xe5;geformul&#xe4;r p&#xe5; webben. Svaren skickas tillbaka med e-post, i br&#xf6;dtexten eller som bilaga.</skos:definition>
   </rdf:Description>
   <rdf:Description rdf:about="http://rdf-vocabulary.ddialliance.org/cv/ModeOfCollection/3.0.0/6255fce">
      <rdf:type rdf:resource="http://www.w3.org/2004/02/skos/core#Concept"/>
      <skos:inScheme rdf:resource="http://rdf-vocabulary.ddialliance.org/cv/ModeOfCollection/3.0.0/"/>
      <skos:notation xml:lang="en">SelfAdministeredQuestionnaire.Paper</skos:notation>
      <skos:prefLabel xml:lang="en">Self-administered questionnaire: Paper</skos:prefLabel>
      <skos:definition xml:lang="en">Self-administered survey using a traditional paper questionnaire delivered and/or collected by mail (postal services), by fax, or in person by either interviewer, or respondent.</skos:definition>
      <skos:prefLabel xml:lang="da">Selvadministreret sp&#xf8;rgeskema: Papir</skos:prefLabel>
      <skos:definition xml:lang="da">Selvadministreret&#xa0;sp&#xf8;rgeskema ved brug af et traditionelt sp&#xf8;rgeskema p&#xe5; papir leveret og/eller indsamlet som post (posttjenester), p&#xe5; fax eller personligt enten af intervieweren eller respondenten.</skos:definition>
      <skos:prefLabel xml:lang="fi">Itset&#xe4;ytett&#xe4;v&#xe4; lomake: paperinen lomake</skos:prefLabel>
      <skos:definition xml:lang="fi">Osanottaja t&#xe4;ytt&#xe4;&#xe4; perinteisen paperisen kyselylomakkeen itse. Paperilomake voidaan l&#xe4;hett&#xe4;&#xe4; tai palauttaa postissa, tai annetaan henkil&#xf6;kohtaisesti.</skos:definition>
      <skos:prefLabel xml:lang="fr">Questionnaire auto-administr&#xe9; : papier</skos:prefLabel>
      <skos:definition xml:lang="fr">Enqu&#xea;te auto-administr&#xe9;e utilisant un traditionnel questionnaire papier distribu&#xe9; et / ou recueilli par courrier (services postaux), par fax, ou en personne par soit par un enqu&#xea;teur ou par un r&#xe9;pondant.</skos:definition>
      <skos:prefLabel xml:lang="it">Questionario auto-compilato: cartaceo</skos:prefLabel>
      <skos:definition xml:lang="it">Questionario cartaceo tradizionale auto-compilato, consegnato e/o ritirato per posta (servizi postali), via fax o di persona dall&apos;intervistatore oppure dall&apos;intervistato.</skos:definition>
      <skos:prefLabel xml:lang="no">Selvadministrerende sp&#xf8;rreskjema: Papir</skos:prefLabel>
      <skos:definition xml:lang="no">Selvadministrert sp&#xf8;rreskjema som bruker tradisjonelle sp&#xf8;rsm&#xe5;lsformuleringer p&#xe5; papir, som blir levert og/eller samlet inn via post, faks, eller personlig av intervjueren eller respondenten.</skos:definition>
      <skos:prefLabel xml:lang="pt">Question&#xe1;rio de autopreenchimento: Papel</skos:prefLabel>
      <skos:definition xml:lang="pt">Question&#xe1;rio de autopreenchimento utilizando um question&#xe1;rio tradicional em papel entregue e/ou recolhido por correio (servi&#xe7;os postais), por fax ou pessoalmente, seja pelo entrevistador ou pelo respondente.</skos:definition>
      <skos:prefLabel xml:lang="sl">Vpra&#x161;alnik za samoizpolnjevanje: papirnati</skos:prefLabel>
      <skos:definition xml:lang="sl">Vpra&#x161;alnik za samoizpolnjevanje z uporabo tradicionalnega papirnatega vpra&#x161;alnika poslanega in/ali prejetega preko tradicionalne po&#x161;tne storitve, preko faksa ali osebno preko spra&#x161;evalca ali spra&#x161;evanca.</skos:definition>
      <skos:prefLabel xml:lang="sr">Samostalno anketiranje: Papirno</skos:prefLabel>
      <skos:definition xml:lang="sr">Anketa koja se sprovodi samostalno, koristec&#x301;i tradicionalni papirnati upitnik dostavljen i / ili prikupljen po&#x161;tom (po&#x161;tanske usluge), faksom ili li&#x10d;no od strane anketara ili ispitanika.</skos:definition>
      <skos:prefLabel xml:lang="sv">Sj&#xe4;lvadministrerat fr&#xe5;geformul&#xe4;r: papper</skos:prefLabel>
      <skos:definition xml:lang="sv">Sj&#xe4;lvadministrerad surveyunders&#xf6;kning som anv&#xe4;nder traditionella fr&#xe5;geformul&#xe4;r p&#xe5; papper, vilka skickas ut och/eller in via post eller fax, eller l&#xe4;mnas &#xf6;ver personligen av antingen intervjuaren eller intervjuobjektet.</skos:definition>
   </rdf:Description>
   <rdf:Description rdf:about="http://rdf-vocabulary.ddialliance.org/cv/ModeOfCollection/3.0.0/ddaefe8">
      <rdf:type rdf:resource="http://www.w3.org/2004/02/skos/core#Concept"/>
      <skos:inScheme rdf:resource="http://rdf-vocabulary.ddialliance.org/cv/ModeOfCollection/3.0.0/"/>
      <skos:notation xml:lang="en">SelfAdministeredQuestionnaire.SMSorMMS</skos:notation>
      <skos:prefLabel xml:lang="en">Self-administered questionnaire: Messaging (SMS/MMS)</skos:prefLabel>
      <skos:definition xml:lang="en">Self-administered survey in which the respondents receive the questions incorporated in SMS (text messages) or MMS (messages including multimedia content) and send their replies in the same format.</skos:definition>
      <skos:prefLabel xml:lang="da">Selvadministreret sp&#xf8;rgeskema: Beskeder (SMS/MMS)</skos:prefLabel>
      <skos:definition xml:lang="da">Selvadministreret sp&#xf8;rgeskema, hvor respondenterne modtager sp&#xf8;rgsm&#xe5;lene p&#xe5; SMS (tekstbeskeder) eller MMS (beskeder indeholdende multimedieindhold) og sender deres svar i samme format.</skos:definition>
      <skos:prefLabel xml:lang="fi">Itset&#xe4;ytett&#xe4;v&#xe4; lomake: tekstiviesti- tai mobiililaitelomake (SMS tai MMS)</skos:prefLabel>
      <skos:definition xml:lang="fi">Osanottaja t&#xe4;ytt&#xe4;&#xe4; tekstiviestin&#xe4; tai mobiililaitekyselyn&#xe4; v&#xe4;litetyn kyselylomakkeen itse ja palauttaa sen samalla teknologialla.</skos:definition>
      <skos:prefLabel xml:lang="fr">Questionnaire auto-administr&#xe9; : par messagerie (SMS / MMS)</skos:prefLabel>
      <skos:definition xml:lang="fr">Enqu&#xea;te auto-administr&#xe9;e dans laquelle les r&#xe9;pondants re&#xe7;oivent les questions par SMS (messages texte) ou MMS (messages incluant des contenus multim&#xe9;dia) et envoient leurs r&#xe9;ponses dans le m&#xea;me format.</skos:definition>
      <skos:prefLabel xml:lang="it">Questionario auto-compilato: messaggistica (SMS/MMS)</skos:prefLabel>
      <skos:definition xml:lang="it">Questionario auto-compilato in cui gli intervistati ricevono le domande all&apos;interno di in SMS (messaggi di testo) o MMS (messaggi che includono contenuti multimediali) e inviano le loro risposte nello stesso formato.</skos:definition>
      <skos:prefLabel xml:lang="no">Selvadministrerende sp&#xf8;rreskjema: SMS/MMS</skos:prefLabel>
      <skos:definition xml:lang="no">Selvadministrert sp&#xf8;rreskjema hvor respondenten mottar sp&#xf8;rsm&#xe5;l p&#xe5; SMS (tekstmeldinger) eller MMS (meldinger med multimedia innhold) og sender svarene i samme format.</skos:definition>
      <skos:prefLabel xml:lang="pt">Question&#xe1;rio de autopreenchimento: Mensagem (SMS/MMS)</skos:prefLabel>
      <skos:definition xml:lang="pt">Question&#xe1;rio de autopreenchimento em que os respondentes recebem as perguntas incorporadas em SMS (mensagens de texto) ou MMS (mensagens que incluem conte&#xfa;do multim&#xe9;dia) e enviam as suas respostas no mesmo formato.</skos:definition>
      <skos:prefLabel xml:lang="sl">Vpra&#x161;alnik za samoizpolnjevanje: SMS/MMS</skos:prefLabel>
      <skos:definition xml:lang="sl">Vpra&#x161;alnik za samoizpolnjevanje, kjer spra&#x161;evanec prejme vpra&#x161;anja, vklju&#x10d;ena v kratkih sporo&#x10d;ilih v formatu SMS (tekstovna sporo&#x10d;ila) ali MMS (multimedijska sporo&#x10d;ila) in odgovore po&#x161;lje v enakem formatu.</skos:definition>
      <skos:prefLabel xml:lang="sr">Samostalno anketiranje: Porukama (SMS/MMS)</skos:prefLabel>
      <skos:definition xml:lang="sr">Anketa koja se sprovodi samostalno, a u kojoj ispitanici dobijaju pitanja putem SMS (tekstualne poruke) ili MMS (poruke koje uklju&#x10d;ujui multimedijalni sadr&#x17e;aj) i &#x161;alju svoje odgovore u istom formatu.</skos:definition>
      <skos:prefLabel xml:lang="sv">Sj&#xe4;lvadministrerat fr&#xe5;geformul&#xe4;r: SMS/MMS</skos:prefLabel>
      <skos:definition xml:lang="sv">Sj&#xe4;lvadministrerad surveyunders&#xf6;kning d&#xe4;r fr&#xe5;gor och svar inkluderas i SMS (textmeddelanden) eller MMS (meddelanden med multimedia-inneh&#xe5;ll) som skickas mellan mobiltelefoner.</skos:definition>
   </rdf:Description>
   <rdf:Description rdf:about="http://rdf-vocabulary.ddialliance.org/cv/ModeOfCollection/3.0.0/557586d">
      <rdf:type rdf:resource="http://www.w3.org/2004/02/skos/core#Concept"/>
      <skos:inScheme rdf:resource="http://rdf-vocabulary.ddialliance.org/cv/ModeOfCollection/3.0.0/"/>
      <skos:notation xml:lang="en">SelfAdministeredQuestionnaire.CAWI</skos:notation>
      <skos:prefLabel xml:lang="en">Self-administered questionnaire: Web-based (CAWI)</skos:prefLabel>
      <skos:definition xml:lang="en">Computer-assisted web interviewing (CAWI). Data are collected using a web questionnaire, produced with a program for creating web surveys. The program can customize the flow of the questionnaire based on the answers provided, and can allow for the questionnaire to contain pictures, audio and video clips, links to different web pages etc.</skos:definition>
      <skos:prefLabel xml:lang="da">Selvadministreret sp&#xf8;rgeskema: Webbaseret (CAWI)</skos:prefLabel>
      <skos:definition xml:lang="da">Computer-assisted web interviewing (CAWI). Data indsamles ved brug af et websp&#xf8;rgeskema, der er&#xa0;produceret af et program til at skabe webunders&#xf8;gelser. Programmet kan tilpasse sp&#xf8;rgeskemaets flow ud fra de givne svar og giver sp&#xf8;rgeskemaet mulighed for at indeholde billeder, lyd og videoklip, links til forskellige hjemmesider mm.</skos:definition>
      <skos:prefLabel xml:lang="fi">Itset&#xe4;ytett&#xe4;v&#xe4; lomake: verkkolomake</skos:prefLabel>
      <skos:definition xml:lang="fi">Osanottaja t&#xe4;ytt&#xe4;&#xe4; kysely- tai ilmoituslomakkeen verkossa itse (Computer-assisted web interviewing, CAWI). Lomake voi olla dynaaminen tai muuttumaton. Dynaamisessa lomakkeessa kysymysten j&#xe4;rjestys sek&#xe4; esitetyt kysymykset riippuvat edelt&#xe4;viin kysymyksiin annetuista vastauksista. Lomake voi my&#xf6;s sis&#xe4;lt&#xe4;&#xe4; kuvia, video- tai &#xe4;&#xe4;nitiedostoja, linkkej&#xe4; toisiin verkkosivuihin jne.</skos:definition>
      <skos:prefLabel xml:lang="fr">Questionnaire auto-administr&#xe9; : par Internet (CAWI)</skos:prefLabel>
      <skos:definition xml:lang="fr">Entretien par Internet assist&#xe9; par ordinateur (CAWI). Des donn&#xe9;es sont collect&#xe9;es en utilisant un questionnaire en ligne, produit avec un programme de cr&#xe9;ation d&apos;enqu&#xea;te en ligne. Le programme peut personnaliser le d&#xe9;roulement du questionnaire en fonction des r&#xe9;ponses fournies, et peut permettre au questionnaire de contenir des images, des clips audio et vid&#xe9;o, des liens vers diff&#xe9;rentes pages Web, etc.</skos:definition>
      <skos:prefLabel xml:lang="it">Questionario auto-compilato: web (CAWI)</skos:prefLabel>
      <skos:definition xml:lang="it">Intervista web assistita da computer (CAWI). I dati vengono raccolti utilizzando un questionario via web, prodotto con un programma per la creazione di indagini via web. Il programma pu&#xf2; personalizzare la struttura del questionario in base alle risposte fornite, e pu&#xf2; consentire al questionario di contenere immagini, clip audio e video, collegamenti a pagine web diverse, ecc.</skos:definition>
      <skos:prefLabel xml:lang="no">Selvadministrerende sp&#xf8;rreskjema: Webbasert</skos:prefLabel>
      <skos:definition xml:lang="no">Datamaskinaassistert webintervju (CAWI). Data samles ved hjelp av sp&#xf8;rreskjema p&#xe5; nett, som er produsert av et program for internettunders&#xf8;kelser. Programmet kan endre flyten av sp&#xf8;rsm&#xe5;l basert p&#xe5; svarene som blir gitt, og det muliggj&#xf8;r inkludering av bilde, lyd og video, lenker til andre nettsider etc.</skos:definition>
      <skos:prefLabel xml:lang="pt">Question&#xe1;rio de autopreenchimento: via web (CAWI)</skos:prefLabel>
      <skos:definition xml:lang="pt">Entrevista via web, assistida por computador (Computer Assisted Web Interviewing - CAWI). Os dados s&#xe3;o recolhidos atrav&#xe9;s de um question&#xe1;rio na web, produzido com um programa para criar inqu&#xe9;ritos na web. O programa pode personalizar o fluxo do question&#xe1;rio de acordo com as respostas e permite que este contenha imagens, clipes de &#xe1;udio e v&#xed;deo, links para diferentes p&#xe1;ginas da web, etc.</skos:definition>
      <skos:prefLabel xml:lang="sl">Vpra&#x161;alnik za samoizpolnjevanje: spletni</skos:prefLabel>
      <skos:definition xml:lang="sl">Ra&#x10d;unalni&#x161;ko podprto spletno intervjuvanje. Podatki so zbrani z uporabo spletnega vpra&#x161;alnika, ustvarjenega v programskem orodju za spletno anketiranje. Program lahko tok vpra&#x161;alnika prilagodi odgovorom na prej&#x161;nja vpra&#x161;anja, omogo&#x10d;a lahko vstavljanje slik ter avdio in video posnetkov, povezave do spletnih strani itd.</skos:definition>
      <skos:prefLabel xml:lang="sr">Samostalno anketiranje: Veb anketa (CAWI)</skos:prefLabel>
      <skos:definition xml:lang="sr">Podaci se prikupljaju putem veb upitnika, sa&#x10d;injenog uz pomo&#x107; program za kreiranje veb ili onlajn anketa. Program mo&#x17e;e prilagoditi tok upitnika na osnovu ponu&#x111;enih odgovora, a mo&#x17e;e omoguc&#x301;iti da upitnik sadr&#x17e;i slike, audio i video snimke, veze do razli&#x10d;itih veb stranica, i sl.</skos:definition>
      <skos:prefLabel xml:lang="sv">Sj&#xe4;lvadministrerat fr&#xe5;geformul&#xe4;r: webbaserat</skos:prefLabel>
      <skos:definition xml:lang="sv">Computer-assisted web interviewing (CAWI). Data samlas in med ett webbformul&#xe4;r som producerats av ett program som skapar webbsurveyer. Programmet kan anpassa fl&#xf6;det i fr&#xe5;geformul&#xe4;ret utifr&#xe5;n svaren som ges och det g&#xe5;r att inkludera bilder, ljud- och videoklipp, l&#xe4;nkar till andra webbsidor m.m. (Anpassad fr&#xe5;n Wikipedia.)</skos:definition>
   </rdf:Description>
   <rdf:Description rdf:about="http://rdf-vocabulary.ddialliance.org/cv/ModeOfCollection/3.0.0/e48ace5">
      <rdf:type rdf:resource="http://www.w3.org/2004/02/skos/core#Concept"/>
      <skos:inScheme rdf:resource="http://rdf-vocabulary.ddialliance.org/cv/ModeOfCollection/3.0.0/"/>
      <skos:notation xml:lang="en">SelfAdministeredQuestionnaire.CASI</skos:notation>
      <skos:prefLabel xml:lang="en">Self-administered questionnaire: Computer-assisted (CASI)</skos:prefLabel>
      <skos:definition xml:lang="en">Computer-assisted self-interview (CASI). Respondents enter the responses into a computer (desktop, laptop, Palm/PDA, tablet, etc.) by themselves. The administration of the questionnaire is managed by a specifically designed program/application but there is no real-time data transfer as in CAWI, the answers are stored on the device used for the interview. The questionnaire may be fixed form or interactive. Includes VCASI (Video computer-assisted self-interviewing), ACASI (Audio computer-assisted self-interviewing) and TACASI (Telephone audio computer-assisted self-interviewing).</skos:definition>
      <skos:prefLabel xml:lang="da">Selvadministreret sp&#xf8;rgeskema: Computerassisteret (CASI)</skos:prefLabel>
      <skos:definition xml:lang="da">Computer-assisted self-interview (CASI). Respondenter indtaster selv svarene p&#xe5; en computer (skrivebord, b&#xe6;rbar, Palm/PDA, tablet etc.) af dem selv. Administrationen af sp&#xf8;rgeskemaet styres af et specifikt designet program/applikation, men der er ingen real-time dataoverf&#xf8;rsel som i CAWI, svarene lagres p&#xe5; enheden, der anvendes til interviewet. Sp&#xf8;rgeskemaet kan v&#xe6;re i fast form eller interaktiv. Inkluderer VCASI (Video computer-assisted self-interviewing), ACASI (Audio computer-assisted self-interviewing) og TACASI (Telephone audio computer-assisted self-interviewing).</skos:definition>
      <skos:prefLabel xml:lang="fi">Itset&#xe4;ytett&#xe4;v&#xe4; lomake: tietokoneavusteinen (CASI)</skos:prefLabel>
      <skos:definition xml:lang="fi">Tietokoneavusteinen itset&#xe4;ytett&#xe4;v&#xe4; kyselylomake, jossa vastaaja tallentaa itse vastauksensa tietokoneelle (p&#xf6;yt&#xe4;kone, kannettava tietokone tai k&#xe4;mmentietokone). Tiedot eiv&#xe4;t siirry verkon kautta vaan taltioituvat vain tietokoneelle. Lomake voi olla dynaaminen tai muuttumaton. Termi sis&#xe4;lt&#xe4;&#xe4; my&#xf6;s harvoin k&#xe4;ytetyt VCASI:n (Video computer-assisted self-interviewing), ACASI:n (Audio computer-assisted self-interviewing) ja TACASI:n (Telephone audio computer-assisted self-interviewing).</skos:definition>
      <skos:prefLabel xml:lang="fr">Questionnaire auto-administr&#xe9; : assist&#xe9; par ordinateur (CASI)</skos:prefLabel>
      <skos:definition xml:lang="fr">Entretien auto-administr&#xe9; assist&#xe9; par ordinateur (CASI). Des r&#xe9;pondants entrent les r&#xe9;ponses dans un ordinateur (ordinateur de bureau, ordinateur portable, Palm / assistant personnel, tablette, etc.) par eux-m&#xea;mes. L&apos;administration du questionnaire est g&#xe9;r&#xe9;e par un programme / une application sp&#xe9;cialement con&#xe7;u mais il n&apos;y a pas de transfert de donn&#xe9;es en temps r&#xe9;el comme dans un CAWI, les r&#xe9;ponses sont stock&#xe9;es sur l&apos;appareil utilis&#xe9; pour l&apos;entretien. Le questionnaire peut &#xea;tre fig&#xe9; ou interactif. Sont inclus les VCASI (entretien vid&#xe9;o auto-administr&#xe9; assist&#xe9; par ordinateur), les ACASI (entretien audio auto-administr&#xe9; assist&#xe9; par ordinateur) et les TACASI (entretien auto-administr&#xe9; par t&#xe9;l&#xe9;phone assist&#xe9; par ordinateur).</skos:definition>
      <skos:prefLabel xml:lang="it">Questionario auto-compilato: computer-assistito (CASI)</skos:prefLabel>
      <skos:definition xml:lang="it">Auto-compilazione del questionario assistita da computer (CASI). Gli intervistati inseriscono autonomamente le risposte in un computer (desktop, laptop, palmare, tablet, ecc.). La somministrazione del questionario &#xe8; gestita da un programma/applicazione appositamente progettato, ma non esiste un trasferimento dati in tempo reale come nel CAWI poich&#xe9; le risposte vengono memorizzate sul dispositivo utilizzato per l&apos;intervista. Il questionario pu&#xf2; essere fisso o interattivo. I tipi di questionario possono essere: VCASI (video assistito), ACASI (audio assistito) e TACASI (assistito via telefono).</skos:definition>
      <skos:prefLabel xml:lang="no">Selvadministrerende sp&#xf8;rreskjema: Datamaskinassistert (CASI)</skos:prefLabel>
      <skos:definition xml:lang="no">Datamaskinassistert selvadministrert intervju (CASI). Respondentene registrerer svarene p&#xe5; en datamaskin, b&#xe6;rbar datamaskin, digital personlig assistent, nettbrett etc.) p&#xe5; egenh&#xe5;nd. Administreringen av sp&#xf8;rreskjemaet er styrt av et spesialdesignet program eller en applikasjon men det er ingen fortl&#xf8;pende datautveksling slik som i CAWI, svarene blir lagret p&#xe5; apparatet som brukes for &#xe5; gjennomf&#xf8;re intervjuet. Sp&#xf8;rreskjemaet kan enten v&#xe6;re fastsatt eller interaktivt.Omfatter VCASI (video computer-assisted self-interview), ACASI (audio computer-assisted self-interview) og TCASI (telephone audio computer-assisted self-interview).</skos:definition>
      <skos:prefLabel xml:lang="pt">Question&#xe1;rio de autopreenchimento: Assistido por computador (CASI)</skos:prefLabel>
      <skos:definition xml:lang="pt">Entrevista de autopreenchimento assistida por computador (Computer-assisted self-interview - CASI). Os entrevistados inserem as respostas num computador (desktop, laptop, PDA, tablet, etc.) por eles pr&#xf3;prios. A administra&#xe7;&#xe3;o do question&#xe1;rio &#xe9; gerida por um programa/aplica&#xe7;&#xe3;o especialmente elaborado para o efeito, mas n&#xe3;o h&#xe1; transfer&#xea;ncia de dados em tempo real, como no CAWI, e as respostas s&#xe3;o armazenadas no dispositivo usado para a entrevista. O question&#xe1;rio pode ter um formato fixo ou interativo. Inclui a entrevista auto-administrada de v&#xed;deo assistida por computador (VCASI - Video computer-assisted self-interviewing), a entrevista auto-administrada de &#xe1;udio assistida por computador (ACASI - Audio computer-assisted self-interviewing) e a entrevista de &#xe1;udio e telefone assistida por computador (TACASI - Telephone audio computer-assisted self-interviewing).</skos:definition>
      <skos:prefLabel xml:lang="sl">Vpra&#x161;alnik za samoizpolnjevanje: ra&#x10d;unalni&#x161;ko podprti (CASI)</skos:prefLabel>
      <skos:definition xml:lang="sl">Ra&#x10d;unalni&#x161;ko podprto samoizpolnjevanje (CASI). Spra&#x161;evanec sam vstavlja odgovore v ra&#x10d;unalnik (namizni, prenosni, dlan&#x10d;ni/PDA, tabli&#x10d;ni itd.). Z vpra&#x161;alnikom upravlja posebej zasnovani program/aplikacija, vendar pri tem ni prenosa v realnem &#x10d;asu kot pri CAWI, vpra&#x161;anja se shranjujejo na napravi, ki se uporablja za intervju. Vpra&#x161;alnik je lahko v fiksni obliki ali interaktiven. Vklju&#x10d;uje tudi VCASI (video ra&#x10d;unalni&#x161;ko podprto samoizpolnjevanje), ACASI (avdio ra&#x10d;unalni&#x161;ko podprto samoizpolnjevanje) in TACASI (telefonsko avdio ra&#x10d;unalni&#x161;ko podprto samoizpolnjevanje).</skos:definition>
      <skos:prefLabel xml:lang="sr">Samostalno anketiranje: Podr&#x17e;ano ra&#x10d;unarom (CASI)</skos:prefLabel>
      <skos:definition xml:lang="sr">Ispitanici samostalno unose odgovore u ra&#x10d;unar (desktop, laptop, Palm / PDA, tablet itd.). Administriranje upitnika obavlja posebno dizajniran program / aplikacija, ali ne postoji prijenos podataka u realnom vremenu (kao u CAWI), ve&#x107; se odgovori &#x10d;uvaju na ure&#x111;aju koji se koristi za intervju. Upitnik mo&#x17e;e biti fiksnog oblika ili interaktivan. Uklju&#x10d;uje VCASI (video-ra&#x10d;unarski podr&#x17e;ano samostalno anketiranje), ACASI (audio-ra&#x10d;unarski podr&#x17e;ano samostalno anketiranje) i TACASI (telefonsko audio-ra&#x10d;unarski podr&#x17e;ano samostalno anketiranje).</skos:definition>
      <skos:prefLabel xml:lang="sv">Sj&#xe4;lvadministrerat fr&#xe5;geformul&#xe4;r: med datorst&#xf6;d (CASI)</skos:prefLabel>
      <skos:definition xml:lang="sv">Computer-assisted self-interview (CASI). Respondenterna noterar sj&#xe4;lva sina svar i en dator (station&#xe4;r eller b&#xe4;rbar, Palm/PDA, surfplatta e. dyl.). Fr&#xe5;geformul&#xe4;ret administreras med ett datorprogram som utvecklats f&#xf6;r detta syfte men data &#xf6;verf&#xf6;rs inte i realtid som i fallet med CAWI: svaren lagras p&#xe5; datorn som anv&#xe4;nds f&#xf6;r intervjun. Fr&#xe5;geformul&#xe4;ret kan vara statiskt eller interaktivt. Omfattar VCASI (Video Computer-Assisted Self-Interview), ACASI (Audio computer-assisted self-interview) och TCASI (Telephone audio computer-assisted self-interview).</skos:definition>
   </rdf:Description>
   <rdf:Description rdf:about="http://rdf-vocabulary.ddialliance.org/cv/ModeOfCollection/3.0.0/9ec957d">
      <rdf:type rdf:resource="http://www.w3.org/2004/02/skos/core#Concept"/>
      <skos:inScheme rdf:resource="http://rdf-vocabulary.ddialliance.org/cv/ModeOfCollection/3.0.0/"/>
      <skos:notation xml:lang="en">FocusGroup</skos:notation>
      <skos:prefLabel xml:lang="en">Focus group</skos:prefLabel>
      <skos:definition xml:lang="en">A group discussion on a particular topic, organized for research purposes. The individuals are selected with relevance to the topic, and interaction among the participants is used as part of the method.</skos:definition>
      <skos:prefLabel xml:lang="da">Fokusgruppe</skos:prefLabel>
      <skos:definition xml:lang="da">En gruppediskussion om et bestemt emne organiseret til forskningsform&#xe5;l. Individerne v&#xe6;lges med relevans for emnet, og interaktion mellem deltagerne anvendes som en del af metoden.</skos:definition>
      <skos:prefLabel xml:lang="fi">Kohderyhm&#xe4;keskustelu</skos:prefLabel>
      <skos:definition xml:lang="fi">Tutkimustarkoitusta varten j&#xe4;rjestetty kohderyhm&#xe4;keskustelu tietyst&#xe4; aiheesta. Ryhm&#xe4;n osanottajat valitaan aiheen mukaan ja osanottajien v&#xe4;linen vuorovaikutus on osa tutkimuskohdetta.</skos:definition>
      <skos:prefLabel xml:lang="fr">Focus group</skos:prefLabel>
      <skos:definition xml:lang="fr">Un groupe de discussions sur un sujet particulier, organis&#xe9; &#xe0; des fins de recherche. Les individus sont s&#xe9;lectionn&#xe9;s en fonction du sujet, et les interactions entre participants sont utilis&#xe9;es dans le cadre de la m&#xe9;thode.</skos:definition>
      <skos:prefLabel xml:lang="it">Focus group</skos:prefLabel>
      <skos:definition xml:lang="it">Una discussione di gruppo focalizzata su un argomento particolare, organizzata per scopi di ricerca. I singoli individui sono selezionati in base all&apos;argomento trattato, e l&apos;interazione tra i partecipanti viene utilizzata come parte della tecnica.</skos:definition>
      <skos:prefLabel xml:lang="no">Fokusgruppe</skos:prefLabel>
      <skos:definition xml:lang="no">En gruppediskusjon som omhandler et bestemt tema, organisert for forskningsform&#xe5;l. Individene er valgt med relevans til temaet og samhandlingen mellom deltakerne er brukt som en del av metoden.</skos:definition>
      <skos:prefLabel xml:lang="pt">Focus group (grupo focal)</skos:prefLabel>
      <skos:definition xml:lang="pt">Entrevista de grupo sobre um t&#xf3;pico espec&#xed;fico, organizada para fins de investiga&#xe7;&#xe3;o. Os indiv&#xed;duos s&#xe3;o selecionados em fun&#xe7;&#xe3;o da sua relev&#xe2;ncia para o t&#xf3;pico e a intera&#xe7;&#xe3;o entre os participantes &#xe9; usada como parte do m&#xe9;todo.</skos:definition>
      <skos:prefLabel xml:lang="sl">Fokusna skupina</skos:prefLabel>
      <skos:definition xml:lang="sl">Skupinska razprava o dolo&#x10d;eni temi, organizirana za raziskovalne namene. Posamezniki so izbrani glede na temo, interakcija med udele&#x17e;enci pa se uporablja kot del metode.</skos:definition>
      <skos:prefLabel xml:lang="sr">Fokus grupa</skos:prefLabel>
      <skos:definition xml:lang="sr">Grupna diskusija o odre&#x111;enoj temi, organizovana u istra&#x17e;iva&#x10d;ke svrhe. Pojedinci su odabrani u skladu sa temom, a interakcija izme&#x111;u u&#x10d;esnika koristi se kao deo metode.</skos:definition>
      <skos:prefLabel xml:lang="sv">Fokusgrupp</skos:prefLabel>
      <skos:definition xml:lang="sv">En gruppdiskussion om ett visst &#xe4;mne som anordnats i forskningssyfte. Deltagarna har valts ut med h&#xe4;nsyn till &#xe4;mnet och interaktionen mellan deltagarna utg&#xf6;r en del av forskningsmetoden.</skos:definition>
      <skos:narrower rdf:resource="http://rdf-vocabulary.ddialliance.org/cv/ModeOfCollection/3.0.0/00b3692"/>
      <skos:narrower rdf:resource="http://rdf-vocabulary.ddialliance.org/cv/ModeOfCollection/3.0.0/2b4ef44"/>
      <skos:narrower rdf:resource="http://rdf-vocabulary.ddialliance.org/cv/ModeOfCollection/3.0.0/4da1255"/>
   </rdf:Description>
   <rdf:Description rdf:about="http://rdf-vocabulary.ddialliance.org/cv/ModeOfCollection/3.0.0/00b3692">
      <rdf:type rdf:resource="http://www.w3.org/2004/02/skos/core#Concept"/>
      <skos:inScheme rdf:resource="http://rdf-vocabulary.ddialliance.org/cv/ModeOfCollection/3.0.0/"/>
      <skos:notation xml:lang="en">FocusGroup.FaceToFace</skos:notation>
      <skos:prefLabel xml:lang="en">Face-to-face focus group</skos:prefLabel>
      <skos:definition xml:lang="en">The focus group participants meet in person to conduct the discussion.</skos:definition>
      <skos:prefLabel xml:lang="da">Personlig fokusgruppe</skos:prefLabel>
      <skos:definition xml:lang="da">Fokusgruppens deltagere m&#xf8;des personligt for at gennemf&#xf8;re diskussionen.</skos:definition>
      <skos:prefLabel xml:lang="fi">Kohderyhm&#xe4;keskustelu: kasvokkainen keskustelu</skos:prefLabel>
      <skos:definition xml:lang="fi">Tutkimustarkoitusta varten j&#xe4;rjestetty kohderyhm&#xe4;keskustelu tietyst&#xe4; aiheesta. Keskustelu k&#xe4;yd&#xe4;&#xe4;n kasvokkain.</skos:definition>
      <skos:prefLabel xml:lang="fr">Focus group en face-&#xe0;-face</skos:prefLabel>
      <skos:definition xml:lang="fr">Les participants du focus group se rencontrent en personne pour mener la discussion.</skos:definition>
      <skos:prefLabel xml:lang="it">Focus group faccia a faccia</skos:prefLabel>
      <skos:definition xml:lang="it">I partecipanti al focus group si incontrano di persona per condurre la discussione.</skos:definition>
      <skos:prefLabel xml:lang="no">Fokusgruppe: Ansikt til ansikt</skos:prefLabel>
      <skos:definition xml:lang="no">Deltakerne i fokusgruppen m&#xf8;tes fysisk for &#xe5; gjennomf&#xf8;re diskusjonen.</skos:definition>
      <skos:prefLabel xml:lang="pt">Focus group presencial</skos:prefLabel>
      <skos:definition xml:lang="pt">Os participantes do grupo focal encontram-se pessoalmente para participar na discuss&#xe3;o.</skos:definition>
      <skos:prefLabel xml:lang="sl">Fokusna skupina v &#x17e;ivo</skos:prefLabel>
      <skos:definition xml:lang="sl">Udele&#x17e;enci fokusne skupine se osebno sestanejo za vodenje razprave.</skos:definition>
      <skos:prefLabel xml:lang="sr">Fokus grupa licem u lice</skos:prefLabel>
      <skos:definition xml:lang="sr">U&#x10d;esnici fokus grupe sastaju se li&#x10d;no kako bi vodili diskusiju.</skos:definition>
      <skos:prefLabel xml:lang="sv">Fokusgrupp: traditionell</skos:prefLabel>
      <skos:definition xml:lang="sv">Fokusgruppens medlemmar tr&#xe4;ffas p&#xe5; samma plats f&#xf6;r att diskutera.</skos:definition>
   </rdf:Description>
   <rdf:Description rdf:about="http://rdf-vocabulary.ddialliance.org/cv/ModeOfCollection/3.0.0/2b4ef44">
      <rdf:type rdf:resource="http://www.w3.org/2004/02/skos/core#Concept"/>
      <skos:inScheme rdf:resource="http://rdf-vocabulary.ddialliance.org/cv/ModeOfCollection/3.0.0/"/>
      <skos:notation xml:lang="en">FocusGroup.Telephone</skos:notation>
      <skos:prefLabel xml:lang="en">Telephone focus group</skos:prefLabel>
      <skos:definition xml:lang="en">The focus group discussion is conducted over the telephone.</skos:definition>
      <skos:prefLabel xml:lang="da">Telefonfokusgruppe</skos:prefLabel>
      <skos:definition xml:lang="da">Fokusgruppediskussionen gennemf&#xf8;res over telefonen.</skos:definition>
      <skos:prefLabel xml:lang="fi">Kohderyhm&#xe4;keskustelu: puhelinkeskustelu</skos:prefLabel>
      <skos:definition xml:lang="fi">Tutkimustarkoitusta varten j&#xe4;rjestetty kohderyhm&#xe4;keskustelu tietyst&#xe4; aiheesta. Keskustelu k&#xe4;yd&#xe4;&#xe4;n puhelimen v&#xe4;lityksell&#xe4;.</skos:definition>
      <skos:prefLabel xml:lang="fr">Focus group par t&#xe9;l&#xe9;phone</skos:prefLabel>
      <skos:definition xml:lang="fr">Les discussions du focus group se font par t&#xe9;l&#xe9;phone.</skos:definition>
      <skos:prefLabel xml:lang="it">Focus group telefonico</skos:prefLabel>
      <skos:definition xml:lang="it">La discussione del focus group &#xe8; condotta via telefono.</skos:definition>
      <skos:prefLabel xml:lang="no">Fokusgruppe: Telefon</skos:prefLabel>
      <skos:definition xml:lang="no">Fokusgruppediskusjonen er gjennomf&#xf8;rt over telefonen.</skos:definition>
      <skos:prefLabel xml:lang="pt">Focus group por telefone</skos:prefLabel>
      <skos:definition xml:lang="pt">A discuss&#xe3;o do grupo focal &#xe9; realizada por telefone.</skos:definition>
      <skos:prefLabel xml:lang="sl">Telefonska fokusna skupina</skos:prefLabel>
      <skos:definition xml:lang="sl">Fokusna skupina, kjer razprava poteka preko telefona.</skos:definition>
      <skos:prefLabel xml:lang="sr">Telefonska fokus grupa</skos:prefLabel>
      <skos:definition xml:lang="sr">Diskusija u okviru fokus grupe vodi se telefonom.</skos:definition>
      <skos:prefLabel xml:lang="sv">Fokusgrupp: telefon</skos:prefLabel>
      <skos:definition xml:lang="sv">Fokusgruppens diskussion f&#xf6;rs &#xf6;ver telefon.</skos:definition>
   </rdf:Description>
   <rdf:Description rdf:about="http://rdf-vocabulary.ddialliance.org/cv/ModeOfCollection/3.0.0/4da1255">
      <rdf:type rdf:resource="http://www.w3.org/2004/02/skos/core#Concept"/>
      <skos:inScheme rdf:resource="http://rdf-vocabulary.ddialliance.org/cv/ModeOfCollection/3.0.0/"/>
      <skos:notation xml:lang="en">FocusGroup.Online</skos:notation>
      <skos:prefLabel xml:lang="en">Online focus group</skos:prefLabel>
      <skos:definition xml:lang="en">The focus group discussion is conducted over the Internet in an interactive manner.</skos:definition>
      <skos:prefLabel xml:lang="da">Online-fokusgruppe</skos:prefLabel>
      <skos:definition xml:lang="da">Fokusgruppediskussionen gennemf&#xf8;res over internettet p&#xe5; en interaktiv m&#xe5;de.</skos:definition>
      <skos:prefLabel xml:lang="fi">Kohderyhm&#xe4;keskustelu: verkkokeskustelu</skos:prefLabel>
      <skos:definition xml:lang="fi">Tutkimustarkoitusta varten j&#xe4;rjestetty kohderyhm&#xe4;keskustelu tietyst&#xe4; aiheesta. Keskustelu k&#xe4;yd&#xe4;&#xe4;n verkossa.</skos:definition>
      <skos:prefLabel xml:lang="fr">Focus group en ligne</skos:prefLabel>
      <skos:definition xml:lang="fr">Les discussions du focus group se font par l&apos;Internet de fa&#xe7;on interactive.</skos:definition>
      <skos:prefLabel xml:lang="it">Focus group online</skos:prefLabel>
      <skos:definition xml:lang="it">La discussione del focus group &#xe8; condotta via Internet in modo interattivo.</skos:definition>
      <skos:prefLabel xml:lang="no">Fokusgruppe: Online</skos:prefLabel>
      <skos:definition xml:lang="no">Fokusgruppediskusjonen er gjennomf&#xf8;rt over internett p&#xe5; en interaktiv m&#xe5;te.</skos:definition>
      <skos:prefLabel xml:lang="pt">Focus group online</skos:prefLabel>
      <skos:definition xml:lang="pt">A discuss&#xe3;o do grupo focal &#xe9; conduzida pela Internet de forma interativa.</skos:definition>
      <skos:prefLabel xml:lang="sl">Spletna fokusna skupina</skos:prefLabel>
      <skos:definition xml:lang="sl">Fokusna skupina, kjer razprava poteka preko spleta na interaktiven na&#x10d;in.</skos:definition>
      <skos:prefLabel xml:lang="sr">Onlajn fokus grupa</skos:prefLabel>
      <skos:definition xml:lang="sr">Diskusija u okviru fokus grupe odvija se putem Interneta na interaktivan na&#x10d;in.</skos:definition>
      <skos:prefLabel xml:lang="sv">Fokusgrupp: virtuell</skos:prefLabel>
      <skos:definition xml:lang="sv">Fokusgruppens diskussion f&#xf6;rs interaktivt &#xf6;ver Internet. Kallas &#xe4;ven IT-st&#xf6;dd fokusgrupp.</skos:definition>
   </rdf:Description>
   <rdf:Description rdf:about="http://rdf-vocabulary.ddialliance.org/cv/ModeOfCollection/3.0.0/08e658a">
      <rdf:type rdf:resource="http://www.w3.org/2004/02/skos/core#Concept"/>
      <skos:inScheme rdf:resource="http://rdf-vocabulary.ddialliance.org/cv/ModeOfCollection/3.0.0/"/>
      <skos:notation xml:lang="en">SelfAdministeredWritingsAndDiaries</skos:notation>
      <skos:prefLabel xml:lang="en">Self-administered writings and/or diaries</skos:prefLabel>
      <skos:definition xml:lang="en">Narratives, stories, diaries, and written texts created by the research subject.</skos:definition>
      <skos:prefLabel xml:lang="da">Selvadministrerede tekster og/eller dagb&#xf8;ger</skos:prefLabel>
      <skos:definition xml:lang="da">Fort&#xe6;llinger, historier, dagb&#xf8;ger og nedskrevne tekster skabt af forskningssubjektet.</skos:definition>
      <skos:prefLabel xml:lang="fi">Oma kirjoitus tai p&#xe4;iv&#xe4;kirja</skos:prefLabel>
      <skos:definition xml:lang="fi">Osanottajien itse kirjoittamat el&#xe4;m&#xe4;kerrat, tarinat, p&#xe4;iv&#xe4;kirjat ja muut kirjoitukset.</skos:definition>
      <skos:prefLabel xml:lang="fr">&#xc9;crits et / ou journaux intimes auto-administr&#xe9;s</skos:prefLabel>
      <skos:definition xml:lang="fr">Des r&#xe9;cits, des histoires, des journaux intimes, et des textes &#xe9;crits cr&#xe9;es par le sujet de recherche.</skos:definition>
      <skos:prefLabel xml:lang="it">Scritti/diari auto-compilati</skos:prefLabel>
      <skos:definition xml:lang="it">Narrazioni, storie, diari e testi scritti creati dai soggetti coinvolti nella ricerca.</skos:definition>
      <skos:prefLabel xml:lang="no">Selvadministrerende tekst og/eller dagbok</skos:prefLabel>
      <skos:definition xml:lang="no">Fortellinger, historier, dagb&#xf8;ker og tekster skrevet av studieobjektene.</skos:definition>
      <skos:prefLabel xml:lang="pt">Textos e/ou di&#xe1;rios de autopreenchimento</skos:prefLabel>
      <skos:definition xml:lang="pt">Narrativas, hist&#xf3;rias, di&#xe1;rios e textos escritos criados/produzidos pelo(s) sujeito(s) da pesquisa.</skos:definition>
      <skos:prefLabel xml:lang="sl">Samoizpolnjevanje zapisov in/ali dnevnikov</skos:prefLabel>
      <skos:definition xml:lang="sl">Pripovedi, zgodbe, dnevniki in napisana besedila, ki jih ustvari subjekt raziskave.</skos:definition>
      <skos:prefLabel xml:lang="sr">Samostalni zapisi i/ili dnevnici</skos:prefLabel>
      <skos:definition xml:lang="sr">Narativi (besede), pri&#x10d;e, dnevnici i pisani tekstovi koje je kreirao subjekat istra&#x17e;ivanja.</skos:definition>
      <skos:prefLabel xml:lang="sv">Sj&#xe4;lvadministrerad text och/eller dagb&#xf6;cker</skos:prefLabel>
      <skos:definition xml:lang="sv">Narrativ, ber&#xe4;ttelser, dagb&#xf6;cker och andra nedskrivna texter skapade av forskningspersonerna.</skos:definition>
      <skos:narrower rdf:resource="http://rdf-vocabulary.ddialliance.org/cv/ModeOfCollection/3.0.0/fe226ad"/>
      <skos:narrower rdf:resource="http://rdf-vocabulary.ddialliance.org/cv/ModeOfCollection/3.0.0/e5bef42"/>
      <skos:narrower rdf:resource="http://rdf-vocabulary.ddialliance.org/cv/ModeOfCollection/3.0.0/9e67a7c"/>
   </rdf:Description>
   <rdf:Description rdf:about="http://rdf-vocabulary.ddialliance.org/cv/ModeOfCollection/3.0.0/fe226ad">
      <rdf:type rdf:resource="http://www.w3.org/2004/02/skos/core#Concept"/>
      <skos:inScheme rdf:resource="http://rdf-vocabulary.ddialliance.org/cv/ModeOfCollection/3.0.0/"/>
      <skos:notation xml:lang="en">SelfAdministeredWritingsAndDiaries.Email</skos:notation>
      <skos:prefLabel xml:lang="en">Self-administered writings and/or diaries: E-mail</skos:prefLabel>
      <skos:definition xml:lang="en">Narratives, stories, diaries, and written texts submitted via e-mail messages.</skos:definition>
      <skos:prefLabel xml:lang="da">Selvadministrerede tekster og/eller dagb&#xf8;ger: E-mail</skos:prefLabel>
      <skos:definition xml:lang="da">Fort&#xe6;llinger, historier, dagb&#xf8;ger og nedskrevne tekster afleveret via e-mail-beskeder.</skos:definition>
      <skos:prefLabel xml:lang="fi">Oma kirjoitus tai p&#xe4;iv&#xe4;kirja: s&#xe4;hk&#xf6;postilla saatu</skos:prefLabel>
      <skos:definition xml:lang="fi">Osanottajien s&#xe4;hk&#xf6;postin v&#xe4;lityksell&#xe4; annetut omat kirjoitukset ja p&#xe4;iv&#xe4;kirjat.</skos:definition>
      <skos:prefLabel xml:lang="fr">crits et / ou journaux intimes auto-administr&#xe9;s : e-mail</skos:prefLabel>
      <skos:definition xml:lang="fr">Des r&#xe9;cits, des histoires, des journaux intimes, et des textes &#xe9;crits soumis par courriel.</skos:definition>
      <skos:prefLabel xml:lang="it">Scritti/diari auto-compilati: e-mail</skos:prefLabel>
      <skos:definition xml:lang="it">Narrazioni, storie, diari e testi scritti inviati tramite e-mail.</skos:definition>
      <skos:prefLabel xml:lang="no">Selvadministrerende tekst og/eller dagbok: E-post</skos:prefLabel>
      <skos:definition xml:lang="no">Fortellinger, historier, dagb&#xf8;ker og tekster som har blitt samlet inn via e-post.</skos:definition>
      <skos:prefLabel xml:lang="pt">Textos e/ou di&#xe1;rios de autopreenchimento: Email</skos:prefLabel>
      <skos:definition xml:lang="pt">Narrativas, hist&#xf3;rias, di&#xe1;rios e textos escritos enviados por mensagens de email.</skos:definition>
      <skos:prefLabel xml:lang="sl">Samoizpolnjevanje zapisov in/ali dnevnikov: elektronska po&#x161;ta</skos:prefLabel>
      <skos:definition xml:lang="sl">Pripovedi, zgodbe, dnevniki in napisana besedila, ki so posredovana preko elektronskih po&#x161;tnih sporo&#x10d;il.</skos:definition>
      <skos:prefLabel xml:lang="sr">Samostalni zapisi i/ili dnevnici: Elektronskom po&#x161;tom</skos:prefLabel>
      <skos:definition xml:lang="sr">Narativi (besede), pri&#x10d;e, dnevnici i pisani tekstovi koje ispitanik &#x161;alje elektronskom po&#x161;tom.</skos:definition>
      <skos:prefLabel xml:lang="sv">Sj&#xe4;lvadministrerad text och/eller dagb&#xf6;cker: e-post</skos:prefLabel>
      <skos:definition xml:lang="sv">Narrativ, ber&#xe4;ttelser, dagb&#xf6;cker och andra nedskrivna texter som skickas in via e-post.</skos:definition>
   </rdf:Description>
   <rdf:Description rdf:about="http://rdf-vocabulary.ddialliance.org/cv/ModeOfCollection/3.0.0/e5bef42">
      <rdf:type rdf:resource="http://www.w3.org/2004/02/skos/core#Concept"/>
      <skos:inScheme rdf:resource="http://rdf-vocabulary.ddialliance.org/cv/ModeOfCollection/3.0.0/"/>
      <skos:notation xml:lang="en">SelfAdministeredWritingsAndDiaries.Paper</skos:notation>
      <skos:prefLabel xml:lang="en">Self-administered writings and/or diaries: Paper</skos:prefLabel>
      <skos:definition xml:lang="en">Narratives, stories, diaries, and written texts created and collected in paper form.</skos:definition>
      <skos:prefLabel xml:lang="da">Selvadministrerede tekster og/eller dagb&#xf8;ger: Papir</skos:prefLabel>
      <skos:definition xml:lang="da">Fort&#xe6;llinger, historier, dagb&#xf8;ger og nedskrevne tekster skabt og indsamlet i papirform.</skos:definition>
      <skos:prefLabel xml:lang="fi">Oma kirjoitus tai p&#xe4;iv&#xe4;kirja: paperimuotoinen kirjoitus</skos:prefLabel>
      <skos:definition xml:lang="fi">Osanottajien paperimuotoiset omat kirjoitukset ja p&#xe4;iv&#xe4;kirjat.</skos:definition>
      <skos:prefLabel xml:lang="fr">&#xc9;crits et / ou journaux intimes auto-administr&#xe9;s : papier</skos:prefLabel>
      <skos:definition xml:lang="fr">Des r&#xe9;cits, des histoires, des journaux intimes, et des textes &#xe9;crits cr&#xe9;es et rassembl&#xe9;s sous forme papier.</skos:definition>
      <skos:prefLabel xml:lang="it">Scritti/diari auto-compilati: cartaceo</skos:prefLabel>
      <skos:definition xml:lang="it">Narrazioni, storie, diari e testi scritti creati e raccolti in forma cartacea.</skos:definition>
      <skos:prefLabel xml:lang="no">Selvadministrerende tekst og/eller dagbok: Papir</skos:prefLabel>
      <skos:definition xml:lang="no">Fortellinger, historier, dagb&#xf8;ker og tekster skrevet og samlet i papirformat.</skos:definition>
      <skos:prefLabel xml:lang="pt">Textos e/ou di&#xe1;rios de autopreenchimento: Papel</skos:prefLabel>
      <skos:definition xml:lang="pt">Narrativas, hist&#xf3;rias, di&#xe1;rios e textos escritos criados e recolhidos em papel.</skos:definition>
      <skos:prefLabel xml:lang="sl">Samoizpolnjevanje zapisov in/ali dnevnikov: papir</skos:prefLabel>
      <skos:definition xml:lang="sl">Pripovedi, zgodbe, dnevniki in napisana besedila, ki so ustvarjena in zbrana na papirju.</skos:definition>
      <skos:prefLabel xml:lang="sr">Samostalni zapisi i/ili dnevnici: Papirni</skos:prefLabel>
      <skos:definition xml:lang="sr">Narativi (besede), pri&#x10d;e, dnevnici i pisani tekstovi koje ispitanik prila&#x17e;e u papirnom obliku.</skos:definition>
      <skos:prefLabel xml:lang="sv">Sj&#xe4;lvadministrerad text och/eller dagb&#xf6;cker: papper</skos:prefLabel>
      <skos:definition xml:lang="sv">Narrativ, ber&#xe4;ttelser, dagb&#xf6;cker och andra nedskrivna texter som skapats och samlats in p&#xe5; papper.</skos:definition>
   </rdf:Description>
   <rdf:Description rdf:about="http://rdf-vocabulary.ddialliance.org/cv/ModeOfCollection/3.0.0/9e67a7c">
      <rdf:type rdf:resource="http://www.w3.org/2004/02/skos/core#Concept"/>
      <skos:inScheme rdf:resource="http://rdf-vocabulary.ddialliance.org/cv/ModeOfCollection/3.0.0/"/>
      <skos:notation xml:lang="en">SelfAdministeredWritingsAndDiaries.WebBased</skos:notation>
      <skos:prefLabel xml:lang="en">Self-administered writings and/or diaries: Web-based</skos:prefLabel>
      <skos:definition xml:lang="en">Narratives, stories, diaries, and written texts gathered from Internet sources, e.g. websites, blogs, discussion forums.</skos:definition>
      <skos:prefLabel xml:lang="da">Selvadministrerede tekster og/eller dagb&#xf8;ger: Webbaseret</skos:prefLabel>
      <skos:definition xml:lang="da">Fort&#xe6;llinger, historier, dagb&#xf8;ger og nedskrevne tekster indsamlet fra internetkilder, for eksempel hjemmesider, blogs og diskussionsfora.</skos:definition>
      <skos:prefLabel xml:lang="fi">Oma kirjoitus tai p&#xe4;iv&#xe4;kirja: verkon kautta saatu</skos:prefLabel>
      <skos:definition xml:lang="fi">Osanottajien verkossa kirjoitetut omat kirjoitukset ja p&#xe4;iv&#xe4;kirjat.</skos:definition>
      <skos:prefLabel xml:lang="fr">&#xc9;crits et / ou journaux intimes auto-administr&#xe9;s : en ligne</skos:prefLabel>
      <skos:definition xml:lang="fr">Des r&#xe9;cits, des histoires, des journaux intimes, et des textes &#xe9;crits provenant d&apos;Internet, e. g. des sites Internet, des blogs, des forums de discussion.</skos:definition>
      <skos:prefLabel xml:lang="it">Scritti/diari auto-compilati: web</skos:prefLabel>
      <skos:definition xml:lang="it">Narrazioni, storie, diari e testi scritti raccolti su Internet, ad esempio da siti web, blog, forum di discussione.</skos:definition>
      <skos:prefLabel xml:lang="no">Selvadministrerende tekst og/eller dagbok: Webbasert</skos:prefLabel>
      <skos:definition xml:lang="no">Fortellinger, historier, dagb&#xf8;ker og tekster samlet fra internett, e.g. nettsider, blogger, diskusjonsforumer.</skos:definition>
      <skos:prefLabel xml:lang="pt">Textos e/ou di&#xe1;rios de autopreenchimento: Online/via web</skos:prefLabel>
      <skos:definition xml:lang="pt">Narrativas, hist&#xf3;rias, di&#xe1;rios e textos escritos recolhidos de fontes da Internet, por ex. sites, blogs, f&#xf3;runs de discuss&#xe3;o.</skos:definition>
      <skos:prefLabel xml:lang="sl">Samoizpolnjevanje zapisov in/ali dnevnikov: spletno</skos:prefLabel>
      <skos:definition xml:lang="sl">Pripovedi, zgodbe, dnevniki in napisana besedila, ki so zbrana preko internetnih virov, npr. spletne strani, blogi, forumi.</skos:definition>
      <skos:prefLabel xml:lang="sr">Samostalni zapisi i/ili dnevnici: Veb</skos:prefLabel>
      <skos:definition xml:lang="sr">Narativi (besede), pri&#x10d;e, dnevnici i pisani tekstovi prikupljeni iz Internet izvora, na primer veb sajtova, blogova, diskusionih grupa.</skos:definition>
      <skos:prefLabel xml:lang="sv">Sj&#xe4;lvadministrerad text och/eller dagb&#xf6;cker: webbaserat</skos:prefLabel>
      <skos:definition xml:lang="sv">Narrativ, ber&#xe4;ttelser, dagb&#xf6;cker och andra nedskrivna texter som samlats in fr&#xe5;n Internet-k&#xe4;llor, t.ex. webbplatser, bloggar, diskussionsforum.</skos:definition>
   </rdf:Description>
   <rdf:Description rdf:about="http://rdf-vocabulary.ddialliance.org/cv/ModeOfCollection/3.0.0/c680d43">
      <rdf:type rdf:resource="http://www.w3.org/2004/02/skos/core#Concept"/>
      <skos:inScheme rdf:resource="http://rdf-vocabulary.ddialliance.org/cv/ModeOfCollection/3.0.0/"/>
      <skos:notation xml:lang="en">Observation</skos:notation>
      <skos:prefLabel xml:lang="en">Observation</skos:prefLabel>
      <skos:definition xml:lang="en">Research method that involves collecting data as they occur (for example, observing behaviors, events, development of condition or disease, etc.), without attempting to manipulate any of the independent variables.</skos:definition>
      <skos:prefLabel xml:lang="da">Observation</skos:prefLabel>
      <skos:definition xml:lang="da">Forskningsmetode, der involverer at indsamle data, som de opst&#xe5;r (for eksempel observering af opf&#xf8;rsel, begivenheder, udviklingen af tilstand eller sygdom mm.) uden at fors&#xf8;ge at manipulere&#xa0;de uafh&#xe6;ngige variable.</skos:definition>
      <skos:prefLabel xml:lang="fi">Havainnointi</skos:prefLabel>
      <skos:definition xml:lang="fi">Keruumenetelm&#xe4;, jossa tarkkaillaan tapahtumia, k&#xe4;ytt&#xe4;ytymist&#xe4;, vuorovaikutusta jne. niiden tapahtuessa, ilman mink&#xe4;&#xe4;n riippumattoman muuttujan manipulointia.</skos:definition>
      <skos:prefLabel xml:lang="fr">Observation</skos:prefLabel>
      <skos:definition xml:lang="fr">M&#xe9;thode de recherche qui consiste &#xe0; collecter des donn&#xe9;es au fur et &#xe0; mesure qu&apos;elle se produisent (par exemple, observation de comportements, d&#x2019;&#xe9;v&#xe9;nements, de l&apos;&#xe9;volution d&apos;un &#xe9;tat ou d&apos;une maladie, etc.), sans tentative de manipuler aucune des variables ind&#xe9;pendantes.</skos:definition>
      <skos:prefLabel xml:lang="it">Osservazione</skos:prefLabel>
      <skos:definition xml:lang="it">Tecnica di rilevazione che implica la raccolta di dati nel momento in cui si generano (ad esempio osservando comportamenti, eventi, sviluppo di condizioni o malattie, ecc.), senza tentare di manipolare nessuna delle variabili indipendenti.</skos:definition>
      <skos:prefLabel xml:lang="no">Observasjon</skos:prefLabel>
      <skos:definition xml:lang="no">Forskningsmetode som inneb&#xe6;rer &#xe5; samle inn data etterhvert som de opptr&#xe5;r (for eksempel, observere atferd, hendelser, utviklingen av helsetilstand eller sykdom, etc.) uten &#xe5; pr&#xf8;ve &#xe5; manipulere noen av de uavhengige variablene.</skos:definition>
      <skos:prefLabel xml:lang="pt">Observa&#xe7;&#xe3;o</skos:prefLabel>
      <skos:definition xml:lang="pt">M&#xe9;todo de investiga&#xe7;&#xe3;o que envolve a recolha de dados conforme eles ocorrem (por exemplo, observando comportamentos, eventos, desenvolvimento de uma condi&#xe7;&#xe3;o ou doen&#xe7;a, etc.), sem tentar manipular nenhuma das vari&#xe1;veis independentes.</skos:definition>
      <skos:prefLabel xml:lang="sl">Opazovanje</skos:prefLabel>
      <skos:definition xml:lang="sl">Raziskovalna metoda, ki vklju&#x10d;uje zbiranje podatkov, ko se pojavijo (npr. opazovanje vedenj, dogodkov, razvoja stanja ali bolezni itd.), ne da bi posku&#x161;ali manipulirati s katero od neodvisnih spremenljivk.</skos:definition>
      <skos:prefLabel xml:lang="sr">Opservacije / posmatranje</skos:prefLabel>
      <skos:definition xml:lang="sr">Metoda istra&#x17e;ivanja koja uklju&#x10d;uje prikupljanje podataka kako se pojavljuju (na primer, posmatranje pona&#x161;anja, doga&#x111;aja, razvoj stanja ili bolesti itd.), bez poku&#x161;aja manipulacije bilo kojom nezavisnom promenljivom.</skos:definition>
      <skos:prefLabel xml:lang="sv">Observation</skos:prefLabel>
      <skos:definition xml:lang="sv">Forskningsmetod som omfattar att samla in data om f&#xf6;reteelser n&#xe4;r de upptr&#xe4;der (t.ex. observationer av beteenden, h&#xe4;ndelser m.m.) utan att f&#xf6;rs&#xf6;ka p&#xe5;verka n&#xe5;gra av de oberoende variablerna.</skos:definition>
      <skos:narrower rdf:resource="http://rdf-vocabulary.ddialliance.org/cv/ModeOfCollection/3.0.0/bdc4aac"/>
      <skos:narrower rdf:resource="http://rdf-vocabulary.ddialliance.org/cv/ModeOfCollection/3.0.0/e679c7f"/>
      <skos:narrower rdf:resource="http://rdf-vocabulary.ddialliance.org/cv/ModeOfCollection/3.0.0/40b8b0c"/>
   </rdf:Description>
   <rdf:Description rdf:about="http://rdf-vocabulary.ddialliance.org/cv/ModeOfCollection/3.0.0/bdc4aac">
      <rdf:type rdf:resource="http://www.w3.org/2004/02/skos/core#Concept"/>
      <skos:inScheme rdf:resource="http://rdf-vocabulary.ddialliance.org/cv/ModeOfCollection/3.0.0/"/>
      <skos:notation xml:lang="en">Observation.Field</skos:notation>
      <skos:prefLabel xml:lang="en">Field observation</skos:prefLabel>
      <skos:definition xml:lang="en">Observation that is conducted in a natural environment.</skos:definition>
      <skos:prefLabel xml:lang="da">Feltobservation</skos:prefLabel>
      <skos:definition xml:lang="da">Observation, som udf&#xf8;res i et naturligt milj&#xf8;.</skos:definition>
      <skos:prefLabel xml:lang="fi">Havainnointi: kentt&#xe4;havainnointi</skos:prefLabel>
      <skos:definition xml:lang="fi">Havainnointi suoritetaan luonnollisessa, kontrolloimattomassa ymp&#xe4;rist&#xf6;ss&#xe4;. K&#xe4;yt&#xe4; termi&#xe4; mik&#xe4;li ei tiedossa onko osallistuvaa vai ei-osallistuvaa.</skos:definition>
      <skos:prefLabel xml:lang="fr">Observation sur le terrain</skos:prefLabel>
      <skos:definition xml:lang="fr">Observation qui a &#xe9;t&#xe9; conduite dans un environnement naturel.</skos:definition>
      <skos:prefLabel xml:lang="it">Osservazione sul campo</skos:prefLabel>
      <skos:definition xml:lang="it">Osservazione condotta in un ambiente naturale.</skos:definition>
      <skos:prefLabel xml:lang="no">Feltobservasjon</skos:prefLabel>
      <skos:definition xml:lang="no">Observasjon som utf&#xf8;res i et naturlig milj&#xf8;.</skos:definition>
      <skos:prefLabel xml:lang="pt">Observa&#xe7;&#xe3;o de campo</skos:prefLabel>
      <skos:definition xml:lang="pt">Observa&#xe7;&#xe3;o conduzida em ambiente natural.</skos:definition>
      <skos:prefLabel xml:lang="sl">Opazovanje na terenu</skos:prefLabel>
      <skos:definition xml:lang="sl">Opazovanje, ki se izvaja v naravnem okolju.</skos:definition>
      <skos:prefLabel xml:lang="sr">Terenska posmatranja</skos:prefLabel>
      <skos:definition xml:lang="sr">Opservacije koje se sprovode u prirodnom okru&#x17e;enju.</skos:definition>
      <skos:prefLabel xml:lang="sv">F&#xe4;ltobservation</skos:prefLabel>
      <skos:definition xml:lang="sv">Observation som utf&#xf6;rs i en naturlig milj&#xf6;.</skos:definition>
      <skos:narrower rdf:resource="http://rdf-vocabulary.ddialliance.org/cv/ModeOfCollection/3.0.0/3cee522"/>
      <skos:narrower rdf:resource="http://rdf-vocabulary.ddialliance.org/cv/ModeOfCollection/3.0.0/8245871"/>
   </rdf:Description>
   <rdf:Description rdf:about="http://rdf-vocabulary.ddialliance.org/cv/ModeOfCollection/3.0.0/e679c7f">
      <rdf:type rdf:resource="http://www.w3.org/2004/02/skos/core#Concept"/>
      <skos:inScheme rdf:resource="http://rdf-vocabulary.ddialliance.org/cv/ModeOfCollection/3.0.0/"/>
      <skos:notation xml:lang="en">Observation.Laboratory</skos:notation>
      <skos:prefLabel xml:lang="en">Laboratory observation</skos:prefLabel>
      <skos:definition xml:lang="en">Observation that is conducted in a controlled, artificially created setting. For example, observing children&apos;s play in a laboratory playroom.</skos:definition>
      <skos:prefLabel xml:lang="da">Laboratorieobservation</skos:prefLabel>
      <skos:definition xml:lang="da">Observation, der udf&#xf8;res i en kontrolleret, kunstig skabt ops&#xe6;tning. For eksempel observering af b&#xf8;rns leg i et laboratoriums legerum.</skos:definition>
      <skos:prefLabel xml:lang="fi">Havainnointi: laboratoriohavainnointi</skos:prefLabel>
      <skos:definition xml:lang="fi">Kokeellinen havainnointi kontrolloidussa, tarkoitusta varten luodussa tilassa tai ymp&#xe4;rist&#xf6;ss&#xe4;. Esimerkki: Lasten leikkien havainnointi laboratorioon rakennetussa leikkihuoneessa. K&#xe4;yt&#xe4; t&#xe4;t&#xe4; termi&#xe4; mik&#xe4;li ei ole tiedossa onko laboratoriohavainnointi osallistuvaa vai ei-osallistuvaa.</skos:definition>
      <skos:prefLabel xml:lang="fr">Observation en laboratoire</skos:prefLabel>
      <skos:definition xml:lang="fr">Observation qui a &#xe9;t&#xe9; conduite dans un configuration contr&#xf4;l&#xe9;e, artificiellement cr&#xe9;&#xe9;e. Par exemple, l&apos;observation du jeu des enfants dans une salle de jeux de laboratoire.</skos:definition>
      <skos:prefLabel xml:lang="it">Osservazione in laboratorio</skos:prefLabel>
      <skos:definition xml:lang="it">Osservazione condotta in un ambiente controllato, creato artificialmente. Ad esempio, osservazione del gioco dei bambini in una stanza da gioco ricreata in laboratorio.</skos:definition>
      <skos:prefLabel xml:lang="no">Laboratorieobservasjon</skos:prefLabel>
      <skos:definition xml:lang="no">Observasjon som er utf&#xf8;rt i et kontrollert, kunstig konstruert milj&#xf8;. For eksempel observasjon av barns lek i et lekerom i laboratoriet.</skos:definition>
      <skos:prefLabel xml:lang="pt">Observa&#xe7;&#xe3;o em laborat&#xf3;rio</skos:prefLabel>
      <skos:definition xml:lang="pt">Observa&#xe7;&#xe3;o que &#xe9; conduzida/realizada em ambiente controlado e artificialmente criado. Por exemplo, observa&#xe7;&#xe3;o das brincadeiras das crian&#xe7;as numa sala de jogos de laborat&#xf3;rio.</skos:definition>
      <skos:prefLabel xml:lang="sl">Laboratorijsko opazovanje</skos:prefLabel>
      <skos:definition xml:lang="sl">Opazovanje, ki se izvaja v nadzorovanem, umetno ustvarjenem okolju. Na primer, opazovanje otro&#x161;ke igre v laboratorijski igralnici.</skos:definition>
      <skos:prefLabel xml:lang="sr">Laboratorijsko posmatranje</skos:prefLabel>
      <skos:definition xml:lang="sr">Posmatranje koje se izvodi u kontrolisanom, ve&#x161;ta&#x10d;ki stvorenom okru&#x17e;enju. Na primer, posmatranje igre dece u laboratorijskoj igraonici.</skos:definition>
      <skos:prefLabel xml:lang="sv">Laboratorieobservation</skos:prefLabel>
      <skos:definition xml:lang="sv">Observation som utf&#xf6;rs i en kontrollerad, konstgjord milj&#xf6;. Exempel: observation av barns lek i ett laboratorielekrum.</skos:definition>
      <skos:narrower rdf:resource="http://rdf-vocabulary.ddialliance.org/cv/ModeOfCollection/3.0.0/2a58349"/>
      <skos:narrower rdf:resource="http://rdf-vocabulary.ddialliance.org/cv/ModeOfCollection/3.0.0/68b02fb"/>
   </rdf:Description>
   <rdf:Description rdf:about="http://rdf-vocabulary.ddialliance.org/cv/ModeOfCollection/3.0.0/2a58349">
      <rdf:type rdf:resource="http://www.w3.org/2004/02/skos/core#Concept"/>
      <skos:inScheme rdf:resource="http://rdf-vocabulary.ddialliance.org/cv/ModeOfCollection/3.0.0/"/>
      <skos:notation xml:lang="en">Observation.Laboratory.Participant</skos:notation>
      <skos:prefLabel xml:lang="en">Participant laboratory observation</skos:prefLabel>
      <skos:definition xml:lang="en">Type of laboratory observation in which the researcher interacts with the subjects and often plays a role in the social situation under observation. For example, observing children&apos;s play in a laboratory playroom with the researcher taking part in the play.</skos:definition>
      <skos:prefLabel xml:lang="da">Laboratorieobservation med deltager</skos:prefLabel>
      <skos:definition xml:lang="da">Type af laboratorieobservation, hvor forskeren interagerer med subjekterne og ofte spiller en rolle i den sociale situation under observation. For eksempel observering af b&#xf8;rns leg i et laboratorielegerum med forskeren, der deltager i legen.</skos:definition>
      <skos:prefLabel xml:lang="fi">Havainnointi: laboratoriohavainnointi: osallistuva</skos:prefLabel>
      <skos:definition xml:lang="fi">Kokeellinen havainnointi kontrolloidussa, tarkoitusta varten luodussa tilassa. Tutkija on vuorovaikutuksessa tutkittavien kanssa ja h&#xe4;nell&#xe4; on usein jokin rooli tutkimuksen kohteena olevassa sosiaalisessa tilanteessa. Esimerkki: Lasten leikkien havainnointi laboratorioon rakennetussa leikkihuoneessa, jossa tutkija ottaa osaa leikkiin.</skos:definition>
      <skos:prefLabel xml:lang="fr">Observation participante en laboratoire</skos:prefLabel>
      <skos:definition xml:lang="fr">Type d&apos;observation en laboratoire dans lequel le sujet interagit avec les sujets et joue souvent un r&#xf4;le dans la situation sociale sous observation. Par exemple, l&apos;observation du jeu des enfants dans une salle de jeux de laboratoire avec le chercheur prenant part au jeu.</skos:definition>
      <skos:prefLabel xml:lang="it">Osservazione partecipante in laboratorio</skos:prefLabel>
      <skos:definition xml:lang="it">Tipo di osservazione in laboratorio in cui il ricercatore interagisce con i soggetti e spesso gioca un ruolo nella situazione sociale sotto osservazione. Ad esempio, osservando il gioco dei bambini in una stanza da gioco ricreata in laboratorio con il ricercatore che partecipa al gioco.</skos:definition>
      <skos:prefLabel xml:lang="no">Deltagende laboratorieobservasjon</skos:prefLabel>
      <skos:definition xml:lang="no">En type laboratorieobservasjon hvor forskeren samhandler med forskningsobjektene, og ofte spiller en rolle i den sosiale situasjonen som er under observasjon. For eksempel observere barns lek i et lekerom i laboratoriet, der forsker deltar i leken.</skos:definition>
      <skos:prefLabel xml:lang="pt">Observa&#xe7;&#xe3;o participante em laborat&#xf3;rio</skos:prefLabel>
      <skos:definition xml:lang="pt">Tipo de observa&#xe7;&#xe3;o em laborat&#xf3;rio em que o investigador interage com os sujeitos e, muitas vezes, desempenha um papel na situa&#xe7;&#xe3;o social em observa&#xe7;&#xe3;o. Por exemplo, observa&#xe7;&#xe3;o das brincadeiras das crian&#xe7;as numa sala de jogos de laborat&#xf3;rio com o investigador a participar no jogo.</skos:definition>
      <skos:prefLabel xml:lang="sl">Laboratorijsko opazovanje z udele&#x17e;bo</skos:prefLabel>
      <skos:definition xml:lang="sl">Vrsta laboratorijskega opazovanja, kjer je raziskovalec v interkaciji s subjekti in pogosto igra vlogo v opazovani dru&#x17e;beni situaciji. Na primer, opazovanje otro&#x161;ke igre v laboratorijski igralnici, kjer ima raziskovalec vlogo v igri.</skos:definition>
      <skos:prefLabel xml:lang="sr">Laboratorijsko posmatranje sa u&#x10d;e&#x161;&#x107;em</skos:prefLabel>
      <skos:definition xml:lang="sr">Vrsta laboratorijskog posmatranja u kome istra&#x17e;iva&#x10d; komunicira sa subjektima i &#x10d;esto igra ulogu u posmatranom socijalnom stanju. Na primer, posmatranje igre dece u laboratorijskoj igraonici sa istra&#x17e;iva&#x10d;em koji u&#x10d;estvuje u predstavi.</skos:definition>
      <skos:prefLabel xml:lang="sv">Deltagande laboratorieobservation</skos:prefLabel>
      <skos:definition xml:lang="sv">Laboratorieobservation d&#xe4;r forskaren interagerar med forskningsobjekten och ofta har en funktion i den sociala situation som observeras. Exempel: observation av barns lek i ett laboratorielekrum d&#xe4;r forskaren deltar i leken.</skos:definition>
   </rdf:Description>
   <rdf:Description rdf:about="http://rdf-vocabulary.ddialliance.org/cv/ModeOfCollection/3.0.0/40b8b0c">
      <rdf:type rdf:resource="http://www.w3.org/2004/02/skos/core#Concept"/>
      <skos:inScheme rdf:resource="http://rdf-vocabulary.ddialliance.org/cv/ModeOfCollection/3.0.0/"/>
      <skos:notation xml:lang="en">Observation.ComputerBased</skos:notation>
      <skos:prefLabel xml:lang="en">Computer-based observation</skos:prefLabel>
      <skos:definition xml:lang="en">Type of observation in which data regarding computer usage are being collected by software that can be built into the computer program itself or can be a separate program. Information may be collected about the number of users, the ways in which users interact with the program(s), how much time they spend on a page, how they use specific sections of applications, how they navigate from page to page or from one application to another, etc.</skos:definition>
      <skos:prefLabel xml:lang="da">Computerbaseret observation</skos:prefLabel>
      <skos:definition xml:lang="da">Observationstype, hvor data vedr&#xf8;rende computerbrug indsamles af software, der kan indbygges i selve computerprogrammet eller kan v&#xe6;re et s&#xe6;rskilt program. Oplysninger kan indsamles om antallet af brugere, hvordan brugere interagerer med programmet (programmerne), hvor meget tid de bruger p&#xe5; en side, hvordan de anvender bestemte sektioner af applikationer, hvordan de navigerer fra side til side eller fra en applikation til en anden mm.</skos:definition>
      <skos:prefLabel xml:lang="fi">Havainnointi: tietokonepohjainen havainnointi</skos:prefLabel>
      <skos:definition xml:lang="fi">Havainnointimenetelm&#xe4;, jossa ker&#xe4;t&#xe4;&#xe4;n tietoa ihmisten tietokoneen k&#xe4;yt&#xf6;st&#xe4; ohjelmallisesti. Havainnointiohjelma voi olla sis&#xe4;&#xe4;nrakennettu tietokoneohjelmaan tai se voi olla erillinen ohjelma. Tietoa voidaan ker&#xe4;t&#xe4; k&#xe4;ytt&#xe4;jien m&#xe4;&#xe4;rist&#xe4;, heid&#xe4;n tavoistaan k&#xe4;ytt&#xe4;&#xe4; ohjelmaa ja sen toimintoja, navigoinnista jne.</skos:definition>
      <skos:prefLabel xml:lang="fr">Observation assist&#xe9; par ordinateur</skos:prefLabel>
      <skos:definition xml:lang="fr">Type d&apos;observation dans lequel les donn&#xe9;es relatives &#xe0; l&apos;utilisation de l&apos;ordinateur ont &#xe9;t&#xe9; collect&#xe9;es par un logiciel qui peut &#xea;tre int&#xe9;gr&#xe9; dans un programme informatique lui-m&#xea;me ou qui peut &#xea;tre un programme s&#xe9;par&#xe9;. Des informations peuvent &#xea;tre collect&#xe9;es &#xe0; propos du nombre d&apos;utilisateurs, les fa&#xe7;ons dans lesquels les utilisateurs interagissent avec le(s) programme(s), combien de temps ils passent sur une page, comment ils utilisent des sections sp&#xe9;cifiques des applications, comment ils naviguent d&apos;une page &#xe0; l&apos;autre ou d&apos;une application &#xe0; l&apos;autre, etc.</skos:definition>
      <skos:prefLabel xml:lang="it">Osservazione basata su computer</skos:prefLabel>
      <skos:definition xml:lang="it">Tipo di osservazione in cui vengono raccolti dati riguardanti l&apos;uso del computer, attraverso software che pu&#xf2; essere incorporato nel programma informatico stesso, oppure essere un programma separato. Con questo metodo si possono raccogliere informazioni sul numero di utenti, sui modi in cui gli utenti interagiscono con il programma, sulla quantit&#xe0; di tempo che trascorrono su una pagina, su come utilizzano specifiche sezioni di applicazioni, su come navigano da una pagina all&apos;altra o da una applicazione all&apos;altra, ecc.</skos:definition>
      <skos:prefLabel xml:lang="no">Datamaskinbasert observasjon</skos:prefLabel>
      <skos:definition xml:lang="no">Type observasjon hvor data om datamaskinbruk blir samlet av program som kan v&#xe6;re inkludert i dataprogrammet en &#xf8;nsker informasjon om, eller kan forekomme som et eget program. Informasjon om antall brukere, m&#xe5;ten brukere samhandler med program(met/mene), hvor mye tid de bruker p&#xe5; siden, hvordan de bruker bestemte deler av en applikasjon, hvordan de navigerer fra side til side eller fra en applikasjon til en annen etc., kan bli samlet.</skos:definition>
      <skos:prefLabel xml:lang="pt">Observa&#xe7;&#xe3;o assistida por computador</skos:prefLabel>
      <skos:definition xml:lang="pt">Tipo de observa&#xe7;&#xe3;o em que os dados referentes ao uso do computador s&#xe3;o recolhidos atrav&#xe9;s de software que pode estar incorporado no pr&#xf3;prio programa do computador, ou pode constituir um programa separado. Pode ser recolhida informa&#xe7;&#xe3;o sobre o n&#xfa;mero de utilizadores, a forma como os utilizadores interagem com o(s) programa(s), quanto tempo passam numa p&#xe1;gina, como usam sec&#xe7;&#xf5;es espec&#xed;ficas de aplica&#xe7;&#xf5;es, como navegam de uma p&#xe1;gina para outra ou de uma aplica&#xe7;&#xe3;o para outra, etc.</skos:definition>
      <skos:prefLabel xml:lang="sl">Ra&#x10d;unalni&#x161;ko podprto opazovanje</skos:prefLabel>
      <skos:definition xml:lang="sl">Vrsta opazovanja, kjer se podatki o uporabi ra&#x10d;unalnika zbirajo s programsko opremo, ki se jo lahko vgradi v sam ra&#x10d;unalni&#x161;ki program ali pa predstavlja lo&#x10d;en program. Lahko se zbirajo informacije o &#x161;tevilu uporabnikov, o na&#x10d;inih interakcije uporabnikov z ra&#x10d;unalni&#x161;kim(i) programom(-mi), koliko &#x10d;asa porabijo na strani, kako uporabljajo dolo&#x10d;ene dele aplikacije, kako krmarijo po straneh ali med aplikacijami itd.</skos:definition>
      <skos:prefLabel xml:lang="sr">Posmatranje podr&#x17e;ano ra&#x10d;unarom</skos:prefLabel>
      <skos:definition xml:lang="sr">Vrsta posmatranja u kome se podaci o upotrebi ra&#x10d;unara prikupljaju softverom koji mo&#x17e;e biti ugra&#x111;en u sam ra&#x10d;unar ili mo&#x17e;e biti zaseban program. Mogu se prikupiti informacije o broju korisnika, na&#x10d;inima na koji korisnici komuniciraju sa programima, koliko vremena provode na veb stranici, kako koriste odre&#x111;ene odeljke aplikacija, kako prelaze sa stranice na stranicu ili sa jedne aplikacije na drugu, itd.</skos:definition>
      <skos:prefLabel xml:lang="sv">Datorbaserade observation</skos:prefLabel>
      <skos:definition xml:lang="sv">Observation d&#xe4;r data om datoranv&#xe4;ndning samlas in av programvara som inkluderats i ett datorprogram eller som kan vara ett separat program. Information kan samlas in om antal anv&#xe4;ndare, hur anv&#xe4;ndare interagerar med programmet, hur l&#xe4;nge de stannar p&#xe5; en sida, hur de anv&#xe4;nder best&#xe4;mda delar av program, hur de navigerar fr&#xe5;n en sida till en annan eller v&#xe4;xlar mellan program m.m.</skos:definition>
   </rdf:Description>
   <rdf:Description rdf:about="http://rdf-vocabulary.ddialliance.org/cv/ModeOfCollection/3.0.0/3cee522">
      <rdf:type rdf:resource="http://www.w3.org/2004/02/skos/core#Concept"/>
      <skos:inScheme rdf:resource="http://rdf-vocabulary.ddialliance.org/cv/ModeOfCollection/3.0.0/"/>
      <skos:notation xml:lang="en">Observation.Field.Participant</skos:notation>
      <skos:prefLabel xml:lang="en">Participant field observation</skos:prefLabel>
      <skos:definition xml:lang="en">Type of field observation in which the researcher interacts with the subjects and often plays a role in the social situation under observation.</skos:definition>
      <skos:prefLabel xml:lang="da">Feltobservation med deltager</skos:prefLabel>
      <skos:definition xml:lang="da">Type af feltobservation, hvor forskeren interagerer med subjekterne og ofte spiller en rolle i den sociale situation under observation.</skos:definition>
      <skos:prefLabel xml:lang="fi">Havainnointi: kentt&#xe4;havainnointi: osallistuva</skos:prefLabel>
      <skos:definition xml:lang="fi">Havainnointi suoritetaan luonnollisessa, kontrolloimattomassa ymp&#xe4;rist&#xf6;ss&#xe4;. Tutkija on vuorovaikutuksessa tutkittavien kanssa ja h&#xe4;nell&#xe4; on usein jokin rooli tutkinnan kohteena olevassa sosiaalisessa tilanteessa.</skos:definition>
      <skos:prefLabel xml:lang="fr">Observation participante sur le terrain</skos:prefLabel>
      <skos:definition xml:lang="fr">Type d&apos;observation sur le terrain dans lequel le chercheur interagit avec les sujets et joue souvent un r&#xf4;le dans la situation sociale sous observation.</skos:definition>
      <skos:prefLabel xml:lang="it">Osservazione partecipante sul campo</skos:prefLabel>
      <skos:definition xml:lang="it">Tipo di osservazione sul campo nella quale il ricercatore interagisce con i soggetti e spesso ricopre un ruolo nella situazione sociale sotto osservazione.</skos:definition>
      <skos:prefLabel xml:lang="no">Deltagende feltobservasjon</skos:prefLabel>
      <skos:definition xml:lang="no">Type feltobservasjon hvor forskeren samhandler og ofte spiller en rolle i de sosiale situasjonene som observeres.</skos:definition>
      <skos:prefLabel xml:lang="pt">Observa&#xe7;&#xe3;o participante </skos:prefLabel>
      <skos:definition xml:lang="pt">Tipo de observa&#xe7;&#xe3;o no trabalho de campo em que o investigador interage com os sujeitos e, muitas vezes, desempenha um papel na situa&#xe7;&#xe3;o social em observa&#xe7;&#xe3;o.</skos:definition>
      <skos:prefLabel xml:lang="sl">Opazovanje na terenu z udele&#x17e;bo</skos:prefLabel>
      <skos:definition xml:lang="sl">Vrsta opazovanja, kjer je raziskovalec v interakciji z raziskovalnim subjektom in pogosto igra vlogo v opazovani dru&#x17e;beni situaciji.</skos:definition>
      <skos:prefLabel xml:lang="sr">Terensko posmatranje sa u&#x10d;e&#x161;&#x107;em</skos:prefLabel>
      <skos:definition xml:lang="sr">Vrsta terenskog posmatranja u kome istra&#x17e;iva&#x10d; komunicira sa subjektima i &#x10d;esto igra ulogu u posmatranom socijalnom stanju.</skos:definition>
      <skos:prefLabel xml:lang="sv">Deltagande f&#xe4;ltobservation</skos:prefLabel>
      <skos:definition xml:lang="sv">F&#xe4;ltobservation d&#xe4;r forskaren interagerar med forskningsobjekten och ofta har en funktion i den sociala situation som observeras.</skos:definition>
   </rdf:Description>
   <rdf:Description rdf:about="http://rdf-vocabulary.ddialliance.org/cv/ModeOfCollection/3.0.0/8245871">
      <rdf:type rdf:resource="http://www.w3.org/2004/02/skos/core#Concept"/>
      <skos:inScheme rdf:resource="http://rdf-vocabulary.ddialliance.org/cv/ModeOfCollection/3.0.0/"/>
      <skos:notation xml:lang="en">Observation.Field.Nonparticipant</skos:notation>
      <skos:prefLabel xml:lang="en">Non-participant field observation</skos:prefLabel>
      <skos:definition xml:lang="en">Observation that is conducted in a natural, non-controlled setting without any interaction between the researcher and his/her subjects.</skos:definition>
      <skos:prefLabel xml:lang="da">Feltobservation uden deltager</skos:prefLabel>
      <skos:definition xml:lang="da">Observation, der udf&#xf8;res i en naturlig, ikke-kontrolleret ops&#xe6;tning uden nogen interaktion mellem forsker og hans/hendes subjekter.</skos:definition>
      <skos:prefLabel xml:lang="fi">Havainnointi: kentt&#xe4;havainnointi: ei-osallistuva</skos:prefLabel>
      <skos:definition xml:lang="fi">Havainnointi suoritetaan luonnollisessa, kontrolloimattomassa ymp&#xe4;rist&#xf6;ss&#xe4;. Tutkija ja tutkittavat eiv&#xe4;t ole lainkaan vuorovaikutuksessa kesken&#xe4;&#xe4;n. Kutsutaan my&#xf6;s suoraksi tai ulkopuoliseksi kentt&#xe4;havainnoinniksi.</skos:definition>
      <skos:prefLabel xml:lang="fr">Observation non-participante sur le terrain</skos:prefLabel>
      <skos:definition xml:lang="fr">Observation qui a &#xe9;t&#xe9; conduite dans une configuration naturelle et non contr&#xf4;l&#xe9;e sans aucune interaction entre le chercheur et ses sujets.</skos:definition>
      <skos:prefLabel xml:lang="it">Osservazione non partecipante sul campo</skos:prefLabel>
      <skos:definition xml:lang="it">Osservazione condotta in un ambiente naturale non controllato senza alcuna interazione tra il ricercatore e i soggetti.</skos:definition>
      <skos:prefLabel xml:lang="no">Ikke-deltagende feltobservasjon</skos:prefLabel>
      <skos:definition xml:lang="no">Observasjon som er gjennomf&#xf8;rt i et naturlig, ikke kontrollert milj&#xf8; uten interaksjon mellom forskeren og studieobjektene.</skos:definition>
      <skos:prefLabel xml:lang="pt">Observa&#xe7;&#xe3;o n&#xe3;o participante</skos:prefLabel>
      <skos:definition xml:lang="pt">Observa&#xe7;&#xe3;o que &#xe9; conduzida/realizada em ambiente natural, n&#xe3;o controlado, sem qualquer intera&#xe7;&#xe3;o entre o investigador e os sujeitos observados.</skos:definition>
      <skos:prefLabel xml:lang="sl">Opazovanje na terenu brez udele&#x17e;be</skos:prefLabel>
      <skos:definition xml:lang="sl">Opazovanje, ki se izvaja v naravnem, nekontroliranem okolju brez kakr&#x161;nekoli interakcije med raziskovalcem in njegovimi/njenimi subjekti.</skos:definition>
      <skos:prefLabel xml:lang="sr">Terensko posmatranje bez u&#x10d;e&#x161;&#x107;a</skos:prefLabel>
      <skos:definition xml:lang="sr">Posmatranje koje se izvodi u prirodnom, nekontrolisanom okru&#x17e;enju bez ikakve interakcije izme&#x111;u istra&#x17e;iva&#x10d;a i njegovih subjekata.</skos:definition>
      <skos:prefLabel xml:lang="sv">Icke-deltagande f&#xe4;ltobservation</skos:prefLabel>
      <skos:definition xml:lang="sv">Observation som utf&#xf6;rs i en naturlig, icke-kontrollerad milj&#xf6; utan interaktion mellan forskaren och dennes forskningsobjekt.</skos:definition>
   </rdf:Description>
   <rdf:Description rdf:about="http://rdf-vocabulary.ddialliance.org/cv/ModeOfCollection/3.0.0/68b02fb">
      <rdf:type rdf:resource="http://www.w3.org/2004/02/skos/core#Concept"/>
      <skos:inScheme rdf:resource="http://rdf-vocabulary.ddialliance.org/cv/ModeOfCollection/3.0.0/"/>
      <skos:notation xml:lang="en">Observation.Laboratory.Nonparticipant</skos:notation>
      <skos:prefLabel xml:lang="en">Non-participant laboratory observation</skos:prefLabel>
      <skos:definition xml:lang="en">Type of laboratory observation that is conducted without any interaction between the researcher and his/her subjects.</skos:definition>
      <skos:prefLabel xml:lang="da">Laboratorieobservation uden deltager</skos:prefLabel>
      <skos:definition xml:lang="da">Type af laboratorieobservation, der udf&#xf8;res uden nogen interaktion mellem forskeren og hans/hendes subjekter.</skos:definition>
      <skos:prefLabel xml:lang="fi">Havainnointi: laboratoriohavainnointi: ei-osallistuva</skos:prefLabel>
      <skos:definition xml:lang="fi">Kokeellinen havainnointi kontrolloidussa, tarkoitusta varten luodussa tilassa. Tutkija ei ole miss&#xe4;&#xe4;n vuorovaikutuksessa tutkittavien kanssa. Kutsutaan my&#xf6;s tarkkailevaksi laboratoriohavainnoinniksi. Esimerkki: Lasten leikkien havainnointi laboratorioon rakennetussa leikkihuoneessa, jossa tutkija ei ota osaa leikkiin.</skos:definition>
      <skos:prefLabel xml:lang="fr">Observation non-participante en laboratoire</skos:prefLabel>
      <skos:definition xml:lang="fr">Type d&apos;observation en laboratoire qui a &#xe9;t&#xe9; conduite sans aucune interaction entre le chercheur et ses sujets.</skos:definition>
      <skos:prefLabel xml:lang="it">Osservazione non partecipante in laboratorio</skos:prefLabel>
      <skos:definition xml:lang="it">Osservazione condotta in laboratorio senza alcuna interazione tra il ricercatore e i soggetti.</skos:definition>
      <skos:prefLabel xml:lang="no">Ikke-deltagende laboratorieobservasjon</skos:prefLabel>
      <skos:definition xml:lang="no">En type laboratorieobservasjon som blir gjennomf&#xf8;rt uten interaksjon mellom forskeren og studieobjektene.</skos:definition>
      <skos:prefLabel xml:lang="pt">Observa&#xe7;&#xe3;o n&#xe3;o participante em laborat&#xf3;rio</skos:prefLabel>
      <skos:definition xml:lang="pt">Tipo de observa&#xe7;&#xe3;o em laborat&#xf3;rio realizada sem qualquer intera&#xe7;&#xe3;o entre o investigador e os sujeitos observados.</skos:definition>
      <skos:prefLabel xml:lang="sl">Laboratorijsko opazovanje brez udele&#x17e;be</skos:prefLabel>
      <skos:definition xml:lang="sl">Vrsta laboratorijskega opazovanja, ki se izvaja brez kakr&#x161;nekoli interakcije med raziskovalcem in njegovimi/njenimi subjekti.</skos:definition>
      <skos:prefLabel xml:lang="sr">Laboratorijsko posmatranje bez u&#x10d;e&#x161;&#x107;a</skos:prefLabel>
      <skos:definition xml:lang="sr">Vrsta laboratorijskog posmatranja koje se sprovodi bez ikakve interakcije izme&#x111;u istra&#x17e;iva&#x10d;a i njegovih subjekata.</skos:definition>
      <skos:prefLabel xml:lang="sv">Icke-deltagande laboratorieobservation</skos:prefLabel>
      <skos:definition xml:lang="sv">Laboratorieobservation som utf&#xf6;rs utan interaktion mellan forskaren och dennes forskningsobjekt.</skos:definition>
   </rdf:Description>
   <rdf:Description rdf:about="http://rdf-vocabulary.ddialliance.org/cv/ModeOfCollection/3.0.0/05aeba4">
      <rdf:type rdf:resource="http://www.w3.org/2004/02/skos/core#Concept"/>
      <skos:inScheme rdf:resource="http://rdf-vocabulary.ddialliance.org/cv/ModeOfCollection/3.0.0/"/>
      <skos:notation xml:lang="en">Experiment</skos:notation>
      <skos:prefLabel xml:lang="en">Experiment</skos:prefLabel>
      <skos:definition xml:lang="en">Research method involving the manipulation of some or all of the independent variables included in the hypotheses.</skos:definition>
      <skos:prefLabel xml:lang="da">Eksperiment</skos:prefLabel>
      <skos:definition xml:lang="da">Forskningsmetode, der involverer manipulationen af nogle eller alle af de uafh&#xe6;ngige variabler inkludereret i hypoteserne.</skos:definition>
      <skos:prefLabel xml:lang="fi">Kontrolloitu koe</skos:prefLabel>
      <skos:definition xml:lang="fi">Tutkimusasetelma, jossa tutkimushypoteesin mukaisesti manipuloidaan yht&#xe4; tai useampaa riippumatonta muuttujaa.</skos:definition>
      <skos:prefLabel xml:lang="fr">Exp&#xe9;rimentation</skos:prefLabel>
      <skos:definition xml:lang="fr">M&#xe9;thode de recherche impliquant la manipulation d&apos;une partie ou de toutes les variables ind&#xe9;pendantes incluses dans les hypoth&#xe8;ses.</skos:definition>
      <skos:prefLabel xml:lang="it">Esperimento</skos:prefLabel>
      <skos:definition xml:lang="it">Metodo di ricerca che coinvolge la manipolazione di alcune o tutte le variabili indipendenti incluse nelle ipotesi.</skos:definition>
      <skos:prefLabel xml:lang="no">Eksperiment</skos:prefLabel>
      <skos:definition xml:lang="no">Forskningsmetode som inneb&#xe6;rer manipulering av noen eller alle de uavhengige variablene inkludert i hypotesene.</skos:definition>
      <skos:prefLabel xml:lang="pt">Estudo experimental</skos:prefLabel>
      <skos:definition xml:lang="pt">M&#xe9;todo de pesquisa que envolve a manipula&#xe7;&#xe3;o de algumas ou de todas as vari&#xe1;veis independentes inclu&#xed;das nas hip&#xf3;teses.</skos:definition>
      <skos:prefLabel xml:lang="sl">Eksperiment</skos:prefLabel>
      <skos:definition xml:lang="sl">Raziskovalna metoda, ki vklju&#x10d;uje manipulacijo nekaterih ali vseh neodvisnih spremenljivk, vklju&#x10d;enih v hipoteze.</skos:definition>
      <skos:prefLabel xml:lang="sr">Ekspertiment</skos:prefLabel>
      <skos:definition xml:lang="sr">Metoda istra&#x17e;ivanja koja uklju&#x10d;uje manipulaciju nekim ili svim nezavisnim varijablama uklju&#x10d;enim u hipoteze.</skos:definition>
      <skos:prefLabel xml:lang="sv">Experiment</skos:prefLabel>
      <skos:definition xml:lang="sv">Forskningsmetod som omfattar att styra vissa eller alla oberoende variabler som ing&#xe5;r i hypotesen.</skos:definition>
      <skos:narrower rdf:resource="http://rdf-vocabulary.ddialliance.org/cv/ModeOfCollection/3.0.0/28a60a6"/>
      <skos:narrower rdf:resource="http://rdf-vocabulary.ddialliance.org/cv/ModeOfCollection/3.0.0/5ff61de"/>
      <skos:narrower rdf:resource="http://rdf-vocabulary.ddialliance.org/cv/ModeOfCollection/3.0.0/ed0d083"/>
   </rdf:Description>
   <rdf:Description rdf:about="http://rdf-vocabulary.ddialliance.org/cv/ModeOfCollection/3.0.0/28a60a6">
      <rdf:type rdf:resource="http://www.w3.org/2004/02/skos/core#Concept"/>
      <skos:inScheme rdf:resource="http://rdf-vocabulary.ddialliance.org/cv/ModeOfCollection/3.0.0/"/>
      <skos:notation xml:lang="en">Experiment.Laboratory</skos:notation>
      <skos:prefLabel xml:lang="en">Laboratory experiment</skos:prefLabel>
      <skos:definition xml:lang="en">An experiment conducted in a controlled, artificially created physical setting, in which a researcher manipulates one or several independent variables and measures its/their effect on the dependent variable.</skos:definition>
      <skos:prefLabel xml:lang="da">Laboratorieeksperiment</skos:prefLabel>
      <skos:definition xml:lang="da">Et eksperiment udf&#xf8;rt i en kontrolleret, kunstigt skabt fysisk ops&#xe6;tning, hvor en forsker manipulerer en eller flere uafh&#xe6;ngige variabler og m&#xe5;ler dens/deres effekt p&#xe5; den afh&#xe6;ngige variabel.</skos:definition>
      <skos:prefLabel xml:lang="fi">Kontrolloitu koe: laboratoriokoe</skos:prefLabel>
      <skos:definition xml:lang="fi">Kontrolloidussa, tarkoitusta varten luodussa ymp&#xe4;rist&#xf6;ss&#xe4; suoritettu koe, jossa tutkija(t) manipuloivat yht&#xe4; tai useampaa riippumatonta muuttujaa ja mittaavat sen vaikutusta riippuvaan muuttujaan.</skos:definition>
      <skos:prefLabel xml:lang="fr">Exp&#xe9;rimentation en laboratoire</skos:prefLabel>
      <skos:definition xml:lang="fr">Une exp&#xe9;rimentation conduite dans une configuration physique contr&#xf4;l&#xe9;e, cr&#xe9;&#xe9;e artificiellement, dans laquelle un chercheur manipule une ou plusieurs variables ind&#xe9;pendantes et mesure son / leur effet sur la variable d&#xe9;pendante.</skos:definition>
      <skos:prefLabel xml:lang="it">Esperimento in laboratorio</skos:prefLabel>
      <skos:definition xml:lang="it">Un esperimento condotto in un ambiente fisico controllato, creato artificialmente, in cui un ricercatore manipola una o pi&#xf9; variabili indipendenti e misura il loro effetto sulla variabile dipendente.</skos:definition>
      <skos:prefLabel xml:lang="no">Laboratorieeksperiment</skos:prefLabel>
      <skos:definition xml:lang="no">Et eksperiment som utf&#xf8;res i et kontrollert, kunstig utformet milj&#xf8;, hvor forskeren manipulerer &#xe9;n eller flere av de uavhengige variablene og m&#xe5;ler effekten det har p&#xe5; den avhengige variabelen.</skos:definition>
      <skos:prefLabel xml:lang="pt">Estudo experimental em laborat&#xf3;rio</skos:prefLabel>
      <skos:definition xml:lang="pt">Experi&#xea;ncia/experimento conduzida/o em ambiente f&#xed;sico controlado, artificialmente criado, no qual o investigador manipula uma ou v&#xe1;rias vari&#xe1;veis independentes e mede o seu efeito sobre a vari&#xe1;vel dependente.</skos:definition>
      <skos:prefLabel xml:lang="sl">Laboratorijski eksperiment</skos:prefLabel>
      <skos:definition xml:lang="sl">Eksperiment, ki se izvaja v nadzorovanem, umetno ustvarjenem fizi&#x10d;nem okolju, v katerem raziskovalec manipulira z eno ali ve&#x10d; neodvisnimi spremenljivkami in meri svoj vpliv na odvisno spremenljivko.</skos:definition>
      <skos:prefLabel xml:lang="sr">Laboratorijski eksperiment</skos:prefLabel>
      <skos:definition xml:lang="sr">Eksperiment sproveden u kontrolisanom, ve&#x161;ta&#x10d;ki stvorenom fizi&#x10d;kom okru&#x17e;enju, u kome istra&#x17e;iva&#x10d; manipuli&#x161;e jednom ili vi&#x161;e nezavisnih varijabli i meri njen / njihov uticaj na zavisnu promenljivu.</skos:definition>
      <skos:prefLabel xml:lang="sv">Laboratorieexperiment</skos:prefLabel>
      <skos:definition xml:lang="sv">Ett experiment som utf&#xf6;rs i en kontrollerad, konstgjord fysisk milj&#xf6; d&#xe4;r forskaren styr en eller flera oberoende variabler och m&#xe4;ter dess/deras effekt p&#xe5; den beroende variabeln.</skos:definition>
   </rdf:Description>
   <rdf:Description rdf:about="http://rdf-vocabulary.ddialliance.org/cv/ModeOfCollection/3.0.0/5ff61de">
      <rdf:type rdf:resource="http://www.w3.org/2004/02/skos/core#Concept"/>
      <skos:inScheme rdf:resource="http://rdf-vocabulary.ddialliance.org/cv/ModeOfCollection/3.0.0/"/>
      <skos:notation xml:lang="en">Experiment.FieldIntervention</skos:notation>
      <skos:prefLabel xml:lang="en">Field/Intervention experiment</skos:prefLabel>
      <skos:definition xml:lang="en">An experiment conducted in a natural, uncontrolled setting, in which the researcher manipulates one or several independent variables. Intervention/clinical studies are one example of field experiments.</skos:definition>
      <skos:prefLabel xml:lang="da">Felt/Interventionseksperiment</skos:prefLabel>
      <skos:definition xml:lang="da">Et eksperiment udf&#xf8;rt i en naturlig, ukontrolleret ops&#xe6;tning, hvor forskeren manipulerer en eller flere uafh&#xe6;ngige variabler. Intervention/kliniske studier er et eksempel p&#xe5; felteksperimenter.</skos:definition>
      <skos:prefLabel xml:lang="fi">Kontrolloitu koe: kentt&#xe4;- tai interventiokoe</skos:prefLabel>
      <skos:definition xml:lang="fi">Luonnollisessa, kontrolloimattomassa ymp&#xe4;rist&#xf6;ss&#xe4; suoritettu koe, jossa tutkija(t) manipuloivat yht&#xe4; tai useampaa riippumatonta muuttujaa. Esimerkkej&#xe4;: kliiniset tutkimukset.</skos:definition>
      <skos:prefLabel xml:lang="fr">Exp&#xe9;rimentation sur le terrain</skos:prefLabel>
      <skos:definition xml:lang="fr">Une exp&#xe9;rimentation conduite dans une configuration naturelle, non contr&#xf4;l&#xe9;e, dans laquelle le chercheur manipule une ou plusieurs variables ind&#xe9;pendantes. Des &#xe9;tudes cliniques sont un exemple d&apos;exp&#xe9;rimentations sur le terrain.</skos:definition>
      <skos:prefLabel xml:lang="it">Esperimento sul campo / Intervento</skos:prefLabel>
      <skos:definition xml:lang="it">Un esperimento condotto in un ambiente naturale, non controllato, in cui il ricercatore manipola una o pi&#xf9; variabili indipendenti. Gli interventi o studi clinici sono un esempio di esperimenti sul campo.</skos:definition>
      <skos:prefLabel xml:lang="no">Felt/felteksperiment</skos:prefLabel>
      <skos:definition xml:lang="no">Et eksperiment som utf&#xf8;res i et naturlig, ukontrollert milj&#xf8;, hvor forskeren manipulerer &#xe9;n eller flere av de uavhengige variablene. Intervensjon/kliniske studier er et eksempel p&#xe5; felteksperiment.</skos:definition>
      <skos:prefLabel xml:lang="pt">Estudo experimental de campo (com interven&#xe7;&#xe3;o)</skos:prefLabel>
      <skos:definition xml:lang="pt">Experi&#xea;ncia/experimento conduzida/o em ambiente natural e n&#xe3;o controlado, no qual o investigador manipula uma ou v&#xe1;rias vari&#xe1;veis independentes. Estudos cl&#xed;nicos ou de interven&#xe7;&#xe3;o s&#xe3;o um exemplo de experimenta&#xe7;&#xf5;es de campo.</skos:definition>
      <skos:prefLabel xml:lang="sl">Terenski/intervencijski eksperiment</skos:prefLabel>
      <skos:definition xml:lang="sl">Eksperiment, ki se izvaja v naravnem, nekontroliranem okolju, v katerem raziskovalec manipulira z eno ali ve&#x10d; neodvisnimi spremenljivkami. Intervencija/klini&#x10d;ne &#x161;tudije so en primer terenskih eksperimentov.</skos:definition>
      <skos:prefLabel xml:lang="sr">Terenski ekspertiment / intervencija</skos:prefLabel>
      <skos:definition xml:lang="sr">Eksperiment sproveden u prirodnom, nekontrolisanom okru&#x17e;enju, u kome istra&#x17e;iva&#x10d; manipuli&#x161;e jednom ili vi&#x161;e nezavisnih varijabli. Interventne / klini&#x10d;ke studije su jedan primer terenskih eksperimenata.</skos:definition>
      <skos:prefLabel xml:lang="sv">F&#xe4;ltexperiment</skos:prefLabel>
      <skos:definition xml:lang="sv">Ett experiment som utf&#xf6;rs i en naturlig, okontrollerad milj&#xf6; d&#xe4;r forskaren styr en eller flera oberoende variabler. Interventionsstudier och kliniska studier &#xe4;r exempel p&#xe5; f&#xe4;ltexperiment.</skos:definition>
   </rdf:Description>
   <rdf:Description rdf:about="http://rdf-vocabulary.ddialliance.org/cv/ModeOfCollection/3.0.0/ed0d083">
      <rdf:type rdf:resource="http://www.w3.org/2004/02/skos/core#Concept"/>
      <skos:inScheme rdf:resource="http://rdf-vocabulary.ddialliance.org/cv/ModeOfCollection/3.0.0/"/>
      <skos:notation xml:lang="en">Experiment.WebBased</skos:notation>
      <skos:prefLabel xml:lang="en">Web-based experiment</skos:prefLabel>
      <skos:definition xml:lang="en">An experiment conducted in the virtual setting of the World Wide Web, in which experimental materials are programmed to implement artificial situations or events to be investigated in a distributed environment. (Reips, U.-D. (2002). Theory and techniques of Web experimenting. In B. Batinic, U.-D. Reips, &amp; M. Bosnjak (Eds.), Online Social Sciences. Seattle: Hogrefe &amp; Huber. Available at: http://www.websm.org/uploadi/editor/Reips_2002_Theory_and_techniques.pdf [07 June 2013])</skos:definition>
      <skos:prefLabel xml:lang="da">Webbaseret eksperiment</skos:prefLabel>
      <skos:definition xml:lang="da">Et eksperiment udf&#xf8;rt i den virtuelle ops&#xe6;tning p&#xe5; World Wibe Web, hvor eksperimentelle materialer er programmeret til at implementere kunstige situationer eller begivenheder, der skal unders&#xf8;ges i et spredt milj&#xf8;. (Reips, U.-D. (2002). Theory and techniques of Web experimenting. In B. Batinic, U.-D. Reips, &amp; M. Bosnjak (Eds.), Online Social Sciences. Seattle: Hogrefe &amp; Huber. Available at: http://www.websm.org/uploadi/editor/Reips_2002_Theory_and_techniques.pdf [07 June 2013])</skos:definition>
      <skos:prefLabel xml:lang="fi">Kontrolloitu koe: virtuaalinen koe</skos:prefLabel>
      <skos:definition xml:lang="fi">Internetiss&#xe4; toteutettu kokeellinen tutkimus, jossa on ohjelmallisesti luotu keinotekoisia virtuaalisia ymp&#xe4;rist&#xf6;j&#xe4; tai tapahtumia tutkimusta varten. Esimerkki: Keinotekoisen kielen oppimiskoe, virtuaalisen pelik&#xe4;ytt&#xe4;ytymisen koe.</skos:definition>
      <skos:prefLabel xml:lang="fr">Exp&#xe9;rimentation par Internet</skos:prefLabel>
      <skos:definition xml:lang="fr">Une exp&#xe9;rimentation conduite dans une configuration virtuelle du Web, dans laquelle des mat&#xe9;riaux exp&#xe9;rimentaux sont programm&#xe9;s pour mettre en &#x153;uvre des situations ou des &#xe9;v&#xe8;nements artificiels pour &#xea;tre &#xe9;tudi&#xe9;s dans un environnement distribu&#xe9;. (Reips, U.-D. (2002). Theory and techniques of Web experimenting. In B. Batinic, U.-D. Reips, &amp;amp; M. Bosnjak (Eds.), Online Social Sciences. Seattle: Hogrefe &amp;amp; Huber. Available at: http://www.websm.org/uploadi/editor/Reips_2002_Theory_and_techniques.pdf [07 June 2013])</skos:definition>
      <skos:prefLabel xml:lang="it">Esperimento web</skos:prefLabel>
      <skos:definition xml:lang="it">Un esperimento condotto nell&apos;ambiente virtuale del World Wide Web, in cui i materiali sperimentali sono programmati per ricreare situazioni o eventi artificiali da indagare in un ambiente distribuito.</skos:definition>
      <skos:prefLabel xml:lang="no">Webbasert eksperiment</skos:prefLabel>
      <skos:definition xml:lang="no">Et eksperiment som utf&#xf8;res i et vituelt milj&#xf8; p&#xe5; internett (World Wide Web), hvor eksperimentelt materiale er programmert til &#xe5; sette i gang kunstige situasjoner eller hendelser som kan unders&#xf8;kes i et gitt milj&#xf8;. (Reips, U.-D. (2002). Theory and techniques of Web experimenting. In B. Batinic, U.-D. Reips, &amp; M. Bosnjak (Eds.), Online Social Sciences. Seattle: Hogrefe &amp; Huber. Available at: http://www.websm.org/uploadi/editor/Reips_2002_Theory_and_techniques.pdf [07 June 2013])</skos:definition>
      <skos:prefLabel xml:lang="pt">Estudo experimental online/via web</skos:prefLabel>
      <skos:definition xml:lang="pt">Experi&#xea;ncia/experimento conduzida/o em ambiente virtual da World Wide Web, no qual materiais experimentais s&#xe3;o programados para implementar situa&#xe7;&#xf5;es ou eventos artificiais para pesquisa num ambiente distribu&#xed;do. (Reips, U.-D. (2002). Theory and techniques of Web experimenting. In B. Batinic, U.-D. Reips, &amp;amp; M. Bosnjak (Eds.), Online Social Sciences. Seattle: Hogrefe &amp;amp; Huber. Dispon&#xed;vel em: http://www.websm.org/uploadi/editor/Reips_2002_Theory_and_techniques.pdf [07 June 2013])</skos:definition>
      <skos:prefLabel xml:lang="sl">Spletni eksperiment</skos:prefLabel>
      <skos:definition xml:lang="sl">Eksperiment, ki se izvaja v virtualnem okolju svetovnega spleta, v katerem so eksperimentalni materiali programirani za izvajanje umetnih situacij ali dogodkov, ki jih je treba raziskati v porazdeljenem okolju.</skos:definition>
      <skos:prefLabel xml:lang="sr">Ekspertiment na vebu</skos:prefLabel>
      <skos:definition xml:lang="sr">Eksperiment sproveden u virtuelnom okru&#x17e;enju World Wide Web-a, u kome se eksperimentalni materijali programiraju za primenu ve&#x161;ta&#x10d;kih situacija ili doga&#x111;aja koji se istra&#x17e;uju u distribuisanoj sredini. (Reips, U.D. (2002). Teorija i tehnike veb eksperimentiranja. U B. Batinic, U.D. Reips i M. Bosnjak (ur.), Online Social Sciences. Seattle: Hogrefe &amp;amp; Huber. Dostupno na: http://www.websm.org/uploadi/editor/Reips_2002_Theori_and_techniques.pdf [07. juni 2013.])</skos:definition>
      <skos:prefLabel xml:lang="sv">Webbaserat experiment</skos:prefLabel>
      <skos:definition xml:lang="sv">Ett experiment som utf&#xf6;rs i en virtuell milj&#xf6; p&#xe5; webben, d&#xe4;r experimentella material programmeras f&#xf6;r att skapa artificiella situationer eller h&#xe4;ndelser som unders&#xf6;ks i en distribuerad milj&#xf6;.  (Reips, U.-D. (2002). Theory and techniques of Web experimenting. In B. Batinic, U.-D. Reips, &amp; M. Bosnjak (Eds.), Online Social Sciences. Seattle: Hogrefe &amp; Huber. Tillg&#xe4;nglig: http://www.websm.org/uploadi/editor/Reips_2002_Theory_and_techniques.pdf [8 september, 2016])</skos:definition>
   </rdf:Description>
   <rdf:Description rdf:about="http://rdf-vocabulary.ddialliance.org/cv/ModeOfCollection/3.0.0/c5564d2">
      <rdf:type rdf:resource="http://www.w3.org/2004/02/skos/core#Concept"/>
      <skos:inScheme rdf:resource="http://rdf-vocabulary.ddialliance.org/cv/ModeOfCollection/3.0.0/"/>
      <skos:notation xml:lang="en">Recording</skos:notation>
      <skos:prefLabel xml:lang="en">Recording</skos:prefLabel>
      <skos:definition xml:lang="en">Registering by mechanical or electronic means, in a form that allows the information to be retrieved and/or reproduced. For example, images or sounds on disc or magnetic tape.</skos:definition>
      <skos:prefLabel xml:lang="da">Optagelse</skos:prefLabel>
      <skos:definition xml:lang="da">Registrering p&#xe5; mekanisk eller elektronisk vis i en form, der muligg&#xf8;r, at information kan genfindes og/eller genskabes. For eksempel billeder eller lyd p&#xe5; disk eller magnetb&#xe5;nd.</skos:definition>
      <skos:prefLabel xml:lang="fi">Taltiointi</skos:prefLabel>
      <skos:definition xml:lang="fi">Aineiston taltioiminen mekaanisesti tai elektronisesti tavalla, joka mahdollistaa sen kuuntelun, katselun tai monistamisen. Sis&#xe4;lt&#xe4;&#xe4; mm. valokuvien, videon tai &#xe4;&#xe4;nen taltioimisen. Esimerkki: Kokousten tai vastaanottojen videoiminen ilman tutkijan l&#xe4;sn&#xe4;oloa, valokuvista muodostuva aineisto.</skos:definition>
      <skos:prefLabel xml:lang="fr">Enregistrement</skos:prefLabel>
      <skos:definition xml:lang="fr">Enregistrement par des moyens m&#xe9;caniques ou &#xe9;lectroniques, sous une forme qui permet que les informations soient r&#xe9;cup&#xe9;r&#xe9;es et / ou reproduites. Par exemple, des images ou des sons sur disque ou bande magn&#xe9;tique.</skos:definition>
      <skos:prefLabel xml:lang="it">Registrazione</skos:prefLabel>
      <skos:definition xml:lang="it">Registrazione tramite mezzi meccanici o elettronici, in una forma che consente di recuperare e/o riprodurre le informazioni. Ad esempio, registrazioni di immagini o suoni su disco o supporto magnetico.</skos:definition>
      <skos:prefLabel xml:lang="no">Opptak</skos:prefLabel>
      <skos:definition xml:lang="no">Mekanisk eller elektronisk registrering i et format som gj&#xf8;r det mulig &#xe5; gjeninnhente og/eller gjenskape informasjonen. For eksempel bilder eller lyd p&#xe5; disk eller magnetb&#xe5;nd.</skos:definition>
      <skos:prefLabel xml:lang="pt">Grava&#xe7;&#xe3;o</skos:prefLabel>
      <skos:definition xml:lang="pt">Registo por meios mec&#xe2;nicos ou electr&#xf3;nicos, de forma a permitir que a informa&#xe7;&#xe3;o seja recuperada e/ou reproduzida. Por exemplo, imagens ou sons em disco ou fita magn&#xe9;tica.</skos:definition>
      <skos:prefLabel xml:lang="sl">Snemanje</skos:prefLabel>
      <skos:definition xml:lang="sl">Snemanje z mehanskimi ali elektronskimi sredstvi v obliki, ki omogo&#x10d;a, da se informacije prikli&#x10d;ejo in/ali reproducirajo. Na primer slike ali zvoki na disku ali magnetnem traku.</skos:definition>
      <skos:prefLabel xml:lang="sr">Snimanje</skos:prefLabel>
      <skos:definition xml:lang="sr">Registrovanje mehani&#x10d;kim ili elektronskim sredstvima, u obliku koji omoguc&#x301;ava preuzimanje i / ili reprodukciju informacija. Na primer, slike ili zvukovi na disku ili magnetnoj traci.</skos:definition>
      <skos:prefLabel xml:lang="sv">Inspelning</skos:prefLabel>
      <skos:definition xml:lang="sv">Upptagning, p&#xe5; mekanisk eller elektronisk v&#xe4;g, p&#xe5; s&#xe5;dant s&#xe4;tt att informationen kan &#xe5;terf&#xe5;s och/eller &#xe5;terskapas. Exempel: bilder eller ljud p&#xe5; en cd eller ett magnetband.</skos:definition>
   </rdf:Description>
   <rdf:Description rdf:about="http://rdf-vocabulary.ddialliance.org/cv/ModeOfCollection/3.0.0/4848ed5">
      <rdf:type rdf:resource="http://www.w3.org/2004/02/skos/core#Concept"/>
      <skos:inScheme rdf:resource="http://rdf-vocabulary.ddialliance.org/cv/ModeOfCollection/3.0.0/"/>
      <skos:notation xml:lang="en">ContentCoding</skos:notation>
      <skos:prefLabel xml:lang="en">Content coding</skos:prefLabel>
      <skos:definition xml:lang="en">As a mode of secondary data collection, content coding applies coding techniques to transform qualitative data (textual, video, audio or still-image) originally produced for other purposes into quantitative data (expressed in unit-by-variable matrices) in accordance with pre-defined categorization schemes. For example, coded party manifesto data like the &quot;European Parliament Election Study 2009, Manifesto Study&quot; (doi:10.4232/1.10204).</skos:definition>
      <skos:prefLabel xml:lang="da">Indholdskodning</skos:prefLabel>
      <skos:definition xml:lang="da">Som en metode til sekund&#xe6;r dataindsamling anvender indholdskodning kodningsteknikker til at transformere kvalitative data (tekst, video, lyd eller stillbilleder), der oprindeligt blev produceret til andre form&#xe5;l, til kvantitative data (udtrykt ved enhed-til-variabel-matricer) i overensstemmelse med forh&#xe5;ndsdefinerede kategoriseringsskemaer. For eksempel, kodede partimanifestdata som &quot;European Parliament Election Study 2009, Manifesto Study&quot; (doi:10.4232/1.10204).</skos:definition>
      <skos:prefLabel xml:lang="fi">Sis&#xe4;ll&#xf6;nkoodaus</skos:prefLabel>
      <skos:definition xml:lang="fi">Jo olemassa olevasta, alun perin toisiin tarkoituksiin luodusta kvalitatiivisesta aineistosta (esim. tekstiaineistot, &#xe4;&#xe4;ni- ja kuvatiedostot, valokuvat) muodostetaan kvantitatiivinen aineisto (matriisi) sovittua koodausohjetta k&#xe4;ytt&#xe4;en. Esimerkki: sanomalehtiartikkeleiden sis&#xe4;ll&#xf6;n luokittelu annettujen kriteerien mukaan.</skos:definition>
      <skos:prefLabel xml:lang="fr">Codage de contenu</skos:prefLabel>
      <skos:definition xml:lang="fr">Comme un mode secondaire de collecte de donn&#xe9;es, le codage de contenu applique des techniques de codage pour transformer des donn&#xe9;es qualitatives (textuel, vid&#xe9;o, audio, ou image fixe) originalement produites &#xe0; d&apos;autres finalit&#xe9;s en donn&#xe9;es quantitatives (exprim&#xe9;es dans des matrices unit&#xe9;-par-variable) en accord avec des sch&#xe9;mas de cat&#xe9;gorisations pr&#xe9;d&#xe9;finis. Par exemple, les donn&#xe9;es recod&#xe9;es des programmes des partis politiques comme les &quot;L&apos;&#xc9;tude &#xe9;lectorale du parlement europ&#xe9;ens 2019, &#xe9;tude des programmes&quot; (doi:10.4232/1.10204).</skos:definition>
      <skos:prefLabel xml:lang="it">Codifica del contenuto</skos:prefLabel>
      <skos:definition xml:lang="it">Metodo di raccolta secondaria dei dati, in cui si applicano le tecniche di codifica del contenuto per trasformare dati qualitativi originariamente prodotti per altri scopi (testi, video, audio o immagini) in dati quantitativi (espressi in forma di matrici) secondo schemi di categorizzazione definiti. Ad esempio, codifica dei dati relativi ai manifesti di partito, come il &quot;European Parliament Election Study 2009, Manifesto Study&quot; (doi:10.4232/1.10204)</skos:definition>
      <skos:prefLabel xml:lang="no">Innholdskoding</skos:prefLabel>
      <skos:definition xml:lang="no">Som metode for sekund&#xe6;r datainnsamling, innholdskoding omfatter kodeteknikker for &#xe5; omgj&#xf8;re kvalitative data (tekst, video, lyd eller bilde), som opprinnelig var utarbeidet for andre form&#xe5;l, til kvantitative data (uttrykket i en matrise med enheter og variabler) i henhold til bestemte kategoriseringssystem. For eksempel, kodede partimanifesto som i &apos;European Parliament Election Study 2009, Manifesto Study&apos; (doi:10.4232/1.10204).</skos:definition>
      <skos:prefLabel xml:lang="pt">Codifica&#xe7;&#xe3;o de conte&#xfa;do</skos:prefLabel>
      <skos:definition xml:lang="pt">Como modo de recolha de dados secund&#xe1;rios, a codifica&#xe7;&#xe3;o de conte&#xfa;do aplica t&#xe9;cnicas de codifica&#xe7;&#xe3;o para transformar dados qualitativos (textual, v&#xed;deo, &#xe1;udio ou imagem parada) originalmente produzidos para outros prop&#xf3;sitos em dados quantitativos (expressos em matrizes unidade-por-vari&#xe1;vel) de acordo com esquemas de categoriza&#xe7;&#xe3;o predefinidos. Por exemplo, dados codificados de um programa de partido pol&#xed;tico, como o &quot;European Parliament Election Study 2009, Manifesto Study&quot; (doi:10.4232/1.10204).</skos:definition>
      <skos:prefLabel xml:lang="sl">Kodiranje vsebine</skos:prefLabel>
      <skos:definition xml:lang="sl">Kot na&#x10d;in sekundarnega zbiranja podatkov, kodiranje vsebine uporablja kodirne tehnike za preoblikovanje kvalitativnih podatkov (besedilni podatki, video, avdio ali mirujo&#x10d;e slike), ki so bili prvotno ustvarjeni za druge namene, v kvantitativne podatke (izra&#x17e;ene z matricami enot po spremenljivkah) v skladu s vnaprej opredeljenimi kategorizacijskimi shemami. Na primer, kodiranje manifestov politi&#x10d;nih strank, kot npr. &#x161;tudija o volitvah v Evropski parlament 2009.</skos:definition>
      <skos:prefLabel xml:lang="sr">Kodiranje sadr&#x17e;aja</skos:prefLabel>
      <skos:definition xml:lang="sr">Kao na&#x10d;in sekundarnog prikupljanja podataka, kodiranje sadr&#x17e;aja primenjuje tehnike kodiranja kako bi se kvalitativni podaci (tekstualni, video, audio ili nepokretni snimci) prvobitno proizvedeni u druge svrhe pretvorili u kvantitativne podatke u skladu sa prethodno definisanom &#x161;emom kategorizacije. Na primer, podaci o manifestu kodiranih strana poput &quot;European Parliament Election Study 2009, Manifesto Study&quot; (doi:10.4232/1.10204)&quot;.</skos:definition>
      <skos:prefLabel xml:lang="sv">Kodning av inneh&#xe5;ll</skos:prefLabel>
      <skos:definition xml:lang="sv">Som en metod f&#xf6;r sekund&#xe4;r datainsamling till&#xe4;mpar inneh&#xe5;llskodning  kodningstekniker f&#xf6;r att omvandla kvalitativa data (text-, ljud-, video-, eller stillbildsdata) som ursprungligen skapats f&#xf6;r andra syften till kvantitativa data (uttryckta i en matris med enheter och variabler) enligt f&#xf6;rdefinierade kategoriseringsscheman. Exempel: kodade partiprogramsdata som i &quot;European Parliament Election Study 2009, Manifesto Study&quot; (DOI: 10.4232/1.10204).</skos:definition>
   </rdf:Description>
   <rdf:Description rdf:about="http://rdf-vocabulary.ddialliance.org/cv/ModeOfCollection/3.0.0/df9aac3">
      <rdf:type rdf:resource="http://www.w3.org/2004/02/skos/core#Concept"/>
      <skos:inScheme rdf:resource="http://rdf-vocabulary.ddialliance.org/cv/ModeOfCollection/3.0.0/"/>
      <skos:notation xml:lang="en">Transcription</skos:notation>
      <skos:prefLabel xml:lang="en">Transcription</skos:prefLabel>
      <skos:definition xml:lang="en">Capturing information in writing from a different source, or from a different medium, alphabet, or form of notation, like scientific formulae, or musical notes. For transcribed interviews or observations, it is recommended to document the primary mode of collection, using one of the interview or observation terms.</skos:definition>
      <skos:prefLabel xml:lang="da">Transskription</skos:prefLabel>
      <skos:definition xml:lang="da">Indfangning af skriftlige oplysninger fra en anden kilde eller fra et andet medium, alfabet eller form for notation, s&#xe5;som videnskabelige formler eller musikalske noder. For transskriberede interviews eller observationer anbefales det at dokumentere den prim&#xe6;re indsamlingsform ved brug af et af interview- eller observationsbetingelserne.</skos:definition>
      <skos:prefLabel xml:lang="fi">Litterointi</skos:prefLabel>
      <skos:definition xml:lang="fi">Informaation siirt&#xe4;minen k&#xe4;sin kirjaamalla toisesta l&#xe4;hteest&#xe4; tai toisesta formaatista, muodosta tai aakkosj&#xe4;rjestelm&#xe4;st&#xe4;. Esimerkki: Musiikin esitt&#xe4;minen nuotteina, kemialliset kaavat. Jos aineisto muodostuu havaintomuistiinpanoista tai haastattelulitteroinneista, suositellaan kuvattavaksi ensisijainen keruumenetelm&#xe4; k&#xe4;ytt&#xe4;m&#xe4;ll&#xe4; sopivaa havainnointi- tai haastattelutermi&#xe4;.</skos:definition>
      <skos:prefLabel xml:lang="fr">Transcription</skos:prefLabel>
      <skos:definition xml:lang="fr">Collecte des informations par &#xe9;crit &#xe0; partir d&apos;une source diff&#xe9;rente, ou &#xe0; partir d&apos;un support diff&#xe9;rent, d&apos;un alphabet, ou d&apos;une forme de notation, comme des formules scientifiques, ou des notes de musique. Pour des entretiens ou des observations transcrits, il est recommand&#xe9; de documenter le mode de collecte initial, en utilisant l&apos;un des termes propres &#xe0; l&apos;entretien ou &#xe0; l&apos;observation.</skos:definition>
      <skos:prefLabel xml:lang="it">Trascrizione</skos:prefLabel>
      <skos:definition xml:lang="it">Raccolta di informazioni per iscritto da un&apos;altra fonte, o da un altro mezzo, alfabeto o forma di notazione, come formule scientifiche o note musicali. Per le interviste o le osservazioni trascritte, si consiglia di documentare la modalit&#xe0; di raccolta dei dati utilizzando uno dei termini del vocabolario relativi all&apos;intervista o all&apos;osservazione.</skos:definition>
      <skos:prefLabel xml:lang="no">Transkripsjon</skos:prefLabel>
      <skos:definition xml:lang="no">Nedtegning av informasjon i skrift fra en annen kilde, eller et annet medium, alfabet, eller fra notasjoner, som vitenskapelige formler, eller musikknoter. For transkriberte intervju eller observasjoner er det anbefalt &#xe5; dokumentere den opprinnelige formen for datainnsamling, ved &#xe5; bruke et av intervju- eller observasjonsbegrepene.</skos:definition>
      <skos:prefLabel xml:lang="pt">Transcri&#xe7;&#xe3;o</skos:prefLabel>
      <skos:definition xml:lang="pt">Recolha de informa&#xe7;&#xf5;es por escrito de uma fonte diferente ou atrav&#xe9;s de um meio diferente, alfabeto ou forma de anota&#xe7;&#xe3;o, como f&#xf3;rmulas cient&#xed;ficas ou notas musicais. Para entrevistas ou observa&#xe7;&#xf5;es transcritas, recomenda-se documentar o modo de recolha principal, usando um dos termos no &#xe2;mbito dos t&#xf3;picos mais gerais &apos;entrevista&apos; ou &apos;observa&#xe7;&#xe3;o&apos;.</skos:definition>
      <skos:prefLabel xml:lang="sl">Prepis</skos:prefLabel>
      <skos:definition xml:lang="sl">Zajemanje podatkov v pisni obliki iz drugega vira ali iz drugega medija, abecede, ali oblika zapisa, kot so znanstvene formule ali glasbene note. Pri transkriptih intervjujev ali opazovanj je priporo&#x10d;ljivo dokumentirati primarni na&#x10d;in zbiranja podatkov z uporabo enega od razgovornih ali opazovalnih pogojev.</skos:definition>
      <skos:prefLabel xml:lang="sr">Transkripcija</skos:prefLabel>
      <skos:definition xml:lang="sr">Obuhvat podataka u pisanom obliku iz drugog izvora ili iz drugog medija, pisma ili oblika notacije, poput nau&#x10d;nih formula ili muzi&#x10d;kih nota. Za prepisane intervjue ili zapa&#x17e;anja preporu&#x10d;uje se dokumentovanje primarnog na&#x10d;ina prikupljanja, koristec&#x301;i jedan od termina intervjua ili opservacije.</skos:definition>
      <skos:prefLabel xml:lang="sv">Transkription</skos:prefLabel>
      <skos:definition xml:lang="sv">Att nedteckna information fr&#xe5;n en annan k&#xe4;lla eller fr&#xe5;n ett annat medium, alfabet eller notationssystem, som till exempel vetenskapliga formler eller noter f&#xf6;r musik. F&#xf6;r transkriberade intervjuer och observationer rekommenderas det att man dokumenterar den prim&#xe4;ra insamlingsmetoden med n&#xe5;gon av termerna f&#xf6;r intervjuer eller observationer.</skos:definition>
   </rdf:Description>
   <rdf:Description rdf:about="http://rdf-vocabulary.ddialliance.org/cv/ModeOfCollection/3.0.0/6decc77">
      <rdf:type rdf:resource="http://www.w3.org/2004/02/skos/core#Concept"/>
      <skos:inScheme rdf:resource="http://rdf-vocabulary.ddialliance.org/cv/ModeOfCollection/3.0.0/"/>
      <skos:notation xml:lang="en">CompilationSynthesis</skos:notation>
      <skos:prefLabel xml:lang="en">Compilation/Synthesis</skos:prefLabel>
      <skos:definition xml:lang="en">Collecting and assembling data from multiple, often heterogeneous sources that have one or more reference points in common, and at least one of the sources was originally produced for other purposes. The data are incorporated in a new entity. For example, providing data on the number of universities in the last 150 years using a variety of available sources (e.g. finance documents, official statistics, university registers), combining survey data with information about geographical areas from official statistics (e.g. population density, doctors per capita, etc.), or using RSS to collect blog posts or tweets, etc.</skos:definition>
      <skos:prefLabel xml:lang="da">Kompilering/Syntese</skos:prefLabel>
      <skos:definition xml:lang="da">Indsamling og samling af data fra flere, ofte heterogene, kilder, der har en eller flere referencepunkter til f&#xe6;lles, og mindst en af kilderne oprindeligt blev produceret til andre form&#xe5;l. Dataene inkorporeres i en ny enhed. For eksempel, give data om antallet af universiteter i de sidste 150 &#xe5;r ved brug af en r&#xe6;kke af tilg&#xe6;ngelige kilder (f.eks. finansielle dokumenter, officielle statistikker, universitetsregistre), kombinere unders&#xf8;gelsesdata med oplysninger om geografiske omr&#xe5;der fra officielle statistikker (f.eks. befolkningst&#xe6;thed, l&#xe6;ger pr. indbygger etc.) eller brug af RSS til at indsamle blogindl&#xe6;g eller tweets mm.</skos:definition>
      <skos:prefLabel xml:lang="fi">Kooste- tai synteesiaineisto</skos:prefLabel>
      <skos:definition xml:lang="fi">Tietojen ker&#xe4;&#xe4;minen ja kokoaminen useista, usein heterogeenisist&#xe4; l&#xe4;hdemateriaaleista, joilla yksi tai useampi yhteinen referenssi. Ainakin yksi l&#xe4;hteist&#xe4; on olemassa valmiina jo ennest&#xe4;&#xe4;n muita tarkoituksia varten. Ker&#xe4;tyt tiedot yhdistet&#xe4;&#xe4;n uudeksi tutkimusaineistoksi. Esimerkkej&#xe4;: Tiedon ker&#xe4;&#xe4;minen suomalaisten yliopistojen historiasta k&#xe4;ytt&#xe4;m&#xe4;ll&#xe4; monia eri l&#xe4;hteit&#xe4;, tai kyselytutkimuksen tietojen yhdist&#xe4;minen muista tietol&#xe4;hteist&#xe4; saatuihin tietoihin.</skos:definition>
      <skos:prefLabel xml:lang="fr">Compilation / synth&#xe8;se</skos:prefLabel>
      <skos:definition xml:lang="fr">Collecte et assemblage de donn&#xe9;es depuis de multiples sources souvent h&#xe9;t&#xe9;rog&#xe8;nes qui ont un ou plusieurs points de r&#xe9;f&#xe9;rence en commun, et dont au moins une des sources a &#xe9;t&#xe9; produite &#xe0; l&apos;origine &#xe0; d&apos;autres fins. Les donn&#xe9;es sont incorpor&#xe9;es dans une nouvelle entit&#xe9;. Par exemple, fournir des donn&#xe9;es sur le nombre d&apos;universit&#xe9;s au cours des 150 derni&#xe8;res ann&#xe9;es utilisant une vari&#xe9;t&#xe9; de sources disponibles (e. g. des documents financiers, des statistiques officielles, des registres universitaires), en combinant les donn&#xe9;es d&apos;enqu&#xea;te avec des informations sur les zones g&#xe9;ographiques provenant des statistiques officielles (e. g. la densit&#xe9; de population, m&#xe9;decins par habitants, etc.), ou en utilisant RSS pour collecter des articles de blogs ou des tweets, etc.</skos:definition>
      <skos:prefLabel xml:lang="it">Raccolta/sintesi</skos:prefLabel>
      <skos:definition xml:lang="it">Raccolta e assemblaggio di dati da pi&#xf9; fonti, spesso eterogenee, che hanno uno o pi&#xf9; punti di riferimento in comune, e dove almeno una delle fonti sia stata originariamente prodotta per altri scopi di ricerca. I dati sono incorporati in una nuova base di dati. Ad esempio, la raccolta di dati sul numero di universit&#xe0; negli ultimi 150 anni attraverso diverse fonti disponibili (ad esempio documenti finanziari, statistiche ufficiali, registri universitari), successivamente combinati con le statistiche ufficiali relative alle aree geografiche (ad es. densit&#xe0; di popolazione, medici pro-capite, ecc.) o tramite RSS per raccogliere post o tweet del blog, ecc.</skos:definition>
      <skos:prefLabel xml:lang="no">Kompilering/Syntese</skos:prefLabel>
      <skos:definition xml:lang="no">Innsamling og sammensetting av data fra flere, ofte heterogene, kilder som har en eller flere felles referansepunkter, og minst &#xe9;n av kildene var opprinnelig utarbeidet for andre form&#xe5;l. Dataene blir integrert i en ny enhet. For eksempel utarbeide data om antallet universitet de siste 150 &#xe5;rene ved &#xe5; bruke flere tilgjengelige kilder (e.g. finansdokumenter, offisiell statistikk, universitetsregistre), kombinere sp&#xf8;rreunders&#xf8;kelsesdata med informasjon om geografiske omr&#xe5;der fra offisiell statistikk (e.g. befolkningstetthet, antall leger per innbygger, etc.), eller bruke RSS for &#xe5; samle blogginnlegg eller tweets etc.</skos:definition>
      <skos:prefLabel xml:lang="pt">Compila&#xe7;&#xe3;o/s&#xed;ntese</skos:prefLabel>
      <skos:definition xml:lang="pt">Recolha e compila&#xe7;&#xe3;o de dados de fontes m&#xfa;ltiplas, muitas vezes heterog&#xe9;neas, que possuem um ou mais pontos de refer&#xea;ncia em comum, e pelo menos uma das fontes foi originalmente produzida para outras finalidades. Os dados s&#xe3;o incorporados numa nova entidade. Por exemplo, providenciar dados sobre o n&#xfa;mero de universidades nos &#xfa;ltimos 150 anos usando uma variedade de fontes dispon&#xed;veis (por exemplo, documentos financeiros, estat&#xed;sticas oficiais, registos universit&#xe1;rios), combinando dados de inqu&#xe9;ritos com informa&#xe7;&#xf5;es sobre &#xe1;reas geogr&#xe1;ficas a partir de estat&#xed;sticas oficiais (por exemplo, densidade populacional, m&#xe9;dicos per capita, etc.), ou usando o RSS (Really Simple Syndication) para recolher publica&#xe7;&#xf5;es de blogs ou tweets, etc.</skos:definition>
      <skos:prefLabel xml:lang="sl">Kompilacija/sinteza</skos:prefLabel>
      <skos:definition xml:lang="sl">Zbiranje in sestavljanje podatkov iz ve&#x10d;, pogosto heterogenih virov, ki imajo eno ali ve&#x10d; skupnih referen&#x10d;nih to&#x10d;k in kjer je bil vsaj eden od virov prvotno produciran v druge namene. Podatki so vklju&#x10d;eni v novo entiteto. Na primer z zagotavljanjem podatkov o &#x161;tevilu univerz v zadnjih 150 letih z uporabo razli&#x10d;nih razpolo&#x17e;ljivih virov (npr. finan&#x10d;ni dokumenti, uradne statistike, univerzitetni registri), kombiniranjem anketnih podatkov z informacijami o geografskih obmo&#x10d;jih iz uradnih statisti&#x10d;nih podatkov (npr. gostota prebivalstva, &#x161;tevilo zdravnikov na prebivalca itd.) ali z uporabo RSS za zbiranje objav bloga ali tvitov itd.</skos:definition>
      <skos:prefLabel xml:lang="sr">Kompilacija / sinteza</skos:prefLabel>
      <skos:definition xml:lang="sr">Prikupljanje i objedinjavanje podataka iz vi&#x161;e, &#x10d;esto heterogenih izvora koji imaju jednu ili vi&#x161;e referentnih ta&#x10d;aka, a bar jedan izvor originalno je proizveden u druge svrhe. Podaci su ugra&#x111;eni u novi entitet. Na primer, pru&#x17e;anje podataka o broju univerziteta u poslednjih 150 godina koristec&#x301;i razne dostupne izvore (npr. finansijska dokumenta, zvani&#x10d;na statistika, univerzitetski registri), kombinujuc&#x301;i podatke ankete sa podacima o geografskim oblastima iz zvani&#x10d;ne statistike (npr. gustina naseljenosti, broj lekara po glavi stanovnika itd.) ili koristec&#x301;i RSS za prikupljanje postova na blogovima ili tvitova, itd.</skos:definition>
      <skos:prefLabel xml:lang="sv">Kompilering/Syntes</skos:prefLabel>
      <skos:definition xml:lang="sv">Att samla in och sammanst&#xe4;lla data fr&#xe5;n flera, ofta heterogena, k&#xe4;llor som har en eller flera gemensamma referenspunkter, och d&#xe4;r minst en av k&#xe4;llorna ursprungligen producerades f&#xf6;r andra syften. Datamaterialet har inf&#xf6;rlivats i ett nytt material. Exempel: data om antalet universitet under de senaste 150 &#xe5;ren som tas fram med hj&#xe4;lp av ett antal olika k&#xe4;llor (t.ex. r&#xe4;kenskaper, offentlig statistik och universitetsrullor); en kombination av surveydata med information om geografiska omr&#xe5;den fr&#xe5;n offentlig statistik (t.ex. befolkningst&#xe4;thet, l&#xe4;kare per capita osv); eller bloggposter, tweetar, m.m. som samlats in med hj&#xe4;lp av RSS.</skos:definition>
   </rdf:Description>
   <rdf:Description rdf:about="http://rdf-vocabulary.ddialliance.org/cv/ModeOfCollection/3.0.0/2906121">
      <rdf:type rdf:resource="http://www.w3.org/2004/02/skos/core#Concept"/>
      <skos:inScheme rdf:resource="http://rdf-vocabulary.ddialliance.org/cv/ModeOfCollection/3.0.0/"/>
      <skos:notation xml:lang="en">Summary</skos:notation>
      <skos:prefLabel xml:lang="en">Summary</skos:prefLabel>
      <skos:definition xml:lang="en">Presentation of information in a condensed form, by reducing it to its main points. For example, abstracts of interviews or reports that are published and used as data rather than the full-length interviews or reports.</skos:definition>
      <skos:prefLabel xml:lang="da">Resum&#xe9;</skos:prefLabel>
      <skos:definition xml:lang="da">Pr&#xe6;sentation af oplysninger i kondenseret form, ved at reducere den til dens hovedpunkter. For eksempel abstracts af interviews eller reporter, der publiceres og anvendes som data frem for interviews og rapporter i fuld l&#xe6;ngde.</skos:definition>
      <skos:prefLabel xml:lang="fi">Yhteenveto,  lyhennelm&#xe4; tai tiivistelm&#xe4;</skos:prefLabel>
      <skos:definition xml:lang="fi">Tietoa ker&#xe4;t&#xe4;&#xe4;n muodostamalla yhteenveto tai tiivistelm&#xe4; olennaisista seikoista. Esimerkiksi: Haastatteluista ei tehd&#xe4; translitteraatioita vaan aineisto muodostuu haastattelujen tiivistelmist&#xe4;, tai sanomalehtiuutisisten aiheista muodostetaan aineisto tiivist&#xe4;m&#xe4;ll&#xe4; ne pariin lauseeseen. Mik&#xe4;li kvalitatiivisesta l&#xe4;hdeaineistosta muodostetaan kvantitatiivinen aineisto, k&#xe4;yt&#xe4; termi&#xe4; &apos;Sis&#xe4;ll&#xf6;nkoodaus&apos;.</skos:definition>
      <skos:prefLabel xml:lang="fr">R&#xe9;sum&#xe9;</skos:prefLabel>
      <skos:definition xml:lang="fr">Pr&#xe9;sentation d&apos;informations dans une forme condens&#xe9;e, en les r&#xe9;duisant &#xe0; leurs points importants. Par exemple, des r&#xe9;sum&#xe9;s d&apos;entretiens ou de rapports qui sont publi&#xe9;s et utilis&#xe9;s comme des donn&#xe9;es plut&#xf4;t que des entretiens ou des rapports complets.</skos:definition>
      <skos:prefLabel xml:lang="it">Sintesi</skos:prefLabel>
      <skos:definition xml:lang="it">Presentazione di informazioni in forma sintetica, riducendole ai punti principali. Ad esempio, abstract di interviste o report che vengono pubblicati e utilizzati come dati, al posto delle interviste o dei report completi.</skos:definition>
      <skos:prefLabel xml:lang="no">Sammendrag</skos:prefLabel>
      <skos:definition xml:lang="no">Presentasjon av informasjon i en konsentrert form, ved &#xe5; redusere den til dens hovedpoeng. For eksempel, sammendrag av intervjuer eller rapporter som er publisert og brukt som data til fordel for de fulle intervjuene eller rapportene.</skos:definition>
      <skos:prefLabel xml:lang="pt">Sum&#xe1;rio/resumo</skos:prefLabel>
      <skos:definition xml:lang="pt">Apresenta&#xe7;&#xe3;o de informa&#xe7;&#xe3;o de forma resumida, reduzindo-a aos seus pontos principais. Por exemplo, resumos de entrevistas ou de relat&#xf3;rios que s&#xe3;o publicados e usados como dados, em vez de entrevistas ou relat&#xf3;rios completos.</skos:definition>
      <skos:prefLabel xml:lang="sl">Povzetek</skos:prefLabel>
      <skos:definition xml:lang="sl">Predstavitev informacij v zgo&#x161;&#x10d;eni obliki z reduciranjem na glavne to&#x10d;ke. Na primer, povzetki intervjujev ali poro&#x10d;il, ki so objavljeni in uporabljeni kot podatki in ne kot celoviti intervjuji ali poro&#x10d;ila.</skos:definition>
      <skos:prefLabel xml:lang="sr">Rezime</skos:prefLabel>
      <skos:definition xml:lang="sr">Predstavljanje informacija u skrac&#x301;enom obliku, svodec&#x301;i je na glavne ta&#x10d;ke. Na primer, sa&#x17e;eci intervjua ili izvje&#x161;taji koji se objavljuju i koriste kao podaci, a ne celoviti intervjui ili izve&#x161;taji.</skos:definition>
      <skos:prefLabel xml:lang="sv">Sammanfattning</skos:prefLabel>
      <skos:definition xml:lang="sv">Presentation av information i sammandrag, som reducerats till sitt viktigaste inneh&#xe5;ll. Exempel: Abstrakt fr&#xe5;n intervjuer eller rapporter publiceras och anv&#xe4;nds som data ist&#xe4;llet f&#xf6;r de fullst&#xe4;ndiga intervjuerna eller rapporterna.</skos:definition>
   </rdf:Description>
   <rdf:Description rdf:about="http://rdf-vocabulary.ddialliance.org/cv/ModeOfCollection/3.0.0/d9ceca6">
      <rdf:type rdf:resource="http://www.w3.org/2004/02/skos/core#Concept"/>
      <skos:inScheme rdf:resource="http://rdf-vocabulary.ddialliance.org/cv/ModeOfCollection/3.0.0/"/>
      <skos:notation xml:lang="en">Aggregation</skos:notation>
      <skos:prefLabel xml:lang="en">Aggregation</skos:prefLabel>
      <skos:definition xml:lang="en">Statistics that relate to broad classes, groups, or categories. The data are averaged, totaled, or otherwise derived from individual-level data, and it is no longer possible to distinguish the characteristics of individuals within those classes, groups, or categories. For example, the number and age group of the unemployed in specific geographic regions, or national level statistics on the occurrence of specific offences, originally derived from the statistics of individual police districts.</skos:definition>
      <skos:prefLabel xml:lang="da">Aggregering</skos:prefLabel>
      <skos:definition xml:lang="da">Statistik, der vedr&#xf8;rer bredere klasser, grupper eller kategorier. Dataene er i gennemsnit, summeret eller p&#xe5; anden vis afledt af data p&#xe5; individuelt niveau, og det er ikke l&#xe6;ngere muligt at adskille individers karakteristika inden for disse klasser, grupper eller kategorier. For eksempel antallet eller aldersgruppen for de ledige i en bestemt geografisk region eller statistik p&#xe5; et nationalt plan om forekomsten af specifikke lovovertr&#xe6;delser, der oprindeligt er afledt af statistikkerne for de enkelte politidistrikter.</skos:definition>
      <skos:prefLabel xml:lang="fi">Aggregointi</skos:prefLabel>
      <skos:definition xml:lang="fi">Tilastollinen tieto, jossa yksitt&#xe4;isi&#xe4; havaintoyksik&#xf6;it&#xe4; koskevat tiedot ovat keskiarvoistettu, yhteenlaskettu tai jotenkin muuten yhdistetty laajempaa ryhm&#xe4;&#xe4; koskevaksi tiedoksi siten, ett&#xe4; yksitt&#xe4;isen havaintoyksik&#xf6;iden tiedot eiv&#xe4;t ole en&#xe4;&#xe4; erotettavissa. Esimerkkej&#xe4;: Kansallinen rikostilasto, joka yhteenlaskettu yksitt&#xe4;isten poliisipiirien tilastoista, tai kuukausittainen hintaindeksi, joka on keskiarvo yksitt&#xe4;isten hy&#xf6;dykkeiden hinnoista.</skos:definition>
      <skos:prefLabel xml:lang="fr">Agr&#xe9;gation</skos:prefLabel>
      <skos:definition xml:lang="fr">Statistiques qui concernent des classes, des groupes, ou des cat&#xe9;gories. Les donn&#xe9;es sont calcul&#xe9;es en moyenne, additionn&#xe9;es, ou autrement d&#xe9;riv&#xe9;es des donn&#xe9;es au niveau individuel, et il n&apos;est plus possible de distinguer les caract&#xe9;ristiques des individus au sein de ces classes, groupes, ou cat&#xe9;gories. Par exemple, le nombre et le groupe d&apos;&#xe2;ge des ch&#xf4;meurs dans des r&#xe9;gions g&#xe9;ographiques sp&#xe9;cifiques, ou des statistiques nationales sur l&apos;apparition de certaines infractions, tir&#xe9;es originellement des statistiques de diff&#xe9;rents districts de police.</skos:definition>
      <skos:prefLabel xml:lang="it">Aggregazione</skos:prefLabel>
      <skos:definition xml:lang="it">Statistiche relative a classi, gruppi o categorie. I dati rappresentano il valore medio, la somma o altre derivazioni dei dati raccolti a livello individuale, che non consentono pi&#xf9; di distinguere le caratteristiche degli individui all&apos;interno di tali classi, gruppi o categorie. Ad esempio, il numero e la fascia di et&#xe0; dei disoccupati in specifiche regioni geografiche, o le statistiche a livello nazionale sul verificarsi di reati specifici, originariamente desunti dalle statistiche dei singoli distretti di polizia.</skos:definition>
      <skos:prefLabel xml:lang="no">Aggregering</skos:prefLabel>
      <skos:definition xml:lang="no">Statistikk som relateres til store klasser, grupper eller kategorier. Dataene er tatt gjennomsnittet av, summert, eller p&#xe5; andre m&#xe5;ter utvunnet av data p&#xe5; individniv&#xe5;, og det er ikke lengre mulig &#xe5; skille mellom egenskapene til individer innad i disse klassene, gruppene eller kategoriene. For eksempel, antallet og aldersgruppen til de arbeidsledige i bestemte regioner, eller statistikk p&#xe5; nasjonalt niv&#xe5; om forekomsten av bestemte overtredelser, opprinnelig utarbeidet fra statistikk om individuelle politidistrikt.</skos:definition>
      <skos:prefLabel xml:lang="pt">Agrega&#xe7;&#xe3;o</skos:prefLabel>
      <skos:definition xml:lang="pt">Estat&#xed;sticas relacionadas com classes, grupos ou categorias amplas. Os dados s&#xe3;o representados por m&#xe9;dias, totais, ou derivados de dados registados a um n&#xed;vel individual, n&#xe3;o sendo mais poss&#xed;vel distinguir as caracter&#xed;sticas dos indiv&#xed;duos dentro dessas classes, grupos ou categorias. Por exemplo, o n&#xfa;mero e a faixa et&#xe1;ria dos desempregados em regi&#xf5;es geogr&#xe1;ficas espec&#xed;ficas, ou estat&#xed;sticas de &#xe2;mbito nacional sobre a ocorr&#xea;ncia de crimes espec&#xed;ficos, originalmente derivadas das estat&#xed;sticas policiais de cada distrito.</skos:definition>
      <skos:prefLabel xml:lang="sl">Agregacija</skos:prefLabel>
      <skos:definition xml:lang="sl">Statistike, ki se nana&#x161;ajo na &#x161;ir&#x161;e razrede, skupine ali kategorije. Podatki so predstavljeni kot povpre&#x10d;ja, vsote ali druge izpeljave, na podlagi katerih ni ve&#x10d; mo&#x17e;no razlikovati med zna&#x10d;ilnostmi posameznikov znotraj teh razredov, skupin ali kategorij. Na primer, &#x161;tevilo in starostna skupina brezposelnih v posebnih geografskih regijah ali nacionalne statistike o pojavu poosameznih kaznivih dejanj, ki so bila prvotno izpeljana iz statisti&#x10d;nih podatkov posameznih policijskih okro&#x17e;ij.</skos:definition>
      <skos:prefLabel xml:lang="sr">Agregacija</skos:prefLabel>
      <skos:definition xml:lang="sr">Statistika koja se odnosi na &#x161;iroke klase, grupe ili kategorije. Podaci su dati na nivou proseka, zbira ili su na neki drugi na&#x10d;in izvedeni iz podataka prikupljenih na nivou pojedinaca i vi&#x161;e nije moguc&#x301;e razlikovati karakteristike pojedinaca u tim klasama, grupama ili kategorijama. Na primer, broj i starosna grupa nezaposlenih u odre&#x111;enim geografskim regionima ili statistika na nacionalnom nivou o pojavljivanju odre&#x111;enih krivi&#x10d;nih dela, izvorno izvedena iz statistika pojedinih policijskih okruga.</skos:definition>
      <skos:prefLabel xml:lang="sv">Aggregation</skos:prefLabel>
      <skos:definition xml:lang="sv">Statistik som r&#xf6;r breda klasser, grupper eller kategorier. Datamaterialet best&#xe5;r av genomsnitt, totalsummor eller andra v&#xe4;rden som har h&#xe4;rletts fr&#xe5;n data p&#xe5; individniv&#xe5;, och det g&#xe5;r inte l&#xe4;ngre att utl&#xe4;sa individernas egenskaper inom dessa klasser, grupper eller kategorier. Exempel: antal och &#xe5;lderskategorier f&#xf6;r arbetsl&#xf6;sa inom s&#xe4;rskilda geografiska omr&#xe5;den, eller statistik p&#xe5; nationsniv&#xe5; &#xf6;ver f&#xf6;rekomsten av s&#xe4;rskilda brott som ursprungligen h&#xe4;rletts fr&#xe5;n statistik fr&#xe5;n enskilda polisdistrikt.</skos:definition>
   </rdf:Description>
   <rdf:Description rdf:about="http://rdf-vocabulary.ddialliance.org/cv/ModeOfCollection/3.0.0/4f502b5">
      <rdf:type rdf:resource="http://www.w3.org/2004/02/skos/core#Concept"/>
      <skos:inScheme rdf:resource="http://rdf-vocabulary.ddialliance.org/cv/ModeOfCollection/3.0.0/"/>
      <skos:notation xml:lang="en">Simulation</skos:notation>
      <skos:prefLabel xml:lang="en">Simulation</skos:prefLabel>
      <skos:definition xml:lang="en">Modeling or imitative representation of real-world processes, events, or systems, often using computer programs. For example, a program modeling household consumption responses to indirect tax changes; or a dataset on hypothetical patients and their drug exposure, background conditions, and known adverse events.</skos:definition>
      <skos:prefLabel xml:lang="da">Simulation</skos:prefLabel>
      <skos:definition xml:lang="da">Modellering eller imitativ repr&#xe6;sentation af processer i den virkelige verden, h&#xe6;ndelser eller systemer, ofte ved brug af computerprogrammer. For eksempel et program, der modellerer husholdningsforbrug, som responderer til indirekte skatte&#xe6;ndringer; eller et datas&#xe6;t om hypotetiske patienter og deres l&#xe6;gemiddeleksponering, baggrundsforhold og kendte bivirkninger.</skos:definition>
      <skos:prefLabel xml:lang="fi">Simulointi</skos:prefLabel>
      <skos:definition xml:lang="fi">Todellisten prosessien, tapahtumien ja systeemien piirteiden tai mahdollisen muuttumisen tutkiminen mallintamalla, usein tietokoneohjelmia k&#xe4;ytt&#xe4;en.</skos:definition>
      <skos:prefLabel xml:lang="fr">Simulation</skos:prefLabel>
      <skos:definition xml:lang="fr">Mod&#xe9;lisation ou repr&#xe9;sentation imitative de processus, d&#x2019;&#xe9;v&#xe9;nements ou de syst&#xe8;mes r&#xe9;els, utilisant souvent des programmes informatiques. Par exemple, un programme mod&#xe9;lisant des r&#xe9;actions de la consommation des m&#xe9;nages aux changement des imp&#xf4;ts indirects ; ou un jeu de donn&#xe9;es sur des patients hypoth&#xe9;tiques et leur exposition aux m&#xe9;dicaments, aux conditions environnementales, et aux effets ind&#xe9;sirables connus.</skos:definition>
      <skos:prefLabel xml:lang="it">Simulazione</skos:prefLabel>
      <skos:definition xml:lang="it">Modellazione o rappresentazione finalizzata alla riproduzione di processi, eventi o sistemi reali, spesso utilizzando programmi per computer. Ad esempio, un programma che modella le risposte dei consumi delle famiglie alle variazioni delle imposte indirette; o un dataset relativo a pazienti ipotetici e alla loro esposizione a farmaci, alle condizioni di fondo e ad eventi avversi conosciuti.</skos:definition>
      <skos:prefLabel xml:lang="no">Simulering</skos:prefLabel>
      <skos:definition xml:lang="no">Modellering eller etterlignende representasjon av virkelige prosesser, hendelser eller systemer, ofte ved bruk av dataprogrammer. For eksempel et program som modellerer hvordan en husholdnings forbruk svarer p&#xe5; endringer i indirekte skatter; eller et datasett om hypotetiske pasienter og deres eksponering for narkotiske stoffer, bakgrunnsforhold, og kjente ugunstige hendelser.</skos:definition>
      <skos:prefLabel xml:lang="pt">Simula&#xe7;&#xe3;o</skos:prefLabel>
      <skos:definition xml:lang="pt">Modela&#xe7;&#xe3;o ou representa&#xe7;&#xe3;o por imita&#xe7;&#xe3;o de processos, eventos ou sistemas do mundo real, utilizando geralmente programas de computador. Por exemplo, um programa que modela as respostas do consumo das fam&#xed;lias &#xe0;s mudan&#xe7;as tribut&#xe1;rias indiretas; ou um conjunto de dados em pacientes hipot&#xe9;ticos e a sua exposi&#xe7;&#xe3;o a drogas, condi&#xe7;&#xf5;es do contexto e eventos adversos conhecidos.</skos:definition>
      <skos:prefLabel xml:lang="sl">Simulacija</skos:prefLabel>
      <skos:definition xml:lang="sl">Modeliranje ali opona&#x161;ajo&#x10d;e predstavljanje procesov, dogodkov ali sistemov v realnem svetu, pogosto z uporabo ra&#x10d;unalni&#x161;kih programov. Na primer program, ki modelira odziv potro&#x161;nje gospodinjstev na posredne dav&#x10d;ne spremembe; ali podatkovje o hipoteti&#x10d;nih pacientih in njihovi izpostavljenosti zdravilu, pogojih v ozadju in znanih ne&#x17e;elenih doogodkih.</skos:definition>
      <skos:prefLabel xml:lang="sr">Simulacija</skos:prefLabel>
      <skos:definition xml:lang="sr">Modeliranje ili imitacija reprezentacije procesa, doga&#x111;aja ili sistema u stvarnom svetu, &#x10d;esto koristec&#x301;i ra&#x10d;unarske programe. Na primer, program koji modelira reakcije potro&#x161;nje domac&#x301;instava na indirektne promene poreza ili skup podataka o hipoteti&#x10d;kim pacijentima i njihovoj izlo&#x17e;enosti lekovima, pozadinskim uslovima i poznatim ne&#x17e;eljenim doga&#x111;ajima.</skos:definition>
      <skos:prefLabel xml:lang="sv">Simulering</skos:prefLabel>
      <skos:definition xml:lang="sv">Modellering eller imiterande representation av processer, h&#xe4;ndelser eller system i den verkliga v&#xe4;rlden, ofta skapade med datorprogram. Exempel: ett program som modellerar hur hush&#xe5;llens konsumtion svarar p&#xe5; f&#xf6;r&#xe4;ndringar i indirekta skatter; eller ett dataset &#xf6;ver hypotetiska patienter och deras droganv&#xe4;ndning, bakgrundsf&#xf6;rh&#xe5;llanden och k&#xe4;nda negativa h&#xe4;ndelser.</skos:definition>
   </rdf:Description>
   <rdf:Description rdf:about="http://rdf-vocabulary.ddialliance.org/cv/ModeOfCollection/3.0.0/38ceaa4">
      <rdf:type rdf:resource="http://www.w3.org/2004/02/skos/core#Concept"/>
      <skos:inScheme rdf:resource="http://rdf-vocabulary.ddialliance.org/cv/ModeOfCollection/3.0.0/"/>
      <skos:notation xml:lang="en">MeasurementsAndTests</skos:notation>
      <skos:prefLabel xml:lang="en">Measurements and tests</skos:prefLabel>
      <skos:definition xml:lang="en">Assessing specific properties (or characteristics) of beings, things, phenomena, (and/ or processes) by applying pre-established standards and/or specialized instruments or techniques.</skos:definition>
      <skos:prefLabel xml:lang="da">M&#xe5;linger og tests</skos:prefLabel>
      <skos:definition xml:lang="da">Vurdere specifikke egenskaber (eller karakteristika) af v&#xe6;sener, ting, f&#xe6;nomener (og/eller processer) ved at anvende forudbestemte standarder og/eller specialiserede instrumenter eller teknikker.</skos:definition>
      <skos:prefLabel xml:lang="fi">Mittaukset ja testit</skos:prefLabel>
      <skos:definition xml:lang="fi">Ihmisten ja muiden elollisten olioiden, esineiden, materiaalien ja ilmi&#xf6;iden ominaisuuksien mittaaminen k&#xe4;ytt&#xe4;en etuk&#xe4;teen m&#xe4;&#xe4;riteltyj&#xe4; standardeja tai tarkoitukseen kehitettyj&#xe4; mittareita ja tekniikoita.</skos:definition>
      <skos:prefLabel xml:lang="fr">Mesures et tests</skos:prefLabel>
      <skos:definition xml:lang="fr">&#xc9;valuer des propri&#xe9;t&#xe9;s sp&#xe9;cifiques (ou caract&#xe9;ristiques) d&apos;&#xea;tres, de choses, de ph&#xe9;nom&#xe8;nes, (et / ou processus) en appliquant des standards pr&#xe9;&#xe9;tablis et / ou des instruments ou des techniques sp&#xe9;cialis&#xe9;s.</skos:definition>
      <skos:prefLabel xml:lang="it">Misurazioni e test</skos:prefLabel>
      <skos:definition xml:lang="it">Valutazione di specifiche propriet&#xe0; (o caratteristiche) di esseri viventi, cose, fenomeni (e/o processi) applicando standard prestabiliti e/o strumenti o tecniche specializzate.</skos:definition>
      <skos:prefLabel xml:lang="no">M&#xe5;linger og tester</skos:prefLabel>
      <skos:definition xml:lang="no">Vurdering av bestemte egenskaper (eller karakteristika) ved vesener, ting, fenomen (og/eller prosesser) ved &#xe5; anvende forutbestemte standarder og/eller spesialiserte instrumenter eller teknikker.</skos:definition>
      <skos:prefLabel xml:lang="pt">Medidas e testes</skos:prefLabel>
      <skos:definition xml:lang="pt">Avalia&#xe7;&#xe3;o de propriedades espec&#xed;ficas (ou caracter&#xed;sticas) de seres, coisas, fen&#xf3;menos (e/ou processos) aplicando padr&#xf5;es pr&#xe9;-estabelecidos e/ou t&#xe9;cnicas e instrumentos espec&#xed;ficos.</skos:definition>
      <skos:prefLabel xml:lang="sl">Merjenje in testiranje</skos:prefLabel>
      <skos:definition xml:lang="sl">Ocenjevanje specifi&#x10d;nih lastnosti (ali zna&#x10d;ilnosti) bitij, stvari, pojavov (in/ali procesov), z uporabo vnaprej dolo&#x10d;enih standardov in/ali specializiranih instrumentov ali tehnik.</skos:definition>
      <skos:prefLabel xml:lang="sr">Merenje i testiranje</skos:prefLabel>
      <skos:definition xml:lang="sr">Procena specifi&#x10d;nih svojstava (ili karakteristika) bic&#x301;a, stvari, pojava (i / ili procesa) primenom unapred utvr&#x111;enih standarda i / ili specijalizovanih instrumenata ili tehnika.</skos:definition>
      <skos:prefLabel xml:lang="sv">M&#xe4;tningar och tester</skos:prefLabel>
      <skos:definition xml:lang="sv">Bed&#xf6;mning av varelsers, f&#xf6;rem&#xe5;ls, fenomens (och/eller processers) s&#xe4;rskilda egenskaper (eller karakteristiska) genom att till&#xe4;mpa f&#xf6;rutbest&#xe4;mda standarder och/eller specialiserade instrument eller tekniker.</skos:definition>
      <skos:narrower rdf:resource="http://rdf-vocabulary.ddialliance.org/cv/ModeOfCollection/3.0.0/4b9776b"/>
      <skos:narrower rdf:resource="http://rdf-vocabulary.ddialliance.org/cv/ModeOfCollection/3.0.0/c2a25a6"/>
      <skos:narrower rdf:resource="http://rdf-vocabulary.ddialliance.org/cv/ModeOfCollection/3.0.0/27daf03"/>
   </rdf:Description>
   <rdf:Description rdf:about="http://rdf-vocabulary.ddialliance.org/cv/ModeOfCollection/3.0.0/4b9776b">
      <rdf:type rdf:resource="http://www.w3.org/2004/02/skos/core#Concept"/>
      <skos:inScheme rdf:resource="http://rdf-vocabulary.ddialliance.org/cv/ModeOfCollection/3.0.0/"/>
      <skos:notation xml:lang="en">MeasurementsAndTests.Educational</skos:notation>
      <skos:prefLabel xml:lang="en">Educational measurements and tests</skos:prefLabel>
      <skos:definition xml:lang="en">Assessment of knowledge, skills, aptitude, or educational achievement by means of specialized measures or tests.</skos:definition>
      <skos:prefLabel xml:lang="da">Udannelsesm&#xe6;ssige m&#xe5;linger og tests</skos:prefLabel>
      <skos:definition xml:lang="da">Vurdering af viden, f&#xe6;rdigheder, egnethed eller uddannelsesm&#xe6;ssig pr&#xe6;station ved brug af specialiserede m&#xe5;linger eller tests.</skos:definition>
      <skos:prefLabel xml:lang="fi">Mittaukset ja testit: tiet&#xe4;myksen, taipumusten, soveltuvuuden ja oppimistulosten mittaaminen</skos:prefLabel>
      <skos:definition xml:lang="fi">Mittaamalla tai testaamalla saadut tiedot tutkittavien tietotasosta, synnynn&#xe4;isist&#xe4; taipumuksista, soveltuvuudesta tai oppimistuloksista. Esimerkkej&#xe4;: PISA-testit, ylioppilaskokeiden tulokset, yhteiskunnallisen tiet&#xe4;myksen mittari, tai kielellist&#xe4; tai matemaattista lahjakkuutta mittaavat testit.</skos:definition>
      <skos:prefLabel xml:lang="fr">Mesures et tests d&apos;enseignement</skos:prefLabel>
      <skos:definition xml:lang="fr">&#xc9;valuation de connaissances, de comp&#xe9;tences, d&apos;aptitudes, ou de r&#xe9;sultats scolaires au moyen de mesures ou tests sp&#xe9;cialis&#xe9;s.</skos:definition>
      <skos:prefLabel xml:lang="it">Misurazioni e test in ambito educativo</skos:prefLabel>
      <skos:definition xml:lang="it">Valutazione delle conoscenze, abilit&#xe0;, attitudini o risultati in ambito educativo mediante misure o test specializzati.</skos:definition>
      <skos:prefLabel xml:lang="no">Pedagogiske m&#xe5;linger og tester</skos:prefLabel>
      <skos:definition xml:lang="no">Vurdering av kunnskap, ferdighet, egnethet, eller utdanningsoppn&#xe5;elser ved spesialiserte m&#xe5;l eller tester.</skos:definition>
      <skos:prefLabel xml:lang="pt">Medidas e testes educacionais</skos:prefLabel>
      <skos:definition xml:lang="pt">Avalia&#xe7;&#xe3;o de conhecimentos, compet&#xea;ncias, aptid&#xf5;es ou desempenhos educacionais por meio de medidas ou testes espec&#xed;ficos.</skos:definition>
      <skos:prefLabel xml:lang="sl">Meritve in testiranja v vzgoji in izobra&#x17e;evanju</skos:prefLabel>
      <skos:definition xml:lang="sl">Ocenjevanje znanja, spretnosti, sposobnosti ali izobra&#x17e;evalnih dose&#x17e;kov s pomo&#x10d;jo specializiranih meritev ali testov.</skos:definition>
      <skos:prefLabel xml:lang="sr">Obrazovno merenje i testiranje</skos:prefLabel>
      <skos:definition xml:lang="sr">Procena znanja, ve&#x161;tina, sposobnosti ili obrazovnog dostignuc&#x301;a pomoc&#x301;u specijalizovanih mera ili testova.</skos:definition>
      <skos:prefLabel xml:lang="sv">Pedagogiska m&#xe4;tningar och tester</skos:prefLabel>
      <skos:definition xml:lang="sv">Bed&#xf6;mning av kunskap, f&#xf6;rm&#xe5;gor, beg&#xe5;vning eller inl&#xe4;rningsf&#xf6;rm&#xe5;ga med hj&#xe4;lp av specialiserade m&#xe4;tredskap och tester.</skos:definition>
   </rdf:Description>
   <rdf:Description rdf:about="http://rdf-vocabulary.ddialliance.org/cv/ModeOfCollection/3.0.0/c2a25a6">
      <rdf:type rdf:resource="http://www.w3.org/2004/02/skos/core#Concept"/>
      <skos:inScheme rdf:resource="http://rdf-vocabulary.ddialliance.org/cv/ModeOfCollection/3.0.0/"/>
      <skos:notation xml:lang="en">MeasurementsAndTests.Physical</skos:notation>
      <skos:prefLabel xml:lang="en">Physical measurements and tests</skos:prefLabel>
      <skos:definition xml:lang="en">Assessment of physical properties of living beings, objects, materials, or natural phenomena. For example, findings from hands-on medical examination (e.g., palpation or auscultation), clinical measurements and lab tests like blood analysis, blood pressure, heart rate, body weight and height, as well as general measurements like time, distance, mass, temperature, force, power, speed, GPS data on physical movement and other physical parameters or variables, like geospatial data.</skos:definition>
      <skos:prefLabel xml:lang="da">Fysiske m&#xe5;linger og tests</skos:prefLabel>
      <skos:definition xml:lang="da">Vurdering af fysiske egenskaber hos levende v&#xe6;sener, objekter, materialer eller naturlige f&#xe6;nomener. For eksempel resultater fra praktisk l&#xe6;geunders&#xf8;gelse (f.eks. palpation eller auskultation), kliniske m&#xe5;linger og laboratorietests s&#xe5;som blodanalyse, blodtryk, hjerterytme, kropsv&#xe6;gt og h&#xf8;jde, s&#xe5;vel som generelle m&#xe5;linger s&#xe5;som tid, afstand, masse, temperatur, styrke, kraft, hastighed, GPS-data om fysisk bev&#xe6;gelse og andre fysiske parametre eller variabler, s&#xe5;som geospatiale data.</skos:definition>
      <skos:prefLabel xml:lang="fi">Mittaukset ja testit: fyysisten ominaisuuksien mittaaminen</skos:prefLabel>
      <skos:definition xml:lang="fi">Ihmisten ja muiden elollisten olioiden, esineiden, materiaalien ja luonnonilmi&#xf6;iden fyysisten ominaisuuksien mittaaminen. Esimerkkej&#xe4;: verenpaine, paino ja pituus, voima, et&#xe4;isyys, l&#xe4;mp&#xf6;tila, nopeus, seismografiset mittaukset, GPS-koordinaatit.</skos:definition>
      <skos:prefLabel xml:lang="fr">Mesures et tests de caract&#xe9;ristiques physiques</skos:prefLabel>
      <skos:definition xml:lang="fr">&#xc9;valuation des propri&#xe9;t&#xe9;s physiques d&apos;&#xea;tres vivants, d&apos;objets, de mat&#xe9;riaux, ou de ph&#xe9;nom&#xe8;nes naturels. Par exemple, des r&#xe9;sultats d&apos;examens cliniques (e. g. palpation, auscultation), mesures cliniques and tests de laboratoire comme analyse de sang, pression sanguine, rythme cardiaque, poids et taille du corps, de m&#xea;me que des mesures g&#xe9;n&#xe9;rales de temps, de distance, de masse, de temp&#xe9;rature, de force, de puissance, de vitesse, de donn&#xe9;es de localisation sur des mouvements physiques ou d&apos;autres param&#xe8;tres ou variables physiques comme des donn&#xe9;es g&#xe9;ospatiales.</skos:definition>
      <skos:prefLabel xml:lang="it">Misurazioni e test fisici</skos:prefLabel>
      <skos:definition xml:lang="it">Valutazione delle propriet&#xe0; fisiche di esseri viventi, oggetti, materiali o fenomeni naturali. Per esempio, risultati di esami pratici a livello medico (ad esempio, palpazione o auscultazione), misurazioni cliniche e test di laboratorio come analisi del sangue, pressione sanguigna, frequenza cardiaca, peso corporeo e altezza, nonch&#xe9; misure generali come tempo, distanza, massa, temperatura, forza, potenza, velocit&#xe0;, dati GPS sul movimento fisico e altri parametri o variabili fisici, come i dati geospaziali.</skos:definition>
      <skos:prefLabel xml:lang="no">Fysiske m&#xe5;linger og tester</skos:prefLabel>
      <skos:definition xml:lang="no">Vurdering av fysiske egenskaper hos levende vesener, objekter, materiale, eller naturlige fenomen. For eksempel, funn fra fysiske medisinske unders&#xf8;kelser (e.g., palpasjon eller auskultasjon), kliniske m&#xe5;l og laboratorietester som blodanalyse, blodtrykksm&#xe5;l, hjerterytme, kroppsvekt og h&#xf8;yde, og generelle m&#xe5;l som tid, distanse, masse, temperatur, kraft, energi, fart, GPS data p&#xe5; fysisk bevegelse og andre m&#xe5;l p&#xe5; fysiske parameter eller variabler.</skos:definition>
      <skos:prefLabel xml:lang="pt">Medidas e testes f&#xed;sicos</skos:prefLabel>
      <skos:definition xml:lang="pt">Avalia&#xe7;&#xe3;o de propriedades f&#xed;sicas de seres vivos, objetos, materiais ou fen&#xf3;menos naturais. Por exemplo, descobertas de exames m&#xe9;dicos pr&#xe1;ticos (por exemplo, palpa&#xe7;&#xe3;o ou ausculta&#xe7;&#xe3;o), medi&#xe7;&#xf5;es cl&#xed;nicas e testes laboratoriais, como an&#xe1;lise sangu&#xed;nea, press&#xe3;o arterial, frequ&#xea;ncia card&#xed;aca, peso e altura, assim como medidas gerais, por exemplo, de tempo, dist&#xe2;ncia, massa, temperatura, for&#xe7;a, pot&#xea;ncia, velocidade, dados de GPS sobre movimento f&#xed;sico e outros par&#xe2;metros ou vari&#xe1;veis f&#xed;sicos, como dados geoespaciais.</skos:definition>
      <skos:prefLabel xml:lang="sl">Meritve in testiranja fizi&#x10d;nih lastnosti</skos:prefLabel>
      <skos:definition xml:lang="sl">Ocenjevanje fizi&#x10d;nih lastnosti &#x17e;ivih bitij, predmetov, materialov ali naravnih pojavov. Na primer ugotovitve prakti&#x10d;nega zdravni&#x161;kega pregleda (npr. palpacije ali auskultacije), klini&#x10d;nih meritev in laboratorijskih preiskav, kot so analiza krvi, krvni talak, sr&#x10d;ni utrip, telesna te&#x17e;a in vi&#x161;ina ter splo&#x161;ne meritve, kot so &#x10d;as, razdalja, temperatura, sila, mo&#x10d;, hitrost, podatki GPS o fizi&#x10d;nem gibanju in drugih fizi&#x10d;nih parametrih ali spremenljivkah, kot so geoprostorski podatki.</skos:definition>
      <skos:prefLabel xml:lang="sr">Fizi&#x10d;ko merenje i testiranje</skos:prefLabel>
      <skos:definition xml:lang="sr">Procena fizi&#x10d;kih svojstava &#x17e;ivih bic&#x301;a, predmeta, materijala ili prirodnih pojava. Na primer, nalaz iz prakti&#x10d;nog medicinskog pregleda (npr. palpacije ili auskultacije), klini&#x10d;kih merenja i laboratorijskih testova poput analize krvi, krvnog pritiska, otkucaja srca, telesne te&#x17e;ine i visine, kao i op&#x161;tih merenja kao &#x161;to su vreme, udaljenost, masa, temperatura, sila, snaga, brzina, GPS podaci o fizi&#x10d;kom kretanju i drugi fizi&#x10d;ki parametri ili promenljive, poput geoprostornih podataka.</skos:definition>
      <skos:prefLabel xml:lang="sv">Fysiska m&#xe4;tningar och tester</skos:prefLabel>
      <skos:definition xml:lang="sv">Bed&#xf6;mning av levande varelsers, f&#xf6;rem&#xe5;ls, materials eller naturliga fenomens fysiska egenskaper. Till exempel: blodtryck, puls, kroppsvikt och l&#xe4;ngd, men &#xe4;ven tid, avst&#xe5;nd, massa, temperatur, kraft, effekt, hastighet, GPS-data f&#xf6;r fysisk r&#xf6;relse och andra fysiska parametrar eller variabler, som t.ex. geospatiala data.</skos:definition>
   </rdf:Description>
   <rdf:Description rdf:about="http://rdf-vocabulary.ddialliance.org/cv/ModeOfCollection/3.0.0/27daf03">
      <rdf:type rdf:resource="http://www.w3.org/2004/02/skos/core#Concept"/>
      <skos:inScheme rdf:resource="http://rdf-vocabulary.ddialliance.org/cv/ModeOfCollection/3.0.0/"/>
      <skos:notation xml:lang="en">MeasurementsAndTests.Psychological</skos:notation>
      <skos:prefLabel xml:lang="en">Psychological measurements and tests</skos:prefLabel>
      <skos:definition xml:lang="en">Assessment of personality traits or psychological/behavioral responses by means of specialized measures or tests. For example, objective tests like self-report measures with a restricted response format, or projective methods allowing free responses, including word association, sentence or story completion, vignettes, cartoon test, thematic apperception tests, role play, drawing tests, inkblot tests, choice ordering exercises, etc.</skos:definition>
      <skos:prefLabel xml:lang="da">Psykologiske m&#xe5;linger og tests</skos:prefLabel>
      <skos:definition xml:lang="da">Vurdering af personlighedskarakterer eller psykologiske/adf&#xe6;rdsm&#xe6;ssige reaktioner ved hj&#xe6;lp af specialiserede m&#xe5;linger og tests. For eksempel objektive tests s&#xe5;som selvrapporterende m&#xe5;linger med et begr&#xe6;nset responsformat eller projektive metoder, der tillader fri respons, inklusiv associering af ord, s&#xe6;tninger eller historief&#xe6;rdigg&#xf8;relse, vignetter, tegneserietests, tematiske accerceptionstests, rollespil, tegnetests, bl&#xe6;kklattests, &#xf8;velser om valgprioritering mm.</skos:definition>
      <skos:prefLabel xml:lang="fi">Mittaukset ja testit: psykologisten ominaisuuksien mittaaminen</skos:prefLabel>
      <skos:definition xml:lang="fi">Luonteenpiirteiden ja k&#xe4;ytt&#xe4;ytymismallien tutkiminen tarkoitusta varten kehitettyjen testien avulla. Esimerkiksi: Luonteenpiirteiden itseraportointi, el&#xe4;ytymismenetelm&#xe4;t. Tarvittaessa voidaan k&#xe4;ytt&#xe4;&#xe4; yhdess&#xe4; muiden aineistonkeruumenetelm&#xe4;termien kanssa (esimerkiksi masentuneisuusaste-testi osana kyselylomaketta).</skos:definition>
      <skos:prefLabel xml:lang="fr">Mesures et tests psychologiques</skos:prefLabel>
      <skos:definition xml:lang="fr">&#xc9;valuation des traits de personnalit&#xe9;s ou de r&#xe9;ponses psychologiques / comportementales au moyen de mesures ou tests sp&#xe9;cialis&#xe9;s. Par exemple, des tests objectifs comme mesure d&apos;auto-&#xe9;valuation avec un format restreint de r&#xe9;ponses, ou des m&#xe9;thodes projectives permettant des r&#xe9;ponses libres, incluant l&apos;association de mots, l&apos;ach&#xe8;vement de phrase ou d&apos;histoire, des vignettes, des tests anim&#xe9;s, des tests th&#xe9;matiques d&apos;apperception, du jeu de r&#xf4;le, des tests de dessin, des tests de t&#xe2;ches d&apos;encre, des exercices de classement, etc.</skos:definition>
      <skos:prefLabel xml:lang="it">Misurazioni e test psicologici</skos:prefLabel>
      <skos:definition xml:lang="it">Valutazione dei tratti di personalit&#xe0; o risposte psicologiche/comportamentali mediante misure o test specializzati. Ad esempio, test oggettivi come misure di autovalutazione con un range predefinito, o test proiettivi che consentono risposte libere, incluse associazione di parole, completamento di frasi o storie, vignette, fumetti, test di appercezione tematica, giochi di ruolo, prove di disegno, test macchie di inchiostri, esercizi sulle scelte di ordinamento, ecc.</skos:definition>
      <skos:prefLabel xml:lang="no">Psykologiske m&#xe5;linger og tester</skos:prefLabel>
      <skos:definition xml:lang="no">Vurdering av personlighetstrekk eller psykologiske/atferdsmessige reaksjoner ved bruk av spesialiserte m&#xe5;l og tester. For eksempel, objektive tester som selvrapporteringsm&#xe5;l med mer begrenset svarformat, eller projektive metoder som gj&#xf8;r det mulig &#xe5; svare helt fritt, inkludert ordassosiasjon, setning eller fortellingsfullf&#xf8;ring, korte beskrivelser, tematiske appersepsjonstester, rollespill, tegnetester, blekk-kladd tester, prioriterings&#xf8;velser etc.</skos:definition>
      <skos:prefLabel xml:lang="pt">Medidas e testes psicol&#xf3;gicos</skos:prefLabel>
      <skos:definition xml:lang="pt">Avalia&#xe7;&#xe3;o de tra&#xe7;os de personalidade ou respostas psicol&#xf3;gicas/comportamentais por meio de medidas espec&#xed;ficas e testes. Por exemplo, testes objetivos como medidas autorreportadas com um formato restrito de resposta, ou m&#xe9;todos projetivos que permitem respostas livres, incluindo associa&#xe7;&#xe3;o de palavras, conclus&#xe3;o de frases ou hist&#xf3;rias, vinhetas, teste de desenho animado, testes tem&#xe1;ticos de percep&#xe7;&#xe3;o, dramatiza&#xe7;&#xe3;o, testes de desenho, testes de mancha de tinta, exerc&#xed;cios de ordena&#xe7;&#xe3;o de escolha, etc.</skos:definition>
      <skos:prefLabel xml:lang="sl">Meritve in testiranja psiholo&#x161;kih lastnosti</skos:prefLabel>
      <skos:definition xml:lang="sl">Ocena osebnostnih lastnosti ali psiholo&#x161;kih/vedenjskih odzivov s pomo&#x10d;jo posebnih meritev ali testov. Na primer objektivni testi, kot so samoporo&#x10d;anje z zaprtim formatom odgovorov ali projekcijske tehnike, ki omogo&#x10d;ajo proste odgovore, vklju&#x10d;no z besednimi asociacijami, dopolnjevanjem stavkov ali zgodb, vinjetami, testi s karikaturami, testi tematske apercepcije, igranjem vlog, testi risanja, testi pack, testi izbire itd.</skos:definition>
      <skos:prefLabel xml:lang="sr">Psiholo&#x161;ko merenje i testiranje</skos:prefLabel>
      <skos:definition xml:lang="sr">Procena osobina li&#x10d;nosti ili psiholo&#x161;kih / bihevioralnih odgovora pomoc&#x301;u specijalizovanih mera ili testova. Na primer, objektivni testovi kao &#x161;to su mere samoizve&#x161;tavanja sa ograni&#x10d;enim formatom odgovora ili projektivne metode koje omogu&#x107;uju slobodne odgovore, uklju&#x10d;ujuc&#x301;i povezivanje re&#x10d;i, dovr&#x161;avanje re&#x10d;enica ili pri&#x10d;e, vinjete, test crte&#x17e;a, tematski testovi prikazivanja, igranje uloga, testovi crtanja, ve&#x17e;be ure&#x111;ivanja izbora itd.</skos:definition>
      <skos:prefLabel xml:lang="sv">Psykologiska m&#xe4;tningar och tester</skos:prefLabel>
      <skos:definition xml:lang="sv">Bed&#xf6;mning av personlighetsdrag eller psykologiska/beteendem&#xe4;ssiga responser genom specialiserade m&#xe4;tredskap eller tester. Exempel: objektiva tester som sj&#xe4;lvskattning med begr&#xe4;nsade svarsformat, eller projektiva tester som till&#xe5;ter &#xf6;ppna svar, inklusive ordassociation, menings- eller ber&#xe4;ttelsekomplettering, vinjetter, &quot;cartoon tests&quot;, tematiska apperceptionstester (TAT), rollspel, teckningstester, Rorschachtester, &quot;choice ordering exercises&quot; m.m.</skos:definition>
   </rdf:Description>
   <rdf:Description rdf:about="http://rdf-vocabulary.ddialliance.org/cv/ModeOfCollection/3.0.0/6311ae1">
      <rdf:type rdf:resource="http://www.w3.org/2004/02/skos/core#Concept"/>
      <skos:inScheme rdf:resource="http://rdf-vocabulary.ddialliance.org/cv/ModeOfCollection/3.0.0/"/>
      <skos:notation xml:lang="en">Other</skos:notation>
      <skos:prefLabel xml:lang="en">Other</skos:prefLabel>
      <skos:definition xml:lang="en">Use if the mode of data collection is known, but not found in the list.</skos:definition>
      <skos:prefLabel xml:lang="da">Andet</skos:prefLabel>
      <skos:definition xml:lang="da">Anvend, hvis dataindsamlingsm&#xe5;den er kendt, men ikke findes p&#xe5; listen.</skos:definition>
      <skos:prefLabel xml:lang="fi">Muu keruumenetelm&#xe4;</skos:prefLabel>
      <skos:definition xml:lang="fi">K&#xe4;yt&#xe4; mik&#xe4;li keruumenetelm&#xe4; on tiedossa, mutta ei sanastossa. Lis&#xe4;&#xe4; tarkempi selostus.</skos:definition>
      <skos:prefLabel xml:lang="fr">Autre</skos:prefLabel>
      <skos:definition xml:lang="fr">Utilisez si le mode de collecte est connu, mais pas pr&#xe9;sent dans la liste.</skos:definition>
      <skos:prefLabel xml:lang="it">Altro</skos:prefLabel>
      <skos:definition xml:lang="it">Utilizzare quando la tecnica di raccolta dei dati &#xe8; conosciuta, ma non &#xe8; presente nell&apos;elenco.</skos:definition>
      <skos:prefLabel xml:lang="no">Annet</skos:prefLabel>
      <skos:definition xml:lang="no">Bruk dersom metode for datainnsamling er kjent, men ikke finnes i listen.</skos:definition>
      <skos:prefLabel xml:lang="pt">Outro</skos:prefLabel>
      <skos:definition xml:lang="pt">Usar se o m&#xe9;todo de recolha de dados for conhecido, mas n&#xe3;o se encontrar na lista.</skos:definition>
      <skos:prefLabel xml:lang="sl">Drugo</skos:prefLabel>
      <skos:definition xml:lang="sl">Uporabite, &#x10d;e je na&#x10d;in zbiranja podatkov znan, vendar ga ni na tem seznamu.</skos:definition>
      <skos:prefLabel xml:lang="sr">Ostalo</skos:prefLabel>
      <skos:definition xml:lang="sr">Koristite ako je na&#x10d;in prikupljanja podataka poznat, ali nije prona&#x111;en na ovoj listi.</skos:definition>
      <skos:prefLabel xml:lang="sv">&#xd6;vrigt</skos:prefLabel>
      <skos:definition xml:lang="sv">Anv&#xe4;nds n&#xe4;r datainsamlingsmetoden &#xe4;r k&#xe4;nd men saknas i listan.</skos:definition>
   </rdf:Description>
</rdf:RDF>
