<?xml version="1.0" encoding="UTF-8"?>
<rdf:RDF xmlns:dcterms="http://purl.org/dc/terms/"
          xmlns:owl="http://www.w3.org/2002/07/owl#"
          xmlns:rdf="http://www.w3.org/1999/02/22-rdf-syntax-ns#"
          xmlns:rdfs="http://www.w3.org/2000/01/rdf-schema#"
          xmlns:skos="http://www.w3.org/2004/02/skos/core#">
   <rdf:Description rdf:about="http://rdf-vocabulary.ddialliance.org/cv/ModeOfCollection/4.0/">
      <rdf:type rdf:resource="http://www.w3.org/2004/02/skos/core#ConceptScheme"/>
      <dcterms:isVersionOf rdf:resource="http://rdf-vocabulary.ddialliance.org/cv/ModeOfCollection"/>
      <skos:notation>ModeOfCollection</skos:notation>
      <skos:prefLabel xml:lang="en">Mode Of Collection</skos:prefLabel>
      <skos:prefLabel xml:lang="de">Erhebungsmodus</skos:prefLabel>
      <skos:prefLabel xml:lang="fi">Keruumenetelmä</skos:prefLabel>
      <skos:prefLabel xml:lang="fi">Keruumenetelmä</skos:prefLabel>
      <skos:prefLabel xml:lang="it">Metodo di raccolta dei dati</skos:prefLabel>
      <skos:prefLabel xml:lang="ja">調査方法</skos:prefLabel>
      <skos:prefLabel xml:lang="lt">Surinkimo būdas</skos:prefLabel>
      <skos:prefLabel xml:lang="nl">Verzamelmethode</skos:prefLabel>
      <skos:prefLabel xml:lang="no">Innsamlingsmetode</skos:prefLabel>
      <skos:prefLabel xml:lang="no">Innsamlingsmetode</skos:prefLabel>
      <skos:prefLabel xml:lang="pt">Método de recolha de dados</skos:prefLabel>
      <skos:prefLabel xml:lang="sl">Način zbiranja podatkov</skos:prefLabel>
      <skos:prefLabel xml:lang="sv">Insamlingsmetod</skos:prefLabel>
      <skos:definition xml:lang="en">The procedure, technique, or mode of inquiry used to attain the data.</skos:definition>
      <skos:definition xml:lang="de">Prozedur, Technik oder Art der Erhebung, die verwendet wurde, um Daten zu bekommen.</skos:definition>
      <skos:definition xml:lang="fi">Kuvailtavan aineiston ensisijainen keruumenetelmä.</skos:definition>
      <skos:definition xml:lang="fi">Kuvailtavan aineiston ensisijainen keruumenetelmä.</skos:definition>
      <skos:definition xml:lang="it">La procedura, la tecnica o la modalità di indagine utilizzata per ottenere i dati.</skos:definition>
      <skos:definition xml:lang="ja">データを取得するにあたり利用された調査の手続き、技術あるいは方法。</skos:definition>
      <skos:definition xml:lang="lt">Tyrimo procedūra, technika ar būdas, naudojami gauti duomenis.</skos:definition>
      <skos:definition xml:lang="nl">De procedure, techniek of methode die is gebruikt om de gegevens te verzamelen. </skos:definition>
      <skos:definition xml:lang="no">Framgangsmåten, teknikken, eller metoden som er anvendt for å samle inn data.</skos:definition>
      <skos:definition xml:lang="no">Framgangsmåten, teknikken, eller metoden som er anvendt for å samle inn data.</skos:definition>
      <skos:definition xml:lang="pt">Procedimentos, técnicas ou métodos de recolha de dados.</skos:definition>
      <skos:definition xml:lang="sl">Postopki, tehnike ali načini raziskovanja, uporabljeni za pridobivanje podatkov.</skos:definition>
      <skos:definition xml:lang="sv">Den process, metod eller teknik som användes för att samla in data.</skos:definition>
      <owl:versionInfo>4.0</owl:versionInfo>
      <dcterms:license rdf:resource="Creative Commons Attribution 4.0 International"/>
      <dcterms:rights>Copyright ©DDI Alliance 2020</dcterms:rights>
      <skos:hasTopConcept rdf:resource="http://rdf-vocabulary.ddialliance.org/cv/ModeOfCollection/4.0/d50e136"/>
      <skos:hasTopConcept rdf:resource="http://rdf-vocabulary.ddialliance.org/cv/ModeOfCollection/4.0/d50e874"/>
      <skos:hasTopConcept rdf:resource="http://rdf-vocabulary.ddialliance.org/cv/ModeOfCollection/4.0/d50e1426"/>
      <skos:hasTopConcept rdf:resource="http://rdf-vocabulary.ddialliance.org/cv/ModeOfCollection/4.0/d50e1794"/>
      <skos:hasTopConcept rdf:resource="http://rdf-vocabulary.ddialliance.org/cv/ModeOfCollection/4.0/d50e2162"/>
      <skos:hasTopConcept rdf:resource="http://rdf-vocabulary.ddialliance.org/cv/ModeOfCollection/4.0/d50e2900"/>
      <skos:hasTopConcept rdf:resource="http://rdf-vocabulary.ddialliance.org/cv/ModeOfCollection/4.0/d50e3268"/>
      <skos:hasTopConcept rdf:resource="http://rdf-vocabulary.ddialliance.org/cv/ModeOfCollection/4.0/d50e3451"/>
      <skos:hasTopConcept rdf:resource="http://rdf-vocabulary.ddialliance.org/cv/ModeOfCollection/4.0/d50e3819"/>
      <skos:hasTopConcept rdf:resource="http://rdf-vocabulary.ddialliance.org/cv/ModeOfCollection/4.0/d50e3909"/>
      <skos:hasTopConcept rdf:resource="http://rdf-vocabulary.ddialliance.org/cv/ModeOfCollection/4.0/d50e3999"/>
      <skos:hasTopConcept rdf:resource="http://rdf-vocabulary.ddialliance.org/cv/ModeOfCollection/4.0/d50e4089"/>
      <skos:hasTopConcept rdf:resource="http://rdf-vocabulary.ddialliance.org/cv/ModeOfCollection/4.0/d50e4179"/>
      <skos:hasTopConcept rdf:resource="http://rdf-vocabulary.ddialliance.org/cv/ModeOfCollection/4.0/d50e4269"/>
      <skos:hasTopConcept rdf:resource="http://rdf-vocabulary.ddialliance.org/cv/ModeOfCollection/4.0/d50e4360"/>
      <skos:hasTopConcept rdf:resource="http://rdf-vocabulary.ddialliance.org/cv/ModeOfCollection/4.0/d50e4727"/>
   </rdf:Description>
   <rdf:Description rdf:about="http://rdf-vocabulary.ddialliance.org/cv/ModeOfCollection/4.0/d50e136">
      <rdf:type rdf:resource="http://www.w3.org/2004/02/skos/core#Concept"/>
      <skos:inScheme rdf:resource="http://rdf-vocabulary.ddialliance.org/cv/ModeOfCollection/4.0/"/>
      <skos:notation>Interview</skos:notation>
      <skos:prefLabel xml:lang="en">Interview</skos:prefLabel>
      <skos:definition xml:lang="en">A pre-planned communication between two (or more) people - the interviewer(s) and the interviewee(s) - in which information is obtained by the interviewer(s) from the interviewee(s). If group interaction is part of the method, use "Focus group".</skos:definition>
      <skos:prefLabel xml:lang="de">Interview</skos:prefLabel>
      <skos:definition xml:lang="de">Eine im Voraus geplante Kommunikation zwischen zwei (oder mehr) Personen - dem/der Interviewer*in bzw. den Interviewern und dem/der/den Befragten -, bei der der/die Interviewer Informationen von dem/der/den Befragten erhalten. Wenn die Interaktion innerhalb einer Gruppe Teil der Methode ist, verwenden Sie die Kategorie "Fokusgruppe".</skos:definition>
      <skos:prefLabel xml:lang="fi">Haastattelu</skos:prefLabel>
      <skos:definition xml:lang="fi">Ennalta suunniteltu, haastattelijan ja yhden tai useamman haastateltavan välinen keskustelu, jossa haastattelija saa tietoa tutkimustarkoituksiin. Käytä tarkempaa haastattelutermiä, mikäli mahdollista. Jos haastateltavia on enemmän kuin yksi ja ryhmän keskinäinen vuorovaikutus on tärkeää, käytetään termiä 'Kohderyhmäkeskustelu'.</skos:definition>
      <skos:prefLabel xml:lang="fi">Haastattelu</skos:prefLabel>
      <skos:definition xml:lang="fi">Ennalta suunniteltu, haastattelijan ja yhden tai useamman haastateltavan välinen keskustelu, jossa haastattelija saa tietoa tutkimustarkoituksiin. Käytä tarkempaa haastattelutermiä, mikäli mahdollista. Jos haastateltavia on enemmän kuin yksi ja ryhmän keskinäinen vuorovaikutus on tärkeää, käytetään termiä 'Kohderyhmäkeskustelu'.</skos:definition>
      <skos:prefLabel xml:lang="it">Intervista</skos:prefLabel>
      <skos:definition xml:lang="it">Una comunicazione pianificata tra due (o più) persone - l'intervistatore/i e l'intervistato/i - in cui le informazioni ottenute dall'intervistatore sono state rilasciate dagli intervistati. Se l'interazione di gruppo è parte della tecnica, utilizzare "Focus group".</skos:definition>
      <skos:prefLabel xml:lang="ja">インタビュー</skos:prefLabel>
      <skos:definition xml:lang="ja">インタビュアーとインタビューの対象という２人(あるいはそれよりも多い人々）の間で行われる、事前に計画されたコミュニケーション。インタビュアーはインタビューの対象から情報を取得する。もし、この方法の一環としてグループでのやり取りがある場合は、「フォーカスグループ」を当てはめること。</skos:definition>
      <skos:prefLabel xml:lang="lt">Interviu</skos:prefLabel>
      <skos:definition xml:lang="lt">Iš anksto suplanuotas dviejų (ar daugiau) žmonių – apklausėjo(-ų) ir apklausiamojo(-ųjų) – bendravimas, kurio metu iš apklausiamojo(-ųjų) informaciją gauna apklausėjas(-ai). Jei metodo taikymas reikalauja grupinės sąveikos, naudoti „Tikslinę grupės diskusiją“.</skos:definition>
      <skos:prefLabel xml:lang="nl">Interview</skos:prefLabel>
      <skos:definition xml:lang="nl"/>
      <skos:prefLabel xml:lang="no">Intervju</skos:prefLabel>
      <skos:definition xml:lang="no">En forhåndsplanlagt kommunikasjon mellom to (eller flere) personer – intervjueren(e) og intervjuobjekt(et/ene) – hvor intervjueren(e) henter informasjon fra intervjuobjekt(et/ene). Dersom gruppeinteraksjoner er del av metoden, bruk 'Fokusgruppe'.</skos:definition>
      <skos:prefLabel xml:lang="no">Intervju</skos:prefLabel>
      <skos:definition xml:lang="no">En forhåndsplanlagt kommunikasjon mellom to (eller flere) personer – intervjueren(e) og intervjuobjekt(et/ene) – hvor intervjueren(e) henter informasjon fra intervjuobjekt(et/ene). Dersom gruppeinteraksjoner er del av metoden, bruk 'Fokusgruppe'.</skos:definition>
      <skos:prefLabel xml:lang="pt">Entrevista</skos:prefLabel>
      <skos:definition xml:lang="pt">Uma comunicação pré-planeada entre duas (ou mais) pessoas - o(s) entrevistador(es) e o(s) entrevistado(s) - em que a informação é obtida pelo(s) entrevistador(es) do(s) entrevistado(s). Se a interação no grupo fizer parte do método, usar "Focus group".</skos:definition>
      <skos:prefLabel xml:lang="sl">Intervju</skos:prefLabel>
      <skos:definition xml:lang="sl">Vnaprej načrtovana komunikacija med dvema (ali več) osebami - spraševalcem(-ci) in spraševancem(-ci) -, kjer spraševalec(-ci) pridobi(jo) informacije s strani spraševanca(-cev). Če je v metodo vključena skupinska interakcija, uporabite izraz "fokusna skupina".</skos:definition>
      <skos:prefLabel xml:lang="sv">Intervju</skos:prefLabel>
      <skos:definition xml:lang="sv">Planerad kommunikation mellan två (eller flera) personer – intervjuare och intervjuobjekt – där intervjuaren/-na får information från intervjuobjektet/-en. Använd "Fokusgrupp" om gruppinteraktion är del av metoden.</skos:definition>
      <skos:narrower rdf:resource="http://rdf-vocabulary.ddialliance.org/cv/ModeOfCollection/4.0/d50e235"/>
      <skos:narrower rdf:resource="http://rdf-vocabulary.ddialliance.org/cv/ModeOfCollection/4.0/d50e511"/>
      <skos:narrower rdf:resource="http://rdf-vocabulary.ddialliance.org/cv/ModeOfCollection/4.0/d50e694"/>
      <skos:narrower rdf:resource="http://rdf-vocabulary.ddialliance.org/cv/ModeOfCollection/4.0/d50e784"/>
   </rdf:Description>
   <rdf:Description rdf:about="http://rdf-vocabulary.ddialliance.org/cv/ModeOfCollection/4.0/d50e235">
      <rdf:type rdf:resource="http://www.w3.org/2004/02/skos/core#Concept"/>
      <skos:inScheme rdf:resource="http://rdf-vocabulary.ddialliance.org/cv/ModeOfCollection/4.0/"/>
      <skos:notation>Interview.FaceToFace</skos:notation>
      <skos:prefLabel xml:lang="en">Face-to-face interview</skos:prefLabel>
      <skos:definition xml:lang="en">Data collection method in which a live interviewer conducts a personal interview, presenting questions and entering the responses. Use this broader term if not CAPI or PAPI, or if not known whether CAPI/PAPI or not.</skos:definition>
      <skos:prefLabel xml:lang="de">Persönliches Interview</skos:prefLabel>
      <skos:definition xml:lang="de">Datenerhebungsmethode, bei der ein/eine Live-Interviewer*in ein persönliches Interview durchführt, Fragen stellt und die Antworten eingibt. Verwenden Sie diesen weiter gefassten Begriff, wenn es sich nicht um CAPI oder PAPI handelt, oder wenn nicht bekannt ist, ob es sich um CAPI/PAPI handelt oder nicht.</skos:definition>
      <skos:prefLabel xml:lang="fi">Kasvokkainen haastattelu</skos:prefLabel>
      <skos:definition xml:lang="fi">Kasvokkain tehty yksilö- tai ryhmähaastattelu, jossa haastattelija esittää kysymykset ja taltioi vastaukset. Käytetään silloin, kun haastattelija tallentaa saamansa tiedot haastattelumuistiinpanoilla, tai haastattelu äänitetään tai videoidaan (eli ei mene mihinkään kasvokkaisen haastattelun alaluokkaan).</skos:definition>
      <skos:prefLabel xml:lang="fi">Kasvokkainen haastattelu</skos:prefLabel>
      <skos:definition xml:lang="fi">Kasvokkain tehty yksilö- tai ryhmähaastattelu, jossa haastattelija esittää kysymykset ja taltioi vastaukset. Käytetään silloin, kun haastattelija tallentaa saamansa tiedot haastattelumuistiinpanoilla, tai haastattelu äänitetään tai videoidaan (eli ei mene mihinkään kasvokkaisen haastattelun alaluokkaan).</skos:definition>
      <skos:prefLabel xml:lang="it">Intervista faccia a faccia</skos:prefLabel>
      <skos:definition xml:lang="it">Tecnica di raccolta dei dati in cui un intervistatore conduce un colloquio personale in presenza, facendo domande e registrando le risposte. Utilizzare questo termine più ampio se l'intervista non è CAPI o PAPI, o se non si è in grado di stabilire se sia CAPI o PAPI.</skos:definition>
      <skos:prefLabel xml:lang="ja">個別面接法</skos:prefLabel>
      <skos:definition xml:lang="ja">インタビュアーが対面で聞き取りを行い、質問を尋ね、回答を記入するデータ収集方法。CAPIでもPAPIでもない場合、あるいはCAPI/PAPIか不明な場合に、この広義の用語を用いる。</skos:definition>
      <skos:prefLabel xml:lang="lt">Tiesioginis interviu</skos:prefLabel>
      <skos:definition xml:lang="lt">Duomenų rinkimo metodas, kai apklausėjas asmeniškai atlieka interviu, pateikdamas klausimus ir fiksuodamas atsakymus. Naudoti šį platesnį terminą, kai netinka CAPI ar PAPI, arba jei nežinoma, ar tinka CAPI arba PAPI.</skos:definition>
      <skos:prefLabel xml:lang="nl">Face-to-face interview</skos:prefLabel>
      <skos:definition xml:lang="nl"/>
      <skos:prefLabel xml:lang="no">Personlig intervju</skos:prefLabel>
      <skos:definition xml:lang="no">Datainnsamlingsmetode hvor en tilstedeværende intervjuer gjennomfører et personlig intervju, presenterer spørsmål og registrerer svarene. Bruk dette bredere begrepet dersom det ikke er CATI eller PAPI, eller dersom det er uvisst om det er CATI/PAPI.</skos:definition>
      <skos:prefLabel xml:lang="no">Personlig intervju</skos:prefLabel>
      <skos:definition xml:lang="no">Datainnsamlingsmetode hvor en tilstedeværende intervjuer gjennomfører et personlig intervju, presenterer spørsmål og registrerer svarene. Bruk dette bredere begrepet dersom det ikke er CATI eller PAPI, eller dersom det er uvisst om det er CATI/PAPI.</skos:definition>
      <skos:prefLabel xml:lang="pt">Entrevista presencial</skos:prefLabel>
      <skos:definition xml:lang="pt">Método de recolha de dados em que um entrevistador presencial realiza uma entrevista pessoal, colocando as perguntas e inserindo as respostas. Usar este termo mais amplo se não for CAPI ou PAPI, ou se não souber se é CAPI/PAPI.</skos:definition>
      <skos:prefLabel xml:lang="sl">Osebni intervju</skos:prefLabel>
      <skos:definition xml:lang="sl">Metoda zbiranja podatkov, kjer spraševalec izvede osebni intervju, postavlja vprašanja in vnese odgovore. Uporabite ta širši izraz, če ne morete uporabiti CAPI ali PAPI ozioma ni znano, ali gre za CAPI/PAPI.</skos:definition>
      <skos:prefLabel xml:lang="sv">Personlig intervju</skos:prefLabel>
      <skos:definition xml:lang="sv">En närvarande intervjuare genomför en personlig intervju genom att ställa frågor och notera svaren. Använd denna bredare term om det inte rör sig om CAPI eller PAPI, eller om det inte är känt huruvida det rör sig om CAPI/PAPI eller inte.</skos:definition>
      <skos:narrower rdf:resource="http://rdf-vocabulary.ddialliance.org/cv/ModeOfCollection/4.0/d50e330"/>
      <skos:narrower rdf:resource="http://rdf-vocabulary.ddialliance.org/cv/ModeOfCollection/4.0/d50e420"/>
      <skos:broader rdf:resource="http://rdf-vocabulary.ddialliance.org/cv/ModeOfCollection/4.0/d50e136"/>
   </rdf:Description>
   <rdf:Description rdf:about="http://rdf-vocabulary.ddialliance.org/cv/ModeOfCollection/4.0/d50e330">
      <rdf:type rdf:resource="http://www.w3.org/2004/02/skos/core#Concept"/>
      <skos:inScheme rdf:resource="http://rdf-vocabulary.ddialliance.org/cv/ModeOfCollection/4.0/"/>
      <skos:notation>Interview.FaceToFace.CAPIorCAMI</skos:notation>
      <skos:prefLabel xml:lang="en">Face-to-face interview: Computer-assisted (CAPI/CAMI)</skos:prefLabel>
      <skos:definition xml:lang="en">Computer-assisted personal interviewing (CAPI), or computer-assisted mobile interviewing (CAMI). Data collection method in which the interviewer reads questions to the respondents from the screen of a computer, laptop, or a mobile device like tablet or smartphone, and enters the answers in the same device. The administration of the interview is managed by a specifically designed program/application.</skos:definition>
      <skos:prefLabel xml:lang="de">Persönliches Interview : Computerunterstützte Befragung (CAPI/CAMI)</skos:prefLabel>
      <skos:definition xml:lang="de">Computerunterstützte persönliche Befragung (CAPI) oder computerunterstützte mobile Befragung (CAMI). Eine Datenerhebungsmethode, bei der der/die Interviewer*in den Befragten die Fragen vom Bildschirm eines Computers, Laptops oder eines mobilen Geräts wie Tablet oder Smartphone vorliest und die Antworten in dasselbe Gerät eingibt. Die Durchführung des Interviews wird von einem speziell entwickelten Programm/einer Anwendung gesteuert.</skos:definition>
      <skos:prefLabel xml:lang="fi">Kasvokkainen haastattelu: tietokoneavusteinen (CAPI tai CAMI)</skos:prefLabel>
      <skos:definition xml:lang="fi">Computer-assisted personal interviewing (CAPI) tai Computer-assisted mobile interviewing (CAMI). Haastattelija lukee kysymykset kannettavalta tietokoneelta, kämmentietokoneelta, tabletista tai älypuhelimesta ja tallentaa haastateltavan vastaukset suoraan laitteeseen.</skos:definition>
      <skos:prefLabel xml:lang="fi">Kasvokkainen haastattelu: tietokoneavusteinen (CAPI tai CAMI)</skos:prefLabel>
      <skos:definition xml:lang="fi">Computer-assisted personal interviewing (CAPI) tai Computer-assisted mobile interviewing (CAMI). Haastattelija lukee kysymykset kannettavalta tietokoneelta, kämmentietokoneelta, tabletista tai älypuhelimesta ja tallentaa haastateltavan vastaukset suoraan laitteeseen.</skos:definition>
      <skos:prefLabel xml:lang="it">Intervista faccia a faccia: computer-assistita (CAPI/CAMI)</skos:prefLabel>
      <skos:definition xml:lang="it">Interviste personali assistite da computer (CAPI) o da cellulare (CAMI). Metodo di raccolta dei dati in cui l'intervistatore legge le domande ai rispondenti dallo schermo di un computer, laptop o dispositivo mobile come un tablet o uno smartphone e inserisce le risposte nello stesso dispositivo. L'intervista è gestita da un programma/applicazione appositamente progettata.</skos:definition>
      <skos:prefLabel xml:lang="ja">個別面接法：コンピューター支援型（CAPI/CAMI）</skos:prefLabel>
      <skos:definition xml:lang="ja">コンピュータ支援による対面インタビュー(CAPI)あるいはコンピュータ支援によるモバイルインタビュー(CAMI)。インタビュアーがコンピュータやラップトップ、あるいはタブレットやスマートフォンといったモバイル端末の画面から回答者に質問を読み上げ、その端末に答えを入力していく方法。インタビューの進行は専用のプログラム/アプリケーションにより管理される。</skos:definition>
      <skos:prefLabel xml:lang="lt">Tiesioginis interviu: kompiuterizuotas interviu (CAPI/CAMI)</skos:prefLabel>
      <skos:definition xml:lang="lt">Kompiuterizuotas tiesioginis interviu (CAPI) arba kompiuterizuotas interviu mobiliaisiais įrenginiais (CAMI). Duomenų rinkimo metodas, kai apklausėjas skaito klausimus respondentams iš kompiuterio, nešiojamojo kompiuterio ar mobiliojo prietaiso, pavyzdžiui, planšetinio kompiuterio ar išmaniojo telefono, ekrano ir įveda atsakymus į tą patį įrenginį. Interviu administravimas vykdomas specialiai sukurta kompiuterine programa.</skos:definition>
      <skos:prefLabel xml:lang="nl">Face-to-face interview: Computer-assisted (CAPI/CAMI)</skos:prefLabel>
      <skos:definition xml:lang="nl"/>
      <skos:prefLabel xml:lang="no">Personlig intervju: CAPI/CAMI</skos:prefLabel>
      <skos:definition xml:lang="no">Dataassistert personlig intervjuing (CAPI), eller dataassistert mobil intervjuing (CAMI). Datainnsamlingsmetode hvor intervjueren leser opp spørsmål for respondenten fra skjermen til en datamaskin, bærbar datamaskin, smarttelefon eller nettbrett, og registrerer svarene på det samme apparatet. Administreringen av intervjuet er styrt av et spesialdesignet program eller en applikasjon.</skos:definition>
      <skos:prefLabel xml:lang="no">Personlig intervju: CAPI/CAMI</skos:prefLabel>
      <skos:definition xml:lang="no">Dataassistert personlig intervjuing (CAPI), eller dataassistert mobil intervjuing (CAMI). Datainnsamlingsmetode hvor intervjueren leser opp spørsmål for respondenten fra skjermen til en datamaskin, bærbar datamaskin, smarttelefon eller nettbrett, og registrerer svarene på det samme apparatet. Administreringen av intervjuet er styrt av et spesialdesignet program eller en applikasjon.</skos:definition>
      <skos:prefLabel xml:lang="pt">Entrevista presencial: Assistida por computador (CAPI/CAMI)</skos:prefLabel>
      <skos:definition xml:lang="pt">Entrevista pessoal assistida por computador (Computer Assisted Personal Interviewing - CAPI) ou entrevista móvel assistida por computador (Computer Assisted Mobile Interviewing - CAMI). Modo de recolha de dados em que o entrevistador lê perguntas aos entrevistados na tela de um computador, laptop ou dispositivo móvel, como tablet ou smartphone, e insere as respostas no mesmo dispositivo. A administração da entrevista é gerida por um programa especialmente elaborado para o efeito.</skos:definition>
      <skos:prefLabel xml:lang="sl">Osebni intervju: CAPI/CAMI</skos:prefLabel>
      <skos:definition xml:lang="sl">Računalniško podprto osebno intervjuvanje (CAPI) ali računalniško podprto mobilno intervjuvanje (CAMI). Metoda zbiranja podatkov, kjer spraševalec prebere vprašanja spraševancu z zaslona na računalniku, prenosnem računalniku ali mobilni napravi, kot na primer na tablici ali pametnemu telefonu, in vnese odgovore v isto napravo. Intervju izvedemo s pomočjo posebej zasnovanega programa/ aplikacije.</skos:definition>
      <skos:prefLabel xml:lang="sv">Personlig intervju: CAPI/CAMI</skos:prefLabel>
      <skos:definition xml:lang="sv">Datorstödd personlig intervju. Intervjuaren läser frågor för respondenterna från en datorskärm eller mobil enhet (t.ex. surfplatta eller mobiltelefon) och skriver in svaren direkt i datorn. Intervjun hanteras med ett program som utvecklats för detta syfte.</skos:definition>
      <skos:broader rdf:resource="http://rdf-vocabulary.ddialliance.org/cv/ModeOfCollection/4.0/d50e235"/>
   </rdf:Description>
   <rdf:Description rdf:about="http://rdf-vocabulary.ddialliance.org/cv/ModeOfCollection/4.0/d50e420">
      <rdf:type rdf:resource="http://www.w3.org/2004/02/skos/core#Concept"/>
      <skos:inScheme rdf:resource="http://rdf-vocabulary.ddialliance.org/cv/ModeOfCollection/4.0/"/>
      <skos:notation>Interview.FaceToFace.PAPI</skos:notation>
      <skos:prefLabel xml:lang="en">Face-to-face interview: Paper-and-pencil (PAPI)</skos:prefLabel>
      <skos:definition xml:lang="en">Paper-and-pencil interviewing (PAPI). The interviewer uses a traditional paper questionnaire to read the questions and enter the answers.</skos:definition>
      <skos:prefLabel xml:lang="de">Persönliches Interview : Papier-und-Bleistift (PAPI)</skos:prefLabel>
      <skos:definition xml:lang="de">Der/die Interviewer*in verwendet einen traditionellen Papierfragebogen, um die Fragen zu vorzulesen und die Antworten einzutragen.</skos:definition>
      <skos:prefLabel xml:lang="fi">Kasvokkainen haastattelu: paperikyselylomake (PAPI)</skos:prefLabel>
      <skos:definition xml:lang="fi">Paper-and-pencil interviewing (PAPI). Paperilomaketta käyttäen tehty henkilökohtainen haastattelu. Haastattelija lukee kysymykset paperilomakkeelta ja kirjoittaa haastateltavan vastaukset lomakkeelle.</skos:definition>
      <skos:prefLabel xml:lang="fi">Kasvokkainen haastattelu: paperikyselylomake (PAPI)</skos:prefLabel>
      <skos:definition xml:lang="fi">Paper-and-pencil interviewing (PAPI). Paperilomaketta käyttäen tehty henkilökohtainen haastattelu. Haastattelija lukee kysymykset paperilomakkeelta ja kirjoittaa haastateltavan vastaukset lomakkeelle.</skos:definition>
      <skos:prefLabel xml:lang="it">Intervista faccia a faccia: carta e penna (PAPI)</skos:prefLabel>
      <skos:definition xml:lang="it">Interviste con carta e penna (PAPI). L'intervistatore utilizza un tradizionale questionario cartaceo per leggere le domande e inserire le risposte.</skos:definition>
      <skos:prefLabel xml:lang="ja">個別面接法： 紙と鉛筆 （PAPI）</skos:prefLabel>
      <skos:definition xml:lang="ja">紙と鉛筆でのインタビュー(PAPI)。インタビュアーは伝統的な紙の調査票を使って質問を読み上げ、答えを記入していく。</skos:definition>
      <skos:prefLabel xml:lang="lt">Tiesioginis interviu: interviu popieriumi ir pieštuku (PAPI)</skos:prefLabel>
      <skos:definition xml:lang="lt">Interviu popieriumi ir pieštuku (PAPI). Apklausėjas naudojasi tradiciniu popieriniu klausimynu, skaitydamas klausimus ir fiksuodamas atsakymus.</skos:definition>
      <skos:prefLabel xml:lang="nl">Face-to-face interview: Paper-and-pencil (PAPI)</skos:prefLabel>
      <skos:definition xml:lang="nl"/>
      <skos:prefLabel xml:lang="no">Personlig intervju: PAPI</skos:prefLabel>
      <skos:definition xml:lang="no">Penn og papir intervju. Intervjueren bruker et tradisjonelt papirspørreskjema for å lese opp spørsmålene og til å registrere svarene.</skos:definition>
      <skos:prefLabel xml:lang="no">Personlig intervju: PAPI</skos:prefLabel>
      <skos:definition xml:lang="no">Penn og papir intervju. Intervjueren bruker et tradisjonelt papirspørreskjema for å lese opp spørsmålene og til å registrere svarene.</skos:definition>
      <skos:prefLabel xml:lang="pt">Entrevista presencial: Papel e lápis (PAPI)</skos:prefLabel>
      <skos:definition xml:lang="pt">Entrevista de papel e lápis (PAPI - Paper-and-pencil interviewing). O entrevistador usa um questionário tradicional em papel para ler as perguntas e inserir as respostas.</skos:definition>
      <skos:prefLabel xml:lang="sl">Osebni intervju: PAPI</skos:prefLabel>
      <skos:definition xml:lang="sl">"Intervjuvanje s papirjem in svinčnikom". Spraševalec uporabi tradicionalni papirnati vprašalnik, s katerega prebere vprašanja in vnese odgovore.</skos:definition>
      <skos:prefLabel xml:lang="sv">Personlig intervju: PAPI</skos:prefLabel>
      <skos:definition xml:lang="sv">Papper-och-penna-intervju. Intervjuaren använder ett traditionellt frågeformulär på papper för att läsa frågorna och skriva ned svaren.</skos:definition>
      <skos:broader rdf:resource="http://rdf-vocabulary.ddialliance.org/cv/ModeOfCollection/4.0/d50e235"/>
   </rdf:Description>
   <rdf:Description rdf:about="http://rdf-vocabulary.ddialliance.org/cv/ModeOfCollection/4.0/d50e511">
      <rdf:type rdf:resource="http://www.w3.org/2004/02/skos/core#Concept"/>
      <skos:inScheme rdf:resource="http://rdf-vocabulary.ddialliance.org/cv/ModeOfCollection/4.0/"/>
      <skos:notation>Interview.Telephone</skos:notation>
      <skos:prefLabel xml:lang="en">Telephone interview</skos:prefLabel>
      <skos:definition xml:lang="en">Interview administered on the telephone. Use this broader term if not CATI, or if not known whether CATI or not.</skos:definition>
      <skos:prefLabel xml:lang="de">Telefonisches Interview</skos:prefLabel>
      <skos:definition xml:lang="de">Interview, das am Telefon durchgeführt wird. Verwenden Sie diesen weiter gefassten Begriff, wenn es sich nicht um CATI handelt, oder wenn nicht bekannt ist, ob es sich um CATI handelt oder nicht.</skos:definition>
      <skos:prefLabel xml:lang="fi">Puhelinhaastattelu</skos:prefLabel>
      <skos:definition xml:lang="fi">Puhelimitse tehty haastattelu. Termiä voi käyttää sekä kvalitatiivisesta että kvantitatiivisesta haastattelusta.</skos:definition>
      <skos:prefLabel xml:lang="fi">Puhelinhaastattelu</skos:prefLabel>
      <skos:definition xml:lang="fi">Puhelimitse tehty haastattelu. Termiä voi käyttää sekä kvalitatiivisesta että kvantitatiivisesta haastattelusta.</skos:definition>
      <skos:prefLabel xml:lang="it">Intervista telefonica</skos:prefLabel>
      <skos:definition xml:lang="it">Intervista somministrata via telefono. Utilizzare questo termine più generale se non è CATI, o se non si è in grado di stabilire se lo sia.</skos:definition>
      <skos:prefLabel xml:lang="ja">電話法</skos:prefLabel>
      <skos:definition xml:lang="ja">電話で行われるインタビュー。CATIではない、あるいはCATIかどうか不明な場合に、この広義の用語を用いる。</skos:definition>
      <skos:prefLabel xml:lang="lt">Interviu telefonu</skos:prefLabel>
      <skos:definition xml:lang="lt">Interviu vykdomas telefonu. Naudoti šį platesnį terminą, kai netinka CATI, arba jei nežinoma, ar tinka CATI.</skos:definition>
      <skos:prefLabel xml:lang="nl">Telefonisch interview</skos:prefLabel>
      <skos:definition xml:lang="nl"/>
      <skos:prefLabel xml:lang="no">Telefonintervju</skos:prefLabel>
      <skos:definition xml:lang="no">Intervju som gjennomføres over telefon. Bruk dette bredere begrepet dersom det ikke er CATI, eller dersom det er uvisst om det er CATI.</skos:definition>
      <skos:prefLabel xml:lang="no">Telefonintervju</skos:prefLabel>
      <skos:definition xml:lang="no">Intervju som gjennomføres over telefon. Bruk dette bredere begrepet dersom det ikke er CATI, eller dersom det er uvisst om det er CATI.</skos:definition>
      <skos:prefLabel xml:lang="pt">Entrevista telefónica</skos:prefLabel>
      <skos:definition xml:lang="pt">Entrevista realizada pelo telefone. Usar este termo mais amplo se não for CATI, ou se não souber se é CATI ou não.</skos:definition>
      <skos:prefLabel xml:lang="sl">Telefonski intervju</skos:prefLabel>
      <skos:definition xml:lang="sl">Intervju, izveden preko telefona. Uporabite ta širši izraz, če ni CATI, oziroma ne veste, ali je CATI ali ne.</skos:definition>
      <skos:prefLabel xml:lang="sv">Telefonintervju</skos:prefLabel>
      <skos:definition xml:lang="sv">Intervju som genomförs över telefon. Använd denna bredare term om det inte rör sig om CATI, eller om det inte är känt huruvida det rör sig om CATI.</skos:definition>
      <skos:narrower rdf:resource="http://rdf-vocabulary.ddialliance.org/cv/ModeOfCollection/4.0/d50e604"/>
      <skos:broader rdf:resource="http://rdf-vocabulary.ddialliance.org/cv/ModeOfCollection/4.0/d50e136"/>
   </rdf:Description>
   <rdf:Description rdf:about="http://rdf-vocabulary.ddialliance.org/cv/ModeOfCollection/4.0/d50e604">
      <rdf:type rdf:resource="http://www.w3.org/2004/02/skos/core#Concept"/>
      <skos:inScheme rdf:resource="http://rdf-vocabulary.ddialliance.org/cv/ModeOfCollection/4.0/"/>
      <skos:notation>Interview.Telephone.CATI</skos:notation>
      <skos:prefLabel xml:lang="en">Telephone interview: Computer-assisted (CATI)</skos:prefLabel>
      <skos:definition xml:lang="en">Computer-assisted telephone interviewing (CATI). The interviewer asks questions as directed by a computer, responses are keyed directly into the computer and the administration of the interview is managed by a specifically designed program.</skos:definition>
      <skos:prefLabel xml:lang="de">Telefonisches Interview: Computerunterstützte Befragung (CATI)</skos:prefLabel>
      <skos:definition xml:lang="de">Computerunterstützte telefonische Befragung (CATI). Der/die Interviewer*in stellt Fragen, die von einem Computer gesteuert werden, die Antworten werden direkt in den Computer eingegeben und die Durchführung des Interviews wird von einem speziell entwickelten Programm gesteuert.</skos:definition>
      <skos:prefLabel xml:lang="fi">Puhelinhaastattelu: tietokoneavusteinen (CATI)</skos:prefLabel>
      <skos:definition xml:lang="fi">Computer-assisted telephone interviewing (CATI). Haastattelija lukee kysymykset tietokoneelta puhelimessa ja tallentaa haastateltavan vastaukset suoraan tietokoneelle.</skos:definition>
      <skos:prefLabel xml:lang="fi">Puhelinhaastattelu: tietokoneavusteinen (CATI)</skos:prefLabel>
      <skos:definition xml:lang="fi">Computer-assisted telephone interviewing (CATI). Haastattelija lukee kysymykset tietokoneelta puhelimessa ja tallentaa haastateltavan vastaukset suoraan tietokoneelle.</skos:definition>
      <skos:prefLabel xml:lang="it">Intervista telefonica: assistita da computer (CATI)</skos:prefLabel>
      <skos:definition xml:lang="it">Intervista telefonica assistita da computer (CATI). L'intervistatore pone le domande indicate dal computer, le risposte sono immesse direttamente nel computer e l'intervista è gestita da un programma appositamente progettato.</skos:definition>
      <skos:prefLabel xml:lang="ja">電話法：コンピュータ支援 （CATI）</skos:prefLabel>
      <skos:definition xml:lang="ja">コンピュータ支援による電話インタビュー(CATI)。インタビュアーはコンピュータからの指示の通りに質問をし、回答はコンピュータに直接入力される。インタビューの進行は専用に設計されたプログラムにより管理される。</skos:definition>
      <skos:prefLabel xml:lang="lt">Telefoninis interviu: kompiuterizuotas interviu (CATI)</skos:prefLabel>
      <skos:definition xml:lang="lt">Kompiuterizuotas interviu telefonu (CATI). Apklausėjas užduoda klausimus pagal kompiuterio nurodymus, atsakymus įvesdamas tiesiai į kompiuterį, o pokalbio administravimą vykdo specialiai tam sukurta kompiuterinė programa.</skos:definition>
      <skos:prefLabel xml:lang="nl">Telefonisch interview: Computer-assisted (CATI)</skos:prefLabel>
      <skos:definition xml:lang="nl"/>
      <skos:prefLabel xml:lang="no">Telefonintervju: CATI</skos:prefLabel>
      <skos:definition xml:lang="no">Dataassistert telefonintervju (CATI). Intervjueren stiller spørsmål ifølge instrukser fra en datamaskin, registrerer svarene direkte på datamaskinen og administreringen av intervjuet er styrt av et spesialdesignet dataprogram.</skos:definition>
      <skos:prefLabel xml:lang="no">Telefonintervju: CATI</skos:prefLabel>
      <skos:definition xml:lang="no">Dataassistert telefonintervju (CATI). Intervjueren stiller spørsmål ifølge instrukser fra en datamaskin, registrerer svarene direkte på datamaskinen og administreringen av intervjuet er styrt av et spesialdesignet dataprogram.</skos:definition>
      <skos:prefLabel xml:lang="pt">Entrevista telefónica: Assistida por computador  (CATI)</skos:prefLabel>
      <skos:definition xml:lang="pt">Entrevista telefónica assistida por computador (Computer Assisted Telephone Interviewing - CATI). O entrevistador faz perguntas orientado por um computador, as respostas são inseridas diretamente no computador e a realização da entrevista é gerida por um programa especialmente elaborado para o efeito.</skos:definition>
      <skos:prefLabel xml:lang="sl">Telefonski intervju: CATI</skos:prefLabel>
      <skos:definition xml:lang="sl">Računalniško podprto telefonsko intervjuvanje. Spraševanec postavlja vprašanja, ki jih ponuja računalnik, odgovori se vnašajo neposredno v računalnik in intervju upravlja posebej za to zasnovan program.</skos:definition>
      <skos:prefLabel xml:lang="sv">Telefonintervju: CATI</skos:prefLabel>
      <skos:definition xml:lang="sv">Datorstödd telefonintervju. Intervjuaren läser frågor för respondenterna från en datorskärm och skriver in svaren direkt i datorn. Intervjun hanteras genom ett program som utvecklats för detta syfte.</skos:definition>
      <skos:broader rdf:resource="http://rdf-vocabulary.ddialliance.org/cv/ModeOfCollection/4.0/d50e511"/>
   </rdf:Description>
   <rdf:Description rdf:about="http://rdf-vocabulary.ddialliance.org/cv/ModeOfCollection/4.0/d50e694">
      <rdf:type rdf:resource="http://www.w3.org/2004/02/skos/core#Concept"/>
      <skos:inScheme rdf:resource="http://rdf-vocabulary.ddialliance.org/cv/ModeOfCollection/4.0/"/>
      <skos:notation>Interview.Email</skos:notation>
      <skos:prefLabel xml:lang="en">E-mail interview</skos:prefLabel>
      <skos:definition xml:lang="en">Interviews conducted via e-mail, usually consisting of several e-mail messages that allow the discussion to continue beyond the first set of questions and answers, or the first e-mail exchange.</skos:definition>
      <skos:prefLabel xml:lang="de">E-Mail Interview</skos:prefLabel>
      <skos:definition xml:lang="de">Interviews, die per E-Mail durchgeführt werden und in der Regel aus mehreren E-Mail-Nachrichten bestehen, die es ermöglichen, die Diskussion über den ersten Satz von Fragen und Antworten bzw. den ersten E-Mail-Austausch hinaus fortzusetzen.</skos:definition>
      <skos:prefLabel xml:lang="fi">Sähköpostihaastattelu</skos:prefLabel>
      <skos:definition xml:lang="fi">Haastattelu tehdään sähköpostin välityksellä. Usein sisältää useita sähköpostiviestejä, jotka mahdollistavat keskustelun jatkumisen alussa esitettyjen kysymysten ja niihin saatujen vastausten jälkeen.</skos:definition>
      <skos:prefLabel xml:lang="fi">Sähköpostihaastattelu</skos:prefLabel>
      <skos:definition xml:lang="fi">Haastattelu tehdään sähköpostin välityksellä. Usein sisältää useita sähköpostiviestejä, jotka mahdollistavat keskustelun jatkumisen alussa esitettyjen kysymysten ja niihin saatujen vastausten jälkeen.</skos:definition>
      <skos:prefLabel xml:lang="it">Intervista e-mail</skos:prefLabel>
      <skos:definition xml:lang="it">Interviste condotte via e-mail, di solito costituite da diversi messaggi di posta elettronica che consentono alla discussione di continuare oltre la prima serie di domande e risposte, oppure dopo il primo scambio di e-mail.</skos:definition>
      <skos:prefLabel xml:lang="ja">電子メール・インタビュー</skos:prefLabel>
      <skos:definition xml:lang="ja">電子メールによるインタビュー。多くの場合、最初の質疑応答や最初の電子メールでのやり取りだけでは終わらず、議論を続けるために複数の電子メールメッセージをやり取りする。</skos:definition>
      <skos:prefLabel xml:lang="lt">Interviu elektroniniu paštu</skos:prefLabel>
      <skos:definition xml:lang="lt">Interviu vykdomi elektroniniu paštu, dažniausiai susidedantys iš kelių elektroninio pašto laiškų, leidžiančių tęsti diskusiją po pirmos klausimų ir atsakymų sesijos arba po pirmojo apsikeitimo elektroniniais laiškais.</skos:definition>
      <skos:prefLabel xml:lang="nl">E-mail interview</skos:prefLabel>
      <skos:definition xml:lang="nl"/>
      <skos:prefLabel xml:lang="no">E-post intervju</skos:prefLabel>
      <skos:definition xml:lang="no">Intervjuer gjennomført over e-post, vanligvis bestående av en rekke e-poster som gjør at diskusjonen kan fortsette utover de første settene med spørsmål og svar, eller den første e-postutvekslingen.</skos:definition>
      <skos:prefLabel xml:lang="no">E-post intervju</skos:prefLabel>
      <skos:definition xml:lang="no">Intervjuer gjennomført over e-post, vanligvis bestående av en rekke e-poster som gjør at diskusjonen kan fortsette utover de første settene med spørsmål og svar, eller den første e-postutvekslingen.</skos:definition>
      <skos:prefLabel xml:lang="pt">Entrevista por email/correio eletrónico</skos:prefLabel>
      <skos:definition xml:lang="pt">Entrevistas realizadas via email, consistindo geralmente em várias mensagens de email que permitem que a discussão continue além do primeiro conjunto de perguntas e respostas, ou da primeira troca de emails.</skos:definition>
      <skos:prefLabel xml:lang="sl">Intervju preko elektronske pošte</skos:prefLabel>
      <skos:definition xml:lang="sl">Intervju, izveden preko elektronske pošte. Običajno ga sestavlja več elektronskih sporočil, ki omogočajo, da se pogovor nadaljuje tudi po prvem nizu vprašanj in odgovorov, ali po prvi izmenjavi elektronskih sporočil.</skos:definition>
      <skos:prefLabel xml:lang="sv">E-postintervju</skos:prefLabel>
      <skos:definition xml:lang="sv">Intervju som genomförs via e-post, vanligtvis över flera meddelanden som möjliggör att diskussionen fortsätter från den första uppsättningen av frågor och svar eller det första utbytet av e-brev.</skos:definition>
      <skos:broader rdf:resource="http://rdf-vocabulary.ddialliance.org/cv/ModeOfCollection/4.0/d50e136"/>
   </rdf:Description>
   <rdf:Description rdf:about="http://rdf-vocabulary.ddialliance.org/cv/ModeOfCollection/4.0/d50e784">
      <rdf:type rdf:resource="http://www.w3.org/2004/02/skos/core#Concept"/>
      <skos:inScheme rdf:resource="http://rdf-vocabulary.ddialliance.org/cv/ModeOfCollection/4.0/"/>
      <skos:notation>Interview.WebBased</skos:notation>
      <skos:prefLabel xml:lang="en">Web-based interview</skos:prefLabel>
      <skos:definition xml:lang="en">An interview conducted via the Internet. For example, interviews conducted within online forums or using web-based audio-visual technology that enables the interviewer(s) and interviewee(s) to communicate in real time.</skos:definition>
      <skos:prefLabel xml:lang="de">Webbasiertes Interview</skos:prefLabel>
      <skos:definition xml:lang="de">Ein Interview, das über das Internet geführt wird. Zum Beispiel Interviews, die in Online-Foren oder mit webbasierter audiovisueller Technologie durchgeführt werden, die es dem/der Interviewer*in bzw. den Interviewern und dem/der/den Befragten ermöglicht, in Echtzeit zu kommunizieren.</skos:definition>
      <skos:prefLabel xml:lang="fi">Verkkohaastattelu</skos:prefLabel>
      <skos:definition xml:lang="fi">Verkon välityksellä tehty haastattelu, esimerkiksi verkkokeskustelufoorumilla tai käyttäen teknologiaa, jonka avulla haastattelija ja haastateltava(t) voivat keskustella samanaikaisesti (chat, skype, videokonferenssit).</skos:definition>
      <skos:prefLabel xml:lang="fi">Verkkohaastattelu</skos:prefLabel>
      <skos:definition xml:lang="fi">Verkon välityksellä tehty haastattelu, esimerkiksi verkkokeskustelufoorumilla tai käyttäen teknologiaa, jonka avulla haastattelija ja haastateltava(t) voivat keskustella samanaikaisesti (chat, skype, videokonferenssit).</skos:definition>
      <skos:prefLabel xml:lang="it">Intervista web</skos:prefLabel>
      <skos:definition xml:lang="it">Un'intervista condotta via Internet. Ad esempio, interviste condotte all'interno di forum online o utilizzando la tecnologia audiovisiva basata sul web che consente all'intervistatore e agli intervistati di comunicare in tempo reale.</skos:definition>
      <skos:prefLabel xml:lang="ja">Webベースのインタビュー</skos:prefLabel>
      <skos:definition xml:lang="ja">インターネット経由で行われるインタビュー。例えば、オンラインフォーラム内で行われる、あるいはインタビュアーとインタビュー対象のリアルタイムでのやり取りを可能とするようなWebベースの視聴覚技術を使って行われるインタビュー。</skos:definition>
      <skos:prefLabel xml:lang="lt">Interviu internetu </skos:prefLabel>
      <skos:definition xml:lang="lt">Interviu atliekami internetu. Pavyzdžiui, interviu atliekami internetiniuose forumuose arba naudojant internetines garso ir vaizdo technologijas, leidžiančias apklausėjui (-ams) ir apklausiamajam (-siems) bendrauti realiu laiku.</skos:definition>
      <skos:prefLabel xml:lang="nl">Webgebaseerd interview</skos:prefLabel>
      <skos:definition xml:lang="nl"/>
      <skos:prefLabel xml:lang="no">Webbasert intervju</skos:prefLabel>
      <skos:definition xml:lang="no">Intervju gjennomført over internett. For eksempel, intervjuer gjennomført på internettforum eller ved bruk av internettbasert audiovisuell teknologi som muliggjør fortløpende kommunikasjon mellom intervjuer(e) og Intervjuobjekt(er).</skos:definition>
      <skos:prefLabel xml:lang="no">Webbasert intervju</skos:prefLabel>
      <skos:definition xml:lang="no">Intervju gjennomført over internett. For eksempel, intervjuer gjennomført på internettforum eller ved bruk av internettbasert audiovisuell teknologi som muliggjør fortløpende kommunikasjon mellom intervjuer(e) og Intervjuobjekt(er).</skos:definition>
      <skos:prefLabel xml:lang="pt">Entrevista via web (online)</skos:prefLabel>
      <skos:definition xml:lang="pt">Entrevistas realizadas via Internet. Por exemplo, entrevistas conduzidas em fóruns online ou utilizando tecnologia audiovisual baseada na web que permite ao(s) entrevistador(es) e entrevistado(s) comunicar em tempo real.</skos:definition>
      <skos:prefLabel xml:lang="sl">Spletni intervju</skos:prefLabel>
      <skos:definition xml:lang="sl">Intervju preko spleta. Na primer, intervjuji izvedeni znotraj spletnih forumov ali z uporabo spletno osnovanih avdio-vizualnih tehnologij, ki omogočajo komunikacijo spraševalca(-cev) in spraševanca(-cev) v realnem času.</skos:definition>
      <skos:prefLabel xml:lang="sv">Webbaserad intervju</skos:prefLabel>
      <skos:definition xml:lang="sv">Intervju som genomförs över Internet. Exempel inkluderar intervjuer genomförda på onlineforum eller med hjälp av webbaserad audiovisuell teknik som tillåter att intervjuare och intervjuobjekt kan kommunicera i realtid.</skos:definition>
      <skos:broader rdf:resource="http://rdf-vocabulary.ddialliance.org/cv/ModeOfCollection/4.0/d50e136"/>
   </rdf:Description>
   <rdf:Description rdf:about="http://rdf-vocabulary.ddialliance.org/cv/ModeOfCollection/4.0/d50e874">
      <rdf:type rdf:resource="http://www.w3.org/2004/02/skos/core#Concept"/>
      <skos:inScheme rdf:resource="http://rdf-vocabulary.ddialliance.org/cv/ModeOfCollection/4.0/"/>
      <skos:notation>SelfAdministeredQuestionnaire</skos:notation>
      <skos:prefLabel xml:lang="en">Self-administered questionnaire</skos:prefLabel>
      <skos:definition xml:lang="en">Data collection method in which the respondent reads or listens to the questions, and enters the responses by him/herself; no live interviewer is present, or participates in the questionnaire administration. If possible, use a narrower term. Use this broader term if the method is not described by any of the narrower terms - for example, for PDF and diskette questionnaires.</skos:definition>
      <skos:prefLabel xml:lang="de">Selbstausgefüllter Fragebogen</skos:prefLabel>
      <skos:definition xml:lang="de">Datenerhebungsmethode, bei der Befragte die Fragen lesen oder hören und die Antworten selbst eingeben; es ist kein Live-Interviewer anwesend oder beteiligt sich an der Fragebogenverwaltung. Wenn möglich, verwenden Sie einen engeren Begriff. Verwenden Sie diesen breiteren Begriff, wenn die Erhebungsmethode durch keinen der engeren Begriffe beschrieben wird - zum Beispiel für PDF- und Diskettenfragebögen.</skos:definition>
      <skos:prefLabel xml:lang="fi">Itsetäytettävä lomake</skos:prefLabel>
      <skos:definition xml:lang="fi">Tutkimuksen osanottaja täyttää kysely- tai ilmoituslomakkeen itsenäisesti. Pääluokkaa käytetään, jos ei tiedetä missä muodossa lomake on saatu ja palautettu tai jos ei puhtaasti mikään suppeampi termi.</skos:definition>
      <skos:prefLabel xml:lang="fi">Itsetäytettävä lomake</skos:prefLabel>
      <skos:definition xml:lang="fi">Tutkimuksen osanottaja täyttää kysely- tai ilmoituslomakkeen itsenäisesti. Pääluokkaa käytetään, jos ei tiedetä missä muodossa lomake on saatu ja palautettu tai jos ei puhtaasti mikään suppeampi termi.</skos:definition>
      <skos:prefLabel xml:lang="it">Questionario auto-compilato</skos:prefLabel>
      <skos:definition xml:lang="it">Tecnica di raccolta dei dati in cui il rispondente legge o ascolta le domande e inserisce autonomamente le risposte; nessun intervistatore è presente o partecipa alla somministrazione del questionario. Se possibile, utilizzare un termine più specifico. Utilizzare questo termine più ampio se il metodo non è descritto da nessuno dei termini più specifici, ad esempio per i questionari PDF o trasmessi via floppy disk.</skos:definition>
      <skos:prefLabel xml:lang="ja">自記式調査票</skos:prefLabel>
      <skos:definition xml:lang="ja">回答者が質問を読み、あるいは聞き、そのうえで自分自身で回答を記入するデータ収集方法。その場にインタビュアーはおらず、調査票の管理者としても参加しない。可能であれば意味を狭く限定した用語を用いること。この広義の用語は、例えばPDFやフロッピーディスクの調査票等、より限定的な言い方では表現できない方法に対して用いる。</skos:definition>
      <skos:prefLabel xml:lang="lt">Savipildos klausimynas</skos:prefLabel>
      <skos:definition xml:lang="lt">Duomenų rinkimo būdas, kai pats respondentas skaito ar klauso klausimus, ir pats įveda atsakymus; tiesioginio apklausėjo nėra, arba jis nedalyvauja administruojant klausimyną. Jei įmanoma, vartoti siauresnį terminą. Naudoti šį platesnį terminą, kai metodui apibūdinti netinka nė vienas siauresnis terminas, pavyzdžiui, PDF ir diskelių klausimynai.</skos:definition>
      <skos:prefLabel xml:lang="nl">Zelf ingevulde vragenlijst</skos:prefLabel>
      <skos:definition xml:lang="nl"/>
      <skos:prefLabel xml:lang="no">Selvadministrert spørreskjema</skos:prefLabel>
      <skos:definition xml:lang="no">Datainnsamlingsmetode hvor respondenten leser eller lytter til spørsmålene, og registrerer svarene på egenhånd; ingen intervjuer er til stede, eller deltar i administreringen av spørreskjemaet. Bruk et smalere begrep dersom det er mulig. Bruk dette bredere begrepet dersom metoden ikke kan defineres av de smalere begrepene, for eksempel for PDF eller diskett spørreskjemaer.</skos:definition>
      <skos:prefLabel xml:lang="no">Selvadministrert spørreskjema</skos:prefLabel>
      <skos:definition xml:lang="no">Datainnsamlingsmetode hvor respondenten leser eller lytter til spørsmålene, og registrerer svarene på egenhånd; ingen intervjuer er til stede, eller deltar i administreringen av spørreskjemaet. Bruk et smalere begrep dersom det er mulig. Bruk dette bredere begrepet dersom metoden ikke kan defineres av de smalere begrepene, for eksempel for PDF eller diskett spørreskjemaer.</skos:definition>
      <skos:prefLabel xml:lang="pt">Questionário de autopreenchimento</skos:prefLabel>
      <skos:definition xml:lang="pt">Método de recolha de dados em que o respondente lê ou ouve as perguntas e ele mesmo insere as respostas; nenhum entrevistador está presente, ou participa da administração do questionário. Se possível, usar um termo mais restrito. Usar este termo mais amplo se o método não for descrito por nenhum dos termos mais restritos - por exemplo, questionários em pdf ou em disquete.</skos:definition>
      <skos:prefLabel xml:lang="sl">Vprašalnik za samoizpolnjevanje</skos:prefLabel>
      <skos:definition xml:lang="sl">Metoda zbiranja podatkov, pri kateri spraševanec bere ali posluša vprašanja in sam vnaša odgovore; spraševalec ni prisoten niti ne sodeluje pri upravljanju vprašalnika. Če je možno, uporabite ožji izraz. Ta širši izraz uporabite le, če metoda ni opisana z nobenem od ožjih izrazov, npr. za PDF ali vprašalnike na disketi.</skos:definition>
      <skos:prefLabel xml:lang="sv">Självadministrerat frågeformulär</skos:prefLabel>
      <skos:definition xml:lang="sv">Respondenten läser eller lyssnar på frågorna och skriver själv in svaren; ingen intervjuare är närvarande eller deltar i administrerandet av frågeformuläret. Använd om möjligt en smalare term. Använd denna bredare term om metoden inte beskrivits av någon av de mer precisa termerna, till exempel för frågeformulär i PDF-format eller på diskett.</skos:definition>
      <skos:narrower rdf:resource="http://rdf-vocabulary.ddialliance.org/cv/ModeOfCollection/4.0/d50e975"/>
      <skos:narrower rdf:resource="http://rdf-vocabulary.ddialliance.org/cv/ModeOfCollection/4.0/d50e1066"/>
      <skos:narrower rdf:resource="http://rdf-vocabulary.ddialliance.org/cv/ModeOfCollection/4.0/d50e1156"/>
      <skos:narrower rdf:resource="http://rdf-vocabulary.ddialliance.org/cv/ModeOfCollection/4.0/d50e1246"/>
      <skos:narrower rdf:resource="http://rdf-vocabulary.ddialliance.org/cv/ModeOfCollection/4.0/d50e1336"/>
   </rdf:Description>
   <rdf:Description rdf:about="http://rdf-vocabulary.ddialliance.org/cv/ModeOfCollection/4.0/d50e975">
      <rdf:type rdf:resource="http://www.w3.org/2004/02/skos/core#Concept"/>
      <skos:inScheme rdf:resource="http://rdf-vocabulary.ddialliance.org/cv/ModeOfCollection/4.0/"/>
      <skos:notation>SelfAdministeredQuestionnaire.Email</skos:notation>
      <skos:prefLabel xml:lang="en">Self-administered questionnaire: E-mail</skos:prefLabel>
      <skos:definition xml:lang="en">Self-administered survey in which questions are presented to the respondent in the text body of an e-mail or as an attachment to an e-mail, but not as a link to a web-based questionnaire. Responses are also sent back via e-mail, in the e-mail body or as an attachment.</skos:definition>
      <skos:prefLabel xml:lang="de">Selbstausgefüllter Fragebogen: E-Mail</skos:prefLabel>
      <skos:definition xml:lang="de">Selbstverwaltete Umfrage, bei der die Fragen den Befragten im Textkörper einer E-Mail oder als Anhang zu einer E-Mail präsentiert werden, nicht aber als Link zu einem webbasierten Fragebogen. Die Antworten werden ebenfalls per E-Mail zurückgeschickt, im E-Mail-Textkörper oder als Anhang.</skos:definition>
      <skos:prefLabel xml:lang="fi">Itsetäytettävä lomake: sähköpostilomake</skos:prefLabel>
      <skos:definition xml:lang="fi">Osanottaja täyttää sähköpostin tekstiosiossa tai sähköpostin liitetiedostona tulleen kyselylomakkeen ja palauttaa sen sähköpostilla. Jos sähköpostissa on vain linkki verkkokyselylomakkeeseen, käytä termiä 'Itsetäytettävä lomake: verkkolomake'.</skos:definition>
      <skos:prefLabel xml:lang="fi">Itsetäytettävä lomake: sähköpostilomake</skos:prefLabel>
      <skos:definition xml:lang="fi">Osanottaja täyttää sähköpostin tekstiosiossa tai sähköpostin liitetiedostona tulleen kyselylomakkeen ja palauttaa sen sähköpostilla. Jos sähköpostissa on vain linkki verkkokyselylomakkeeseen, käytä termiä 'Itsetäytettävä lomake: verkkolomake'.</skos:definition>
      <skos:prefLabel xml:lang="it">Questionario auto-compilato: e-mail</skos:prefLabel>
      <skos:definition xml:lang="it">Questionario auto-compilato in cui le domande vengono presentate all'intervistato nel corpo del testo di un'e-mail o come allegato a un'e-mail, ma non come un collegamento a un questionario somministrato via web. Anche le risposte vengono rispedite via e-mail, nel corpo dell'e-mail o come allegato.</skos:definition>
      <skos:prefLabel xml:lang="ja">自記式調査票：電子メール</skos:prefLabel>
      <skos:definition xml:lang="ja">回答者に、電子メールのテキスト本文あるいは添付ファイルとして送られる自記式の調査。Webベースの調査票へのリンクを送付する場合は該当しない。回答も電子メールを通して電子メール本文あるいは添付ファイルとして返送される。</skos:definition>
      <skos:prefLabel xml:lang="lt">Savipildos klausimynas: elektroniniu paštu</skos:prefLabel>
      <skos:definition xml:lang="lt">Savipildos būdu atliekama apklausa, kurios metu respondentui klausimai pateikiami elektroninio laiško tekste arba prie elektroninio laiško pridedant priedą, bet ne kaip nuoroda į internetinę anketą. Atsakymai taip pat siunčiami elektroniniu laišku, jo pagrindiniame tekste arba kaip priedas.</skos:definition>
      <skos:prefLabel xml:lang="nl">Zelf ingevulde vragenlijst: E-mail</skos:prefLabel>
      <skos:definition xml:lang="nl"/>
      <skos:prefLabel xml:lang="no">Selvadministrert spørreskjema: E-post</skos:prefLabel>
      <skos:definition xml:lang="no">Undersøkelse hvor spørsmål blir presentert til respondenten som tekst i en e-post eller som et vedlegg i en e-post, men ikke som lenke til et web-basert spørreskjema. Svarene sendes også tilbake med e-post, enten som tekst i e-posten eller som et vedlegg.</skos:definition>
      <skos:prefLabel xml:lang="no">Selvadministrert spørreskjema: E-post</skos:prefLabel>
      <skos:definition xml:lang="no">Undersøkelse hvor spørsmål blir presentert til respondenten som tekst i en e-post eller som et vedlegg i en e-post, men ikke som lenke til et web-basert spørreskjema. Svarene sendes også tilbake med e-post, enten som tekst i e-posten eller som et vedlegg.</skos:definition>
      <skos:prefLabel xml:lang="pt">Questionário de autopreenchimento: Email/correio eletrónico</skos:prefLabel>
      <skos:definition xml:lang="pt">Questionário de autopreenchimento em que as perguntas são apresentadas ao respondente no corpo do texto de um email ou num anexo de um email, mas não como um link para um questionário baseado na web. As respostas são também devolvidas via email, no corpo do email ou como anexo.</skos:definition>
      <skos:prefLabel xml:lang="sl">Vprašalnik za samoizpolnjevanje: elektronska pošta</skos:prefLabel>
      <skos:definition xml:lang="sl">Vprašalnik za samoizpolnjevanje, kjer so spraševancu vprašanja prikazana bodisi kot besedilo v telesu elektronskega sporočila bodisi v priponki, vendar ne kot povezava do spletnega vprašalnika. Prav tako so tudi odgovori poslani preko elektronskega sporočila, bodisi v telesu elektronskega sporočila, bodisi kot priponka.</skos:definition>
      <skos:prefLabel xml:lang="sv">Självadministrerat frågeformulär: e-post</skos:prefLabel>
      <skos:definition xml:lang="sv">Självadministrerad surveyundersökning där frågor skickas till respondenten i brödtexten på, eller som en bilaga till, ett e-brev, inte som en länk till ett frågeformulär på webben. Svaren skickas tillbaka med e-post, i brödtexten eller som bilaga.</skos:definition>
      <skos:broader rdf:resource="http://rdf-vocabulary.ddialliance.org/cv/ModeOfCollection/4.0/d50e874"/>
   </rdf:Description>
   <rdf:Description rdf:about="http://rdf-vocabulary.ddialliance.org/cv/ModeOfCollection/4.0/d50e1066">
      <rdf:type rdf:resource="http://www.w3.org/2004/02/skos/core#Concept"/>
      <skos:inScheme rdf:resource="http://rdf-vocabulary.ddialliance.org/cv/ModeOfCollection/4.0/"/>
      <skos:notation>SelfAdministeredQuestionnaire.Paper</skos:notation>
      <skos:prefLabel xml:lang="en">Self-administered questionnaire: Paper</skos:prefLabel>
      <skos:definition xml:lang="en">Self-administered survey using a traditional paper questionnaire delivered and/or collected by mail (postal services), by fax, or in person by either interviewer, or respondent.</skos:definition>
      <skos:prefLabel xml:lang="de">Selbstausgefüllter Fragebogen: Papier</skos:prefLabel>
      <skos:definition xml:lang="de">Selbstverwaltete Umfrage unter Verwendung eines traditionellen Papierfragebogens, der per Post (Postdienste), per Fax oder persönlich entweder durch die Interviewer oder die Befragten zugestellt und/oder abgeholt wird.</skos:definition>
      <skos:prefLabel xml:lang="fi">Itsetäytettävä lomake: paperinen lomake</skos:prefLabel>
      <skos:definition xml:lang="fi">Osanottaja täyttää perinteisen paperisen kyselylomakkeen itse. Paperilomake voidaan lähettää tai palauttaa postissa, tai annetaan henkilökohtaisesti.</skos:definition>
      <skos:prefLabel xml:lang="fi">Itsetäytettävä lomake: paperinen lomake</skos:prefLabel>
      <skos:definition xml:lang="fi">Osanottaja täyttää perinteisen paperisen kyselylomakkeen itse. Paperilomake voidaan lähettää tai palauttaa postissa, tai annetaan henkilökohtaisesti.</skos:definition>
      <skos:prefLabel xml:lang="it">Questionario auto-compilato: cartaceo</skos:prefLabel>
      <skos:definition xml:lang="it">Questionario cartaceo tradizionale auto-compilato, consegnato e/o ritirato per posta (servizi postali), via fax o di persona dall'intervistatore oppure dall'intervistato.</skos:definition>
      <skos:prefLabel xml:lang="ja">自記式調査票：紙</skos:prefLabel>
      <skos:definition xml:lang="ja">伝統的な紙の調査票を用いた自記式の調査。調査票は郵送、ファックス、あるいは調査員により対面で配布、収集される。回答者自身が調査票を受け取り、あるいは届ける場合を含む。</skos:definition>
      <skos:prefLabel xml:lang="lt">Savipildos klausimynas: popieriuje </skos:prefLabel>
      <skos:definition xml:lang="lt">Savipildos būdu atliekama apklausa, naudojant tradicinį popierinį klausimyną, kai klausimynas pateikiamas ir (arba) surenkamas paštu (pašto paslauga), faksu arba asmeniškai paties apklausėjo ar respondento.</skos:definition>
      <skos:prefLabel xml:lang="nl">Zelf ingevulde vragenlijst: Papier</skos:prefLabel>
      <skos:definition xml:lang="nl"/>
      <skos:prefLabel xml:lang="no">Selvadministrert spørreskjema: Papir</skos:prefLabel>
      <skos:definition xml:lang="no">Selvadministrert spørreskjema som bruker tradisjonelle spørsmålsformuleringer på papir, som blir levert og/eller samlet inn via post, faks, eller personlig av intervjueren eller respondenten.</skos:definition>
      <skos:prefLabel xml:lang="no">Selvadministrert spørreskjema: Papir</skos:prefLabel>
      <skos:definition xml:lang="no">Selvadministrert spørreskjema som bruker tradisjonelle spørsmålsformuleringer på papir, som blir levert og/eller samlet inn via post, faks, eller personlig av intervjueren eller respondenten.</skos:definition>
      <skos:prefLabel xml:lang="pt">Questionário de autopreenchimento: Papel</skos:prefLabel>
      <skos:definition xml:lang="pt">Questionário de autopreenchimento utilizando um questionário tradicional em papel entregue e/ou recolhido por correio (serviços postais), por fax ou pessoalmente, seja pelo entrevistador ou pelo respondente.</skos:definition>
      <skos:prefLabel xml:lang="sl">Vprašalnik za samoizpolnjevanje: papirnati</skos:prefLabel>
      <skos:definition xml:lang="sl">Vprašalnik za samoizpolnjevanje z uporabo tradicionalnega papirnatega vprašalnika poslanega in/ali prejetega preko tradicionalne poštne storitve, preko faksa ali osebno preko spraševalca ali spraševanca.</skos:definition>
      <skos:prefLabel xml:lang="sv">Självadministrerat frågeformulär: papper</skos:prefLabel>
      <skos:definition xml:lang="sv">Självadministrerad surveyundersökning som använder traditionella frågeformulär på papper, vilka skickas ut och/eller in via post eller fax, eller lämnas över personligen av antingen intervjuaren eller intervjuobjektet.</skos:definition>
      <skos:broader rdf:resource="http://rdf-vocabulary.ddialliance.org/cv/ModeOfCollection/4.0/d50e874"/>
   </rdf:Description>
   <rdf:Description rdf:about="http://rdf-vocabulary.ddialliance.org/cv/ModeOfCollection/4.0/d50e1156">
      <rdf:type rdf:resource="http://www.w3.org/2004/02/skos/core#Concept"/>
      <skos:inScheme rdf:resource="http://rdf-vocabulary.ddialliance.org/cv/ModeOfCollection/4.0/"/>
      <skos:notation>SelfAdministeredQuestionnaire.SMSorMMS</skos:notation>
      <skos:prefLabel xml:lang="en">Self-administered questionnaire: Messaging (SMS/MMS)</skos:prefLabel>
      <skos:definition xml:lang="en">Self-administered survey in which the respondents receive the questions incorporated in SMS (text messages) or MMS (messages including multimedia content) and send their replies in the same format.</skos:definition>
      <skos:prefLabel xml:lang="de">Selbstausgefüllter Fragebogen: Nachrichtenübermittlung (SMS/MMS)</skos:prefLabel>
      <skos:definition xml:lang="de">Selbstverwaltete Umfrage, bei der die Befragten die Fragen in SMS (Textnachrichten) oder MMS (Nachrichten mit multimedialen Inhalten) eingebunden erhalten und ihre Antworten im gleichen Format senden.</skos:definition>
      <skos:prefLabel xml:lang="fi">Itsetäytettävä lomake: tekstiviesti- tai mobiililaitelomake (SMS tai MMS)</skos:prefLabel>
      <skos:definition xml:lang="fi">Osanottaja täyttää tekstiviestinä tai mobiililaitekyselynä välitetyn kyselylomakkeen itse ja palauttaa sen samalla teknologialla.</skos:definition>
      <skos:prefLabel xml:lang="fi">Itsetäytettävä lomake: tekstiviesti- tai mobiililaitelomake (SMS tai MMS)</skos:prefLabel>
      <skos:definition xml:lang="fi">Osanottaja täyttää tekstiviestinä tai mobiililaitekyselynä välitetyn kyselylomakkeen itse ja palauttaa sen samalla teknologialla.</skos:definition>
      <skos:prefLabel xml:lang="it">Questionario auto-compilato: messaggistica (SMS/MMS)</skos:prefLabel>
      <skos:definition xml:lang="it">Questionario auto-compilato in cui gli intervistati ricevono le domande all'interno di in SMS (messaggi di testo) o MMS (messaggi che includono contenuti multimediali) e inviano le loro risposte nello stesso formato.</skos:definition>
      <skos:prefLabel xml:lang="ja">自記式調査票：メッセージング（SMS/MMS）</skos:prefLabel>
      <skos:definition xml:lang="ja">回答者がSMS（テキストメッセージ）かMMS（動画や音声、静止画、文章等を組み合わせたメッセージ）に記されてる質問を受け取り、同じフォーマットで回答を送る自記式の調査。</skos:definition>
      <skos:prefLabel xml:lang="lt">Savipildos klausimynas: žinutėmis (SMS/MMS)</skos:prefLabel>
      <skos:definition xml:lang="lt">Savipildos būdu atliekama apklausa, kurios metu respondentai gauna klausimus kaip SMS (tekstine žinute) arba MMS (žinutes, įtraukiančias daugialypės terpės turinį), ir siunčia savo atsakymus tuo pačiu formatu.</skos:definition>
      <skos:prefLabel xml:lang="nl">Zelf ingevulde vragenlijst: Bericht (SMS/MMS)</skos:prefLabel>
      <skos:definition xml:lang="nl"/>
      <skos:prefLabel xml:lang="no">Selvadministrert spørreskjema: SMS/MMS</skos:prefLabel>
      <skos:definition xml:lang="no">Selvadministrert spørreskjema hvor respondenten mottar spørsmål på SMS (tekstmeldinger) eller MMS (meldinger med multimedia innhold) og sender svarene i samme format.</skos:definition>
      <skos:prefLabel xml:lang="no">Selvadministrert spørreskjema: SMS/MMS</skos:prefLabel>
      <skos:definition xml:lang="no">Selvadministrert spørreskjema hvor respondenten mottar spørsmål på SMS (tekstmeldinger) eller MMS (meldinger med multimedia innhold) og sender svarene i samme format.</skos:definition>
      <skos:prefLabel xml:lang="pt">Questionário de autopreenchimento: Mensagem (SMS/MMS)</skos:prefLabel>
      <skos:definition xml:lang="pt">Questionário de autopreenchimento em que os respondentes recebem as perguntas incorporadas em SMS (mensagens de texto) ou MMS (mensagens que incluem conteúdo multimédia) e enviam as suas respostas no mesmo formato.</skos:definition>
      <skos:prefLabel xml:lang="sl">Vprašalnik za samoizpolnjevanje: SMS/MMS</skos:prefLabel>
      <skos:definition xml:lang="sl">Vprašalnik za samoizpolnjevanje, kjer spraševanec prejme vprašanja, vključena v kratkih sporočilih v formatu SMS (tekstovna sporočila) ali MMS (multimedijska sporočila) in odgovore pošlje v enakem formatu.</skos:definition>
      <skos:prefLabel xml:lang="sv">Självadministrerat frågeformulär: SMS/MMS</skos:prefLabel>
      <skos:definition xml:lang="sv">Självadministrerad surveyundersökning där frågor och svar inkluderas i SMS (textmeddelanden) eller MMS (meddelanden med multimedia-innehåll) som skickas mellan mobiltelefoner.</skos:definition>
      <skos:broader rdf:resource="http://rdf-vocabulary.ddialliance.org/cv/ModeOfCollection/4.0/d50e874"/>
   </rdf:Description>
   <rdf:Description rdf:about="http://rdf-vocabulary.ddialliance.org/cv/ModeOfCollection/4.0/d50e1246">
      <rdf:type rdf:resource="http://www.w3.org/2004/02/skos/core#Concept"/>
      <skos:inScheme rdf:resource="http://rdf-vocabulary.ddialliance.org/cv/ModeOfCollection/4.0/"/>
      <skos:notation>SelfAdministeredQuestionnaire.CAWI</skos:notation>
      <skos:prefLabel xml:lang="en">Self-administered questionnaire: Web-based (CAWI)</skos:prefLabel>
      <skos:definition xml:lang="en">Computer-assisted web interviewing (CAWI). Data are collected using a web questionnaire, produced with a program for creating web surveys. The program can customize the flow of the questionnaire based on the answers provided, and can allow for the questionnaire to contain pictures, audio and video clips, links to different web pages etc.</skos:definition>
      <skos:prefLabel xml:lang="de">Selbstausgefüllter Fragebogen: Webbasiert (CAWI)</skos:prefLabel>
      <skos:definition xml:lang="de">Computerunterstützte Webbefragung (CAWI). Die Daten werden mithilfe eines Web-Fragebogens erhoben, der mit einem Programm zur Erstellung von Web-Umfragen erstellt wird. Das Programm kann den Ablauf des Fragebogens auf der Grundlage der gegebenen Antworten anpassen und es ermöglichen, dass der Fragebogen Bilder, Audio- und Videoclips, sowie Links zu verschiedenen Webseiten usw. enthält.</skos:definition>
      <skos:prefLabel xml:lang="fi">Itsetäytettävä lomake: verkkolomake</skos:prefLabel>
      <skos:definition xml:lang="fi">Osanottaja täyttää kysely- tai ilmoituslomakkeen verkossa itse (Computer-assisted web interviewing, CAWI). Lomake voi olla dynaaminen tai muuttumaton. Dynaamisessa lomakkeessa kysymysten järjestys sekä esitetyt kysymykset riippuvat edeltäviin kysymyksiin annetuista vastauksista. Lomake voi myös sisältää kuvia, video- tai äänitiedostoja, linkkejä toisiin verkkosivuihin jne.</skos:definition>
      <skos:prefLabel xml:lang="fi">Itsetäytettävä lomake: verkkolomake</skos:prefLabel>
      <skos:definition xml:lang="fi">Osanottaja täyttää kysely- tai ilmoituslomakkeen verkossa itse (Computer-assisted web interviewing, CAWI). Lomake voi olla dynaaminen tai muuttumaton. Dynaamisessa lomakkeessa kysymysten järjestys sekä esitetyt kysymykset riippuvat edeltäviin kysymyksiin annetuista vastauksista. Lomake voi myös sisältää kuvia, video- tai äänitiedostoja, linkkejä toisiin verkkosivuihin jne.</skos:definition>
      <skos:prefLabel xml:lang="it">Questionario auto-compilato: web (CAWI)</skos:prefLabel>
      <skos:definition xml:lang="it">Intervista web assistita da computer (CAWI). I dati vengono raccolti utilizzando un questionario via web, prodotto con un programma per la creazione di indagini via web. Il programma può personalizzare la struttura del questionario in base alle risposte fornite, e può consentire al questionario di contenere immagini, clip audio e video, collegamenti a pagine web diverse, ecc.</skos:definition>
      <skos:prefLabel xml:lang="ja">自記式調査票：Webベース（CAWI）</skos:prefLabel>
      <skos:definition xml:lang="ja">コンピュータ支援によるWebインタビュー(CAWI)。Web調査の作成プログラムで制作したWeb調査票を使ってデータは収集される。このプログラムは回答をもとに調査票の流れをカスタマイズできるほか、調査票に写真、音声、そしてビデオクリップ、別のWebサイトへのリンク等を含めることもできる。</skos:definition>
      <skos:prefLabel xml:lang="lt">Savipildos klausimynas: internetu (CAWI)</skos:prefLabel>
      <skos:definition xml:lang="lt">Kompiuterizuotas interviu internetu (CAWI). Duomenys renkami naudojant internetinį klausimyną, parengtą su internetinių apklausų kūrimo programa. Priklausomai nuo pateikiamų atsakymų, programa gali pritaikyti klausimų eiliškumą. Tokia programa taip pat leidžia į klausimyną įdėti paveikslėlius, garso ir vaizdo įrašus, nuorodas į įvairius tinklalapius ir kt.</skos:definition>
      <skos:prefLabel xml:lang="nl">Zelf ingevulde vragenlijst: Webgebaseerd (CAWI)</skos:prefLabel>
      <skos:definition xml:lang="nl"/>
      <skos:prefLabel xml:lang="no">Selvadministrert spørreskjema: Webbasert (CAWI)</skos:prefLabel>
      <skos:definition xml:lang="no">Datamaskinaassistert webintervju (CAWI). Data samles ved hjelp av spørreskjema på nett, som er produsert av et program for internettundersøkelser. Programmet kan endre flyten av spørsmål basert på svarene som blir gitt, og det muliggjør inkludering av bilde, lyd og video, lenker til andre nettsider etc.</skos:definition>
      <skos:prefLabel xml:lang="no">Selvadministrert spørreskjema: Webbasert (CAWI)</skos:prefLabel>
      <skos:definition xml:lang="no">Datamaskinaassistert webintervju (CAWI). Data samles ved hjelp av spørreskjema på nett, som er produsert av et program for internettundersøkelser. Programmet kan endre flyten av spørsmål basert på svarene som blir gitt, og det muliggjør inkludering av bilde, lyd og video, lenker til andre nettsider etc.</skos:definition>
      <skos:prefLabel xml:lang="pt">Questionário de autopreenchimento: via web (CAWI)</skos:prefLabel>
      <skos:definition xml:lang="pt">Entrevista via web, assistida por computador (Computer Assisted Web Interviewing - CAWI). Os dados são recolhidos através de um questionário na web, produzido com um programa para criar inquéritos na web. O programa pode personalizar o fluxo do questionário de acordo com as respostas e permite que este contenha imagens, clipes de áudio e vídeo, links para diferentes páginas da web, etc.</skos:definition>
      <skos:prefLabel xml:lang="sl">Vprašalnik za samoizpolnjevanje: spletni</skos:prefLabel>
      <skos:definition xml:lang="sl">Računalniško podprto spletno intervjuvanje (CAWI). Podatki so zbrani z uporabo spletnega vprašalnika, ustvarjenega v programskem orodju za spletno anketiranje. Program lahko tok vprašalnika prilagodi odgovorom na prejšnja vprašanja, omogoča lahko vstavljanje slik ter avdio in video posnetkov, povezave do spletnih strani itd.</skos:definition>
      <skos:prefLabel xml:lang="sv">Självadministrerat frågeformulär: webbaserat</skos:prefLabel>
      <skos:definition xml:lang="sv">Computer-assisted web interviewing (CAWI). Data samlas in med ett webbformulär som producerats av ett program som skapar webbsurveyer. Programmet kan anpassa flödet i frågeformuläret utifrån svaren som ges och det går att inkludera bilder, ljud- och videoklipp, länkar till andra webbsidor m.m. (Anpassad från Wikipedia.)</skos:definition>
      <skos:broader rdf:resource="http://rdf-vocabulary.ddialliance.org/cv/ModeOfCollection/4.0/d50e874"/>
   </rdf:Description>
   <rdf:Description rdf:about="http://rdf-vocabulary.ddialliance.org/cv/ModeOfCollection/4.0/d50e1336">
      <rdf:type rdf:resource="http://www.w3.org/2004/02/skos/core#Concept"/>
      <skos:inScheme rdf:resource="http://rdf-vocabulary.ddialliance.org/cv/ModeOfCollection/4.0/"/>
      <skos:notation>SelfAdministeredQuestionnaire.CASI</skos:notation>
      <skos:prefLabel xml:lang="en">Self-administered questionnaire: Computer-assisted (CASI)</skos:prefLabel>
      <skos:definition xml:lang="en">Computer-assisted self-interview (CASI). Respondents enter the responses into a computer (desktop, laptop, Palm/PDA, tablet, etc.) by themselves. The administration of the questionnaire is managed by a specifically designed program/application but there is no real-time data transfer as in CAWI, the answers are stored on the device used for the interview. The questionnaire may be fixed form or interactive. Includes VCASI (Video computer-assisted self-interviewing), ACASI (Audio computer-assisted self-interviewing) and TACASI (Telephone audio computer-assisted self-interviewing).</skos:definition>
      <skos:prefLabel xml:lang="de">Selbstausgefüllter Fragebogen: Computerunterstützt (CASI)</skos:prefLabel>
      <skos:definition xml:lang="de">Computerunterstütztes Selbstinterview (CASI). Die Befragten geben die Antworten selbst in einen Computer (Desktop, Laptop, Palm/PDA, Tablet, etc.) ein. Die Steuerung des Fragebogens wird von einem speziell entwickelten Programm/einer Anwendung verwaltet, aber es gibt keine Echtzeit-Datenübertragung wie bei CAWI, sondern die Antworten werden auf dem für das Interview verwendeten Gerät gespeichert. Der Fragebogen kann in starrer Form oder interaktiv sein. Beinhaltet VCASI (Video computer-assisted self-interviewing), ACASI (Audio computer-assisted self-interviewing) und TACASI (Telephone audio computer-assisted self-interviewing).</skos:definition>
      <skos:prefLabel xml:lang="fi">Itsetäytettävä lomake: tietokoneavusteinen (CASI)</skos:prefLabel>
      <skos:definition xml:lang="fi">Tietokoneavusteinen itsetäytettävä kyselylomake, jossa vastaaja tallentaa itse vastauksensa tietokoneelle (pöytäkone, kannettava tietokone tai kämmentietokone). Tiedot eivät siirry verkon kautta vaan taltioituvat vain tietokoneelle. Lomake voi olla dynaaminen tai muuttumaton. Termi sisältää myös harvoin käytetyt VCASI:n (Video computer-assisted self-interviewing), ACASI:n (Audio computer-assisted self-interviewing) ja TACASI:n (Telephone audio computer-assisted self-interviewing).</skos:definition>
      <skos:prefLabel xml:lang="fi">Itsetäytettävä lomake: tietokoneavusteinen (CASI)</skos:prefLabel>
      <skos:definition xml:lang="fi">Tietokoneavusteinen itsetäytettävä kyselylomake, jossa vastaaja tallentaa itse vastauksensa tietokoneelle (pöytäkone, kannettava tietokone tai kämmentietokone). Tiedot eivät siirry verkon kautta vaan taltioituvat vain tietokoneelle. Lomake voi olla dynaaminen tai muuttumaton. Termi sisältää myös harvoin käytetyt VCASI:n (Video computer-assisted self-interviewing), ACASI:n (Audio computer-assisted self-interviewing) ja TACASI:n (Telephone audio computer-assisted self-interviewing).</skos:definition>
      <skos:prefLabel xml:lang="it">Questionario auto-compilato: computer-assistito (CASI)</skos:prefLabel>
      <skos:definition xml:lang="it">Auto-compilazione del questionario assistita da computer (CASI). Gli intervistati inseriscono autonomamente le risposte in un computer (desktop, laptop, palmare, tablet, ecc.). La somministrazione del questionario è gestita da un programma/applicazione appositamente progettato, ma non esiste un trasferimento dati in tempo reale come nel CAWI poiché le risposte vengono memorizzate sul dispositivo utilizzato per l'intervista. Il questionario può essere fisso o interattivo. I tipi di questionario possono essere: VCASI (video assistito), ACASI (audio assistito) e TACASI (assistito via telefono).</skos:definition>
      <skos:prefLabel xml:lang="ja">自記式調査票：コンピュータ支援型（CASI）</skos:prefLabel>
      <skos:definition xml:lang="ja">コンピュータ支援による自記式調査（CASI）。回答者は自分でコンピュータ（デスクトップ、ラップトップ、パーム/PDA、タブレット等）に回答を入力する。調査票の進行は専用に設計されたプログラム/アプリケーションにより管理されるものの、CAWIのようにリアルタイムでデータが転送されることはなく、回答は調査に使われる端末に保存される。調査票は固定式、あるいは対話方式のいずれもありうる。VCASI (ビデオコンピュータ支援による自記式調査)、 ACASI (音声コンピュータ支援による自記式調査)、およびTACASI (電話音声コンピュータ支援による自記式調査)を含む。</skos:definition>
      <skos:prefLabel xml:lang="lt">Savipildos klausimynas: kompiuteriu (CASI)</skos:prefLabel>
      <skos:definition xml:lang="lt">Savarankiškas interviu kompiuteriu (CASI). Respondentai patys įveda atsakymus į kompiuterį (stalinį, nešiojamą, delninį, planšetinį kompiuterį ir kt.). Klausimyno administravimas vykdomas specialiai sukurta kompiuterine programa, tačiau duomenų perdavimas realiuoju laiku nevyksta, kaip CAWI, atsakymai saugomi apklausai naudojamame įrenginyje. Klausimynas gali būti fiksuotos formos arba interaktyvus. Apima VCASI (savarankiškas vaizdo interviu kompiuteriu), ACASI (savarankiškas garso interviu kompiuteriu) ir TACASI (savarankiškas telefoninio garso interviu kompiuteriu).</skos:definition>
      <skos:prefLabel xml:lang="nl">Zelf ingevulde vragenlijst: Computer-assisted (CASI)</skos:prefLabel>
      <skos:definition xml:lang="nl"/>
      <skos:prefLabel xml:lang="no">Selvadministrert spørreskjema: Datamaskinassistert (CASI)</skos:prefLabel>
      <skos:definition xml:lang="no">Datamaskinassistert selvadministrert intervju (CASI). Respondentene registrerer svarene på en datamaskin (stasjonær, bærbar, digital personlig assistent, nettbrett etc.) på egenhånd. Administreringen av spørreskjemaet er styrt av et spesialdesignet program eller en applikasjon men det er ingen fortløpende datautveksling slik som i CAWI, svarene blir lagret på apparatet som brukes for å gjennomføre intervjuet. Spørreskjemaet kan enten være fastsatt eller interaktivt. Omfatter VCASI (video computer-assisted self-interview), ACASI (audio computer-assisted self-interview) og TACASI (telephone audio computer-assisted self-interview).</skos:definition>
      <skos:prefLabel xml:lang="no">Selvadministrert spørreskjema: Datamaskinassistert (CASI)</skos:prefLabel>
      <skos:definition xml:lang="no">Datamaskinassistert selvadministrert intervju (CASI). Respondentene registrerer svarene på en datamaskin (stasjonær, bærbar, digital personlig assistent, nettbrett etc.) på egenhånd. Administreringen av spørreskjemaet er styrt av et spesialdesignet program eller en applikasjon men det er ingen fortløpende datautveksling slik som i CAWI, svarene blir lagret på apparatet som brukes for å gjennomføre intervjuet. Spørreskjemaet kan enten være fastsatt eller interaktivt. Omfatter VCASI (video computer-assisted self-interview), ACASI (audio computer-assisted self-interview) og TACASI (telephone audio computer-assisted self-interview).</skos:definition>
      <skos:prefLabel xml:lang="pt">Questionário de autopreenchimento: Assistido por computador (CASI)</skos:prefLabel>
      <skos:definition xml:lang="pt">Entrevista de autopreenchimento assistida por computador (Computer-assisted self-interview - CASI). Os entrevistados inserem as respostas num computador (desktop, laptop, PDA, tablet, etc.) por eles próprios. A administração do questionário é gerida por um programa/aplicação especialmente elaborado para o efeito, mas não há transferência de dados em tempo real, como no CAWI, e as respostas são armazenadas no dispositivo usado para a entrevista. O questionário pode ter um formato fixo ou interativo. Inclui a entrevista auto-administrada de vídeo assistida por computador (VCASI - Video computer-assisted self-interviewing), a entrevista auto-administrada de áudio assistida por computador (ACASI - Audio computer-assisted self-interviewing) e a entrevista de áudio e telefone assistida por computador (TACASI - Telephone audio computer-assisted self-interviewing).</skos:definition>
      <skos:prefLabel xml:lang="sl">Vprašalnik za samoizpolnjevanje: računalniško podprti (CASI)</skos:prefLabel>
      <skos:definition xml:lang="sl">Računalniško podprto samoizpolnjevanje (CASI). Spraševanec sam vstavlja odgovore v računalnik (namizni, prenosni, dlančni/PDA, tablični itd.). Z vprašalnikom upravlja posebej zasnovani program/aplikacija, vendar pri tem ni prenosa v realnem času kot pri CAWI, vprašanja se shranjujejo na napravi, ki se uporablja za intervju. Vprašalnik je lahko v fiksni obliki ali interaktiven. Vključuje tudi VCASI (video računalniško podprto samoizpolnjevanje), ACASI (avdio računalniško podprto samoizpolnjevanje) in TACASI (telefonsko avdio računalniško podprto samoizpolnjevanje).</skos:definition>
      <skos:prefLabel xml:lang="sv">Självadministrerat frågeformulär: med datorstöd (CASI)</skos:prefLabel>
      <skos:definition xml:lang="sv">Computer-assisted self-interview (CASI). Respondenterna noterar själva sina svar i en dator (stationär eller bärbar, Palm/PDA, surfplatta e. dyl.). Frågeformuläret administreras med ett datorprogram som utvecklats för detta syfte men data överförs inte i realtid som i fallet med CAWI: svaren lagras på datorn som används för intervjun. Frågeformuläret kan vara statiskt eller interaktivt. Omfattar VCASI (Video Computer-Assisted Self-Interview), ACASI (Audio computer-assisted self-interview) och TCASI (Telephone audio computer-assisted self-interview).</skos:definition>
      <skos:broader rdf:resource="http://rdf-vocabulary.ddialliance.org/cv/ModeOfCollection/4.0/d50e874"/>
   </rdf:Description>
   <rdf:Description rdf:about="http://rdf-vocabulary.ddialliance.org/cv/ModeOfCollection/4.0/d50e1426">
      <rdf:type rdf:resource="http://www.w3.org/2004/02/skos/core#Concept"/>
      <skos:inScheme rdf:resource="http://rdf-vocabulary.ddialliance.org/cv/ModeOfCollection/4.0/"/>
      <skos:notation>FocusGroup</skos:notation>
      <skos:prefLabel xml:lang="en">Focus group</skos:prefLabel>
      <skos:definition xml:lang="en">A group discussion on a particular topic, organized for research purposes. The individuals are selected with relevance to the topic, and interaction among the participants is used as part of the method.</skos:definition>
      <skos:prefLabel xml:lang="de">Fokusgruppe</skos:prefLabel>
      <skos:definition xml:lang="de">Eine für Forschungszwecke organisierte Gruppendiskussion zu einem bestimmten Thema. Individuen mit Bezug zum Thema werden ausgewählt und die Interaktion zwischen den Teilnehmern wird als Teil der Methode verwendet.</skos:definition>
      <skos:prefLabel xml:lang="fi">Kohderyhmäkeskustelu</skos:prefLabel>
      <skos:definition xml:lang="fi">Tutkimustarkoitusta varten järjestetty kohderyhmäkeskustelu tietystä aiheesta. Ryhmän osanottajat valitaan aiheen mukaan ja osanottajien välinen vuorovaikutus on osa tutkimuskohdetta.</skos:definition>
      <skos:prefLabel xml:lang="fi">Kohderyhmäkeskustelu</skos:prefLabel>
      <skos:definition xml:lang="fi">Tutkimustarkoitusta varten järjestetty kohderyhmäkeskustelu tietystä aiheesta. Ryhmän osanottajat valitaan aiheen mukaan ja osanottajien välinen vuorovaikutus on osa tutkimuskohdetta.</skos:definition>
      <skos:prefLabel xml:lang="it">Focus group</skos:prefLabel>
      <skos:definition xml:lang="it">Una discussione di gruppo focalizzata su un argomento particolare, organizzata per scopi di ricerca. I singoli individui sono selezionati in base all'argomento trattato, e l'interazione tra i partecipanti viene utilizzata come parte della tecnica.</skos:definition>
      <skos:prefLabel xml:lang="ja">フォーカスグループ</skos:prefLabel>
      <skos:definition xml:lang="ja">調査目的で組織された、特定の話題に関する集団討論。個々の参加者は話題との関連性をもとに選択され、参加者間のやりとりも方法の一部として用いられる。</skos:definition>
      <skos:prefLabel xml:lang="lt">Tikslinė grupės diskusija</skos:prefLabel>
      <skos:definition xml:lang="lt">Tyrimo tikslais organizuojama tikslinė grupės diskusija tam tikra tema. Asmenys parenkami atsižvelgiant į temą, o metodo taikymas reikalauja grupinės sąveikos.</skos:definition>
      <skos:prefLabel xml:lang="nl">Focusgroep</skos:prefLabel>
      <skos:definition xml:lang="nl"/>
      <skos:prefLabel xml:lang="no">Fokusgruppe</skos:prefLabel>
      <skos:definition xml:lang="no">En gruppediskusjon som omhandler et bestemt tema, organisert for forskningsformål. Individene er valgt med relevans til temaet og samhandlingen mellom deltakerne er brukt som en del av metoden.</skos:definition>
      <skos:prefLabel xml:lang="no">Fokusgruppe</skos:prefLabel>
      <skos:definition xml:lang="no">En gruppediskusjon som omhandler et bestemt tema, organisert for forskningsformål. Individene er valgt med relevans til temaet og samhandlingen mellom deltakerne er brukt som en del av metoden.</skos:definition>
      <skos:prefLabel xml:lang="pt">Focus group (grupo focal)</skos:prefLabel>
      <skos:definition xml:lang="pt">Entrevista de grupo sobre um tópico específico, organizada para fins de investigação. Os indivíduos são selecionados em função da sua relevância para o tópico e a interação entre os participantes é usada como parte do método.</skos:definition>
      <skos:prefLabel xml:lang="sl">Fokusna skupina</skos:prefLabel>
      <skos:definition xml:lang="sl">Skupinska razprava o določeni temi, organizirana za raziskovalne namene. Posamezniki so izbrani glede na temo, interakcija med udeleženci pa se uporablja kot del metode.</skos:definition>
      <skos:prefLabel xml:lang="sv">Fokusgrupp</skos:prefLabel>
      <skos:definition xml:lang="sv">En gruppdiskussion om ett visst ämne som anordnats i forskningssyfte. Deltagarna har valts ut med hänsyn till ämnet och interaktionen mellan deltagarna utgör en del av forskningsmetoden.</skos:definition>
      <skos:narrower rdf:resource="http://rdf-vocabulary.ddialliance.org/cv/ModeOfCollection/4.0/d50e1523"/>
      <skos:narrower rdf:resource="http://rdf-vocabulary.ddialliance.org/cv/ModeOfCollection/4.0/d50e1614"/>
      <skos:narrower rdf:resource="http://rdf-vocabulary.ddialliance.org/cv/ModeOfCollection/4.0/d50e1704"/>
   </rdf:Description>
   <rdf:Description rdf:about="http://rdf-vocabulary.ddialliance.org/cv/ModeOfCollection/4.0/d50e1523">
      <rdf:type rdf:resource="http://www.w3.org/2004/02/skos/core#Concept"/>
      <skos:inScheme rdf:resource="http://rdf-vocabulary.ddialliance.org/cv/ModeOfCollection/4.0/"/>
      <skos:notation>FocusGroup.FaceToFace</skos:notation>
      <skos:prefLabel xml:lang="en">Face-to-face focus group</skos:prefLabel>
      <skos:definition xml:lang="en">The focus group participants meet in person to conduct the discussion.</skos:definition>
      <skos:prefLabel xml:lang="de">Fokusgruppe: Persönlich</skos:prefLabel>
      <skos:definition xml:lang="de">Die Teilnehmer der Fokusgruppe treffen sich persönlich zur Diskussion.</skos:definition>
      <skos:prefLabel xml:lang="fi">Kohderyhmäkeskustelu: kasvokkainen keskustelu</skos:prefLabel>
      <skos:definition xml:lang="fi">Tutkimustarkoitusta varten järjestetty kohderyhmäkeskustelu tietystä aiheesta. Keskustelu käydään kasvokkain.</skos:definition>
      <skos:prefLabel xml:lang="fi">Kohderyhmäkeskustelu: kasvokkainen keskustelu</skos:prefLabel>
      <skos:definition xml:lang="fi">Tutkimustarkoitusta varten järjestetty kohderyhmäkeskustelu tietystä aiheesta. Keskustelu käydään kasvokkain.</skos:definition>
      <skos:prefLabel xml:lang="it">Focus group faccia a faccia</skos:prefLabel>
      <skos:definition xml:lang="it">I partecipanti al focus group si incontrano di persona per condurre la discussione.</skos:definition>
      <skos:prefLabel xml:lang="ja">対面フォーカスグループ</skos:prefLabel>
      <skos:definition xml:lang="ja">フォーカスグループの参加者は討論を行うため直接対面する。</skos:definition>
      <skos:prefLabel xml:lang="lt">Tiesioginė tikslinė grupės diskusija </skos:prefLabel>
      <skos:definition xml:lang="lt">Tikslinės grupės diskusijos dalyviai susitinka ir diskutuoja tiesiogiai.</skos:definition>
      <skos:prefLabel xml:lang="nl">Face-to-face focusgroep</skos:prefLabel>
      <skos:definition xml:lang="nl"/>
      <skos:prefLabel xml:lang="no">Fokusgruppe: Ansikt til ansikt</skos:prefLabel>
      <skos:definition xml:lang="no">Deltakerne i fokusgruppen møtes fysisk for å gjennomføre diskusjonen.</skos:definition>
      <skos:prefLabel xml:lang="no">Fokusgruppe: Ansikt til ansikt</skos:prefLabel>
      <skos:definition xml:lang="no">Deltakerne i fokusgruppen møtes fysisk for å gjennomføre diskusjonen.</skos:definition>
      <skos:prefLabel xml:lang="pt">Focus group presencial</skos:prefLabel>
      <skos:definition xml:lang="pt">Os participantes do grupo focal encontram-se pessoalmente para participar na discussão.</skos:definition>
      <skos:prefLabel xml:lang="sl">Fokusna skupina v živo</skos:prefLabel>
      <skos:definition xml:lang="sl">Udeleženci fokusne skupine se osebno sestanejo za vodenje razprave.</skos:definition>
      <skos:prefLabel xml:lang="sv">Fokusgrupp: traditionell</skos:prefLabel>
      <skos:definition xml:lang="sv">Fokusgruppens medlemmar träffas på samma plats för att diskutera.</skos:definition>
      <skos:broader rdf:resource="http://rdf-vocabulary.ddialliance.org/cv/ModeOfCollection/4.0/d50e1426"/>
   </rdf:Description>
   <rdf:Description rdf:about="http://rdf-vocabulary.ddialliance.org/cv/ModeOfCollection/4.0/d50e1614">
      <rdf:type rdf:resource="http://www.w3.org/2004/02/skos/core#Concept"/>
      <skos:inScheme rdf:resource="http://rdf-vocabulary.ddialliance.org/cv/ModeOfCollection/4.0/"/>
      <skos:notation>FocusGroup.Telephone</skos:notation>
      <skos:prefLabel xml:lang="en">Telephone focus group</skos:prefLabel>
      <skos:definition xml:lang="en">The focus group discussion is conducted over the telephone.</skos:definition>
      <skos:prefLabel xml:lang="de">Fokusgruppe: Telefonisch</skos:prefLabel>
      <skos:definition xml:lang="de">Die Fokusgruppendiskussion wird über das Telefon durchgeführt.</skos:definition>
      <skos:prefLabel xml:lang="fi">Kohderyhmäkeskustelu: puhelinkeskustelu</skos:prefLabel>
      <skos:definition xml:lang="fi">Tutkimustarkoitusta varten järjestetty kohderyhmäkeskustelu tietystä aiheesta. Keskustelu käydään puhelimen välityksellä.</skos:definition>
      <skos:prefLabel xml:lang="fi">Kohderyhmäkeskustelu: puhelinkeskustelu</skos:prefLabel>
      <skos:definition xml:lang="fi">Tutkimustarkoitusta varten järjestetty kohderyhmäkeskustelu tietystä aiheesta. Keskustelu käydään puhelimen välityksellä.</skos:definition>
      <skos:prefLabel xml:lang="it">Focus group telefonico</skos:prefLabel>
      <skos:definition xml:lang="it">La discussione del focus group è condotta via telefono.</skos:definition>
      <skos:prefLabel xml:lang="ja">電話フォーカスグループ</skos:prefLabel>
      <skos:definition xml:lang="ja">フォーカスグループの討論は電話で行われる。</skos:definition>
      <skos:prefLabel xml:lang="lt">Tikslinė grupės diskusija telefonu</skos:prefLabel>
      <skos:definition xml:lang="lt">Tikslinė grupės diskusija vedama telefonu.</skos:definition>
      <skos:prefLabel xml:lang="nl">Telefonische focusgroep</skos:prefLabel>
      <skos:definition xml:lang="nl"/>
      <skos:prefLabel xml:lang="no">Fokusgruppe: Telefon</skos:prefLabel>
      <skos:definition xml:lang="no">Fokusgruppediskusjonen er gjennomført over telefonen.</skos:definition>
      <skos:prefLabel xml:lang="no">Fokusgruppe: Telefon</skos:prefLabel>
      <skos:definition xml:lang="no">Fokusgruppediskusjonen er gjennomført over telefonen.</skos:definition>
      <skos:prefLabel xml:lang="pt">Focus group por telefone</skos:prefLabel>
      <skos:definition xml:lang="pt">A discussão do grupo focal é realizada por telefone.</skos:definition>
      <skos:prefLabel xml:lang="sl">Telefonska fokusna skupina</skos:prefLabel>
      <skos:definition xml:lang="sl">Fokusna skupina, kjer razprava poteka preko telefona.</skos:definition>
      <skos:prefLabel xml:lang="sv">Fokusgrupp: telefon</skos:prefLabel>
      <skos:definition xml:lang="sv">Fokusgruppens diskussion förs över telefon.</skos:definition>
      <skos:broader rdf:resource="http://rdf-vocabulary.ddialliance.org/cv/ModeOfCollection/4.0/d50e1426"/>
   </rdf:Description>
   <rdf:Description rdf:about="http://rdf-vocabulary.ddialliance.org/cv/ModeOfCollection/4.0/d50e1704">
      <rdf:type rdf:resource="http://www.w3.org/2004/02/skos/core#Concept"/>
      <skos:inScheme rdf:resource="http://rdf-vocabulary.ddialliance.org/cv/ModeOfCollection/4.0/"/>
      <skos:notation>FocusGroup.Online</skos:notation>
      <skos:prefLabel xml:lang="en">Online focus group</skos:prefLabel>
      <skos:definition xml:lang="en">The focus group discussion is conducted over the Internet in an interactive manner.</skos:definition>
      <skos:prefLabel xml:lang="de">Fokusgruppe: Online</skos:prefLabel>
      <skos:definition xml:lang="de">Die Fokusgruppendiskussion wird interaktiv über das Internet durchgeführt.</skos:definition>
      <skos:prefLabel xml:lang="fi">Kohderyhmäkeskustelu: verkkokeskustelu</skos:prefLabel>
      <skos:definition xml:lang="fi">Tutkimustarkoitusta varten järjestetty kohderyhmäkeskustelu tietystä aiheesta. Keskustelu käydään verkossa.</skos:definition>
      <skos:prefLabel xml:lang="fi">Kohderyhmäkeskustelu: verkkokeskustelu</skos:prefLabel>
      <skos:definition xml:lang="fi">Tutkimustarkoitusta varten järjestetty kohderyhmäkeskustelu tietystä aiheesta. Keskustelu käydään verkossa.</skos:definition>
      <skos:prefLabel xml:lang="it">Focus group online</skos:prefLabel>
      <skos:definition xml:lang="it">La discussione del focus group è condotta via Internet in modo interattivo.</skos:definition>
      <skos:prefLabel xml:lang="ja">オンライン・フォーカスグループ</skos:prefLabel>
      <skos:definition xml:lang="ja">フォーカスグループの討論はインターネット上でインタラクティブに行われる。</skos:definition>
      <skos:prefLabel xml:lang="lt">Tikslinė grupės diskusija internetu</skos:prefLabel>
      <skos:definition xml:lang="lt">Tikslinė grupės diskusija interaktyviai vedama internetu.</skos:definition>
      <skos:prefLabel xml:lang="nl">Online focusgroep</skos:prefLabel>
      <skos:definition xml:lang="nl"/>
      <skos:prefLabel xml:lang="no">Fokusgruppe: Online</skos:prefLabel>
      <skos:definition xml:lang="no">Fokusgruppediskusjonen er gjennomført over internett på en interaktiv måte.</skos:definition>
      <skos:prefLabel xml:lang="no">Fokusgruppe: Online</skos:prefLabel>
      <skos:definition xml:lang="no">Fokusgruppediskusjonen er gjennomført over internett på en interaktiv måte.</skos:definition>
      <skos:prefLabel xml:lang="pt">Focus group online</skos:prefLabel>
      <skos:definition xml:lang="pt">A discussão do grupo focal é conduzida pela Internet de forma interativa.</skos:definition>
      <skos:prefLabel xml:lang="sl">Spletna fokusna skupina</skos:prefLabel>
      <skos:definition xml:lang="sl">Fokusna skupina, kjer razprava poteka preko spleta na interaktiven način.</skos:definition>
      <skos:prefLabel xml:lang="sv">Fokusgrupp: virtuell</skos:prefLabel>
      <skos:definition xml:lang="sv">Fokusgruppens diskussion förs interaktivt över Internet. Kallas även IT-stödd fokusgrupp.</skos:definition>
      <skos:broader rdf:resource="http://rdf-vocabulary.ddialliance.org/cv/ModeOfCollection/4.0/d50e1426"/>
   </rdf:Description>
   <rdf:Description rdf:about="http://rdf-vocabulary.ddialliance.org/cv/ModeOfCollection/4.0/d50e1794">
      <rdf:type rdf:resource="http://www.w3.org/2004/02/skos/core#Concept"/>
      <skos:inScheme rdf:resource="http://rdf-vocabulary.ddialliance.org/cv/ModeOfCollection/4.0/"/>
      <skos:notation>SelfAdministeredWritingsAndDiaries</skos:notation>
      <skos:prefLabel xml:lang="en">Self-administered writings and/or diaries</skos:prefLabel>
      <skos:definition xml:lang="en">Narratives, stories, diaries, and written texts created by the research subject.</skos:definition>
      <skos:prefLabel xml:lang="de">Selbstverfasste Schriften und/oder Tagebücher</skos:prefLabel>
      <skos:definition xml:lang="de">Erzählungen, Geschichten, Tagebücher und schriftliche Texte, die vom Forschungssubjekt erstellt wurden.</skos:definition>
      <skos:prefLabel xml:lang="fi">Oma kirjoitus tai päiväkirja</skos:prefLabel>
      <skos:definition xml:lang="fi">Osanottajien itse kirjoittamat elämäkerrat, tarinat, päiväkirjat ja muut kirjoitukset.</skos:definition>
      <skos:prefLabel xml:lang="fi">Oma kirjoitus tai päiväkirja</skos:prefLabel>
      <skos:definition xml:lang="fi">Osanottajien itse kirjoittamat elämäkerrat, tarinat, päiväkirjat ja muut kirjoitukset.</skos:definition>
      <skos:prefLabel xml:lang="it">Scritti/diari auto-compilati</skos:prefLabel>
      <skos:definition xml:lang="it">Narrazioni, storie, diari e testi scritti creati dai soggetti coinvolti nella ricerca.</skos:definition>
      <skos:prefLabel xml:lang="ja">自記式の文章／日記</skos:prefLabel>
      <skos:definition xml:lang="ja">調査対象により作成された語り、物語、日記、テキスト。</skos:definition>
      <skos:prefLabel xml:lang="lt">Savarankiškai rašomi užrašai ir (arba) dienoraščiai</skos:prefLabel>
      <skos:definition xml:lang="lt">Tiriamųjų sukuriami naratyvai, pasakojimai, dienoraščiai ir rašytiniai tekstai.</skos:definition>
      <skos:prefLabel xml:lang="nl">Zelf ingevulde antwoorden/of dagboeken</skos:prefLabel>
      <skos:definition xml:lang="nl"/>
      <skos:prefLabel xml:lang="no">Selvadministrert tekst og/eller dagbok</skos:prefLabel>
      <skos:definition xml:lang="no">Fortellinger, historier, dagbøker og tekster skrevet av studieobjektene.</skos:definition>
      <skos:prefLabel xml:lang="no">Selvadministrert tekst og/eller dagbok</skos:prefLabel>
      <skos:definition xml:lang="no">Fortellinger, historier, dagbøker og tekster skrevet av studieobjektene.</skos:definition>
      <skos:prefLabel xml:lang="pt">Textos e/ou diários de autopreenchimento</skos:prefLabel>
      <skos:definition xml:lang="pt">Narrativas, histórias, diários e textos escritos criados/produzidos pelo(s) sujeito(s) da pesquisa.</skos:definition>
      <skos:prefLabel xml:lang="sl">Samoizpolnjevanje zapisov in/ali dnevnikov</skos:prefLabel>
      <skos:definition xml:lang="sl">Pripovedi, zgodbe, dnevniki in napisana besedila, ki jih ustvari subjekt raziskave.</skos:definition>
      <skos:prefLabel xml:lang="sv">Självadministrerad text och/eller dagböcker</skos:prefLabel>
      <skos:definition xml:lang="sv">Narrativ, berättelser, dagböcker och andra nedskrivna texter skapade av forskningspersonerna.</skos:definition>
      <skos:narrower rdf:resource="http://rdf-vocabulary.ddialliance.org/cv/ModeOfCollection/4.0/d50e1891"/>
      <skos:narrower rdf:resource="http://rdf-vocabulary.ddialliance.org/cv/ModeOfCollection/4.0/d50e1981"/>
      <skos:narrower rdf:resource="http://rdf-vocabulary.ddialliance.org/cv/ModeOfCollection/4.0/d50e2071"/>
   </rdf:Description>
   <rdf:Description rdf:about="http://rdf-vocabulary.ddialliance.org/cv/ModeOfCollection/4.0/d50e1891">
      <rdf:type rdf:resource="http://www.w3.org/2004/02/skos/core#Concept"/>
      <skos:inScheme rdf:resource="http://rdf-vocabulary.ddialliance.org/cv/ModeOfCollection/4.0/"/>
      <skos:notation>SelfAdministeredWritingsAndDiaries.Email</skos:notation>
      <skos:prefLabel xml:lang="en">Self-administered writings and/or diaries: E-mail</skos:prefLabel>
      <skos:definition xml:lang="en">Narratives, stories, diaries, and written texts submitted via e-mail messages.</skos:definition>
      <skos:prefLabel xml:lang="de">Selbstverfasste Schriften und/oder Tagebücher: E-Mail</skos:prefLabel>
      <skos:definition xml:lang="de">Erzählungen, Geschichten, Tagebücher und schriftliche Texte, die über E-Mail-Nachrichten eingereicht werden.</skos:definition>
      <skos:prefLabel xml:lang="fi">Oma kirjoitus tai päiväkirja: sähköpostilla saatu</skos:prefLabel>
      <skos:definition xml:lang="fi">Osanottajien sähköpostin välityksellä annetut omat kirjoitukset ja päiväkirjat.</skos:definition>
      <skos:prefLabel xml:lang="fi">Oma kirjoitus tai päiväkirja: sähköpostilla saatu</skos:prefLabel>
      <skos:definition xml:lang="fi">Osanottajien sähköpostin välityksellä annetut omat kirjoitukset ja päiväkirjat.</skos:definition>
      <skos:prefLabel xml:lang="it">Scritti/diari auto-compilati: e-mail</skos:prefLabel>
      <skos:definition xml:lang="it">Narrazioni, storie, diari e testi scritti inviati tramite e-mail.</skos:definition>
      <skos:prefLabel xml:lang="ja">自記式の日記：電子メール</skos:prefLabel>
      <skos:definition xml:lang="ja">電子メールのメッセージにより提出された語り、物語、日記、テキスト。</skos:definition>
      <skos:prefLabel xml:lang="lt">Savarankiškai rašomi užrašai ir (arba) dienoraščiai: elektroniniu paštu</skos:prefLabel>
      <skos:definition xml:lang="lt">Elektroniniu paštu pateikiami naratyvai, pasakojimai, dienoraščiai ir rašytiniai tekstai.</skos:definition>
      <skos:prefLabel xml:lang="nl">Zelf ingevulde antwoorden/of dagboeken: E-mail</skos:prefLabel>
      <skos:definition xml:lang="nl"/>
      <skos:prefLabel xml:lang="no">Selvadministrert tekst og/eller dagbok: E-post</skos:prefLabel>
      <skos:definition xml:lang="no">Fortellinger, historier, dagbøker og tekster som har blitt samlet inn via e-post.</skos:definition>
      <skos:prefLabel xml:lang="no">Selvadministrert tekst og/eller dagbok: E-post</skos:prefLabel>
      <skos:definition xml:lang="no">Fortellinger, historier, dagbøker og tekster som har blitt samlet inn via e-post.</skos:definition>
      <skos:prefLabel xml:lang="pt">Textos e/ou diários de autopreenchimento: Email</skos:prefLabel>
      <skos:definition xml:lang="pt">Narrativas, histórias, diários e textos escritos enviados por mensagens de email.</skos:definition>
      <skos:prefLabel xml:lang="sl">Samoizpolnjevanje zapisov in/ali dnevnikov: elektronska pošta</skos:prefLabel>
      <skos:definition xml:lang="sl">Pripovedi, zgodbe, dnevniki in napisana besedila, ki so posredovana preko elektronskih poštnih sporočil.</skos:definition>
      <skos:prefLabel xml:lang="sv">Självadministrerad text och/eller dagböcker: e-post</skos:prefLabel>
      <skos:definition xml:lang="sv">Narrativ, berättelser, dagböcker och andra nedskrivna texter som skickas in via e-post.</skos:definition>
      <skos:broader rdf:resource="http://rdf-vocabulary.ddialliance.org/cv/ModeOfCollection/4.0/d50e1794"/>
   </rdf:Description>
   <rdf:Description rdf:about="http://rdf-vocabulary.ddialliance.org/cv/ModeOfCollection/4.0/d50e1981">
      <rdf:type rdf:resource="http://www.w3.org/2004/02/skos/core#Concept"/>
      <skos:inScheme rdf:resource="http://rdf-vocabulary.ddialliance.org/cv/ModeOfCollection/4.0/"/>
      <skos:notation>SelfAdministeredWritingsAndDiaries.Paper</skos:notation>
      <skos:prefLabel xml:lang="en">Self-administered writings and/or diaries: Paper</skos:prefLabel>
      <skos:definition xml:lang="en">Narratives, stories, diaries, and written texts created and collected in paper form.</skos:definition>
      <skos:prefLabel xml:lang="de">Selbstverfasste Schriften und/oder Tagebücher: Papier</skos:prefLabel>
      <skos:definition xml:lang="de">Erzählungen, Geschichten, Tagebücher und schriftliche Texte, die in Papierform erstellt und gesammelt wurden.</skos:definition>
      <skos:prefLabel xml:lang="fi">Oma kirjoitus tai päiväkirja: paperimuotoinen kirjoitus</skos:prefLabel>
      <skos:definition xml:lang="fi">Osanottajien paperimuotoiset omat kirjoitukset ja päiväkirjat.</skos:definition>
      <skos:prefLabel xml:lang="fi">Oma kirjoitus tai päiväkirja: paperimuotoinen kirjoitus</skos:prefLabel>
      <skos:definition xml:lang="fi">Osanottajien paperimuotoiset omat kirjoitukset ja päiväkirjat.</skos:definition>
      <skos:prefLabel xml:lang="it">Scritti/diari auto-compilati: cartaceo</skos:prefLabel>
      <skos:definition xml:lang="it">Narrazioni, storie, diari e testi scritti creati e raccolti in forma cartacea.</skos:definition>
      <skos:prefLabel xml:lang="ja">自記式の文章／日記：紙</skos:prefLabel>
      <skos:definition xml:lang="ja">紙に記された形で収集された語り、物語、日記、テキスト。</skos:definition>
      <skos:prefLabel xml:lang="lt">Savarankiškai rašomi užrašai ir (arba) dienoraščiai: popieriuje</skos:prefLabel>
      <skos:definition xml:lang="lt">Naratyvai, pasakojimai, dienoraščiai ir rašytiniai tekstai sukuriami ir renkami popierine forma.</skos:definition>
      <skos:prefLabel xml:lang="nl">Zelf ingevulde antwoorden/of dagboeken: Papier</skos:prefLabel>
      <skos:definition xml:lang="nl"/>
      <skos:prefLabel xml:lang="no">Selvadministrert tekst og/eller dagbok: Papir</skos:prefLabel>
      <skos:definition xml:lang="no">Fortellinger, historier, dagbøker og tekster skrevet og samlet i papirformat.</skos:definition>
      <skos:prefLabel xml:lang="no">Selvadministrert tekst og/eller dagbok: Papir</skos:prefLabel>
      <skos:definition xml:lang="no">Fortellinger, historier, dagbøker og tekster skrevet og samlet i papirformat.</skos:definition>
      <skos:prefLabel xml:lang="pt">Textos e/ou diários de autopreenchimento: Papel</skos:prefLabel>
      <skos:definition xml:lang="pt">Narrativas, histórias, diários e textos escritos criados e recolhidos em papel.</skos:definition>
      <skos:prefLabel xml:lang="sl">Samoizpolnjevanje zapisov in/ali dnevnikov: papir</skos:prefLabel>
      <skos:definition xml:lang="sl">Pripovedi, zgodbe, dnevniki in napisana besedila, ki so ustvarjena in zbrana na papirju.</skos:definition>
      <skos:prefLabel xml:lang="sv">Självadministrerad text och/eller dagböcker: papper</skos:prefLabel>
      <skos:definition xml:lang="sv">Narrativ, berättelser, dagböcker och andra nedskrivna texter som skapats och samlats in på papper.</skos:definition>
      <skos:broader rdf:resource="http://rdf-vocabulary.ddialliance.org/cv/ModeOfCollection/4.0/d50e1794"/>
   </rdf:Description>
   <rdf:Description rdf:about="http://rdf-vocabulary.ddialliance.org/cv/ModeOfCollection/4.0/d50e2071">
      <rdf:type rdf:resource="http://www.w3.org/2004/02/skos/core#Concept"/>
      <skos:inScheme rdf:resource="http://rdf-vocabulary.ddialliance.org/cv/ModeOfCollection/4.0/"/>
      <skos:notation>SelfAdministeredWritingsAndDiaries.WebBased</skos:notation>
      <skos:prefLabel xml:lang="en">Self-administered writings and/or diaries: Web-based</skos:prefLabel>
      <skos:definition xml:lang="en">Narratives, stories, diaries, and written texts gathered from Internet sources, e.g. websites, blogs, discussion forums.</skos:definition>
      <skos:prefLabel xml:lang="de">Selbstverfasste Schriften und/oder Tagebücher: Webbasiert</skos:prefLabel>
      <skos:definition xml:lang="de">Erzählungen, Geschichten, Tagebücher und schriftliche Texte aus Internetquellen, z. B. Webseiten, Blogs, Diskussionsforen.</skos:definition>
      <skos:prefLabel xml:lang="fi">Oma kirjoitus tai päiväkirja: verkon kautta saatu</skos:prefLabel>
      <skos:definition xml:lang="fi">Osanottajien verkossa kirjoitetut omat kirjoitukset ja päiväkirjat.</skos:definition>
      <skos:prefLabel xml:lang="fi">Oma kirjoitus tai päiväkirja: verkon kautta saatu</skos:prefLabel>
      <skos:definition xml:lang="fi">Osanottajien verkossa kirjoitetut omat kirjoitukset ja päiväkirjat.</skos:definition>
      <skos:prefLabel xml:lang="it">Scritti/diari auto-compilati: web</skos:prefLabel>
      <skos:definition xml:lang="it">Narrazioni, storie, diari e testi scritti raccolti su Internet, ad esempio da siti web, blog, forum di discussione.</skos:definition>
      <skos:prefLabel xml:lang="ja">自記式の文章／日記：Webベース</skos:prefLabel>
      <skos:definition xml:lang="ja">インターネット上の情報源から収集された語り、物語、日記、テキスト。例えば、Webサイト、ブログ、ディスカッションフォーラム等がある。</skos:definition>
      <skos:prefLabel xml:lang="lt">Savarankiškai rašomi užrašai ir (arba) dienoraščiai: internete</skos:prefLabel>
      <skos:definition xml:lang="lt">Naratyvai, pasakojimai, dienoraščiai ir rašytiniai tekstai surenkami iš internetinių šaltinių, pavyzdžiui, svetainių, tinklaraščių, diskusijų forumų.</skos:definition>
      <skos:prefLabel xml:lang="nl">Zelf ingevulde antwoorden/of dagboeken: Webgebaseerd</skos:prefLabel>
      <skos:definition xml:lang="nl"/>
      <skos:prefLabel xml:lang="no">Selvadministrert tekst og/eller dagbok: Webbasert</skos:prefLabel>
      <skos:definition xml:lang="no">Fortellinger, historier, dagbøker og tekster samlet fra internett, e.g. nettsider, blogger, diskusjonsforumer.</skos:definition>
      <skos:prefLabel xml:lang="no">Selvadministrert tekst og/eller dagbok: Webbasert</skos:prefLabel>
      <skos:definition xml:lang="no">Fortellinger, historier, dagbøker og tekster samlet fra internett, e.g. nettsider, blogger, diskusjonsforumer.</skos:definition>
      <skos:prefLabel xml:lang="pt">Textos e/ou diários de autopreenchimento: Online/via web</skos:prefLabel>
      <skos:definition xml:lang="pt">Narrativas, histórias, diários e textos escritos recolhidos de fontes da Internet, por ex. sites, blogs, fóruns de discussão.</skos:definition>
      <skos:prefLabel xml:lang="sl">Samoizpolnjevanje zapisov in/ali dnevnikov: spletno</skos:prefLabel>
      <skos:definition xml:lang="sl">Pripovedi, zgodbe, dnevniki in napisana besedila, ki so zbrana preko internetnih virov, npr. spletne strani, blogi, forumi.</skos:definition>
      <skos:prefLabel xml:lang="sv">Självadministrerad text och/eller dagböcker: webbaserat</skos:prefLabel>
      <skos:definition xml:lang="sv">Narrativ, berättelser, dagböcker och andra nedskrivna texter som samlats in från Internet-källor, t.ex. webbplatser, bloggar, diskussionsforum.</skos:definition>
      <skos:broader rdf:resource="http://rdf-vocabulary.ddialliance.org/cv/ModeOfCollection/4.0/d50e1794"/>
   </rdf:Description>
   <rdf:Description rdf:about="http://rdf-vocabulary.ddialliance.org/cv/ModeOfCollection/4.0/d50e2162">
      <rdf:type rdf:resource="http://www.w3.org/2004/02/skos/core#Concept"/>
      <skos:inScheme rdf:resource="http://rdf-vocabulary.ddialliance.org/cv/ModeOfCollection/4.0/"/>
      <skos:notation>Observation</skos:notation>
      <skos:prefLabel xml:lang="en">Observation</skos:prefLabel>
      <skos:definition xml:lang="en">Research method that involves collecting data as they occur (for example, observing behaviors, events, development of condition or disease, etc.), without attempting to manipulate any of the independent variables.</skos:definition>
      <skos:prefLabel xml:lang="de">Beobachtung</skos:prefLabel>
      <skos:definition xml:lang="de">Forschungsmethode, bei der Daten gesammelt werden, während sie auftreten (z. B. Beobachtung von Verhaltensweisen, Ereignissen, Entwicklung eines Zustands oder einer Krankheit usw.), ohne dass versucht wird, eine der unabhängigen Variablen zu manipulieren.</skos:definition>
      <skos:prefLabel xml:lang="fi">Havainnointi</skos:prefLabel>
      <skos:definition xml:lang="fi">Keruumenetelmä, jossa tarkkaillaan tapahtumia, käyttäytymistä, vuorovaikutusta jne. niiden tapahtuessa, ilman minkään riippumattoman muuttujan manipulointia.</skos:definition>
      <skos:prefLabel xml:lang="fi">Havainnointi</skos:prefLabel>
      <skos:definition xml:lang="fi">Keruumenetelmä, jossa tarkkaillaan tapahtumia, käyttäytymistä, vuorovaikutusta jne. niiden tapahtuessa, ilman minkään riippumattoman muuttujan manipulointia.</skos:definition>
      <skos:prefLabel xml:lang="it">Osservazione</skos:prefLabel>
      <skos:definition xml:lang="it">Tecnica di rilevazione che implica la raccolta di dati nel momento in cui si generano (ad esempio osservando comportamenti, eventi, sviluppo di condizioni o malattie, ecc.), senza tentare di manipolare nessuna delle variabili indipendenti.</skos:definition>
      <skos:prefLabel xml:lang="ja">観察</skos:prefLabel>
      <skos:definition xml:lang="ja">独立変数を操作することなく、事象が発生したらそのままデータを収集する調査方法（例えば、行動、イベント、状況や病気の進行の観察等)。</skos:definition>
      <skos:prefLabel xml:lang="lt">Stebėjimas</skos:prefLabel>
      <skos:definition xml:lang="lt">Tyrimo metodas, kai duomenys renkami tiesiogiai realiu laiku (pavyzdžiui, stebint elgseną, įvykius, ligos būklę ir raidą ir kt.), nebandant manipuliuoti jokiais nepriklausomais kintamaisiais.</skos:definition>
      <skos:prefLabel xml:lang="nl">Observatie</skos:prefLabel>
      <skos:definition xml:lang="nl"/>
      <skos:prefLabel xml:lang="no">Observasjon</skos:prefLabel>
      <skos:definition xml:lang="no">Forskningsmetode som innebærer å samle inn data etterhvert som de opptrår (for eksempel, observere atferd, hendelser, utviklingen av helsetilstand eller sykdom, etc.) uten å prøve å manipulere noen av de uavhengige variablene.</skos:definition>
      <skos:prefLabel xml:lang="no">Observasjon</skos:prefLabel>
      <skos:definition xml:lang="no">Forskningsmetode som innebærer å samle inn data etterhvert som de opptrår (for eksempel, observere atferd, hendelser, utviklingen av helsetilstand eller sykdom, etc.) uten å prøve å manipulere noen av de uavhengige variablene.</skos:definition>
      <skos:prefLabel xml:lang="pt">Observação</skos:prefLabel>
      <skos:definition xml:lang="pt">Método de investigação que envolve a recolha de dados conforme eles ocorrem (por exemplo, observando comportamentos, eventos, desenvolvimento de uma condição ou doença, etc.), sem tentar manipular nenhuma das variáveis independentes.</skos:definition>
      <skos:prefLabel xml:lang="sl">Opazovanje</skos:prefLabel>
      <skos:definition xml:lang="sl">Raziskovalna metoda, ki vključuje zbiranje podatkov, ko se pojavijo (npr. opazovanje vedenj, dogodkov, razvoja stanja ali bolezni itd.), ne da bi poskušali manipulirati s katero od neodvisnih spremenljivk.</skos:definition>
      <skos:prefLabel xml:lang="sv">Observation</skos:prefLabel>
      <skos:definition xml:lang="sv">Forskningsmetod som omfattar att samla in data om företeelser när de uppträder (t.ex. observationer av beteenden, händelser m.m.) utan att försöka påverka några av de oberoende variablerna.</skos:definition>
      <skos:narrower rdf:resource="http://rdf-vocabulary.ddialliance.org/cv/ModeOfCollection/4.0/d50e2259"/>
      <skos:narrower rdf:resource="http://rdf-vocabulary.ddialliance.org/cv/ModeOfCollection/4.0/d50e2534"/>
      <skos:narrower rdf:resource="http://rdf-vocabulary.ddialliance.org/cv/ModeOfCollection/4.0/d50e2810"/>
   </rdf:Description>
   <rdf:Description rdf:about="http://rdf-vocabulary.ddialliance.org/cv/ModeOfCollection/4.0/d50e2259">
      <rdf:type rdf:resource="http://www.w3.org/2004/02/skos/core#Concept"/>
      <skos:inScheme rdf:resource="http://rdf-vocabulary.ddialliance.org/cv/ModeOfCollection/4.0/"/>
      <skos:notation>Observation.Field</skos:notation>
      <skos:prefLabel xml:lang="en">Field observation</skos:prefLabel>
      <skos:definition xml:lang="en">Observation that is conducted in a natural environment.</skos:definition>
      <skos:prefLabel xml:lang="de">Feldbeobachtung</skos:prefLabel>
      <skos:definition xml:lang="de">Beobachtung, die in einer natürlichen Umgebung durchgeführt wird.</skos:definition>
      <skos:prefLabel xml:lang="fi">Havainnointi: kenttähavainnointi</skos:prefLabel>
      <skos:definition xml:lang="fi">Havainnointi suoritetaan luonnollisessa, kontrolloimattomassa ympäristössä. Käytä termiä mikäli ei tiedossa onko osallistuvaa vai ei-osallistuvaa.</skos:definition>
      <skos:prefLabel xml:lang="fi">Havainnointi: kenttähavainnointi</skos:prefLabel>
      <skos:definition xml:lang="fi">Havainnointi suoritetaan luonnollisessa, kontrolloimattomassa ympäristössä. Käytä termiä mikäli ei tiedossa onko osallistuvaa vai ei-osallistuvaa.</skos:definition>
      <skos:prefLabel xml:lang="it">Osservazione sul campo</skos:prefLabel>
      <skos:definition xml:lang="it">Osservazione condotta in un ambiente naturale.</skos:definition>
      <skos:prefLabel xml:lang="ja">フィールド観察</skos:prefLabel>
      <skos:definition xml:lang="ja">自然な環境で行われる観察。</skos:definition>
      <skos:prefLabel xml:lang="lt">Lauko stebėjimas</skos:prefLabel>
      <skos:definition xml:lang="lt">Stebėjimas atliekamas natūralioje aplinkoje.</skos:definition>
      <skos:prefLabel xml:lang="nl">Observatie in het veld</skos:prefLabel>
      <skos:definition xml:lang="nl"/>
      <skos:prefLabel xml:lang="no">Feltobservasjon</skos:prefLabel>
      <skos:definition xml:lang="no">Observasjon som utføres i et naturlig miljø.</skos:definition>
      <skos:prefLabel xml:lang="no">Feltobservasjon</skos:prefLabel>
      <skos:definition xml:lang="no">Observasjon som utføres i et naturlig miljø.</skos:definition>
      <skos:prefLabel xml:lang="pt">Observação de campo</skos:prefLabel>
      <skos:definition xml:lang="pt">Observação conduzida em ambiente natural.</skos:definition>
      <skos:prefLabel xml:lang="sl">Opazovanje na terenu</skos:prefLabel>
      <skos:definition xml:lang="sl">Opazovanje, ki se izvaja v naravnem okolju.</skos:definition>
      <skos:prefLabel xml:lang="sv">Fältobservation</skos:prefLabel>
      <skos:definition xml:lang="sv">Observation som utförs i en naturlig miljö.</skos:definition>
      <skos:narrower rdf:resource="http://rdf-vocabulary.ddialliance.org/cv/ModeOfCollection/4.0/d50e2354"/>
      <skos:narrower rdf:resource="http://rdf-vocabulary.ddialliance.org/cv/ModeOfCollection/4.0/d50e2444"/>
      <skos:broader rdf:resource="http://rdf-vocabulary.ddialliance.org/cv/ModeOfCollection/4.0/d50e2162"/>
   </rdf:Description>
   <rdf:Description rdf:about="http://rdf-vocabulary.ddialliance.org/cv/ModeOfCollection/4.0/d50e2354">
      <rdf:type rdf:resource="http://www.w3.org/2004/02/skos/core#Concept"/>
      <skos:inScheme rdf:resource="http://rdf-vocabulary.ddialliance.org/cv/ModeOfCollection/4.0/"/>
      <skos:notation>Observation.Field.Participant</skos:notation>
      <skos:prefLabel xml:lang="en">Participant field observation</skos:prefLabel>
      <skos:definition xml:lang="en">Type of field observation in which the researcher interacts with the subjects and often plays a role in the social situation under observation.</skos:definition>
      <skos:prefLabel xml:lang="de">Teilnehmende Feldbeobachtung</skos:prefLabel>
      <skos:definition xml:lang="de">Eine Art der Feldbeobachtung, in der der Forscher mit den Probanden interagiert und oft selbst eine Rolle in der sozialen Situation unter Beobachtung einnimmt.</skos:definition>
      <skos:prefLabel xml:lang="fi">Havainnointi: kenttähavainnointi: osallistuva</skos:prefLabel>
      <skos:definition xml:lang="fi">Havainnointi suoritetaan luonnollisessa, kontrolloimattomassa ympäristössä. Tutkija on vuorovaikutuksessa tutkittavien kanssa ja hänellä on usein jokin rooli tutkinnan kohteena olevassa sosiaalisessa tilanteessa.</skos:definition>
      <skos:prefLabel xml:lang="fi">Havainnointi: kenttähavainnointi: osallistuva</skos:prefLabel>
      <skos:definition xml:lang="fi">Havainnointi suoritetaan luonnollisessa, kontrolloimattomassa ympäristössä. Tutkija on vuorovaikutuksessa tutkittavien kanssa ja hänellä on usein jokin rooli tutkinnan kohteena olevassa sosiaalisessa tilanteessa.</skos:definition>
      <skos:prefLabel xml:lang="it">Osservazione partecipante sul campo</skos:prefLabel>
      <skos:definition xml:lang="it">Tipo di osservazione sul campo nella quale il ricercatore interagisce con i soggetti e spesso ricopre un ruolo nella situazione sociale sotto osservazione.</skos:definition>
      <skos:prefLabel xml:lang="ja">参与観察</skos:prefLabel>
      <skos:definition xml:lang="ja">研究者が調査対象者とやり取りを行い、しばしば観察下の社会状況において一定の役割を果たしながら行うフィールドでの観察。</skos:definition>
      <skos:prefLabel xml:lang="lt">Lauko stebėjimas dalyvaujant</skos:prefLabel>
      <skos:definition xml:lang="lt">Lauko stebėjimo tipas, kai tyrėjas sąveikauja su tiriamaisiais ir stebimoje socialinėje situacijoje paprastai turi tam tikrą vaidmenį.</skos:definition>
      <skos:prefLabel xml:lang="nl">Participerende observatie in het veld</skos:prefLabel>
      <skos:definition xml:lang="nl"/>
      <skos:prefLabel xml:lang="no">Deltagende feltobservasjon</skos:prefLabel>
      <skos:definition xml:lang="no">Type feltobservasjon hvor forskeren samhandler og ofte spiller en rolle i de sosiale situasjonene som observeres.</skos:definition>
      <skos:prefLabel xml:lang="no">Deltagende feltobservasjon</skos:prefLabel>
      <skos:definition xml:lang="no">Type feltobservasjon hvor forskeren samhandler og ofte spiller en rolle i de sosiale situasjonene som observeres.</skos:definition>
      <skos:prefLabel xml:lang="pt">Observação participante </skos:prefLabel>
      <skos:definition xml:lang="pt">Tipo de observação no trabalho de campo em que o investigador interage com os sujeitos e, muitas vezes, desempenha um papel na situação social em observação.</skos:definition>
      <skos:prefLabel xml:lang="sl">Opazovanje na terenu z udeležbo</skos:prefLabel>
      <skos:definition xml:lang="sl">Vrsta opazovanja, kjer je raziskovalec v interakciji z raziskovalnim subjektom in pogosto igra vlogo v opazovani družbeni situaciji.</skos:definition>
      <skos:prefLabel xml:lang="sv">Deltagande fältobservation</skos:prefLabel>
      <skos:definition xml:lang="sv">Fältobservation där forskaren interagerar med forskningsobjekten och ofta har en funktion i den sociala situation som observeras.</skos:definition>
      <skos:broader rdf:resource="http://rdf-vocabulary.ddialliance.org/cv/ModeOfCollection/4.0/d50e2259"/>
   </rdf:Description>
   <rdf:Description rdf:about="http://rdf-vocabulary.ddialliance.org/cv/ModeOfCollection/4.0/d50e2444">
      <rdf:type rdf:resource="http://www.w3.org/2004/02/skos/core#Concept"/>
      <skos:inScheme rdf:resource="http://rdf-vocabulary.ddialliance.org/cv/ModeOfCollection/4.0/"/>
      <skos:notation>Observation.Field.Nonparticipant</skos:notation>
      <skos:prefLabel xml:lang="en">Non-participant field observation</skos:prefLabel>
      <skos:definition xml:lang="en">Observation that is conducted in a natural, non-controlled setting without any interaction between the researcher and his/her subjects.</skos:definition>
      <skos:prefLabel xml:lang="de">Nicht-teilnehmende Feldbeobachtung</skos:prefLabel>
      <skos:definition xml:lang="de">Eine Art der Feldbeobachtung, die in einer natürlichen, nicht kontrollierten Umgebung durchgeführt wird - ohne jegliche Interaktion zwischen dem/der Forscher*in und seinen/ihren Probanden*innen.</skos:definition>
      <skos:prefLabel xml:lang="fi">Havainnointi: kenttähavainnointi: ei-osallistuva</skos:prefLabel>
      <skos:definition xml:lang="fi">Havainnointi suoritetaan luonnollisessa, kontrolloimattomassa ympäristössä. Tutkija ja tutkittavat eivät ole lainkaan vuorovaikutuksessa keskenään. Kutsutaan myös suoraksi tai ulkopuoliseksi kenttähavainnoinniksi.</skos:definition>
      <skos:prefLabel xml:lang="fi">Havainnointi: kenttähavainnointi: ei-osallistuva</skos:prefLabel>
      <skos:definition xml:lang="fi">Havainnointi suoritetaan luonnollisessa, kontrolloimattomassa ympäristössä. Tutkija ja tutkittavat eivät ole lainkaan vuorovaikutuksessa keskenään. Kutsutaan myös suoraksi tai ulkopuoliseksi kenttähavainnoinniksi.</skos:definition>
      <skos:prefLabel xml:lang="it">Osservazione non partecipante sul campo</skos:prefLabel>
      <skos:definition xml:lang="it">Osservazione condotta in un ambiente naturale non controllato senza alcuna interazione tra il ricercatore e i soggetti.</skos:definition>
      <skos:prefLabel xml:lang="ja">非参与型のフィールド観察</skos:prefLabel>
      <skos:definition xml:lang="ja">研究者と調査対象者の間でなんらやり取りがない、統制されない自然な環境で行われる観察。</skos:definition>
      <skos:prefLabel xml:lang="lt">Lauko stebėjimas nedalyvaujant</skos:prefLabel>
      <skos:definition xml:lang="lt">Stebėjimas vykdomas natūralioje, nekontroliuojamoje aplinkoje be jokios sąveikos tarp tyrėjo ir tiriamųjų.</skos:definition>
      <skos:prefLabel xml:lang="nl">Niet-participerende observatie in het veld</skos:prefLabel>
      <skos:definition xml:lang="nl"/>
      <skos:prefLabel xml:lang="no">Ikke-deltagende feltobservasjon</skos:prefLabel>
      <skos:definition xml:lang="no">Observasjon som er gjennomført i et naturlig, ikke kontrollert miljø uten interaksjon mellom forskeren og studieobjektene.</skos:definition>
      <skos:prefLabel xml:lang="no">Ikke-deltagende feltobservasjon</skos:prefLabel>
      <skos:definition xml:lang="no">Observasjon som er gjennomført i et naturlig, ikke kontrollert miljø uten interaksjon mellom forskeren og studieobjektene.</skos:definition>
      <skos:prefLabel xml:lang="pt">Observação não participante</skos:prefLabel>
      <skos:definition xml:lang="pt">Observação que é conduzida/realizada em ambiente natural, não controlado, sem qualquer interação entre o investigador e os sujeitos observados.</skos:definition>
      <skos:prefLabel xml:lang="sl">Opazovanje na terenu brez udeležbe</skos:prefLabel>
      <skos:definition xml:lang="sl">Opazovanje, ki se izvaja v naravnem, nekontroliranem okolju brez kakršnekoli interakcije med raziskovalcem in njegovimi/njenimi subjekti.</skos:definition>
      <skos:prefLabel xml:lang="sv">Icke-deltagande fältobservation</skos:prefLabel>
      <skos:definition xml:lang="sv">Observation som utförs i en naturlig, icke-kontrollerad miljö utan interaktion mellan forskaren och dennes forskningsobjekt.</skos:definition>
      <skos:broader rdf:resource="http://rdf-vocabulary.ddialliance.org/cv/ModeOfCollection/4.0/d50e2259"/>
   </rdf:Description>
   <rdf:Description rdf:about="http://rdf-vocabulary.ddialliance.org/cv/ModeOfCollection/4.0/d50e2534">
      <rdf:type rdf:resource="http://www.w3.org/2004/02/skos/core#Concept"/>
      <skos:inScheme rdf:resource="http://rdf-vocabulary.ddialliance.org/cv/ModeOfCollection/4.0/"/>
      <skos:notation>Observation.Laboratory</skos:notation>
      <skos:prefLabel xml:lang="en">Laboratory observation</skos:prefLabel>
      <skos:definition xml:lang="en">Observation that is conducted in a controlled, artificially created setting. For example, observing children's play in a laboratory playroom.</skos:definition>
      <skos:prefLabel xml:lang="de">Laborbeobachtung</skos:prefLabel>
      <skos:definition xml:lang="de">Beobachtung, die in einer kontrollierten, künstlich geschaffenen Umgebung durchgeführt wird. Zum Beispiel, die Beobachtung spielender Kinder in einem Labor-Spielzimmer.</skos:definition>
      <skos:prefLabel xml:lang="fi">Havainnointi: laboratoriohavainnointi</skos:prefLabel>
      <skos:definition xml:lang="fi">Kokeellinen havainnointi kontrolloidussa, tarkoitusta varten luodussa tilassa tai ympäristössä. Esimerkki: Lasten leikkien havainnointi laboratorioon rakennetussa leikkihuoneessa. Käytä tätä termiä mikäli ei ole tiedossa onko laboratoriohavainnointi osallistuvaa vai ei-osallistuvaa.</skos:definition>
      <skos:prefLabel xml:lang="fi">Havainnointi: laboratoriohavainnointi</skos:prefLabel>
      <skos:definition xml:lang="fi">Kokeellinen havainnointi kontrolloidussa, tarkoitusta varten luodussa tilassa tai ympäristössä. Esimerkki: Lasten leikkien havainnointi laboratorioon rakennetussa leikkihuoneessa. Käytä tätä termiä mikäli ei ole tiedossa onko laboratoriohavainnointi osallistuvaa vai ei-osallistuvaa.</skos:definition>
      <skos:prefLabel xml:lang="it">Osservazione in laboratorio</skos:prefLabel>
      <skos:definition xml:lang="it">Osservazione condotta in un ambiente controllato, creato artificialmente. Ad esempio, osservazione del gioco dei bambini in una stanza da gioco ricreata in laboratorio.</skos:definition>
      <skos:prefLabel xml:lang="ja">実験室観察</skos:prefLabel>
      <skos:definition xml:lang="ja">統制された人工的な環境で行われる観察。例えば、実験用の遊戯室で子どもの遊びを観察する等。</skos:definition>
      <skos:prefLabel xml:lang="lt">Laboratorinis stebėjimas</skos:prefLabel>
      <skos:definition xml:lang="lt">Stebėjimas atliekamas kontroliuojamoje, dirbtinai sukurtoje aplinkoje. Pavyzdžiui, vaikų žaidimo stebėjimas laboratoriniame žaidimų kambaryje.</skos:definition>
      <skos:prefLabel xml:lang="nl">Observatie in het lab</skos:prefLabel>
      <skos:definition xml:lang="nl"/>
      <skos:prefLabel xml:lang="no">Laboratorieobservasjon</skos:prefLabel>
      <skos:definition xml:lang="no">Observasjon som er utført i et kontrollert, kunstig konstruert miljø. For eksempel observasjon av barns lek i et lekerom i laboratoriet.</skos:definition>
      <skos:prefLabel xml:lang="no">Laboratorieobservasjon</skos:prefLabel>
      <skos:definition xml:lang="no">Observasjon som er utført i et kontrollert, kunstig konstruert miljø. For eksempel observasjon av barns lek i et lekerom i laboratoriet.</skos:definition>
      <skos:prefLabel xml:lang="pt">Observação em laboratório</skos:prefLabel>
      <skos:definition xml:lang="pt">Observação que é conduzida/realizada em ambiente controlado e artificialmente criado. Por exemplo, observação das brincadeiras das crianças numa sala de jogos de laboratório.</skos:definition>
      <skos:prefLabel xml:lang="sl">Laboratorijsko opazovanje</skos:prefLabel>
      <skos:definition xml:lang="sl">Opazovanje, ki se izvaja v nadzorovanem, umetno ustvarjenem okolju. Na primer, opazovanje otroške igre v laboratorijski igralnici.</skos:definition>
      <skos:prefLabel xml:lang="sv">Laboratorieobservation</skos:prefLabel>
      <skos:definition xml:lang="sv">Observation som utförs i en kontrollerad, konstgjord miljö. Exempel: observation av barns lek i ett laboratorielekrum.</skos:definition>
      <skos:narrower rdf:resource="http://rdf-vocabulary.ddialliance.org/cv/ModeOfCollection/4.0/d50e2629"/>
      <skos:narrower rdf:resource="http://rdf-vocabulary.ddialliance.org/cv/ModeOfCollection/4.0/d50e2720"/>
      <skos:broader rdf:resource="http://rdf-vocabulary.ddialliance.org/cv/ModeOfCollection/4.0/d50e2162"/>
   </rdf:Description>
   <rdf:Description rdf:about="http://rdf-vocabulary.ddialliance.org/cv/ModeOfCollection/4.0/d50e2629">
      <rdf:type rdf:resource="http://www.w3.org/2004/02/skos/core#Concept"/>
      <skos:inScheme rdf:resource="http://rdf-vocabulary.ddialliance.org/cv/ModeOfCollection/4.0/"/>
      <skos:notation>Observation.Laboratory.Participant</skos:notation>
      <skos:prefLabel xml:lang="en">Participant laboratory observation</skos:prefLabel>
      <skos:definition xml:lang="en">Type of laboratory observation in which the researcher interacts with the subjects and often plays a role in the social situation under observation. For example, observing children's play in a laboratory playroom with the researcher taking part in the play.</skos:definition>
      <skos:prefLabel xml:lang="de">Teilnehmende Laborbeobachtung</skos:prefLabel>
      <skos:definition xml:lang="de">Eine Art der Laborbeobachtung, in der Forschende mit den Probanden interagieren und oft selbst ein Rolle in der sozialen Situation unter Beobachtung einnehmen. Zum Beispiel, die Beobachtung spielender Kinder in einem Labor-Spielzimmer, wobei der/die Forscher*in selbst am Spiel teilnimmt.</skos:definition>
      <skos:prefLabel xml:lang="fi">Havainnointi: laboratoriohavainnointi: osallistuva</skos:prefLabel>
      <skos:definition xml:lang="fi">Kokeellinen havainnointi kontrolloidussa, tarkoitusta varten luodussa tilassa. Tutkija on vuorovaikutuksessa tutkittavien kanssa ja hänellä on usein jokin rooli tutkimuksen kohteena olevassa sosiaalisessa tilanteessa. Esimerkki: Lasten leikkien havainnointi laboratorioon rakennetussa leikkihuoneessa, jossa tutkija ottaa osaa leikkiin.</skos:definition>
      <skos:prefLabel xml:lang="fi">Havainnointi: laboratoriohavainnointi: osallistuva</skos:prefLabel>
      <skos:definition xml:lang="fi">Kokeellinen havainnointi kontrolloidussa, tarkoitusta varten luodussa tilassa. Tutkija on vuorovaikutuksessa tutkittavien kanssa ja hänellä on usein jokin rooli tutkimuksen kohteena olevassa sosiaalisessa tilanteessa. Esimerkki: Lasten leikkien havainnointi laboratorioon rakennetussa leikkihuoneessa, jossa tutkija ottaa osaa leikkiin.</skos:definition>
      <skos:prefLabel xml:lang="it">Osservazione partecipante in laboratorio</skos:prefLabel>
      <skos:definition xml:lang="it">Tipo di osservazione in laboratorio in cui il ricercatore interagisce con i soggetti e spesso gioca un ruolo nella situazione sociale sotto osservazione. Ad esempio, osservando il gioco dei bambini in una stanza da gioco ricreata in laboratorio con il ricercatore che partecipa al gioco.</skos:definition>
      <skos:prefLabel xml:lang="ja">参与型実験室観察</skos:prefLabel>
      <skos:definition xml:lang="ja">研究者が調査対象者とやり取りを行い、しばしば観察下の社会状況において一定の役割を果たしながら行う実験室での観察。例えば、実験用の遊戯室で、研究者が遊びに参加しながら、子どもの遊びを観察する場合。</skos:definition>
      <skos:prefLabel xml:lang="lt">Laboratorinis stebėjimas dalyvaujant</skos:prefLabel>
      <skos:definition xml:lang="lt">Laboratorinio stebėjimo rūšis, kai tyrėjas sąveikauja su tiriamaisiais ir stebimoje socialinėje situacijoje paprastai turi tam tikrą vaidmenį. Pavyzdžiui, vaikų žaidimo stebėjimas laboratoriniame žaidimų kambaryje tyrėjui pačiam įsitraukiant į žaidimą.</skos:definition>
      <skos:prefLabel xml:lang="nl">Participerende observatie in het lab</skos:prefLabel>
      <skos:definition xml:lang="nl"/>
      <skos:prefLabel xml:lang="no">Deltagende laboratorieobservasjon</skos:prefLabel>
      <skos:definition xml:lang="no">En type laboratorieobservasjon hvor forskeren samhandler med forskningsobjektene, og ofte spiller en rolle i den sosiale situasjonen som er under observasjon. For eksempel observere barns lek i et lekerom i laboratoriet, der forsker deltar i leken.</skos:definition>
      <skos:prefLabel xml:lang="no">Deltagende laboratorieobservasjon</skos:prefLabel>
      <skos:definition xml:lang="no">En type laboratorieobservasjon hvor forskeren samhandler med forskningsobjektene, og ofte spiller en rolle i den sosiale situasjonen som er under observasjon. For eksempel observere barns lek i et lekerom i laboratoriet, der forsker deltar i leken.</skos:definition>
      <skos:prefLabel xml:lang="pt">Observação participante em laboratório</skos:prefLabel>
      <skos:definition xml:lang="pt">Tipo de observação em laboratório em que o investigador interage com os sujeitos e, muitas vezes, desempenha um papel na situação social em observação. Por exemplo, observação das brincadeiras das crianças numa sala de jogos de laboratório com o investigador a participar no jogo.</skos:definition>
      <skos:prefLabel xml:lang="sl">Laboratorijsko opazovanje z udeležbo</skos:prefLabel>
      <skos:definition xml:lang="sl">Vrsta laboratorijskega opazovanja, kjer je raziskovalec v interkaciji s subjekti in pogosto igra vlogo v opazovani družbeni situaciji. Na primer, opazovanje otroške igre v laboratorijski igralnici, kjer ima raziskovalec vlogo v igri.</skos:definition>
      <skos:prefLabel xml:lang="sv">Deltagande laboratorieobservation</skos:prefLabel>
      <skos:definition xml:lang="sv">Laboratorieobservation där forskaren interagerar med forskningsobjekten och ofta har en funktion i den sociala situation som observeras. Exempel: observation av barns lek i ett laboratorielekrum där forskaren deltar i leken.</skos:definition>
      <skos:broader rdf:resource="http://rdf-vocabulary.ddialliance.org/cv/ModeOfCollection/4.0/d50e2534"/>
   </rdf:Description>
   <rdf:Description rdf:about="http://rdf-vocabulary.ddialliance.org/cv/ModeOfCollection/4.0/d50e2720">
      <rdf:type rdf:resource="http://www.w3.org/2004/02/skos/core#Concept"/>
      <skos:inScheme rdf:resource="http://rdf-vocabulary.ddialliance.org/cv/ModeOfCollection/4.0/"/>
      <skos:notation>Observation.Laboratory.Nonparticipant</skos:notation>
      <skos:prefLabel xml:lang="en">Non-participant laboratory observation</skos:prefLabel>
      <skos:definition xml:lang="en">Type of laboratory observation that is conducted without any interaction between the researcher and his/her subjects.</skos:definition>
      <skos:prefLabel xml:lang="de">Nicht-teilnehmende Laborbeobachtung</skos:prefLabel>
      <skos:definition xml:lang="de">Eine Art der Laborbeobachtung, die ohne jegliche Interaktion zwischen dem/der Forscher*in und seinen/ihren Probanden*innen durchgeführt wird.</skos:definition>
      <skos:prefLabel xml:lang="fi">Havainnointi: laboratoriohavainnointi: ei-osallistuva</skos:prefLabel>
      <skos:definition xml:lang="fi">Kokeellinen havainnointi kontrolloidussa, tarkoitusta varten luodussa tilassa. Tutkija ei ole missään vuorovaikutuksessa tutkittavien kanssa. Kutsutaan myös tarkkailevaksi laboratoriohavainnoinniksi. Esimerkki: Lasten leikkien havainnointi laboratorioon rakennetussa leikkihuoneessa, jossa tutkija ei ota osaa leikkiin.</skos:definition>
      <skos:prefLabel xml:lang="fi">Havainnointi: laboratoriohavainnointi: ei-osallistuva</skos:prefLabel>
      <skos:definition xml:lang="fi">Kokeellinen havainnointi kontrolloidussa, tarkoitusta varten luodussa tilassa. Tutkija ei ole missään vuorovaikutuksessa tutkittavien kanssa. Kutsutaan myös tarkkailevaksi laboratoriohavainnoinniksi. Esimerkki: Lasten leikkien havainnointi laboratorioon rakennetussa leikkihuoneessa, jossa tutkija ei ota osaa leikkiin.</skos:definition>
      <skos:prefLabel xml:lang="it">Osservazione non partecipante in laboratorio</skos:prefLabel>
      <skos:definition xml:lang="it">Osservazione condotta in laboratorio senza alcuna interazione tra il ricercatore e i soggetti.</skos:definition>
      <skos:prefLabel xml:lang="ja">非参与型実験室観察</skos:prefLabel>
      <skos:definition xml:lang="ja">研究者と調査対象者の間でなんらやり取りをすることなく行われる実験室での観察。</skos:definition>
      <skos:prefLabel xml:lang="lt">Laboratorinis stebėjimas nedalyvaujant</skos:prefLabel>
      <skos:definition xml:lang="lt">Laboratorinio stebėjimo, kuris atliekamas be jokio tyrėjo ir tiriamųjų sąveikos, tipas.</skos:definition>
      <skos:prefLabel xml:lang="nl">Niet-participerende observatie in het lab</skos:prefLabel>
      <skos:definition xml:lang="nl"/>
      <skos:prefLabel xml:lang="no">Ikke-deltagende laboratorieobservasjon</skos:prefLabel>
      <skos:definition xml:lang="no">En type laboratorieobservasjon som blir gjennomført uten interaksjon mellom forskeren og studieobjektene.</skos:definition>
      <skos:prefLabel xml:lang="no">Ikke-deltagende laboratorieobservasjon</skos:prefLabel>
      <skos:definition xml:lang="no">En type laboratorieobservasjon som blir gjennomført uten interaksjon mellom forskeren og studieobjektene.</skos:definition>
      <skos:prefLabel xml:lang="pt">Observação não participante em laboratório</skos:prefLabel>
      <skos:definition xml:lang="pt">Tipo de observação em laboratório realizada sem qualquer interação entre o investigador e os sujeitos observados.</skos:definition>
      <skos:prefLabel xml:lang="sl">Laboratorijsko opazovanje brez udeležbe</skos:prefLabel>
      <skos:definition xml:lang="sl">Vrsta laboratorijskega opazovanja, ki se izvaja brez kakršnekoli interakcije med raziskovalcem in njegovimi/njenimi subjekti.</skos:definition>
      <skos:prefLabel xml:lang="sv">Icke-deltagande laboratorieobservation</skos:prefLabel>
      <skos:definition xml:lang="sv">Laboratorieobservation som utförs utan interaktion mellan forskaren och dennes forskningsobjekt.</skos:definition>
      <skos:broader rdf:resource="http://rdf-vocabulary.ddialliance.org/cv/ModeOfCollection/4.0/d50e2534"/>
   </rdf:Description>
   <rdf:Description rdf:about="http://rdf-vocabulary.ddialliance.org/cv/ModeOfCollection/4.0/d50e2810">
      <rdf:type rdf:resource="http://www.w3.org/2004/02/skos/core#Concept"/>
      <skos:inScheme rdf:resource="http://rdf-vocabulary.ddialliance.org/cv/ModeOfCollection/4.0/"/>
      <skos:notation>Observation.ComputerBased</skos:notation>
      <skos:prefLabel xml:lang="en">Computer-based observation</skos:prefLabel>
      <skos:definition xml:lang="en">Type of observation in which data regarding computer usage are being collected by software that can be built into the computer program itself or can be a separate program. Information may be collected about the number of users, the ways in which users interact with the program(s), how much time they spend on a page, how they use specific sections of applications, how they navigate from page to page or from one application to another, etc.</skos:definition>
      <skos:prefLabel xml:lang="de">Computer-basierte Beobachtung</skos:prefLabel>
      <skos:definition xml:lang="de">Art der Beobachtung, bei der Daten über die Computernutzung von einer Software gesammelt werden, die in das Computerprogramm selbst eingebaut sein kann oder ein separates Programm ist. Es können Informationen über die Anzahl der Benutzer, die Art und Weise, wie die Benutzer mit dem/den Programm(en) interagieren, wie viel Zeit sie auf einer Seite verbringen, wie sie bestimmte Abschnitte von Anwendungen nutzen, wie sie von Seite zu Seite oder von einer Anwendung zu einer anderen navigieren, usw. gesammelt werden.</skos:definition>
      <skos:prefLabel xml:lang="fi">Havainnointi: tietokonepohjainen havainnointi</skos:prefLabel>
      <skos:definition xml:lang="fi">Havainnointimenetelmä, jossa kerätään tietoa ihmisten tietokoneen käytöstä ohjelmallisesti. Havainnointiohjelma voi olla sisäänrakennettu tietokoneohjelmaan tai se voi olla erillinen ohjelma. Tietoa voidaan kerätä käyttäjien määristä, heidän tavoistaan käyttää ohjelmaa ja sen toimintoja, navigoinnista jne.</skos:definition>
      <skos:prefLabel xml:lang="fi">Havainnointi: tietokonepohjainen havainnointi</skos:prefLabel>
      <skos:definition xml:lang="fi">Havainnointimenetelmä, jossa kerätään tietoa ihmisten tietokoneen käytöstä ohjelmallisesti. Havainnointiohjelma voi olla sisäänrakennettu tietokoneohjelmaan tai se voi olla erillinen ohjelma. Tietoa voidaan kerätä käyttäjien määristä, heidän tavoistaan käyttää ohjelmaa ja sen toimintoja, navigoinnista jne.</skos:definition>
      <skos:prefLabel xml:lang="it">Osservazione basata su computer</skos:prefLabel>
      <skos:definition xml:lang="it">Tipo di osservazione in cui vengono raccolti dati riguardanti l'uso del computer, attraverso software che può essere incorporato nel programma informatico stesso, oppure essere un programma separato. Con questo metodo si possono raccogliere informazioni sul numero di utenti, sui modi in cui gli utenti interagiscono con il programma, sulla quantità di tempo che trascorrono su una pagina, su come utilizzano specifiche sezioni di applicazioni, su come navigano da una pagina all'altra o da una applicazione all'altra, ecc.</skos:definition>
      <skos:prefLabel xml:lang="ja">コンピューターによる観察</skos:prefLabel>
      <skos:definition xml:lang="ja">コンピュータの使用状況に関するデータをソフトウェアにより収集する種類の観察。このソフトウェアはコンピュータのプログラムそのものに組み込むことも、あるいは別のプログラムにすることも可能。収集される情報としては、利用者数、利用者によるプログラムの利用方法、利用者が１ページに費やす時間、アプリケーションの個々のセクションの使い方、ページからページ、アプリケーションからアプリケーションにどう移動するか等である。</skos:definition>
      <skos:prefLabel xml:lang="lt">Kompiuterinis stebėjimas</skos:prefLabel>
      <skos:definition xml:lang="lt">Stebėjimo tipas, kai duomenis apie kompiuterio naudojimą renka programinė įranga. Ji gali būti išorinė arba integruota. Informacija gali būti renkama apie vartotojų skaičių, būdus, kaip vartotojai sąveikauja su programa (-omis), kiek laiko praleidžia puslapyje, kaip naudoja tam tikras programos dalis, kaip naršo iš vieno puslapio į kitą, pereina iš vienos programos į kitą ir kt.</skos:definition>
      <skos:prefLabel xml:lang="nl">Computer-gebaseerde observatie</skos:prefLabel>
      <skos:definition xml:lang="nl"/>
      <skos:prefLabel xml:lang="no">Datamaskinbasert observasjon</skos:prefLabel>
      <skos:definition xml:lang="no">Type observasjon hvor data om datamaskinbruk blir samlet av program som kan være inkludert i dataprogrammet en ønsker informasjon om, eller kan forekomme som et eget program. Informasjon om antall brukere, måten brukere samhandler med program(met/mene), hvor mye tid de bruker på siden, hvordan de bruker bestemte deler av en applikasjon, hvordan de navigerer fra side til side eller fra en applikasjon til en annen etc., kan bli samlet.</skos:definition>
      <skos:prefLabel xml:lang="no">Datamaskinbasert observasjon</skos:prefLabel>
      <skos:definition xml:lang="no">Type observasjon hvor data om datamaskinbruk blir samlet av program som kan være inkludert i dataprogrammet en ønsker informasjon om, eller kan forekomme som et eget program. Informasjon om antall brukere, måten brukere samhandler med program(met/mene), hvor mye tid de bruker på siden, hvordan de bruker bestemte deler av en applikasjon, hvordan de navigerer fra side til side eller fra en applikasjon til en annen etc., kan bli samlet.</skos:definition>
      <skos:prefLabel xml:lang="pt">Observação assistida por computador</skos:prefLabel>
      <skos:definition xml:lang="pt">Tipo de observação em que os dados referentes ao uso do computador são recolhidos através de software que pode estar incorporado no próprio programa do computador, ou pode constituir um programa separado. Pode ser recolhida informação sobre o número de utilizadores, a forma como os utilizadores interagem com o(s) programa(s), quanto tempo passam numa página, como usam secções específicas de aplicações, como navegam de uma página para outra ou de uma aplicação para outra, etc.</skos:definition>
      <skos:prefLabel xml:lang="sl">Računalniško podprto opazovanje</skos:prefLabel>
      <skos:definition xml:lang="sl">Vrsta opazovanja, kjer se podatki o uporabi računalnika zbirajo s programsko opremo, ki se jo lahko vgradi v sam računalniški program ali pa predstavlja ločen program. Lahko se zbirajo informacije o številu uporabnikov, o načinih interakcije uporabnikov z računalniškim(i) programom(-mi), koliko časa porabijo na strani, kako uporabljajo določene dele aplikacije, kako krmarijo po straneh ali med aplikacijami itd.</skos:definition>
      <skos:prefLabel xml:lang="sv">Datorbaserad observation</skos:prefLabel>
      <skos:definition xml:lang="sv">Observation där data om datoranvändning samlas in av programvara som inkluderats i ett datorprogram eller som kan vara ett separat program. Information kan samlas in om antal användare, hur användare interagerar med programmet, hur länge de stannar på en sida, hur de använder bestämda delar av program, hur de navigerar från en sida till en annan eller växlar mellan program m.m.</skos:definition>
      <skos:broader rdf:resource="http://rdf-vocabulary.ddialliance.org/cv/ModeOfCollection/4.0/d50e2162"/>
   </rdf:Description>
   <rdf:Description rdf:about="http://rdf-vocabulary.ddialliance.org/cv/ModeOfCollection/4.0/d50e2900">
      <rdf:type rdf:resource="http://www.w3.org/2004/02/skos/core#Concept"/>
      <skos:inScheme rdf:resource="http://rdf-vocabulary.ddialliance.org/cv/ModeOfCollection/4.0/"/>
      <skos:notation>Experiment</skos:notation>
      <skos:prefLabel xml:lang="en">Experiment</skos:prefLabel>
      <skos:definition xml:lang="en">Research method involving the manipulation of some or all of the independent variables included in the hypotheses.</skos:definition>
      <skos:prefLabel xml:lang="de">Experiment</skos:prefLabel>
      <skos:definition xml:lang="de">Forschungsmethode, die die Manipulation einiger oder aller der in den Hypothesen enthaltenen unabhängigen Variablen beinhaltet.</skos:definition>
      <skos:prefLabel xml:lang="fi">Kontrolloitu koe</skos:prefLabel>
      <skos:definition xml:lang="fi">Tutkimusasetelma, jossa tutkimushypoteesin mukaisesti manipuloidaan yhtä tai useampaa riippumatonta muuttujaa.</skos:definition>
      <skos:prefLabel xml:lang="fi">Kontrolloitu koe</skos:prefLabel>
      <skos:definition xml:lang="fi">Tutkimusasetelma, jossa tutkimushypoteesin mukaisesti manipuloidaan yhtä tai useampaa riippumatonta muuttujaa.</skos:definition>
      <skos:prefLabel xml:lang="it">Esperimento</skos:prefLabel>
      <skos:definition xml:lang="it">Metodo di ricerca che coinvolge la manipolazione di alcune o tutte le variabili indipendenti incluse nelle ipotesi.</skos:definition>
      <skos:prefLabel xml:lang="ja">実験</skos:prefLabel>
      <skos:definition xml:lang="ja">仮説に含まれる一部あるいは全部の独立変数を操作して行う研究方法。</skos:definition>
      <skos:prefLabel xml:lang="lt">Eksperimentas</skos:prefLabel>
      <skos:definition xml:lang="lt">Tyrimo metodas apimantis į hipotezes įtrauktų kai kurių ar visų nepriklausomų kintamųjų manipuliavimą.</skos:definition>
      <skos:prefLabel xml:lang="nl">Experiment</skos:prefLabel>
      <skos:definition xml:lang="nl"/>
      <skos:prefLabel xml:lang="no">Eksperiment</skos:prefLabel>
      <skos:definition xml:lang="no">Forskningsmetode som innebærer manipulering av noen eller alle de uavhengige variablene inkludert i hypotesene.</skos:definition>
      <skos:prefLabel xml:lang="no">Eksperiment</skos:prefLabel>
      <skos:definition xml:lang="no">Forskningsmetode som innebærer manipulering av noen eller alle de uavhengige variablene inkludert i hypotesene.</skos:definition>
      <skos:prefLabel xml:lang="pt">Estudo experimental</skos:prefLabel>
      <skos:definition xml:lang="pt">Método de pesquisa que envolve a manipulação de algumas ou de todas as variáveis independentes incluídas nas hipóteses.</skos:definition>
      <skos:prefLabel xml:lang="sl">Eksperiment</skos:prefLabel>
      <skos:definition xml:lang="sl">Raziskovalna metoda, ki vključuje manipulacijo nekaterih ali vseh neodvisnih spremenljivk, vključenih v hipoteze.</skos:definition>
      <skos:prefLabel xml:lang="sv">Experiment</skos:prefLabel>
      <skos:definition xml:lang="sv">Forskningsmetod som omfattar att styra vissa eller alla oberoende variabler som ingår i hypotesen.</skos:definition>
      <skos:narrower rdf:resource="http://rdf-vocabulary.ddialliance.org/cv/ModeOfCollection/4.0/d50e2997"/>
      <skos:narrower rdf:resource="http://rdf-vocabulary.ddialliance.org/cv/ModeOfCollection/4.0/d50e3087"/>
      <skos:narrower rdf:resource="http://rdf-vocabulary.ddialliance.org/cv/ModeOfCollection/4.0/d50e3177"/>
   </rdf:Description>
   <rdf:Description rdf:about="http://rdf-vocabulary.ddialliance.org/cv/ModeOfCollection/4.0/d50e2997">
      <rdf:type rdf:resource="http://www.w3.org/2004/02/skos/core#Concept"/>
      <skos:inScheme rdf:resource="http://rdf-vocabulary.ddialliance.org/cv/ModeOfCollection/4.0/"/>
      <skos:notation>Experiment.Laboratory</skos:notation>
      <skos:prefLabel xml:lang="en">Laboratory experiment</skos:prefLabel>
      <skos:definition xml:lang="en">An experiment conducted in a controlled, artificially created physical setting, in which a researcher manipulates one or several independent variables and measures its/their effect on the dependent variable.</skos:definition>
      <skos:prefLabel xml:lang="de">Laborexperiment</skos:prefLabel>
      <skos:definition xml:lang="de">Ein Experiment, das in einer kontrollierten, künstlich erzeugten Umgebung durchgeführt wird, in der Forschende eine oder mehrere unabhängige Variablen manipulieren und ihre Wirkung auf die abhängige Variable messen.</skos:definition>
      <skos:prefLabel xml:lang="fi">Kontrolloitu koe: laboratoriokoe</skos:prefLabel>
      <skos:definition xml:lang="fi">Kontrolloidussa, tarkoitusta varten luodussa ympäristössä suoritettu koe, jossa tutkija(t) manipuloivat yhtä tai useampaa riippumatonta muuttujaa ja mittaavat sen vaikutusta riippuvaan muuttujaan.</skos:definition>
      <skos:prefLabel xml:lang="fi">Kontrolloitu koe: laboratoriokoe</skos:prefLabel>
      <skos:definition xml:lang="fi">Kontrolloidussa, tarkoitusta varten luodussa ympäristössä suoritettu koe, jossa tutkija(t) manipuloivat yhtä tai useampaa riippumatonta muuttujaa ja mittaavat sen vaikutusta riippuvaan muuttujaan.</skos:definition>
      <skos:prefLabel xml:lang="it">Esperimento in laboratorio</skos:prefLabel>
      <skos:definition xml:lang="it">Un esperimento condotto in un ambiente fisico controllato, creato artificialmente, in cui un ricercatore manipola una o più variabili indipendenti e misura il loro effetto sulla variabile dipendente.</skos:definition>
      <skos:prefLabel xml:lang="ja">実験室実験</skos:prefLabel>
      <skos:definition xml:lang="ja">統制された人工的な物理環境で行われる実験。研究者が1つあるいは複数の独立変数を操作し、それらの変数が従属変数に与える影響を測定する。</skos:definition>
      <skos:prefLabel xml:lang="lt">Laboratorinis eksperimentas</skos:prefLabel>
      <skos:definition xml:lang="lt">Eksperimentas, atliekamas kontroliuojamoje, dirbtinai sukurtoje fizinėje aplinkoje, kurio metu tyrėjas manipuliuoja vienu ar keliais nepriklausomais kintamaisiais ir išmatuoja jų poveikį priklausomam kintamajam.</skos:definition>
      <skos:prefLabel xml:lang="nl">Experiment in het lab</skos:prefLabel>
      <skos:definition xml:lang="nl"/>
      <skos:prefLabel xml:lang="no">Laboratorieeksperiment</skos:prefLabel>
      <skos:definition xml:lang="no">Et eksperiment som utføres i et kontrollert, kunstig utformet miljø, hvor forskeren manipulerer én eller flere av de uavhengige variablene og måler effekten det har på den avhengige variabelen.</skos:definition>
      <skos:prefLabel xml:lang="no">Laboratorieeksperiment</skos:prefLabel>
      <skos:definition xml:lang="no">Et eksperiment som utføres i et kontrollert, kunstig utformet miljø, hvor forskeren manipulerer én eller flere av de uavhengige variablene og måler effekten det har på den avhengige variabelen.</skos:definition>
      <skos:prefLabel xml:lang="pt">Estudo experimental em laboratório</skos:prefLabel>
      <skos:definition xml:lang="pt">Experiência/experimento conduzida/o em ambiente físico controlado, artificialmente criado, no qual o investigador manipula uma ou várias variáveis independentes e mede o seu efeito sobre a variável dependente.</skos:definition>
      <skos:prefLabel xml:lang="sl">Laboratorijski eksperiment</skos:prefLabel>
      <skos:definition xml:lang="sl">Eksperiment, ki se izvaja v nadzorovanem, umetno ustvarjenem fizičnem okolju, v katerem raziskovalec manipulira z eno ali več neodvisnimi spremenljivkami in meri svoj vpliv na odvisno spremenljivko.</skos:definition>
      <skos:prefLabel xml:lang="sv">Laboratorieexperiment</skos:prefLabel>
      <skos:definition xml:lang="sv">Ett experiment som utförs i en kontrollerad, konstgjord fysisk miljö där forskaren styr en eller flera oberoende variabler och mäter dess/deras effekt på den beroende variabeln.</skos:definition>
      <skos:broader rdf:resource="http://rdf-vocabulary.ddialliance.org/cv/ModeOfCollection/4.0/d50e2900"/>
   </rdf:Description>
   <rdf:Description rdf:about="http://rdf-vocabulary.ddialliance.org/cv/ModeOfCollection/4.0/d50e3087">
      <rdf:type rdf:resource="http://www.w3.org/2004/02/skos/core#Concept"/>
      <skos:inScheme rdf:resource="http://rdf-vocabulary.ddialliance.org/cv/ModeOfCollection/4.0/"/>
      <skos:notation>Experiment.FieldIntervention</skos:notation>
      <skos:prefLabel xml:lang="en">Field/Intervention experiment</skos:prefLabel>
      <skos:definition xml:lang="en">An experiment conducted in a natural, uncontrolled setting, in which the researcher manipulates one or several independent variables. Intervention/clinical studies are one example of field experiments.</skos:definition>
      <skos:prefLabel xml:lang="de">Feld-/Interventionsexperiment</skos:prefLabel>
      <skos:definition xml:lang="de">Ein Experiment, das in einer natürlichen, unkontrollierten Umgebung durchgeführt wird, in der Forschende eine oder mehrere unabhängige Variablen manipulieren. Interventions-/klinische Studien sind ein Beispiel für Feldexperimente.</skos:definition>
      <skos:prefLabel xml:lang="fi">Kontrolloitu koe: kenttä- tai interventiokoe</skos:prefLabel>
      <skos:definition xml:lang="fi">Luonnollisessa, kontrolloimattomassa ympäristössä suoritettu koe, jossa tutkija(t) manipuloivat yhtä tai useampaa riippumatonta muuttujaa. Esimerkkejä: kliiniset tutkimukset.</skos:definition>
      <skos:prefLabel xml:lang="fi">Kontrolloitu koe: kenttä- tai interventiokoe</skos:prefLabel>
      <skos:definition xml:lang="fi">Luonnollisessa, kontrolloimattomassa ympäristössä suoritettu koe, jossa tutkija(t) manipuloivat yhtä tai useampaa riippumatonta muuttujaa. Esimerkkejä: kliiniset tutkimukset.</skos:definition>
      <skos:prefLabel xml:lang="it">Esperimento sul campo / Intervento</skos:prefLabel>
      <skos:definition xml:lang="it">Un esperimento condotto in un ambiente naturale, non controllato, in cui il ricercatore manipola una o più variabili indipendenti. Gli interventi o studi clinici sono un esempio di esperimenti sul campo.</skos:definition>
      <skos:prefLabel xml:lang="ja">フィールド／介入実験</skos:prefLabel>
      <skos:definition xml:lang="ja">自然で、統制されていない環境で行われる実験。研究者は1つあるいは複数の独立変数を操作する。フィールド実験の一例として、介入/臨床研究がある。</skos:definition>
      <skos:prefLabel xml:lang="lt">Lauko arba intervencinis eksperimentas</skos:prefLabel>
      <skos:definition xml:lang="lt">Eksperimentas, atliktas natūralioje, nekontroliuojamoje aplinkoje, kurio metu tyrėjas manipuliuoja vienu ar keliais nepriklausomais kintamaisiais. Intervenciniai ar klinikiniai tyrimai yra lauko eksperimentų pavyzdžiai.</skos:definition>
      <skos:prefLabel xml:lang="nl">Experiment in het veld/interventie</skos:prefLabel>
      <skos:definition xml:lang="nl"/>
      <skos:prefLabel xml:lang="no">Felt/felteksperiment</skos:prefLabel>
      <skos:definition xml:lang="no">Et eksperiment som utføres i et naturlig, ukontrollert miljø, hvor forskeren manipulerer én eller flere av de uavhengige variablene. Intervensjon/kliniske studier er et eksempel på felteksperiment.</skos:definition>
      <skos:prefLabel xml:lang="no">Felt/felteksperiment</skos:prefLabel>
      <skos:definition xml:lang="no">Et eksperiment som utføres i et naturlig, ukontrollert miljø, hvor forskeren manipulerer én eller flere av de uavhengige variablene. Intervensjon/kliniske studier er et eksempel på felteksperiment.</skos:definition>
      <skos:prefLabel xml:lang="pt">Estudo experimental de campo (com intervenção)</skos:prefLabel>
      <skos:definition xml:lang="pt">Experiência/experimento conduzida/o em ambiente natural e não controlado, no qual o investigador manipula uma ou várias variáveis independentes. Estudos clínicos ou de intervenção são um exemplo de experimentações de campo.</skos:definition>
      <skos:prefLabel xml:lang="sl">Terenski/intervencijski eksperiment</skos:prefLabel>
      <skos:definition xml:lang="sl">Eksperiment, ki se izvaja v naravnem, nekontroliranem okolju, v katerem raziskovalec manipulira z eno ali več neodvisnimi spremenljivkami. Intervencija/klinične študije so en primer terenskih eksperimentov.</skos:definition>
      <skos:prefLabel xml:lang="sv">Fältexperiment</skos:prefLabel>
      <skos:definition xml:lang="sv">Ett experiment som utförs i en naturlig, okontrollerad miljö där forskaren styr en eller flera oberoende variabler. Interventionsstudier och kliniska studier är exempel på fältexperiment.</skos:definition>
      <skos:broader rdf:resource="http://rdf-vocabulary.ddialliance.org/cv/ModeOfCollection/4.0/d50e2900"/>
   </rdf:Description>
   <rdf:Description rdf:about="http://rdf-vocabulary.ddialliance.org/cv/ModeOfCollection/4.0/d50e3177">
      <rdf:type rdf:resource="http://www.w3.org/2004/02/skos/core#Concept"/>
      <skos:inScheme rdf:resource="http://rdf-vocabulary.ddialliance.org/cv/ModeOfCollection/4.0/"/>
      <skos:notation>Experiment.WebBased</skos:notation>
      <skos:prefLabel xml:lang="en">Web-based experiment</skos:prefLabel>
      <skos:definition xml:lang="en">An experiment conducted in the virtual setting of the World Wide Web, in which experimental materials are programmed to implement artificial situations or events to be investigated in a distributed environment. (Reips, U.-D. (2002). Theory and techniques of Web experimenting. In B. Batinic, U.-D. Reips, &amp; M. Bosnjak (Eds.), Online Social Sciences. Seattle: Hogrefe &amp; Huber. Available at: http://www.websm.org/uploadi/editor/Reips_2002_Theory_and_techniques.pdf [07 June 2013])</skos:definition>
      <skos:prefLabel xml:lang="de">Web-basiertes Experiment</skos:prefLabel>
      <skos:definition xml:lang="de">Ein Experiment, das in der virtuellen Umgebung des World Wide Web durchgeführt wird, in dem experimentelle Materialien programmiert werden, um künstliche Situationen oder Ereignisse zu implementieren, die in einer verteilten Umgebung untersucht werden sollen.</skos:definition>
      <skos:prefLabel xml:lang="fi">Kontrolloitu koe: virtuaalinen koe</skos:prefLabel>
      <skos:definition xml:lang="fi">Internetissä toteutettu kokeellinen tutkimus, jossa on ohjelmallisesti luotu keinotekoisia virtuaalisia ympäristöjä tai tapahtumia tutkimusta varten. Esimerkki: Keinotekoisen kielen oppimiskoe, virtuaalisen pelikäyttäytymisen koe.</skos:definition>
      <skos:prefLabel xml:lang="fi">Kontrolloitu koe: virtuaalinen koe</skos:prefLabel>
      <skos:definition xml:lang="fi">Internetissä toteutettu kokeellinen tutkimus, jossa on ohjelmallisesti luotu keinotekoisia virtuaalisia ympäristöjä tai tapahtumia tutkimusta varten. Esimerkki: Keinotekoisen kielen oppimiskoe, virtuaalisen pelikäyttäytymisen koe.</skos:definition>
      <skos:prefLabel xml:lang="it">Esperimento web</skos:prefLabel>
      <skos:definition xml:lang="it">Un esperimento condotto nell'ambiente virtuale del World Wide Web, in cui i materiali sperimentali sono programmati per ricreare situazioni o eventi artificiali da indagare in un ambiente distribuito.</skos:definition>
      <skos:prefLabel xml:lang="ja">Webベース実験</skos:prefLabel>
      <skos:definition xml:lang="ja">World Wide Webの仮想環境で行われる実験。実験材料をプログラムし、人工的な状況やイベントを作り出すことで、分散した環境において調査を実施する (Reips, U.-D. (2002). Theory and techniques of Web experimenting. In B. Batinic, U.-D. Reips, &amp; M. Bosnjak (Eds.), Online Social Sciences. Seattle: Hogrefe &amp; Huber. http://www.websm.org/uploadi/editor/Reips_2002_Theory_and_techniques.pdf [07 June 2013])。</skos:definition>
      <skos:prefLabel xml:lang="lt">Internetinis eksperimentas</skos:prefLabel>
      <skos:definition xml:lang="lt">Eksperimentas atliekamas virtualioje aplinkoje per internetą, kai suprogramuota eksperimentinė medžiaga sukuria dirbtines situacijas ir įvykius paskirstytoje aplinkoje.  (Reips, U.-D. (2002). Theory and techniques of Web experimenting. In B. Batinic, U.-D. Reips, &amp; M. Bosnjak (Eds.), Online Social Sciences. Seattle: Hogrefe &amp; Huber. Galima rasti: http://www.websm.org/uploadi/editor/Reips_2002_Theory_and_techniques.pdf   [2013 m. birželio 7 d.]).</skos:definition>
      <skos:prefLabel xml:lang="nl">Webgebaseerd experiment</skos:prefLabel>
      <skos:definition xml:lang="nl"/>
      <skos:prefLabel xml:lang="no">Webbasert eksperiment</skos:prefLabel>
      <skos:definition xml:lang="no">Et eksperiment som utføres i et vituelt miljø på internett (World Wide Web), hvor eksperimentelt materiale er programmert til å sette i gang kunstige situasjoner eller hendelser som kan undersøkes i et gitt miljø. (Reips, U.-D. (2002). Theory and techniques of Web experimenting. In B. Batinic, U.-D. Reips, &amp; M. Bosnjak (Eds.), Online Social Sciences. Seattle: Hogrefe &amp; Huber. Available at: http://www.websm.org/uploadi/editor/Reips_2002_Theory_and_techniques.pdf [07 June 2013])</skos:definition>
      <skos:prefLabel xml:lang="no">Webbasert eksperiment</skos:prefLabel>
      <skos:definition xml:lang="no">Et eksperiment som utføres i et vituelt miljø på internett (World Wide Web), hvor eksperimentelt materiale er programmert til å sette i gang kunstige situasjoner eller hendelser som kan undersøkes i et gitt miljø. (Reips, U.-D. (2002). Theory and techniques of Web experimenting. In B. Batinic, U.-D. Reips, &amp; M. Bosnjak (Eds.), Online Social Sciences. Seattle: Hogrefe &amp; Huber. Available at: http://www.websm.org/uploadi/editor/Reips_2002_Theory_and_techniques.pdf [07 June 2013])</skos:definition>
      <skos:prefLabel xml:lang="pt">Estudo experimental online/via web</skos:prefLabel>
      <skos:definition xml:lang="pt">Experiência/experimento conduzida/o em ambiente virtual da World Wide Web, no qual materiais experimentais são programados para implementar situações ou eventos artificiais para pesquisa num ambiente distribuído. (Reips, U.-D. (2002). Theory and techniques of Web experimenting. In B. Batinic, U.-D. Reips, &amp;amp; M. Bosnjak (Eds.), Online Social Sciences. Seattle: Hogrefe &amp;amp; Huber. Disponível em: http://www.websm.org/uploadi/editor/Reips_2002_Theory_and_techniques.pdf [07 June 2013])</skos:definition>
      <skos:prefLabel xml:lang="sl">Spletni eksperiment</skos:prefLabel>
      <skos:definition xml:lang="sl">Eksperiment, ki se izvaja v virtualnem okolju svetovnega spleta, v katerem so eksperimentalni materiali programirani za izvajanje umetnih situacij ali dogodkov, ki jih je treba raziskati v tako vzpostavljenem okolju. (Reips, U.-D. (2002). Theory and techniques of Web experimenting. V B. Batinic, U.-D. Reips, &amp; M. Bosnjak (Eds.), Online Social Sciences. Seattle: Hogrefe &amp; Huber. Dostopno preko: http://www.websm.org/uploadi/editor/Reips_2002_Theory_and_techniques.pdf [07. junij 2013])</skos:definition>
      <skos:prefLabel xml:lang="sv">Webbaserat experiment</skos:prefLabel>
      <skos:definition xml:lang="sv">Ett experiment som utförs i en virtuell miljö på webben, där experimentella material programmeras för att skapa artificiella situationer eller händelser som undersöks i en distribuerad miljö.  (Reips, U.-D. (2002). Theory and techniques of Web experimenting. In B. Batinic, U.-D. Reips, &amp; M. Bosnjak (Eds.), Online Social Sciences. Seattle: Hogrefe &amp; Huber. Tillgänglig: http://www.websm.org/uploadi/editor/Reips_2002_Theory_and_techniques.pdf [8 september, 2016])</skos:definition>
      <skos:broader rdf:resource="http://rdf-vocabulary.ddialliance.org/cv/ModeOfCollection/4.0/d50e2900"/>
   </rdf:Description>
   <rdf:Description rdf:about="http://rdf-vocabulary.ddialliance.org/cv/ModeOfCollection/4.0/d50e3268">
      <rdf:type rdf:resource="http://www.w3.org/2004/02/skos/core#Concept"/>
      <skos:inScheme rdf:resource="http://rdf-vocabulary.ddialliance.org/cv/ModeOfCollection/4.0/"/>
      <skos:notation>Recording</skos:notation>
      <skos:prefLabel xml:lang="en">Recording</skos:prefLabel>
      <skos:definition xml:lang="en">Registering by mechanical or electronic means, in a form that allows the information to be retrieved and/or reproduced. For example, images or sounds on disc or magnetic tape.</skos:definition>
      <skos:prefLabel xml:lang="de">Aufzeichnung (mechanisch/elektronisch)</skos:prefLabel>
      <skos:definition xml:lang="de">Aufzeichnungen, die auf mechanischem oder elektronischem Wege getätigt werden und die es ermöglichen, die Informationen abzurufen und/oder zu reproduzieren. Zum Beispiel Bilder oder Töne auf Diskette oder Magnetband.</skos:definition>
      <skos:prefLabel xml:lang="fi">Taltiointi</skos:prefLabel>
      <skos:definition xml:lang="fi">Aineiston taltioiminen mekaanisesti tai elektronisesti tavalla, joka mahdollistaa sen kuuntelun, katselun tai monistamisen. Sisältää mm. valokuvien, videon tai äänen taltioimisen. Esimerkki: Kokousten tai vastaanottojen videoiminen ilman tutkijan läsnäoloa, valokuvista muodostuva aineisto.</skos:definition>
      <skos:prefLabel xml:lang="fi">Taltiointi</skos:prefLabel>
      <skos:definition xml:lang="fi">Aineiston taltioiminen mekaanisesti tai elektronisesti tavalla, joka mahdollistaa sen kuuntelun, katselun tai monistamisen. Sisältää mm. valokuvien, videon tai äänen taltioimisen. Esimerkki: Kokousten tai vastaanottojen videoiminen ilman tutkijan läsnäoloa, valokuvista muodostuva aineisto.</skos:definition>
      <skos:prefLabel xml:lang="it">Registrazione</skos:prefLabel>
      <skos:definition xml:lang="it">Registrazione tramite mezzi meccanici o elettronici, in una forma che consente di recuperare e/o riprodurre le informazioni. Ad esempio, registrazioni di immagini o suoni su disco o supporto magnetico.</skos:definition>
      <skos:prefLabel xml:lang="ja">記録</skos:prefLabel>
      <skos:definition xml:lang="ja">情報を検索、複製できる形式で機械的あるいは電子的手段により記録すること。例えば、画像や音のディスクや磁気テープへの記録。</skos:definition>
      <skos:prefLabel xml:lang="lt">Įrašas</skos:prefLabel>
      <skos:definition xml:lang="lt">Mechaninėmis ar elektroninėmis priemonėmis atliekamas įrašymas taip, kad informaciją būtų galima pasiekti ir (arba) atkurti. Pavyzdžiui, vaizdai ar garsai diske ar magnetinėje juostoje.</skos:definition>
      <skos:prefLabel xml:lang="nl">Opname</skos:prefLabel>
      <skos:definition xml:lang="nl"/>
      <skos:prefLabel xml:lang="no">Opptak</skos:prefLabel>
      <skos:definition xml:lang="no">Mekanisk eller elektronisk registrering i et format som gjør det mulig å gjeninnhente og/eller gjenskape informasjonen. For eksempel bilder eller lyd på disk eller magnetbånd.</skos:definition>
      <skos:prefLabel xml:lang="no">Opptak</skos:prefLabel>
      <skos:definition xml:lang="no">Mekanisk eller elektronisk registrering i et format som gjør det mulig å gjeninnhente og/eller gjenskape informasjonen. For eksempel bilder eller lyd på disk eller magnetbånd.</skos:definition>
      <skos:prefLabel xml:lang="pt">Gravação</skos:prefLabel>
      <skos:definition xml:lang="pt">Registo por meios mecânicos ou electrónicos, de forma a permitir que a informação seja recuperada e/ou reproduzida. Por exemplo, imagens ou sons em disco ou fita magnética.</skos:definition>
      <skos:prefLabel xml:lang="sl">Snemanje</skos:prefLabel>
      <skos:definition xml:lang="sl">Snemanje z mehanskimi ali elektronskimi sredstvi v obliki, ki omogoča, da se informacije prikličejo in/ali reproducirajo. Na primer slike ali zvoki na disku ali magnetnem traku.</skos:definition>
      <skos:prefLabel xml:lang="sv">Inspelning</skos:prefLabel>
      <skos:definition xml:lang="sv">Upptagning, på mekanisk eller elektronisk väg, på sådant sätt att informationen kan återfås och/eller återskapas. Exempel: bilder eller ljud på en cd eller ett magnetband.</skos:definition>
      <skos:narrower rdf:resource="http://rdf-vocabulary.ddialliance.org/cv/ModeOfCollection/4.0/d50e3361"/>
   </rdf:Description>
   <rdf:Description rdf:about="http://rdf-vocabulary.ddialliance.org/cv/ModeOfCollection/4.0/d50e3361">
      <rdf:type rdf:resource="http://www.w3.org/2004/02/skos/core#Concept"/>
      <skos:inScheme rdf:resource="http://rdf-vocabulary.ddialliance.org/cv/ModeOfCollection/4.0/"/>
      <skos:notation>Recording.RemoteSensing</skos:notation>
      <skos:prefLabel xml:lang="en">Recording: Remote sensing</skos:prefLabel>
      <skos:definition xml:lang="en">Collecting information on objects or phenomena without physical contact with them, using remote sensors on satellites and aircraft (planes, drones, weather balloons). Often used to gather information on the Earth’s surface, atmosphere and oceans. For example, damage assessment after an earthquake or forest fires. The technique is also used for military, commercial, economic and other applications.</skos:definition>
      <skos:prefLabel xml:lang="de">Aufzeichnung: Fernerkundung</skos:prefLabel>
      <skos:definition xml:lang="de">Das Sammeln von Informationen über Objekte oder Phänomene ohne physischen Kontakt mit ihnen, mithilfe von Fernsensoren auf Satelliten und Flugzeugen (Flugzeuge, Drohnen, Wetterballons). Wird oft verwendet, um Informationen über die Erdoberfläche, die Atmosphäre und die Ozeane zu sammeln. Zum Beispiel bei der Schadensbeurteilung nach einem Erdbeben oder bei Waldbränden. Die Technik wird auch für militärische, kommerzielle, wirtschaftliche und andere Anwendungen genutzt.</skos:definition>
      <skos:prefLabel xml:lang="fi">Taltiointi: etämittaus</skos:prefLabel>
      <skos:definition xml:lang="fi">Tiedonkeruu etämittauksella eli kaukokartoituksella, käyttäen satelliitteihin tai ilma-aluksiin (lentokoneet, dronet, helikopterit, sääpallot) sijoitettuja mittalaitteita. Mitattavaan kohteeseen tai ilmiöön ei ole fyysistä kontaktia. Menetelmää käytetään usein Maan pinnan, ilmakehän tai vesistöjen havainnointiin, esimerkiksi vahinkojen arviointiin maanjäristysten tai metsäpalojen jälkeen. Etämittausta voidaan käyttää myös sotilaallisissa, kaupallisissa tai muissa sovelluksissa.</skos:definition>
      <skos:prefLabel xml:lang="fi">Taltiointi: etämittaus</skos:prefLabel>
      <skos:definition xml:lang="fi">Tiedonkeruu etämittauksella eli kaukokartoituksella, käyttäen satelliitteihin tai ilma-aluksiin (lentokoneet, dronet, helikopterit, sääpallot) sijoitettuja mittalaitteita. Mitattavaan kohteeseen tai ilmiöön ei ole fyysistä kontaktia. Menetelmää käytetään usein Maan pinnan, ilmakehän tai vesistöjen havainnointiin, esimerkiksi vahinkojen arviointiin maanjäristysten tai metsäpalojen jälkeen. Etämittausta voidaan käyttää myös sotilaallisissa, kaupallisissa tai muissa sovelluksissa.</skos:definition>
      <skos:prefLabel xml:lang="it">Registrazione: telerilevamento</skos:prefLabel>
      <skos:definition xml:lang="it">Raccolta di informazioni relative ad oggetti o fenomeni senza che vi sia un contatto fisico con essi, utilizzando sensori remoti posizionati su satelliti e apparecchi aeronautici (aerei, droni, palloni sonda). Spesso è utilizzato per raccogliere informazioni sulla superficie terrestre, sull'atmosfera e sugli oceani. Per esempio, viene utilizzato per la valutazione dei danni causati da un terremoto o da incendi boschivi. La tecnica è usata anche per applicazioni in campo militare, commerciale, economico e di altro tipo.</skos:definition>
      <skos:prefLabel xml:lang="ja">記録：リモートセンシング</skos:prefLabel>
      <skos:definition xml:lang="ja">衛星や航空機（飛行機、ドローン、気球）のリモートセンサーを使用して、物理的に接触することなく物体や現象の情報を収集する。多くの場合、地表、大気、そして海洋についての情報を集めるために利用される。例えば、地震や森林火災の後に被害状況を評価するために用いられる。この技術は、軍事、商用、経済分野等にも応用されている。</skos:definition>
      <skos:prefLabel xml:lang="lt">Įrašas: nuotolinis stebėjimas</skos:prefLabel>
      <skos:definition xml:lang="lt">Informacijos apie objektus ar reiškinius rinkimas be fizinio kontakto su jais, naudojant nuotolinius palydovų ir orlaivių (lėktuvų, nepilotuojamų orlaivių, oro balionų) jutiklius. Dažnai naudojamas renkant informaciją apie Žemės paviršių, atmosferą ir vandenynus. Pavyzdžiui, žalos vertinimas po žemės drebėjimų ar miškų gaisrų. Ši technika taip pat naudojama karinėms, komercinėms, ekonominėms ir kitoms reikmėms.</skos:definition>
      <skos:prefLabel xml:lang="nl">Opname: op afstand opgenomen</skos:prefLabel>
      <skos:definition xml:lang="nl"/>
      <skos:prefLabel xml:lang="no">Opptak: Fjernmåling</skos:prefLabel>
      <skos:definition xml:lang="no">Innsamling av informasjon om objekter eller fenomen uten fysisk kontakt med de ved bruk av fjernmålere på satellitter og luftfartøy (fly, droner, værballonger). Ofte brukt for å samle informasjon om jordens overflate, atmosfære og hav. For eksempel, skadevurdering etter et jordskjelv eller skogbrann. Teknikken brukes også av militære, kommersielle, økonomiske og andre formål.</skos:definition>
      <skos:prefLabel xml:lang="no">Opptak: Fjernmåling</skos:prefLabel>
      <skos:definition xml:lang="no">Innsamling av informasjon om objekter eller fenomen uten fysisk kontakt med de ved bruk av fjernmålere på satellitter og luftfartøy (fly, droner, værballonger). Ofte brukt for å samle informasjon om jordens overflate, atmosfære og hav. For eksempel, skadevurdering etter et jordskjelv eller skogbrann. Teknikken brukes også av militære, kommersielle, økonomiske og andre formål.</skos:definition>
      <skos:prefLabel xml:lang="pt">Gravação: Sensoriamento remoto ou deteção remota</skos:prefLabel>
      <skos:definition xml:lang="pt">Recolha de informações sobre objetos ou fenómenos sem contato físico com os mesmos, por meio de sensores remotos em satélites e aeronaves (aviões, drones, balões meteorológicos). Método frequentemente usado para obter informações sobre a superfície da Terra, atmosfera e oceanos. Por exemplo, avaliação de danos após um terramoto ou incêndios florestais. A técnica também é usada para aplicações militares, comerciais, económicas e outras.</skos:definition>
      <skos:prefLabel xml:lang="sl">Snemanje: daljinsko zaznavanje</skos:prefLabel>
      <skos:definition xml:lang="sl">Zbiranje informacij o predmetih ali pojavih brez fizičnega stika z njimi z uporabo daljinskih senzorjev na satelitih in letalih (letala, droni, vremenski baloni). Pogosto se uporablja za zbiranje informacij o zemeljski površini, ozračju in oceanih. Na primer ocena škode po potresu ali gozdnih požarih. Tehnika se uporablja tudi za vojaške, komercialne, gospodarske in druge namene.</skos:definition>
      <skos:prefLabel xml:lang="sv">Inspelning: fjärranalys</skos:prefLabel>
      <skos:definition xml:lang="sv">Insamling av information om objekt eller företeelser utan att ha fysisk kontakt med dem. Insamlingen görs med fjärrsensorer på satelliter och luftfartyg (t.ex. flygplan, drönare, väderballonger). Fjärranalys används ofta för att samla in information om jorden och dess atmosfär och hav, t.ex. skadebedömning efter jordbävningar eller skogsbränder. Tekniken används även för bland annat militära, affärsmässiga och ekonomiska syften.</skos:definition>
      <skos:broader rdf:resource="http://rdf-vocabulary.ddialliance.org/cv/ModeOfCollection/4.0/d50e3268"/>
   </rdf:Description>
   <rdf:Description rdf:about="http://rdf-vocabulary.ddialliance.org/cv/ModeOfCollection/4.0/d50e3451">
      <rdf:type rdf:resource="http://www.w3.org/2004/02/skos/core#Concept"/>
      <skos:inScheme rdf:resource="http://rdf-vocabulary.ddialliance.org/cv/ModeOfCollection/4.0/"/>
      <skos:notation>AutomatedDataExtraction</skos:notation>
      <skos:prefLabel xml:lang="en">Automated data extraction</skos:prefLabel>
      <skos:definition xml:lang="en">Using automated means to retrieve information from data sources and save it to a local file or database for further processing or storage. Use this term if it is not known what kind of automated technique has been used or if the technique is known but not listed as a narrower term.</skos:definition>
      <skos:prefLabel xml:lang="de">Automatisierte Datenextraktion</skos:prefLabel>
      <skos:definition xml:lang="de">Verwendung automatisierter Mittel zum Abrufen von Informationen aus Datenquellen und Speichern in einer lokalen Datei oder Datenbank zur weiteren Verarbeitung oder Speicherung. Verwenden Sie diesen Begriff, wenn nicht bekannt ist, welche Art von automatisierter Technik verwendet wurde, oder wenn die Technik bekannt ist, aber nicht als engerer Begriff aufgeführt ist.</skos:definition>
      <skos:prefLabel xml:lang="fi">Automatisoitu tiedonpoiminta</skos:prefLabel>
      <skos:definition xml:lang="fi">Automatisoidut menetelmät tiedon poimimiseksi erilaisista tietolähteistä. Tieto tallennetaan tiedostoon tai tietokantaan myöhempää käsittelyä tai säilytystä varten. Käytä tätä termiä mikäli ei ole tiedossa millaista automatisoitua tiedonpoimintaa on käytetty tai mikäli menetelmä on tiedossa mutta ei sanastossa.</skos:definition>
      <skos:prefLabel xml:lang="fi">Automatisoitu tiedonpoiminta</skos:prefLabel>
      <skos:definition xml:lang="fi">Automatisoidut menetelmät tiedon poimimiseksi erilaisista tietolähteistä. Tieto tallennetaan tiedostoon tai tietokantaan myöhempää käsittelyä tai säilytystä varten. Käytä tätä termiä mikäli ei ole tiedossa millaista automatisoitua tiedonpoimintaa on käytetty tai mikäli menetelmä on tiedossa mutta ei sanastossa.</skos:definition>
      <skos:prefLabel xml:lang="it">Estrazione automatizzata</skos:prefLabel>
      <skos:definition xml:lang="it">Utilizzo di strumenti automatizzati per recuperare informazioni da fonti di dati e salvarle in un file locale o in un database per una successiva elaborazione o archiviazione. Utilizzare questo termine se non si conosce il tipo di tecnica automatizzata impiegata oppure se la tecnica è nota ma non è presente nell'elenco.</skos:definition>
      <skos:prefLabel xml:lang="ja">自動データ抽出</skos:prefLabel>
      <skos:definition xml:lang="ja">自動的にデータソースから情報を検索し、取得した情報をローカルファイルあるいはデータベースに保存する。その後さらにデータの処理と保管が行われる。どのような自動化の技術が用いられたのか不明な場合や使われた技術はわかっているがより意味を限定した用語がリストに含まれていない場合に、この用語を用いる。</skos:definition>
      <skos:prefLabel xml:lang="lt">Automatinė duomenų gavyba</skos:prefLabel>
      <skos:definition xml:lang="lt">Automatinių priemonių naudojimas, siekiant nuskaityti informaciją iš duomenų šaltinių ir išsaugoti ją vidiniame faile arba duomenų bazėje, skirtoje tolesniam apdorojimui ar saugojimui. Naudoti šį platesnį terminą, kai nėra žinoma, kokia automatinės duomenų gavybos technika buvo naudota, arba jei ji yra žinoma, bet nėra jai skirto siauresnio termino.</skos:definition>
      <skos:prefLabel xml:lang="nl">Geautomatiseerde data-extractie</skos:prefLabel>
      <skos:definition xml:lang="nl"/>
      <skos:prefLabel xml:lang="no">Automatisert datautvinning</skos:prefLabel>
      <skos:definition xml:lang="no">Å bruke automatiske midler for å hente informasjon fra datakilder og lagre det i en lokal fil eller database for ytterligere prosessering eller oppbevaring. Bruk denne termen hvis det er ukjent hvilke automatisk teknikk som har blitt brukt eller teknikken er kjent, men ikke er oppført i et av de smalere begrepene.</skos:definition>
      <skos:prefLabel xml:lang="no">Automatisert datautvinning</skos:prefLabel>
      <skos:definition xml:lang="no">Å bruke automatiske midler for å hente informasjon fra datakilder og lagre det i en lokal fil eller database for ytterligere prosessering eller oppbevaring. Bruk denne termen hvis det er ukjent hvilke automatisk teknikk som har blitt brukt eller teknikken er kjent, men ikke er oppført i et av de smalere begrepene.</skos:definition>
      <skos:prefLabel xml:lang="pt">Extração de dados automatizada</skos:prefLabel>
      <skos:definition xml:lang="pt">Uso de meios automatizados para obter informações de fontes de dados e salvá-las num ficheiro local ou banco de dados, para posterior processamento ou armazenamento. Usar este termo se não se souber o tipo de técnica automatizada que foi usada, ou se a técnica for conhecida, mas não listada como um termo mais restrito.</skos:definition>
      <skos:prefLabel xml:lang="sl">Avtomatizirano pridobivanje podatkov</skos:prefLabel>
      <skos:definition xml:lang="sl">Uporaba avtomatiziranih sredstev za pridobivanje informacij iz virov podatkov in njihov prenos v lokalno datoteko ali bazo podatkov za nadaljnjo obdelavo ali shranjevanje. Uporabite ta izraz, če ni znano, kakšna avtomatizirana tehnika je bila uporabljena ali če je tehnika znana, vendar ni navedena kot ožji izraz.</skos:definition>
      <skos:prefLabel xml:lang="sv">Automatiserad dataextrahering</skos:prefLabel>
      <skos:definition xml:lang="sv">Användning av automatiserade metoder för att hämta information ur datakällor och spara informationen som en lokal fil eller databas för ytterligare behandling eller lagring. Använd den här termen om det inte är känt vilken automatiserad teknik som använts eller om tekniken är känd, men inte finns listad som en smalare term.</skos:definition>
      <skos:narrower rdf:resource="http://rdf-vocabulary.ddialliance.org/cv/ModeOfCollection/4.0/d50e3548"/>
      <skos:narrower rdf:resource="http://rdf-vocabulary.ddialliance.org/cv/ModeOfCollection/4.0/d50e3638"/>
      <skos:narrower rdf:resource="http://rdf-vocabulary.ddialliance.org/cv/ModeOfCollection/4.0/d50e3728"/>
   </rdf:Description>
   <rdf:Description rdf:about="http://rdf-vocabulary.ddialliance.org/cv/ModeOfCollection/4.0/d50e3548">
      <rdf:type rdf:resource="http://www.w3.org/2004/02/skos/core#Concept"/>
      <skos:inScheme rdf:resource="http://rdf-vocabulary.ddialliance.org/cv/ModeOfCollection/4.0/"/>
      <skos:notation>AutomatedDataExtraction.ApiQuery</skos:notation>
      <skos:prefLabel xml:lang="en">Automated data extraction: API query</skos:prefLabel>
      <skos:definition xml:lang="en">Retrieving information from online data sources through an API (application programming interface) to save it to a local file or database for further processing or storage.</skos:definition>
      <skos:prefLabel xml:lang="de">Automatisierte Datenextraktion: API-Abfrage</skos:prefLabel>
      <skos:definition xml:lang="de">Abrufen von Informationen aus Online-Datenquellen über eine API (Application Programming Interface), um sie in einer lokalen Datei oder Datenbank zur weiteren Verarbeitung oder Speicherung zu speichern.</skos:definition>
      <skos:prefLabel xml:lang="fi">Automatisoitu tiedonpoiminta: API-rajapintakysely</skos:prefLabel>
      <skos:definition xml:lang="fi">Tiedonpoiminta verkkolähteistä ohjelmointirajapinnan (API: application programming interface) avulla. Poimittu tieto tallennetaan tiedostoon tai tietokantaan myöhempää käsittelyä tai säilytystä varten.</skos:definition>
      <skos:prefLabel xml:lang="fi">Automatisoitu tiedonpoiminta: API-rajapintakysely</skos:prefLabel>
      <skos:definition xml:lang="fi">Tiedonpoiminta verkkolähteistä ohjelmointirajapinnan (API: application programming interface) avulla. Poimittu tieto tallennetaan tiedostoon tai tietokantaan myöhempää käsittelyä tai säilytystä varten.</skos:definition>
      <skos:prefLabel xml:lang="it">Estrazione automatizzata: interrogazione API</skos:prefLabel>
      <skos:definition xml:lang="it">Recupero di informazioni da fonti di dati online attraverso una API (Application Programming Interface) per salvarle in un file locale o in un database per una successiva elaborazione o archiviazione.</skos:definition>
      <skos:prefLabel xml:lang="ja">自動データ抽出：APIクエリ</skos:prefLabel>
      <skos:definition xml:lang="ja">API（アプリケーションプログラミングインターフェイス）を介してオンライン上のデータソースから情報を検索し、取得した情報をローカルファイルまたはデータベースに保存する。その後さらにデータの処理と保管が行われる。</skos:definition>
      <skos:prefLabel xml:lang="lt">Automatinė duomenų gavyba: API užklausa</skos:prefLabel>
      <skos:definition xml:lang="lt">Informacijos nuskaitymas iš internetinių duomenų šaltinių, naudojant API (programinės įrangos sąsają) ir išsaugant ją vidiniame faile ar duomenų bazėje tolesniam apdorojimui ar saugojimui.</skos:definition>
      <skos:prefLabel xml:lang="nl">Geautomatiseerde data-extractie: API zoekvraag</skos:prefLabel>
      <skos:definition xml:lang="nl"/>
      <skos:prefLabel xml:lang="no">Automatisert datautvinning: API spørring</skos:prefLabel>
      <skos:definition xml:lang="no">Å hente informasjon fra datakilder på nett via en API (programmeringsgrensesnitt) for å lagre det på en lokal fil eller database for ytterligere prosessering eller oppbevaring.</skos:definition>
      <skos:prefLabel xml:lang="no">Automatisert datautvinning: API spørring</skos:prefLabel>
      <skos:definition xml:lang="no">Å hente informasjon fra datakilder på nett via en API (programmeringsgrensesnitt) for å lagre det på en lokal fil eller database for ytterligere prosessering eller oppbevaring.</skos:definition>
      <skos:prefLabel xml:lang="pt">Extração de dados automatizada: consulta de API’s</skos:prefLabel>
      <skos:definition xml:lang="pt">Recolha de informações a partir de fontes de dados online através de uma API (Application Programming Interface) para as salvar num ficheiro local ou banco de dados, para posterior processamento ou armazenamento.</skos:definition>
      <skos:prefLabel xml:lang="sl">Avtomatizirano pridobivanje podatkov: iskanje preko API</skos:prefLabel>
      <skos:definition xml:lang="sl">Pridobivanje informacij iz spletnih virov podatkov preko API-ja (vmesnik uporabniškega programa) in njihov prenos v lokalno datoteko ali bazo podatkov za nadaljnjo obdelavo ali shranjevanje.</skos:definition>
      <skos:prefLabel xml:lang="sv">Automatiserad dataextrahering: API-förfrågan</skos:prefLabel>
      <skos:definition xml:lang="sv">Inhämtning av information från datakällor online via ett API (Application Programming Interface) för att spara informationen som en lokal fil eller databas för ytterligare behandling eller lagring.</skos:definition>
      <skos:broader rdf:resource="http://rdf-vocabulary.ddialliance.org/cv/ModeOfCollection/4.0/d50e3451"/>
   </rdf:Description>
   <rdf:Description rdf:about="http://rdf-vocabulary.ddialliance.org/cv/ModeOfCollection/4.0/d50e3638">
      <rdf:type rdf:resource="http://www.w3.org/2004/02/skos/core#Concept"/>
      <skos:inScheme rdf:resource="http://rdf-vocabulary.ddialliance.org/cv/ModeOfCollection/4.0/"/>
      <skos:notation>AutomatedDataExtraction.DatabaseQuery</skos:notation>
      <skos:prefLabel xml:lang="en">Automated data extraction: Database query</skos:prefLabel>
      <skos:definition xml:lang="en">Retrieving information from databases through a query to the database to extract only the information required, saving it to a local file or database for further processing or storage.</skos:definition>
      <skos:prefLabel xml:lang="de">Automatisierte Datenextraktion: Datenbankabfrage</skos:prefLabel>
      <skos:definition xml:lang="de">Abrufen von Informationen aus Datenbanken durch eine Abfrage an die Datenbank, um nur die benötigten Informationen zu extrahieren und sie in einer lokalen Datei oder Datenbank zur weiteren Verarbeitung oder Speicherung zu speichern.</skos:definition>
      <skos:prefLabel xml:lang="fi">Automatisoitu tiedonpoiminta: tietokantakysely</skos:prefLabel>
      <skos:definition xml:lang="fi">Tiedonpoiminta tietokannoista. Tehtyjen kyselyiden avulla tietokannoista poimitaan vain haluttu tieto, joka tallennetaan tiedostoon tai tietokantaan myöhempää käsittelyä tai säilytystä varten.</skos:definition>
      <skos:prefLabel xml:lang="fi">Automatisoitu tiedonpoiminta: tietokantakysely</skos:prefLabel>
      <skos:definition xml:lang="fi">Tiedonpoiminta tietokannoista. Tehtyjen kyselyiden avulla tietokannoista poimitaan vain haluttu tieto, joka tallennetaan tiedostoon tai tietokantaan myöhempää käsittelyä tai säilytystä varten.</skos:definition>
      <skos:prefLabel xml:lang="it">Estrazione automatizzata: interrogazione database</skos:prefLabel>
      <skos:definition xml:lang="it">Recupero di informazioni da un database attraverso una sua interrogazione con lo scopo di estrarre solo le informazioni necessarie, salvandole in un file locale o in un database per una successiva elaborazione o archiviazione.</skos:definition>
      <skos:prefLabel xml:lang="ja">自動データ抽出：データベースクエリ</skos:prefLabel>
      <skos:definition xml:lang="ja">必要な情報のみを抽出するためにデータベースへのクエリを介して情報を検索し、取得した情報をローカルファイルまたはデータベースに保存する。その後さらにデータの処理と保管が行われる。</skos:definition>
      <skos:prefLabel xml:lang="lt">Automatinė duomenų gavyba: duomenų bazės užklausa</skos:prefLabel>
      <skos:definition xml:lang="lt">Informacijos nuskaitymas iš duomenų bazių per jų užklausas, siekiant išgauti tik reikalingą informaciją ir išsaugoti ją vidiniame faile ar duomenų bazėje tolesniam apdorojimui ar saugojimui.</skos:definition>
      <skos:prefLabel xml:lang="nl">Geautomatiseerde data-extractie: Database zoekvraag</skos:prefLabel>
      <skos:definition xml:lang="nl"/>
      <skos:prefLabel xml:lang="no">Automatisert datautvinning: Databasespørring</skos:prefLabel>
      <skos:definition xml:lang="no">Å hente informasjon fra databaser via en spørring til databasen som tar ut kun den informasjonen som er nødvendig for å lagre det på en lokal fil eller database for ytterligere prosessering eller oppbevaring.</skos:definition>
      <skos:prefLabel xml:lang="no">Automatisert datautvinning: Databasespørring</skos:prefLabel>
      <skos:definition xml:lang="no">Å hente informasjon fra databaser via en spørring til databasen som tar ut kun den informasjonen som er nødvendig for å lagre det på en lokal fil eller database for ytterligere prosessering eller oppbevaring.</skos:definition>
      <skos:prefLabel xml:lang="pt">Extração de dados automatizada: consulta de bases de dados</skos:prefLabel>
      <skos:definition xml:lang="pt">Recolha de informações a partir de bases de dados através duma consulta da base de dados para extrair apenas as informações necessárias, salvando-as num ficheiro local ou banco de dados, para posterior processamento ou armazenamento.</skos:definition>
      <skos:prefLabel xml:lang="sl">Avtomatizirano pridobivanje podatkov: iskanje po zbirki podatkov</skos:prefLabel>
      <skos:definition xml:lang="sl">Pridobivanje informacij iz zbirke podatkov s pomočjo poizvedbe v zbirko podatkov, da se pridobijo samo zahtevane informacije, in njihov prenos v lokalno datoteko ali bazo podatkov za nadaljnjo obdelavo ali shranjevanje.</skos:definition>
      <skos:prefLabel xml:lang="sv">Automatiserad dataextrahering: databasförfrågan</skos:prefLabel>
      <skos:definition xml:lang="sv">Inhämtning av information från databaser via en förfrågan till databasen om att extrahera enbart den önskade informationen och sedan spara den som en lokal fil eller databas för ytterligare behandling eller lagring.</skos:definition>
      <skos:broader rdf:resource="http://rdf-vocabulary.ddialliance.org/cv/ModeOfCollection/4.0/d50e3451"/>
   </rdf:Description>
   <rdf:Description rdf:about="http://rdf-vocabulary.ddialliance.org/cv/ModeOfCollection/4.0/d50e3728">
      <rdf:type rdf:resource="http://www.w3.org/2004/02/skos/core#Concept"/>
      <skos:inScheme rdf:resource="http://rdf-vocabulary.ddialliance.org/cv/ModeOfCollection/4.0/"/>
      <skos:notation>AutomatedDataExtraction.WebScraping</skos:notation>
      <skos:prefLabel xml:lang="en">Automated data extraction: Web scraping</skos:prefLabel>
      <skos:definition xml:lang="en">A technique employed to extract large amounts of data from websites and save it to a local file or database for further processing or storage. Also called screen scraping, web data extraction, web harvesting, etc.</skos:definition>
      <skos:prefLabel xml:lang="de">Automatisierte Datenextraktion: Web Scraping</skos:prefLabel>
      <skos:definition xml:lang="de">Eine Technik, die verwendet wird, um große Datenmengen aus Websites zu extrahieren und sie in einer lokalen Datei oder Datenbank zur weiteren Verarbeitung oder Speicherung zu speichern. Auch Screen Scraping, Webdatenextraktion, Web Harvesting usw. genannt.</skos:definition>
      <skos:prefLabel xml:lang="fi">Automatisoitu tiedonpoiminta: verkkoharavointi</skos:prefLabel>
      <skos:definition xml:lang="fi">Menetelmä suurien tietomäärien haravoimiseksi verkkosivuilta. Sisältää mm. ruutukaappaukset, kuvakaappaukset ja verkkosivujen tiedonharavoinnin. Haravoitu tieto tallennetaan tiedostoon tai tietokantaan myöhempää käsittelyä tai säilytystä varten.</skos:definition>
      <skos:prefLabel xml:lang="fi">Automatisoitu tiedonpoiminta: verkkoharavointi</skos:prefLabel>
      <skos:definition xml:lang="fi">Menetelmä suurien tietomäärien haravoimiseksi verkkosivuilta. Sisältää mm. ruutukaappaukset, kuvakaappaukset ja verkkosivujen tiedonharavoinnin. Haravoitu tieto tallennetaan tiedostoon tai tietokantaan myöhempää käsittelyä tai säilytystä varten.</skos:definition>
      <skos:prefLabel xml:lang="it">Estrazione automatizzata: web scraping</skos:prefLabel>
      <skos:definition xml:lang="it">Tecnica utilizzata per estrarre grandi quantità di dati da siti web e salvarli in un file locale o in un database per una successiva elaborazione o archiviazione. Chiamato anche screen scraping, estrazione di dati web, web harvesting, ecc.</skos:definition>
      <skos:prefLabel xml:lang="ja">自動データ抽出：Webスクレイピング</skos:prefLabel>
      <skos:definition xml:lang="ja">Webサイトから大量のデータを抽出し、取得した情報をローカルファイルまたはデータベースに保存するために用いられる技術。その後さらにデータの処理と保管が行われる。スクリーンスクレイピング、Webデータ抽出、Webハーベスティングなどとも呼ばれる。</skos:definition>
      <skos:prefLabel xml:lang="lt">Automatinė duomenų gavyba: žiniatinklio puslapių nuskaitymas</skos:prefLabel>
      <skos:definition xml:lang="lt">Technika naudojama siekiant iš žiniatinklio nuskaityti didelius duomenų kiekius ir išsaugoti juos vidiniame faile ar duomenų bazėje tolesniam apdorojimui ar saugojimui. Taip pat vadinama ekrano duomenų nuskaitymu, žiniatinklio duomenų gavyba ar kt.</skos:definition>
      <skos:prefLabel xml:lang="nl">Geautomatiseerde data-extractie: Web scrapen</skos:prefLabel>
      <skos:definition xml:lang="nl"/>
      <skos:prefLabel xml:lang="no">Automatisert datautvinning: Nettskraping</skos:prefLabel>
      <skos:definition xml:lang="no">En teknikk som anvendes for å hente ut store mengder data fra nettsider og lagre det på en lokal fil eller database for ytterligere prosessering eller oppbevaring. Også kalt skjermskraping, utvinning av nettdata, netthøsting, etc.</skos:definition>
      <skos:prefLabel xml:lang="no">Automatisert datautvinning: Nettskraping</skos:prefLabel>
      <skos:definition xml:lang="no">En teknikk som anvendes for å hente ut store mengder data fra nettsider og lagre det på en lokal fil eller database for ytterligere prosessering eller oppbevaring. Også kalt skjermskraping, utvinning av nettdata, netthøsting, etc.</skos:definition>
      <skos:prefLabel xml:lang="pt">Extração de dados automatizada: recolha de dados via web ou “raspagem web”</skos:prefLabel>
      <skos:definition xml:lang="pt">Técnica usada para extrair grandes quantidades de dados a partir de sites e salvá-los num ficheiro local ou banco de dados, para posterior processamento ou armazenamento. Também designada “raspagem de tela”, extração de dados da web, “raspagem web”, etc.</skos:definition>
      <skos:prefLabel xml:lang="sl">Avtomatizirano pridobivanje podatkov: strganje zaslona</skos:prefLabel>
      <skos:definition xml:lang="sl">Tehnika, ki se uporablja za pridobivanje velikih količin podatkov s spletnih mest. Pridobljeni podatki se prenesejo v lokalno datoteko ali bazo podatkov za nadaljnjo obdelavo ali shranjevanje. Imenuje se tudi luščenje podatkov, pridobivanje spletnih podatkov, zbiranje spletnih strani itd.</skos:definition>
      <skos:prefLabel xml:lang="sv">Automatiserad dataextrahering: webbskrapning</skos:prefLabel>
      <skos:definition xml:lang="sv">En teknik som används för att extrahera stora mängder data från webbplatser och spara dem som en lokal fil eller databas för ytterligare behandling eller lagring. Tekniken kallas även för web scraping, skärmskrapning (screen scraping), webbskördning m.m.</skos:definition>
      <skos:broader rdf:resource="http://rdf-vocabulary.ddialliance.org/cv/ModeOfCollection/4.0/d50e3451"/>
   </rdf:Description>
   <rdf:Description rdf:about="http://rdf-vocabulary.ddialliance.org/cv/ModeOfCollection/4.0/d50e3819">
      <rdf:type rdf:resource="http://www.w3.org/2004/02/skos/core#Concept"/>
      <skos:inScheme rdf:resource="http://rdf-vocabulary.ddialliance.org/cv/ModeOfCollection/4.0/"/>
      <skos:notation>ContentCoding</skos:notation>
      <skos:prefLabel xml:lang="en">Content coding</skos:prefLabel>
      <skos:definition xml:lang="en">As a mode of secondary data collection, content coding applies coding techniques to transform qualitative data (textual, video, audio or still-image) originally produced for other purposes into quantitative data (expressed in unit-by-variable matrices) in accordance with pre-defined categorization schemes. For example, coded party manifesto data like the "European Parliament Election Study 2009, Manifesto Study" (doi:10.4232/1.10204).</skos:definition>
      <skos:prefLabel xml:lang="de">Inhaltsanalyse</skos:prefLabel>
      <skos:definition xml:lang="de">Als eine Form der sekundären Datenerhebung wendet die Inhaltsanalyse Kodierungstechniken an, um qualitative Daten (Text-, Video-, Audio- oder Standbilddaten), die ursprünglich für andere Zwecke produziert wurden, mithilfe von vordefinierten Kategorisierungsschemata in quantitative Daten zu transformieren. Zum Beispiel die Kodierung von Parteiprogrammen.</skos:definition>
      <skos:prefLabel xml:lang="fi">Sisällönkoodaus</skos:prefLabel>
      <skos:definition xml:lang="fi">Jo olemassa olevasta, alun perin toisiin tarkoituksiin luodusta kvalitatiivisesta aineistosta (esim. tekstiaineistot, ääni- ja kuvatiedostot, valokuvat) muodostetaan kvantitatiivinen aineisto (matriisi) sovittua koodausohjetta käyttäen. Esimerkki: sanomalehtiartikkeleiden sisällön luokittelu annettujen kriteerien mukaan.</skos:definition>
      <skos:prefLabel xml:lang="fi">Sisällönkoodaus</skos:prefLabel>
      <skos:definition xml:lang="fi">Jo olemassa olevasta, alun perin toisiin tarkoituksiin luodusta kvalitatiivisesta aineistosta (esim. tekstiaineistot, ääni- ja kuvatiedostot, valokuvat) muodostetaan kvantitatiivinen aineisto (matriisi) sovittua koodausohjetta käyttäen. Esimerkki: sanomalehtiartikkeleiden sisällön luokittelu annettujen kriteerien mukaan.</skos:definition>
      <skos:prefLabel xml:lang="it">Codifica del contenuto</skos:prefLabel>
      <skos:definition xml:lang="it">Metodo di raccolta secondaria dei dati, in cui si applicano le tecniche di codifica del contenuto per trasformare dati qualitativi originariamente prodotti per altri scopi (testi, video, audio o immagini) in dati quantitativi (espressi in forma di matrici) secondo schemi di categorizzazione definiti. Ad esempio, codifica dei dati relativi ai manifesti di partito, come il "European Parliament Election Study 2009, Manifesto Study" (doi:10.4232/1.10204)</skos:definition>
      <skos:prefLabel xml:lang="ja">内容コーディング</skos:prefLabel>
      <skos:definition xml:lang="ja">二次的なデータ収集手段として、内容コーディングはあらかじめ定義済の分類基準に従い、本来他の目的のために作られた定性的データ(文字、映像、音声、静止画)を定量的データ(変数単位のマトリックスで表現)に変換するためにコーディング手法を適用する。例えば、"European Parliament Election Study 2009, Manifesto Study" (doi:10.4232/1.10204)"のような、分類（コーディング）された政党マニフェストデータがそれに当たる。</skos:definition>
      <skos:prefLabel xml:lang="lt">Turinio kodavimas</skos:prefLabel>
      <skos:definition xml:lang="lt">Turinio kodavimas yra toks antrinių duomenų rinkimo būdas, kuriame kitais tikslais sukurti kokybiniai duomenys (tekstiniai, video, garso ar statinių vaizdų) transformuojami į kiekybinius duomenis (išreikštus kintamųjų-atvejų matricomis), koduojant pagal išankstines kategorijų schemas. Pavyzdžiui, partijų manifestų kodavimo duomenys tokie kaip "European Parliament Election Study 2009, Manifesto Study" (doi:10.4232/1.10204).</skos:definition>
      <skos:prefLabel xml:lang="nl">Content coding</skos:prefLabel>
      <skos:definition xml:lang="nl"/>
      <skos:prefLabel xml:lang="no">Innholdskoding</skos:prefLabel>
      <skos:definition xml:lang="no">Som metode for sekundær datainnsamling, innholdskoding omfatter kodeteknikker for å omgjøre kvalitative data (tekst, video, lyd eller bilde), som opprinnelig var utarbeidet for andre formål, til kvantitative data (uttrykket i en matrise med enheter og variabler) i henhold til bestemte kategoriseringssystem. For eksempel, kodede partimanifesto som i 'European Parliament Election Study 2009, Manifesto Study' (doi:10.4232/1.10204).</skos:definition>
      <skos:prefLabel xml:lang="no">Innholdskoding</skos:prefLabel>
      <skos:definition xml:lang="no">Som metode for sekundær datainnsamling, innholdskoding omfatter kodeteknikker for å omgjøre kvalitative data (tekst, video, lyd eller bilde), som opprinnelig var utarbeidet for andre formål, til kvantitative data (uttrykket i en matrise med enheter og variabler) i henhold til bestemte kategoriseringssystem. For eksempel, kodede partimanifesto som i 'European Parliament Election Study 2009, Manifesto Study' (doi:10.4232/1.10204).</skos:definition>
      <skos:prefLabel xml:lang="pt">Codificação de conteúdo</skos:prefLabel>
      <skos:definition xml:lang="pt">Como modo de recolha de dados secundários, a codificação de conteúdo aplica técnicas de codificação para transformar dados qualitativos (textual, vídeo, áudio ou imagem parada) originalmente produzidos para outros propósitos em dados quantitativos (expressos em matrizes unidade-por-variável) de acordo com esquemas de categorização predefinidos. Por exemplo, dados codificados de um programa de partido político, como o "European Parliament Election Study 2009, Manifesto Study" (doi:10.4232/1.10204).</skos:definition>
      <skos:prefLabel xml:lang="sl">Kodiranje vsebine</skos:prefLabel>
      <skos:definition xml:lang="sl">Kot način sekundarnega zbiranja podatkov, kodiranje vsebine uporablja kodirne tehnike za preoblikovanje kvalitativnih podatkov (besedilni podatki, video, avdio ali mirujoče slike), ki so bili prvotno ustvarjeni za druge namene, v kvantitativne podatke (izražene z matricami enot po spremenljivkah) v skladu s vnaprej opredeljenimi kategorizacijskimi shemami. Na primer, kodiranje manifestov političnih strank, kot npr. študija o volitvah v Evropski parlament 2009 (doi:10.4232/1.10204).</skos:definition>
      <skos:prefLabel xml:lang="sv">Kodning av innehåll</skos:prefLabel>
      <skos:definition xml:lang="sv">Som en metod för sekundär datainsamling tillämpar innehållskodning  kodningstekniker för att omvandla kvalitativa data (text-, ljud-, video-, eller stillbildsdata) som ursprungligen skapats för andra syften till kvantitativa data (uttryckta i en matris med enheter och variabler) enligt fördefinierade kategoriseringsscheman. Exempel: kodade partiprogramsdata som i "European Parliament Election Study 2009, Manifesto Study" (DOI: 10.4232/1.10204).</skos:definition>
   </rdf:Description>
   <rdf:Description rdf:about="http://rdf-vocabulary.ddialliance.org/cv/ModeOfCollection/4.0/d50e3909">
      <rdf:type rdf:resource="http://www.w3.org/2004/02/skos/core#Concept"/>
      <skos:inScheme rdf:resource="http://rdf-vocabulary.ddialliance.org/cv/ModeOfCollection/4.0/"/>
      <skos:notation>Transcription</skos:notation>
      <skos:prefLabel xml:lang="en">Transcription</skos:prefLabel>
      <skos:definition xml:lang="en">Capturing information in writing from a different source, or from a different medium, alphabet, or form of notation, like scientific formulae, or musical notes. For transcribed interviews or observations, it is recommended to document the primary mode of collection, using one of the interview or observation terms.</skos:definition>
      <skos:prefLabel xml:lang="de">Transkription</skos:prefLabel>
      <skos:definition xml:lang="de">Das schriftliche Erfassen von Informationen aus einer anderen Quelle oder aus einem anderen Medium, Alphabet oder einer anderen Notationsform, wie z. B. wissenschaftliche Formeln oder Musiknoten. Bei transkribierten Interviews oder Beobachtungen wird empfohlen, die primäre Methode der Datenerhebung zu dokumentieren, indem einer der Interview- oder Beobachtungsbegriffe verwendet wird.</skos:definition>
      <skos:prefLabel xml:lang="fi">Litterointi</skos:prefLabel>
      <skos:definition xml:lang="fi">Informaation siirtäminen käsin kirjaamalla toisesta lähteestä tai toisesta formaatista, muodosta tai aakkosjärjestelmästä. Esimerkki: Musiikin esittäminen nuotteina, kemialliset kaavat. Jos aineisto muodostuu havaintomuistiinpanoista tai haastattelulitteroinneista, suositellaan kuvattavaksi ensisijainen keruumenetelmä käyttämällä sopivaa havainnointi- tai haastattelutermiä.</skos:definition>
      <skos:prefLabel xml:lang="fi">Litterointi</skos:prefLabel>
      <skos:definition xml:lang="fi">Informaation siirtäminen käsin kirjaamalla toisesta lähteestä tai toisesta formaatista, muodosta tai aakkosjärjestelmästä. Esimerkki: Musiikin esittäminen nuotteina, kemialliset kaavat. Jos aineisto muodostuu havaintomuistiinpanoista tai haastattelulitteroinneista, suositellaan kuvattavaksi ensisijainen keruumenetelmä käyttämällä sopivaa havainnointi- tai haastattelutermiä.</skos:definition>
      <skos:prefLabel xml:lang="it">Trascrizione</skos:prefLabel>
      <skos:definition xml:lang="it">Raccolta di informazioni per iscritto da un'altra fonte, o da un altro mezzo, alfabeto o forma di notazione, come formule scientifiche o note musicali. Per le interviste o le osservazioni trascritte, si consiglia di documentare la modalità di raccolta dei dati utilizzando uno dei termini del vocabolario relativi all'intervista o all'osservazione.</skos:definition>
      <skos:prefLabel xml:lang="ja">トランスクリプション</skos:prefLabel>
      <skos:definition xml:lang="ja">科学の公式や楽譜等、別の情報源、別の媒体、文字、表記方法から情報を取得し文字に起こす方法。インタビューや観察結果の書き起こしについては、インタビュー法や観察法の用語を使い、主なデータ収集方法について記録を残すことが推奨される。</skos:definition>
      <skos:prefLabel xml:lang="lt">Transkripcija </skos:prefLabel>
      <skos:definition xml:lang="lt">Informacijos fiksavimas perrašant iš kitokio tipo šaltinių ar medijų, iš kitų alfabetų ar žymėjimo formų, pavyzdžiui, mokslinių formulių ar muzikos natų. Transkribuotus interviu ar stebėjimus (stebėjimo užrašus) rekomenduojama dokumentuoti pagal pirminį duomenų rinkimo būdą, naudojant atitinkamai interviu arba stebėjimo terminus.</skos:definition>
      <skos:prefLabel xml:lang="nl">Transcriptie</skos:prefLabel>
      <skos:definition xml:lang="nl"/>
      <skos:prefLabel xml:lang="no">Transkripsjon</skos:prefLabel>
      <skos:definition xml:lang="no">Nedtegning av informasjon i skrift fra en annen kilde, eller et annet medium, alfabet, eller fra notasjoner, som vitenskapelige formler, eller musikknoter. For transkriberte intervju eller observasjoner er det anbefalt å dokumentere den opprinnelige formen for datainnsamling, ved å bruke et av intervju- eller observasjonsbegrepene.</skos:definition>
      <skos:prefLabel xml:lang="no">Transkripsjon</skos:prefLabel>
      <skos:definition xml:lang="no">Nedtegning av informasjon i skrift fra en annen kilde, eller et annet medium, alfabet, eller fra notasjoner, som vitenskapelige formler, eller musikknoter. For transkriberte intervju eller observasjoner er det anbefalt å dokumentere den opprinnelige formen for datainnsamling, ved å bruke et av intervju- eller observasjonsbegrepene.</skos:definition>
      <skos:prefLabel xml:lang="pt">Transcrição</skos:prefLabel>
      <skos:definition xml:lang="pt">Recolha de informações por escrito de uma fonte diferente ou através de um meio diferente, alfabeto ou forma de anotação, como fórmulas científicas ou notas musicais. Para entrevistas ou observações transcritas, recomenda-se documentar o modo de recolha principal, usando um dos termos no âmbito dos tópicos mais gerais 'entrevista' ou 'observação'.</skos:definition>
      <skos:prefLabel xml:lang="sl">Prepis</skos:prefLabel>
      <skos:definition xml:lang="sl">Zajemanje podatkov v pisni obliki iz drugega vira ali iz drugega medija, abecede, ali oblika zapisa, kot so znanstvene formule ali glasbene note. Pri transkriptih intervjujev ali opazovanj je priporočljivo dokumentirati primarni način zbiranja podatkov z uporabo enega od razgovornih ali opazovalnih pogojev.</skos:definition>
      <skos:prefLabel xml:lang="sv">Transkription</skos:prefLabel>
      <skos:definition xml:lang="sv">Att nedteckna information från en annan källa eller från ett annat medium, alfabet eller notationssystem, som till exempel vetenskapliga formler eller noter för musik. För transkriberade intervjuer och observationer rekommenderas det att man dokumenterar den primära insamlingsmetoden med någon av termerna för intervjuer eller observationer.</skos:definition>
   </rdf:Description>
   <rdf:Description rdf:about="http://rdf-vocabulary.ddialliance.org/cv/ModeOfCollection/4.0/d50e3999">
      <rdf:type rdf:resource="http://www.w3.org/2004/02/skos/core#Concept"/>
      <skos:inScheme rdf:resource="http://rdf-vocabulary.ddialliance.org/cv/ModeOfCollection/4.0/"/>
      <skos:notation>CompilationSynthesis</skos:notation>
      <skos:prefLabel xml:lang="en">Compilation/Synthesis</skos:prefLabel>
      <skos:definition xml:lang="en">Collecting and assembling data from multiple, often heterogeneous sources that have one or more reference points in common, and at least one of the sources was originally produced for other purposes. The data are incorporated in a new entity. For example, providing data on the number of universities in the last 150 years using a variety of available sources (e.g. finance documents, official statistics, university registers), combining survey data with information about geographical areas from official statistics (e.g. population density, doctors per capita, etc.), or with social media data, etc.</skos:definition>
      <skos:prefLabel xml:lang="de">Kompilation/Synthese</skos:prefLabel>
      <skos:definition xml:lang="de">Sammeln und Zusammenstellen von Daten aus mehreren, oft heterogenen Quellen, die einen oder mehrere Bezugspunkte gemeinsam haben, wobei mindestens eine der Quellen ursprünglich für andere Zwecke erstellt wurde. Die Daten werden in eine neue Einheit integriert. Zum Beispiel die Bereitstellung von Daten über die Anzahl der Universitäten in den letzten 150 Jahren unter Verwendung einer Vielzahl verfügbarer Quellen (z. B. Finanzdokumente, amtliche Statistiken, Universitätsregister), die Kombination von Umfragedaten mit Informationen über geografische Gebiete aus amtlichen Statistiken (z. B. Bevölkerungsdichte, Ärzte pro Kopf usw.) oder mit Daten aus sozialen Medien usw.</skos:definition>
      <skos:prefLabel xml:lang="fi">Kooste- tai synteesiaineisto</skos:prefLabel>
      <skos:definition xml:lang="fi">Tietojen kerääminen ja kokoaminen useista, usein heterogeenisistä lähdemateriaaleista, joilla yksi tai useampi yhteinen referenssi. Ainakin yksi lähteistä on olemassa valmiina jo ennestään muita tarkoituksia varten. Kerätyt tiedot yhdistetään uudeksi tutkimusaineistoksi. Esimerkkejä: Tiedon kerääminen suomalaisten yliopistojen historiasta käyttämällä monia eri lähteitä, tai kyselytutkimuksen tietojen yhdistäminen muista tietolähteistä saatuihin tietoihin.</skos:definition>
      <skos:prefLabel xml:lang="fi">Kooste- tai synteesiaineisto</skos:prefLabel>
      <skos:definition xml:lang="fi">Tietojen kerääminen ja kokoaminen useista, usein heterogeenisistä lähdemateriaaleista, joilla yksi tai useampi yhteinen referenssi. Ainakin yksi lähteistä on olemassa valmiina jo ennestään muita tarkoituksia varten. Kerätyt tiedot yhdistetään uudeksi tutkimusaineistoksi. Esimerkkejä: Tiedon kerääminen suomalaisten yliopistojen historiasta käyttämällä monia eri lähteitä, tai kyselytutkimuksen tietojen yhdistäminen muista tietolähteistä saatuihin tietoihin.</skos:definition>
      <skos:prefLabel xml:lang="it">Raccolta/sintesi</skos:prefLabel>
      <skos:definition xml:lang="it">Raccolta e assemblaggio di dati da più fonti, spesso eterogenee, che hanno uno o più punti di riferimento in comune, e dove almeno una delle fonti è stata originariamente prodotta per altri scopi. I dati sono incorporati in una nuova base di dati. Ad esempio, la raccolta di dati sul numero di università negli ultimi 150 anni attraverso diverse fonti disponibili (ad esempio documenti finanziari, statistiche ufficiali, registri universitari), successivamente combinati con le statistiche ufficiali relative alle aree geografiche (ad es. densità di popolazione, medici pro-capite, ecc.) o con dati provenienti dai social media, ecc.</skos:definition>
      <skos:prefLabel xml:lang="ja">編集／統合</skos:prefLabel>
      <skos:definition xml:lang="ja">複数の情報源、たいてい少なくとも1つの点を共有した多様な情報源からデータを収集し、整理すること。少なくとも1つの情報源は他の目的のために作成されたものである。集めたデータを統合することで、新しく統一的な情報が生みだされる。例えば、様々な入手可能な情報源（例えば会計書類、公的統計、大学の登録簿）を使って過去150年間の大学に関するデータを提供すること、調査データと公的統計から得られる地域情報の連結（例えば、人口密度、千人あたり医師の数等）、あるいは、ソーシャル・メディアのデータを集めること等があげられる。</skos:definition>
      <skos:prefLabel xml:lang="lt">Kompiliacija ar sintezė</skos:prefLabel>
      <skos:definition xml:lang="lt">Duomenų rinkimas ir integravimas iš kelių skirtingų šaltinių, kuriuos jungia viena ar kelios bendros charakteristikos, o bent vienas iš šaltinių buvo kurtas kitiems tikslams. Duomenys integruojami naujame objekte. Pavyzdžiui, teikiant duomenis apie universitetų skaičių už praėjusius 150 metų, naudojami įvairūs prieinami šaltiniai (pavyzdžiui, finansiniai dokumentai, oficiali statistika, universitetų registrai); apklausų duomenys jungiami su oficialia statistine informacijos apie geografines vietoves (pavyzdžiui, gyventojų tankis, mokslo daktarų skaičius vienam gyventojui ir kt.); arba su socialinių medijų duomenimis ir kt.</skos:definition>
      <skos:prefLabel xml:lang="nl">Compilatie/Synthese</skos:prefLabel>
      <skos:definition xml:lang="nl"/>
      <skos:prefLabel xml:lang="no">Kompilering/Syntese</skos:prefLabel>
      <skos:definition xml:lang="no">Innsamling og sammensetting av data fra flere, ofte heterogene, kilder som har en eller flere felles referansepunkter, og minst én av kildene var opprinnelig utarbeidet for andre formål. Dataene blir integrert i en ny enhet. For eksempel utarbeide data om antallet universitet de siste 150 årene ved å bruke flere tilgjengelige kilder (e.g. finansdokumenter, offisiell statistikk, universitetsregistre), kombinere spørreundersøkelsesdata med informasjon om geografiske områder fra offisiell statistikk (e.g. befolkningstetthet, antall leger per innbygger, etc.), eller bruke RSS for å samle blogginnlegg eller tweets etc.</skos:definition>
      <skos:prefLabel xml:lang="no">Kompilering/Syntese</skos:prefLabel>
      <skos:definition xml:lang="no">Innsamling og sammensetting av data fra flere, ofte heterogene, kilder som har en eller flere felles referansepunkter, og minst én av kildene var opprinnelig utarbeidet for andre formål. Dataene blir integrert i en ny enhet. For eksempel utarbeide data om antallet universitet de siste 150 årene ved å bruke flere tilgjengelige kilder (e.g. finansdokumenter, offisiell statistikk, universitetsregistre), kombinere spørreundersøkelsesdata med informasjon om geografiske områder fra offisiell statistikk (e.g. befolkningstetthet, antall leger per innbygger, etc.), eller bruke RSS for å samle blogginnlegg eller tweets etc.</skos:definition>
      <skos:prefLabel xml:lang="pt">Compilação/síntese</skos:prefLabel>
      <skos:definition xml:lang="pt">Recolha e compilação de dados de fontes múltiplas, muitas vezes heterogéneas, que possuem um ou mais pontos de referência em comum, e pelo menos uma das fontes foi originalmente produzida para outras finalidades. Os dados são incorporados numa nova entidade. Por exemplo, providenciar dados sobre o número de universidades nos últimos 150 anos usando uma variedade de fontes disponíveis (por exemplo, documentos financeiros, estatísticas oficiais, registos universitários), combinando dados de inquéritos com informações sobre áreas geográficas a partir de estatísticas oficiais (por exemplo, densidade populacional, médicos per capita, etc.), ou com dados dos media sociais, etc.</skos:definition>
      <skos:prefLabel xml:lang="sl">Kompilacija/sinteza</skos:prefLabel>
      <skos:definition xml:lang="sl">Zbiranje in sestavljanje podatkov iz več, pogosto heterogenih virov, ki imajo eno ali več skupnih referenčnih točk in kjer je bil vsaj eden od virov prvotno produciran v druge namene. Podatki so vključeni v novo entiteto. Na primer z zagotavljanjem podatkov o številu univerz v zadnjih 150 letih z uporabo različnih razpoložljivih virov (npr. finančni dokumenti, uradne statistike, univerzitetni registri), kombiniranjem anketnih podatkov z informacijami o geografskih območjih iz uradnih statističnih podatkov (npr. gostota prebivalstva, število zdravnikov na prebivalca itd.) ali z uporabo RSS za zbiranje objav bloga ali tvitov itd.</skos:definition>
      <skos:prefLabel xml:lang="sv">Kompilering/Syntes</skos:prefLabel>
      <skos:definition xml:lang="sv">Att samla in och sammanställa data från flera, ofta heterogena, källor som har en eller flera gemensamma referenspunkter, och där minst en av källorna ursprungligen producerades för andra syften. Datamaterialet har införlivats i ett nytt material. Exempel: data om antalet universitet under de senaste 150 åren som tas fram med hjälp av ett antal olika källor (t.ex. räkenskaper, offentlig statistik och universitetsrullor); en kombination av surveydata med information om geografiska områden från offentlig statistik (t.ex. befolkningstäthet, läkare per capita osv); eller bloggposter, tweetar, m.m. som samlats in med hjälp av RSS.</skos:definition>
   </rdf:Description>
   <rdf:Description rdf:about="http://rdf-vocabulary.ddialliance.org/cv/ModeOfCollection/4.0/d50e4089">
      <rdf:type rdf:resource="http://www.w3.org/2004/02/skos/core#Concept"/>
      <skos:inScheme rdf:resource="http://rdf-vocabulary.ddialliance.org/cv/ModeOfCollection/4.0/"/>
      <skos:notation>Summary</skos:notation>
      <skos:prefLabel xml:lang="en">Summary</skos:prefLabel>
      <skos:definition xml:lang="en">Presentation of information in a condensed form, by reducing it to its main points. For example, abstracts of interviews or reports that are published and used as data rather than the full-length interviews or reports.</skos:definition>
      <skos:prefLabel xml:lang="de">Zusammenfassung</skos:prefLabel>
      <skos:definition xml:lang="de">Darstellung von Informationen in komprimierter Form, indem sie auf die wesentlichen Punkte reduziert werden. Zum Beispiel Zusammenfassungen von Interviews oder Berichten, die veröffentlicht und als Daten verwendet werden, anstatt die Interviews oder Berichte in deren voller Länge.</skos:definition>
      <skos:prefLabel xml:lang="fi">Yhteenveto,  lyhennelmä tai tiivistelmä</skos:prefLabel>
      <skos:definition xml:lang="fi">Tietoa kerätään muodostamalla yhteenveto tai tiivistelmä olennaisista seikoista. Esimerkiksi: Haastatteluista ei tehdä translitteraatioita vaan aineisto muodostuu haastattelujen tiivistelmistä, tai sanomalehtiuutisisten aiheista muodostetaan aineisto tiivistämällä ne pariin lauseeseen. Mikäli kvalitatiivisesta lähdeaineistosta muodostetaan kvantitatiivinen aineisto, käytä termiä 'Sisällönkoodaus'.</skos:definition>
      <skos:prefLabel xml:lang="fi">Yhteenveto,  lyhennelmä tai tiivistelmä</skos:prefLabel>
      <skos:definition xml:lang="fi">Tietoa kerätään muodostamalla yhteenveto tai tiivistelmä olennaisista seikoista. Esimerkiksi: Haastatteluista ei tehdä translitteraatioita vaan aineisto muodostuu haastattelujen tiivistelmistä, tai sanomalehtiuutisisten aiheista muodostetaan aineisto tiivistämällä ne pariin lauseeseen. Mikäli kvalitatiivisesta lähdeaineistosta muodostetaan kvantitatiivinen aineisto, käytä termiä 'Sisällönkoodaus'.</skos:definition>
      <skos:prefLabel xml:lang="it">Sintesi</skos:prefLabel>
      <skos:definition xml:lang="it">Presentazione di informazioni in forma sintetica, riducendole ai punti principali. Ad esempio, abstract di interviste o report che vengono pubblicati e utilizzati come dati, al posto delle interviste o dei report completi.</skos:definition>
      <skos:prefLabel xml:lang="ja">要約</skos:prefLabel>
      <skos:definition xml:lang="ja">要点をまとめることで情報を簡潔に提示すること。例えば、インタビューや報告の全文ではなく、それらの概要をまとめて、発表したりデータに用いたりすること等を指す。</skos:definition>
      <skos:prefLabel xml:lang="lt">Santrauka</skos:prefLabel>
      <skos:definition xml:lang="lt">Informacijos glaustas išdėstymas, ją sutrumpinant iki pagrindinės esmės. Pavyzdžiui, interviu ar ataskaitos santrauka, kuri publikuojama ir naudojama kaip duomenys, vietoje pilnos trukmės interviu ar ataskaitos.</skos:definition>
      <skos:prefLabel xml:lang="nl">Samenvatting</skos:prefLabel>
      <skos:definition xml:lang="nl"/>
      <skos:prefLabel xml:lang="no">Sammendrag</skos:prefLabel>
      <skos:definition xml:lang="no">Presentasjon av informasjon i en konsentrert form, ved å redusere den til dens hovedpoeng. For eksempel, sammendrag av intervjuer eller rapporter som er publisert og brukt som data til fordel for de fulle intervjuene eller rapportene.</skos:definition>
      <skos:prefLabel xml:lang="no">Sammendrag</skos:prefLabel>
      <skos:definition xml:lang="no">Presentasjon av informasjon i en konsentrert form, ved å redusere den til dens hovedpoeng. For eksempel, sammendrag av intervjuer eller rapporter som er publisert og brukt som data til fordel for de fulle intervjuene eller rapportene.</skos:definition>
      <skos:prefLabel xml:lang="pt">Sumário/resumo</skos:prefLabel>
      <skos:definition xml:lang="pt">Apresentação de informação de forma resumida, reduzindo-a aos seus pontos principais. Por exemplo, resumos de entrevistas ou de relatórios que são publicados e usados como dados, em vez de entrevistas ou relatórios completos.</skos:definition>
      <skos:prefLabel xml:lang="sl">Povzetek</skos:prefLabel>
      <skos:definition xml:lang="sl">Predstavitev informacij v zgoščeni obliki z reduciranjem na glavne točke. Na primer, povzetki intervjujev ali poročil, ki so objavljeni in uporabljeni kot podatki in ne kot celoviti intervjuji ali poročila.</skos:definition>
      <skos:prefLabel xml:lang="sv">Sammanfattning</skos:prefLabel>
      <skos:definition xml:lang="sv">Presentation av information i sammandrag, som reducerats till sitt viktigaste innehåll. Exempel: Abstrakt från intervjuer eller rapporter publiceras och används som data istället för de fullständiga intervjuerna eller rapporterna.</skos:definition>
   </rdf:Description>
   <rdf:Description rdf:about="http://rdf-vocabulary.ddialliance.org/cv/ModeOfCollection/4.0/d50e4179">
      <rdf:type rdf:resource="http://www.w3.org/2004/02/skos/core#Concept"/>
      <skos:inScheme rdf:resource="http://rdf-vocabulary.ddialliance.org/cv/ModeOfCollection/4.0/"/>
      <skos:notation>Aggregation</skos:notation>
      <skos:prefLabel xml:lang="en">Aggregation</skos:prefLabel>
      <skos:definition xml:lang="en">Statistics that relate to broad classes, groups, or categories. The data are averaged, totaled, or otherwise derived from individual-level data, and it is no longer possible to distinguish the characteristics of individuals within those classes, groups, or categories. For example, the number and age group of the unemployed in specific geographic regions, or national level statistics on the occurrence of specific offences, originally derived from the statistics of individual police districts.</skos:definition>
      <skos:prefLabel xml:lang="de">Aggregation</skos:prefLabel>
      <skos:definition xml:lang="de">Statistiken, die sich auf breite Klassen, Gruppen oder Kategorien beziehen. Die Daten werden gemittelt, summiert oder auf andere Weise aus Daten auf individueller Ebene abgeleitet, und es ist nicht mehr möglich, die Merkmale von Einzelpersonen innerhalb dieser Klassen, Gruppen oder Kategorien zu unterscheiden. Zum Beispiel die Anzahl und Altersgruppe der Arbeitslosen in bestimmten geografischen Regionen oder Statistiken auf nationaler Ebene über das Auftreten bestimmter Straftaten, die ursprünglich aus den Statistiken einzelner Polizeibezirke abgeleitet wurden.</skos:definition>
      <skos:prefLabel xml:lang="fi">Aggregointi</skos:prefLabel>
      <skos:definition xml:lang="fi">Tilastollinen tieto, jossa yksittäisiä havaintoyksiköitä koskevat tiedot ovat keskiarvoistettu, yhteenlaskettu tai jotenkin muuten yhdistetty laajempaa ryhmää koskevaksi tiedoksi siten, että yksittäisen havaintoyksiköiden tiedot eivät ole enää erotettavissa. Esimerkkejä: Kansallinen rikostilasto, joka yhteenlaskettu yksittäisten poliisipiirien tilastoista, tai kuukausittainen hintaindeksi, joka on keskiarvo yksittäisten hyödykkeiden hinnoista.</skos:definition>
      <skos:prefLabel xml:lang="fi">Aggregointi</skos:prefLabel>
      <skos:definition xml:lang="fi">Tilastollinen tieto, jossa yksittäisiä havaintoyksiköitä koskevat tiedot ovat keskiarvoistettu, yhteenlaskettu tai jotenkin muuten yhdistetty laajempaa ryhmää koskevaksi tiedoksi siten, että yksittäisen havaintoyksiköiden tiedot eivät ole enää erotettavissa. Esimerkkejä: Kansallinen rikostilasto, joka yhteenlaskettu yksittäisten poliisipiirien tilastoista, tai kuukausittainen hintaindeksi, joka on keskiarvo yksittäisten hyödykkeiden hinnoista.</skos:definition>
      <skos:prefLabel xml:lang="it">Aggregazione</skos:prefLabel>
      <skos:definition xml:lang="it">Statistiche relative a classi, gruppi o categorie. I dati rappresentano il valore medio, la somma o altre derivazioni dei dati raccolti a livello individuale, che non consentono più di distinguere le caratteristiche degli individui all'interno di tali classi, gruppi o categorie. Ad esempio, il numero e la fascia di età dei disoccupati in specifiche regioni geografiche, o le statistiche a livello nazionale sul verificarsi di reati specifici, originariamente desunti dalle statistiche dei singoli distretti di polizia.</skos:definition>
      <skos:prefLabel xml:lang="ja">集計</skos:prefLabel>
      <skos:definition xml:lang="ja">広範な分類、集団、あるいは範疇に関する統計。個人レベルのデータから平均、合計等の数値が導出されており、それらの分類、集団あるいは範疇に属する個人の特性を判別することは不可能である。例えば、失業者数とその年齢層に関する特定の地域の統計、各警察管区の統計から導かれた特定の犯罪の発生件数についての全国統計等があげられる。</skos:definition>
      <skos:prefLabel xml:lang="lt">Agregavimas</skos:prefLabel>
      <skos:definition xml:lang="lt">Statistika apie didesnes klases, grupes ar kategorijas. Skaičiuojami duomenų vidurkiai, duomenys susumuojami arba kitaip išvedami iš individualaus lygmens duomenų ir nebėra įmanoma atskirti asmenų charakteristikų tose klasėse, grupėse ar kategorijose. Pavyzdžiui, bedarbių skaičius amžiaus grupėse konkrečiuose geografiniuose regionuose, arba nacionalinio lygmens statistiniai duomenys apie tam tikrus nusikaltimus, išvesti iš atskirų rajonų policijos statistinės informacijos.</skos:definition>
      <skos:prefLabel xml:lang="nl">Aggregatie</skos:prefLabel>
      <skos:definition xml:lang="nl"/>
      <skos:prefLabel xml:lang="no">Aggregering</skos:prefLabel>
      <skos:definition xml:lang="no">Statistikk som relateres til store klasser, grupper eller kategorier. Dataene er tatt gjennomsnittet av, summert, eller på andre måter utvunnet av data på individnivå, og det er ikke lengre mulig å skille mellom egenskapene til individer innad i disse klassene, gruppene eller kategoriene. For eksempel, antallet og aldersgruppen til de arbeidsledige i bestemte regioner, eller statistikk på nasjonalt nivå om forekomsten av bestemte overtredelser, opprinnelig utarbeidet fra statistikk om individuelle politidistrikt.</skos:definition>
      <skos:prefLabel xml:lang="no">Aggregering</skos:prefLabel>
      <skos:definition xml:lang="no">Statistikk som relateres til store klasser, grupper eller kategorier. Dataene er tatt gjennomsnittet av, summert, eller på andre måter utvunnet av data på individnivå, og det er ikke lengre mulig å skille mellom egenskapene til individer innad i disse klassene, gruppene eller kategoriene. For eksempel, antallet og aldersgruppen til de arbeidsledige i bestemte regioner, eller statistikk på nasjonalt nivå om forekomsten av bestemte overtredelser, opprinnelig utarbeidet fra statistikk om individuelle politidistrikt.</skos:definition>
      <skos:prefLabel xml:lang="pt">Agregação</skos:prefLabel>
      <skos:definition xml:lang="pt">Estatísticas relacionadas com classes, grupos ou categorias amplas. Os dados são representados por médias, totais, ou derivados de dados registados a um nível individual, não sendo mais possível distinguir as características dos indivíduos dentro dessas classes, grupos ou categorias. Por exemplo, o número e a faixa etária dos desempregados em regiões geográficas específicas, ou estatísticas de âmbito nacional sobre a ocorrência de crimes específicos, originalmente derivadas das estatísticas policiais de cada distrito.</skos:definition>
      <skos:prefLabel xml:lang="sl">Agregacija</skos:prefLabel>
      <skos:definition xml:lang="sl">Statistike, ki se nanašajo na širše razrede, skupine ali kategorije. Podatki so predstavljeni kot povprečja, vsote ali druge izpeljave, na podlagi katerih ni več možno razlikovati med značilnostmi posameznikov znotraj teh razredov, skupin ali kategorij. Na primer, število in starostna skupina brezposelnih v posebnih geografskih regijah ali nacionalne statistike o pojavu poosameznih kaznivih dejanj, ki so bila prvotno izpeljana iz statističnih podatkov posameznih policijskih okrožij.</skos:definition>
      <skos:prefLabel xml:lang="sv">Aggregation</skos:prefLabel>
      <skos:definition xml:lang="sv">Statistik som rör breda klasser, grupper eller kategorier. Datamaterialet består av genomsnitt, totalsummor eller andra värden som har härletts från data på individnivå, och det går inte längre att utläsa individernas egenskaper inom dessa klasser, grupper eller kategorier. Exempel: antal och ålderskategorier för arbetslösa inom särskilda geografiska områden, eller statistik på nationsnivå över förekomsten av särskilda brott som ursprungligen härletts från statistik från enskilda polisdistrikt.</skos:definition>
   </rdf:Description>
   <rdf:Description rdf:about="http://rdf-vocabulary.ddialliance.org/cv/ModeOfCollection/4.0/d50e4269">
      <rdf:type rdf:resource="http://www.w3.org/2004/02/skos/core#Concept"/>
      <skos:inScheme rdf:resource="http://rdf-vocabulary.ddialliance.org/cv/ModeOfCollection/4.0/"/>
      <skos:notation>Simulation</skos:notation>
      <skos:prefLabel xml:lang="en">Simulation</skos:prefLabel>
      <skos:definition xml:lang="en">Modeling or imitative representation of real-world processes, events, or systems, often using computer programs. For example, a program modeling household consumption responses to indirect tax changes; or a dataset on hypothetical patients and their drug exposure, background conditions, and known adverse events.</skos:definition>
      <skos:prefLabel xml:lang="de">Simulation</skos:prefLabel>
      <skos:definition xml:lang="de">Modellierung oder nachahmende Darstellung von realen Prozessen, Ereignissen oder Systemen, oft unter Verwendung von Computerprogrammen. Zum Beispiel ein Programm, das die Reaktionen des Haushaltskonsums auf Veränderung indirekter Steuern modelliert; oder ein Datensatz über hypothetische Patienten und deren Medikamentenbelastung, Hintergrundbedingungen und bekannte unerwünschte Ereignisse.</skos:definition>
      <skos:prefLabel xml:lang="fi">Simulointi</skos:prefLabel>
      <skos:definition xml:lang="fi">Todellisten prosessien, tapahtumien ja systeemien piirteiden tai mahdollisen muuttumisen tutkiminen mallintamalla, usein tietokoneohjelmia käyttäen.</skos:definition>
      <skos:prefLabel xml:lang="fi">Simulointi</skos:prefLabel>
      <skos:definition xml:lang="fi">Todellisten prosessien, tapahtumien ja systeemien piirteiden tai mahdollisen muuttumisen tutkiminen mallintamalla, usein tietokoneohjelmia käyttäen.</skos:definition>
      <skos:prefLabel xml:lang="it">Simulazione</skos:prefLabel>
      <skos:definition xml:lang="it">Modellazione o rappresentazione finalizzata alla riproduzione di processi, eventi o sistemi reali, spesso utilizzando programmi per computer. Ad esempio, un programma che modella le risposte dei consumi delle famiglie alle variazioni delle imposte indirette; o un dataset relativo a pazienti ipotetici e alla loro esposizione a farmaci, alle condizioni di fondo e ad eventi avversi conosciuti.</skos:definition>
      <skos:prefLabel xml:lang="ja">シミュレーション</skos:prefLabel>
      <skos:definition xml:lang="ja">主にコンピュータプログラムを使い、現実世界のプロセス、イベント、システムのモデルを構築する、あるいは模倣すること。例えば、間接税の税率変更に伴い家計の消費がどう変わるのかをモデル化するプログラムや、仮想の患者と彼らの薬物服用、背景条件、既知の有害作用に関するデータセット等があげられる。</skos:definition>
      <skos:prefLabel xml:lang="lt">Simuliavimas</skos:prefLabel>
      <skos:definition xml:lang="lt">Realaus pasaulio procesų, įvykių ar sistemų modeliavimas arba imitavimas, dažniausiai naudojant kompiuterines programas. Pavyzdžiui, programa modeliuojanti netiesioginių mokesčių pakeitimų poveikį namų ūkių vartojimo įpročiams; arba duomenų rinkinys apie hipotetinius pacientus ir jų vaistų vartojimą, gyvenimo sąlygas ir žinomas šalutines reakcijas.</skos:definition>
      <skos:prefLabel xml:lang="nl">Simulatie</skos:prefLabel>
      <skos:definition xml:lang="nl"/>
      <skos:prefLabel xml:lang="no">Simulering</skos:prefLabel>
      <skos:definition xml:lang="no">Modellering eller etterlignende representasjon av virkelige prosesser, hendelser eller systemer, ofte ved bruk av dataprogrammer. For eksempel et program som modellerer hvordan en husholdnings forbruk svarer på endringer i indirekte skatter; eller et datasett om hypotetiske pasienter og deres eksponering for narkotiske stoffer, bakgrunnsforhold, og kjente ugunstige hendelser.</skos:definition>
      <skos:prefLabel xml:lang="no">Simulering</skos:prefLabel>
      <skos:definition xml:lang="no">Modellering eller etterlignende representasjon av virkelige prosesser, hendelser eller systemer, ofte ved bruk av dataprogrammer. For eksempel et program som modellerer hvordan en husholdnings forbruk svarer på endringer i indirekte skatter; eller et datasett om hypotetiske pasienter og deres eksponering for narkotiske stoffer, bakgrunnsforhold, og kjente ugunstige hendelser.</skos:definition>
      <skos:prefLabel xml:lang="pt">Simulação</skos:prefLabel>
      <skos:definition xml:lang="pt">Modelação ou representação por imitação de processos, eventos ou sistemas do mundo real, utilizando geralmente programas de computador. Por exemplo, um programa que modela as respostas do consumo das famílias às mudanças tributárias indiretas; ou um conjunto de dados em pacientes hipotéticos e a sua exposição a drogas, condições do contexto e eventos adversos conhecidos.</skos:definition>
      <skos:prefLabel xml:lang="sl">Simulacija</skos:prefLabel>
      <skos:definition xml:lang="sl">Modeliranje ali oponašajoče predstavljanje procesov, dogodkov ali sistemov v realnem svetu, pogosto z uporabo računalniških programov. Na primer program, ki modelira odziv potrošnje gospodinjstev na posredne davčne spremembe; ali podatkovje o hipotetičnih pacientih in njihovi izpostavljenosti zdravilu, pogojih v ozadju in znanih neželenih doogodkih.</skos:definition>
      <skos:prefLabel xml:lang="sv">Simulering</skos:prefLabel>
      <skos:definition xml:lang="sv">Modellering eller imiterande representation av processer, händelser eller system i den verkliga världen, ofta skapade med datorprogram. Exempel: ett program som modellerar hur hushållens konsumtion svarar på förändringar i indirekta skatter; eller ett dataset över hypotetiska patienter och deras droganvändning, bakgrundsförhållanden och kända negativa händelser.</skos:definition>
   </rdf:Description>
   <rdf:Description rdf:about="http://rdf-vocabulary.ddialliance.org/cv/ModeOfCollection/4.0/d50e4360">
      <rdf:type rdf:resource="http://www.w3.org/2004/02/skos/core#Concept"/>
      <skos:inScheme rdf:resource="http://rdf-vocabulary.ddialliance.org/cv/ModeOfCollection/4.0/"/>
      <skos:notation>MeasurementsAndTests</skos:notation>
      <skos:prefLabel xml:lang="en">Measurements and tests</skos:prefLabel>
      <skos:definition xml:lang="en">Assessing specific properties (or characteristics) of beings, things, phenomena, (and/ or processes) by applying pre-established standards and/or specialized instruments or techniques.</skos:definition>
      <skos:prefLabel xml:lang="de">Messungen und Tests</skos:prefLabel>
      <skos:definition xml:lang="de">Beurteilung spezifischer Eigenschaften (oder Merkmale) von Wesen, Dingen, Phänomenen (und/oder Prozessen) durch Anwendung vorher festgelegter Standards und/oder spezieller Instrumente oder Techniken.</skos:definition>
      <skos:prefLabel xml:lang="fi">Mittaukset ja testit</skos:prefLabel>
      <skos:definition xml:lang="fi">Ihmisten ja muiden elollisten olioiden, esineiden, materiaalien ja ilmiöiden ominaisuuksien mittaaminen käyttäen etukäteen määriteltyjä standardeja tai tarkoitukseen kehitettyjä mittareita ja tekniikoita.</skos:definition>
      <skos:prefLabel xml:lang="fi">Mittaukset ja testit</skos:prefLabel>
      <skos:definition xml:lang="fi">Ihmisten ja muiden elollisten olioiden, esineiden, materiaalien ja ilmiöiden ominaisuuksien mittaaminen käyttäen etukäteen määriteltyjä standardeja tai tarkoitukseen kehitettyjä mittareita ja tekniikoita.</skos:definition>
      <skos:prefLabel xml:lang="it">Misurazioni e test</skos:prefLabel>
      <skos:definition xml:lang="it">Valutazione di specifiche proprietà (o caratteristiche) di esseri viventi, cose, fenomeni (e/o processi) applicando standard prestabiliti e/o strumenti o tecniche specializzate.</skos:definition>
      <skos:prefLabel xml:lang="ja">測定・テスト</skos:prefLabel>
      <skos:definition xml:lang="ja">事前に定められた基準や専用の測定方法や技術を適用することで、対象となる存在、物事、現象(あるいはプロセス)の特性(あるいは特徴)を評価すること。</skos:definition>
      <skos:prefLabel xml:lang="lt">Matavimai ir testai</skos:prefLabel>
      <skos:definition xml:lang="lt">Organizmų, daiktų, reiškinių (ir (arba) procesų) tam tikrų savybių (ar charakteristikų) vertinimas, naudojant visuotinai priimtus standartus ir (arba) specializuotus instrumentus ar technikas.</skos:definition>
      <skos:prefLabel xml:lang="nl">Metingen en tests</skos:prefLabel>
      <skos:definition xml:lang="nl"/>
      <skos:prefLabel xml:lang="no">Målinger og tester</skos:prefLabel>
      <skos:definition xml:lang="no">Vurdering av bestemte egenskaper (eller karakteristika) ved vesener, ting, fenomen (og/eller prosesser) ved å anvende forutbestemte standarder og/eller spesialiserte instrumenter eller teknikker.</skos:definition>
      <skos:prefLabel xml:lang="no">Målinger og tester</skos:prefLabel>
      <skos:definition xml:lang="no">Vurdering av bestemte egenskaper (eller karakteristika) ved vesener, ting, fenomen (og/eller prosesser) ved å anvende forutbestemte standarder og/eller spesialiserte instrumenter eller teknikker.</skos:definition>
      <skos:prefLabel xml:lang="pt">Medidas e testes</skos:prefLabel>
      <skos:definition xml:lang="pt">Avaliação de propriedades específicas (ou características) de seres, coisas, fenómenos (e/ou processos) aplicando padrões pré-estabelecidos e/ou técnicas e instrumentos específicos.</skos:definition>
      <skos:prefLabel xml:lang="sl">Merjenje in testiranje</skos:prefLabel>
      <skos:definition xml:lang="sl">Ocenjevanje specifičnih lastnosti (ali značilnosti) bitij, stvari, pojavov (in/ali procesov), z uporabo vnaprej določenih standardov in/ali specializiranih instrumentov ali tehnik.</skos:definition>
      <skos:prefLabel xml:lang="sv">Mätningar och tester</skos:prefLabel>
      <skos:definition xml:lang="sv">Bedömning av varelsers, föremåls, fenomens (och/eller processers) särskilda egenskaper (eller karakteristiska) genom att tillämpa förutbestämda standarder och/eller specialiserade instrument eller tekniker.</skos:definition>
      <skos:narrower rdf:resource="http://rdf-vocabulary.ddialliance.org/cv/ModeOfCollection/4.0/d50e4457"/>
      <skos:narrower rdf:resource="http://rdf-vocabulary.ddialliance.org/cv/ModeOfCollection/4.0/d50e4547"/>
      <skos:narrower rdf:resource="http://rdf-vocabulary.ddialliance.org/cv/ModeOfCollection/4.0/d50e4637"/>
   </rdf:Description>
   <rdf:Description rdf:about="http://rdf-vocabulary.ddialliance.org/cv/ModeOfCollection/4.0/d50e4457">
      <rdf:type rdf:resource="http://www.w3.org/2004/02/skos/core#Concept"/>
      <skos:inScheme rdf:resource="http://rdf-vocabulary.ddialliance.org/cv/ModeOfCollection/4.0/"/>
      <skos:notation>MeasurementsAndTests.Educational</skos:notation>
      <skos:prefLabel xml:lang="en">Educational measurements and tests</skos:prefLabel>
      <skos:definition xml:lang="en">Assessment of knowledge, skills, aptitude, or educational achievement by means of specialized measures or tests.</skos:definition>
      <skos:prefLabel xml:lang="de">Messungen und Tests: Leistungs- und Kompetenztests</skos:prefLabel>
      <skos:definition xml:lang="de">Beurteilung von Kenntnissen, Fähigkeiten, Eignung oder Bildungsstand mittels spezieller Messungen oder Tests.</skos:definition>
      <skos:prefLabel xml:lang="fi">Mittaukset ja testit: tietämyksen, taipumusten, soveltuvuuden ja oppimistulosten mittaaminen</skos:prefLabel>
      <skos:definition xml:lang="fi">Mittaamalla tai testaamalla saadut tiedot tutkittavien tietotasosta, synnynnäisistä taipumuksista, soveltuvuudesta tai oppimistuloksista. Esimerkkejä: PISA-testit, ylioppilaskokeiden tulokset, yhteiskunnallisen tietämyksen mittari, tai kielellistä tai matemaattista lahjakkuutta mittaavat testit.</skos:definition>
      <skos:prefLabel xml:lang="fi">Mittaukset ja testit: tietämyksen, taipumusten, soveltuvuuden ja oppimistulosten mittaaminen</skos:prefLabel>
      <skos:definition xml:lang="fi">Mittaamalla tai testaamalla saadut tiedot tutkittavien tietotasosta, synnynnäisistä taipumuksista, soveltuvuudesta tai oppimistuloksista. Esimerkkejä: PISA-testit, ylioppilaskokeiden tulokset, yhteiskunnallisen tietämyksen mittari, tai kielellistä tai matemaattista lahjakkuutta mittaavat testit.</skos:definition>
      <skos:prefLabel xml:lang="it">Misurazioni e test in ambito educativo</skos:prefLabel>
      <skos:definition xml:lang="it">Valutazione delle conoscenze, abilità, attitudini o risultati in ambito educativo mediante misure o test specializzati.</skos:definition>
      <skos:prefLabel xml:lang="ja">教育測定・テスト</skos:prefLabel>
      <skos:definition xml:lang="ja">知識、技能、適正あるいは学業達成度を専用の尺度や試験により評価すること。</skos:definition>
      <skos:prefLabel xml:lang="lt">Edukologiniai matavimai ir testai</skos:prefLabel>
      <skos:definition xml:lang="lt">Žinių, įgūdžių, gabumų ar mokymosi pasiekimų vertinimas, naudojant specialius matus ar testus.</skos:definition>
      <skos:prefLabel xml:lang="nl">Metingen en tests: Kennis/bekwaamheid</skos:prefLabel>
      <skos:definition xml:lang="nl"/>
      <skos:prefLabel xml:lang="no">Pedagogiske målinger og tester</skos:prefLabel>
      <skos:definition xml:lang="no">Vurdering av kunnskap, ferdighet, egnethet, eller utdanningsoppnåelser ved spesialiserte mål eller tester.</skos:definition>
      <skos:prefLabel xml:lang="no">Pedagogiske målinger og tester</skos:prefLabel>
      <skos:definition xml:lang="no">Vurdering av kunnskap, ferdighet, egnethet, eller utdanningsoppnåelser ved spesialiserte mål eller tester.</skos:definition>
      <skos:prefLabel xml:lang="pt">Medidas e testes educacionais</skos:prefLabel>
      <skos:definition xml:lang="pt">Avaliação de conhecimentos, competências, aptidões ou desempenhos educacionais por meio de medidas ou testes específicos.</skos:definition>
      <skos:prefLabel xml:lang="sl">Meritve in testiranja v vzgoji in izobraževanju</skos:prefLabel>
      <skos:definition xml:lang="sl">Ocenjevanje znanja, spretnosti, sposobnosti ali izobraževalnih dosežkov s pomočjo specializiranih meritev ali testov.</skos:definition>
      <skos:prefLabel xml:lang="sv">Pedagogiska mätningar och tester</skos:prefLabel>
      <skos:definition xml:lang="sv">Bedömning av kunskap, förmågor, begåvning eller inlärningsförmåga med hjälp av specialiserade mätredskap och tester.</skos:definition>
      <skos:broader rdf:resource="http://rdf-vocabulary.ddialliance.org/cv/ModeOfCollection/4.0/d50e4360"/>
   </rdf:Description>
   <rdf:Description rdf:about="http://rdf-vocabulary.ddialliance.org/cv/ModeOfCollection/4.0/d50e4547">
      <rdf:type rdf:resource="http://www.w3.org/2004/02/skos/core#Concept"/>
      <skos:inScheme rdf:resource="http://rdf-vocabulary.ddialliance.org/cv/ModeOfCollection/4.0/"/>
      <skos:notation>MeasurementsAndTests.Physical</skos:notation>
      <skos:prefLabel xml:lang="en">Physical measurements and tests</skos:prefLabel>
      <skos:definition xml:lang="en">Assessment of physical properties of living beings, objects, materials, or natural phenomena. For example, findings from hands-on medical examination (e.g., palpation or auscultation), clinical measurements and lab tests like blood analysis, blood pressure, heart rate, body weight and height, as well as general measurements like time, distance, mass, temperature, force, power, speed, GPS data on physical movement and other physical parameters or variables, like geospatial data.</skos:definition>
      <skos:prefLabel xml:lang="de">Messungen und Tests: Physische Tests</skos:prefLabel>
      <skos:definition xml:lang="de">Beurteilung von physikalischen Eigenschaften von Lebewesen, Gegenständen, Materialien oder Naturphänomenen. Zum Beispiel Befunde aus der praktischen medizinischen Untersuchung (z. B. Abtasten oder Abhören), klinische Messungen und Labortests wie Blutanalyse, Blutdruck, Herzfrequenz, Körpergewicht und -größe sowie allgemeine Messungen wie Zeit, Entfernung, Masse, Temperatur, Kraft, Leistung, Geschwindigkeit, GPS-Daten zu körperlichen Bewegungen und andere physikalische Parameter oder Variablen, wie Geodaten.</skos:definition>
      <skos:prefLabel xml:lang="fi">Mittaukset ja testit: fyysisten ominaisuuksien mittaaminen</skos:prefLabel>
      <skos:definition xml:lang="fi">Ihmisten ja muiden elollisten olioiden, esineiden, materiaalien ja luonnonilmiöiden fyysisten ominaisuuksien mittaaminen. Esimerkkejä: verenpaine, paino ja pituus, voima, etäisyys, lämpötila, nopeus, seismografiset mittaukset, GPS-koordinaatit.</skos:definition>
      <skos:prefLabel xml:lang="fi">Mittaukset ja testit: fyysisten ominaisuuksien mittaaminen</skos:prefLabel>
      <skos:definition xml:lang="fi">Ihmisten ja muiden elollisten olioiden, esineiden, materiaalien ja luonnonilmiöiden fyysisten ominaisuuksien mittaaminen. Esimerkkejä: verenpaine, paino ja pituus, voima, etäisyys, lämpötila, nopeus, seismografiset mittaukset, GPS-koordinaatit.</skos:definition>
      <skos:prefLabel xml:lang="it">Misurazioni e test fisici</skos:prefLabel>
      <skos:definition xml:lang="it">Valutazione delle proprietà fisiche di esseri viventi, oggetti, materiali o fenomeni naturali. Per esempio, risultati di esami pratici a livello medico (ad esempio, palpazione o auscultazione), misurazioni cliniche e test di laboratorio come analisi del sangue, pressione sanguigna, frequenza cardiaca, peso corporeo e altezza, nonché misure generali come tempo, distanza, massa, temperatura, forza, potenza, velocità, dati GPS sul movimento fisico e altri parametri o variabili fisici, come i dati geospaziali.</skos:definition>
      <skos:prefLabel xml:lang="ja">肉体的／物理的測定・テスト</skos:prefLabel>
      <skos:definition xml:lang="ja">生物、物、素材、自然現象の物理的特性の評価。例えば、直接的に確かめる健康診断（例：触診や聴診）の結果や、血液検査、血圧、心拍数、体重や身長といった臨床測定・臨床試験の結果等。同様に、一般的な測定値も例としてあげられる。例えば、時間、距離、質量、温度、物理的な力、動力、速度、物理的移動に関するGPSデータ、そして地理空間データ等のその他の物理的変数やパラメーター等がある。</skos:definition>
      <skos:prefLabel xml:lang="lt">Fiziniai matavimai ir testai</skos:prefLabel>
      <skos:definition xml:lang="lt">Gyvų organizmų, objektų, medžiagų ar gamtos reiškinių fizinių savybių vertinimas. Pavyzdžiui, praktinės medicininės apžiūros (pavyzdžiui, palpacijos ar auskultacijos) rezultatai, klinikinių matavimų ir laboratorinių tyrimų testai (pavyzdžiui, kraujo tyrimai, kraujospūdžio, širdies ritmo, kūno svorio ir ūgio matavimai), taip pat bendrieji matavimo vienetai (pavyzdžiui, laikas, atstumas, masė, temperatūra, jėga, galia, greitis, GPS duomenys apie fizinį judėjimą) ir kiti fiziniai parametrai ar kintamieji (pavyzdžiui, geoerdviniai duomenys).</skos:definition>
      <skos:prefLabel xml:lang="nl">Fysieke metingen en tests</skos:prefLabel>
      <skos:definition xml:lang="nl"/>
      <skos:prefLabel xml:lang="no">Fysiske målinger og tester</skos:prefLabel>
      <skos:definition xml:lang="no">Vurdering av fysiske egenskaper hos levende vesener, objekter, materiale, eller naturlige fenomen. For eksempel, funn fra fysiske medisinske undersøkelser (e.g., palpasjon eller auskultasjon), kliniske mål og laboratorietester som blodanalyse, blodtrykksmål, hjerterytme, kroppsvekt og høyde, og generelle mål som tid, distanse, masse, temperatur, kraft, energi, fart, GPS data på fysisk bevegelse og andre mål på fysiske parameter eller variabler.</skos:definition>
      <skos:prefLabel xml:lang="no">Fysiske målinger og tester</skos:prefLabel>
      <skos:definition xml:lang="no">Vurdering av fysiske egenskaper hos levende vesener, objekter, materiale, eller naturlige fenomen. For eksempel, funn fra fysiske medisinske undersøkelser (e.g., palpasjon eller auskultasjon), kliniske mål og laboratorietester som blodanalyse, blodtrykksmål, hjerterytme, kroppsvekt og høyde, og generelle mål som tid, distanse, masse, temperatur, kraft, energi, fart, GPS data på fysisk bevegelse og andre mål på fysiske parameter eller variabler.</skos:definition>
      <skos:prefLabel xml:lang="pt">Medidas e testes físicos</skos:prefLabel>
      <skos:definition xml:lang="pt">Avaliação de propriedades físicas de seres vivos, objetos, materiais ou fenómenos naturais. Por exemplo, descobertas de exames médicos práticos (por exemplo, palpação ou auscultação), medições clínicas e testes laboratoriais, como análise sanguínea, pressão arterial, frequência cardíaca, peso e altura, assim como medidas gerais, por exemplo, de tempo, distância, massa, temperatura, força, potência, velocidade, dados de GPS sobre movimento físico e outros parâmetros ou variáveis físicos, como dados geoespaciais.</skos:definition>
      <skos:prefLabel xml:lang="sl">Meritve in testiranja fizičnih lastnosti</skos:prefLabel>
      <skos:definition xml:lang="sl">Ocenjevanje fizičnih lastnosti živih bitij, predmetov, materialov ali naravnih pojavov. Na primer ugotovitve praktičnega zdravniškega pregleda (npr. palpacije ali auskultacije), kliničnih meritev in laboratorijskih preiskav, kot so analiza krvi, krvni talak, srčni utrip, telesna teža in višina ter splošne meritve, kot so čas, razdalja, temperatura, sila, moč, hitrost, podatki GPS o fizičnem gibanju in drugih fizičnih parametrih ali spremenljivkah, kot so geoprostorski podatki.</skos:definition>
      <skos:prefLabel xml:lang="sv">Fysiska mätningar och tester</skos:prefLabel>
      <skos:definition xml:lang="sv">Bedömning av levande varelsers, föremåls, materials eller naturliga fenomens fysiska egenskaper. Till exempel: blodtryck, puls, kroppsvikt och längd, men även tid, avstånd, massa, temperatur, kraft, effekt, hastighet, GPS-data för fysisk rörelse och andra fysiska parametrar eller variabler, som t.ex. geospatiala data.</skos:definition>
      <skos:broader rdf:resource="http://rdf-vocabulary.ddialliance.org/cv/ModeOfCollection/4.0/d50e4360"/>
   </rdf:Description>
   <rdf:Description rdf:about="http://rdf-vocabulary.ddialliance.org/cv/ModeOfCollection/4.0/d50e4637">
      <rdf:type rdf:resource="http://www.w3.org/2004/02/skos/core#Concept"/>
      <skos:inScheme rdf:resource="http://rdf-vocabulary.ddialliance.org/cv/ModeOfCollection/4.0/"/>
      <skos:notation>MeasurementsAndTests.Psychological</skos:notation>
      <skos:prefLabel xml:lang="en">Psychological measurements and tests</skos:prefLabel>
      <skos:definition xml:lang="en">Assessment of personality traits or psychological/behavioral responses by means of specialized measures or tests. For example, objective tests like self-report measures with a restricted response format, or projective methods allowing free responses, including word association, sentence or story completion, vignettes, cartoon test, thematic apperception tests, role play, drawing tests, inkblot tests, choice ordering exercises, etc.</skos:definition>
      <skos:prefLabel xml:lang="de">Messungen und Tests: Psychologische Tests</skos:prefLabel>
      <skos:definition xml:lang="de">Beurteilung von Persönlichkeitsmerkmalen oder psychologischen/verhaltensbezogenen Reaktionen mittels spezieller Messungen oder Tests. Zum Beispiel objektive Tests wie Selbstauskünfte mit eingeschränktem Antwortformat oder projektive Methoden, die freie Antworten erlauben, einschließlich Wortassoziation, Vervollständigung von Sätzen- oder Geschichten, Vignetten, Karikatur-Tests, thematische Apperzeptionstests, Rollenspiele, Zeichentests, Tintenkleckstests, Zuordnungsaufgaben usw.</skos:definition>
      <skos:prefLabel xml:lang="fi">Mittaukset ja testit: psykologisten ominaisuuksien mittaaminen</skos:prefLabel>
      <skos:definition xml:lang="fi">Luonteenpiirteiden ja käyttäytymismallien tutkiminen tarkoitusta varten kehitettyjen testien avulla. Esimerkiksi: Luonteenpiirteiden itseraportointi, eläytymismenetelmät. Tarvittaessa voidaan käyttää yhdessä muiden aineistonkeruumenetelmätermien kanssa (esimerkiksi masentuneisuusaste-testi osana kyselylomaketta).</skos:definition>
      <skos:prefLabel xml:lang="fi">Mittaukset ja testit: psykologisten ominaisuuksien mittaaminen</skos:prefLabel>
      <skos:definition xml:lang="fi">Luonteenpiirteiden ja käyttäytymismallien tutkiminen tarkoitusta varten kehitettyjen testien avulla. Esimerkiksi: Luonteenpiirteiden itseraportointi, eläytymismenetelmät. Tarvittaessa voidaan käyttää yhdessä muiden aineistonkeruumenetelmätermien kanssa (esimerkiksi masentuneisuusaste-testi osana kyselylomaketta).</skos:definition>
      <skos:prefLabel xml:lang="it">Misurazioni e test psicologici</skos:prefLabel>
      <skos:definition xml:lang="it">Valutazione dei tratti di personalità o risposte psicologiche/comportamentali mediante misure o test specializzati. Ad esempio, test oggettivi come misure di autovalutazione con un range predefinito, o test proiettivi che consentono risposte libere, incluse associazione di parole, completamento di frasi o storie, vignette, fumetti, test di appercezione tematica, giochi di ruolo, prove di disegno, test macchie di inchiostri, esercizi sulle scelte di ordinamento, ecc.</skos:definition>
      <skos:prefLabel xml:lang="ja">心理測定・テスト</skos:prefLabel>
      <skos:definition xml:lang="ja">特別な尺度やテストにより性格的な特徴や心理的あるいは行動における反応を評価すること。例えば、限られた選択肢から自己報告式で回答する客観的テスト等がある。同様に、自由に回答できる投影法を用いたテストもある。例えば、単語の連想、文や物語の完成、ビネット調査、漫画を用いたテスト、主題統覚検査、ロールプレイ、作図テスト、ロールシャッハ・テスト、選択肢の並べ替え課題等が例としてあげられる。</skos:definition>
      <skos:prefLabel xml:lang="lt">Psichologiniai matavimai ir testai</skos:prefLabel>
      <skos:definition xml:lang="lt">Asmenybės bruožų arba psichologinių ar elgsenos reakcijų vertinimas, naudojant specialius matavimo instrumentus ar testus. Pavyzdžiui, standartizuoti testai (pavyzdžiui, savipildos instrumentai) su uždarais klausimais, ar projekciniai metodai naudojant atvirus klausimus (įskaitant žodžių asociacijas, sakinio ar pasakojimo užbaigimą, vinjetes, animuotus testus, teminius suvokimo testus, vaidmenų žaidimus, piešimo testus, rašalo dėmių testus, pasirinkimų rangavimo pratimus ir kt.).</skos:definition>
      <skos:prefLabel xml:lang="nl">Psychologische metingen en tests </skos:prefLabel>
      <skos:definition xml:lang="nl"/>
      <skos:prefLabel xml:lang="no">Psykologiske målinger og tester</skos:prefLabel>
      <skos:definition xml:lang="no">Vurdering av personlighetstrekk eller psykologiske/atferdsmessige reaksjoner ved bruk av spesialiserte mål og tester. For eksempel, objektive tester som selvrapporteringsmål med mer begrenset svarformat, eller projektive metoder som gjør det mulig å svare helt fritt, inkludert ordassosiasjon, setning eller fortellingsfullføring, korte beskrivelser, tematiske appersepsjonstester, rollespill, tegnetester, blekk-kladd tester, prioriteringsøvelser etc.</skos:definition>
      <skos:prefLabel xml:lang="no">Psykologiske målinger og tester</skos:prefLabel>
      <skos:definition xml:lang="no">Vurdering av personlighetstrekk eller psykologiske/atferdsmessige reaksjoner ved bruk av spesialiserte mål og tester. For eksempel, objektive tester som selvrapporteringsmål med mer begrenset svarformat, eller projektive metoder som gjør det mulig å svare helt fritt, inkludert ordassosiasjon, setning eller fortellingsfullføring, korte beskrivelser, tematiske appersepsjonstester, rollespill, tegnetester, blekk-kladd tester, prioriteringsøvelser etc.</skos:definition>
      <skos:prefLabel xml:lang="pt">Medidas e testes psicológicos</skos:prefLabel>
      <skos:definition xml:lang="pt">Avaliação de traços de personalidade ou respostas psicológicas/comportamentais por meio de medidas específicas e testes. Por exemplo, testes objetivos como medidas autorreportadas com um formato restrito de resposta, ou métodos projetivos que permitem respostas livres, incluindo associação de palavras, conclusão de frases ou histórias, vinhetas, teste de desenho animado, testes temáticos de percepção, dramatização, testes de desenho, testes de mancha de tinta, exercícios de ordenação de escolha, etc.</skos:definition>
      <skos:prefLabel xml:lang="sl">Meritve in testiranja psiholoških lastnosti</skos:prefLabel>
      <skos:definition xml:lang="sl">Ocena osebnostnih lastnosti ali psiholoških/vedenjskih odzivov s pomočjo posebnih meritev ali testov. Na primer objektivni testi, kot so samoporočanje z zaprtim formatom odgovorov ali projekcijske tehnike, ki omogočajo proste odgovore, vključno z besednimi asociacijami, dopolnjevanjem stavkov ali zgodb, vinjetami, testi s karikaturami, testi tematske apercepcije, igranjem vlog, testi risanja, testi pack, testi izbire itd.</skos:definition>
      <skos:prefLabel xml:lang="sv">Psykologiska mätningar och tester</skos:prefLabel>
      <skos:definition xml:lang="sv">Bedömning av personlighetsdrag eller psykologiska/beteendemässiga responser genom specialiserade mätredskap eller tester. Exempel: objektiva tester som självskattning med begränsade svarsformat, eller projektiva tester som tillåter öppna svar, inklusive ordassociation, menings- eller berättelsekomplettering, vinjetter, "cartoon tests", tematiska apperceptionstester (TAT), rollspel, teckningstester, Rorschachtester, "choice ordering exercises" m.m.</skos:definition>
      <skos:broader rdf:resource="http://rdf-vocabulary.ddialliance.org/cv/ModeOfCollection/4.0/d50e4360"/>
   </rdf:Description>
   <rdf:Description rdf:about="http://rdf-vocabulary.ddialliance.org/cv/ModeOfCollection/4.0/d50e4727">
      <rdf:type rdf:resource="http://www.w3.org/2004/02/skos/core#Concept"/>
      <skos:inScheme rdf:resource="http://rdf-vocabulary.ddialliance.org/cv/ModeOfCollection/4.0/"/>
      <skos:notation>Other</skos:notation>
      <skos:prefLabel xml:lang="en">Other</skos:prefLabel>
      <skos:definition xml:lang="en">Use if the mode of data collection is known, but not found in the list.</skos:definition>
      <skos:prefLabel xml:lang="de">Andere</skos:prefLabel>
      <skos:definition xml:lang="de">Verwenden Sie diese Kategorie, wenn die Art der Datenerhebung bekannt, aber nicht in der Liste vertreten ist.</skos:definition>
      <skos:prefLabel xml:lang="fi">Muu keruumenetelmä</skos:prefLabel>
      <skos:definition xml:lang="fi">Käytä mikäli keruumenetelmä on tiedossa, mutta ei sanastossa. Lisää tarkempi selostus.</skos:definition>
      <skos:prefLabel xml:lang="fi">Muu keruumenetelmä</skos:prefLabel>
      <skos:definition xml:lang="fi">Käytä mikäli keruumenetelmä on tiedossa, mutta ei sanastossa. Lisää tarkempi selostus.</skos:definition>
      <skos:prefLabel xml:lang="it">Altro</skos:prefLabel>
      <skos:definition xml:lang="it">Utilizzare quando la tecnica di raccolta dei dati è conosciuta, ma non è presente nell'elenco.</skos:definition>
      <skos:prefLabel xml:lang="ja">その他</skos:prefLabel>
      <skos:definition xml:lang="ja">データ収集方法は既知であるが、このリストに載っていない場合に用いる。</skos:definition>
      <skos:prefLabel xml:lang="lt">Kita </skos:prefLabel>
      <skos:definition xml:lang="lt">Naudoti, kai duomenų rinkimo būdas yra žinomas, bet jo nėra sąraše.</skos:definition>
      <skos:prefLabel xml:lang="nl">Anders</skos:prefLabel>
      <skos:definition xml:lang="nl"/>
      <skos:prefLabel xml:lang="no">Annet</skos:prefLabel>
      <skos:definition xml:lang="no">Bruk dersom metode for datainnsamling er kjent, men ikke finnes i listen.</skos:definition>
      <skos:prefLabel xml:lang="no">Annet</skos:prefLabel>
      <skos:definition xml:lang="no">Bruk dersom metode for datainnsamling er kjent, men ikke finnes i listen.</skos:definition>
      <skos:prefLabel xml:lang="pt">Outro</skos:prefLabel>
      <skos:definition xml:lang="pt">Usar se o método de recolha de dados for conhecido, mas não se encontrar na lista.</skos:definition>
      <skos:prefLabel xml:lang="sl">Drugo</skos:prefLabel>
      <skos:definition xml:lang="sl">Uporabite, če je način zbiranja podatkov znan, vendar ga ni na tem seznamu.</skos:definition>
      <skos:prefLabel xml:lang="sv">Övrigt</skos:prefLabel>
      <skos:definition xml:lang="sv">Används när datainsamlingsmetoden är känd men saknas i listan.</skos:definition>
   </rdf:Description>
</rdf:RDF>
