<?xml version="1.0" encoding="UTF-8"?>
<rdf:RDF xmlns:rdf="http://www.w3.org/1999/02/22-rdf-syntax-ns#"
         xmlns:skos="http://www.w3.org/2004/02/skos/core#"
         xmlns:owl="http://www.w3.org/2002/07/owl#"
         xmlns:dcterms="http://purl.org/dc/terms/"
>
   <rdf:Description rdf:about="http://rdf-vocabulary.ddialliance.org/cv/NumericType/1.0.0/">
      <rdf:type rdf:resource="http://www.w3.org/2004/02/skos/core#ConceptScheme"/>
      <dcterms:isVersionOf rdf:resource="http://rdf-vocabulary.ddialliance.org/cv/NumericType/"/>
      <skos:notation xml:lang="en">NumericType</skos:notation>
      <dcterms:title xml:lang="en">Numeric Type</dcterms:title>
      <dcterms:description xml:lang="en">Specifies the type of numeric data.</dcterms:description>
      <skos:prefLabel xml:lang="en">Numeric Type</skos:prefLabel>
      <owl:versionInfo>1.0.0</owl:versionInfo>
      <dcterms:license rdf:resource="http://creativecommons.org/licenses/by/4.0/"/>
      <dcterms:rights>Copyright &#xa9;DDI Alliance 2019</dcterms:rights>
      <skos:hasTopConcept rdf:resource="http://rdf-vocabulary.ddialliance.org/cv/NumericType/1.0.0/a0faef0"/>
      <skos:hasTopConcept rdf:resource="http://rdf-vocabulary.ddialliance.org/cv/NumericType/1.0.0/1686a6c"/>
      <skos:hasTopConcept rdf:resource="http://rdf-vocabulary.ddialliance.org/cv/NumericType/1.0.0/8394f03"/>
      <skos:hasTopConcept rdf:resource="http://rdf-vocabulary.ddialliance.org/cv/NumericType/1.0.0/30bb747"/>
      <skos:hasTopConcept rdf:resource="http://rdf-vocabulary.ddialliance.org/cv/NumericType/1.0.0/937504f"/>
      <skos:hasTopConcept rdf:resource="http://rdf-vocabulary.ddialliance.org/cv/NumericType/1.0.0/22ae0e2"/>
      <skos:hasTopConcept rdf:resource="http://rdf-vocabulary.ddialliance.org/cv/NumericType/1.0.0/d909d38"/>
      <skos:hasTopConcept rdf:resource="http://rdf-vocabulary.ddialliance.org/cv/NumericType/1.0.0/e93f994"/>
      <skos:hasTopConcept rdf:resource="http://rdf-vocabulary.ddialliance.org/cv/NumericType/1.0.0/482be0d"/>
      <skos:hasTopConcept rdf:resource="http://rdf-vocabulary.ddialliance.org/cv/NumericType/1.0.0/6311ae1"/>
   </rdf:Description>
   <rdf:Description rdf:about="http://rdf-vocabulary.ddialliance.org/cv/NumericType/1.0.0/a0faef0">
      <rdf:type rdf:resource="http://www.w3.org/2004/02/skos/core#Concept"/>
      <skos:inScheme rdf:resource="http://rdf-vocabulary.ddialliance.org/cv/NumericType/1.0.0/"/>
      <skos:notation xml:lang="en">Integer</skos:notation>
      <skos:prefLabel xml:lang="en">Integer</skos:prefLabel>
      <skos:definition xml:lang="en">Whole numbers,  the infinite set of integers, no minimum or maximum value.  An integer datatype corresponding to the W3C XML Schema&apos;s xs:integer datatype.</skos:definition>
   </rdf:Description>
   <rdf:Description rdf:about="http://rdf-vocabulary.ddialliance.org/cv/NumericType/1.0.0/1686a6c">
      <rdf:type rdf:resource="http://www.w3.org/2004/02/skos/core#Concept"/>
      <skos:inScheme rdf:resource="http://rdf-vocabulary.ddialliance.org/cv/NumericType/1.0.0/"/>
      <skos:notation xml:lang="en">Int</skos:notation>
      <skos:prefLabel xml:lang="en">Int </skos:prefLabel>
      <skos:definition xml:lang="en">Whole numbers in the range -2147483648 .. 2147483647. An integer datatype corresponding to the W3C XML Schema&apos;s xs:int datatype.</skos:definition>
   </rdf:Description>
   <rdf:Description rdf:about="http://rdf-vocabulary.ddialliance.org/cv/NumericType/1.0.0/8394f03">
      <rdf:type rdf:resource="http://www.w3.org/2004/02/skos/core#Concept"/>
      <skos:inScheme rdf:resource="http://rdf-vocabulary.ddialliance.org/cv/NumericType/1.0.0/"/>
      <skos:notation xml:lang="en">Long</skos:notation>
      <skos:prefLabel xml:lang="en">Long</skos:prefLabel>
      <skos:definition xml:lang="en">Whole numbers in the range -9223372036854775808 .. 9223372036854775807. A numeric datatype corresponding to the W3C XML Schema&apos;s xs:long datatype.</skos:definition>
   </rdf:Description>
   <rdf:Description rdf:about="http://rdf-vocabulary.ddialliance.org/cv/NumericType/1.0.0/30bb747">
      <rdf:type rdf:resource="http://www.w3.org/2004/02/skos/core#Concept"/>
      <skos:inScheme rdf:resource="http://rdf-vocabulary.ddialliance.org/cv/NumericType/1.0.0/"/>
      <skos:notation xml:lang="en">Short</skos:notation>
      <skos:prefLabel xml:lang="en">Short</skos:prefLabel>
      <skos:definition xml:lang="en">Whole numbers in the range -32768 .. 32767. A numeric datatype corresponding to the W3C XML Schema&apos;s xs:short datatype.</skos:definition>
   </rdf:Description>
   <rdf:Description rdf:about="http://rdf-vocabulary.ddialliance.org/cv/NumericType/1.0.0/937504f">
      <rdf:type rdf:resource="http://www.w3.org/2004/02/skos/core#Concept"/>
      <skos:inScheme rdf:resource="http://rdf-vocabulary.ddialliance.org/cv/NumericType/1.0.0/"/>
      <skos:notation xml:lang="en">Decimal</skos:notation>
      <skos:prefLabel xml:lang="en">Decimal</skos:prefLabel>
      <skos:definition xml:lang="en">A subset of real numbers, which can be represented by a finite-length sequence of decimal digits (0-9) separated by a period as a decimal indicator. An optional leading sign is allowed. If the sign is omitted, &quot;+&quot; is assumed. Leading and trailing zeroes are optional. If the fractional part is zero, the period and following zero(es) can be omitted. For example: -1.23, 12678967.543233, +100000.00, 210. A numeric datatype corresponding to the W3C XML Schema&apos;s xs:decimal datatype.</skos:definition>
   </rdf:Description>
   <rdf:Description rdf:about="http://rdf-vocabulary.ddialliance.org/cv/NumericType/1.0.0/22ae0e2">
      <rdf:type rdf:resource="http://www.w3.org/2004/02/skos/core#Concept"/>
      <skos:inScheme rdf:resource="http://rdf-vocabulary.ddialliance.org/cv/NumericType/1.0.0/"/>
      <skos:notation xml:lang="en">Float</skos:notation>
      <skos:prefLabel xml:lang="en">Float</skos:prefLabel>
      <skos:definition xml:lang="en">Single-precision 32-bit floating point type: The basic value space of float consists of the values m&#xfffd;2^e, where m is an integer whose absolute value is less than 2^24, and e is an integer between -149 and 104, inclusive. In addition, it also contains the following three special values: positive and negative infinity and not-a-number (NaN). The special values positive and negative infinity and not-a-number have lexical representations INF, -INF and NaN, respectively. Lexical representations for zero may take a positive or negative sign. For example, -1E4, 1267.43233E12, 12.78e-2, 12 , -0, 0 and INF are all legal literals for float. A numeric datatype corresponding to the W3C XML Schema&apos;s xs:float datatype.</skos:definition>
   </rdf:Description>
   <rdf:Description rdf:about="http://rdf-vocabulary.ddialliance.org/cv/NumericType/1.0.0/d909d38">
      <rdf:type rdf:resource="http://www.w3.org/2004/02/skos/core#Concept"/>
      <skos:inScheme rdf:resource="http://rdf-vocabulary.ddialliance.org/cv/NumericType/1.0.0/"/>
      <skos:notation xml:lang="en">Double</skos:notation>
      <skos:prefLabel xml:lang="en">Double</skos:prefLabel>
      <skos:definition xml:lang="en">Double-precision 64-bit floating point type. The basic value space of double consists of the values m&#xfffd;2^e, where m is an integer whose absolute value is less than 2^53, and e is an integer between -1075 and 970, inclusive. In addition to the basic value space described above, the value space of double also contains the following three special values: positive and negative infinity and not-a-number (NaN). The special values positive and negative infinity and not-a-number have lexical representations INF, -INF and NaN, respectively. Lexical representations for zero may take a positive or negative sign. For example, -1E4, 1267.43233E12, 12.78e-2, 12 , -0, 0 and INF are all legal literals for double. A numeric datatype corresponding to the W3C XML Schema&apos;s xs:double datatype.</skos:definition>
   </rdf:Description>
   <rdf:Description rdf:about="http://rdf-vocabulary.ddialliance.org/cv/NumericType/1.0.0/e93f994">
      <rdf:type rdf:resource="http://www.w3.org/2004/02/skos/core#Concept"/>
      <skos:inScheme rdf:resource="http://rdf-vocabulary.ddialliance.org/cv/NumericType/1.0.0/"/>
      <skos:notation xml:lang="en">Count</skos:notation>
      <skos:prefLabel xml:lang="en">Count</skos:prefLabel>
      <skos:definition xml:lang="en">Ordinal number of objects in a finite set, discrete. A simple incrementing Integer type. When using in DDI-L, the &quot;isSequence&quot; facet must be set to true, and the &quot;interval&quot; facet must be set to &quot;1&quot;.</skos:definition>
   </rdf:Description>
   <rdf:Description rdf:about="http://rdf-vocabulary.ddialliance.org/cv/NumericType/1.0.0/482be0d">
      <rdf:type rdf:resource="http://www.w3.org/2004/02/skos/core#Concept"/>
      <skos:inScheme rdf:resource="http://rdf-vocabulary.ddialliance.org/cv/NumericType/1.0.0/"/>
      <skos:notation xml:lang="en">Incremental</skos:notation>
      <skos:prefLabel xml:lang="en">Incremental</skos:prefLabel>
      <skos:definition xml:lang="en">A value that increases continuously and infinitely by a given amount. Use of this term in DDI-L indicates that the value increases by the amount provided in the &quot;interval&quot; facet; the &quot;isSequence&quot; facet will be set to &quot;true&quot;.</skos:definition>
   </rdf:Description>
   <rdf:Description rdf:about="http://rdf-vocabulary.ddialliance.org/cv/NumericType/1.0.0/6311ae1">
      <rdf:type rdf:resource="http://www.w3.org/2004/02/skos/core#Concept"/>
      <skos:inScheme rdf:resource="http://rdf-vocabulary.ddialliance.org/cv/NumericType/1.0.0/"/>
      <skos:notation xml:lang="en">Other</skos:notation>
      <skos:prefLabel xml:lang="en">Other</skos:prefLabel>
      <skos:definition xml:lang="en">Use if the numeric type is known, but not found in the list.</skos:definition>
   </rdf:Description>
</rdf:RDF>
