<?xml version="1.0" encoding="UTF-8"?>
<rdf:RDF xmlns:rdf="http://www.w3.org/1999/02/22-rdf-syntax-ns#"
         xmlns:skos="http://www.w3.org/2004/02/skos/core#"
         xmlns:owl="http://www.w3.org/2002/07/owl#"
         xmlns:dcterms="http://purl.org/dc/terms/"
>
   <rdf:Description rdf:about="http://rdf-vocabulary.ddialliance.org/cv/AnalysisUnit/2.1.0/">
      <rdf:type rdf:resource="http://www.w3.org/2004/02/skos/core#ConceptScheme"/>
      <dcterms:isVersionOf rdf:resource="http://rdf-vocabulary.ddialliance.org/cv/AnalysisUnit/"/>
      <skos:notation xml:lang="en">AnalysisUnit</skos:notation>
      <dcterms:title xml:lang="sl">Enota analize</dcterms:title>
      <dcterms:description xml:lang="sl">Opisuje enoto, ki jo analiziramo v raziskavi ali v spremenljivki.</dcterms:description>
      <skos:prefLabel xml:lang="sl">Enota analize</skos:prefLabel>
      <dcterms:title xml:lang="lt">Analiz&#x117;s vienetas</dcterms:title>
      <dcterms:description xml:lang="lt">Apib&#x16b;dina tyrime ar kintamajame stebim&#x105; ar analizuojam&#x105; objekt&#x105;. &#x160;is &#x17e;odynas taip pat gali b&#x16b;ti naudojamas apib&#x16b;dinant steb&#x117;jimo vienetus, kurie patys gali b&#x16b;ti steb&#x117;jimo objektais, arba i&#x161; kuri&#x173; gali b&#x16b;ti renkami duomenys. Steb&#x117;jimo vienetas gali sutapti arba skirtis nuo analiz&#x117;s vieneto.</dcterms:description>
      <skos:prefLabel xml:lang="lt">Analiz&#x117;s vienetas</skos:prefLabel>
      <dcterms:title xml:lang="sv">Analysenhet</dcterms:title>
      <dcterms:description xml:lang="sv">Beskriver den enhet som analyseras i studien eller i variabeln. Den h&#xe4;r vokabul&#xe4;ren kan &#xe4;ven anv&#xe4;ndas f&#xf6;r att beskriva unders&#xf6;kningsenhet, som &#xe4;r den enhet som unders&#xf6;ks eller observeras, eller som data samlas in fr&#xe5;n. Unders&#xf6;kningsenheten kan vara densamma som eller &#xe5;tskild fr&#xe5;n analysenheten. </dcterms:description>
      <skos:prefLabel xml:lang="sv">Analysenhet</skos:prefLabel>
      <dcterms:title xml:lang="fi">Havainto/aineistoyksikk&#xf6;tyyppi</dcterms:title>
      <dcterms:description xml:lang="fi">M&#xe4;&#xe4;rittelee yksik&#xf6;n, jota tutkimuksessa/muuttujassa analysoidaan. Sanastoa voidaan k&#xe4;ytt&#xe4;&#xe4; my&#xf6;s m&#xe4;&#xe4;rittelem&#xe4;&#xe4;n havaintoyksikk&#xf6;, jota tutkimuksessa havannoidaan tai josta aineistoa ker&#xe4;t&#xe4;&#xe4;n. Havaintoyksikk&#xf6; voi olla sama tai eri kuin analyysiyksikk&#xf6;.
</dcterms:description>
      <skos:prefLabel xml:lang="fi">Havainto/aineistoyksikk&#xf6;tyyppi</skos:prefLabel>
      <dcterms:title xml:lang="it">Unit&#xe0; di analisi</dcterms:title>
      <dcterms:description xml:lang="it">Descrive l&apos;entit&#xe0; analizzata nello studio o nella variabile. Questo vocabolario pu&#xf2; essere usato anche per descrivere l&apos;unit&#xe0; di raccolta, che &#xe8; l&apos;unit&#xe0; che viene osservata, o sulla base della quale vengono raccolti i dati. L&apos;unit&#xe0; di raccolta pu&#xf2; coincidere con l&apos;unit&#xe0; di analisi oppure pu&#xf2; essere differente.</dcterms:description>
      <skos:prefLabel xml:lang="it">Unit&#xe0; di analisi</skos:prefLabel>
      <dcterms:title xml:lang="pt">Unidade de An&#xe1;lise</dcterms:title>
      <dcterms:description xml:lang="pt">Descreve a entidade que est&#xe1; a ser observada ou analisada no estudo ou na vari&#xe1;vel.</dcterms:description>
      <skos:prefLabel xml:lang="pt">Unidade de An&#xe1;lise</skos:prefLabel>
      <dcterms:title xml:lang="en">Analysis Unit</dcterms:title>
      <dcterms:description xml:lang="en">Describes the entity being analyzed in the study or variable. This vocabulary can also be used to describe the unit of observation, which is the unit being observed, or from which data are collected. The unit of observation can be the same as, or different from the unit of analysis. </dcterms:description>
      <skos:prefLabel xml:lang="en">Analysis Unit</skos:prefLabel>
      <dcterms:title xml:lang="de">Analyseeinheit</dcterms:title>
      <dcterms:description xml:lang="de">Beschreibt die Entit&#xe4;t, die in der Studie oder in der Variable analysiert wird. Dieses Vokabular kann auch verwendet werden, um die Beobachtungseinheit zu beschreiben, d. h. die Einheit, die beobachtet wird oder von der Daten gesammelt werden. Die Beobachtungseinheit kann mit der Analyseeinheit identisch sein oder sich von ihr unterscheiden.</dcterms:description>
      <skos:prefLabel xml:lang="de">Analyseeinheit</skos:prefLabel>
      <dcterms:title xml:lang="nl">Analyse Eenheid</dcterms:title>
      <dcterms:description xml:lang="nl">Beschrijft de eenheid die geanalyseerd wordt in een bepaalde studie of variabele. De termen kunnen ook gebruikt worden om de waargenomen eenheid te beschrijven - dit is de eenheid die geobserveerd wordt of waarvan data wordt verzameld. De waargenomen eenheid kan hetzelfde zijn als de analyse eenheid, of ze kunnen van elkaar verschillen.</dcterms:description>
      <skos:prefLabel xml:lang="nl">Analyse Eenheid</skos:prefLabel>
      <dcterms:title xml:lang="no">Analyseenhet</dcterms:title>
      <dcterms:description xml:lang="no">Beskrivelse av enhet som blir analysert i studien eller i variablene. Dette vokabularet kan ogs&#xe5; bli brukt for &#xe5; beskrive observasjonsenheten, som er enheten som blir observert, eller enheten data er samlet inn fra. Observasjonsenhten kan v&#xe6;re det samme eller forskjellig fra analyseenheten.</dcterms:description>
      <skos:prefLabel xml:lang="no">Analyseenhet</skos:prefLabel>
      <owl:versionInfo>2.1.1</owl:versionInfo>
      <dcterms:license rdf:resource="http://creativecommons.org/licenses/by/4.0/"/>
      <dcterms:rights>Copyright &#xa9;DDI Alliance 2020</dcterms:rights>
      <skos:hasTopConcept rdf:resource="http://rdf-vocabulary.ddialliance.org/cv/AnalysisUnit/2.1.0/2dd4472"/>
      <skos:hasTopConcept rdf:resource="http://rdf-vocabulary.ddialliance.org/cv/AnalysisUnit/2.1.0/63eefb7"/>
      <skos:hasTopConcept rdf:resource="http://rdf-vocabulary.ddialliance.org/cv/AnalysisUnit/2.1.0/cefc4f7"/>
      <skos:hasTopConcept rdf:resource="http://rdf-vocabulary.ddialliance.org/cv/AnalysisUnit/2.1.0/ea4be67"/>
      <skos:hasTopConcept rdf:resource="http://rdf-vocabulary.ddialliance.org/cv/AnalysisUnit/2.1.0/4358d21"/>
      <skos:hasTopConcept rdf:resource="http://rdf-vocabulary.ddialliance.org/cv/AnalysisUnit/2.1.0/fa83853"/>
      <skos:hasTopConcept rdf:resource="http://rdf-vocabulary.ddialliance.org/cv/AnalysisUnit/2.1.0/435eb71"/>
      <skos:hasTopConcept rdf:resource="http://rdf-vocabulary.ddialliance.org/cv/AnalysisUnit/2.1.0/75fa5c6"/>
      <skos:hasTopConcept rdf:resource="http://rdf-vocabulary.ddialliance.org/cv/AnalysisUnit/2.1.0/8b62b80"/>
      <skos:hasTopConcept rdf:resource="http://rdf-vocabulary.ddialliance.org/cv/AnalysisUnit/2.1.0/9658ae5"/>
      <skos:hasTopConcept rdf:resource="http://rdf-vocabulary.ddialliance.org/cv/AnalysisUnit/2.1.0/0393713"/>
      <skos:hasTopConcept rdf:resource="http://rdf-vocabulary.ddialliance.org/cv/AnalysisUnit/2.1.0/4970317"/>
      <skos:hasTopConcept rdf:resource="http://rdf-vocabulary.ddialliance.org/cv/AnalysisUnit/2.1.0/6311ae1"/>
   </rdf:Description>
   <rdf:Description rdf:about="http://rdf-vocabulary.ddialliance.org/cv/AnalysisUnit/2.1.0/2dd4472">
      <rdf:type rdf:resource="http://www.w3.org/2004/02/skos/core#Concept"/>
      <skos:inScheme rdf:resource="http://rdf-vocabulary.ddialliance.org/cv/AnalysisUnit/2.1.0/"/>
      <skos:notation xml:lang="en">Individual</skos:notation>
      <skos:prefLabel xml:lang="sl">Posameznik</skos:prefLabel>
      <skos:definition xml:lang="sl">Katerikoli posameznik.</skos:definition>
      <skos:prefLabel xml:lang="lt">Asmuo</skos:prefLabel>
      <skos:definition xml:lang="lt">Bet kuris atskiras asmuo.</skos:definition>
      <skos:prefLabel xml:lang="sv">Individ</skos:prefLabel>
      <skos:definition xml:lang="sv">En enskild person.</skos:definition>
      <skos:prefLabel xml:lang="fi">Henkil&#xf6;</skos:prefLabel>
      <skos:definition xml:lang="fi">Tutkimuksen tarkastelukohteena ovat yksitt&#xe4;iset henkil&#xf6;t</skos:definition>
      <skos:prefLabel xml:lang="it">Individuo</skos:prefLabel>
      <skos:definition xml:lang="it">Qualsiasi persona.</skos:definition>
      <skos:prefLabel xml:lang="pt">Indiv&#xed;duo</skos:prefLabel>
      <skos:definition xml:lang="pt">Qualquer sujeito individual.</skos:definition>
      <skos:prefLabel xml:lang="en">Individual</skos:prefLabel>
      <skos:definition xml:lang="en">Any individual person.</skos:definition>
      <skos:prefLabel xml:lang="de">Individuum</skos:prefLabel>
      <skos:definition xml:lang="de">Jede einzelne Person, unabh&#xe4;ngig von demographischen Merkmalen, dem Beruf, dem sozialen Status oder Rechtsstatus.</skos:definition>
      <skos:prefLabel xml:lang="nl">Individueel</skos:prefLabel>
      <skos:definition xml:lang="nl"></skos:definition>
      <skos:prefLabel xml:lang="no">Individ</skos:prefLabel>
      <skos:definition xml:lang="no">Enhver individuell person.</skos:definition>
   </rdf:Description>
   <rdf:Description rdf:about="http://rdf-vocabulary.ddialliance.org/cv/AnalysisUnit/2.1.0/63eefb7">
      <rdf:type rdf:resource="http://www.w3.org/2004/02/skos/core#Concept"/>
      <skos:inScheme rdf:resource="http://rdf-vocabulary.ddialliance.org/cv/AnalysisUnit/2.1.0/"/>
      <skos:notation xml:lang="en">OrganizationOrInstitution</skos:notation>
      <skos:prefLabel xml:lang="sl">Organizacija/Institucija</skos:prefLabel>
      <skos:definition xml:lang="sl">Katerakoli formalna upravna in funkcionalna oblika ali vrsta organizacije - vklju&#x10d;uje zdru&#x17e;enja, institucije, agencije, podjetja, politi&#x10d;ne stranke, &#x161;ole itd. Podatki se zbirajo o organizacijah ali ustanovah, tudi &#x10d;e na vpra&#x161;anja odgovarjajo posamezniki. Na primer podatki o okoljski politiki podjetij, podatki o stopnjah vpisa ali diplome na nacionalnih univerzah itd.</skos:definition>
      <skos:prefLabel xml:lang="lt">Organizacija ar institucija</skos:prefLabel>
      <skos:definition xml:lang="lt">Bet kokia formali administracin&#x117; ir funkcin&#x117; strukt&#x16b;ra &#x2013; apima asociacijas, institucijas, agent&#x16b;ras, &#x12f;mones, politines partijas, mokyklas ir kt. Duomenys renkami apie organizacijas ar institucijas, net jei &#x12f; klausimus atsako individual&#x16b;s asmenys. Pavyzd&#x17e;iui, duomenys apie verslo aplinkosaugin&#x119; politik&#x105;, duomenys apie stojan&#x10d;i&#x173;j&#x173; ar absolvent&#x173; skai&#x10d;i&#x173; nacionaliniuose universitetuose ir kt.</skos:definition>
      <skos:prefLabel xml:lang="sv">Organisation/institution</skos:prefLabel>
      <skos:definition xml:lang="sv">En formell administrativ och funktionell struktur. Detta inkluderar f&#xf6;reningar, institutioner, myndigheter, f&#xf6;retag, politiska partier, skolor m.m. Data om organisationerna eller institutionerna samlas in &#xe4;ven om fr&#xe5;gorna besvaras av enskilda personer. Det g&#xe4;ller till exempel data om f&#xf6;retags milj&#xf6;policyer, data om antagningar eller examensfrekvens vid nationella universitet m.m.</skos:definition>
      <skos:prefLabel xml:lang="fi">Organisaatio</skos:prefLabel>
      <skos:definition xml:lang="fi">Mik&#xe4; tahansa hallinnollinen tai toiminnallinen organisaatio, esimerkiksi j&#xe4;rjest&#xf6;, koulu, instituutti, toimisto, yritys, poliittinen puolue, jne. Kysymykset kohdistuvat itse organisaatioon vaikka vastaajina ovatkin yksitt&#xe4;iset henkil&#xf6;t. Esimerkiksi tutkittaessa yritysten ymp&#xe4;rist&#xf6;politiikkaa tai korkeakouluista valmistuneiden m&#xe4;&#xe4;ri&#xe4; suhteessa opiskelijoihin jne.</skos:definition>
      <skos:prefLabel xml:lang="it">Organizzazione/Istituzione</skos:prefLabel>
      <skos:definition xml:lang="it">Qualsiasi tipo di struttura amministrativa e funzionale formale - incluse associazioni, istituzioni, agenzie, imprese, partiti politici, scuole, ecc. I dati raccolti si riferiscono alle organizzazioni o alle istituzioni, anche se le risposte alle domande sono fornite da singoli individui. Ad esempio, dati sulle politiche ambientali delle imprese, dati sui tassi di iscrizione o di laurea presso le universit&#xe0; nazionali, ecc.</skos:definition>
      <skos:prefLabel xml:lang="pt">Organiza&#xe7;&#xe3;o/Institui&#xe7;&#xe3;o</skos:prefLabel>
      <skos:definition xml:lang="pt">Qualquer tipo de estrutura funcional e administrativa formal. Inclui associa&#xe7;&#xf5;es, institui&#xe7;&#xf5;es, ag&#xea;ncias, empresas, partidos pol&#xed;ticos, escolas, etc. Os dados s&#xe3;o recolhidos sobre as organiza&#xe7;&#xf5;es e as institui&#xe7;&#xf5;es, mesmo que as quest&#xf5;es sejam respondidas por indiv&#xed;duos. Por exemplo, dados sobre pol&#xed;ticas ambientais nas empresas, dados sobre taxas de sucesso nas universidades nacionais, etc.</skos:definition>
      <skos:prefLabel xml:lang="en">Organization/Institution</skos:prefLabel>
      <skos:definition xml:lang="en">Any kind of formal administrative and functional structure - includes associations, institutions, agencies, businesses, political parties, schools, etc. The data are collected about the organizations or institutions, even if the questions are answered by individuals. For example, data on the environmental policies of businesses, data on enrollment or graduation rates at national universities, etc.</skos:definition>
      <skos:prefLabel xml:lang="de">Organisation/Institution</skos:prefLabel>
      <skos:definition xml:lang="de">Jede Art von formaler Verwaltungsstruktur und funktionaler Struktur - schlie&#xdf;t Verb&#xe4;nde, Institutionen, Agenturen, Unternehmen, politische Parteien, Schulen usw. ein. Die Daten werden &#xfc;ber die Organisationen oder Institutionen erhoben, auch wenn die Fragen von Individuen beantwortet werden. Zum Beispiel Daten zur Umweltpolitik von Unternehmen, Daten zu Immatrikulations- oder Absolventenquoten an Universit&#xe4;ten usw.</skos:definition>
      <skos:prefLabel xml:lang="nl">Organisatie/Instituut</skos:prefLabel>
      <skos:definition xml:lang="nl"></skos:definition>
      <skos:prefLabel xml:lang="no">Organisasjon/Institusjon</skos:prefLabel>
      <skos:definition xml:lang="no">Former for formelle administrative og funksjonelle strukturerer - inkluderer foreninger, institusjoner, foretak, bedrifter, politiske partier, skoler etc. Data er samlet om organisasjoner eller institusjoner selv om sp&#xf8;rsm&#xe5;lene er besvart av individer. For eksempel data om virksomheters milj&#xf8;politikk, data om opptak eller avgangsgrader ved nasjonale universitet, etc.</skos:definition>
   </rdf:Description>
   <rdf:Description rdf:about="http://rdf-vocabulary.ddialliance.org/cv/AnalysisUnit/2.1.0/cefc4f7">
      <rdf:type rdf:resource="http://www.w3.org/2004/02/skos/core#Concept"/>
      <skos:inScheme rdf:resource="http://rdf-vocabulary.ddialliance.org/cv/AnalysisUnit/2.1.0/"/>
      <skos:notation xml:lang="en">Family</skos:notation>
      <skos:prefLabel xml:lang="sl">Dru&#x17e;ina</skos:prefLabel>
      <skos:definition xml:lang="sl">Dva ali ve&#x10d; posameznikov, ki so medseboj sorodstveno povezani, ali z zakonsko oz. zunanjzakonsko partnersko zvezo (vklju&#x10d;uje tudi vzpostavljeno dru&#x17e;ino), ali s posvojitvijo ali z rejni&#x161;tvom. Ti posamezniki lahko &#x17e;ivijo skupaj ali pa ne (National Community Services Data Dictionary, Vers 3, AIHW, 2004). Na primer podatki o tem, kak&#x161;ne javne storitve dru&#x17e;ina uporablja ali bi jih potrebovala; ali kako pogosto so dru&#x17e;inski &#x10d;lani v medsebojnem stiku.</skos:definition>
      <skos:prefLabel xml:lang="lt">&#x160;eima</skos:prefLabel>
      <skos:definition xml:lang="lt">Kartu gyvenantys ar negyvenantys du ar daugiau &#x17e;moni&#x173;, kuriuos sieja kraujo ry&#x161;ys, santuoka (&#x12f;skaitant pat&#x117;vius, podukras, pos&#x16b;nius), bendro gyvenimo sutartis ar registruota partneryst&#x117;, &#x12f;vaikinimas ar globa. Pavyzd&#x17e;iui, duomenys apie tai, kokias vie&#x161;&#x105;sias paslaugas &#x161;eima naudoja ar nor&#x117;t&#x173; naudoti; arba kaip da&#x17e;nai &#x161;eimos nariai bendrauja tarpusavyje.</skos:definition>
      <skos:prefLabel xml:lang="sv">Familj</skos:prefLabel>
      <skos:definition xml:lang="sv">Tv&#xe5; eller fler personer som &#xe4;r sl&#xe4;kt genom blodsband, &#xe4;ktenskap (inklusive styvsyskon, -f&#xf6;r&#xe4;ldrar, -barn m.m.), samboskap eller registrerat partnerskap, adoption eller fosterfamiljeskap, men som inte n&#xf6;dv&#xe4;ndigtvis bor tillsammans. Till exempel data om vilka offentliga tj&#xe4;nster familjen anv&#xe4;nder eller skulle vara i behov av, eller hur ofta familjemedlemmar har kontakt med varandra.</skos:definition>
      <skos:prefLabel xml:lang="fi">Perhe</skos:prefLabel>
      <skos:definition xml:lang="fi">Kaksi tai useampia henkil&#xf6;it&#xe4;, jotka liittyv&#xe4;t toisiinsa sukulaisuuden, avo- tai avioliiton (laskien mukaan esim. sisar- ja velipuolet), rekister&#xf6;idyn parisuhteen, adoption tai sijaisvanhemmuuden kautta, riippumatta siit&#xe4;, asuvatko he yhdess&#xe4; vai eiv&#xe4;t. Esimerkiksi tutkittaessa mit&#xe4; julkisia palveluja perhe k&#xe4;ytt&#xe4;&#xe4;; tai kuinka usein perheenj&#xe4;senet ovat yhteydess&#xe4; toisiinsa.</skos:definition>
      <skos:prefLabel xml:lang="it">Famiglia</skos:prefLabel>
      <skos:definition xml:lang="it">Due o pi&#xf9; persone legate da vincolo di sangue, matrimonio (compresi i rapporti allargati), coabitazione o convivenza di fatto, adozione o affidamento che possono o meno vivere insieme. Ad esempio, dati sul tipo di servizi pubblici di cui la famiglia usufruisce o di cui avrebbe bisogno; oppure dati sulla frequenza con cui i membri della famiglia sono in contatto tra loro.</skos:definition>
      <skos:prefLabel xml:lang="pt">Fam&#xed;lia</skos:prefLabel>
      <skos:definition xml:lang="pt">Duas ou mais pessoas relacionadas por sangue, casamento (incluindo rela&#xe7;&#xf5;es de fam&#xed;lias recompostas), coabita&#xe7;&#xe3;o ou parentalidade registada, adop&#xe7;&#xe3;o ou guarda de crian&#xe7;as, e que podem ou n&#xe3;o viver juntas. Por exemplo, dados sobre que tipo de servi&#xe7;os p&#xfa;blicos as fam&#xed;lias usam ou poderiam requerer; ou sobre qu&#xe3;o frequentemente os membros duma fam&#xed;lia est&#xe3;o em contacto uns com os outros.</skos:definition>
      <skos:prefLabel xml:lang="en">Family</skos:prefLabel>
      <skos:definition xml:lang="en">Two or more people related by blood, marriage (including step-relations), co-habitation or registered partnership, adoption or fostering, and who may or may not live together. For example, data on what kind of public services the family uses or would require; or how often family members are in contact with each other.</skos:definition>
      <skos:prefLabel xml:lang="de">Familie</skos:prefLabel>
      <skos:definition xml:lang="de">Zwei oder mehr Menschen, die miteinander blutsverwandt sind, oder durch Heirat (einschlie&#xdf;lich der Verwandtschaft des Ehepartners), Adoption oder Pflege (Pflegeeltern, Pflegekinder etc.) anverwandt sind - unabh&#xe4;ngig davon, ob sie zusammenleben oder nicht. Zum Beispiel Daten dar&#xfc;ber, welche Art von &#xf6;ffentlichen Dienstleistungen die Familie nutzt oder ben&#xf6;tigen w&#xfc;rde; oder wie oft die Familienmitglieder miteinander in Kontakt stehen.</skos:definition>
      <skos:prefLabel xml:lang="nl">Familie</skos:prefLabel>
      <skos:definition xml:lang="nl"></skos:definition>
      <skos:prefLabel xml:lang="no">Familie</skos:prefLabel>
      <skos:definition xml:lang="no">To eller flere mennesker som er i slekt med blod, ekteskap (inkludert ste-relasjoner), samboerskap eller registrerte partnere, adopsjon eller fosterbarn som enten lever eller ikke lever sammen. For eksempel, data om hvilke typer offentlige tjenster familien bruker eller har behov for; eller hvor ofte familiemedlemmene er i kontakt med hverandre.</skos:definition>
      <skos:narrower rdf:resource="http://rdf-vocabulary.ddialliance.org/cv/AnalysisUnit/2.1.0/4a75b73"/>
   </rdf:Description>
   <rdf:Description rdf:about="http://rdf-vocabulary.ddialliance.org/cv/AnalysisUnit/2.1.0/4a75b73">
      <rdf:type rdf:resource="http://www.w3.org/2004/02/skos/core#Concept"/>
      <skos:inScheme rdf:resource="http://rdf-vocabulary.ddialliance.org/cv/AnalysisUnit/2.1.0/"/>
      <skos:notation xml:lang="en">Family.HouseholdFamily</skos:notation>
      <skos:prefLabel xml:lang="sl">Dru&#x17e;ina: dru&#x17e;ina znotraj gospodinjstva</skos:prefLabel>
      <skos:definition xml:lang="sl">Bolj dolo&#x10d;en izraz, nana&#x161;a se le na sorodnike (glej definicijo &quot;Dru&#x17e;ina&quot;), ki v dolo&#x10d;enem trenutku &#x17e;ivijo v istem gospodinjstvu. &#x10c;e ni znano, ali je enota analize &quot;Dru&#x17e;ina&quot; ali &quot;Dru&#x17e;ina znotraj gospodinjstva&quot;, uporabite izraz &quot;Dru&#x17e;ina&quot;.</skos:definition>
      <skos:prefLabel xml:lang="lt">&#x160;eima: &#x161;eiminis nam&#x173; &#x16b;kis</skos:prefLabel>
      <skos:definition xml:lang="lt">Konkretesnis terminas, nurodantis tik &#x17e;mones, kurie yra susij&#x119; &#x161;eimos ry&#x161;iais (&#x17e;r. apibr&#x117;&#x17e;im&#x105; &#x201e;&#x160;eima&#x201c;) ir tuo pa&#x10d;iu metu gyvena tame pa&#x10d;iame nam&#x173; &#x16b;kyje. Jei ne&#x17e;inoma, ar analiz&#x117;s vienetas yra &#x201e;&#x160;eima&#x201c;, ar &#x201e;&#x160;eimos nam&#x173; &#x16b;kis&#x201c;, naudoti &#x201e;&#x160;eima&#x201c;.</skos:definition>
      <skos:prefLabel xml:lang="sv">Familj: Familjehush&#xe5;ll</skos:prefLabel>
      <skos:definition xml:lang="sv">En mer specifik term &#xe4;n &quot;Familj&quot;. Betecknar endast m&#xe4;nniskor som &#xe4;r sl&#xe4;kt genom familjeband (se definitionen f&#xf6;r &quot;Familj&quot;) och som bor tillsammans i samma hush&#xe5;ll vid en given tidpunkt. Om det inte &#xe4;r k&#xe4;nt huruvida analysenheten &#xe4;r &quot;Familj&quot; eller &quot;Familjehush&#xe5;ll&quot; ska &quot;Familj&quot; anv&#xe4;ndas.</skos:definition>
      <skos:prefLabel xml:lang="fi">Perhe: perhekotitalous</skos:prefLabel>
      <skos:definition xml:lang="fi">Spesifimpi termi, joka viittaa kotitalouteen, jossa tietyll&#xe4; hetkell&#xe4; yhdess&#xe4; asuvat henkil&#xf6;t my&#xf6;s kuuluvat perheeseen (katso m&#xe4;&#xe4;ritelm&#xe4; termille &apos;Perhe&apos;). Jos ei tiedossa, onko kyseess&#xe4; &apos;Perhe&apos; vai &apos;Perhekotitalous&apos;, k&#xe4;yt&#xe4; &apos;Perhe&apos;.</skos:definition>
      <skos:prefLabel xml:lang="it">Famiglia: Famiglia convivente</skos:prefLabel>
      <skos:definition xml:lang="it">Un termine pi&#xf9; specifico che si riferisce solo a persone che sono legate da vincoli familiari (si veda la definizione di &quot;Famiglia&quot;) e che vivono nella stessa abitazione in un determinato momento. Se non &#xe8; possibile distinguere tra &quot;Famiglia&quot; e &quot;Famiglia convivente&quot; come unit&#xe0; di analisi, utilizzare &quot;Famiglia&quot;</skos:definition>
      <skos:prefLabel xml:lang="pt">Fam&#xed;lia: Agregado familiar</skos:prefLabel>
      <skos:definition xml:lang="pt">Termo mais espec&#xed;fico que se refere apenas a pessoas que est&#xe3;o relacionadas atrav&#xe9;s de liga&#xe7;&#xf5;es familiares (ver defini&#xe7;&#xe3;o de &apos;Fam&#xed;lia&apos;) e que moram no mesmo domic&#xed;lio em determinado momento. Se n&#xe3;o souber se a unidade de an&#xe1;lise &#xe9; &apos;Fam&#xed;lia&apos; ou &apos;Agregado familiar&apos;, usar &apos;Fam&#xed;lia&apos;.</skos:definition>
      <skos:prefLabel xml:lang="en">Family: Household family</skos:prefLabel>
      <skos:definition xml:lang="en">A more specific term that refers only to people who are related through family ties (see definition for &apos;Family&apos;) and live in the same household at a point in time. If not known whether the analysis unit is &apos;Family&apos; or &apos;Household family&apos;, use &apos;Family&apos;.</skos:definition>
      <skos:prefLabel xml:lang="de">Familie: Familienhaushalt</skos:prefLabel>
      <skos:definition xml:lang="de">Ein spezifischerer Begriff, der sich nur auf Personen bezieht, die durch famili&#xe4;re Bindungen miteinander verbunden sind (siehe Definition f&#xfc;r &quot;Familie&quot;) und zu einem bestimmten Zeitpunkt im selben Haushalt leben. Wenn nicht bekannt ist, ob die Analyseeinheit &quot;Familie&quot; oder &quot;Familienhaushalt&quot; ist, verwenden Sie &quot;Familie&quot;.</skos:definition>
      <skos:prefLabel xml:lang="nl">Gezin</skos:prefLabel>
      <skos:definition xml:lang="nl"></skos:definition>
      <skos:prefLabel xml:lang="no">Familie: familiehusholdning</skos:prefLabel>
      <skos:definition xml:lang="no">Et mer spesifikt begrep som kun referer til personer som er beslektet gjennom familierelasjoner (se definisjonen for &apos;Familie&apos;) og som bor i den samme husholdningen p&#xe5; et gitt tidspunkt. Om det ikke er kjent om analyseenheten er &apos;Familie&apos; eller &apos;Familiehusholdning&apos; skal begrepet &apos;Familie&apos; benyttes.</skos:definition>
   </rdf:Description>
   <rdf:Description rdf:about="http://rdf-vocabulary.ddialliance.org/cv/AnalysisUnit/2.1.0/ea4be67">
      <rdf:type rdf:resource="http://www.w3.org/2004/02/skos/core#Concept"/>
      <skos:inScheme rdf:resource="http://rdf-vocabulary.ddialliance.org/cv/AnalysisUnit/2.1.0/"/>
      <skos:notation xml:lang="en">Household</skos:notation>
      <skos:prefLabel xml:lang="sl">Gospodinjstvo</skos:prefLabel>
      <skos:definition xml:lang="sl">Oseba ali skupina oseb, ki si delijo isto stanovanjsko enoto in ureditev skupnega &#x17e;ivljenja. Te ureditve skupnega &#x17e;ivljenja lahko vklju&#x10d;ujejo zdru&#x17e;evanje nekaterih ali vseh prihodkov in premo&#x17e;enja ter skupno (u)porabo dolo&#x10d;enih vrst blaga in storitev, predvsem stanovanja in hrane (Eurostat).</skos:definition>
      <skos:prefLabel xml:lang="lt">Nam&#x173; &#x16b;kis</skos:prefLabel>
      <skos:definition xml:lang="lt">Asmuo ar asmen&#x173; grup&#x117;, kuri dalinasi tuo pa&#x10d;iu b&#x16b;sto vienetu ir bendra gyvenimo tvarka. &#x160;i bendro gyvenimo tvarka gali apimti kai kuri&#x173; arba vis&#x173; pajam&#x173; ir turto bendr&#x105; kaupim&#x105;, tam tikr&#x173; tip&#x173; preki&#x173; ir paslaug&#x173; vartojim&#x105;, da&#x17e;niausiai susijus&#x12f; su b&#x16b;stu ir maistu (pagal Eurostat&#x105;).</skos:definition>
      <skos:prefLabel xml:lang="sv">Hush&#xe5;ll</skos:prefLabel>
      <skos:definition xml:lang="sv">En person eller grupp av personer som delar bostad och levnadsf&#xf6;rh&#xe5;llanden. Dessa gemensamma levnadsf&#xf6;rh&#xe5;llanden kan inkludera att viss eller all inkomst och egendom &#xe4;r gemensam och att vissa sorters varor och tj&#xe4;nster konsumeras gemensamt, f&#xf6;retr&#xe4;delsevis bostad och mat (Eurostat).</skos:definition>
      <skos:prefLabel xml:lang="fi">Kotitalous</skos:prefLabel>
      <skos:definition xml:lang="fi">Kotitalouden muodostaa yksi henkil&#xf6; tai ryhm&#xe4; henkil&#xf6;it&#xe4;, jotka asuvat yhdess&#xe4; ja joilla on kokonaan tai osittain yhteinen ruokatalous tai jotka muuten k&#xe4;ytt&#xe4;v&#xe4;t tulojaan ja varallisuuttaan ainakin osittain yhdess&#xe4;.</skos:definition>
      <skos:prefLabel xml:lang="it">Conviventi</skos:prefLabel>
      <skos:definition xml:lang="it">Una persona o un gruppo di persone che condividono la stessa unit&#xe0; abitativa e le stesse modalit&#xe0; di vita comuni. Queste modalit&#xe0; di vita comuni possono includere la condivisione di alcuni oppure di tutti i redditi e ricchezze, e il consumo collettivo di determinati tipi di beni e servizi, principalmente alloggi e cibo (Eurostat)</skos:definition>
      <skos:prefLabel xml:lang="pt">Agregado dom&#xe9;stico</skos:prefLabel>
      <skos:definition xml:lang="pt">Uma pessoa ou um grupo de pessoas que compartilham a mesma unidade de habita&#xe7;&#xe3;o e vida em comum. Esta &#xfa;ltima pode incluir a agrega&#xe7;&#xe3;o de alguns ou de todos os rendimentos e riqueza e o consumo colectivo de certos tipos de bens e servi&#xe7;os, principalmente alojamento e alimenta&#xe7;&#xe3;o (Eurostat).</skos:definition>
      <skos:prefLabel xml:lang="en">Household</skos:prefLabel>
      <skos:definition xml:lang="en">A person or a group of persons who share the same dwelling unit and common living arrangements. These common living arrangements may include pooling some, or all, of their income and wealth, and consuming certain types of goods and services collectively, mainly housing and food (Eurostat).</skos:definition>
      <skos:prefLabel xml:lang="de">Haushalt</skos:prefLabel>
      <skos:definition xml:lang="de">Eine Person oder eine Gruppe von Personen, die dieselbe Wohneinheit und gemeinsame Wohnverh&#xe4;ltnisse teilen. Zu diesen gemeinsamen Wohnverh&#xe4;ltnissen kann es geh&#xf6;ren, dass sie einen Teil oder ihr gesamtes Einkommen und Verm&#xf6;gen zusammenlegen und bestimmte Arten von Waren und Dienstleistungen gemeinsam konsumieren, vor allem Wohnraum und Lebensmittel (Eurostat).</skos:definition>
      <skos:prefLabel xml:lang="nl">Huishouden</skos:prefLabel>
      <skos:definition xml:lang="nl"></skos:definition>
      <skos:prefLabel xml:lang="no">Husholdning</skos:prefLabel>
      <skos:definition xml:lang="no">En person eller en gruppe av personer som har samme boligenhet og leveforhold. Disse felles leveforholdene kan inkludere at deler av, eller alt av inntekt og eiendom er felles, og at visse type varer og tjenester konsumeres i fellesskap, hovedsakelig bosted og mat (Eurostat).</skos:definition>
   </rdf:Description>
   <rdf:Description rdf:about="http://rdf-vocabulary.ddialliance.org/cv/AnalysisUnit/2.1.0/4358d21">
      <rdf:type rdf:resource="http://www.w3.org/2004/02/skos/core#Concept"/>
      <skos:inScheme rdf:resource="http://rdf-vocabulary.ddialliance.org/cv/AnalysisUnit/2.1.0/"/>
      <skos:notation xml:lang="en">HousingUnit</skos:notation>
      <skos:prefLabel xml:lang="sl">Bivalna enota</skos:prefLabel>
      <skos:definition xml:lang="sl">Popis ZDA: Bivalna enota je hi&#x161;a, stanovanje, mobilna hi&#x161;ica, skupina sob ali enoposteljna soba, ki se uporablja kot lo&#x10d;en bivalni prostor (oziroma je v primeru, da je prazna, namenjena bivanju). Lo&#x10d;eni bivalni prostori so tisti, v katerih stanovalci &#x17e;ivijo in se prehranjujejo lo&#x10d;eno od drugih oseb v stavbi in imajo neposreden dostop do prostora pred stavbo ali do skupnega hodnika.</skos:definition>
      <skos:prefLabel xml:lang="lt">B&#x16b;sto vienetas</skos:prefLabel>
      <skos:definition xml:lang="lt">JAV visuotinis gyventoj&#x173; sura&#x161;ymas: b&#x16b;sto vienetas &#x2013; namas, butas, mobilus namelis, kambari&#x173; grup&#x117; arba atskiras kambarys, kuris yra u&#x17e;imtas (arba jei laisvas, tai skirtas apgyvendinimui), kaip atskira gyvenamoji patalpa. Atskiros gyvenamosios patalpos yra tokios, kuriose gyventojai gyvena bei valgo atskirai nuo kit&#x173; pastate esan&#x10d;i&#x173; asmen&#x173;, ir &#x12f; kurias galima tiesiogiai patekti i&#x161; pastato i&#x161;or&#x117;s arba per bendr&#x105; koridori&#x173;.</skos:definition>
      <skos:prefLabel xml:lang="sv">Bostadsenhet</skos:prefLabel>
      <skos:definition xml:lang="sv">En bostadsenhet &#xe4;r ett hus, en l&#xe4;genhet, en husvagn, eller ett eller flera rum som bebos (eller, om den &#xe4;r tom, &#xe4;r avsedd att bebos) som avskild inkvartering. Med avskild inkvartering menas att de som &#xe4;r inkvarterade d&#xe4;r bor och &#xe4;ter avskilda fr&#xe5;n andra personer i byggnaden och kan komma in direkt utifr&#xe5;n eller via en gemensam entr&#xe9; (U.S. Census).</skos:definition>
      <skos:prefLabel xml:lang="fi">Asuntokunta</skos:prefLabel>
      <skos:definition xml:lang="fi">Asuntokunta voi sijaita talossa, huoneistossa, asuntovaunussa, tai asunnon tietyss&#xe4; huoneessa tai huoneissa. Asuntokunnnan asuintilassa el&#xe4;vill&#xe4; henkil&#xf6;ill&#xe4; on oma erillinen ruokataloutensa ja j&#xe4;rjestelyns&#xe4;. Yhdess&#xe4; asunnossa voi olla useampia asuntokuntia. Esimerkiksi soluasunnoissa asuvilla opiskelijoilla voi kullakin olla oma ruoka- ja asuntokuntansa. Termi k&#xe4;yt&#xf6;ss&#xe4; etenkin Yhdysvalloissa.</skos:definition>
      <skos:prefLabel xml:lang="it">Unit&#xe0; abitativa</skos:prefLabel>
      <skos:definition xml:lang="it">Un&apos;unit&#xe0; abitativa &#xe8; una casa, un appartamento, una casa mobile, un gruppo di stanze o una stanza singola occupata (oppure, se non occupata, destinata ad ospitare) come abitazione separata. Le abitazioni separate sono quelli in cui gli occupanti vivono e mangiano separatamente da qualsiasi altra persona presente nell&apos;edificio, e che hanno un accesso diretto dall&apos;esterno dell&apos;edificio oppure attraverso un ingresso comune.</skos:definition>
      <skos:prefLabel xml:lang="pt">Unidade residencial</skos:prefLabel>
      <skos:definition xml:lang="pt">Censo dos EUA: Uma unidade residencial &#xe9; uma casa, um apartamento, uma casa m&#xf3;vel, um grupo de quartos ou um quarto individual que &#xe9; ocupado (ou, se for vago, destinado a ocupa&#xe7;&#xe3;o) enquanto alojamentos/aposentos separados. Alojamentos separados s&#xe3;o aqueles em que os ocupantes vivem e comem separadamente de quaisquer outras pessoas no edif&#xed;cio e que t&#xea;m acesso direto a partir do exterior do edif&#xed;cio ou atrav&#xe9;s de um hall comum.</skos:definition>
      <skos:prefLabel xml:lang="en">Housing unit</skos:prefLabel>
      <skos:definition xml:lang="en">U.S. Census: A housing unit is a house, an apartment, a mobile home, a group of rooms, or a single room that is occupied (or if vacant, is intended for occupancy) as separate living quarters. Separate living quarters are those in which the occupants live and eat separately from any other persons in the building and which have direct access from the outside of the building or through a common hall.</skos:definition>
      <skos:prefLabel xml:lang="de">Wohneinheit</skos:prefLabel>
      <skos:definition xml:lang="de">Eine Wohneinheit ist ein Haus, eine Wohnung, ein Wohnmobil, eine Gruppe von R&#xe4;umen oder ein einzelner Raum, der als separater Wohnbereich genutzt wird (oder, wenn er leer steht, zur Nutzung vorgesehen ist). Geschlossene Wohneinheiten sind solche, in denen die Bewohner getrennt von allen anderen Personen im Geb&#xe4;ude leben und essen und die einen direkten Zugang von der Au&#xdf;enseite des Geb&#xe4;udes oder durch einen gemeinsamen Flur haben.</skos:definition>
      <skos:prefLabel xml:lang="nl">Wooneenheid</skos:prefLabel>
      <skos:definition xml:lang="nl"></skos:definition>
      <skos:prefLabel xml:lang="no">Boenhet</skos:prefLabel>
      <skos:definition xml:lang="no">USAs folketelling: En boenhet er et hus, en leilighet, et mobilt hjem (campingvogn), eller ett eller flere rom som er bebodd (eventuelt ledig, men som er ment &#xe5; v&#xe6;re bebodd), som adskilte enheter. Med adskilte enheter menes det at personer bor og spiser uavhengig av andre personer i samme boenhet, og som har direkte tilgang til enheten utenfra, eller gjennom en felles inngang.</skos:definition>
   </rdf:Description>
   <rdf:Description rdf:about="http://rdf-vocabulary.ddialliance.org/cv/AnalysisUnit/2.1.0/fa83853">
      <rdf:type rdf:resource="http://www.w3.org/2004/02/skos/core#Concept"/>
      <skos:inScheme rdf:resource="http://rdf-vocabulary.ddialliance.org/cv/AnalysisUnit/2.1.0/"/>
      <skos:notation xml:lang="en">EventOrProcessOrActivity</skos:notation>
      <skos:prefLabel xml:lang="sl">Dogodek/proces/dejavnost</skos:prefLabel>
      <skos:definition xml:lang="sl">Katerakoli vrsta dogodka, pojava ali dejavnosti. Dogodki so obi&#x10d;ajno enkratni, posamezni pojavi, omejenega ali kratkega trajanja. Primeri: kazniva dejanja, neredi, sestanki, volitve, &#x161;portna tekmovanja, teroristi&#x10d;ni napadi, naravne nesre&#x10d;e, kot so poplave ipd. Procesi obi&#x10d;ajno potekajo dalj &#x10d;asa in lahko vklju&#x10d;ujejo ve&#x10d; &quot;dogodkov&quot; ali postopnih sprememb, ki na koncu vodijo ali bodo predvidoma vodili do dolo&#x10d;enega rezultata. Primeri: sodni postopki, kazenske preiskave, politi&#x10d;ne kampanje, zdravljenje, izobra&#x17e;evanje, &#x161;portni trening itd. Uporabite, kadar je glavni poudarek bolj na dogodku, postopku ali sami dejavnosti. Na primer terenska raziskava z opazovanjem igranja na sre&#x10d;o na igralnih avtomatih; ali zbrani podatki o primerih zlorabe otrok, kot so vrsta in trajanje zlorabe, vloga vpletenih oseb itd.</skos:definition>
      <skos:prefLabel xml:lang="lt">&#x12e;vykis, procesas ar veikla</skos:prefLabel>
      <skos:definition xml:lang="lt">Bet kokio tipo atsitikimas, atvejis ar veikla. &#x12e;vykiai paprastai b&#x16b;na vienkartiniai, atskiri, ribotos arba trumpos trukm&#x117;s. Pavyzd&#x17e;iai: nusikalstamos veikos, riau&#x161;&#x117;s, susitikimai, rinkimai, sporto var&#x17e;ybos, teroristiniai i&#x161;puoliai, stichin&#x117;s nelaim&#x117;s (pvz.  potvyniai) ir kt. Procesai paprastai vyksta tam tikr&#x105; laik&#x105; ir gali apimti kelis &#x201e;&#x12f;vykius&#x201c; ar laipsni&#x161;kus poky&#x10d;ius, kurie gal&#x173; gale lemia arba, kaip tikimasi, veda prie konkretaus rezultato. Pavyzd&#x17e;iai: teismo procesai, kriminaliniai tyrimai, politin&#x117;s kampanijos, medicininis gydymas, ugdymas, sportinink&#x173; rengimas ir kt. Naudoti, kai pagrindinis d&#x117;mesys skiriamas labiau pa&#x10d;iam &#x12f;vykiui, procesui ar veiklai. Pavyzd&#x17e;iui, lauko steb&#x117;jimo tyrimas apie lo&#x161;im&#x105; &#x17e;aidim&#x173; automatais; arba duomen&#x173; rinkimas apie vaik&#x173; i&#x161;naudojimo atvejus, pvz. i&#x161;naudojimo r&#x16b;&#x161;is ir trukm&#x119;, dalyvaujan&#x10d;i&#x173; asmen&#x173; vaidmenis ir kt.</skos:definition>
      <skos:prefLabel xml:lang="sv">H&#xe4;ndelse/process/aktivitet</skos:prefLabel>
      <skos:definition xml:lang="sv">En f&#xf6;reteelse, tilldragelse eller aktivitet. H&#xe4;ndelser &#xe4;r vanligtvis enstaka f&#xf6;reteelser med begr&#xe4;nsad eller kort varaktighet. Exempel: brott, upplopp, m&#xf6;ten, val, idrottst&#xe4;vlingar, terroristangrepp, naturkatastrofer som &#xf6;versv&#xe4;mningar o.dyl. Processer utspelar sig vanligtvis &#xf6;ver tid och kan omfatta flera &quot;h&#xe4;ndelser&quot; eller gradvisa f&#xf6;r&#xe4;ndringar som slutligen resulterar i, eller kan t&#xe4;nkas resultera i, en viss utg&#xe5;ng. Exempel: r&#xe4;tteg&#xe5;ngar, brottsutredningar, politiska kampanjer, medicinska behandlingar, utbildning, en idrottsut&#xf6;vares tr&#xe4;ning, m.m. Anv&#xe4;nd detta begrepp n&#xe4;r fokus ligger p&#xe5; sj&#xe4;lva h&#xe4;ndelsen, processen eller aktiviteten. Till exempel en f&#xe4;ltobservationsstudie om spel p&#xe5; spelautomater; eller data om fall av &#xf6;vergrepp p&#xe5; barn, som typ av och varaktighet f&#xf6;r &#xf6;vergreppet, de inblandade personernas roller osv.</skos:definition>
      <skos:prefLabel xml:lang="fi">Tapahtuma/prosessi/toiminta</skos:prefLabel>
      <skos:definition xml:lang="fi">Tapahtuma, tapahtumasarja, toiminta tai prosessi. Tapahtumat ovat usein lyhytaikaisia ja kertaluonteisia, esimerkiksi mellakat, kokoukset, urheilukilpailut, terroristihy&#xf6;kk&#xe4;ykset ja luonnonkatastrofit. Prosessit ovat tyypillisesti pidempikestoisia, voivat sis&#xe4;lt&#xe4;&#xe4; useampia tapahtumia tai v&#xe4;hitt&#xe4;isi&#xe4; muutoksia, jotka lopuksi johtavat tiettyyn tulokseen. Esimerkiksi oikeusjutut, rikostutkimukset, poliittiset kampanjat, kuntoutushoidot, koulutus. Tapahtuma/prosessi/toiminta -termi&#xe4; k&#xe4;ytet&#xe4;&#xe4;n silloin, kun tutkimuksessa keskityt&#xe4;&#xe4;n kyseiseen tapahtumaan, prosessiin tai toimintaan, ei henkil&#xf6;ihin sin&#xe4;ns&#xe4;. Esimerkiksi havainnointitutkimus peliautomaattipelaamisesta; tutkimus lasten pahoinpitelytapauksista, niiden tyypist&#xe4; ja kestosta, osallistuvien henkil&#xf6;iden roolista niiss&#xe4;.</skos:definition>
      <skos:prefLabel xml:lang="it">Evento/Processo/Attivit&#xe0;</skos:prefLabel>
      <skos:definition xml:lang="it">Qualsiasi tipo di episodio, evento o attivit&#xe0;. Gli eventi sono generalmente occorrenze singole, con una durata limitata oppure breve. Esempi: reati, rivolte, riunioni, elezioni, competizioni sportive, attacchi terroristici, calamit&#xe0; naturali come inondazioni, ecc. I processi generalmente durano nel tempo, e possono includere &quot;eventi&quot; multipli o cambiamenti graduali che alla fine conducono, oppure tendono a condurre, a un risultato particolare. Esempi: processi giudiziari, indagini penali, campagne politiche, trattamenti sanitari, istruzione, allenamenti sportivi, ecc. Utilizzare quando l&apos;attenzione &#xe8; riposta principalmente sull&apos;evento, sul processo o sull&apos;attivit&#xe0; stessa. Ad esempio, uno studio che prevede un&apos;osservazione sul campo relativa al gioco d&apos;azzardo attraverso slot machine; oppure dati raccolti su casi di abuso su minori, come il tipo e la durata dell&apos;abuso, il ruolo delle persone coinvolte, ecc.</skos:definition>
      <skos:prefLabel xml:lang="pt">Evento/Processo/Atividade</skos:prefLabel>
      <skos:definition xml:lang="pt">Qualquer tipo de incidente, ocorr&#xea;ncia ou atividade. Os eventos s&#xe3;o geralmente ocorr&#xea;ncias &#xfa;nicas e isoladas, com dura&#xe7;&#xe3;o limitada ou curta. Exemplos: infra&#xe7;&#xf5;es criminais, tumultos, reuni&#xf5;es, elei&#xe7;&#xf5;es, competi&#xe7;&#xf5;es desportivas, ataques terroristas, desastres naturais como inunda&#xe7;&#xf5;es, etc. Os processos geralmente ocorrem ao longo do tempo e podem incluir m&#xfa;ltiplos &apos;eventos&apos; ou mudan&#xe7;as graduais que conduzem ou podem conduzir a um resultado particular. Exemplos: julgamentos em tribunal, investiga&#xe7;&#xf5;es criminais, campanhas pol&#xed;ticas, tratamentos m&#xe9;dicos, educa&#xe7;&#xe3;o, forma&#xe7;&#xe3;o de atletas, etc. Usar quando o principal foco &#xe9; mais no evento, processo ou atividade. Por exemplo, um estudo de observa&#xe7;&#xe3;o no terreno sobre m&#xe1;quinas autom&#xe1;ticas de jogos; ou dados recolhidos sobre casos de abuso de crian&#xe7;as, como o tipo e a dura&#xe7;&#xe3;o do abuso, o papel das pessoas envolvidas, etc.</skos:definition>
      <skos:prefLabel xml:lang="en">Event/Process/Activity</skos:prefLabel>
      <skos:definition xml:lang="en">Any type of incident, occurrence, or activity. Events are usually one-time, individual occurrences, with a limited or short duration. Examples: criminal offenses, riots, meetings, elections, sports competitions, terrorist attacks, natural disasters like floods, etc. Processes typically take place over time, and may include multiple &apos;events&apos; or gradual changes that ultimately lead, or are projected to lead, to a particular result. Examples: court trials, criminal investigations, political campaigns, medical treatments, education, athletes&apos; training, etc. Use when the main focus is more on the event, process or activity itself. For example, a field observation study on slot machine gambling; or data collected on child abuse cases, such as the type and duration of abuse, the role of the persons involved, etc.</skos:definition>
      <skos:prefLabel xml:lang="de">Ereignis/Prozess/Aktivit&#xe4;t</skos:prefLabel>
      <skos:definition xml:lang="de">Jede Art von Vorfall, Vorkommnis oder Aktivit&#xe4;t. Ereignisse sind in der Regel einmalige, individuelle Vorkommnisse, mit einer begrenzten oder kurzen Dauer. Beispiele: Straftaten, Unruhen, Versammlungen, Wahlen, Sportwettk&#xe4;mpfe, Terroranschl&#xe4;ge, Naturkatastrophen wie &#xdc;berschwemmungen usw. Prozesse finden typischerweise im Laufe der Zeit statt und k&#xf6;nnen mehrere &quot;Ereignisse&quot; oder allm&#xe4;hliche Ver&#xe4;nderungen umfassen, die letztendlich zu einem bestimmten Ergebnis f&#xfc;hren oder f&#xfc;hren sollen. Beispiele: Gerichtsverhandlungen, strafrechtliche Ermittlungen, politische Kampagnen, medizinische Behandlungen, Bildung, Training von Sportlern usw. Der Begriff wird verwendet, wenn das Hauptaugenmerk eher auf dem Ereignis, dem Prozess oder der Aktivit&#xe4;t selbst liegt. Beispiele: eine Feldbeobachtungsstudie zum Gl&#xfc;cksspiel an Spielautomaten.</skos:definition>
      <skos:prefLabel xml:lang="nl">Event/Proces/Activteit</skos:prefLabel>
      <skos:definition xml:lang="nl"></skos:definition>
      <skos:prefLabel xml:lang="no">Hendelse/prosess/aktivitet</skos:prefLabel>
      <skos:definition xml:lang="no">Enhver form for hendelse, begivenhet eller aktivitet. Hendelser er som oftest enkeltst&#xe5;ende med begrenset eller kort varighet. For eksempel: kriminell handling, oppt&#xf8;yer, m&#xf8;ter, valg, idrettsbegivenheter, terroristangrep, naturkatastrofer osv. Prosesser finner som regel sted over tid, og kan inkludere flere &apos;hendelser&apos; eller gradvise endringer som etterhvert f&#xf8;rer til, eller er ansl&#xe5;tt &#xe5; f&#xf8;re til, et bestemt resultat. For eksempel: rettsaker, kriminaletterforskning, politiske kampanjer, medisinsk behandling, utdanning, idrettsut&#xf8;veres treninger etc. Bruk n&#xe5;r selve fokuset er mer p&#xe5; hendelsen, prosessen eller aktiviteten. For eksempel: feltobservasjonsstudie p&#xe5; spillemaskiner; eller data samlet inn om barnemishandlingssaker, med hensyn til type og varigheten til mishandlingen og rollen personer involvert har etc.</skos:definition>
   </rdf:Description>
   <rdf:Description rdf:about="http://rdf-vocabulary.ddialliance.org/cv/AnalysisUnit/2.1.0/435eb71">
      <rdf:type rdf:resource="http://www.w3.org/2004/02/skos/core#Concept"/>
      <skos:inScheme rdf:resource="http://rdf-vocabulary.ddialliance.org/cv/AnalysisUnit/2.1.0/"/>
      <skos:notation xml:lang="en">GeographicUnit</skos:notation>
      <skos:prefLabel xml:lang="sl">Geografska enota</skos:prefLabel>
      <skos:definition xml:lang="sl">Vsaka enota, ki je prostorsko opredeljena kot geografsko obmo&#x10d;je z naravnimi (fizi&#x10d;nimi) ali administrativnimi mejami. Na primer podatki o prodaji nepremi&#x10d;nin, spremembah krajine, novogradnjah ali demografski sestavi nekaterih regij ali okro&#x17e;ij.</skos:definition>
      <skos:prefLabel xml:lang="lt">Geografinis vienetas</skos:prefLabel>
      <skos:definition xml:lang="lt">Bet kuris objektas, kuris gali b&#x16b;ti apibr&#x117;&#x17e;tas geografine teritorija, turin&#x10d;ia nat&#x16b;ralias (fizines) arba administracines ribas. Pavyzd&#x17e;iui, duomenys apie nam&#x173; pardavimus, kra&#x161;tovaizd&#x17e;io poky&#x10d;ius, naujus statinius ar demografin&#x117;s sud&#x117;ties poky&#x10d;ius tam tikruose regionuose ar rajonuose.</skos:definition>
      <skos:prefLabel xml:lang="sv">Geografisk enhet</skos:prefLabel>
      <skos:definition xml:lang="sv">En enhet som kan definieras spatialt som ett geografiskt omr&#xe5;de med antingen naturliga (fysiska) eller administrativa gr&#xe4;nser. Till exempel data om husf&#xf6;rs&#xe4;ljning, landskapsf&#xf6;r&#xe4;ndringar, nybyggen eller f&#xf6;r&#xe4;ndringar av den demografiska sammans&#xe4;ttningen i vissa regioner eller distrikt.</skos:definition>
      <skos:prefLabel xml:lang="fi">Maantieteellinen yksikk&#xf6;</skos:prefLabel>
      <skos:definition xml:lang="fi">Mik&#xe4; tahansa maantieteellisesti m&#xe4;&#xe4;ritelt&#xe4;viss&#xe4; oleva alue, jolla on joko luontaiset fyysiset rajat tai hallinnolliset rajat. Esimerkiksi muutokset tiettyjen alueiden v&#xe4;est&#xf6;ss&#xe4; tai asuntojen myyntiluvut tai rakennusluvat tietyll&#xe4; alueella.</skos:definition>
      <skos:prefLabel xml:lang="it">Unit&#xe0; geografica</skos:prefLabel>
      <skos:definition xml:lang="it">Qualsiasi entit&#xe0; che possa essere definita nello spazio, come un&apos;area geografica, con confini naturali (fisici) o amministrativi. Ad esempio, i dati sulle vendite di case, sui mutamenti del paesaggio, sulle nuove costruzioni o sui cambiamenti nella composizione demografica di alcune regioni o distretti territoriali.</skos:definition>
      <skos:prefLabel xml:lang="pt">Unidade geogr&#xe1;fica</skos:prefLabel>
      <skos:definition xml:lang="pt">Qualquer entidade que possa ser definida espacialmente como uma &#xe1;rea geogr&#xe1;fica, com limites naturais (f&#xed;sicos) ou administrativos. Por exemplo, dados sobre venda de casas, mudan&#xe7;as paisag&#xed;sticas, novas constru&#xe7;&#xf5;es, ou mudan&#xe7;as na composi&#xe7;&#xe3;o demogr&#xe1;fica de certas regi&#xf5;es ou distritos.</skos:definition>
      <skos:prefLabel xml:lang="en">Geographic unit</skos:prefLabel>
      <skos:definition xml:lang="en">Any entity that can be spatially defined as a geographic area, with either natural (physical) or administrative boundaries. For example, data on home sales, landscaping changes, new constructions, or changes in the demographic composition of certain regions or districts.</skos:definition>
      <skos:prefLabel xml:lang="de">Geographische Einheit</skos:prefLabel>
      <skos:definition xml:lang="de">Jede Einheit, die r&#xe4;umlich als ein geographisches Gebiet definiert werden kann, entweder mit nat&#xfc;rlichen (physischen) oder administrativen Grenzen. Zum Beispiel Daten &#xfc;ber Hausverk&#xe4;ufe, Landschaftsver&#xe4;nderungen, Neubauten oder Ver&#xe4;nderungen in der demographischen Zusammensetzung bestimmter Regionen oder Bezirke.</skos:definition>
      <skos:prefLabel xml:lang="nl">Geografische eenheid</skos:prefLabel>
      <skos:definition xml:lang="nl"></skos:definition>
      <skos:prefLabel xml:lang="no">Geografisk enhet</skos:prefLabel>
      <skos:definition xml:lang="no">Enhver enhet som romlig kan defineres som et geografisk omr&#xe5;de, med enten naturlige (fysiske) eller administrative grenser. For eksempel: data om boligsalg, landskapsforandringer, nye konstruksjoner eller endringer i den demografiske sammensetningen i bestemte regioner eller distrikter.</skos:definition>
   </rdf:Description>
   <rdf:Description rdf:about="http://rdf-vocabulary.ddialliance.org/cv/AnalysisUnit/2.1.0/75fa5c6">
      <rdf:type rdf:resource="http://www.w3.org/2004/02/skos/core#Concept"/>
      <skos:inScheme rdf:resource="http://rdf-vocabulary.ddialliance.org/cv/AnalysisUnit/2.1.0/"/>
      <skos:notation xml:lang="en">PoliticalAdministrativeArea</skos:notation>
      <skos:prefLabel xml:lang="sl">Politi&#x10d;no-upravno obmo&#x10d;je</skos:prefLabel>
      <skos:definition xml:lang="sl">Geografsko obmo&#x10d;je, ki ga vodi suverena oblast, ki ima lastno pristojnost za sprejemanje upravnih ali politi&#x10d;nih odlo&#x10d;itev za to obmo&#x10d;je. To vklju&#x10d;uje nadnacionalna obmo&#x10d;ja (npr. zveze dr&#x17e;av, kot je Evropska unija), nacionalna (npr. posamezne dr&#x17e;avne uprave ali dr&#x17e;ave), podnacionalna (npr. upravna podobmo&#x10d;ja, kot so zvezne dr&#x17e;ave, province itd.) In lokalna (npr. ob&#x10d;ine).</skos:definition>
      <skos:prefLabel xml:lang="lt">Politin&#x117; administracin&#x117; teritorija</skos:prefLabel>
      <skos:definition xml:lang="lt">Geografin&#x117; teritorija valdoma suverenios vald&#x17e;ios, kuri turi gali&#x105; joje priimti administracinius ar politinius sprendimus. Tai apima vir&#x161;nacionalin&#x12f; (pavyzd&#x17e;iui, valstybi&#x173; s&#x105;jungos, kaip Europos S&#x105;junga), nacionalin&#x12f; (pavyzd&#x17e;iui, atskiros valstyb&#x117;s ar &#x161;alys), regionin&#x12f; (pavyzd&#x17e;iui, administraciniai vienetai, kaip federalin&#x117;s &#x17e;em&#x117;s, provincijos, apskritys ir kt.) ir vietos (pavyzd&#x17e;iui, savivaldybi&#x173;) lygmenis.</skos:definition>
      <skos:prefLabel xml:lang="sv">Politiskt f&#xf6;rvaltningsomr&#xe5;de</skos:prefLabel>
      <skos:definition xml:lang="sv">Ett geografiskt omr&#xe5;de som styrs av en best&#xe4;mmande myndighet med makt att fatta administrativa eller politiska beslut f&#xf6;r omr&#xe5;det. Detta inkluderar omr&#xe5;den p&#xe5; &#xf6;verstatlig (t.ex. unioner av stater som EU), statlig (t.ex. delstater eller l&#xe4;nder), subnationell/regional (t.ex. f&#xf6;rvaltningsomr&#xe5;den som federala delstater, provinser osv.) och lokal (t.ex. kommuner) niv&#xe5;.</skos:definition>
      <skos:prefLabel xml:lang="fi">Poliittis-hallinnollinen alue</skos:prefLabel>
      <skos:definition xml:lang="fi">Maantieteellinen alue, jota hallinnoivilla viranomaisilla tai p&#xe4;&#xe4;t&#xe4;nt&#xe4;elimill&#xe4; on oikeus tehd&#xe4; aluetta koskevia hallinnollisia tai poliittisia p&#xe4;&#xe4;t&#xf6;ksi&#xe4;. Sis&#xe4;lt&#xe4;&#xe4; ylikansalliset (esim. Euroopan unioni), kansalliset (esim. valtiot), maansis&#xe4;iset (esim. maakunnat) ja paikalliset (esim. kunnat) alueet.</skos:definition>
      <skos:prefLabel xml:lang="it">Area politico-amministrativa</skos:prefLabel>
      <skos:definition xml:lang="it">Un&apos;area geografica governata da un&apos;autorit&#xe0; che ha il potere di prendere decisioni amministrative o politiche relative a quell&apos;area. Comprende aree a livello sovranazionale (ad esempio unioni di stati come l&apos;Unione Europea), nazionale (ad esempio singoli stati o paesi), subnazionale (ad esempio suddivisioni amministrative come stati federali, province, ecc.), e locale (ad esempio comuni).</skos:definition>
      <skos:prefLabel xml:lang="pt">&#xc1;rea pol&#xed;tico-administrativa</skos:prefLabel>
      <skos:definition xml:lang="pt">Uma &#xe1;rea geogr&#xe1;fica governada por autoridade soberana que tem o poder de tomar decis&#xf5;es pol&#xed;ticas ou administrativas para aquela &#xe1;rea. Isto inclui &#xe1;reas ao n&#xed;vel supranacional (por exemplo, uni&#xf5;es de v&#xe1;rios estados como a Uni&#xe3;o Europeia), nacional (por exemplo, estados individuais ou pa&#xed;ses), subnacional (por exemplo, subdivis&#xf5;es administrativas como estados federais, prov&#xed;ncias, etc.), e local (por exemplo, munic&#xed;pios).</skos:definition>
      <skos:prefLabel xml:lang="en">Political-administrative area</skos:prefLabel>
      <skos:definition xml:lang="en">A geographical area governed by a sovereign authority that has the power to take administrative or policy decisions for that area. This includes&#xa0;areas at the supranational (e.g., unions of states like the European Union),  national (e.g., individual states or countries), sub-national (e.g., administrative subdivisions like federal states, provinces, etc.), and local (e.g., municipalities) levels.</skos:definition>
      <skos:prefLabel xml:lang="de">Politisch-administratives Gebiet</skos:prefLabel>
      <skos:definition xml:lang="de">Ein geographisches Gebiet, das von einer souver&#xe4;nen Staatsgewalt regiert wird, die die Befugnis hat, administrative oder politische Entscheidungen f&#xfc;r dieses Gebiet zu treffen. Dazu geh&#xf6;ren Gebiete auf supranationaler (z. B. Staatenb&#xfc;nde wie die Europ&#xe4;ische Union), nationaler (z. B. einzelne Staaten oder L&#xe4;nder), subnationaler (z. B. Verwaltungsgliederungen wie Bundesl&#xe4;nder, Provinzen usw.) und lokaler (z. B. Gemeinden) Ebene.</skos:definition>
      <skos:prefLabel xml:lang="nl">Poltiek administratief gebied</skos:prefLabel>
      <skos:definition xml:lang="nl"></skos:definition>
      <skos:prefLabel xml:lang="no">Politisk administrativt omr&#xe5;de</skos:prefLabel>
      <skos:definition xml:lang="no">Et geografisk omr&#xe5;de styrt av en suveren myndighet som har makten til beslutte administrative eller politiske avgj&#xf8;relser for det omr&#xe5;det. Dette inkluderer omr&#xe5;der p&#xe5; overstatlig (f.eks sammenslutninger av stater som Den Europeiske Union), nasjonalt (f.eks individuelle stater eller land), subnasjonalt (f.eks administrative oppdelinger som f&#xf8;derale stater, provinser etc.) og lokalt (f.eks kommuner) niv&#xe5;.</skos:definition>
   </rdf:Description>
   <rdf:Description rdf:about="http://rdf-vocabulary.ddialliance.org/cv/AnalysisUnit/2.1.0/8b62b80">
      <rdf:type rdf:resource="http://www.w3.org/2004/02/skos/core#Concept"/>
      <skos:inScheme rdf:resource="http://rdf-vocabulary.ddialliance.org/cv/AnalysisUnit/2.1.0/"/>
      <skos:notation xml:lang="en">TimeUnit</skos:notation>
      <skos:prefLabel xml:lang="sl">&#x10c;asovna enota</skos:prefLabel>
      <skos:definition xml:lang="sl">Katerokoli &#x10d;asovno obdobje: leto, teden, mesec, dan, dvomese&#x10d;no ali &#x10d;etrtletno obdobje itd.</skos:definition>
      <skos:prefLabel xml:lang="lt">Laiko vienetas</skos:prefLabel>
      <skos:definition xml:lang="lt">Bet koks laikotarpis: metai, savait&#x117;, m&#x117;nuo, diena, du m&#x117;nesiai, ketvirtis ir kt.</skos:definition>
      <skos:prefLabel xml:lang="sv">Tidsenhet</skos:prefLabel>
      <skos:definition xml:lang="sv">En tidsperiod: &#xe5;r, m&#xe5;nad, vecka, dag, kvartal, tv&#xe5;m&#xe5;nadersperiod osv.</skos:definition>
      <skos:prefLabel xml:lang="fi">Aikajakso</skos:prefLabel>
      <skos:definition xml:lang="fi">Mink&#xe4; mittainen aikajakso tahansa: sekunti, tunti, vuorokausi, viikko, kuukausi, vuosi yms.</skos:definition>
      <skos:prefLabel xml:lang="it">Unit&#xe0; temporale</skos:prefLabel>
      <skos:definition xml:lang="it">Qualsiasi periodo di tempo: anno, settimana, mese, giorno, bimestre, trimestre, ecc.</skos:definition>
      <skos:prefLabel xml:lang="pt">Unidade de tempo</skos:prefLabel>
      <skos:definition xml:lang="pt">Qualquer per&#xed;odo de tempo: ano, semana, m&#xea;s, dia, ou per&#xed;odos bimestrais ou trimestrais, etc.</skos:definition>
      <skos:prefLabel xml:lang="en">Time unit</skos:prefLabel>
      <skos:definition xml:lang="en">Any period of time: year, week, month, day, or bimonthly or quarterly periods, etc.</skos:definition>
      <skos:prefLabel xml:lang="de">Zeiteinheit</skos:prefLabel>
      <skos:definition xml:lang="de">Beliebiger Zeitraum: Jahr, Woche, Monat, Tag, oder zweimonatliche oder viertelj&#xe4;hrliche Zeitr&#xe4;ume, usw.</skos:definition>
      <skos:prefLabel xml:lang="nl">Tijdseenheid</skos:prefLabel>
      <skos:definition xml:lang="nl"></skos:definition>
      <skos:prefLabel xml:lang="no">Tidsenhet</skos:prefLabel>
      <skos:definition xml:lang="no">Tidsperiode: &#xe5;r, uke, m&#xe5;ned, dag, annenhver m&#xe5;ned eller kvartal etc.</skos:definition>
   </rdf:Description>
   <rdf:Description rdf:about="http://rdf-vocabulary.ddialliance.org/cv/AnalysisUnit/2.1.0/9658ae5">
      <rdf:type rdf:resource="http://www.w3.org/2004/02/skos/core#Concept"/>
      <skos:inScheme rdf:resource="http://rdf-vocabulary.ddialliance.org/cv/AnalysisUnit/2.1.0/"/>
      <skos:notation xml:lang="en">MediaUnit</skos:notation>
      <skos:prefLabel xml:lang="sl">Medijska enota</skos:prefLabel>
      <skos:definition xml:lang="sl">Enota, ki vsebuje dolo&#x10d;eno multimedijsko vsebino: besedilo, mirujo&#x10d;o sliko, posnetek in zvok.</skos:definition>
      <skos:prefLabel xml:lang="lt">Medijos vienetas</skos:prefLabel>
      <skos:definition xml:lang="lt">Apima tekstus, statinius vaizdus, vaizdo ir garso &#x12f;ra&#x161;us.</skos:definition>
      <skos:prefLabel xml:lang="sv">Mediaenhet</skos:prefLabel>
      <skos:definition xml:lang="sv">Inkluderar text, stillbilder, video och ljud.</skos:definition>
      <skos:prefLabel xml:lang="fi">Mediatyyppi (teksti, &#xe4;&#xe4;ni, still-kuva, liikkuva kuva)</skos:prefLabel>
      <skos:definition xml:lang="fi">Sis&#xe4;lt&#xe4;&#xe4; teksti-, kuva- ja &#xe4;&#xe4;nimuodossa olevan viestinn&#xe4;n.</skos:definition>
      <skos:prefLabel xml:lang="it">Unit&#xe0; di supporto</skos:prefLabel>
      <skos:definition xml:lang="it">Include testi, immagini, video e suoni.</skos:definition>
      <skos:prefLabel xml:lang="pt">Unidade de Media</skos:prefLabel>
      <skos:definition xml:lang="pt">Inclui texto, imagem, v&#xed;deo e som.</skos:definition>
      <skos:prefLabel xml:lang="en">Media unit</skos:prefLabel>
      <skos:definition xml:lang="en">Includes text, still image, video and sound.</skos:definition>
      <skos:prefLabel xml:lang="de">Medieneinheit</skos:prefLabel>
      <skos:definition xml:lang="de">Beinhaltet Text, Standbild, Video und Ton.</skos:definition>
      <skos:prefLabel xml:lang="nl">Media-eenheid</skos:prefLabel>
      <skos:definition xml:lang="nl"></skos:definition>
      <skos:prefLabel xml:lang="no">Medieenhet</skos:prefLabel>
      <skos:definition xml:lang="no">Inkluderer tekst, stillbilder, video og lyd.</skos:definition>
      <skos:narrower rdf:resource="http://rdf-vocabulary.ddialliance.org/cv/AnalysisUnit/2.1.0/8ab1c50"/>
      <skos:narrower rdf:resource="http://rdf-vocabulary.ddialliance.org/cv/AnalysisUnit/2.1.0/a0a6f8d"/>
      <skos:narrower rdf:resource="http://rdf-vocabulary.ddialliance.org/cv/AnalysisUnit/2.1.0/45ab7c1"/>
      <skos:narrower rdf:resource="http://rdf-vocabulary.ddialliance.org/cv/AnalysisUnit/2.1.0/75ea575"/>
   </rdf:Description>
   <rdf:Description rdf:about="http://rdf-vocabulary.ddialliance.org/cv/AnalysisUnit/2.1.0/8ab1c50">
      <rdf:type rdf:resource="http://www.w3.org/2004/02/skos/core#Concept"/>
      <skos:inScheme rdf:resource="http://rdf-vocabulary.ddialliance.org/cv/AnalysisUnit/2.1.0/"/>
      <skos:notation xml:lang="en">MediaUnit.Sound</skos:notation>
      <skos:prefLabel xml:lang="sl">Medijska enota: zvok</skos:prefLabel>
      <skos:definition xml:lang="sl">Posneti zvok, vklju&#x10d;no z glasom, glasbo itd.</skos:definition>
      <skos:prefLabel xml:lang="lt">Medijos vienetas: garso &#x12f;ra&#x161;as</skos:prefLabel>
      <skos:definition xml:lang="lt">&#x12e;ra&#x161;ytas garsas, &#x12f;skaitant bals&#x105;, muzik&#x105; ir kt.</skos:definition>
      <skos:prefLabel xml:lang="sv">Mediaenhet: Ljud</skos:prefLabel>
      <skos:definition xml:lang="sv">Inspelat ljud, som r&#xf6;st, musik m.m.</skos:definition>
      <skos:prefLabel xml:lang="fi">Mediatyyppi: &#xe4;&#xe4;ni</skos:prefLabel>
      <skos:definition xml:lang="fi">Taltioitu &#xe4;&#xe4;ni, esimerkiksi puhe, musiikki jne.</skos:definition>
      <skos:prefLabel xml:lang="it">Unit&#xe0; di supporto: suono</skos:prefLabel>
      <skos:definition xml:lang="it">Suoni registrati, inclusa la voce, la musica, ecc.</skos:definition>
      <skos:prefLabel xml:lang="pt">Unidade de Media: Som</skos:prefLabel>
      <skos:definition xml:lang="pt">Som gravado, incluindo voz, m&#xfa;sica, etc.</skos:definition>
      <skos:prefLabel xml:lang="en">Media unit: Sound</skos:prefLabel>
      <skos:definition xml:lang="en">Recorded sound, including voice, music, etc.</skos:definition>
      <skos:prefLabel xml:lang="de">Medieneinheit: Ton</skos:prefLabel>
      <skos:definition xml:lang="de">Aufgenommener Ton, einschlie&#xdf;lich Sprache, Musik usw.</skos:definition>
      <skos:prefLabel xml:lang="nl">Media-eenheid: Geluid</skos:prefLabel>
      <skos:definition xml:lang="nl"></skos:definition>
      <skos:prefLabel xml:lang="no">Medieenhet: Lyd</skos:prefLabel>
      <skos:definition xml:lang="no">Lydopptak, inkludert stemme, musikk, etc.</skos:definition>
   </rdf:Description>
   <rdf:Description rdf:about="http://rdf-vocabulary.ddialliance.org/cv/AnalysisUnit/2.1.0/a0a6f8d">
      <rdf:type rdf:resource="http://www.w3.org/2004/02/skos/core#Concept"/>
      <skos:inScheme rdf:resource="http://rdf-vocabulary.ddialliance.org/cv/AnalysisUnit/2.1.0/"/>
      <skos:notation xml:lang="en">MediaUnit.StillImage</skos:notation>
      <skos:prefLabel xml:lang="sl">Medijska enota: mirujo&#x10d;a slika</skos:prefLabel>
      <skos:definition xml:lang="sl">Stati&#x10d;ne slike, kot so grafi, risbe, fotografije, diagnosti&#x10d;ne/medicinske slike, kot so rentgenske slike in druge vrste slikovnih testov itd.</skos:definition>
      <skos:prefLabel xml:lang="lt">Medijos vienetas: statinis vaizdas</skos:prefLabel>
      <skos:definition xml:lang="lt">Statiniai vaizdai, tokie kaip grafikai, br&#x117;&#x17e;iniai, nuotraukos, diagnostiniai ar medicininiai vaizdai (rentgeno nuotraukos ir kitokio tipo vaizdo tyrimai) ir kt.</skos:definition>
      <skos:prefLabel xml:lang="sv">Mediaenhet: Stillbild</skos:prefLabel>
      <skos:definition xml:lang="sv">Statiska bilder, som diagram, ritningar, fotografier, diagnostiska/medicinska bilder som r&#xf6;ntgenbilder eller andra typer av bilddiagnostiska unders&#xf6;kningar&amp;nbsp;osv.</skos:definition>
      <skos:prefLabel xml:lang="fi">Mediatyyppi: still-kuva</skos:prefLabel>
      <skos:definition xml:lang="fi">Still-kuvat kuten esimerkiksi graafit, piirrokset, valokuvat, r&#xf6;ntgenkuvat tai muut l&#xe4;&#xe4;ketieteelliset still-kuvat.</skos:definition>
      <skos:prefLabel xml:lang="it">Unit&#xe0; di supporto: immagine</skos:prefLabel>
      <skos:definition xml:lang="it">Immagini statiche, come grafici, disegni, fotografie, immagini diagnostiche/mediche come radiografie e altri tipi di esami per immagini, ecc.</skos:definition>
      <skos:prefLabel xml:lang="pt">Unidade de Media: Imagem</skos:prefLabel>
      <skos:definition xml:lang="pt">Imagens est&#xe1;ticas, como gr&#xe1;ficos, desenhos, fotografias, imagens m&#xe9;dicas/de diagn&#xf3;stico como raio-x e outros tipos de testes de imagem, etc.</skos:definition>
      <skos:prefLabel xml:lang="en">Media unit: Still image</skos:prefLabel>
      <skos:definition xml:lang="en">Static images, such as graphs, drawings, photographs, diagnostic/medical images like X-rays and other types of imaging tests, etc.</skos:definition>
      <skos:prefLabel xml:lang="de">Medieneinheit: Unbewegtes Bild</skos:prefLabel>
      <skos:definition xml:lang="de">Statische Bilder, wie z. B. Diagramme, Zeichnungen, Fotos, diagnostische/medizinische Bilder wie R&#xf6;ntgenbilder und andere Arten von bildgebenden Tests usw.</skos:definition>
      <skos:prefLabel xml:lang="nl">Media-eenheid: Beeld</skos:prefLabel>
      <skos:definition xml:lang="nl"></skos:definition>
      <skos:prefLabel xml:lang="no">Medieenhet: Stillbilde</skos:prefLabel>
      <skos:definition xml:lang="no">Statiske bilder som grafer, tegninger, fotografier, diagnostiske/medisinske bilder som r&#xf8;ntgen og andre bildetester, etc.</skos:definition>
   </rdf:Description>
   <rdf:Description rdf:about="http://rdf-vocabulary.ddialliance.org/cv/AnalysisUnit/2.1.0/45ab7c1">
      <rdf:type rdf:resource="http://www.w3.org/2004/02/skos/core#Concept"/>
      <skos:inScheme rdf:resource="http://rdf-vocabulary.ddialliance.org/cv/AnalysisUnit/2.1.0/"/>
      <skos:notation xml:lang="en">MediaUnit.Text</skos:notation>
      <skos:prefLabel xml:lang="sl">Medijska enota: besedilo</skos:prefLabel>
      <skos:definition xml:lang="sl">Vsak pisni izdelek/entiteta, na primer knjige, &#x10d;lanki, tviti, blogi itd. Na primer &#x161;tudija o sovra&#x17e;nem govoru v tvitih ali &#x161;tudija o tem, kako &#x10d;asopisi predstavljajo dolo&#x10d;ena politi&#x10d;na/dru&#x17e;bena vpra&#x161;anja v &#x10d;asu, na primer pravice &#x17e;ensk ali manj&#x161;in itd.</skos:definition>
      <skos:prefLabel xml:lang="lt">Medijos vienetas: tekstas</skos:prefLabel>
      <skos:definition xml:lang="lt">Bet koks para&#x161;ytas k&#x16b;rinys ar objektas, pavyzd&#x17e;iui, knygos, straipsniai, socialini&#x173; medij&#x173; &#x17e;inut&#x117;s, tinklara&#x161;&#x10d;iai ir kt. Pavyzd&#x17e;iui, tyrimas apie neapykantos kalb&#x105; socialini&#x173; medij&#x173; &#x17e;inut&#x117;se arba tyrimas apie tai, kaip laikra&#x161;&#x10d;iai pateikia tam tikras politines ar socialines problemas, pavyzd&#x17e;iui, moter&#x173; ar ma&#x17e;um&#x173; teises ir kt.</skos:definition>
      <skos:prefLabel xml:lang="sv">Mediaenhet: Text</skos:prefLabel>
      <skos:definition xml:lang="sv">Skrivna texter, som b&#xf6;cker, artiklar, tweets, bloggar m.m. Till exempel en studie om hets mot folkgrupp i tweets, eller en studie om hur tidningar beskriver olika politiska/sociala &#xe4;mnen &#xf6;ver tid, som kvinnors eller minoriteters r&#xe4;ttigheter osv.</skos:definition>
      <skos:prefLabel xml:lang="fi">Mediatyyppi: teksti</skos:prefLabel>
      <skos:definition xml:lang="fi">Kirja, artikkeli, tweet, blogikirjoitus tai mik&#xe4; tahansa muu tekstiyksikk&#xf6;. Esimerkiksi tutkittaessa miten sanomalehdet ovat k&#xe4;sitelleet tietty&#xe4; aihetta ajan saatossa tai tutkittaessa vihapuhetta blogikirjoituksissa.</skos:definition>
      <skos:prefLabel xml:lang="it">Unit&#xe0; di supporto: testo</skos:prefLabel>
      <skos:definition xml:lang="it">Qualsiasi entit&#xe0; scritta, come libri, articoli, tweet, blog, ecc. Ad esempio, uno studio sugli hate speech nei tweet, oppure uno studio sul modo in cui i giornali presentano nel tempo alcuni temi politici/sociali, come i diritti delle donne o delle minoranze, ecc.</skos:definition>
      <skos:prefLabel xml:lang="pt">Unidade de Media: Texto</skos:prefLabel>
      <skos:definition xml:lang="pt">Qualquer entidade/pe&#xe7;a escrita, como livros, artigos, tweets, blogues, etc. Por exemplo, um estudo sobre discurso de &#xf3;dio nos tweets, ou um estudo sobre a forma como os jornais apresentam certos fen&#xf3;menos pol&#xed;ticos/sociais ao longo do tempo, como os direitos das mulheres ou de outras minorias, etc.</skos:definition>
      <skos:prefLabel xml:lang="en">Media unit: Text</skos:prefLabel>
      <skos:definition xml:lang="en">Any written piece/entity, such as books, articles, tweets, blogs, etc. For example, a study on hate speech in tweets, or a study of the way newspapers present certain political/social issues over time, like women&apos;s or minorities&apos; rights, etc.</skos:definition>
      <skos:prefLabel xml:lang="de">Medieneinheit: Text</skos:prefLabel>
      <skos:definition xml:lang="de">Jede schriftliche Arbeit/Einheit, wie B&#xfc;cher, Artikel, Tweets, Blogbeitr&#xe4;ge usw. Zum Beispiel eine Studie &#xfc;ber Hassreden in Tweets oder eine Studie &#xfc;ber die Art und Weise, wie Zeitungen bestimmte politische/soziale Themen im Laufe der Zeit darstellen, wie z. B. die Rechte von Frauen oder Minderheiten, usw.</skos:definition>
      <skos:prefLabel xml:lang="nl">Media-eenheid: Tekst</skos:prefLabel>
      <skos:definition xml:lang="nl"></skos:definition>
      <skos:prefLabel xml:lang="no">Medieenhet: Tekst</skos:prefLabel>
      <skos:definition xml:lang="no">Alle skrevne tekster/enheter som b&#xf8;ker, artikler, tweets, blogger, etc. For eksempel: en studie om hatefulle ytringer i tweets, en studie om m&#xe5;ten nyhetsaviser fremstiller enkelte politiske/sosiale problemer over tid, som kvinners eller minoriteters rettigheter.</skos:definition>
   </rdf:Description>
   <rdf:Description rdf:about="http://rdf-vocabulary.ddialliance.org/cv/AnalysisUnit/2.1.0/75ea575">
      <rdf:type rdf:resource="http://www.w3.org/2004/02/skos/core#Concept"/>
      <skos:inScheme rdf:resource="http://rdf-vocabulary.ddialliance.org/cv/AnalysisUnit/2.1.0/"/>
      <skos:notation xml:lang="en">MediaUnit.Video</skos:notation>
      <skos:prefLabel xml:lang="sl">Medijska enota: video</skos:prefLabel>
      <skos:definition xml:lang="sl">Premi&#x10d;ne slike. Vklju&#x10d;ujejo lahko filme, animacije, digitalne posnetke, vizualne rezultate simulacij, posnete televizijske programe, diagnosti&#x10d;ne/medicinske video posnetke, kot so ultrazvo&#x10d;ni pregledi itd.</skos:definition>
      <skos:prefLabel xml:lang="lt">Medijos vienetas: vaizdo &#x12f;ra&#x161;as</skos:prefLabel>
      <skos:definition xml:lang="lt">Judantys vaizdai. Gali apimti filmus, animacij&#x105;, skaitmeninius &#x12f;ra&#x161;us, simuliacij&#x173; vaizdinius produktus, &#x12f;ra&#x161;ytas televizijos programas, diagnostinius ar medicininius vaizdo &#x12f;ra&#x161;us, tokius kaip ultragarso tyrimai ir kt. Gali b&#x16b;ti be garso ar tur&#x117;ti garso sinchronizacij&#x105;.</skos:definition>
      <skos:prefLabel xml:lang="sv">Mediaenhet: Video</skos:prefLabel>
      <skos:definition xml:lang="sv">R&#xf6;rliga bilder. Det kan inkludera filmer, animationer, digitala inspelningar, visuella utdata fr&#xe5;n simuleringar, inspelade tv-program, diagnostiska/medicinska videor som ultraljudsunders&#xf6;kningar osv. De kan vara utan ljud eller med synkroniserat ljud.</skos:definition>
      <skos:prefLabel xml:lang="fi">Mediatyyppi: liikkuva kuva</skos:prefLabel>
      <skos:definition xml:lang="fi">Liikkuva kuva &#xe4;&#xe4;nell&#xe4; tai ilman. Esimerkiksi elokuvat, animaatiot, digitaaliset taltiot, simulaatioiden liikkuvat kuvat, taltioidut televisio-ohjelmat ja ultra&#xe4;&#xe4;nikuvat.</skos:definition>
      <skos:prefLabel xml:lang="it">Unit&#xe0; di supporto: video</skos:prefLabel>
      <skos:definition xml:lang="it">Immagini in movimento. Pu&#xf2; includere film, animazioni, registrazioni digitali, output visivi prodotti da simulazioni, programmi televisivi registrati, video medico/diagnostici come ecografie, ecc. Pu&#xf2; essere muto o pu&#xf2; includere il suono sincronizzato.</skos:definition>
      <skos:prefLabel xml:lang="pt">Unidade de Media: V&#xed;deo</skos:prefLabel>
      <skos:definition xml:lang="pt">Imagens em movimento. Pode incluir filmes, anima&#xe7;&#xe3;o, grava&#xe7;&#xf5;es digitais, output visual de simula&#xe7;&#xf5;es, programas televisivos gravados, v&#xed;deos m&#xe9;dicos/de diagn&#xf3;stico como ultrasons, etc. Podem ser silenciosos ou podem incluir som sincronizado.</skos:definition>
      <skos:prefLabel xml:lang="en">Media unit: Video</skos:prefLabel>
      <skos:definition xml:lang="en">Moving images. May include films, animation, digital recordings, visual output from simulations, recorded television programs, diagnostic/medical videos like ultrasound scans, etc. May be mute or may include synchronized sound.</skos:definition>
      <skos:prefLabel xml:lang="de">Medieneinheit: Video</skos:prefLabel>
      <skos:definition xml:lang="de">Bewegte Bilder. Das kann Filme, Animationen, digitale Aufnahmen, visuelle Ausgaben von Simulationen, aufgezeichnete Fernsehsendungen, diagnostische/medizinische Videos wie Ultraschalluntersuchungen usw. beinhalten. Das kann stummgeschalteten oder synchronisierten Ton beinhalten.</skos:definition>
      <skos:prefLabel xml:lang="nl">Media-eenheid: Video</skos:prefLabel>
      <skos:definition xml:lang="nl"></skos:definition>
      <skos:prefLabel xml:lang="no">Medieenhet: video</skos:prefLabel>
      <skos:definition xml:lang="no">Bevegelige bilder. Kan inkludere filmer, animasjoner, digitale opptak, visuell produksjon fra simuleringer, innspilte fjernsynsprogram, diagnostiske/medisinske videor som ultralyd skanninger, etc. Kan v&#xe6;re uten lyd eller med synkronisert lyd.</skos:definition>
   </rdf:Description>
   <rdf:Description rdf:about="http://rdf-vocabulary.ddialliance.org/cv/AnalysisUnit/2.1.0/0393713">
      <rdf:type rdf:resource="http://www.w3.org/2004/02/skos/core#Concept"/>
      <skos:inScheme rdf:resource="http://rdf-vocabulary.ddialliance.org/cv/AnalysisUnit/2.1.0/"/>
      <skos:notation xml:lang="en">Group</skos:notation>
      <skos:prefLabel xml:lang="sl">Skupina</skos:prefLabel>
      <skos:definition xml:lang="sl">Dva ali ve&#x10d; posameznikov, zbranih skupaj oziroma vklju&#x10d;enih v medsebojen odnos. V anketnih raziskavah so vpra&#x161;anja osredoto&#x10d;ena predvsem na skupino in stali&#x161;&#x10d;a / izku&#x161;nje skupine, ne pa na stali&#x161;&#x10d;a posameznih anketirancev. &#x10c;e se vpra&#x161;anja nana&#x161;ajo skupino in posameznika, uporabite oba kot enoti za analizo.</skos:definition>
      <skos:prefLabel xml:lang="lt">Grup&#x117; </skos:prefLabel>
      <skos:definition xml:lang="lt">Du ar daugiau asmen&#x173;, susib&#x16b;rusi&#x173; kartu arba turin&#x10d;i&#x173; tam tikr&#x173; vienijan&#x10d;i&#x173; ry&#x161;i&#x173; ar savybi&#x173;. Atliekant apklausas klausimai gali b&#x16b;ti nukreipti &#x12f; grup&#x119; ir grup&#x117;s, o ne atskir&#x173; respondent&#x173;, po&#x17e;i&#x16b;rius ar patirtis. Jei klausimai apima tiek grup&#x119;, tiek asmen&#x12f;, naudoti abu kaip analiz&#x117;s vienetus.</skos:definition>
      <skos:prefLabel xml:lang="sv">Grupp</skos:prefLabel>
      <skos:definition xml:lang="sv">Tv&#xe5; eller fler personer som samlats eller som har n&#xe5;gon form av relation eller egenskap som f&#xf6;renar dem. I surveyunders&#xf6;kningar fokuserar fr&#xe5;gorna framf&#xf6;r allt p&#xe5; gruppen och gruppens attityder/erfarenheter, snarare &#xe4;n p&#xe5; de enskilda respondenterna. Om fr&#xe5;gorna g&#xe4;ller b&#xe5;de gruppen och individen, anv&#xe4;nd b&#xe5;da som analysenheter.</skos:definition>
      <skos:prefLabel xml:lang="fi">Ryhm&#xe4;</skos:prefLabel>
      <skos:definition xml:lang="fi">Kaksi tai useampia henkil&#xf6;it&#xe4;, jotka ovat joko kokoontuneet yhteen tai joita yhdist&#xe4;&#xe4; jokin muu tekij&#xe4;. Mik&#xe4;li kyselytutkimus, kysymykset koskevat p&#xe4;&#xe4;asiassa itse ryhm&#xe4;&#xe4;, ryhm&#xe4;n kokemuksia ja asenteita ryhm&#xe4;&#xe4; kohtaan, ei henkil&#xf6;&#xe4; itse&#xe4;&#xe4;n. Mik&#xe4;li kysymykset koskevat sek&#xe4; ryhm&#xe4;&#xe4; ett&#xe4; henkil&#xf6;&#xe4;, k&#xe4;yt&#xe4; havaintoyksikk&#xf6;n&#xe4; molempia.</skos:definition>
      <skos:prefLabel xml:lang="it">Gruppo</skos:prefLabel>
      <skos:definition xml:lang="it">Due o pi&#xf9; individui riuniti oppure che possiedono una qualsiasi relazione o caratteristica unificante. Nelle indagini le domande si concentrano principalmente sul gruppo e sugli atteggiamenti/esperienze del gruppo, piuttosto che su quelle dei singoli intervistati. Se le domande riguardano sia il gruppo che l&apos;individuo, utilizzare entrambi come unit&#xe0; di analisi.</skos:definition>
      <skos:prefLabel xml:lang="pt">Grupo</skos:prefLabel>
      <skos:definition xml:lang="pt">Dois ou mais indiv&#xed;duos que se assemelham ou que t&#xea;m uma rela&#xe7;&#xe3;o ou caracter&#xed;stica unificadora. Nos inqu&#xe9;ritos, as quest&#xf5;es s&#xe3;o principalmente focadas no grupo e nas atitudes e experi&#xea;ncias do grupo, e n&#xe3;o tanto nos indiv&#xed;duos entrevistados. Se as quest&#xf5;es abrangem o indiv&#xed;duo e o grupo, usar ambos como unidades de an&#xe1;lise.</skos:definition>
      <skos:prefLabel xml:lang="en">Group</skos:prefLabel>
      <skos:definition xml:lang="en">Two or more individuals assembled together or having some unifying relationship or characteristic. In surveys, the questions are mainly focused on the group and the attitudes/experiences of the group, rather than on those of the individual respondents. If questions cover both the group and the individual, use  both as analysis units.</skos:definition>
      <skos:prefLabel xml:lang="de">Gruppe</skos:prefLabel>
      <skos:definition xml:lang="de">Zwei oder mehr Individuen, die zusammen versammelt sind oder eine verbindende Beziehung oder Eigenschaft haben. In Umfragen konzentrieren sich die Fragen haupts&#xe4;chlich auf die Gruppe und die Einstellungen/Erfahrungen der Gruppe und nicht auf die der einzelnen Befragten. Wenn sich die Fragen sowohl auf die Gruppe als auch auf das Individuum beziehen, k&#xf6;nnen beide Analyseeinheiten verwendet werden.</skos:definition>
      <skos:prefLabel xml:lang="nl">Groep</skos:prefLabel>
      <skos:definition xml:lang="nl"></skos:definition>
      <skos:prefLabel xml:lang="no">Gruppe</skos:prefLabel>
      <skos:definition xml:lang="no">To eller flere personer som samles eller som har et forhold som forener dem. I sp&#xf8;rreunders&#xf8;kelser er sp&#xf8;rsm&#xe5;lene hovedsaklig rettet mot gruppen og holdningen/opplevelsene til gruppen i steden for de individuelle respondentene. Hvis sp&#xf8;rsm&#xe5;l ang&#xe5;r b&#xe5;de gruppen og individene, bruk begge som analyseenhet.</skos:definition>
   </rdf:Description>
   <rdf:Description rdf:about="http://rdf-vocabulary.ddialliance.org/cv/AnalysisUnit/2.1.0/4970317">
      <rdf:type rdf:resource="http://www.w3.org/2004/02/skos/core#Concept"/>
      <skos:inScheme rdf:resource="http://rdf-vocabulary.ddialliance.org/cv/AnalysisUnit/2.1.0/"/>
      <skos:notation xml:lang="en">Object</skos:notation>
      <skos:prefLabel xml:lang="sl">Predmet</skos:prefLabel>
      <skos:definition xml:lang="sl">Karkoli materialnega, toda ne&#x17e;ivega, kar ima neodvisen obstoj in ga lahko zaznamo s &#x10d;utili. Primeri: umetni&#x161;ki predmeti (slike, skulpture itd.), oro&#x17e;je, vozila itd.</skos:definition>
      <skos:prefLabel xml:lang="lt">Objektas</skos:prefLabel>
      <skos:definition xml:lang="lt">Visa, kas materialu, bet negyva, egzistuoja savaranki&#x161;kai ir gali b&#x16b;ti juntama jusl&#x117;mis. Pavyzd&#x17e;iai: meno k&#x16b;riniai (paveikslai, skulpt&#x16b;ros ir kt.), ginklai ar transporto priemon&#x117;s ir kt.</skos:definition>
      <skos:prefLabel xml:lang="sv">F&#xf6;rem&#xe5;l</skos:prefLabel>
      <skos:definition xml:lang="sv">N&#xe5;got fysiskt men icke levande som existerar som en oberoende enhet och kan uppfattas av sinnena. Exempel: konstf&#xf6;rem&#xe5;l (tavlor, skulpturer, o.dyl.), vapen, fordon m.m.</skos:definition>
      <skos:prefLabel xml:lang="fi">Eloton objekti/esine</skos:prefLabel>
      <skos:definition xml:lang="fi">Mik&#xe4; tahansa konkreettinen, eloton esine/kohde, joka voidaan aistein havaita. Esimerkiksi taideteokset (veistokset, maalaukset), aseet, ajoneuvot jne.</skos:definition>
      <skos:prefLabel xml:lang="it">Oggetto</skos:prefLabel>
      <skos:definition xml:lang="it">Tutto ci&#xf2; che &#xe8; materiale, inanimato, che ha un&apos;esistenza indipendente e che pu&#xf2; essere percepito attraverso i sensi. Esempi: oggetti d&apos;arte (dipinti, sculture, ecc.), armi, veicoli, ecc.</skos:definition>
      <skos:prefLabel xml:lang="pt">Objeto</skos:prefLabel>
      <skos:definition xml:lang="pt">Qualquer coisa material, mas inanimada, que tenha uma exist&#xea;ncia independente e possa ser percebida pelos sentidos. Exemplos: objetos de arte (pinturas, esculturas, etc.) ou armas, ou ve&#xed;culos, etc.</skos:definition>
      <skos:prefLabel xml:lang="en">Object</skos:prefLabel>
      <skos:definition xml:lang="en">Anything material, but inanimate, that has an independent existence and may be perceived by the senses. Examples: objects of art (paintings, sculptures, etc.) or weapons, or vehicles, etc.</skos:definition>
      <skos:prefLabel xml:lang="de">Objekt</skos:prefLabel>
      <skos:definition xml:lang="de">Alle nicht lebenden Stoffe, die eine unabh&#xe4;ngige Existenz haben und mit den Sinnen wahrgenommen werden k&#xf6;nnen. Beispiele: Kunstobjekte (Gem&#xe4;lde, Skulpturen, etc.) oder Waffen oder Fahrzeuge usw.</skos:definition>
      <skos:prefLabel xml:lang="nl">Voorwerp</skos:prefLabel>
      <skos:definition xml:lang="nl"></skos:definition>
      <skos:prefLabel xml:lang="no">Objekt</skos:prefLabel>
      <skos:definition xml:lang="no">Noe fysisk, men ikke levende som eksisterer som en uavhengig enhet og som kan oppfattes av sansene. For eksempel: kunst (malerier, skulpturer osv.), v&#xe5;pen, kj&#xf8;ret&#xf8;y etc.</skos:definition>
   </rdf:Description>
   <rdf:Description rdf:about="http://rdf-vocabulary.ddialliance.org/cv/AnalysisUnit/2.1.0/6311ae1">
      <rdf:type rdf:resource="http://www.w3.org/2004/02/skos/core#Concept"/>
      <skos:inScheme rdf:resource="http://rdf-vocabulary.ddialliance.org/cv/AnalysisUnit/2.1.0/"/>
      <skos:notation xml:lang="en">Other</skos:notation>
      <skos:prefLabel xml:lang="sl">Drugo</skos:prefLabel>
      <skos:definition xml:lang="sl">Uporabite, &#x10d;e je enota analize poznana, a je ne najdete na seznamu.</skos:definition>
      <skos:prefLabel xml:lang="lt">Kita</skos:prefLabel>
      <skos:definition xml:lang="lt">Naudoti, kai analiz&#x117;s vienetas yra &#x17e;inomas, bet s&#x105;ra&#x161;e jo n&#x117;ra.</skos:definition>
      <skos:prefLabel xml:lang="sv">&#xd6;vrigt</skos:prefLabel>
      <skos:definition xml:lang="sv">Anv&#xe4;nd om analysenheten &#xe4;r k&#xe4;nd men saknas i listan.</skos:definition>
      <skos:prefLabel xml:lang="fi">Muu havainto/aineistoyksikk&#xf6;tyyppi</skos:prefLabel>
      <skos:definition xml:lang="fi">K&#xe4;yt&#xe4; mik&#xe4;li havaintoyksikk&#xf6; on tiedossa, mutta ei l&#xf6;ydy sanastosta.</skos:definition>
      <skos:prefLabel xml:lang="it">Altro</skos:prefLabel>
      <skos:definition xml:lang="it">Utilizzare se l&apos;unit&#xe0; di analisi &#xe8; nota, ma non riconducibile a nessun termine presente nell&apos;elenco.</skos:definition>
      <skos:prefLabel xml:lang="pt">Outro </skos:prefLabel>
      <skos:definition xml:lang="pt">Usar se a unidade de an&#xe1;lise for conhecida, mas n&#xe3;o se encontrar na lista.</skos:definition>
      <skos:prefLabel xml:lang="en">Other</skos:prefLabel>
      <skos:definition xml:lang="en">Use if the unit of analysis is known, but not found in the list.</skos:definition>
      <skos:prefLabel xml:lang="de">Sonstiges</skos:prefLabel>
      <skos:definition xml:lang="de">Wird verwendet, wenn die Analyseeinheit bekannt ist, aber nicht in der Liste vertreten ist.</skos:definition>
      <skos:prefLabel xml:lang="nl">Anders</skos:prefLabel>
      <skos:definition xml:lang="nl"></skos:definition>
      <skos:prefLabel xml:lang="no">Annet</skos:prefLabel>
      <skos:definition xml:lang="no">Benytt hvis analyseenheten er kjent, men ikke finnes i listen.</skos:definition>
   </rdf:Description>
</rdf:RDF>
