<?xml version="1.0" encoding="UTF-8"?>
<rdf:RDF xmlns:rdf="http://www.w3.org/1999/02/22-rdf-syntax-ns#"
         xmlns:skos="http://www.w3.org/2004/02/skos/core#"
         xmlns:owl="http://www.w3.org/2002/07/owl#"
         xmlns:dcterms="http://purl.org/dc/terms/"
>
   <rdf:Description rdf:about="http://rdf-vocabulary.ddialliance.org/cv/ModeOfCollection/5.0.0/">
      <rdf:type rdf:resource="http://www.w3.org/2004/02/skos/core#ConceptScheme"/>
      <dcterms:isVersionOf rdf:resource="http://rdf-vocabulary.ddialliance.org/cv/ModeOfCollection/"/>
      <skos:notation xml:lang="en">ModeOfCollection</skos:notation>
      <dcterms:title xml:lang="sl">Na&#x10d;in zbiranja podatkov</dcterms:title>
      <dcterms:description xml:lang="sl">Postopki, tehnike ali na&#x10d;ini raziskovanja, uporabljeni za pridobivanje podatkov.</dcterms:description>
      <skos:prefLabel xml:lang="sl">Na&#x10d;in zbiranja podatkov</skos:prefLabel>
      <dcterms:title xml:lang="sv">Insamlingsmetod</dcterms:title>
      <dcterms:description xml:lang="sv">Den process, metod eller teknik som anv&#xe4;ndes f&#xf6;r att samla in data.</dcterms:description>
      <skos:prefLabel xml:lang="sv">Insamlingsmetod</skos:prefLabel>
      <dcterms:title xml:lang="en">Mode Of Collection</dcterms:title>
      <dcterms:description xml:lang="en">The procedure, technique, or mode of inquiry used to attain the data.</dcterms:description>
      <skos:prefLabel xml:lang="en">Mode Of Collection</skos:prefLabel>
      <dcterms:title xml:lang="de">Erhebungsmodus</dcterms:title>
      <dcterms:description xml:lang="de">Prozedur, Technik oder Art der Erhebung, die verwendet wurde, um Daten zu bekommen.</dcterms:description>
      <skos:prefLabel xml:lang="de">Erhebungsmodus</skos:prefLabel>
      <dcterms:title xml:lang="no">Innsamlingsmetode</dcterms:title>
      <dcterms:description xml:lang="no">Framgangsm&#xe5;ten, teknikken, eller metoden som er anvendt for &#xe5; samle inn data.</dcterms:description>
      <skos:prefLabel xml:lang="no">Innsamlingsmetode</skos:prefLabel>
      <dcterms:title xml:lang="lt">Surinkimo b&#x16b;das</dcterms:title>
      <dcterms:description xml:lang="lt">Tyrimo proced&#x16b;ra, technika ar b&#x16b;das, naudojami gauti duomenis.</dcterms:description>
      <skos:prefLabel xml:lang="lt">Surinkimo b&#x16b;das</skos:prefLabel>
      <dcterms:title xml:lang="it">Metodo di raccolta dei dati</dcterms:title>
      <dcterms:description xml:lang="it">La procedura, la tecnica o la modalit&#xe0; di indagine utilizzata per ottenere i dati.</dcterms:description>
      <skos:prefLabel xml:lang="it">Metodo di raccolta dei dati</skos:prefLabel>
      <dcterms:title xml:lang="fr">Mode de collecte</dcterms:title>
      <dcterms:description xml:lang="fr">La proc&#xe9;dure, la technique ou le mode d&apos;enqu&#xea;te utilis&#xe9; pour obtenir les donn&#xe9;es.</dcterms:description>
      <skos:prefLabel xml:lang="fr">Mode de collecte</skos:prefLabel>
      <dcterms:title xml:lang="nl">Verzamelmethode</dcterms:title>
      <dcterms:description xml:lang="nl">De procedure, techniek of methode die is gebruikt om de gegevens te verzamelen. </dcterms:description>
      <skos:prefLabel xml:lang="nl">Verzamelmethode</skos:prefLabel>
      <owl:versionInfo>5.0.0</owl:versionInfo>
      <dcterms:license rdf:resource="http://creativecommons.org/licenses/by/4.0/"/>
      <dcterms:rights>Copyright &#xa9;DDI Alliance 2025</dcterms:rights>
      <skos:hasTopConcept rdf:resource="http://rdf-vocabulary.ddialliance.org/cv/ModeOfCollection/5.0.0/cb20d17"/>
      <skos:hasTopConcept rdf:resource="http://rdf-vocabulary.ddialliance.org/cv/ModeOfCollection/5.0.0/35e4248"/>
      <skos:hasTopConcept rdf:resource="http://rdf-vocabulary.ddialliance.org/cv/ModeOfCollection/5.0.0/9ec957d"/>
      <skos:hasTopConcept rdf:resource="http://rdf-vocabulary.ddialliance.org/cv/ModeOfCollection/5.0.0/08e658a"/>
      <skos:hasTopConcept rdf:resource="http://rdf-vocabulary.ddialliance.org/cv/ModeOfCollection/5.0.0/c680d43"/>
      <skos:hasTopConcept rdf:resource="http://rdf-vocabulary.ddialliance.org/cv/ModeOfCollection/5.0.0/05aeba4"/>
      <skos:hasTopConcept rdf:resource="http://rdf-vocabulary.ddialliance.org/cv/ModeOfCollection/5.0.0/c5564d2"/>
      <skos:hasTopConcept rdf:resource="http://rdf-vocabulary.ddialliance.org/cv/ModeOfCollection/5.0.0/c867d80"/>
      <skos:hasTopConcept rdf:resource="http://rdf-vocabulary.ddialliance.org/cv/ModeOfCollection/5.0.0/4848ed5"/>
      <skos:hasTopConcept rdf:resource="http://rdf-vocabulary.ddialliance.org/cv/ModeOfCollection/5.0.0/df9aac3"/>
      <skos:hasTopConcept rdf:resource="http://rdf-vocabulary.ddialliance.org/cv/ModeOfCollection/5.0.0/6decc77"/>
      <skos:hasTopConcept rdf:resource="http://rdf-vocabulary.ddialliance.org/cv/ModeOfCollection/5.0.0/2906121"/>
      <skos:hasTopConcept rdf:resource="http://rdf-vocabulary.ddialliance.org/cv/ModeOfCollection/5.0.0/d9ceca6"/>
      <skos:hasTopConcept rdf:resource="http://rdf-vocabulary.ddialliance.org/cv/ModeOfCollection/5.0.0/4f502b5"/>
      <skos:hasTopConcept rdf:resource="http://rdf-vocabulary.ddialliance.org/cv/ModeOfCollection/5.0.0/38ceaa4"/>
      <skos:hasTopConcept rdf:resource="http://rdf-vocabulary.ddialliance.org/cv/ModeOfCollection/5.0.0/6311ae1"/>
   </rdf:Description>
   <rdf:Description rdf:about="http://rdf-vocabulary.ddialliance.org/cv/ModeOfCollection/5.0.0/cb20d17">
      <rdf:type rdf:resource="http://www.w3.org/2004/02/skos/core#Concept"/>
      <skos:inScheme rdf:resource="http://rdf-vocabulary.ddialliance.org/cv/ModeOfCollection/5.0.0/"/>
      <skos:notation xml:lang="en">Interview</skos:notation>
      <skos:prefLabel xml:lang="sl">Intervju</skos:prefLabel>
      <skos:definition xml:lang="sl">Vnaprej na&#x10d;rtovana komunikacija med dvema (ali ve&#x10d;) osebami - spra&#x161;evalcem(-ci) in spra&#x161;evancem(-ci) -, kjer spra&#x161;evalec(-ci) pridobi(jo) informacije s strani spra&#x161;evanca(-cev). &#x10c;e je v metodo vklju&#x10d;ena skupinska interakcija, uporabite izraz &quot;fokusna skupina&quot;.</skos:definition>
      <skos:prefLabel xml:lang="sv">Intervju</skos:prefLabel>
      <skos:definition xml:lang="sv">Planerad kommunikation mellan tv&#xe5; (eller flera) personer &#x2013; intervjuare och intervjuobjekt &#x2013; d&#xe4;r intervjuaren/-na f&#xe5;r information fr&#xe5;n intervjuobjektet/-en. Anv&#xe4;nd &quot;Fokusgrupp&quot; om gruppinteraktion &#xe4;r del av metoden.</skos:definition>
      <skos:prefLabel xml:lang="en">Interview</skos:prefLabel>
      <skos:definition xml:lang="en">A pre-planned communication between two (or more) people - the interviewer(s) and the interviewee(s) - in which information is obtained by the interviewer(s) from the interviewee(s). If group interaction is part of the method, use &quot;Focus group&quot;.</skos:definition>
      <skos:prefLabel xml:lang="de">Interview</skos:prefLabel>
      <skos:definition xml:lang="de">Eine im Voraus geplante Kommunikation zwischen zwei (oder mehr) Personen - dem/der Interviewer*in bzw. den Interviewern und dem/der/den Befragten -, bei der der/die Interviewer Informationen von dem/der/den Befragten erhalten. Wenn die Interaktion innerhalb einer Gruppe Teil der Methode ist, verwenden Sie die Kategorie &quot;Fokusgruppe&quot;.</skos:definition>
      <skos:prefLabel xml:lang="no">Intervju</skos:prefLabel>
      <skos:definition xml:lang="no">En forh&#xe5;ndsplanlagt kommunikasjon mellom to (eller flere) personer &#x2013; intervjueren(e) og intervjuobjekt(et/ene) &#x2013; hvor intervjueren(e) henter informasjon fra intervjuobjekt(et/ene). Dersom gruppeinteraksjoner er del av metoden, bruk &apos;Fokusgruppe&apos;.</skos:definition>
      <skos:prefLabel xml:lang="lt">Interviu</skos:prefLabel>
      <skos:definition xml:lang="lt">I&#x161; anksto suplanuotas dviej&#x173; (ar daugiau) &#x17e;moni&#x173; &#x2013; apklaus&#x117;jo(-&#x173;) ir apklausiamojo(-&#x173;j&#x173;) &#x2013; bendravimas, kurio metu i&#x161; apklausiamojo(-&#x173;j&#x173;) informacij&#x105; gauna apklaus&#x117;jas(-ai). Jei metodo taikymas reikalauja grupin&#x117;s s&#x105;veikos, naudoti &#x201e;Tikslin&#x119; grup&#x117;s diskusij&#x105;&#x201c;.</skos:definition>
      <skos:prefLabel xml:lang="it">Intervista</skos:prefLabel>
      <skos:definition xml:lang="it">Una comunicazione pianificata tra due (o pi&#xf9;) persone - l&apos;intervistatore/i e l&apos;intervistato/i - in cui le informazioni ottenute dall&apos;intervistatore sono state rilasciate dagli intervistati. Se l&apos;interazione di gruppo &#xe8; parte della tecnica, utilizzare &quot;Focus group&quot;.</skos:definition>
      <skos:prefLabel xml:lang="fr">Entretien</skos:prefLabel>
      <skos:definition xml:lang="fr">Un &#xe9;change pr&#xe9;vu entre deux (ou plusieurs) personnes - l(es) enqu&#xea;teur(s) et l(es) enqu&#xea;t&#xe9;(s) - au cours duquel des informations sont obtenues par l(es) enqu&#xea;teur(s) sur l(es) enqu&#xea;t&#xe9;(s). Si la m&#xe9;thode implique des interactions groupales, utilisez le terme &quot;Focus group&quot;.</skos:definition>
      <skos:prefLabel xml:lang="nl">Interview</skos:prefLabel>
      <skos:definition xml:lang="nl"></skos:definition>
      <skos:narrower rdf:resource="http://rdf-vocabulary.ddialliance.org/cv/ModeOfCollection/5.0.0/9f669a4"/>
      <skos:narrower rdf:resource="http://rdf-vocabulary.ddialliance.org/cv/ModeOfCollection/5.0.0/ae68e25"/>
      <skos:narrower rdf:resource="http://rdf-vocabulary.ddialliance.org/cv/ModeOfCollection/5.0.0/b0b2868"/>
      <skos:narrower rdf:resource="http://rdf-vocabulary.ddialliance.org/cv/ModeOfCollection/5.0.0/1af2bfa"/>
   </rdf:Description>
   <rdf:Description rdf:about="http://rdf-vocabulary.ddialliance.org/cv/ModeOfCollection/5.0.0/9f669a4">
      <rdf:type rdf:resource="http://www.w3.org/2004/02/skos/core#Concept"/>
      <skos:inScheme rdf:resource="http://rdf-vocabulary.ddialliance.org/cv/ModeOfCollection/5.0.0/"/>
      <skos:notation xml:lang="en">Interview.FaceToFace</skos:notation>
      <skos:prefLabel xml:lang="sl">Osebni intervju</skos:prefLabel>
      <skos:definition xml:lang="sl">Metoda zbiranja podatkov, kjer spra&#x161;evalec izvede osebni intervju, postavlja vpra&#x161;anja in vnese odgovore. Uporabite ta &#x161;ir&#x161;i izraz, &#x10d;e ne morete uporabiti CAPI ali PAPI ozioma ni znano, ali gre za CAPI/PAPI.</skos:definition>
      <skos:prefLabel xml:lang="sv">Personlig intervju</skos:prefLabel>
      <skos:definition xml:lang="sv">En n&#xe4;rvarande intervjuare genomf&#xf6;r en personlig intervju genom att st&#xe4;lla fr&#xe5;gor och notera svaren. Anv&#xe4;nd denna bredare term om det inte r&#xf6;r sig om CAPI eller PAPI, eller om det inte &#xe4;r k&#xe4;nt huruvida det r&#xf6;r sig om CAPI/PAPI eller inte.</skos:definition>
      <skos:prefLabel xml:lang="en">Face-to-face interview</skos:prefLabel>
      <skos:definition xml:lang="en">Data collection method in which a live interviewer conducts a personal interview, presenting questions and entering the responses. Use this broader term if not CAPI or PAPI, or if not known whether CAPI/PAPI or not.</skos:definition>
      <skos:prefLabel xml:lang="de">Pers&#xf6;nliches Interview</skos:prefLabel>
      <skos:definition xml:lang="de">Datenerhebungsmethode, bei der ein/eine Live-Interviewer*in ein pers&#xf6;nliches Interview durchf&#xfc;hrt, Fragen stellt und die Antworten eingibt. Verwenden Sie diesen weiter gefassten Begriff, wenn es sich nicht um CAPI oder PAPI handelt, oder wenn nicht bekannt ist, ob es sich um CAPI/PAPI handelt oder nicht.</skos:definition>
      <skos:prefLabel xml:lang="no">Personlig intervju</skos:prefLabel>
      <skos:definition xml:lang="no">Datainnsamlingsmetode hvor en tilstedev&#xe6;rende intervjuer gjennomf&#xf8;rer et personlig intervju, presenterer sp&#xf8;rsm&#xe5;l og registrerer svarene. Bruk dette bredere begrepet dersom det ikke er CATI eller PAPI, eller dersom det er uvisst om det er CATI/PAPI.</skos:definition>
      <skos:prefLabel xml:lang="lt">Tiesioginis interviu</skos:prefLabel>
      <skos:definition xml:lang="lt">Duomen&#x173; rinkimo metodas, kai apklaus&#x117;jas asmeni&#x161;kai atlieka interviu, pateikdamas klausimus ir fiksuodamas atsakymus. Naudoti &#x161;&#x12f; platesn&#x12f; termin&#x105;, kai netinka CAPI ar PAPI, arba jei ne&#x17e;inoma, ar tinka CAPI arba PAPI.</skos:definition>
      <skos:prefLabel xml:lang="it">Intervista faccia a faccia</skos:prefLabel>
      <skos:definition xml:lang="it">Tecnica di raccolta dei dati in cui un intervistatore conduce un colloquio personale in presenza, facendo domande e registrando le risposte. Utilizzare questo termine pi&#xf9; ampio se l&apos;intervista non &#xe8; CAPI o PAPI, o se non si &#xe8; in grado di stabilire se sia CAPI o PAPI.</skos:definition>
      <skos:prefLabel xml:lang="fr">Entretien en face-&#xe0;-face</skos:prefLabel>
      <skos:definition xml:lang="fr">M&#xe9;thode de recueil de donn&#xe9;es dans laquelle un enqu&#xea;teur m&#xe8;ne un entretien, pose des questions et saisit les r&#xe9;ponses. Utilisez ce terme si ce n&#x2019;est ni CAPI ni PAPI, ou si vous ne savez pas si CAPI / PAPI ou pas.</skos:definition>
      <skos:prefLabel xml:lang="nl">Face-to-face interview</skos:prefLabel>
      <skos:definition xml:lang="nl"></skos:definition>
      <skos:narrower rdf:resource="http://rdf-vocabulary.ddialliance.org/cv/ModeOfCollection/5.0.0/89e4fb4"/>
      <skos:narrower rdf:resource="http://rdf-vocabulary.ddialliance.org/cv/ModeOfCollection/5.0.0/e477963"/>
   </rdf:Description>
   <rdf:Description rdf:about="http://rdf-vocabulary.ddialliance.org/cv/ModeOfCollection/5.0.0/89e4fb4">
      <rdf:type rdf:resource="http://www.w3.org/2004/02/skos/core#Concept"/>
      <skos:inScheme rdf:resource="http://rdf-vocabulary.ddialliance.org/cv/ModeOfCollection/5.0.0/"/>
      <skos:notation xml:lang="en">Interview.FaceToFace.CAPIorCAMI</skos:notation>
      <skos:prefLabel xml:lang="sl">Osebni intervju: CAPI/CAMI</skos:prefLabel>
      <skos:definition xml:lang="sl">Ra&#x10d;unalni&#x161;ko podprto osebno intervjuvanje (CAPI) ali ra&#x10d;unalni&#x161;ko podprto mobilno intervjuvanje (CAMI). Metoda zbiranja podatkov, kjer spra&#x161;evalec prebere vpra&#x161;anja spra&#x161;evancu z zaslona na ra&#x10d;unalniku, prenosnem ra&#x10d;unalniku ali mobilni napravi, kot na primer na tablici ali pametnemu telefonu, in vnese odgovore v isto napravo. Intervju izvedemo s pomo&#x10d;jo posebej zasnovanega programa/ aplikacije.</skos:definition>
      <skos:prefLabel xml:lang="sv">Personlig intervju: CAPI/CAMI</skos:prefLabel>
      <skos:definition xml:lang="sv">Datorst&#xf6;dd personlig intervju. Intervjuaren l&#xe4;ser fr&#xe5;gor f&#xf6;r respondenterna fr&#xe5;n en datorsk&#xe4;rm eller mobil enhet (t.ex. surfplatta eller mobiltelefon) och skriver in svaren direkt i datorn. Intervjun hanteras med ett program som utvecklats f&#xf6;r detta syfte.</skos:definition>
      <skos:prefLabel xml:lang="en">Face-to-face interview: Computer-assisted (CAPI/CAMI)</skos:prefLabel>
      <skos:definition xml:lang="en">Computer-assisted personal interviewing (CAPI), or computer-assisted mobile interviewing (CAMI). Data collection method in which the interviewer reads questions to the respondents from the screen of a computer, laptop, or a mobile device like tablet or smartphone, and enters the answers in the same device. The administration of the interview is managed by a specifically designed program/application.</skos:definition>
      <skos:prefLabel xml:lang="de">Pers&#xf6;nliches Interview: Computerunterst&#xfc;tzte Befragung (CAPI/CAMI)</skos:prefLabel>
      <skos:definition xml:lang="de">Computerunterst&#xfc;tzte pers&#xf6;nliche Befragung (CAPI) oder computerunterst&#xfc;tzte mobile Befragung (CAMI). Eine Datenerhebungsmethode, bei der der/die Interviewer*in den Befragten die Fragen vom Bildschirm eines Computers, Laptops oder eines mobilen Ger&#xe4;ts wie Tablet oder Smartphone vorliest und die Antworten in dasselbe Ger&#xe4;t eingibt. Die Durchf&#xfc;hrung des Interviews wird von einem speziell entwickelten Programm/einer Anwendung gesteuert.</skos:definition>
      <skos:prefLabel xml:lang="no">Personlig intervju: CAPI/CAMI</skos:prefLabel>
      <skos:definition xml:lang="no">Dataassistert personlig intervjuing (CAPI), eller dataassistert mobil intervjuing (CAMI). Datainnsamlingsmetode hvor intervjueren leser opp sp&#xf8;rsm&#xe5;l for respondenten fra skjermen til en datamaskin, b&#xe6;rbar datamaskin, smarttelefon eller nettbrett, og registrerer svarene p&#xe5; det samme apparatet. Administreringen av intervjuet er styrt av et spesialdesignet program eller en applikasjon.</skos:definition>
      <skos:prefLabel xml:lang="lt">Tiesioginis interviu: kompiuterizuotas interviu (CAPI/CAMI)</skos:prefLabel>
      <skos:definition xml:lang="lt">Kompiuterizuotas tiesioginis interviu (CAPI) arba kompiuterizuotas interviu mobiliaisiais &#x12f;renginiais (CAMI). Duomen&#x173; rinkimo metodas, kai apklaus&#x117;jas skaito klausimus respondentams i&#x161; kompiuterio, ne&#x161;iojamojo kompiuterio ar mobiliojo prietaiso, pavyzd&#x17e;iui, plan&#x161;etinio kompiuterio ar i&#x161;maniojo telefono, ekrano ir &#x12f;veda atsakymus &#x12f; t&#x105; pat&#x12f; &#x12f;rengin&#x12f;. Interviu administravimas vykdomas specialiai sukurta kompiuterine programa.</skos:definition>
      <skos:prefLabel xml:lang="it">Intervista faccia a faccia: computer-assistita (CAPI/CAMI)</skos:prefLabel>
      <skos:definition xml:lang="it">Interviste personali assistite da computer (CAPI) o da cellulare (CAMI). Metodo di raccolta dei dati in cui l&apos;intervistatore legge le domande ai rispondenti dallo schermo di un computer, laptop o dispositivo mobile come un tablet o uno smartphone e inserisce le risposte nello stesso dispositivo. L&apos;intervista &#xe8; gestita da un programma/applicazione appositamente progettata.</skos:definition>
      <skos:prefLabel xml:lang="fr">Entretien en face-&#xe0;-face : assist&#xe9; par ordinateur (CAPI / CAMI)</skos:prefLabel>
      <skos:definition xml:lang="fr">Entretien assist&#xe9; par ordinateur (CAPI), ou entretien assist&#xe9; par un appareil mobile (CAMI). M&#xe9;thode de collecte des donn&#xe9;es dans laquelle l&apos;enqu&#xea;teur lit les questions aux r&#xe9;pondants depuis l&apos;&#xe9;cran d&apos;un ordinateur (fixe ou portable) ou d&apos;un appareil mobile tel qu&apos;une tablette ou un smartphone, et saisit les r&#xe9;ponses sur le m&#xea;me appareil. L&apos;administration de l&apos;entretien est g&#xe9;r&#xe9;e par un programme ou une application d&#xe9;velopp&#xe9; sp&#xe9;cifiquement.</skos:definition>
      <skos:prefLabel xml:lang="nl">Face-to-face interview: Computer-assisted (CAPI/CAMI)</skos:prefLabel>
      <skos:definition xml:lang="nl"></skos:definition>
   </rdf:Description>
   <rdf:Description rdf:about="http://rdf-vocabulary.ddialliance.org/cv/ModeOfCollection/5.0.0/e477963">
      <rdf:type rdf:resource="http://www.w3.org/2004/02/skos/core#Concept"/>
      <skos:inScheme rdf:resource="http://rdf-vocabulary.ddialliance.org/cv/ModeOfCollection/5.0.0/"/>
      <skos:notation xml:lang="en">Interview.FaceToFace.PAPI</skos:notation>
      <skos:prefLabel xml:lang="sl">Osebni intervju: PAPI</skos:prefLabel>
      <skos:definition xml:lang="sl">&quot;Intervjuvanje s papirjem in svin&#x10d;nikom&quot;. Spra&#x161;evalec uporabi tradicionalni papirnati vpra&#x161;alnik, s katerega prebere vpra&#x161;anja in vnese odgovore.</skos:definition>
      <skos:prefLabel xml:lang="sv">Personlig intervju: PAPI</skos:prefLabel>
      <skos:definition xml:lang="sv">Papper-och-penna-intervju. Intervjuaren anv&#xe4;nder ett traditionellt fr&#xe5;geformul&#xe4;r p&#xe5; papper f&#xf6;r att l&#xe4;sa fr&#xe5;gorna och skriva ned svaren.</skos:definition>
      <skos:prefLabel xml:lang="en">Face-to-face interview: Paper-and-pencil (PAPI)</skos:prefLabel>
      <skos:definition xml:lang="en">Paper-and-pencil interviewing (PAPI). The interviewer uses a traditional paper questionnaire to read the questions and enter the answers.</skos:definition>
      <skos:prefLabel xml:lang="de">Pers&#xf6;nliches Interview: Papier-und-Bleistift (PAPI)</skos:prefLabel>
      <skos:definition xml:lang="de">Der/die Interviewer*in verwendet einen traditionellen Papierfragebogen, um die Fragen zu vorzulesen und die Antworten einzutragen.</skos:definition>
      <skos:prefLabel xml:lang="no">Personlig intervju: PAPI</skos:prefLabel>
      <skos:definition xml:lang="no">Penn og papir intervju. Intervjueren bruker et tradisjonelt papirsp&#xf8;rreskjema for &#xe5; lese opp sp&#xf8;rsm&#xe5;lene og til &#xe5; registrere svarene.</skos:definition>
      <skos:prefLabel xml:lang="lt">Tiesioginis interviu: interviu popieriumi ir pie&#x161;tuku (PAPI)</skos:prefLabel>
      <skos:definition xml:lang="lt">Interviu popieriumi ir pie&#x161;tuku (PAPI). Apklaus&#x117;jas naudojasi tradiciniu popieriniu klausimynu, skaitydamas klausimus ir fiksuodamas atsakymus.</skos:definition>
      <skos:prefLabel xml:lang="it">Intervista faccia a faccia: carta e penna (PAPI)</skos:prefLabel>
      <skos:definition xml:lang="it">Interviste con carta e penna (PAPI). L&apos;intervistatore utilizza un tradizionale questionario cartaceo per leggere le domande e inserire le risposte.</skos:definition>
      <skos:prefLabel xml:lang="fr">Entretien en face-&#xe0;-face : papier et crayon (PAPI)</skos:prefLabel>
      <skos:definition xml:lang="fr">Entretien avec papier et crayon (PAPI). L&apos;enqu&#xea;teur utilise un questionnaire papier traditionnel pour lire les questions et &#xe9;crire les r&#xe9;ponses.</skos:definition>
      <skos:prefLabel xml:lang="nl">Face-to-face interview: Paper-and-pencil (PAPI)</skos:prefLabel>
      <skos:definition xml:lang="nl"></skos:definition>
   </rdf:Description>
   <rdf:Description rdf:about="http://rdf-vocabulary.ddialliance.org/cv/ModeOfCollection/5.0.0/ae68e25">
      <rdf:type rdf:resource="http://www.w3.org/2004/02/skos/core#Concept"/>
      <skos:inScheme rdf:resource="http://rdf-vocabulary.ddialliance.org/cv/ModeOfCollection/5.0.0/"/>
      <skos:notation xml:lang="en">Interview.Telephone</skos:notation>
      <skos:prefLabel xml:lang="sl">Telefonski intervju</skos:prefLabel>
      <skos:definition xml:lang="sl">Intervju, izveden preko telefona. Uporabite ta &#x161;ir&#x161;i izraz, &#x10d;e ni CATI, oziroma ne veste, ali je CATI ali ne.</skos:definition>
      <skos:prefLabel xml:lang="sv">Telefonintervju</skos:prefLabel>
      <skos:definition xml:lang="sv">Intervju som genomf&#xf6;rs &#xf6;ver telefon. Anv&#xe4;nd denna bredare term om det inte r&#xf6;r sig om CATI, eller om det inte &#xe4;r k&#xe4;nt huruvida det r&#xf6;r sig om CATI.</skos:definition>
      <skos:prefLabel xml:lang="en">Telephone interview</skos:prefLabel>
      <skos:definition xml:lang="en">Interview administered on the telephone. Use this broader term if not CATI, or if not known whether CATI or not.</skos:definition>
      <skos:prefLabel xml:lang="de">Telefonisches Interview</skos:prefLabel>
      <skos:definition xml:lang="de">Interview, das am Telefon durchgef&#xfc;hrt wird. Verwenden Sie diesen weiter gefassten Begriff, wenn es sich nicht um CATI handelt, oder wenn nicht bekannt ist, ob es sich um CATI handelt oder nicht.</skos:definition>
      <skos:prefLabel xml:lang="no">Telefonintervju</skos:prefLabel>
      <skos:definition xml:lang="no">Intervju som gjennomf&#xf8;res over telefon. Bruk dette bredere begrepet dersom det ikke er CATI, eller dersom det er uvisst om det er CATI.</skos:definition>
      <skos:prefLabel xml:lang="lt">Interviu telefonu</skos:prefLabel>
      <skos:definition xml:lang="lt">Interviu vykdomas telefonu. Naudoti &#x161;&#x12f; platesn&#x12f; termin&#x105;, kai netinka CATI, arba jei ne&#x17e;inoma, ar tinka CATI.</skos:definition>
      <skos:prefLabel xml:lang="it">Intervista telefonica</skos:prefLabel>
      <skos:definition xml:lang="it">Intervista somministrata via telefono. Utilizzare questo termine pi&#xf9; generale se non &#xe8; CATI, o se non si &#xe8; in grado di stabilire se lo sia.</skos:definition>
      <skos:prefLabel xml:lang="fr">Entretien t&#xe9;l&#xe9;phonique</skos:prefLabel>
      <skos:definition xml:lang="fr">Entretien administr&#xe9; par t&#xe9;l&#xe9;phone. Utilisez ce terme si pas CATI, ou si vous ne savez pas si CATI ou pas.</skos:definition>
      <skos:prefLabel xml:lang="nl">Telefonisch interview</skos:prefLabel>
      <skos:definition xml:lang="nl"></skos:definition>
      <skos:narrower rdf:resource="http://rdf-vocabulary.ddialliance.org/cv/ModeOfCollection/5.0.0/1498dd4"/>
   </rdf:Description>
   <rdf:Description rdf:about="http://rdf-vocabulary.ddialliance.org/cv/ModeOfCollection/5.0.0/1498dd4">
      <rdf:type rdf:resource="http://www.w3.org/2004/02/skos/core#Concept"/>
      <skos:inScheme rdf:resource="http://rdf-vocabulary.ddialliance.org/cv/ModeOfCollection/5.0.0/"/>
      <skos:notation xml:lang="en">Interview.Telephone.CATI</skos:notation>
      <skos:prefLabel xml:lang="sl">Telefonski intervju: CATI</skos:prefLabel>
      <skos:definition xml:lang="sl">Ra&#x10d;unalni&#x161;ko podprto telefonsko intervjuvanje. Spra&#x161;evanec postavlja vpra&#x161;anja, ki jih ponuja ra&#x10d;unalnik, odgovori se vna&#x161;ajo neposredno v ra&#x10d;unalnik in intervju upravlja posebej za to zasnovan program.</skos:definition>
      <skos:prefLabel xml:lang="sv">Telefonintervju: CATI</skos:prefLabel>
      <skos:definition xml:lang="sv">Datorst&#xf6;dd telefonintervju. Intervjuaren l&#xe4;ser fr&#xe5;gor f&#xf6;r respondenterna fr&#xe5;n en datorsk&#xe4;rm och skriver in svaren direkt i datorn. Intervjun hanteras genom ett program som utvecklats f&#xf6;r detta syfte.</skos:definition>
      <skos:prefLabel xml:lang="en">Telephone interview: Computer-assisted (CATI)</skos:prefLabel>
      <skos:definition xml:lang="en">Computer-assisted telephone interviewing (CATI). The interviewer asks questions as directed by a computer, responses are keyed directly into the computer and the administration of the interview is managed by a specifically designed program.</skos:definition>
      <skos:prefLabel xml:lang="de">Telefonisches Interview: Computerunterst&#xfc;tzte Befragung (CATI)</skos:prefLabel>
      <skos:definition xml:lang="de">Computerunterst&#xfc;tzte telefonische Befragung (CATI). Der/die Interviewer*in stellt Fragen, die von einem Computer gesteuert werden, die Antworten werden direkt in den Computer eingegeben und die Durchf&#xfc;hrung des Interviews wird von einem speziell entwickelten Programm gesteuert.</skos:definition>
      <skos:prefLabel xml:lang="no">Telefonintervju: CATI</skos:prefLabel>
      <skos:definition xml:lang="no">Dataassistert telefonintervju (CATI). Intervjueren stiller sp&#xf8;rsm&#xe5;l if&#xf8;lge instrukser fra en datamaskin, registrerer svarene direkte p&#xe5; datamaskinen og administreringen av intervjuet er styrt av et spesialdesignet dataprogram.</skos:definition>
      <skos:prefLabel xml:lang="lt">Telefoninis interviu: kompiuterizuotas interviu (CATI)</skos:prefLabel>
      <skos:definition xml:lang="lt">Kompiuterizuotas interviu telefonu (CATI). Apklaus&#x117;jas u&#x17e;duoda klausimus pagal kompiuterio nurodymus, atsakymus &#x12f;vesdamas tiesiai &#x12f; kompiuter&#x12f;, o pokalbio administravim&#x105; vykdo specialiai tam sukurta kompiuterin&#x117; programa.</skos:definition>
      <skos:prefLabel xml:lang="it">Intervista telefonica: assistita da computer (CATI)</skos:prefLabel>
      <skos:definition xml:lang="it">Intervista telefonica assistita da computer (CATI). L&apos;intervistatore pone le domande indicate dal computer, le risposte sono immesse direttamente nel computer e l&apos;intervista &#xe8; gestita da un programma appositamente progettato.</skos:definition>
      <skos:prefLabel xml:lang="fr">Entretien t&#xe9;l&#xe9;phonique : assist&#xe9; par ordinateur (CATI)</skos:prefLabel>
      <skos:definition xml:lang="fr">Entretien t&#xe9;l&#xe9;phonique assist&#xe9; par ordinateur (CATI). L&apos;enqu&#xea;teur pose des questions selon les directives de l&apos;ordinateur, des r&#xe9;ponses sont saisies directement dans l&apos;ordinateur et l&apos;administration de l&apos;entretien est g&#xe9;r&#xe9;e pas un programme d&#xe9;velopp&#xe9; sp&#xe9;cialement.</skos:definition>
      <skos:prefLabel xml:lang="nl">Telefonisch interview: Computer-assisted (CATI)</skos:prefLabel>
      <skos:definition xml:lang="nl"></skos:definition>
   </rdf:Description>
   <rdf:Description rdf:about="http://rdf-vocabulary.ddialliance.org/cv/ModeOfCollection/5.0.0/b0b2868">
      <rdf:type rdf:resource="http://www.w3.org/2004/02/skos/core#Concept"/>
      <skos:inScheme rdf:resource="http://rdf-vocabulary.ddialliance.org/cv/ModeOfCollection/5.0.0/"/>
      <skos:notation xml:lang="en">Interview.Email</skos:notation>
      <skos:prefLabel xml:lang="sl">Intervju preko elektronske po&#x161;te</skos:prefLabel>
      <skos:definition xml:lang="sl">Intervju, izveden preko elektronske po&#x161;te. Obi&#x10d;ajno ga sestavlja ve&#x10d; elektronskih sporo&#x10d;il, ki omogo&#x10d;ajo, da se pogovor nadaljuje tudi po prvem nizu vpra&#x161;anj in odgovorov, ali po prvi izmenjavi elektronskih sporo&#x10d;il.</skos:definition>
      <skos:prefLabel xml:lang="sv">E-postintervju</skos:prefLabel>
      <skos:definition xml:lang="sv">Intervju som genomf&#xf6;rs via e-post, vanligtvis &#xf6;ver flera meddelanden som m&#xf6;jligg&#xf6;r att diskussionen forts&#xe4;tter fr&#xe5;n den f&#xf6;rsta upps&#xe4;ttningen av fr&#xe5;gor och svar eller det f&#xf6;rsta utbytet av e-brev.</skos:definition>
      <skos:prefLabel xml:lang="en">E-mail interview</skos:prefLabel>
      <skos:definition xml:lang="en">Interviews conducted via e-mail, usually consisting of several e-mail messages that allow the discussion to continue beyond the first set of questions and answers, or the first e-mail exchange.</skos:definition>
      <skos:prefLabel xml:lang="de">E-Mail Interview</skos:prefLabel>
      <skos:definition xml:lang="de">Interviews, die per E-Mail durchgef&#xfc;hrt werden und in der Regel aus mehreren E-Mail-Nachrichten bestehen, die es erm&#xf6;glichen, die Diskussion &#xfc;ber den ersten Satz von Fragen und Antworten bzw. den ersten E-Mail-Austausch hinaus fortzusetzen.</skos:definition>
      <skos:prefLabel xml:lang="no">E-post intervju</skos:prefLabel>
      <skos:definition xml:lang="no">Intervjuer gjennomf&#xf8;rt over e-post, vanligvis best&#xe5;ende av en rekke e-poster som gj&#xf8;r at diskusjonen kan fortsette utover de f&#xf8;rste settene med sp&#xf8;rsm&#xe5;l og svar, eller den f&#xf8;rste e-postutvekslingen.</skos:definition>
      <skos:prefLabel xml:lang="lt">Interviu elektroniniu pa&#x161;tu</skos:prefLabel>
      <skos:definition xml:lang="lt">Interviu vykdomi elektroniniu pa&#x161;tu, da&#x17e;niausiai susidedantys i&#x161; keli&#x173; elektroninio pa&#x161;to lai&#x161;k&#x173;, leid&#x17e;ian&#x10d;i&#x173; t&#x119;sti diskusij&#x105; po pirmos klausim&#x173; ir atsakym&#x173; sesijos arba po pirmojo apsikeitimo elektroniniais lai&#x161;kais.</skos:definition>
      <skos:prefLabel xml:lang="it">Intervista e-mail</skos:prefLabel>
      <skos:definition xml:lang="it">Interviste condotte via e-mail, di solito costituite da diversi messaggi di posta elettronica che consentono alla discussione di continuare oltre la prima serie di domande e risposte, oppure dopo il primo scambio di e-mail.</skos:definition>
      <skos:prefLabel xml:lang="fr">Entretien par e-mail</skos:prefLabel>
      <skos:definition xml:lang="fr">Entretiens conduits par e-mail, habituellement consistant en plusieurs e-mails qui permettent &#xe0; la discussion de se poursuivre au-del&#xe0; d&#x2019;une premi&#xe8;re s&#xe9;rie de questions et de r&#xe9;ponses, ou d&apos;un premier &#xe9;change d&apos;e-mails.</skos:definition>
      <skos:prefLabel xml:lang="nl">E-mail interview</skos:prefLabel>
      <skos:definition xml:lang="nl"></skos:definition>
   </rdf:Description>
   <rdf:Description rdf:about="http://rdf-vocabulary.ddialliance.org/cv/ModeOfCollection/5.0.0/1af2bfa">
      <rdf:type rdf:resource="http://www.w3.org/2004/02/skos/core#Concept"/>
      <skos:inScheme rdf:resource="http://rdf-vocabulary.ddialliance.org/cv/ModeOfCollection/5.0.0/"/>
      <skos:notation xml:lang="en">Interview.WebBased</skos:notation>
      <skos:prefLabel xml:lang="sl">Spletni intervju</skos:prefLabel>
      <skos:definition xml:lang="sl">Intervju preko spleta. Na primer, intervjuji izvedeni znotraj spletnih forumov ali z uporabo spletno osnovanih avdio-vizualnih tehnologij, ki omogo&#x10d;ajo komunikacijo spra&#x161;evalca(-cev) in spra&#x161;evanca(-cev) v realnem &#x10d;asu.</skos:definition>
      <skos:prefLabel xml:lang="sv">Webbaserad intervju</skos:prefLabel>
      <skos:definition xml:lang="sv">Intervju som genomf&#xf6;rs &#xf6;ver Internet. Exempel inkluderar intervjuer genomf&#xf6;rda p&#xe5; onlineforum eller med hj&#xe4;lp av webbaserad audiovisuell teknik som till&#xe5;ter att intervjuare och intervjuobjekt kan kommunicera i realtid.</skos:definition>
      <skos:prefLabel xml:lang="en">Web-based interview</skos:prefLabel>
      <skos:definition xml:lang="en">An interview conducted via the Internet. For example, interviews conducted within online forums or using web-based audio-visual technology that enables the interviewer(s) and interviewee(s) to communicate in real time.</skos:definition>
      <skos:prefLabel xml:lang="de">Webbasiertes Interview</skos:prefLabel>
      <skos:definition xml:lang="de">Ein Interview, das &#xfc;ber das Internet gef&#xfc;hrt wird. Zum Beispiel Interviews, die in Online-Foren oder mit webbasierter audiovisueller Technologie durchgef&#xfc;hrt werden, die es dem/der Interviewer*in bzw. den Interviewern und dem/der/den Befragten erm&#xf6;glicht, in Echtzeit zu kommunizieren.</skos:definition>
      <skos:prefLabel xml:lang="no">Webbasert intervju</skos:prefLabel>
      <skos:definition xml:lang="no">Intervju gjennomf&#xf8;rt over internett. For eksempel, intervjuer gjennomf&#xf8;rt p&#xe5; internettforum eller ved bruk av internettbasert audiovisuell teknologi som muliggj&#xf8;r fortl&#xf8;pende kommunikasjon mellom intervjuer(e) og Intervjuobjekt(er).</skos:definition>
      <skos:prefLabel xml:lang="lt">Interviu internetu </skos:prefLabel>
      <skos:definition xml:lang="lt">Interviu atliekami internetu. Pavyzd&#x17e;iui, interviu atliekami internetiniuose forumuose arba naudojant internetines garso ir vaizdo technologijas, leid&#x17e;ian&#x10d;ias apklaus&#x117;jui (-ams) ir apklausiamajam (-siems) bendrauti realiu laiku.</skos:definition>
      <skos:prefLabel xml:lang="it">Intervista web</skos:prefLabel>
      <skos:definition xml:lang="it">Un&apos;intervista condotta via Internet. Ad esempio, interviste condotte all&apos;interno di forum online o utilizzando la tecnologia audiovisiva basata sul web che consente all&apos;intervistatore e agli intervistati di comunicare in tempo reale.</skos:definition>
      <skos:prefLabel xml:lang="fr">Entretien par Internet</skos:prefLabel>
      <skos:definition xml:lang="fr">Un entretien conduit via Internet. Par exemple, des entretiens men&#xe9;s dans des forums en ligne ou utilisant des technologies web audio-vid&#xe9;o qui permettent au(x) enqu&#xea;teur(s) et au(x) r&#xe9;pondant(s) de communiquer en temps r&#xe9;el.</skos:definition>
      <skos:prefLabel xml:lang="nl">Webgebaseerd interview</skos:prefLabel>
      <skos:definition xml:lang="nl"></skos:definition>
   </rdf:Description>
   <rdf:Description rdf:about="http://rdf-vocabulary.ddialliance.org/cv/ModeOfCollection/5.0.0/35e4248">
      <rdf:type rdf:resource="http://www.w3.org/2004/02/skos/core#Concept"/>
      <skos:inScheme rdf:resource="http://rdf-vocabulary.ddialliance.org/cv/ModeOfCollection/5.0.0/"/>
      <skos:notation xml:lang="en">SelfAdministeredQuestionnaire</skos:notation>
      <skos:prefLabel xml:lang="sl">Vpra&#x161;alnik za samoizpolnjevanje</skos:prefLabel>
      <skos:definition xml:lang="sl">Metoda zbiranja podatkov, pri kateri spra&#x161;evanec bere ali poslu&#x161;a vpra&#x161;anja in sam vna&#x161;a odgovore; spra&#x161;evalec ni prisoten niti ne sodeluje pri upravljanju vpra&#x161;alnika. &#x10c;e je mo&#x17e;no, uporabite o&#x17e;ji izraz. Ta &#x161;ir&#x161;i izraz uporabite le, &#x10d;e metoda ni opisana z nobenem od o&#x17e;jih izrazov, npr. za PDF ali vpra&#x161;alnike na disketi.</skos:definition>
      <skos:prefLabel xml:lang="sv">Sj&#xe4;lvadministrerat fr&#xe5;geformul&#xe4;r</skos:prefLabel>
      <skos:definition xml:lang="sv">Respondenten l&#xe4;ser eller lyssnar p&#xe5; fr&#xe5;gorna och skriver sj&#xe4;lv in svaren; ingen intervjuare &#xe4;r n&#xe4;rvarande eller deltar i administrerandet av fr&#xe5;geformul&#xe4;ret. Anv&#xe4;nd om m&#xf6;jligt en smalare term. Anv&#xe4;nd denna bredare term om metoden inte beskrivits av n&#xe5;gon av de mer precisa termerna, till exempel f&#xf6;r fr&#xe5;geformul&#xe4;r i PDF-format eller p&#xe5; diskett.</skos:definition>
      <skos:prefLabel xml:lang="en">Self-administered questionnaire</skos:prefLabel>
      <skos:definition xml:lang="en">Data collection method in which the respondent reads or listens to the questions, and enters the responses by him/herself; no live interviewer is present, or participates in the questionnaire administration. If possible, use a narrower term. Use this broader term if the method is not described by any of the narrower terms - for example, for PDF and diskette questionnaires.</skos:definition>
      <skos:prefLabel xml:lang="de">Selbstausgef&#xfc;llter Fragebogen</skos:prefLabel>
      <skos:definition xml:lang="de">Datenerhebungsmethode, bei der Befragte die Fragen lesen oder h&#xf6;ren und die Antworten selbst eingeben; es ist kein Live-Interviewer anwesend oder beteiligt sich an der Fragebogenverwaltung. Wenn m&#xf6;glich, verwenden Sie einen engeren Begriff. Verwenden Sie diesen breiteren Begriff, wenn die Erhebungsmethode durch keinen der engeren Begriffe beschrieben wird - zum Beispiel f&#xfc;r PDF- und Diskettenfrageb&#xf6;gen.</skos:definition>
      <skos:prefLabel xml:lang="no">Selvadministrert sp&#xf8;rreskjema</skos:prefLabel>
      <skos:definition xml:lang="no">Datainnsamlingsmetode hvor respondenten leser eller lytter til sp&#xf8;rsm&#xe5;lene, og registrerer svarene p&#xe5; egenh&#xe5;nd; ingen intervjuer er til stede, eller deltar i administreringen av sp&#xf8;rreskjemaet. Bruk et smalere begrep dersom det er mulig. Bruk dette bredere begrepet dersom metoden ikke kan defineres av de smalere begrepene, for eksempel for PDF eller diskett sp&#xf8;rreskjemaer.</skos:definition>
      <skos:prefLabel xml:lang="lt">Savipildos klausimynas</skos:prefLabel>
      <skos:definition xml:lang="lt">Duomen&#x173; rinkimo b&#x16b;das, kai pats respondentas skaito ar klauso klausimus, ir pats &#x12f;veda atsakymus; tiesioginio apklaus&#x117;jo n&#x117;ra, arba jis nedalyvauja administruojant klausimyn&#x105;. Jei &#x12f;manoma, vartoti siauresn&#x12f; termin&#x105;. Naudoti &#x161;&#x12f; platesn&#x12f; termin&#x105;, kai metodui apib&#x16b;dinti netinka n&#x117; vienas siauresnis terminas, pavyzd&#x17e;iui, PDF ir diskeli&#x173; klausimynai.</skos:definition>
      <skos:prefLabel xml:lang="it">Questionario auto-compilato</skos:prefLabel>
      <skos:definition xml:lang="it">Tecnica di raccolta dei dati in cui il rispondente legge o ascolta le domande e inserisce autonomamente le risposte; nessun intervistatore &#xe8; presente o partecipa alla somministrazione del questionario. Se possibile, utilizzare un termine pi&#xf9; specifico. Utilizzare questo termine pi&#xf9; ampio se il metodo non &#xe8; descritto da nessuno dei termini pi&#xf9; specifici, ad esempio per i questionari PDF o trasmessi via floppy disk.</skos:definition>
      <skos:prefLabel xml:lang="fr">Questionnaire auto-administr&#xe9;</skos:prefLabel>
      <skos:definition xml:lang="fr">M&#xe9;thode de collecte de donn&#xe9;es dans laquelle l&apos;enqu&#xea;t&#xe9; lit ou &#xe9;coute les questions et saisit lui-m&#xea;me les r&#xe9;ponses ; aucun enqu&#xea;teur n&#x2019;est pr&#xe9;sent ni ne participe &#xe0; l&#x2019;administration du questionnaire. Si possible, utilisez un terme plus pr&#xe9;cis. Utilisez ce terme si la m&#xe9;thode n&apos;est d&#xe9;crite par aucun termes plus pr&#xe9;cis - par exemple, pour les questionnaires PDF ou sur disquette.</skos:definition>
      <skos:prefLabel xml:lang="nl">Zelf ingevulde vragenlijst</skos:prefLabel>
      <skos:definition xml:lang="nl"></skos:definition>
      <skos:narrower rdf:resource="http://rdf-vocabulary.ddialliance.org/cv/ModeOfCollection/5.0.0/69a46ca"/>
      <skos:narrower rdf:resource="http://rdf-vocabulary.ddialliance.org/cv/ModeOfCollection/5.0.0/6255fce"/>
      <skos:narrower rdf:resource="http://rdf-vocabulary.ddialliance.org/cv/ModeOfCollection/5.0.0/ddaefe8"/>
      <skos:narrower rdf:resource="http://rdf-vocabulary.ddialliance.org/cv/ModeOfCollection/5.0.0/557586d"/>
      <skos:narrower rdf:resource="http://rdf-vocabulary.ddialliance.org/cv/ModeOfCollection/5.0.0/e48ace5"/>
   </rdf:Description>
   <rdf:Description rdf:about="http://rdf-vocabulary.ddialliance.org/cv/ModeOfCollection/5.0.0/69a46ca">
      <rdf:type rdf:resource="http://www.w3.org/2004/02/skos/core#Concept"/>
      <skos:inScheme rdf:resource="http://rdf-vocabulary.ddialliance.org/cv/ModeOfCollection/5.0.0/"/>
      <skos:notation xml:lang="en">SelfAdministeredQuestionnaire.Email</skos:notation>
      <skos:prefLabel xml:lang="sl">Vpra&#x161;alnik za samoizpolnjevanje: elektronska po&#x161;ta</skos:prefLabel>
      <skos:definition xml:lang="sl">Vpra&#x161;alnik za samoizpolnjevanje, kjer so spra&#x161;evancu vpra&#x161;anja prikazana bodisi kot besedilo v telesu elektronskega sporo&#x10d;ila bodisi v priponki, vendar ne kot povezava do spletnega vpra&#x161;alnika. Prav tako so tudi odgovori poslani preko elektronskega sporo&#x10d;ila, bodisi v telesu elektronskega sporo&#x10d;ila, bodisi kot priponka.</skos:definition>
      <skos:prefLabel xml:lang="sv">Sj&#xe4;lvadministrerat fr&#xe5;geformul&#xe4;r: e-post</skos:prefLabel>
      <skos:definition xml:lang="sv">Sj&#xe4;lvadministrerad surveyunders&#xf6;kning d&#xe4;r fr&#xe5;gor skickas till respondenten i br&#xf6;dtexten p&#xe5;, eller som en bilaga till, ett e-brev, inte som en l&#xe4;nk till ett fr&#xe5;geformul&#xe4;r p&#xe5; webben. Svaren skickas tillbaka med e-post, i br&#xf6;dtexten eller som bilaga.</skos:definition>
      <skos:prefLabel xml:lang="en">Self-administered questionnaire: E-mail</skos:prefLabel>
      <skos:definition xml:lang="en">Self-administered survey in which questions are presented to the respondent in the text body of an e-mail or as an attachment to an e-mail, but not as a link to a web-based questionnaire. Responses are also sent back via e-mail, in the e-mail body or as an attachment.</skos:definition>
      <skos:prefLabel xml:lang="de">Selbstausgef&#xfc;llter Fragebogen: E-Mail</skos:prefLabel>
      <skos:definition xml:lang="de">Selbstverwaltete Umfrage, bei der die Fragen den Befragten im Textk&#xf6;rper einer E-Mail oder als Anhang zu einer E-Mail pr&#xe4;sentiert werden, nicht aber als Link zu einem webbasierten Fragebogen. Die Antworten werden ebenfalls per E-Mail zur&#xfc;ckgeschickt, im E-Mail-Textk&#xf6;rper oder als Anhang.</skos:definition>
      <skos:prefLabel xml:lang="no">Selvadministrert sp&#xf8;rreskjema: E-post</skos:prefLabel>
      <skos:definition xml:lang="no">Unders&#xf8;kelse hvor sp&#xf8;rsm&#xe5;l blir presentert til respondenten som tekst i en e-post eller som et vedlegg i en e-post, men ikke som lenke til et web-basert sp&#xf8;rreskjema. Svarene sendes ogs&#xe5; tilbake med e-post, enten som tekst i e-posten eller som et vedlegg.</skos:definition>
      <skos:prefLabel xml:lang="lt">Savipildos klausimynas: elektroniniu pa&#x161;tu</skos:prefLabel>
      <skos:definition xml:lang="lt">Savipildos b&#x16b;du atliekama apklausa, kurios metu respondentui klausimai pateikiami elektroninio lai&#x161;ko tekste arba prie elektroninio lai&#x161;ko pridedant pried&#x105;, bet ne kaip nuoroda &#x12f; internetin&#x119; anket&#x105;. Atsakymai taip pat siun&#x10d;iami elektroniniu lai&#x161;ku, jo pagrindiniame tekste arba kaip priedas.</skos:definition>
      <skos:prefLabel xml:lang="it">Questionario auto-compilato: e-mail</skos:prefLabel>
      <skos:definition xml:lang="it">Questionario auto-compilato in cui le domande vengono presentate all&apos;intervistato nel corpo del testo di un&apos;e-mail o come allegato a un&apos;e-mail, ma non come un collegamento a un questionario somministrato via web. Anche le risposte vengono rispedite via e-mail, nel corpo dell&apos;e-mail o come allegato.</skos:definition>
      <skos:prefLabel xml:lang="fr">Questionnaire auto-administr&#xe9; : e-mail</skos:prefLabel>
      <skos:definition xml:lang="fr">Enqu&#xea;te auto-administr&#xe9;e dans laquelle les questions sont pr&#xe9;sent&#xe9;es au r&#xe9;pondant dans le corps d&apos;un e-mail ou dans une pi&#xe8;ce jointe, mais pas comme un lien vers une enqu&#xea;te par Internet.  Les r&#xe9;ponses sont ensuite renvoy&#xe9;es par e-mail, soit dans le corps du message, soit en pi&#xe8;ce jointe.</skos:definition>
      <skos:prefLabel xml:lang="nl">Zelf ingevulde vragenlijst: E-mail</skos:prefLabel>
      <skos:definition xml:lang="nl"></skos:definition>
   </rdf:Description>
   <rdf:Description rdf:about="http://rdf-vocabulary.ddialliance.org/cv/ModeOfCollection/5.0.0/6255fce">
      <rdf:type rdf:resource="http://www.w3.org/2004/02/skos/core#Concept"/>
      <skos:inScheme rdf:resource="http://rdf-vocabulary.ddialliance.org/cv/ModeOfCollection/5.0.0/"/>
      <skos:notation xml:lang="en">SelfAdministeredQuestionnaire.Paper</skos:notation>
      <skos:prefLabel xml:lang="sl">Vpra&#x161;alnik za samoizpolnjevanje: papirnati</skos:prefLabel>
      <skos:definition xml:lang="sl">Vpra&#x161;alnik za samoizpolnjevanje z uporabo tradicionalnega papirnatega vpra&#x161;alnika poslanega in/ali prejetega preko tradicionalne po&#x161;tne storitve, preko faksa ali osebno preko spra&#x161;evalca ali spra&#x161;evanca.</skos:definition>
      <skos:prefLabel xml:lang="sv">Sj&#xe4;lvadministrerat fr&#xe5;geformul&#xe4;r: papper</skos:prefLabel>
      <skos:definition xml:lang="sv">Sj&#xe4;lvadministrerad surveyunders&#xf6;kning som anv&#xe4;nder traditionella fr&#xe5;geformul&#xe4;r p&#xe5; papper, vilka skickas ut och/eller in via post eller fax, eller l&#xe4;mnas &#xf6;ver personligen av antingen intervjuaren eller intervjuobjektet.</skos:definition>
      <skos:prefLabel xml:lang="en">Self-administered questionnaire: Paper</skos:prefLabel>
      <skos:definition xml:lang="en">Self-administered survey using a traditional paper questionnaire delivered and/or collected by mail (postal services), by fax, or in person by either interviewer, or respondent.</skos:definition>
      <skos:prefLabel xml:lang="de">Selbstausgef&#xfc;llter Fragebogen: Papier</skos:prefLabel>
      <skos:definition xml:lang="de">Selbstverwaltete Umfrage unter Verwendung eines traditionellen Papierfragebogens, der per Post (Postdienste), per Fax oder pers&#xf6;nlich entweder durch die Interviewer oder die Befragten zugestellt und/oder abgeholt wird.</skos:definition>
      <skos:prefLabel xml:lang="no">Selvadministrert sp&#xf8;rreskjema: Papir</skos:prefLabel>
      <skos:definition xml:lang="no">Selvadministrert sp&#xf8;rreskjema som bruker tradisjonelle sp&#xf8;rsm&#xe5;lsformuleringer p&#xe5; papir, som blir levert og/eller samlet inn via post, faks, eller personlig av intervjueren eller respondenten.</skos:definition>
      <skos:prefLabel xml:lang="lt">Savipildos klausimynas: popieriuje </skos:prefLabel>
      <skos:definition xml:lang="lt">Savipildos b&#x16b;du atliekama apklausa, naudojant tradicin&#x12f; popierin&#x12f; klausimyn&#x105;, kai klausimynas pateikiamas ir (arba) surenkamas pa&#x161;tu (pa&#x161;to paslauga), faksu arba asmeni&#x161;kai paties apklaus&#x117;jo ar respondento.</skos:definition>
      <skos:prefLabel xml:lang="it">Questionario auto-compilato: cartaceo</skos:prefLabel>
      <skos:definition xml:lang="it">Questionario cartaceo tradizionale auto-compilato, consegnato e/o ritirato per posta (servizi postali), via fax o di persona dall&apos;intervistatore oppure dall&apos;intervistato.</skos:definition>
      <skos:prefLabel xml:lang="fr">Questionnaire auto-administr&#xe9; : papier</skos:prefLabel>
      <skos:definition xml:lang="fr">Enqu&#xea;te auto-administr&#xe9;e utilisant un questionnaire papier traditionnel distribu&#xe9; et / ou recueilli par courrier (services postaux), par fax ou en personne, soit par un enqu&#xea;teur, soit par un r&#xe9;pondant.</skos:definition>
      <skos:prefLabel xml:lang="nl">Zelf ingevulde vragenlijst: Papier</skos:prefLabel>
      <skos:definition xml:lang="nl"></skos:definition>
   </rdf:Description>
   <rdf:Description rdf:about="http://rdf-vocabulary.ddialliance.org/cv/ModeOfCollection/5.0.0/ddaefe8">
      <rdf:type rdf:resource="http://www.w3.org/2004/02/skos/core#Concept"/>
      <skos:inScheme rdf:resource="http://rdf-vocabulary.ddialliance.org/cv/ModeOfCollection/5.0.0/"/>
      <skos:notation xml:lang="en">SelfAdministeredQuestionnaire.SMSorMMS</skos:notation>
      <skos:prefLabel xml:lang="sl">Vpra&#x161;alnik za samoizpolnjevanje: SMS/MMS</skos:prefLabel>
      <skos:definition xml:lang="sl">Vpra&#x161;alnik za samoizpolnjevanje, kjer spra&#x161;evanec prejme vpra&#x161;anja, vklju&#x10d;ena v kratkih sporo&#x10d;ilih v formatu SMS (tekstovna sporo&#x10d;ila) ali MMS (multimedijska sporo&#x10d;ila) in odgovore po&#x161;lje v enakem formatu.</skos:definition>
      <skos:prefLabel xml:lang="sv">Sj&#xe4;lvadministrerat fr&#xe5;geformul&#xe4;r: SMS/MMS</skos:prefLabel>
      <skos:definition xml:lang="sv">Sj&#xe4;lvadministrerad surveyunders&#xf6;kning d&#xe4;r fr&#xe5;gor och svar inkluderas i SMS (textmeddelanden) eller MMS (meddelanden med multimedia-inneh&#xe5;ll) som skickas mellan mobiltelefoner.</skos:definition>
      <skos:prefLabel xml:lang="en">Self-administered questionnaire: Messaging (SMS/MMS)</skos:prefLabel>
      <skos:definition xml:lang="en">Self-administered survey in which the respondents receive the questions incorporated in SMS (text messages) or MMS (messages including multimedia content) and send their replies in the same format.</skos:definition>
      <skos:prefLabel xml:lang="de">Selbstausgef&#xfc;llter Fragebogen: Nachrichten&#xfc;bermittlung (SMS/MMS)</skos:prefLabel>
      <skos:definition xml:lang="de">Selbstverwaltete Umfrage, bei der die Befragten die Fragen in SMS (Textnachrichten) oder MMS (Nachrichten mit multimedialen Inhalten) eingebunden erhalten und ihre Antworten im gleichen Format senden.</skos:definition>
      <skos:prefLabel xml:lang="no">Selvadministrert sp&#xf8;rreskjema: SMS/MMS</skos:prefLabel>
      <skos:definition xml:lang="no">Selvadministrert sp&#xf8;rreskjema hvor respondenten mottar sp&#xf8;rsm&#xe5;l p&#xe5; SMS (tekstmeldinger) eller MMS (meldinger med multimedia innhold) og sender svarene i samme format.</skos:definition>
      <skos:prefLabel xml:lang="lt">Savipildos klausimynas: &#x17e;inut&#x117;mis (SMS/MMS)</skos:prefLabel>
      <skos:definition xml:lang="lt">Savipildos b&#x16b;du atliekama apklausa, kurios metu respondentai gauna klausimus kaip SMS (tekstine &#x17e;inute) arba MMS (&#x17e;inutes, &#x12f;traukian&#x10d;ias daugialyp&#x117;s terp&#x117;s turin&#x12f;), ir siun&#x10d;ia savo atsakymus tuo pa&#x10d;iu formatu.</skos:definition>
      <skos:prefLabel xml:lang="it">Questionario auto-compilato: messaggistica (SMS/MMS)</skos:prefLabel>
      <skos:definition xml:lang="it">Questionario auto-compilato in cui gli intervistati ricevono le domande all&apos;interno di in SMS (messaggi di testo) o MMS (messaggi che includono contenuti multimediali) e inviano le loro risposte nello stesso formato.</skos:definition>
      <skos:prefLabel xml:lang="fr">Questionnaire auto-administr&#xe9; : par messagerie (SMS / MMS)</skos:prefLabel>
      <skos:definition xml:lang="fr">Enqu&#xea;te auto-administr&#xe9;e dans laquelle les r&#xe9;pondants re&#xe7;oivent les questions par SMS (texte uniquement) ou MMS (messages incluant des contenus multim&#xe9;dia) et envoient leurs r&#xe9;ponses dans le m&#xea;me format.</skos:definition>
      <skos:prefLabel xml:lang="nl">Zelf ingevulde vragenlijst: Bericht (SMS/MMS)</skos:prefLabel>
      <skos:definition xml:lang="nl"></skos:definition>
   </rdf:Description>
   <rdf:Description rdf:about="http://rdf-vocabulary.ddialliance.org/cv/ModeOfCollection/5.0.0/557586d">
      <rdf:type rdf:resource="http://www.w3.org/2004/02/skos/core#Concept"/>
      <skos:inScheme rdf:resource="http://rdf-vocabulary.ddialliance.org/cv/ModeOfCollection/5.0.0/"/>
      <skos:notation xml:lang="en">SelfAdministeredQuestionnaire.CAWI</skos:notation>
      <skos:prefLabel xml:lang="sl">Vpra&#x161;alnik za samoizpolnjevanje: spletni</skos:prefLabel>
      <skos:definition xml:lang="sl">Ra&#x10d;unalni&#x161;ko podprto spletno intervjuvanje (CAWI). Podatki so zbrani z uporabo spletnega vpra&#x161;alnika, ustvarjenega v programskem orodju za spletno anketiranje. Program lahko tok vpra&#x161;alnika prilagodi odgovorom na prej&#x161;nja vpra&#x161;anja, omogo&#x10d;a lahko vstavljanje slik ter avdio in video posnetkov, povezave do spletnih strani itd.</skos:definition>
      <skos:prefLabel xml:lang="sv">Sj&#xe4;lvadministrerat fr&#xe5;geformul&#xe4;r: webbaserat</skos:prefLabel>
      <skos:definition xml:lang="sv">Computer-assisted web interviewing (CAWI). Data samlas in med ett webbformul&#xe4;r som producerats av ett program som skapar webbsurveyer. Programmet kan anpassa fl&#xf6;det i fr&#xe5;geformul&#xe4;ret utifr&#xe5;n svaren som ges och det g&#xe5;r att inkludera bilder, ljud- och videoklipp, l&#xe4;nkar till andra webbsidor m.m. (Anpassad fr&#xe5;n Wikipedia.)</skos:definition>
      <skos:prefLabel xml:lang="en">Self-administered questionnaire: Web-based (CAWI)</skos:prefLabel>
      <skos:definition xml:lang="en">Computer-assisted web interviewing (CAWI). Data are collected using a web questionnaire, produced with a program for creating web surveys. The program can customize the flow of the questionnaire based on the answers provided, and can allow for the questionnaire to contain pictures, audio and video clips, links to different web pages etc.</skos:definition>
      <skos:prefLabel xml:lang="de">Selbstausgef&#xfc;llter Fragebogen: Webbasiert (CAWI)</skos:prefLabel>
      <skos:definition xml:lang="de">Computerunterst&#xfc;tzte Webbefragung (CAWI). Die Daten werden mithilfe eines Web-Fragebogens erhoben, der mit einem Programm zur Erstellung von Web-Umfragen erstellt wird. Das Programm kann den Ablauf des Fragebogens auf der Grundlage der gegebenen Antworten anpassen und es erm&#xf6;glichen, dass der Fragebogen Bilder, Audio- und Videoclips, sowie Links zu verschiedenen Webseiten usw. enth&#xe4;lt.</skos:definition>
      <skos:prefLabel xml:lang="no">Selvadministrert sp&#xf8;rreskjema: Webbasert (CAWI)</skos:prefLabel>
      <skos:definition xml:lang="no">Datamaskinaassistert webintervju (CAWI). Data samles ved hjelp av sp&#xf8;rreskjema p&#xe5; nett, som er produsert av et program for internettunders&#xf8;kelser. Programmet kan endre flyten av sp&#xf8;rsm&#xe5;l basert p&#xe5; svarene som blir gitt, og det muliggj&#xf8;r inkludering av bilde, lyd og video, lenker til andre nettsider etc.</skos:definition>
      <skos:prefLabel xml:lang="lt">Savipildos klausimynas: internetu (CAWI)</skos:prefLabel>
      <skos:definition xml:lang="lt">Kompiuterizuotas interviu internetu (CAWI). Duomenys renkami naudojant internetin&#x12f; klausimyn&#x105;, parengt&#x105; su internetini&#x173; apklaus&#x173; k&#x16b;rimo programa. Priklausomai nuo pateikiam&#x173; atsakym&#x173;, programa gali pritaikyti klausim&#x173; eili&#x161;kum&#x105;. Tokia programa taip pat leid&#x17e;ia &#x12f; klausimyn&#x105; &#x12f;d&#x117;ti paveiksl&#x117;lius, garso ir vaizdo &#x12f;ra&#x161;us, nuorodas &#x12f; &#x12f;vairius tinklalapius ir kt.</skos:definition>
      <skos:prefLabel xml:lang="it">Questionario auto-compilato: web (CAWI)</skos:prefLabel>
      <skos:definition xml:lang="it">Intervista web assistita da computer (CAWI). I dati vengono raccolti utilizzando un questionario via web, prodotto con un programma per la creazione di indagini via web. Il programma pu&#xf2; personalizzare la struttura del questionario in base alle risposte fornite, e pu&#xf2; consentire al questionario di contenere immagini, clip audio e video, collegamenti a pagine web diverse, ecc.</skos:definition>
      <skos:prefLabel xml:lang="fr">Questionnaire auto-administr&#xe9; : par Internet (CAWI)</skos:prefLabel>
      <skos:definition xml:lang="fr">Entretien par Internet assist&#xe9; par ordinateur (CAWI). Les donn&#xe9;es sont collect&#xe9;es &#xe0; l&#x2019;aide d&#x2019;un questionnaire en ligne, cr&#xe9;&#xe9; avec un programme de conception d&#x2019;enqu&#xea;tes en ligne. Le programme peut personnaliser le d&#xe9;roulement du questionnaire en fonction des r&#xe9;ponses fournies, et peut permettre au questionnaire de contenir des images, des clips audio et vid&#xe9;o, des liens vers diff&#xe9;rentes pages Web, etc.</skos:definition>
      <skos:prefLabel xml:lang="nl">Zelf ingevulde vragenlijst: Webgebaseerd (CAWI)</skos:prefLabel>
      <skos:definition xml:lang="nl"></skos:definition>
   </rdf:Description>
   <rdf:Description rdf:about="http://rdf-vocabulary.ddialliance.org/cv/ModeOfCollection/5.0.0/e48ace5">
      <rdf:type rdf:resource="http://www.w3.org/2004/02/skos/core#Concept"/>
      <skos:inScheme rdf:resource="http://rdf-vocabulary.ddialliance.org/cv/ModeOfCollection/5.0.0/"/>
      <skos:notation xml:lang="en">SelfAdministeredQuestionnaire.CASI</skos:notation>
      <skos:prefLabel xml:lang="sl">Vpra&#x161;alnik za samoizpolnjevanje: ra&#x10d;unalni&#x161;ko podprti (CASI)</skos:prefLabel>
      <skos:definition xml:lang="sl">Ra&#x10d;unalni&#x161;ko podprto samoizpolnjevanje (CASI). Spra&#x161;evanec sam vstavlja odgovore v ra&#x10d;unalnik (namizni, prenosni, dlan&#x10d;ni/PDA, tabli&#x10d;ni itd.). Z vpra&#x161;alnikom upravlja posebej zasnovani program/aplikacija, vendar pri tem ni prenosa v realnem &#x10d;asu kot pri CAWI, vpra&#x161;anja se shranjujejo na napravi, ki se uporablja za intervju. Vpra&#x161;alnik je lahko v fiksni obliki ali interaktiven. Vklju&#x10d;uje tudi VCASI (video ra&#x10d;unalni&#x161;ko podprto samoizpolnjevanje), ACASI (avdio ra&#x10d;unalni&#x161;ko podprto samoizpolnjevanje) in TACASI (telefonsko avdio ra&#x10d;unalni&#x161;ko podprto samoizpolnjevanje).</skos:definition>
      <skos:prefLabel xml:lang="sv">Sj&#xe4;lvadministrerat fr&#xe5;geformul&#xe4;r: med datorst&#xf6;d (CASI)</skos:prefLabel>
      <skos:definition xml:lang="sv">Computer-assisted self-interview (CASI). Respondenterna noterar sj&#xe4;lva sina svar i en dator (station&#xe4;r eller b&#xe4;rbar, Palm/PDA, surfplatta e. dyl.). Fr&#xe5;geformul&#xe4;ret administreras med ett datorprogram som utvecklats f&#xf6;r detta syfte men data &#xf6;verf&#xf6;rs inte i realtid som i fallet med CAWI: svaren lagras p&#xe5; datorn som anv&#xe4;nds f&#xf6;r intervjun. Fr&#xe5;geformul&#xe4;ret kan vara statiskt eller interaktivt. Omfattar VCASI (Video Computer-Assisted Self-Interview), ACASI (Audio computer-assisted self-interview) och TCASI (Telephone audio computer-assisted self-interview).</skos:definition>
      <skos:prefLabel xml:lang="en">Self-administered questionnaire: Computer-assisted (CASI)</skos:prefLabel>
      <skos:definition xml:lang="en">Computer-assisted self-interview (CASI). Respondents enter the responses into a computer (desktop, laptop, Palm/PDA, tablet, etc.) by themselves. The administration of the questionnaire is managed by a specifically designed program/application but there is no real-time data transfer as in CAWI, the answers are stored on the device used for the interview. The questionnaire may be fixed form or interactive. Includes VCASI (Video computer-assisted self-interviewing), ACASI (Audio computer-assisted self-interviewing) and TACASI (Telephone audio computer-assisted self-interviewing).</skos:definition>
      <skos:prefLabel xml:lang="de">Selbstausgef&#xfc;llter Fragebogen: Computerunterst&#xfc;tzt (CASI)</skos:prefLabel>
      <skos:definition xml:lang="de">Computerunterst&#xfc;tztes Selbstinterview (CASI). Die Befragten geben die Antworten selbst in einen Computer (Desktop, Laptop, Palm/PDA, Tablet, etc.) ein. Die Steuerung des Fragebogens wird von einem speziell entwickelten Programm/einer Anwendung verwaltet, aber es gibt keine Echtzeit-Daten&#xfc;bertragung wie bei CAWI, sondern die Antworten werden auf dem f&#xfc;r das Interview verwendeten Ger&#xe4;t gespeichert. Der Fragebogen kann in starrer Form oder interaktiv sein. Beinhaltet VCASI (Video computer-assisted self-interviewing), ACASI (Audio computer-assisted self-interviewing) und TACASI (Telephone audio computer-assisted self-interviewing).</skos:definition>
      <skos:prefLabel xml:lang="no">Selvadministrert sp&#xf8;rreskjema: Datamaskinassistert (CASI)</skos:prefLabel>
      <skos:definition xml:lang="no">Datamaskinassistert selvadministrert intervju (CASI). Respondentene registrerer svarene p&#xe5; en datamaskin (stasjon&#xe6;r, b&#xe6;rbar, digital personlig assistent, nettbrett etc.) p&#xe5; egenh&#xe5;nd. Administreringen av sp&#xf8;rreskjemaet er styrt av et spesialdesignet program eller en applikasjon men det er ingen fortl&#xf8;pende datautveksling slik som i CAWI, svarene blir lagret p&#xe5; apparatet som brukes for &#xe5; gjennomf&#xf8;re intervjuet. Sp&#xf8;rreskjemaet kan enten v&#xe6;re fastsatt eller interaktivt. Omfatter VCASI (video computer-assisted self-interview), ACASI (audio computer-assisted self-interview) og TACASI (telephone audio computer-assisted self-interview).</skos:definition>
      <skos:prefLabel xml:lang="lt">Savipildos klausimynas: kompiuteriu (CASI)</skos:prefLabel>
      <skos:definition xml:lang="lt">Savaranki&#x161;kas interviu kompiuteriu (CASI). Respondentai patys &#x12f;veda atsakymus &#x12f; kompiuter&#x12f; (stalin&#x12f;, ne&#x161;iojam&#x105;, delnin&#x12f;, plan&#x161;etin&#x12f; kompiuter&#x12f; ir kt.). Klausimyno administravimas vykdomas specialiai sukurta kompiuterine programa, ta&#x10d;iau duomen&#x173; perdavimas realiuoju laiku nevyksta, kaip CAWI, atsakymai saugomi apklausai naudojamame &#x12f;renginyje. Klausimynas gali b&#x16b;ti fiksuotos formos arba interaktyvus. Apima VCASI (savaranki&#x161;kas vaizdo interviu kompiuteriu), ACASI (savaranki&#x161;kas garso interviu kompiuteriu) ir TACASI (savaranki&#x161;kas telefoninio garso interviu kompiuteriu).</skos:definition>
      <skos:prefLabel xml:lang="it">Questionario auto-compilato: computer-assistito (CASI)</skos:prefLabel>
      <skos:definition xml:lang="it">Auto-compilazione del questionario assistita da computer (CASI). Gli intervistati inseriscono autonomamente le risposte in un computer (desktop, laptop, palmare, tablet, ecc.). La somministrazione del questionario &#xe8; gestita da un programma/applicazione appositamente progettato, ma non esiste un trasferimento dati in tempo reale come nel CAWI poich&#xe9; le risposte vengono memorizzate sul dispositivo utilizzato per l&apos;intervista. Il questionario pu&#xf2; essere fisso o interattivo. I tipi di questionario possono essere: VCASI (video assistito), ACASI (audio assistito) e TACASI (assistito via telefono).</skos:definition>
      <skos:prefLabel xml:lang="fr">Questionnaire auto-administr&#xe9; : assist&#xe9; par ordinateur (CASI)</skos:prefLabel>
      <skos:definition xml:lang="fr">Entretien auto-administr&#xe9; assist&#xe9; par ordinateur (CASI). Des r&#xe9;pondants saisissent eux-m&#xea;mes les r&#xe9;ponses dans un ordinateur (ordinateur de bureau, ordinateur portable, Palm / assistant personnel, tablette, etc.). L&apos;administration du questionnaire est g&#xe9;r&#xe9;e par un programme ou une application sp&#xe9;cialement d&#xe9;velopp&#xe9;(e) mais il n&apos;y a pas de transfert de donn&#xe9;es en temps r&#xe9;el comme dans un CAWI, les r&#xe9;ponses sont stock&#xe9;es sur l&apos;appareil utilis&#xe9; pour l&apos;entretien. Le questionnaire peut &#xea;tre fig&#xe9; ou interactif. Sont inclus les VCASI (entretien vid&#xe9;o auto-administr&#xe9; assist&#xe9; par ordinateur), les ACASI (entretien audio auto-administr&#xe9; assist&#xe9; par ordinateur) et les TACASI (entretien auto-administr&#xe9; par t&#xe9;l&#xe9;phone assist&#xe9; par ordinateur).</skos:definition>
      <skos:prefLabel xml:lang="nl">Zelf ingevulde vragenlijst: Computer-assisted (CASI)</skos:prefLabel>
      <skos:definition xml:lang="nl"></skos:definition>
   </rdf:Description>
   <rdf:Description rdf:about="http://rdf-vocabulary.ddialliance.org/cv/ModeOfCollection/5.0.0/9ec957d">
      <rdf:type rdf:resource="http://www.w3.org/2004/02/skos/core#Concept"/>
      <skos:inScheme rdf:resource="http://rdf-vocabulary.ddialliance.org/cv/ModeOfCollection/5.0.0/"/>
      <skos:notation xml:lang="en">FocusGroup</skos:notation>
      <skos:prefLabel xml:lang="sl">Fokusna skupina</skos:prefLabel>
      <skos:definition xml:lang="sl">Skupinska razprava o dolo&#x10d;eni temi, organizirana za raziskovalne namene. Posamezniki so izbrani glede na temo, interakcija med udele&#x17e;enci pa se uporablja kot del metode.</skos:definition>
      <skos:prefLabel xml:lang="sv">Fokusgrupp</skos:prefLabel>
      <skos:definition xml:lang="sv">En gruppdiskussion om ett visst &#xe4;mne som anordnats i forskningssyfte. Deltagarna har valts ut med h&#xe4;nsyn till &#xe4;mnet och interaktionen mellan deltagarna utg&#xf6;r en del av forskningsmetoden.</skos:definition>
      <skos:prefLabel xml:lang="en">Focus group</skos:prefLabel>
      <skos:definition xml:lang="en">A group discussion on a particular topic, organized for research purposes. The individuals are selected with relevance to the topic, and interaction among the participants is used as part of the method.</skos:definition>
      <skos:prefLabel xml:lang="de">Fokusgruppe</skos:prefLabel>
      <skos:definition xml:lang="de">Eine f&#xfc;r Forschungszwecke organisierte Gruppendiskussion zu einem bestimmten Thema. Individuen mit Bezug zum Thema werden ausgew&#xe4;hlt und die Interaktion zwischen den Teilnehmern wird als Teil der Methode verwendet.</skos:definition>
      <skos:prefLabel xml:lang="no">Fokusgruppe</skos:prefLabel>
      <skos:definition xml:lang="no">En gruppediskusjon som omhandler et bestemt tema, organisert for forskningsform&#xe5;l. Individene er valgt med relevans til temaet og samhandlingen mellom deltakerne er brukt som en del av metoden.</skos:definition>
      <skos:prefLabel xml:lang="lt">Tikslin&#x117; grup&#x117;s diskusija</skos:prefLabel>
      <skos:definition xml:lang="lt">Tyrimo tikslais organizuojama tikslin&#x117; grup&#x117;s diskusija tam tikra tema. Asmenys parenkami atsi&#x17e;velgiant &#x12f; tem&#x105;, o metodo taikymas reikalauja grupin&#x117;s s&#x105;veikos.</skos:definition>
      <skos:prefLabel xml:lang="it">Focus group</skos:prefLabel>
      <skos:definition xml:lang="it">Una discussione di gruppo focalizzata su un argomento particolare, organizzata per scopi di ricerca. I singoli individui sono selezionati in base all&apos;argomento trattato, e l&apos;interazione tra i partecipanti viene utilizzata come parte della tecnica.</skos:definition>
      <skos:prefLabel xml:lang="fr">Focus group</skos:prefLabel>
      <skos:definition xml:lang="fr">Un groupe de discussions sur un sujet particulier, organis&#xe9; &#xe0; des fins de recherche. Les individus sont s&#xe9;lectionn&#xe9;s en fonction du sujet, et les interactions entre participants sont utilis&#xe9;es dans le cadre de la m&#xe9;thode.</skos:definition>
      <skos:prefLabel xml:lang="nl">Focusgroep</skos:prefLabel>
      <skos:definition xml:lang="nl"></skos:definition>
      <skos:narrower rdf:resource="http://rdf-vocabulary.ddialliance.org/cv/ModeOfCollection/5.0.0/00b3692"/>
      <skos:narrower rdf:resource="http://rdf-vocabulary.ddialliance.org/cv/ModeOfCollection/5.0.0/2b4ef44"/>
      <skos:narrower rdf:resource="http://rdf-vocabulary.ddialliance.org/cv/ModeOfCollection/5.0.0/4da1255"/>
   </rdf:Description>
   <rdf:Description rdf:about="http://rdf-vocabulary.ddialliance.org/cv/ModeOfCollection/5.0.0/00b3692">
      <rdf:type rdf:resource="http://www.w3.org/2004/02/skos/core#Concept"/>
      <skos:inScheme rdf:resource="http://rdf-vocabulary.ddialliance.org/cv/ModeOfCollection/5.0.0/"/>
      <skos:notation xml:lang="en">FocusGroup.FaceToFace</skos:notation>
      <skos:prefLabel xml:lang="sl">Fokusna skupina v &#x17e;ivo</skos:prefLabel>
      <skos:definition xml:lang="sl">Udele&#x17e;enci fokusne skupine se osebno sestanejo za vodenje razprave.</skos:definition>
      <skos:prefLabel xml:lang="sv">Fokusgrupp: traditionell</skos:prefLabel>
      <skos:definition xml:lang="sv">Fokusgruppens medlemmar tr&#xe4;ffas p&#xe5; samma plats f&#xf6;r att diskutera.</skos:definition>
      <skos:prefLabel xml:lang="en">Face-to-face focus group</skos:prefLabel>
      <skos:definition xml:lang="en">The focus group participants meet in person to conduct the discussion.</skos:definition>
      <skos:prefLabel xml:lang="de">Fokusgruppe: Pers&#xf6;nlich</skos:prefLabel>
      <skos:definition xml:lang="de">Die Teilnehmer der Fokusgruppe treffen sich pers&#xf6;nlich zur Diskussion.</skos:definition>
      <skos:prefLabel xml:lang="no">Fokusgruppe: Ansikt til ansikt</skos:prefLabel>
      <skos:definition xml:lang="no">Deltakerne i fokusgruppen m&#xf8;tes fysisk for &#xe5; gjennomf&#xf8;re diskusjonen.</skos:definition>
      <skos:prefLabel xml:lang="lt">Tiesiogin&#x117; tikslin&#x117; grup&#x117;s diskusija </skos:prefLabel>
      <skos:definition xml:lang="lt">Tikslin&#x117;s grup&#x117;s diskusijos dalyviai susitinka ir diskutuoja tiesiogiai.</skos:definition>
      <skos:prefLabel xml:lang="it">Focus group faccia a faccia</skos:prefLabel>
      <skos:definition xml:lang="it">I partecipanti al focus group si incontrano di persona per condurre la discussione.</skos:definition>
      <skos:prefLabel xml:lang="fr">Focus group en face-&#xe0;-face</skos:prefLabel>
      <skos:definition xml:lang="fr">Les participants du focus group se rencontrent en personne pour mener la discussion.</skos:definition>
      <skos:prefLabel xml:lang="nl">Face-to-face focusgroep</skos:prefLabel>
      <skos:definition xml:lang="nl"></skos:definition>
   </rdf:Description>
   <rdf:Description rdf:about="http://rdf-vocabulary.ddialliance.org/cv/ModeOfCollection/5.0.0/2b4ef44">
      <rdf:type rdf:resource="http://www.w3.org/2004/02/skos/core#Concept"/>
      <skos:inScheme rdf:resource="http://rdf-vocabulary.ddialliance.org/cv/ModeOfCollection/5.0.0/"/>
      <skos:notation xml:lang="en">FocusGroup.Telephone</skos:notation>
      <skos:prefLabel xml:lang="sl">Telefonska fokusna skupina</skos:prefLabel>
      <skos:definition xml:lang="sl">Fokusna skupina, kjer razprava poteka preko telefona.</skos:definition>
      <skos:prefLabel xml:lang="sv">Fokusgrupp: telefon</skos:prefLabel>
      <skos:definition xml:lang="sv">Fokusgruppens diskussion f&#xf6;rs &#xf6;ver telefon.</skos:definition>
      <skos:prefLabel xml:lang="en">Telephone focus group</skos:prefLabel>
      <skos:definition xml:lang="en">The focus group discussion is conducted over the telephone.</skos:definition>
      <skos:prefLabel xml:lang="de">Fokusgruppe: Telefonisch</skos:prefLabel>
      <skos:definition xml:lang="de">Die Fokusgruppendiskussion wird &#xfc;ber das Telefon durchgef&#xfc;hrt.</skos:definition>
      <skos:prefLabel xml:lang="no">Fokusgruppe: Telefon</skos:prefLabel>
      <skos:definition xml:lang="no">Fokusgruppediskusjonen er gjennomf&#xf8;rt over telefonen.</skos:definition>
      <skos:prefLabel xml:lang="lt">Tikslin&#x117; grup&#x117;s diskusija telefonu</skos:prefLabel>
      <skos:definition xml:lang="lt">Tikslin&#x117; grup&#x117;s diskusija vedama telefonu.</skos:definition>
      <skos:prefLabel xml:lang="it">Focus group telefonico</skos:prefLabel>
      <skos:definition xml:lang="it">La discussione del focus group &#xe8; condotta via telefono.</skos:definition>
      <skos:prefLabel xml:lang="fr">Focus group par t&#xe9;l&#xe9;phone</skos:prefLabel>
      <skos:definition xml:lang="fr">Les discussions du focus group se font par t&#xe9;l&#xe9;phone.</skos:definition>
      <skos:prefLabel xml:lang="nl">Telefonische focusgroep</skos:prefLabel>
      <skos:definition xml:lang="nl"></skos:definition>
   </rdf:Description>
   <rdf:Description rdf:about="http://rdf-vocabulary.ddialliance.org/cv/ModeOfCollection/5.0.0/4da1255">
      <rdf:type rdf:resource="http://www.w3.org/2004/02/skos/core#Concept"/>
      <skos:inScheme rdf:resource="http://rdf-vocabulary.ddialliance.org/cv/ModeOfCollection/5.0.0/"/>
      <skos:notation xml:lang="en">FocusGroup.Online</skos:notation>
      <skos:prefLabel xml:lang="sl">Spletna fokusna skupina</skos:prefLabel>
      <skos:definition xml:lang="sl">Fokusna skupina, kjer razprava poteka preko spleta na interaktiven na&#x10d;in.</skos:definition>
      <skos:prefLabel xml:lang="sv">Fokusgrupp: virtuell</skos:prefLabel>
      <skos:definition xml:lang="sv">Fokusgruppens diskussion f&#xf6;rs interaktivt &#xf6;ver Internet. Kallas &#xe4;ven IT-st&#xf6;dd fokusgrupp.</skos:definition>
      <skos:prefLabel xml:lang="en">Online focus group</skos:prefLabel>
      <skos:definition xml:lang="en">The focus group discussion is conducted over the Internet in an interactive manner.</skos:definition>
      <skos:prefLabel xml:lang="de">Fokusgruppe: Online</skos:prefLabel>
      <skos:definition xml:lang="de">Die Fokusgruppendiskussion wird interaktiv &#xfc;ber das Internet durchgef&#xfc;hrt.</skos:definition>
      <skos:prefLabel xml:lang="no">Fokusgruppe: Online</skos:prefLabel>
      <skos:definition xml:lang="no">Fokusgruppediskusjonen er gjennomf&#xf8;rt over internett p&#xe5; en interaktiv m&#xe5;te.</skos:definition>
      <skos:prefLabel xml:lang="lt">Tikslin&#x117; grup&#x117;s diskusija internetu</skos:prefLabel>
      <skos:definition xml:lang="lt">Tikslin&#x117; grup&#x117;s diskusija interaktyviai vedama internetu.</skos:definition>
      <skos:prefLabel xml:lang="it">Focus group online</skos:prefLabel>
      <skos:definition xml:lang="it">La discussione del focus group &#xe8; condotta via Internet in modo interattivo.</skos:definition>
      <skos:prefLabel xml:lang="fr">Focus group en ligne</skos:prefLabel>
      <skos:definition xml:lang="fr">Les discussions du focus group se d&#xe9;roulent de mani&#xe8;re interactive via Internet.</skos:definition>
      <skos:prefLabel xml:lang="nl">Online focusgroep</skos:prefLabel>
      <skos:definition xml:lang="nl"></skos:definition>
   </rdf:Description>
   <rdf:Description rdf:about="http://rdf-vocabulary.ddialliance.org/cv/ModeOfCollection/5.0.0/08e658a">
      <rdf:type rdf:resource="http://www.w3.org/2004/02/skos/core#Concept"/>
      <skos:inScheme rdf:resource="http://rdf-vocabulary.ddialliance.org/cv/ModeOfCollection/5.0.0/"/>
      <skos:notation xml:lang="en">SelfAdministeredWritingsAndDiaries</skos:notation>
      <skos:prefLabel xml:lang="sl">Samoizpolnjevanje zapisov in/ali dnevnikov</skos:prefLabel>
      <skos:definition xml:lang="sl">Pripovedi, zgodbe, dnevniki in napisana besedila, ki jih ustvari subjekt raziskave.</skos:definition>
      <skos:prefLabel xml:lang="sv">Sj&#xe4;lvadministrerad text och/eller dagb&#xf6;cker</skos:prefLabel>
      <skos:definition xml:lang="sv">Narrativ, ber&#xe4;ttelser, dagb&#xf6;cker och andra nedskrivna texter skapade av forskningspersonerna.</skos:definition>
      <skos:prefLabel xml:lang="en">Self-administered writings and/or diaries</skos:prefLabel>
      <skos:definition xml:lang="en">Narratives, stories, diaries, and written texts created by the research subject.</skos:definition>
      <skos:prefLabel xml:lang="de">Selbstverfasste Schriften und/oder Tageb&#xfc;cher</skos:prefLabel>
      <skos:definition xml:lang="de">Erz&#xe4;hlungen, Geschichten, Tageb&#xfc;cher und schriftliche Texte, die vom Forschungssubjekt erstellt wurden.</skos:definition>
      <skos:prefLabel xml:lang="no">Selvadministrert tekst og/eller dagbok</skos:prefLabel>
      <skos:definition xml:lang="no">Fortellinger, historier, dagb&#xf8;ker og tekster skrevet av studieobjektene.</skos:definition>
      <skos:prefLabel xml:lang="lt">Savaranki&#x161;kai ra&#x161;omi u&#x17e;ra&#x161;ai ir (arba) dienora&#x161;&#x10d;iai</skos:prefLabel>
      <skos:definition xml:lang="lt">Tiriam&#x173;j&#x173; sukuriami naratyvai, pasakojimai, dienora&#x161;&#x10d;iai ir ra&#x161;ytiniai tekstai.</skos:definition>
      <skos:prefLabel xml:lang="it">Scritti/diari auto-compilati</skos:prefLabel>
      <skos:definition xml:lang="it">Narrazioni, storie, diari e testi scritti creati dai soggetti coinvolti nella ricerca.</skos:definition>
      <skos:prefLabel xml:lang="fr">&#xc9;crits et / ou journaux intimes auto-administr&#xe9;s</skos:prefLabel>
      <skos:definition xml:lang="fr">Des r&#xe9;cits, des histoires, des journaux intimes et des textes &#xe9;crits cr&#xe9;&#xe9;s par le sujet de recherche.</skos:definition>
      <skos:prefLabel xml:lang="nl">Zelf ingevulde antwoorden/of dagboeken</skos:prefLabel>
      <skos:definition xml:lang="nl"></skos:definition>
      <skos:narrower rdf:resource="http://rdf-vocabulary.ddialliance.org/cv/ModeOfCollection/5.0.0/fe226ad"/>
      <skos:narrower rdf:resource="http://rdf-vocabulary.ddialliance.org/cv/ModeOfCollection/5.0.0/e5bef42"/>
      <skos:narrower rdf:resource="http://rdf-vocabulary.ddialliance.org/cv/ModeOfCollection/5.0.0/9e67a7c"/>
   </rdf:Description>
   <rdf:Description rdf:about="http://rdf-vocabulary.ddialliance.org/cv/ModeOfCollection/5.0.0/fe226ad">
      <rdf:type rdf:resource="http://www.w3.org/2004/02/skos/core#Concept"/>
      <skos:inScheme rdf:resource="http://rdf-vocabulary.ddialliance.org/cv/ModeOfCollection/5.0.0/"/>
      <skos:notation xml:lang="en">SelfAdministeredWritingsAndDiaries.Email</skos:notation>
      <skos:prefLabel xml:lang="sl">Samoizpolnjevanje zapisov in/ali dnevnikov: elektronska po&#x161;ta</skos:prefLabel>
      <skos:definition xml:lang="sl">Pripovedi, zgodbe, dnevniki in napisana besedila, ki so posredovana preko elektronskih po&#x161;tnih sporo&#x10d;il.</skos:definition>
      <skos:prefLabel xml:lang="sv">Sj&#xe4;lvadministrerad text och/eller dagb&#xf6;cker: e-post</skos:prefLabel>
      <skos:definition xml:lang="sv">Narrativ, ber&#xe4;ttelser, dagb&#xf6;cker och andra nedskrivna texter som skickas in via e-post.</skos:definition>
      <skos:prefLabel xml:lang="en">Self-administered writings and/or diaries: E-mail</skos:prefLabel>
      <skos:definition xml:lang="en">Narratives, stories, diaries, and written texts submitted via e-mail messages.</skos:definition>
      <skos:prefLabel xml:lang="de">Selbstverfasste Schriften und/oder Tageb&#xfc;cher: E-Mail</skos:prefLabel>
      <skos:definition xml:lang="de">Erz&#xe4;hlungen, Geschichten, Tageb&#xfc;cher und schriftliche Texte, die &#xfc;ber E-Mail-Nachrichten eingereicht werden.</skos:definition>
      <skos:prefLabel xml:lang="no">Selvadministrert tekst og/eller dagbok: E-post</skos:prefLabel>
      <skos:definition xml:lang="no">Fortellinger, historier, dagb&#xf8;ker og tekster som har blitt samlet inn via e-post.</skos:definition>
      <skos:prefLabel xml:lang="lt">Savaranki&#x161;kai ra&#x161;omi u&#x17e;ra&#x161;ai ir (arba) dienora&#x161;&#x10d;iai: elektroniniu pa&#x161;tu</skos:prefLabel>
      <skos:definition xml:lang="lt">Elektroniniu pa&#x161;tu pateikiami naratyvai, pasakojimai, dienora&#x161;&#x10d;iai ir ra&#x161;ytiniai tekstai.</skos:definition>
      <skos:prefLabel xml:lang="it">Scritti/diari auto-compilati: e-mail</skos:prefLabel>
      <skos:definition xml:lang="it">Narrazioni, storie, diari e testi scritti inviati tramite e-mail.</skos:definition>
      <skos:prefLabel xml:lang="fr">&#xc9;crits et / ou journaux intimes auto-administr&#xe9;s : e-mail</skos:prefLabel>
      <skos:definition xml:lang="fr">Des r&#xe9;cits, des histoires, des journaux intimes et des textes &#xe9;crits soumis par courriel.</skos:definition>
      <skos:prefLabel xml:lang="nl">Zelf ingevulde antwoorden/of dagboeken: E-mail</skos:prefLabel>
      <skos:definition xml:lang="nl"></skos:definition>
   </rdf:Description>
   <rdf:Description rdf:about="http://rdf-vocabulary.ddialliance.org/cv/ModeOfCollection/5.0.0/e5bef42">
      <rdf:type rdf:resource="http://www.w3.org/2004/02/skos/core#Concept"/>
      <skos:inScheme rdf:resource="http://rdf-vocabulary.ddialliance.org/cv/ModeOfCollection/5.0.0/"/>
      <skos:notation xml:lang="en">SelfAdministeredWritingsAndDiaries.Paper</skos:notation>
      <skos:prefLabel xml:lang="sl">Samoizpolnjevanje zapisov in/ali dnevnikov: papir</skos:prefLabel>
      <skos:definition xml:lang="sl">Pripovedi, zgodbe, dnevniki in napisana besedila, ki so ustvarjena in zbrana na papirju.</skos:definition>
      <skos:prefLabel xml:lang="sv">Sj&#xe4;lvadministrerad text och/eller dagb&#xf6;cker: papper</skos:prefLabel>
      <skos:definition xml:lang="sv">Narrativ, ber&#xe4;ttelser, dagb&#xf6;cker och andra nedskrivna texter som skapats och samlats in p&#xe5; papper.</skos:definition>
      <skos:prefLabel xml:lang="en">Self-administered writings and/or diaries: Paper</skos:prefLabel>
      <skos:definition xml:lang="en">Narratives, stories, diaries, and written texts created and collected in paper form.</skos:definition>
      <skos:prefLabel xml:lang="de">Selbstverfasste Schriften und/oder Tageb&#xfc;cher: Papier</skos:prefLabel>
      <skos:definition xml:lang="de">Erz&#xe4;hlungen, Geschichten, Tageb&#xfc;cher und schriftliche Texte, die in Papierform erstellt und gesammelt wurden.</skos:definition>
      <skos:prefLabel xml:lang="no">Selvadministrert tekst og/eller dagbok: Papir</skos:prefLabel>
      <skos:definition xml:lang="no">Fortellinger, historier, dagb&#xf8;ker og tekster skrevet og samlet i papirformat.</skos:definition>
      <skos:prefLabel xml:lang="lt">Savaranki&#x161;kai ra&#x161;omi u&#x17e;ra&#x161;ai ir (arba) dienora&#x161;&#x10d;iai: popieriuje</skos:prefLabel>
      <skos:definition xml:lang="lt">Naratyvai, pasakojimai, dienora&#x161;&#x10d;iai ir ra&#x161;ytiniai tekstai sukuriami ir renkami popierine forma.</skos:definition>
      <skos:prefLabel xml:lang="it">Scritti/diari auto-compilati: cartaceo</skos:prefLabel>
      <skos:definition xml:lang="it">Narrazioni, storie, diari e testi scritti creati e raccolti in forma cartacea.</skos:definition>
      <skos:prefLabel xml:lang="fr">&#xc9;crits et / ou journaux intimes auto-administr&#xe9;s : papier</skos:prefLabel>
      <skos:definition xml:lang="fr">Des r&#xe9;cits, des histoires, des journaux intimes, et des textes &#xe9;crits cr&#xe9;&#xe9;s et rassembl&#xe9;s sous forme papier.</skos:definition>
      <skos:prefLabel xml:lang="nl">Zelf ingevulde antwoorden/of dagboeken: Papier</skos:prefLabel>
      <skos:definition xml:lang="nl"></skos:definition>
   </rdf:Description>
   <rdf:Description rdf:about="http://rdf-vocabulary.ddialliance.org/cv/ModeOfCollection/5.0.0/9e67a7c">
      <rdf:type rdf:resource="http://www.w3.org/2004/02/skos/core#Concept"/>
      <skos:inScheme rdf:resource="http://rdf-vocabulary.ddialliance.org/cv/ModeOfCollection/5.0.0/"/>
      <skos:notation xml:lang="en">SelfAdministeredWritingsAndDiaries.WebBased</skos:notation>
      <skos:prefLabel xml:lang="sl">Samoizpolnjevanje zapisov in/ali dnevnikov: spletno</skos:prefLabel>
      <skos:definition xml:lang="sl">Pripovedi, zgodbe, dnevniki in napisana besedila, ki so zbrana preko internetnih virov, npr. spletne strani, blogi, forumi.</skos:definition>
      <skos:prefLabel xml:lang="sv">Sj&#xe4;lvadministrerad text och/eller dagb&#xf6;cker: webbaserat</skos:prefLabel>
      <skos:definition xml:lang="sv">Narrativ, ber&#xe4;ttelser, dagb&#xf6;cker och andra nedskrivna texter som samlats in fr&#xe5;n Internet-k&#xe4;llor, t.ex. webbplatser, bloggar, diskussionsforum.</skos:definition>
      <skos:prefLabel xml:lang="en">Self-administered writings and/or diaries: Web-based</skos:prefLabel>
      <skos:definition xml:lang="en">Narratives, stories, diaries, and written texts gathered from Internet sources, e.g. websites, blogs, discussion forums.</skos:definition>
      <skos:prefLabel xml:lang="de">Selbstverfasste Schriften und/oder Tageb&#xfc;cher: Webbasiert</skos:prefLabel>
      <skos:definition xml:lang="de">Erz&#xe4;hlungen, Geschichten, Tageb&#xfc;cher und schriftliche Texte aus Internetquellen, z. B. Webseiten, Blogs, Diskussionsforen.</skos:definition>
      <skos:prefLabel xml:lang="no">Selvadministrert tekst og/eller dagbok: Webbasert</skos:prefLabel>
      <skos:definition xml:lang="no">Fortellinger, historier, dagb&#xf8;ker og tekster samlet fra internett, e.g. nettsider, blogger, diskusjonsforumer.</skos:definition>
      <skos:prefLabel xml:lang="lt">Savaranki&#x161;kai ra&#x161;omi u&#x17e;ra&#x161;ai ir (arba) dienora&#x161;&#x10d;iai: internete</skos:prefLabel>
      <skos:definition xml:lang="lt">Naratyvai, pasakojimai, dienora&#x161;&#x10d;iai ir ra&#x161;ytiniai tekstai surenkami i&#x161; internetini&#x173; &#x161;altini&#x173;, pavyzd&#x17e;iui, svetaini&#x173;, tinklara&#x161;&#x10d;i&#x173;, diskusij&#x173; forum&#x173;.</skos:definition>
      <skos:prefLabel xml:lang="it">Scritti/diari auto-compilati: web</skos:prefLabel>
      <skos:definition xml:lang="it">Narrazioni, storie, diari e testi scritti raccolti su Internet, ad esempio da siti web, blog, forum di discussione.</skos:definition>
      <skos:prefLabel xml:lang="fr">&#xc9;crits et / ou journaux intimes auto-administr&#xe9;s : en ligne</skos:prefLabel>
      <skos:definition xml:lang="fr">Des r&#xe9;cits, des histoires, des journaux intimes, et des textes &#xe9;crits provenant d&apos;Internet, e. g. des sites Internet, des blogs, des forums de discussion.</skos:definition>
      <skos:prefLabel xml:lang="nl">Zelf ingevulde antwoorden/of dagboeken: Webgebaseerd</skos:prefLabel>
      <skos:definition xml:lang="nl"></skos:definition>
   </rdf:Description>
   <rdf:Description rdf:about="http://rdf-vocabulary.ddialliance.org/cv/ModeOfCollection/5.0.0/c680d43">
      <rdf:type rdf:resource="http://www.w3.org/2004/02/skos/core#Concept"/>
      <skos:inScheme rdf:resource="http://rdf-vocabulary.ddialliance.org/cv/ModeOfCollection/5.0.0/"/>
      <skos:notation xml:lang="en">Observation</skos:notation>
      <skos:prefLabel xml:lang="sl">Opazovanje</skos:prefLabel>
      <skos:definition xml:lang="sl">Raziskovalna metoda, ki vklju&#x10d;uje zbiranje podatkov, ko se pojavijo (npr. opazovanje vedenj, dogodkov, razvoja stanja ali bolezni itd.), ne da bi posku&#x161;ali manipulirati s katero od neodvisnih spremenljivk.</skos:definition>
      <skos:prefLabel xml:lang="sv">Observation</skos:prefLabel>
      <skos:definition xml:lang="sv">Forskningsmetod som omfattar att samla in data om f&#xf6;reteelser n&#xe4;r de upptr&#xe4;der (t.ex. observationer av beteenden, h&#xe4;ndelser m.m.) utan att f&#xf6;rs&#xf6;ka p&#xe5;verka n&#xe5;gra av de oberoende variablerna.</skos:definition>
      <skos:prefLabel xml:lang="en">Observation</skos:prefLabel>
      <skos:definition xml:lang="en">Research method that involves collecting data as they occur (for example, observing behaviors, events, development of condition or disease, etc.), without attempting to manipulate any of the independent variables.</skos:definition>
      <skos:prefLabel xml:lang="de">Beobachtung</skos:prefLabel>
      <skos:definition xml:lang="de">Forschungsmethode, bei der Daten gesammelt werden, w&#xe4;hrend sie auftreten (z. B. Beobachtung von Verhaltensweisen, Ereignissen, Entwicklung eines Zustands oder einer Krankheit usw.), ohne dass versucht wird, eine der unabh&#xe4;ngigen Variablen zu manipulieren.</skos:definition>
      <skos:prefLabel xml:lang="no">Observasjon</skos:prefLabel>
      <skos:definition xml:lang="no">Forskningsmetode som inneb&#xe6;rer &#xe5; samle inn data etterhvert som de opptr&#xe5;r (for eksempel, observere atferd, hendelser, utviklingen av helsetilstand eller sykdom, etc.) uten &#xe5; pr&#xf8;ve &#xe5; manipulere noen av de uavhengige variablene.</skos:definition>
      <skos:prefLabel xml:lang="lt">Steb&#x117;jimas</skos:prefLabel>
      <skos:definition xml:lang="lt">Tyrimo metodas, kai duomenys renkami tiesiogiai realiu laiku (pavyzd&#x17e;iui, stebint elgsen&#x105;, &#x12f;vykius, ligos b&#x16b;kl&#x119; ir raid&#x105; ir kt.), nebandant manipuliuoti jokiais nepriklausomais kintamaisiais.</skos:definition>
      <skos:prefLabel xml:lang="it">Osservazione</skos:prefLabel>
      <skos:definition xml:lang="it">Tecnica di rilevazione che implica la raccolta di dati nel momento in cui si generano (ad esempio osservando comportamenti, eventi, sviluppo di condizioni o malattie, ecc.), senza tentare di manipolare nessuna delle variabili indipendenti.</skos:definition>
      <skos:prefLabel xml:lang="fr">Observation</skos:prefLabel>
      <skos:definition xml:lang="fr">M&#xe9;thode de recherche qui consiste &#xe0; collecter des donn&#xe9;es au fur et &#xe0; mesure de leur apparition (par exemple, observation de comportements, d&#x2019;&#xe9;v&#xe9;nements, de l&apos;&#xe9;volution d&apos;un &#xe9;tat ou d&apos;une maladie, etc.), sans tentative de manipuler les variables ind&#xe9;pendantes.</skos:definition>
      <skos:prefLabel xml:lang="nl">Observatie</skos:prefLabel>
      <skos:definition xml:lang="nl"></skos:definition>
      <skos:narrower rdf:resource="http://rdf-vocabulary.ddialliance.org/cv/ModeOfCollection/5.0.0/bdc4aac"/>
      <skos:narrower rdf:resource="http://rdf-vocabulary.ddialliance.org/cv/ModeOfCollection/5.0.0/e679c7f"/>
      <skos:narrower rdf:resource="http://rdf-vocabulary.ddialliance.org/cv/ModeOfCollection/5.0.0/40b8b0c"/>
   </rdf:Description>
   <rdf:Description rdf:about="http://rdf-vocabulary.ddialliance.org/cv/ModeOfCollection/5.0.0/bdc4aac">
      <rdf:type rdf:resource="http://www.w3.org/2004/02/skos/core#Concept"/>
      <skos:inScheme rdf:resource="http://rdf-vocabulary.ddialliance.org/cv/ModeOfCollection/5.0.0/"/>
      <skos:notation xml:lang="en">Observation.Field</skos:notation>
      <skos:prefLabel xml:lang="sl">Opazovanje na terenu</skos:prefLabel>
      <skos:definition xml:lang="sl">Opazovanje, ki se izvaja v naravnem okolju.</skos:definition>
      <skos:prefLabel xml:lang="sv">F&#xe4;ltobservation</skos:prefLabel>
      <skos:definition xml:lang="sv">Observation som utf&#xf6;rs i en naturlig milj&#xf6;.</skos:definition>
      <skos:prefLabel xml:lang="en">Field observation</skos:prefLabel>
      <skos:definition xml:lang="en">Observation that is conducted in a natural environment.</skos:definition>
      <skos:prefLabel xml:lang="de">Feldbeobachtung</skos:prefLabel>
      <skos:definition xml:lang="de">Beobachtung, die in einer nat&#xfc;rlichen Umgebung durchgef&#xfc;hrt wird.</skos:definition>
      <skos:prefLabel xml:lang="no">Feltobservasjon</skos:prefLabel>
      <skos:definition xml:lang="no">Observasjon som utf&#xf8;res i et naturlig milj&#xf8;.</skos:definition>
      <skos:prefLabel xml:lang="lt">Lauko steb&#x117;jimas</skos:prefLabel>
      <skos:definition xml:lang="lt">Steb&#x117;jimas atliekamas nat&#x16b;ralioje aplinkoje.</skos:definition>
      <skos:prefLabel xml:lang="it">Osservazione sul campo</skos:prefLabel>
      <skos:definition xml:lang="it">Osservazione condotta in un ambiente naturale.</skos:definition>
      <skos:prefLabel xml:lang="fr">Observation sur le terrain</skos:prefLabel>
      <skos:definition xml:lang="fr">Observation qui a &#xe9;t&#xe9; conduite dans un environnement naturel.</skos:definition>
      <skos:prefLabel xml:lang="nl">Observatie in het veld</skos:prefLabel>
      <skos:definition xml:lang="nl"></skos:definition>
      <skos:narrower rdf:resource="http://rdf-vocabulary.ddialliance.org/cv/ModeOfCollection/5.0.0/3cee522"/>
      <skos:narrower rdf:resource="http://rdf-vocabulary.ddialliance.org/cv/ModeOfCollection/5.0.0/8245871"/>
   </rdf:Description>
   <rdf:Description rdf:about="http://rdf-vocabulary.ddialliance.org/cv/ModeOfCollection/5.0.0/3cee522">
      <rdf:type rdf:resource="http://www.w3.org/2004/02/skos/core#Concept"/>
      <skos:inScheme rdf:resource="http://rdf-vocabulary.ddialliance.org/cv/ModeOfCollection/5.0.0/"/>
      <skos:notation xml:lang="en">Observation.Field.Participant</skos:notation>
      <skos:prefLabel xml:lang="sl">Opazovanje na terenu z udele&#x17e;bo</skos:prefLabel>
      <skos:definition xml:lang="sl">Vrsta opazovanja, kjer je raziskovalec v interakciji z raziskovalnim subjektom in pogosto igra vlogo v opazovani dru&#x17e;beni situaciji.</skos:definition>
      <skos:prefLabel xml:lang="sv">Deltagande f&#xe4;ltobservation</skos:prefLabel>
      <skos:definition xml:lang="sv">F&#xe4;ltobservation d&#xe4;r forskaren interagerar med forskningsobjekten och ofta har en funktion i den sociala situation som observeras.</skos:definition>
      <skos:prefLabel xml:lang="en">Participant field observation</skos:prefLabel>
      <skos:definition xml:lang="en">Type of field observation in which the researcher interacts with the subjects and often plays a role in the social situation under observation.</skos:definition>
      <skos:prefLabel xml:lang="de">Teilnehmende Feldbeobachtung</skos:prefLabel>
      <skos:definition xml:lang="de">Eine Art der Feldbeobachtung, in der der Forscher mit den Probanden interagiert und oft selbst eine Rolle in der sozialen Situation unter Beobachtung einnimmt.</skos:definition>
      <skos:prefLabel xml:lang="no">Deltagende feltobservasjon</skos:prefLabel>
      <skos:definition xml:lang="no">Type feltobservasjon hvor forskeren samhandler og ofte spiller en rolle i de sosiale situasjonene som observeres.</skos:definition>
      <skos:prefLabel xml:lang="lt">Lauko steb&#x117;jimas dalyvaujant</skos:prefLabel>
      <skos:definition xml:lang="lt">Lauko steb&#x117;jimo tipas, kai tyr&#x117;jas s&#x105;veikauja su tiriamaisiais ir stebimoje socialin&#x117;je situacijoje paprastai turi tam tikr&#x105; vaidmen&#x12f;.</skos:definition>
      <skos:prefLabel xml:lang="it">Osservazione partecipante sul campo</skos:prefLabel>
      <skos:definition xml:lang="it">Tipo di osservazione sul campo nella quale il ricercatore interagisce con i soggetti e spesso ricopre un ruolo nella situazione sociale sotto osservazione.</skos:definition>
      <skos:prefLabel xml:lang="fr">Observation participante sur le terrain</skos:prefLabel>
      <skos:definition xml:lang="fr">Type d&apos;observation sur le terrain dans lequel le chercheur interagit avec les sujets et joue souvent un r&#xf4;le au sein de la situation sociale sous observation.</skos:definition>
      <skos:prefLabel xml:lang="nl">Participerende observatie in het veld</skos:prefLabel>
      <skos:definition xml:lang="nl"></skos:definition>
   </rdf:Description>
   <rdf:Description rdf:about="http://rdf-vocabulary.ddialliance.org/cv/ModeOfCollection/5.0.0/8245871">
      <rdf:type rdf:resource="http://www.w3.org/2004/02/skos/core#Concept"/>
      <skos:inScheme rdf:resource="http://rdf-vocabulary.ddialliance.org/cv/ModeOfCollection/5.0.0/"/>
      <skos:notation xml:lang="en">Observation.Field.Nonparticipant</skos:notation>
      <skos:prefLabel xml:lang="sl">Opazovanje na terenu brez udele&#x17e;be</skos:prefLabel>
      <skos:definition xml:lang="sl">Opazovanje, ki se izvaja v naravnem, nekontroliranem okolju brez kakr&#x161;nekoli interakcije med raziskovalcem in njegovimi/njenimi subjekti.</skos:definition>
      <skos:prefLabel xml:lang="sv">Icke-deltagande f&#xe4;ltobservation</skos:prefLabel>
      <skos:definition xml:lang="sv">Observation som utf&#xf6;rs i en naturlig, icke-kontrollerad milj&#xf6; utan interaktion mellan forskaren och dennes forskningsobjekt.</skos:definition>
      <skos:prefLabel xml:lang="en">Non-participant field observation</skos:prefLabel>
      <skos:definition xml:lang="en">Observation that is conducted in a natural, non-controlled setting without any interaction between the researcher and his/her subjects.</skos:definition>
      <skos:prefLabel xml:lang="de">Nicht-teilnehmende Feldbeobachtung</skos:prefLabel>
      <skos:definition xml:lang="de">Eine Art der Feldbeobachtung, die in einer nat&#xfc;rlichen, nicht kontrollierten Umgebung durchgef&#xfc;hrt wird - ohne jegliche Interaktion zwischen dem/der Forscher*in und seinen/ihren Probanden*innen.</skos:definition>
      <skos:prefLabel xml:lang="no">Ikke-deltagende feltobservasjon</skos:prefLabel>
      <skos:definition xml:lang="no">Observasjon som er gjennomf&#xf8;rt i et naturlig, ikke kontrollert milj&#xf8; uten interaksjon mellom forskeren og studieobjektene.</skos:definition>
      <skos:prefLabel xml:lang="lt">Lauko steb&#x117;jimas nedalyvaujant</skos:prefLabel>
      <skos:definition xml:lang="lt">Steb&#x117;jimas vykdomas nat&#x16b;ralioje, nekontroliuojamoje aplinkoje be jokios s&#x105;veikos tarp tyr&#x117;jo ir tiriam&#x173;j&#x173;.</skos:definition>
      <skos:prefLabel xml:lang="it">Osservazione non partecipante sul campo</skos:prefLabel>
      <skos:definition xml:lang="it">Osservazione condotta in un ambiente naturale non controllato senza alcuna interazione tra il ricercatore e i soggetti.</skos:definition>
      <skos:prefLabel xml:lang="fr">Observation non-participante sur le terrain</skos:prefLabel>
      <skos:definition xml:lang="fr">Observation qui a &#xe9;t&#xe9; conduite dans un environnement naturel et non contr&#xf4;l&#xe9; sans aucune interaction entre le chercheur et ses sujets.</skos:definition>
      <skos:prefLabel xml:lang="nl">Niet-participerende observatie in het veld</skos:prefLabel>
      <skos:definition xml:lang="nl"></skos:definition>
   </rdf:Description>
   <rdf:Description rdf:about="http://rdf-vocabulary.ddialliance.org/cv/ModeOfCollection/5.0.0/e679c7f">
      <rdf:type rdf:resource="http://www.w3.org/2004/02/skos/core#Concept"/>
      <skos:inScheme rdf:resource="http://rdf-vocabulary.ddialliance.org/cv/ModeOfCollection/5.0.0/"/>
      <skos:notation xml:lang="en">Observation.Laboratory</skos:notation>
      <skos:prefLabel xml:lang="sl">Laboratorijsko opazovanje</skos:prefLabel>
      <skos:definition xml:lang="sl">Opazovanje, ki se izvaja v nadzorovanem, umetno ustvarjenem okolju. Na primer, opazovanje otro&#x161;ke igre v laboratorijski igralnici.</skos:definition>
      <skos:prefLabel xml:lang="sv">Laboratorieobservation</skos:prefLabel>
      <skos:definition xml:lang="sv">Observation som utf&#xf6;rs i en kontrollerad, konstgjord milj&#xf6;. Exempel: observation av barns lek i ett laboratorielekrum.</skos:definition>
      <skos:prefLabel xml:lang="en">Laboratory observation</skos:prefLabel>
      <skos:definition xml:lang="en">Observation that is conducted in a controlled, artificially created setting. For example, observing children&apos;s play in a laboratory playroom.</skos:definition>
      <skos:prefLabel xml:lang="de">Laborbeobachtung</skos:prefLabel>
      <skos:definition xml:lang="de">Beobachtung, die in einer kontrollierten, k&#xfc;nstlich geschaffenen Umgebung durchgef&#xfc;hrt wird. Zum Beispiel, die Beobachtung spielender Kinder in einem Labor-Spielzimmer.</skos:definition>
      <skos:prefLabel xml:lang="no">Laboratorieobservasjon</skos:prefLabel>
      <skos:definition xml:lang="no">Observasjon som er utf&#xf8;rt i et kontrollert, kunstig konstruert milj&#xf8;. For eksempel observasjon av barns lek i et lekerom i laboratoriet.</skos:definition>
      <skos:prefLabel xml:lang="lt">Laboratorinis steb&#x117;jimas</skos:prefLabel>
      <skos:definition xml:lang="lt">Steb&#x117;jimas atliekamas kontroliuojamoje, dirbtinai sukurtoje aplinkoje. Pavyzd&#x17e;iui, vaik&#x173; &#x17e;aidimo steb&#x117;jimas laboratoriniame &#x17e;aidim&#x173; kambaryje.</skos:definition>
      <skos:prefLabel xml:lang="it">Osservazione in laboratorio</skos:prefLabel>
      <skos:definition xml:lang="it">Osservazione condotta in un ambiente controllato, creato artificialmente. Ad esempio, osservazione del gioco dei bambini in una stanza da gioco ricreata in laboratorio.</skos:definition>
      <skos:prefLabel xml:lang="fr">Observation en laboratoire</skos:prefLabel>
      <skos:definition xml:lang="fr">Observation qui a &#xe9;t&#xe9; conduite dans un environnement contr&#xf4;l&#xe9;, cr&#xe9;&#xe9; artificiellement. Par exemple, l&apos;observation du jeu des enfants dans une salle de jeux de laboratoire.</skos:definition>
      <skos:prefLabel xml:lang="nl">Observatie in het lab</skos:prefLabel>
      <skos:definition xml:lang="nl"></skos:definition>
      <skos:narrower rdf:resource="http://rdf-vocabulary.ddialliance.org/cv/ModeOfCollection/5.0.0/2a58349"/>
      <skos:narrower rdf:resource="http://rdf-vocabulary.ddialliance.org/cv/ModeOfCollection/5.0.0/68b02fb"/>
   </rdf:Description>
   <rdf:Description rdf:about="http://rdf-vocabulary.ddialliance.org/cv/ModeOfCollection/5.0.0/2a58349">
      <rdf:type rdf:resource="http://www.w3.org/2004/02/skos/core#Concept"/>
      <skos:inScheme rdf:resource="http://rdf-vocabulary.ddialliance.org/cv/ModeOfCollection/5.0.0/"/>
      <skos:notation xml:lang="en">Observation.Laboratory.Participant</skos:notation>
      <skos:prefLabel xml:lang="sl">Laboratorijsko opazovanje z udele&#x17e;bo</skos:prefLabel>
      <skos:definition xml:lang="sl">Vrsta laboratorijskega opazovanja, kjer je raziskovalec v interkaciji s subjekti in pogosto igra vlogo v opazovani dru&#x17e;beni situaciji. Na primer, opazovanje otro&#x161;ke igre v laboratorijski igralnici, kjer ima raziskovalec vlogo v igri.</skos:definition>
      <skos:prefLabel xml:lang="sv">Deltagande laboratorieobservation</skos:prefLabel>
      <skos:definition xml:lang="sv">Laboratorieobservation d&#xe4;r forskaren interagerar med forskningsobjekten och ofta har en funktion i den sociala situation som observeras. Exempel: observation av barns lek i ett laboratorielekrum d&#xe4;r forskaren deltar i leken.</skos:definition>
      <skos:prefLabel xml:lang="en">Participant laboratory observation</skos:prefLabel>
      <skos:definition xml:lang="en">Type of laboratory observation in which the researcher interacts with the subjects and often plays a role in the social situation under observation. For example, observing children&apos;s play in a laboratory playroom with the researcher taking part in the play.</skos:definition>
      <skos:prefLabel xml:lang="de">Teilnehmende Laborbeobachtung</skos:prefLabel>
      <skos:definition xml:lang="de">Eine Art der Laborbeobachtung, in der Forschende mit den Probanden interagieren und oft selbst ein Rolle in der sozialen Situation unter Beobachtung einnehmen. Zum Beispiel, die Beobachtung spielender Kinder in einem Labor-Spielzimmer, wobei der/die Forscher*in selbst am Spiel teilnimmt.</skos:definition>
      <skos:prefLabel xml:lang="no">Deltagende laboratorieobservasjon</skos:prefLabel>
      <skos:definition xml:lang="no">En type laboratorieobservasjon hvor forskeren samhandler med forskningsobjektene, og ofte spiller en rolle i den sosiale situasjonen som er under observasjon. For eksempel observere barns lek i et lekerom i laboratoriet, der forsker deltar i leken.</skos:definition>
      <skos:prefLabel xml:lang="lt">Laboratorinis steb&#x117;jimas dalyvaujant</skos:prefLabel>
      <skos:definition xml:lang="lt">Laboratorinio steb&#x117;jimo r&#x16b;&#x161;is, kai tyr&#x117;jas s&#x105;veikauja su tiriamaisiais ir stebimoje socialin&#x117;je situacijoje paprastai turi tam tikr&#x105; vaidmen&#x12f;. Pavyzd&#x17e;iui, vaik&#x173; &#x17e;aidimo steb&#x117;jimas laboratoriniame &#x17e;aidim&#x173; kambaryje tyr&#x117;jui pa&#x10d;iam &#x12f;sitraukiant &#x12f; &#x17e;aidim&#x105;.</skos:definition>
      <skos:prefLabel xml:lang="it">Osservazione partecipante in laboratorio</skos:prefLabel>
      <skos:definition xml:lang="it">Tipo di osservazione in laboratorio in cui il ricercatore interagisce con i soggetti e spesso gioca un ruolo nella situazione sociale sotto osservazione. Ad esempio, osservando il gioco dei bambini in una stanza da gioco ricreata in laboratorio con il ricercatore che partecipa al gioco.</skos:definition>
      <skos:prefLabel xml:lang="fr">Observation participante en laboratoire</skos:prefLabel>
      <skos:definition xml:lang="fr">Type d&apos;observation en laboratoire dans lequel le chercheur interagit avec les sujets et joue souvent un r&#xf4;le dans la situation sociale sous observation. Par exemple, l&apos;observation du jeu des enfants dans une salle de jeux de laboratoire avec le chercheur prenant part au jeu.</skos:definition>
      <skos:prefLabel xml:lang="nl">Participerende observatie in het lab</skos:prefLabel>
      <skos:definition xml:lang="nl"></skos:definition>
   </rdf:Description>
   <rdf:Description rdf:about="http://rdf-vocabulary.ddialliance.org/cv/ModeOfCollection/5.0.0/68b02fb">
      <rdf:type rdf:resource="http://www.w3.org/2004/02/skos/core#Concept"/>
      <skos:inScheme rdf:resource="http://rdf-vocabulary.ddialliance.org/cv/ModeOfCollection/5.0.0/"/>
      <skos:notation xml:lang="en">Observation.Laboratory.Nonparticipant</skos:notation>
      <skos:prefLabel xml:lang="sl">Laboratorijsko opazovanje brez udele&#x17e;be</skos:prefLabel>
      <skos:definition xml:lang="sl">Vrsta laboratorijskega opazovanja, ki se izvaja brez kakr&#x161;nekoli interakcije med raziskovalcem in njegovimi/njenimi subjekti.</skos:definition>
      <skos:prefLabel xml:lang="sv">Icke-deltagande laboratorieobservation</skos:prefLabel>
      <skos:definition xml:lang="sv">Laboratorieobservation som utf&#xf6;rs utan interaktion mellan forskaren och dennes forskningsobjekt.</skos:definition>
      <skos:prefLabel xml:lang="en">Non-participant laboratory observation</skos:prefLabel>
      <skos:definition xml:lang="en">Type of laboratory observation that is conducted without any interaction between the researcher and his/her subjects.</skos:definition>
      <skos:prefLabel xml:lang="de">Nicht-teilnehmende Laborbeobachtung</skos:prefLabel>
      <skos:definition xml:lang="de">Eine Art der Laborbeobachtung, die ohne jegliche Interaktion zwischen dem/der Forscher*in und seinen/ihren Probanden*innen durchgef&#xfc;hrt wird.</skos:definition>
      <skos:prefLabel xml:lang="no">Ikke-deltagende laboratorieobservasjon</skos:prefLabel>
      <skos:definition xml:lang="no">En type laboratorieobservasjon som blir gjennomf&#xf8;rt uten interaksjon mellom forskeren og studieobjektene.</skos:definition>
      <skos:prefLabel xml:lang="lt">Laboratorinis steb&#x117;jimas nedalyvaujant</skos:prefLabel>
      <skos:definition xml:lang="lt">Laboratorinio steb&#x117;jimo, kuris atliekamas be jokio tyr&#x117;jo ir tiriam&#x173;j&#x173; s&#x105;veikos, tipas.</skos:definition>
      <skos:prefLabel xml:lang="it">Osservazione non partecipante in laboratorio</skos:prefLabel>
      <skos:definition xml:lang="it">Osservazione condotta in laboratorio senza alcuna interazione tra il ricercatore e i soggetti.</skos:definition>
      <skos:prefLabel xml:lang="fr">Observation non-participante en laboratoire</skos:prefLabel>
      <skos:definition xml:lang="fr">Type d&apos;observation en laboratoire qui a &#xe9;t&#xe9; conduite sans aucune interaction entre le chercheur et ses sujets.</skos:definition>
      <skos:prefLabel xml:lang="nl">Niet-participerende observatie in het lab</skos:prefLabel>
      <skos:definition xml:lang="nl"></skos:definition>
   </rdf:Description>
   <rdf:Description rdf:about="http://rdf-vocabulary.ddialliance.org/cv/ModeOfCollection/5.0.0/40b8b0c">
      <rdf:type rdf:resource="http://www.w3.org/2004/02/skos/core#Concept"/>
      <skos:inScheme rdf:resource="http://rdf-vocabulary.ddialliance.org/cv/ModeOfCollection/5.0.0/"/>
      <skos:notation xml:lang="en">Observation.ComputerBased</skos:notation>
      <skos:prefLabel xml:lang="sl">Ra&#x10d;unalni&#x161;ko podprto opazovanje</skos:prefLabel>
      <skos:definition xml:lang="sl">Vrsta opazovanja, kjer se podatki o uporabi ra&#x10d;unalnika zbirajo s programsko opremo, ki se jo lahko vgradi v sam ra&#x10d;unalni&#x161;ki program ali pa predstavlja lo&#x10d;en program. Lahko se zbirajo informacije o &#x161;tevilu uporabnikov, o na&#x10d;inih interakcije uporabnikov z ra&#x10d;unalni&#x161;kim(i) programom(-mi), koliko &#x10d;asa porabijo na strani, kako uporabljajo dolo&#x10d;ene dele aplikacije, kako krmarijo po straneh ali med aplikacijami itd.</skos:definition>
      <skos:prefLabel xml:lang="sv">Datorbaserad observation</skos:prefLabel>
      <skos:definition xml:lang="sv">Observation d&#xe4;r data om datoranv&#xe4;ndning samlas in av programvara som inkluderats i ett datorprogram eller som kan vara ett separat program. Information kan samlas in om antal anv&#xe4;ndare, hur anv&#xe4;ndare interagerar med programmet, hur l&#xe4;nge de stannar p&#xe5; en sida, hur de anv&#xe4;nder best&#xe4;mda delar av program, hur de navigerar fr&#xe5;n en sida till en annan eller v&#xe4;xlar mellan program m.m.</skos:definition>
      <skos:prefLabel xml:lang="en">Computer-based observation</skos:prefLabel>
      <skos:definition xml:lang="en">Type of observation in which data regarding computer usage are being collected by software that can be built into the computer program itself or can be a separate program. Information may be collected about the number of users, the ways in which users interact with the program(s), how much time they spend on a page, how they use specific sections of applications, how they navigate from page to page or from one application to another, etc.</skos:definition>
      <skos:prefLabel xml:lang="de">Computer-basierte Beobachtung</skos:prefLabel>
      <skos:definition xml:lang="de">Art der Beobachtung, bei der Daten &#xfc;ber die Computernutzung von einer Software gesammelt werden, die in das Computerprogramm selbst eingebaut sein kann oder ein separates Programm ist. Es k&#xf6;nnen Informationen &#xfc;ber die Anzahl der Benutzer, die Art und Weise, wie die Benutzer mit dem/den Programm(en) interagieren, wie viel Zeit sie auf einer Seite verbringen, wie sie bestimmte Abschnitte von Anwendungen nutzen, wie sie von Seite zu Seite oder von einer Anwendung zu einer anderen navigieren, usw. gesammelt werden.</skos:definition>
      <skos:prefLabel xml:lang="no">Datamaskinbasert observasjon</skos:prefLabel>
      <skos:definition xml:lang="no">Type observasjon hvor data om datamaskinbruk blir samlet av program som kan v&#xe6;re inkludert i dataprogrammet en &#xf8;nsker informasjon om, eller kan forekomme som et eget program. Informasjon om antall brukere, m&#xe5;ten brukere samhandler med program(met/mene), hvor mye tid de bruker p&#xe5; siden, hvordan de bruker bestemte deler av en applikasjon, hvordan de navigerer fra side til side eller fra en applikasjon til en annen etc., kan bli samlet.</skos:definition>
      <skos:prefLabel xml:lang="lt">Kompiuterinis steb&#x117;jimas</skos:prefLabel>
      <skos:definition xml:lang="lt">Steb&#x117;jimo tipas, kai duomenis apie kompiuterio naudojim&#x105; renka programin&#x117; &#x12f;ranga. Ji gali b&#x16b;ti i&#x161;orin&#x117; arba integruota. Informacija gali b&#x16b;ti renkama apie vartotoj&#x173; skai&#x10d;i&#x173;, b&#x16b;dus, kaip vartotojai s&#x105;veikauja su programa (-omis), kiek laiko praleid&#x17e;ia puslapyje, kaip naudoja tam tikras programos dalis, kaip nar&#x161;o i&#x161; vieno puslapio &#x12f; kit&#x105;, pereina i&#x161; vienos programos &#x12f; kit&#x105; ir kt.</skos:definition>
      <skos:prefLabel xml:lang="it">Osservazione basata su computer</skos:prefLabel>
      <skos:definition xml:lang="it">Tipo di osservazione in cui vengono raccolti dati riguardanti l&apos;uso del computer, attraverso software che pu&#xf2; essere incorporato nel programma informatico stesso, oppure essere un programma separato. Con questo metodo si possono raccogliere informazioni sul numero di utenti, sui modi in cui gli utenti interagiscono con il programma, sulla quantit&#xe0; di tempo che trascorrono su una pagina, su come utilizzano specifiche sezioni di applicazioni, su come navigano da una pagina all&apos;altra o da una applicazione all&apos;altra, ecc.</skos:definition>
      <skos:prefLabel xml:lang="fr">Observation assist&#xe9;e par ordinateur</skos:prefLabel>
      <skos:definition xml:lang="fr">Type d&apos;observation dans lequel les donn&#xe9;es relatives &#xe0; l&apos;utilisation de l&apos;ordinateur ont &#xe9;t&#xe9; collect&#xe9;es par un logiciel qui peut &#xea;tre int&#xe9;gr&#xe9; au programme informatique ou &#xea;tre un programme s&#xe9;par&#xe9;. Des informations peuvent &#xea;tre collect&#xe9;es sur le nombre d&apos;utilisateurs, la fa&#xe7;on dont les utilisateurs interagissent avec le(s) programme(s), le temps qu&apos;ils passent sur une page, la fa&#xe7;on dont ils utilisent des sections sp&#xe9;cifiques des applications, dont ils naviguent d&apos;une page &#xe0; l&apos;autre ou d&apos;une application &#xe0; l&apos;autre, etc.</skos:definition>
      <skos:prefLabel xml:lang="nl">Computer-gebaseerde observatie</skos:prefLabel>
      <skos:definition xml:lang="nl"></skos:definition>
   </rdf:Description>
   <rdf:Description rdf:about="http://rdf-vocabulary.ddialliance.org/cv/ModeOfCollection/5.0.0/05aeba4">
      <rdf:type rdf:resource="http://www.w3.org/2004/02/skos/core#Concept"/>
      <skos:inScheme rdf:resource="http://rdf-vocabulary.ddialliance.org/cv/ModeOfCollection/5.0.0/"/>
      <skos:notation xml:lang="en">Experiment</skos:notation>
      <skos:prefLabel xml:lang="sl">Eksperiment</skos:prefLabel>
      <skos:definition xml:lang="sl">Raziskovalna metoda, ki vklju&#x10d;uje manipulacijo nekaterih ali vseh neodvisnih spremenljivk, vklju&#x10d;enih v hipoteze.</skos:definition>
      <skos:prefLabel xml:lang="sv">Experiment</skos:prefLabel>
      <skos:definition xml:lang="sv">Forskningsmetod som omfattar att styra vissa eller alla oberoende variabler som ing&#xe5;r i hypotesen.</skos:definition>
      <skos:prefLabel xml:lang="en">Experiment</skos:prefLabel>
      <skos:definition xml:lang="en">Research method involving the manipulation of some or all of the independent variables included in the hypotheses.</skos:definition>
      <skos:prefLabel xml:lang="de">Experiment</skos:prefLabel>
      <skos:definition xml:lang="de">Forschungsmethode, die die Manipulation einiger oder aller der in den Hypothesen enthaltenen unabh&#xe4;ngigen Variablen beinhaltet.</skos:definition>
      <skos:prefLabel xml:lang="no">Eksperiment</skos:prefLabel>
      <skos:definition xml:lang="no">Forskningsmetode som inneb&#xe6;rer manipulering av noen eller alle de uavhengige variablene inkludert i hypotesene.</skos:definition>
      <skos:prefLabel xml:lang="lt">Eksperimentas</skos:prefLabel>
      <skos:definition xml:lang="lt">Tyrimo metodas apimantis &#x12f; hipotezes &#x12f;traukt&#x173; kai kuri&#x173; ar vis&#x173; nepriklausom&#x173; kintam&#x173;j&#x173; manipuliavim&#x105;.</skos:definition>
      <skos:prefLabel xml:lang="it">Esperimento</skos:prefLabel>
      <skos:definition xml:lang="it">Metodo di ricerca che coinvolge la manipolazione di alcune o tutte le variabili indipendenti incluse nelle ipotesi.</skos:definition>
      <skos:prefLabel xml:lang="fr">Exp&#xe9;rimentation</skos:prefLabel>
      <skos:definition xml:lang="fr">M&#xe9;thode de recherche impliquant la manipulation d&apos;une partie ou de toutes les variables ind&#xe9;pendantes incluses dans les hypoth&#xe8;ses.</skos:definition>
      <skos:prefLabel xml:lang="nl">Experiment</skos:prefLabel>
      <skos:definition xml:lang="nl"></skos:definition>
      <skos:narrower rdf:resource="http://rdf-vocabulary.ddialliance.org/cv/ModeOfCollection/5.0.0/28a60a6"/>
      <skos:narrower rdf:resource="http://rdf-vocabulary.ddialliance.org/cv/ModeOfCollection/5.0.0/5ff61de"/>
      <skos:narrower rdf:resource="http://rdf-vocabulary.ddialliance.org/cv/ModeOfCollection/5.0.0/ed0d083"/>
   </rdf:Description>
   <rdf:Description rdf:about="http://rdf-vocabulary.ddialliance.org/cv/ModeOfCollection/5.0.0/28a60a6">
      <rdf:type rdf:resource="http://www.w3.org/2004/02/skos/core#Concept"/>
      <skos:inScheme rdf:resource="http://rdf-vocabulary.ddialliance.org/cv/ModeOfCollection/5.0.0/"/>
      <skos:notation xml:lang="en">Experiment.Laboratory</skos:notation>
      <skos:prefLabel xml:lang="sl">Laboratorijski eksperiment</skos:prefLabel>
      <skos:definition xml:lang="sl">Eksperiment, ki se izvaja v nadzorovanem, umetno ustvarjenem fizi&#x10d;nem okolju, v katerem raziskovalec manipulira z eno ali ve&#x10d; neodvisnimi spremenljivkami in meri svoj vpliv na odvisno spremenljivko.</skos:definition>
      <skos:prefLabel xml:lang="sv">Laboratorieexperiment</skos:prefLabel>
      <skos:definition xml:lang="sv">Ett experiment som utf&#xf6;rs i en kontrollerad, konstgjord fysisk milj&#xf6; d&#xe4;r forskaren styr en eller flera oberoende variabler och m&#xe4;ter dess/deras effekt p&#xe5; den beroende variabeln.</skos:definition>
      <skos:prefLabel xml:lang="en">Laboratory experiment</skos:prefLabel>
      <skos:definition xml:lang="en">An experiment conducted in a controlled, artificially created physical setting, in which a researcher manipulates one or several independent variables and measures its/their effect on the dependent variable.</skos:definition>
      <skos:prefLabel xml:lang="de">Laborexperiment</skos:prefLabel>
      <skos:definition xml:lang="de">Ein Experiment, das in einer kontrollierten, k&#xfc;nstlich erzeugten Umgebung durchgef&#xfc;hrt wird, in der Forschende eine oder mehrere unabh&#xe4;ngige Variablen manipulieren und ihre Wirkung auf die abh&#xe4;ngige Variable messen.</skos:definition>
      <skos:prefLabel xml:lang="no">Laboratorieeksperiment</skos:prefLabel>
      <skos:definition xml:lang="no">Et eksperiment som utf&#xf8;res i et kontrollert, kunstig utformet milj&#xf8;, hvor forskeren manipulerer &#xe9;n eller flere av de uavhengige variablene og m&#xe5;ler effekten det har p&#xe5; den avhengige variabelen.</skos:definition>
      <skos:prefLabel xml:lang="lt">Laboratorinis eksperimentas</skos:prefLabel>
      <skos:definition xml:lang="lt">Eksperimentas, atliekamas kontroliuojamoje, dirbtinai sukurtoje fizin&#x117;je aplinkoje, kurio metu tyr&#x117;jas manipuliuoja vienu ar keliais nepriklausomais kintamaisiais ir i&#x161;matuoja j&#x173; poveik&#x12f; priklausomam kintamajam.</skos:definition>
      <skos:prefLabel xml:lang="it">Esperimento in laboratorio</skos:prefLabel>
      <skos:definition xml:lang="it">Un esperimento condotto in un ambiente fisico controllato, creato artificialmente, in cui un ricercatore manipola una o pi&#xf9; variabili indipendenti e misura il loro effetto sulla variabile dipendente.</skos:definition>
      <skos:prefLabel xml:lang="fr">Exp&#xe9;rimentation en laboratoire</skos:prefLabel>
      <skos:definition xml:lang="fr">Une exp&#xe9;rimentation conduite dans un environnement physique contr&#xf4;l&#xe9;, cr&#xe9;&#xe9; artificiellement, dans lequel un chercheur manipule une ou plusieurs variables ind&#xe9;pendantes et mesure son / leur effet sur la variable d&#xe9;pendante.</skos:definition>
      <skos:prefLabel xml:lang="nl">Experiment in het lab</skos:prefLabel>
      <skos:definition xml:lang="nl"></skos:definition>
   </rdf:Description>
   <rdf:Description rdf:about="http://rdf-vocabulary.ddialliance.org/cv/ModeOfCollection/5.0.0/5ff61de">
      <rdf:type rdf:resource="http://www.w3.org/2004/02/skos/core#Concept"/>
      <skos:inScheme rdf:resource="http://rdf-vocabulary.ddialliance.org/cv/ModeOfCollection/5.0.0/"/>
      <skos:notation xml:lang="en">Experiment.FieldIntervention</skos:notation>
      <skos:prefLabel xml:lang="sl">Terenski/intervencijski eksperiment</skos:prefLabel>
      <skos:definition xml:lang="sl">Eksperiment, ki se izvaja v naravnem, nekontroliranem okolju, v katerem raziskovalec manipulira z eno ali ve&#x10d; neodvisnimi spremenljivkami. Intervencija/klini&#x10d;ne &#x161;tudije so en primer terenskih eksperimentov.</skos:definition>
      <skos:prefLabel xml:lang="sv">F&#xe4;ltexperiment</skos:prefLabel>
      <skos:definition xml:lang="sv">Ett experiment som utf&#xf6;rs i en naturlig, okontrollerad milj&#xf6; d&#xe4;r forskaren styr en eller flera oberoende variabler. Interventionsstudier och kliniska studier &#xe4;r exempel p&#xe5; f&#xe4;ltexperiment.</skos:definition>
      <skos:prefLabel xml:lang="en">Field/Intervention experiment</skos:prefLabel>
      <skos:definition xml:lang="en">An experiment conducted in a natural, uncontrolled setting, in which the researcher manipulates one or several independent variables. Intervention/clinical studies are one example of field experiments.</skos:definition>
      <skos:prefLabel xml:lang="de">Feld-/Interventionsexperiment</skos:prefLabel>
      <skos:definition xml:lang="de">Ein Experiment, das in einer nat&#xfc;rlichen, unkontrollierten Umgebung durchgef&#xfc;hrt wird, in der Forschende eine oder mehrere unabh&#xe4;ngige Variablen manipulieren. Interventions-/klinische Studien sind ein Beispiel f&#xfc;r Feldexperimente.</skos:definition>
      <skos:prefLabel xml:lang="no">Felt/felteksperiment</skos:prefLabel>
      <skos:definition xml:lang="no">Et eksperiment som utf&#xf8;res i et naturlig, ukontrollert milj&#xf8;, hvor forskeren manipulerer &#xe9;n eller flere av de uavhengige variablene. Intervensjon/kliniske studier er et eksempel p&#xe5; felteksperiment.</skos:definition>
      <skos:prefLabel xml:lang="lt">Lauko arba intervencinis eksperimentas</skos:prefLabel>
      <skos:definition xml:lang="lt">Eksperimentas, atliktas nat&#x16b;ralioje, nekontroliuojamoje aplinkoje, kurio metu tyr&#x117;jas manipuliuoja vienu ar keliais nepriklausomais kintamaisiais. Intervenciniai ar klinikiniai tyrimai yra lauko eksperiment&#x173; pavyzd&#x17e;iai.</skos:definition>
      <skos:prefLabel xml:lang="it">Esperimento sul campo / Intervento</skos:prefLabel>
      <skos:definition xml:lang="it">Un esperimento condotto in un ambiente naturale, non controllato, in cui il ricercatore manipola una o pi&#xf9; variabili indipendenti. Gli interventi o studi clinici sono un esempio di esperimenti sul campo.</skos:definition>
      <skos:prefLabel xml:lang="fr">Exp&#xe9;rimentation sur le terrain</skos:prefLabel>
      <skos:definition xml:lang="fr">Une exp&#xe9;rimentation conduite dans un environnement naturel, non contr&#xf4;l&#xe9;, dans lequel le chercheur manipule une ou plusieurs variables ind&#xe9;pendantes. Des &#xe9;tudes cliniques sont un exemple d&apos;exp&#xe9;rimentations sur le terrain.</skos:definition>
      <skos:prefLabel xml:lang="nl">Experiment in het veld/interventie</skos:prefLabel>
      <skos:definition xml:lang="nl"></skos:definition>
   </rdf:Description>
   <rdf:Description rdf:about="http://rdf-vocabulary.ddialliance.org/cv/ModeOfCollection/5.0.0/ed0d083">
      <rdf:type rdf:resource="http://www.w3.org/2004/02/skos/core#Concept"/>
      <skos:inScheme rdf:resource="http://rdf-vocabulary.ddialliance.org/cv/ModeOfCollection/5.0.0/"/>
      <skos:notation xml:lang="en">Experiment.WebBased</skos:notation>
      <skos:prefLabel xml:lang="sl">Spletni eksperiment</skos:prefLabel>
      <skos:definition xml:lang="sl">Eksperiment, ki se izvaja v virtualnem okolju svetovnega spleta, v katerem so eksperimentalni materiali programirani za izvajanje umetnih situacij ali dogodkov, ki jih je treba raziskati v tako vzpostavljenem okolju. (Reips, U.-D. (2002). Theory and techniques of Web experimenting. V B. Batinic, U.-D. Reips, &amp; M. Bosnjak (Eds.), Online Social Sciences. Seattle: Hogrefe &amp; Huber. Dostopno preko: http://www.websm.org/uploadi/editor/Reips_2002_Theory_and_techniques.pdf [07. junij 2013])</skos:definition>
      <skos:prefLabel xml:lang="sv">Webbaserat experiment</skos:prefLabel>
      <skos:definition xml:lang="sv">Ett experiment som utf&#xf6;rs i en virtuell milj&#xf6; p&#xe5; webben, d&#xe4;r experimentella material programmeras f&#xf6;r att skapa artificiella situationer eller h&#xe4;ndelser som unders&#xf6;ks i en distribuerad milj&#xf6;.  (Reips, U.-D. (2002). Theory and techniques of Web experimenting. In B. Batinic, U.-D. Reips, &amp; M. Bosnjak (Eds.), Online Social Sciences. Seattle: Hogrefe &amp; Huber. Tillg&#xe4;nglig: http://www.websm.org/uploadi/editor/Reips_2002_Theory_and_techniques.pdf [8 september, 2016])</skos:definition>
      <skos:prefLabel xml:lang="en">Web-based experiment</skos:prefLabel>
      <skos:definition xml:lang="en">An experiment conducted in the virtual setting of the World Wide Web, in which experimental materials are programmed to implement artificial situations or events to be investigated in a distributed environment. (Reips, U.-D. (2002). Theory and techniques of Web experimenting. In B. Batinic, U.-D. Reips, &amp; M. Bosnjak (Eds.), Online Social Sciences. Seattle: Hogrefe &amp; Huber. Available at: http://www.websm.org/uploadi/editor/Reips_2002_Theory_and_techniques.pdf [07 June 2013])</skos:definition>
      <skos:prefLabel xml:lang="de">Web-basiertes Experiment</skos:prefLabel>
      <skos:definition xml:lang="de">Ein Experiment, das in der virtuellen Umgebung des World Wide Web durchgef&#xfc;hrt wird, in dem experimentelle Materialien programmiert werden, um k&#xfc;nstliche Situationen oder Ereignisse zu implementieren, die in einer verteilten Umgebung untersucht werden sollen.</skos:definition>
      <skos:prefLabel xml:lang="no">Webbasert eksperiment</skos:prefLabel>
      <skos:definition xml:lang="no">Et eksperiment som utf&#xf8;res i et vituelt milj&#xf8; p&#xe5; internett (World Wide Web), hvor eksperimentelt materiale er programmert til &#xe5; sette i gang kunstige situasjoner eller hendelser som kan unders&#xf8;kes i et gitt milj&#xf8;. (Reips, U.-D. (2002). Theory and techniques of Web experimenting. In B. Batinic, U.-D. Reips, &amp; M. Bosnjak (Eds.), Online Social Sciences. Seattle: Hogrefe &amp; Huber. Available at: http://www.websm.org/uploadi/editor/Reips_2002_Theory_and_techniques.pdf [07 June 2013])</skos:definition>
      <skos:prefLabel xml:lang="lt">Internetinis eksperimentas</skos:prefLabel>
      <skos:definition xml:lang="lt">Eksperimentas atliekamas virtualioje aplinkoje per internet&#x105;, kai suprogramuota eksperimentin&#x117; med&#x17e;iaga sukuria dirbtines situacijas ir &#x12f;vykius paskirstytoje aplinkoje.  (Reips, U.-D. (2002). Theory and techniques of Web experimenting. In B. Batinic, U.-D. Reips, &amp; M. Bosnjak (Eds.), Online Social Sciences. Seattle: Hogrefe &amp; Huber. Galima rasti: http://www.websm.org/uploadi/editor/Reips_2002_Theory_and_techniques.pdf   [2013 m. bir&#x17e;elio 7 d.]).</skos:definition>
      <skos:prefLabel xml:lang="it">Esperimento web</skos:prefLabel>
      <skos:definition xml:lang="it">Un esperimento condotto nell&apos;ambiente virtuale del World Wide Web, in cui i materiali sperimentali sono programmati per ricreare situazioni o eventi artificiali da indagare in un ambiente distribuito.</skos:definition>
      <skos:prefLabel xml:lang="fr">Exp&#xe9;rimentation par Internet</skos:prefLabel>
      <skos:definition xml:lang="fr">Une exp&#xe9;rimentation conduite dans une configuration virtuelle sur le Web, dans laquelle des mat&#xe9;riaux exp&#xe9;rimentaux sont programm&#xe9;s pour mettre en &#x153;uvre des situations ou des &#xe9;v&#xe9;nements artificiels &#xe0; &#xe9;tudier dans un environnement distribu&#xe9;.  (Reips, U.-D. (2002). Theory and techniques of Web experimenting. In B. Batinic, U.-D. Reips, &amp; M. Bosnjak (Eds.), Online Social Sciences. Seattle: Hogrefe &amp; Huber. Available at: http://www.websm.org/uploadi/editor/Reips_2002_Theory_and_techniques.pdf [07 June 2013])</skos:definition>
      <skos:prefLabel xml:lang="nl">Webgebaseerd experiment</skos:prefLabel>
      <skos:definition xml:lang="nl"></skos:definition>
   </rdf:Description>
   <rdf:Description rdf:about="http://rdf-vocabulary.ddialliance.org/cv/ModeOfCollection/5.0.0/c5564d2">
      <rdf:type rdf:resource="http://www.w3.org/2004/02/skos/core#Concept"/>
      <skos:inScheme rdf:resource="http://rdf-vocabulary.ddialliance.org/cv/ModeOfCollection/5.0.0/"/>
      <skos:notation xml:lang="en">Recording</skos:notation>
      <skos:prefLabel xml:lang="sl">Snemanje</skos:prefLabel>
      <skos:definition xml:lang="sl">Snemanje z mehanskimi ali elektronskimi sredstvi v obliki, ki omogo&#x10d;a, da se informacije prikli&#x10d;ejo in/ali reproducirajo. Na primer slike ali zvoki na disku ali magnetnem traku.</skos:definition>
      <skos:prefLabel xml:lang="sv">Inspelning</skos:prefLabel>
      <skos:definition xml:lang="sv">Upptagning, p&#xe5; mekanisk eller elektronisk v&#xe4;g, p&#xe5; s&#xe5;dant s&#xe4;tt att informationen kan &#xe5;terf&#xe5;s och/eller &#xe5;terskapas. Exempel: bilder eller ljud p&#xe5; en cd eller ett magnetband.</skos:definition>
      <skos:prefLabel xml:lang="en">Recording</skos:prefLabel>
      <skos:definition xml:lang="en">Registering by mechanical or electronic means, in a form that allows the information to be retrieved and/or reproduced. For example, images or sounds on disc or magnetic tape.</skos:definition>
      <skos:prefLabel xml:lang="de">Aufzeichnung (mechanisch/elektronisch)</skos:prefLabel>
      <skos:definition xml:lang="de">Aufzeichnungen, die auf mechanischem oder elektronischem Wege get&#xe4;tigt werden und die es erm&#xf6;glichen, die Informationen abzurufen und/oder zu reproduzieren. Zum Beispiel Bilder oder T&#xf6;ne auf Diskette oder Magnetband.</skos:definition>
      <skos:prefLabel xml:lang="no">Opptak</skos:prefLabel>
      <skos:definition xml:lang="no">Mekanisk eller elektronisk registrering i et format som gj&#xf8;r det mulig &#xe5; gjeninnhente og/eller gjenskape informasjonen. For eksempel bilder eller lyd p&#xe5; disk eller magnetb&#xe5;nd.</skos:definition>
      <skos:prefLabel xml:lang="lt">&#x12e;ra&#x161;as</skos:prefLabel>
      <skos:definition xml:lang="lt">Mechanin&#x117;mis ar elektronin&#x117;mis priemon&#x117;mis atliekamas &#x12f;ra&#x161;ymas taip, kad informacij&#x105; b&#x16b;t&#x173; galima pasiekti ir (arba) atkurti. Pavyzd&#x17e;iui, vaizdai ar garsai diske ar magnetin&#x117;je juostoje.</skos:definition>
      <skos:prefLabel xml:lang="it">Registrazione</skos:prefLabel>
      <skos:definition xml:lang="it">Registrazione tramite mezzi meccanici o elettronici, in una forma che consente di recuperare e/o riprodurre le informazioni. Ad esempio, registrazioni di immagini o suoni su disco o supporto magnetico.</skos:definition>
      <skos:prefLabel xml:lang="fr">Enregistrement</skos:prefLabel>
      <skos:definition xml:lang="fr">Enregistrement par des moyens m&#xe9;caniques ou &#xe9;lectroniques, sous une forme permettant la r&#xe9;cup&#xe9;ration et / ou la reproduction des informations. Par exemple, des images ou des sons sur disque ou bande magn&#xe9;tique.</skos:definition>
      <skos:prefLabel xml:lang="nl">Opname</skos:prefLabel>
      <skos:definition xml:lang="nl"></skos:definition>
      <skos:narrower rdf:resource="http://rdf-vocabulary.ddialliance.org/cv/ModeOfCollection/5.0.0/f25ffb0"/>
   </rdf:Description>
   <rdf:Description rdf:about="http://rdf-vocabulary.ddialliance.org/cv/ModeOfCollection/5.0.0/f25ffb0">
      <rdf:type rdf:resource="http://www.w3.org/2004/02/skos/core#Concept"/>
      <skos:inScheme rdf:resource="http://rdf-vocabulary.ddialliance.org/cv/ModeOfCollection/5.0.0/"/>
      <skos:notation xml:lang="en">Recording.RemoteSensing</skos:notation>
      <skos:prefLabel xml:lang="sl">Snemanje: daljinsko zaznavanje</skos:prefLabel>
      <skos:definition xml:lang="sl">Zbiranje informacij o predmetih ali pojavih brez fizi&#x10d;nega stika z njimi z uporabo daljinskih senzorjev na satelitih in letalih (letala, droni, vremenski baloni). Pogosto se uporablja za zbiranje informacij o zemeljski povr&#x161;ini, ozra&#x10d;ju in oceanih. Na primer ocena &#x161;kode po potresu ali gozdnih po&#x17e;arih. Tehnika se uporablja tudi za voja&#x161;ke, komercialne, gospodarske in druge namene.</skos:definition>
      <skos:prefLabel xml:lang="sv">Inspelning: fj&#xe4;rranalys</skos:prefLabel>
      <skos:definition xml:lang="sv">Insamling av information om objekt eller f&#xf6;reteelser utan att ha fysisk kontakt med dem. Insamlingen g&#xf6;rs med fj&#xe4;rrsensorer p&#xe5; satelliter och luftfartyg (t.ex. flygplan, dr&#xf6;nare, v&#xe4;derballonger). Fj&#xe4;rranalys anv&#xe4;nds ofta f&#xf6;r att samla in information om jorden och dess atmosf&#xe4;r och hav, t.ex. skadebed&#xf6;mning efter jordb&#xe4;vningar eller skogsbr&#xe4;nder. Tekniken anv&#xe4;nds &#xe4;ven f&#xf6;r bland annat milit&#xe4;ra, aff&#xe4;rsm&#xe4;ssiga och ekonomiska syften.</skos:definition>
      <skos:prefLabel xml:lang="en">Recording: Remote sensing</skos:prefLabel>
      <skos:definition xml:lang="en">Collecting information on objects or phenomena without physical contact with them, using remote sensors on satellites and aircraft (planes, drones, weather balloons). Often used to gather information on the Earth&#x2019;s surface, atmosphere and oceans. For example, damage assessment after an earthquake or forest fires. The technique is also used for military, commercial, economic and other applications.</skos:definition>
      <skos:prefLabel xml:lang="de">Aufzeichnung: Fernerkundung</skos:prefLabel>
      <skos:definition xml:lang="de">Das Sammeln von Informationen &#xfc;ber Objekte oder Ph&#xe4;nomene ohne physischen Kontakt mit ihnen, mithilfe von Fernsensoren auf Satelliten und Flugzeugen (Flugzeuge, Drohnen, Wetterballons). Wird oft verwendet, um Informationen &#xfc;ber die Erdoberfl&#xe4;che, die Atmosph&#xe4;re und die Ozeane zu sammeln. Zum Beispiel bei der Schadensbeurteilung nach einem Erdbeben oder bei Waldbr&#xe4;nden. Die Technik wird auch f&#xfc;r milit&#xe4;rische, kommerzielle, wirtschaftliche und andere Anwendungen genutzt.</skos:definition>
      <skos:prefLabel xml:lang="no">Opptak: Fjernm&#xe5;ling</skos:prefLabel>
      <skos:definition xml:lang="no">Innsamling av informasjon om objekter eller fenomen uten fysisk kontakt med de ved bruk av fjernm&#xe5;lere p&#xe5; satellitter og luftfart&#xf8;y (fly, droner, v&#xe6;rballonger). Ofte brukt for &#xe5; samle informasjon om jordens overflate, atmosf&#xe6;re og hav. For eksempel, skadevurdering etter et jordskjelv eller skogbrann. Teknikken brukes ogs&#xe5; av milit&#xe6;re, kommersielle, &#xf8;konomiske og andre form&#xe5;l.</skos:definition>
      <skos:prefLabel xml:lang="lt">&#x12e;ra&#x161;as: nuotolinis steb&#x117;jimas</skos:prefLabel>
      <skos:definition xml:lang="lt">Informacijos apie objektus ar rei&#x161;kinius rinkimas be fizinio kontakto su jais, naudojant nuotolinius palydov&#x173; ir orlaivi&#x173; (l&#x117;ktuv&#x173;, nepilotuojam&#x173; orlaivi&#x173;, oro balion&#x173;) jutiklius. Da&#x17e;nai naudojamas renkant informacij&#x105; apie &#x17d;em&#x117;s pavir&#x161;i&#x173;, atmosfer&#x105; ir vandenynus. Pavyzd&#x17e;iui, &#x17e;alos vertinimas po &#x17e;em&#x117;s dreb&#x117;jim&#x173; ar mi&#x161;k&#x173; gaisr&#x173;. &#x160;i technika taip pat naudojama karin&#x117;ms, komercin&#x117;ms, ekonomin&#x117;ms ir kitoms reikm&#x117;ms.</skos:definition>
      <skos:prefLabel xml:lang="it">Registrazione: telerilevamento</skos:prefLabel>
      <skos:definition xml:lang="it">Raccolta di informazioni relative ad oggetti o fenomeni senza che vi sia un contatto fisico con essi, utilizzando sensori remoti posizionati su satelliti e apparecchi aeronautici (aerei, droni, palloni sonda). Spesso &#xe8; utilizzato per raccogliere informazioni sulla superficie terrestre, sull&apos;atmosfera e sugli oceani. Per esempio, viene utilizzato per la valutazione dei danni causati da un terremoto o da incendi boschivi. La tecnica &#xe8; usata anche per applicazioni in campo militare, commerciale, economico e di altro tipo.</skos:definition>
      <skos:prefLabel xml:lang="fr">Enregistrement : t&#xe9;l&#xe9;d&#xe9;tection</skos:prefLabel>
      <skos:definition xml:lang="fr">Collecte d&#x2019;informations sur des objets ou des ph&#xe9;nom&#xe8;nes sans contact physique avec ceux-ci, en utilisant des capteurs &#xe0; distance install&#xe9;s sur des satellites et des a&#xe9;ronefs (avions, drones, ballons m&#xe9;t&#xe9;orologiques). Cette m&#xe9;thode est souvent utilis&#xe9;e pour recueillir des donn&#xe9;es sur la surface terrestre, l&#x2019;atmosph&#xe8;re et les oc&#xe9;ans. Par exemple, pour l&#x2019;&#xe9;valuation des d&#xe9;g&#xe2;ts apr&#xe8;s un tremblement de terre ou des incendies de for&#xea;t. Cette technique est &#xe9;galement employ&#xe9;e dans des domaines militaires, commerciaux, &#xe9;conomiques et autres.</skos:definition>
      <skos:prefLabel xml:lang="nl">Opname: op afstand opgenomen</skos:prefLabel>
      <skos:definition xml:lang="nl"></skos:definition>
   </rdf:Description>
   <rdf:Description rdf:about="http://rdf-vocabulary.ddialliance.org/cv/ModeOfCollection/5.0.0/c867d80">
      <rdf:type rdf:resource="http://www.w3.org/2004/02/skos/core#Concept"/>
      <skos:inScheme rdf:resource="http://rdf-vocabulary.ddialliance.org/cv/ModeOfCollection/5.0.0/"/>
      <skos:notation xml:lang="en">AutomatedDataExtraction</skos:notation>
      <skos:prefLabel xml:lang="sl">Avtomatizirano pridobivanje podatkov</skos:prefLabel>
      <skos:definition xml:lang="sl">Uporaba avtomatiziranih sredstev za pridobivanje informacij iz virov podatkov in njihov prenos v lokalno datoteko ali bazo podatkov za nadaljnjo obdelavo ali shranjevanje. Uporabite ta izraz, &#x10d;e ni znano, kak&#x161;na avtomatizirana tehnika je bila uporabljena ali &#x10d;e je tehnika znana, vendar ni navedena kot o&#x17e;ji izraz.</skos:definition>
      <skos:prefLabel xml:lang="sv">Automatiserad dataextrahering</skos:prefLabel>
      <skos:definition xml:lang="sv">Anv&#xe4;ndning av automatiserade metoder f&#xf6;r att h&#xe4;mta information ur datak&#xe4;llor och spara informationen som en lokal fil eller databas f&#xf6;r ytterligare behandling eller lagring. Anv&#xe4;nd den h&#xe4;r termen om det inte &#xe4;r k&#xe4;nt vilken automatiserad teknik som anv&#xe4;nts eller om tekniken &#xe4;r k&#xe4;nd, men inte finns listad som en smalare term.</skos:definition>
      <skos:prefLabel xml:lang="en">Automated data extraction</skos:prefLabel>
      <skos:definition xml:lang="en">Using automated means to retrieve information from data sources and save it to a local file or database for further processing or storage. Use this term if it is not known what kind of automated technique has been used or if the technique is known but not listed as a narrower term.</skos:definition>
      <skos:prefLabel xml:lang="de">Automatisierte Datenextraktion</skos:prefLabel>
      <skos:definition xml:lang="de">Verwendung automatisierter Mittel zum Abrufen von Informationen aus Datenquellen und Speichern in einer lokalen Datei oder Datenbank zur weiteren Verarbeitung oder Speicherung. Verwenden Sie diesen Begriff, wenn nicht bekannt ist, welche Art von automatisierter Technik verwendet wurde, oder wenn die Technik bekannt ist, aber nicht als engerer Begriff aufgef&#xfc;hrt ist.</skos:definition>
      <skos:prefLabel xml:lang="no">Automatisert datautvinning</skos:prefLabel>
      <skos:definition xml:lang="no">&#xc5; bruke automatiske midler for &#xe5; hente informasjon fra datakilder og lagre det i en lokal fil eller database for ytterligere prosessering eller oppbevaring. Bruk denne termen hvis det er ukjent hvilke automatisk teknikk som har blitt brukt eller teknikken er kjent, men ikke er oppf&#xf8;rt i et av de smalere begrepene.</skos:definition>
      <skos:prefLabel xml:lang="lt">Automatin&#x117; duomen&#x173; gavyba</skos:prefLabel>
      <skos:definition xml:lang="lt">Automatini&#x173; priemoni&#x173; naudojimas, siekiant nuskaityti informacij&#x105; i&#x161; duomen&#x173; &#x161;altini&#x173; ir i&#x161;saugoti j&#x105; vidiniame faile arba duomen&#x173; baz&#x117;je, skirtoje tolesniam apdorojimui ar saugojimui. Naudoti &#x161;&#x12f; platesn&#x12f; termin&#x105;, kai n&#x117;ra &#x17e;inoma, kokia automatin&#x117;s duomen&#x173; gavybos technika buvo naudota, arba jei ji yra &#x17e;inoma, bet n&#x117;ra jai skirto siauresnio termino.</skos:definition>
      <skos:prefLabel xml:lang="it">Estrazione automatizzata</skos:prefLabel>
      <skos:definition xml:lang="it">Utilizzo di strumenti automatizzati per recuperare informazioni da fonti di dati e salvarle in un file locale o in un database per una successiva elaborazione o archiviazione. Utilizzare questo termine se non si conosce il tipo di tecnica automatizzata impiegata oppure se la tecnica &#xe8; nota ma non &#xe8; presente nell&apos;elenco.</skos:definition>
      <skos:prefLabel xml:lang="fr">Extraction automatis&#xe9;e des donn&#xe9;es</skos:prefLabel>
      <skos:definition xml:lang="fr">Utilisation de moyens automatis&#xe9;s pour extraire des informations de sources de donn&#xe9;es et les enregistrer dans un fichier local ou une base de donn&#xe9;es en vue d&#x2019;un traitement ou d&#x2019;un stockage ult&#xe9;rieur. Utilisez ce terme lorsque la technique automatis&#xe9;e employ&#xe9;e est inconnue ou lorsqu&#x2019;elle est connue mais non r&#xe9;pertori&#xe9;e en des termes plus sp&#xe9;cifiques.</skos:definition>
      <skos:prefLabel xml:lang="nl">Geautomatiseerde data-extractie</skos:prefLabel>
      <skos:definition xml:lang="nl"></skos:definition>
      <skos:narrower rdf:resource="http://rdf-vocabulary.ddialliance.org/cv/ModeOfCollection/5.0.0/0998f59"/>
      <skos:narrower rdf:resource="http://rdf-vocabulary.ddialliance.org/cv/ModeOfCollection/5.0.0/613d44d"/>
      <skos:narrower rdf:resource="http://rdf-vocabulary.ddialliance.org/cv/ModeOfCollection/5.0.0/d759f9a"/>
   </rdf:Description>
   <rdf:Description rdf:about="http://rdf-vocabulary.ddialliance.org/cv/ModeOfCollection/5.0.0/0998f59">
      <rdf:type rdf:resource="http://www.w3.org/2004/02/skos/core#Concept"/>
      <skos:inScheme rdf:resource="http://rdf-vocabulary.ddialliance.org/cv/ModeOfCollection/5.0.0/"/>
      <skos:notation xml:lang="en">AutomatedDataExtraction.ApiQuery</skos:notation>
      <skos:prefLabel xml:lang="sl">Avtomatizirano pridobivanje podatkov: iskanje preko API</skos:prefLabel>
      <skos:definition xml:lang="sl">Pridobivanje informacij iz spletnih virov podatkov preko API-ja (vmesnik uporabni&#x161;kega programa) in njihov prenos v lokalno datoteko ali bazo podatkov za nadaljnjo obdelavo ali shranjevanje.</skos:definition>
      <skos:prefLabel xml:lang="sv">Automatiserad dataextrahering: API-f&#xf6;rfr&#xe5;gan</skos:prefLabel>
      <skos:definition xml:lang="sv">Inh&#xe4;mtning av information fr&#xe5;n datak&#xe4;llor online via ett API (Application Programming Interface) f&#xf6;r att spara informationen som en lokal fil eller databas f&#xf6;r ytterligare behandling eller lagring.</skos:definition>
      <skos:prefLabel xml:lang="en">Automated data extraction: API query</skos:prefLabel>
      <skos:definition xml:lang="en">Retrieving information from online data sources through an API (application programming interface) to save it to a local file or database for further processing or storage.</skos:definition>
      <skos:prefLabel xml:lang="de">Automatisierte Datenextraktion: API-Abfrage</skos:prefLabel>
      <skos:definition xml:lang="de">Abrufen von Informationen aus Online-Datenquellen &#xfc;ber eine API (Application Programming Interface), um sie in einer lokalen Datei oder Datenbank zur weiteren Verarbeitung oder Speicherung zu speichern.</skos:definition>
      <skos:prefLabel xml:lang="no">Automatisert datautvinning: API sp&#xf8;rring</skos:prefLabel>
      <skos:definition xml:lang="no">&#xc5; hente informasjon fra datakilder p&#xe5; nett via en API (programmeringsgrensesnitt) for &#xe5; lagre det p&#xe5; en lokal fil eller database for ytterligere prosessering eller oppbevaring.</skos:definition>
      <skos:prefLabel xml:lang="lt">Automatin&#x117; duomen&#x173; gavyba: API u&#x17e;klausa</skos:prefLabel>
      <skos:definition xml:lang="lt">Informacijos nuskaitymas i&#x161; internetini&#x173; duomen&#x173; &#x161;altini&#x173;, naudojant API (programin&#x117;s &#x12f;rangos s&#x105;saj&#x105;) ir i&#x161;saugant j&#x105; vidiniame faile ar duomen&#x173; baz&#x117;je tolesniam apdorojimui ar saugojimui.</skos:definition>
      <skos:prefLabel xml:lang="it">Estrazione automatizzata: interrogazione API</skos:prefLabel>
      <skos:definition xml:lang="it">Recupero di informazioni da fonti di dati online attraverso una API (Application Programming Interface) per salvarle in un file locale o in un database per una successiva elaborazione o archiviazione.</skos:definition>
      <skos:prefLabel xml:lang="fr">Extraction automatis&#xe9;e des donn&#xe9;es : requ&#xea;te API</skos:prefLabel>
      <skos:definition xml:lang="fr">R&#xe9;cup&#xe9;ration d&#x2019;informations &#xe0; partir de sources de donn&#xe9;es en ligne via une API (interface de programmation applicative) pour les enregistrer dans un fichier local ou une base de donn&#xe9;es en vue d&#x2019;un traitement ou d&#x2019;un stockage ult&#xe9;rieur.</skos:definition>
      <skos:prefLabel xml:lang="nl">Geautomatiseerde data-extractie: API zoekvraag</skos:prefLabel>
      <skos:definition xml:lang="nl"></skos:definition>
   </rdf:Description>
   <rdf:Description rdf:about="http://rdf-vocabulary.ddialliance.org/cv/ModeOfCollection/5.0.0/613d44d">
      <rdf:type rdf:resource="http://www.w3.org/2004/02/skos/core#Concept"/>
      <skos:inScheme rdf:resource="http://rdf-vocabulary.ddialliance.org/cv/ModeOfCollection/5.0.0/"/>
      <skos:notation xml:lang="en">AutomatedDataExtraction.DatabaseQuery</skos:notation>
      <skos:prefLabel xml:lang="sl">Avtomatizirano pridobivanje podatkov: iskanje po zbirki podatkov</skos:prefLabel>
      <skos:definition xml:lang="sl">Pridobivanje informacij iz zbirke podatkov s pomo&#x10d;jo poizvedbe v zbirko podatkov, da se pridobijo samo zahtevane informacije, in njihov prenos v lokalno datoteko ali bazo podatkov za nadaljnjo obdelavo ali shranjevanje.</skos:definition>
      <skos:prefLabel xml:lang="sv">Automatiserad dataextrahering: databasf&#xf6;rfr&#xe5;gan</skos:prefLabel>
      <skos:definition xml:lang="sv">Inh&#xe4;mtning av information fr&#xe5;n databaser via en f&#xf6;rfr&#xe5;gan till databasen om att extrahera enbart den &#xf6;nskade informationen och sedan spara den som en lokal fil eller databas f&#xf6;r ytterligare behandling eller lagring.</skos:definition>
      <skos:prefLabel xml:lang="en">Automated data extraction: Database query</skos:prefLabel>
      <skos:definition xml:lang="en">Retrieving information from databases through a query to the database to extract only the information required, saving it to a local file or database for further processing or storage.</skos:definition>
      <skos:prefLabel xml:lang="de">Automatisierte Datenextraktion: Datenbankabfrage</skos:prefLabel>
      <skos:definition xml:lang="de">Abrufen von Informationen aus Datenbanken durch eine Abfrage an die Datenbank, um nur die ben&#xf6;tigten Informationen zu extrahieren und sie in einer lokalen Datei oder Datenbank zur weiteren Verarbeitung oder Speicherung zu speichern.</skos:definition>
      <skos:prefLabel xml:lang="no">Automatisert datautvinning: Databasesp&#xf8;rring</skos:prefLabel>
      <skos:definition xml:lang="no">&#xc5; hente informasjon fra databaser via en sp&#xf8;rring til databasen som tar ut kun den informasjonen som er n&#xf8;dvendig for &#xe5; lagre det p&#xe5; en lokal fil eller database for ytterligere prosessering eller oppbevaring.</skos:definition>
      <skos:prefLabel xml:lang="lt">Automatin&#x117; duomen&#x173; gavyba: duomen&#x173; baz&#x117;s u&#x17e;klausa</skos:prefLabel>
      <skos:definition xml:lang="lt">Informacijos nuskaitymas i&#x161; duomen&#x173; bazi&#x173; per j&#x173; u&#x17e;klausas, siekiant i&#x161;gauti tik reikaling&#x105; informacij&#x105; ir i&#x161;saugoti j&#x105; vidiniame faile ar duomen&#x173; baz&#x117;je tolesniam apdorojimui ar saugojimui.</skos:definition>
      <skos:prefLabel xml:lang="it">Estrazione automatizzata: interrogazione database</skos:prefLabel>
      <skos:definition xml:lang="it">Recupero di informazioni da un database attraverso una sua interrogazione con lo scopo di estrarre solo le informazioni necessarie, salvandole in un file locale o in un database per una successiva elaborazione o archiviazione.</skos:definition>
      <skos:prefLabel xml:lang="fr">Extraction automatis&#xe9;e des donn&#xe9;es : requ&#xea;te dans une base de donn&#xe9;es</skos:prefLabel>
      <skos:definition xml:lang="fr">R&#xe9;cup&#xe9;ration d&#x2019;informations &#xe0; partir de bases de donn&#xe9;es via une requ&#xea;te permettant d&#x2019;extraire uniquement les informations n&#xe9;cessaires, puis enregistrement dans un fichier local ou une base de donn&#xe9;es pour un traitement ou un stockage ult&#xe9;rieur.</skos:definition>
      <skos:prefLabel xml:lang="nl">Geautomatiseerde data-extractie: Database zoekvraag</skos:prefLabel>
      <skos:definition xml:lang="nl"></skos:definition>
   </rdf:Description>
   <rdf:Description rdf:about="http://rdf-vocabulary.ddialliance.org/cv/ModeOfCollection/5.0.0/d759f9a">
      <rdf:type rdf:resource="http://www.w3.org/2004/02/skos/core#Concept"/>
      <skos:inScheme rdf:resource="http://rdf-vocabulary.ddialliance.org/cv/ModeOfCollection/5.0.0/"/>
      <skos:notation xml:lang="en">AutomatedDataExtraction.WebScraping</skos:notation>
      <skos:prefLabel xml:lang="sl">Avtomatizirano pridobivanje podatkov: strganje zaslona</skos:prefLabel>
      <skos:definition xml:lang="sl">Tehnika, ki se uporablja za pridobivanje velikih koli&#x10d;in podatkov s spletnih mest. Pridobljeni podatki se prenesejo v lokalno datoteko ali bazo podatkov za nadaljnjo obdelavo ali shranjevanje. Imenuje se tudi lu&#x161;&#x10d;enje podatkov, pridobivanje spletnih podatkov, zbiranje spletnih strani itd.</skos:definition>
      <skos:prefLabel xml:lang="sv">Automatiserad dataextrahering: webbskrapning</skos:prefLabel>
      <skos:definition xml:lang="sv">En teknik som anv&#xe4;nds f&#xf6;r att extrahera stora m&#xe4;ngder data fr&#xe5;n webbplatser och spara dem som en lokal fil eller databas f&#xf6;r ytterligare behandling eller lagring. Tekniken kallas &#xe4;ven f&#xf6;r web scraping, sk&#xe4;rmskrapning (screen scraping), webbsk&#xf6;rdning m.m.</skos:definition>
      <skos:prefLabel xml:lang="en">Automated data extraction: Web scraping</skos:prefLabel>
      <skos:definition xml:lang="en">A technique employed to extract large amounts of data from websites and save it to a local file or database for further processing or storage. Also called screen scraping, web data extraction, web harvesting, etc.</skos:definition>
      <skos:prefLabel xml:lang="de">Automatisierte Datenextraktion: Web Scraping</skos:prefLabel>
      <skos:definition xml:lang="de">Eine Technik, die verwendet wird, um gro&#xdf;e Datenmengen aus Websites zu extrahieren und sie in einer lokalen Datei oder Datenbank zur weiteren Verarbeitung oder Speicherung zu speichern. Auch Screen Scraping, Webdatenextraktion, Web Harvesting usw. genannt.</skos:definition>
      <skos:prefLabel xml:lang="no">Automatisert datautvinning: Nettskraping</skos:prefLabel>
      <skos:definition xml:lang="no">En teknikk som anvendes for &#xe5; hente ut store mengder data fra nettsider og lagre det p&#xe5; en lokal fil eller database for ytterligere prosessering eller oppbevaring. Ogs&#xe5; kalt skjermskraping, utvinning av nettdata, netth&#xf8;sting, etc.</skos:definition>
      <skos:prefLabel xml:lang="lt">Automatin&#x117; duomen&#x173; gavyba: &#x17e;iniatinklio puslapi&#x173; nuskaitymas</skos:prefLabel>
      <skos:definition xml:lang="lt">Technika naudojama siekiant i&#x161; &#x17e;iniatinklio nuskaityti didelius duomen&#x173; kiekius ir i&#x161;saugoti juos vidiniame faile ar duomen&#x173; baz&#x117;je tolesniam apdorojimui ar saugojimui. Taip pat vadinama ekrano duomen&#x173; nuskaitymu, &#x17e;iniatinklio duomen&#x173; gavyba ar kt.</skos:definition>
      <skos:prefLabel xml:lang="it">Estrazione automatizzata: web scraping</skos:prefLabel>
      <skos:definition xml:lang="it">Tecnica utilizzata per estrarre grandi quantit&#xe0; di dati da siti web e salvarli in un file locale o in un database per una successiva elaborazione o archiviazione. Chiamato anche screen scraping, estrazione di dati web, web harvesting, ecc.</skos:definition>
      <skos:prefLabel xml:lang="fr">Extraction automatis&#xe9;e des donn&#xe9;es : Web scraping</skos:prefLabel>
      <skos:definition xml:lang="fr">Technique utilis&#xe9;e pour extraire de grandes quantit&#xe9;s de donn&#xe9;es &#xe0; partir de sites Web et les enregistrer dans un fichier local ou une base de donn&#xe9;es en vue d&#x2019;un traitement ou d&#x2019;un stockage ult&#xe9;rieur. &#xc9;galement appel&#xe9;e capture d&#x2019;&#xe9;cran automatis&#xe9;e, extraction de donn&#xe9;es Web, collecte de donn&#xe9;es Web, etc.</skos:definition>
      <skos:prefLabel xml:lang="nl">Geautomatiseerde data-extractie: Web scrapen</skos:prefLabel>
      <skos:definition xml:lang="nl"></skos:definition>
   </rdf:Description>
   <rdf:Description rdf:about="http://rdf-vocabulary.ddialliance.org/cv/ModeOfCollection/5.0.0/4848ed5">
      <rdf:type rdf:resource="http://www.w3.org/2004/02/skos/core#Concept"/>
      <skos:inScheme rdf:resource="http://rdf-vocabulary.ddialliance.org/cv/ModeOfCollection/5.0.0/"/>
      <skos:notation xml:lang="en">ContentCoding</skos:notation>
      <skos:prefLabel xml:lang="sl">Kodiranje vsebine</skos:prefLabel>
      <skos:definition xml:lang="sl">Kot na&#x10d;in sekundarnega zbiranja podatkov, kodiranje vsebine uporablja kodirne tehnike za preoblikovanje kvalitativnih podatkov (besedilni podatki, video, avdio ali mirujo&#x10d;e slike), ki so bili prvotno ustvarjeni za druge namene, v kvantitativne podatke (izra&#x17e;ene z matricami enot po spremenljivkah) v skladu s vnaprej opredeljenimi kategorizacijskimi shemami. Na primer, kodiranje manifestov politi&#x10d;nih strank, kot npr. &#x161;tudija o volitvah v Evropski parlament 2009 (doi:10.4232/1.10204).</skos:definition>
      <skos:prefLabel xml:lang="sv">Inneh&#xe5;llskodning</skos:prefLabel>
      <skos:definition xml:lang="sv">Som en metod f&#xf6;r sekund&#xe4;r datainsamling inneb&#xe4;r inneh&#xe5;llskodning att kodningstekniker anv&#xe4;nds f&#xf6;r att omvandla kvalitativa data (text, video, ljud eller stillbilder), som ursprungligen skapats f&#xf6;r andra syften, till kvantitativa data (uttryckta i matriser med antal enheter per variabel) enligt f&#xf6;rdefinierade kategoriseringsscheman. Exempel &#xe4;r kodade partiprogramdata som i &quot;European Parliament Election Study 2009, Manifesto Study&quot; (DOI: 10.4232/1.10204).</skos:definition>
      <skos:prefLabel xml:lang="en">Content coding</skos:prefLabel>
      <skos:definition xml:lang="en">As a mode of secondary data collection, content coding applies coding techniques to transform qualitative data (textual, video, audio or still-image) originally produced for other purposes into quantitative data (expressed in unit-by-variable matrices) in accordance with pre-defined categorization schemes. For example, coded party manifesto data like the &quot;European Parliament Election Study 2009, Manifesto Study&quot; (doi:10.4232/1.10204).</skos:definition>
      <skos:prefLabel xml:lang="de">Inhaltsanalyse</skos:prefLabel>
      <skos:definition xml:lang="de">Als eine Form der sekund&#xe4;ren Datenerhebung wendet die Inhaltsanalyse Kodierungstechniken an, um qualitative Daten (Text-, Video-, Audio- oder Standbilddaten), die urspr&#xfc;nglich f&#xfc;r andere Zwecke produziert wurden, mithilfe von vordefinierten Kategorisierungsschemata in quantitative Daten zu transformieren. Zum Beispiel die Kodierung von Parteiprogrammen.</skos:definition>
      <skos:prefLabel xml:lang="no">Innholdskoding</skos:prefLabel>
      <skos:definition xml:lang="no">Som metode for sekund&#xe6;r datainnsamling, innholdskoding omfatter kodeteknikker for &#xe5; omgj&#xf8;re kvalitative data (tekst, video, lyd eller bilde), som opprinnelig var utarbeidet for andre form&#xe5;l, til kvantitative data (uttrykket i en matrise med enheter og variabler) i henhold til bestemte kategoriseringssystem. For eksempel, kodede partimanifesto som i &apos;European Parliament Election Study 2009, Manifesto Study&apos; (doi:10.4232/1.10204).</skos:definition>
      <skos:prefLabel xml:lang="lt">Turinio kodavimas</skos:prefLabel>
      <skos:definition xml:lang="lt">Turinio kodavimas yra toks antrini&#x173; duomen&#x173; rinkimo b&#x16b;das, kuriame kitais tikslais sukurti kokybiniai duomenys (tekstiniai, video, garso ar statini&#x173; vaizd&#x173;) transformuojami &#x12f; kiekybinius duomenis (i&#x161;reik&#x161;tus kintam&#x173;j&#x173;-atvej&#x173; matricomis), koduojant pagal i&#x161;ankstines kategorij&#x173; schemas. Pavyzd&#x17e;iui, partij&#x173; manifest&#x173; kodavimo duomenys tokie kaip &quot;European Parliament Election Study 2009, Manifesto Study&quot; (doi:10.4232/1.10204).</skos:definition>
      <skos:prefLabel xml:lang="it">Codifica del contenuto</skos:prefLabel>
      <skos:definition xml:lang="it">Metodo di raccolta secondaria dei dati, in cui si applicano le tecniche di codifica del contenuto per trasformare dati qualitativi originariamente prodotti per altri scopi (testi, video, audio o immagini) in dati quantitativi (espressi in forma di matrici) secondo schemi di categorizzazione definiti. Ad esempio, codifica dei dati relativi ai manifesti di partito, come il &quot;European Parliament Election Study 2009, Manifesto Study&quot; (doi:10.4232/1.10204)</skos:definition>
      <skos:prefLabel xml:lang="fr">Codage de contenu</skos:prefLabel>
      <skos:definition xml:lang="fr">Le codage de contenu, en tant que mode de collecte secondaire, met en oeuvre des techniques de codage pour transformer des donn&#xe9;es qualitatives (textuel, vid&#xe9;o, audio, ou image fixe), initialement produites &#xe0; d&apos;autres fins, en donn&#xe9;es quantitatives (exprim&#xe9;es dans des matrices unit&#xe9;-par-variable) en accord avec des sch&#xe9;mas de cat&#xe9;gorisations pr&#xe9;d&#xe9;finis. Par exemple, les donn&#xe9;es recod&#xe9;es des programmes des partis politiques comme &quot;European Parliament Election Study 2009, Manifesto Study&quot; (doi:10.4232/1.10204).</skos:definition>
      <skos:prefLabel xml:lang="nl">Content coding</skos:prefLabel>
      <skos:definition xml:lang="nl"></skos:definition>
   </rdf:Description>
   <rdf:Description rdf:about="http://rdf-vocabulary.ddialliance.org/cv/ModeOfCollection/5.0.0/df9aac3">
      <rdf:type rdf:resource="http://www.w3.org/2004/02/skos/core#Concept"/>
      <skos:inScheme rdf:resource="http://rdf-vocabulary.ddialliance.org/cv/ModeOfCollection/5.0.0/"/>
      <skos:notation xml:lang="en">Transcription</skos:notation>
      <skos:prefLabel xml:lang="sl">Prepis</skos:prefLabel>
      <skos:definition xml:lang="sl">Zajemanje podatkov v pisni obliki iz drugega vira ali iz drugega medija, abecede, ali oblika zapisa, kot so znanstvene formule ali glasbene note. Pri transkriptih intervjujev ali opazovanj je priporo&#x10d;ljivo dokumentirati primarni na&#x10d;in zbiranja podatkov z uporabo enega od razgovornih ali opazovalnih pogojev.</skos:definition>
      <skos:prefLabel xml:lang="sv">Transkription</skos:prefLabel>
      <skos:definition xml:lang="sv">Att nedteckna information fr&#xe5;n en annan k&#xe4;lla eller fr&#xe5;n ett annat medium, alfabet eller notationssystem, som till exempel vetenskapliga formler eller noter f&#xf6;r musik. F&#xf6;r transkriberade intervjuer och observationer rekommenderas det att man dokumenterar den prim&#xe4;ra insamlingsmetoden med n&#xe5;gon av termerna f&#xf6;r intervjuer eller observationer.</skos:definition>
      <skos:prefLabel xml:lang="en">Transcription</skos:prefLabel>
      <skos:definition xml:lang="en">Capturing information in writing from a different source, or from a different medium, alphabet, or form of notation, like scientific formulae, or musical notes. For transcribed interviews or observations, it is recommended to document the primary mode of collection, using one of the interview or observation terms.</skos:definition>
      <skos:prefLabel xml:lang="de">Transkription</skos:prefLabel>
      <skos:definition xml:lang="de">Das schriftliche Erfassen von Informationen aus einer anderen Quelle oder aus einem anderen Medium, Alphabet oder einer anderen Notationsform, wie z. B. wissenschaftliche Formeln oder Musiknoten. Bei transkribierten Interviews oder Beobachtungen wird empfohlen, die prim&#xe4;re Methode der Datenerhebung zu dokumentieren, indem einer der Interview- oder Beobachtungsbegriffe verwendet wird.</skos:definition>
      <skos:prefLabel xml:lang="no">Transkripsjon</skos:prefLabel>
      <skos:definition xml:lang="no">Nedtegning av informasjon i skrift fra en annen kilde, eller et annet medium, alfabet, eller fra notasjoner, som vitenskapelige formler, eller musikknoter. For transkriberte intervju eller observasjoner er det anbefalt &#xe5; dokumentere den opprinnelige formen for datainnsamling, ved &#xe5; bruke et av intervju- eller observasjonsbegrepene.</skos:definition>
      <skos:prefLabel xml:lang="lt">Transkripcija </skos:prefLabel>
      <skos:definition xml:lang="lt">Informacijos fiksavimas perra&#x161;ant i&#x161; kitokio tipo &#x161;altini&#x173; ar medij&#x173;, i&#x161; kit&#x173; alfabet&#x173; ar &#x17e;ym&#x117;jimo form&#x173;, pavyzd&#x17e;iui, mokslini&#x173; formuli&#x173; ar muzikos nat&#x173;. Transkribuotus interviu ar steb&#x117;jimus (steb&#x117;jimo u&#x17e;ra&#x161;us) rekomenduojama dokumentuoti pagal pirmin&#x12f; duomen&#x173; rinkimo b&#x16b;d&#x105;, naudojant atitinkamai interviu arba steb&#x117;jimo terminus.</skos:definition>
      <skos:prefLabel xml:lang="it">Trascrizione</skos:prefLabel>
      <skos:definition xml:lang="it">Raccolta di informazioni per iscritto da un&apos;altra fonte, o da un altro mezzo, alfabeto o forma di notazione, come formule scientifiche o note musicali. Per le interviste o le osservazioni trascritte, si consiglia di documentare la modalit&#xe0; di raccolta dei dati utilizzando uno dei termini del vocabolario relativi all&apos;intervista o all&apos;osservazione.</skos:definition>
      <skos:prefLabel xml:lang="fr">Transcription</skos:prefLabel>
      <skos:definition xml:lang="fr">Collecte des informations par &#xe9;crit &#xe0; partir d&apos;une source diff&#xe9;rente, ou &#xe0; partir d&apos;un support diff&#xe9;rent, d&apos;un alphabet, ou d&apos;une forme de notation, comme des formules scientifiques, ou des notes de musique. Pour des retranscriptions d&apos;entretiens ou d&apos;observations, il est recommand&#xe9; de documenter le mode de collecte initial, en utilisant l&apos;un des termes d&#xe9;di&#xe9;s &#xe0; l&apos;entretien ou &#xe0; l&apos;observation.</skos:definition>
      <skos:prefLabel xml:lang="nl">Transcriptie</skos:prefLabel>
      <skos:definition xml:lang="nl"></skos:definition>
   </rdf:Description>
   <rdf:Description rdf:about="http://rdf-vocabulary.ddialliance.org/cv/ModeOfCollection/5.0.0/6decc77">
      <rdf:type rdf:resource="http://www.w3.org/2004/02/skos/core#Concept"/>
      <skos:inScheme rdf:resource="http://rdf-vocabulary.ddialliance.org/cv/ModeOfCollection/5.0.0/"/>
      <skos:notation xml:lang="en">CompilationSynthesis</skos:notation>
      <skos:prefLabel xml:lang="sl">Kompilacija/sinteza</skos:prefLabel>
      <skos:definition xml:lang="sl">Zbiranje in sestavljanje podatkov iz ve&#x10d;, pogosto heterogenih virov, ki imajo eno ali ve&#x10d; skupnih referen&#x10d;nih to&#x10d;k in kjer je bil vsaj eden od virov prvotno produciran v druge namene. Podatki so vklju&#x10d;eni v novo entiteto. Na primer z zagotavljanjem podatkov o &#x161;tevilu univerz v zadnjih 150 letih z uporabo razli&#x10d;nih razpolo&#x17e;ljivih virov (npr. finan&#x10d;ni dokumenti, uradne statistike, univerzitetni registri), kombiniranjem anketnih podatkov z informacijami o geografskih obmo&#x10d;jih iz uradnih statisti&#x10d;nih podatkov (npr. gostota prebivalstva, &#x161;tevilo zdravnikov na prebivalca itd.) ali z uporabo RSS za zbiranje objav bloga ali tvitov itd.</skos:definition>
      <skos:prefLabel xml:lang="sv">Kompilering/Syntes</skos:prefLabel>
      <skos:definition xml:lang="sv">Att samla in och sammanst&#xe4;lla data fr&#xe5;n flera, ofta heterogena, k&#xe4;llor som har en eller flera gemensamma referenspunkter, och d&#xe4;r minst en av k&#xe4;llorna ursprungligen producerades f&#xf6;r andra syften. Datamaterialet har inf&#xf6;rlivats i ett nytt material. Exempel: data om antalet universitet under de senaste 150 &#xe5;ren som tas fram med hj&#xe4;lp av ett antal olika k&#xe4;llor (t.ex. r&#xe4;kenskaper, offentlig statistik och universitetsrullor); en kombination av surveydata med information om geografiska omr&#xe5;den fr&#xe5;n offentlig statistik (t.ex. befolkningst&#xe4;thet, l&#xe4;kare per capita osv); eller bloggposter, tweetar, m.m. som samlats in med hj&#xe4;lp av RSS.</skos:definition>
      <skos:prefLabel xml:lang="en">Compilation/Synthesis</skos:prefLabel>
      <skos:definition xml:lang="en">Collecting and assembling data from multiple, often heterogeneous sources that have one or more reference points in common, and at least one of the sources was originally produced for other purposes. The data are incorporated in a new entity. For example, providing data on the number of universities in the last 150 years using a variety of available sources (e.g. finance documents, official statistics, university registers), combining survey data with information about geographical areas from official statistics (e.g. population density, doctors per capita, etc.), or with social media data, etc.</skos:definition>
      <skos:prefLabel xml:lang="de">Kompilation/Synthese</skos:prefLabel>
      <skos:definition xml:lang="de">Sammeln und Zusammenstellen von Daten aus mehreren, oft heterogenen Quellen, die einen oder mehrere Bezugspunkte gemeinsam haben, wobei mindestens eine der Quellen urspr&#xfc;nglich f&#xfc;r andere Zwecke erstellt wurde. Die Daten werden in eine neue Einheit integriert. Zum Beispiel die Bereitstellung von Daten &#xfc;ber die Anzahl der Universit&#xe4;ten in den letzten 150 Jahren unter Verwendung einer Vielzahl verf&#xfc;gbarer Quellen (z. B. Finanzdokumente, amtliche Statistiken, Universit&#xe4;tsregister), die Kombination von Umfragedaten mit Informationen &#xfc;ber geografische Gebiete aus amtlichen Statistiken (z. B. Bev&#xf6;lkerungsdichte, &#xc4;rzte pro Kopf usw.) oder mit Daten aus sozialen Medien usw.</skos:definition>
      <skos:prefLabel xml:lang="no">Kompilering/Syntese</skos:prefLabel>
      <skos:definition xml:lang="no">Innsamling og sammensetting av data fra flere, ofte heterogene, kilder som har en eller flere felles referansepunkter, og minst &#xe9;n av kildene var opprinnelig utarbeidet for andre form&#xe5;l. Dataene blir integrert i en ny enhet. For eksempel utarbeide data om antallet universitet de siste 150 &#xe5;rene ved &#xe5; bruke flere tilgjengelige kilder (e.g. finansdokumenter, offisiell statistikk, universitetsregistre), kombinere sp&#xf8;rreunders&#xf8;kelsesdata med informasjon om geografiske omr&#xe5;der fra offisiell statistikk (e.g. befolkningstetthet, antall leger per innbygger, etc.), eller bruke RSS for &#xe5; samle blogginnlegg eller tweets etc.</skos:definition>
      <skos:prefLabel xml:lang="lt">Kompiliacija ar sintez&#x117;</skos:prefLabel>
      <skos:definition xml:lang="lt">Duomen&#x173; rinkimas ir integravimas i&#x161; keli&#x173; skirting&#x173; &#x161;altini&#x173;, kuriuos jungia viena ar kelios bendros charakteristikos, o bent vienas i&#x161; &#x161;altini&#x173; buvo kurtas kitiems tikslams. Duomenys integruojami naujame objekte. Pavyzd&#x17e;iui, teikiant duomenis apie universitet&#x173; skai&#x10d;i&#x173; u&#x17e; pra&#x117;jusius 150 met&#x173;, naudojami &#x12f;vair&#x16b;s prieinami &#x161;altiniai (pavyzd&#x17e;iui, finansiniai dokumentai, oficiali statistika, universitet&#x173; registrai); apklaus&#x173; duomenys jungiami su oficialia statistine informacijos apie geografines vietoves (pavyzd&#x17e;iui, gyventoj&#x173; tankis, mokslo daktar&#x173; skai&#x10d;ius vienam gyventojui ir kt.); arba su socialini&#x173; medij&#x173; duomenimis ir kt.</skos:definition>
      <skos:prefLabel xml:lang="it">Raccolta/sintesi</skos:prefLabel>
      <skos:definition xml:lang="it">Raccolta e assemblaggio di dati da pi&#xf9; fonti, spesso eterogenee, che hanno uno o pi&#xf9; punti di riferimento in comune, e dove almeno una delle fonti &#xe8; stata originariamente prodotta per altri scopi. I dati sono incorporati in una nuova base di dati. Ad esempio, la raccolta di dati sul numero di universit&#xe0; negli ultimi 150 anni attraverso diverse fonti disponibili (ad esempio documenti finanziari, statistiche ufficiali, registri universitari), successivamente combinati con le statistiche ufficiali relative alle aree geografiche (ad es. densit&#xe0; di popolazione, medici pro-capite, ecc.) o con dati provenienti dai social media, ecc.</skos:definition>
      <skos:prefLabel xml:lang="fr">Compilation / synth&#xe8;se</skos:prefLabel>
      <skos:definition xml:lang="fr">Collecte et assemblage de donn&#xe9;es depuis de multiples sources souvent h&#xe9;t&#xe9;rog&#xe8;nes qui ont un ou plusieurs points de r&#xe9;f&#xe9;rence en commun, et dont au moins une des sources a &#xe9;t&#xe9; produite &#xe0; l&apos;origine &#xe0; d&apos;autres fins. Les donn&#xe9;es sont incorpor&#xe9;es dans une nouvelle entit&#xe9;. Par exemple, fournir des donn&#xe9;es sur le nombre d&apos;universit&#xe9;s au cours des 150 derni&#xe8;res ann&#xe9;es en utilisant une vari&#xe9;t&#xe9; de sources disponibles (e. g. documents financiers, statistiques officielles, registres universitaires), en combinant les donn&#xe9;es d&apos;enqu&#xea;te avec des informations sur les zones g&#xe9;ographiques provenant des statistiques officielles (e. g. la densit&#xe9; de population, nombre de m&#xe9;decins par habitants, etc.), ou les donn&#xe9;es des r&#xe9;seaux sociaux, etc.</skos:definition>
      <skos:prefLabel xml:lang="nl">Compilatie/Synthese</skos:prefLabel>
      <skos:definition xml:lang="nl"></skos:definition>
   </rdf:Description>
   <rdf:Description rdf:about="http://rdf-vocabulary.ddialliance.org/cv/ModeOfCollection/5.0.0/2906121">
      <rdf:type rdf:resource="http://www.w3.org/2004/02/skos/core#Concept"/>
      <skos:inScheme rdf:resource="http://rdf-vocabulary.ddialliance.org/cv/ModeOfCollection/5.0.0/"/>
      <skos:notation xml:lang="en">Summary</skos:notation>
      <skos:prefLabel xml:lang="sl">Povzetek</skos:prefLabel>
      <skos:definition xml:lang="sl">Predstavitev informacij v zgo&#x161;&#x10d;eni obliki z reduciranjem na glavne to&#x10d;ke. Na primer, povzetki intervjujev ali poro&#x10d;il, ki so objavljeni in uporabljeni kot podatki in ne kot celoviti intervjuji ali poro&#x10d;ila.</skos:definition>
      <skos:prefLabel xml:lang="sv">Sammanfattning</skos:prefLabel>
      <skos:definition xml:lang="sv">Presentation av information i sammandrag, som reducerats till sitt viktigaste inneh&#xe5;ll. Exempel: Abstrakt fr&#xe5;n intervjuer eller rapporter publiceras och anv&#xe4;nds som data ist&#xe4;llet f&#xf6;r de fullst&#xe4;ndiga intervjuerna eller rapporterna.</skos:definition>
      <skos:prefLabel xml:lang="en">Summary</skos:prefLabel>
      <skos:definition xml:lang="en">Presentation of information in a condensed form, by reducing it to its main points. For example, abstracts of interviews or reports that are published and used as data rather than the full-length interviews or reports.</skos:definition>
      <skos:prefLabel xml:lang="de">Zusammenfassung</skos:prefLabel>
      <skos:definition xml:lang="de">Darstellung von Informationen in komprimierter Form, indem sie auf die wesentlichen Punkte reduziert werden. Zum Beispiel Zusammenfassungen von Interviews oder Berichten, die ver&#xf6;ffentlicht und als Daten verwendet werden, anstatt die Interviews oder Berichte in deren voller L&#xe4;nge.</skos:definition>
      <skos:prefLabel xml:lang="no">Sammendrag</skos:prefLabel>
      <skos:definition xml:lang="no">Presentasjon av informasjon i en konsentrert form, ved &#xe5; redusere den til dens hovedpoeng. For eksempel, sammendrag av intervjuer eller rapporter som er publisert og brukt som data til fordel for de fulle intervjuene eller rapportene.</skos:definition>
      <skos:prefLabel xml:lang="lt">Santrauka</skos:prefLabel>
      <skos:definition xml:lang="lt">Informacijos glaustas i&#x161;d&#x117;stymas, j&#x105; sutrumpinant iki pagrindin&#x117;s esm&#x117;s. Pavyzd&#x17e;iui, interviu ar ataskaitos santrauka, kuri publikuojama ir naudojama kaip duomenys, vietoje pilnos trukm&#x117;s interviu ar ataskaitos.</skos:definition>
      <skos:prefLabel xml:lang="it">Sintesi</skos:prefLabel>
      <skos:definition xml:lang="it">Presentazione di informazioni in forma sintetica, riducendole ai punti principali. Ad esempio, abstract di interviste o report che vengono pubblicati e utilizzati come dati, al posto delle interviste o dei report completi.</skos:definition>
      <skos:prefLabel xml:lang="fr">R&#xe9;sum&#xe9;</skos:prefLabel>
      <skos:definition xml:lang="fr">Pr&#xe9;sentation d&apos;informations dans une forme condens&#xe9;e, en les r&#xe9;duisant &#xe0; leurs points principaux. Par exemple, des r&#xe9;sum&#xe9;s d&apos;entretiens ou de rapports qui sont publi&#xe9;s et utilis&#xe9;s comme des donn&#xe9;es plut&#xf4;t que des entretiens ou des rapports complets.</skos:definition>
      <skos:prefLabel xml:lang="nl">Samenvatting</skos:prefLabel>
      <skos:definition xml:lang="nl"></skos:definition>
   </rdf:Description>
   <rdf:Description rdf:about="http://rdf-vocabulary.ddialliance.org/cv/ModeOfCollection/5.0.0/d9ceca6">
      <rdf:type rdf:resource="http://www.w3.org/2004/02/skos/core#Concept"/>
      <skos:inScheme rdf:resource="http://rdf-vocabulary.ddialliance.org/cv/ModeOfCollection/5.0.0/"/>
      <skos:notation xml:lang="en">Aggregation</skos:notation>
      <skos:prefLabel xml:lang="sl">Agregacija</skos:prefLabel>
      <skos:definition xml:lang="sl">Statistike, ki se nana&#x161;ajo na &#x161;ir&#x161;e razrede, skupine ali kategorije. Podatki so predstavljeni kot povpre&#x10d;ja, vsote ali druge izpeljave, na podlagi katerih ni ve&#x10d; mo&#x17e;no razlikovati med zna&#x10d;ilnostmi posameznikov znotraj teh razredov, skupin ali kategorij. Na primer, &#x161;tevilo in starostna skupina brezposelnih v posebnih geografskih regijah ali nacionalne statistike o pojavu poosameznih kaznivih dejanj, ki so bila prvotno izpeljana iz statisti&#x10d;nih podatkov posameznih policijskih okro&#x17e;ij.</skos:definition>
      <skos:prefLabel xml:lang="sv">Aggregation</skos:prefLabel>
      <skos:definition xml:lang="sv">Statistik som r&#xf6;r breda klasser, grupper eller kategorier. Datamaterialet best&#xe5;r av genomsnitt, totalsummor eller andra v&#xe4;rden som har h&#xe4;rletts fr&#xe5;n data p&#xe5; individniv&#xe5;, och det g&#xe5;r inte l&#xe4;ngre att utl&#xe4;sa individernas egenskaper inom dessa klasser, grupper eller kategorier. Exempel: antal och &#xe5;lderskategorier f&#xf6;r arbetsl&#xf6;sa inom s&#xe4;rskilda geografiska omr&#xe5;den, eller statistik p&#xe5; nationsniv&#xe5; &#xf6;ver f&#xf6;rekomsten av s&#xe4;rskilda brott som ursprungligen h&#xe4;rletts fr&#xe5;n statistik fr&#xe5;n enskilda polisdistrikt.</skos:definition>
      <skos:prefLabel xml:lang="en">Aggregation</skos:prefLabel>
      <skos:definition xml:lang="en">Statistics that relate to broad classes, groups, or categories. The data are averaged, totaled, or otherwise derived from individual-level data, and it is no longer possible to distinguish the characteristics of individuals within those classes, groups, or categories. For example, the number and age group of the unemployed in specific geographic regions, or national level statistics on the occurrence of specific offences, originally derived from the statistics of individual police districts.</skos:definition>
      <skos:prefLabel xml:lang="de">Aggregation</skos:prefLabel>
      <skos:definition xml:lang="de">Statistiken, die sich auf breite Klassen, Gruppen oder Kategorien beziehen. Die Daten werden gemittelt, summiert oder auf andere Weise aus Daten auf individueller Ebene abgeleitet, und es ist nicht mehr m&#xf6;glich, die Merkmale von Einzelpersonen innerhalb dieser Klassen, Gruppen oder Kategorien zu unterscheiden. Zum Beispiel die Anzahl und Altersgruppe der Arbeitslosen in bestimmten geografischen Regionen oder Statistiken auf nationaler Ebene &#xfc;ber das Auftreten bestimmter Straftaten, die urspr&#xfc;nglich aus den Statistiken einzelner Polizeibezirke abgeleitet wurden.</skos:definition>
      <skos:prefLabel xml:lang="no">Aggregering</skos:prefLabel>
      <skos:definition xml:lang="no">Statistikk som relateres til store klasser, grupper eller kategorier. Dataene er tatt gjennomsnittet av, summert, eller p&#xe5; andre m&#xe5;ter utvunnet av data p&#xe5; individniv&#xe5;, og det er ikke lengre mulig &#xe5; skille mellom egenskapene til individer innad i disse klassene, gruppene eller kategoriene. For eksempel, antallet og aldersgruppen til de arbeidsledige i bestemte regioner, eller statistikk p&#xe5; nasjonalt niv&#xe5; om forekomsten av bestemte overtredelser, opprinnelig utarbeidet fra statistikk om individuelle politidistrikt.</skos:definition>
      <skos:prefLabel xml:lang="lt">Agregavimas</skos:prefLabel>
      <skos:definition xml:lang="lt">Statistika apie didesnes klases, grupes ar kategorijas. Skai&#x10d;iuojami duomen&#x173; vidurkiai, duomenys susumuojami arba kitaip i&#x161;vedami i&#x161; individualaus lygmens duomen&#x173; ir neb&#x117;ra &#x12f;manoma atskirti asmen&#x173; charakteristik&#x173; tose klas&#x117;se, grup&#x117;se ar kategorijose. Pavyzd&#x17e;iui, bedarbi&#x173; skai&#x10d;ius am&#x17e;iaus grup&#x117;se konkre&#x10d;iuose geografiniuose regionuose, arba nacionalinio lygmens statistiniai duomenys apie tam tikrus nusikaltimus, i&#x161;vesti i&#x161; atskir&#x173; rajon&#x173; policijos statistin&#x117;s informacijos.</skos:definition>
      <skos:prefLabel xml:lang="it">Aggregazione</skos:prefLabel>
      <skos:definition xml:lang="it">Statistiche relative a classi, gruppi o categorie. I dati rappresentano il valore medio, la somma o altre derivazioni dei dati raccolti a livello individuale, che non consentono pi&#xf9; di distinguere le caratteristiche degli individui all&apos;interno di tali classi, gruppi o categorie. Ad esempio, il numero e la fascia di et&#xe0; dei disoccupati in specifiche regioni geografiche, o le statistiche a livello nazionale sul verificarsi di reati specifici, originariamente desunti dalle statistiche dei singoli distretti di polizia.</skos:definition>
      <skos:prefLabel xml:lang="fr">Agr&#xe9;gation</skos:prefLabel>
      <skos:definition xml:lang="fr">Statistiques qui concernent des classes, des groupes, ou des cat&#xe9;gories. Les donn&#xe9;es sont recalcul&#xe9;es en moyenne, additionn&#xe9;es, ou proposent un autre d&#xe9;riv&#xe9; des donn&#xe9;es individuelles, et il n&apos;est plus possible de distinguer les caract&#xe9;ristiques des individus au sein de ces classes, groupes, ou cat&#xe9;gories. Par exemple, le nombre et le groupe d&apos;&#xe2;ge des ch&#xf4;meurs dans des r&#xe9;gions g&#xe9;ographiques sp&#xe9;cifiques, ou des statistiques nationales sur l&apos;apparition de certaines infractions, initialement tir&#xe9;es des statistiques de diff&#xe9;rents districts de police.</skos:definition>
      <skos:prefLabel xml:lang="nl">Aggregatie</skos:prefLabel>
      <skos:definition xml:lang="nl"></skos:definition>
   </rdf:Description>
   <rdf:Description rdf:about="http://rdf-vocabulary.ddialliance.org/cv/ModeOfCollection/5.0.0/4f502b5">
      <rdf:type rdf:resource="http://www.w3.org/2004/02/skos/core#Concept"/>
      <skos:inScheme rdf:resource="http://rdf-vocabulary.ddialliance.org/cv/ModeOfCollection/5.0.0/"/>
      <skos:notation xml:lang="en">Simulation</skos:notation>
      <skos:prefLabel xml:lang="sl">Simulacija</skos:prefLabel>
      <skos:definition xml:lang="sl">Modeliranje ali opona&#x161;ajo&#x10d;e predstavljanje procesov, dogodkov ali sistemov v realnem svetu, pogosto z uporabo ra&#x10d;unalni&#x161;kih programov. Na primer program, ki modelira odziv potro&#x161;nje gospodinjstev na posredne dav&#x10d;ne spremembe; ali podatkovje o hipoteti&#x10d;nih pacientih in njihovi izpostavljenosti zdravilu, pogojih v ozadju in znanih ne&#x17e;elenih doogodkih.</skos:definition>
      <skos:prefLabel xml:lang="sv">Simulering</skos:prefLabel>
      <skos:definition xml:lang="sv">Modellering eller imiterande representation av processer, h&#xe4;ndelser eller system i den verkliga v&#xe4;rlden, ofta skapade med datorprogram. Exempel: ett program som modellerar hur hush&#xe5;llens konsumtion svarar p&#xe5; f&#xf6;r&#xe4;ndringar i indirekta skatter; eller ett dataset &#xf6;ver hypotetiska patienter och deras droganv&#xe4;ndning, bakgrundsf&#xf6;rh&#xe5;llanden och k&#xe4;nda negativa h&#xe4;ndelser.</skos:definition>
      <skos:prefLabel xml:lang="en">Simulation</skos:prefLabel>
      <skos:definition xml:lang="en">Modeling or imitative representation of real-world processes, events, or systems, often using computer programs. For example, a program modeling household consumption responses to indirect tax changes; or a dataset on hypothetical patients and their drug exposure, background conditions, and known adverse events.</skos:definition>
      <skos:prefLabel xml:lang="de">Simulation</skos:prefLabel>
      <skos:definition xml:lang="de">Modellierung oder nachahmende Darstellung von realen Prozessen, Ereignissen oder Systemen, oft unter Verwendung von Computerprogrammen. Zum Beispiel ein Programm, das die Reaktionen des Haushaltskonsums auf Ver&#xe4;nderung indirekter Steuern modelliert; oder ein Datensatz &#xfc;ber hypothetische Patienten und deren Medikamentenbelastung, Hintergrundbedingungen und bekannte unerw&#xfc;nschte Ereignisse.</skos:definition>
      <skos:prefLabel xml:lang="no">Simulering</skos:prefLabel>
      <skos:definition xml:lang="no">Modellering eller etterlignende representasjon av virkelige prosesser, hendelser eller systemer, ofte ved bruk av dataprogrammer. For eksempel et program som modellerer hvordan en husholdnings forbruk svarer p&#xe5; endringer i indirekte skatter; eller et datasett om hypotetiske pasienter og deres eksponering for narkotiske stoffer, bakgrunnsforhold, og kjente ugunstige hendelser.</skos:definition>
      <skos:prefLabel xml:lang="lt">Simuliavimas</skos:prefLabel>
      <skos:definition xml:lang="lt">Realaus pasaulio proces&#x173;, &#x12f;vyki&#x173; ar sistem&#x173; modeliavimas arba imitavimas, da&#x17e;niausiai naudojant kompiuterines programas. Pavyzd&#x17e;iui, programa modeliuojanti netiesiogini&#x173; mokes&#x10d;i&#x173; pakeitim&#x173; poveik&#x12f; nam&#x173; &#x16b;ki&#x173; vartojimo &#x12f;pro&#x10d;iams; arba duomen&#x173; rinkinys apie hipotetinius pacientus ir j&#x173; vaist&#x173; vartojim&#x105;, gyvenimo s&#x105;lygas ir &#x17e;inomas &#x161;alutines reakcijas.</skos:definition>
      <skos:prefLabel xml:lang="it">Simulazione</skos:prefLabel>
      <skos:definition xml:lang="it">Modellazione o rappresentazione finalizzata alla riproduzione di processi, eventi o sistemi reali, spesso utilizzando programmi per computer. Ad esempio, un programma che modella le risposte dei consumi delle famiglie alle variazioni delle imposte indirette; o un dataset relativo a pazienti ipotetici e alla loro esposizione a farmaci, alle condizioni di fondo e ad eventi avversi conosciuti.</skos:definition>
      <skos:prefLabel xml:lang="fr">Simulation</skos:prefLabel>
      <skos:definition xml:lang="fr">Mod&#xe9;lisation ou repr&#xe9;sentation imitative de processus, d&#x2019;&#xe9;v&#xe9;nements ou de syst&#xe8;mes r&#xe9;els, utilisant souvent des programmes informatiques. Par exemple, un programme mod&#xe9;lisant des r&#xe9;actions de la consommation des m&#xe9;nages aux changement des imp&#xf4;ts indirects ; ou un jeu de donn&#xe9;es sur des patients hypoth&#xe9;tiques et leur exposition aux m&#xe9;dicaments, aux conditions environnementales, et aux effets ind&#xe9;sirables connus.</skos:definition>
      <skos:prefLabel xml:lang="nl">Simulatie</skos:prefLabel>
      <skos:definition xml:lang="nl"></skos:definition>
   </rdf:Description>
   <rdf:Description rdf:about="http://rdf-vocabulary.ddialliance.org/cv/ModeOfCollection/5.0.0/38ceaa4">
      <rdf:type rdf:resource="http://www.w3.org/2004/02/skos/core#Concept"/>
      <skos:inScheme rdf:resource="http://rdf-vocabulary.ddialliance.org/cv/ModeOfCollection/5.0.0/"/>
      <skos:notation xml:lang="en">MeasurementsAndTests</skos:notation>
      <skos:prefLabel xml:lang="sl">Merjenje in testiranje</skos:prefLabel>
      <skos:definition xml:lang="sl">Ocenjevanje specifi&#x10d;nih lastnosti (ali zna&#x10d;ilnosti) bitij, stvari, pojavov (in/ali procesov), z uporabo vnaprej dolo&#x10d;enih standardov in/ali specializiranih instrumentov ali tehnik.</skos:definition>
      <skos:prefLabel xml:lang="sv">M&#xe4;tningar och tester</skos:prefLabel>
      <skos:definition xml:lang="sv">Bed&#xf6;mning av varelsers, f&#xf6;rem&#xe5;ls, fenomens (och/eller processers) s&#xe4;rskilda egenskaper (eller karakteristiska) genom att till&#xe4;mpa f&#xf6;rutbest&#xe4;mda standarder och/eller specialiserade instrument eller tekniker.</skos:definition>
      <skos:prefLabel xml:lang="en">Measurements and tests</skos:prefLabel>
      <skos:definition xml:lang="en">Assessing specific properties (or characteristics) of beings, things, phenomena, (and/ or processes) by applying pre-established standards and/or specialized instruments or techniques.</skos:definition>
      <skos:prefLabel xml:lang="de">Messungen und Tests</skos:prefLabel>
      <skos:definition xml:lang="de">Beurteilung spezifischer Eigenschaften (oder Merkmale) von Wesen, Dingen, Ph&#xe4;nomenen (und/oder Prozessen) durch Anwendung vorher festgelegter Standards und/oder spezieller Instrumente oder Techniken.</skos:definition>
      <skos:prefLabel xml:lang="no">M&#xe5;linger og tester</skos:prefLabel>
      <skos:definition xml:lang="no">Vurdering av bestemte egenskaper (eller karakteristika) ved vesener, ting, fenomen (og/eller prosesser) ved &#xe5; anvende forutbestemte standarder og/eller spesialiserte instrumenter eller teknikker.</skos:definition>
      <skos:prefLabel xml:lang="lt">Matavimai ir testai</skos:prefLabel>
      <skos:definition xml:lang="lt">Organizm&#x173;, daikt&#x173;, rei&#x161;kini&#x173; (ir (arba) proces&#x173;) tam tikr&#x173; savybi&#x173; (ar charakteristik&#x173;) vertinimas, naudojant visuotinai priimtus standartus ir (arba) specializuotus instrumentus ar technikas.</skos:definition>
      <skos:prefLabel xml:lang="it">Misurazioni e test</skos:prefLabel>
      <skos:definition xml:lang="it">Valutazione di specifiche propriet&#xe0; (o caratteristiche) di esseri viventi, cose, fenomeni (e/o processi) applicando standard prestabiliti e/o strumenti o tecniche specializzate.</skos:definition>
      <skos:prefLabel xml:lang="fr">Mesures et tests</skos:prefLabel>
      <skos:definition xml:lang="fr">&#xc9;valuer des propri&#xe9;t&#xe9;s sp&#xe9;cifiques (ou caract&#xe9;ristiques) d&apos;&#xea;tres, de choses, de ph&#xe9;nom&#xe8;nes, (et / ou processus) en appliquant des standards pr&#xe9;&#xe9;tablis et / ou des instruments ou des techniques sp&#xe9;cialis&#xe9;s.</skos:definition>
      <skos:prefLabel xml:lang="nl">Metingen en tests</skos:prefLabel>
      <skos:definition xml:lang="nl"></skos:definition>
      <skos:narrower rdf:resource="http://rdf-vocabulary.ddialliance.org/cv/ModeOfCollection/5.0.0/47bfda9"/>
      <skos:narrower rdf:resource="http://rdf-vocabulary.ddialliance.org/cv/ModeOfCollection/5.0.0/4b9776b"/>
      <skos:narrower rdf:resource="http://rdf-vocabulary.ddialliance.org/cv/ModeOfCollection/5.0.0/c2a25a6"/>
      <skos:narrower rdf:resource="http://rdf-vocabulary.ddialliance.org/cv/ModeOfCollection/5.0.0/27daf03"/>
   </rdf:Description>
   <rdf:Description rdf:about="http://rdf-vocabulary.ddialliance.org/cv/ModeOfCollection/5.0.0/47bfda9">
      <rdf:type rdf:resource="http://www.w3.org/2004/02/skos/core#Concept"/>
      <skos:inScheme rdf:resource="http://rdf-vocabulary.ddialliance.org/cv/ModeOfCollection/5.0.0/"/>
      <skos:notation xml:lang="en">MeasurementsAndTests.Cognitive</skos:notation>
      <skos:prefLabel xml:lang="sl">Meritve in testiranja kognitivnih sposobnosti</skos:prefLabel>
      <skos:definition xml:lang="sl">Standardizirane naloge ali ocenjevanja, zasnovana za ocenjevanje du&#x161;evnih procesov, kot so spomin, pozornost, zaznavanje, sklepanje, re&#x161;evanje problemov in razumevanje jezika. Namen teh testov je objektivno meriti kognitivne sposobnosti in se pogosto uporabljajo v raziskavah o staranju, delovanju mo&#x17e;ganov in v klini&#x10d;ni diagnostiki. Primeri vklju&#x10d;ujejo teste inteligentnosti, kot sta Wechslerjeva lestvica inteligentnosti za odrasle (WAIS) in Ravenove progresivne matrice.</skos:definition>
      <skos:prefLabel xml:lang="sv">Kognitiva m&#xe4;tningar och tester</skos:prefLabel>
      <skos:definition xml:lang="sv">Standardiserade uppgifter eller bed&#xf6;mningar som &#xe4;r utformade f&#xf6;r att utv&#xe4;rdera mentala processer som minne, uppm&#xe4;rksamhet, perception, logiskt t&#xe4;nkande, probleml&#xf6;sning och spr&#xe5;kf&#xf6;rst&#xe5;else. Testerna syftar till att ge objektiva m&#xe5;tt p&#xe5; kognitiva f&#xf6;rm&#xe5;gor och anv&#xe4;nds ofta inom forskning om &#xe5;ldrande, hj&#xe4;rnfunktion och klinisk diagnostik. N&#xe5;gra exempel &#xe4;r intelligenstester som Wechsler Adult Intelligence Scale (WAIS) och Raven&apos;s Progressive Matrices (eller Ravens Progressiva Matriser); tester som utv&#xe4;rderar uppm&#xe4;rksamhet, koncentration och arbetsminne, till exempel Montreal Cognitive Assessment (MoCA); samt bland annat reaktionstidstester och tester av verbalt fl&#xf6;de.</skos:definition>
      <skos:prefLabel xml:lang="en">Cognitive measurements and tests</skos:prefLabel>
      <skos:definition xml:lang="en">Standardized tasks or assessments designed to evaluate mental processes such as memory, attention, perception, reasoning, problem solving, and language comprehension. These tests aim to objectively measure cognitive abilities and are commonly used in research on aging, brain function, and clinical diagnostics. Examples include intelligence tests such as the Wechsler Adult Intelligence Scale (WAIS) and Raven&apos;s Progressive Matrices; tasks evaluating attention, concentration, and working memory such as the Montreal Cognitive Assessment (MoCA); as well as reaction time experiments, verbal fluency tests, and others.</skos:definition>
      <skos:prefLabel xml:lang="de">Messungen und Tests: Kognitive Tests</skos:prefLabel>
      <skos:definition xml:lang="de">Standardisierte Aufgaben oder Tests, um geistige Prozesse zu beurteilen, wie Ged&#xe4;chtnis, Aufmerksamkeit, Wahrnehmung, logisches Denken, Probleml&#xf6;sung und Sprachverst&#xe4;ndnis. Diese Tests dienen der objektiven Messung kognitiver F&#xe4;higkeiten und werden h&#xe4;ufig in der Forschung zu Alterung, Gehirnfunktion und klinischer Diagnostik eingesetzt. Beispiele hierf&#xfc;r sind Intelligenztests wie die Wechsler Adult Intelligence Scale (WAIS) oder Ravens Progressive Matrizen, Aufgaben zur Bewertung von Aufmerksamkeit, Konzentration und Arbeitsged&#xe4;chtnis wie der Montreal Cognitive Assessment (MoCA) sowie Reaktionszeit-Experimente, Tests zur verbalen Fl&#xfc;ssigkeit und andere.</skos:definition>
      <skos:prefLabel xml:lang="no">Kognitive m&#xe5;linger og tester</skos:prefLabel>
      <skos:definition xml:lang="no">Standardiserte oppgaver eller tester utviklet for &#xe5; evaluare mentale prosesser som hukommelse, oppmerksomhet, persepsjon, resonnering, probleml&#xf8;sning og spr&#xe5;kforst&#xe5;else. Disse testene har som m&#xe5;l &#xe5; m&#xe5;le kognitive evner p&#xe5; en objektiv m&#xe5;te og brukes ofte i forskning p&#xe5; aldring, hjernefunksjon og klinisk diagnostikk. Eksempler inkluderer intelligenstester som Wechsler Adult Intelligence Scale (WAIS) og Raven&apos;s Progressive Matrices; oppgaver som evaluerer oppmerksomhet, konsentrasjon og arbeidsminne slik som Montreal Cognitive Assessment (MoCA); samt reaksjonstidseksperimenter, verbal flyt-tester og andre.</skos:definition>
      <skos:prefLabel xml:lang="lt">Kognityvinis vertinimas ir testai</skos:prefLabel>
      <skos:definition xml:lang="lt">Standartizuotos u&#x17e;duotys ar testai, skirti &#x12f;vertinti kognityvinius procesus, tokius kaip atmintis, d&#x117;mesys, suvokimas, m&#x105;stymas, problem&#x173; sprendimas ir kalbos supratimas. &#x160;iais testais siekiama objektyviai &#x12f;vertinti kognityvinius geb&#x117;jimus. Jie da&#x17e;nai naudojami sen&#x117;jimo, smegen&#x173; funkcij&#x173; tyrimuose bei klinikin&#x117;je diagnostikoje. Pavyzd&#x17e;iai apima intelekto testus, tokius kaip Wechslerio suaugusi&#x173;j&#x173; intelekto skal&#x117; (WAIS) ir Raveno progresyvi&#x173;j&#x173; matric&#x173; testas; d&#x117;mesio, koncentracijos ir darbin&#x117;s atminties vertinimo u&#x17e;duotis, pvz., Monrealio kognityvin&#x12f; test&#x105; (MoCA); taip pat reakcijos laiko eksperimentus, &#x17e;odinio sklandumo testus ir kitus vertinimus.</skos:definition>
      <skos:prefLabel xml:lang="it">Misurazioni e test cognitivi</skos:prefLabel>
      <skos:definition xml:lang="it">Compiti o valutazioni standardizzati progettati per valutare i processi mentali quali la memoria, l&apos;attenzione, la percezione, il ragionamento, la risoluzione dei problemi e la comprensione del linguaggio. Questi test mirano a misurare oggettivamente le capacit&#xe0; cognitive e sono comunemente utilizzati nella ricerca sull&apos;invecchiamento, sulle funzioni cerebrali e nella diagnostica clinica. Sono inclusi, ad esempio, i test di intelligenza come la Wechsler Adult Intelligence Scale (WAIS) e le Matrici Progressive di Raven; i compiti che valutano l&apos;attenzione, la concentrazione e la memoria di lavoro come il Montreal Cognitive Assessment (MoCA); esperimenti sui tempi di reazione, test di fluenza verbale e altri simili.</skos:definition>
      <skos:prefLabel xml:lang="fr">Mesures et tests cognitifs</skos:prefLabel>
      <skos:definition xml:lang="fr">Des t&#xe2;ches ou &#xe9;valuations standardis&#xe9;es con&#xe7;ues pour &#xe9;valuer des processus mentaux tels que la m&#xe9;moire, l&#x2019;attention, la perception, le raisonnement, la r&#xe9;solution de probl&#xe8;mes et la compr&#xe9;hension du langage. Ces tests visent &#xe0; mesurer de mani&#xe8;re objective les capacit&#xe9;s cognitives et sont couramment utilis&#xe9;s dans la recherche sur le vieillissement, le fonctionnement c&#xe9;r&#xe9;bral et le diagnostic clinique. Parmi les exemples figurent des tests d&#x2019;intelligence tels que l&#x2019;&#xc9;chelle d&apos;intelligence pour adultes selon Wechsler (WAIS) et les Matrices progressives de Raven ; des t&#xe2;ches &#xe9;valuant l&#x2019;attention, la concentration et la m&#xe9;moire de travail comme l&#x2019;&#xc9;valuation cognitive de Montr&#xe9;al (MoCA) ; ainsi que des exp&#xe9;riences de temps de r&#xe9;action, des tests de fluence verbale et d&#x2019;autres encore.</skos:definition>
      <skos:prefLabel xml:lang="nl">Cognitieve metingen en tests</skos:prefLabel>
      <skos:definition xml:lang="nl"></skos:definition>
   </rdf:Description>
   <rdf:Description rdf:about="http://rdf-vocabulary.ddialliance.org/cv/ModeOfCollection/5.0.0/4b9776b">
      <rdf:type rdf:resource="http://www.w3.org/2004/02/skos/core#Concept"/>
      <skos:inScheme rdf:resource="http://rdf-vocabulary.ddialliance.org/cv/ModeOfCollection/5.0.0/"/>
      <skos:notation xml:lang="en">MeasurementsAndTests.Educational</skos:notation>
      <skos:prefLabel xml:lang="sl">Meritve in testiranja v vzgoji in izobra&#x17e;evanju</skos:prefLabel>
      <skos:definition xml:lang="sl">Ocenjevanje znanja, spretnosti, sposobnosti ali izobra&#x17e;evalnih dose&#x17e;kov s pomo&#x10d;jo specializiranih meritev ali testov.</skos:definition>
      <skos:prefLabel xml:lang="sv">Pedagogiska m&#xe4;tningar och tester</skos:prefLabel>
      <skos:definition xml:lang="sv">Bed&#xf6;mning av kunskap, f&#xf6;rm&#xe5;gor, beg&#xe5;vning eller inl&#xe4;rningsf&#xf6;rm&#xe5;ga med hj&#xe4;lp av specialiserade m&#xe4;tredskap och tester.</skos:definition>
      <skos:prefLabel xml:lang="en">Educational measurements and tests</skos:prefLabel>
      <skos:definition xml:lang="en">Assessment of knowledge, skills, aptitude, or educational achievement by means of specialized measures or tests.</skos:definition>
      <skos:prefLabel xml:lang="de">Messungen und Tests: Leistungs- und Kompetenztests</skos:prefLabel>
      <skos:definition xml:lang="de">Beurteilung von Kenntnissen, F&#xe4;higkeiten, Eignung oder Bildungsstand mittels spezieller Messungen oder Tests.</skos:definition>
      <skos:prefLabel xml:lang="no">Pedagogiske m&#xe5;linger og tester</skos:prefLabel>
      <skos:definition xml:lang="no">Vurdering av kunnskap, ferdighet, egnethet, eller utdanningsoppn&#xe5;elser ved spesialiserte m&#xe5;l eller tester.</skos:definition>
      <skos:prefLabel xml:lang="lt">Edukologiniai matavimai ir testai</skos:prefLabel>
      <skos:definition xml:lang="lt">&#x17d;ini&#x173;, &#x12f;g&#x16b;d&#x17e;i&#x173;, gabum&#x173; ar mokymosi pasiekim&#x173; vertinimas, naudojant specialius matus ar testus.</skos:definition>
      <skos:prefLabel xml:lang="it">Misurazioni e test in ambito educativo</skos:prefLabel>
      <skos:definition xml:lang="it">Valutazione delle conoscenze, abilit&#xe0;, attitudini o risultati in ambito educativo mediante misure o test specializzati.</skos:definition>
      <skos:prefLabel xml:lang="fr">Mesures et tests d&apos;enseignement</skos:prefLabel>
      <skos:definition xml:lang="fr">&#xc9;valuation de connaissances, de comp&#xe9;tences, d&apos;aptitudes, ou de r&#xe9;sultats scolaires au moyen de mesures ou tests sp&#xe9;cialis&#xe9;s.</skos:definition>
      <skos:prefLabel xml:lang="nl">Metingen en tests: Kennis/bekwaamheid</skos:prefLabel>
      <skos:definition xml:lang="nl"></skos:definition>
   </rdf:Description>
   <rdf:Description rdf:about="http://rdf-vocabulary.ddialliance.org/cv/ModeOfCollection/5.0.0/c2a25a6">
      <rdf:type rdf:resource="http://www.w3.org/2004/02/skos/core#Concept"/>
      <skos:inScheme rdf:resource="http://rdf-vocabulary.ddialliance.org/cv/ModeOfCollection/5.0.0/"/>
      <skos:notation xml:lang="en">MeasurementsAndTests.Physical</skos:notation>
      <skos:prefLabel xml:lang="sl">Meritve in testiranja fizi&#x10d;nih lastnosti</skos:prefLabel>
      <skos:definition xml:lang="sl">Ocenjevanje fizi&#x10d;nih lastnosti &#x17e;ivih bitij, predmetov, materialov ali naravnih pojavov. Na primer ugotovitve prakti&#x10d;nega zdravni&#x161;kega pregleda (npr. palpacije ali auskultacije), klini&#x10d;nih meritev in laboratorijskih preiskav, kot so analiza krvi, krvni talak, sr&#x10d;ni utrip, telesna te&#x17e;a in vi&#x161;ina ter splo&#x161;ne meritve, kot so &#x10d;as, razdalja, temperatura, sila, mo&#x10d;, hitrost, podatki GPS o fizi&#x10d;nem gibanju in drugih fizi&#x10d;nih parametrih ali spremenljivkah, kot so geoprostorski podatki.</skos:definition>
      <skos:prefLabel xml:lang="sv">Fysiska m&#xe4;tningar och tester</skos:prefLabel>
      <skos:definition xml:lang="sv">Bed&#xf6;mning av levande varelsers, f&#xf6;rem&#xe5;ls, materials eller naturliga fenomens fysiska egenskaper. Till exempel: blodtryck, puls, kroppsvikt och l&#xe4;ngd, men &#xe4;ven tid, avst&#xe5;nd, massa, temperatur, kraft, effekt, hastighet, GPS-data f&#xf6;r fysisk r&#xf6;relse och andra fysiska parametrar eller variabler, som t.ex. geospatiala data.</skos:definition>
      <skos:prefLabel xml:lang="en">Physical measurements and tests</skos:prefLabel>
      <skos:definition xml:lang="en">Assessment of physical properties of living beings, objects, materials, or natural phenomena. For example, findings from hands-on medical examination (e.g., palpation or auscultation), clinical measurements and lab tests like blood analysis, blood pressure, heart rate, body weight and height, as well as general measurements like time, distance, mass, temperature, force, power, speed, GPS data on physical movement and other physical parameters or variables, like geospatial data.</skos:definition>
      <skos:prefLabel xml:lang="de">Messungen und Tests: Physische Tests</skos:prefLabel>
      <skos:definition xml:lang="de">Beurteilung von physikalischen Eigenschaften von Lebewesen, Gegenst&#xe4;nden, Materialien oder Naturph&#xe4;nomenen. Zum Beispiel Befunde aus der praktischen medizinischen Untersuchung (z. B. Abtasten oder Abh&#xf6;ren), klinische Messungen und Labortests wie Blutanalyse, Blutdruck, Herzfrequenz, K&#xf6;rpergewicht und -gr&#xf6;&#xdf;e sowie allgemeine Messungen wie Zeit, Entfernung, Masse, Temperatur, Kraft, Leistung, Geschwindigkeit, GPS-Daten zu k&#xf6;rperlichen Bewegungen und andere physikalische Parameter oder Variablen, wie Geodaten.</skos:definition>
      <skos:prefLabel xml:lang="no">Fysiske m&#xe5;linger og tester</skos:prefLabel>
      <skos:definition xml:lang="no">Vurdering av fysiske egenskaper hos levende vesener, objekter, materiale, eller naturlige fenomen. For eksempel, funn fra fysiske medisinske unders&#xf8;kelser (e.g., palpasjon eller auskultasjon), kliniske m&#xe5;l og laboratorietester som blodanalyse, blodtrykksm&#xe5;l, hjerterytme, kroppsvekt og h&#xf8;yde, og generelle m&#xe5;l som tid, distanse, masse, temperatur, kraft, energi, fart, GPS data p&#xe5; fysisk bevegelse og andre m&#xe5;l p&#xe5; fysiske parameter eller variabler.</skos:definition>
      <skos:prefLabel xml:lang="lt">Fiziniai matavimai ir testai</skos:prefLabel>
      <skos:definition xml:lang="lt">Gyv&#x173; organizm&#x173;, objekt&#x173;, med&#x17e;iag&#x173; ar gamtos rei&#x161;kini&#x173; fizini&#x173; savybi&#x173; vertinimas. Pavyzd&#x17e;iui, praktin&#x117;s medicinin&#x117;s ap&#x17e;i&#x16b;ros (pavyzd&#x17e;iui, palpacijos ar auskultacijos) rezultatai, klinikini&#x173; matavim&#x173; ir laboratorini&#x173; tyrim&#x173; testai (pavyzd&#x17e;iui, kraujo tyrimai, kraujosp&#x16b;d&#x17e;io, &#x161;irdies ritmo, k&#x16b;no svorio ir &#x16b;gio matavimai), taip pat bendrieji matavimo vienetai (pavyzd&#x17e;iui, laikas, atstumas, mas&#x117;, temperat&#x16b;ra, j&#x117;ga, galia, greitis, GPS duomenys apie fizin&#x12f; jud&#x117;jim&#x105;) ir kiti fiziniai parametrai ar kintamieji (pavyzd&#x17e;iui, geoerdviniai duomenys).</skos:definition>
      <skos:prefLabel xml:lang="it">Misurazioni e test fisici</skos:prefLabel>
      <skos:definition xml:lang="it">Valutazione delle propriet&#xe0; fisiche di esseri viventi, oggetti, materiali o fenomeni naturali. Per esempio, risultati di esami pratici a livello medico (ad esempio, palpazione o auscultazione), misurazioni cliniche e test di laboratorio come analisi del sangue, pressione sanguigna, frequenza cardiaca, peso corporeo e altezza, nonch&#xe9; misure generali come tempo, distanza, massa, temperatura, forza, potenza, velocit&#xe0;, dati GPS sul movimento fisico e altri parametri o variabili fisici, come i dati geospaziali.</skos:definition>
      <skos:prefLabel xml:lang="fr">Mesures et tests de caract&#xe9;ristiques physiques</skos:prefLabel>
      <skos:definition xml:lang="fr">&#xc9;valuation des propri&#xe9;t&#xe9;s physiques d&apos;&#xea;tres vivants, d&apos;objets, de mat&#xe9;riaux, ou de ph&#xe9;nom&#xe8;nes naturels. Par exemple, des r&#xe9;sultats d&apos;examens cliniques (e. g. palpation, auscultation), de mesures cliniques et de tests de laboratoire, comme des analyses de sang, de pression sanguine, de rythme cardiaque, de poids et de taille du corps, de m&#xea;me que des mesures g&#xe9;n&#xe9;rales de temps, de distance, de masse, de temp&#xe9;rature, de force, de puissance, de vitesse, de donn&#xe9;es de localisation sur des mouvements physiques ou d&apos;autres param&#xe8;tres ou variables physiques comme des donn&#xe9;es g&#xe9;ospatiales.</skos:definition>
      <skos:prefLabel xml:lang="nl">Fysieke metingen en tests</skos:prefLabel>
      <skos:definition xml:lang="nl"></skos:definition>
   </rdf:Description>
   <rdf:Description rdf:about="http://rdf-vocabulary.ddialliance.org/cv/ModeOfCollection/5.0.0/27daf03">
      <rdf:type rdf:resource="http://www.w3.org/2004/02/skos/core#Concept"/>
      <skos:inScheme rdf:resource="http://rdf-vocabulary.ddialliance.org/cv/ModeOfCollection/5.0.0/"/>
      <skos:notation xml:lang="en">MeasurementsAndTests.Psychological</skos:notation>
      <skos:prefLabel xml:lang="sl">Meritve in testiranja psiholo&#x161;kih lastnosti</skos:prefLabel>
      <skos:definition xml:lang="sl">Ocena osebnostnih lastnosti ali psiholo&#x161;kih/vedenjskih odzivov s pomo&#x10d;jo posebnih meritev ali testov. Na primer objektivni testi, kot so samoporo&#x10d;anje z zaprtim formatom odgovorov ali projekcijske tehnike, ki omogo&#x10d;ajo proste odgovore, vklju&#x10d;no z besednimi asociacijami, dopolnjevanjem stavkov ali zgodb, vinjetami, testi s karikaturami, testi tematske apercepcije, igranjem vlog, testi risanja, testi pack, testi izbire itd.</skos:definition>
      <skos:prefLabel xml:lang="sv">Psykologiska m&#xe4;tningar och tester</skos:prefLabel>
      <skos:definition xml:lang="sv">Bed&#xf6;mning av personlighetsdrag eller psykologiska/beteendem&#xe4;ssiga responser genom specialiserade m&#xe4;tredskap eller tester. Exempel: objektiva tester som sj&#xe4;lvskattning med begr&#xe4;nsade svarsformat, eller projektiva tester som till&#xe5;ter &#xf6;ppna svar, inklusive ordassociation, menings- eller ber&#xe4;ttelsekomplettering, vinjetter, &quot;cartoon tests&quot;, tematiska apperceptionstester (TAT), rollspel, teckningstester, Rorschachtester, &quot;choice ordering exercises&quot; m.m.</skos:definition>
      <skos:prefLabel xml:lang="en">Psychological measurements and tests</skos:prefLabel>
      <skos:definition xml:lang="en">Assessment of personality traits or psychological/behavioral responses by means of specialized measures or tests. For example, objective tests like self-report measures with a restricted response format, or projective methods allowing free responses, including word association, sentence or story completion, vignettes, cartoon test, thematic apperception tests, role play, drawing tests, inkblot tests, choice ordering exercises, etc.</skos:definition>
      <skos:prefLabel xml:lang="de">Messungen und Tests: Psychologische Tests</skos:prefLabel>
      <skos:definition xml:lang="de">Beurteilung von Pers&#xf6;nlichkeitsmerkmalen oder psychologischen/verhaltensbezogenen Reaktionen mittels spezieller Messungen oder Tests. Zum Beispiel objektive Tests wie Selbstausk&#xfc;nfte mit eingeschr&#xe4;nktem Antwortformat oder projektive Methoden, die freie Antworten erlauben, einschlie&#xdf;lich Wortassoziation, Vervollst&#xe4;ndigung von S&#xe4;tzen- oder Geschichten, Vignetten, Karikatur-Tests, thematische Apperzeptionstests, Rollenspiele, Zeichentests, Tintenkleckstests, Zuordnungsaufgaben usw.</skos:definition>
      <skos:prefLabel xml:lang="no">Psykologiske m&#xe5;linger og tester</skos:prefLabel>
      <skos:definition xml:lang="no">Vurdering av personlighetstrekk eller psykologiske/atferdsmessige reaksjoner ved bruk av spesialiserte m&#xe5;l og tester. For eksempel, objektive tester som selvrapporteringsm&#xe5;l med mer begrenset svarformat, eller projektive metoder som gj&#xf8;r det mulig &#xe5; svare helt fritt, inkludert ordassosiasjon, setning eller fortellingsfullf&#xf8;ring, korte beskrivelser, tematiske appersepsjonstester, rollespill, tegnetester, blekk-kladd tester, prioriterings&#xf8;velser etc.</skos:definition>
      <skos:prefLabel xml:lang="lt">Psichologiniai matavimai ir testai</skos:prefLabel>
      <skos:definition xml:lang="lt">Asmenyb&#x117;s bruo&#x17e;&#x173; arba psichologini&#x173; ar elgsenos reakcij&#x173; vertinimas, naudojant specialius matavimo instrumentus ar testus. Pavyzd&#x17e;iui, standartizuoti testai (pavyzd&#x17e;iui, savipildos instrumentai) su u&#x17e;darais klausimais, ar projekciniai metodai naudojant atvirus klausimus (&#x12f;skaitant &#x17e;od&#x17e;i&#x173; asociacijas, sakinio ar pasakojimo u&#x17e;baigim&#x105;, vinjetes, animuotus testus, teminius suvokimo testus, vaidmen&#x173; &#x17e;aidimus, pie&#x161;imo testus, ra&#x161;alo d&#x117;mi&#x173; testus, pasirinkim&#x173; rangavimo pratimus ir kt.).</skos:definition>
      <skos:prefLabel xml:lang="it">Misurazioni e test psicologici</skos:prefLabel>
      <skos:definition xml:lang="it">Valutazione dei tratti di personalit&#xe0; o risposte psicologiche/comportamentali mediante misure o test specializzati. Ad esempio, test oggettivi come misure di autovalutazione con un range predefinito, o test proiettivi che consentono risposte libere, incluse associazione di parole, completamento di frasi o storie, vignette, fumetti, test di appercezione tematica, giochi di ruolo, prove di disegno, test macchie di inchiostri, esercizi sulle scelte di ordinamento, ecc.</skos:definition>
      <skos:prefLabel xml:lang="fr">Mesures et tests psychologiques</skos:prefLabel>
      <skos:definition xml:lang="fr">&#xc9;valuation des traits de personnalit&#xe9;s ou de r&#xe9;ponses psychologiques / comportementales au moyen de mesures ou tests sp&#xe9;cialis&#xe9;s. Par exemple, des tests objectifs comme des mesures auto-&#xe9;valu&#xe9;es avec un format de r&#xe9;ponses restreint, ou des m&#xe9;thodes projectives permettant des r&#xe9;ponses libres, incluant l&apos;association de mots, l&apos;ach&#xe8;vement de phrase ou d&apos;histoire, des vignettes, des tests anim&#xe9;s, des tests th&#xe9;matiques d&apos;aperception, du jeu de r&#xf4;le, des tests de dessin, des tests de t&#xe2;ches d&apos;encre, des exercices de classement, etc.</skos:definition>
      <skos:prefLabel xml:lang="nl">Psychologische metingen en tests </skos:prefLabel>
      <skos:definition xml:lang="nl"></skos:definition>
   </rdf:Description>
   <rdf:Description rdf:about="http://rdf-vocabulary.ddialliance.org/cv/ModeOfCollection/5.0.0/6311ae1">
      <rdf:type rdf:resource="http://www.w3.org/2004/02/skos/core#Concept"/>
      <skos:inScheme rdf:resource="http://rdf-vocabulary.ddialliance.org/cv/ModeOfCollection/5.0.0/"/>
      <skos:notation xml:lang="en">Other</skos:notation>
      <skos:prefLabel xml:lang="sl">Drugo</skos:prefLabel>
      <skos:definition xml:lang="sl">Uporabite, &#x10d;e je na&#x10d;in zbiranja podatkov znan, vendar ga ni na tem seznamu.</skos:definition>
      <skos:prefLabel xml:lang="sv">&#xd6;vrigt</skos:prefLabel>
      <skos:definition xml:lang="sv">Anv&#xe4;nds n&#xe4;r datainsamlingsmetoden &#xe4;r k&#xe4;nd men saknas i listan.</skos:definition>
      <skos:prefLabel xml:lang="en">Other</skos:prefLabel>
      <skos:definition xml:lang="en">Use if the mode of data collection is known, but not found in the list.</skos:definition>
      <skos:prefLabel xml:lang="de">Andere</skos:prefLabel>
      <skos:definition xml:lang="de">Verwenden Sie diese Kategorie, wenn die Art der Datenerhebung bekannt, aber nicht in der Liste vertreten ist.</skos:definition>
      <skos:prefLabel xml:lang="no">Annet</skos:prefLabel>
      <skos:definition xml:lang="no">Bruk dersom metode for datainnsamling er kjent, men ikke finnes i listen.</skos:definition>
      <skos:prefLabel xml:lang="lt">Kita </skos:prefLabel>
      <skos:definition xml:lang="lt">Naudoti, kai duomen&#x173; rinkimo b&#x16b;das yra &#x17e;inomas, bet jo n&#x117;ra s&#x105;ra&#x161;e.</skos:definition>
      <skos:prefLabel xml:lang="it">Altro</skos:prefLabel>
      <skos:definition xml:lang="it">Utilizzare quando la tecnica di raccolta dei dati &#xe8; conosciuta, ma non &#xe8; presente nell&apos;elenco.</skos:definition>
      <skos:prefLabel xml:lang="fr">Autre</skos:prefLabel>
      <skos:definition xml:lang="fr">Utilisez si le mode de collecte est connu, mais pas pr&#xe9;sent dans la liste.</skos:definition>
      <skos:prefLabel xml:lang="nl">Anders</skos:prefLabel>
      <skos:definition xml:lang="nl"></skos:definition>
   </rdf:Description>
</rdf:RDF>
