<?xml version="1.0" encoding="UTF-8"?>
<rdf:RDF xmlns:dcterms="http://purl.org/dc/terms/"
          xmlns:owl="http://www.w3.org/2002/07/owl#"
          xmlns:rdf="http://www.w3.org/1999/02/22-rdf-syntax-ns#"
          xmlns:rdfs="http://www.w3.org/2000/01/rdf-schema#"
          xmlns:skos="http://www.w3.org/2004/02/skos/core#">
   <rdf:Description rdf:about="http://rdf-vocabulary.ddialliance.org/cv/TypeOfInstrument/1.1.2/">
      <rdf:type rdf:resource="http://www.w3.org/2004/02/skos/core#ConceptScheme"/>
      <dcterms:isVersionOf rdf:resource="http://rdf-vocabulary.ddialliance.org/cv/TypeOfInstrument"/>
      <skos:notation>TypeOfInstrument</skos:notation>
      <skos:prefLabel xml:lang="en">Type of Instrument</skos:prefLabel>
      <skos:prefLabel xml:lang="en">Type of Instrument</skos:prefLabel>
      <skos:prefLabel xml:lang="da">Instrumenttype</skos:prefLabel>
      <skos:prefLabel xml:lang="da">Instrumenttype</skos:prefLabel>
      <skos:prefLabel xml:lang="fi">Keruuväline</skos:prefLabel>
      <skos:prefLabel xml:lang="fi">Keruuväline</skos:prefLabel>
      <skos:prefLabel xml:lang="fr">Type d'instrument</skos:prefLabel>
      <skos:prefLabel xml:lang="fr">Type d'instrument</skos:prefLabel>
      <skos:prefLabel xml:lang="it">Tipo di Strumento</skos:prefLabel>
      <skos:prefLabel xml:lang="it">Tipo di Strumento</skos:prefLabel>
      <skos:prefLabel xml:lang="lt">Instrumento tipas</skos:prefLabel>
      <skos:prefLabel xml:lang="lt">Instrumento tipas</skos:prefLabel>
      <skos:prefLabel xml:lang="nl">Type meetinstrument</skos:prefLabel>
      <skos:prefLabel xml:lang="nl">Type meetinstrument</skos:prefLabel>
      <skos:prefLabel xml:lang="no">Type instrument</skos:prefLabel>
      <skos:prefLabel xml:lang="no">Type instrument</skos:prefLabel>
      <skos:prefLabel xml:lang="pt">Tipo de instrumento de recolha de dados</skos:prefLabel>
      <skos:prefLabel xml:lang="pt">Tipo de instrumento de recolha de dados</skos:prefLabel>
      <skos:prefLabel xml:lang="sl">Vrste instrumentov</skos:prefLabel>
      <skos:prefLabel xml:lang="sl">Vrste instrumentov</skos:prefLabel>
      <skos:prefLabel xml:lang="sr">Vrsta Instrumenta</skos:prefLabel>
      <skos:prefLabel xml:lang="sr">Vrsta Instrumenta</skos:prefLabel>
      <skos:prefLabel xml:lang="sv">Typ av instrument</skos:prefLabel>
      <skos:prefLabel xml:lang="sv">Typ av instrument</skos:prefLabel>
      <skos:definition xml:lang="en">Includes a typology of data collection instruments.</skos:definition>
      <skos:definition xml:lang="en">Includes a typology of data collection instruments.</skos:definition>
      <skos:definition xml:lang="da">Indeholder en typologi af dataindsamlingsinstrumenter.</skos:definition>
      <skos:definition xml:lang="da">Indeholder en typologi af dataindsamlingsinstrumenter.</skos:definition>
      <skos:definition xml:lang="fi">Tyyppiluokittelu tutkimusaineiston muodostamisessa käytetyille keruuvälineille, -ohjeistuksille tai -suunnitelmille.</skos:definition>
      <skos:definition xml:lang="fi">Tyyppiluokittelu tutkimusaineiston muodostamisessa käytetyille keruuvälineille, -ohjeistuksille tai -suunnitelmille.</skos:definition>
      <skos:definition xml:lang="fr">Inclut une typologie des instruments de collecte de données</skos:definition>
      <skos:definition xml:lang="fr">Inclut une typologie des instruments de collecte de données</skos:definition>
      <skos:definition xml:lang="it">Include una tipologia di strumenti per la raccolta dei dati.</skos:definition>
      <skos:definition xml:lang="it">Include una tipologia di strumenti per la raccolta dei dati.</skos:definition>
      <skos:definition xml:lang="lt">Apima duomenų rinkimo instrumentų tipologiją.</skos:definition>
      <skos:definition xml:lang="lt">Apima duomenų rinkimo instrumentų tipologiją.</skos:definition>
      <skos:definition xml:lang="nl">Bevat een indeling van meetinstrumenten voor data verzameling. </skos:definition>
      <skos:definition xml:lang="nl">Bevat een indeling van meetinstrumenten voor data verzameling. </skos:definition>
      <skos:definition xml:lang="no">Inneholder en typologi av ulike instrumenter for datainnsamling.</skos:definition>
      <skos:definition xml:lang="no">Inneholder en typologi av ulike instrumenter for datainnsamling.</skos:definition>
      <skos:definition xml:lang="pt">Inclui uma tipologia de instrumentos de recolha de dados.</skos:definition>
      <skos:definition xml:lang="pt">Inclui uma tipologia de instrumentos de recolha de dados.</skos:definition>
      <skos:definition xml:lang="sl">Vključuje razvrstitev instrumentov za zbiranje podatkov.</skos:definition>
      <skos:definition xml:lang="sl">Vključuje razvrstitev instrumentov za zbiranje podatkov.</skos:definition>
      <skos:definition xml:lang="sr">Sadrži tipologiju instrumenata za prikupljanje podataka.</skos:definition>
      <skos:definition xml:lang="sr">Sadrži tipologiju instrumenata za prikupljanje podataka.</skos:definition>
      <skos:definition xml:lang="sv">Innehåller en typologi av olika instrument för datainsamling.</skos:definition>
      <skos:definition xml:lang="sv">Innehåller en typologi av olika instrument för datainsamling.</skos:definition>
      <owl:versionInfo>1.1.0</owl:versionInfo>
      <dcterms:license rdf:resource="Creative Commons Attribution 4.0 International"/>
      <dcterms:rights>Copyright ©DDI Alliance 2019</dcterms:rights>
      <skos:hasTopConcept rdf:resource="http://rdf-vocabulary.ddialliance.org/cv/TypeOfInstrument/1.1.2/d12e186"/>
      <skos:hasTopConcept rdf:resource="http://rdf-vocabulary.ddialliance.org/cv/TypeOfInstrument/1.1.2/d12e830"/>
      <skos:hasTopConcept rdf:resource="http://rdf-vocabulary.ddialliance.org/cv/TypeOfInstrument/1.1.2/d12e989"/>
      <skos:hasTopConcept rdf:resource="http://rdf-vocabulary.ddialliance.org/cv/TypeOfInstrument/1.1.2/d12e1794"/>
      <skos:hasTopConcept rdf:resource="http://rdf-vocabulary.ddialliance.org/cv/TypeOfInstrument/1.1.2/d12e1953"/>
      <skos:hasTopConcept rdf:resource="http://rdf-vocabulary.ddialliance.org/cv/TypeOfInstrument/1.1.2/d12e2112"/>
      <skos:hasTopConcept rdf:resource="http://rdf-vocabulary.ddialliance.org/cv/TypeOfInstrument/1.1.2/d12e2271"/>
   </rdf:Description>
   <rdf:Description rdf:about="http://rdf-vocabulary.ddialliance.org/cv/TypeOfInstrument/1.1.2/d12e186">
      <rdf:type rdf:resource="http://www.w3.org/2004/02/skos/core#Concept"/>
      <skos:inScheme rdf:resource="http://rdf-vocabulary.ddialliance.org/cv/TypeOfInstrument/1.1.2/"/>
      <skos:notation>Questionnaire</skos:notation>
      <skos:prefLabel xml:lang="en">Questionnaire</skos:prefLabel>
      <skos:definition xml:lang="en">Set of pre-determined questions presented to study participants.</skos:definition>
      <skos:prefLabel xml:lang="en">Questionnaire</skos:prefLabel>
      <skos:definition xml:lang="en">Set of pre-determined questions presented to study participants.</skos:definition>
      <skos:prefLabel xml:lang="da">Spørgeskema</skos:prefLabel>
      <skos:definition xml:lang="da">Sæt af forudbestemte spørgsmål præsenteret for undersøgelsesdeltagerne.</skos:definition>
      <skos:prefLabel xml:lang="da">Spørgeskema</skos:prefLabel>
      <skos:definition xml:lang="da">Sæt af forudbestemte spørgsmål præsenteret for undersøgelsesdeltagerne.</skos:definition>
      <skos:prefLabel xml:lang="fi">Lomake</skos:prefLabel>
      <skos:definition xml:lang="fi">Kysely- tai ilmoituslomake. Kysymykset ovat ennalta määriteltyjä.</skos:definition>
      <skos:prefLabel xml:lang="fi">Lomake</skos:prefLabel>
      <skos:definition xml:lang="fi">Kysely- tai ilmoituslomake. Kysymykset ovat ennalta määriteltyjä.</skos:definition>
      <skos:prefLabel xml:lang="fr">Questionnaire</skos:prefLabel>
      <skos:definition xml:lang="fr">Ensemble de questions prédéterminées présentées aux participants de l'étude</skos:definition>
      <skos:prefLabel xml:lang="fr">Questionnaire</skos:prefLabel>
      <skos:definition xml:lang="fr">Ensemble de questions prédéterminées présentées aux participants de l'étude</skos:definition>
      <skos:prefLabel xml:lang="it">Questionario</skos:prefLabel>
      <skos:definition xml:lang="it">Insieme di domande pre-determinate presentate ai partecipanti allo studio.</skos:definition>
      <skos:prefLabel xml:lang="it">Questionario</skos:prefLabel>
      <skos:definition xml:lang="it">Insieme di domande pre-determinate presentate ai partecipanti allo studio.</skos:definition>
      <skos:prefLabel xml:lang="lt">Klausimynas</skos:prefLabel>
      <skos:definition xml:lang="lt">Iš anksto parengtų klausimų, pateikiamų tyrimo dalyviams, rinkinys.</skos:definition>
      <skos:prefLabel xml:lang="lt">Klausimynas</skos:prefLabel>
      <skos:definition xml:lang="lt">Iš anksto parengtų klausimų, pateikiamų tyrimo dalyviams, rinkinys.</skos:definition>
      <skos:prefLabel xml:lang="nl">Vragenlijst</skos:prefLabel>
      <skos:definition xml:lang="nl"/>
      <skos:prefLabel xml:lang="nl">Vragenlijst</skos:prefLabel>
      <skos:definition xml:lang="nl"/>
      <skos:prefLabel xml:lang="no">Spørreskjema</skos:prefLabel>
      <skos:definition xml:lang="no">Oppsett med forhåndsbestemte spørsmål som blir presentert for studiedeltakerne.</skos:definition>
      <skos:prefLabel xml:lang="no">Spørreskjema</skos:prefLabel>
      <skos:definition xml:lang="no">Oppsett med forhåndsbestemte spørsmål som blir presentert for studiedeltakerne.</skos:definition>
      <skos:prefLabel xml:lang="pt">Questionário</skos:prefLabel>
      <skos:definition xml:lang="pt">Conjunto de questões pré-determinadas apresentadas aos participantes do estudo.</skos:definition>
      <skos:prefLabel xml:lang="pt">Questionário</skos:prefLabel>
      <skos:definition xml:lang="pt">Conjunto de questões pré-determinadas apresentadas aos participantes do estudo.</skos:definition>
      <skos:prefLabel xml:lang="sl">Vprašalnik</skos:prefLabel>
      <skos:definition xml:lang="sl">Nabor vnaprej določenih vprašanj, predstavljenih udeležencem raziskave.</skos:definition>
      <skos:prefLabel xml:lang="sl">Vprašalnik</skos:prefLabel>
      <skos:definition xml:lang="sl">Nabor vnaprej določenih vprašanj, predstavljenih udeležencem raziskave.</skos:definition>
      <skos:prefLabel xml:lang="sr">Upitnik</skos:prefLabel>
      <skos:definition xml:lang="sr">Skup unapred utvrđenih pitanja koja su predstavljena učesnicima studije.</skos:definition>
      <skos:prefLabel xml:lang="sr">Upitnik</skos:prefLabel>
      <skos:definition xml:lang="sr">Skup unapred utvrđenih pitanja koja su predstavljena učesnicima studije.</skos:definition>
      <skos:prefLabel xml:lang="sv">Frågeformulär</skos:prefLabel>
      <skos:definition xml:lang="sv">En uppsättning förutbestämda frågor som ställs till deltagare i studien.</skos:definition>
      <skos:prefLabel xml:lang="sv">Frågeformulär</skos:prefLabel>
      <skos:definition xml:lang="sv">En uppsättning förutbestämda frågor som ställs till deltagare i studien.</skos:definition>
      <skos:narrower rdf:resource="http://rdf-vocabulary.ddialliance.org/cv/TypeOfInstrument/1.1.2/d12e352"/>
      <skos:narrower rdf:resource="http://rdf-vocabulary.ddialliance.org/cv/TypeOfInstrument/1.1.2/d12e511"/>
      <skos:narrower rdf:resource="http://rdf-vocabulary.ddialliance.org/cv/TypeOfInstrument/1.1.2/d12e670"/>
   </rdf:Description>
   <rdf:Description rdf:about="http://rdf-vocabulary.ddialliance.org/cv/TypeOfInstrument/1.1.2/d12e352">
      <rdf:type rdf:resource="http://www.w3.org/2004/02/skos/core#Concept"/>
      <skos:inScheme rdf:resource="http://rdf-vocabulary.ddialliance.org/cv/TypeOfInstrument/1.1.2/"/>
      <skos:notation>Questionnaire.Structured</skos:notation>
      <skos:prefLabel xml:lang="en">Structured questionnaire</skos:prefLabel>
      <skos:definition xml:lang="en">Set of pre-determined questions, a great majority of which are closed-ended, although there may be a small proportion of open-ended questions.</skos:definition>
      <skos:prefLabel xml:lang="en">Structured questionnaire</skos:prefLabel>
      <skos:definition xml:lang="en">Set of pre-determined questions, a great majority of which are closed-ended, although there may be a small proportion of open-ended questions.</skos:definition>
      <skos:prefLabel xml:lang="da">Struktureret spørgeskema</skos:prefLabel>
      <skos:definition xml:lang="da">Sæt af forudbestemte spørgsmål, hvoraf en størstedel er lukkede, selvom der kan være en mindre del af åbne spørgsmål.</skos:definition>
      <skos:prefLabel xml:lang="da">Struktureret spørgeskema</skos:prefLabel>
      <skos:definition xml:lang="da">Sæt af forudbestemte spørgsmål, hvoraf en størstedel er lukkede, selvom der kan være en mindre del af åbne spørgsmål.</skos:definition>
      <skos:prefLabel xml:lang="fi">Strukturoitu lomake</skos:prefLabel>
      <skos:definition xml:lang="fi">Kysely- tai ilmoituslomake. Kysymykset ovat ennalta määriteltyjä. Kysymyksiin on useimmiten laadittu valmiit vastausvaihtoehdot, joskin mukana saattaa olla pieni määrä avokysymyksiä.</skos:definition>
      <skos:prefLabel xml:lang="fi">Strukturoitu lomake</skos:prefLabel>
      <skos:definition xml:lang="fi">Kysely- tai ilmoituslomake. Kysymykset ovat ennalta määriteltyjä. Kysymyksiin on useimmiten laadittu valmiit vastausvaihtoehdot, joskin mukana saattaa olla pieni määrä avokysymyksiä.</skos:definition>
      <skos:prefLabel xml:lang="fr">Questionnaire structuré</skos:prefLabel>
      <skos:definition xml:lang="fr">Ensemble de questions prédéterminées, une grande majorité d'entre elles sont fermées, bien qu'il y ait peut-être une petite proportion de questions ouvertes.</skos:definition>
      <skos:prefLabel xml:lang="fr">Questionnaire structuré</skos:prefLabel>
      <skos:definition xml:lang="fr">Ensemble de questions prédéterminées, une grande majorité d'entre elles sont fermées, bien qu'il y ait peut-être une petite proportion de questions ouvertes.</skos:definition>
      <skos:prefLabel xml:lang="it">Questionario strutturato</skos:prefLabel>
      <skos:definition xml:lang="it">Insieme di domande pre-determinate, la maggior parte delle quali prevede risposte chiuse, sebbene possa esserci una piccola percentuale di domande a risposta aperta.</skos:definition>
      <skos:prefLabel xml:lang="it">Questionario strutturato</skos:prefLabel>
      <skos:definition xml:lang="it">Insieme di domande pre-determinate, la maggior parte delle quali prevede risposte chiuse, sebbene possa esserci una piccola percentuale di domande a risposta aperta.</skos:definition>
      <skos:prefLabel xml:lang="lt">Struktūruotas klausimynas</skos:prefLabel>
      <skos:definition xml:lang="lt">Iš anksto parengtų klausimų rinkinys, kuriame dauguma klausimų yra uždari, bet gali būti ir nedidelė dalis atvirų klausimų.</skos:definition>
      <skos:prefLabel xml:lang="lt">Struktūruotas klausimynas</skos:prefLabel>
      <skos:definition xml:lang="lt">Iš anksto parengtų klausimų rinkinys, kuriame dauguma klausimų yra uždari, bet gali būti ir nedidelė dalis atvirų klausimų.</skos:definition>
      <skos:prefLabel xml:lang="nl">Gestructureerde vragenlijst</skos:prefLabel>
      <skos:definition xml:lang="nl"/>
      <skos:prefLabel xml:lang="nl">Gestructureerde vragenlijst</skos:prefLabel>
      <skos:definition xml:lang="nl"/>
      <skos:prefLabel xml:lang="no">Strukturert spørreskjema</skos:prefLabel>
      <skos:definition xml:lang="no">Oppsett med forhåndsbestemte spørsmål hvor de fleste er lukkede. Det kan forekomme en liten andel åpne spørsmål.</skos:definition>
      <skos:prefLabel xml:lang="no">Strukturert spørreskjema</skos:prefLabel>
      <skos:definition xml:lang="no">Oppsett med forhåndsbestemte spørsmål hvor de fleste er lukkede. Det kan forekomme en liten andel åpne spørsmål.</skos:definition>
      <skos:prefLabel xml:lang="pt">Questionário estruturado</skos:prefLabel>
      <skos:definition xml:lang="pt">Conjunto de questões pré-determinadas, das quais a grande maioria são fechadas, embora possa haver uma pequena proporção de questões abertas.</skos:definition>
      <skos:prefLabel xml:lang="pt">Questionário estruturado</skos:prefLabel>
      <skos:definition xml:lang="pt">Conjunto de questões pré-determinadas, das quais a grande maioria são fechadas, embora possa haver uma pequena proporção de questões abertas.</skos:definition>
      <skos:prefLabel xml:lang="sl">Strukturiran vprašalnik</skos:prefLabel>
      <skos:definition xml:lang="sl">Nabor vnaprej določenih vprašanj, izmed katerih je velika večina vprašanj zaprtega tipa, čeprav je lahko majhen delež vprašanj tudi odprtega tipa.</skos:definition>
      <skos:prefLabel xml:lang="sl">Strukturiran vprašalnik</skos:prefLabel>
      <skos:definition xml:lang="sl">Nabor vnaprej določenih vprašanj, izmed katerih je velika večina vprašanj zaprtega tipa, čeprav je lahko majhen delež vprašanj tudi odprtega tipa.</skos:definition>
      <skos:prefLabel xml:lang="sr">Strukturirana anketa</skos:prefLabel>
      <skos:definition xml:lang="sr">Skup unapred utvrđenih pitanja, od kojih je velika većina zatvorenih, mada može postojati i mali procenat otvorenih pitanja.</skos:definition>
      <skos:prefLabel xml:lang="sr">Strukturirana anketa</skos:prefLabel>
      <skos:definition xml:lang="sr">Skup unapred utvrđenih pitanja, od kojih je velika većina zatvorenih, mada može postojati i mali procenat otvorenih pitanja.</skos:definition>
      <skos:prefLabel xml:lang="sv">Strukturerat frågeformulär</skos:prefLabel>
      <skos:definition xml:lang="sv">En uppsättning förutbestämda frågor, av vilka en stor majoritet är slutna, även om det kan finnas en liten andel öppna frågor.</skos:definition>
      <skos:prefLabel xml:lang="sv">Strukturerat frågeformulär</skos:prefLabel>
      <skos:definition xml:lang="sv">En uppsättning förutbestämda frågor, av vilka en stor majoritet är slutna, även om det kan finnas en liten andel öppna frågor.</skos:definition>
      <skos:broader rdf:resource="http://rdf-vocabulary.ddialliance.org/cv/TypeOfInstrument/1.1.2/d12e186"/>
   </rdf:Description>
   <rdf:Description rdf:about="http://rdf-vocabulary.ddialliance.org/cv/TypeOfInstrument/1.1.2/d12e511">
      <rdf:type rdf:resource="http://www.w3.org/2004/02/skos/core#Concept"/>
      <skos:inScheme rdf:resource="http://rdf-vocabulary.ddialliance.org/cv/TypeOfInstrument/1.1.2/"/>
      <skos:notation>Questionnaire.Semistructured</skos:notation>
      <skos:prefLabel xml:lang="en">Semi-structured questionnaire</skos:prefLabel>
      <skos:definition xml:lang="en">Set of pre-determined questions, a significant proportion of which are open-ended (roughly one third to two thirds), and the rest are closed-ended.</skos:definition>
      <skos:prefLabel xml:lang="en">Semi-structured questionnaire</skos:prefLabel>
      <skos:definition xml:lang="en">Set of pre-determined questions, a significant proportion of which are open-ended (roughly one third to two thirds), and the rest are closed-ended.</skos:definition>
      <skos:prefLabel xml:lang="da">Semistruktueret spørgeskema</skos:prefLabel>
      <skos:definition xml:lang="da">Sæt af forudbestemte spørgsmål, hvoraf en væsentlig del er åbne (rundt regnet en til to tredjedele), og resten er lukkede.</skos:definition>
      <skos:prefLabel xml:lang="da">Semistruktueret spørgeskema</skos:prefLabel>
      <skos:definition xml:lang="da">Sæt af forudbestemte spørgsmål, hvoraf en væsentlig del er åbne (rundt regnet en til to tredjedele), og resten er lukkede.</skos:definition>
      <skos:prefLabel xml:lang="fi">Puolistrukturoitu lomake</skos:prefLabel>
      <skos:definition xml:lang="fi">Kysely- tai ilmoituslomake. Kysymykset ovat ennalta määriteltyjä. Avokysymysten osuus on merkittävä ja vaihtelee suunnilleen kolmasosasta kahteen kolmasosaan. Lopuissa kysymyksissä on valmiit vastausvaihtoehdot.</skos:definition>
      <skos:prefLabel xml:lang="fi">Puolistrukturoitu lomake</skos:prefLabel>
      <skos:definition xml:lang="fi">Kysely- tai ilmoituslomake. Kysymykset ovat ennalta määriteltyjä. Avokysymysten osuus on merkittävä ja vaihtelee suunnilleen kolmasosasta kahteen kolmasosaan. Lopuissa kysymyksissä on valmiit vastausvaihtoehdot.</skos:definition>
      <skos:prefLabel xml:lang="fr">Questionnaire semi-structuré</skos:prefLabel>
      <skos:definition xml:lang="fr">Ensemble de questions prédéterminées, une proportion significative d'entre elles sont ouvertes (environ un tiers à deux tiers), et les restantes sont fermées.</skos:definition>
      <skos:prefLabel xml:lang="fr">Questionnaire semi-structuré</skos:prefLabel>
      <skos:definition xml:lang="fr">Ensemble de questions prédéterminées, une proportion significative d'entre elles sont ouvertes (environ un tiers à deux tiers), et les restantes sont fermées.</skos:definition>
      <skos:prefLabel xml:lang="it">Questionario semi-strutturato</skos:prefLabel>
      <skos:definition xml:lang="it">Insieme di domande pre-determinate, di cui una parte significativa presenta risposta aperte (indicativamente tra un terzo e due terzi del totale), e le restanti sono chiuse.</skos:definition>
      <skos:prefLabel xml:lang="it">Questionario semi-strutturato</skos:prefLabel>
      <skos:definition xml:lang="it">Insieme di domande pre-determinate, di cui una parte significativa presenta risposta aperte (indicativamente tra un terzo e due terzi del totale), e le restanti sono chiuse.</skos:definition>
      <skos:prefLabel xml:lang="lt">Pusiau struktūruotas klausimynas</skos:prefLabel>
      <skos:definition xml:lang="lt">Iš anksto parengtų klausimų rinkinys, kuriame didelė dalis (maždaug nuo vieno iki dviejų trečdalių) klausimų yra atviri, o kiti – uždari.</skos:definition>
      <skos:prefLabel xml:lang="lt">Pusiau struktūruotas klausimynas</skos:prefLabel>
      <skos:definition xml:lang="lt">Iš anksto parengtų klausimų rinkinys, kuriame didelė dalis (maždaug nuo vieno iki dviejų trečdalių) klausimų yra atviri, o kiti – uždari.</skos:definition>
      <skos:prefLabel xml:lang="nl">Semi-gestructureerde vragenlijst</skos:prefLabel>
      <skos:definition xml:lang="nl"/>
      <skos:prefLabel xml:lang="nl">Semi-gestructureerde vragenlijst</skos:prefLabel>
      <skos:definition xml:lang="nl"/>
      <skos:prefLabel xml:lang="no">Semistrukturert spørreskjema</skos:prefLabel>
      <skos:definition xml:lang="no">Oppsett med forhåndsbestemte spørsmål hvor en betydelig andel er åpne (ca. én til to tredjedeler), og resten er lukket.</skos:definition>
      <skos:prefLabel xml:lang="no">Semistrukturert spørreskjema</skos:prefLabel>
      <skos:definition xml:lang="no">Oppsett med forhåndsbestemte spørsmål hvor en betydelig andel er åpne (ca. én til to tredjedeler), og resten er lukket.</skos:definition>
      <skos:prefLabel xml:lang="pt">Questionário semiestruturado</skos:prefLabel>
      <skos:definition xml:lang="pt">Conjunto de questões pré-determinadas, das quais uma parte significativa são abertas (cerca de um terço a dois terços), sendo as restantes fechadas.</skos:definition>
      <skos:prefLabel xml:lang="pt">Questionário semiestruturado</skos:prefLabel>
      <skos:definition xml:lang="pt">Conjunto de questões pré-determinadas, das quais uma parte significativa são abertas (cerca de um terço a dois terços), sendo as restantes fechadas.</skos:definition>
      <skos:prefLabel xml:lang="sl">Polstrukturiran vprašalnik</skos:prefLabel>
      <skos:definition xml:lang="sl">Nabor vnaprej določenih vprašanj, izmed katerih je pomemben delež vprašanj odprtega tipa (približno ena do dve tretjini), preostali del pa zaprtega tipa.</skos:definition>
      <skos:prefLabel xml:lang="sl">Polstrukturiran vprašalnik</skos:prefLabel>
      <skos:definition xml:lang="sl">Nabor vnaprej določenih vprašanj, izmed katerih je pomemben delež vprašanj odprtega tipa (približno ena do dve tretjini), preostali del pa zaprtega tipa.</skos:definition>
      <skos:prefLabel xml:lang="sr">Polustrukturirana anketa</skos:prefLabel>
      <skos:definition xml:lang="sr">Skup unapred utvrđenih pitanja, čiji je značajan deo otvoren (otprilike jedna trećina do dve trećine), a ostala su zatvorena.</skos:definition>
      <skos:prefLabel xml:lang="sr">Polustrukturirana anketa</skos:prefLabel>
      <skos:definition xml:lang="sr">Skup unapred utvrđenih pitanja, čiji je značajan deo otvoren (otprilike jedna trećina do dve trećine), a ostala su zatvorena.</skos:definition>
      <skos:prefLabel xml:lang="sv">Semistrukturerat frågeformulär</skos:prefLabel>
      <skos:definition xml:lang="sv">En uppsättning förutbestämda frågor, av vilka en signifikant majoritet är öppna (cirka en till två tredjedelar), och resten är slutna.</skos:definition>
      <skos:prefLabel xml:lang="sv">Semistrukturerat frågeformulär</skos:prefLabel>
      <skos:definition xml:lang="sv">En uppsättning förutbestämda frågor, av vilka en signifikant majoritet är öppna (cirka en till två tredjedelar), och resten är slutna.</skos:definition>
      <skos:broader rdf:resource="http://rdf-vocabulary.ddialliance.org/cv/TypeOfInstrument/1.1.2/d12e186"/>
   </rdf:Description>
   <rdf:Description rdf:about="http://rdf-vocabulary.ddialliance.org/cv/TypeOfInstrument/1.1.2/d12e670">
      <rdf:type rdf:resource="http://www.w3.org/2004/02/skos/core#Concept"/>
      <skos:inScheme rdf:resource="http://rdf-vocabulary.ddialliance.org/cv/TypeOfInstrument/1.1.2/"/>
      <skos:notation>Questionnaire.Unstructured</skos:notation>
      <skos:prefLabel xml:lang="en">Unstructured questionnaire</skos:prefLabel>
      <skos:definition xml:lang="en">Set of pre-determined questions, a great majority of which are open-ended, although there may be a small proportion of close-ended questions.</skos:definition>
      <skos:prefLabel xml:lang="en">Unstructured questionnaire</skos:prefLabel>
      <skos:definition xml:lang="en">Set of pre-determined questions, a great majority of which are open-ended, although there may be a small proportion of close-ended questions.</skos:definition>
      <skos:prefLabel xml:lang="da">Ustruktureret spørgeskema</skos:prefLabel>
      <skos:definition xml:lang="da">Sæt af forudbestemte spørgsmål, hvoraf en størstedel er åbne, selvom der kan være en mindre del af lukkede spørgsmål.</skos:definition>
      <skos:prefLabel xml:lang="da">Ustruktureret spørgeskema</skos:prefLabel>
      <skos:definition xml:lang="da">Sæt af forudbestemte spørgsmål, hvoraf en størstedel er åbne, selvom der kan være en mindre del af lukkede spørgsmål.</skos:definition>
      <skos:prefLabel xml:lang="fi">Strukturoimaton lomake</skos:prefLabel>
      <skos:definition xml:lang="fi">Kysely- tai ilmoituslomake. Kysymykset ovat ennalta määriteltyjä. Ne ovat useimmiten avokysymyksiä, vaikkakin mukana saattaa olla pieni määrä kysymyksiä, joissa on valmiit vastausvaihtoehdot.</skos:definition>
      <skos:prefLabel xml:lang="fi">Strukturoimaton lomake</skos:prefLabel>
      <skos:definition xml:lang="fi">Kysely- tai ilmoituslomake. Kysymykset ovat ennalta määriteltyjä. Ne ovat useimmiten avokysymyksiä, vaikkakin mukana saattaa olla pieni määrä kysymyksiä, joissa on valmiit vastausvaihtoehdot.</skos:definition>
      <skos:prefLabel xml:lang="fr">Questionnaire non structuré</skos:prefLabel>
      <skos:definition xml:lang="fr">Ensemble de questions prédéterminées, une grande majorité d'entre elles sont ouvertes, bien qu'il y ait peut-être une petite proportion de questions fermées.</skos:definition>
      <skos:prefLabel xml:lang="fr">Questionnaire non structuré</skos:prefLabel>
      <skos:definition xml:lang="fr">Ensemble de questions prédéterminées, une grande majorité d'entre elles sont ouvertes, bien qu'il y ait peut-être une petite proportion de questions fermées.</skos:definition>
      <skos:prefLabel xml:lang="it">Questionario non strutturato</skos:prefLabel>
      <skos:definition xml:lang="it">Insieme di domande pre-determinate, la maggior parte delle quali prevede risposte aperte, sebbene possa esserci una piccola percentuale di domande a risposta chiusa.</skos:definition>
      <skos:prefLabel xml:lang="it">Questionario non strutturato</skos:prefLabel>
      <skos:definition xml:lang="it">Insieme di domande pre-determinate, la maggior parte delle quali prevede risposte aperte, sebbene possa esserci una piccola percentuale di domande a risposta chiusa.</skos:definition>
      <skos:prefLabel xml:lang="lt">Nestruktūruotas klausimynas</skos:prefLabel>
      <skos:definition xml:lang="lt">Iš anksto parengtų klausimų rinkinys, kuriame dauguma klausimų yra atviri, bet gali būti ir nedidelė dalis uždarų klausimų.</skos:definition>
      <skos:prefLabel xml:lang="lt">Nestruktūruotas klausimynas</skos:prefLabel>
      <skos:definition xml:lang="lt">Iš anksto parengtų klausimų rinkinys, kuriame dauguma klausimų yra atviri, bet gali būti ir nedidelė dalis uždarų klausimų.</skos:definition>
      <skos:prefLabel xml:lang="nl">Ongestructureerde vragenlijst</skos:prefLabel>
      <skos:definition xml:lang="nl"/>
      <skos:prefLabel xml:lang="nl">Ongestructureerde vragenlijst</skos:prefLabel>
      <skos:definition xml:lang="nl"/>
      <skos:prefLabel xml:lang="no">Ustrukturert spørreskjema</skos:prefLabel>
      <skos:definition xml:lang="no">Oppsett med forhåndsbestemte spørsmål hvor de fleste er åpne. Det kan forekomme en liten andel lukkede spørsmål.</skos:definition>
      <skos:prefLabel xml:lang="no">Ustrukturert spørreskjema</skos:prefLabel>
      <skos:definition xml:lang="no">Oppsett med forhåndsbestemte spørsmål hvor de fleste er åpne. Det kan forekomme en liten andel lukkede spørsmål.</skos:definition>
      <skos:prefLabel xml:lang="pt">Questionário aberto/não estruturado</skos:prefLabel>
      <skos:definition xml:lang="pt">Conjunto de questões pré-determinadas, das quais a grande maioria são abertas, embora possa haver uma pequena proporção de questões fechadas.</skos:definition>
      <skos:prefLabel xml:lang="pt">Questionário aberto/não estruturado</skos:prefLabel>
      <skos:definition xml:lang="pt">Conjunto de questões pré-determinadas, das quais a grande maioria são abertas, embora possa haver uma pequena proporção de questões fechadas.</skos:definition>
      <skos:prefLabel xml:lang="sl">Nestrukturiran vprašalnik</skos:prefLabel>
      <skos:definition xml:lang="sl">Nabor vnaprej določenih vprašanj, izmed katerih je velika večina vprašanj odprtega tipa, čeprav je lahko majhen delež vprašanj tudi zaprtega tipa.</skos:definition>
      <skos:prefLabel xml:lang="sl">Nestrukturiran vprašalnik</skos:prefLabel>
      <skos:definition xml:lang="sl">Nabor vnaprej določenih vprašanj, izmed katerih je velika večina vprašanj odprtega tipa, čeprav je lahko majhen delež vprašanj tudi zaprtega tipa.</skos:definition>
      <skos:prefLabel xml:lang="sr">Nestrukturirana anketa</skos:prefLabel>
      <skos:definition xml:lang="sr">Skup unapred utvrđenih pitanja, od kojih je velika većina otvorena, mada može postojati mali deo bliskih pitanja.</skos:definition>
      <skos:prefLabel xml:lang="sr">Nestrukturirana anketa</skos:prefLabel>
      <skos:definition xml:lang="sr">Skup unapred utvrđenih pitanja, od kojih je velika većina otvorena, mada može postojati mali deo bliskih pitanja.</skos:definition>
      <skos:prefLabel xml:lang="sv">Ostrukturerat frågeformulär</skos:prefLabel>
      <skos:definition xml:lang="sv">En uppsättning förutbestämda frågor, av vilka en stor majoritet är öppna, även om det kan finnas en liten andel slutna frågor.</skos:definition>
      <skos:prefLabel xml:lang="sv">Ostrukturerat frågeformulär</skos:prefLabel>
      <skos:definition xml:lang="sv">En uppsättning förutbestämda frågor, av vilka en stor majoritet är öppna, även om det kan finnas en liten andel slutna frågor.</skos:definition>
      <skos:broader rdf:resource="http://rdf-vocabulary.ddialliance.org/cv/TypeOfInstrument/1.1.2/d12e186"/>
   </rdf:Description>
   <rdf:Description rdf:about="http://rdf-vocabulary.ddialliance.org/cv/TypeOfInstrument/1.1.2/d12e830">
      <rdf:type rdf:resource="http://www.w3.org/2004/02/skos/core#Concept"/>
      <skos:inScheme rdf:resource="http://rdf-vocabulary.ddialliance.org/cv/TypeOfInstrument/1.1.2/"/>
      <skos:notation>InterviewSchemeAndThemes</skos:notation>
      <skos:prefLabel xml:lang="en">Interview scheme and/or themes</skos:prefLabel>
      <skos:definition xml:lang="en">Themes, topics, and/or questions used in an interview. Can vary between loosely defined themes to more exactly formulated questions. There is more flexibility than in an unstructured questionnaire regarding which questions are asked of each participant and how they are conveyed.</skos:definition>
      <skos:prefLabel xml:lang="en">Interview scheme and/or themes</skos:prefLabel>
      <skos:definition xml:lang="en">Themes, topics, and/or questions used in an interview. Can vary between loosely defined themes to more exactly formulated questions. There is more flexibility than in an unstructured questionnaire regarding which questions are asked of each participant and how they are conveyed.</skos:definition>
      <skos:prefLabel xml:lang="da">Interviewskema og/eller temaer</skos:prefLabel>
      <skos:definition xml:lang="da">Temaer, emner, og/eller spørgsmål anvendt i et interview. Kan variere mellem løst definerede temaer til mere præcist formulerede spørgsmål. Der er mere fleksibilitet end i et ustruktureret spørgeskema i forhold til, hvilke spørgsmål deltageren stilles, og hvordan de stilles.</skos:definition>
      <skos:prefLabel xml:lang="da">Interviewskema og/eller temaer</skos:prefLabel>
      <skos:definition xml:lang="da">Temaer, emner, og/eller spørgsmål anvendt i et interview. Kan variere mellem løst definerede temaer til mere præcist formulerede spørgsmål. Der er mere fleksibilitet end i et ustruktureret spørgeskema i forhold til, hvilke spørgsmål deltageren stilles, og hvordan de stilles.</skos:definition>
      <skos:prefLabel xml:lang="fi">Haastatteluteemat tai haastattelurunko</skos:prefLabel>
      <skos:definition xml:lang="fi">Haastattelututkimuksessa käytetyt haastatteluteemat tai -kysymykset. Vaihtelevat väljästi muotoilluista teemoista melko tarkasti muotoiltuihin kysymyksiin. Jälkimmäisessä tapauksessa ero strukturoimattomaan lomakkeeseen on siinä, että kaikille osanottajille ei esitetä kaikkia kysymyksiä tai kysymysten muotoilu on vapaampaa.</skos:definition>
      <skos:prefLabel xml:lang="fi">Haastatteluteemat tai haastattelurunko</skos:prefLabel>
      <skos:definition xml:lang="fi">Haastattelututkimuksessa käytetyt haastatteluteemat tai -kysymykset. Vaihtelevat väljästi muotoilluista teemoista melko tarkasti muotoiltuihin kysymyksiin. Jälkimmäisessä tapauksessa ero strukturoimattomaan lomakkeeseen on siinä, että kaikille osanottajille ei esitetä kaikkia kysymyksiä tai kysymysten muotoilu on vapaampaa.</skos:definition>
      <skos:prefLabel xml:lang="fr">Schéma et / ou thèmes d'entretien</skos:prefLabel>
      <skos:definition xml:lang="fr">Thèmes, sujets, et / ou questions utilisés dans un entretien. Peut varier entre des thèmes vaguement définis et des questions formulées plus précisément. Il y a plus de souplesse que dans un questionnaire non structuré en ce qui concerne les questions qui sont posées à chaque participant et la manière dont elles sont transmises.</skos:definition>
      <skos:prefLabel xml:lang="fr">Schéma et / ou thèmes d'entretien</skos:prefLabel>
      <skos:definition xml:lang="fr">Thèmes, sujets, et / ou questions utilisés dans un entretien. Peut varier entre des thèmes vaguement définis et des questions formulées plus précisément. Il y a plus de souplesse que dans un questionnaire non structuré en ce qui concerne les questions qui sont posées à chaque participant et la manière dont elles sont transmises.</skos:definition>
      <skos:prefLabel xml:lang="it">Traccia e/o temi di intervista</skos:prefLabel>
      <skos:definition xml:lang="it">Temi, argomenti e/o domande utilizzate in un'intervista. Può variare tra temi definiti in modo ampio e domande formulate in modo più preciso. Rispetto a un questionario non strutturato c'è una maggiore flessibilità riguardo a quali domande vengono effettivamente poste a ciascun partecipante e come esse vengono poste.</skos:definition>
      <skos:prefLabel xml:lang="it">Traccia e/o temi di intervista</skos:prefLabel>
      <skos:definition xml:lang="it">Temi, argomenti e/o domande utilizzate in un'intervista. Può variare tra temi definiti in modo ampio e domande formulate in modo più preciso. Rispetto a un questionario non strutturato c'è una maggiore flessibilità riguardo a quali domande vengono effettivamente poste a ciascun partecipante e come esse vengono poste.</skos:definition>
      <skos:prefLabel xml:lang="lt">Interviu planas ir (arba) temos</skos:prefLabel>
      <skos:definition xml:lang="lt">Temos ir (arba) klausimai, naudojami interviu metu. Gali apimti ir laisvai apibrėžtas temas ir tiksliau suformuluotus klausimus. Lyginant su nestruktūruotu klausimynu, čia daugiau lankstumo pateikiant klausimus ar juos užduodant skirtingiems dalyviams.</skos:definition>
      <skos:prefLabel xml:lang="lt">Interviu planas ir (arba) temos</skos:prefLabel>
      <skos:definition xml:lang="lt">Temos ir (arba) klausimai, naudojami interviu metu. Gali apimti ir laisvai apibrėžtas temas ir tiksliau suformuluotus klausimus. Lyginant su nestruktūruotu klausimynu, čia daugiau lankstumo pateikiant klausimus ar juos užduodant skirtingiems dalyviams.</skos:definition>
      <skos:prefLabel xml:lang="nl">Interviewschema en/of thema's</skos:prefLabel>
      <skos:definition xml:lang="nl"/>
      <skos:prefLabel xml:lang="nl">Interviewschema en/of thema's</skos:prefLabel>
      <skos:definition xml:lang="nl"/>
      <skos:prefLabel xml:lang="no">Intervjuskjema og/eller tema</skos:prefLabel>
      <skos:definition xml:lang="no">Tema, emner og/eller spørsmål brukt i et intervju. Kan variere mellom løst definerte tema til mer nøyaktig formulerte spørsmål. Mer fleksibilitet enn i ustrukturerte spørreskjema når det kommer til hvilke spørsmål som blir stilt hver deltaker og hvordan de blir stilt.</skos:definition>
      <skos:prefLabel xml:lang="no">Intervjuskjema og/eller tema</skos:prefLabel>
      <skos:definition xml:lang="no">Tema, emner og/eller spørsmål brukt i et intervju. Kan variere mellom løst definerte tema til mer nøyaktig formulerte spørsmål. Mer fleksibilitet enn i ustrukturerte spørreskjema når det kommer til hvilke spørsmål som blir stilt hver deltaker og hvordan de blir stilt.</skos:definition>
      <skos:prefLabel xml:lang="pt">Esquema/temas de entrevista</skos:prefLabel>
      <skos:definition xml:lang="pt">Temas, tópicos e/ou questões usados numa entrevista. Pode variar entre temas vagamente definidos para questões mais especificamente formuladas. Há mais flexibilidade do que num questionário não estruturado relativamente a que questões são colocadas a cada participante e como elas são abordadas.</skos:definition>
      <skos:prefLabel xml:lang="pt">Esquema/temas de entrevista</skos:prefLabel>
      <skos:definition xml:lang="pt">Temas, tópicos e/ou questões usados numa entrevista. Pode variar entre temas vagamente definidos para questões mais especificamente formuladas. Há mais flexibilidade do que num questionário não estruturado relativamente a que questões são colocadas a cada participante e como elas são abordadas.</skos:definition>
      <skos:prefLabel xml:lang="sl">Načrt intervjuja in/ali teme</skos:prefLabel>
      <skos:definition xml:lang="sl">Teme in/ali vprašanja, uporabljena v intervjuju. Lahko se razteza od široko opredeljenih tem do natančneje oblikovanih vprašanj. V primerjavi z nestrukturiranim vprašalnikom je več prožnosti glede vprašanj, ki jih postavimo udeležencem, in načina, kako jih posredujemo.</skos:definition>
      <skos:prefLabel xml:lang="sl">Načrt intervjuja in/ali teme</skos:prefLabel>
      <skos:definition xml:lang="sl">Teme in/ali vprašanja, uporabljena v intervjuju. Lahko se razteza od široko opredeljenih tem do natančneje oblikovanih vprašanj. V primerjavi z nestrukturiranim vprašalnikom je več prožnosti glede vprašanj, ki jih postavimo udeležencem, in načina, kako jih posredujemo.</skos:definition>
      <skos:prefLabel xml:lang="sr">Okvir intervjua i/ili teme</skos:prefLabel>
      <skos:definition xml:lang="sr">Teme i/ili pitanja koja se koriste u intervjuu. Mogu varirati između okvirno definisanih tema do precizno formulisanih pitanja. Postoji veća fleksibilnost nego u nestrukturiranom upitniku u vezi sa tim koja se pitanja postavljaju svakom učesniku i kako se prenose.</skos:definition>
      <skos:prefLabel xml:lang="sr">Okvir intervjua i/ili teme</skos:prefLabel>
      <skos:definition xml:lang="sr">Teme i/ili pitanja koja se koriste u intervjuu. Mogu varirati između okvirno definisanih tema do precizno formulisanih pitanja. Postoji veća fleksibilnost nego u nestrukturiranom upitniku u vezi sa tim koja se pitanja postavljaju svakom učesniku i kako se prenose.</skos:definition>
      <skos:prefLabel xml:lang="sv">Intervjuschema och/eller teman</skos:prefLabel>
      <skos:definition xml:lang="sv">Teman, ämnen och/eller frågor som används i en intervju. Kan variera mellan löst definierade teman och mer exakt formulerade frågor. Det finns mer flexibilitet än i ett ostrukturerat frågeformulär angående vilka frågor som ställs till varje deltagare och hur de förmedlas.</skos:definition>
      <skos:prefLabel xml:lang="sv">Intervjuschema och/eller teman</skos:prefLabel>
      <skos:definition xml:lang="sv">Teman, ämnen och/eller frågor som används i en intervju. Kan variera mellan löst definierade teman och mer exakt formulerade frågor. Det finns mer flexibilitet än i ett ostrukturerat frågeformulär angående vilka frågor som ställs till varje deltagare och hur de förmedlas.</skos:definition>
   </rdf:Description>
   <rdf:Description rdf:about="http://rdf-vocabulary.ddialliance.org/cv/TypeOfInstrument/1.1.2/d12e989">
      <rdf:type rdf:resource="http://www.w3.org/2004/02/skos/core#Concept"/>
      <skos:inScheme rdf:resource="http://rdf-vocabulary.ddialliance.org/cv/TypeOfInstrument/1.1.2/"/>
      <skos:notation>DataCollectionGuidelines</skos:notation>
      <skos:prefLabel xml:lang="en">Data collection guidelines</skos:prefLabel>
      <skos:definition xml:lang="en">Directions or instructions regarding the methods and procedures to be used for collecting the data. Use a more specific term if possible.</skos:definition>
      <skos:prefLabel xml:lang="en">Data collection guidelines</skos:prefLabel>
      <skos:definition xml:lang="en">Directions or instructions regarding the methods and procedures to be used for collecting the data. Use a more specific term if possible.</skos:definition>
      <skos:prefLabel xml:lang="da">Retningslinjer for dataindsamling</skos:prefLabel>
      <skos:definition xml:lang="da">Retningslinjer eller instruktioner vedrørende metoder og procedurer, der bør anvendes til indsamling af dataene. Anvend et mere specifikt begreb, hvis muligt.</skos:definition>
      <skos:prefLabel xml:lang="da">Retningslinjer for dataindsamling</skos:prefLabel>
      <skos:definition xml:lang="da">Retningslinjer eller instruktioner vedrørende metoder og procedurer, der bør anvendes til indsamling af dataene. Anvend et mere specifikt begreb, hvis muligt.</skos:definition>
      <skos:prefLabel xml:lang="fi">Aineistonkeruuohjeistus</skos:prefLabel>
      <skos:definition xml:lang="fi">Suunnitelma tai ohjeet, jotka määrittelevät aineistonkeruun menetelmät ja prosessit. Käytä tarkempaa termiä mikäli mahdollista.</skos:definition>
      <skos:prefLabel xml:lang="fi">Aineistonkeruuohjeistus</skos:prefLabel>
      <skos:definition xml:lang="fi">Suunnitelma tai ohjeet, jotka määrittelevät aineistonkeruun menetelmät ja prosessit. Käytä tarkempaa termiä mikäli mahdollista.</skos:definition>
      <skos:prefLabel xml:lang="fr">Consignes de collecte de données</skos:prefLabel>
      <skos:definition xml:lang="fr">Directions ou instructions concernant les méthodes et les procédures à utiliser pour collecter les données. Utilisez un terme plus précis si possible.</skos:definition>
      <skos:prefLabel xml:lang="fr">Consignes de collecte de données</skos:prefLabel>
      <skos:definition xml:lang="fr">Directions ou instructions concernant les méthodes et les procédures à utiliser pour collecter les données. Utilisez un terme plus précis si possible.</skos:definition>
      <skos:prefLabel xml:lang="it">Linee guida per la raccolta dei dati</skos:prefLabel>
      <skos:definition xml:lang="it">Indicazioni o istruzioni relative ai metodi e alle procedure da utilizzare per la raccolta dei dati. Utilizzare un termine più specifico, se possibile.</skos:definition>
      <skos:prefLabel xml:lang="it">Linee guida per la raccolta dei dati</skos:prefLabel>
      <skos:definition xml:lang="it">Indicazioni o istruzioni relative ai metodi e alle procedure da utilizzare per la raccolta dei dati. Utilizzare un termine più specifico, se possibile.</skos:definition>
      <skos:prefLabel xml:lang="lt">Duomenų rinkimo gairės</skos:prefLabel>
      <skos:definition xml:lang="lt">Duomenų rinkimo metodų ir procedūrų taikymo nurodymai ar instrukcijos. Jei įmanoma, naudoti konkretesnį terminą.</skos:definition>
      <skos:prefLabel xml:lang="lt">Duomenų rinkimo gairės</skos:prefLabel>
      <skos:definition xml:lang="lt">Duomenų rinkimo metodų ir procedūrų taikymo nurodymai ar instrukcijos. Jei įmanoma, naudoti konkretesnį terminą.</skos:definition>
      <skos:prefLabel xml:lang="nl">Richtlijnen voor gegevensverzameling</skos:prefLabel>
      <skos:definition xml:lang="nl"/>
      <skos:prefLabel xml:lang="nl">Richtlijnen voor gegevensverzameling</skos:prefLabel>
      <skos:definition xml:lang="nl"/>
      <skos:prefLabel xml:lang="no">Retningslinjer for datainnsamling</skos:prefLabel>
      <skos:definition xml:lang="no">Retningslinjer og framgangsmåter som skal brukes for å samle inn dataene. Bruk et smalere begrep om mulig.</skos:definition>
      <skos:prefLabel xml:lang="no">Retningslinjer for datainnsamling</skos:prefLabel>
      <skos:definition xml:lang="no">Retningslinjer og framgangsmåter som skal brukes for å samle inn dataene. Bruk et smalere begrep om mulig.</skos:definition>
      <skos:prefLabel xml:lang="pt">Orientações para a recolha de dados</skos:prefLabel>
      <skos:definition xml:lang="pt">Orientações ou instruções sobre os métodos e procedimentos a utilizar para recolher os dados. Se possível, usar um termo mais específico.</skos:definition>
      <skos:prefLabel xml:lang="pt">Orientações para a recolha de dados</skos:prefLabel>
      <skos:definition xml:lang="pt">Orientações ou instruções sobre os métodos e procedimentos a utilizar para recolher os dados. Se possível, usar um termo mais específico.</skos:definition>
      <skos:prefLabel xml:lang="sl">Smernice za zbiranje podatkov</skos:prefLabel>
      <skos:definition xml:lang="sl">Smernice in navodila, ki opredeljujejo vsebino zajema podatkov. Če je mogoče, uporabite ožji izraz.</skos:definition>
      <skos:prefLabel xml:lang="sl">Smernice za zbiranje podatkov</skos:prefLabel>
      <skos:definition xml:lang="sl">Smernice in navodila, ki opredeljujejo vsebino zajema podatkov. Če je mogoče, uporabite ožji izraz.</skos:definition>
      <skos:prefLabel xml:lang="sr">Smernice za prikupljanje podataka</skos:prefLabel>
      <skos:definition xml:lang="sr">Uputstva ili smernice u vezi sa metodama i postupcima koji će se koristiti za prikupljanje podataka. Koristite precizniji izraz ako je moguće.</skos:definition>
      <skos:prefLabel xml:lang="sr">Smernice za prikupljanje podataka</skos:prefLabel>
      <skos:definition xml:lang="sr">Uputstva ili smernice u vezi sa metodama i postupcima koji će se koristiti za prikupljanje podataka. Koristite precizniji izraz ako je moguće.</skos:definition>
      <skos:prefLabel xml:lang="sv">Datainsamlingsguide</skos:prefLabel>
      <skos:definition xml:lang="sv">Guide och anvisningar som definierar innehållet i datainsamlingen. Använd en smalare term om möjligt.</skos:definition>
      <skos:prefLabel xml:lang="sv">Datainsamlingsguide</skos:prefLabel>
      <skos:definition xml:lang="sv">Guide och anvisningar som definierar innehållet i datainsamlingen. Använd en smalare term om möjligt.</skos:definition>
      <skos:narrower rdf:resource="http://rdf-vocabulary.ddialliance.org/cv/TypeOfInstrument/1.1.2/d12e1157"/>
      <skos:narrower rdf:resource="http://rdf-vocabulary.ddialliance.org/cv/TypeOfInstrument/1.1.2/d12e1316"/>
      <skos:narrower rdf:resource="http://rdf-vocabulary.ddialliance.org/cv/TypeOfInstrument/1.1.2/d12e1475"/>
      <skos:narrower rdf:resource="http://rdf-vocabulary.ddialliance.org/cv/TypeOfInstrument/1.1.2/d12e1634"/>
   </rdf:Description>
   <rdf:Description rdf:about="http://rdf-vocabulary.ddialliance.org/cv/TypeOfInstrument/1.1.2/d12e1157">
      <rdf:type rdf:resource="http://www.w3.org/2004/02/skos/core#Concept"/>
      <skos:inScheme rdf:resource="http://rdf-vocabulary.ddialliance.org/cv/TypeOfInstrument/1.1.2/"/>
      <skos:notation>DataCollectionGuidelines.ObservationGuide</skos:notation>
      <skos:prefLabel xml:lang="en">Data collection guidelines: Observation guide</skos:prefLabel>
      <skos:definition xml:lang="en">Guidelines regarding what will be observed. Depending on the study design, an observation guide can be more or less structured, ranging from exact specifications and scales to loosely formulated ideas.</skos:definition>
      <skos:prefLabel xml:lang="en">Data collection guidelines: Observation guide</skos:prefLabel>
      <skos:definition xml:lang="en">Guidelines regarding what will be observed. Depending on the study design, an observation guide can be more or less structured, ranging from exact specifications and scales to loosely formulated ideas.</skos:definition>
      <skos:prefLabel xml:lang="da">Retningslinjer for dataindsamling: Observationsguide</skos:prefLabel>
      <skos:definition xml:lang="da">Retningslinjer for, hvad der vil blive observeret. Afhængigt af undersøgelsesdesign kan en observationsvejledning være mere eller mindre struktureret, rangerende fra nøjagtige specifikationer og skaleringer til løst formulerede idéer.</skos:definition>
      <skos:prefLabel xml:lang="da">Retningslinjer for dataindsamling: Observationsguide</skos:prefLabel>
      <skos:definition xml:lang="da">Retningslinjer for, hvad der vil blive observeret. Afhængigt af undersøgelsesdesign kan en observationsvejledning være mere eller mindre struktureret, rangerende fra nøjagtige specifikationer og skaleringer til løst formulerede idéer.</skos:definition>
      <skos:prefLabel xml:lang="fi">Aineistonkeruuohjeistus: havainnointiohje tai -suunnitelma</skos:prefLabel>
      <skos:definition xml:lang="fi">Havainnointitutkimuksessa käytetty suunnitelma siitä, mitä havainnoidaan. Tutkimusasetelmasta riippuen havainnointisuunnitelma voi olla enemmän tai vähemmän strukturoitu, vaihdellen tarkoista määrittelyistä ja asteikoista väljästi muotoiltuihin ideoihin.</skos:definition>
      <skos:prefLabel xml:lang="fi">Aineistonkeruuohjeistus: havainnointiohje tai -suunnitelma</skos:prefLabel>
      <skos:definition xml:lang="fi">Havainnointitutkimuksessa käytetty suunnitelma siitä, mitä havainnoidaan. Tutkimusasetelmasta riippuen havainnointisuunnitelma voi olla enemmän tai vähemmän strukturoitu, vaihdellen tarkoista määrittelyistä ja asteikoista väljästi muotoiltuihin ideoihin.</skos:definition>
      <skos:prefLabel xml:lang="fr">Consignes de collecte de données : guide d'observation</skos:prefLabel>
      <skos:definition xml:lang="fr">Consignes concernant ce qui devra être observé. En fonction de la conception de l'étude, un guide d'observation peut être plus ou moins structuré, allant de spécifications et d'échelle à des idées vagues formulées.</skos:definition>
      <skos:prefLabel xml:lang="fr">Consignes de collecte de données : guide d'observation</skos:prefLabel>
      <skos:definition xml:lang="fr">Consignes concernant ce qui devra être observé. En fonction de la conception de l'étude, un guide d'observation peut être plus ou moins structuré, allant de spécifications et d'échelle à des idées vagues formulées.</skos:definition>
      <skos:prefLabel xml:lang="it">Linee guida per la raccolta dei dati: traccia di osservazione</skos:prefLabel>
      <skos:definition xml:lang="it">Linee guida riguardanti ciò che verrà osservato. A seconda della disegno della ricerca, una guida all'osservazione può essere più o meno strutturata, variando da indicazioni e scale precise a idee formulate in modo generale.</skos:definition>
      <skos:prefLabel xml:lang="it">Linee guida per la raccolta dei dati: traccia di osservazione</skos:prefLabel>
      <skos:definition xml:lang="it">Linee guida riguardanti ciò che verrà osservato. A seconda della disegno della ricerca, una guida all'osservazione può essere più o meno strutturata, variando da indicazioni e scale precise a idee formulate in modo generale.</skos:definition>
      <skos:prefLabel xml:lang="lt">Duomenų rinkimo gairės: stebėjimo vadovas</skos:prefLabel>
      <skos:definition xml:lang="lt">Gairės apibrėžiančios, kas bus stebima. Priklausomai nuo tyrimo plano, stebėjimo vadovas gali būti daugiau ar mažiau struktūruotas. Gairės gali pateikti tikslias taisykles ir skales, arba tik laisvai suformuluotas idėjas.</skos:definition>
      <skos:prefLabel xml:lang="lt">Duomenų rinkimo gairės: stebėjimo vadovas</skos:prefLabel>
      <skos:definition xml:lang="lt">Gairės apibrėžiančios, kas bus stebima. Priklausomai nuo tyrimo plano, stebėjimo vadovas gali būti daugiau ar mažiau struktūruotas. Gairės gali pateikti tikslias taisykles ir skales, arba tik laisvai suformuluotas idėjas.</skos:definition>
      <skos:prefLabel xml:lang="nl">Richtlijnen voor gegevensverzameling: Observatie handleiding</skos:prefLabel>
      <skos:definition xml:lang="nl"/>
      <skos:prefLabel xml:lang="nl">Richtlijnen voor gegevensverzameling: Observatie handleiding</skos:prefLabel>
      <skos:definition xml:lang="nl"/>
      <skos:prefLabel xml:lang="no">Retningslinjer for datainnsamling: Observasjonsguide</skos:prefLabel>
      <skos:definition xml:lang="no">Retningslinjer til det som skal observeres. En observasjonsguide kan være mer eller mindre strukturert avhengig av studiedesignet. Den kan variere fra eksakte spesifikasjoner og skalaer til løst formulerte ideer.</skos:definition>
      <skos:prefLabel xml:lang="no">Retningslinjer for datainnsamling: Observasjonsguide</skos:prefLabel>
      <skos:definition xml:lang="no">Retningslinjer til det som skal observeres. En observasjonsguide kan være mer eller mindre strukturert avhengig av studiedesignet. Den kan variere fra eksakte spesifikasjoner og skalaer til løst formulerte ideer.</skos:definition>
      <skos:prefLabel xml:lang="pt">Orientações para a recolha de dados: Grelha de observação</skos:prefLabel>
      <skos:definition xml:lang="pt">Orientações ou instruções sobre o que será observado. Dependendo da concepção do estudo, uma grelha de observação pode ser mais ou menos estruturada, variando de especificações exatas e escalas a ideias formuladas de uma forma vaga.</skos:definition>
      <skos:prefLabel xml:lang="pt">Orientações para a recolha de dados: Grelha de observação</skos:prefLabel>
      <skos:definition xml:lang="pt">Orientações ou instruções sobre o que será observado. Dependendo da concepção do estudo, uma grelha de observação pode ser mais ou menos estruturada, variando de especificações exatas e escalas a ideias formuladas de uma forma vaga.</skos:definition>
      <skos:prefLabel xml:lang="sl">Smernice za zbiranje podatkov: vodnik za opazovanje</skos:prefLabel>
      <skos:definition xml:lang="sl">Smernice za opazovanje. Glede na načrt raziskave je vodnik za opazovanje lahko bolj ali manj strukturiran, od natančnih določitev in lestvic do ohlapno oblikovanih idej.</skos:definition>
      <skos:prefLabel xml:lang="sl">Smernice za zbiranje podatkov: vodnik za opazovanje</skos:prefLabel>
      <skos:definition xml:lang="sl">Smernice za opazovanje. Glede na načrt raziskave je vodnik za opazovanje lahko bolj ali manj strukturiran, od natančnih določitev in lestvic do ohlapno oblikovanih idej.</skos:definition>
      <skos:prefLabel xml:lang="sr">Smernice za prikupljanje podataka: Uputstvo za posmatranje</skos:prefLabel>
      <skos:definition xml:lang="sr">Smernice o tome šta će se posmatrati. U zavisnosti od dizajna studije, uputstvo za posmatranje može biti manje ili više struktuirano, u rasponu od tačnih specifikacija i skala, do slabo formulisanih ideja.</skos:definition>
      <skos:prefLabel xml:lang="sr">Smernice za prikupljanje podataka: Uputstvo za posmatranje</skos:prefLabel>
      <skos:definition xml:lang="sr">Smernice o tome šta će se posmatrati. U zavisnosti od dizajna studije, uputstvo za posmatranje može biti manje ili više struktuirano, u rasponu od tačnih specifikacija i skala, do slabo formulisanih ideja.</skos:definition>
      <skos:prefLabel xml:lang="sv">Datainsamlingsguide: Observationsguide</skos:prefLabel>
      <skos:definition xml:lang="sv">Guide till det som ska observeras. Beroende på studiedesign kan en observationsguide vara mer eller mindre strukturerad, allt från exakta specifikationer och skalor till löst formulerade idéer.</skos:definition>
      <skos:prefLabel xml:lang="sv">Datainsamlingsguide: Observationsguide</skos:prefLabel>
      <skos:definition xml:lang="sv">Guide till det som ska observeras. Beroende på studiedesign kan en observationsguide vara mer eller mindre strukturerad, allt från exakta specifikationer och skalor till löst formulerade idéer.</skos:definition>
      <skos:broader rdf:resource="http://rdf-vocabulary.ddialliance.org/cv/TypeOfInstrument/1.1.2/d12e989"/>
   </rdf:Description>
   <rdf:Description rdf:about="http://rdf-vocabulary.ddialliance.org/cv/TypeOfInstrument/1.1.2/d12e1316">
      <rdf:type rdf:resource="http://www.w3.org/2004/02/skos/core#Concept"/>
      <skos:inScheme rdf:resource="http://rdf-vocabulary.ddialliance.org/cv/TypeOfInstrument/1.1.2/"/>
      <skos:notation>DataCollectionGuidelines.DiscussionGuide</skos:notation>
      <skos:prefLabel xml:lang="en">Data collection guidelines: Discussion guide</skos:prefLabel>
      <skos:definition xml:lang="en">Guidelines for a group discussion. Depending on the study design, a discussion guide can be more or less structured, ranging from exactly formulated questions to general ideas on what to discuss. For example, a list of topics to be discussed in a focus group, or themes formulated by a researcher to direct a blog discussion, etc.</skos:definition>
      <skos:prefLabel xml:lang="en">Data collection guidelines: Discussion guide</skos:prefLabel>
      <skos:definition xml:lang="en">Guidelines for a group discussion. Depending on the study design, a discussion guide can be more or less structured, ranging from exactly formulated questions to general ideas on what to discuss. For example, a list of topics to be discussed in a focus group, or themes formulated by a researcher to direct a blog discussion, etc.</skos:definition>
      <skos:prefLabel xml:lang="da">Retningslinjer for dataindsamling: Diskussionsguide</skos:prefLabel>
      <skos:definition xml:lang="da">Retningslinjer for en gruppediskussion. Afhængigt af undersøgelsesdesignet kan en diskussion være mere eller mindre struktureret, rangererende fra præcist formulerede spørgsmål til generelle idéer om, hvad man skal diskutere. For eksempel en liste over emner, der skal diskuteres i en fokusgruppe eller temaer formuleret af en forsker, der skal lede en blogdiskussion mm.</skos:definition>
      <skos:prefLabel xml:lang="da">Retningslinjer for dataindsamling: Diskussionsguide</skos:prefLabel>
      <skos:definition xml:lang="da">Retningslinjer for en gruppediskussion. Afhængigt af undersøgelsesdesignet kan en diskussion være mere eller mindre struktureret, rangererende fra præcist formulerede spørgsmål til generelle idéer om, hvad man skal diskutere. For eksempel en liste over emner, der skal diskuteres i en fokusgruppe eller temaer formuleret af en forsker, der skal lede en blogdiskussion mm.</skos:definition>
      <skos:prefLabel xml:lang="fi">Aineistonkeruuohjeistus: keskusteluohje</skos:prefLabel>
      <skos:definition xml:lang="fi">Ryhmäkeskusteluun annetut ohjeet. Tutkimusasetelmasta riippuen saattavat olla enemmän tai vähemmän strukturoituja, vaihdellen väljästi muotoilluista keskusteluteemoista tarkasti muotoiltuihin kysymyksiin. Esimerkkejä: Lista keskustelun teemoista, tutkijan esille ottamat tarkat aiheet ja muu ohjaus blogikeskusteluun jne.</skos:definition>
      <skos:prefLabel xml:lang="fi">Aineistonkeruuohjeistus: keskusteluohje</skos:prefLabel>
      <skos:definition xml:lang="fi">Ryhmäkeskusteluun annetut ohjeet. Tutkimusasetelmasta riippuen saattavat olla enemmän tai vähemmän strukturoituja, vaihdellen väljästi muotoilluista keskusteluteemoista tarkasti muotoiltuihin kysymyksiin. Esimerkkejä: Lista keskustelun teemoista, tutkijan esille ottamat tarkat aiheet ja muu ohjaus blogikeskusteluun jne.</skos:definition>
      <skos:prefLabel xml:lang="fr">Consignes de collecte de données : guide de discussion</skos:prefLabel>
      <skos:definition xml:lang="fr">Consignes pour un groupe de discussion. En fonction de la conception de l'étude, un guide de discussion peut être plus ou moins structuré, allant de questions formulées précisément à des idées générales sur quoi discuter. Par exemple, une liste de sujets à discutés dans un focus group, ou des thèmes formulés par un chercheur pour diriger une discussion sur un blog, etc.</skos:definition>
      <skos:prefLabel xml:lang="fr">Consignes de collecte de données : guide de discussion</skos:prefLabel>
      <skos:definition xml:lang="fr">Consignes pour un groupe de discussion. En fonction de la conception de l'étude, un guide de discussion peut être plus ou moins structuré, allant de questions formulées précisément à des idées générales sur quoi discuter. Par exemple, une liste de sujets à discutés dans un focus group, ou des thèmes formulés par un chercheur pour diriger une discussion sur un blog, etc.</skos:definition>
      <skos:prefLabel xml:lang="it">Linee guida per la raccolta dei dati: traccia di discussione</skos:prefLabel>
      <skos:definition xml:lang="it">Linee guida per una discussione di gruppo. A seconda del progetto del disegno della ricerca, una guida alla discussione può essere più o meno strutturata, variando tra domande formulate con precisione a idee generali sui temi da sottoporre alla discussione. Ad esempio, un elenco di argomenti da discutere in un focus group o temi formulati da un ricercatore per indirizzare una discussione su un blog, ecc.</skos:definition>
      <skos:prefLabel xml:lang="it">Linee guida per la raccolta dei dati: traccia di discussione</skos:prefLabel>
      <skos:definition xml:lang="it">Linee guida per una discussione di gruppo. A seconda del progetto del disegno della ricerca, una guida alla discussione può essere più o meno strutturata, variando tra domande formulate con precisione a idee generali sui temi da sottoporre alla discussione. Ad esempio, un elenco di argomenti da discutere in un focus group o temi formulati da un ricercatore per indirizzare una discussione su un blog, ecc.</skos:definition>
      <skos:prefLabel xml:lang="lt">Duomenų rinkimo gairės: diskusijų vadovas</skos:prefLabel>
      <skos:definition xml:lang="lt">Grupinės diskusijos gairės. Priklausomai nuo tyrimo plano, diskusijų vadovas gali būti daugiau ar mažiau struktūruotas (pateikti tiksliai suformuluotus klausimus ar tik bendras diskusijos idėjas). Pavyzdžiui, temų sąrašas tikslinei grupės diskusijai, arba tematikos, kurias tyrėjas suformuluoja norėdamas kryptingai valdyti diskusiją tinklaraštyje ir kt.</skos:definition>
      <skos:prefLabel xml:lang="lt">Duomenų rinkimo gairės: diskusijų vadovas</skos:prefLabel>
      <skos:definition xml:lang="lt">Grupinės diskusijos gairės. Priklausomai nuo tyrimo plano, diskusijų vadovas gali būti daugiau ar mažiau struktūruotas (pateikti tiksliai suformuluotus klausimus ar tik bendras diskusijos idėjas). Pavyzdžiui, temų sąrašas tikslinei grupės diskusijai, arba tematikos, kurias tyrėjas suformuluoja norėdamas kryptingai valdyti diskusiją tinklaraštyje ir kt.</skos:definition>
      <skos:prefLabel xml:lang="nl">Richtlijnen voor gegevensverzameling: Discussie handleiding</skos:prefLabel>
      <skos:definition xml:lang="nl"/>
      <skos:prefLabel xml:lang="nl">Richtlijnen voor gegevensverzameling: Discussie handleiding</skos:prefLabel>
      <skos:definition xml:lang="nl"/>
      <skos:prefLabel xml:lang="no">Retningslinjer for datainnsamling: Diskusjonsguide</skos:prefLabel>
      <skos:definition xml:lang="no">Retningslinjer for en gruppediskusjon. En diskusjonsguide kan være mer eller mindre strukturert avhengig av studiedesignet. Den kan variere mellom nøyaktig formulerte spørsmål og løst formulerte ideer om hva en ønsker å diskutere. For eksempel en liste med tema å diskutere i en fokusgruppe, eller tema formulert av forsker for å lede en bloggdiskusjon, etc.</skos:definition>
      <skos:prefLabel xml:lang="no">Retningslinjer for datainnsamling: Diskusjonsguide</skos:prefLabel>
      <skos:definition xml:lang="no">Retningslinjer for en gruppediskusjon. En diskusjonsguide kan være mer eller mindre strukturert avhengig av studiedesignet. Den kan variere mellom nøyaktig formulerte spørsmål og løst formulerte ideer om hva en ønsker å diskutere. For eksempel en liste med tema å diskutere i en fokusgruppe, eller tema formulert av forsker for å lede en bloggdiskusjon, etc.</skos:definition>
      <skos:prefLabel xml:lang="pt">Orientações para a recolha de dados: Guião de debate</skos:prefLabel>
      <skos:definition xml:lang="pt">Orientações ou instruções para uma discussão de grupo. Dependendo da concepção do estudo, um guião de discussão pode ser mais ou menos estruturado, variando de questões especificamente formuladas a ideias gerais sobre o que discutir/debater. Por exemplo, uma lista de tópicos a serem discutidos num grupo de foco, ou temas formulados por um investigador para orientar uma discussão num blog, etc.</skos:definition>
      <skos:prefLabel xml:lang="pt">Orientações para a recolha de dados: Guião de debate</skos:prefLabel>
      <skos:definition xml:lang="pt">Orientações ou instruções para uma discussão de grupo. Dependendo da concepção do estudo, um guião de discussão pode ser mais ou menos estruturado, variando de questões especificamente formuladas a ideias gerais sobre o que discutir/debater. Por exemplo, uma lista de tópicos a serem discutidos num grupo de foco, ou temas formulados por um investigador para orientar uma discussão num blog, etc.</skos:definition>
      <skos:prefLabel xml:lang="sl">Smernice za zbiranje podatkov: vodnik za razpravo</skos:prefLabel>
      <skos:definition xml:lang="sl">Smernice za skupinsko razpravo. Glede na načrt raziskave je lahko vodnik za razpravo bolj ali manj strukturiran, od natančno oblikovanih vprašanj do splošnih idej o predmetu razprave. Na primer, seznam tem, o katerih bo razpravljala fokusna skupina, ali teme, ki jih oblikuje raziskovalec za usmerjanje razprave na spletnem blogu, itd.</skos:definition>
      <skos:prefLabel xml:lang="sl">Smernice za zbiranje podatkov: vodnik za razpravo</skos:prefLabel>
      <skos:definition xml:lang="sl">Smernice za skupinsko razpravo. Glede na načrt raziskave je lahko vodnik za razpravo bolj ali manj strukturiran, od natančno oblikovanih vprašanj do splošnih idej o predmetu razprave. Na primer, seznam tem, o katerih bo razpravljala fokusna skupina, ali teme, ki jih oblikuje raziskovalec za usmerjanje razprave na spletnem blogu, itd.</skos:definition>
      <skos:prefLabel xml:lang="sr">Smernice za prikupljanje podataka: Uputstvo za razgovor (diskusiju)</skos:prefLabel>
      <skos:definition xml:lang="sr">Smernice za grupnu diskusiju. Zavisno od dizajna studije, vodič za diskusiju može biti manje ili više strukturiran, u rasponu od tačno formulisanih pitanja do opštih ideja o tome o čemu treba razgovarati. Na primer, spisak tema o kojima će se razgovarati u fokus grupi ili teme koje je formulisao istraživač kako bi usmeravao raspravu na blogu, itd.</skos:definition>
      <skos:prefLabel xml:lang="sr">Smernice za prikupljanje podataka: Uputstvo za razgovor (diskusiju)</skos:prefLabel>
      <skos:definition xml:lang="sr">Smernice za grupnu diskusiju. Zavisno od dizajna studije, vodič za diskusiju može biti manje ili više strukturiran, u rasponu od tačno formulisanih pitanja do opštih ideja o tome o čemu treba razgovarati. Na primer, spisak tema o kojima će se razgovarati u fokus grupi ili teme koje je formulisao istraživač kako bi usmeravao raspravu na blogu, itd.</skos:definition>
      <skos:prefLabel xml:lang="sv">Datainsamlingsguide: Diskussionsguide</skos:prefLabel>
      <skos:definition xml:lang="sv">Guide för en gruppdiskussion. Beroende på studiedesign kan en diskussionsguide vara mer eller mindre strukturerad, allt från exakt formulerade frågor till allmänna idéer om vad man ska diskutera. Till exempel en lista över ämnen som ska diskuteras i en fokusgrupp eller teman formulerade av en forskare för att styra en bloggdiskussion osv.</skos:definition>
      <skos:prefLabel xml:lang="sv">Datainsamlingsguide: Diskussionsguide</skos:prefLabel>
      <skos:definition xml:lang="sv">Guide för en gruppdiskussion. Beroende på studiedesign kan en diskussionsguide vara mer eller mindre strukturerad, allt från exakt formulerade frågor till allmänna idéer om vad man ska diskutera. Till exempel en lista över ämnen som ska diskuteras i en fokusgrupp eller teman formulerade av en forskare för att styra en bloggdiskussion osv.</skos:definition>
      <skos:broader rdf:resource="http://rdf-vocabulary.ddialliance.org/cv/TypeOfInstrument/1.1.2/d12e989"/>
   </rdf:Description>
   <rdf:Description rdf:about="http://rdf-vocabulary.ddialliance.org/cv/TypeOfInstrument/1.1.2/d12e1475">
      <rdf:type rdf:resource="http://www.w3.org/2004/02/skos/core#Concept"/>
      <skos:inScheme rdf:resource="http://rdf-vocabulary.ddialliance.org/cv/TypeOfInstrument/1.1.2/"/>
      <skos:notation>DataCollectionGuidelines.SelfAdministeredWritingsGuide</skos:notation>
      <skos:prefLabel xml:lang="en">Data collection guidelines: Self-administered writings guide</skos:prefLabel>
      <skos:definition xml:lang="en">Guidelines regarding the desired, or expected content of self-written personal accounts or narratives from potential participants. The instructions can be supplied as part of the writing invitation or separately. For example, an invitation asking people suffering from a specific disease or disability to describe how it affects their feelings, social relations, and everyday life; or a writing invitation asking people to keep a diary of books read during a period of six months and the thoughts provoked by the books.</skos:definition>
      <skos:prefLabel xml:lang="en">Data collection guidelines: Self-administered writings guide</skos:prefLabel>
      <skos:definition xml:lang="en">Guidelines regarding the desired, or expected content of self-written personal accounts or narratives from potential participants. The instructions can be supplied as part of the writing invitation or separately. For example, an invitation asking people suffering from a specific disease or disability to describe how it affects their feelings, social relations, and everyday life; or a writing invitation asking people to keep a diary of books read during a period of six months and the thoughts provoked by the books.</skos:definition>
      <skos:prefLabel xml:lang="da">Retningslinjer for dataindsamling: Selvadministreret skriveguide</skos:prefLabel>
      <skos:definition xml:lang="da">Retningslinjer vedrørende det ønskede eller forventede indhold af selvskrevne, personlige beretninger eller fortællinger fra potentielle deltagere. Instruktionerne kan leveres som del af den skriftlige invitation eller separat. For eksempel en invitation, der beder folk, som lider af en specifik sygdom eller handicap om at beskrive, hvordan det påvirker deres følelser, sociale relationer og hverdagsliv; eller en skriftlig invitation, der beder folk om at holde en dagbog om bøger læst over seks måneder og de tanker, som bøger fremkalder.</skos:definition>
      <skos:prefLabel xml:lang="da">Retningslinjer for dataindsamling: Selvadministreret skriveguide</skos:prefLabel>
      <skos:definition xml:lang="da">Retningslinjer vedrørende det ønskede eller forventede indhold af selvskrevne, personlige beretninger eller fortællinger fra potentielle deltagere. Instruktionerne kan leveres som del af den skriftlige invitation eller separat. For eksempel en invitation, der beder folk, som lider af en specifik sygdom eller handicap om at beskrive, hvordan det påvirker deres følelser, sociale relationer og hverdagsliv; eller en skriftlig invitation, der beder folk om at holde en dagbog om bøger læst over seks måneder og de tanker, som bøger fremkalder.</skos:definition>
      <skos:prefLabel xml:lang="fi">Aineistonkeruuohjeistus: kirjoitusohje</skos:prefLabel>
      <skos:definition xml:lang="fi">Kirjoitusaineistojen keräämistä varten annetut kirjoitusohjeet joko kirjoituskutsun osana tai erillisenä. Esimerkkejä: Kirjoituskutsussa pyydetään tietyn sairauden tai vamman omaavia ihmisiä  kuvailemaan kuinka se vaikuttaa heidän tunteisiinsa, ihmissuhteisiinsa ja jokapäiväiseen elämäänsä; ohjeistus lukupäiväkirjalle, johon osanottaja kirjaa lukemansa kirjat ja niiden herättämät ajatukset.</skos:definition>
      <skos:prefLabel xml:lang="fi">Aineistonkeruuohjeistus: kirjoitusohje</skos:prefLabel>
      <skos:definition xml:lang="fi">Kirjoitusaineistojen keräämistä varten annetut kirjoitusohjeet joko kirjoituskutsun osana tai erillisenä. Esimerkkejä: Kirjoituskutsussa pyydetään tietyn sairauden tai vamman omaavia ihmisiä  kuvailemaan kuinka se vaikuttaa heidän tunteisiinsa, ihmissuhteisiinsa ja jokapäiväiseen elämäänsä; ohjeistus lukupäiväkirjalle, johon osanottaja kirjaa lukemansa kirjat ja niiden herättämät ajatukset.</skos:definition>
      <skos:prefLabel xml:lang="fr">Consignes de collecte de données : guide des écrits auto-administrés</skos:prefLabel>
      <skos:definition xml:lang="fr">Consignes concernant le contenu attendu ou désiré des écrits personnels ou narratifs de participants potentiels. Les instructions peuvent être fournies dans le cadre de l'invitation écrite ou séparément. Par exemple, une invitation demandant aux personnes souffrant d'une maladie ou un handicap spécifique de décrire comment cela affecte leurs sentiments, leurs relations sociales et la vie quotidienne ; ou une invitation écrite demandant aux personnes de tenir un journal des livres lus pendant une période de six mois et les pensées provoquées par les livres.</skos:definition>
      <skos:prefLabel xml:lang="fr">Consignes de collecte de données : guide des écrits auto-administrés</skos:prefLabel>
      <skos:definition xml:lang="fr">Consignes concernant le contenu attendu ou désiré des écrits personnels ou narratifs de participants potentiels. Les instructions peuvent être fournies dans le cadre de l'invitation écrite ou séparément. Par exemple, une invitation demandant aux personnes souffrant d'une maladie ou un handicap spécifique de décrire comment cela affecte leurs sentiments, leurs relations sociales et la vie quotidienne ; ou une invitation écrite demandant aux personnes de tenir un journal des livres lus pendant une période de six mois et les pensées provoquées par les livres.</skos:definition>
      <skos:prefLabel xml:lang="it">Linee guida per la raccolta dei dati: scritti autocompilati</skos:prefLabel>
      <skos:definition xml:lang="it">Linee guida relative al contenuto desiderato o atteso di documenti o narrazioni personali dei potenziali partecipanti allo studio. Le istruzioni possono essere fornite come parte dell'invito a partecipare oppure separatamente. Ad esempio, un invito che chiede alle persone che soffrono di una specifica malattia o disabilità di descrivere come essa influisca sui loro sentimenti, sulle relazioni sociali e sulla vita quotidiana; oppure un invito a tenere un diario dei libri letti durante un periodo di sei mesi con la richiesta di riportare i pensieri suscitati dai libri.</skos:definition>
      <skos:prefLabel xml:lang="it">Linee guida per la raccolta dei dati: scritti autocompilati</skos:prefLabel>
      <skos:definition xml:lang="it">Linee guida relative al contenuto desiderato o atteso di documenti o narrazioni personali dei potenziali partecipanti allo studio. Le istruzioni possono essere fornite come parte dell'invito a partecipare oppure separatamente. Ad esempio, un invito che chiede alle persone che soffrono di una specifica malattia o disabilità di descrivere come essa influisca sui loro sentimenti, sulle relazioni sociali e sulla vita quotidiana; oppure un invito a tenere un diario dei libri letti durante un periodo di sei mesi con la richiesta di riportare i pensieri suscitati dai libri.</skos:definition>
      <skos:prefLabel xml:lang="lt">Duomenų rinkimo gairės: savarankiškai rašomų tekstų vadovas</skos:prefLabel>
      <skos:definition xml:lang="lt">Potencialių dalyvių savarankiškai rašomų asmeninių pasakojimų ar naratyvų turinio kūrimo gairės. Instrukcijos gali būti pateiktos kartu su kvietimu rašyti arba atskirai. Pavyzdžiui, kvietimas, kuriame žmonių, kenčiančių nuo konkrečios ligos ar negalios, prašoma aprašyti, kaip tai veikia jų jausmus, socialinius ryšius ir kasdienį gyvenimą; arba kvietimas, kuriame žmonių prašoma šešis mėnesius rašyti perskaitytų knygų dienoraštį ir kilusias mintis.</skos:definition>
      <skos:prefLabel xml:lang="lt">Duomenų rinkimo gairės: savarankiškai rašomų tekstų vadovas</skos:prefLabel>
      <skos:definition xml:lang="lt">Potencialių dalyvių savarankiškai rašomų asmeninių pasakojimų ar naratyvų turinio kūrimo gairės. Instrukcijos gali būti pateiktos kartu su kvietimu rašyti arba atskirai. Pavyzdžiui, kvietimas, kuriame žmonių, kenčiančių nuo konkrečios ligos ar negalios, prašoma aprašyti, kaip tai veikia jų jausmus, socialinius ryšius ir kasdienį gyvenimą; arba kvietimas, kuriame žmonių prašoma šešis mėnesius rašyti perskaitytų knygų dienoraštį ir kilusias mintis.</skos:definition>
      <skos:prefLabel xml:lang="nl">Richtlijnen voor gegevensverzameling: Instructie voor zelf invullen</skos:prefLabel>
      <skos:definition xml:lang="nl"/>
      <skos:prefLabel xml:lang="nl">Richtlijnen voor gegevensverzameling: Instructie voor zelf invullen</skos:prefLabel>
      <skos:definition xml:lang="nl"/>
      <skos:prefLabel xml:lang="no">Retningslinjer for datainnsamling: Selvadministrert skriveguide</skos:prefLabel>
      <skos:definition xml:lang="no">Retningslinjer angående ønsket eller forventet innhold i selvskrevne personlige fortellinger fra potensielle deltakere. Instruksjonene kan bli utdelt som del av invitasjonen til å skrive, eller den kan gis ut separat. For eksempel en invitasjon som ber folk med livstruende sykdommer beskrive hvordan sykdommen påvirker deres følelser, sosiale relasjoner og hverdagsliv; eller en skriveinvitasjon som ber folk føre en dagbok over hvilke bøker de leser over en seksmånedersperiode og hvilke tanker bøkene vekker.</skos:definition>
      <skos:prefLabel xml:lang="no">Retningslinjer for datainnsamling: Selvadministrert skriveguide</skos:prefLabel>
      <skos:definition xml:lang="no">Retningslinjer angående ønsket eller forventet innhold i selvskrevne personlige fortellinger fra potensielle deltakere. Instruksjonene kan bli utdelt som del av invitasjonen til å skrive, eller den kan gis ut separat. For eksempel en invitasjon som ber folk med livstruende sykdommer beskrive hvordan sykdommen påvirker deres følelser, sosiale relasjoner og hverdagsliv; eller en skriveinvitasjon som ber folk føre en dagbok over hvilke bøker de leser over en seksmånedersperiode og hvilke tanker bøkene vekker.</skos:definition>
      <skos:prefLabel xml:lang="pt">Orientações para a recolha de dados: Guião para registos  de autopreenchimento</skos:prefLabel>
      <skos:definition xml:lang="pt">Orientações ou instruções sobre o conteúdo esperado ou desejado de relatos ou narrativas pessoais de potenciais participantes. As instruções podem ser fornecidas como parte do guião ou separadamente. Por exemplo, um convite pedindo/solicitando às pessoas que sofrem de uma doença específica ou incapacidade/limitação para descrever como isso afeta os sentimentos, as relações sociais e a vida quotidiana; ou um convite por escrito pedindo às pessoas para manterem um diário dos livros lidos durante um período de seis meses e dos pensamentos por eles suscitados.</skos:definition>
      <skos:prefLabel xml:lang="pt">Orientações para a recolha de dados: Guião para registos  de autopreenchimento</skos:prefLabel>
      <skos:definition xml:lang="pt">Orientações ou instruções sobre o conteúdo esperado ou desejado de relatos ou narrativas pessoais de potenciais participantes. As instruções podem ser fornecidas como parte do guião ou separadamente. Por exemplo, um convite pedindo/solicitando às pessoas que sofrem de uma doença específica ou incapacidade/limitação para descrever como isso afeta os sentimentos, as relações sociais e a vida quotidiana; ou um convite por escrito pedindo às pessoas para manterem um diário dos livros lidos durante um período de seis meses e dos pensamentos por eles suscitados.</skos:definition>
      <skos:prefLabel xml:lang="sl">Smernice za zbiranje podatkov: vodnik za samoizpolnjevanje</skos:prefLabel>
      <skos:definition xml:lang="sl">Smernice o želeni ali pričakovani vsebini samoizpolnjenih osebnih dnevnikov ali pripovedi potencialnih udeležencev. Navodila so lahko na voljo kot del napisanega vabila ali ločeno. Na primer, obvestilo o literarnem natečaju, ki vabi ljudi z življenjsko nevarno boleznijo, da opišejo, kako bolezen vpliva na njihove občutke, medsebojne odnose in vsakdanje življenje; ali pisno vabilo posameznikom, naj vodijo dnevnik prebranih knjig v šestih mesecih in si zapisujejo misli, ki se jim porajajo ob branju.</skos:definition>
      <skos:prefLabel xml:lang="sl">Smernice za zbiranje podatkov: vodnik za samoizpolnjevanje</skos:prefLabel>
      <skos:definition xml:lang="sl">Smernice o želeni ali pričakovani vsebini samoizpolnjenih osebnih dnevnikov ali pripovedi potencialnih udeležencev. Navodila so lahko na voljo kot del napisanega vabila ali ločeno. Na primer, obvestilo o literarnem natečaju, ki vabi ljudi z življenjsko nevarno boleznijo, da opišejo, kako bolezen vpliva na njihove občutke, medsebojne odnose in vsakdanje življenje; ali pisno vabilo posameznikom, naj vodijo dnevnik prebranih knjig v šestih mesecih in si zapisujejo misli, ki se jim porajajo ob branju.</skos:definition>
      <skos:prefLabel xml:lang="sr">Smernice za prikupljanje podataka: Vodič za samostalno upravljanje zapisima</skos:prefLabel>
      <skos:definition xml:lang="sr">Smernice o željenom ili očekivanom sadržaju samostalno sastavljenih ličnih zapisa ili svedočanstvima potencijalnih učesnika. Uputstva se mogu biti deo pismenog poziva ili odvojena. Na primer, poziv koji traži od ljudi koji pate od određene bolesti ili invaliditeta da opišu kako to utiče na njihova osećanja, društvene odnose i svakodnevni život; ili poziv za pisanje kojim se traži da ljudi vode dnevnik čitanja knjiga tokom perioda od šest meseci i misli koje izazivaju knjige.</skos:definition>
      <skos:prefLabel xml:lang="sr">Smernice za prikupljanje podataka: Vodič za samostalno upravljanje zapisima</skos:prefLabel>
      <skos:definition xml:lang="sr">Smernice o željenom ili očekivanom sadržaju samostalno sastavljenih ličnih zapisa ili svedočanstvima potencijalnih učesnika. Uputstva se mogu biti deo pismenog poziva ili odvojena. Na primer, poziv koji traži od ljudi koji pate od određene bolesti ili invaliditeta da opišu kako to utiče na njihova osećanja, društvene odnose i svakodnevni život; ili poziv za pisanje kojim se traži da ljudi vode dnevnik čitanja knjiga tokom perioda od šest meseci i misli koje izazivaju knjige.</skos:definition>
      <skos:prefLabel xml:lang="sv">Datainsamlingsguide: Guide för självadministrerade skriftliga uppgifter</skos:prefLabel>
      <skos:definition xml:lang="sv">Guide för önskat eller förväntat innehåll i självskrivna personliga redogörelser eller berättelser från potentiella deltagare. Anvisningarna kan levereras separat eller som en del av inbjudan att delta i skrivandet. Till exempel en inbjudan till människor med en viss sjukdom eller funktionsnedsättning om att beskriva hur det påverkar deras känslor, sociala relationer och vardagsliv. Eller en skrivinbjudan som ber människor att föra dagbok om vilka böcker de läser under en period av sex månader och de tankar som väcks av böckerna.</skos:definition>
      <skos:prefLabel xml:lang="sv">Datainsamlingsguide: Guide för självadministrerade skriftliga uppgifter</skos:prefLabel>
      <skos:definition xml:lang="sv">Guide för önskat eller förväntat innehåll i självskrivna personliga redogörelser eller berättelser från potentiella deltagare. Anvisningarna kan levereras separat eller som en del av inbjudan att delta i skrivandet. Till exempel en inbjudan till människor med en viss sjukdom eller funktionsnedsättning om att beskriva hur det påverkar deras känslor, sociala relationer och vardagsliv. Eller en skrivinbjudan som ber människor att föra dagbok om vilka böcker de läser under en period av sex månader och de tankar som väcks av böckerna.</skos:definition>
      <skos:broader rdf:resource="http://rdf-vocabulary.ddialliance.org/cv/TypeOfInstrument/1.1.2/d12e989"/>
   </rdf:Description>
   <rdf:Description rdf:about="http://rdf-vocabulary.ddialliance.org/cv/TypeOfInstrument/1.1.2/d12e1634">
      <rdf:type rdf:resource="http://www.w3.org/2004/02/skos/core#Concept"/>
      <skos:inScheme rdf:resource="http://rdf-vocabulary.ddialliance.org/cv/TypeOfInstrument/1.1.2/"/>
      <skos:notation>DataCollectionGuidelines.SecondaryDataCollectionGuide</skos:notation>
      <skos:prefLabel xml:lang="en">Data collection guidelines: Secondary data collection guide</skos:prefLabel>
      <skos:definition xml:lang="en">Guidelines specifying what data are to be collected from previously existing sources originally created for other purposes. For example, directions on how to select and code data from qualitative sources to create a quantitative dataset.</skos:definition>
      <skos:prefLabel xml:lang="en">Data collection guidelines: Secondary data collection guide</skos:prefLabel>
      <skos:definition xml:lang="en">Guidelines specifying what data are to be collected from previously existing sources originally created for other purposes. For example, directions on how to select and code data from qualitative sources to create a quantitative dataset.</skos:definition>
      <skos:prefLabel xml:lang="da">Retningslinjer for dataindsamling: Guide for indsamling af sekundærdata</skos:prefLabel>
      <skos:definition xml:lang="da">Retningslinjer, der angiver, hvilke data, som skal indsamles fra tidligere eksisterende kilder oprindeligt skabt til andre formål. For eksempel vejledning til, hvordan man vælger og koder data fra kvalitative kilder for at oprette et kvantitativt datasæt.</skos:definition>
      <skos:prefLabel xml:lang="da">Retningslinjer for dataindsamling: Guide for indsamling af sekundærdata</skos:prefLabel>
      <skos:definition xml:lang="da">Retningslinjer, der angiver, hvilke data, som skal indsamles fra tidligere eksisterende kilder oprindeligt skabt til andre formål. For eksempel vejledning til, hvordan man vælger og koder data fra kvalitative kilder for at oprette et kvantitativt datasæt.</skos:definition>
      <skos:prefLabel xml:lang="fi">Aineistonkeruuohjeistus: poimintaohje tai -suunnitelma</skos:prefLabel>
      <skos:definition xml:lang="fi">Keruuohje tai -suunnitelma siitä, miten tutkimusaineisto muodostetaan jo aiemmin olemassa olevasta, muuta tarkoitusta varten tehdystä lähdemateriaalista. Esimerkiksi ohje sanomalehtimateriaalin poimimiseksi tutkimukseen tai poiminta- ja käsittelyohjeet jos jostain kvalitatiivisesta lähdemateriaalista muodostetaan numeerinen aineisto.</skos:definition>
      <skos:prefLabel xml:lang="fi">Aineistonkeruuohjeistus: poimintaohje tai -suunnitelma</skos:prefLabel>
      <skos:definition xml:lang="fi">Keruuohje tai -suunnitelma siitä, miten tutkimusaineisto muodostetaan jo aiemmin olemassa olevasta, muuta tarkoitusta varten tehdystä lähdemateriaalista. Esimerkiksi ohje sanomalehtimateriaalin poimimiseksi tutkimukseen tai poiminta- ja käsittelyohjeet jos jostain kvalitatiivisesta lähdemateriaalista muodostetaan numeerinen aineisto.</skos:definition>
      <skos:prefLabel xml:lang="fr">Consignes de collecte de données : Guide de collecte de données secondaires</skos:prefLabel>
      <skos:definition xml:lang="fr">Consignes spécifiant quelles données sont collectées à partir de sources existantes précédemment créées pour d'autres fins. Par exemple, des directives sur comment sélectionner et coder des données à partir de sources qualitatives pour créer un ensemble de données quantitatives.</skos:definition>
      <skos:prefLabel xml:lang="fr">Consignes de collecte de données : Guide de collecte de données secondaires</skos:prefLabel>
      <skos:definition xml:lang="fr">Consignes spécifiant quelles données sont collectées à partir de sources existantes précédemment créées pour d'autres fins. Par exemple, des directives sur comment sélectionner et coder des données à partir de sources qualitatives pour créer un ensemble de données quantitatives.</skos:definition>
      <skos:prefLabel xml:lang="it">Linee guida per la raccolta dei dati: dati secondari</skos:prefLabel>
      <skos:definition xml:lang="it">Linee guida che specificano quali dati devono essere raccolti da fonti precedentemente esistenti ma create originariamente per altri scopi. Ad esempio, indicazioni su come selezionare e codificare i dati da fonti qualitative per creare un dataset quantitativo.</skos:definition>
      <skos:prefLabel xml:lang="it">Linee guida per la raccolta dei dati: dati secondari</skos:prefLabel>
      <skos:definition xml:lang="it">Linee guida che specificano quali dati devono essere raccolti da fonti precedentemente esistenti ma create originariamente per altri scopi. Ad esempio, indicazioni su come selezionare e codificare i dati da fonti qualitative per creare un dataset quantitativo.</skos:definition>
      <skos:prefLabel xml:lang="lt">Duomenų rinkimo gairės: antrinių duomenų rinkimo vadovas</skos:prefLabel>
      <skos:definition xml:lang="lt">Gairės nurodančios, kokie duomenys turi būti renkami iš egzistuojančių šaltinių, sukurtų kitiems tikslams. Pavyzdžiui, nurodymai, kaip atrinkti ir koduoti duomenis iš kokybinių šaltinių, norint sukurti kiekybinių duomenų rinkinį.</skos:definition>
      <skos:prefLabel xml:lang="lt">Duomenų rinkimo gairės: antrinių duomenų rinkimo vadovas</skos:prefLabel>
      <skos:definition xml:lang="lt">Gairės nurodančios, kokie duomenys turi būti renkami iš egzistuojančių šaltinių, sukurtų kitiems tikslams. Pavyzdžiui, nurodymai, kaip atrinkti ir koduoti duomenis iš kokybinių šaltinių, norint sukurti kiekybinių duomenų rinkinį.</skos:definition>
      <skos:prefLabel xml:lang="nl">Richtlijnen voor gegevensverzameling: Handleiding voor de verzameling van secundaire gegevens</skos:prefLabel>
      <skos:definition xml:lang="nl"/>
      <skos:prefLabel xml:lang="nl">Richtlijnen voor gegevensverzameling: Handleiding voor de verzameling van secundaire gegevens</skos:prefLabel>
      <skos:definition xml:lang="nl"/>
      <skos:prefLabel xml:lang="no">Retningslinjer for datainnsamling: Guide for andregangsinnsamling av data</skos:prefLabel>
      <skos:definition xml:lang="no">Retningslinjer som spesifiserer hvilke opplysninger som skal hentes fra eksisterende datakilder som opprinnelig ble samlet for andre formål. For eksempel retningslinjer for hvordan opplysninger fra kvalitative kilder skal velges og kodes for å utarbeide kvantitative datasett.</skos:definition>
      <skos:prefLabel xml:lang="no">Retningslinjer for datainnsamling: Guide for andregangsinnsamling av data</skos:prefLabel>
      <skos:definition xml:lang="no">Retningslinjer som spesifiserer hvilke opplysninger som skal hentes fra eksisterende datakilder som opprinnelig ble samlet for andre formål. For eksempel retningslinjer for hvordan opplysninger fra kvalitative kilder skal velges og kodes for å utarbeide kvantitative datasett.</skos:definition>
      <skos:prefLabel xml:lang="pt">Orientações para a recolha de dados: Guião para recolha de dados secundários</skos:prefLabel>
      <skos:definition xml:lang="pt">Orientações ou instruções que especificam que dados devem ser recolhidos de fontes anteriormente existentes criadas originalmente para outros fins. Por exemplo, instruções sobre como selecionar e codificar dados de fontes qualitativas para criar um conjunto de dados quantitativos.</skos:definition>
      <skos:prefLabel xml:lang="pt">Orientações para a recolha de dados: Guião para recolha de dados secundários</skos:prefLabel>
      <skos:definition xml:lang="pt">Orientações ou instruções que especificam que dados devem ser recolhidos de fontes anteriormente existentes criadas originalmente para outros fins. Por exemplo, instruções sobre como selecionar e codificar dados de fontes qualitativas para criar um conjunto de dados quantitativos.</skos:definition>
      <skos:prefLabel xml:lang="sl">Smernice za zbiranje podatkov: vodnik za zbiranje sekundarnih podatkov</skos:prefLabel>
      <skos:definition xml:lang="sl">Smernice, ki določajo, katere podatke je potrebno zbrati iz že obstoječih virov, ki so bili prvotno ustvarjeni za druge namene. Na primer navodila za izbiranje in kodiranje podatkov iz kakovostnih virov z namenom oblikovanja kvantitativnega nabora podatkov.</skos:definition>
      <skos:prefLabel xml:lang="sl">Smernice za zbiranje podatkov: vodnik za zbiranje sekundarnih podatkov</skos:prefLabel>
      <skos:definition xml:lang="sl">Smernice, ki določajo, katere podatke je potrebno zbrati iz že obstoječih virov, ki so bili prvotno ustvarjeni za druge namene. Na primer navodila za izbiranje in kodiranje podatkov iz kakovostnih virov z namenom oblikovanja kvantitativnega nabora podatkov.</skos:definition>
      <skos:prefLabel xml:lang="sr">Smernice za prikupljanje podataka: Vodič za prikupljanje sekundarnih podataka</skos:prefLabel>
      <skos:definition xml:lang="sr">Smernice koje određuju koji se podaci prikupljaju iz prethodno postojećih izvora prvobitno kreiranih u druge svrhe. Na primer, uputstva o tome kako da odaberete i kodirate podatke iz kvalitativnih izvora kako biste stvorili kvantitativni skup podataka.</skos:definition>
      <skos:prefLabel xml:lang="sr">Smernice za prikupljanje podataka: Vodič za prikupljanje sekundarnih podataka</skos:prefLabel>
      <skos:definition xml:lang="sr">Smernice koje određuju koji se podaci prikupljaju iz prethodno postojećih izvora prvobitno kreiranih u druge svrhe. Na primer, uputstva o tome kako da odaberete i kodirate podatke iz kvalitativnih izvora kako biste stvorili kvantitativni skup podataka.</skos:definition>
      <skos:prefLabel xml:lang="sv">Datainsamlingsguide: Guide för insamling av sekundärdata</skos:prefLabel>
      <skos:definition xml:lang="sv">Guide som anger vilka data som ska samlas in från befintliga källor som ursprungligen skapats för andra ändamål. Till exempel anvisningar om hur man väljer och kodar data från kvalitativa källor för att skapa ett kvantitativt dataset.</skos:definition>
      <skos:prefLabel xml:lang="sv">Datainsamlingsguide: Guide för insamling av sekundärdata</skos:prefLabel>
      <skos:definition xml:lang="sv">Guide som anger vilka data som ska samlas in från befintliga källor som ursprungligen skapats för andra ändamål. Till exempel anvisningar om hur man väljer och kodar data från kvalitativa källor för att skapa ett kvantitativt dataset.</skos:definition>
      <skos:broader rdf:resource="http://rdf-vocabulary.ddialliance.org/cv/TypeOfInstrument/1.1.2/d12e989"/>
   </rdf:Description>
   <rdf:Description rdf:about="http://rdf-vocabulary.ddialliance.org/cv/TypeOfInstrument/1.1.2/d12e1794">
      <rdf:type rdf:resource="http://www.w3.org/2004/02/skos/core#Concept"/>
      <skos:inScheme rdf:resource="http://rdf-vocabulary.ddialliance.org/cv/TypeOfInstrument/1.1.2/"/>
      <skos:notation>ParticipantTasks</skos:notation>
      <skos:prefLabel xml:lang="en">Participant tasks</skos:prefLabel>
      <skos:definition xml:lang="en">A description of tasks that participants are asked to carry out as a part of the data collection process. For example, marking places on a map, taking photographs, telling a fairy tale, etc.</skos:definition>
      <skos:prefLabel xml:lang="en">Participant tasks</skos:prefLabel>
      <skos:definition xml:lang="en">A description of tasks that participants are asked to carry out as a part of the data collection process. For example, marking places on a map, taking photographs, telling a fairy tale, etc.</skos:definition>
      <skos:prefLabel xml:lang="da">Deltageropgaver</skos:prefLabel>
      <skos:definition xml:lang="da">En beskrivelse af opgaver, som deltagerne bliver bedt om at udføre som en del af dataindsamlingsprocessen. For eksempel markering af steder på et kort, tage fotografier, fortælle et eventyr mm.</skos:definition>
      <skos:prefLabel xml:lang="da">Deltageropgaver</skos:prefLabel>
      <skos:definition xml:lang="da">En beskrivelse af opgaver, som deltagerne bliver bedt om at udføre som en del af dataindsamlingsprocessen. For eksempel markering af steder på et kort, tage fotografier, fortælle et eventyr mm.</skos:definition>
      <skos:prefLabel xml:lang="fi">Osallistujatehtävä</skos:prefLabel>
      <skos:definition xml:lang="fi">Osanottajille annettu tehtävänanto, joka on osa aineistonkeruuprosessia. Esimerkiksi: Lempipaikkojen merkitseminen virtuaalikarttaan, valokuvien ottaminen, vitsien tai satujen kertominen.</skos:definition>
      <skos:prefLabel xml:lang="fi">Osallistujatehtävä</skos:prefLabel>
      <skos:definition xml:lang="fi">Osanottajille annettu tehtävänanto, joka on osa aineistonkeruuprosessia. Esimerkiksi: Lempipaikkojen merkitseminen virtuaalikarttaan, valokuvien ottaminen, vitsien tai satujen kertominen.</skos:definition>
      <skos:prefLabel xml:lang="fr">Tâches des participants</skos:prefLabel>
      <skos:definition xml:lang="fr">Une description de tâches que les participants sont invités à effectuer dans le cadre du processus de collecte des données. Par exemple, marquer des endroits sur une carte, prendre des photographies, raconter un conte de fées, etc.</skos:definition>
      <skos:prefLabel xml:lang="fr">Tâches des participants</skos:prefLabel>
      <skos:definition xml:lang="fr">Une description de tâches que les participants sont invités à effectuer dans le cadre du processus de collecte des données. Par exemple, marquer des endroits sur une carte, prendre des photographies, raconter un conte de fées, etc.</skos:definition>
      <skos:prefLabel xml:lang="it">Compiti del partecipante</skos:prefLabel>
      <skos:definition xml:lang="it">Una descrizione delle attività che i partecipanti sono invitati a svolgere come parte del processo di raccolta dei dati. Ad esempio, segnare i luoghi su una mappa, scattare fotografie, raccontare una fiaba, ecc.</skos:definition>
      <skos:prefLabel xml:lang="it">Compiti del partecipante</skos:prefLabel>
      <skos:definition xml:lang="it">Una descrizione delle attività che i partecipanti sono invitati a svolgere come parte del processo di raccolta dei dati. Ad esempio, segnare i luoghi su una mappa, scattare fotografie, raccontare una fiaba, ecc.</skos:definition>
      <skos:prefLabel xml:lang="lt">Užduotys dalyviams</skos:prefLabel>
      <skos:definition xml:lang="lt">Užduočių, kurias dalyvių prašoma atlikti renkant duomenis, aprašas. Pavyzdžiui, pažymėti vietas žemėlapyje, fotografuoti, pasekti pasaką ir kt.</skos:definition>
      <skos:prefLabel xml:lang="lt">Užduotys dalyviams</skos:prefLabel>
      <skos:definition xml:lang="lt">Užduočių, kurias dalyvių prašoma atlikti renkant duomenis, aprašas. Pavyzdžiui, pažymėti vietas žemėlapyje, fotografuoti, pasekti pasaką ir kt.</skos:definition>
      <skos:prefLabel xml:lang="nl">Taken voor de deelnemers</skos:prefLabel>
      <skos:definition xml:lang="nl"/>
      <skos:prefLabel xml:lang="nl">Taken voor de deelnemers</skos:prefLabel>
      <skos:definition xml:lang="nl"/>
      <skos:prefLabel xml:lang="no">Deltakeroppgaver</skos:prefLabel>
      <skos:definition xml:lang="no">En beskrivelse av oppgavene deltakere blir bedt om å utføre som del av datainnsamlingsprosessen. For eksempel markere steder på et kart, ta bilder, fortelle et eventyr, etc.</skos:definition>
      <skos:prefLabel xml:lang="no">Deltakeroppgaver</skos:prefLabel>
      <skos:definition xml:lang="no">En beskrivelse av oppgavene deltakere blir bedt om å utføre som del av datainnsamlingsprosessen. For eksempel markere steder på et kart, ta bilder, fortelle et eventyr, etc.</skos:definition>
      <skos:prefLabel xml:lang="pt">Tarefas para os participantes</skos:prefLabel>
      <skos:definition xml:lang="pt">Descrição das tarefas que os participantes são convidados a realizar como parte do processo de recolha de dados. Por exemplo, marcar lugares num mapa, tirar fotografias, contar uma história infantil, etc.</skos:definition>
      <skos:prefLabel xml:lang="pt">Tarefas para os participantes</skos:prefLabel>
      <skos:definition xml:lang="pt">Descrição das tarefas que os participantes são convidados a realizar como parte do processo de recolha de dados. Por exemplo, marcar lugares num mapa, tirar fotografias, contar uma história infantil, etc.</skos:definition>
      <skos:prefLabel xml:lang="sl">Naloge udeležencev</skos:prefLabel>
      <skos:definition xml:lang="sl">Opis nalog, ki jih morajo udeleženci opraviti kot del postopka zbiranja podatkov. Na primer, označevanje mest na zemljevidu, fotografiranje, pripovedovanje pravljice itd.</skos:definition>
      <skos:prefLabel xml:lang="sl">Naloge udeležencev</skos:prefLabel>
      <skos:definition xml:lang="sl">Opis nalog, ki jih morajo udeleženci opraviti kot del postopka zbiranja podatkov. Na primer, označevanje mest na zemljevidu, fotografiranje, pripovedovanje pravljice itd.</skos:definition>
      <skos:prefLabel xml:lang="sr">Zadaci učesnika</skos:prefLabel>
      <skos:definition xml:lang="sr">Opis zadataka koji se od učesnika traže da izvrše kao deo procesa prikupljanja podataka. Na primer, obeležavanje mesta na mapi, fotografisanje, pričanje bajke itd.</skos:definition>
      <skos:prefLabel xml:lang="sr">Zadaci učesnika</skos:prefLabel>
      <skos:definition xml:lang="sr">Opis zadataka koji se od učesnika traže da izvrše kao deo procesa prikupljanja podataka. Na primer, obeležavanje mesta na mapi, fotografisanje, pričanje bajke itd.</skos:definition>
      <skos:prefLabel xml:lang="sv">Uppgifter för deltagarna</skos:prefLabel>
      <skos:definition xml:lang="sv">En beskrivning av uppgifter som deltagare ombeds att utföra som en del av datainsamlingsprocessen. Till exempel att markera platser på en karta, fotografera, berätta en saga osv.</skos:definition>
      <skos:prefLabel xml:lang="sv">Uppgifter för deltagarna</skos:prefLabel>
      <skos:definition xml:lang="sv">En beskrivning av uppgifter som deltagare ombeds att utföra som en del av datainsamlingsprocessen. Till exempel att markera platser på en karta, fotografera, berätta en saga osv.</skos:definition>
   </rdf:Description>
   <rdf:Description rdf:about="http://rdf-vocabulary.ddialliance.org/cv/TypeOfInstrument/1.1.2/d12e1953">
      <rdf:type rdf:resource="http://www.w3.org/2004/02/skos/core#Concept"/>
      <skos:inScheme rdf:resource="http://rdf-vocabulary.ddialliance.org/cv/TypeOfInstrument/1.1.2/"/>
      <skos:notation>TechnicalInstruments</skos:notation>
      <skos:prefLabel xml:lang="en">Technical instrument(s)</skos:prefLabel>
      <skos:definition xml:lang="en">Instruments used to collect objective data like measurements, images, etc. For example, chronometers, scales, speedometers, blood pressure monitors, thermometers, x-ray machines, etc.</skos:definition>
      <skos:prefLabel xml:lang="en">Technical instrument(s)</skos:prefLabel>
      <skos:definition xml:lang="en">Instruments used to collect objective data like measurements, images, etc. For example, chronometers, scales, speedometers, blood pressure monitors, thermometers, x-ray machines, etc.</skos:definition>
      <skos:prefLabel xml:lang="da">Teknisk(e) instrument(er)</skos:prefLabel>
      <skos:definition xml:lang="da">Instrumenter anvendt til at indsamle objektive data såsom målinger, billeder mm. For eksempel kronometer, vægte, hastighedsmålere, blodtryksmålere, termometre, røntgenapparater mm.</skos:definition>
      <skos:prefLabel xml:lang="da">Teknisk(e) instrument(er)</skos:prefLabel>
      <skos:definition xml:lang="da">Instrumenter anvendt til at indsamle objektive data såsom målinger, billeder mm. For eksempel kronometer, vægte, hastighedsmålere, blodtryksmålere, termometre, røntgenapparater mm.</skos:definition>
      <skos:prefLabel xml:lang="fi">Tekniset keruuvälineet</skos:prefLabel>
      <skos:definition xml:lang="fi">Objektiivisten havaintojen keräämiseen käytetyt välineet. Esimerkiksi verenpainemittarit, röntgenkuvat, ajanmittaus, nopeus- ja lämpötilamittarit jne.</skos:definition>
      <skos:prefLabel xml:lang="fi">Tekniset keruuvälineet</skos:prefLabel>
      <skos:definition xml:lang="fi">Objektiivisten havaintojen keräämiseen käytetyt välineet. Esimerkiksi verenpainemittarit, röntgenkuvat, ajanmittaus, nopeus- ja lämpötilamittarit jne.</skos:definition>
      <skos:prefLabel xml:lang="fr">Instrument(s) technique(s)</skos:prefLabel>
      <skos:definition xml:lang="fr">Instruments utilisé pour collecter des données objectives comme des mesures, des images, etc. Par exemple, chronomètres, balances, compteurs de vitesse, tensiomètres, thermomètres, appareils à rayons X, etc.</skos:definition>
      <skos:prefLabel xml:lang="fr">Instrument(s) technique(s)</skos:prefLabel>
      <skos:definition xml:lang="fr">Instruments utilisé pour collecter des données objectives comme des mesures, des images, etc. Par exemple, chronomètres, balances, compteurs de vitesse, tensiomètres, thermomètres, appareils à rayons X, etc.</skos:definition>
      <skos:prefLabel xml:lang="it">Strumenti tecnici</skos:prefLabel>
      <skos:definition xml:lang="it">Strumenti utilizzati per raccogliere dati oggettivi come misurazioni, immagini, ecc. Ad esempio, cronometri, scale, tachimetri, misuratori della pressione sanguigna, termometri, macchine a raggi X, ecc.</skos:definition>
      <skos:prefLabel xml:lang="it">Strumenti tecnici</skos:prefLabel>
      <skos:definition xml:lang="it">Strumenti utilizzati per raccogliere dati oggettivi come misurazioni, immagini, ecc. Ad esempio, cronometri, scale, tachimetri, misuratori della pressione sanguigna, termometri, macchine a raggi X, ecc.</skos:definition>
      <skos:prefLabel xml:lang="lt">Techninis (-iai) instrumentas (-ai)</skos:prefLabel>
      <skos:definition xml:lang="lt">Instrumentai naudojami objektyviems duomenims (tokiems kaip išmatavimai, nuotraukos ir kt.) rinkti. Pavyzdžiui, chronometrai, svarstyklės, spidometrai, kraujospūdžio matuokliai, termometrai, rentgeno aparatai ir kt.</skos:definition>
      <skos:prefLabel xml:lang="lt">Techninis (-iai) instrumentas (-ai)</skos:prefLabel>
      <skos:definition xml:lang="lt">Instrumentai naudojami objektyviems duomenims (tokiems kaip išmatavimai, nuotraukos ir kt.) rinkti. Pavyzdžiui, chronometrai, svarstyklės, spidometrai, kraujospūdžio matuokliai, termometrai, rentgeno aparatai ir kt.</skos:definition>
      <skos:prefLabel xml:lang="nl">Technische hulpmiddelen</skos:prefLabel>
      <skos:definition xml:lang="nl"/>
      <skos:prefLabel xml:lang="nl">Technische hulpmiddelen</skos:prefLabel>
      <skos:definition xml:lang="nl"/>
      <skos:prefLabel xml:lang="no">Tekniske instrument(er)</skos:prefLabel>
      <skos:definition xml:lang="no">Instrumenter brukt for å samle inn objektive data, slik som mål, bilder, etc. For eksempel kronometre, vekter, speedometre, blodtrykksmonitorer, termometere, røntgenmaskiner, etc.</skos:definition>
      <skos:prefLabel xml:lang="no">Tekniske instrument(er)</skos:prefLabel>
      <skos:definition xml:lang="no">Instrumenter brukt for å samle inn objektive data, slik som mål, bilder, etc. For eksempel kronometre, vekter, speedometre, blodtrykksmonitorer, termometere, røntgenmaskiner, etc.</skos:definition>
      <skos:prefLabel xml:lang="pt">Instrumento(s) técnico(s)</skos:prefLabel>
      <skos:definition xml:lang="pt">Instrumentos usados para recolher dados objetivos, como medições, imagens, etc. Por exemplo, cronómetros, balanças, velocímetros, monitores de pressão arterial, termómetros, máquinas de raio-x, etc.</skos:definition>
      <skos:prefLabel xml:lang="pt">Instrumento(s) técnico(s)</skos:prefLabel>
      <skos:definition xml:lang="pt">Instrumentos usados para recolher dados objetivos, como medições, imagens, etc. Por exemplo, cronómetros, balanças, velocímetros, monitores de pressão arterial, termómetros, máquinas de raio-x, etc.</skos:definition>
      <skos:prefLabel xml:lang="sl">Tehnični inštrument(i)</skos:prefLabel>
      <skos:definition xml:lang="sl">Pripomočki, ki se uporabljajo za zbiranje objektivnih podatkov, kot so meritve, slike itd. Na primer kronometri, lestvice, merilniki hitrosti, naprave za merjenje krvnega tlaka, termometri, rentgen itd.</skos:definition>
      <skos:prefLabel xml:lang="sl">Tehnični inštrument(i)</skos:prefLabel>
      <skos:definition xml:lang="sl">Pripomočki, ki se uporabljajo za zbiranje objektivnih podatkov, kot so meritve, slike itd. Na primer kronometri, lestvice, merilniki hitrosti, naprave za merjenje krvnega tlaka, termometri, rentgen itd.</skos:definition>
      <skos:prefLabel xml:lang="sr">Tehnički instrument(i)</skos:prefLabel>
      <skos:definition xml:lang="sr">Instrumenti koji se koriste za prikupljanje objektivnih podataka kao što su merenja, slike, itd. Na primer, hronometri, vage, brzinomeri, merači krvnog pritiska, termometri, rendgenski aparati, itd.</skos:definition>
      <skos:prefLabel xml:lang="sr">Tehnički instrument(i)</skos:prefLabel>
      <skos:definition xml:lang="sr">Instrumenti koji se koriste za prikupljanje objektivnih podataka kao što su merenja, slike, itd. Na primer, hronometri, vage, brzinomeri, merači krvnog pritiska, termometri, rendgenski aparati, itd.</skos:definition>
      <skos:prefLabel xml:lang="sv">Tekniskt/-a instrument</skos:prefLabel>
      <skos:definition xml:lang="sv">Instrument som används för att samla in objektiva data som mätningar, bilder osv. Till exempel kronometrar, vågar, hastighetsmätare, blodtrycksmätare, termometrar, röntgenapparater osv.</skos:definition>
      <skos:prefLabel xml:lang="sv">Tekniskt/-a instrument</skos:prefLabel>
      <skos:definition xml:lang="sv">Instrument som används för att samla in objektiva data som mätningar, bilder osv. Till exempel kronometrar, vågar, hastighetsmätare, blodtrycksmätare, termometrar, röntgenapparater osv.</skos:definition>
   </rdf:Description>
   <rdf:Description rdf:about="http://rdf-vocabulary.ddialliance.org/cv/TypeOfInstrument/1.1.2/d12e2112">
      <rdf:type rdf:resource="http://www.w3.org/2004/02/skos/core#Concept"/>
      <skos:inScheme rdf:resource="http://rdf-vocabulary.ddialliance.org/cv/TypeOfInstrument/1.1.2/"/>
      <skos:notation>ProgrammingScript</skos:notation>
      <skos:prefLabel xml:lang="en">Programming script</skos:prefLabel>
      <skos:definition xml:lang="en">Programming script written in a data query language that is used to extract specific data, for instance from online social networks.</skos:definition>
      <skos:prefLabel xml:lang="en">Programming script</skos:prefLabel>
      <skos:definition xml:lang="en">Programming script written in a data query language that is used to extract specific data, for instance from online social networks.</skos:definition>
      <skos:prefLabel xml:lang="da">Programmeringsscript</skos:prefLabel>
      <skos:definition xml:lang="da">Programmeringsscript skrevet på et programmeringssprog, der anvendes til at udtrække specifikke data, eksempelvis fra online sociale netværk.</skos:definition>
      <skos:prefLabel xml:lang="da">Programmeringsscript</skos:prefLabel>
      <skos:definition xml:lang="da">Programmeringsscript skrevet på et programmeringssprog, der anvendes til at udtrække specifikke data, eksempelvis fra online sociale netværk.</skos:definition>
      <skos:prefLabel xml:lang="fi">Ohjelmointikoodi</skos:prefLabel>
      <skos:definition xml:lang="fi">Halutun kaltaista dataa on poimittu ohjelmallisesti, esimerkiksi sosiaalisesta mediasta tai muista verkkolähteistä.</skos:definition>
      <skos:prefLabel xml:lang="fi">Ohjelmointikoodi</skos:prefLabel>
      <skos:definition xml:lang="fi">Halutun kaltaista dataa on poimittu ohjelmallisesti, esimerkiksi sosiaalisesta mediasta tai muista verkkolähteistä.</skos:definition>
      <skos:prefLabel xml:lang="fr">Script de programmation</skos:prefLabel>
      <skos:definition xml:lang="fr">Script de programmation écrit dans un langage de requête de données qui est utilisé pour extraire des données spécifiques, par exemple des réseaux sociaux en ligne.</skos:definition>
      <skos:prefLabel xml:lang="fr">Script de programmation</skos:prefLabel>
      <skos:definition xml:lang="fr">Script de programmation écrit dans un langage de requête de données qui est utilisé pour extraire des données spécifiques, par exemple des réseaux sociaux en ligne.</skos:definition>
      <skos:prefLabel xml:lang="it">Script di programmazione</skos:prefLabel>
      <skos:definition xml:lang="it">Script di programmazione sviluppato in un linguaggio di interrogazione dei dati che viene utilizzato per estrarre dati specifici, ad esempio dai social network online.</skos:definition>
      <skos:prefLabel xml:lang="it">Script di programmazione</skos:prefLabel>
      <skos:definition xml:lang="it">Script di programmazione sviluppato in un linguaggio di interrogazione dei dati che viene utilizzato per estrarre dati specifici, ad esempio dai social network online.</skos:definition>
      <skos:prefLabel xml:lang="lt">Programavimo skriptas</skos:prefLabel>
      <skos:definition xml:lang="lt">Programavimo skriptas, parašytas duomenų užklausos kalba, ir naudojamas konkrečių duomenų gavybai, pavyzdžiui, iš internetinių socialinių tinklų.</skos:definition>
      <skos:prefLabel xml:lang="lt">Programavimo skriptas</skos:prefLabel>
      <skos:definition xml:lang="lt">Programavimo skriptas, parašytas duomenų užklausos kalba, ir naudojamas konkrečių duomenų gavybai, pavyzdžiui, iš internetinių socialinių tinklų.</skos:definition>
      <skos:prefLabel xml:lang="nl">Programmeerscript</skos:prefLabel>
      <skos:definition xml:lang="nl"/>
      <skos:prefLabel xml:lang="nl">Programmeerscript</skos:prefLabel>
      <skos:definition xml:lang="nl"/>
      <skos:prefLabel xml:lang="no">Programmeringsskript</skos:prefLabel>
      <skos:definition xml:lang="no">Programmeringsskript som er skrevet i et skriptprogrammeringsspråk som blir brukt til å trekke ut bestemte opplysninger, for eksempel fra sosiale nettverk på internett.</skos:definition>
      <skos:prefLabel xml:lang="no">Programmeringsskript</skos:prefLabel>
      <skos:definition xml:lang="no">Programmeringsskript som er skrevet i et skriptprogrammeringsspråk som blir brukt til å trekke ut bestemte opplysninger, for eksempel fra sosiale nettverk på internett.</skos:definition>
      <skos:prefLabel xml:lang="pt">Script/Esquema de programação</skos:prefLabel>
      <skos:definition xml:lang="pt">Script de programação escrito numa linguagem de pesquisa de dados, que é usado para extrair dados específicos, nomeadamente de redes sociais online.</skos:definition>
      <skos:prefLabel xml:lang="pt">Script/Esquema de programação</skos:prefLabel>
      <skos:definition xml:lang="pt">Script de programação escrito numa linguagem de pesquisa de dados, que é usado para extrair dados específicos, nomeadamente de redes sociais online.</skos:definition>
      <skos:prefLabel xml:lang="sl">Programska koda</skos:prefLabel>
      <skos:definition xml:lang="sl">Koda za programiranje, napisana v jeziku poizvedbe, ki se uporablja za pridobivanje določenih podatkov, na primer iz spletnih socialnih omrežij.</skos:definition>
      <skos:prefLabel xml:lang="sl">Programska koda</skos:prefLabel>
      <skos:definition xml:lang="sl">Koda za programiranje, napisana v jeziku poizvedbe, ki se uporablja za pridobivanje določenih podatkov, na primer iz spletnih socialnih omrežij.</skos:definition>
      <skos:prefLabel xml:lang="sr">Programska skripta</skos:prefLabel>
      <skos:definition xml:lang="sr">Programska skripta napisana na Data Query jeziku (DQL) koja se koriste za izvlačenje određenih podataka, na primer, iz društvenih mreža.</skos:definition>
      <skos:prefLabel xml:lang="sr">Programska skripta</skos:prefLabel>
      <skos:definition xml:lang="sr">Programska skripta napisana na Data Query jeziku (DQL) koja se koriste za izvlačenje određenih podataka, na primer, iz društvenih mreža.</skos:definition>
      <skos:prefLabel xml:lang="sv">Skript</skos:prefLabel>
      <skos:definition xml:lang="sv">Ett skript som är skrivet i ett förfrågningsspråk (data query language) och som används för att extrahera specifika data, t.ex. från sociala nätverk på nätet.</skos:definition>
      <skos:prefLabel xml:lang="sv">Skript</skos:prefLabel>
      <skos:definition xml:lang="sv">Ett skript som är skrivet i ett förfrågningsspråk (data query language) och som används för att extrahera specifika data, t.ex. från sociala nätverk på nätet.</skos:definition>
   </rdf:Description>
   <rdf:Description rdf:about="http://rdf-vocabulary.ddialliance.org/cv/TypeOfInstrument/1.1.2/d12e2271">
      <rdf:type rdf:resource="http://www.w3.org/2004/02/skos/core#Concept"/>
      <skos:inScheme rdf:resource="http://rdf-vocabulary.ddialliance.org/cv/TypeOfInstrument/1.1.2/"/>
      <skos:notation>Other</skos:notation>
      <skos:prefLabel xml:lang="en">Other</skos:prefLabel>
      <skos:definition xml:lang="en">Use when the type of instrument is known, but not found in the list.</skos:definition>
      <skos:prefLabel xml:lang="en">Other</skos:prefLabel>
      <skos:definition xml:lang="en">Use when the type of instrument is known, but not found in the list.</skos:definition>
      <skos:prefLabel xml:lang="da">Andet</skos:prefLabel>
      <skos:definition xml:lang="da">Anvend, når typen af instrument er kendt, men ikke findes i listen.</skos:definition>
      <skos:prefLabel xml:lang="da">Andet</skos:prefLabel>
      <skos:definition xml:lang="da">Anvend, når typen af instrument er kendt, men ikke findes i listen.</skos:definition>
      <skos:prefLabel xml:lang="fi">Muu keruuväline</skos:prefLabel>
      <skos:definition xml:lang="fi">Käytetään jos keruuväline on tiedossa mutta ei listassa.</skos:definition>
      <skos:prefLabel xml:lang="fi">Muu keruuväline</skos:prefLabel>
      <skos:definition xml:lang="fi">Käytetään jos keruuväline on tiedossa mutta ei listassa.</skos:definition>
      <skos:prefLabel xml:lang="fr">Autre</skos:prefLabel>
      <skos:definition xml:lang="fr">Utilisez quand le type d'instrument est connu, mais pas présent dans la liste.</skos:definition>
      <skos:prefLabel xml:lang="fr">Autre</skos:prefLabel>
      <skos:definition xml:lang="fr">Utilisez quand le type d'instrument est connu, mais pas présent dans la liste.</skos:definition>
      <skos:prefLabel xml:lang="it">Altro</skos:prefLabel>
      <skos:definition xml:lang="it">Utilizzare quando il tipo di strumento è conosciuto, ma non è presente nell'elenco.</skos:definition>
      <skos:prefLabel xml:lang="it">Altro</skos:prefLabel>
      <skos:definition xml:lang="it">Utilizzare quando il tipo di strumento è conosciuto, ma non è presente nell'elenco.</skos:definition>
      <skos:prefLabel xml:lang="lt">Kita </skos:prefLabel>
      <skos:definition xml:lang="lt">Naudoti, kai instrumento tipas yra žinomas, bet jo sąraše nėra.</skos:definition>
      <skos:prefLabel xml:lang="lt">Kita </skos:prefLabel>
      <skos:definition xml:lang="lt">Naudoti, kai instrumento tipas yra žinomas, bet jo sąraše nėra.</skos:definition>
      <skos:prefLabel xml:lang="nl">Anders</skos:prefLabel>
      <skos:definition xml:lang="nl"/>
      <skos:prefLabel xml:lang="nl">Anders</skos:prefLabel>
      <skos:definition xml:lang="nl"/>
      <skos:prefLabel xml:lang="no">Annet</skos:prefLabel>
      <skos:definition xml:lang="no">Bruk når instrumenttypen er kjent, men ikke finnes i listen.</skos:definition>
      <skos:prefLabel xml:lang="no">Annet</skos:prefLabel>
      <skos:definition xml:lang="no">Bruk når instrumenttypen er kjent, men ikke finnes i listen.</skos:definition>
      <skos:prefLabel xml:lang="pt">Outro</skos:prefLabel>
      <skos:definition xml:lang="pt">Usar se o tipo de instrumento for conhecido, mas não se encontrar na lista.</skos:definition>
      <skos:prefLabel xml:lang="pt">Outro</skos:prefLabel>
      <skos:definition xml:lang="pt">Usar se o tipo de instrumento for conhecido, mas não se encontrar na lista.</skos:definition>
      <skos:prefLabel xml:lang="sl">Drugo</skos:prefLabel>
      <skos:definition xml:lang="sl">Uporabite, ko je vrsta uporabljenega instrumenta znana, a je ne najdete na seznamu.</skos:definition>
      <skos:prefLabel xml:lang="sl">Drugo</skos:prefLabel>
      <skos:definition xml:lang="sl">Uporabite, ko je vrsta uporabljenega instrumenta znana, a je ne najdete na seznamu.</skos:definition>
      <skos:prefLabel xml:lang="sr">Ostalo</skos:prefLabel>
      <skos:definition xml:lang="sr">Koristiti kada je vrsta instrumenta poznata, ali se ne nalazi na listi.</skos:definition>
      <skos:prefLabel xml:lang="sr">Ostalo</skos:prefLabel>
      <skos:definition xml:lang="sr">Koristiti kada je vrsta instrumenta poznata, ali se ne nalazi na listi.</skos:definition>
      <skos:prefLabel xml:lang="sv">Övrigt</skos:prefLabel>
      <skos:definition xml:lang="sv">Använd när typ av instrument är känt men saknas i listan.</skos:definition>
      <skos:prefLabel xml:lang="sv">Övrigt</skos:prefLabel>
      <skos:definition xml:lang="sv">Använd när typ av instrument är känt men saknas i listan.</skos:definition>
   </rdf:Description>
</rdf:RDF>
