<?xml version="1.0" encoding="UTF-8"?>
<rdf:RDF xmlns:rdf="http://www.w3.org/1999/02/22-rdf-syntax-ns#"
         xmlns:rdfs="http://www.w3.org/2000/01/rdf-schema#"
         xmlns:skos="http://www.w3.org/2004/02/skos/core#"
         xmlns:owl="http://www.w3.org/2002/07/owl#"
         xmlns:dcterms="http://purl.org/dc/terms/">
   <rdf:Description rdf:about="http://rdf-vocabulary.ddialliance.org/cv/ModeOfCollection/3.0">
      <rdf:type rdf:resource="http://www.w3.org/2004/02/skos/core#ConceptScheme"/>
      <dcterms:isVersionOf rdf:resource="http://rdf-vocabulary.ddialliance.org/cv/ModeOfCollection"/>
      <skos:notation>ModeOfCollection</skos:notation>
      <skos:prefLabel xml:lang="en">Mode Of Collection</skos:prefLabel>
      <skos:prefLabel xml:lang="da">Indsamlingsmetode</skos:prefLabel>
      <skos:prefLabel xml:lang="fi">Keruumenetelmä</skos:prefLabel>
      <skos:prefLabel xml:lang="fr">Mode de collecte</skos:prefLabel>
      <skos:prefLabel xml:lang="fr">Mode de collecte</skos:prefLabel>
      <skos:prefLabel xml:lang="it">Metodo di raccolta dei dati</skos:prefLabel>
      <skos:prefLabel xml:lang="no">Innsamlingsmetode</skos:prefLabel>
      <skos:prefLabel xml:lang="pt">Método de recolha de dados</skos:prefLabel>
      <skos:prefLabel xml:lang="sl">Način zbiranja podatkov</skos:prefLabel>
      <skos:prefLabel xml:lang="sr">Način prikupljanja</skos:prefLabel>
      <skos:prefLabel xml:lang="sv">Insamlingsmetod</skos:prefLabel>
      <skos:definition xml:lang="en">The procedure, technique, or mode of inquiry used to attain the data.</skos:definition>
      <skos:definition xml:lang="da">Fremgangsmåden, teknikken eller undersøgelsesmetoden, der er anvendt til at opnå dataene.</skos:definition>
      <skos:definition xml:lang="fi">Kuvailtavan aineiston ensisijainen keruumenetelmä.</skos:definition>
      <skos:definition xml:lang="fr">La procédure, la technique ou le mode d'enquête utilisé pour obtenir les données.</skos:definition>
      <skos:definition xml:lang="fr">La procédure, la technique ou le mode d'enquête utilisé pour obtenir les données.</skos:definition>
      <skos:definition xml:lang="it">La procedura, la tecnica o la modalità di indagine utilizzata per ottenere i dati.</skos:definition>
      <skos:definition xml:lang="no">Framgangsmåten, teknikken, eller metoden som er anvendt for å samle inn data.</skos:definition>
      <skos:definition xml:lang="pt">Procedimentos, técnicas ou métodos de recolha de dados.</skos:definition>
      <skos:definition xml:lang="sl">Postopki, tehnike ali načini raziskovanja, uporabljeni za pridobivanje podatkov.</skos:definition>
      <skos:definition xml:lang="sr">Postupak, tehnika ili način ispitivanja koji se koristi za dobijanje podataka.</skos:definition>
      <skos:definition xml:lang="sv">Den process, metod eller teknik som användes för att samla in data.</skos:definition>
      <owl:versionInfo>3.0</owl:versionInfo>
      <dcterms:license rdf:resource="Creative Commons Attribution 4.0 International"/>
      <dcterms:rights>Copyright ©DDI Alliance 2020</dcterms:rights>
      <skos:hasTopConcept rdf:resource="http://rdf-vocabulary.ddialliance.org/cv/ModeOfCollection/3.0/d64e136"/>
      <skos:hasTopConcept rdf:resource="http://rdf-vocabulary.ddialliance.org/cv/ModeOfCollection/3.0/d64e874"/>
      <skos:hasTopConcept rdf:resource="http://rdf-vocabulary.ddialliance.org/cv/ModeOfCollection/3.0/d64e1426"/>
      <skos:hasTopConcept rdf:resource="http://rdf-vocabulary.ddialliance.org/cv/ModeOfCollection/3.0/d64e1794"/>
      <skos:hasTopConcept rdf:resource="http://rdf-vocabulary.ddialliance.org/cv/ModeOfCollection/3.0/d64e2162"/>
      <skos:hasTopConcept rdf:resource="http://rdf-vocabulary.ddialliance.org/cv/ModeOfCollection/3.0/d64e2900"/>
      <skos:hasTopConcept rdf:resource="http://rdf-vocabulary.ddialliance.org/cv/ModeOfCollection/3.0/d64e3268"/>
      <skos:hasTopConcept rdf:resource="http://rdf-vocabulary.ddialliance.org/cv/ModeOfCollection/3.0/d64e3819"/>
      <skos:hasTopConcept rdf:resource="http://rdf-vocabulary.ddialliance.org/cv/ModeOfCollection/3.0/d64e3909"/>
      <skos:hasTopConcept rdf:resource="http://rdf-vocabulary.ddialliance.org/cv/ModeOfCollection/3.0/d64e3999"/>
      <skos:hasTopConcept rdf:resource="http://rdf-vocabulary.ddialliance.org/cv/ModeOfCollection/3.0/d64e4089"/>
      <skos:hasTopConcept rdf:resource="http://rdf-vocabulary.ddialliance.org/cv/ModeOfCollection/3.0/d64e4179"/>
      <skos:hasTopConcept rdf:resource="http://rdf-vocabulary.ddialliance.org/cv/ModeOfCollection/3.0/d64e4269"/>
      <skos:hasTopConcept rdf:resource="http://rdf-vocabulary.ddialliance.org/cv/ModeOfCollection/3.0/d64e4360"/>
      <skos:hasTopConcept rdf:resource="http://rdf-vocabulary.ddialliance.org/cv/ModeOfCollection/3.0/d64e4727"/>
   </rdf:Description>
   <rdf:Description rdf:about="http://rdf-vocabulary.ddialliance.org/cv/ModeOfCollection/3.0/d64e136">
      <rdf:type rdf:resource="http://www.w3.org/2004/02/skos/core#Concept"/>
      <skos:inScheme rdf:resource="http://rdf-vocabulary.ddialliance.org/cv/ModeOfCollection/3.0"/>
      <skos:notation>Interview</skos:notation>
      <skos:prefLabel xml:lang="en">Interview</skos:prefLabel>
      <skos:definition xml:lang="en">A pre-planned communication between two (or more) people - the interviewer(s) and the interviewee(s) - in which information is obtained by the interviewer(s) from the interviewee(s). If group interaction is part of the method, use "Focus group".</skos:definition>
      <skos:prefLabel xml:lang="da">Interview</skos:prefLabel>
      <skos:definition xml:lang="da">En forudplanlagt kommunikation mellem to (eller flere) personer – interviewere(n) og de(n) interviewede - hvor intervieweren(ne) får information fra de(n) interviewede. Hvis gruppeinteraktion er en del af metoden, anvend ”Fokusgruppe”.</skos:definition>
      <skos:prefLabel xml:lang="fi">Haastattelu</skos:prefLabel>
      <skos:definition xml:lang="fi">Ennalta suunniteltu, haastattelijan ja yhden tai useamman haastateltavan välinen keskustelu, jossa haastattelija saa tietoa tutkimustarkoituksiin. Käytä tarkempaa haastattelutermiä, mikäli mahdollista. Jos haastateltavia on enemmän kuin yksi ja ryhmän keskinäinen vuorovaikutus on tärkeää, käytetään termiä 'Kohderyhmäkeskustelu'.</skos:definition>
      <skos:prefLabel xml:lang="fr">Entretien</skos:prefLabel>
      <skos:definition xml:lang="fr">Un échange prévu entre deux (ou plusieurs) personnes - l(es) enquêteur(s) et l(es) enquêté(s) - dans lequel des informations sont obtenus par l(es) enquêteur(s) d(es) enquêté(s). Si l'interaction de groupe fait partie de la méthode, utilisez "Focus group"</skos:definition>
      <skos:prefLabel xml:lang="fr">Entretien</skos:prefLabel>
      <skos:definition xml:lang="fr">Un échange prévu entre deux (ou plusieurs) personnes - l(es) enquêteur(s) et l(es) enquêté(s) - dans lequel des informations sont obtenus par l(es) enquêteur(s) d(es) enquêté(s). Si l'interaction de groupe fait partie de la méthode, utilisez "Focus group"</skos:definition>
      <skos:prefLabel xml:lang="it">Intervista</skos:prefLabel>
      <skos:definition xml:lang="it">Una comunicazione pianificata tra due (o più) persone - l'intervistatore/i e l'intervistato/i - in cui le informazioni ottenute dall'intervistatore sono state rilasciate dagli intervistati. Se l'interazione di gruppo è parte della tecnica, utilizzare "Focus group".</skos:definition>
      <skos:prefLabel xml:lang="no">Intervju</skos:prefLabel>
      <skos:definition xml:lang="no">En forhåndsbestemt kommunikasjon mellom to (eller flere) personer – intervjueren(e) og intervjuobjekt(et/ene) – hvor intervjueren(e) henter informasjon fra intervjuobjekt(et/ene). Dersom gruppeinteraksjoner er del av metoden, bruk 'Fokusgruppe'.</skos:definition>
      <skos:prefLabel xml:lang="pt">Entrevista</skos:prefLabel>
      <skos:definition xml:lang="pt">Uma comunicação pré-planeada entre duas (ou mais) pessoas - o(s) entrevistador(es) e o(s) entrevistado(s) - em que a informação é obtida pelo(s) entrevistador(es) do(s) entrevistado(s). Se a interação no grupo fizer parte do método, usar "Focus group".</skos:definition>
      <skos:prefLabel xml:lang="sl">Intervju</skos:prefLabel>
      <skos:definition xml:lang="sl">Vnaprej načrtovana komunikacija med dvema (ali več) osebami - spraševalcem(-ci) in spraševancem(-ci) -, kjer spraševalec(-ci) pridobi(jo) informacije s strani spraševanca(-cev). Če je v metodo vključena skupinska interakcija, uporabite izraz "fokusna skupina".</skos:definition>
      <skos:prefLabel xml:lang="sr">Intervju</skos:prefLabel>
      <skos:definition xml:lang="sr">Unapred planirana komunikacija između dve (ili više) osoba - anketara i sagovornika (anketiranog), u kojoj informacije dobija anketar od anketiranog. Ukoliko je grupna interakcija deo ove metode, koristite termin „Fokus grupa“.</skos:definition>
      <skos:prefLabel xml:lang="sv">Intervju</skos:prefLabel>
      <skos:definition xml:lang="sv">Planerad kommunikation mellan två (eller flera) personer – intervjuaren/-na och intervjuobjektet/-en – där intervjuaren/-na får information från intervjuobjektet/-en. Om gruppinteraktion är del av metoden, använd "Fokusgrupp".</skos:definition>
      <skos:narrower rdf:resource="http://rdf-vocabulary.ddialliance.org/cv/ModeOfCollection/3.0/d64e235"/>
      <skos:narrower rdf:resource="http://rdf-vocabulary.ddialliance.org/cv/ModeOfCollection/3.0/d64e511"/>
      <skos:narrower rdf:resource="http://rdf-vocabulary.ddialliance.org/cv/ModeOfCollection/3.0/d64e694"/>
      <skos:narrower rdf:resource="http://rdf-vocabulary.ddialliance.org/cv/ModeOfCollection/3.0/d64e784"/>
   </rdf:Description>
   <rdf:Description rdf:about="http://rdf-vocabulary.ddialliance.org/cv/ModeOfCollection/3.0/d64e235">
      <rdf:type rdf:resource="http://www.w3.org/2004/02/skos/core#Concept"/>
      <skos:inScheme rdf:resource="http://rdf-vocabulary.ddialliance.org/cv/ModeOfCollection/3.0"/>
      <skos:notation>Interview.FaceToFace</skos:notation>
      <skos:prefLabel xml:lang="en">Face-to-face interview</skos:prefLabel>
      <skos:definition xml:lang="en">Data collection method in which a live interviewer conducts a personal interview, presenting questions and entering the responses. Use this broader term if not CAPI or PAPI, or if not known whether CAPI/PAPI or not.</skos:definition>
      <skos:prefLabel xml:lang="da">Personligt interview</skos:prefLabel>
      <skos:definition xml:lang="da">Dataindsamlingsmetode, hvor en tilstedeværende interviewer foretager et personligt interview, stiller spørgsmål og noterer svar. Brug dette bredere begreb, hvis det ikke er CAPI eller PAPI, eller hvis det ikke vides, om det er CAPI eller PAPI.</skos:definition>
      <skos:prefLabel xml:lang="fi">Kasvokkainen haastattelu</skos:prefLabel>
      <skos:definition xml:lang="fi">Kasvokkain tehty yksilö- tai ryhmähaastattelu, jossa haastattelija esittää kysymykset ja taltioi vastaukset. Käytetään silloin, kun haastattelija tallentaa saamansa tiedot haastattelumuistiinpanoilla, tai haastattelu äänitetään tai videoidaan (eli ei mene mihinkään kasvokkaisen haastattelun alaluokkaan).</skos:definition>
      <skos:prefLabel xml:lang="fr">Entretien en face-à-face</skos:prefLabel>
      <skos:definition xml:lang="fr">Méthode de recueil de données dans laquelle un enquêteur conduit un entretien personnel, posant des questions et écrivant les réponses. Utilisez ce terme si pas CAPI ou PAPI, ou si vous ne savez pas si CAPI/PAPI ou pas.</skos:definition>
      <skos:prefLabel xml:lang="fr">Entretien en face-à-face</skos:prefLabel>
      <skos:definition xml:lang="fr">Méthode de recueil de données dans laquelle un enquêteur conduit un entretien personnel, posant des questions et écrivant les réponses. Utilisez ce terme si pas CAPI ou PAPI, ou si vous ne savez pas si CAPI/PAPI ou pas.</skos:definition>
      <skos:prefLabel xml:lang="it">Intervista faccia a faccia</skos:prefLabel>
      <skos:definition xml:lang="it">Tecnica di raccolta dei dati in cui un intervistatore conduce un colloquio personale in presenza, facendo domande e registrando le risposte. Utilizzare questo termine più ampio se l'intervista non è CAPI o PAPI, o se non si è in grado di stabilire se sia CAPI o PAPI.</skos:definition>
      <skos:prefLabel xml:lang="no">Personlig intervju</skos:prefLabel>
      <skos:definition xml:lang="no">Datainnsamlingsmetode hvor en tilstedeværende intervjuer gjennomfører et personlig intervju, presenterer spørsmål og registrerer svarene. Bruk dette bredere begrepet dersom det ikke er CATI eller PAPI, eller dersom det er uvisst om det er CATI/PAPI.</skos:definition>
      <skos:prefLabel xml:lang="pt">Entrevista presencial</skos:prefLabel>
      <skos:definition xml:lang="pt">Método de recolha de dados em que um entrevistador presencial realiza uma entrevista pessoal, colocando as perguntas e inserindo as respostas. Usar este termo mais amplo se não for CAPI ou PAPI, ou se não souber se é CAPI/PAPI.</skos:definition>
      <skos:prefLabel xml:lang="sl">Osebni intervju</skos:prefLabel>
      <skos:definition xml:lang="sl">Metoda zbiranja podatkov, kjer spraševalec izvede osebni intervju, postavlja vprašanja in vnese odgovore. Uporabite ta širši izraz, če ne morete uporabiti CAPI ali PAPI ozioma ni znano, ali gre za CAPI/PAPI.</skos:definition>
      <skos:prefLabel xml:lang="sr">Intervju licem u lice</skos:prefLabel>
      <skos:definition xml:lang="sr">Način prikupljanja podataka u kojem anketar uživo vodi usmeni razgovor, postavljajući pitanja i unoseći odgovore. Koristite ovaj širi pojam ukoliko nije tačno navedno da se radi o CAPI (Intervju licem u lice: podržan računarom) ili PAPI (Intervju licem u lice: beleži se na papiru) ili ukoliko vama nije poznato da li je u pitanju CAPI ili PAPI.</skos:definition>
      <skos:prefLabel xml:lang="sv">Personlig intervju</skos:prefLabel>
      <skos:definition xml:lang="sv">En närvarande intervjuare genomför en personlig intervju genom att ställa frågor och notera svaren. Använd denna bredare term om det inte rör sig om CAPI eller PAPI, eller om det inte är känt huruvida det rör sig om CAPI/PAPI eller inte.</skos:definition>
      <skos:narrower rdf:resource="http://rdf-vocabulary.ddialliance.org/cv/ModeOfCollection/3.0/d64e330"/>
      <skos:narrower rdf:resource="http://rdf-vocabulary.ddialliance.org/cv/ModeOfCollection/3.0/d64e420"/>
      <skos:broader rdf:resource="http://rdf-vocabulary.ddialliance.org/cv/ModeOfCollection/3.0/d64e136"/>
   </rdf:Description>
   <rdf:Description rdf:about="http://rdf-vocabulary.ddialliance.org/cv/ModeOfCollection/3.0/d64e330">
      <rdf:type rdf:resource="http://www.w3.org/2004/02/skos/core#Concept"/>
      <skos:inScheme rdf:resource="http://rdf-vocabulary.ddialliance.org/cv/ModeOfCollection/3.0"/>
      <skos:notation>Interview.FaceToFace.CAPIorCAMI</skos:notation>
      <skos:prefLabel xml:lang="en">Face-to-face interview: Computer-assisted (CAPI/CAMI)</skos:prefLabel>
      <skos:definition xml:lang="en">Computer-assisted personal interviewing (CAPI), or computer-assisted mobile interviewing (CAMI). Data collection method in which the interviewer reads questions to the respondents from the screen of a computer, laptop, or a mobile device like tablet or smartphone, and enters the answers in the same device. The administration of the interview is managed by a specifically designed program/application.</skos:definition>
      <skos:prefLabel xml:lang="da">Personligt interview: Computerassisteret (CAPI/CAMI)</skos:prefLabel>
      <skos:definition xml:lang="da">Computer-assisted personal interviewing (CAPI) eller computer-assisted mobile interviewing (CAMI). Dataindsamlingsmetode, hvor intervieweren læser spørgsmål op til respondenterne fra skærmen på en computer, bærbar eller en mobil enhed såsom tablet eller smartphone og indtaster svarene på den samme enhed. Administrationen af interviewet styres af et specifikt designet program/applikation.</skos:definition>
      <skos:prefLabel xml:lang="fi">Kasvokkainen haastattelu: tietokoneavusteinen (CAPI tai CAMI)</skos:prefLabel>
      <skos:definition xml:lang="fi">Computer-assisted personal interviewing (CAPI) tai Computer-assisted mobile interviewing (CAMI). Haastattelija lukee kysymykset kannettavalta tietokoneelta, kämmentietokoneelta, tabletista tai älypuhelimesta ja tallentaa haastateltavan vastaukset suoraan laitteeseen.</skos:definition>
      <skos:prefLabel xml:lang="fr">Entretien en face-à-face : assisté par ordinateur (CAPI / CAMI)</skos:prefLabel>
      <skos:definition xml:lang="fr">Entretien assisté par ordinateur (CAPI), ou entretien assisté par un appareil mobile (CAMI). Méthode de collecte des données dans laquelle l'enquêteur lit les questions aux répondants depuis l'écran d'un ordinateur, d'un ordinateur portable ou d'un appareil mobile tel qu'une tablette ou un smartphone, et entre les réponses sur le même appareil. L'administration de l'entretien est géré par un programme / application spécialement conçue.</skos:definition>
      <skos:prefLabel xml:lang="fr">Entretien en face-à-face : assisté par ordinateur (CAPI / CAMI)</skos:prefLabel>
      <skos:definition xml:lang="fr">Entretien assisté par ordinateur (CAPI), ou entretien assisté par un appareil mobile (CAMI). Méthode de collecte des données dans laquelle l'enquêteur lit les questions aux répondants depuis l'écran d'un ordinateur, d'un ordinateur portable ou d'un appareil mobile tel qu'une tablette ou un smartphone, et entre les réponses sur le même appareil. L'administration de l'entretien est géré par un programme / application spécialement conçue.</skos:definition>
      <skos:prefLabel xml:lang="it">Intervista faccia a faccia: computer-assistita (CAPI/CAMI)</skos:prefLabel>
      <skos:definition xml:lang="it">Interviste personali assistite da computer (CAPI) o da cellulare (CAMI). Metodo di raccolta dei dati in cui l'intervistatore legge le domande ai rispondenti dallo schermo di un computer, laptop o dispositivo mobile come un tablet o uno smartphone e inserisce le risposte nello stesso dispositivo. L'intervista è gestita da un programma/applicazione appositamente progettata.</skos:definition>
      <skos:prefLabel xml:lang="no">Personlig intervju: CAPI/CAMI</skos:prefLabel>
      <skos:definition xml:lang="no">Dataassistert personlig intervjuing (CAPI). Datainnsamlingsmetode hvor intervjueren leser opp spørsmål for respondenten fra skjermen til en datamaskin, bærbar datamaskin, smarttelefon eller nettbrett, og registrerer svarene på det samme apparatet. Administreringen av intervjuet er styrt av et spesialdesignet program eller en applikasjon.</skos:definition>
      <skos:prefLabel xml:lang="pt">Entrevista presencial: Assistida por computador (CAPI/CAMI)</skos:prefLabel>
      <skos:definition xml:lang="pt">Entrevista pessoal assistida por computador (Computer Assisted Personal Interviewing - CAPI) ou entrevista móvel assistida por computador (Computer Assisted Mobile Interviewing - CAMI). Modo de recolha de dados em que o entrevistador lê perguntas aos entrevistados na tela de um computador, laptop ou dispositivo móvel, como tablet ou smartphone, e insere as respostas no mesmo dispositivo. A administração da entrevista é gerida por um programa especialmente elaborado para o efeito.</skos:definition>
      <skos:prefLabel xml:lang="sl">Osebni intervju: CAPI/CAMI</skos:prefLabel>
      <skos:definition xml:lang="sl">Računalniško podprto osebno intervjuvanje (CAPI). Metoda zbiranja podatkov, kjer spraševalec prebere vprašanja spraševancu z zaslona na računalniku, prenosnem računalniku ali mobilni napravi, kot na primer na tablici ali pametnemu telefonu, in vnese odgovore v isto napravo. Intervju izvedemo s pomočjo posebej zasnovanega programa/ aplikacije.</skos:definition>
      <skos:prefLabel xml:lang="sr">Intervju licem u lice: Podržan računarom (CAPI/CAMI)</skos:prefLabel>
      <skos:definition xml:lang="sr">Računarsko lično intervjuisanje (CAPI) ili računarsko potpomognuto mobilno intervjuisanje (CAMI). Način prikupljanja podataka u kojem anketar čita pitanja anketiranima sa ekrana računara, laptopa ili mobilnog uređaja poput tableta ili pametnog telefona i unosi odgovore u isti uređaj. Administriranjem intervjua upravlja se posebno dizajniranim programom / aplikacijom.</skos:definition>
      <skos:prefLabel xml:lang="sv">Personlig intervju: CAPI/CAMI</skos:prefLabel>
      <skos:definition xml:lang="sv">Datorstödd personlig intervju. Intervjuaren läser frågor för respondenterna från en datorskärm eller mobil enhet (t.ex. surfplatta eller mobiltelefon) och skriver in svaren direkt i datorn. Intervjun hanteras med ett program som utvecklats för detta syfte.</skos:definition>
      <skos:broader rdf:resource="http://rdf-vocabulary.ddialliance.org/cv/ModeOfCollection/3.0/d64e235"/>
   </rdf:Description>
   <rdf:Description rdf:about="http://rdf-vocabulary.ddialliance.org/cv/ModeOfCollection/3.0/d64e420">
      <rdf:type rdf:resource="http://www.w3.org/2004/02/skos/core#Concept"/>
      <skos:inScheme rdf:resource="http://rdf-vocabulary.ddialliance.org/cv/ModeOfCollection/3.0"/>
      <skos:notation>Interview.FaceToFace.PAPI</skos:notation>
      <skos:prefLabel xml:lang="en">Face-to-face interview: Paper-and-pencil (PAPI)</skos:prefLabel>
      <skos:definition xml:lang="en">Paper-and-pencil interviewing (PAPI). The interviewer uses a traditional paper questionnaire to read the questions and enter the answers.</skos:definition>
      <skos:prefLabel xml:lang="da">Personligt interview: Papir og pen (PAPI)</skos:prefLabel>
      <skos:definition xml:lang="da">Paper-and-pencil interviewing (PAPI). Intervieweren anvender et traditionelt spørgeskema på papir til at oplæse spørgsmålene og registrere svarene.</skos:definition>
      <skos:prefLabel xml:lang="fi">Kasvokkainen haastattelu: paperikyselylomake (PAPI)</skos:prefLabel>
      <skos:definition xml:lang="fi">Paper-and-pencil interviewing (PAPI). Paperilomaketta käyttäen tehty henkilökohtainen haastattelu. Haastattelija lukee kysymykset paperilomakkeelta ja kirjoittaa haastateltavan vastaukset lomakkeelle.</skos:definition>
      <skos:prefLabel xml:lang="fr">Entretien en face-à-face : papier et crayon (PAPI)</skos:prefLabel>
      <skos:definition xml:lang="fr">Entretien avec papier et crayon (PAPI). L'enquêteur utilise un questionnaire papier traditionnel pour lire les questions et écrire les réponses.</skos:definition>
      <skos:prefLabel xml:lang="fr">Entretien en face-à-face : papier et crayon (PAPI)</skos:prefLabel>
      <skos:definition xml:lang="fr">Entretien avec papier et crayon (PAPI). L'enquêteur utilise un questionnaire papier traditionnel pour lire les questions et écrire les réponses.</skos:definition>
      <skos:prefLabel xml:lang="it">Intervista faccia a faccia: carta e penna (PAPI)</skos:prefLabel>
      <skos:definition xml:lang="it">Interviste con carta e penna (PAPI). L'intervistatore utilizza un tradizionale questionario cartaceo per leggere le domande e inserire le risposte.</skos:definition>
      <skos:prefLabel xml:lang="no">Personlig intervju: PAPI</skos:prefLabel>
      <skos:definition xml:lang="no">Penn og papir intervju. Intervjueren bruker et tradisjonelt papirspørreskjema for å lese opp spørsmålene og til å registrere svarene.</skos:definition>
      <skos:prefLabel xml:lang="pt">Entrevista presencial: Papel e lápis (PAPI)</skos:prefLabel>
      <skos:definition xml:lang="pt">Entrevista de papel e lápis (PAPI - Paper-and-pencil interviewing). O entrevistador usa um questionário tradicional em papel para ler as perguntas e inserir as respostas.</skos:definition>
      <skos:prefLabel xml:lang="sl">Osebni intervju: PAPI</skos:prefLabel>
      <skos:definition xml:lang="sl">"Intervjuvanje s papirjem in svinčnikom". Spraševalec uporabi tradicionalni papirnati vprašalnik, s katerega prebere vprašanja in vnese odgovore.</skos:definition>
      <skos:prefLabel xml:lang="sr">Intervju licem u lice: beleži se na papiru (PAPI)</skos:prefLabel>
      <skos:definition xml:lang="sr">Intervju sa papirom i olovkom (PAPI). Anketar koristi tradicionalni papirni upitnik za čitanje pitanja i unos odgovora.</skos:definition>
      <skos:prefLabel xml:lang="sv">Personlig intervju: PAPI</skos:prefLabel>
      <skos:definition xml:lang="sv">Papper-och-penna-intervju. Intervjuaren använder ett traditionellt frågeformulär på papper för att läsa frågorna och skriva ned svaren.</skos:definition>
      <skos:broader rdf:resource="http://rdf-vocabulary.ddialliance.org/cv/ModeOfCollection/3.0/d64e235"/>
   </rdf:Description>
   <rdf:Description rdf:about="http://rdf-vocabulary.ddialliance.org/cv/ModeOfCollection/3.0/d64e511">
      <rdf:type rdf:resource="http://www.w3.org/2004/02/skos/core#Concept"/>
      <skos:inScheme rdf:resource="http://rdf-vocabulary.ddialliance.org/cv/ModeOfCollection/3.0"/>
      <skos:notation>Interview.Telephone</skos:notation>
      <skos:prefLabel xml:lang="en">Telephone interview</skos:prefLabel>
      <skos:definition xml:lang="en">Interview administered on the telephone. Use this broader term if not CATI, or if not known whether CATI or not.</skos:definition>
      <skos:prefLabel xml:lang="da">Telefoninterview</skos:prefLabel>
      <skos:definition xml:lang="da">Interview gennemført over telefon. Brug dette bredere begreb, hvis det ikke er CATI, eller hvis det ikke vides, om det er CATI.</skos:definition>
      <skos:prefLabel xml:lang="fi">Puhelinhaastattelu</skos:prefLabel>
      <skos:definition xml:lang="fi">Puhelimitse tehty haastattelu. Termiä voi käyttää sekä kvalitatiivisesta että kvantitatiivisesta haastattelusta.</skos:definition>
      <skos:prefLabel xml:lang="fr">Entretien téléphonique</skos:prefLabel>
      <skos:definition xml:lang="fr">Entretien administré par téléphone. Utilisez ce terme si pas CATI, ou si vous ne savez pas si CATI ou pas.</skos:definition>
      <skos:prefLabel xml:lang="fr">Entretien téléphonique</skos:prefLabel>
      <skos:definition xml:lang="fr">Entretien administré par téléphone. Utilisez ce terme si pas CATI, ou si vous ne savez pas si CATI ou pas.</skos:definition>
      <skos:prefLabel xml:lang="it">Intervista telefonica</skos:prefLabel>
      <skos:definition xml:lang="it">Intervista somministrata via telefono. Utilizzare questo termine più generale se non è CATI, o se non si è in grado di stabilire se lo sia.</skos:definition>
      <skos:prefLabel xml:lang="no">Telefonintervju</skos:prefLabel>
      <skos:definition xml:lang="no">Intervju som gjennomføres over telefon. Bruk dette bredere begrepet dersom det ikke er CATI, eller dersom det er uvisst om det er CATI.</skos:definition>
      <skos:prefLabel xml:lang="pt">Entrevista telefónica</skos:prefLabel>
      <skos:definition xml:lang="pt">Entrevista realizada pelo telefone. Usar este termo mais amplo se não for CATI, ou se não souber se é CATI ou não.</skos:definition>
      <skos:prefLabel xml:lang="sl">Telefonski intervju</skos:prefLabel>
      <skos:definition xml:lang="sl">Intervju, izveden preko telefona. Uporabite ta širši izraz, če ni CATI, oziroma ne veste, ali je CATI ali ne.</skos:definition>
      <skos:prefLabel xml:lang="sr">Telefonski upitnik</skos:prefLabel>
      <skos:definition xml:lang="sr">Intervju administriran telefonom. Koristite ovaj širi pojam ukoliko nije spcifikovano da je u pitanu telefonski upitnik podržan računarom (CATI) ili ako vam nije poznato koji tip telefonskog upitnika je korišćen.</skos:definition>
      <skos:prefLabel xml:lang="sv">Telefonintervju</skos:prefLabel>
      <skos:definition xml:lang="sv">Intervju som genomförs över telefon. Använd denna bredare term om det inte rör sig om CATI, eller om det inte är känt huruvida det rör sig om CATI.</skos:definition>
      <skos:narrower rdf:resource="http://rdf-vocabulary.ddialliance.org/cv/ModeOfCollection/3.0/d64e604"/>
      <skos:broader rdf:resource="http://rdf-vocabulary.ddialliance.org/cv/ModeOfCollection/3.0/d64e136"/>
   </rdf:Description>
   <rdf:Description rdf:about="http://rdf-vocabulary.ddialliance.org/cv/ModeOfCollection/3.0/d64e604">
      <rdf:type rdf:resource="http://www.w3.org/2004/02/skos/core#Concept"/>
      <skos:inScheme rdf:resource="http://rdf-vocabulary.ddialliance.org/cv/ModeOfCollection/3.0"/>
      <skos:notation>Interview.Telephone.CATI</skos:notation>
      <skos:prefLabel xml:lang="en">Telephone interview: Computer-assisted (CATI)</skos:prefLabel>
      <skos:definition xml:lang="en">Computer-assisted telephone interviewing (CATI). The interviewer asks questions as directed by a computer, responses are keyed directly into the computer and the administration of the interview is managed by a specifically designed program.</skos:definition>
      <skos:prefLabel xml:lang="da">Telefoninterview: Computerassisteret (CATI)</skos:prefLabel>
      <skos:definition xml:lang="da">Computer-assisted telephone interviewing (CATI). Intervieweren stiller spørgsmål ved hjælp af en computer, svarene indtastes direkte i computeren, og administrationen af interviewet styres af et specifikt designet program.</skos:definition>
      <skos:prefLabel xml:lang="fi">Puhelinhaastattelu: tietokoneavusteinen (CATI)</skos:prefLabel>
      <skos:definition xml:lang="fi">Computer-assisted telephone interviewing (CATI). Haastattelija lukee kysymykset tietokoneelta puhelimessa ja tallentaa haastateltavan vastaukset suoraan tietokoneelle.</skos:definition>
      <skos:prefLabel xml:lang="fr">Entretien téléphonique : assisté par ordinateur (CATI)</skos:prefLabel>
      <skos:definition xml:lang="fr">Entretien téléphonique assisté par ordinateur (CATI). L'enquêteur pose des questions selon les directives de l'ordinateur, des réponses sont saisies directement dans l'ordinateur et l'administration de l'entretien est géré pas un programme spécialement conçu.</skos:definition>
      <skos:prefLabel xml:lang="fr">Entretien téléphonique : assisté par ordinateur (CATI)</skos:prefLabel>
      <skos:definition xml:lang="fr">Entretien téléphonique assisté par ordinateur (CATI). L'enquêteur pose des questions selon les directives de l'ordinateur, des réponses sont saisies directement dans l'ordinateur et l'administration de l'entretien est géré pas un programme spécialement conçu.</skos:definition>
      <skos:prefLabel xml:lang="it">Intervista telefonica: assistita da computer (CATI)</skos:prefLabel>
      <skos:definition xml:lang="it">Intervista telefonica assistita da computer (CATI). L'intervistatore pone le domande indicate dal computer, le risposte sono immesse direttamente nel computer e l'intervista è gestita da un programma appositamente progettato.</skos:definition>
      <skos:prefLabel xml:lang="no">Telefonintervju: CATI</skos:prefLabel>
      <skos:definition xml:lang="no">Dataassistert telefonintervju. Intervjueren stiller spørsmål ifølge instrukser fra en datamaskin, registrerer svarene direkte på datamaskinen og administreringen av intervjuet er styrt av et spesialdesignet dataprogram.</skos:definition>
      <skos:prefLabel xml:lang="pt">Entrevista telefónica: Assistida por computador  (CATI)</skos:prefLabel>
      <skos:definition xml:lang="pt">Entrevista telefónica assistida por computador (Computer Assisted Telephone Interviewing - CATI). O entrevistador faz perguntas orientado por um computador, as respostas são inseridas diretamente no computador e a realização da entrevista é gerida por um programa especialmente elaborado para o efeito.</skos:definition>
      <skos:prefLabel xml:lang="sl">Telefonski intervju: CATI</skos:prefLabel>
      <skos:definition xml:lang="sl">Računalniško podprto telefonsko intervjuvanje. Spraševanec postavlja vprašanja, ki jih ponuja računalnik, odgovori se vnašajo neposredno v računalnik in intervju upravlja posebej za to zasnovan program.</skos:definition>
      <skos:prefLabel xml:lang="sr">Telefonski intervju: Podržan računarom (CATI)</skos:prefLabel>
      <skos:definition xml:lang="sr">Telefonski intervju (CATI) podržan računarom je onaj u kome anketar postavlja pitanja u skladu sa uputstvom računara, odgovori se unose direktno u računar, a administracijom intervjua upravlja posebno dizajniran program.</skos:definition>
      <skos:prefLabel xml:lang="sv">Telefonintervju: CATI</skos:prefLabel>
      <skos:definition xml:lang="sv">Datorstödd telefonintervju. Intervjuaren läser frågor för respondenterna från en datorskärm och skriver in svaren direkt i datorn. Intervjun hanteras genom ett program som utvecklats för detta syfte.</skos:definition>
      <skos:broader rdf:resource="http://rdf-vocabulary.ddialliance.org/cv/ModeOfCollection/3.0/d64e511"/>
   </rdf:Description>
   <rdf:Description rdf:about="http://rdf-vocabulary.ddialliance.org/cv/ModeOfCollection/3.0/d64e694">
      <rdf:type rdf:resource="http://www.w3.org/2004/02/skos/core#Concept"/>
      <skos:inScheme rdf:resource="http://rdf-vocabulary.ddialliance.org/cv/ModeOfCollection/3.0"/>
      <skos:notation>Interview.Email</skos:notation>
      <skos:prefLabel xml:lang="en">E-mail interview</skos:prefLabel>
      <skos:definition xml:lang="en">Interviews conducted via e-mail, usually consisting of several e-mail messages that allow the discussion to continue beyond the first set of questions and answers, or the first e-mail exchange.</skos:definition>
      <skos:prefLabel xml:lang="da">E-mail-interview</skos:prefLabel>
      <skos:definition xml:lang="da">Interviews gennemført via e-mail, som regel bestående af flere e-mail-beskeder, der tillader diskussionen at fortsætte efter det første sæt af spørgsmål og svar eller den første udveksling af e-mails.</skos:definition>
      <skos:prefLabel xml:lang="fi">Sähköpostihaastattelu</skos:prefLabel>
      <skos:definition xml:lang="fi">Haastattelu tehdään sähköpostin välityksellä. Usein sisältää useita sähköpostiviestejä, jotka mahdollistavat keskustelun jatkumisen alussa esitettyjen kysymysten ja niihin saatujen vastausten jälkeen.</skos:definition>
      <skos:prefLabel xml:lang="fr">Entretien par e-mail</skos:prefLabel>
      <skos:definition xml:lang="fr">Entretiens conduits via e-mail, habituellement consistant en plusieurs courriels qui permettent la discussion qui continue au-delà d'une première série de questions et de réponses, ou d'un premier échange de courriels.</skos:definition>
      <skos:prefLabel xml:lang="fr">Entretien par e-mail</skos:prefLabel>
      <skos:definition xml:lang="fr">Entretiens conduits via e-mail, habituellement consistant en plusieurs courriels qui permettent la discussion qui continue au-delà d'une première série de questions et de réponses, ou d'un premier échange de courriels.</skos:definition>
      <skos:prefLabel xml:lang="it">Intervista e-mail</skos:prefLabel>
      <skos:definition xml:lang="it">Interviste condotte via e-mail, di solito costituite da diversi messaggi di posta elettronica che consentono alla discussione di continuare oltre la prima serie di domande e risposte, oppure dopo il primo scambio di e-mail.</skos:definition>
      <skos:prefLabel xml:lang="no">E-post intervju</skos:prefLabel>
      <skos:definition xml:lang="no">Intervjuer gjennomført over e-post, vanligvis bestående av en rekke e-poster som gjør at diskusjonen kan fortsette utover de første settene med spørsmål og svar, eller den første e-postutvekslingen.</skos:definition>
      <skos:prefLabel xml:lang="pt">Entrevista por email/correio eletrónico</skos:prefLabel>
      <skos:definition xml:lang="pt">Entrevistas realizadas via email, consistindo geralmente em várias mensagens de email que permitem que a discussão continue além do primeiro conjunto de perguntas e respostas, ou da primeira troca de emails.</skos:definition>
      <skos:prefLabel xml:lang="sl">Intervju preko elektronske pošte</skos:prefLabel>
      <skos:definition xml:lang="sl">Intervju, izveden preko elektronske pošte. Običajno ga sestavlja več elektronskih sporočil, ki omogočajo, da se pogovor nadaljuje tudi po prvem nizu vprašanj in odgovorov, ali po prvi izmenjavi elektronskih sporočil.</skos:definition>
      <skos:prefLabel xml:lang="sr">Upitnik putem elektronske pošte</skos:prefLabel>
      <skos:definition xml:lang="sr">Intervju koji se vodi putem elektronske pošte, koji se obično sastoji od nekoliko poruka e-pošte koje omogućavaju da se diskusija nastavi izvan prvog skupa pitanja i odgovora ili prve razmene e-pošte.</skos:definition>
      <skos:prefLabel xml:lang="sv">E-postintervju</skos:prefLabel>
      <skos:definition xml:lang="sv">Intervju som genomförs via e-post, vanligtvis över flera meddelanden som möjliggör att diskussionen fortsätter från den första uppsättningen av frågor och svar eller det första utbytet av e-brev.</skos:definition>
      <skos:broader rdf:resource="http://rdf-vocabulary.ddialliance.org/cv/ModeOfCollection/3.0/d64e136"/>
   </rdf:Description>
   <rdf:Description rdf:about="http://rdf-vocabulary.ddialliance.org/cv/ModeOfCollection/3.0/d64e784">
      <rdf:type rdf:resource="http://www.w3.org/2004/02/skos/core#Concept"/>
      <skos:inScheme rdf:resource="http://rdf-vocabulary.ddialliance.org/cv/ModeOfCollection/3.0"/>
      <skos:notation>Interview.WebBased</skos:notation>
      <skos:prefLabel xml:lang="en">Web-based interview</skos:prefLabel>
      <skos:definition xml:lang="en">An interview conducted via the Internet. For example, interviews conducted within online forums or using web-based audio-visual technology that enables the interviewer(s) and interviewee(s) to communicate in real time.</skos:definition>
      <skos:prefLabel xml:lang="da">Webbaseret interview</skos:prefLabel>
      <skos:definition xml:lang="da">Et interview gennemført via internettet. For eksempel interviews gennemført på online fora eller ved brug af webbaseret audiovisuel teknologi, der gør det muligt for interviewere(n) og de(n) interviewede at kommunikere i realtid.</skos:definition>
      <skos:prefLabel xml:lang="fi">Verkkohaastattelu</skos:prefLabel>
      <skos:definition xml:lang="fi">Verkon välityksellä tehty haastattelu, esimerkiksi verkkokeskustelufoorumilla tai käyttäen teknologiaa, jonka avulla haastattelija ja haastateltava(t) voivat keskustella samanaikaisesti (chat, skype, videokonferenssit).</skos:definition>
      <skos:prefLabel xml:lang="fr">Entretien par Internet</skos:prefLabel>
      <skos:definition xml:lang="fr">Un entretien conduit via l'Internet. Par exemple, des entretiens conduits à l'intérieur de forums en ligne ou en utilisant des technologies web audio-vidéo qui permettent au(x) enquêteur(s) et au(x) répondant(s) de communiquer en temps réel.</skos:definition>
      <skos:prefLabel xml:lang="fr">Entretien par Internet</skos:prefLabel>
      <skos:definition xml:lang="fr">Un entretien conduit via l'Internet. Par exemple, des entretiens conduits à l'intérieur de forums en ligne ou en utilisant des technologies web audio-vidéo qui permettent au(x) enquêteur(s) et au(x) répondant(s) de communiquer en temps réel.</skos:definition>
      <skos:prefLabel xml:lang="it">Intervista web</skos:prefLabel>
      <skos:definition xml:lang="it">Un'intervista condotta via Internet. Ad esempio, interviste condotte all'interno di forum online o utilizzando la tecnologia audiovisiva basata sul web che consente all'intervistatore e agli intervistati di comunicare in tempo reale.</skos:definition>
      <skos:prefLabel xml:lang="no">Webbasert intervju</skos:prefLabel>
      <skos:definition xml:lang="no">Intervju gjennomført over internett. For eksempel, intervjuer gjennomført på internettforum eller ved bruk av internettbasert audiovisuell teknologi som muliggjør fortløpende kommunikasjon mellom intervjuer(e) og Intervjuobjekt(er).</skos:definition>
      <skos:prefLabel xml:lang="pt">Entrevista via web (online)</skos:prefLabel>
      <skos:definition xml:lang="pt">Entrevistas realizadas via Internet. Por exemplo, entrevistas conduzidas em fóruns online ou utilizando tecnologia audiovisual baseada na web que permite ao(s) entrevistador(es) e entrevistado(s) comunicar em tempo real.</skos:definition>
      <skos:prefLabel xml:lang="sl">Spletni intervju</skos:prefLabel>
      <skos:definition xml:lang="sl">Intervju preko spleta. Na primer, intervjuji izvedeni znotraj spletnih forumov ali z uporabo spletno osnovanih avdio-vizualnih tehnologij, ki omogočajo komunikacijo spraševalca(-cev) in spraševanca(-cev) v realnem času.</skos:definition>
      <skos:prefLabel xml:lang="sr">Veb upitnik</skos:prefLabel>
      <skos:definition xml:lang="sr">Intervju koji se sprovodi putem interneta. Na primer, intervjui vođeni na internet forumima ili korišćenjem internet audio-vizuelne tehnologije koja omogućava anketarima i anketiranim licima da komuniciraju u realnom vremenu.</skos:definition>
      <skos:prefLabel xml:lang="sv">Webbaserad intervju</skos:prefLabel>
      <skos:definition xml:lang="sv">Intervju som genomförs över Internet. Exempel inkluderar intervjuer genomförda på onlineforum eller med hjälp av webbaserad audiovisuell teknik som tillåter att intervjuare och intervjuobjekt kan kommunicera i realtid.</skos:definition>
      <skos:broader rdf:resource="http://rdf-vocabulary.ddialliance.org/cv/ModeOfCollection/3.0/d64e136"/>
   </rdf:Description>
   <rdf:Description rdf:about="http://rdf-vocabulary.ddialliance.org/cv/ModeOfCollection/3.0/d64e874">
      <rdf:type rdf:resource="http://www.w3.org/2004/02/skos/core#Concept"/>
      <skos:inScheme rdf:resource="http://rdf-vocabulary.ddialliance.org/cv/ModeOfCollection/3.0"/>
      <skos:notation>SelfAdministeredQuestionnaire</skos:notation>
      <skos:prefLabel xml:lang="en">Self-administered questionnaire</skos:prefLabel>
      <skos:definition xml:lang="en">Data collection method in which the respondent reads or listens to the questions, and enters the responses by him/herself; no live interviewer is present, or participates in the questionnaire administration. If possible, use a narrower term. Use this broader term if the method is not described by any of the narrower terms - for example, for PDF and diskette questionnaires.</skos:definition>
      <skos:prefLabel xml:lang="da">Selvadministreret spørgeskema</skos:prefLabel>
      <skos:definition xml:lang="da">Dataindsamlingsmetode, hvor respondenten læser eller hører spørgsmålene og selv indtaster svarene; ingen interviewer er til stede eller deltager i administrationen af spørgeskemaet. Hvis det er muligt, brug da et smallere begreb. Brug dette begreb, hvis metoden ikke er beskrevet af nogle af de smallere begreber - for eksempel til PDF- eller diskettespørgeskemaer.</skos:definition>
      <skos:prefLabel xml:lang="fi">Itsetäytettävä lomake</skos:prefLabel>
      <skos:definition xml:lang="fi">Tutkimuksen osanottaja täyttää kysely- tai ilmoituslomakkeen itsenäisesti. Pääluokkaa käytetään, jos ei tiedetä missä muodossa lomake on saatu ja palautettu tai jos ei puhtaasti mikään suppeampi termi.</skos:definition>
      <skos:prefLabel xml:lang="fr">Questionnaire auto-administré</skos:prefLabel>
      <skos:definition xml:lang="fr">Méthode de collecte de données dans laquelle l'enquêté lit ou écoute les questions et saisit les réponses par lui-même ; aucun enquêteur n'est présent, ou participe à l'administration du questionnaire. Si possible, utilisez un terme plus précis. Utilisez ce terme si la méthode n'est pas décrite par aucun des termes plus précis - par exemple, pour les questionnaires PDF ou sur disquette.</skos:definition>
      <skos:prefLabel xml:lang="fr">Questionnaire auto-administré</skos:prefLabel>
      <skos:definition xml:lang="fr">Méthode de collecte de données dans laquelle l'enquêté lit ou écoute les questions et saisit les réponses par lui-même ; aucun enquêteur n'est présent, ou participe à l'administration du questionnaire. Si possible, utilisez un terme plus précis. Utilisez ce terme si la méthode n'est pas décrite par aucun des termes plus précis - par exemple, pour les questionnaires PDF ou sur disquette.</skos:definition>
      <skos:prefLabel xml:lang="it">Questionario auto-compilato</skos:prefLabel>
      <skos:definition xml:lang="it">Tecnica di raccolta dei dati in cui il rispondente legge o ascolta le domande e inserisce autonomamente le risposte; nessun intervistatore è presente o partecipa alla somministrazione del questionario. Se possibile, utilizzare un termine più specifico. Utilizzare questo termine più ampio se il metodo non è descritto da nessuno dei termini più specifici, ad esempio per i questionari PDF o trasmessi via floppy disk.</skos:definition>
      <skos:prefLabel xml:lang="no">Selvadministrerende spørreskjema</skos:prefLabel>
      <skos:definition xml:lang="no">Datainnsamlingsmetode hvor respondenten leser eller lytter til spørsmålene, og registrerer svarene på egenhånd; ingen intervjuer er til stede, eller deltar i administreringen av spørreskjemaet. Bruk et smalere begrep dersom det er mulig. Bruk dette bredere begrepet dersom ingen av de smalere begrepene passer.</skos:definition>
      <skos:prefLabel xml:lang="pt">Questionário de autopreenchimento</skos:prefLabel>
      <skos:definition xml:lang="pt">Método de recolha de dados em que o respondente lê ou ouve as perguntas e ele mesmo insere as respostas; nenhum entrevistador está presente, ou participa da administração do questionário. Se possível, usar um termo mais restrito. Usar este termo mais amplo se o método não for descrito por nenhum dos termos mais restritos - por exemplo, questionários em pdf ou em disquete.</skos:definition>
      <skos:prefLabel xml:lang="sl">Vprašalnik za samoizpolnjevanje</skos:prefLabel>
      <skos:definition xml:lang="sl">Metoda zbiranja podatkov, pri kateri spraševanec bere ali posluša vprašanja in sam vnaša odgovore; spraševalec ni prisoten niti ne sodeluje pri upravljanju vprašalnika. Če je možno, uporabite ožji izraz. Ta širši izraz uporabite le, če metoda ni opisana z nobenem od ožjih izrazov, npr. za PDF ali vprašalnike na disketi.</skos:definition>
      <skos:prefLabel xml:lang="sr">Samostalni upitnik</skos:prefLabel>
      <skos:definition xml:lang="sr">Metoda prikupljanja podataka u kojoj ispitanik čita ili sluša pitanja i unosi odgovore; nema živog anketara ili on ne učestvuje u administraciji upitnika. Ako je moguće, koristite uži termin. Upotrebite ovaj širi pojam ako metod nije opisan nijednim užim terminom.</skos:definition>
      <skos:prefLabel xml:lang="sv">Självadministrerat frågeformulär</skos:prefLabel>
      <skos:definition xml:lang="sv">Respondenten läser eller lyssnar på frågorna och noterar själv svaren; ingen intervjuare är närvarande eller deltar i administrerandet av frågeformuläret. Använd om möjligt en smalare term. Använd denna bredare term om metoden inte beskrivits av någon av de mer precisa termerna.</skos:definition>
      <skos:narrower rdf:resource="http://rdf-vocabulary.ddialliance.org/cv/ModeOfCollection/3.0/d64e975"/>
      <skos:narrower rdf:resource="http://rdf-vocabulary.ddialliance.org/cv/ModeOfCollection/3.0/d64e1066"/>
      <skos:narrower rdf:resource="http://rdf-vocabulary.ddialliance.org/cv/ModeOfCollection/3.0/d64e1156"/>
      <skos:narrower rdf:resource="http://rdf-vocabulary.ddialliance.org/cv/ModeOfCollection/3.0/d64e1246"/>
      <skos:narrower rdf:resource="http://rdf-vocabulary.ddialliance.org/cv/ModeOfCollection/3.0/d64e1336"/>
   </rdf:Description>
   <rdf:Description rdf:about="http://rdf-vocabulary.ddialliance.org/cv/ModeOfCollection/3.0/d64e975">
      <rdf:type rdf:resource="http://www.w3.org/2004/02/skos/core#Concept"/>
      <skos:inScheme rdf:resource="http://rdf-vocabulary.ddialliance.org/cv/ModeOfCollection/3.0"/>
      <skos:notation>SelfAdministeredQuestionnaire.Email</skos:notation>
      <skos:prefLabel xml:lang="en">Self-administered questionnaire: E-mail</skos:prefLabel>
      <skos:definition xml:lang="en">Self-administered survey in which questions are presented to the respondent in the text body of an e-mail or as an attachment to an e-mail, but not as a link to a web-based questionnaire. Responses are also sent back via e-mail, in the e-mail body or as an attachment.</skos:definition>
      <skos:prefLabel xml:lang="da">Selvadministreret spørgeskema: E-mail</skos:prefLabel>
      <skos:definition xml:lang="da">Selvadministreret spørgeskema, hvor spørgsmålene stilles til respondenten i en e-mails tekstfelt eller som en vedhæftning i en e-mail, men ikke som et link til et webbaseret spørgeskema. Svarene er også sendt tilbage via e-mail, enten som tekst eller som vedhæftet fil.</skos:definition>
      <skos:prefLabel xml:lang="fi">Itsetäytettävä lomake: sähköpostilomake</skos:prefLabel>
      <skos:definition xml:lang="fi">Osanottaja täyttää sähköpostin tekstiosiossa tai sähköpostin liitetiedostona tulleen kyselylomakkeen ja palauttaa sen sähköpostilla. Jos sähköpostissa on vain linkki verkkokyselylomakkeeseen, käytä termiä 'Itsetäytettävä lomake: verkkolomake'.</skos:definition>
      <skos:prefLabel xml:lang="fr">Questionnaire auto-administré : e-mail</skos:prefLabel>
      <skos:definition xml:lang="fr">Enquête auto-administrée dans laquelle les questions sont présentées au répondant dans le corps d'un e-mail ou dans une pièce jointe, mais pas comme un lien vers une enquête par Internet. Les réponses sont alors renvoyées via e-mail, dans le corps du message ou comme une pièce jointe.</skos:definition>
      <skos:prefLabel xml:lang="fr">Questionnaire auto-administré : e-mail</skos:prefLabel>
      <skos:definition xml:lang="fr">Enquête auto-administrée dans laquelle les questions sont présentées au répondant dans le corps d'un e-mail ou dans une pièce jointe, mais pas comme un lien vers une enquête par Internet. Les réponses sont alors renvoyées via e-mail, dans le corps du message ou comme une pièce jointe.</skos:definition>
      <skos:prefLabel xml:lang="it">Questionario auto-compilato: e-mail</skos:prefLabel>
      <skos:definition xml:lang="it">Questionario auto-compilato in cui le domande vengono presentate all'intervistato nel corpo del testo di un'e-mail o come allegato a un'e-mail, ma non come un collegamento a un questionario somministrato via web. Anche le risposte vengono rispedite via e-mail, nel corpo dell'e-mail o come allegato.</skos:definition>
      <skos:prefLabel xml:lang="no">Selvadministrerende spørreskjema: E-post</skos:prefLabel>
      <skos:definition xml:lang="no">Undersøkelse hvor spørsmål blir presentert til respondenten som tekst i en e-post eller som et vedlegg i en e-post, men ikke som lenke til et web-basert spørreskjema. Svarene sendes også tilbake med e-post, enten som tekst i e-posten eller som et vedlegg.</skos:definition>
      <skos:prefLabel xml:lang="pt">Questionário de autopreenchimento: Email/correio eletrónico</skos:prefLabel>
      <skos:definition xml:lang="pt">Questionário de autopreenchimento em que as perguntas são apresentadas ao respondente no corpo do texto de um email ou num anexo de um email, mas não como um link para um questionário baseado na web. As respostas são também devolvidas via email, no corpo do email ou como anexo.</skos:definition>
      <skos:prefLabel xml:lang="sl">Vprašalnik za samoizpolnjevanje: elektronska pošta</skos:prefLabel>
      <skos:definition xml:lang="sl">Vprašalnik za samoizpolnjevanje, kjer so spraševancu vprašanja prikazana bodisi kot besedilo v telesu elektronskega sporočila bodisi v priponki, vendar ne kot povezava do spletnega vprašalnika. Prav tako so tudi odgovori poslani preko elektronskega sporočila, bodisi v telesu elektronskega sporočila, bodisi kot priponka.</skos:definition>
      <skos:prefLabel xml:lang="sr">Samostalno anketiranje: Elektronskom poštom</skos:prefLabel>
      <skos:definition xml:lang="sr">Samostalno anketiranje u kome se ispitanicima postavljaju pitanja u tekstu e-pošte ili kao prilog e-pošti, ali ne kao hiperlink do veb-upitnika. Odgovori se takođe šalju nazad e-poštom, u poruci e-pošte ili kao prilog.</skos:definition>
      <skos:prefLabel xml:lang="sv">Självadministrerat frågeformulär: e-post</skos:prefLabel>
      <skos:definition xml:lang="sv">Frågor skickas till respondenten i brödtexten på, eller som en bilaga till, ett e-brev, inte som en länk till ett frågeformulär på webben. Svaren skickas tillbaka med e-post, i brödtexten eller som bilaga.</skos:definition>
      <skos:broader rdf:resource="http://rdf-vocabulary.ddialliance.org/cv/ModeOfCollection/3.0/d64e874"/>
   </rdf:Description>
   <rdf:Description rdf:about="http://rdf-vocabulary.ddialliance.org/cv/ModeOfCollection/3.0/d64e1066">
      <rdf:type rdf:resource="http://www.w3.org/2004/02/skos/core#Concept"/>
      <skos:inScheme rdf:resource="http://rdf-vocabulary.ddialliance.org/cv/ModeOfCollection/3.0"/>
      <skos:notation>SelfAdministeredQuestionnaire.Paper</skos:notation>
      <skos:prefLabel xml:lang="en">Self-administered questionnaire: Paper</skos:prefLabel>
      <skos:definition xml:lang="en">Self-administered survey using a traditional paper questionnaire delivered and/or collected by mail (postal services), by fax, or in person by either interviewer, or respondent.</skos:definition>
      <skos:prefLabel xml:lang="da">Selvadministreret spørgeskema: Papir</skos:prefLabel>
      <skos:definition xml:lang="da">Selvadministreret spørgeskema ved brug af et traditionelt spørgeskema på papir leveret og/eller indsamlet som post (posttjenester), på fax eller personligt enten af intervieweren eller respondenten.</skos:definition>
      <skos:prefLabel xml:lang="fi">Itsetäytettävä lomake: paperinen lomake</skos:prefLabel>
      <skos:definition xml:lang="fi">Osanottaja täyttää perinteisen paperisen kyselylomakkeen itse. Paperilomake voidaan lähettää tai palauttaa postissa, tai annetaan henkilökohtaisesti.</skos:definition>
      <skos:prefLabel xml:lang="fr">Questionnaire auto-administré : papier</skos:prefLabel>
      <skos:definition xml:lang="fr">Enquête auto-administrée utilisant un traditionnel questionnaire papier distribué et / ou recueilli par courrier (services postaux), par fax, ou en personne par soit par un enquêteur ou par un répondant.</skos:definition>
      <skos:prefLabel xml:lang="fr">Questionnaire auto-administré : papier</skos:prefLabel>
      <skos:definition xml:lang="fr">Enquête auto-administrée utilisant un traditionnel questionnaire papier distribué et / ou recueilli par courrier (services postaux), par fax, ou en personne par soit par un enquêteur ou par un répondant.</skos:definition>
      <skos:prefLabel xml:lang="it">Questionario auto-compilato: cartaceo</skos:prefLabel>
      <skos:definition xml:lang="it">Questionario cartaceo tradizionale auto-compilato, consegnato e/o ritirato per posta (servizi postali), via fax o di persona dall'intervistatore oppure dall'intervistato.</skos:definition>
      <skos:prefLabel xml:lang="no">Selvadministrerende spørreskjema: Papir</skos:prefLabel>
      <skos:definition xml:lang="no">Selvadministrert spørreskjema som bruker tradisjonelle spørsmålsformuleringer på papir, som blir levert og/eller samlet inn via post, faks, eller personlig av intervjueren eller respondenten.</skos:definition>
      <skos:prefLabel xml:lang="pt">Questionário de autopreenchimento: Papel</skos:prefLabel>
      <skos:definition xml:lang="pt">Questionário de autopreenchimento utilizando um questionário tradicional em papel entregue e/ou recolhido por correio (serviços postais), por fax ou pessoalmente, seja pelo entrevistador ou pelo respondente.</skos:definition>
      <skos:prefLabel xml:lang="sl">Vprašalnik za samoizpolnjevanje: papirnati</skos:prefLabel>
      <skos:definition xml:lang="sl">Vprašalnik za samoizpolnjevanje z uporabo tradicionalnega papirnatega vprašalnika poslanega in/ali prejetega preko tradicionalne poštne storitve, preko faksa ali osebno preko spraševalca ali spraševanca.</skos:definition>
      <skos:prefLabel xml:lang="sr">Samostalno anketiranje: Papirno</skos:prefLabel>
      <skos:definition xml:lang="sr">Anketa koja se sprovodi samostalno, koristeći tradicionalni papirnati upitnik dostavljen i / ili prikupljen poštom (poštanske usluge), faksom ili lično od strane anketara ili ispitanika.</skos:definition>
      <skos:prefLabel xml:lang="sv">Självadministrerat frågeformulär: papper</skos:prefLabel>
      <skos:definition xml:lang="sv">Självadministrerad surveyundersökning som använder traditionella frågeformulär på papper, vilka skickas ut och/eller in via post eller fax, eller lämnas över personligen av antingen intervjuaren eller intervjuobjektet.</skos:definition>
      <skos:broader rdf:resource="http://rdf-vocabulary.ddialliance.org/cv/ModeOfCollection/3.0/d64e874"/>
   </rdf:Description>
   <rdf:Description rdf:about="http://rdf-vocabulary.ddialliance.org/cv/ModeOfCollection/3.0/d64e1156">
      <rdf:type rdf:resource="http://www.w3.org/2004/02/skos/core#Concept"/>
      <skos:inScheme rdf:resource="http://rdf-vocabulary.ddialliance.org/cv/ModeOfCollection/3.0"/>
      <skos:notation>SelfAdministeredQuestionnaire.SMSorMMS</skos:notation>
      <skos:prefLabel xml:lang="en">Self-administered questionnaire: Messaging (SMS/MMS)</skos:prefLabel>
      <skos:definition xml:lang="en">Self-administered survey in which the respondents receive the questions incorporated in SMS (text messages) or MMS (messages including multimedia content) and send their replies in the same format.</skos:definition>
      <skos:prefLabel xml:lang="da">Selvadministreret spørgeskema: Beskeder (SMS/MMS)</skos:prefLabel>
      <skos:definition xml:lang="da">Selvadministreret spørgeskema, hvor respondenterne modtager spørgsmålene på SMS (tekstbeskeder) eller MMS (beskeder indeholdende multimedieindhold) og sender deres svar i samme format.</skos:definition>
      <skos:prefLabel xml:lang="fi">Itsetäytettävä lomake: tekstiviesti- tai mobiililaitelomake (SMS tai MMS)</skos:prefLabel>
      <skos:definition xml:lang="fi">Osanottaja täyttää tekstiviestinä tai mobiililaitekyselynä välitetyn kyselylomakkeen itse ja palauttaa sen samalla teknologialla.</skos:definition>
      <skos:prefLabel xml:lang="fr">Questionnaire auto-administré : par messagerie (SMS / MMS)</skos:prefLabel>
      <skos:definition xml:lang="fr">Enquête auto-administrée dans laquelle les répondants reçoivent les questions par SMS (messages texte) ou MMS (messages incluant des contenus multimédia) et envoient leurs réponses dans le même format.</skos:definition>
      <skos:prefLabel xml:lang="fr">Questionnaire auto-administré : par messagerie (SMS / MMS)</skos:prefLabel>
      <skos:definition xml:lang="fr">Enquête auto-administrée dans laquelle les répondants reçoivent les questions par SMS (messages texte) ou MMS (messages incluant des contenus multimédia) et envoient leurs réponses dans le même format.</skos:definition>
      <skos:prefLabel xml:lang="it">Questionario auto-compilato: messaggistica (SMS/MMS)</skos:prefLabel>
      <skos:definition xml:lang="it">Questionario auto-compilato in cui gli intervistati ricevono le domande all'interno di in SMS (messaggi di testo) o MMS (messaggi che includono contenuti multimediali) e inviano le loro risposte nello stesso formato.</skos:definition>
      <skos:prefLabel xml:lang="no">Selvadministrerende spørreskjema: SMS/MMS</skos:prefLabel>
      <skos:definition xml:lang="no">Selvadministrert spørreskjema hvor respondenten mottar spørsmål på SMS (tekstmeldinger) eller MMS (meldinger med multimedia innhold) og sender svarene i samme format.</skos:definition>
      <skos:prefLabel xml:lang="pt">Questionário de autopreenchimento: Mensagem (SMS/MMS)</skos:prefLabel>
      <skos:definition xml:lang="pt">Questionário de autopreenchimento em que os respondentes recebem as perguntas incorporadas em SMS (mensagens de texto) ou MMS (mensagens que incluem conteúdo multimédia) e enviam as suas respostas no mesmo formato.</skos:definition>
      <skos:prefLabel xml:lang="sl">Vprašalnik za samoizpolnjevanje: SMS/MMS</skos:prefLabel>
      <skos:definition xml:lang="sl">Vprašalnik za samoizpolnjevanje, kjer spraševanec prejme vprašanja, vključena v kratkih sporočilih v formatu SMS (tekstovna sporočila) ali MMS (multimedijska sporočila) in odgovore pošlje v enakem formatu.</skos:definition>
      <skos:prefLabel xml:lang="sr">Samostalno anketiranje: Porukama (SMS/MMS)</skos:prefLabel>
      <skos:definition xml:lang="sr">Anketa koja se sprovodi samostalno, a u kojoj ispitanici dobijaju pitanja putem SMS (tekstualne poruke) ili MMS (poruke koje uključujui multimedijalni sadržaj) i šalju svoje odgovore u istom formatu.</skos:definition>
      <skos:prefLabel xml:lang="sv">Självadministrerat frågeformulär: SMS/MMS</skos:prefLabel>
      <skos:definition xml:lang="sv">Självadministrerad surveyundersökning där frågor och svar inkluderas i SMS (textmeddelanden) eller MMS (meddelanden med multimedia-innehåll) som skickas mellan mobiltelefoner.</skos:definition>
      <skos:broader rdf:resource="http://rdf-vocabulary.ddialliance.org/cv/ModeOfCollection/3.0/d64e874"/>
   </rdf:Description>
   <rdf:Description rdf:about="http://rdf-vocabulary.ddialliance.org/cv/ModeOfCollection/3.0/d64e1246">
      <rdf:type rdf:resource="http://www.w3.org/2004/02/skos/core#Concept"/>
      <skos:inScheme rdf:resource="http://rdf-vocabulary.ddialliance.org/cv/ModeOfCollection/3.0"/>
      <skos:notation>SelfAdministeredQuestionnaire.CAWI</skos:notation>
      <skos:prefLabel xml:lang="en">Self-administered questionnaire: Web-based (CAWI)</skos:prefLabel>
      <skos:definition xml:lang="en">Computer-assisted web interviewing (CAWI). Data are collected using a web questionnaire, produced with a program for creating web surveys. The program can customize the flow of the questionnaire based on the answers provided, and can allow for the questionnaire to contain pictures, audio and video clips, links to different web pages etc.</skos:definition>
      <skos:prefLabel xml:lang="da">Selvadministreret spørgeskema: Webbaseret (CAWI)</skos:prefLabel>
      <skos:definition xml:lang="da">Computer-assisted web interviewing (CAWI). Data indsamles ved brug af et webspørgeskema, der er produceret af et program til at skabe webundersøgelser. Programmet kan tilpasse spørgeskemaets flow ud fra de givne svar og giver spørgeskemaet mulighed for at indeholde billeder, lyd og videoklip, links til forskellige hjemmesider mm.</skos:definition>
      <skos:prefLabel xml:lang="fi">Itsetäytettävä lomake: verkkolomake</skos:prefLabel>
      <skos:definition xml:lang="fi">Osanottaja täyttää kysely- tai ilmoituslomakkeen verkossa itse (Computer-assisted web interviewing, CAWI). Lomake voi olla dynaaminen tai muuttumaton. Dynaamisessa lomakkeessa kysymysten järjestys sekä esitetyt kysymykset riippuvat edeltäviin kysymyksiin annetuista vastauksista. Lomake voi myös sisältää kuvia, video- tai äänitiedostoja, linkkejä toisiin verkkosivuihin jne.</skos:definition>
      <skos:prefLabel xml:lang="fr">Questionnaire auto-administré : par Internet (CAWI)</skos:prefLabel>
      <skos:definition xml:lang="fr">Entretien par Internet assisté par ordinateur (CAWI). Des données sont collectées en utilisant un questionnaire en ligne, produit avec un programme de création d'enquête en ligne. Le programme peut personnaliser le déroulement du questionnaire en fonction des réponses fournies, et peut permettre au questionnaire de contenir des images, des clips audio et vidéo, des liens vers différentes pages Web, etc.</skos:definition>
      <skos:prefLabel xml:lang="fr">Questionnaire auto-administré : par Internet (CAWI)</skos:prefLabel>
      <skos:definition xml:lang="fr">Entretien par Internet assisté par ordinateur (CAWI). Des données sont collectées en utilisant un questionnaire en ligne, produit avec un programme de création d'enquête en ligne. Le programme peut personnaliser le déroulement du questionnaire en fonction des réponses fournies, et peut permettre au questionnaire de contenir des images, des clips audio et vidéo, des liens vers différentes pages Web, etc.</skos:definition>
      <skos:prefLabel xml:lang="it">Questionario auto-compilato: web (CAWI)</skos:prefLabel>
      <skos:definition xml:lang="it">Intervista web assistita da computer (CAWI). I dati vengono raccolti utilizzando un questionario via web, prodotto con un programma per la creazione di indagini via web. Il programma può personalizzare la struttura del questionario in base alle risposte fornite, e può consentire al questionario di contenere immagini, clip audio e video, collegamenti a pagine web diverse, ecc.</skos:definition>
      <skos:prefLabel xml:lang="no">Selvadministrerende spørreskjema: Webbasert</skos:prefLabel>
      <skos:definition xml:lang="no">Datamaskinaassistert webintervju (CAWI). Data samles ved hjelp av spørreskjema på nett, som er produsert av et program for internettundersøkelser. Programmet kan endre flyten av spørsmål basert på svarene som blir gitt, og det muliggjør inkludering av bilde, lyd og video, lenker til andre nettsider etc.</skos:definition>
      <skos:prefLabel xml:lang="pt">Questionário de autopreenchimento: via web (CAWI)</skos:prefLabel>
      <skos:definition xml:lang="pt">Entrevista via web, assistida por computador (Computer Assisted Web Interviewing - CAWI). Os dados são recolhidos através de um questionário na web, produzido com um programa para criar inquéritos na web. O programa pode personalizar o fluxo do questionário de acordo com as respostas e permite que este contenha imagens, clipes de áudio e vídeo, links para diferentes páginas da web, etc.</skos:definition>
      <skos:prefLabel xml:lang="sl">Vprašalnik za samoizpolnjevanje: spletni</skos:prefLabel>
      <skos:definition xml:lang="sl">Računalniško podprto spletno intervjuvanje. Podatki so zbrani z uporabo spletnega vprašalnika, ustvarjenega v programskem orodju za spletno anketiranje. Program lahko tok vprašalnika prilagodi odgovorom na prejšnja vprašanja, omogoča lahko vstavljanje slik ter avdio in video posnetkov, povezave do spletnih strani itd.</skos:definition>
      <skos:prefLabel xml:lang="sr">Samostalno anketiranje: Veb anketa (CAWI)</skos:prefLabel>
      <skos:definition xml:lang="sr">Podaci se prikupljaju putem veb upitnika, sačinjenog uz pomoć program za kreiranje veb ili onlajn anketa. Program može prilagoditi tok upitnika na osnovu ponuđenih odgovora, a može omogućiti da upitnik sadrži slike, audio i video snimke, veze do različitih veb stranica, i sl.</skos:definition>
      <skos:prefLabel xml:lang="sv">Självadministrerat frågeformulär: webbaserat</skos:prefLabel>
      <skos:definition xml:lang="sv">Computer-assisted web interviewing (CAWI). Data samlas in med ett webbformulär som producerats av ett program som skapar webbsurveyer. Programmet kan anpassa flödet i frågeformuläret utifrån svaren som ges och det går att inkludera bilder, ljud- och videoklipp, länkar till andra webbsidor m.m. (Anpassad från Wikipedia.)</skos:definition>
      <skos:broader rdf:resource="http://rdf-vocabulary.ddialliance.org/cv/ModeOfCollection/3.0/d64e874"/>
   </rdf:Description>
   <rdf:Description rdf:about="http://rdf-vocabulary.ddialliance.org/cv/ModeOfCollection/3.0/d64e1336">
      <rdf:type rdf:resource="http://www.w3.org/2004/02/skos/core#Concept"/>
      <skos:inScheme rdf:resource="http://rdf-vocabulary.ddialliance.org/cv/ModeOfCollection/3.0"/>
      <skos:notation>SelfAdministeredQuestionnaire.CASI</skos:notation>
      <skos:prefLabel xml:lang="en">Self-administered questionnaire: Computer-assisted (CASI)</skos:prefLabel>
      <skos:definition xml:lang="en">Computer-assisted self-interview (CASI). Respondents enter the responses into a computer (desktop, laptop, Palm/PDA, tablet, etc.) by themselves. The administration of the questionnaire is managed by a specifically designed program/application but there is no real-time data transfer as in CAWI, the answers are stored on the device used for the interview. The questionnaire may be fixed form or interactive. Includes VCASI (Video computer-assisted self-interviewing), ACASI (Audio computer-assisted self-interviewing) and TACASI (Telephone audio computer-assisted self-interviewing).</skos:definition>
      <skos:prefLabel xml:lang="da">Selvadministreret spørgeskema: Computerassisteret (CASI)</skos:prefLabel>
      <skos:definition xml:lang="da">Computer-assisted self-interview (CASI). Respondenter indtaster selv svarene på en computer (skrivebord, bærbar, Palm/PDA, tablet etc.) af dem selv. Administrationen af spørgeskemaet styres af et specifikt designet program/applikation, men der er ingen real-time dataoverførsel som i CAWI, svarene lagres på enheden, der anvendes til interviewet. Spørgeskemaet kan være i fast form eller interaktiv. Inkluderer VCASI (Video computer-assisted self-interviewing), ACASI (Audio computer-assisted self-interviewing) og TACASI (Telephone audio computer-assisted self-interviewing).</skos:definition>
      <skos:prefLabel xml:lang="fi">Itsetäytettävä lomake: tietokoneavusteinen (CASI)</skos:prefLabel>
      <skos:definition xml:lang="fi">Tietokoneavusteinen itsetäytettävä kyselylomake, jossa vastaaja tallentaa itse vastauksensa tietokoneelle (pöytäkone, kannettava tietokone tai kämmentietokone). Tiedot eivät siirry verkon kautta vaan taltioituvat vain tietokoneelle. Lomake voi olla dynaaminen tai muuttumaton. Termi sisältää myös harvoin käytetyt VCASI:n (Video computer-assisted self-interviewing), ACASI:n (Audio computer-assisted self-interviewing) ja TACASI:n (Telephone audio computer-assisted self-interviewing).</skos:definition>
      <skos:prefLabel xml:lang="fr">Questionnaire auto-administré : assisté par ordinateur (CASI)</skos:prefLabel>
      <skos:definition xml:lang="fr">Entretien auto-administré assisté par ordinateur (CASI). Des répondants entrent les réponses dans un ordinateur (ordinateur de bureau, ordinateur portable, Palm / assistant personnel, tablette, etc.) par eux-mêmes. L'administration du questionnaire est gérée par un programme / une application spécialement conçu mais il n'y a pas de transfert de données en temps réel comme dans un CAWI, les réponses sont stockées sur l'appareil utilisé pour l'entretien. Le questionnaire peut être figé ou interactif. Sont inclus les VCASI (entretien vidéo auto-administré assisté par ordinateur), les ACASI (entretien audio auto-administré assisté par ordinateur) et les TACASI (entretien auto-administré par téléphone assisté par ordinateur).</skos:definition>
      <skos:prefLabel xml:lang="fr">Questionnaire auto-administré : assisté par ordinateur (CASI)</skos:prefLabel>
      <skos:definition xml:lang="fr">Entretien auto-administré assisté par ordinateur (CASI). Des répondants entrent les réponses dans un ordinateur (ordinateur de bureau, ordinateur portable, Palm / assistant personnel, tablette, etc.) par eux-mêmes. L'administration du questionnaire est gérée par un programme / une application spécialement conçu mais il n'y a pas de transfert de données en temps réel comme dans un CAWI, les réponses sont stockées sur l'appareil utilisé pour l'entretien. Le questionnaire peut être figé ou interactif. Sont inclus les VCASI (entretien vidéo auto-administré assisté par ordinateur), les ACASI (entretien audio auto-administré assisté par ordinateur) et les TACASI (entretien auto-administré par téléphone assisté par ordinateur).</skos:definition>
      <skos:prefLabel xml:lang="it">Questionario auto-compilato: computer-assistito (CASI)</skos:prefLabel>
      <skos:definition xml:lang="it">Auto-compilazione del questionario assistita da computer (CASI). Gli intervistati inseriscono autonomamente le risposte in un computer (desktop, laptop, palmare, tablet, ecc.). La somministrazione del questionario è gestita da un programma/applicazione appositamente progettato, ma non esiste un trasferimento dati in tempo reale come nel CAWI poiché le risposte vengono memorizzate sul dispositivo utilizzato per l'intervista. Il questionario può essere fisso o interattivo. I tipi di questionario possono essere: VCASI (video assistito), ACASI (audio assistito) e TACASI (assistito via telefono).</skos:definition>
      <skos:prefLabel xml:lang="no">Selvadministrerende spørreskjema: Datamaskinassistert (CASI)</skos:prefLabel>
      <skos:definition xml:lang="no">Datamaskinassistert selvadministrert intervju (CASI). Respondentene registrerer svarene på en datamaskin, bærbar datamaskin, digital personlig assistent, nettbrett etc.) på egenhånd. Administreringen av spørreskjemaet er styrt av et spesialdesignet program eller en applikasjon men det er ingen fortløpende datautveksling slik som i CAWI, svarene blir lagret på apparatet som brukes for å gjennomføre intervjuet. Spørreskjemaet kan enten være fastsatt eller interaktivt.Omfatter VCASI (video computer-assisted self-interview), ACASI (audio computer-assisted self-interview) og TCASI (telephone audio computer-assisted self-interview).</skos:definition>
      <skos:prefLabel xml:lang="pt">Questionário de autopreenchimento: Assistido por computador (CASI)</skos:prefLabel>
      <skos:definition xml:lang="pt">Entrevista de autopreenchimento assistida por computador (Computer-assisted self-interview - CASI). Os entrevistados inserem as respostas num computador (desktop, laptop, PDA, tablet, etc.) por eles próprios. A administração do questionário é gerida por um programa/aplicação especialmente elaborado para o efeito, mas não há transferência de dados em tempo real, como no CAWI, e as respostas são armazenadas no dispositivo usado para a entrevista. O questionário pode ter um formato fixo ou interativo. Inclui a entrevista auto-administrada de vídeo assistida por computador (VCASI - Video computer-assisted self-interviewing), a entrevista auto-administrada de áudio assistida por computador (ACASI - Audio computer-assisted self-interviewing) e a entrevista de áudio e telefone assistida por computador (TACASI - Telephone audio computer-assisted self-interviewing).</skos:definition>
      <skos:prefLabel xml:lang="sl">Vprašalnik za samoizpolnjevanje: računalniško podprti (CASI)</skos:prefLabel>
      <skos:definition xml:lang="sl">Računalniško podprto samoizpolnjevanje (CASI). Spraševanec sam vstavlja odgovore v računalnik (namizni, prenosni, dlančni/PDA, tablični itd.). Z vprašalnikom upravlja posebej zasnovani program/aplikacija, vendar pri tem ni prenosa v realnem času kot pri CAWI, vprašanja se shranjujejo na napravi, ki se uporablja za intervju. Vprašalnik je lahko v fiksni obliki ali interaktiven. Vključuje tudi VCASI (video računalniško podprto samoizpolnjevanje), ACASI (avdio računalniško podprto samoizpolnjevanje) in TACASI (telefonsko avdio računalniško podprto samoizpolnjevanje).</skos:definition>
      <skos:prefLabel xml:lang="sr">Samostalno anketiranje: Podržano računarom (CASI)</skos:prefLabel>
      <skos:definition xml:lang="sr">Ispitanici samostalno unose odgovore u računar (desktop, laptop, Palm / PDA, tablet itd.). Administriranje upitnika obavlja posebno dizajniran program / aplikacija, ali ne postoji prijenos podataka u realnom vremenu (kao u CAWI), već se odgovori čuvaju na uređaju koji se koristi za intervju. Upitnik može biti fiksnog oblika ili interaktivan. Uključuje VCASI (video-računarski podržano samostalno anketiranje), ACASI (audio-računarski podržano samostalno anketiranje) i TACASI (telefonsko audio-računarski podržano samostalno anketiranje).</skos:definition>
      <skos:prefLabel xml:lang="sv">Självadministrerat frågeformulär: med datorstöd (CASI)</skos:prefLabel>
      <skos:definition xml:lang="sv">Computer-assisted self-interview (CASI). Respondenterna noterar själva sina svar i en dator (stationär eller bärbar, Palm/PDA, surfplatta e. dyl.). Frågeformuläret administreras med ett datorprogram som utvecklats för detta syfte men data överförs inte i realtid som i fallet med CAWI: svaren lagras på datorn som används för intervjun. Frågeformuläret kan vara statiskt eller interaktivt. Omfattar VCASI (Video Computer-Assisted Self-Interview), ACASI (Audio computer-assisted self-interview) och TCASI (Telephone audio computer-assisted self-interview).</skos:definition>
      <skos:broader rdf:resource="http://rdf-vocabulary.ddialliance.org/cv/ModeOfCollection/3.0/d64e874"/>
   </rdf:Description>
   <rdf:Description rdf:about="http://rdf-vocabulary.ddialliance.org/cv/ModeOfCollection/3.0/d64e1426">
      <rdf:type rdf:resource="http://www.w3.org/2004/02/skos/core#Concept"/>
      <skos:inScheme rdf:resource="http://rdf-vocabulary.ddialliance.org/cv/ModeOfCollection/3.0"/>
      <skos:notation>FocusGroup</skos:notation>
      <skos:prefLabel xml:lang="en">Focus group</skos:prefLabel>
      <skos:definition xml:lang="en">A group discussion on a particular topic, organized for research purposes. The individuals are selected with relevance to the topic, and interaction among the participants is used as part of the method.</skos:definition>
      <skos:prefLabel xml:lang="da">Fokusgruppe</skos:prefLabel>
      <skos:definition xml:lang="da">En gruppediskussion om et bestemt emne organiseret til forskningsformål. Individerne vælges med relevans for emnet, og interaktion mellem deltagerne anvendes som en del af metoden.</skos:definition>
      <skos:prefLabel xml:lang="fi">Kohderyhmäkeskustelu</skos:prefLabel>
      <skos:definition xml:lang="fi">Tutkimustarkoitusta varten järjestetty kohderyhmäkeskustelu tietystä aiheesta. Ryhmän osanottajat valitaan aiheen mukaan ja osanottajien välinen vuorovaikutus on osa tutkimuskohdetta.</skos:definition>
      <skos:prefLabel xml:lang="fr">Focus group</skos:prefLabel>
      <skos:definition xml:lang="fr">Un groupe de discussions sur un sujet particulier, organisé à des fins de recherche. Les individus sont sélectionnés en fonction du sujet, et les interactions entre participants sont utilisées dans le cadre de la méthode.</skos:definition>
      <skos:prefLabel xml:lang="fr">Focus group</skos:prefLabel>
      <skos:definition xml:lang="fr">Un groupe de discussions sur un sujet particulier, organisé à des fins de recherche. Les individus sont sélectionnés en fonction du sujet, et les interactions entre participants sont utilisées dans le cadre de la méthode.</skos:definition>
      <skos:prefLabel xml:lang="it">Focus group</skos:prefLabel>
      <skos:definition xml:lang="it">Una discussione di gruppo focalizzata su un argomento particolare, organizzata per scopi di ricerca. I singoli individui sono selezionati in base all'argomento trattato, e l'interazione tra i partecipanti viene utilizzata come parte della tecnica.</skos:definition>
      <skos:prefLabel xml:lang="no">Fokusgruppe</skos:prefLabel>
      <skos:definition xml:lang="no">En gruppediskusjon som omhandler et bestemt tema, organisert for forskningsformål. Individene er valgt med relevans til temaet og samhandlingen mellom deltakerne er brukt som en del av metoden.</skos:definition>
      <skos:prefLabel xml:lang="pt">Focus group (grupo focal)</skos:prefLabel>
      <skos:definition xml:lang="pt">Entrevista de grupo sobre um tópico específico, organizada para fins de investigação. Os indivíduos são selecionados em função da sua relevância para o tópico e a interação entre os participantes é usada como parte do método.</skos:definition>
      <skos:prefLabel xml:lang="sl">Fokusna skupina</skos:prefLabel>
      <skos:definition xml:lang="sl">Skupinska razprava o določeni temi, organizirana za raziskovalne namene. Posamezniki so izbrani glede na temo, interakcija med udeleženci pa se uporablja kot del metode.</skos:definition>
      <skos:prefLabel xml:lang="sr">Fokus grupa</skos:prefLabel>
      <skos:definition xml:lang="sr">Grupna diskusija o određenoj temi, organizovana u istraživačke svrhe. Pojedinci su odabrani u skladu sa temom, a interakcija između učesnika koristi se kao deo metode.</skos:definition>
      <skos:prefLabel xml:lang="sv">Fokusgrupp</skos:prefLabel>
      <skos:definition xml:lang="sv">En gruppdiskussion om ett visst ämne som anordnats i forskningssyfte. Deltagarna har valts ut med hänsyn till ämnet och interaktionen mellan deltagarna utgör en del av forskningsmetoden.</skos:definition>
      <skos:narrower rdf:resource="http://rdf-vocabulary.ddialliance.org/cv/ModeOfCollection/3.0/d64e1523"/>
      <skos:narrower rdf:resource="http://rdf-vocabulary.ddialliance.org/cv/ModeOfCollection/3.0/d64e1614"/>
      <skos:narrower rdf:resource="http://rdf-vocabulary.ddialliance.org/cv/ModeOfCollection/3.0/d64e1704"/>
   </rdf:Description>
   <rdf:Description rdf:about="http://rdf-vocabulary.ddialliance.org/cv/ModeOfCollection/3.0/d64e1523">
      <rdf:type rdf:resource="http://www.w3.org/2004/02/skos/core#Concept"/>
      <skos:inScheme rdf:resource="http://rdf-vocabulary.ddialliance.org/cv/ModeOfCollection/3.0"/>
      <skos:notation>FocusGroup.FaceToFace</skos:notation>
      <skos:prefLabel xml:lang="en">Face-to-face focus group</skos:prefLabel>
      <skos:definition xml:lang="en">The focus group participants meet in person to conduct the discussion.</skos:definition>
      <skos:prefLabel xml:lang="da">Personlig fokusgruppe</skos:prefLabel>
      <skos:definition xml:lang="da">Fokusgruppens deltagere mødes personligt for at gennemføre diskussionen.</skos:definition>
      <skos:prefLabel xml:lang="fi">Kohderyhmäkeskustelu: kasvokkainen keskustelu</skos:prefLabel>
      <skos:definition xml:lang="fi">Tutkimustarkoitusta varten järjestetty kohderyhmäkeskustelu tietystä aiheesta. Keskustelu käydään kasvokkain.</skos:definition>
      <skos:prefLabel xml:lang="fr">Focus group en face-à-face</skos:prefLabel>
      <skos:definition xml:lang="fr">Les participants du focus group se rencontrent en personne pour mener la discussion.</skos:definition>
      <skos:prefLabel xml:lang="fr">Focus group en face-à-face</skos:prefLabel>
      <skos:definition xml:lang="fr">Les participants du focus group se rencontrent en personne pour mener la discussion.</skos:definition>
      <skos:prefLabel xml:lang="it">Focus group faccia a faccia</skos:prefLabel>
      <skos:definition xml:lang="it">I partecipanti al focus group si incontrano di persona per condurre la discussione.</skos:definition>
      <skos:prefLabel xml:lang="no">Fokusgruppe: Ansikt til ansikt</skos:prefLabel>
      <skos:definition xml:lang="no">Deltakerne i fokusgruppen møtes fysisk for å gjennomføre diskusjonen.</skos:definition>
      <skos:prefLabel xml:lang="pt">Focus group presencial</skos:prefLabel>
      <skos:definition xml:lang="pt">Os participantes do grupo focal encontram-se pessoalmente para participar na discussão.</skos:definition>
      <skos:prefLabel xml:lang="sl">Fokusna skupina v živo</skos:prefLabel>
      <skos:definition xml:lang="sl">Udeleženci fokusne skupine se osebno sestanejo za vodenje razprave.</skos:definition>
      <skos:prefLabel xml:lang="sr">Fokus grupa licem u lice</skos:prefLabel>
      <skos:definition xml:lang="sr">Učesnici fokus grupe sastaju se lično kako bi vodili diskusiju.</skos:definition>
      <skos:prefLabel xml:lang="sv">Fokusgrupp: traditionell</skos:prefLabel>
      <skos:definition xml:lang="sv">Fokusgruppens medlemmar träffas på samma plats för att diskutera.</skos:definition>
      <skos:broader rdf:resource="http://rdf-vocabulary.ddialliance.org/cv/ModeOfCollection/3.0/d64e1426"/>
   </rdf:Description>
   <rdf:Description rdf:about="http://rdf-vocabulary.ddialliance.org/cv/ModeOfCollection/3.0/d64e1614">
      <rdf:type rdf:resource="http://www.w3.org/2004/02/skos/core#Concept"/>
      <skos:inScheme rdf:resource="http://rdf-vocabulary.ddialliance.org/cv/ModeOfCollection/3.0"/>
      <skos:notation>FocusGroup.Telephone</skos:notation>
      <skos:prefLabel xml:lang="en">Telephone focus group</skos:prefLabel>
      <skos:definition xml:lang="en">The focus group discussion is conducted over the telephone.</skos:definition>
      <skos:prefLabel xml:lang="da">Telefonfokusgruppe</skos:prefLabel>
      <skos:definition xml:lang="da">Fokusgruppediskussionen gennemføres over telefonen.</skos:definition>
      <skos:prefLabel xml:lang="fi">Kohderyhmäkeskustelu: puhelinkeskustelu</skos:prefLabel>
      <skos:definition xml:lang="fi">Tutkimustarkoitusta varten järjestetty kohderyhmäkeskustelu tietystä aiheesta. Keskustelu käydään puhelimen välityksellä.</skos:definition>
      <skos:prefLabel xml:lang="fr">Focus group par téléphone</skos:prefLabel>
      <skos:definition xml:lang="fr">Les discussions du focus group se font par téléphone.</skos:definition>
      <skos:prefLabel xml:lang="fr">Focus group par téléphone</skos:prefLabel>
      <skos:definition xml:lang="fr">Les discussions du focus group se font par téléphone.</skos:definition>
      <skos:prefLabel xml:lang="it">Focus group telefonico</skos:prefLabel>
      <skos:definition xml:lang="it">La discussione del focus group è condotta via telefono.</skos:definition>
      <skos:prefLabel xml:lang="no">Fokusgruppe: Telefon</skos:prefLabel>
      <skos:definition xml:lang="no">Fokusgruppediskusjonen er gjennomført over telefonen.</skos:definition>
      <skos:prefLabel xml:lang="pt">Focus group por telefone</skos:prefLabel>
      <skos:definition xml:lang="pt">A discussão do grupo focal é realizada por telefone.</skos:definition>
      <skos:prefLabel xml:lang="sl">Telefonska fokusna skupina</skos:prefLabel>
      <skos:definition xml:lang="sl">Fokusna skupina, kjer razprava poteka preko telefona.</skos:definition>
      <skos:prefLabel xml:lang="sr">Telefonska fokus grupa</skos:prefLabel>
      <skos:definition xml:lang="sr">Diskusija u okviru fokus grupe vodi se telefonom.</skos:definition>
      <skos:prefLabel xml:lang="sv">Fokusgrupp: telefon</skos:prefLabel>
      <skos:definition xml:lang="sv">Fokusgruppens diskussion förs över telefon.</skos:definition>
      <skos:broader rdf:resource="http://rdf-vocabulary.ddialliance.org/cv/ModeOfCollection/3.0/d64e1426"/>
   </rdf:Description>
   <rdf:Description rdf:about="http://rdf-vocabulary.ddialliance.org/cv/ModeOfCollection/3.0/d64e1704">
      <rdf:type rdf:resource="http://www.w3.org/2004/02/skos/core#Concept"/>
      <skos:inScheme rdf:resource="http://rdf-vocabulary.ddialliance.org/cv/ModeOfCollection/3.0"/>
      <skos:notation>FocusGroup.Online</skos:notation>
      <skos:prefLabel xml:lang="en">Online focus group</skos:prefLabel>
      <skos:definition xml:lang="en">The focus group discussion is conducted over the Internet in an interactive manner.</skos:definition>
      <skos:prefLabel xml:lang="da">Online-fokusgruppe</skos:prefLabel>
      <skos:definition xml:lang="da">Fokusgruppediskussionen gennemføres over internettet på en interaktiv måde.</skos:definition>
      <skos:prefLabel xml:lang="fi">Kohderyhmäkeskustelu: verkkokeskustelu</skos:prefLabel>
      <skos:definition xml:lang="fi">Tutkimustarkoitusta varten järjestetty kohderyhmäkeskustelu tietystä aiheesta. Keskustelu käydään verkossa.</skos:definition>
      <skos:prefLabel xml:lang="fr">Focus group en ligne</skos:prefLabel>
      <skos:definition xml:lang="fr">Les discussions du focus group se font par l'Internet de façon interactive.</skos:definition>
      <skos:prefLabel xml:lang="fr">Focus group en ligne</skos:prefLabel>
      <skos:definition xml:lang="fr">Les discussions du focus group se font par l'Internet de façon interactive.</skos:definition>
      <skos:prefLabel xml:lang="it">Focus group online</skos:prefLabel>
      <skos:definition xml:lang="it">La discussione del focus group è condotta via Internet in modo interattivo.</skos:definition>
      <skos:prefLabel xml:lang="no">Fokusgruppe: Online</skos:prefLabel>
      <skos:definition xml:lang="no">Fokusgruppediskusjonen er gjennomført over internett på en interaktiv måte.</skos:definition>
      <skos:prefLabel xml:lang="pt">Focus group online</skos:prefLabel>
      <skos:definition xml:lang="pt">A discussão do grupo focal é conduzida pela Internet de forma interativa.</skos:definition>
      <skos:prefLabel xml:lang="sl">Spletna fokusna skupina</skos:prefLabel>
      <skos:definition xml:lang="sl">Fokusna skupina, kjer razprava poteka preko spleta na interaktiven način.</skos:definition>
      <skos:prefLabel xml:lang="sr">Onlajn fokus grupa</skos:prefLabel>
      <skos:definition xml:lang="sr">Diskusija u okviru fokus grupe odvija se putem Interneta na interaktivan način.</skos:definition>
      <skos:prefLabel xml:lang="sv">Fokusgrupp: virtuell</skos:prefLabel>
      <skos:definition xml:lang="sv">Fokusgruppens diskussion förs interaktivt över Internet. Kallas även IT-stödd fokusgrupp.</skos:definition>
      <skos:broader rdf:resource="http://rdf-vocabulary.ddialliance.org/cv/ModeOfCollection/3.0/d64e1426"/>
   </rdf:Description>
   <rdf:Description rdf:about="http://rdf-vocabulary.ddialliance.org/cv/ModeOfCollection/3.0/d64e1794">
      <rdf:type rdf:resource="http://www.w3.org/2004/02/skos/core#Concept"/>
      <skos:inScheme rdf:resource="http://rdf-vocabulary.ddialliance.org/cv/ModeOfCollection/3.0"/>
      <skos:notation>SelfAdministeredWritingsAndDiaries</skos:notation>
      <skos:prefLabel xml:lang="en">Self-administered writings and/or diaries</skos:prefLabel>
      <skos:definition xml:lang="en">Narratives, stories, diaries, and written texts created by the research subject.</skos:definition>
      <skos:prefLabel xml:lang="da">Selvadministrerede tekster og/eller dagbøger</skos:prefLabel>
      <skos:definition xml:lang="da">Fortællinger, historier, dagbøger og nedskrevne tekster skabt af forskningssubjektet.</skos:definition>
      <skos:prefLabel xml:lang="fi">Oma kirjoitus tai päiväkirja</skos:prefLabel>
      <skos:definition xml:lang="fi">Osanottajien itse kirjoittamat elämäkerrat, tarinat, päiväkirjat ja muut kirjoitukset.</skos:definition>
      <skos:prefLabel xml:lang="fr">Écrits et / ou journaux intimes auto-administrés</skos:prefLabel>
      <skos:definition xml:lang="fr">Des récits, des histoires, des journaux intimes, et des textes écrits crées par le sujet de recherche.</skos:definition>
      <skos:prefLabel xml:lang="fr">Écrits et / ou journaux intimes auto-administrés</skos:prefLabel>
      <skos:definition xml:lang="fr">Des récits, des histoires, des journaux intimes, et des textes écrits crées par le sujet de recherche.</skos:definition>
      <skos:prefLabel xml:lang="it">Scritti/diari auto-compilati</skos:prefLabel>
      <skos:definition xml:lang="it">Narrazioni, storie, diari e testi scritti creati dai soggetti coinvolti nella ricerca.</skos:definition>
      <skos:prefLabel xml:lang="no">Selvadministrerende tekst og/eller dagbok</skos:prefLabel>
      <skos:definition xml:lang="no">Fortellinger, historier, dagbøker og tekster skrevet av studieobjektene.</skos:definition>
      <skos:prefLabel xml:lang="pt">Textos e/ou diários de autopreenchimento</skos:prefLabel>
      <skos:definition xml:lang="pt">Narrativas, histórias, diários e textos escritos criados/produzidos pelo(s) sujeito(s) da pesquisa.</skos:definition>
      <skos:prefLabel xml:lang="sl">Samoizpolnjevanje zapisov in/ali dnevnikov</skos:prefLabel>
      <skos:definition xml:lang="sl">Pripovedi, zgodbe, dnevniki in napisana besedila, ki jih ustvari subjekt raziskave.</skos:definition>
      <skos:prefLabel xml:lang="sr">Samostalni zapisi i/ili dnevnici</skos:prefLabel>
      <skos:definition xml:lang="sr">Narativi (besede), priče, dnevnici i pisani tekstovi koje je kreirao subjekat istraživanja.</skos:definition>
      <skos:prefLabel xml:lang="sv">Självadministrerad text och/eller dagböcker</skos:prefLabel>
      <skos:definition xml:lang="sv">Narrativ, berättelser, dagböcker och andra nedskrivna texter skapade av forskningspersonerna.</skos:definition>
      <skos:narrower rdf:resource="http://rdf-vocabulary.ddialliance.org/cv/ModeOfCollection/3.0/d64e1891"/>
      <skos:narrower rdf:resource="http://rdf-vocabulary.ddialliance.org/cv/ModeOfCollection/3.0/d64e1981"/>
      <skos:narrower rdf:resource="http://rdf-vocabulary.ddialliance.org/cv/ModeOfCollection/3.0/d64e2071"/>
   </rdf:Description>
   <rdf:Description rdf:about="http://rdf-vocabulary.ddialliance.org/cv/ModeOfCollection/3.0/d64e1891">
      <rdf:type rdf:resource="http://www.w3.org/2004/02/skos/core#Concept"/>
      <skos:inScheme rdf:resource="http://rdf-vocabulary.ddialliance.org/cv/ModeOfCollection/3.0"/>
      <skos:notation>SelfAdministeredWritingsAndDiaries.Email</skos:notation>
      <skos:prefLabel xml:lang="en">Self-administered writings and/or diaries: E-mail</skos:prefLabel>
      <skos:definition xml:lang="en">Narratives, stories, diaries, and written texts submitted via e-mail messages.</skos:definition>
      <skos:prefLabel xml:lang="da">Selvadministrerede tekster og/eller dagbøger: E-mail</skos:prefLabel>
      <skos:definition xml:lang="da">Fortællinger, historier, dagbøger og nedskrevne tekster afleveret via e-mail-beskeder.</skos:definition>
      <skos:prefLabel xml:lang="fi">Oma kirjoitus tai päiväkirja: sähköpostilla saatu</skos:prefLabel>
      <skos:definition xml:lang="fi">Osanottajien sähköpostin välityksellä annetut omat kirjoitukset ja päiväkirjat.</skos:definition>
      <skos:prefLabel xml:lang="fr">crits et / ou journaux intimes auto-administrés : e-mail</skos:prefLabel>
      <skos:definition xml:lang="fr">Des récits, des histoires, des journaux intimes, et des textes écrits soumis par courriel.</skos:definition>
      <skos:prefLabel xml:lang="fr">crits et / ou journaux intimes auto-administrés : e-mail</skos:prefLabel>
      <skos:definition xml:lang="fr">Des récits, des histoires, des journaux intimes, et des textes écrits soumis par courriel.</skos:definition>
      <skos:prefLabel xml:lang="it">Scritti/diari auto-compilati: e-mail</skos:prefLabel>
      <skos:definition xml:lang="it">Narrazioni, storie, diari e testi scritti inviati tramite e-mail.</skos:definition>
      <skos:prefLabel xml:lang="no">Selvadministrerende tekst og/eller dagbok: E-post</skos:prefLabel>
      <skos:definition xml:lang="no">Fortellinger, historier, dagbøker og tekster som har blitt samlet inn via e-post.</skos:definition>
      <skos:prefLabel xml:lang="pt">Textos e/ou diários de autopreenchimento: Email</skos:prefLabel>
      <skos:definition xml:lang="pt">Narrativas, histórias, diários e textos escritos enviados por mensagens de email.</skos:definition>
      <skos:prefLabel xml:lang="sl">Samoizpolnjevanje zapisov in/ali dnevnikov: elektronska pošta</skos:prefLabel>
      <skos:definition xml:lang="sl">Pripovedi, zgodbe, dnevniki in napisana besedila, ki so posredovana preko elektronskih poštnih sporočil.</skos:definition>
      <skos:prefLabel xml:lang="sr">Samostalni zapisi i/ili dnevnici: Elektronskom poštom</skos:prefLabel>
      <skos:definition xml:lang="sr">Narativi (besede), priče, dnevnici i pisani tekstovi koje ispitanik šalje elektronskom poštom.</skos:definition>
      <skos:prefLabel xml:lang="sv">Självadministrerad text och/eller dagböcker: e-post</skos:prefLabel>
      <skos:definition xml:lang="sv">Narrativ, berättelser, dagböcker och andra nedskrivna texter som skickas in via e-post.</skos:definition>
      <skos:broader rdf:resource="http://rdf-vocabulary.ddialliance.org/cv/ModeOfCollection/3.0/d64e1794"/>
   </rdf:Description>
   <rdf:Description rdf:about="http://rdf-vocabulary.ddialliance.org/cv/ModeOfCollection/3.0/d64e1981">
      <rdf:type rdf:resource="http://www.w3.org/2004/02/skos/core#Concept"/>
      <skos:inScheme rdf:resource="http://rdf-vocabulary.ddialliance.org/cv/ModeOfCollection/3.0"/>
      <skos:notation>SelfAdministeredWritingsAndDiaries.Paper</skos:notation>
      <skos:prefLabel xml:lang="en">Self-administered writings and/or diaries: Paper</skos:prefLabel>
      <skos:definition xml:lang="en">Narratives, stories, diaries, and written texts created and collected in paper form.</skos:definition>
      <skos:prefLabel xml:lang="da">Selvadministrerede tekster og/eller dagbøger: Papir</skos:prefLabel>
      <skos:definition xml:lang="da">Fortællinger, historier, dagbøger og nedskrevne tekster skabt og indsamlet i papirform.</skos:definition>
      <skos:prefLabel xml:lang="fi">Oma kirjoitus tai päiväkirja: paperimuotoinen kirjoitus</skos:prefLabel>
      <skos:definition xml:lang="fi">Osanottajien paperimuotoiset omat kirjoitukset ja päiväkirjat.</skos:definition>
      <skos:prefLabel xml:lang="fr">Écrits et / ou journaux intimes auto-administrés : papier</skos:prefLabel>
      <skos:definition xml:lang="fr">Des récits, des histoires, des journaux intimes, et des textes écrits crées et rassemblés sous forme papier.</skos:definition>
      <skos:prefLabel xml:lang="fr">Écrits et / ou journaux intimes auto-administrés : papier</skos:prefLabel>
      <skos:definition xml:lang="fr">Des récits, des histoires, des journaux intimes, et des textes écrits crées et rassemblés sous forme papier.</skos:definition>
      <skos:prefLabel xml:lang="it">Scritti/diari auto-compilati: cartaceo</skos:prefLabel>
      <skos:definition xml:lang="it">Narrazioni, storie, diari e testi scritti creati e raccolti in forma cartacea.</skos:definition>
      <skos:prefLabel xml:lang="no">Selvadministrerende tekst og/eller dagbok: Papir</skos:prefLabel>
      <skos:definition xml:lang="no">Fortellinger, historier, dagbøker og tekster skrevet og samlet i papirformat.</skos:definition>
      <skos:prefLabel xml:lang="pt">Textos e/ou diários de autopreenchimento: Papel</skos:prefLabel>
      <skos:definition xml:lang="pt">Narrativas, histórias, diários e textos escritos criados e recolhidos em papel.</skos:definition>
      <skos:prefLabel xml:lang="sl">Samoizpolnjevanje zapisov in/ali dnevnikov: papir</skos:prefLabel>
      <skos:definition xml:lang="sl">Pripovedi, zgodbe, dnevniki in napisana besedila, ki so ustvarjena in zbrana na papirju.</skos:definition>
      <skos:prefLabel xml:lang="sr">Samostalni zapisi i/ili dnevnici: Papirni</skos:prefLabel>
      <skos:definition xml:lang="sr">Narativi (besede), priče, dnevnici i pisani tekstovi koje ispitanik prilaže u papirnom obliku.</skos:definition>
      <skos:prefLabel xml:lang="sv">Självadministrerad text och/eller dagböcker: papper</skos:prefLabel>
      <skos:definition xml:lang="sv">Narrativ, berättelser, dagböcker och andra nedskrivna texter som skapats och samlats in på papper.</skos:definition>
      <skos:broader rdf:resource="http://rdf-vocabulary.ddialliance.org/cv/ModeOfCollection/3.0/d64e1794"/>
   </rdf:Description>
   <rdf:Description rdf:about="http://rdf-vocabulary.ddialliance.org/cv/ModeOfCollection/3.0/d64e2071">
      <rdf:type rdf:resource="http://www.w3.org/2004/02/skos/core#Concept"/>
      <skos:inScheme rdf:resource="http://rdf-vocabulary.ddialliance.org/cv/ModeOfCollection/3.0"/>
      <skos:notation>SelfAdministeredWritingsAndDiaries.WebBased</skos:notation>
      <skos:prefLabel xml:lang="en">Self-administered writings and/or diaries: Web-based</skos:prefLabel>
      <skos:definition xml:lang="en">Narratives, stories, diaries, and written texts gathered from Internet sources, e.g. websites, blogs, discussion forums.</skos:definition>
      <skos:prefLabel xml:lang="da">Selvadministrerede tekster og/eller dagbøger: Webbaseret</skos:prefLabel>
      <skos:definition xml:lang="da">Fortællinger, historier, dagbøger og nedskrevne tekster indsamlet fra internetkilder, for eksempel hjemmesider, blogs og diskussionsfora.</skos:definition>
      <skos:prefLabel xml:lang="fi">Oma kirjoitus tai päiväkirja: verkon kautta saatu</skos:prefLabel>
      <skos:definition xml:lang="fi">Osanottajien verkossa kirjoitetut omat kirjoitukset ja päiväkirjat.</skos:definition>
      <skos:prefLabel xml:lang="fr">Écrits et / ou journaux intimes auto-administrés : en ligne</skos:prefLabel>
      <skos:definition xml:lang="fr">Des récits, des histoires, des journaux intimes, et des textes écrits provenant d'Internet, e. g. des sites Internet, des blogs, des forums de discussion.</skos:definition>
      <skos:prefLabel xml:lang="fr">Écrits et / ou journaux intimes auto-administrés : en ligne</skos:prefLabel>
      <skos:definition xml:lang="fr">Des récits, des histoires, des journaux intimes, et des textes écrits provenant d'Internet, e. g. des sites Internet, des blogs, des forums de discussion.</skos:definition>
      <skos:prefLabel xml:lang="it">Scritti/diari auto-compilati: web</skos:prefLabel>
      <skos:definition xml:lang="it">Narrazioni, storie, diari e testi scritti raccolti su Internet, ad esempio da siti web, blog, forum di discussione.</skos:definition>
      <skos:prefLabel xml:lang="no">Selvadministrerende tekst og/eller dagbok: Webbasert</skos:prefLabel>
      <skos:definition xml:lang="no">Fortellinger, historier, dagbøker og tekster samlet fra internett, e.g. nettsider, blogger, diskusjonsforumer.</skos:definition>
      <skos:prefLabel xml:lang="pt">Textos e/ou diários de autopreenchimento: Online/via web</skos:prefLabel>
      <skos:definition xml:lang="pt">Narrativas, histórias, diários e textos escritos recolhidos de fontes da Internet, por ex. sites, blogs, fóruns de discussão.</skos:definition>
      <skos:prefLabel xml:lang="sl">Samoizpolnjevanje zapisov in/ali dnevnikov: spletno</skos:prefLabel>
      <skos:definition xml:lang="sl">Pripovedi, zgodbe, dnevniki in napisana besedila, ki so zbrana preko internetnih virov, npr. spletne strani, blogi, forumi.</skos:definition>
      <skos:prefLabel xml:lang="sr">Samostalni zapisi i/ili dnevnici: Veb</skos:prefLabel>
      <skos:definition xml:lang="sr">Narativi (besede), priče, dnevnici i pisani tekstovi prikupljeni iz Internet izvora, na primer veb sajtova, blogova, diskusionih grupa.</skos:definition>
      <skos:prefLabel xml:lang="sv">Självadministrerad text och/eller dagböcker: webbaserat</skos:prefLabel>
      <skos:definition xml:lang="sv">Narrativ, berättelser, dagböcker och andra nedskrivna texter som samlats in från Internet-källor, t.ex. webbplatser, bloggar, diskussionsforum.</skos:definition>
      <skos:broader rdf:resource="http://rdf-vocabulary.ddialliance.org/cv/ModeOfCollection/3.0/d64e1794"/>
   </rdf:Description>
   <rdf:Description rdf:about="http://rdf-vocabulary.ddialliance.org/cv/ModeOfCollection/3.0/d64e2162">
      <rdf:type rdf:resource="http://www.w3.org/2004/02/skos/core#Concept"/>
      <skos:inScheme rdf:resource="http://rdf-vocabulary.ddialliance.org/cv/ModeOfCollection/3.0"/>
      <skos:notation>Observation</skos:notation>
      <skos:prefLabel xml:lang="en">Observation</skos:prefLabel>
      <skos:definition xml:lang="en">Research method that involves collecting data as they occur (for example, observing behaviors, events, development of condition or disease, etc.), without attempting to manipulate any of the independent variables.</skos:definition>
      <skos:prefLabel xml:lang="da">Observation</skos:prefLabel>
      <skos:definition xml:lang="da">Forskningsmetode, der involverer at indsamle data, som de opstår (for eksempel observering af opførsel, begivenheder, udviklingen af tilstand eller sygdom mm.) uden at forsøge at manipulere de uafhængige variable.</skos:definition>
      <skos:prefLabel xml:lang="fi">Havainnointi</skos:prefLabel>
      <skos:definition xml:lang="fi">Keruumenetelmä, jossa tarkkaillaan tapahtumia, käyttäytymistä, vuorovaikutusta jne. niiden tapahtuessa, ilman minkään riippumattoman muuttujan manipulointia.</skos:definition>
      <skos:prefLabel xml:lang="fr">Observation</skos:prefLabel>
      <skos:definition xml:lang="fr">Méthode de recherche qui consiste à collecter des données au fur et à mesure qu'elle se produisent (par exemple, observation de comportements, d’événements, de l'évolution d'un état ou d'une maladie, etc.), sans tentative de manipuler aucune des variables indépendantes.</skos:definition>
      <skos:prefLabel xml:lang="fr">Observation</skos:prefLabel>
      <skos:definition xml:lang="fr">Méthode de recherche qui consiste à collecter des données au fur et à mesure qu'elle se produisent (par exemple, observation de comportements, d’événements, de l'évolution d'un état ou d'une maladie, etc.), sans tentative de manipuler aucune des variables indépendantes.</skos:definition>
      <skos:prefLabel xml:lang="it">Osservazione</skos:prefLabel>
      <skos:definition xml:lang="it">Tecnica di rilevazione che implica la raccolta di dati nel momento in cui si generano (ad esempio osservando comportamenti, eventi, sviluppo di condizioni o malattie, ecc.), senza tentare di manipolare nessuna delle variabili indipendenti.</skos:definition>
      <skos:prefLabel xml:lang="no">Observasjon</skos:prefLabel>
      <skos:definition xml:lang="no">Forskningsmetode som innebærer å samle inn data etterhvert som de opptrår (for eksempel, observere atferd, hendelser, utviklingen av helsetilstand eller sykdom, etc.) uten å prøve å manipulere noen av de uavhengige variablene.</skos:definition>
      <skos:prefLabel xml:lang="pt">Observação</skos:prefLabel>
      <skos:definition xml:lang="pt">Método de investigação que envolve a recolha de dados conforme eles ocorrem (por exemplo, observando comportamentos, eventos, desenvolvimento de uma condição ou doença, etc.), sem tentar manipular nenhuma das variáveis independentes.</skos:definition>
      <skos:prefLabel xml:lang="sl">Opazovanje</skos:prefLabel>
      <skos:definition xml:lang="sl">Raziskovalna metoda, ki vključuje zbiranje podatkov, ko se pojavijo (npr. opazovanje vedenj, dogodkov, razvoja stanja ali bolezni itd.), ne da bi poskušali manipulirati s katero od neodvisnih spremenljivk.</skos:definition>
      <skos:prefLabel xml:lang="sr">Opservacije / posmatranje</skos:prefLabel>
      <skos:definition xml:lang="sr">Metoda istraživanja koja uključuje prikupljanje podataka kako se pojavljuju (na primer, posmatranje ponašanja, događaja, razvoj stanja ili bolesti itd.), bez pokušaja manipulacije bilo kojom nezavisnom promenljivom.</skos:definition>
      <skos:prefLabel xml:lang="sv">Observation</skos:prefLabel>
      <skos:definition xml:lang="sv">Forskningsmetod som omfattar att samla in data om företeelser när de uppträder (t.ex. observationer av beteenden, händelser m.m.) utan att försöka påverka några av de oberoende variablerna.</skos:definition>
      <skos:narrower rdf:resource="http://rdf-vocabulary.ddialliance.org/cv/ModeOfCollection/3.0/d64e2259"/>
      <skos:narrower rdf:resource="http://rdf-vocabulary.ddialliance.org/cv/ModeOfCollection/3.0/d64e2534"/>
      <skos:narrower rdf:resource="http://rdf-vocabulary.ddialliance.org/cv/ModeOfCollection/3.0/d64e2810"/>
   </rdf:Description>
   <rdf:Description rdf:about="http://rdf-vocabulary.ddialliance.org/cv/ModeOfCollection/3.0/d64e2259">
      <rdf:type rdf:resource="http://www.w3.org/2004/02/skos/core#Concept"/>
      <skos:inScheme rdf:resource="http://rdf-vocabulary.ddialliance.org/cv/ModeOfCollection/3.0"/>
      <skos:notation>Observation.Field</skos:notation>
      <skos:prefLabel xml:lang="en">Field observation</skos:prefLabel>
      <skos:definition xml:lang="en">Observation that is conducted in a natural environment.</skos:definition>
      <skos:prefLabel xml:lang="da">Feltobservation</skos:prefLabel>
      <skos:definition xml:lang="da">Observation, som udføres i et naturligt miljø.</skos:definition>
      <skos:prefLabel xml:lang="fi">Havainnointi: kenttähavainnointi</skos:prefLabel>
      <skos:definition xml:lang="fi">Havainnointi suoritetaan luonnollisessa, kontrolloimattomassa ympäristössä. Käytä termiä mikäli ei tiedossa onko osallistuvaa vai ei-osallistuvaa.</skos:definition>
      <skos:prefLabel xml:lang="fr">Observation sur le terrain</skos:prefLabel>
      <skos:definition xml:lang="fr">Observation qui a été conduite dans un environnement naturel.</skos:definition>
      <skos:prefLabel xml:lang="fr">Observation sur le terrain</skos:prefLabel>
      <skos:definition xml:lang="fr">Observation qui a été conduite dans un environnement naturel.</skos:definition>
      <skos:prefLabel xml:lang="it">Osservazione sul campo</skos:prefLabel>
      <skos:definition xml:lang="it">Osservazione condotta in un ambiente naturale.</skos:definition>
      <skos:prefLabel xml:lang="no">Feltobservasjon</skos:prefLabel>
      <skos:definition xml:lang="no">Observasjon som utføres i et naturlig miljø.</skos:definition>
      <skos:prefLabel xml:lang="pt">Observação de campo</skos:prefLabel>
      <skos:definition xml:lang="pt">Observação conduzida em ambiente natural.</skos:definition>
      <skos:prefLabel xml:lang="sl">Opazovanje na terenu</skos:prefLabel>
      <skos:definition xml:lang="sl">Opazovanje, ki se izvaja v naravnem okolju.</skos:definition>
      <skos:prefLabel xml:lang="sr">Terenska posmatranja</skos:prefLabel>
      <skos:definition xml:lang="sr">Opservacije koje se sprovode u prirodnom okruženju.</skos:definition>
      <skos:prefLabel xml:lang="sv">Fältobservation</skos:prefLabel>
      <skos:definition xml:lang="sv">Observation som utförs i en naturlig miljö.</skos:definition>
      <skos:narrower rdf:resource="http://rdf-vocabulary.ddialliance.org/cv/ModeOfCollection/3.0/d64e2354"/>
      <skos:narrower rdf:resource="http://rdf-vocabulary.ddialliance.org/cv/ModeOfCollection/3.0/d64e2444"/>
      <skos:broader rdf:resource="http://rdf-vocabulary.ddialliance.org/cv/ModeOfCollection/3.0/d64e2162"/>
   </rdf:Description>
   <rdf:Description rdf:about="http://rdf-vocabulary.ddialliance.org/cv/ModeOfCollection/3.0/d64e2534">
      <rdf:type rdf:resource="http://www.w3.org/2004/02/skos/core#Concept"/>
      <skos:inScheme rdf:resource="http://rdf-vocabulary.ddialliance.org/cv/ModeOfCollection/3.0"/>
      <skos:notation>Observation.Laboratory</skos:notation>
      <skos:prefLabel xml:lang="en">Laboratory observation</skos:prefLabel>
      <skos:definition xml:lang="en">Observation that is conducted in a controlled, artificially created setting. For example, observing children's play in a laboratory playroom.</skos:definition>
      <skos:prefLabel xml:lang="da">Laboratorieobservation</skos:prefLabel>
      <skos:definition xml:lang="da">Observation, der udføres i en kontrolleret, kunstig skabt opsætning. For eksempel observering af børns leg i et laboratoriums legerum.</skos:definition>
      <skos:prefLabel xml:lang="fi">Havainnointi: laboratoriohavainnointi</skos:prefLabel>
      <skos:definition xml:lang="fi">Kokeellinen havainnointi kontrolloidussa, tarkoitusta varten luodussa tilassa tai ympäristössä. Esimerkki: Lasten leikkien havainnointi laboratorioon rakennetussa leikkihuoneessa. Käytä tätä termiä mikäli ei ole tiedossa onko laboratoriohavainnointi osallistuvaa vai ei-osallistuvaa.</skos:definition>
      <skos:prefLabel xml:lang="fr">Observation en laboratoire</skos:prefLabel>
      <skos:definition xml:lang="fr">Observation qui a été conduite dans un configuration contrôlée, artificiellement créée. Par exemple, l'observation du jeu des enfants dans une salle de jeux de laboratoire.</skos:definition>
      <skos:prefLabel xml:lang="fr">Observation en laboratoire</skos:prefLabel>
      <skos:definition xml:lang="fr">Observation qui a été conduite dans un configuration contrôlée, artificiellement créée. Par exemple, l'observation du jeu des enfants dans une salle de jeux de laboratoire.</skos:definition>
      <skos:prefLabel xml:lang="it">Osservazione in laboratorio</skos:prefLabel>
      <skos:definition xml:lang="it">Osservazione condotta in un ambiente controllato, creato artificialmente. Ad esempio, osservazione del gioco dei bambini in una stanza da gioco ricreata in laboratorio.</skos:definition>
      <skos:prefLabel xml:lang="no">Laboratorieobservasjon</skos:prefLabel>
      <skos:definition xml:lang="no">Observasjon som er utført i et kontrollert, kunstig konstruert miljø. For eksempel observasjon av barns lek i et lekerom i laboratoriet.</skos:definition>
      <skos:prefLabel xml:lang="pt">Observação em laboratório</skos:prefLabel>
      <skos:definition xml:lang="pt">Observação que é conduzida/realizada em ambiente controlado e artificialmente criado. Por exemplo, observação das brincadeiras das crianças numa sala de jogos de laboratório.</skos:definition>
      <skos:prefLabel xml:lang="sl">Laboratorijsko opazovanje</skos:prefLabel>
      <skos:definition xml:lang="sl">Opazovanje, ki se izvaja v nadzorovanem, umetno ustvarjenem okolju. Na primer, opazovanje otroške igre v laboratorijski igralnici.</skos:definition>
      <skos:prefLabel xml:lang="sr">Laboratorijsko posmatranje</skos:prefLabel>
      <skos:definition xml:lang="sr">Posmatranje koje se izvodi u kontrolisanom, veštački stvorenom okruženju. Na primer, posmatranje igre dece u laboratorijskoj igraonici.</skos:definition>
      <skos:prefLabel xml:lang="sv">Laboratorieobservation</skos:prefLabel>
      <skos:definition xml:lang="sv">Observation som utförs i en kontrollerad, konstgjord miljö. Exempel: observation av barns lek i ett laboratorielekrum.</skos:definition>
      <skos:narrower rdf:resource="http://rdf-vocabulary.ddialliance.org/cv/ModeOfCollection/3.0/d64e2629"/>
      <skos:narrower rdf:resource="http://rdf-vocabulary.ddialliance.org/cv/ModeOfCollection/3.0/d64e2720"/>
      <skos:broader rdf:resource="http://rdf-vocabulary.ddialliance.org/cv/ModeOfCollection/3.0/d64e2162"/>
   </rdf:Description>
   <rdf:Description rdf:about="http://rdf-vocabulary.ddialliance.org/cv/ModeOfCollection/3.0/d64e2629">
      <rdf:type rdf:resource="http://www.w3.org/2004/02/skos/core#Concept"/>
      <skos:inScheme rdf:resource="http://rdf-vocabulary.ddialliance.org/cv/ModeOfCollection/3.0"/>
      <skos:notation>Observation.Laboratory.Participant</skos:notation>
      <skos:prefLabel xml:lang="en">Participant laboratory observation</skos:prefLabel>
      <skos:definition xml:lang="en">Type of laboratory observation in which the researcher interacts with the subjects and often plays a role in the social situation under observation. For example, observing children's play in a laboratory playroom with the researcher taking part in the play.</skos:definition>
      <skos:prefLabel xml:lang="da">Laboratorieobservation med deltager</skos:prefLabel>
      <skos:definition xml:lang="da">Type af laboratorieobservation, hvor forskeren interagerer med subjekterne og ofte spiller en rolle i den sociale situation under observation. For eksempel observering af børns leg i et laboratorielegerum med forskeren, der deltager i legen.</skos:definition>
      <skos:prefLabel xml:lang="fi">Havainnointi: laboratoriohavainnointi: osallistuva</skos:prefLabel>
      <skos:definition xml:lang="fi">Kokeellinen havainnointi kontrolloidussa, tarkoitusta varten luodussa tilassa. Tutkija on vuorovaikutuksessa tutkittavien kanssa ja hänellä on usein jokin rooli tutkimuksen kohteena olevassa sosiaalisessa tilanteessa. Esimerkki: Lasten leikkien havainnointi laboratorioon rakennetussa leikkihuoneessa, jossa tutkija ottaa osaa leikkiin.</skos:definition>
      <skos:prefLabel xml:lang="fr">Observation participante en laboratoire</skos:prefLabel>
      <skos:definition xml:lang="fr">Type d'observation en laboratoire dans lequel le sujet interagit avec les sujets et joue souvent un rôle dans la situation sociale sous observation. Par exemple, l'observation du jeu des enfants dans une salle de jeux de laboratoire avec le chercheur prenant part au jeu.</skos:definition>
      <skos:prefLabel xml:lang="fr">Observation participante en laboratoire</skos:prefLabel>
      <skos:definition xml:lang="fr">Type d'observation en laboratoire dans lequel le sujet interagit avec les sujets et joue souvent un rôle dans la situation sociale sous observation. Par exemple, l'observation du jeu des enfants dans une salle de jeux de laboratoire avec le chercheur prenant part au jeu.</skos:definition>
      <skos:prefLabel xml:lang="it">Osservazione partecipante in laboratorio</skos:prefLabel>
      <skos:definition xml:lang="it">Tipo di osservazione in laboratorio in cui il ricercatore interagisce con i soggetti e spesso gioca un ruolo nella situazione sociale sotto osservazione. Ad esempio, osservando il gioco dei bambini in una stanza da gioco ricreata in laboratorio con il ricercatore che partecipa al gioco.</skos:definition>
      <skos:prefLabel xml:lang="no">Deltagende laboratorieobservasjon</skos:prefLabel>
      <skos:definition xml:lang="no">En type laboratorieobservasjon hvor forskeren samhandler med forskningsobjektene, og ofte spiller en rolle i den sosiale situasjonen som er under observasjon. For eksempel observere barns lek i et lekerom i laboratoriet, der forsker deltar i leken.</skos:definition>
      <skos:prefLabel xml:lang="pt">Observação participante em laboratório</skos:prefLabel>
      <skos:definition xml:lang="pt">Tipo de observação em laboratório em que o investigador interage com os sujeitos e, muitas vezes, desempenha um papel na situação social em observação. Por exemplo, observação das brincadeiras das crianças numa sala de jogos de laboratório com o investigador a participar no jogo.</skos:definition>
      <skos:prefLabel xml:lang="sl">Laboratorijsko opazovanje z udeležbo</skos:prefLabel>
      <skos:definition xml:lang="sl">Vrsta laboratorijskega opazovanja, kjer je raziskovalec v interkaciji s subjekti in pogosto igra vlogo v opazovani družbeni situaciji. Na primer, opazovanje otroške igre v laboratorijski igralnici, kjer ima raziskovalec vlogo v igri.</skos:definition>
      <skos:prefLabel xml:lang="sr">Laboratorijsko posmatranje sa učešćem</skos:prefLabel>
      <skos:definition xml:lang="sr">Vrsta laboratorijskog posmatranja u kome istraživač komunicira sa subjektima i često igra ulogu u posmatranom socijalnom stanju. Na primer, posmatranje igre dece u laboratorijskoj igraonici sa istraživačem koji učestvuje u predstavi.</skos:definition>
      <skos:prefLabel xml:lang="sv">Deltagande laboratorieobservation</skos:prefLabel>
      <skos:definition xml:lang="sv">Laboratorieobservation där forskaren interagerar med forskningsobjekten och ofta har en funktion i den sociala situation som observeras. Exempel: observation av barns lek i ett laboratorielekrum där forskaren deltar i leken.</skos:definition>
      <skos:broader rdf:resource="http://rdf-vocabulary.ddialliance.org/cv/ModeOfCollection/3.0/d64e2534"/>
   </rdf:Description>
   <rdf:Description rdf:about="http://rdf-vocabulary.ddialliance.org/cv/ModeOfCollection/3.0/d64e2810">
      <rdf:type rdf:resource="http://www.w3.org/2004/02/skos/core#Concept"/>
      <skos:inScheme rdf:resource="http://rdf-vocabulary.ddialliance.org/cv/ModeOfCollection/3.0"/>
      <skos:notation>Observation.ComputerBased</skos:notation>
      <skos:prefLabel xml:lang="en">Computer-based observation</skos:prefLabel>
      <skos:definition xml:lang="en">Type of observation in which data regarding computer usage are being collected by software that can be built into the computer program itself or can be a separate program. Information may be collected about the number of users, the ways in which users interact with the program(s), how much time they spend on a page, how they use specific sections of applications, how they navigate from page to page or from one application to another, etc.</skos:definition>
      <skos:prefLabel xml:lang="da">Computerbaseret observation</skos:prefLabel>
      <skos:definition xml:lang="da">Observationstype, hvor data vedrørende computerbrug indsamles af software, der kan indbygges i selve computerprogrammet eller kan være et særskilt program. Oplysninger kan indsamles om antallet af brugere, hvordan brugere interagerer med programmet (programmerne), hvor meget tid de bruger på en side, hvordan de anvender bestemte sektioner af applikationer, hvordan de navigerer fra side til side eller fra en applikation til en anden mm.</skos:definition>
      <skos:prefLabel xml:lang="fi">Havainnointi: tietokonepohjainen havainnointi</skos:prefLabel>
      <skos:definition xml:lang="fi">Havainnointimenetelmä, jossa kerätään tietoa ihmisten tietokoneen käytöstä ohjelmallisesti. Havainnointiohjelma voi olla sisäänrakennettu tietokoneohjelmaan tai se voi olla erillinen ohjelma. Tietoa voidaan kerätä käyttäjien määristä, heidän tavoistaan käyttää ohjelmaa ja sen toimintoja, navigoinnista jne.</skos:definition>
      <skos:prefLabel xml:lang="fr">Observation assisté par ordinateur</skos:prefLabel>
      <skos:definition xml:lang="fr">Type d'observation dans lequel les données relatives à l'utilisation de l'ordinateur ont été collectées par un logiciel qui peut être intégré dans un programme informatique lui-même ou qui peut être un programme séparé. Des informations peuvent être collectées à propos du nombre d'utilisateurs, les façons dans lesquels les utilisateurs interagissent avec le(s) programme(s), combien de temps ils passent sur une page, comment ils utilisent des sections spécifiques des applications, comment ils naviguent d'une page à l'autre ou d'une application à l'autre, etc.</skos:definition>
      <skos:prefLabel xml:lang="fr">Observation assisté par ordinateur</skos:prefLabel>
      <skos:definition xml:lang="fr">Type d'observation dans lequel les données relatives à l'utilisation de l'ordinateur ont été collectées par un logiciel qui peut être intégré dans un programme informatique lui-même ou qui peut être un programme séparé. Des informations peuvent être collectées à propos du nombre d'utilisateurs, les façons dans lesquels les utilisateurs interagissent avec le(s) programme(s), combien de temps ils passent sur une page, comment ils utilisent des sections spécifiques des applications, comment ils naviguent d'une page à l'autre ou d'une application à l'autre, etc.</skos:definition>
      <skos:prefLabel xml:lang="it">Osservazione basata su computer</skos:prefLabel>
      <skos:definition xml:lang="it">Tipo di osservazione in cui vengono raccolti dati riguardanti l'uso del computer, attraverso software che può essere incorporato nel programma informatico stesso, oppure essere un programma separato. Con questo metodo si possono raccogliere informazioni sul numero di utenti, sui modi in cui gli utenti interagiscono con il programma, sulla quantità di tempo che trascorrono su una pagina, su come utilizzano specifiche sezioni di applicazioni, su come navigano da una pagina all'altra o da una applicazione all'altra, ecc.</skos:definition>
      <skos:prefLabel xml:lang="no">Datamaskinbasert observasjon</skos:prefLabel>
      <skos:definition xml:lang="no">Type observasjon hvor data om datamaskinbruk blir samlet av program som kan være inkludert i dataprogrammet en ønsker informasjon om, eller kan forekomme som et eget program. Informasjon om antall brukere, måten brukere samhandler med program(met/mene), hvor mye tid de bruker på siden, hvordan de bruker bestemte deler av en applikasjon, hvordan de navigerer fra side til side eller fra en applikasjon til en annen etc., kan bli samlet.</skos:definition>
      <skos:prefLabel xml:lang="pt">Observação assistida por computador</skos:prefLabel>
      <skos:definition xml:lang="pt">Tipo de observação em que os dados referentes ao uso do computador são recolhidos através de software que pode estar incorporado no próprio programa do computador, ou pode constituir um programa separado. Pode ser recolhida informação sobre o número de utilizadores, a forma como os utilizadores interagem com o(s) programa(s), quanto tempo passam numa página, como usam secções específicas de aplicações, como navegam de uma página para outra ou de uma aplicação para outra, etc.</skos:definition>
      <skos:prefLabel xml:lang="sl">Računalniško podprto opazovanje</skos:prefLabel>
      <skos:definition xml:lang="sl">Vrsta opazovanja, kjer se podatki o uporabi računalnika zbirajo s programsko opremo, ki se jo lahko vgradi v sam računalniški program ali pa predstavlja ločen program. Lahko se zbirajo informacije o številu uporabnikov, o načinih interakcije uporabnikov z računalniškim(i) programom(-mi), koliko časa porabijo na strani, kako uporabljajo določene dele aplikacije, kako krmarijo po straneh ali med aplikacijami itd.</skos:definition>
      <skos:prefLabel xml:lang="sr">Posmatranje podržano računarom</skos:prefLabel>
      <skos:definition xml:lang="sr">Vrsta posmatranja u kome se podaci o upotrebi računara prikupljaju softverom koji može biti ugrađen u sam računar ili može biti zaseban program. Mogu se prikupiti informacije o broju korisnika, načinima na koji korisnici komuniciraju sa programima, koliko vremena provode na veb stranici, kako koriste određene odeljke aplikacija, kako prelaze sa stranice na stranicu ili sa jedne aplikacije na drugu, itd.</skos:definition>
      <skos:prefLabel xml:lang="sv">Datorbaserade observation</skos:prefLabel>
      <skos:definition xml:lang="sv">Observation där data om datoranvändning samlas in av programvara som inkluderats i ett datorprogram eller som kan vara ett separat program. Information kan samlas in om antal användare, hur användare interagerar med programmet, hur länge de stannar på en sida, hur de använder bestämda delar av program, hur de navigerar från en sida till en annan eller växlar mellan program m.m.</skos:definition>
      <skos:broader rdf:resource="http://rdf-vocabulary.ddialliance.org/cv/ModeOfCollection/3.0/d64e2162"/>
   </rdf:Description>
   <rdf:Description rdf:about="http://rdf-vocabulary.ddialliance.org/cv/ModeOfCollection/3.0/d64e2354">
      <rdf:type rdf:resource="http://www.w3.org/2004/02/skos/core#Concept"/>
      <skos:inScheme rdf:resource="http://rdf-vocabulary.ddialliance.org/cv/ModeOfCollection/3.0"/>
      <skos:notation>Observation.Field.Participant</skos:notation>
      <skos:prefLabel xml:lang="en">Participant field observation</skos:prefLabel>
      <skos:definition xml:lang="en">Type of field observation in which the researcher interacts with the subjects and often plays a role in the social situation under observation.</skos:definition>
      <skos:prefLabel xml:lang="da">Feltobservation med deltager</skos:prefLabel>
      <skos:definition xml:lang="da">Type af feltobservation, hvor forskeren interagerer med subjekterne og ofte spiller en rolle i den sociale situation under observation.</skos:definition>
      <skos:prefLabel xml:lang="fi">Havainnointi: kenttähavainnointi: osallistuva</skos:prefLabel>
      <skos:definition xml:lang="fi">Havainnointi suoritetaan luonnollisessa, kontrolloimattomassa ympäristössä. Tutkija on vuorovaikutuksessa tutkittavien kanssa ja hänellä on usein jokin rooli tutkinnan kohteena olevassa sosiaalisessa tilanteessa.</skos:definition>
      <skos:prefLabel xml:lang="fr">Observation participante sur le terrain</skos:prefLabel>
      <skos:definition xml:lang="fr">Type d'observation sur le terrain dans lequel le chercheur interagit avec les sujets et joue souvent un rôle dans la situation sociale sous observation.</skos:definition>
      <skos:prefLabel xml:lang="fr">Observation participante sur le terrain</skos:prefLabel>
      <skos:definition xml:lang="fr">Type d'observation sur le terrain dans lequel le chercheur interagit avec les sujets et joue souvent un rôle dans la situation sociale sous observation.</skos:definition>
      <skos:prefLabel xml:lang="it">Osservazione partecipante sul campo</skos:prefLabel>
      <skos:definition xml:lang="it">Tipo di osservazione sul campo nella quale il ricercatore interagisce con i soggetti e spesso ricopre un ruolo nella situazione sociale sotto osservazione.</skos:definition>
      <skos:prefLabel xml:lang="no">Deltagende feltobservasjon</skos:prefLabel>
      <skos:definition xml:lang="no">Type feltobservasjon hvor forskeren samhandler og ofte spiller en rolle i de sosiale situasjonene som observeres.</skos:definition>
      <skos:prefLabel xml:lang="pt">Observação participante </skos:prefLabel>
      <skos:definition xml:lang="pt">Tipo de observação no trabalho de campo em que o investigador interage com os sujeitos e, muitas vezes, desempenha um papel na situação social em observação.</skos:definition>
      <skos:prefLabel xml:lang="sl">Opazovanje na terenu z udeležbo</skos:prefLabel>
      <skos:definition xml:lang="sl">Vrsta opazovanja, kjer je raziskovalec v interakciji z raziskovalnim subjektom in pogosto igra vlogo v opazovani družbeni situaciji.</skos:definition>
      <skos:prefLabel xml:lang="sr">Terensko posmatranje sa učešćem</skos:prefLabel>
      <skos:definition xml:lang="sr">Vrsta terenskog posmatranja u kome istraživač komunicira sa subjektima i često igra ulogu u posmatranom socijalnom stanju.</skos:definition>
      <skos:prefLabel xml:lang="sv">Deltagande fältobservation</skos:prefLabel>
      <skos:definition xml:lang="sv">Fältobservation där forskaren interagerar med forskningsobjekten och ofta har en funktion i den sociala situation som observeras.</skos:definition>
      <skos:broader rdf:resource="http://rdf-vocabulary.ddialliance.org/cv/ModeOfCollection/3.0/d64e2259"/>
   </rdf:Description>
   <rdf:Description rdf:about="http://rdf-vocabulary.ddialliance.org/cv/ModeOfCollection/3.0/d64e2444">
      <rdf:type rdf:resource="http://www.w3.org/2004/02/skos/core#Concept"/>
      <skos:inScheme rdf:resource="http://rdf-vocabulary.ddialliance.org/cv/ModeOfCollection/3.0"/>
      <skos:notation>Observation.Field.Nonparticipant</skos:notation>
      <skos:prefLabel xml:lang="en">Non-participant field observation</skos:prefLabel>
      <skos:definition xml:lang="en">Observation that is conducted in a natural, non-controlled setting without any interaction between the researcher and his/her subjects.</skos:definition>
      <skos:prefLabel xml:lang="da">Feltobservation uden deltager</skos:prefLabel>
      <skos:definition xml:lang="da">Observation, der udføres i en naturlig, ikke-kontrolleret opsætning uden nogen interaktion mellem forsker og hans/hendes subjekter.</skos:definition>
      <skos:prefLabel xml:lang="fi">Havainnointi: kenttähavainnointi: ei-osallistuva</skos:prefLabel>
      <skos:definition xml:lang="fi">Havainnointi suoritetaan luonnollisessa, kontrolloimattomassa ympäristössä. Tutkija ja tutkittavat eivät ole lainkaan vuorovaikutuksessa keskenään. Kutsutaan myös suoraksi tai ulkopuoliseksi kenttähavainnoinniksi.</skos:definition>
      <skos:prefLabel xml:lang="fr">Observation non-participante sur le terrain</skos:prefLabel>
      <skos:definition xml:lang="fr">Observation qui a été conduite dans une configuration naturelle et non contrôlée sans aucune interaction entre le chercheur et ses sujets.</skos:definition>
      <skos:prefLabel xml:lang="fr">Observation non-participante sur le terrain</skos:prefLabel>
      <skos:definition xml:lang="fr">Observation qui a été conduite dans une configuration naturelle et non contrôlée sans aucune interaction entre le chercheur et ses sujets.</skos:definition>
      <skos:prefLabel xml:lang="it">Osservazione non partecipante sul campo</skos:prefLabel>
      <skos:definition xml:lang="it">Osservazione condotta in un ambiente naturale non controllato senza alcuna interazione tra il ricercatore e i soggetti.</skos:definition>
      <skos:prefLabel xml:lang="no">Ikke-deltagende feltobservasjon</skos:prefLabel>
      <skos:definition xml:lang="no">Observasjon som er gjennomført i et naturlig, ikke kontrollert miljø uten interaksjon mellom forskeren og studieobjektene.</skos:definition>
      <skos:prefLabel xml:lang="pt">Observação não participante</skos:prefLabel>
      <skos:definition xml:lang="pt">Observação que é conduzida/realizada em ambiente natural, não controlado, sem qualquer interação entre o investigador e os sujeitos observados.</skos:definition>
      <skos:prefLabel xml:lang="sl">Opazovanje na terenu brez udeležbe</skos:prefLabel>
      <skos:definition xml:lang="sl">Opazovanje, ki se izvaja v naravnem, nekontroliranem okolju brez kakršnekoli interakcije med raziskovalcem in njegovimi/njenimi subjekti.</skos:definition>
      <skos:prefLabel xml:lang="sr">Terensko posmatranje bez učešća</skos:prefLabel>
      <skos:definition xml:lang="sr">Posmatranje koje se izvodi u prirodnom, nekontrolisanom okruženju bez ikakve interakcije između istraživača i njegovih subjekata.</skos:definition>
      <skos:prefLabel xml:lang="sv">Icke-deltagande fältobservation</skos:prefLabel>
      <skos:definition xml:lang="sv">Observation som utförs i en naturlig, icke-kontrollerad miljö utan interaktion mellan forskaren och dennes forskningsobjekt.</skos:definition>
      <skos:broader rdf:resource="http://rdf-vocabulary.ddialliance.org/cv/ModeOfCollection/3.0/d64e2259"/>
   </rdf:Description>
   <rdf:Description rdf:about="http://rdf-vocabulary.ddialliance.org/cv/ModeOfCollection/3.0/d64e2720">
      <rdf:type rdf:resource="http://www.w3.org/2004/02/skos/core#Concept"/>
      <skos:inScheme rdf:resource="http://rdf-vocabulary.ddialliance.org/cv/ModeOfCollection/3.0"/>
      <skos:notation>Observation.Laboratory.Nonparticipant</skos:notation>
      <skos:prefLabel xml:lang="en">Non-participant laboratory observation</skos:prefLabel>
      <skos:definition xml:lang="en">Type of laboratory observation that is conducted without any interaction between the researcher and his/her subjects.</skos:definition>
      <skos:prefLabel xml:lang="da">Laboratorieobservation uden deltager</skos:prefLabel>
      <skos:definition xml:lang="da">Type af laboratorieobservation, der udføres uden nogen interaktion mellem forskeren og hans/hendes subjekter.</skos:definition>
      <skos:prefLabel xml:lang="fi">Havainnointi: laboratoriohavainnointi: ei-osallistuva</skos:prefLabel>
      <skos:definition xml:lang="fi">Kokeellinen havainnointi kontrolloidussa, tarkoitusta varten luodussa tilassa. Tutkija ei ole missään vuorovaikutuksessa tutkittavien kanssa. Kutsutaan myös tarkkailevaksi laboratoriohavainnoinniksi. Esimerkki: Lasten leikkien havainnointi laboratorioon rakennetussa leikkihuoneessa, jossa tutkija ei ota osaa leikkiin.</skos:definition>
      <skos:prefLabel xml:lang="fr">Observation non-participante en laboratoire</skos:prefLabel>
      <skos:definition xml:lang="fr">Type d'observation en laboratoire qui a été conduite sans aucune interaction entre le chercheur et ses sujets.</skos:definition>
      <skos:prefLabel xml:lang="fr">Observation non-participante en laboratoire</skos:prefLabel>
      <skos:definition xml:lang="fr">Type d'observation en laboratoire qui a été conduite sans aucune interaction entre le chercheur et ses sujets.</skos:definition>
      <skos:prefLabel xml:lang="it">Osservazione non partecipante in laboratorio</skos:prefLabel>
      <skos:definition xml:lang="it">Osservazione condotta in laboratorio senza alcuna interazione tra il ricercatore e i soggetti.</skos:definition>
      <skos:prefLabel xml:lang="no">Ikke-deltagende laboratorieobservasjon</skos:prefLabel>
      <skos:definition xml:lang="no">En type laboratorieobservasjon som blir gjennomført uten interaksjon mellom forskeren og studieobjektene.</skos:definition>
      <skos:prefLabel xml:lang="pt">Observação não participante em laboratório</skos:prefLabel>
      <skos:definition xml:lang="pt">Tipo de observação em laboratório realizada sem qualquer interação entre o investigador e os sujeitos observados.</skos:definition>
      <skos:prefLabel xml:lang="sl">Laboratorijsko opazovanje brez udeležbe</skos:prefLabel>
      <skos:definition xml:lang="sl">Vrsta laboratorijskega opazovanja, ki se izvaja brez kakršnekoli interakcije med raziskovalcem in njegovimi/njenimi subjekti.</skos:definition>
      <skos:prefLabel xml:lang="sr">Laboratorijsko posmatranje bez učešća</skos:prefLabel>
      <skos:definition xml:lang="sr">Vrsta laboratorijskog posmatranja koje se sprovodi bez ikakve interakcije između istraživača i njegovih subjekata.</skos:definition>
      <skos:prefLabel xml:lang="sv">Icke-deltagande laboratorieobservation</skos:prefLabel>
      <skos:definition xml:lang="sv">Laboratorieobservation som utförs utan interaktion mellan forskaren och dennes forskningsobjekt.</skos:definition>
      <skos:broader rdf:resource="http://rdf-vocabulary.ddialliance.org/cv/ModeOfCollection/3.0/d64e2534"/>
   </rdf:Description>
   <rdf:Description rdf:about="http://rdf-vocabulary.ddialliance.org/cv/ModeOfCollection/3.0/d64e2900">
      <rdf:type rdf:resource="http://www.w3.org/2004/02/skos/core#Concept"/>
      <skos:inScheme rdf:resource="http://rdf-vocabulary.ddialliance.org/cv/ModeOfCollection/3.0"/>
      <skos:notation>Experiment</skos:notation>
      <skos:prefLabel xml:lang="en">Experiment</skos:prefLabel>
      <skos:definition xml:lang="en">Research method involving the manipulation of some or all of the independent variables included in the hypotheses.</skos:definition>
      <skos:prefLabel xml:lang="da">Eksperiment</skos:prefLabel>
      <skos:definition xml:lang="da">Forskningsmetode, der involverer manipulationen af nogle eller alle af de uafhængige variabler inkludereret i hypoteserne.</skos:definition>
      <skos:prefLabel xml:lang="fi">Kontrolloitu koe</skos:prefLabel>
      <skos:definition xml:lang="fi">Tutkimusasetelma, jossa tutkimushypoteesin mukaisesti manipuloidaan yhtä tai useampaa riippumatonta muuttujaa.</skos:definition>
      <skos:prefLabel xml:lang="fr">Expérimentation</skos:prefLabel>
      <skos:definition xml:lang="fr">Méthode de recherche impliquant la manipulation d'une partie ou de toutes les variables indépendantes incluses dans les hypothèses.</skos:definition>
      <skos:prefLabel xml:lang="fr">Expérimentation</skos:prefLabel>
      <skos:definition xml:lang="fr">Méthode de recherche impliquant la manipulation d'une partie ou de toutes les variables indépendantes incluses dans les hypothèses.</skos:definition>
      <skos:prefLabel xml:lang="it">Esperimento</skos:prefLabel>
      <skos:definition xml:lang="it">Metodo di ricerca che coinvolge la manipolazione di alcune o tutte le variabili indipendenti incluse nelle ipotesi.</skos:definition>
      <skos:prefLabel xml:lang="no">Eksperiment</skos:prefLabel>
      <skos:definition xml:lang="no">Forskningsmetode som innebærer manipulering av noen eller alle de uavhengige variablene inkludert i hypotesene.</skos:definition>
      <skos:prefLabel xml:lang="pt">Estudo experimental</skos:prefLabel>
      <skos:definition xml:lang="pt">Método de pesquisa que envolve a manipulação de algumas ou de todas as variáveis independentes incluídas nas hipóteses.</skos:definition>
      <skos:prefLabel xml:lang="sl">Eksperiment</skos:prefLabel>
      <skos:definition xml:lang="sl">Raziskovalna metoda, ki vključuje manipulacijo nekaterih ali vseh neodvisnih spremenljivk, vključenih v hipoteze.</skos:definition>
      <skos:prefLabel xml:lang="sr">Ekspertiment</skos:prefLabel>
      <skos:definition xml:lang="sr">Metoda istraživanja koja uključuje manipulaciju nekim ili svim nezavisnim varijablama uključenim u hipoteze.</skos:definition>
      <skos:prefLabel xml:lang="sv">Experiment</skos:prefLabel>
      <skos:definition xml:lang="sv">Forskningsmetod som omfattar att styra vissa eller alla oberoende variabler som ingår i hypotesen.</skos:definition>
      <skos:narrower rdf:resource="http://rdf-vocabulary.ddialliance.org/cv/ModeOfCollection/3.0/d64e2997"/>
      <skos:narrower rdf:resource="http://rdf-vocabulary.ddialliance.org/cv/ModeOfCollection/3.0/d64e3087"/>
      <skos:narrower rdf:resource="http://rdf-vocabulary.ddialliance.org/cv/ModeOfCollection/3.0/d64e3177"/>
   </rdf:Description>
   <rdf:Description rdf:about="http://rdf-vocabulary.ddialliance.org/cv/ModeOfCollection/3.0/d64e2997">
      <rdf:type rdf:resource="http://www.w3.org/2004/02/skos/core#Concept"/>
      <skos:inScheme rdf:resource="http://rdf-vocabulary.ddialliance.org/cv/ModeOfCollection/3.0"/>
      <skos:notation>Experiment.Laboratory</skos:notation>
      <skos:prefLabel xml:lang="en">Laboratory experiment</skos:prefLabel>
      <skos:definition xml:lang="en">An experiment conducted in a controlled, artificially created physical setting, in which a researcher manipulates one or several independent variables and measures its/their effect on the dependent variable.</skos:definition>
      <skos:prefLabel xml:lang="da">Laboratorieeksperiment</skos:prefLabel>
      <skos:definition xml:lang="da">Et eksperiment udført i en kontrolleret, kunstigt skabt fysisk opsætning, hvor en forsker manipulerer en eller flere uafhængige variabler og måler dens/deres effekt på den afhængige variabel.</skos:definition>
      <skos:prefLabel xml:lang="fi">Kontrolloitu koe: laboratoriokoe</skos:prefLabel>
      <skos:definition xml:lang="fi">Kontrolloidussa, tarkoitusta varten luodussa ympäristössä suoritettu koe, jossa tutkija(t) manipuloivat yhtä tai useampaa riippumatonta muuttujaa ja mittaavat sen vaikutusta riippuvaan muuttujaan.</skos:definition>
      <skos:prefLabel xml:lang="fr">Expérimentation en laboratoire</skos:prefLabel>
      <skos:definition xml:lang="fr">Une expérimentation conduite dans une configuration physique contrôlée, créée artificiellement, dans laquelle un chercheur manipule une ou plusieurs variables indépendantes et mesure son / leur effet sur la variable dépendante.</skos:definition>
      <skos:prefLabel xml:lang="fr">Expérimentation en laboratoire</skos:prefLabel>
      <skos:definition xml:lang="fr">Une expérimentation conduite dans une configuration physique contrôlée, créée artificiellement, dans laquelle un chercheur manipule une ou plusieurs variables indépendantes et mesure son / leur effet sur la variable dépendante.</skos:definition>
      <skos:prefLabel xml:lang="it">Esperimento in laboratorio</skos:prefLabel>
      <skos:definition xml:lang="it">Un esperimento condotto in un ambiente fisico controllato, creato artificialmente, in cui un ricercatore manipola una o più variabili indipendenti e misura il loro effetto sulla variabile dipendente.</skos:definition>
      <skos:prefLabel xml:lang="no">Laboratorieeksperiment</skos:prefLabel>
      <skos:definition xml:lang="no">Et eksperiment som utføres i et kontrollert, kunstig utformet miljø, hvor forskeren manipulerer én eller flere av de uavhengige variablene og måler effekten det har på den avhengige variabelen.</skos:definition>
      <skos:prefLabel xml:lang="pt">Estudo experimental em laboratório</skos:prefLabel>
      <skos:definition xml:lang="pt">Experiência/experimento conduzida/o em ambiente físico controlado, artificialmente criado, no qual o investigador manipula uma ou várias variáveis independentes e mede o seu efeito sobre a variável dependente.</skos:definition>
      <skos:prefLabel xml:lang="sl">Laboratorijski eksperiment</skos:prefLabel>
      <skos:definition xml:lang="sl">Eksperiment, ki se izvaja v nadzorovanem, umetno ustvarjenem fizičnem okolju, v katerem raziskovalec manipulira z eno ali več neodvisnimi spremenljivkami in meri svoj vpliv na odvisno spremenljivko.</skos:definition>
      <skos:prefLabel xml:lang="sr">Laboratorijski eksperiment</skos:prefLabel>
      <skos:definition xml:lang="sr">Eksperiment sproveden u kontrolisanom, veštački stvorenom fizičkom okruženju, u kome istraživač manipuliše jednom ili više nezavisnih varijabli i meri njen / njihov uticaj na zavisnu promenljivu.</skos:definition>
      <skos:prefLabel xml:lang="sv">Laboratorieexperiment</skos:prefLabel>
      <skos:definition xml:lang="sv">Ett experiment som utförs i en kontrollerad, konstgjord fysisk miljö där forskaren styr en eller flera oberoende variabler och mäter dess/deras effekt på den beroende variabeln.</skos:definition>
      <skos:broader rdf:resource="http://rdf-vocabulary.ddialliance.org/cv/ModeOfCollection/3.0/d64e2900"/>
   </rdf:Description>
   <rdf:Description rdf:about="http://rdf-vocabulary.ddialliance.org/cv/ModeOfCollection/3.0/d64e3087">
      <rdf:type rdf:resource="http://www.w3.org/2004/02/skos/core#Concept"/>
      <skos:inScheme rdf:resource="http://rdf-vocabulary.ddialliance.org/cv/ModeOfCollection/3.0"/>
      <skos:notation>Experiment.FieldIntervention</skos:notation>
      <skos:prefLabel xml:lang="en">Field/Intervention experiment</skos:prefLabel>
      <skos:definition xml:lang="en">An experiment conducted in a natural, uncontrolled setting, in which the researcher manipulates one or several independent variables. Intervention/clinical studies are one example of field experiments.</skos:definition>
      <skos:prefLabel xml:lang="da">Felt/Interventionseksperiment</skos:prefLabel>
      <skos:definition xml:lang="da">Et eksperiment udført i en naturlig, ukontrolleret opsætning, hvor forskeren manipulerer en eller flere uafhængige variabler. Intervention/kliniske studier er et eksempel på felteksperimenter.</skos:definition>
      <skos:prefLabel xml:lang="fi">Kontrolloitu koe: kenttä- tai interventiokoe</skos:prefLabel>
      <skos:definition xml:lang="fi">Luonnollisessa, kontrolloimattomassa ympäristössä suoritettu koe, jossa tutkija(t) manipuloivat yhtä tai useampaa riippumatonta muuttujaa. Esimerkkejä: kliiniset tutkimukset.</skos:definition>
      <skos:prefLabel xml:lang="fr">Expérimentation sur le terrain</skos:prefLabel>
      <skos:definition xml:lang="fr">Une expérimentation conduite dans une configuration naturelle, non contrôlée, dans laquelle le chercheur manipule une ou plusieurs variables indépendantes. Des études cliniques sont un exemple d'expérimentations sur le terrain.</skos:definition>
      <skos:prefLabel xml:lang="fr">Expérimentation sur le terrain</skos:prefLabel>
      <skos:definition xml:lang="fr">Une expérimentation conduite dans une configuration naturelle, non contrôlée, dans laquelle le chercheur manipule une ou plusieurs variables indépendantes. Des études cliniques sont un exemple d'expérimentations sur le terrain.</skos:definition>
      <skos:prefLabel xml:lang="it">Esperimento sul campo / Intervento</skos:prefLabel>
      <skos:definition xml:lang="it">Un esperimento condotto in un ambiente naturale, non controllato, in cui il ricercatore manipola una o più variabili indipendenti. Gli interventi o studi clinici sono un esempio di esperimenti sul campo.</skos:definition>
      <skos:prefLabel xml:lang="no">Felt/felteksperiment</skos:prefLabel>
      <skos:definition xml:lang="no">Et eksperiment som utføres i et naturlig, ukontrollert miljø, hvor forskeren manipulerer én eller flere av de uavhengige variablene. Intervensjon/kliniske studier er et eksempel på felteksperiment.</skos:definition>
      <skos:prefLabel xml:lang="pt">Estudo experimental de campo (com intervenção)</skos:prefLabel>
      <skos:definition xml:lang="pt">Experiência/experimento conduzida/o em ambiente natural e não controlado, no qual o investigador manipula uma ou várias variáveis independentes. Estudos clínicos ou de intervenção são um exemplo de experimentações de campo.</skos:definition>
      <skos:prefLabel xml:lang="sl">Terenski/intervencijski eksperiment</skos:prefLabel>
      <skos:definition xml:lang="sl">Eksperiment, ki se izvaja v naravnem, nekontroliranem okolju, v katerem raziskovalec manipulira z eno ali več neodvisnimi spremenljivkami. Intervencija/klinične študije so en primer terenskih eksperimentov.</skos:definition>
      <skos:prefLabel xml:lang="sr">Terenski ekspertiment / intervencija</skos:prefLabel>
      <skos:definition xml:lang="sr">Eksperiment sproveden u prirodnom, nekontrolisanom okruženju, u kome istraživač manipuliše jednom ili više nezavisnih varijabli. Interventne / kliničke studije su jedan primer terenskih eksperimenata.</skos:definition>
      <skos:prefLabel xml:lang="sv">Fältexperiment</skos:prefLabel>
      <skos:definition xml:lang="sv">Ett experiment som utförs i en naturlig, okontrollerad miljö där forskaren styr en eller flera oberoende variabler. Interventionsstudier och kliniska studier är exempel på fältexperiment.</skos:definition>
      <skos:broader rdf:resource="http://rdf-vocabulary.ddialliance.org/cv/ModeOfCollection/3.0/d64e2900"/>
   </rdf:Description>
   <rdf:Description rdf:about="http://rdf-vocabulary.ddialliance.org/cv/ModeOfCollection/3.0/d64e3177">
      <rdf:type rdf:resource="http://www.w3.org/2004/02/skos/core#Concept"/>
      <skos:inScheme rdf:resource="http://rdf-vocabulary.ddialliance.org/cv/ModeOfCollection/3.0"/>
      <skos:notation>Experiment.WebBased</skos:notation>
      <skos:prefLabel xml:lang="en">Web-based experiment</skos:prefLabel>
      <skos:definition xml:lang="en">An experiment conducted in the virtual setting of the World Wide Web, in which experimental materials are programmed to implement artificial situations or events to be investigated in a distributed environment. (Reips, U.-D. (2002). Theory and techniques of Web experimenting. In B. Batinic, U.-D. Reips, &amp; M. Bosnjak (Eds.), Online Social Sciences. Seattle: Hogrefe &amp; Huber. Available at: http://www.websm.org/uploadi/editor/Reips_2002_Theory_and_techniques.pdf [07 June 2013])</skos:definition>
      <skos:prefLabel xml:lang="da">Webbaseret eksperiment</skos:prefLabel>
      <skos:definition xml:lang="da">Et eksperiment udført i den virtuelle opsætning på World Wibe Web, hvor eksperimentelle materialer er programmeret til at implementere kunstige situationer eller begivenheder, der skal undersøges i et spredt miljø. (Reips, U.-D. (2002). Theory and techniques of Web experimenting. In B. Batinic, U.-D. Reips, &amp; M. Bosnjak (Eds.), Online Social Sciences. Seattle: Hogrefe &amp; Huber. Available at: http://www.websm.org/uploadi/editor/Reips_2002_Theory_and_techniques.pdf [07 June 2013])</skos:definition>
      <skos:prefLabel xml:lang="fi">Kontrolloitu koe: virtuaalinen koe</skos:prefLabel>
      <skos:definition xml:lang="fi">Internetissä toteutettu kokeellinen tutkimus, jossa on ohjelmallisesti luotu keinotekoisia virtuaalisia ympäristöjä tai tapahtumia tutkimusta varten. Esimerkki: Keinotekoisen kielen oppimiskoe, virtuaalisen pelikäyttäytymisen koe.</skos:definition>
      <skos:prefLabel xml:lang="fr">Expérimentation par Internet</skos:prefLabel>
      <skos:definition xml:lang="fr">Une expérimentation conduite dans une configuration virtuelle du Web, dans laquelle des matériaux expérimentaux sont programmés pour mettre en œuvre des situations ou des évènements artificiels pour être étudiés dans un environnement distribué. (Reips, U.-D. (2002). Theory and techniques of Web experimenting. In B. Batinic, U.-D. Reips, &amp;amp; M. Bosnjak (Eds.), Online Social Sciences. Seattle: Hogrefe &amp;amp; Huber. Available at: http://www.websm.org/uploadi/editor/Reips_2002_Theory_and_techniques.pdf [07 June 2013])</skos:definition>
      <skos:prefLabel xml:lang="fr">Expérimentation par Internet</skos:prefLabel>
      <skos:definition xml:lang="fr">Une expérimentation conduite dans une configuration virtuelle du Web, dans laquelle des matériaux expérimentaux sont programmés pour mettre en œuvre des situations ou des évènements artificiels pour être étudiés dans un environnement distribué. (Reips, U.-D. (2002). Theory and techniques of Web experimenting. In B. Batinic, U.-D. Reips, &amp;amp; M. Bosnjak (Eds.), Online Social Sciences. Seattle: Hogrefe &amp;amp; Huber. Available at: http://www.websm.org/uploadi/editor/Reips_2002_Theory_and_techniques.pdf [07 June 2013])</skos:definition>
      <skos:prefLabel xml:lang="it">Esperimento web</skos:prefLabel>
      <skos:definition xml:lang="it">Un esperimento condotto nell'ambiente virtuale del World Wide Web, in cui i materiali sperimentali sono programmati per ricreare situazioni o eventi artificiali da indagare in un ambiente distribuito.</skos:definition>
      <skos:prefLabel xml:lang="no">Webbasert eksperiment</skos:prefLabel>
      <skos:definition xml:lang="no">Et eksperiment som utføres i et vituelt miljø på internett (World Wide Web), hvor eksperimentelt materiale er programmert til å sette i gang kunstige situasjoner eller hendelser som kan undersøkes i et gitt miljø. (Reips, U.-D. (2002). Theory and techniques of Web experimenting. In B. Batinic, U.-D. Reips, &amp; M. Bosnjak (Eds.), Online Social Sciences. Seattle: Hogrefe &amp; Huber. Available at: http://www.websm.org/uploadi/editor/Reips_2002_Theory_and_techniques.pdf [07 June 2013])</skos:definition>
      <skos:prefLabel xml:lang="pt">Estudo experimental online/via web</skos:prefLabel>
      <skos:definition xml:lang="pt">Experiência/experimento conduzida/o em ambiente virtual da World Wide Web, no qual materiais experimentais são programados para implementar situações ou eventos artificiais para pesquisa num ambiente distribuído. (Reips, U.-D. (2002). Theory and techniques of Web experimenting. In B. Batinic, U.-D. Reips, &amp;amp; M. Bosnjak (Eds.), Online Social Sciences. Seattle: Hogrefe &amp;amp; Huber. Disponível em: http://www.websm.org/uploadi/editor/Reips_2002_Theory_and_techniques.pdf [07 June 2013])</skos:definition>
      <skos:prefLabel xml:lang="sl">Spletni eksperiment</skos:prefLabel>
      <skos:definition xml:lang="sl">Eksperiment, ki se izvaja v virtualnem okolju svetovnega spleta, v katerem so eksperimentalni materiali programirani za izvajanje umetnih situacij ali dogodkov, ki jih je treba raziskati v porazdeljenem okolju.</skos:definition>
      <skos:prefLabel xml:lang="sr">Ekspertiment na vebu</skos:prefLabel>
      <skos:definition xml:lang="sr">Eksperiment sproveden u virtuelnom okruženju World Wide Web-a, u kome se eksperimentalni materijali programiraju za primenu veštačkih situacija ili događaja koji se istražuju u distribuisanoj sredini. (Reips, U.D. (2002). Teorija i tehnike veb eksperimentiranja. U B. Batinic, U.D. Reips i M. Bosnjak (ur.), Online Social Sciences. Seattle: Hogrefe &amp;amp; Huber. Dostupno na: http://www.websm.org/uploadi/editor/Reips_2002_Theori_and_techniques.pdf [07. juni 2013.])</skos:definition>
      <skos:prefLabel xml:lang="sv">Webbaserat experiment</skos:prefLabel>
      <skos:definition xml:lang="sv">Ett experiment som utförs i en virtuell miljö på webben, där experimentella material programmeras för att skapa artificiella situationer eller händelser som undersöks i en distribuerad miljö.  (Reips, U.-D. (2002). Theory and techniques of Web experimenting. In B. Batinic, U.-D. Reips, &amp; M. Bosnjak (Eds.), Online Social Sciences. Seattle: Hogrefe &amp; Huber. Tillgänglig: http://www.websm.org/uploadi/editor/Reips_2002_Theory_and_techniques.pdf [8 september, 2016])</skos:definition>
      <skos:broader rdf:resource="http://rdf-vocabulary.ddialliance.org/cv/ModeOfCollection/3.0/d64e2900"/>
   </rdf:Description>
   <rdf:Description rdf:about="http://rdf-vocabulary.ddialliance.org/cv/ModeOfCollection/3.0/d64e3268">
      <rdf:type rdf:resource="http://www.w3.org/2004/02/skos/core#Concept"/>
      <skos:inScheme rdf:resource="http://rdf-vocabulary.ddialliance.org/cv/ModeOfCollection/3.0"/>
      <skos:notation>Recording</skos:notation>
      <skos:prefLabel xml:lang="en">Recording</skos:prefLabel>
      <skos:definition xml:lang="en">Registering by mechanical or electronic means, in a form that allows the information to be retrieved and/or reproduced. For example, images or sounds on disc or magnetic tape.</skos:definition>
      <skos:prefLabel xml:lang="da">Optagelse</skos:prefLabel>
      <skos:definition xml:lang="da">Registrering på mekanisk eller elektronisk vis i en form, der muliggør, at information kan genfindes og/eller genskabes. For eksempel billeder eller lyd på disk eller magnetbånd.</skos:definition>
      <skos:prefLabel xml:lang="fi">Taltiointi</skos:prefLabel>
      <skos:definition xml:lang="fi">Aineiston taltioiminen mekaanisesti tai elektronisesti tavalla, joka mahdollistaa sen kuuntelun, katselun tai monistamisen. Sisältää mm. valokuvien, videon tai äänen taltioimisen. Esimerkki: Kokousten tai vastaanottojen videoiminen ilman tutkijan läsnäoloa, valokuvista muodostuva aineisto.</skos:definition>
      <skos:prefLabel xml:lang="fr">Enregistrement</skos:prefLabel>
      <skos:definition xml:lang="fr">Enregistrement par des moyens mécaniques ou électroniques, sous une forme qui permet que les informations soient récupérées et / ou reproduites. Par exemple, des images ou des sons sur disque ou bande magnétique.</skos:definition>
      <skos:prefLabel xml:lang="fr">Enregistrement</skos:prefLabel>
      <skos:definition xml:lang="fr">Enregistrement par des moyens mécaniques ou électroniques, sous une forme qui permet que les informations soient récupérées et / ou reproduites. Par exemple, des images ou des sons sur disque ou bande magnétique.</skos:definition>
      <skos:prefLabel xml:lang="it">Registrazione</skos:prefLabel>
      <skos:definition xml:lang="it">Registrazione tramite mezzi meccanici o elettronici, in una forma che consente di recuperare e/o riprodurre le informazioni. Ad esempio, registrazioni di immagini o suoni su disco o supporto magnetico.</skos:definition>
      <skos:prefLabel xml:lang="no">Opptak</skos:prefLabel>
      <skos:definition xml:lang="no">Mekanisk eller elektronisk registrering i et format som gjør det mulig å gjeninnhente og/eller gjenskape informasjonen. For eksempel bilder eller lyd på disk eller magnetbånd.</skos:definition>
      <skos:prefLabel xml:lang="pt">Gravação</skos:prefLabel>
      <skos:definition xml:lang="pt">Registo por meios mecânicos ou electrónicos, de forma a permitir que a informação seja recuperada e/ou reproduzida. Por exemplo, imagens ou sons em disco ou fita magnética.</skos:definition>
      <skos:prefLabel xml:lang="sl">Snemanje</skos:prefLabel>
      <skos:definition xml:lang="sl">Snemanje z mehanskimi ali elektronskimi sredstvi v obliki, ki omogoča, da se informacije prikličejo in/ali reproducirajo. Na primer slike ali zvoki na disku ali magnetnem traku.</skos:definition>
      <skos:prefLabel xml:lang="sr">Snimanje</skos:prefLabel>
      <skos:definition xml:lang="sr">Registrovanje mehaničkim ili elektronskim sredstvima, u obliku koji omogućava preuzimanje i / ili reprodukciju informacija. Na primer, slike ili zvukovi na disku ili magnetnoj traci.</skos:definition>
      <skos:prefLabel xml:lang="sv">Inspelning</skos:prefLabel>
      <skos:definition xml:lang="sv">Upptagning, på mekanisk eller elektronisk väg, på sådant sätt att informationen kan återfås och/eller återskapas. Exempel: bilder eller ljud på en cd eller ett magnetband.</skos:definition>
   </rdf:Description>
   <rdf:Description rdf:about="http://rdf-vocabulary.ddialliance.org/cv/ModeOfCollection/3.0/d64e3819">
      <rdf:type rdf:resource="http://www.w3.org/2004/02/skos/core#Concept"/>
      <skos:inScheme rdf:resource="http://rdf-vocabulary.ddialliance.org/cv/ModeOfCollection/3.0"/>
      <skos:notation>ContentCoding</skos:notation>
      <skos:prefLabel xml:lang="en">Content coding</skos:prefLabel>
      <skos:definition xml:lang="en">As a mode of secondary data collection, content coding applies coding techniques to transform qualitative data (textual, video, audio or still-image) originally produced for other purposes into quantitative data (expressed in unit-by-variable matrices) in accordance with pre-defined categorization schemes. For example, coded party manifesto data like the "European Parliament Election Study 2009, Manifesto Study" (doi:10.4232/1.10204).</skos:definition>
      <skos:prefLabel xml:lang="da">Indholdskodning</skos:prefLabel>
      <skos:definition xml:lang="da">Som en metode til sekundær dataindsamling anvender indholdskodning kodningsteknikker til at transformere kvalitative data (tekst, video, lyd eller stillbilleder), der oprindeligt blev produceret til andre formål, til kvantitative data (udtrykt ved enhed-til-variabel-matricer) i overensstemmelse med forhåndsdefinerede kategoriseringsskemaer. For eksempel, kodede partimanifestdata som "European Parliament Election Study 2009, Manifesto Study" (doi:10.4232/1.10204).</skos:definition>
      <skos:prefLabel xml:lang="fi">Sisällönkoodaus</skos:prefLabel>
      <skos:definition xml:lang="fi">Jo olemassa olevasta, alun perin toisiin tarkoituksiin luodusta kvalitatiivisesta aineistosta (esim. tekstiaineistot, ääni- ja kuvatiedostot, valokuvat) muodostetaan kvantitatiivinen aineisto (matriisi) sovittua koodausohjetta käyttäen. Esimerkki: sanomalehtiartikkeleiden sisällön luokittelu annettujen kriteerien mukaan.</skos:definition>
      <skos:prefLabel xml:lang="fr">Codage de contenu</skos:prefLabel>
      <skos:definition xml:lang="fr">Comme un mode secondaire de collecte de données, le codage de contenu applique des techniques de codage pour transformer des données qualitatives (textuel, vidéo, audio, ou image fixe) originalement produites à d'autres finalités en données quantitatives (exprimées dans des matrices unité-par-variable) en accord avec des schémas de catégorisations prédéfinis. Par exemple, les données recodées des programmes des partis politiques comme les "L'Étude électorale du parlement européens 2019, étude des programmes" (doi:10.4232/1.10204).</skos:definition>
      <skos:prefLabel xml:lang="fr">Codage de contenu</skos:prefLabel>
      <skos:definition xml:lang="fr">Comme un mode secondaire de collecte de données, le codage de contenu applique des techniques de codage pour transformer des données qualitatives (textuel, vidéo, audio, ou image fixe) originalement produites à d'autres finalités en données quantitatives (exprimées dans des matrices unité-par-variable) en accord avec des schémas de catégorisations prédéfinis. Par exemple, les données recodées des programmes des partis politiques comme les "L'Étude électorale du parlement européens 2019, étude des programmes" (doi:10.4232/1.10204).</skos:definition>
      <skos:prefLabel xml:lang="it">Codifica del contenuto</skos:prefLabel>
      <skos:definition xml:lang="it">Metodo di raccolta secondaria dei dati, in cui si applicano le tecniche di codifica del contenuto per trasformare dati qualitativi originariamente prodotti per altri scopi (testi, video, audio o immagini) in dati quantitativi (espressi in forma di matrici) secondo schemi di categorizzazione definiti. Ad esempio, codifica dei dati relativi ai manifesti di partito, come il "European Parliament Election Study 2009, Manifesto Study" (doi:10.4232/1.10204)</skos:definition>
      <skos:prefLabel xml:lang="no">Innholdskoding</skos:prefLabel>
      <skos:definition xml:lang="no">Som metode for sekundær datainnsamling, innholdskoding omfatter kodeteknikker for å omgjøre kvalitative data (tekst, video, lyd eller bilde), som opprinnelig var utarbeidet for andre formål, til kvantitative data (uttrykket i en matrise med enheter og variabler) i henhold til bestemte kategoriseringssystem. For eksempel, kodede partimanifesto som i 'European Parliament Election Study 2009, Manifesto Study' (doi:10.4232/1.10204).</skos:definition>
      <skos:prefLabel xml:lang="pt">Codificação de conteúdo</skos:prefLabel>
      <skos:definition xml:lang="pt">Como modo de recolha de dados secundários, a codificação de conteúdo aplica técnicas de codificação para transformar dados qualitativos (textual, vídeo, áudio ou imagem parada) originalmente produzidos para outros propósitos em dados quantitativos (expressos em matrizes unidade-por-variável) de acordo com esquemas de categorização predefinidos. Por exemplo, dados codificados de um programa de partido político, como o "European Parliament Election Study 2009, Manifesto Study" (doi:10.4232/1.10204).</skos:definition>
      <skos:prefLabel xml:lang="sl">Kodiranje vsebine</skos:prefLabel>
      <skos:definition xml:lang="sl">Kot način sekundarnega zbiranja podatkov, kodiranje vsebine uporablja kodirne tehnike za preoblikovanje kvalitativnih podatkov (besedilni podatki, video, avdio ali mirujoče slike), ki so bili prvotno ustvarjeni za druge namene, v kvantitativne podatke (izražene z matricami enot po spremenljivkah) v skladu s vnaprej opredeljenimi kategorizacijskimi shemami. Na primer, kodiranje manifestov političnih strank, kot npr. študija o volitvah v Evropski parlament 2009.</skos:definition>
      <skos:prefLabel xml:lang="sr">Kodiranje sadržaja</skos:prefLabel>
      <skos:definition xml:lang="sr">Kao način sekundarnog prikupljanja podataka, kodiranje sadržaja primenjuje tehnike kodiranja kako bi se kvalitativni podaci (tekstualni, video, audio ili nepokretni snimci) prvobitno proizvedeni u druge svrhe pretvorili u kvantitativne podatke u skladu sa prethodno definisanom šemom kategorizacije. Na primer, podaci o manifestu kodiranih strana poput "European Parliament Election Study 2009, Manifesto Study" (doi:10.4232/1.10204)".</skos:definition>
      <skos:prefLabel xml:lang="sv">Kodning av innehåll</skos:prefLabel>
      <skos:definition xml:lang="sv">Som en metod för sekundär datainsamling tillämpar innehållskodning  kodningstekniker för att omvandla kvalitativa data (text-, ljud-, video-, eller stillbildsdata) som ursprungligen skapats för andra syften till kvantitativa data (uttryckta i en matris med enheter och variabler) enligt fördefinierade kategoriseringsscheman. Exempel: kodade partiprogramsdata som i "European Parliament Election Study 2009, Manifesto Study" (DOI: 10.4232/1.10204).</skos:definition>
   </rdf:Description>
   <rdf:Description rdf:about="http://rdf-vocabulary.ddialliance.org/cv/ModeOfCollection/3.0/d64e3909">
      <rdf:type rdf:resource="http://www.w3.org/2004/02/skos/core#Concept"/>
      <skos:inScheme rdf:resource="http://rdf-vocabulary.ddialliance.org/cv/ModeOfCollection/3.0"/>
      <skos:notation>Transcription</skos:notation>
      <skos:prefLabel xml:lang="en">Transcription</skos:prefLabel>
      <skos:definition xml:lang="en">Capturing information in writing from a different source, or from a different medium, alphabet, or form of notation, like scientific formulae, or musical notes. For transcribed interviews or observations, it is recommended to document the primary mode of collection, using one of the interview or observation terms.</skos:definition>
      <skos:prefLabel xml:lang="da">Transskription</skos:prefLabel>
      <skos:definition xml:lang="da">Indfangning af skriftlige oplysninger fra en anden kilde eller fra et andet medium, alfabet eller form for notation, såsom videnskabelige formler eller musikalske noder. For transskriberede interviews eller observationer anbefales det at dokumentere den primære indsamlingsform ved brug af et af interview- eller observationsbetingelserne.</skos:definition>
      <skos:prefLabel xml:lang="fi">Litterointi</skos:prefLabel>
      <skos:definition xml:lang="fi">Informaation siirtäminen käsin kirjaamalla toisesta lähteestä tai toisesta formaatista, muodosta tai aakkosjärjestelmästä. Esimerkki: Musiikin esittäminen nuotteina, kemialliset kaavat. Jos aineisto muodostuu havaintomuistiinpanoista tai haastattelulitteroinneista, suositellaan kuvattavaksi ensisijainen keruumenetelmä käyttämällä sopivaa havainnointi- tai haastattelutermiä.</skos:definition>
      <skos:prefLabel xml:lang="fr">Transcription</skos:prefLabel>
      <skos:definition xml:lang="fr">Collecte des informations par écrit à partir d'une source différente, ou à partir d'un support différent, d'un alphabet, ou d'une forme de notation, comme des formules scientifiques, ou des notes de musique. Pour des entretiens ou des observations transcrits, il est recommandé de documenter le mode de collecte initial, en utilisant l'un des termes propres à l'entretien ou à l'observation.</skos:definition>
      <skos:prefLabel xml:lang="fr">Transcription</skos:prefLabel>
      <skos:definition xml:lang="fr">Collecte des informations par écrit à partir d'une source différente, ou à partir d'un support différent, d'un alphabet, ou d'une forme de notation, comme des formules scientifiques, ou des notes de musique. Pour des entretiens ou des observations transcrits, il est recommandé de documenter le mode de collecte initial, en utilisant l'un des termes propres à l'entretien ou à l'observation.</skos:definition>
      <skos:prefLabel xml:lang="it">Trascrizione</skos:prefLabel>
      <skos:definition xml:lang="it">Raccolta di informazioni per iscritto da un'altra fonte, o da un altro mezzo, alfabeto o forma di notazione, come formule scientifiche o note musicali. Per le interviste o le osservazioni trascritte, si consiglia di documentare la modalità di raccolta dei dati utilizzando uno dei termini del vocabolario relativi all'intervista o all'osservazione.</skos:definition>
      <skos:prefLabel xml:lang="no">Transkripsjon</skos:prefLabel>
      <skos:definition xml:lang="no">Nedtegning av informasjon i skrift fra en annen kilde, eller et annet medium, alfabet, eller fra notasjoner, som vitenskapelige formler, eller musikknoter. For transkriberte intervju eller observasjoner er det anbefalt å dokumentere den opprinnelige formen for datainnsamling, ved å bruke et av intervju- eller observasjonsbegrepene.</skos:definition>
      <skos:prefLabel xml:lang="pt">Transcrição</skos:prefLabel>
      <skos:definition xml:lang="pt">Recolha de informações por escrito de uma fonte diferente ou através de um meio diferente, alfabeto ou forma de anotação, como fórmulas científicas ou notas musicais. Para entrevistas ou observações transcritas, recomenda-se documentar o modo de recolha principal, usando um dos termos no âmbito dos tópicos mais gerais 'entrevista' ou 'observação'.</skos:definition>
      <skos:prefLabel xml:lang="sl">Prepis</skos:prefLabel>
      <skos:definition xml:lang="sl">Zajemanje podatkov v pisni obliki iz drugega vira ali iz drugega medija, abecede, ali oblika zapisa, kot so znanstvene formule ali glasbene note. Pri transkriptih intervjujev ali opazovanj je priporočljivo dokumentirati primarni način zbiranja podatkov z uporabo enega od razgovornih ali opazovalnih pogojev.</skos:definition>
      <skos:prefLabel xml:lang="sr">Transkripcija</skos:prefLabel>
      <skos:definition xml:lang="sr">Obuhvat podataka u pisanom obliku iz drugog izvora ili iz drugog medija, pisma ili oblika notacije, poput naučnih formula ili muzičkih nota. Za prepisane intervjue ili zapažanja preporučuje se dokumentovanje primarnog načina prikupljanja, koristeći jedan od termina intervjua ili opservacije.</skos:definition>
      <skos:prefLabel xml:lang="sv">Transkription</skos:prefLabel>
      <skos:definition xml:lang="sv">Att nedteckna information från en annan källa eller från ett annat medium, alfabet eller notationssystem, som till exempel vetenskapliga formler eller noter för musik. För transkriberade intervjuer och observationer rekommenderas det att man dokumenterar den primära insamlingsmetoden med någon av termerna för intervjuer eller observationer.</skos:definition>
   </rdf:Description>
   <rdf:Description rdf:about="http://rdf-vocabulary.ddialliance.org/cv/ModeOfCollection/3.0/d64e3999">
      <rdf:type rdf:resource="http://www.w3.org/2004/02/skos/core#Concept"/>
      <skos:inScheme rdf:resource="http://rdf-vocabulary.ddialliance.org/cv/ModeOfCollection/3.0"/>
      <skos:notation>CompilationSynthesis</skos:notation>
      <skos:prefLabel xml:lang="en">Compilation/Synthesis</skos:prefLabel>
      <skos:definition xml:lang="en">Collecting and assembling data from multiple, often heterogeneous sources that have one or more reference points in common, and at least one of the sources was originally produced for other purposes. The data are incorporated in a new entity. For example, providing data on the number of universities in the last 150 years using a variety of available sources (e.g. finance documents, official statistics, university registers), combining survey data with information about geographical areas from official statistics (e.g. population density, doctors per capita, etc.), or using RSS to collect blog posts or tweets, etc.</skos:definition>
      <skos:prefLabel xml:lang="da">Kompilering/Syntese</skos:prefLabel>
      <skos:definition xml:lang="da">Indsamling og samling af data fra flere, ofte heterogene, kilder, der har en eller flere referencepunkter til fælles, og mindst en af kilderne oprindeligt blev produceret til andre formål. Dataene inkorporeres i en ny enhed. For eksempel, give data om antallet af universiteter i de sidste 150 år ved brug af en række af tilgængelige kilder (f.eks. finansielle dokumenter, officielle statistikker, universitetsregistre), kombinere undersøgelsesdata med oplysninger om geografiske områder fra officielle statistikker (f.eks. befolkningstæthed, læger pr. indbygger etc.) eller brug af RSS til at indsamle blogindlæg eller tweets mm.</skos:definition>
      <skos:prefLabel xml:lang="fi">Kooste- tai synteesiaineisto</skos:prefLabel>
      <skos:definition xml:lang="fi">Tietojen kerääminen ja kokoaminen useista, usein heterogeenisistä lähdemateriaaleista, joilla yksi tai useampi yhteinen referenssi. Ainakin yksi lähteistä on olemassa valmiina jo ennestään muita tarkoituksia varten. Kerätyt tiedot yhdistetään uudeksi tutkimusaineistoksi. Esimerkkejä: Tiedon kerääminen suomalaisten yliopistojen historiasta käyttämällä monia eri lähteitä, tai kyselytutkimuksen tietojen yhdistäminen muista tietolähteistä saatuihin tietoihin.</skos:definition>
      <skos:prefLabel xml:lang="fr">Compilation / synthèse</skos:prefLabel>
      <skos:definition xml:lang="fr">Collecte et assemblage de données depuis de multiples sources souvent hétérogènes qui ont un ou plusieurs points de référence en commun, et dont au moins une des sources a été produite à l'origine à d'autres fins. Les données sont incorporées dans une nouvelle entité. Par exemple, fournir des données sur le nombre d'universités au cours des 150 dernières années utilisant une variété de sources disponibles (e. g. des documents financiers, des statistiques officielles, des registres universitaires), en combinant les données d'enquête avec des informations sur les zones géographiques provenant des statistiques officielles (e. g. la densité de population, médecins par habitants, etc.), ou en utilisant RSS pour collecter des articles de blogs ou des tweets, etc.</skos:definition>
      <skos:prefLabel xml:lang="fr">Compilation / synthèse</skos:prefLabel>
      <skos:definition xml:lang="fr">Collecte et assemblage de données depuis de multiples sources souvent hétérogènes qui ont un ou plusieurs points de référence en commun, et dont au moins une des sources a été produite à l'origine à d'autres fins. Les données sont incorporées dans une nouvelle entité. Par exemple, fournir des données sur le nombre d'universités au cours des 150 dernières années utilisant une variété de sources disponibles (e. g. des documents financiers, des statistiques officielles, des registres universitaires), en combinant les données d'enquête avec des informations sur les zones géographiques provenant des statistiques officielles (e. g. la densité de population, médecins par habitants, etc.), ou en utilisant RSS pour collecter des articles de blogs ou des tweets, etc.</skos:definition>
      <skos:prefLabel xml:lang="it">Raccolta/sintesi</skos:prefLabel>
      <skos:definition xml:lang="it">Raccolta e assemblaggio di dati da più fonti, spesso eterogenee, che hanno uno o più punti di riferimento in comune, e dove almeno una delle fonti sia stata originariamente prodotta per altri scopi di ricerca. I dati sono incorporati in una nuova base di dati. Ad esempio, la raccolta di dati sul numero di università negli ultimi 150 anni attraverso diverse fonti disponibili (ad esempio documenti finanziari, statistiche ufficiali, registri universitari), successivamente combinati con le statistiche ufficiali relative alle aree geografiche (ad es. densità di popolazione, medici pro-capite, ecc.) o tramite RSS per raccogliere post o tweet del blog, ecc.</skos:definition>
      <skos:prefLabel xml:lang="no">Kompilering/Syntese</skos:prefLabel>
      <skos:definition xml:lang="no">Innsamling og sammensetting av data fra flere, ofte heterogene, kilder som har en eller flere felles referansepunkter, og minst én av kildene var opprinnelig utarbeidet for andre formål. Dataene blir integrert i en ny enhet. For eksempel utarbeide data om antallet universitet de siste 150 årene ved å bruke flere tilgjengelige kilder (e.g. finansdokumenter, offisiell statistikk, universitetsregistre), kombinere spørreundersøkelsesdata med informasjon om geografiske områder fra offisiell statistikk (e.g. befolkningstetthet, antall leger per innbygger, etc.), eller bruke RSS for å samle blogginnlegg eller tweets etc.</skos:definition>
      <skos:prefLabel xml:lang="pt">Compilação/síntese</skos:prefLabel>
      <skos:definition xml:lang="pt">Recolha e compilação de dados de fontes múltiplas, muitas vezes heterogéneas, que possuem um ou mais pontos de referência em comum, e pelo menos uma das fontes foi originalmente produzida para outras finalidades. Os dados são incorporados numa nova entidade. Por exemplo, providenciar dados sobre o número de universidades nos últimos 150 anos usando uma variedade de fontes disponíveis (por exemplo, documentos financeiros, estatísticas oficiais, registos universitários), combinando dados de inquéritos com informações sobre áreas geográficas a partir de estatísticas oficiais (por exemplo, densidade populacional, médicos per capita, etc.), ou usando o RSS (Really Simple Syndication) para recolher publicações de blogs ou tweets, etc.</skos:definition>
      <skos:prefLabel xml:lang="sl">Kompilacija/sinteza</skos:prefLabel>
      <skos:definition xml:lang="sl">Zbiranje in sestavljanje podatkov iz več, pogosto heterogenih virov, ki imajo eno ali več skupnih referenčnih točk in kjer je bil vsaj eden od virov prvotno produciran v druge namene. Podatki so vključeni v novo entiteto. Na primer z zagotavljanjem podatkov o številu univerz v zadnjih 150 letih z uporabo različnih razpoložljivih virov (npr. finančni dokumenti, uradne statistike, univerzitetni registri), kombiniranjem anketnih podatkov z informacijami o geografskih območjih iz uradnih statističnih podatkov (npr. gostota prebivalstva, število zdravnikov na prebivalca itd.) ali z uporabo RSS za zbiranje objav bloga ali tvitov itd.</skos:definition>
      <skos:prefLabel xml:lang="sr">Kompilacija / sinteza</skos:prefLabel>
      <skos:definition xml:lang="sr">Prikupljanje i objedinjavanje podataka iz više, često heterogenih izvora koji imaju jednu ili više referentnih tačaka, a bar jedan izvor originalno je proizveden u druge svrhe. Podaci su ugrađeni u novi entitet. Na primer, pružanje podataka o broju univerziteta u poslednjih 150 godina koristeći razne dostupne izvore (npr. finansijska dokumenta, zvanična statistika, univerzitetski registri), kombinujući podatke ankete sa podacima o geografskim oblastima iz zvanične statistike (npr. gustina naseljenosti, broj lekara po glavi stanovnika itd.) ili koristeći RSS za prikupljanje postova na blogovima ili tvitova, itd.</skos:definition>
      <skos:prefLabel xml:lang="sv">Kompilering/Syntes</skos:prefLabel>
      <skos:definition xml:lang="sv">Att samla in och sammanställa data från flera, ofta heterogena, källor som har en eller flera gemensamma referenspunkter, och där minst en av källorna ursprungligen producerades för andra syften. Datamaterialet har införlivats i ett nytt material. Exempel: data om antalet universitet under de senaste 150 åren som tas fram med hjälp av ett antal olika källor (t.ex. räkenskaper, offentlig statistik och universitetsrullor); en kombination av surveydata med information om geografiska områden från offentlig statistik (t.ex. befolkningstäthet, läkare per capita osv); eller bloggposter, tweetar, m.m. som samlats in med hjälp av RSS.</skos:definition>
   </rdf:Description>
   <rdf:Description rdf:about="http://rdf-vocabulary.ddialliance.org/cv/ModeOfCollection/3.0/d64e4089">
      <rdf:type rdf:resource="http://www.w3.org/2004/02/skos/core#Concept"/>
      <skos:inScheme rdf:resource="http://rdf-vocabulary.ddialliance.org/cv/ModeOfCollection/3.0"/>
      <skos:notation>Summary</skos:notation>
      <skos:prefLabel xml:lang="en">Summary</skos:prefLabel>
      <skos:definition xml:lang="en">Presentation of information in a condensed form, by reducing it to its main points. For example, abstracts of interviews or reports that are published and used as data rather than the full-length interviews or reports.</skos:definition>
      <skos:prefLabel xml:lang="da">Resumé</skos:prefLabel>
      <skos:definition xml:lang="da">Præsentation af oplysninger i kondenseret form, ved at reducere den til dens hovedpunkter. For eksempel abstracts af interviews eller reporter, der publiceres og anvendes som data frem for interviews og rapporter i fuld længde.</skos:definition>
      <skos:prefLabel xml:lang="fi">Yhteenveto,  lyhennelmä tai tiivistelmä</skos:prefLabel>
      <skos:definition xml:lang="fi">Tietoa kerätään muodostamalla yhteenveto tai tiivistelmä olennaisista seikoista. Esimerkiksi: Haastatteluista ei tehdä translitteraatioita vaan aineisto muodostuu haastattelujen tiivistelmistä, tai sanomalehtiuutisisten aiheista muodostetaan aineisto tiivistämällä ne pariin lauseeseen. Mikäli kvalitatiivisesta lähdeaineistosta muodostetaan kvantitatiivinen aineisto, käytä termiä 'Sisällönkoodaus'.</skos:definition>
      <skos:prefLabel xml:lang="fr">Résumé</skos:prefLabel>
      <skos:definition xml:lang="fr">Présentation d'informations dans une forme condensée, en les réduisant à leurs points importants. Par exemple, des résumés d'entretiens ou de rapports qui sont publiés et utilisés comme des données plutôt que des entretiens ou des rapports complets.</skos:definition>
      <skos:prefLabel xml:lang="fr">Résumé</skos:prefLabel>
      <skos:definition xml:lang="fr">Présentation d'informations dans une forme condensée, en les réduisant à leurs points importants. Par exemple, des résumés d'entretiens ou de rapports qui sont publiés et utilisés comme des données plutôt que des entretiens ou des rapports complets.</skos:definition>
      <skos:prefLabel xml:lang="it">Sintesi</skos:prefLabel>
      <skos:definition xml:lang="it">Presentazione di informazioni in forma sintetica, riducendole ai punti principali. Ad esempio, abstract di interviste o report che vengono pubblicati e utilizzati come dati, al posto delle interviste o dei report completi.</skos:definition>
      <skos:prefLabel xml:lang="no">Sammendrag</skos:prefLabel>
      <skos:definition xml:lang="no">Presentasjon av informasjon i en konsentrert form, ved å redusere den til dens hovedpoeng. For eksempel, sammendrag av intervjuer eller rapporter som er publisert og brukt som data til fordel for de fulle intervjuene eller rapportene.</skos:definition>
      <skos:prefLabel xml:lang="pt">Sumário/resumo</skos:prefLabel>
      <skos:definition xml:lang="pt">Apresentação de informação de forma resumida, reduzindo-a aos seus pontos principais. Por exemplo, resumos de entrevistas ou de relatórios que são publicados e usados como dados, em vez de entrevistas ou relatórios completos.</skos:definition>
      <skos:prefLabel xml:lang="sl">Povzetek</skos:prefLabel>
      <skos:definition xml:lang="sl">Predstavitev informacij v zgoščeni obliki z reduciranjem na glavne točke. Na primer, povzetki intervjujev ali poročil, ki so objavljeni in uporabljeni kot podatki in ne kot celoviti intervjuji ali poročila.</skos:definition>
      <skos:prefLabel xml:lang="sr">Rezime</skos:prefLabel>
      <skos:definition xml:lang="sr">Predstavljanje informacija u skraćenom obliku, svodeći je na glavne tačke. Na primer, sažeci intervjua ili izvještaji koji se objavljuju i koriste kao podaci, a ne celoviti intervjui ili izveštaji.</skos:definition>
      <skos:prefLabel xml:lang="sv">Sammanfattning</skos:prefLabel>
      <skos:definition xml:lang="sv">Presentation av information i sammandrag, som reducerats till sitt viktigaste innehåll. Exempel: Abstrakt från intervjuer eller rapporter publiceras och används som data istället för de fullständiga intervjuerna eller rapporterna.</skos:definition>
   </rdf:Description>
   <rdf:Description rdf:about="http://rdf-vocabulary.ddialliance.org/cv/ModeOfCollection/3.0/d64e4179">
      <rdf:type rdf:resource="http://www.w3.org/2004/02/skos/core#Concept"/>
      <skos:inScheme rdf:resource="http://rdf-vocabulary.ddialliance.org/cv/ModeOfCollection/3.0"/>
      <skos:notation>Aggregation</skos:notation>
      <skos:prefLabel xml:lang="en">Aggregation</skos:prefLabel>
      <skos:definition xml:lang="en">Statistics that relate to broad classes, groups, or categories. The data are averaged, totaled, or otherwise derived from individual-level data, and it is no longer possible to distinguish the characteristics of individuals within those classes, groups, or categories. For example, the number and age group of the unemployed in specific geographic regions, or national level statistics on the occurrence of specific offences, originally derived from the statistics of individual police districts.</skos:definition>
      <skos:prefLabel xml:lang="da">Aggregering</skos:prefLabel>
      <skos:definition xml:lang="da">Statistik, der vedrører bredere klasser, grupper eller kategorier. Dataene er i gennemsnit, summeret eller på anden vis afledt af data på individuelt niveau, og det er ikke længere muligt at adskille individers karakteristika inden for disse klasser, grupper eller kategorier. For eksempel antallet eller aldersgruppen for de ledige i en bestemt geografisk region eller statistik på et nationalt plan om forekomsten af specifikke lovovertrædelser, der oprindeligt er afledt af statistikkerne for de enkelte politidistrikter.</skos:definition>
      <skos:prefLabel xml:lang="fi">Aggregointi</skos:prefLabel>
      <skos:definition xml:lang="fi">Tilastollinen tieto, jossa yksittäisiä havaintoyksiköitä koskevat tiedot ovat keskiarvoistettu, yhteenlaskettu tai jotenkin muuten yhdistetty laajempaa ryhmää koskevaksi tiedoksi siten, että yksittäisen havaintoyksiköiden tiedot eivät ole enää erotettavissa. Esimerkkejä: Kansallinen rikostilasto, joka yhteenlaskettu yksittäisten poliisipiirien tilastoista, tai kuukausittainen hintaindeksi, joka on keskiarvo yksittäisten hyödykkeiden hinnoista.</skos:definition>
      <skos:prefLabel xml:lang="fr">Agrégation</skos:prefLabel>
      <skos:definition xml:lang="fr">Statistiques qui concernent des classes, des groupes, ou des catégories. Les données sont calculées en moyenne, additionnées, ou autrement dérivées des données au niveau individuel, et il n'est plus possible de distinguer les caractéristiques des individus au sein de ces classes, groupes, ou catégories. Par exemple, le nombre et le groupe d'âge des chômeurs dans des régions géographiques spécifiques, ou des statistiques nationales sur l'apparition de certaines infractions, tirées originellement des statistiques de différents districts de police.</skos:definition>
      <skos:prefLabel xml:lang="fr">Agrégation</skos:prefLabel>
      <skos:definition xml:lang="fr">Statistiques qui concernent des classes, des groupes, ou des catégories. Les données sont calculées en moyenne, additionnées, ou autrement dérivées des données au niveau individuel, et il n'est plus possible de distinguer les caractéristiques des individus au sein de ces classes, groupes, ou catégories. Par exemple, le nombre et le groupe d'âge des chômeurs dans des régions géographiques spécifiques, ou des statistiques nationales sur l'apparition de certaines infractions, tirées originellement des statistiques de différents districts de police.</skos:definition>
      <skos:prefLabel xml:lang="it">Aggregazione</skos:prefLabel>
      <skos:definition xml:lang="it">Statistiche relative a classi, gruppi o categorie. I dati rappresentano il valore medio, la somma o altre derivazioni dei dati raccolti a livello individuale, che non consentono più di distinguere le caratteristiche degli individui all'interno di tali classi, gruppi o categorie. Ad esempio, il numero e la fascia di età dei disoccupati in specifiche regioni geografiche, o le statistiche a livello nazionale sul verificarsi di reati specifici, originariamente desunti dalle statistiche dei singoli distretti di polizia.</skos:definition>
      <skos:prefLabel xml:lang="no">Aggregering</skos:prefLabel>
      <skos:definition xml:lang="no">Statistikk som relateres til store klasser, grupper eller kategorier. Dataene er tatt gjennomsnittet av, summert, eller på andre måter utvunnet av data på individnivå, og det er ikke lengre mulig å skille mellom egenskapene til individer innad i disse klassene, gruppene eller kategoriene. For eksempel, antallet og aldersgruppen til de arbeidsledige i bestemte regioner, eller statistikk på nasjonalt nivå om forekomsten av bestemte overtredelser, opprinnelig utarbeidet fra statistikk om individuelle politidistrikt.</skos:definition>
      <skos:prefLabel xml:lang="pt">Agregação</skos:prefLabel>
      <skos:definition xml:lang="pt">Estatísticas relacionadas com classes, grupos ou categorias amplas. Os dados são representados por médias, totais, ou derivados de dados registados a um nível individual, não sendo mais possível distinguir as características dos indivíduos dentro dessas classes, grupos ou categorias. Por exemplo, o número e a faixa etária dos desempregados em regiões geográficas específicas, ou estatísticas de âmbito nacional sobre a ocorrência de crimes específicos, originalmente derivadas das estatísticas policiais de cada distrito.</skos:definition>
      <skos:prefLabel xml:lang="sl">Agregacija</skos:prefLabel>
      <skos:definition xml:lang="sl">Statistike, ki se nanašajo na širše razrede, skupine ali kategorije. Podatki so predstavljeni kot povprečja, vsote ali druge izpeljave, na podlagi katerih ni več možno razlikovati med značilnostmi posameznikov znotraj teh razredov, skupin ali kategorij. Na primer, število in starostna skupina brezposelnih v posebnih geografskih regijah ali nacionalne statistike o pojavu poosameznih kaznivih dejanj, ki so bila prvotno izpeljana iz statističnih podatkov posameznih policijskih okrožij.</skos:definition>
      <skos:prefLabel xml:lang="sr">Agregacija</skos:prefLabel>
      <skos:definition xml:lang="sr">Statistika koja se odnosi na široke klase, grupe ili kategorije. Podaci su dati na nivou proseka, zbira ili su na neki drugi način izvedeni iz podataka prikupljenih na nivou pojedinaca i više nije moguće razlikovati karakteristike pojedinaca u tim klasama, grupama ili kategorijama. Na primer, broj i starosna grupa nezaposlenih u određenim geografskim regionima ili statistika na nacionalnom nivou o pojavljivanju određenih krivičnih dela, izvorno izvedena iz statistika pojedinih policijskih okruga.</skos:definition>
      <skos:prefLabel xml:lang="sv">Aggregation</skos:prefLabel>
      <skos:definition xml:lang="sv">Statistik som rör breda klasser, grupper eller kategorier. Datamaterialet består av genomsnitt, totalsummor eller andra värden som har härletts från data på individnivå, och det går inte längre att utläsa individernas egenskaper inom dessa klasser, grupper eller kategorier. Exempel: antal och ålderskategorier för arbetslösa inom särskilda geografiska områden, eller statistik på nationsnivå över förekomsten av särskilda brott som ursprungligen härletts från statistik från enskilda polisdistrikt.</skos:definition>
   </rdf:Description>
   <rdf:Description rdf:about="http://rdf-vocabulary.ddialliance.org/cv/ModeOfCollection/3.0/d64e4269">
      <rdf:type rdf:resource="http://www.w3.org/2004/02/skos/core#Concept"/>
      <skos:inScheme rdf:resource="http://rdf-vocabulary.ddialliance.org/cv/ModeOfCollection/3.0"/>
      <skos:notation>Simulation</skos:notation>
      <skos:prefLabel xml:lang="en">Simulation</skos:prefLabel>
      <skos:definition xml:lang="en">Modeling or imitative representation of real-world processes, events, or systems, often using computer programs. For example, a program modeling household consumption responses to indirect tax changes; or a dataset on hypothetical patients and their drug exposure, background conditions, and known adverse events.</skos:definition>
      <skos:prefLabel xml:lang="da">Simulation</skos:prefLabel>
      <skos:definition xml:lang="da">Modellering eller imitativ repræsentation af processer i den virkelige verden, hændelser eller systemer, ofte ved brug af computerprogrammer. For eksempel et program, der modellerer husholdningsforbrug, som responderer til indirekte skatteændringer; eller et datasæt om hypotetiske patienter og deres lægemiddeleksponering, baggrundsforhold og kendte bivirkninger.</skos:definition>
      <skos:prefLabel xml:lang="fi">Simulointi</skos:prefLabel>
      <skos:definition xml:lang="fi">Todellisten prosessien, tapahtumien ja systeemien piirteiden tai mahdollisen muuttumisen tutkiminen mallintamalla, usein tietokoneohjelmia käyttäen.</skos:definition>
      <skos:prefLabel xml:lang="fr">Simulation</skos:prefLabel>
      <skos:definition xml:lang="fr">Modélisation ou représentation imitative de processus, d’événements ou de systèmes réels, utilisant souvent des programmes informatiques. Par exemple, un programme modélisant des réactions de la consommation des ménages aux changement des impôts indirects ; ou un jeu de données sur des patients hypothétiques et leur exposition aux médicaments, aux conditions environnementales, et aux effets indésirables connus.</skos:definition>
      <skos:prefLabel xml:lang="fr">Simulation</skos:prefLabel>
      <skos:definition xml:lang="fr">Modélisation ou représentation imitative de processus, d’événements ou de systèmes réels, utilisant souvent des programmes informatiques. Par exemple, un programme modélisant des réactions de la consommation des ménages aux changement des impôts indirects ; ou un jeu de données sur des patients hypothétiques et leur exposition aux médicaments, aux conditions environnementales, et aux effets indésirables connus.</skos:definition>
      <skos:prefLabel xml:lang="it">Simulazione</skos:prefLabel>
      <skos:definition xml:lang="it">Modellazione o rappresentazione finalizzata alla riproduzione di processi, eventi o sistemi reali, spesso utilizzando programmi per computer. Ad esempio, un programma che modella le risposte dei consumi delle famiglie alle variazioni delle imposte indirette; o un dataset relativo a pazienti ipotetici e alla loro esposizione a farmaci, alle condizioni di fondo e ad eventi avversi conosciuti.</skos:definition>
      <skos:prefLabel xml:lang="no">Simulering</skos:prefLabel>
      <skos:definition xml:lang="no">Modellering eller etterlignende representasjon av virkelige prosesser, hendelser eller systemer, ofte ved bruk av dataprogrammer. For eksempel et program som modellerer hvordan en husholdnings forbruk svarer på endringer i indirekte skatter; eller et datasett om hypotetiske pasienter og deres eksponering for narkotiske stoffer, bakgrunnsforhold, og kjente ugunstige hendelser.</skos:definition>
      <skos:prefLabel xml:lang="pt">Simulação</skos:prefLabel>
      <skos:definition xml:lang="pt">Modelação ou representação por imitação de processos, eventos ou sistemas do mundo real, utilizando geralmente programas de computador. Por exemplo, um programa que modela as respostas do consumo das famílias às mudanças tributárias indiretas; ou um conjunto de dados em pacientes hipotéticos e a sua exposição a drogas, condições do contexto e eventos adversos conhecidos.</skos:definition>
      <skos:prefLabel xml:lang="sl">Simulacija</skos:prefLabel>
      <skos:definition xml:lang="sl">Modeliranje ali oponašajoče predstavljanje procesov, dogodkov ali sistemov v realnem svetu, pogosto z uporabo računalniških programov. Na primer program, ki modelira odziv potrošnje gospodinjstev na posredne davčne spremembe; ali podatkovje o hipotetičnih pacientih in njihovi izpostavljenosti zdravilu, pogojih v ozadju in znanih neželenih doogodkih.</skos:definition>
      <skos:prefLabel xml:lang="sr">Simulacija</skos:prefLabel>
      <skos:definition xml:lang="sr">Modeliranje ili imitacija reprezentacije procesa, događaja ili sistema u stvarnom svetu, često koristeći računarske programe. Na primer, program koji modelira reakcije potrošnje domaćinstava na indirektne promene poreza ili skup podataka o hipotetičkim pacijentima i njihovoj izloženosti lekovima, pozadinskim uslovima i poznatim neželjenim događajima.</skos:definition>
      <skos:prefLabel xml:lang="sv">Simulering</skos:prefLabel>
      <skos:definition xml:lang="sv">Modellering eller imiterande representation av processer, händelser eller system i den verkliga världen, ofta skapade med datorprogram. Exempel: ett program som modellerar hur hushållens konsumtion svarar på förändringar i indirekta skatter; eller ett dataset över hypotetiska patienter och deras droganvändning, bakgrundsförhållanden och kända negativa händelser.</skos:definition>
   </rdf:Description>
   <rdf:Description rdf:about="http://rdf-vocabulary.ddialliance.org/cv/ModeOfCollection/3.0/d64e4360">
      <rdf:type rdf:resource="http://www.w3.org/2004/02/skos/core#Concept"/>
      <skos:inScheme rdf:resource="http://rdf-vocabulary.ddialliance.org/cv/ModeOfCollection/3.0"/>
      <skos:notation>MeasurementsAndTests</skos:notation>
      <skos:prefLabel xml:lang="en">Measurements and tests</skos:prefLabel>
      <skos:definition xml:lang="en">Assessing specific properties (or characteristics) of beings, things, phenomena, (and/ or processes) by applying pre-established standards and/or specialized instruments or techniques.</skos:definition>
      <skos:prefLabel xml:lang="da">Målinger og tests</skos:prefLabel>
      <skos:definition xml:lang="da">Vurdere specifikke egenskaber (eller karakteristika) af væsener, ting, fænomener (og/eller processer) ved at anvende forudbestemte standarder og/eller specialiserede instrumenter eller teknikker.</skos:definition>
      <skos:prefLabel xml:lang="fi">Mittaukset ja testit</skos:prefLabel>
      <skos:definition xml:lang="fi">Ihmisten ja muiden elollisten olioiden, esineiden, materiaalien ja ilmiöiden ominaisuuksien mittaaminen käyttäen etukäteen määriteltyjä standardeja tai tarkoitukseen kehitettyjä mittareita ja tekniikoita.</skos:definition>
      <skos:prefLabel xml:lang="fr">Mesures et tests</skos:prefLabel>
      <skos:definition xml:lang="fr">Évaluer des propriétés spécifiques (ou caractéristiques) d'êtres, de choses, de phénomènes, (et / ou processus) en appliquant des standards préétablis et / ou des instruments ou des techniques spécialisés.</skos:definition>
      <skos:prefLabel xml:lang="fr">Mesures et tests</skos:prefLabel>
      <skos:definition xml:lang="fr">Évaluer des propriétés spécifiques (ou caractéristiques) d'êtres, de choses, de phénomènes, (et / ou processus) en appliquant des standards préétablis et / ou des instruments ou des techniques spécialisés.</skos:definition>
      <skos:prefLabel xml:lang="it">Misurazioni e test</skos:prefLabel>
      <skos:definition xml:lang="it">Valutazione di specifiche proprietà (o caratteristiche) di esseri viventi, cose, fenomeni (e/o processi) applicando standard prestabiliti e/o strumenti o tecniche specializzate.</skos:definition>
      <skos:prefLabel xml:lang="no">Målinger og tester</skos:prefLabel>
      <skos:definition xml:lang="no">Vurdering av bestemte egenskaper (eller karakteristika) ved vesener, ting, fenomen (og/eller prosesser) ved å anvende forutbestemte standarder og/eller spesialiserte instrumenter eller teknikker.</skos:definition>
      <skos:prefLabel xml:lang="pt">Medidas e testes</skos:prefLabel>
      <skos:definition xml:lang="pt">Avaliação de propriedades específicas (ou características) de seres, coisas, fenómenos (e/ou processos) aplicando padrões pré-estabelecidos e/ou técnicas e instrumentos específicos.</skos:definition>
      <skos:prefLabel xml:lang="sl">Merjenje in testiranje</skos:prefLabel>
      <skos:definition xml:lang="sl">Ocenjevanje specifičnih lastnosti (ali značilnosti) bitij, stvari, pojavov (in/ali procesov), z uporabo vnaprej določenih standardov in/ali specializiranih instrumentov ali tehnik.</skos:definition>
      <skos:prefLabel xml:lang="sr">Merenje i testiranje</skos:prefLabel>
      <skos:definition xml:lang="sr">Procena specifičnih svojstava (ili karakteristika) bića, stvari, pojava (i / ili procesa) primenom unapred utvrđenih standarda i / ili specijalizovanih instrumenata ili tehnika.</skos:definition>
      <skos:prefLabel xml:lang="sv">Mätningar och tester</skos:prefLabel>
      <skos:definition xml:lang="sv">Bedömning av varelsers, föremåls, fenomens (och/eller processers) särskilda egenskaper (eller karakteristiska) genom att tillämpa förutbestämda standarder och/eller specialiserade instrument eller tekniker.</skos:definition>
      <skos:narrower rdf:resource="http://rdf-vocabulary.ddialliance.org/cv/ModeOfCollection/3.0/d64e4457"/>
      <skos:narrower rdf:resource="http://rdf-vocabulary.ddialliance.org/cv/ModeOfCollection/3.0/d64e4547"/>
      <skos:narrower rdf:resource="http://rdf-vocabulary.ddialliance.org/cv/ModeOfCollection/3.0/d64e4637"/>
   </rdf:Description>
   <rdf:Description rdf:about="http://rdf-vocabulary.ddialliance.org/cv/ModeOfCollection/3.0/d64e4457">
      <rdf:type rdf:resource="http://www.w3.org/2004/02/skos/core#Concept"/>
      <skos:inScheme rdf:resource="http://rdf-vocabulary.ddialliance.org/cv/ModeOfCollection/3.0"/>
      <skos:notation>MeasurementsAndTests.Educational</skos:notation>
      <skos:prefLabel xml:lang="en">Educational measurements and tests</skos:prefLabel>
      <skos:definition xml:lang="en">Assessment of knowledge, skills, aptitude, or educational achievement by means of specialized measures or tests.</skos:definition>
      <skos:prefLabel xml:lang="da">Udannelsesmæssige målinger og tests</skos:prefLabel>
      <skos:definition xml:lang="da">Vurdering af viden, færdigheder, egnethed eller uddannelsesmæssig præstation ved brug af specialiserede målinger eller tests.</skos:definition>
      <skos:prefLabel xml:lang="fi">Mittaukset ja testit: tietämyksen, taipumusten, soveltuvuuden ja oppimistulosten mittaaminen</skos:prefLabel>
      <skos:definition xml:lang="fi">Mittaamalla tai testaamalla saadut tiedot tutkittavien tietotasosta, synnynnäisistä taipumuksista, soveltuvuudesta tai oppimistuloksista. Esimerkkejä: PISA-testit, ylioppilaskokeiden tulokset, yhteiskunnallisen tietämyksen mittari, tai kielellistä tai matemaattista lahjakkuutta mittaavat testit.</skos:definition>
      <skos:prefLabel xml:lang="fr">Mesures et tests d'enseignement</skos:prefLabel>
      <skos:definition xml:lang="fr">Évaluation de connaissances, de compétences, d'aptitudes, ou de résultats scolaires au moyen de mesures ou tests spécialisés.</skos:definition>
      <skos:prefLabel xml:lang="fr">Mesures et tests d'enseignement</skos:prefLabel>
      <skos:definition xml:lang="fr">Évaluation de connaissances, de compétences, d'aptitudes, ou de résultats scolaires au moyen de mesures ou tests spécialisés.</skos:definition>
      <skos:prefLabel xml:lang="it">Misurazioni e test in ambito educativo</skos:prefLabel>
      <skos:definition xml:lang="it">Valutazione delle conoscenze, abilità, attitudini o risultati in ambito educativo mediante misure o test specializzati.</skos:definition>
      <skos:prefLabel xml:lang="no">Pedagogiske målinger og tester</skos:prefLabel>
      <skos:definition xml:lang="no">Vurdering av kunnskap, ferdighet, egnethet, eller utdanningsoppnåelser ved spesialiserte mål eller tester.</skos:definition>
      <skos:prefLabel xml:lang="pt">Medidas e testes educacionais</skos:prefLabel>
      <skos:definition xml:lang="pt">Avaliação de conhecimentos, competências, aptidões ou desempenhos educacionais por meio de medidas ou testes específicos.</skos:definition>
      <skos:prefLabel xml:lang="sl">Meritve in testiranja v vzgoji in izobraževanju</skos:prefLabel>
      <skos:definition xml:lang="sl">Ocenjevanje znanja, spretnosti, sposobnosti ali izobraževalnih dosežkov s pomočjo specializiranih meritev ali testov.</skos:definition>
      <skos:prefLabel xml:lang="sr">Obrazovno merenje i testiranje</skos:prefLabel>
      <skos:definition xml:lang="sr">Procena znanja, veština, sposobnosti ili obrazovnog dostignuća pomoću specijalizovanih mera ili testova.</skos:definition>
      <skos:prefLabel xml:lang="sv">Pedagogiska mätningar och tester</skos:prefLabel>
      <skos:definition xml:lang="sv">Bedömning av kunskap, förmågor, begåvning eller inlärningsförmåga med hjälp av specialiserade mätredskap och tester.</skos:definition>
      <skos:broader rdf:resource="http://rdf-vocabulary.ddialliance.org/cv/ModeOfCollection/3.0/d64e4360"/>
   </rdf:Description>
   <rdf:Description rdf:about="http://rdf-vocabulary.ddialliance.org/cv/ModeOfCollection/3.0/d64e4547">
      <rdf:type rdf:resource="http://www.w3.org/2004/02/skos/core#Concept"/>
      <skos:inScheme rdf:resource="http://rdf-vocabulary.ddialliance.org/cv/ModeOfCollection/3.0"/>
      <skos:notation>MeasurementsAndTests.Physical</skos:notation>
      <skos:prefLabel xml:lang="en">Physical measurements and tests</skos:prefLabel>
      <skos:definition xml:lang="en">Assessment of physical properties of living beings, objects, materials, or natural phenomena. For example, findings from hands-on medical examination (e.g., palpation or auscultation), clinical measurements and lab tests like blood analysis, blood pressure, heart rate, body weight and height, as well as general measurements like time, distance, mass, temperature, force, power, speed, GPS data on physical movement and other physical parameters or variables, like geospatial data.</skos:definition>
      <skos:prefLabel xml:lang="da">Fysiske målinger og tests</skos:prefLabel>
      <skos:definition xml:lang="da">Vurdering af fysiske egenskaber hos levende væsener, objekter, materialer eller naturlige fænomener. For eksempel resultater fra praktisk lægeundersøgelse (f.eks. palpation eller auskultation), kliniske målinger og laboratorietests såsom blodanalyse, blodtryk, hjerterytme, kropsvægt og højde, såvel som generelle målinger såsom tid, afstand, masse, temperatur, styrke, kraft, hastighed, GPS-data om fysisk bevægelse og andre fysiske parametre eller variabler, såsom geospatiale data.</skos:definition>
      <skos:prefLabel xml:lang="fi">Mittaukset ja testit: fyysisten ominaisuuksien mittaaminen</skos:prefLabel>
      <skos:definition xml:lang="fi">Ihmisten ja muiden elollisten olioiden, esineiden, materiaalien ja luonnonilmiöiden fyysisten ominaisuuksien mittaaminen. Esimerkkejä: verenpaine, paino ja pituus, voima, etäisyys, lämpötila, nopeus, seismografiset mittaukset, GPS-koordinaatit.</skos:definition>
      <skos:prefLabel xml:lang="fr">Mesures et tests de caractéristiques physiques</skos:prefLabel>
      <skos:definition xml:lang="fr">Évaluation des propriétés physiques d'êtres vivants, d'objets, de matériaux, ou de phénomènes naturels. Par exemple, des résultats d'examens cliniques (e. g. palpation, auscultation), mesures cliniques and tests de laboratoire comme analyse de sang, pression sanguine, rythme cardiaque, poids et taille du corps, de même que des mesures générales de temps, de distance, de masse, de température, de force, de puissance, de vitesse, de données de localisation sur des mouvements physiques ou d'autres paramètres ou variables physiques comme des données géospatiales.</skos:definition>
      <skos:prefLabel xml:lang="fr">Mesures et tests de caractéristiques physiques</skos:prefLabel>
      <skos:definition xml:lang="fr">Évaluation des propriétés physiques d'êtres vivants, d'objets, de matériaux, ou de phénomènes naturels. Par exemple, des résultats d'examens cliniques (e. g. palpation, auscultation), mesures cliniques and tests de laboratoire comme analyse de sang, pression sanguine, rythme cardiaque, poids et taille du corps, de même que des mesures générales de temps, de distance, de masse, de température, de force, de puissance, de vitesse, de données de localisation sur des mouvements physiques ou d'autres paramètres ou variables physiques comme des données géospatiales.</skos:definition>
      <skos:prefLabel xml:lang="it">Misurazioni e test fisici</skos:prefLabel>
      <skos:definition xml:lang="it">Valutazione delle proprietà fisiche di esseri viventi, oggetti, materiali o fenomeni naturali. Per esempio, risultati di esami pratici a livello medico (ad esempio, palpazione o auscultazione), misurazioni cliniche e test di laboratorio come analisi del sangue, pressione sanguigna, frequenza cardiaca, peso corporeo e altezza, nonché misure generali come tempo, distanza, massa, temperatura, forza, potenza, velocità, dati GPS sul movimento fisico e altri parametri o variabili fisici, come i dati geospaziali.</skos:definition>
      <skos:prefLabel xml:lang="no">Fysiske målinger og tester</skos:prefLabel>
      <skos:definition xml:lang="no">Vurdering av fysiske egenskaper hos levende vesener, objekter, materiale, eller naturlige fenomen. For eksempel, funn fra fysiske medisinske undersøkelser (e.g., palpasjon eller auskultasjon), kliniske mål og laboratorietester som blodanalyse, blodtrykksmål, hjerterytme, kroppsvekt og høyde, og generelle mål som tid, distanse, masse, temperatur, kraft, energi, fart, GPS data på fysisk bevegelse og andre mål på fysiske parameter eller variabler.</skos:definition>
      <skos:prefLabel xml:lang="pt">Medidas e testes físicos</skos:prefLabel>
      <skos:definition xml:lang="pt">Avaliação de propriedades físicas de seres vivos, objetos, materiais ou fenómenos naturais. Por exemplo, descobertas de exames médicos práticos (por exemplo, palpação ou auscultação), medições clínicas e testes laboratoriais, como análise sanguínea, pressão arterial, frequência cardíaca, peso e altura, assim como medidas gerais, por exemplo, de tempo, distância, massa, temperatura, força, potência, velocidade, dados de GPS sobre movimento físico e outros parâmetros ou variáveis físicos, como dados geoespaciais.</skos:definition>
      <skos:prefLabel xml:lang="sl">Meritve in testiranja fizičnih lastnosti</skos:prefLabel>
      <skos:definition xml:lang="sl">Ocenjevanje fizičnih lastnosti živih bitij, predmetov, materialov ali naravnih pojavov. Na primer ugotovitve praktičnega zdravniškega pregleda (npr. palpacije ali auskultacije), kliničnih meritev in laboratorijskih preiskav, kot so analiza krvi, krvni talak, srčni utrip, telesna teža in višina ter splošne meritve, kot so čas, razdalja, temperatura, sila, moč, hitrost, podatki GPS o fizičnem gibanju in drugih fizičnih parametrih ali spremenljivkah, kot so geoprostorski podatki.</skos:definition>
      <skos:prefLabel xml:lang="sr">Fizičko merenje i testiranje</skos:prefLabel>
      <skos:definition xml:lang="sr">Procena fizičkih svojstava živih bića, predmeta, materijala ili prirodnih pojava. Na primer, nalaz iz praktičnog medicinskog pregleda (npr. palpacije ili auskultacije), kliničkih merenja i laboratorijskih testova poput analize krvi, krvnog pritiska, otkucaja srca, telesne težine i visine, kao i opštih merenja kao što su vreme, udaljenost, masa, temperatura, sila, snaga, brzina, GPS podaci o fizičkom kretanju i drugi fizički parametri ili promenljive, poput geoprostornih podataka.</skos:definition>
      <skos:prefLabel xml:lang="sv">Fysiska mätningar och tester</skos:prefLabel>
      <skos:definition xml:lang="sv">Bedömning av levande varelsers, föremåls, materials eller naturliga fenomens fysiska egenskaper. Till exempel: blodtryck, puls, kroppsvikt och längd, men även tid, avstånd, massa, temperatur, kraft, effekt, hastighet, GPS-data för fysisk rörelse och andra fysiska parametrar eller variabler, som t.ex. geospatiala data.</skos:definition>
      <skos:broader rdf:resource="http://rdf-vocabulary.ddialliance.org/cv/ModeOfCollection/3.0/d64e4360"/>
   </rdf:Description>
   <rdf:Description rdf:about="http://rdf-vocabulary.ddialliance.org/cv/ModeOfCollection/3.0/d64e4637">
      <rdf:type rdf:resource="http://www.w3.org/2004/02/skos/core#Concept"/>
      <skos:inScheme rdf:resource="http://rdf-vocabulary.ddialliance.org/cv/ModeOfCollection/3.0"/>
      <skos:notation>MeasurementsAndTests.Psychological</skos:notation>
      <skos:prefLabel xml:lang="en">Psychological measurements and tests</skos:prefLabel>
      <skos:definition xml:lang="en">Assessment of personality traits or psychological/behavioral responses by means of specialized measures or tests. For example, objective tests like self-report measures with a restricted response format, or projective methods allowing free responses, including word association, sentence or story completion, vignettes, cartoon test, thematic apperception tests, role play, drawing tests, inkblot tests, choice ordering exercises, etc.</skos:definition>
      <skos:prefLabel xml:lang="da">Psykologiske målinger og tests</skos:prefLabel>
      <skos:definition xml:lang="da">Vurdering af personlighedskarakterer eller psykologiske/adfærdsmæssige reaktioner ved hjælp af specialiserede målinger og tests. For eksempel objektive tests såsom selvrapporterende målinger med et begrænset responsformat eller projektive metoder, der tillader fri respons, inklusiv associering af ord, sætninger eller historiefærdiggørelse, vignetter, tegneserietests, tematiske accerceptionstests, rollespil, tegnetests, blækklattests, øvelser om valgprioritering mm.</skos:definition>
      <skos:prefLabel xml:lang="fi">Mittaukset ja testit: psykologisten ominaisuuksien mittaaminen</skos:prefLabel>
      <skos:definition xml:lang="fi">Luonteenpiirteiden ja käyttäytymismallien tutkiminen tarkoitusta varten kehitettyjen testien avulla. Esimerkiksi: Luonteenpiirteiden itseraportointi, eläytymismenetelmät. Tarvittaessa voidaan käyttää yhdessä muiden aineistonkeruumenetelmätermien kanssa (esimerkiksi masentuneisuusaste-testi osana kyselylomaketta).</skos:definition>
      <skos:prefLabel xml:lang="fr">Mesures et tests psychologiques</skos:prefLabel>
      <skos:definition xml:lang="fr">Évaluation des traits de personnalités ou de réponses psychologiques / comportementales au moyen de mesures ou tests spécialisés. Par exemple, des tests objectifs comme mesure d'auto-évaluation avec un format restreint de réponses, ou des méthodes projectives permettant des réponses libres, incluant l'association de mots, l'achèvement de phrase ou d'histoire, des vignettes, des tests animés, des tests thématiques d'apperception, du jeu de rôle, des tests de dessin, des tests de tâches d'encre, des exercices de classement, etc.</skos:definition>
      <skos:prefLabel xml:lang="fr">Mesures et tests psychologiques</skos:prefLabel>
      <skos:definition xml:lang="fr">Évaluation des traits de personnalités ou de réponses psychologiques / comportementales au moyen de mesures ou tests spécialisés. Par exemple, des tests objectifs comme mesure d'auto-évaluation avec un format restreint de réponses, ou des méthodes projectives permettant des réponses libres, incluant l'association de mots, l'achèvement de phrase ou d'histoire, des vignettes, des tests animés, des tests thématiques d'apperception, du jeu de rôle, des tests de dessin, des tests de tâches d'encre, des exercices de classement, etc.</skos:definition>
      <skos:prefLabel xml:lang="it">Misurazioni e test psicologici</skos:prefLabel>
      <skos:definition xml:lang="it">Valutazione dei tratti di personalità o risposte psicologiche/comportamentali mediante misure o test specializzati. Ad esempio, test oggettivi come misure di autovalutazione con un range predefinito, o test proiettivi che consentono risposte libere, incluse associazione di parole, completamento di frasi o storie, vignette, fumetti, test di appercezione tematica, giochi di ruolo, prove di disegno, test macchie di inchiostri, esercizi sulle scelte di ordinamento, ecc.</skos:definition>
      <skos:prefLabel xml:lang="no">Psykologiske målinger og tester</skos:prefLabel>
      <skos:definition xml:lang="no">Vurdering av personlighetstrekk eller psykologiske/atferdsmessige reaksjoner ved bruk av spesialiserte mål og tester. For eksempel, objektive tester som selvrapporteringsmål med mer begrenset svarformat, eller projektive metoder som gjør det mulig å svare helt fritt, inkludert ordassosiasjon, setning eller fortellingsfullføring, korte beskrivelser, tematiske appersepsjonstester, rollespill, tegnetester, blekk-kladd tester, prioriteringsøvelser etc.</skos:definition>
      <skos:prefLabel xml:lang="pt">Medidas e testes psicológicos</skos:prefLabel>
      <skos:definition xml:lang="pt">Avaliação de traços de personalidade ou respostas psicológicas/comportamentais por meio de medidas específicas e testes. Por exemplo, testes objetivos como medidas autorreportadas com um formato restrito de resposta, ou métodos projetivos que permitem respostas livres, incluindo associação de palavras, conclusão de frases ou histórias, vinhetas, teste de desenho animado, testes temáticos de percepção, dramatização, testes de desenho, testes de mancha de tinta, exercícios de ordenação de escolha, etc.</skos:definition>
      <skos:prefLabel xml:lang="sl">Meritve in testiranja psiholoških lastnosti</skos:prefLabel>
      <skos:definition xml:lang="sl">Ocena osebnostnih lastnosti ali psiholoških/vedenjskih odzivov s pomočjo posebnih meritev ali testov. Na primer objektivni testi, kot so samoporočanje z zaprtim formatom odgovorov ali projekcijske tehnike, ki omogočajo proste odgovore, vključno z besednimi asociacijami, dopolnjevanjem stavkov ali zgodb, vinjetami, testi s karikaturami, testi tematske apercepcije, igranjem vlog, testi risanja, testi pack, testi izbire itd.</skos:definition>
      <skos:prefLabel xml:lang="sr">Psihološko merenje i testiranje</skos:prefLabel>
      <skos:definition xml:lang="sr">Procena osobina ličnosti ili psiholoških / bihevioralnih odgovora pomoću specijalizovanih mera ili testova. Na primer, objektivni testovi kao što su mere samoizveštavanja sa ograničenim formatom odgovora ili projektivne metode koje omogućuju slobodne odgovore, uključujući povezivanje reči, dovršavanje rečenica ili priče, vinjete, test crteža, tematski testovi prikazivanja, igranje uloga, testovi crtanja, vežbe uređivanja izbora itd.</skos:definition>
      <skos:prefLabel xml:lang="sv">Psykologiska mätningar och tester</skos:prefLabel>
      <skos:definition xml:lang="sv">Bedömning av personlighetsdrag eller psykologiska/beteendemässiga responser genom specialiserade mätredskap eller tester. Exempel: objektiva tester som självskattning med begränsade svarsformat, eller projektiva tester som tillåter öppna svar, inklusive ordassociation, menings- eller berättelsekomplettering, vinjetter, "cartoon tests", tematiska apperceptionstester (TAT), rollspel, teckningstester, Rorschachtester, "choice ordering exercises" m.m.</skos:definition>
      <skos:broader rdf:resource="http://rdf-vocabulary.ddialliance.org/cv/ModeOfCollection/3.0/d64e4360"/>
   </rdf:Description>
   <rdf:Description rdf:about="http://rdf-vocabulary.ddialliance.org/cv/ModeOfCollection/3.0/d64e4727">
      <rdf:type rdf:resource="http://www.w3.org/2004/02/skos/core#Concept"/>
      <skos:inScheme rdf:resource="http://rdf-vocabulary.ddialliance.org/cv/ModeOfCollection/3.0"/>
      <skos:notation>Other</skos:notation>
      <skos:prefLabel xml:lang="en">Other</skos:prefLabel>
      <skos:definition xml:lang="en">Use if the mode of data collection is known, but not found in the list.</skos:definition>
      <skos:prefLabel xml:lang="da">Andet</skos:prefLabel>
      <skos:definition xml:lang="da">Anvend, hvis dataindsamlingsmåden er kendt, men ikke findes på listen.</skos:definition>
      <skos:prefLabel xml:lang="fi">Muu keruumenetelmä</skos:prefLabel>
      <skos:definition xml:lang="fi">Käytä mikäli keruumenetelmä on tiedossa, mutta ei sanastossa. Lisää tarkempi selostus.</skos:definition>
      <skos:prefLabel xml:lang="fr">Autre</skos:prefLabel>
      <skos:definition xml:lang="fr">Utilisez si le mode de collecte est connu, mais pas présent dans la liste.</skos:definition>
      <skos:prefLabel xml:lang="fr">Autre</skos:prefLabel>
      <skos:definition xml:lang="fr">Utilisez si le mode de collecte est connu, mais pas présent dans la liste.</skos:definition>
      <skos:prefLabel xml:lang="it">Altro</skos:prefLabel>
      <skos:definition xml:lang="it">Utilizzare quando la tecnica di raccolta dei dati è conosciuta, ma non è presente nell'elenco.</skos:definition>
      <skos:prefLabel xml:lang="no">Annet</skos:prefLabel>
      <skos:definition xml:lang="no">Bruk dersom metode for datainnsamling er kjent, men ikke finnes i listen.</skos:definition>
      <skos:prefLabel xml:lang="pt">Outro</skos:prefLabel>
      <skos:definition xml:lang="pt">Usar se o método de recolha de dados for conhecido, mas não se encontrar na lista.</skos:definition>
      <skos:prefLabel xml:lang="sl">Drugo</skos:prefLabel>
      <skos:definition xml:lang="sl">Uporabite, če je način zbiranja podatkov znan, vendar ga ni na tem seznamu.</skos:definition>
      <skos:prefLabel xml:lang="sr">Ostalo</skos:prefLabel>
      <skos:definition xml:lang="sr">Koristite ako je način prikupljanja podataka poznat, ali nije pronađen na ovoj listi.</skos:definition>
      <skos:prefLabel xml:lang="sv">Övrigt</skos:prefLabel>
      <skos:definition xml:lang="sv">Används när datainsamlingsmetoden är känd men saknas i listan.</skos:definition>
   </rdf:Description>
</rdf:RDF>
