<?xml version="1.0" encoding="UTF-8"?>
<rdf:RDF xmlns:rdf="http://www.w3.org/1999/02/22-rdf-syntax-ns#"
         xmlns:skos="http://www.w3.org/2004/02/skos/core#"
         xmlns:owl="http://www.w3.org/2002/07/owl#"
         xmlns:dcterms="http://purl.org/dc/terms/"
>
   <rdf:Description rdf:about="http://rdf-vocabulary.ddialliance.org/cv/TypeOfConceptGroup/1.0.0/">
      <rdf:type rdf:resource="http://www.w3.org/2004/02/skos/core#ConceptScheme"/>
      <dcterms:isVersionOf rdf:resource="http://rdf-vocabulary.ddialliance.org/cv/TypeOfConceptGroup/"/>
      <skos:notation xml:lang="en">TypeOfConceptGroup</skos:notation>
      <dcterms:title xml:lang="en">Type of Concept Group</dcterms:title>
      <dcterms:description xml:lang="en">Specifies the rationale for creating a concept group.</dcterms:description>
      <skos:prefLabel xml:lang="en">Type of Concept Group</skos:prefLabel>
      <dcterms:title xml:lang="no">Type konseptgruppe</dcterms:title>
      <dcterms:description xml:lang="no">Spesifiserer rasjonale for &#xe5; lage en konseptgruppe.</dcterms:description>
      <skos:prefLabel xml:lang="no">Type konseptgruppe</skos:prefLabel>
      <owl:versionInfo>1.0.0</owl:versionInfo>
      <dcterms:license rdf:resource="http://creativecommons.org/licenses/by/4.0/"/>
      <dcterms:rights>Copyright &#xa9;DDI Alliance 2020</dcterms:rights>
      <skos:hasTopConcept rdf:resource="http://rdf-vocabulary.ddialliance.org/cv/TypeOfConceptGroup/1.0.0/9ef1541"/>
      <skos:hasTopConcept rdf:resource="http://rdf-vocabulary.ddialliance.org/cv/TypeOfConceptGroup/1.0.0/39872cc"/>
      <skos:hasTopConcept rdf:resource="http://rdf-vocabulary.ddialliance.org/cv/TypeOfConceptGroup/1.0.0/6311ae1"/>
   </rdf:Description>
   <rdf:Description rdf:about="http://rdf-vocabulary.ddialliance.org/cv/TypeOfConceptGroup/1.0.0/9ef1541">
      <rdf:type rdf:resource="http://www.w3.org/2004/02/skos/core#Concept"/>
      <skos:inScheme rdf:resource="http://rdf-vocabulary.ddialliance.org/cv/TypeOfConceptGroup/1.0.0/"/>
      <skos:notation xml:lang="en">Administrative</skos:notation>
      <skos:prefLabel xml:lang="en">Administrative</skos:prefLabel>
      <skos:definition xml:lang="en">A concept group created for administrative purposes, for instance for subsetting or reorganizing data.</skos:definition>
      <skos:prefLabel xml:lang="no">Administrativ</skos:prefLabel>
      <skos:definition xml:lang="no">En konseptgruppe som lages for administrative form&#xe5;l, for eksempel for &#xe5; subsette eller reorganisere data.</skos:definition>
   </rdf:Description>
   <rdf:Description rdf:about="http://rdf-vocabulary.ddialliance.org/cv/TypeOfConceptGroup/1.0.0/39872cc">
      <rdf:type rdf:resource="http://www.w3.org/2004/02/skos/core#Concept"/>
      <skos:inScheme rdf:resource="http://rdf-vocabulary.ddialliance.org/cv/TypeOfConceptGroup/1.0.0/"/>
      <skos:notation xml:lang="en">Thematic</skos:notation>
      <skos:prefLabel xml:lang="en">Thematic</skos:prefLabel>
      <skos:definition xml:lang="en">A concept group created to bring together concepts reflecting the same general theme, or topic; for example, a group called &quot;Trust&quot; can include trust in institutions, trust in government, as well as interpersonal trust.</skos:definition>
      <skos:prefLabel xml:lang="no">Tematisk</skos:prefLabel>
      <skos:definition xml:lang="no">En konseptgruppe som lages for &#xe5; knytte sammen konsepter som gjenspeiler det samme generelle tema eller emne; for eksempel, en gruppe kalt &quot;Tillit&quot; kan inkludere tillit til institusjoner, tillit til styresmakter, s&#xe5; vel som mellommenneskelige tillit.</skos:definition>
   </rdf:Description>
   <rdf:Description rdf:about="http://rdf-vocabulary.ddialliance.org/cv/TypeOfConceptGroup/1.0.0/6311ae1">
      <rdf:type rdf:resource="http://www.w3.org/2004/02/skos/core#Concept"/>
      <skos:inScheme rdf:resource="http://rdf-vocabulary.ddialliance.org/cv/TypeOfConceptGroup/1.0.0/"/>
      <skos:notation xml:lang="en">Other</skos:notation>
      <skos:prefLabel xml:lang="en">Other</skos:prefLabel>
      <skos:definition xml:lang="en">Use when the type of concept group is known, but not found in the list.</skos:definition>
      <skos:prefLabel xml:lang="no">Annen</skos:prefLabel>
      <skos:definition xml:lang="no">Bruk n&#xe5;r typen konseptgruppe er kjent, men ikke finnes p&#xe5; listen.</skos:definition>
   </rdf:Description>
</rdf:RDF>
