<?xml version="1.0" encoding="UTF-8"?>
<rdf:RDF xmlns:dcterms="http://purl.org/dc/terms/"
          xmlns:owl="http://www.w3.org/2002/07/owl#"
          xmlns:rdf="http://www.w3.org/1999/02/22-rdf-syntax-ns#"
          xmlns:rdfs="http://www.w3.org/2000/01/rdf-schema#"
          xmlns:skos="http://www.w3.org/2004/02/skos/core#">
   <rdf:Description rdf:about="http://rdf-vocabulary.ddialliance.org/cv/TypeOfAddress/1.1.1/">
      <rdf:type rdf:resource="http://www.w3.org/2004/02/skos/core#ConceptScheme"/>
      <dcterms:isVersionOf rdf:resource="http://rdf-vocabulary.ddialliance.org/cv/TypeOfAddress"/>
      <skos:notation>TypeOfAddress</skos:notation>
      <skos:prefLabel xml:lang="en">Type of Address</skos:prefLabel>
      <skos:prefLabel xml:lang="en">Type of Address</skos:prefLabel>
      <skos:definition xml:lang="en">Identifies the type of address entered as contact information for an individual or an organization.
</skos:definition>
      <skos:definition xml:lang="en">Identifies the type of address entered as contact information for an individual or an organization.
</skos:definition>
      <owl:versionInfo>1.1.0</owl:versionInfo>
      <dcterms:license rdf:resource="Creative Commons Attribution 4.0 International"/>
      <dcterms:rights>Copyright Â©DDI Alliance 2020</dcterms:rights>
      <skos:hasTopConcept rdf:resource="http://rdf-vocabulary.ddialliance.org/cv/TypeOfAddress/1.1.1/d108e31"/>
      <skos:hasTopConcept rdf:resource="http://rdf-vocabulary.ddialliance.org/cv/TypeOfAddress/1.1.1/d108e81"/>
      <skos:hasTopConcept rdf:resource="http://rdf-vocabulary.ddialliance.org/cv/TypeOfAddress/1.1.1/d108e132"/>
   </rdf:Description>
   <rdf:Description rdf:about="http://rdf-vocabulary.ddialliance.org/cv/TypeOfAddress/1.1.1/d108e31">
      <rdf:type rdf:resource="http://www.w3.org/2004/02/skos/core#Concept"/>
      <skos:inScheme rdf:resource="http://rdf-vocabulary.ddialliance.org/cv/TypeOfAddress/1.1.1/"/>
      <skos:notation>Mailing</skos:notation>
      <skos:prefLabel xml:lang="en">Mailing address</skos:prefLabel>
      <skos:definition xml:lang="en">Includes both "street", and P.O. Box addresses used for sending and receiving physical/conventional mail through the postal system.</skos:definition>
      <skos:prefLabel xml:lang="en">Mailing address</skos:prefLabel>
      <skos:definition xml:lang="en">Includes both "street", and P.O. Box addresses used for sending and receiving physical/conventional mail through the postal system.</skos:definition>
      <skos:narrower rdf:resource="http://rdf-vocabulary.ddialliance.org/cv/TypeOfAddress/1.1.1/d108e51"/>
      <skos:narrower rdf:resource="http://rdf-vocabulary.ddialliance.org/cv/TypeOfAddress/1.1.1/d108e66"/>
   </rdf:Description>
   <rdf:Description rdf:about="http://rdf-vocabulary.ddialliance.org/cv/TypeOfAddress/1.1.1/d108e51">
      <rdf:type rdf:resource="http://www.w3.org/2004/02/skos/core#Concept"/>
      <skos:inScheme rdf:resource="http://rdf-vocabulary.ddialliance.org/cv/TypeOfAddress/1.1.1/"/>
      <skos:notation>Mailing.Residential</skos:notation>
      <skos:prefLabel xml:lang="en">Mailing address: Residential</skos:prefLabel>
      <skos:definition xml:lang="en">Address for directing physical/conventional mail to a person's residence, including institutional residence.</skos:definition>
      <skos:prefLabel xml:lang="en">Mailing address: Residential</skos:prefLabel>
      <skos:definition xml:lang="en">Address for directing physical/conventional mail to a person's residence, including institutional residence.</skos:definition>
      <skos:broader rdf:resource="http://rdf-vocabulary.ddialliance.org/cv/TypeOfAddress/1.1.1/d108e31"/>
   </rdf:Description>
   <rdf:Description rdf:about="http://rdf-vocabulary.ddialliance.org/cv/TypeOfAddress/1.1.1/d108e66">
      <rdf:type rdf:resource="http://www.w3.org/2004/02/skos/core#Concept"/>
      <skos:inScheme rdf:resource="http://rdf-vocabulary.ddialliance.org/cv/TypeOfAddress/1.1.1/"/>
      <skos:notation>Mailing.Nonresidential</skos:notation>
      <skos:prefLabel xml:lang="en">Mailing address: Nonresidential</skos:prefLabel>
      <skos:definition xml:lang="en">Address for directing physical/conventional mail to a business, organization, or other type of association.</skos:definition>
      <skos:prefLabel xml:lang="en">Mailing address: Nonresidential</skos:prefLabel>
      <skos:definition xml:lang="en">Address for directing physical/conventional mail to a business, organization, or other type of association.</skos:definition>
      <skos:broader rdf:resource="http://rdf-vocabulary.ddialliance.org/cv/TypeOfAddress/1.1.1/d108e31"/>
   </rdf:Description>
   <rdf:Description rdf:about="http://rdf-vocabulary.ddialliance.org/cv/TypeOfAddress/1.1.1/d108e81">
      <rdf:type rdf:resource="http://www.w3.org/2004/02/skos/core#Concept"/>
      <skos:inScheme rdf:resource="http://rdf-vocabulary.ddialliance.org/cv/TypeOfAddress/1.1.1/"/>
      <skos:notation>Visiting</skos:notation>
      <skos:prefLabel xml:lang="en">Visiting address</skos:prefLabel>
      <skos:definition xml:lang="en">Address used to identify a physical location (typically a building or a unit in a building) that may be accessed in person.</skos:definition>
      <skos:prefLabel xml:lang="en">Visiting address</skos:prefLabel>
      <skos:definition xml:lang="en">Address used to identify a physical location (typically a building or a unit in a building) that may be accessed in person.</skos:definition>
      <skos:narrower rdf:resource="http://rdf-vocabulary.ddialliance.org/cv/TypeOfAddress/1.1.1/d108e102"/>
      <skos:narrower rdf:resource="http://rdf-vocabulary.ddialliance.org/cv/TypeOfAddress/1.1.1/d108e117"/>
   </rdf:Description>
   <rdf:Description rdf:about="http://rdf-vocabulary.ddialliance.org/cv/TypeOfAddress/1.1.1/d108e102">
      <rdf:type rdf:resource="http://www.w3.org/2004/02/skos/core#Concept"/>
      <skos:inScheme rdf:resource="http://rdf-vocabulary.ddialliance.org/cv/TypeOfAddress/1.1.1/"/>
      <skos:notation>Visiting.Residential</skos:notation>
      <skos:prefLabel xml:lang="en">Visiting address: Residential</skos:prefLabel>
      <skos:definition xml:lang="en">Visiting address for a person's residence, including institutional residence.</skos:definition>
      <skos:prefLabel xml:lang="en">Visiting address: Residential</skos:prefLabel>
      <skos:definition xml:lang="en">Visiting address for a person's residence, including institutional residence.</skos:definition>
      <skos:broader rdf:resource="http://rdf-vocabulary.ddialliance.org/cv/TypeOfAddress/1.1.1/d108e81"/>
   </rdf:Description>
   <rdf:Description rdf:about="http://rdf-vocabulary.ddialliance.org/cv/TypeOfAddress/1.1.1/d108e117">
      <rdf:type rdf:resource="http://www.w3.org/2004/02/skos/core#Concept"/>
      <skos:inScheme rdf:resource="http://rdf-vocabulary.ddialliance.org/cv/TypeOfAddress/1.1.1/"/>
      <skos:notation>Visiting.Nonresidential</skos:notation>
      <skos:prefLabel xml:lang="en">Visiting address: Nonresidential</skos:prefLabel>
      <skos:definition xml:lang="en">Visiting address for a business, organization, or other type of association.</skos:definition>
      <skos:prefLabel xml:lang="en">Visiting address: Nonresidential</skos:prefLabel>
      <skos:definition xml:lang="en">Visiting address for a business, organization, or other type of association.</skos:definition>
      <skos:broader rdf:resource="http://rdf-vocabulary.ddialliance.org/cv/TypeOfAddress/1.1.1/d108e81"/>
   </rdf:Description>
   <rdf:Description rdf:about="http://rdf-vocabulary.ddialliance.org/cv/TypeOfAddress/1.1.1/d108e132">
      <rdf:type rdf:resource="http://www.w3.org/2004/02/skos/core#Concept"/>
      <skos:inScheme rdf:resource="http://rdf-vocabulary.ddialliance.org/cv/TypeOfAddress/1.1.1/"/>
      <skos:notation>Other</skos:notation>
      <skos:prefLabel xml:lang="en">Other</skos:prefLabel>
      <skos:definition xml:lang="en">Use if type of address is known, but not found in the list.</skos:definition>
      <skos:prefLabel xml:lang="en">Other</skos:prefLabel>
      <skos:definition xml:lang="en">Use if type of address is known, but not found in the list.</skos:definition>
   </rdf:Description>
</rdf:RDF>
