<?xml version="1.0" encoding="UTF-8"?>
<rdf:RDF xmlns:rdf="http://www.w3.org/1999/02/22-rdf-syntax-ns#"
         xmlns:skos="http://www.w3.org/2004/02/skos/core#"
         xmlns:owl="http://www.w3.org/2002/07/owl#"
         xmlns:dcterms="http://purl.org/dc/terms/"
>
   <rdf:Description rdf:about="http://rdf-vocabulary.ddialliance.org/cv/TypeOfNote/1.0.0/">
      <rdf:type rdf:resource="http://www.w3.org/2004/02/skos/core#ConceptScheme"/>
      <dcterms:isVersionOf rdf:resource="http://rdf-vocabulary.ddialliance.org/cv/TypeOfNote/"/>
      <skos:notation xml:lang="en">TypeOfNote</skos:notation>
      <dcterms:title xml:lang="en">Type of Note</dcterms:title>
      <dcterms:description xml:lang="en">Includes a typology of notes.</dcterms:description>
      <skos:prefLabel xml:lang="en">Type of Note</skos:prefLabel>
      <owl:versionInfo>1.0.0</owl:versionInfo>
      <dcterms:license rdf:resource="http://creativecommons.org/licenses/by/4.0/"/>
      <dcterms:rights>Copyright &#xa9;DDI Alliance 2020</dcterms:rights>
      <skos:hasTopConcept rdf:resource="http://rdf-vocabulary.ddialliance.org/cv/TypeOfNote/1.0.0/643562a"/>
      <skos:hasTopConcept rdf:resource="http://rdf-vocabulary.ddialliance.org/cv/TypeOfNote/1.0.0/efcfc2f"/>
      <skos:hasTopConcept rdf:resource="http://rdf-vocabulary.ddialliance.org/cv/TypeOfNote/1.0.0/a45da96"/>
      <skos:hasTopConcept rdf:resource="http://rdf-vocabulary.ddialliance.org/cv/TypeOfNote/1.0.0/c680d43"/>
      <skos:hasTopConcept rdf:resource="http://rdf-vocabulary.ddialliance.org/cv/TypeOfNote/1.0.0/0be8406"/>
      <skos:hasTopConcept rdf:resource="http://rdf-vocabulary.ddialliance.org/cv/TypeOfNote/1.0.0/6311ae1"/>
   </rdf:Description>
   <rdf:Description rdf:about="http://rdf-vocabulary.ddialliance.org/cv/TypeOfNote/1.0.0/643562a">
      <rdf:type rdf:resource="http://www.w3.org/2004/02/skos/core#Concept"/>
      <skos:inScheme rdf:resource="http://rdf-vocabulary.ddialliance.org/cv/TypeOfNote/1.0.0/"/>
      <skos:notation xml:lang="en">Processing</skos:notation>
      <skos:prefLabel xml:lang="en">Processing Note</skos:prefLabel>
      <skos:definition xml:lang="en">A note related to the processing of the data, or metadata, or both.</skos:definition>
   </rdf:Description>
   <rdf:Description rdf:about="http://rdf-vocabulary.ddialliance.org/cv/TypeOfNote/1.0.0/efcfc2f">
      <rdf:type rdf:resource="http://www.w3.org/2004/02/skos/core#Concept"/>
      <skos:inScheme rdf:resource="http://rdf-vocabulary.ddialliance.org/cv/TypeOfNote/1.0.0/"/>
      <skos:notation xml:lang="en">Addendum</skos:notation>
      <skos:prefLabel xml:lang="en">Addendum</skos:prefLabel>
      <skos:definition xml:lang="en">Additional information, usually of a factual nature (as opposed to a comment), intended to clarify the content of a DDI section or module.</skos:definition>
   </rdf:Description>
   <rdf:Description rdf:about="http://rdf-vocabulary.ddialliance.org/cv/TypeOfNote/1.0.0/a45da96">
      <rdf:type rdf:resource="http://www.w3.org/2004/02/skos/core#Concept"/>
      <skos:inScheme rdf:resource="http://rdf-vocabulary.ddialliance.org/cv/TypeOfNote/1.0.0/"/>
      <skos:notation xml:lang="en">System</skos:notation>
      <skos:prefLabel xml:lang="en">System Note</skos:prefLabel>
      <skos:definition xml:lang="en">A note generated by the processing system used to produce the data, or metadata, or both.</skos:definition>
   </rdf:Description>
   <rdf:Description rdf:about="http://rdf-vocabulary.ddialliance.org/cv/TypeOfNote/1.0.0/c680d43">
      <rdf:type rdf:resource="http://www.w3.org/2004/02/skos/core#Concept"/>
      <skos:inScheme rdf:resource="http://rdf-vocabulary.ddialliance.org/cv/TypeOfNote/1.0.0/"/>
      <skos:notation xml:lang="en">Observation</skos:notation>
      <skos:prefLabel xml:lang="en">Observation</skos:prefLabel>
      <skos:definition xml:lang="en">A note providing information on an aspect relevant for data usage that is likely to remain permanent, or a temporary note providing information for further review and correction. May be an observation entered by a human user or a system-generated note on any inconsistencies or deviations.</skos:definition>
   </rdf:Description>
   <rdf:Description rdf:about="http://rdf-vocabulary.ddialliance.org/cv/TypeOfNote/1.0.0/0be8406">
      <rdf:type rdf:resource="http://www.w3.org/2004/02/skos/core#Concept"/>
      <skos:inScheme rdf:resource="http://rdf-vocabulary.ddialliance.org/cv/TypeOfNote/1.0.0/"/>
      <skos:notation xml:lang="en">Comment</skos:notation>
      <skos:prefLabel xml:lang="en">Comment</skos:prefLabel>
      <skos:definition xml:lang="en">A human-readable comment, typically of a more subjective nature than an addendum.</skos:definition>
   </rdf:Description>
   <rdf:Description rdf:about="http://rdf-vocabulary.ddialliance.org/cv/TypeOfNote/1.0.0/6311ae1">
      <rdf:type rdf:resource="http://www.w3.org/2004/02/skos/core#Concept"/>
      <skos:inScheme rdf:resource="http://rdf-vocabulary.ddialliance.org/cv/TypeOfNote/1.0.0/"/>
      <skos:notation xml:lang="en">Other</skos:notation>
      <skos:prefLabel xml:lang="en">Other</skos:prefLabel>
      <skos:definition xml:lang="en">Use when the type of note is known, but not found in the list.</skos:definition>
   </rdf:Description>
</rdf:RDF>
