<?xml version="1.0" encoding="UTF-8"?>
<rdf:RDF xmlns:dcterms="http://purl.org/dc/terms/"
          xmlns:owl="http://www.w3.org/2002/07/owl#"
          xmlns:rdf="http://www.w3.org/1999/02/22-rdf-syntax-ns#"
          xmlns:rdfs="http://www.w3.org/2000/01/rdf-schema#"
          xmlns:skos="http://www.w3.org/2004/02/skos/core#">
   <rdf:Description rdf:about="http://rdf-vocabulary.ddialliance.org/cv/LifecycleEventType/1.0">
      <rdf:type rdf:resource="http://www.w3.org/2004/02/skos/core#ConceptScheme"/>
      <dcterms:isVersionOf rdf:resource="http://rdf-vocabulary.ddialliance.org/cv/LifecycleEventType"/>
      <skos:notation>LifecycleEventType</skos:notation>
      <skos:prefLabel xml:lang="en">Lifecycle Event Type</skos:prefLabel>
      <skos:prefLabel xml:lang="no">Livssyklus hendelsestype</skos:prefLabel>
      <skos:definition xml:lang="en">Specifies the event happening over the data life cycle that is considered significant enough to document.</skos:definition>
      <skos:definition xml:lang="no">Spesifiserer hendelser som skjer i data livssyklusen som anses som signifikante nok til å bli dokumentert.</skos:definition>
      <owl:versionInfo>1.0</owl:versionInfo>
      <dcterms:license rdf:resource="Creative Commons Attribution 4.0 International"/>
      <dcterms:rights>Copyright ©DDI Alliance 2020</dcterms:rights>
      <skos:hasTopConcept rdf:resource="http://rdf-vocabulary.ddialliance.org/cv/LifecycleEventType/1.0/d80e92"/>
      <skos:hasTopConcept rdf:resource="http://rdf-vocabulary.ddialliance.org/cv/LifecycleEventType/1.0/d80e114"/>
      <skos:hasTopConcept rdf:resource="http://rdf-vocabulary.ddialliance.org/cv/LifecycleEventType/1.0/d80e136"/>
      <skos:hasTopConcept rdf:resource="http://rdf-vocabulary.ddialliance.org/cv/LifecycleEventType/1.0/d80e158"/>
      <skos:hasTopConcept rdf:resource="http://rdf-vocabulary.ddialliance.org/cv/LifecycleEventType/1.0/d80e181"/>
      <skos:hasTopConcept rdf:resource="http://rdf-vocabulary.ddialliance.org/cv/LifecycleEventType/1.0/d80e203"/>
      <skos:hasTopConcept rdf:resource="http://rdf-vocabulary.ddialliance.org/cv/LifecycleEventType/1.0/d80e225"/>
      <skos:hasTopConcept rdf:resource="http://rdf-vocabulary.ddialliance.org/cv/LifecycleEventType/1.0/d80e247"/>
      <skos:hasTopConcept rdf:resource="http://rdf-vocabulary.ddialliance.org/cv/LifecycleEventType/1.0/d80e269"/>
      <skos:hasTopConcept rdf:resource="http://rdf-vocabulary.ddialliance.org/cv/LifecycleEventType/1.0/d80e291"/>
      <skos:hasTopConcept rdf:resource="http://rdf-vocabulary.ddialliance.org/cv/LifecycleEventType/1.0/d80e314"/>
      <skos:hasTopConcept rdf:resource="http://rdf-vocabulary.ddialliance.org/cv/LifecycleEventType/1.0/d80e336"/>
      <skos:hasTopConcept rdf:resource="http://rdf-vocabulary.ddialliance.org/cv/LifecycleEventType/1.0/d80e358"/>
      <skos:hasTopConcept rdf:resource="http://rdf-vocabulary.ddialliance.org/cv/LifecycleEventType/1.0/d80e380"/>
      <skos:hasTopConcept rdf:resource="http://rdf-vocabulary.ddialliance.org/cv/LifecycleEventType/1.0/d80e402"/>
      <skos:hasTopConcept rdf:resource="http://rdf-vocabulary.ddialliance.org/cv/LifecycleEventType/1.0/d80e692"/>
      <skos:hasTopConcept rdf:resource="http://rdf-vocabulary.ddialliance.org/cv/LifecycleEventType/1.0/d80e714"/>
      <skos:hasTopConcept rdf:resource="http://rdf-vocabulary.ddialliance.org/cv/LifecycleEventType/1.0/d80e737"/>
      <skos:hasTopConcept rdf:resource="http://rdf-vocabulary.ddialliance.org/cv/LifecycleEventType/1.0/d80e759"/>
      <skos:hasTopConcept rdf:resource="http://rdf-vocabulary.ddialliance.org/cv/LifecycleEventType/1.0/d80e781"/>
      <skos:hasTopConcept rdf:resource="http://rdf-vocabulary.ddialliance.org/cv/LifecycleEventType/1.0/d80e803"/>
      <skos:hasTopConcept rdf:resource="http://rdf-vocabulary.ddialliance.org/cv/LifecycleEventType/1.0/d80e825"/>
      <skos:hasTopConcept rdf:resource="http://rdf-vocabulary.ddialliance.org/cv/LifecycleEventType/1.0/d80e847"/>
      <skos:hasTopConcept rdf:resource="http://rdf-vocabulary.ddialliance.org/cv/LifecycleEventType/1.0/d80e870"/>
      <skos:hasTopConcept rdf:resource="http://rdf-vocabulary.ddialliance.org/cv/LifecycleEventType/1.0/d80e892"/>
      <skos:hasTopConcept rdf:resource="http://rdf-vocabulary.ddialliance.org/cv/LifecycleEventType/1.0/d80e914"/>
      <skos:hasTopConcept rdf:resource="http://rdf-vocabulary.ddialliance.org/cv/LifecycleEventType/1.0/d80e936"/>
      <skos:hasTopConcept rdf:resource="http://rdf-vocabulary.ddialliance.org/cv/LifecycleEventType/1.0/d80e958"/>
   </rdf:Description>
   <rdf:Description rdf:about="http://rdf-vocabulary.ddialliance.org/cv/LifecycleEventType/1.0/d80e92">
      <rdf:type rdf:resource="http://www.w3.org/2004/02/skos/core#Concept"/>
      <skos:inScheme rdf:resource="http://rdf-vocabulary.ddialliance.org/cv/LifecycleEventType/1.0"/>
      <skos:notation>StudyProposal</skos:notation>
      <skos:prefLabel xml:lang="en">Study proposal</skos:prefLabel>
      <skos:definition xml:lang="en">Defining outlines for a new study/data collection, including needs for information and general  research  objectives, as well  as main concepts, study scope and methodology, usually to be presented for approval to funders, partners, or other relevant bodies.</skos:definition>
      <skos:prefLabel xml:lang="no">Studieforslag</skos:prefLabel>
      <skos:definition xml:lang="no">Definere rammene for en ny studie/datainnsamling, inkluderer behovet for informasjon og de generelle forskningsmålene, samt hovedkonsepter, studieomfang og metodologi, som regel presenteres dette for godkjenning hos finansiere, partnere og andre relevante aktører.</skos:definition>
   </rdf:Description>
   <rdf:Description rdf:about="http://rdf-vocabulary.ddialliance.org/cv/LifecycleEventType/1.0/d80e114">
      <rdf:type rdf:resource="http://www.w3.org/2004/02/skos/core#Concept"/>
      <skos:inScheme rdf:resource="http://rdf-vocabulary.ddialliance.org/cv/LifecycleEventType/1.0"/>
      <skos:notation>Funding</skos:notation>
      <skos:prefLabel xml:lang="en">Funding</skos:prefLabel>
      <skos:definition xml:lang="en">Decisions to extend financial support for the study/data collection.</skos:definition>
      <skos:prefLabel xml:lang="no">Finansiering</skos:prefLabel>
      <skos:definition xml:lang="no">Avgjørelser om å forlenge finansiell støtte for en studie/datainnsamling.</skos:definition>
   </rdf:Description>
   <rdf:Description rdf:about="http://rdf-vocabulary.ddialliance.org/cv/LifecycleEventType/1.0/d80e136">
      <rdf:type rdf:resource="http://www.w3.org/2004/02/skos/core#Concept"/>
      <skos:inScheme rdf:resource="http://rdf-vocabulary.ddialliance.org/cv/LifecycleEventType/1.0"/>
      <skos:notation>StudyDesign</skos:notation>
      <skos:prefLabel xml:lang="en">Study design</skos:prefLabel>
      <skos:definition xml:lang="en">Detailed planning for carrying out the study/data collection: refining concepts and identifying ways to measure them, defining the target population, time dimension, sampling frame and sample selection, data collection methodology, production systems and workflows, etc.</skos:definition>
      <skos:prefLabel xml:lang="no">Studie design</skos:prefLabel>
      <skos:definition xml:lang="no">Detaljert planlegging for å gjennomføre studien/datainnsamlingen: raffinere konsepter og identifisere måter å måle de, definere mål populasjonen, tidsdimensjonen, utvalgsrammeverket og utvalgstrekning, datainnsamlings metodologi, produksjonssystemer og arbeidsflyt, etc.</skos:definition>
   </rdf:Description>
   <rdf:Description rdf:about="http://rdf-vocabulary.ddialliance.org/cv/LifecycleEventType/1.0/d80e158">
      <rdf:type rdf:resource="http://www.w3.org/2004/02/skos/core#Concept"/>
      <skos:inScheme rdf:resource="http://rdf-vocabulary.ddialliance.org/cv/LifecycleEventType/1.0"/>
      <skos:notation>InstrumentDesign</skos:notation>
      <skos:prefLabel xml:lang="en">Instrument design</skos:prefLabel>
      <skos:definition xml:lang="en">Building the data collection instrument, for example, the questionnaire or interview questions, focus group topics, observation forms for an observational design, standardized record review, independent and dependent variables for an experimental design, etc.</skos:definition>
      <skos:prefLabel xml:lang="no">Instrumentdesign</skos:prefLabel>
      <skos:definition xml:lang="no">Utvikle datainnsamlingsinstrumentet, for eksempel, spørreskjemaet eller intervjuspørsmålene, fokusgruppe emner, observasjonsskjema for observasjonsdesign, standardisert journalgjennomgang, uavhengig og avhengig variabler for eksperimentelt design.</skos:definition>
   </rdf:Description>
   <rdf:Description rdf:about="http://rdf-vocabulary.ddialliance.org/cv/LifecycleEventType/1.0/d80e181">
      <rdf:type rdf:resource="http://www.w3.org/2004/02/skos/core#Concept"/>
      <skos:inScheme rdf:resource="http://rdf-vocabulary.ddialliance.org/cv/LifecycleEventType/1.0"/>
      <skos:notation>QuestionnaireTranslation</skos:notation>
      <skos:prefLabel xml:lang="en">Questionnaire translation</skos:prefLabel>
      <skos:definition xml:lang="en">Translating the source questionnaire into other languages, for example, in cross-national surveys or in national surveys conducted in multilingual countries.</skos:definition>
      <skos:prefLabel xml:lang="no">Spørreskjema oversettelse</skos:prefLabel>
      <skos:definition xml:lang="no">Oversette kildespørreskjemaet til andre språk, for eksempel, i tverrnasjonale spørreskjema eller i nasjonale spørreskjema gjennomført i flerspråklige land.</skos:definition>
   </rdf:Description>
   <rdf:Description rdf:about="http://rdf-vocabulary.ddialliance.org/cv/LifecycleEventType/1.0/d80e203">
      <rdf:type rdf:resource="http://www.w3.org/2004/02/skos/core#Concept"/>
      <skos:inScheme rdf:resource="http://rdf-vocabulary.ddialliance.org/cv/LifecycleEventType/1.0"/>
      <skos:notation>QuestionnaireAdaptation</skos:notation>
      <skos:prefLabel xml:lang="en">Questionnaire adaptation</skos:prefLabel>
      <skos:definition xml:lang="en">Changing the wording of questions to reflect cultural or institutional differences if same-language questionnaires are administered in different regions or countries.</skos:definition>
      <skos:prefLabel xml:lang="no">Spørreskjema tilpasning</skos:prefLabel>
      <skos:definition xml:lang="no">Endring av språkformulering i spørsmål for å belyse kulturelle eller institusjonelle forskjeller, hvis spørreskjema i samme språk utføres i forskjellige regioner eller land.</skos:definition>
   </rdf:Description>
   <rdf:Description rdf:about="http://rdf-vocabulary.ddialliance.org/cv/LifecycleEventType/1.0/d80e225">
      <rdf:type rdf:resource="http://www.w3.org/2004/02/skos/core#Concept"/>
      <skos:inScheme rdf:resource="http://rdf-vocabulary.ddialliance.org/cv/LifecycleEventType/1.0"/>
      <skos:notation>InterviewerTraining</skos:notation>
      <skos:prefLabel xml:lang="en">Interviewer training</skos:prefLabel>
      <skos:definition xml:lang="en">Training the interviewers that administer questionnaires in survey-type studies.</skos:definition>
      <skos:prefLabel xml:lang="no">Intervjueropplæring</skos:prefLabel>
      <skos:definition xml:lang="no">Opplæring av intervjuere som administrerer spørreskjemaet i spørreskjemaundersøkelser.</skos:definition>
   </rdf:Description>
   <rdf:Description rdf:about="http://rdf-vocabulary.ddialliance.org/cv/LifecycleEventType/1.0/d80e247">
      <rdf:type rdf:resource="http://www.w3.org/2004/02/skos/core#Concept"/>
      <skos:inScheme rdf:resource="http://rdf-vocabulary.ddialliance.org/cv/LifecycleEventType/1.0"/>
      <skos:notation>EthicsReview</skos:notation>
      <skos:prefLabel xml:lang="en">Ethics review</skos:prefLabel>
      <skos:definition xml:lang="en">Review of the study/data collection to ensure that it complies with statutory ethics requirements or regulations, including verification of the informed consent statement, performed by a qualified body, like a Research Ethics Committee, or Institutional Review Board.</skos:definition>
      <skos:prefLabel xml:lang="no">Etisk godkjenning</skos:prefLabel>
      <skos:definition xml:lang="no">Gjennomgang av studien/datainnsamlingen for å forsikre at den samsvarer med lovpålagte etiske krav eller forskrifter, inkludert verifisering av informert samtykke, gjennomført av et godkjent organ, som en forskningsetisk komité eller institusjonell vurderingsnemd.</skos:definition>
   </rdf:Description>
   <rdf:Description rdf:about="http://rdf-vocabulary.ddialliance.org/cv/LifecycleEventType/1.0/d80e269">
      <rdf:type rdf:resource="http://www.w3.org/2004/02/skos/core#Concept"/>
      <skos:inScheme rdf:resource="http://rdf-vocabulary.ddialliance.org/cv/LifecycleEventType/1.0"/>
      <skos:notation>LegalReview</skos:notation>
      <skos:prefLabel xml:lang="en">Legal review</skos:prefLabel>
      <skos:definition xml:lang="en">Review of the study/data collection in terms of compliance with the law  (legislation concerning confidentiality, the protection of children, etc.).</skos:definition>
      <skos:prefLabel xml:lang="no">Lovlig godkjenning</skos:prefLabel>
      <skos:definition xml:lang="no">Gjennomgang av studien/datainnsamling i forhold til samsvar med loven (lovgivning som omhandler konfidensialitet, beskyttelse av barn, etc.).</skos:definition>
   </rdf:Description>
   <rdf:Description rdf:about="http://rdf-vocabulary.ddialliance.org/cv/LifecycleEventType/1.0/d80e291">
      <rdf:type rdf:resource="http://www.w3.org/2004/02/skos/core#Concept"/>
      <skos:inScheme rdf:resource="http://rdf-vocabulary.ddialliance.org/cv/LifecycleEventType/1.0"/>
      <skos:notation>Sampling</skos:notation>
      <skos:prefLabel xml:lang="en">Sampling</skos:prefLabel>
      <skos:definition xml:lang="en">Selecting the sample for the study/data collection.</skos:definition>
      <skos:prefLabel xml:lang="no">Utvalgstrekking</skos:prefLabel>
      <skos:definition xml:lang="no">Velge utvalget for studien/datainnsamlingen.</skos:definition>
   </rdf:Description>
   <rdf:Description rdf:about="http://rdf-vocabulary.ddialliance.org/cv/LifecycleEventType/1.0/d80e314">
      <rdf:type rdf:resource="http://www.w3.org/2004/02/skos/core#Concept"/>
      <skos:inScheme rdf:resource="http://rdf-vocabulary.ddialliance.org/cv/LifecycleEventType/1.0"/>
      <skos:notation>InstrumentPreTesting</skos:notation>
      <skos:prefLabel xml:lang="en">Instrument pre-testing</skos:prefLabel>
      <skos:definition xml:lang="en">Small-scale application of the data collection instrument designed to identify potential problems before using it for the entire study.</skos:definition>
      <skos:prefLabel xml:lang="no">Instrumenttest</skos:prefLabel>
      <skos:definition xml:lang="no">Småskala anvendelse av datainnsamling instrumentet med hensikt å identifisere potensielle problemer før en tar det i bruk i fullskala for hele studien.</skos:definition>
   </rdf:Description>
   <rdf:Description rdf:about="http://rdf-vocabulary.ddialliance.org/cv/LifecycleEventType/1.0/d80e336">
      <rdf:type rdf:resource="http://www.w3.org/2004/02/skos/core#Concept"/>
      <skos:inScheme rdf:resource="http://rdf-vocabulary.ddialliance.org/cv/LifecycleEventType/1.0"/>
      <skos:notation>PilotStudy</skos:notation>
      <skos:prefLabel xml:lang="en">Pilot study</skos:prefLabel>
      <skos:definition xml:lang="en">Dress rehearsal of the full project, for example, by administering the questionnaire to a small number of people, then coding and analyzing results, etc.</skos:definition>
      <skos:prefLabel xml:lang="no">Pilotstudie</skos:prefLabel>
      <skos:definition xml:lang="no">Generalprøve for hele prosjektet, for eksempel ved å gjennomføre datainnsamling via spørreskjema til et lite antall mennesker, så kode og analysere resultatene, etc.</skos:definition>
   </rdf:Description>
   <rdf:Description rdf:about="http://rdf-vocabulary.ddialliance.org/cv/LifecycleEventType/1.0/d80e358">
      <rdf:type rdf:resource="http://www.w3.org/2004/02/skos/core#Concept"/>
      <skos:inScheme rdf:resource="http://rdf-vocabulary.ddialliance.org/cv/LifecycleEventType/1.0"/>
      <skos:notation>DataCollection</skos:notation>
      <skos:prefLabel xml:lang="en">Data collection</skos:prefLabel>
      <skos:definition xml:lang="en">Setting up, running and finalizing the data collection process, including follow-up procedures, etc.</skos:definition>
      <skos:prefLabel xml:lang="no">Datainnsamling</skos:prefLabel>
      <skos:definition xml:lang="no">Klargjøre, gjennomføre og ferdigstille datainnsamling prosessen, inkludert oppfølging prosedyrer, etc.</skos:definition>
   </rdf:Description>
   <rdf:Description rdf:about="http://rdf-vocabulary.ddialliance.org/cv/LifecycleEventType/1.0/d80e380">
      <rdf:type rdf:resource="http://www.w3.org/2004/02/skos/core#Concept"/>
      <skos:inScheme rdf:resource="http://rdf-vocabulary.ddialliance.org/cv/LifecycleEventType/1.0"/>
      <skos:notation>DataCollectionReports</skos:notation>
      <skos:prefLabel xml:lang="en">Data collection reports</skos:prefLabel>
      <skos:definition xml:lang="en">Reports on designing and conducting the data collection process, including methodological decisions and problems encountered. These may take the form of conference posters or presentations, journal articles or online publications, book chapters, etc.</skos:definition>
      <skos:prefLabel xml:lang="no">Datainnsamling rapporter</skos:prefLabel>
      <skos:definition xml:lang="no">Rapporter på designet og gjennomførelsen av datainnsamling prosessen, inkludert metodologiske avgjørelser og utfordringer som har oppstått. Disse kan være konferansepresentasjoner, tidsskriftartikler eller online publikasjoner, bokkapitler, etc.</skos:definition>
   </rdf:Description>
   <rdf:Description rdf:about="http://rdf-vocabulary.ddialliance.org/cv/LifecycleEventType/1.0/d80e402">
      <rdf:type rdf:resource="http://www.w3.org/2004/02/skos/core#Concept"/>
      <skos:inScheme rdf:resource="http://rdf-vocabulary.ddialliance.org/cv/LifecycleEventType/1.0"/>
      <skos:notation>DataProcessing</skos:notation>
      <skos:prefLabel xml:lang="en">Data processing</skos:prefLabel>
      <skos:definition xml:lang="en">Changes, additions or deletions brought to the data at any point in time after collection.</skos:definition>
      <skos:prefLabel xml:lang="no">Databehandling</skos:prefLabel>
      <skos:definition xml:lang="no">Endringer, tillegg eller sletting gjennomført på data på hvilket som helst tidspunkt etter innsamlingen.</skos:definition>
      <skos:narrower rdf:resource="http://rdf-vocabulary.ddialliance.org/cv/LifecycleEventType/1.0/d80e448"/>
      <skos:narrower rdf:resource="http://rdf-vocabulary.ddialliance.org/cv/LifecycleEventType/1.0/d80e471"/>
      <skos:narrower rdf:resource="http://rdf-vocabulary.ddialliance.org/cv/LifecycleEventType/1.0/d80e493"/>
      <skos:narrower rdf:resource="http://rdf-vocabulary.ddialliance.org/cv/LifecycleEventType/1.0/d80e515"/>
      <skos:narrower rdf:resource="http://rdf-vocabulary.ddialliance.org/cv/LifecycleEventType/1.0/d80e537"/>
      <skos:narrower rdf:resource="http://rdf-vocabulary.ddialliance.org/cv/LifecycleEventType/1.0/d80e559"/>
      <skos:narrower rdf:resource="http://rdf-vocabulary.ddialliance.org/cv/LifecycleEventType/1.0/d80e581"/>
      <skos:narrower rdf:resource="http://rdf-vocabulary.ddialliance.org/cv/LifecycleEventType/1.0/d80e604"/>
      <skos:narrower rdf:resource="http://rdf-vocabulary.ddialliance.org/cv/LifecycleEventType/1.0/d80e626"/>
      <skos:narrower rdf:resource="http://rdf-vocabulary.ddialliance.org/cv/LifecycleEventType/1.0/d80e648"/>
      <skos:narrower rdf:resource="http://rdf-vocabulary.ddialliance.org/cv/LifecycleEventType/1.0/d80e670"/>
   </rdf:Description>
   <rdf:Description rdf:about="http://rdf-vocabulary.ddialliance.org/cv/LifecycleEventType/1.0/d80e448">
      <rdf:type rdf:resource="http://www.w3.org/2004/02/skos/core#Concept"/>
      <skos:inScheme rdf:resource="http://rdf-vocabulary.ddialliance.org/cv/LifecycleEventType/1.0"/>
      <skos:notation>DataProcessing.Coding</skos:notation>
      <skos:prefLabel xml:lang="en">Data processing: Coding</skos:prefLabel>
      <skos:definition xml:lang="en">Converting raw data into machine-readable codes.</skos:definition>
      <skos:prefLabel xml:lang="no">Databehandling: Koding</skos:prefLabel>
      <skos:definition xml:lang="no">Konvertering av rådata til maskinlesbare koder.</skos:definition>
      <skos:broader rdf:resource="http://rdf-vocabulary.ddialliance.org/cv/LifecycleEventType/1.0/d80e402"/>
   </rdf:Description>
   <rdf:Description rdf:about="http://rdf-vocabulary.ddialliance.org/cv/LifecycleEventType/1.0/d80e471">
      <rdf:type rdf:resource="http://www.w3.org/2004/02/skos/core#Concept"/>
      <skos:inScheme rdf:resource="http://rdf-vocabulary.ddialliance.org/cv/LifecycleEventType/1.0"/>
      <skos:notation>DataProcessing.Classification</skos:notation>
      <skos:prefLabel xml:lang="en">Data processing: Classification</skos:prefLabel>
      <skos:definition xml:lang="en">Documenting the meaning/substance of coded data.</skos:definition>
      <skos:prefLabel xml:lang="no">Databehandling: Klassifisering</skos:prefLabel>
      <skos:definition xml:lang="no">Dokumentering av meningen/innholdet av kodede data.</skos:definition>
      <skos:broader rdf:resource="http://rdf-vocabulary.ddialliance.org/cv/LifecycleEventType/1.0/d80e402"/>
   </rdf:Description>
   <rdf:Description rdf:about="http://rdf-vocabulary.ddialliance.org/cv/LifecycleEventType/1.0/d80e493">
      <rdf:type rdf:resource="http://www.w3.org/2004/02/skos/core#Concept"/>
      <skos:inScheme rdf:resource="http://rdf-vocabulary.ddialliance.org/cv/LifecycleEventType/1.0"/>
      <skos:notation>DataProcessing.InterviewTranscriptions</skos:notation>
      <skos:prefLabel xml:lang="en">Data processing: Transcriptions of interviews</skos:prefLabel>
      <skos:definition xml:lang="en">Transferring video- or audio-taped data into written form.</skos:definition>
      <skos:prefLabel xml:lang="no">Databehandling: Transkibering av intervjuer</skos:prefLabel>
      <skos:definition xml:lang="no">Overføring av video- eller lydopptak data til skriftlig format.</skos:definition>
      <skos:broader rdf:resource="http://rdf-vocabulary.ddialliance.org/cv/LifecycleEventType/1.0/d80e402"/>
   </rdf:Description>
   <rdf:Description rdf:about="http://rdf-vocabulary.ddialliance.org/cv/LifecycleEventType/1.0/d80e515">
      <rdf:type rdf:resource="http://www.w3.org/2004/02/skos/core#Concept"/>
      <skos:inScheme rdf:resource="http://rdf-vocabulary.ddialliance.org/cv/LifecycleEventType/1.0"/>
      <skos:notation>DataProcessing.Weighting</skos:notation>
      <skos:prefLabel xml:lang="en">Data processing: Weighting</skos:prefLabel>
      <skos:definition xml:lang="en">Calculating weight variables and adding them to the data.</skos:definition>
      <skos:prefLabel xml:lang="no">Databehandling: Vekting</skos:prefLabel>
      <skos:definition xml:lang="no">Utregning av vektevariabler og legge de til datamaterialet.</skos:definition>
      <skos:broader rdf:resource="http://rdf-vocabulary.ddialliance.org/cv/LifecycleEventType/1.0/d80e402"/>
   </rdf:Description>
   <rdf:Description rdf:about="http://rdf-vocabulary.ddialliance.org/cv/LifecycleEventType/1.0/d80e537">
      <rdf:type rdf:resource="http://www.w3.org/2004/02/skos/core#Concept"/>
      <skos:inScheme rdf:resource="http://rdf-vocabulary.ddialliance.org/cv/LifecycleEventType/1.0"/>
      <skos:notation>DataProcessing.Aggregation</skos:notation>
      <skos:prefLabel xml:lang="en">Data processing: Aggregation</skos:prefLabel>
      <skos:definition xml:lang="en">Calculating cumulative measures of individual-level data or microdata.</skos:definition>
      <skos:prefLabel xml:lang="no">Databehandling: Aggregering</skos:prefLabel>
      <skos:definition xml:lang="no">Utregning av kumulative mål på individnivå data eller mikrodata.</skos:definition>
      <skos:broader rdf:resource="http://rdf-vocabulary.ddialliance.org/cv/LifecycleEventType/1.0/d80e402"/>
   </rdf:Description>
   <rdf:Description rdf:about="http://rdf-vocabulary.ddialliance.org/cv/LifecycleEventType/1.0/d80e559">
      <rdf:type rdf:resource="http://www.w3.org/2004/02/skos/core#Concept"/>
      <skos:inScheme rdf:resource="http://rdf-vocabulary.ddialliance.org/cv/LifecycleEventType/1.0"/>
      <skos:notation>DataProcessing.CompositeMeasures</skos:notation>
      <skos:prefLabel xml:lang="en">Data processing: Composite measures</skos:prefLabel>
      <skos:definition xml:lang="en">Calculating scales, indexes, or typologies and adding them to the data.</skos:definition>
      <skos:prefLabel xml:lang="no">Databehandling: Sammensatte mål</skos:prefLabel>
      <skos:definition xml:lang="no">Utregning av skalaer, indekser eller typologier og legge de til datamaterialet.</skos:definition>
      <skos:broader rdf:resource="http://rdf-vocabulary.ddialliance.org/cv/LifecycleEventType/1.0/d80e402"/>
   </rdf:Description>
   <rdf:Description rdf:about="http://rdf-vocabulary.ddialliance.org/cv/LifecycleEventType/1.0/d80e581">
      <rdf:type rdf:resource="http://www.w3.org/2004/02/skos/core#Concept"/>
      <skos:inScheme rdf:resource="http://rdf-vocabulary.ddialliance.org/cv/LifecycleEventType/1.0"/>
      <skos:notation>DataProcessing.Derivation</skos:notation>
      <skos:prefLabel xml:lang="en">Data processing: Derivation</skos:prefLabel>
      <skos:definition xml:lang="en">Calculating new variables from measured variables, usually by recodes.</skos:definition>
      <skos:prefLabel xml:lang="no">Databehandling: Avledning</skos:prefLabel>
      <skos:definition xml:lang="no">Utregning av nye variabler fra målte variabler, som regel gjennom rekoding.</skos:definition>
      <skos:broader rdf:resource="http://rdf-vocabulary.ddialliance.org/cv/LifecycleEventType/1.0/d80e402"/>
   </rdf:Description>
   <rdf:Description rdf:about="http://rdf-vocabulary.ddialliance.org/cv/LifecycleEventType/1.0/d80e604">
      <rdf:type rdf:resource="http://www.w3.org/2004/02/skos/core#Concept"/>
      <skos:inScheme rdf:resource="http://rdf-vocabulary.ddialliance.org/cv/LifecycleEventType/1.0"/>
      <skos:notation>DataProcessing.DataQualityChecks</skos:notation>
      <skos:prefLabel xml:lang="en">Data processing: Quality checks</skos:prefLabel>
      <skos:definition xml:lang="en">Checks for consistency, undocumented codes, missing data representation, etc.</skos:definition>
      <skos:prefLabel xml:lang="no">Databehandling: Kvalitetskontroll</skos:prefLabel>
      <skos:definition xml:lang="no">Kontrollere overensstemmelser, udokumenterte koder, missing data representasjoner, etc.</skos:definition>
      <skos:broader rdf:resource="http://rdf-vocabulary.ddialliance.org/cv/LifecycleEventType/1.0/d80e402"/>
   </rdf:Description>
   <rdf:Description rdf:about="http://rdf-vocabulary.ddialliance.org/cv/LifecycleEventType/1.0/d80e626">
      <rdf:type rdf:resource="http://www.w3.org/2004/02/skos/core#Concept"/>
      <skos:inScheme rdf:resource="http://rdf-vocabulary.ddialliance.org/cv/LifecycleEventType/1.0"/>
      <skos:notation>DataProcessing.DataIntegration</skos:notation>
      <skos:prefLabel xml:lang="en">Data processing: Data integration</skos:prefLabel>
      <skos:definition xml:lang="en">Creating complex datasets by merging related data, for example, hierarchical datasets with multiple but related  analysis units, or multiple-wave datasets, or data collected in different countries for a cross-national study, etc.</skos:definition>
      <skos:prefLabel xml:lang="no">Databehandling: Dataintegrering</skos:prefLabel>
      <skos:definition xml:lang="no">Opprette komplekse datasett med å koble sammen relaterte data, for eksempel, hierarkiske datasett med flere, men sammenliknbare, analyseenheter, eller datasett fra flere runder av en undersøkelse, eller data samlet inn i forskjellige land for en tverrnasjonal studie, etc.</skos:definition>
      <skos:broader rdf:resource="http://rdf-vocabulary.ddialliance.org/cv/LifecycleEventType/1.0/d80e402"/>
   </rdf:Description>
   <rdf:Description rdf:about="http://rdf-vocabulary.ddialliance.org/cv/LifecycleEventType/1.0/d80e648">
      <rdf:type rdf:resource="http://www.w3.org/2004/02/skos/core#Concept"/>
      <skos:inScheme rdf:resource="http://rdf-vocabulary.ddialliance.org/cv/LifecycleEventType/1.0"/>
      <skos:notation>DataProcessing.DisclosureLimitation</skos:notation>
      <skos:prefLabel xml:lang="en">Data processing: Disclosure limitation</skos:prefLabel>
      <skos:definition xml:lang="en">Editing the data to prevent identification of subjects, for example, performing anonymization measures like recoding or top-coding sensitive variables like income levels, suppressing some geographic indicators, or replacing personal names with pseudonyms and/or categorizing background or demographic information in qualitative data.</skos:definition>
      <skos:prefLabel xml:lang="no">Databehandling: Begrensning om avsløring</skos:prefLabel>
      <skos:definition xml:lang="no">Å endre dataene for å forhindre identifisering av subjekter, for eksempel, å utføre anonymiseringstiltak som å rekode eller topp-kode sensitive variabler som inntektsnivå, aggregere eller holde tilbake geografiske indikatorer, eller erstatte personnavn med pseudonymer og/eller kategorisere bakgrunnsopplysninger eller demografisk informasjon i kvalitative data.</skos:definition>
      <skos:broader rdf:resource="http://rdf-vocabulary.ddialliance.org/cv/LifecycleEventType/1.0/d80e402"/>
   </rdf:Description>
   <rdf:Description rdf:about="http://rdf-vocabulary.ddialliance.org/cv/LifecycleEventType/1.0/d80e670">
      <rdf:type rdf:resource="http://www.w3.org/2004/02/skos/core#Concept"/>
      <skos:inScheme rdf:resource="http://rdf-vocabulary.ddialliance.org/cv/LifecycleEventType/1.0"/>
      <skos:notation>DataProcessing.Imputation</skos:notation>
      <skos:prefLabel xml:lang="en">Data processing: Imputation</skos:prefLabel>
      <skos:definition xml:lang="en">Replacing missing data points with values calculated according to an imputation technique.</skos:definition>
      <skos:prefLabel xml:lang="no">Databehandling: Imputasjon</skos:prefLabel>
      <skos:definition xml:lang="no">Erstatte manglende data punkter med verdier utregnet ved bruk av imputasjonsteknikker.</skos:definition>
      <skos:broader rdf:resource="http://rdf-vocabulary.ddialliance.org/cv/LifecycleEventType/1.0/d80e402"/>
   </rdf:Description>
   <rdf:Description rdf:about="http://rdf-vocabulary.ddialliance.org/cv/LifecycleEventType/1.0/d80e692">
      <rdf:type rdf:resource="http://www.w3.org/2004/02/skos/core#Concept"/>
      <skos:inScheme rdf:resource="http://rdf-vocabulary.ddialliance.org/cv/LifecycleEventType/1.0"/>
      <skos:notation>MetadataProduction</skos:notation>
      <skos:prefLabel xml:lang="en">Metadata production</skos:prefLabel>
      <skos:definition xml:lang="en">Documenting the data, for example, by producing study-level and variable descriptions.</skos:definition>
      <skos:prefLabel xml:lang="no">Metadata produksjon</skos:prefLabel>
      <skos:definition xml:lang="no">Dokumentere data, for eksempel ved å produsere studienivå og variabel beskrivelser.</skos:definition>
   </rdf:Description>
   <rdf:Description rdf:about="http://rdf-vocabulary.ddialliance.org/cv/LifecycleEventType/1.0/d80e714">
      <rdf:type rdf:resource="http://www.w3.org/2004/02/skos/core#Concept"/>
      <skos:inScheme rdf:resource="http://rdf-vocabulary.ddialliance.org/cv/LifecycleEventType/1.0"/>
      <skos:notation>MetadataEditing</skos:notation>
      <skos:prefLabel xml:lang="en">Metadata editing</skos:prefLabel>
      <skos:definition xml:lang="en">Amending the metadata to reflect changes in the data or to improve or enhance documentation.</skos:definition>
      <skos:prefLabel xml:lang="no">Metadata redigering</skos:prefLabel>
      <skos:definition xml:lang="no">Å endre metadataene for å gjenspeile endringer i dataene eller for å forbedre eller styrke dokumentasjonen.</skos:definition>
   </rdf:Description>
   <rdf:Description rdf:about="http://rdf-vocabulary.ddialliance.org/cv/LifecycleEventType/1.0/d80e737">
      <rdf:type rdf:resource="http://www.w3.org/2004/02/skos/core#Concept"/>
      <skos:inScheme rdf:resource="http://rdf-vocabulary.ddialliance.org/cv/LifecycleEventType/1.0"/>
      <skos:notation>MetadataTranslation</skos:notation>
      <skos:prefLabel xml:lang="en">Metadata translation</skos:prefLabel>
      <skos:definition xml:lang="en">Translating the metadata into another language.</skos:definition>
      <skos:prefLabel xml:lang="no">Metadata oversettelse</skos:prefLabel>
      <skos:definition xml:lang="no">Å oversette metadata til et annet språk.</skos:definition>
   </rdf:Description>
   <rdf:Description rdf:about="http://rdf-vocabulary.ddialliance.org/cv/LifecycleEventType/1.0/d80e759">
      <rdf:type rdf:resource="http://www.w3.org/2004/02/skos/core#Concept"/>
      <skos:inScheme rdf:resource="http://rdf-vocabulary.ddialliance.org/cv/LifecycleEventType/1.0"/>
      <skos:notation>FinalReport</skos:notation>
      <skos:prefLabel xml:lang="en">Final report</skos:prefLabel>
      <skos:definition xml:lang="en">Complete account on how the study was conducted through all its stages, often required by funders or other administrative bodies.</skos:definition>
      <skos:prefLabel xml:lang="no">Sluttrapport</skos:prefLabel>
      <skos:definition xml:lang="no">Fullstendig redegjørelse for hvordan studien ble gjennomført i alle stadier, ofte påkrevd av finansiør eller andre administrative instanser.</skos:definition>
   </rdf:Description>
   <rdf:Description rdf:about="http://rdf-vocabulary.ddialliance.org/cv/LifecycleEventType/1.0/d80e781">
      <rdf:type rdf:resource="http://www.w3.org/2004/02/skos/core#Concept"/>
      <skos:inScheme rdf:resource="http://rdf-vocabulary.ddialliance.org/cv/LifecycleEventType/1.0"/>
      <skos:notation>Evaluation</skos:notation>
      <skos:prefLabel xml:lang="en">Evaluation</skos:prefLabel>
      <skos:definition xml:lang="en">Analysis of how the study, in all its stages, was managed and/or conducted, including the outcome of methodological, technical, and business decisions. May serve as a basis for changes or improvements in planning future iterations of the data collection, or entirely new projects.</skos:definition>
      <skos:prefLabel xml:lang="no">Evaluering</skos:prefLabel>
      <skos:definition xml:lang="no">Analyse av hvordan studien, i alle stadier, ble administrert og/eller gjennomført, inkludert utfallet av metodologiske-, tekniske- og forretningsbeslutninger. Kan tjene som et grunnlag for endringer eller forbedringer i planleggingen av fremtidige iterasjoner av datainnsamlingen eller helt nye prosjekter.</skos:definition>
   </rdf:Description>
   <rdf:Description rdf:about="http://rdf-vocabulary.ddialliance.org/cv/LifecycleEventType/1.0/d80e803">
      <rdf:type rdf:resource="http://www.w3.org/2004/02/skos/core#Concept"/>
      <skos:inScheme rdf:resource="http://rdf-vocabulary.ddialliance.org/cv/LifecycleEventType/1.0"/>
      <skos:notation>OriginalRelease</skos:notation>
      <skos:prefLabel xml:lang="en">Original release</skos:prefLabel>
      <skos:definition xml:lang="en">First release of data and/or metadata to other individuals and/or agencies than the study producers.</skos:definition>
      <skos:prefLabel xml:lang="no">Original utgivelse</skos:prefLabel>
      <skos:definition xml:lang="no">Første utgivelse av data og/eller metadata til andre individer og/eller byråer enn studiens produsenter.</skos:definition>
   </rdf:Description>
   <rdf:Description rdf:about="http://rdf-vocabulary.ddialliance.org/cv/LifecycleEventType/1.0/d80e825">
      <rdf:type rdf:resource="http://www.w3.org/2004/02/skos/core#Concept"/>
      <skos:inScheme rdf:resource="http://rdf-vocabulary.ddialliance.org/cv/LifecycleEventType/1.0"/>
      <skos:notation>Deposit</skos:notation>
      <skos:prefLabel xml:lang="en">Deposit</skos:prefLabel>
      <skos:definition xml:lang="en">Handing over the data and available metadata (Submission Information Package in OAIS terms) to a data archive or repository for preservation, possible further processing,  and dissemination.</skos:definition>
      <skos:prefLabel xml:lang="no">Deponering</skos:prefLabel>
      <skos:definition xml:lang="no">Overlevering av data og tilgjengelig metadata (Submission Information Package i OAIS terminologi) til ett dataarkiv eller oppbevaringssted for bevaring, mulig videre prosessering, og formidling.</skos:definition>
   </rdf:Description>
   <rdf:Description rdf:about="http://rdf-vocabulary.ddialliance.org/cv/LifecycleEventType/1.0/d80e847">
      <rdf:type rdf:resource="http://www.w3.org/2004/02/skos/core#Concept"/>
      <skos:inScheme rdf:resource="http://rdf-vocabulary.ddialliance.org/cv/LifecycleEventType/1.0"/>
      <skos:notation>PreservationPackageProduction</skos:notation>
      <skos:prefLabel xml:lang="en">Preservation package production</skos:prefLabel>
      <skos:definition xml:lang="en">Producing a preservation package of the data for archiving purposes (Archival Information Package in OAIS terms).</skos:definition>
      <skos:prefLabel xml:lang="no">Produksjon av bevaringspakke</skos:prefLabel>
      <skos:definition xml:lang="no">Produsere en bevaringspakke av datamaterialet for arkivformål (Archival Information Package i OAIS terminologi).</skos:definition>
   </rdf:Description>
   <rdf:Description rdf:about="http://rdf-vocabulary.ddialliance.org/cv/LifecycleEventType/1.0/d80e870">
      <rdf:type rdf:resource="http://www.w3.org/2004/02/skos/core#Concept"/>
      <skos:inScheme rdf:resource="http://rdf-vocabulary.ddialliance.org/cv/LifecycleEventType/1.0"/>
      <skos:notation>DisseminationPackageProduction</skos:notation>
      <skos:prefLabel xml:lang="en">Dissemination package production</skos:prefLabel>
      <skos:definition xml:lang="en">Producing a dissemination package for distribution of the data (Dissemination Information Package in OAIS terms).</skos:definition>
      <skos:prefLabel xml:lang="no">Produksjon av formidlingspakke</skos:prefLabel>
      <skos:definition xml:lang="no">Produsere en formidlingspakke for distribusjon av data (Dissemination Information Package i OAIS terminologi).</skos:definition>
   </rdf:Description>
   <rdf:Description rdf:about="http://rdf-vocabulary.ddialliance.org/cv/LifecycleEventType/1.0/d80e892">
      <rdf:type rdf:resource="http://www.w3.org/2004/02/skos/core#Concept"/>
      <skos:inScheme rdf:resource="http://rdf-vocabulary.ddialliance.org/cv/LifecycleEventType/1.0"/>
      <skos:notation>DisseminationPackageRelease</skos:notation>
      <skos:prefLabel xml:lang="en">Dissemination package release</skos:prefLabel>
      <skos:definition xml:lang="en">Publishing or otherwise making the dissemination package available to users.</skos:definition>
      <skos:prefLabel xml:lang="no">Utgivelse av formidlingspakke</skos:prefLabel>
      <skos:definition xml:lang="no">Publisering, eller annen tilgjengeliggjøring, av formidlingspakken for brukere.</skos:definition>
   </rdf:Description>
   <rdf:Description rdf:about="http://rdf-vocabulary.ddialliance.org/cv/LifecycleEventType/1.0/d80e914">
      <rdf:type rdf:resource="http://www.w3.org/2004/02/skos/core#Concept"/>
      <skos:inScheme rdf:resource="http://rdf-vocabulary.ddialliance.org/cv/LifecycleEventType/1.0"/>
      <skos:notation>DataAnalysisReports</skos:notation>
      <skos:prefLabel xml:lang="en">Data analysis reports</skos:prefLabel>
      <skos:definition xml:lang="en">Reports describing how the data were analyzed,  as well as the resulting findings. These may take the form of conference posters or presentations, journal articles or online publications, books, book chapters, etc.</skos:definition>
      <skos:prefLabel xml:lang="no">Dataanalyse rapport</skos:prefLabel>
      <skos:definition xml:lang="no">Rapport som beskriver hvordan data ble analyser, inklusiv funn. Dette kan være konferansepresentasjoner, tidsskriftartikler eller online publikasjoner, bøker eller bokkapitler, etc.</skos:definition>
   </rdf:Description>
   <rdf:Description rdf:about="http://rdf-vocabulary.ddialliance.org/cv/LifecycleEventType/1.0/d80e936">
      <rdf:type rdf:resource="http://www.w3.org/2004/02/skos/core#Concept"/>
      <skos:inScheme rdf:resource="http://rdf-vocabulary.ddialliance.org/cv/LifecycleEventType/1.0"/>
      <skos:notation>NewVersionRelease</skos:notation>
      <skos:prefLabel xml:lang="en">New version release</skos:prefLabel>
      <skos:definition xml:lang="en">Publishing or otherwise making a new version of the data and/or metadata available to users.</skos:definition>
      <skos:prefLabel xml:lang="no">Ny versjon utgivelse</skos:prefLabel>
      <skos:definition xml:lang="no">Publisering, eller annen tilgjengeliggjøring, av en ny versjon av data og/eller metadata for brukere.</skos:definition>
   </rdf:Description>
   <rdf:Description rdf:about="http://rdf-vocabulary.ddialliance.org/cv/LifecycleEventType/1.0/d80e958">
      <rdf:type rdf:resource="http://www.w3.org/2004/02/skos/core#Concept"/>
      <skos:inScheme rdf:resource="http://rdf-vocabulary.ddialliance.org/cv/LifecycleEventType/1.0"/>
      <skos:notation>Other</skos:notation>
      <skos:prefLabel xml:lang="en">Other</skos:prefLabel>
      <skos:definition xml:lang="en">Use if the event type is known, but not found in the list.</skos:definition>
      <skos:prefLabel xml:lang="no">Annet</skos:prefLabel>
      <skos:definition xml:lang="no">Bruk hvis hendelsestypen er kjent, men ikke finnes på listen.</skos:definition>
   </rdf:Description>
</rdf:RDF>
