<?xml version="1.0" encoding="UTF-8"?>
<rdf:RDF xmlns:dcterms="http://purl.org/dc/terms/"
          xmlns:owl="http://www.w3.org/2002/07/owl#"
          xmlns:rdf="http://www.w3.org/1999/02/22-rdf-syntax-ns#"
          xmlns:rdfs="http://www.w3.org/2000/01/rdf-schema#"
          xmlns:skos="http://www.w3.org/2004/02/skos/core#">
   <rdf:Description rdf:about="http://rdf-vocabulary.ddialliance.org/cv/DataType/1.1/">
      <rdf:type rdf:resource="http://www.w3.org/2004/02/skos/core#ConceptScheme"/>
      <dcterms:isVersionOf rdf:resource="http://rdf-vocabulary.ddialliance.org/cv/DataType"/>
      <skos:notation>DataType</skos:notation>
      <skos:prefLabel xml:lang="en">Data Type</skos:prefLabel>
      <skos:prefLabel xml:lang="da">Datatype</skos:prefLabel>
      <skos:prefLabel xml:lang="no">Data type</skos:prefLabel>
      <skos:definition xml:lang="en">Identifies the type of data, which has a bearing on the acceptable data values, the operations that can be performed with the data, and the ways in which the data are stored.</skos:definition>
      <skos:definition xml:lang="da">Identificerer datatypen, der har betydning for acceptable dataværdier, operationerne, der kan udføres med dataene, og måderne, hvorpå dataene kan lagres.</skos:definition>
      <skos:definition xml:lang="no">Identifisering av datatypen som har betydning for akseptable dataverdier, operasjoner som kan bli gjennomført på dataene og hvordan data kan bli lagret.</skos:definition>
      <owl:versionInfo>1.1</owl:versionInfo>
      <dcterms:license rdf:resource="Creative Commons Attribution 4.0 International"/>
      <dcterms:rights>Copyright ©DDI Alliance 2019</dcterms:rights>
      <skos:hasTopConcept rdf:resource="http://rdf-vocabulary.ddialliance.org/cv/DataType/1.1/d11e107"/>
      <skos:hasTopConcept rdf:resource="http://rdf-vocabulary.ddialliance.org/cv/DataType/1.1/d11e135"/>
      <skos:hasTopConcept rdf:resource="http://rdf-vocabulary.ddialliance.org/cv/DataType/1.1/d11e163"/>
      <skos:hasTopConcept rdf:resource="http://rdf-vocabulary.ddialliance.org/cv/DataType/1.1/d11e191"/>
      <skos:hasTopConcept rdf:resource="http://rdf-vocabulary.ddialliance.org/cv/DataType/1.1/d11e220"/>
      <skos:hasTopConcept rdf:resource="http://rdf-vocabulary.ddialliance.org/cv/DataType/1.1/d11e248"/>
      <skos:hasTopConcept rdf:resource="http://rdf-vocabulary.ddialliance.org/cv/DataType/1.1/d11e276"/>
      <skos:hasTopConcept rdf:resource="http://rdf-vocabulary.ddialliance.org/cv/DataType/1.1/d11e304"/>
      <skos:hasTopConcept rdf:resource="http://rdf-vocabulary.ddialliance.org/cv/DataType/1.1/d11e332"/>
      <skos:hasTopConcept rdf:resource="http://rdf-vocabulary.ddialliance.org/cv/DataType/1.1/d11e360"/>
      <skos:hasTopConcept rdf:resource="http://rdf-vocabulary.ddialliance.org/cv/DataType/1.1/d11e389"/>
      <skos:hasTopConcept rdf:resource="http://rdf-vocabulary.ddialliance.org/cv/DataType/1.1/d11e417"/>
      <skos:hasTopConcept rdf:resource="http://rdf-vocabulary.ddialliance.org/cv/DataType/1.1/d11e445"/>
      <skos:hasTopConcept rdf:resource="http://rdf-vocabulary.ddialliance.org/cv/DataType/1.1/d11e473"/>
      <skos:hasTopConcept rdf:resource="http://rdf-vocabulary.ddialliance.org/cv/DataType/1.1/d11e501"/>
      <skos:hasTopConcept rdf:resource="http://rdf-vocabulary.ddialliance.org/cv/DataType/1.1/d11e529"/>
      <skos:hasTopConcept rdf:resource="http://rdf-vocabulary.ddialliance.org/cv/DataType/1.1/d11e558"/>
      <skos:hasTopConcept rdf:resource="http://rdf-vocabulary.ddialliance.org/cv/DataType/1.1/d11e586"/>
      <skos:hasTopConcept rdf:resource="http://rdf-vocabulary.ddialliance.org/cv/DataType/1.1/d11e614"/>
      <skos:hasTopConcept rdf:resource="http://rdf-vocabulary.ddialliance.org/cv/DataType/1.1/d11e642"/>
      <skos:hasTopConcept rdf:resource="http://rdf-vocabulary.ddialliance.org/cv/DataType/1.1/d11e670"/>
      <skos:hasTopConcept rdf:resource="http://rdf-vocabulary.ddialliance.org/cv/DataType/1.1/d11e698"/>
      <skos:hasTopConcept rdf:resource="http://rdf-vocabulary.ddialliance.org/cv/DataType/1.1/d11e727"/>
      <skos:hasTopConcept rdf:resource="http://rdf-vocabulary.ddialliance.org/cv/DataType/1.1/d11e755"/>
      <skos:hasTopConcept rdf:resource="http://rdf-vocabulary.ddialliance.org/cv/DataType/1.1/d11e783"/>
      <skos:hasTopConcept rdf:resource="http://rdf-vocabulary.ddialliance.org/cv/DataType/1.1/d11e811"/>
      <skos:hasTopConcept rdf:resource="http://rdf-vocabulary.ddialliance.org/cv/DataType/1.1/d11e839"/>
      <skos:hasTopConcept rdf:resource="http://rdf-vocabulary.ddialliance.org/cv/DataType/1.1/d11e867"/>
      <skos:hasTopConcept rdf:resource="http://rdf-vocabulary.ddialliance.org/cv/DataType/1.1/d11e896"/>
      <skos:hasTopConcept rdf:resource="http://rdf-vocabulary.ddialliance.org/cv/DataType/1.1/d11e924"/>
      <skos:hasTopConcept rdf:resource="http://rdf-vocabulary.ddialliance.org/cv/DataType/1.1/d11e952"/>
      <skos:hasTopConcept rdf:resource="http://rdf-vocabulary.ddialliance.org/cv/DataType/1.1/d11e980"/>
   </rdf:Description>
   <rdf:Description rdf:about="http://rdf-vocabulary.ddialliance.org/cv/DataType/1.1/d11e107">
      <rdf:type rdf:resource="http://www.w3.org/2004/02/skos/core#Concept"/>
      <skos:inScheme rdf:resource="http://rdf-vocabulary.ddialliance.org/cv/DataType/1.1/"/>
      <skos:notation>String</skos:notation>
      <skos:prefLabel xml:lang="en">String</skos:prefLabel>
      <skos:definition xml:lang="en">Finite sequences of characters. A character is an atomic unit of written communication; it is not further specified except to note that every character has a corresponding Universal Character Set code point (which is an integer).</skos:definition>
      <skos:prefLabel xml:lang="da">Streng</skos:prefLabel>
      <skos:definition xml:lang="da">Begrænset sekvens af tegn. Et tegn er en atomenhed af skriftlig kommunikation; det er ikke nærmere specifiseret undtagen at bemærke, at hvert tegn har et tilsvarende Universal Character Set-kodepunkt (som er et heltal).</skos:definition>
      <skos:prefLabel xml:lang="no">Streng</skos:prefLabel>
      <skos:definition xml:lang="no">Endelig sekvens av tegn. Et tegn er en atomenhet for skriftlig kommunikasjon; det er ikke nærmere spesifisert, bortsett fra å merke seg at hvert tegn har et tilsvarende Universal Character Set-kodepunkt (som er et heltall).</skos:definition>
   </rdf:Description>
   <rdf:Description rdf:about="http://rdf-vocabulary.ddialliance.org/cv/DataType/1.1/d11e135">
      <rdf:type rdf:resource="http://www.w3.org/2004/02/skos/core#Concept"/>
      <skos:inScheme rdf:resource="http://rdf-vocabulary.ddialliance.org/cv/DataType/1.1/"/>
      <skos:notation>NormalizedString</skos:notation>
      <skos:prefLabel xml:lang="en">Normalized string</skos:prefLabel>
      <skos:definition xml:lang="en">Type of string in which any occurrence of whitespace (including tabs, line feeds, and carriage returns) is replaced by a single space.</skos:definition>
      <skos:prefLabel xml:lang="da">Normaliseret streng</skos:prefLabel>
      <skos:definition xml:lang="da">Type af streng, hvor enhver forekomst af mellemrum (inklusive faneblade, linjeskift og vognretur) erstattes af et enkelt mellemrum.</skos:definition>
      <skos:prefLabel xml:lang="no">Normalisert streng</skos:prefLabel>
      <skos:definition xml:lang="no">En type streng hvor alle forekomster av hvitt mellomrom (inkludert tabulator, linjeskift og vognretur) blir erstattet av et enkelt mellomrom.</skos:definition>
   </rdf:Description>
   <rdf:Description rdf:about="http://rdf-vocabulary.ddialliance.org/cv/DataType/1.1/d11e163">
      <rdf:type rdf:resource="http://www.w3.org/2004/02/skos/core#Concept"/>
      <skos:inScheme rdf:resource="http://rdf-vocabulary.ddialliance.org/cv/DataType/1.1/"/>
      <skos:notation>Boolean</skos:notation>
      <skos:prefLabel xml:lang="en">Boolean</skos:prefLabel>
      <skos:definition xml:lang="en">True or false. Can be represented by 1 and 0 correspondingly.</skos:definition>
      <skos:prefLabel xml:lang="da">Boolsk</skos:prefLabel>
      <skos:definition xml:lang="da">Sandt eller falsk. Kan tilsvarende være repræsenteret af 1 og 0.</skos:definition>
      <skos:prefLabel xml:lang="no">Boolsk</skos:prefLabel>
      <skos:definition xml:lang="no">Sant eller usant. Kan være representert av 1 og 0 henholdsvis.</skos:definition>
   </rdf:Description>
   <rdf:Description rdf:about="http://rdf-vocabulary.ddialliance.org/cv/DataType/1.1/d11e191">
      <rdf:type rdf:resource="http://www.w3.org/2004/02/skos/core#Concept"/>
      <skos:inScheme rdf:resource="http://rdf-vocabulary.ddialliance.org/cv/DataType/1.1/"/>
      <skos:notation>Decimal</skos:notation>
      <skos:prefLabel xml:lang="en">Decimal</skos:prefLabel>
      <skos:definition xml:lang="en">A subset of real numbers, which can be represented by a finite-length sequence of decimal digits (0-9) separated by a period as a decimal indicator. An optional leading sign is allowed. If the sign is omitted, "+" is assumed. Leading and trailing zeroes are optional. If the fractional part is zero, the period and following zero(es) can be omitted. For example: -1.23, 12678967.543233, +100000.00, 210.</skos:definition>
      <skos:prefLabel xml:lang="da">Decimal</skos:prefLabel>
      <skos:definition xml:lang="da">En delmængde af reelle tal, der kan repræsenteres af en sekvens af begrænset længde af decimaltal (0-9) adskilt med et punktum som decimalindikator. Et valgfrit fortegn er tilladt. Hvis tegnet er udeladt, antages "+". Førende og efterfølgende nuller er valgfri. Hvis brøkdelen er nul, kan punktummet og følgende nul(ler) udelades. For eksempel: -1.23, 12678967.543233, +100000.00, 210.</skos:definition>
      <skos:prefLabel xml:lang="no">Desimal</skos:prefLabel>
      <skos:definition xml:lang="no">En delmengde av reelle tall som kan bli representert av en endelig sekvens av desimaltall (0-9) adskilt med et punktum som desimalindikator. Et alternativ tegn før desimalindikatoren er tillatt. Hvis tegnet er utelatt, antas "+". Førende og etterfølgende nuller er valgfri. Hvis brøkdelen er null, kan punktumet og følgende null(er) bli utelatt. For eksempel: -1.23, 12678967.543233, +100000.00, 210.</skos:definition>
   </rdf:Description>
   <rdf:Description rdf:about="http://rdf-vocabulary.ddialliance.org/cv/DataType/1.1/d11e220">
      <rdf:type rdf:resource="http://www.w3.org/2004/02/skos/core#Concept"/>
      <skos:inScheme rdf:resource="http://rdf-vocabulary.ddialliance.org/cv/DataType/1.1/"/>
      <skos:notation>Integer</skos:notation>
      <skos:prefLabel xml:lang="en">Integer</skos:prefLabel>
      <skos:definition xml:lang="en">Whole numbers, the infinite set of integers, no minimum or maximum value.</skos:definition>
      <skos:prefLabel xml:lang="da">Heltal</skos:prefLabel>
      <skos:definition xml:lang="da">Hele tal, det uendelige sæt heltal, ingen minimums- eller maksimumværdi.</skos:definition>
      <skos:prefLabel xml:lang="no">Heltall</skos:prefLabel>
      <skos:definition xml:lang="no">Hele tall, det uendelige settet med heltall, ingen minimum eller maksimum verdi.</skos:definition>
   </rdf:Description>
   <rdf:Description rdf:about="http://rdf-vocabulary.ddialliance.org/cv/DataType/1.1/d11e248">
      <rdf:type rdf:resource="http://www.w3.org/2004/02/skos/core#Concept"/>
      <skos:inScheme rdf:resource="http://rdf-vocabulary.ddialliance.org/cv/DataType/1.1/"/>
      <skos:notation>PositiveInteger</skos:notation>
      <skos:prefLabel xml:lang="en">Positive integer</skos:prefLabel>
      <skos:definition xml:lang="en">Whole numbers greater than 0.</skos:definition>
      <skos:prefLabel xml:lang="da">Positiv heltal</skos:prefLabel>
      <skos:definition xml:lang="da">Hele tal større end 0.</skos:definition>
      <skos:prefLabel xml:lang="no">Positive heltall</skos:prefLabel>
      <skos:definition xml:lang="no">Hele tall større enn 0.</skos:definition>
   </rdf:Description>
   <rdf:Description rdf:about="http://rdf-vocabulary.ddialliance.org/cv/DataType/1.1/d11e276">
      <rdf:type rdf:resource="http://www.w3.org/2004/02/skos/core#Concept"/>
      <skos:inScheme rdf:resource="http://rdf-vocabulary.ddialliance.org/cv/DataType/1.1/"/>
      <skos:notation>NegativeInteger</skos:notation>
      <skos:prefLabel xml:lang="en">Negative integer</skos:prefLabel>
      <skos:definition xml:lang="en">Whole numbers less than 0.</skos:definition>
      <skos:prefLabel xml:lang="da">Negativ heltal</skos:prefLabel>
      <skos:definition xml:lang="da">Hele tal mindre end 0.</skos:definition>
      <skos:prefLabel xml:lang="no">Negative heltall</skos:prefLabel>
      <skos:definition xml:lang="no">Hele tall mindre enn 0.</skos:definition>
   </rdf:Description>
   <rdf:Description rdf:about="http://rdf-vocabulary.ddialliance.org/cv/DataType/1.1/d11e304">
      <rdf:type rdf:resource="http://www.w3.org/2004/02/skos/core#Concept"/>
      <skos:inScheme rdf:resource="http://rdf-vocabulary.ddialliance.org/cv/DataType/1.1/"/>
      <skos:notation>NonNegativeInteger</skos:notation>
      <skos:prefLabel xml:lang="en">Non-negative integer</skos:prefLabel>
      <skos:definition xml:lang="en">Whole numbers greater than -1.</skos:definition>
      <skos:prefLabel xml:lang="da">Ikke-negativ heltal</skos:prefLabel>
      <skos:definition xml:lang="da">Hele tal større end -1.</skos:definition>
      <skos:prefLabel xml:lang="no">Ikke-negative heltall</skos:prefLabel>
      <skos:definition xml:lang="no">Hele tall større enn -1.</skos:definition>
   </rdf:Description>
   <rdf:Description rdf:about="http://rdf-vocabulary.ddialliance.org/cv/DataType/1.1/d11e332">
      <rdf:type rdf:resource="http://www.w3.org/2004/02/skos/core#Concept"/>
      <skos:inScheme rdf:resource="http://rdf-vocabulary.ddialliance.org/cv/DataType/1.1/"/>
      <skos:notation>NonPositiveInteger</skos:notation>
      <skos:prefLabel xml:lang="en">Non-positive integer</skos:prefLabel>
      <skos:definition xml:lang="en">Whole numbers less than 1.</skos:definition>
      <skos:prefLabel xml:lang="da">Ikke-positiv heltal</skos:prefLabel>
      <skos:definition xml:lang="da">Hele tal mindre end 1.</skos:definition>
      <skos:prefLabel xml:lang="no">Ikke-positive heltall</skos:prefLabel>
      <skos:definition xml:lang="no">Hele tall mindre enn 1.</skos:definition>
   </rdf:Description>
   <rdf:Description rdf:about="http://rdf-vocabulary.ddialliance.org/cv/DataType/1.1/d11e360">
      <rdf:type rdf:resource="http://www.w3.org/2004/02/skos/core#Concept"/>
      <skos:inScheme rdf:resource="http://rdf-vocabulary.ddialliance.org/cv/DataType/1.1/"/>
      <skos:notation>Long</skos:notation>
      <skos:prefLabel xml:lang="en">Long</skos:prefLabel>
      <skos:definition xml:lang="en">Whole numbers in the range -9223372036854775808 .. 9223372036854775807.</skos:definition>
      <skos:prefLabel xml:lang="da">Long</skos:prefLabel>
      <skos:definition xml:lang="da">Hele tal i intervallet -9223372036854775808 .. 9223372036854775807.</skos:definition>
      <skos:prefLabel xml:lang="no">Long</skos:prefLabel>
      <skos:definition xml:lang="no">Hele tall i rekkevidden -9223372036854775808 .. 9223372036854775807.</skos:definition>
   </rdf:Description>
   <rdf:Description rdf:about="http://rdf-vocabulary.ddialliance.org/cv/DataType/1.1/d11e389">
      <rdf:type rdf:resource="http://www.w3.org/2004/02/skos/core#Concept"/>
      <skos:inScheme rdf:resource="http://rdf-vocabulary.ddialliance.org/cv/DataType/1.1/"/>
      <skos:notation>Int</skos:notation>
      <skos:prefLabel xml:lang="en">Int</skos:prefLabel>
      <skos:definition xml:lang="en">Whole numbers in the range -2147483648 .. 2147483647.</skos:definition>
      <skos:prefLabel xml:lang="da">Int</skos:prefLabel>
      <skos:definition xml:lang="da">Hele tal i intervallet -2147483648 .. 2147483647.</skos:definition>
      <skos:prefLabel xml:lang="no">Int</skos:prefLabel>
      <skos:definition xml:lang="no">Hele tall i rekkevidden -2147483648 .. 2147483647.</skos:definition>
   </rdf:Description>
   <rdf:Description rdf:about="http://rdf-vocabulary.ddialliance.org/cv/DataType/1.1/d11e417">
      <rdf:type rdf:resource="http://www.w3.org/2004/02/skos/core#Concept"/>
      <skos:inScheme rdf:resource="http://rdf-vocabulary.ddialliance.org/cv/DataType/1.1/"/>
      <skos:notation>Short</skos:notation>
      <skos:prefLabel xml:lang="en">Short</skos:prefLabel>
      <skos:definition xml:lang="en">Whole numbers in the range -32768 .. 32767.</skos:definition>
      <skos:prefLabel xml:lang="da">Short</skos:prefLabel>
      <skos:definition xml:lang="da">Hele tal i intervallet -32768 .. 32767.</skos:definition>
      <skos:prefLabel xml:lang="no">Short</skos:prefLabel>
      <skos:definition xml:lang="no">Hele tall i rekkevidden -32768 .. 32767.</skos:definition>
   </rdf:Description>
   <rdf:Description rdf:about="http://rdf-vocabulary.ddialliance.org/cv/DataType/1.1/d11e445">
      <rdf:type rdf:resource="http://www.w3.org/2004/02/skos/core#Concept"/>
      <skos:inScheme rdf:resource="http://rdf-vocabulary.ddialliance.org/cv/DataType/1.1/"/>
      <skos:notation>Byte</skos:notation>
      <skos:prefLabel xml:lang="en">Byte</skos:prefLabel>
      <skos:definition xml:lang="en">Whole numbers in the range -128 .. 127.</skos:definition>
      <skos:prefLabel xml:lang="da">Byte</skos:prefLabel>
      <skos:definition xml:lang="da">Hele tal i intervallet -128 .. 127.</skos:definition>
      <skos:prefLabel xml:lang="no">Byte</skos:prefLabel>
      <skos:definition xml:lang="no">Hele tall i rekkevidden -128 .. 127.</skos:definition>
   </rdf:Description>
   <rdf:Description rdf:about="http://rdf-vocabulary.ddialliance.org/cv/DataType/1.1/d11e473">
      <rdf:type rdf:resource="http://www.w3.org/2004/02/skos/core#Concept"/>
      <skos:inScheme rdf:resource="http://rdf-vocabulary.ddialliance.org/cv/DataType/1.1/"/>
      <skos:notation>UnsignedLong</skos:notation>
      <skos:prefLabel xml:lang="en">Unsigned long</skos:prefLabel>
      <skos:definition xml:lang="en">Whole numbers in the range 0 .. 18446744073709551615.</skos:definition>
      <skos:prefLabel xml:lang="da">Unsigned long</skos:prefLabel>
      <skos:definition xml:lang="da">Hele tal i intervallet 0 .. 18446744073709551615.</skos:definition>
      <skos:prefLabel xml:lang="no">Unsigned long</skos:prefLabel>
      <skos:definition xml:lang="no">Hele tall i rekkevidden 0 .. 18446744073709551615.</skos:definition>
   </rdf:Description>
   <rdf:Description rdf:about="http://rdf-vocabulary.ddialliance.org/cv/DataType/1.1/d11e501">
      <rdf:type rdf:resource="http://www.w3.org/2004/02/skos/core#Concept"/>
      <skos:inScheme rdf:resource="http://rdf-vocabulary.ddialliance.org/cv/DataType/1.1/"/>
      <skos:notation>UnsignedInt</skos:notation>
      <skos:prefLabel xml:lang="en">Unsigned int</skos:prefLabel>
      <skos:definition xml:lang="en">Whole numbers in the range 0 .. 4294967295.</skos:definition>
      <skos:prefLabel xml:lang="da">Unsigned int</skos:prefLabel>
      <skos:definition xml:lang="da">Hele tal i intervallet 0 .. 4294967295.</skos:definition>
      <skos:prefLabel xml:lang="no">Unsigned int</skos:prefLabel>
      <skos:definition xml:lang="no">Hele tall i rekkevidden 0 .. 4294967295.</skos:definition>
   </rdf:Description>
   <rdf:Description rdf:about="http://rdf-vocabulary.ddialliance.org/cv/DataType/1.1/d11e529">
      <rdf:type rdf:resource="http://www.w3.org/2004/02/skos/core#Concept"/>
      <skos:inScheme rdf:resource="http://rdf-vocabulary.ddialliance.org/cv/DataType/1.1/"/>
      <skos:notation>UnsignedShort</skos:notation>
      <skos:prefLabel xml:lang="en">Unsigned short</skos:prefLabel>
      <skos:definition xml:lang="en">Whole numbers in the range 0 .. 65535.</skos:definition>
      <skos:prefLabel xml:lang="da">Unsigned short</skos:prefLabel>
      <skos:definition xml:lang="da">Hele tal i intervallet 0 .. 65535.</skos:definition>
      <skos:prefLabel xml:lang="no">Unsigned short</skos:prefLabel>
      <skos:definition xml:lang="no">Hele tall i rekkevidden 0 .. 65535.</skos:definition>
   </rdf:Description>
   <rdf:Description rdf:about="http://rdf-vocabulary.ddialliance.org/cv/DataType/1.1/d11e558">
      <rdf:type rdf:resource="http://www.w3.org/2004/02/skos/core#Concept"/>
      <skos:inScheme rdf:resource="http://rdf-vocabulary.ddialliance.org/cv/DataType/1.1/"/>
      <skos:notation>UnsignedByte</skos:notation>
      <skos:prefLabel xml:lang="en">Unsigned byte</skos:prefLabel>
      <skos:definition xml:lang="en">Whole numbers in the range 0 .. 255 (system dependent).</skos:definition>
      <skos:prefLabel xml:lang="da">Unsigned byte</skos:prefLabel>
      <skos:definition xml:lang="da">Hele tal i intervallet 0 .. 255 (systemafhængigt).</skos:definition>
      <skos:prefLabel xml:lang="no">Unsigned byte</skos:prefLabel>
      <skos:definition xml:lang="no">Hele tall i rekkevidden 0 .. 255 (systemavhengig).</skos:definition>
   </rdf:Description>
   <rdf:Description rdf:about="http://rdf-vocabulary.ddialliance.org/cv/DataType/1.1/d11e586">
      <rdf:type rdf:resource="http://www.w3.org/2004/02/skos/core#Concept"/>
      <skos:inScheme rdf:resource="http://rdf-vocabulary.ddialliance.org/cv/DataType/1.1/"/>
      <skos:notation>Float</skos:notation>
      <skos:prefLabel xml:lang="en">Float</skos:prefLabel>
      <skos:definition xml:lang="en">Single-precision 32-bit floating point type: The basic value space of float consists of the values m*2^e, where m is an integer whose absolute value is less than 2^24, and e is an integer between -149 and 104, inclusive. In addition, it also contains the following three special values: positive and negative infinity and not-a-number (NaN). The special values positive and negative infinity and not-a-number have lexical representations INF, -INF and NaN, respectively. Lexical representations for zero may take a positive or negative sign. For example, -1E4, 1267.43233E12, 12.78e-2, 12 , -0, 0 and INF are all legal literals for float.</skos:definition>
      <skos:prefLabel xml:lang="da">Float</skos:prefLabel>
      <skos:definition xml:lang="da">Single-precision 32-bit floating point type: Den grundlæggende float-værdirækkevidde består af værdierne m*2^e, hvor m er et heltal, hvis absolutte værdi er mindre end 2^24, og e er et heltal mellem -149 og 104, inklusiv. I tillæg indeholder det også de følgende tre specialværdier: positiv og negativ uendelighed og not-a-number (NaN). Specialværdierne positiv og negativ uendehlighed og not-a-number har henholdsvis leksikale repræsentationer INF, -INF og NaN. Leksikale repræsentationer for nul kan have positivt eller negativt fortegn. For eksempel, -1E4, 1267.43233E12, 12.78e-2, 12 , -0, 0 og INF er alle lovlige udtryk for float.</skos:definition>
      <skos:prefLabel xml:lang="no">Float</skos:prefLabel>
      <skos:definition xml:lang="no">Single-precision 32-bit floating point type: Den grunnleggende verdirekkevidden til en float består av verdiene m*2^e, hvor m er et heltall med absolutt verdi mindre enn 2^24 og e er et heltall mellom -149 og 104. I tillegg inneholder det også tre spesialverdier: positiv og negativ uendelig og not-a-number (NaN). Spesialverdiene positiv og negativ uendelig og not-a-number har leksikalsk representasjon INF, -INF og NaN, henholdsvis. Leksikalske representasjoner for null kan ha positivt eller negativt fortegn. For eksempel, -1E4, 1267.43233E12, 12.78e-2. -0. 0 og INF er alle lovlige uttrykk for float.</skos:definition>
   </rdf:Description>
   <rdf:Description rdf:about="http://rdf-vocabulary.ddialliance.org/cv/DataType/1.1/d11e614">
      <rdf:type rdf:resource="http://www.w3.org/2004/02/skos/core#Concept"/>
      <skos:inScheme rdf:resource="http://rdf-vocabulary.ddialliance.org/cv/DataType/1.1/"/>
      <skos:notation>Double</skos:notation>
      <skos:prefLabel xml:lang="en">Double</skos:prefLabel>
      <skos:definition xml:lang="en">Double-precision 64-bit floating point type. The basic value space of double consists of the values m*2^e, where m is an integer whose absolute value is less than 2^53, and e is an integer between -1075 and 970, inclusive. In addition to the basic value space described above, the value space of double also contains the following three special values: positive and negative infinity and not-a-number (NaN). The special values positive and negative infinity and not-a-number have lexical representations INF, -INF and NaN, respectively. Lexical representations for zero may take a positive or negative sign. For example, -1E4, 1267.43233E12, 12.78e-2, 12 , -0, 0 and INF are all legal literals for double.</skos:definition>
      <skos:prefLabel xml:lang="da">Double</skos:prefLabel>
      <skos:definition xml:lang="da">Double-precision 64-bit floating point type. Den grundlæggende double-værdirækkevidde består af værdierne m*2^e, hvor m er et heltal, hvis absolutte værdi er mindre end 2^53, og e er et heltal mellem -1075 og 970, inklusiv. I tillæg til den grundlæggende værdirækkevidde beskrevet ovenfor indeholder double-værdirækkevidden også de følgende tre specialværdier: positiv og negativ uendelighed og not-a-number (NaN). Specialværdierne positiv og negativ uendehlighed og not-a-number har henholdsvis leksikale repræsentationer INF, -INF og NaN. Leksikale repræsentationer for nul kan have positivt eller negativt fortegn. For eksempel, -1E4, 1267.43233E12, 12.78e-2, 12 , -0, 0 er alle lovlige udtryk for double.</skos:definition>
      <skos:prefLabel xml:lang="no">Double</skos:prefLabel>
      <skos:definition xml:lang="no">Double-precision 64-bit floating point type. Den grunnleggende verdirekkevidden til en double består av verdiene m*2^e, hvor m er et heltall med absolutt verdi mindre enn 2^53, og e er et heltall mellom -1075 og 970. I tillegg til de grunnleggende verdiene beskrevet ovenfor, inneholder også verdirekkevidden til double også de følgende tre spesialverdiene: positiv og negativ uendelig og not-a-number (NaN). Spesialverdiene positiv og negativ uendelig og not-a-number har leksikalske representasjon INF, -INF og NaN, henholdsvis. Leksikalske representasjoner for null kan ha positivt eller negativt fortegn. For eksempel, -1E4, 1267.43233E12, 12.78e-2, 12, -0, 0 og INF er alle lovlige uttrykk for double.</skos:definition>
   </rdf:Description>
   <rdf:Description rdf:about="http://rdf-vocabulary.ddialliance.org/cv/DataType/1.1/d11e642">
      <rdf:type rdf:resource="http://www.w3.org/2004/02/skos/core#Concept"/>
      <skos:inScheme rdf:resource="http://rdf-vocabulary.ddialliance.org/cv/DataType/1.1/"/>
      <skos:notation>DateTime</skos:notation>
      <skos:prefLabel xml:lang="en">DateTime</skos:prefLabel>
      <skos:definition xml:lang="en">Integer-valued year, month, day, hour and minute, plus decimal-valued second property, and time zone hour and minute (e.g., 2002-10-10T12:00:00-05:00).</skos:definition>
      <skos:prefLabel xml:lang="da">DatoTid</skos:prefLabel>
      <skos:definition xml:lang="da">Heltalsværdi år, måned, dag, time og minut, plus decimalværdi af sekunders egenskaber, og tidszone, time og minut (f.eks. 2002-10-10T12:00:00-05:00).</skos:definition>
      <skos:prefLabel xml:lang="no">DateTime</skos:prefLabel>
      <skos:definition xml:lang="no">Heltall verdi år, måned, dag, time og minutt, pluss desimalverdi av sekunders egenskaper, og tidssone, time og minutt. (f.eks., 2002-10-10T12:00:00-05:00).</skos:definition>
   </rdf:Description>
   <rdf:Description rdf:about="http://rdf-vocabulary.ddialliance.org/cv/DataType/1.1/d11e670">
      <rdf:type rdf:resource="http://www.w3.org/2004/02/skos/core#Concept"/>
      <skos:inScheme rdf:resource="http://rdf-vocabulary.ddialliance.org/cv/DataType/1.1/"/>
      <skos:notation>Time</skos:notation>
      <skos:prefLabel xml:lang="en">Time</skos:prefLabel>
      <skos:definition xml:lang="en">Left-truncated dateTime, e.g., 13:20:00-05:00 (1:20 pm for Eastern Standard Time U.S.).</skos:definition>
      <skos:prefLabel xml:lang="da">Tid</skos:prefLabel>
      <skos:definition xml:lang="da">Venstre-afkortet DatoTid, f.eks. 13:20:00-05:00 (1.20 pm for Eastern Standard Time U.S.</skos:definition>
      <skos:prefLabel xml:lang="no">Tid</skos:prefLabel>
      <skos:definition xml:lang="no">Venstre avkortet dateTime, f.eks., 13:20:00-05:00 (13:20 for Eastern Standard Time U.S.).</skos:definition>
   </rdf:Description>
   <rdf:Description rdf:about="http://rdf-vocabulary.ddialliance.org/cv/DataType/1.1/d11e698">
      <rdf:type rdf:resource="http://www.w3.org/2004/02/skos/core#Concept"/>
      <skos:inScheme rdf:resource="http://rdf-vocabulary.ddialliance.org/cv/DataType/1.1/"/>
      <skos:notation>Date</skos:notation>
      <skos:prefLabel xml:lang="en">Date</skos:prefLabel>
      <skos:definition xml:lang="en">Integer-valued year, month, day, and time zone hour and minutes, e.g., 2003-06-30-05:00 (30 June 2003 Eastern Standard Time U.S.).</skos:definition>
      <skos:prefLabel xml:lang="da">Dato</skos:prefLabel>
      <skos:definition xml:lang="da">Heltalsværdi år, måned, dag, og tidszone og minutter, f.eks. 2003-06-30-05:00 (30. juni 2003 Eastern Standard Time U.S.).</skos:definition>
      <skos:prefLabel xml:lang="no">Dato</skos:prefLabel>
      <skos:definition xml:lang="no">Heltall verdi år, måned, dag og tidssone time og minutter, f.eks., 2003-06-30-05:00 (30 Juni 2003 Eastern Standard Time U.S.).</skos:definition>
   </rdf:Description>
   <rdf:Description rdf:about="http://rdf-vocabulary.ddialliance.org/cv/DataType/1.1/d11e727">
      <rdf:type rdf:resource="http://www.w3.org/2004/02/skos/core#Concept"/>
      <skos:inScheme rdf:resource="http://rdf-vocabulary.ddialliance.org/cv/DataType/1.1/"/>
      <skos:notation>GYearMonth</skos:notation>
      <skos:prefLabel xml:lang="en">YearMonth</skos:prefLabel>
      <skos:definition xml:lang="en">Integer-valued year and month, e.g., 2004-11.</skos:definition>
      <skos:prefLabel xml:lang="da">ÅrMåned</skos:prefLabel>
      <skos:definition xml:lang="da">Heltalsværdi år og måned, f.eks. 2004-11.</skos:definition>
      <skos:prefLabel xml:lang="no">YearMonth</skos:prefLabel>
      <skos:definition xml:lang="no">Heltall verdi år og måned, f.eks., 2004-11.</skos:definition>
   </rdf:Description>
   <rdf:Description rdf:about="http://rdf-vocabulary.ddialliance.org/cv/DataType/1.1/d11e755">
      <rdf:type rdf:resource="http://www.w3.org/2004/02/skos/core#Concept"/>
      <skos:inScheme rdf:resource="http://rdf-vocabulary.ddialliance.org/cv/DataType/1.1/"/>
      <skos:notation>GYear</skos:notation>
      <skos:prefLabel xml:lang="en">Year</skos:prefLabel>
      <skos:definition xml:lang="en">Integer-valued year, e.g., 2005.</skos:definition>
      <skos:prefLabel xml:lang="da">År</skos:prefLabel>
      <skos:definition xml:lang="da">Heltalsværdi år, f.eks. 2005.</skos:definition>
      <skos:prefLabel xml:lang="no">År</skos:prefLabel>
      <skos:definition xml:lang="no">Heltall verdi år, f.eks., 2005.</skos:definition>
   </rdf:Description>
   <rdf:Description rdf:about="http://rdf-vocabulary.ddialliance.org/cv/DataType/1.1/d11e783">
      <rdf:type rdf:resource="http://www.w3.org/2004/02/skos/core#Concept"/>
      <skos:inScheme rdf:resource="http://rdf-vocabulary.ddialliance.org/cv/DataType/1.1/"/>
      <skos:notation>GMonthDay</skos:notation>
      <skos:prefLabel xml:lang="en">MonthDay</skos:prefLabel>
      <skos:definition xml:lang="en">Integer-valued month and day, e.g., 12-31.</skos:definition>
      <skos:prefLabel xml:lang="da">MånedDag</skos:prefLabel>
      <skos:definition xml:lang="da">Heltalsværdi måned og dag, f.eks. 12-31.</skos:definition>
      <skos:prefLabel xml:lang="no">MonthDay</skos:prefLabel>
      <skos:definition xml:lang="no">Heltall verdi måned og dag, f.eks., 12-31.</skos:definition>
   </rdf:Description>
   <rdf:Description rdf:about="http://rdf-vocabulary.ddialliance.org/cv/DataType/1.1/d11e811">
      <rdf:type rdf:resource="http://www.w3.org/2004/02/skos/core#Concept"/>
      <skos:inScheme rdf:resource="http://rdf-vocabulary.ddialliance.org/cv/DataType/1.1/"/>
      <skos:notation>GDay</skos:notation>
      <skos:prefLabel xml:lang="en">Day</skos:prefLabel>
      <skos:definition xml:lang="en">Integer-valued day, e.g., 24.</skos:definition>
      <skos:prefLabel xml:lang="da">Dag</skos:prefLabel>
      <skos:definition xml:lang="da">Heltalsværdi dag, f.eks. 24.</skos:definition>
      <skos:prefLabel xml:lang="no">Dag</skos:prefLabel>
      <skos:definition xml:lang="no">Heltall verdi dag, f.eks., 24.</skos:definition>
   </rdf:Description>
   <rdf:Description rdf:about="http://rdf-vocabulary.ddialliance.org/cv/DataType/1.1/d11e839">
      <rdf:type rdf:resource="http://www.w3.org/2004/02/skos/core#Concept"/>
      <skos:inScheme rdf:resource="http://rdf-vocabulary.ddialliance.org/cv/DataType/1.1/"/>
      <skos:notation>GMonth</skos:notation>
      <skos:prefLabel xml:lang="en">Month</skos:prefLabel>
      <skos:definition xml:lang="en">Integer-valued month, e.g., 03.</skos:definition>
      <skos:prefLabel xml:lang="da">Måned</skos:prefLabel>
      <skos:definition xml:lang="da">Heltalsværdi måned, f.eks. 03.</skos:definition>
      <skos:prefLabel xml:lang="no">Måned</skos:prefLabel>
      <skos:definition xml:lang="no">Heltall verdi, f.eks., 03.</skos:definition>
   </rdf:Description>
   <rdf:Description rdf:about="http://rdf-vocabulary.ddialliance.org/cv/DataType/1.1/d11e867">
      <rdf:type rdf:resource="http://www.w3.org/2004/02/skos/core#Concept"/>
      <skos:inScheme rdf:resource="http://rdf-vocabulary.ddialliance.org/cv/DataType/1.1/"/>
      <skos:notation>Duration</skos:notation>
      <skos:prefLabel xml:lang="en">Duration</skos:prefLabel>
      <skos:definition xml:lang="en">A duration of time. The value space of "duration" is a six-dimensional space in which the coordinates designate the Gregorian year, month, day, hour, minute, and second components as defined in ISO 8601. These components are ordered in their significance by their order of appearance as year, month, day, hour, minute, and second. The lexical representation of duration is the extended format PnYnMnDTnHnMnS, where P is the flag for duration (i.e., Period) and is constant, nY represents the number of years, nM the number of months, nD the number of days, T is the date/time separator, nH the number of hours, nM the number of minutes and nS the number of seconds. The number of seconds can include decimal digits to arbitrary precision. For example, to indicate a duration of 1 year, 2 months, 3 days, 10 hours, and 30 minutes, one would write: "P1Y2M3DT10H30M." An optional preceding minus sign ("-") is allowed, to indicate a negative duration: a duration of minus 120 days would be indicated as: "-P120D" (from: http://www.w3.org/TR/xmlschema-2/#duration).</skos:definition>
      <skos:prefLabel xml:lang="da">Varighed</skos:prefLabel>
      <skos:definition xml:lang="da">En varighed af tid. Værdirummet for "varighed" er et seksdimensionelt rum, hvor koordinaterne udpeger det gregorianske år, måned, dag, time, minut og sekund som komponenter defineret i ISO 8601. Disse komponenter er ordnet i deres betydning efter deres rækkefølge af fremkomst som år, måned, dag, time, minut og sekund. Den leksikale repræsentation af varighed er det udvidede format PnYnMnDTnHnMnS, hvor P er flaget for varighed (dvs. periode) og er konstant, nY repræsenterer antallet af år, nM antallet af måneder, nD antallet af dage, T er dato/tid-separatør, nH antallet af timer, nM antallet af minutter og nS antallet af sekunder. Antallet af sekunder kan indeholde decimaltal til vilkårlig præcision. For at angive en varighed, for eksempel, på 1 år, 2 måneder, 3 dage, 10 timer og 30 minutes ville man skrive: "P1Y2M3DT10H30M." Et valgfrit forudgående minustegn ("-") er tilladt for at angive en negativ varighed: en varighed af minus 120 dage ville angives som: "-P120D" (fra: http://www.w3.org/TR/xmlschema-2/#duration).</skos:definition>
      <skos:prefLabel xml:lang="no">Varighet</skos:prefLabel>
      <skos:definition xml:lang="no">En varighet av tid. Verdirekkevidden til "varighet" er i seks dimensjoner som koordinerer det Gregorianske år, måned, dag, time, minutt og sekund komponenter som er definert i ISO 8601. Disse komponentene er arrangert etter signifikans gjennom rekkefølgen år, måned, dag, time, minutt og sekund. Den leksikalske representasjonen av varighet er i det utvidede formatet PnYnMnDTnHnMnS, hvor P er flagget for varighet (i.e., Period) og er konstant, nY representerer antall
år, nM antall måneder, nD antall dager, T er dato/tid skilletegn, nH antall timer, nM antall minutter og nS antall sekunder. Antallet sekunder kan inkludere desimaltall til skjønnsmessig presisjon. For eksempel, for å indikere en varighet på 1 år, 2 måneder, 3 dager, 10 timer og 30 minutter kan en skrive: "P1Y2M3T10H30M." En valgfri foranledende minustegn ("-") er tillatt, for å indikere negativ varighet: en varighet på minus 120 dager vil bli indikert som "-P120D" (fra: http://www.w3.org/TR/xmlschema-2/#duration).</skos:definition>
   </rdf:Description>
   <rdf:Description rdf:about="http://rdf-vocabulary.ddialliance.org/cv/DataType/1.1/d11e896">
      <rdf:type rdf:resource="http://www.w3.org/2004/02/skos/core#Concept"/>
      <skos:inScheme rdf:resource="http://rdf-vocabulary.ddialliance.org/cv/DataType/1.1/"/>
      <skos:notation>HexBinary</skos:notation>
      <skos:prefLabel xml:lang="en">hexBinary</skos:prefLabel>
      <skos:definition xml:lang="en">Even-lengthed sequence of hexadecimal digits representing an N times 8-bit integer.</skos:definition>
      <skos:prefLabel xml:lang="da">hexBinary</skos:prefLabel>
      <skos:definition xml:lang="da">Sekvens af jævn længde af hexadecimale cifre, der repræsenterer et N-gange 8-bit heltal.</skos:definition>
      <skos:prefLabel xml:lang="no">hexBinary</skos:prefLabel>
      <skos:definition xml:lang="no">Jevnlange sekvenser av heksadesimal sifre som representerer et N ganger 8-bit heltall.</skos:definition>
   </rdf:Description>
   <rdf:Description rdf:about="http://rdf-vocabulary.ddialliance.org/cv/DataType/1.1/d11e924">
      <rdf:type rdf:resource="http://www.w3.org/2004/02/skos/core#Concept"/>
      <skos:inScheme rdf:resource="http://rdf-vocabulary.ddialliance.org/cv/DataType/1.1/"/>
      <skos:notation>Base64Binary</skos:notation>
      <skos:prefLabel xml:lang="en">base64Binary</skos:prefLabel>
      <skos:definition xml:lang="en">Sequence of multiples of four base64 digits, where each 4-tuple represents a 24-bit integer. Each digit (a-z, A-Z, 0-9, +, /) represents a 6-bit integer between 0 and 63.</skos:definition>
      <skos:prefLabel xml:lang="da">base64Binary</skos:prefLabel>
      <skos:definition xml:lang="da">Sekvenser af multipler af fire base64 cifre, hvor hver 4-tuple repræsenterer et 24-bit heltal. Hvert ciffer (a-z, A-Z, 0-9, +, /) repræsenterer et 6-bit heltal mellem 0 og 63.</skos:definition>
      <skos:prefLabel xml:lang="no">base64Binary</skos:prefLabel>
      <skos:definition xml:lang="no">Sekvens av multipler av fire base64 sifre, hvor hver 4-tuppel representerer et 24-bit heltall. Hvert siffer (a-z, A-Z, 0-9, +, /) representerer et 6-bit heltall mellom 0 og 63.</skos:definition>
   </rdf:Description>
   <rdf:Description rdf:about="http://rdf-vocabulary.ddialliance.org/cv/DataType/1.1/d11e952">
      <rdf:type rdf:resource="http://www.w3.org/2004/02/skos/core#Concept"/>
      <skos:inScheme rdf:resource="http://rdf-vocabulary.ddialliance.org/cv/DataType/1.1/"/>
      <skos:notation>AnyURI</skos:notation>
      <skos:prefLabel xml:lang="en">anyURI</skos:prefLabel>
      <skos:definition xml:lang="en">A Uniform Resource Identifier such as ftp, http or mailto, e.g., http://www.w3.org/TR/xmlschema-2.</skos:definition>
      <skos:prefLabel xml:lang="da">anyURI</skos:prefLabel>
      <skos:definition xml:lang="da">En Uniform Resource Identifier such as ftp, http eller mailto, for eksempel http://www.w3.org/TR/xmlschema-2.</skos:definition>
      <skos:prefLabel xml:lang="no">anyURI</skos:prefLabel>
      <skos:definition xml:lang="no">En Uniform Resource Identifier som ftp, http eller mailto, f.eks., http://www.w3.org/TR/xmlschema-2.</skos:definition>
   </rdf:Description>
   <rdf:Description rdf:about="http://rdf-vocabulary.ddialliance.org/cv/DataType/1.1/d11e980">
      <rdf:type rdf:resource="http://www.w3.org/2004/02/skos/core#Concept"/>
      <skos:inScheme rdf:resource="http://rdf-vocabulary.ddialliance.org/cv/DataType/1.1/"/>
      <skos:notation>Other</skos:notation>
      <skos:prefLabel xml:lang="en">Other</skos:prefLabel>
      <skos:definition xml:lang="en">Use if the data type is known, but not found in the list.</skos:definition>
      <skos:prefLabel xml:lang="da">Andet</skos:prefLabel>
      <skos:definition xml:lang="da">Anvend, hvis datatypen er kendt, men ikke findes på listen.</skos:definition>
      <skos:prefLabel xml:lang="no">Annet</skos:prefLabel>
      <skos:definition xml:lang="no">Bruk hvis datatypen er kjent, men ikke er på listen.</skos:definition>
   </rdf:Description>
</rdf:RDF>
