<?xml version="1.0" encoding="UTF-8"?>
<rdf:RDF xmlns:dcterms="http://purl.org/dc/terms/"
          xmlns:owl="http://www.w3.org/2002/07/owl#"
          xmlns:rdf="http://www.w3.org/1999/02/22-rdf-syntax-ns#"
          xmlns:rdfs="http://www.w3.org/2000/01/rdf-schema#"
          xmlns:skos="http://www.w3.org/2004/02/skos/core#">
   <rdf:Description rdf:about="http://rdf-vocabulary.ddialliance.org/cv/SummaryStatisticType/2.1">
      <rdf:type rdf:resource="http://www.w3.org/2004/02/skos/core#ConceptScheme"/>
      <dcterms:isVersionOf rdf:resource="http://rdf-vocabulary.ddialliance.org/cv/SummaryStatisticType"/>
      <skos:notation>SummaryStatisticType</skos:notation>
      <skos:prefLabel xml:lang="en">Summary Statistic Type</skos:prefLabel>
      <skos:prefLabel xml:lang="da">Typen af sammenfattende statistik</skos:prefLabel>
      <skos:prefLabel xml:lang="fi">Tilastollisen tunnusluvun tyyppi</skos:prefLabel>
      <skos:prefLabel xml:lang="it">Tipo di statistiche riassuntive</skos:prefLabel>
      <skos:prefLabel xml:lang="nl">Type samenvattende statistieken</skos:prefLabel>
      <skos:prefLabel xml:lang="no">Oppsummerende statistikk type</skos:prefLabel>
      <skos:prefLabel xml:lang="pt">Tipo de estatística sumária</skos:prefLabel>
      <skos:prefLabel xml:lang="sl">Vrsta zbirne statistike</skos:prefLabel>
      <skos:prefLabel xml:lang="sr">Vrsta zbirne statistike</skos:prefLabel>
      <skos:prefLabel xml:lang="sv">Typ av sammanfattande statistik</skos:prefLabel>
      <skos:definition xml:lang="en">Specifies the type of summary statistic. Summary statistics are a single number representation of the characteristics of a set of values.</skos:definition>
      <skos:definition xml:lang="da">Specificerer typen af sammenfattende statistik. Sammenfattende statistik er en repræsentation af et sæt af værdiers karakteristika ved hjælp af et enkelt tal.</skos:definition>
      <skos:definition xml:lang="fi">Tilastolliset tunnusluvut kuvaavat tietyn arvojoukon, esimerkiksi otoksen havaintojen sisältämää informaatiota. Usein tunnusluvut ovat nimensä mukaisesti yksittäisiä lukuja.</skos:definition>
      <skos:definition xml:lang="it">Specifica il tipo di statistica riassuntiva. Tali statistiche sono una rappresentazione sintetica delle caratteristiche di un insieme di valori.</skos:definition>
      <skos:definition xml:lang="nl">Beschrijft het type samenvattende statistieken. Samenvattende statistieken worden gebruikt om een ​​reeks waarnemingen samen te vatten in een getal.</skos:definition>
      <skos:definition xml:lang="no">Spesifiserer typen av oppsummerende statistikk. Oppsummerende statisitkk er en representasjon av et sett verdiers karakteristika representert ved et enkelt tall.</skos:definition>
      <skos:definition xml:lang="pt">Especifica o tipo de estatística sumária. As estatísticas sumárias são medidas/números/valores usados para descrever as características de um conjunto de dados.</skos:definition>
      <skos:definition xml:lang="sl">Določa vrsto zbirne statistike. Zbirna statistika je številka, s katero predstavimo značilnosti niza vrednosti.</skos:definition>
      <skos:definition xml:lang="sr">Određuje vrstu zbirne statistike. Zbirna statistika predstavlja jednoznačan broj karakteristika skupa vrednosti. </skos:definition>
      <skos:definition xml:lang="sv">Anger typ av sammanfattande statistik. Sammanfattande statistik är ett enda värde som representerar egenskaperna hos en mängd värden.</skos:definition>
      <owl:versionInfo>2.1</owl:versionInfo>
      <dcterms:license rdf:resource="Creative Commons Attribution 4.0 International"/>
      <dcterms:rights>Copyright ©DDI Alliance 2019</dcterms:rights>
      <skos:hasTopConcept rdf:resource="http://rdf-vocabulary.ddialliance.org/cv/SummaryStatisticType/2.1/d40e177"/>
      <skos:hasTopConcept rdf:resource="http://rdf-vocabulary.ddialliance.org/cv/SummaryStatisticType/2.1/d40e248"/>
      <skos:hasTopConcept rdf:resource="http://rdf-vocabulary.ddialliance.org/cv/SummaryStatisticType/2.1/d40e319"/>
      <skos:hasTopConcept rdf:resource="http://rdf-vocabulary.ddialliance.org/cv/SummaryStatisticType/2.1/d40e390"/>
      <skos:hasTopConcept rdf:resource="http://rdf-vocabulary.ddialliance.org/cv/SummaryStatisticType/2.1/d40e462"/>
      <skos:hasTopConcept rdf:resource="http://rdf-vocabulary.ddialliance.org/cv/SummaryStatisticType/2.1/d40e533"/>
      <skos:hasTopConcept rdf:resource="http://rdf-vocabulary.ddialliance.org/cv/SummaryStatisticType/2.1/d40e604"/>
      <skos:hasTopConcept rdf:resource="http://rdf-vocabulary.ddialliance.org/cv/SummaryStatisticType/2.1/d40e675"/>
      <skos:hasTopConcept rdf:resource="http://rdf-vocabulary.ddialliance.org/cv/SummaryStatisticType/2.1/d40e746"/>
      <skos:hasTopConcept rdf:resource="http://rdf-vocabulary.ddialliance.org/cv/SummaryStatisticType/2.1/d40e817"/>
      <skos:hasTopConcept rdf:resource="http://rdf-vocabulary.ddialliance.org/cv/SummaryStatisticType/2.1/d40e889"/>
      <skos:hasTopConcept rdf:resource="http://rdf-vocabulary.ddialliance.org/cv/SummaryStatisticType/2.1/d40e960"/>
      <skos:hasTopConcept rdf:resource="http://rdf-vocabulary.ddialliance.org/cv/SummaryStatisticType/2.1/d40e1031"/>
      <skos:hasTopConcept rdf:resource="http://rdf-vocabulary.ddialliance.org/cv/SummaryStatisticType/2.1/d40e1102"/>
      <skos:hasTopConcept rdf:resource="http://rdf-vocabulary.ddialliance.org/cv/SummaryStatisticType/2.1/d40e1173"/>
      <skos:hasTopConcept rdf:resource="http://rdf-vocabulary.ddialliance.org/cv/SummaryStatisticType/2.1/d40e1244"/>
      <skos:hasTopConcept rdf:resource="http://rdf-vocabulary.ddialliance.org/cv/SummaryStatisticType/2.1/d40e1316"/>
      <skos:hasTopConcept rdf:resource="http://rdf-vocabulary.ddialliance.org/cv/SummaryStatisticType/2.1/d40e1387"/>
      <skos:hasTopConcept rdf:resource="http://rdf-vocabulary.ddialliance.org/cv/SummaryStatisticType/2.1/d40e1458"/>
      <skos:hasTopConcept rdf:resource="http://rdf-vocabulary.ddialliance.org/cv/SummaryStatisticType/2.1/d40e1529"/>
      <skos:hasTopConcept rdf:resource="http://rdf-vocabulary.ddialliance.org/cv/SummaryStatisticType/2.1/d40e1600"/>
      <skos:hasTopConcept rdf:resource="http://rdf-vocabulary.ddialliance.org/cv/SummaryStatisticType/2.1/d40e1671"/>
      <skos:hasTopConcept rdf:resource="http://rdf-vocabulary.ddialliance.org/cv/SummaryStatisticType/2.1/d40e1743"/>
      <skos:hasTopConcept rdf:resource="http://rdf-vocabulary.ddialliance.org/cv/SummaryStatisticType/2.1/d40e1814"/>
      <skos:hasTopConcept rdf:resource="http://rdf-vocabulary.ddialliance.org/cv/SummaryStatisticType/2.1/d40e1885"/>
      <skos:hasTopConcept rdf:resource="http://rdf-vocabulary.ddialliance.org/cv/SummaryStatisticType/2.1/d40e1956"/>
      <skos:hasTopConcept rdf:resource="http://rdf-vocabulary.ddialliance.org/cv/SummaryStatisticType/2.1/d40e2027"/>
      <skos:hasTopConcept rdf:resource="http://rdf-vocabulary.ddialliance.org/cv/SummaryStatisticType/2.1/d40e2098"/>
      <skos:hasTopConcept rdf:resource="http://rdf-vocabulary.ddialliance.org/cv/SummaryStatisticType/2.1/d40e2170"/>
      <skos:hasTopConcept rdf:resource="http://rdf-vocabulary.ddialliance.org/cv/SummaryStatisticType/2.1/d40e2241"/>
      <skos:hasTopConcept rdf:resource="http://rdf-vocabulary.ddialliance.org/cv/SummaryStatisticType/2.1/d40e2312"/>
      <skos:hasTopConcept rdf:resource="http://rdf-vocabulary.ddialliance.org/cv/SummaryStatisticType/2.1/d40e2383"/>
      <skos:hasTopConcept rdf:resource="http://rdf-vocabulary.ddialliance.org/cv/SummaryStatisticType/2.1/d40e2454"/>
      <skos:hasTopConcept rdf:resource="http://rdf-vocabulary.ddialliance.org/cv/SummaryStatisticType/2.1/d40e2525"/>
      <skos:hasTopConcept rdf:resource="http://rdf-vocabulary.ddialliance.org/cv/SummaryStatisticType/2.1/d40e2597"/>
      <skos:hasTopConcept rdf:resource="http://rdf-vocabulary.ddialliance.org/cv/SummaryStatisticType/2.1/d40e2668"/>
      <skos:hasTopConcept rdf:resource="http://rdf-vocabulary.ddialliance.org/cv/SummaryStatisticType/2.1/d40e2739"/>
      <skos:hasTopConcept rdf:resource="http://rdf-vocabulary.ddialliance.org/cv/SummaryStatisticType/2.1/d40e2810"/>
      <skos:hasTopConcept rdf:resource="http://rdf-vocabulary.ddialliance.org/cv/SummaryStatisticType/2.1/d40e2881"/>
      <skos:hasTopConcept rdf:resource="http://rdf-vocabulary.ddialliance.org/cv/SummaryStatisticType/2.1/d40e2952"/>
      <skos:hasTopConcept rdf:resource="http://rdf-vocabulary.ddialliance.org/cv/SummaryStatisticType/2.1/d40e3024"/>
      <skos:hasTopConcept rdf:resource="http://rdf-vocabulary.ddialliance.org/cv/SummaryStatisticType/2.1/d40e3095"/>
      <skos:hasTopConcept rdf:resource="http://rdf-vocabulary.ddialliance.org/cv/SummaryStatisticType/2.1/d40e3166"/>
      <skos:hasTopConcept rdf:resource="http://rdf-vocabulary.ddialliance.org/cv/SummaryStatisticType/2.1/d40e3237"/>
   </rdf:Description>
   <rdf:Description rdf:about="http://rdf-vocabulary.ddialliance.org/cv/SummaryStatisticType/2.1/d40e177">
      <rdf:type rdf:resource="http://www.w3.org/2004/02/skos/core#Concept"/>
      <skos:inScheme rdf:resource="http://rdf-vocabulary.ddialliance.org/cv/SummaryStatisticType/2.1"/>
      <skos:notation>ArithmeticMean</skos:notation>
      <skos:prefLabel xml:lang="en">Arithmetic mean</skos:prefLabel>
      <skos:definition xml:lang="en">Mathematical average of a set of values. The mean is calculated by adding up two or more values and dividing the total by their number. In social/political science, it is usually the sum of the measurements divided by the number of subjects, or cases.</skos:definition>
      <skos:prefLabel xml:lang="da">Aritmetisk gennemsnit</skos:prefLabel>
      <skos:definition xml:lang="da">Matematisk gennemsnit af et sæt af værdier. Gennemsnittet beregnes ved at sammenlægge to eller flere værdier og dividere summen med antallet af værdier. I samfundsvidenskab er det normalt summen af målingerne divideret med antallet af subjekter eller cases.</skos:definition>
      <skos:prefLabel xml:lang="fi">Aritmeettinen keskiarvo</skos:prefLabel>
      <skos:definition xml:lang="fi">Arvojen matemaattinen keskiarvo. Keskiarvo lasketaan laskemalla kaksi tai useampi arvo yhteen ja jakamalla saatu summa arvojen määrällä. Yhteiskuntatieteissä keskiarvo on yleensä mittaustulosten summa jaettuna vastaajien/tapausten määrällä.</skos:definition>
      <skos:prefLabel xml:lang="it">Media aritmetica</skos:prefLabel>
      <skos:definition xml:lang="it">Media matematica di un insieme di valori. La media è calcolata sommando tutti i  valori e dividendo la somma per il loro numero. Nell'ambito delle scienze sociali/politiche identifica il valore medio della misura (ad esempio la somma dei punteggi diviso il numero di unità per cui il punteggio è disponibile).</skos:definition>
      <skos:prefLabel xml:lang="nl">Rekenkundig gemiddelde</skos:prefLabel>
      <skos:definition xml:lang="nl"/>
      <skos:prefLabel xml:lang="no">Aritmetisk gjennomsnitt</skos:prefLabel>
      <skos:definition xml:lang="no">Matematisk gjennomsnitt av et sett av verdier. Gjennomsnittet beregnes ved å legge sammen to eller flere verdier, og dele summen på antallet verdier. I samfunns-/statsvitenskap er det vanligvis summen av målingene delt på antall enheter eller tilfeller.</skos:definition>
      <skos:prefLabel xml:lang="pt">Média aritmética</skos:prefLabel>
      <skos:definition xml:lang="pt">Média matemática de um conjunto de valores. A média é calculada por meio da soma de dois ou mais valores, dividindo o total pelo seu número. Nas ciências sociais e políticas, geralmente é a soma das observações dividida pelo número de sujeitos, ou casos.</skos:definition>
      <skos:prefLabel xml:lang="sl">Aritmetična sredina</skos:prefLabel>
      <skos:definition xml:lang="sl">Matematično povprečje množice vrednosti. Aritmetična sredina se izračuna tako, da se vsota dveh ali več vrednosti deli s številom vrednosti. V družbslovju/ politiologiji je običajno vsota meritev, deljena s številom udeležencev oziroma enot.</skos:definition>
      <skos:prefLabel xml:lang="sr">Aritmetička sredina</skos:prefLabel>
      <skos:definition xml:lang="sr">Aritmetička sredina, srednja vrednost ili prosek je mera centralne tendencija skupa ili uzorka. Srednja vrednost izračunava se sabiranjem dve ili više vrednosti i deljenjem dobijenog zbira sa brojem elemenata u skupu ili uzorku. U društvenim naukama to je obično zbir mera (npr. visina plate ili visina učenika) podeljen sa brojem predmeta ili slučajeva (npr. broj zaposlenih, broj učenika).</skos:definition>
      <skos:prefLabel xml:lang="sv">Aritmetiskt medelvärde</skos:prefLabel>
      <skos:definition xml:lang="sv">Det matematiska medelvärdet av en uppsättning värden. Medelvärdet beräknas genom att addera två eller flera värden och dividera summan med antalet värden. I samhällsvetenskap är det oftast summan av mätningarna dividerat med antalet subjekt eller fall.</skos:definition>
   </rdf:Description>
   <rdf:Description rdf:about="http://rdf-vocabulary.ddialliance.org/cv/SummaryStatisticType/2.1/d40e248">
      <rdf:type rdf:resource="http://www.w3.org/2004/02/skos/core#Concept"/>
      <skos:inScheme rdf:resource="http://rdf-vocabulary.ddialliance.org/cv/SummaryStatisticType/2.1"/>
      <skos:notation>GeometricMean</skos:notation>
      <skos:prefLabel xml:lang="en">Geometric mean</skos:prefLabel>
      <skos:definition xml:lang="en">Average value of all data if extracting the nth root of the product of all (n) values. Rarely used in social sciences.</skos:definition>
      <skos:prefLabel xml:lang="da">Geometrisk gennemsnit</skos:prefLabel>
      <skos:definition xml:lang="da">Gennemsnitsværdien af alle data, hvis n’te rod tages af produktet af alle (n) værdier. Anvendes sjældent i samfundsvidenskab.</skos:definition>
      <skos:prefLabel xml:lang="fi">Geometrinen keskiarvo</skos:prefLabel>
      <skos:definition xml:lang="fi">Keskiluku, jossa otetaan n. juuri kaikkien (n) arvojen tulosta. Käytetään harvoin yhteiskuntatieteissä.</skos:definition>
      <skos:prefLabel xml:lang="it">Media geometrica</skos:prefLabel>
      <skos:definition xml:lang="it">Valore medio di tutti i dati se si estrae l'ennesima radice del prodotto di tutti i valori (n). Utilizzata raramente nelle scienze sociali.</skos:definition>
      <skos:prefLabel xml:lang="nl">Meetkundig gemiddelde</skos:prefLabel>
      <skos:definition xml:lang="nl"/>
      <skos:prefLabel xml:lang="no">Geometrisk gjennomsnitt</skos:prefLabel>
      <skos:definition xml:lang="no">Gjennomsnittsverdi for alle data når en finner den n-te rot til alle (n) verdiene. Sjeldent brukt i samfunnsfag.</skos:definition>
      <skos:prefLabel xml:lang="pt">Média geométrica</skos:prefLabel>
      <skos:definition xml:lang="pt">Valor médio de todos os dados, extraindo a raiz n-ésima do produto de todos (n) os elementos. Raramente é usada nas ciências sociais.</skos:definition>
      <skos:prefLabel xml:lang="sl">Geometrijska sredina</skos:prefLabel>
      <skos:definition xml:lang="sl">Povprečna vrednost vseh podatkov, če izpeljemo n-ti koren zmnožka vseh (n) vrednosti. V družboslovju se redko uporablja.</skos:definition>
      <skos:prefLabel xml:lang="sr">Geometrijska sredina</skos:prefLabel>
      <skos:definition xml:lang="sr">Geometrijska sredina je mera centralne tendencije koja se računa kao n-ti koren proizvoda svih elemenata skupa podataka. Retko se koristi u društvenim naukama.</skos:definition>
      <skos:prefLabel xml:lang="sv">Geometriskt medelvärde</skos:prefLabel>
      <skos:definition xml:lang="sv">Medelvärdet av samtliga värden som man får genom att ta den n:te roten av produkten av alla (n) värden. Används sällan inom samhällsvetenskap.</skos:definition>
   </rdf:Description>
   <rdf:Description rdf:about="http://rdf-vocabulary.ddialliance.org/cv/SummaryStatisticType/2.1/d40e319">
      <rdf:type rdf:resource="http://www.w3.org/2004/02/skos/core#Concept"/>
      <skos:inScheme rdf:resource="http://rdf-vocabulary.ddialliance.org/cv/SummaryStatisticType/2.1"/>
      <skos:notation>HarmonicMean</skos:notation>
      <skos:prefLabel xml:lang="en">Harmonic mean</skos:prefLabel>
      <skos:definition xml:lang="en">Average value of all data if calculating the reciprocal of the arithmetic mean of the reciprocal of values. Rarely used in social sciences.</skos:definition>
      <skos:prefLabel xml:lang="da">Harmonisk gennemsnit</skos:prefLabel>
      <skos:definition xml:lang="da">Gennemsnitlig værdi af alle data ved beregning af den reciprokke af det aritmetiske gennemsnit af den reciprokke af værdier. Anvendes sjældent i samfundsvidenskab.</skos:definition>
      <skos:prefLabel xml:lang="fi">Harmoninen keskiarvo</skos:prefLabel>
      <skos:definition xml:lang="fi">Keskiluku, jossa lasketaan arvojen käänteislukujen aritmeettisen keskiarvon käänteisluku. Käytetään harvoin yhteiskuntatieteissä.</skos:definition>
      <skos:prefLabel xml:lang="it">Media armonica</skos:prefLabel>
      <skos:definition xml:lang="it">Valore medio di tutti i dati se si calcola il reciproco della media aritmetica del reciproco dei valori. Utilizzata raramente nelle scienze sociali.</skos:definition>
      <skos:prefLabel xml:lang="nl">Harmonisch gemiddelde</skos:prefLabel>
      <skos:definition xml:lang="nl"/>
      <skos:prefLabel xml:lang="no">Harmonisk gjennomsnitt</skos:prefLabel>
      <skos:definition xml:lang="no">Gjennomsnittsverdi av alle data hvis man beregener det tilsvarende av det aritmetiske gjennomsnittet av tilsvarende verdier. Sjelden brukt i samfunnsvitenskap.</skos:definition>
      <skos:prefLabel xml:lang="pt">Média harmónica (ou média subcontrária)</skos:prefLabel>
      <skos:definition xml:lang="pt">Valor médio de todos os dados calculado como a razão entre o número de elementos e a soma do inverso desses elementos, ou seja, como a recíproca da média aritmética dos recíprocos dos valores. Raramente é usada nas ciências sociais.</skos:definition>
      <skos:prefLabel xml:lang="sl">Harmonična sredina</skos:prefLabel>
      <skos:definition xml:lang="sl">Povprečna vrednost vseh podatkov, če izračunamo obratno vrednost aritmetične sredine obratnih vrednosti. V družboslovju se redko uporablja.</skos:definition>
      <skos:prefLabel xml:lang="sr">Harmonijska sredina</skos:prefLabel>
      <skos:definition xml:lang="sr">Harmonijska sredina je recipročna vrednost aritmetičke sredine recipročnih vrednosti skupa elemenata.</skos:definition>
      <skos:prefLabel xml:lang="sv">Harmoniskt medelvärde</skos:prefLabel>
      <skos:definition xml:lang="sv">Medelvärdet av samtliga värden som fås genom att beräkna det inverterade aritmetiska medelvärdet av summan av alla inverterade värden. Används sällan inom samhällsvetenskap.</skos:definition>
   </rdf:Description>
   <rdf:Description rdf:about="http://rdf-vocabulary.ddialliance.org/cv/SummaryStatisticType/2.1/d40e390">
      <rdf:type rdf:resource="http://www.w3.org/2004/02/skos/core#Concept"/>
      <skos:inScheme rdf:resource="http://rdf-vocabulary.ddialliance.org/cv/SummaryStatisticType/2.1"/>
      <skos:notation>TrimmedMean</skos:notation>
      <skos:prefLabel xml:lang="en">Trimmed mean</skos:prefLabel>
      <skos:definition xml:lang="en">The (arithmetic) mean calculated after discarding given parts of observations at the high and low end (e.g., interquartile mean when the lowest 25% and the highest 25% are discarded, and the mean of the remaining values is calculated).</skos:definition>
      <skos:prefLabel xml:lang="da">Trimmet gennemsnit</skos:prefLabel>
      <skos:definition xml:lang="da">Det (aritmetiske) gennemsnit beregnet efter frasortering af givne observationer i den høje og den lave ende (fx interkvartil gennemsnit, når de laveste 25 % og de højeste 25 % er frasorteret, og gennemsnittet af de resterende værdier beregnes).</skos:definition>
      <skos:prefLabel xml:lang="fi">Leikattu keskiarvo</skos:prefLabel>
      <skos:definition xml:lang="fi">(Aritmeettinen) keskiarvo, joka lasketaan sen jälkeen, kun tietty osa havaintoarvoista on jätetty pois (leikattu) (esim. kvartiilivälin keskiarvo, jossa ylä- ja alakvartiileille eli ylimpään ja alimpaan 25 %:iin asettuvat havaintoarvot jätetään pois ja jäljelle jäävistä arvoista lasketaan keskiarvo).</skos:definition>
      <skos:prefLabel xml:lang="it">Media troncata</skos:prefLabel>
      <skos:definition xml:lang="it">La media (aritmetica) calcolata senza considerare parte delle osservazioni che nella sequenza ordinata si trovano  all'estremità  superiore e inferiore (ad esempio, la media interquartile è calcolata sulle osservazioni centrali della distribuzione ordinata eludendo il  25% di quelle più basse ed il 25% di quelle più alte).</skos:definition>
      <skos:prefLabel xml:lang="nl">Getrimd gemiddelde</skos:prefLabel>
      <skos:definition xml:lang="nl"/>
      <skos:prefLabel xml:lang="no">Trimmet gjennomsnitt</skos:prefLabel>
      <skos:definition xml:lang="no">Det (aritmetiske) gjennomsnittet beregnet etter å ha fjernet deler av observasjonene ved den høye og den lave enden (f.eks. interkvartilgjennomsnittet når de laveste 25% og de høyeste 25% fjernes, og gjennomsnittet av de gjenværende verdier beregnes).</skos:definition>
      <skos:prefLabel xml:lang="pt">Média aparada</skos:prefLabel>
      <skos:definition xml:lang="pt">A média (aritmética) calculada após excluir determinada percentagem dos valores mais altos e mais baixos (por exemplo, a média interquartil quando os 25% mais baixos e os 25% mais altos são descartados e a média dos valores restantes é calculada).</skos:definition>
      <skos:prefLabel xml:lang="sl">Modificirana aritemtična sredina</skos:prefLabel>
      <skos:definition xml:lang="sl">(Aritmetična) sredina, izračunana po odstranitvi najvišjih in najnižjih vrednosti opazovanj (npr. interkvartilna sredina, kjer odstranimo najnižjih 25% in najvišjih 25% vrednosti, nato pa izračunamo aritmetično sredino preostalih vrednosti).</skos:definition>
      <skos:prefLabel xml:lang="sr">Skraćena srednja vrednosti</skos:prefLabel>
      <skos:definition xml:lang="sr">(Aritmetička) srednja vrednost izračunata nakon odbacivanja ekstremnih vrednosti u skupu ili uzorku, tzv. autlajera (npr. Interkvartilna srednja vrednost kada se odbace najniža 25% i najviša 25%, a izračunava se srednja vrednost preostalih vrednosti).</skos:definition>
      <skos:prefLabel xml:lang="sv">Trunkerat medelvärde</skos:prefLabel>
      <skos:definition xml:lang="sv">Det aritmetiska medelvärdet beräknat efter att man tagit bort givna delar av de höga och låga observationerna (t.ex. medelvärdet för kvartilavståndet, när de lägsta 25 % och de högsta 25 % räknats bort och medelvärdet av de återstående värdena beräknas).</skos:definition>
   </rdf:Description>
   <rdf:Description rdf:about="http://rdf-vocabulary.ddialliance.org/cv/SummaryStatisticType/2.1/d40e462">
      <rdf:type rdf:resource="http://www.w3.org/2004/02/skos/core#Concept"/>
      <skos:inScheme rdf:resource="http://rdf-vocabulary.ddialliance.org/cv/SummaryStatisticType/2.1"/>
      <skos:notation>StandardErrorOfMean</skos:notation>
      <skos:prefLabel xml:lang="en">Standard error of the mean</skos:prefLabel>
      <skos:definition xml:lang="en">Provides an estimate of how much the sample mean differs from the actual mean of the population.</skos:definition>
      <skos:prefLabel xml:lang="da">Standardfejl for gennemsnittet</skos:prefLabel>
      <skos:definition xml:lang="da">Giver et estimate på, hvor meget stikprøvens gennemsnit afgiver fra populationens faktiske gennemsnit.</skos:definition>
      <skos:prefLabel xml:lang="fi">Keskiarvon keskivirhe</skos:prefLabel>
      <skos:definition xml:lang="fi">Antaa arvion siitä, kuinka paljon otoksesta saatu keskiarvo poikkeaa väestön tosiasiallisesta keskiarvosta.</skos:definition>
      <skos:prefLabel xml:lang="it">Errore standard della media</skos:prefLabel>
      <skos:definition xml:lang="it">Fornisce una stima di quanto la media campionaria differisce dalla media effettiva della popolazione.</skos:definition>
      <skos:prefLabel xml:lang="nl">Standaardfout</skos:prefLabel>
      <skos:definition xml:lang="nl"/>
      <skos:prefLabel xml:lang="no">Standardfeil for gjennomsnittet</skos:prefLabel>
      <skos:definition xml:lang="no">Gir et estimat av hvor mye utvalgets gjennomsnitt varierer fra det faktiske populasjonsgjennomsnittet.</skos:definition>
      <skos:prefLabel xml:lang="pt">Erro padrão da média</skos:prefLabel>
      <skos:definition xml:lang="pt">Fornece uma estimativa de quanto a média da amostra difere da média real da população.</skos:definition>
      <skos:prefLabel xml:lang="sl">Standardna napaka aritmetične sredine</skos:prefLabel>
      <skos:definition xml:lang="sl">Standardna napaka (aritmetične) sredine.</skos:definition>
      <skos:prefLabel xml:lang="sr">Standardna greška srednje vrednosti</skos:prefLabel>
      <skos:definition xml:lang="sr">Daje procenu koliko se prosečna vrednost uzorka razlikuje od stvarne prosečne vrednosti populacije.</skos:definition>
      <skos:prefLabel xml:lang="sv">Standardfel för medelvärdet</skos:prefLabel>
      <skos:definition xml:lang="sv">Ger en uppskattning av hur mycket medelvärdet för ett urval avviker från medelvärdet för hela populationen.</skos:definition>
   </rdf:Description>
   <rdf:Description rdf:about="http://rdf-vocabulary.ddialliance.org/cv/SummaryStatisticType/2.1/d40e533">
      <rdf:type rdf:resource="http://www.w3.org/2004/02/skos/core#Concept"/>
      <skos:inScheme rdf:resource="http://rdf-vocabulary.ddialliance.org/cv/SummaryStatisticType/2.1"/>
      <skos:notation>Mode</skos:notation>
      <skos:prefLabel xml:lang="en">Mode</skos:prefLabel>
      <skos:definition xml:lang="en">The most frequently observed data value (Statistics Canada).</skos:definition>
      <skos:prefLabel xml:lang="da">Modus</skos:prefLabel>
      <skos:definition xml:lang="da">Den hyppigst observerede dataværdi (Statistics Canada).</skos:definition>
      <skos:prefLabel xml:lang="fi">Moodi</skos:prefLabel>
      <skos:definition xml:lang="fi">Moodi ilmoittaa, mikä on muuttujan jakauman huippukohta eli eniten tapauksia sisältävä luokka (Tilastokeskus).</skos:definition>
      <skos:prefLabel xml:lang="it">Moda</skos:prefLabel>
      <skos:definition xml:lang="it">Valore a cui corrisponde la massima frequenza.</skos:definition>
      <skos:prefLabel xml:lang="nl">Modus</skos:prefLabel>
      <skos:definition xml:lang="nl"/>
      <skos:prefLabel xml:lang="no">Modus</skos:prefLabel>
      <skos:definition xml:lang="no">Verdien som er observert flest ganger.</skos:definition>
      <skos:prefLabel xml:lang="pt">Moda</skos:prefLabel>
      <skos:definition xml:lang="pt">O valor observado com mais frequência num conjunto de dados.</skos:definition>
      <skos:prefLabel xml:lang="sl">Modus (Mo)</skos:prefLabel>
      <skos:definition xml:lang="sl">Najpogosteje izmerjena vrednost podatkov (Statistics Canada).</skos:definition>
      <skos:prefLabel xml:lang="sr">Modus</skos:prefLabel>
      <skos:definition xml:lang="sr">Vrednost koja se u skupu ili uzorku najčešće pojavljuje.</skos:definition>
      <skos:prefLabel xml:lang="sv">Typvärde</skos:prefLabel>
      <skos:definition xml:lang="sv">Det mest frekvent observerade datavärdet.</skos:definition>
   </rdf:Description>
   <rdf:Description rdf:about="http://rdf-vocabulary.ddialliance.org/cv/SummaryStatisticType/2.1/d40e604">
      <rdf:type rdf:resource="http://www.w3.org/2004/02/skos/core#Concept"/>
      <skos:inScheme rdf:resource="http://rdf-vocabulary.ddialliance.org/cv/SummaryStatisticType/2.1"/>
      <skos:notation>Median</skos:notation>
      <skos:prefLabel xml:lang="en">Median</skos:prefLabel>
      <skos:definition xml:lang="en">The middle value in a set of values arranged in ascending order. Half of the values fall below the median, and half above it. If the set has an even number of values, the median will be the average of the two middle ones.</skos:definition>
      <skos:prefLabel xml:lang="da">Median</skos:prefLabel>
      <skos:definition xml:lang="da">Den midterste værdi i et sæt af værdier arrangeret i stigende rækkefølge. Halvdelen af værdier falder under medianen og halvdelen over den. Hvis sættet har et lige antal af værdier, vil medianen være gennemsnittet af de to midterste.</skos:definition>
      <skos:prefLabel xml:lang="fi">Mediaani</skos:prefLabel>
      <skos:definition xml:lang="fi">Jakauman keskimmäinen havaintoarvo, kun havainnot on järjestetty suuruusjärjestykseen (Tilastokeskus). Puolet jakauman arvoista sijoittuu mediaanin alle ja puolet sen ylle.</skos:definition>
      <skos:prefLabel xml:lang="it">Mediana</skos:prefLabel>
      <skos:definition xml:lang="it">Il valore medio di un insieme di valori disposti in ordine crescente. Metà dei valori si trova al di sotto della mediana e metà al di sopra di essa. Se l'insieme ha un numero pari di valori, la mediana sarà pari alla media dei due valori centrali.</skos:definition>
      <skos:prefLabel xml:lang="nl">Mediaan</skos:prefLabel>
      <skos:definition xml:lang="nl"/>
      <skos:prefLabel xml:lang="no">Median</skos:prefLabel>
      <skos:definition xml:lang="no">Midtverdien i et sett av verdier arrangert i stigende rekkefølge. Halvparten av verdiene er under medianen og halvparten over den. Hvis antallet verdier i settet er et partall vil medianen være gjennomsnittet av de to midterste verdiene.</skos:definition>
      <skos:prefLabel xml:lang="pt">Mediana</skos:prefLabel>
      <skos:definition xml:lang="pt">O valor do meio de um conjunto de dados organizado por ordem ascendente. Metade dos valores estão abaixo da mediana e a outra metade acima. Se o conjunto tiver um número par de valores, a mediana será a média dos dois valores do meio.</skos:definition>
      <skos:prefLabel xml:lang="sl">Mediana (Mdn)</skos:prefLabel>
      <skos:definition xml:lang="sl">Vrednosti, pod katerimi in nad katerimi je polovica vrednosti porazdelitve (50. percentil).</skos:definition>
      <skos:prefLabel xml:lang="sr">Medijana</skos:prefLabel>
      <skos:definition xml:lang="sr">Medijana razdvaja gornju polovinu skupa ili uzorka, od donje polovine, pri čemu vrednosti moraju biti raspoređene u rastućem nizu. Ukoliko skup ima parni broj vrednosti, središnja vrednost (medijana) će biti prosek dve središnje vrednosti.</skos:definition>
      <skos:prefLabel xml:lang="sv">Median</skos:prefLabel>
      <skos:definition xml:lang="sv">Värdena som ligger mellan övre och undre hälften av värdena i en fördelning (50: e percentilen).</skos:definition>
   </rdf:Description>
   <rdf:Description rdf:about="http://rdf-vocabulary.ddialliance.org/cv/SummaryStatisticType/2.1/d40e675">
      <rdf:type rdf:resource="http://www.w3.org/2004/02/skos/core#Concept"/>
      <skos:inScheme rdf:resource="http://rdf-vocabulary.ddialliance.org/cv/SummaryStatisticType/2.1"/>
      <skos:notation>ValidCases</skos:notation>
      <skos:prefLabel xml:lang="en">Valid cases</skos:prefLabel>
      <skos:definition xml:lang="en">Cases with observations which are considered to be valid, i.e., providing substantial information and to be included for calculation.</skos:definition>
      <skos:prefLabel xml:lang="da">Gyldige cases</skos:prefLabel>
      <skos:definition xml:lang="da">Cases med observationer, der betragtes som gyldige, dvs. giver substantiel information og inkluderes i beregning.</skos:definition>
      <skos:prefLabel xml:lang="fi">Validit havainnot</skos:prefLabel>
      <skos:definition xml:lang="fi">Havainnot, joiden katsotaan olevan valideja tai 'oikeita', eli ne tarjoavat olennaista tietoa ja sisällytetään analyyseihin.</skos:definition>
      <skos:prefLabel xml:lang="it">Casi validi</skos:prefLabel>
      <skos:definition xml:lang="it">Valori considerati ammissibili per lo studio, e che pertanto forniscono informazioni sostanziali nelle analisi dei dati.</skos:definition>
      <skos:prefLabel xml:lang="nl">Geldige gevallen</skos:prefLabel>
      <skos:definition xml:lang="nl"/>
      <skos:prefLabel xml:lang="no">Gyldige tilfeller</skos:prefLabel>
      <skos:definition xml:lang="no">Observerte tilfeller som er ansett for å være gyldige, dvs. gir vesentlig informasjon og skal inngå i beregninger.</skos:definition>
      <skos:prefLabel xml:lang="pt">Casos válidos</skos:prefLabel>
      <skos:definition xml:lang="pt">Casos com observações consideradas válidas, isto é, fornecendo informações substanciais e a serem incluídas nos cálculos.</skos:definition>
      <skos:prefLabel xml:lang="sl">Veljavne enote</skos:prefLabel>
      <skos:definition xml:lang="sl">Enote z opazovanji, ki jih štejemo za veljavne, npr. prinašajo bistvene informacije in jih vključimo v analizo.</skos:definition>
      <skos:prefLabel xml:lang="sr">Ispravni (validni) slučajevi</skos:prefLabel>
      <skos:definition xml:lang="sr">Slučajevi sa opservacijama za koja se smatra da su ispravni, tj. da daju značajne informacije i da mogu biti uključeni se u dalju analizu.</skos:definition>
      <skos:prefLabel xml:lang="sv">Giltiga fall</skos:prefLabel>
      <skos:definition xml:lang="sv">Fall med observationer som anses vara giltiga, dvs. ger betydande information och ska ingå i beräkningar.</skos:definition>
   </rdf:Description>
   <rdf:Description rdf:about="http://rdf-vocabulary.ddialliance.org/cv/SummaryStatisticType/2.1/d40e746">
      <rdf:type rdf:resource="http://www.w3.org/2004/02/skos/core#Concept"/>
      <skos:inScheme rdf:resource="http://rdf-vocabulary.ddialliance.org/cv/SummaryStatisticType/2.1"/>
      <skos:notation>InvalidCases</skos:notation>
      <skos:prefLabel xml:lang="en">Invalid cases</skos:prefLabel>
      <skos:definition xml:lang="en">Cases which are considered/defined as "missing" (e.g., not ascertained, not applicable, etc.), usually excluded from calculation.</skos:definition>
      <skos:prefLabel xml:lang="da">Ugyldige cases</skos:prefLabel>
      <skos:definition xml:lang="da">Cases, der betragtes/defineres som “manglende” (fx. ikke fastslået, ikke anvendelig etc.), som regel udeladt fra beregning.</skos:definition>
      <skos:prefLabel xml:lang="fi">Puuttuvat havainnot</skos:prefLabel>
      <skos:definition xml:lang="fi">Havainnot, joiden katsotaan olevan puuttuvia (esim. tyhjäksi jätetty vastaus, näppäilyvirhe jne.) ja jotka yleensä jätetään huomioimatta analyyseissä.</skos:definition>
      <skos:prefLabel xml:lang="it">Casi non validi</skos:prefLabel>
      <skos:definition xml:lang="it">Valori non considerati ammissibili per lo studio (ad esempio, non accertati, non applicabili, ecc.) e che pertanto vengono esclusi  nelle analisi dei dati.</skos:definition>
      <skos:prefLabel xml:lang="nl">Ongeldige gevallen</skos:prefLabel>
      <skos:definition xml:lang="nl"/>
      <skos:prefLabel xml:lang="no">Ugyldige tilfeller</skos:prefLabel>
      <skos:definition xml:lang="no">Observerte tilfeller som er ansett/definert som 'missing' (f.eks. ikke konstantert, ikke aktuelle etc.), vanligvis fjernet fra beregningene.</skos:definition>
      <skos:prefLabel xml:lang="pt">Casos inválidos</skos:prefLabel>
      <skos:definition xml:lang="pt">Casos considerados ou definidos como "missing values" (por exemplo, dados não apurados, não aplicáveis, etc.), geralmente excluídos dos cálculos.</skos:definition>
      <skos:prefLabel xml:lang="sl">Neveljavne enote</skos:prefLabel>
      <skos:definition xml:lang="sl">Enote, ki jih obravnavamo/opredelimo kot 'manjkajoče' (npr. niso določene, se ne uporabljajo, itd.), običajno so izključene iz analiz.</skos:definition>
      <skos:prefLabel xml:lang="sr">Neispravni (nevalidni) slučajevi</skos:prefLabel>
      <skos:definition xml:lang="sr">Slučajevi koji se smatraju / definišu kao "nedostajući" (npr. nisu utvrđeni, nisu primenljivi, itd.), najčešće se isključuju iz analize.</skos:definition>
      <skos:prefLabel xml:lang="sv">Ogiltiga fall</skos:prefLabel>
      <skos:definition xml:lang="sv">Fall som betraktas/definieras som "saknade" (t.ex. inte fastställda, inte tillämpliga osv.), vanligtvis uteslutna ur beräkningar.</skos:definition>
   </rdf:Description>
   <rdf:Description rdf:about="http://rdf-vocabulary.ddialliance.org/cv/SummaryStatisticType/2.1/d40e817">
      <rdf:type rdf:resource="http://www.w3.org/2004/02/skos/core#Concept"/>
      <skos:inScheme rdf:resource="http://rdf-vocabulary.ddialliance.org/cv/SummaryStatisticType/2.1"/>
      <skos:notation>Minimum</skos:notation>
      <skos:prefLabel xml:lang="en">Minimum</skos:prefLabel>
      <skos:definition xml:lang="en">The lowest valid value in a variable.</skos:definition>
      <skos:prefLabel xml:lang="da">Minimum</skos:prefLabel>
      <skos:definition xml:lang="da">Den lavest gyldige værdi i en variabel.</skos:definition>
      <skos:prefLabel xml:lang="fi">Minimi</skos:prefLabel>
      <skos:definition xml:lang="fi">Alin validi muuttujan arvo.</skos:definition>
      <skos:prefLabel xml:lang="it">Minimo</skos:prefLabel>
      <skos:definition xml:lang="it">Il valore valido più basso assunto da una variabile.</skos:definition>
      <skos:prefLabel xml:lang="nl">Minimum</skos:prefLabel>
      <skos:definition xml:lang="nl"/>
      <skos:prefLabel xml:lang="no">Minimum</skos:prefLabel>
      <skos:definition xml:lang="no">Den laveste gyldige verdien i en variabel.</skos:definition>
      <skos:prefLabel xml:lang="pt">Mínimo</skos:prefLabel>
      <skos:definition xml:lang="pt">O menor valor válido de uma variável.</skos:definition>
      <skos:prefLabel xml:lang="sl">Minimum</skos:prefLabel>
      <skos:definition xml:lang="sl">Najnižja veljavna vrednost spremenljivke.</skos:definition>
      <skos:prefLabel xml:lang="sr">Minimum</skos:prefLabel>
      <skos:definition xml:lang="sr">Najniža ispravna vrednost promenljive.</skos:definition>
      <skos:prefLabel xml:lang="sv">Minimum</skos:prefLabel>
      <skos:definition xml:lang="sv">Det lägsta giltiga värdet i en variabel.</skos:definition>
   </rdf:Description>
   <rdf:Description rdf:about="http://rdf-vocabulary.ddialliance.org/cv/SummaryStatisticType/2.1/d40e889">
      <rdf:type rdf:resource="http://www.w3.org/2004/02/skos/core#Concept"/>
      <skos:inScheme rdf:resource="http://rdf-vocabulary.ddialliance.org/cv/SummaryStatisticType/2.1"/>
      <skos:notation>Maximum</skos:notation>
      <skos:prefLabel xml:lang="en">Maximum</skos:prefLabel>
      <skos:definition xml:lang="en">The highest valid value in a variable.</skos:definition>
      <skos:prefLabel xml:lang="da">Maksimum</skos:prefLabel>
      <skos:definition xml:lang="da">Den højest gyldige værdi i en variabel.</skos:definition>
      <skos:prefLabel xml:lang="fi">Maksimi</skos:prefLabel>
      <skos:definition xml:lang="fi">Ylin validi muuttujan arvo.</skos:definition>
      <skos:prefLabel xml:lang="it">Massimo</skos:prefLabel>
      <skos:definition xml:lang="it">Il valore valido più alto assunto da una variabile.</skos:definition>
      <skos:prefLabel xml:lang="nl">Maximum</skos:prefLabel>
      <skos:definition xml:lang="nl"/>
      <skos:prefLabel xml:lang="no">Maksimum</skos:prefLabel>
      <skos:definition xml:lang="no">Den høyeste gyldige verdien i en variabel.</skos:definition>
      <skos:prefLabel xml:lang="pt">Máximo</skos:prefLabel>
      <skos:definition xml:lang="pt">O maior valor válido de uma variável.</skos:definition>
      <skos:prefLabel xml:lang="sl">Maksimum</skos:prefLabel>
      <skos:definition xml:lang="sl">Najvišja veljavna vrednost spremenljivke.</skos:definition>
      <skos:prefLabel xml:lang="sr">Maksimum</skos:prefLabel>
      <skos:definition xml:lang="sr">Najviša ispravna vrednost promenljive.</skos:definition>
      <skos:prefLabel xml:lang="sv">Maximum</skos:prefLabel>
      <skos:definition xml:lang="sv">Det högsta giltiga värdet i en variabel.</skos:definition>
   </rdf:Description>
   <rdf:Description rdf:about="http://rdf-vocabulary.ddialliance.org/cv/SummaryStatisticType/2.1/d40e960">
      <rdf:type rdf:resource="http://www.w3.org/2004/02/skos/core#Concept"/>
      <skos:inScheme rdf:resource="http://rdf-vocabulary.ddialliance.org/cv/SummaryStatisticType/2.1"/>
      <skos:notation>Range</skos:notation>
      <skos:prefLabel xml:lang="en">Range</skos:prefLabel>
      <skos:definition xml:lang="en">The range of valid values, i.e., all values that fall between the lowest and highest valid values.</skos:definition>
      <skos:prefLabel xml:lang="da">Variationsbredde</skos:prefLabel>
      <skos:definition xml:lang="da">Afstanden mellem gyldige værdier, dvs., alle værdier, der falder mellem de laveste og højeste gyldige værdier.</skos:definition>
      <skos:prefLabel xml:lang="fi">Vaihteluväli</skos:prefLabel>
      <skos:definition xml:lang="fi">Validien arvojen vaihteluväli, eli alimman ja ylimmän arvon väliin asettuvat arvot, ts. muuttujan suurimman ja pienimmän arvon välimatka.</skos:definition>
      <skos:prefLabel xml:lang="it">Intervallo</skos:prefLabel>
      <skos:definition xml:lang="it">L'intervallo di valori validi, ossia tutti i valori compresi tra il più basso e il più alto dei valori validi.</skos:definition>
      <skos:prefLabel xml:lang="nl">Bereik</skos:prefLabel>
      <skos:definition xml:lang="nl"/>
      <skos:prefLabel xml:lang="no">Variasjonsbredde</skos:prefLabel>
      <skos:definition xml:lang="no">Variasjonsbredden av gyldige verdier, dvs. alle verdier som befinner seg mellom den høyeste og laveste gyldige verdien.</skos:definition>
      <skos:prefLabel xml:lang="pt">Intervalo</skos:prefLabel>
      <skos:definition xml:lang="pt">O intervalo de valores válidos, ou seja, todos os valores que se encontram entre os valores válidos mais baixo e mais alto.</skos:definition>
      <skos:prefLabel xml:lang="sl">Rang</skos:prefLabel>
      <skos:definition xml:lang="sl">Razpon veljavnih vrednosti, to je vseh vrednosti med najnižjo in najvišjo veljavno vrednostjo.</skos:definition>
      <skos:prefLabel xml:lang="sr">Raspon / opseg</skos:prefLabel>
      <skos:definition xml:lang="sr">Raspon ispravnih vrednosti, tj. razlika između najviše i najniže vrednosti u skupu ili uzorku.</skos:definition>
      <skos:prefLabel xml:lang="sv">Variationsvidd</skos:prefLabel>
      <skos:definition xml:lang="sv">Variationsvidden av giltiga värden, dvs. alla värden som faller mellan det lägsta och det högsta giltiga värdet.</skos:definition>
   </rdf:Description>
   <rdf:Description rdf:about="http://rdf-vocabulary.ddialliance.org/cv/SummaryStatisticType/2.1/d40e1031">
      <rdf:type rdf:resource="http://www.w3.org/2004/02/skos/core#Concept"/>
      <skos:inScheme rdf:resource="http://rdf-vocabulary.ddialliance.org/cv/SummaryStatisticType/2.1"/>
      <skos:notation>Sum</skos:notation>
      <skos:prefLabel xml:lang="en">Sum</skos:prefLabel>
      <skos:definition xml:lang="en">The sum or total of the values, across all valid cases.</skos:definition>
      <skos:prefLabel xml:lang="da">Sum</skos:prefLabel>
      <skos:definition xml:lang="da">Summen af værdierne på tværs af alle gyldige cases.</skos:definition>
      <skos:prefLabel xml:lang="fi">Summa</skos:prefLabel>
      <skos:definition xml:lang="fi">Kaikkien validien havaintojen arvojen summa.</skos:definition>
      <skos:prefLabel xml:lang="it">Somma</skos:prefLabel>
      <skos:definition xml:lang="it">La somma o il totale dei valori di tutti i casi validi.</skos:definition>
      <skos:prefLabel xml:lang="nl">Som</skos:prefLabel>
      <skos:definition xml:lang="nl"/>
      <skos:prefLabel xml:lang="no">Sum</skos:prefLabel>
      <skos:definition xml:lang="no">Summen eller totalen av verdiene på tvers av alle gyldige tilfeller.</skos:definition>
      <skos:prefLabel xml:lang="pt">Soma</skos:prefLabel>
      <skos:definition xml:lang="pt">A soma ou o total dos valores, considerando os casos válidos.</skos:definition>
      <skos:prefLabel xml:lang="sl">Vsota</skos:prefLabel>
      <skos:definition xml:lang="sl">Vsota vrednosti na vseh veljavnih enotah.</skos:definition>
      <skos:prefLabel xml:lang="sr">Zbir</skos:prefLabel>
      <skos:definition xml:lang="sr">Zbir ili ukupna vrednost svih vrednosti ispravnih (validnih) elemenata skupa ili uzroka.</skos:definition>
      <skos:prefLabel xml:lang="sv">Summa</skos:prefLabel>
      <skos:definition xml:lang="sv">Summan av värden för alla giltiga fall.</skos:definition>
   </rdf:Description>
   <rdf:Description rdf:about="http://rdf-vocabulary.ddialliance.org/cv/SummaryStatisticType/2.1/d40e1102">
      <rdf:type rdf:resource="http://www.w3.org/2004/02/skos/core#Concept"/>
      <skos:inScheme rdf:resource="http://rdf-vocabulary.ddialliance.org/cv/SummaryStatisticType/2.1"/>
      <skos:notation>Variance</skos:notation>
      <skos:prefLabel xml:lang="en">Variance</skos:prefLabel>
      <skos:definition xml:lang="en">The variance is the mean square deviation of the variable around the average value. It reflects the dispersion of a frequency distribution around its mean (OECD Glossary of Statistics).</skos:definition>
      <skos:prefLabel xml:lang="da">Varians</skos:prefLabel>
      <skos:definition xml:lang="da">Variansen er den gennemsnitlige kvadratafvigelse for variable omkring gennemsnitsværdien. Den afspejler frekvensfordelingens spredning omkring dens gennemsnit (OECD Glossary of Statistics)</skos:definition>
      <skos:prefLabel xml:lang="fi">Varianssi</skos:prefLabel>
      <skos:definition xml:lang="fi">Varianssi ilmoittaa miten suuria keskimäärin ovat neliöidyt poikkeamat keskiarvosta (Tilastokeskus). Varianssi kuvaa jakauman hajontaa odotusarvon ympärillä.</skos:definition>
      <skos:prefLabel xml:lang="it">Varianza</skos:prefLabel>
      <skos:definition xml:lang="it">La varianza di una variabile è lo scarto quadratico medio dal valore medio. Riflette la dispersione di una distribuzione di frequenza attorno alla sua media.</skos:definition>
      <skos:prefLabel xml:lang="nl">Variantie</skos:prefLabel>
      <skos:definition xml:lang="nl"/>
      <skos:prefLabel xml:lang="no">Varians</skos:prefLabel>
      <skos:definition xml:lang="no">Variansen er det gjennomsnittlige kvadratiske avvik av variabelen rundt gjennomsnittsverdien. Det gjenspeiler spredning rundt dets gjennomsnitt.</skos:definition>
      <skos:prefLabel xml:lang="pt">Variância</skos:prefLabel>
      <skos:definition xml:lang="pt">A variância é a média dos quadrados dos desvios de uma variável em torno do seu valor médio. Ela reflete a dispersão de uma distribuição de frequências em torno da sua média (OECD Glossary of Statistics).</skos:definition>
      <skos:prefLabel xml:lang="sl">Varianca (s2)</skos:prefLabel>
      <skos:definition xml:lang="sl">Varianca je srednji kvadratni odklon spremenljivke okoli povprečne vrednosti. Odraža razpršenost frekvenčne porazdelitve okoli aritmetične sredine (OECD Glossary of Statistics).</skos:definition>
      <skos:prefLabel xml:lang="sr">Varijansa</skos:prefLabel>
      <skos:definition xml:lang="sr">Varijansa je srednje kvadratno odstupanje vrednosti promenljive oko njene prosečne vrednosti. Ukazuje na raspodelu frekvencije oko srednje vrednosti (OECD-ov Statistički rečnik).</skos:definition>
      <skos:prefLabel xml:lang="sv">Varians</skos:prefLabel>
      <skos:definition xml:lang="sv">Variansen är genomsnittet för en variabels kvadrerade avvikelser från sitt medelvärde. Det återspeglar spridningen av en frekvensfördelning runt medelvärdet.</skos:definition>
   </rdf:Description>
   <rdf:Description rdf:about="http://rdf-vocabulary.ddialliance.org/cv/SummaryStatisticType/2.1/d40e1173">
      <rdf:type rdf:resource="http://www.w3.org/2004/02/skos/core#Concept"/>
      <skos:inScheme rdf:resource="http://rdf-vocabulary.ddialliance.org/cv/SummaryStatisticType/2.1"/>
      <skos:notation>StandardDeviation</skos:notation>
      <skos:prefLabel xml:lang="en">Standard deviation</skos:prefLabel>
      <skos:definition xml:lang="en">Indicates the degree to which individuals within the sample differ from the sample mean.</skos:definition>
      <skos:prefLabel xml:lang="da">Standardafvigelse</skos:prefLabel>
      <skos:definition xml:lang="da">Angiver den grad, hvormed individerne i stikprøven afviger fra stikprøvens gennemsnit.</skos:definition>
      <skos:prefLabel xml:lang="fi">Keskihajonta</skos:prefLabel>
      <skos:definition xml:lang="fi">Luku, joka mittaa missä määrin otoksen yksiköiden arvot eroavat koko otoksen keskiarvosta.</skos:definition>
      <skos:prefLabel xml:lang="it">Deviazione standard</skos:prefLabel>
      <skos:definition xml:lang="it">Indica il grado in cui gli individui all'interno del campione differiscono dalla media campionaria.</skos:definition>
      <skos:prefLabel xml:lang="nl">Standaardafwijking</skos:prefLabel>
      <skos:definition xml:lang="nl"/>
      <skos:prefLabel xml:lang="no">Standardavvik</skos:prefLabel>
      <skos:definition xml:lang="no">Indikerer graden av hvorvidt individer i utvalget er forskjellige fra utvalgsgjennomsnittet.</skos:definition>
      <skos:prefLabel xml:lang="pt">Desvio padrão</skos:prefLabel>
      <skos:definition xml:lang="pt">Indica em que medida os indivíduos de uma amostra diferem da média da mesma.</skos:definition>
      <skos:prefLabel xml:lang="sl">Standardni odklon (s)</skos:prefLabel>
      <skos:definition xml:lang="sl">Pozitivni kvadratni koren variance. Najpogosteje uporabljena mera razpršenosti frekvenčne porazdelitve.</skos:definition>
      <skos:prefLabel xml:lang="sr">Standardna devijacija</skos:prefLabel>
      <skos:definition xml:lang="sr">Apsolutna mera disperzije u osnovnom skupu. Ona nam govori koliko u proseku elementi skupa odstupaju od aritmetičke sredine skupa.</skos:definition>
      <skos:prefLabel xml:lang="sv">Standardavvikelse</skos:prefLabel>
      <skos:definition xml:lang="sv">Den positiva kvadratroten ur variansen. Det mest använda måttet på spridningen av en frekvensfördelning.</skos:definition>
   </rdf:Description>
   <rdf:Description rdf:about="http://rdf-vocabulary.ddialliance.org/cv/SummaryStatisticType/2.1/d40e1244">
      <rdf:type rdf:resource="http://www.w3.org/2004/02/skos/core#Concept"/>
      <skos:inScheme rdf:resource="http://rdf-vocabulary.ddialliance.org/cv/SummaryStatisticType/2.1"/>
      <skos:notation>CoefficientOfVariation</skos:notation>
      <skos:prefLabel xml:lang="en">Coefficient of variation</skos:prefLabel>
      <skos:definition xml:lang="en">Standard deviation divided by the mean.</skos:definition>
      <skos:prefLabel xml:lang="da">Variationskoefficient</skos:prefLabel>
      <skos:definition xml:lang="da">Standardafvigelse divideret med gennemsnittet.</skos:definition>
      <skos:prefLabel xml:lang="fi">Variaatiokerroin</skos:prefLabel>
      <skos:definition xml:lang="fi">Keskihajonta jaettuna keskiarvolla.</skos:definition>
      <skos:prefLabel xml:lang="it">Coefficiente di variazione</skos:prefLabel>
      <skos:definition xml:lang="it">Deviazione standard divisa per la media.</skos:definition>
      <skos:prefLabel xml:lang="nl">Variatiecoëfficiënt</skos:prefLabel>
      <skos:definition xml:lang="nl"/>
      <skos:prefLabel xml:lang="no">Variasjonskoeffisienten</skos:prefLabel>
      <skos:definition xml:lang="no">Standardavviket delt på gjennomsnittet.</skos:definition>
      <skos:prefLabel xml:lang="pt">Coeficiente de variação</skos:prefLabel>
      <skos:definition xml:lang="pt">Desvio padrão dividido pela média.</skos:definition>
      <skos:prefLabel xml:lang="sl">Koeficient variacije (CV)</skos:prefLabel>
      <skos:definition xml:lang="sl">Standardni odklon, deljen z aritmetično sredino.</skos:definition>
      <skos:prefLabel xml:lang="sr">Koeficijent varijacije</skos:prefLabel>
      <skos:definition xml:lang="sr">Standardna devijacija podeljena sa srednjom vrednošću.</skos:definition>
      <skos:prefLabel xml:lang="sv">Variationskoefficient</skos:prefLabel>
      <skos:definition xml:lang="sv">Standardavvikelsen dividerad med medelvärdet.</skos:definition>
   </rdf:Description>
   <rdf:Description rdf:about="http://rdf-vocabulary.ddialliance.org/cv/SummaryStatisticType/2.1/d40e1316">
      <rdf:type rdf:resource="http://www.w3.org/2004/02/skos/core#Concept"/>
      <skos:inScheme rdf:resource="http://rdf-vocabulary.ddialliance.org/cv/SummaryStatisticType/2.1"/>
      <skos:notation>AverageAbsoluteDeviation</skos:notation>
      <skos:prefLabel xml:lang="en">Average absolute deviation</skos:prefLabel>
      <skos:definition xml:lang="en">The average of the absolute differences between each value and the overall mean. Measure of statistical dispersion around the mean, alternative to Standard Deviation.</skos:definition>
      <skos:prefLabel xml:lang="da">Gennemsnitlig numerisk afvigelse</skos:prefLabel>
      <skos:definition xml:lang="da">Gennemsnittet af de numeriske forskelle mellem hver værdi og det samlede gennemsnit. Mål for statistisk spredning omkring gennemsnittet, alternativt til standardafvigelse.</skos:definition>
      <skos:prefLabel xml:lang="fi">Absoluuttinen keskipoikkeama</skos:prefLabel>
      <skos:definition xml:lang="fi">Kunkin yksittäisen arvon ja kaikkien arvojen keskiarvon välisten poikkeamien keskiarvo. Hajontaluku, joka kuvaa arvojen vaihtelua keskiarvon ympärillä. Vaihtoehto keskihajonnalle.</skos:definition>
      <skos:prefLabel xml:lang="it">Deviazione media assoluta</skos:prefLabel>
      <skos:definition xml:lang="it">La media delle differenze assolute tra ciascun valore e la media complessiva. Misura la dispersione statistica attorno alla media, alternativa alla deviazione standard.</skos:definition>
      <skos:prefLabel xml:lang="nl">Gemiddelde absolute afwijking</skos:prefLabel>
      <skos:definition xml:lang="nl"/>
      <skos:prefLabel xml:lang="no">Gjennomsnittlig absoluttavvik</skos:prefLabel>
      <skos:definition xml:lang="no">Gjennomsnittet av de absolutte forskjellene mellom hver verdi og gjennomsnittet. Måling av statistisk spredning rundt gjennomsnittet, alternativ til standardavvik.</skos:definition>
      <skos:prefLabel xml:lang="pt">Desvio absoluto médio</skos:prefLabel>
      <skos:definition xml:lang="pt">A média das diferenças absolutas entre cada valor e a média geral. Medida de dispersão estatística em torno da média, alternativa ao desvio padrão.</skos:definition>
      <skos:prefLabel xml:lang="sl">Povprečni absolutni odklon (AAD)</skos:prefLabel>
      <skos:definition xml:lang="sl">Povprečje absolutnih razlik med posamezno vrednostjo in aritmetično sredino. Mera statistične razpršenosti okrog aritmetične sredine, alternativa standardnemu odklonu.</skos:definition>
      <skos:prefLabel xml:lang="sr">Prosečna apsolutna devijacija</skos:prefLabel>
      <skos:definition xml:lang="sr">Prosek apsolutnih razlika između svake vrednosti i ukupne srednje vrednosti. Meri statističku disperziju oko srednje vrednosti, alternativa je standardnoj devijaciji.</skos:definition>
      <skos:prefLabel xml:lang="sv">Genomsnittlig absolut avvikelse</skos:prefLabel>
      <skos:definition xml:lang="sv">Medelvärdet av de absoluta skillnaderna mellan varje värde och det totala medelvärdet. Mått på den statistiska spridningen kring medelvärdet, ett alternativ till standardavvikelsen.</skos:definition>
   </rdf:Description>
   <rdf:Description rdf:about="http://rdf-vocabulary.ddialliance.org/cv/SummaryStatisticType/2.1/d40e1387">
      <rdf:type rdf:resource="http://www.w3.org/2004/02/skos/core#Concept"/>
      <skos:inScheme rdf:resource="http://rdf-vocabulary.ddialliance.org/cv/SummaryStatisticType/2.1"/>
      <skos:notation>MedianAbsoluteDeviation</skos:notation>
      <skos:prefLabel xml:lang="en">Median absolute deviation</skos:prefLabel>
      <skos:definition xml:lang="en">The median absolute deviation from the median. Measure of statistical dispersion around the median.</skos:definition>
      <skos:prefLabel xml:lang="da">Median numerisk afvigelse</skos:prefLabel>
      <skos:definition xml:lang="da">Medianens numeriske afvigelse fra median. Måling af statistisk spredning omkring medianen.</skos:definition>
      <skos:prefLabel xml:lang="fi">Mediaanin absoluuttinen keskipoikkeama</skos:prefLabel>
      <skos:definition xml:lang="fi">Keskipoikkeama mediaanista. Hajontaluku, joka kuvaa arvojen vaihtelua mediaanin ympärillä.</skos:definition>
      <skos:prefLabel xml:lang="it">Deviazione mediana assoluta</skos:prefLabel>
      <skos:definition xml:lang="it">La deviazione mediana assoluta dalla mediana. Misura la dispersione statistica intorno alla mediana.</skos:definition>
      <skos:prefLabel xml:lang="nl">Mediaan absolute afwijking</skos:prefLabel>
      <skos:definition xml:lang="nl"/>
      <skos:prefLabel xml:lang="no">Median absoluttavvik</skos:prefLabel>
      <skos:definition xml:lang="no">Median absoluttavvik fra medianen. Måling av statistisk spredning rundt medianen.</skos:definition>
      <skos:prefLabel xml:lang="pt">Desvio absoluto mediano</skos:prefLabel>
      <skos:definition xml:lang="pt">O desvio absoluto mediano da mediana. Medida de dispersão estatística em torno da mediana.</skos:definition>
      <skos:prefLabel xml:lang="sl">Mediana absolutnega odklona od mediane (MAD)</skos:prefLabel>
      <skos:definition xml:lang="sl">Mediana absolutnega odklona od mediane. Mera statistične razpršenosti okrog mediane.</skos:definition>
      <skos:prefLabel xml:lang="sr">Medijana apsolutne devijacije</skos:prefLabel>
      <skos:definition xml:lang="sr">Mera statističke disperzije oko medijane.</skos:definition>
      <skos:prefLabel xml:lang="sv">Median absolut avvikelse</skos:prefLabel>
      <skos:definition xml:lang="sv">Median absolut avvikelsen från medianen. Mått på spridningen runt medianen.</skos:definition>
   </rdf:Description>
   <rdf:Description rdf:about="http://rdf-vocabulary.ddialliance.org/cv/SummaryStatisticType/2.1/d40e1458">
      <rdf:type rdf:resource="http://www.w3.org/2004/02/skos/core#Concept"/>
      <skos:inScheme rdf:resource="http://rdf-vocabulary.ddialliance.org/cv/SummaryStatisticType/2.1"/>
      <skos:notation>FirstQuartile</skos:notation>
      <skos:prefLabel xml:lang="en">First quartile</skos:prefLabel>
      <skos:definition xml:lang="en">The first of three values which separate the total frequency of a distribution into four equal parts.</skos:definition>
      <skos:prefLabel xml:lang="da">Første kvartil</skos:prefLabel>
      <skos:definition xml:lang="da">Den første af tre værdier, der adskiller den samlede frekvensfordeling i fire lige dele.</skos:definition>
      <skos:prefLabel xml:lang="fi">Ensimmäinen kvartiili</skos:prefLabel>
      <skos:definition xml:lang="fi">Alakvartiili. Ensimmäinen kolmesta arvosta, jotka jakavat jakauman neljään yhtä suureen osaan. Jakauman arvoista 25 % on siis pienempiä tai yhtä suuria kuin ensimmäinen kvartiili.</skos:definition>
      <skos:prefLabel xml:lang="it">Primo quartile</skos:prefLabel>
      <skos:definition xml:lang="it">Il primo dei tre valori che suddividono la frequenza totale di una distribuzione in quattro parti uguali.</skos:definition>
      <skos:prefLabel xml:lang="nl">Eerste kwartiel</skos:prefLabel>
      <skos:definition xml:lang="nl"/>
      <skos:prefLabel xml:lang="no">Første kvartil</skos:prefLabel>
      <skos:definition xml:lang="no">Den første av tre verdier som separerer den totale frekvensen av en fordeling i fire like store deler.</skos:definition>
      <skos:prefLabel xml:lang="pt">Primeiro quartil</skos:prefLabel>
      <skos:definition xml:lang="pt">O primeiro dos três valores que separam a frequência total de uma distribuição em quatro partes iguais.</skos:definition>
      <skos:prefLabel xml:lang="sl">Prvi kvartil</skos:prefLabel>
      <skos:definition xml:lang="sl">Prva od treh vrednosti, ki razdelijo celotno frekvenčno porazdelitev na štiri enake dele.</skos:definition>
      <skos:prefLabel xml:lang="sr">Prvi kvartil</skos:prefLabel>
      <skos:definition xml:lang="sr">Prva od tri vrednosti koja razdvaja ukupnu frekvenciju distribucije u četiri jednaka dela.</skos:definition>
      <skos:prefLabel xml:lang="sv">Första kvartilen</skos:prefLabel>
      <skos:definition xml:lang="sv">Det första av tre värden som separerar den totala frekvensen av en fördelning i fyra lika stora delar.</skos:definition>
   </rdf:Description>
   <rdf:Description rdf:about="http://rdf-vocabulary.ddialliance.org/cv/SummaryStatisticType/2.1/d40e1529">
      <rdf:type rdf:resource="http://www.w3.org/2004/02/skos/core#Concept"/>
      <skos:inScheme rdf:resource="http://rdf-vocabulary.ddialliance.org/cv/SummaryStatisticType/2.1"/>
      <skos:notation>SecondQuartile</skos:notation>
      <skos:prefLabel xml:lang="en">Second quartile</skos:prefLabel>
      <skos:definition xml:lang="en">The second of three values which separate the total frequency of a distribution into four equal parts (= median).</skos:definition>
      <skos:prefLabel xml:lang="da">Anden kvartil</skos:prefLabel>
      <skos:definition xml:lang="da">Den anden af tre værdier, der adskiller den samlede frekvensfordeling i fire lige dele (=median).</skos:definition>
      <skos:prefLabel xml:lang="fi">Toinen kvartiili</skos:prefLabel>
      <skos:definition xml:lang="fi">Toinen kvartiili eli mediaani. Toinen kolmesta arvosta, jotka jakavat jakauman neljään yhtä suureen osaan.</skos:definition>
      <skos:prefLabel xml:lang="it">Secondo quartile</skos:prefLabel>
      <skos:definition xml:lang="it">Il secondo dei tre valori che suddividono la frequenza totale di una distribuzione in quattro parti uguali (= mediana).</skos:definition>
      <skos:prefLabel xml:lang="nl">Tweede kwartiel</skos:prefLabel>
      <skos:definition xml:lang="nl"/>
      <skos:prefLabel xml:lang="no">Andre kvartil</skos:prefLabel>
      <skos:definition xml:lang="no">Den andre av tre verdier som separerer den totale frekvensen av en fordeling i fire like store deler (=median).</skos:definition>
      <skos:prefLabel xml:lang="pt">Segundo quartil</skos:prefLabel>
      <skos:definition xml:lang="pt">O segundo dos três valores que separam a frequência total de uma distribuição em quatro partes iguais. (= mediana).</skos:definition>
      <skos:prefLabel xml:lang="sl">Drugi kvartil</skos:prefLabel>
      <skos:definition xml:lang="sl">Druga od treh vrednosti, ki razdelijo celotno frekvenčno porazdelitev na štiri enake dele (= mediana).</skos:definition>
      <skos:prefLabel xml:lang="sr">Drugi kvartil</skos:prefLabel>
      <skos:definition xml:lang="sr">Druga od tri vrednosti koja razdvaja ukupnu frekvenciju distribucije u četiri jednaka dela.</skos:definition>
      <skos:prefLabel xml:lang="sv">Andra kvartilen</skos:prefLabel>
      <skos:definition xml:lang="sv">Det andra av tre värden som separerar den totala frekvensen av en fördelning i fyra lika delar (= median).</skos:definition>
   </rdf:Description>
   <rdf:Description rdf:about="http://rdf-vocabulary.ddialliance.org/cv/SummaryStatisticType/2.1/d40e1600">
      <rdf:type rdf:resource="http://www.w3.org/2004/02/skos/core#Concept"/>
      <skos:inScheme rdf:resource="http://rdf-vocabulary.ddialliance.org/cv/SummaryStatisticType/2.1"/>
      <skos:notation>ThirdQuartile</skos:notation>
      <skos:prefLabel xml:lang="en">Third quartile</skos:prefLabel>
      <skos:definition xml:lang="en">The third of three values which separate the total frequency of a distribution into four equal parts.</skos:definition>
      <skos:prefLabel xml:lang="da">Tredje kvartil</skos:prefLabel>
      <skos:definition xml:lang="da">Den tredje af tre værdier, der adskiller den samlede frekvensfordeling i fire lige store dele.</skos:definition>
      <skos:prefLabel xml:lang="fi">Kolmas kvartiili</skos:prefLabel>
      <skos:definition xml:lang="fi">Yläkvartiili. Kolmas kolmesta arvosta, jotka jakavat jakauman neljään yhtä suureen osaan.</skos:definition>
      <skos:prefLabel xml:lang="it">Terzo quartile</skos:prefLabel>
      <skos:definition xml:lang="it">Il terzo dei tre valori che suddividono la frequenza totale di una distribuzione in quattro parti uguali.</skos:definition>
      <skos:prefLabel xml:lang="nl">Derde kwartiel</skos:prefLabel>
      <skos:definition xml:lang="nl"/>
      <skos:prefLabel xml:lang="no">Tredje kvartil</skos:prefLabel>
      <skos:definition xml:lang="no">Den tredje av tre verdier som separerer den totale frekvensen av en fordeling i fire like store deler.</skos:definition>
      <skos:prefLabel xml:lang="pt">Terceiro quartil</skos:prefLabel>
      <skos:definition xml:lang="pt">O terceiro dos três valores que separam a frequência total de uma distribuição em quatro partes iguais.</skos:definition>
      <skos:prefLabel xml:lang="sl">Tretji kvartil</skos:prefLabel>
      <skos:definition xml:lang="sl">Tretja od treh vrednosti, ki razdelijo celotno frekvenčno porazdelitev na štiri enake dele.</skos:definition>
      <skos:prefLabel xml:lang="sr">Treći kvatil</skos:prefLabel>
      <skos:definition xml:lang="sr">Treća od tri vrednosti koja razdvaja ukupnu frekvenciju distribucije u četiri jednaka dela.</skos:definition>
      <skos:prefLabel xml:lang="sv">Tredje kvartilen</skos:prefLabel>
      <skos:definition xml:lang="sv">Det tredje av tre värden som separerar den totala frekvensen av en fördelning i fyra lika delar.</skos:definition>
   </rdf:Description>
   <rdf:Description rdf:about="http://rdf-vocabulary.ddialliance.org/cv/SummaryStatisticType/2.1/d40e1671">
      <rdf:type rdf:resource="http://www.w3.org/2004/02/skos/core#Concept"/>
      <skos:inScheme rdf:resource="http://rdf-vocabulary.ddialliance.org/cv/SummaryStatisticType/2.1"/>
      <skos:notation>InterquartileRange</skos:notation>
      <skos:prefLabel xml:lang="en">Interquartile range</skos:prefLabel>
      <skos:definition xml:lang="en">The range between the first and third quartile values.</skos:definition>
      <skos:prefLabel xml:lang="da">Afstanden mellem 1. og 3. kvartil</skos:prefLabel>
      <skos:definition xml:lang="da">Afstanden mellem 1. og 3. kvartils værdier.</skos:definition>
      <skos:prefLabel xml:lang="fi">Kvartiiliväli</skos:prefLabel>
      <skos:definition xml:lang="fi">Väli alakvartiilista (ensimmäinen kvartiili) yläkvartiiliin (kolmas kvartiili).</skos:definition>
      <skos:prefLabel xml:lang="it">Differenza interquartile</skos:prefLabel>
      <skos:definition xml:lang="it">L'intervallo tra il primo e il terzo quartile.</skos:definition>
      <skos:prefLabel xml:lang="nl">Interkwartielafstand</skos:prefLabel>
      <skos:definition xml:lang="nl"/>
      <skos:prefLabel xml:lang="no">Kvartilbredde</skos:prefLabel>
      <skos:definition xml:lang="no">Differansen mellom den første og den tredje kvartilverdien.</skos:definition>
      <skos:prefLabel xml:lang="pt">Amplitude interquartil</skos:prefLabel>
      <skos:definition xml:lang="pt">O intervalo entre os valores do primeiro e do terceiro quartil.</skos:definition>
      <skos:prefLabel xml:lang="sl">Kvartilni razmik</skos:prefLabel>
      <skos:definition xml:lang="sl">Razpon med vrednostjo prvega in tretjega kvartila.</skos:definition>
      <skos:prefLabel xml:lang="sr">Međukvartilni raspon</skos:prefLabel>
      <skos:definition xml:lang="sr">Raspon između prvog i trećeg kvartila.</skos:definition>
      <skos:prefLabel xml:lang="sv">Kvartilavstånd</skos:prefLabel>
      <skos:definition xml:lang="sv">Intervallet mellan första och tredje kvartilen.</skos:definition>
   </rdf:Description>
   <rdf:Description rdf:about="http://rdf-vocabulary.ddialliance.org/cv/SummaryStatisticType/2.1/d40e1743">
      <rdf:type rdf:resource="http://www.w3.org/2004/02/skos/core#Concept"/>
      <skos:inScheme rdf:resource="http://rdf-vocabulary.ddialliance.org/cv/SummaryStatisticType/2.1"/>
      <skos:notation>FirstQuintile</skos:notation>
      <skos:prefLabel xml:lang="en">First quintile</skos:prefLabel>
      <skos:definition xml:lang="en">The first of four values which separate the total frequency of a distribution into five equal parts.</skos:definition>
      <skos:prefLabel xml:lang="da">Første kvintil</skos:prefLabel>
      <skos:definition xml:lang="da">Den første af fire værdier, der adskiller den samlede frekvensfordeling i fem lige dele.</skos:definition>
      <skos:prefLabel xml:lang="fi">Ensimmäinen kvintiili</skos:prefLabel>
      <skos:definition xml:lang="fi">Ensimmäinen neljästä arvosta, jotka jakavat jakauman viiteen yhtä suureen osaan. Jakauman arvoista 20 % on siis pienempiä tai yhtä suuria kuin ensmmäinen kvintiili.</skos:definition>
      <skos:prefLabel xml:lang="it">Primo quintile</skos:prefLabel>
      <skos:definition xml:lang="it">Il primo dei quattro valori che suddividono la frequenza totale di una distribuzione in cinque parti uguali.</skos:definition>
      <skos:prefLabel xml:lang="nl">Eerste kwintiel</skos:prefLabel>
      <skos:definition xml:lang="nl"/>
      <skos:prefLabel xml:lang="no">Første kvintil</skos:prefLabel>
      <skos:definition xml:lang="no">Den første av fire verdier som separerer den totale frekvensen av en fordeling i fem like deler.</skos:definition>
      <skos:prefLabel xml:lang="pt">Primeiro quintil</skos:prefLabel>
      <skos:definition xml:lang="pt">O primeiro dos quatro valores que separam a frequência total de uma distribuição em cinco partes iguais.</skos:definition>
      <skos:prefLabel xml:lang="sl">Prvi kvintil</skos:prefLabel>
      <skos:definition xml:lang="sl">Prva od štirih vrednosti, ki razdelijo celotno frekvenčno porazdelitev na pet enakih delov.</skos:definition>
      <skos:prefLabel xml:lang="sr">Prvi kvintil</skos:prefLabel>
      <skos:definition xml:lang="sr">Prva od četiri vrednosti koja razdvaja ukupnu frekvenciju distribucije na pet jednakih delova.</skos:definition>
      <skos:prefLabel xml:lang="sv">Första kvintilen</skos:prefLabel>
      <skos:definition xml:lang="sv">Det första av fyra värden som separerar den totala frekvensen av en fördelning i fem lika delar.</skos:definition>
   </rdf:Description>
   <rdf:Description rdf:about="http://rdf-vocabulary.ddialliance.org/cv/SummaryStatisticType/2.1/d40e1814">
      <rdf:type rdf:resource="http://www.w3.org/2004/02/skos/core#Concept"/>
      <skos:inScheme rdf:resource="http://rdf-vocabulary.ddialliance.org/cv/SummaryStatisticType/2.1"/>
      <skos:notation>SecondQuintile</skos:notation>
      <skos:prefLabel xml:lang="en">Second quintile</skos:prefLabel>
      <skos:definition xml:lang="en">The second of four values which separate the total frequency of a distribution into five equal parts.</skos:definition>
      <skos:prefLabel xml:lang="da">Anden kvintil</skos:prefLabel>
      <skos:definition xml:lang="da">Den anden af fire værdier, der adskiller den samlede frekvensfordeling i fem lige dele.</skos:definition>
      <skos:prefLabel xml:lang="fi">Toinen kvintiili</skos:prefLabel>
      <skos:definition xml:lang="fi">Toinen neljästä arvosta, jotka jakavat jakauman viiteen yhtä suureen osaan.</skos:definition>
      <skos:prefLabel xml:lang="it">Secondo quintile</skos:prefLabel>
      <skos:definition xml:lang="it">Il secondo dei quattro valori che suddividono la frequenza totale di una distribuzione in cinque parti uguali.</skos:definition>
      <skos:prefLabel xml:lang="nl">Tweede kwintiel</skos:prefLabel>
      <skos:definition xml:lang="nl"/>
      <skos:prefLabel xml:lang="no">Andre kvintil</skos:prefLabel>
      <skos:definition xml:lang="no">Den andre av fire verdier som separerer den totale frekvensen av en fordeling i fem like deler.</skos:definition>
      <skos:prefLabel xml:lang="pt">Segundo quintil</skos:prefLabel>
      <skos:definition xml:lang="pt">O segundo dos quatro valores que separam a frequência total de uma distribuição em cinco partes iguais.</skos:definition>
      <skos:prefLabel xml:lang="sl">Drugi kvintil</skos:prefLabel>
      <skos:definition xml:lang="sl">Druga od štirih vrednosti, ki razdelijo celotno frekvenčno porazdelitev na pet enakih delov.</skos:definition>
      <skos:prefLabel xml:lang="sr">Drugi kvintil</skos:prefLabel>
      <skos:definition xml:lang="sr">Druga od četiri vrednosti koja razdvaja ukupnu frekvenciju distribucije na pet jednakih delova.</skos:definition>
      <skos:prefLabel xml:lang="sv">Andra kvintilen</skos:prefLabel>
      <skos:definition xml:lang="sv">Det andra av fyra värden som separerar den totala frekvensen av en fördelning i fem lika delar.</skos:definition>
   </rdf:Description>
   <rdf:Description rdf:about="http://rdf-vocabulary.ddialliance.org/cv/SummaryStatisticType/2.1/d40e1885">
      <rdf:type rdf:resource="http://www.w3.org/2004/02/skos/core#Concept"/>
      <skos:inScheme rdf:resource="http://rdf-vocabulary.ddialliance.org/cv/SummaryStatisticType/2.1"/>
      <skos:notation>ThirdQuintile</skos:notation>
      <skos:prefLabel xml:lang="en">Third quintile</skos:prefLabel>
      <skos:definition xml:lang="en">The third of four values which separate the total frequency of a distribution into five equal parts.</skos:definition>
      <skos:prefLabel xml:lang="da">Tredje kvintil</skos:prefLabel>
      <skos:definition xml:lang="da">Den tredje af fire værdier, der adskiller den samlede frekvensfordeling i fem lige dele.</skos:definition>
      <skos:prefLabel xml:lang="fi">Kolmas kvintiili</skos:prefLabel>
      <skos:definition xml:lang="fi">Kolmas neljästä arvosta, jotka jakavat jakauman viiteen yhtä suureen osaan.</skos:definition>
      <skos:prefLabel xml:lang="it">Terzo quintile</skos:prefLabel>
      <skos:definition xml:lang="it">Il terzo dei quattro valori che suddividono la frequenza totale di una distribuzione in cinque parti uguali.</skos:definition>
      <skos:prefLabel xml:lang="nl">Derde kwintiel</skos:prefLabel>
      <skos:definition xml:lang="nl"/>
      <skos:prefLabel xml:lang="no">Tredje kvintil</skos:prefLabel>
      <skos:definition xml:lang="no">Den tredje av fire verdier som separerer den totale frekvensen av en fordeling i fem like deler.</skos:definition>
      <skos:prefLabel xml:lang="pt">Terceiro quintil</skos:prefLabel>
      <skos:definition xml:lang="pt">O terceiro dos quatro valores que separam a frequência total de uma distribuição em cinco partes iguais.</skos:definition>
      <skos:prefLabel xml:lang="sl">Tretji kvintil</skos:prefLabel>
      <skos:definition xml:lang="sl">Tretja od štirih vrednosti, ki razdelijo celotno frekvenčno porazdelitev na pet enakih delov.</skos:definition>
      <skos:prefLabel xml:lang="sr">Treći kvintil</skos:prefLabel>
      <skos:definition xml:lang="sr">Treća od četiri vrednosti koja razdvaja ukupnu frekvenciju distribucije na pet jednakih delova.</skos:definition>
      <skos:prefLabel xml:lang="sv">Tredje kvintilen</skos:prefLabel>
      <skos:definition xml:lang="sv">Det tredje av fyra värden som separerar den totala frekvensen av en fördelning i fem lika delar.</skos:definition>
   </rdf:Description>
   <rdf:Description rdf:about="http://rdf-vocabulary.ddialliance.org/cv/SummaryStatisticType/2.1/d40e1956">
      <rdf:type rdf:resource="http://www.w3.org/2004/02/skos/core#Concept"/>
      <skos:inScheme rdf:resource="http://rdf-vocabulary.ddialliance.org/cv/SummaryStatisticType/2.1"/>
      <skos:notation>FourthQuintile</skos:notation>
      <skos:prefLabel xml:lang="en">Fourth quintile</skos:prefLabel>
      <skos:definition xml:lang="en">The fourth of four values which separate the total frequency of a distribution into five equal parts.</skos:definition>
      <skos:prefLabel xml:lang="da">Fjerde kvintil</skos:prefLabel>
      <skos:definition xml:lang="da">Den fjerde af fire værdier, der adskiller den samlede frekvensfordeling i fem lige dele.</skos:definition>
      <skos:prefLabel xml:lang="fi">Neljäs kvintiili</skos:prefLabel>
      <skos:definition xml:lang="fi">Neljäs neljästä arvosta, jotka jakavat jakauman viiteen yhtä suureen osaan.</skos:definition>
      <skos:prefLabel xml:lang="it">Quarto quintile</skos:prefLabel>
      <skos:definition xml:lang="it">Il quarto dei quattro valori che suddividono la frequenza totale di una distribuzione in cinque parti uguali.</skos:definition>
      <skos:prefLabel xml:lang="nl">Vierde kwintiel</skos:prefLabel>
      <skos:definition xml:lang="nl"/>
      <skos:prefLabel xml:lang="no">Fjerde kvintil</skos:prefLabel>
      <skos:definition xml:lang="no">Den fjerde av fire verdier som separerer den totale frekvensen av en fordeling i fem like deler.</skos:definition>
      <skos:prefLabel xml:lang="pt">Quarto quintil</skos:prefLabel>
      <skos:definition xml:lang="pt">O quarto dos quatro valores que separam a frequência total de uma distribuição em cinco partes iguais.</skos:definition>
      <skos:prefLabel xml:lang="sl">Četrti kvintil</skos:prefLabel>
      <skos:definition xml:lang="sl">Četrta od štirih vrednosti, ki razdelijo celotno frekvenčno porazdelitev na pet enakih delov.</skos:definition>
      <skos:prefLabel xml:lang="sr">Četvrti kvintil</skos:prefLabel>
      <skos:definition xml:lang="sr">Četvrta od četiri vrednosti koja razdvaja ukupnu frekvenciju distribucije na pet jednakih delova.</skos:definition>
      <skos:prefLabel xml:lang="sv">Fjärde kvintilen</skos:prefLabel>
      <skos:definition xml:lang="sv">Det fjärde av fyra värden som separerar den totala frekvensen av en fördelning i fem lika delar.</skos:definition>
   </rdf:Description>
   <rdf:Description rdf:about="http://rdf-vocabulary.ddialliance.org/cv/SummaryStatisticType/2.1/d40e2027">
      <rdf:type rdf:resource="http://www.w3.org/2004/02/skos/core#Concept"/>
      <skos:inScheme rdf:resource="http://rdf-vocabulary.ddialliance.org/cv/SummaryStatisticType/2.1"/>
      <skos:notation>InterquintileRange</skos:notation>
      <skos:prefLabel xml:lang="en">Interquintile range</skos:prefLabel>
      <skos:definition xml:lang="en">The range between the first and fourth quintile values.</skos:definition>
      <skos:prefLabel xml:lang="da">Afstanden mellem 1. og 4. kvintil</skos:prefLabel>
      <skos:definition xml:lang="da">Afstanden mellem 1. og 4. kvintils værdier.</skos:definition>
      <skos:prefLabel xml:lang="fi">Kvintiiliväli</skos:prefLabel>
      <skos:definition xml:lang="fi">Väli ensimmäisestä kvintiilistä neljänteen kvintiiliin.</skos:definition>
      <skos:prefLabel xml:lang="it">Ampiezza interquintile</skos:prefLabel>
      <skos:definition xml:lang="it">L'intervallo tra il primo e il quarto quintile.</skos:definition>
      <skos:prefLabel xml:lang="nl">Interkwintielafstand</skos:prefLabel>
      <skos:definition xml:lang="nl"/>
      <skos:prefLabel xml:lang="no">Kvintilbredde</skos:prefLabel>
      <skos:definition xml:lang="no">Intervallet mellom første og fjerde kvintil.</skos:definition>
      <skos:prefLabel xml:lang="pt">Amplitude interquintil</skos:prefLabel>
      <skos:definition xml:lang="pt">O intervalo entre os valores do primeiro e do quarto quintil.</skos:definition>
      <skos:prefLabel xml:lang="sl">Kvintilni razmik</skos:prefLabel>
      <skos:definition xml:lang="sl">Razpon med vrednostjo prvega in četrtega kvintila.</skos:definition>
      <skos:prefLabel xml:lang="sr">Međukvintilni raspon</skos:prefLabel>
      <skos:definition xml:lang="sr">Raspon između prvog i četvrtog kvintila.</skos:definition>
      <skos:prefLabel xml:lang="sv">Kvintilavstånd</skos:prefLabel>
      <skos:definition xml:lang="sv">Intervallet mellan första och fjärde kvintilen.</skos:definition>
   </rdf:Description>
   <rdf:Description rdf:about="http://rdf-vocabulary.ddialliance.org/cv/SummaryStatisticType/2.1/d40e2098">
      <rdf:type rdf:resource="http://www.w3.org/2004/02/skos/core#Concept"/>
      <skos:inScheme rdf:resource="http://rdf-vocabulary.ddialliance.org/cv/SummaryStatisticType/2.1"/>
      <skos:notation>FirstDecile</skos:notation>
      <skos:prefLabel xml:lang="en">First decile</skos:prefLabel>
      <skos:definition xml:lang="en">The first of nine values which separate the total frequency of a distribution into ten equal parts.</skos:definition>
      <skos:prefLabel xml:lang="da">Første decil</skos:prefLabel>
      <skos:definition xml:lang="da">Den første af ni værdier, der adskiller den samlede frekvensfordeling i ti lige dele.</skos:definition>
      <skos:prefLabel xml:lang="fi">Ensimmäinen desiili</skos:prefLabel>
      <skos:definition xml:lang="fi">Ensimmäinen yhdeksästä arvosta, jotka jakavat jakauman kymmeneen yhtä suureen osaan. Jakauman arvoista 10 % on siis pienempiä tai yhtä suuria kuin ensimmäinen desiili.</skos:definition>
      <skos:prefLabel xml:lang="it">Primo decile</skos:prefLabel>
      <skos:definition xml:lang="it">Il primo dei nove valori che suddividono la frequenza totale di una distribuzione in dieci parti uguali.</skos:definition>
      <skos:prefLabel xml:lang="nl">Eerste deciel</skos:prefLabel>
      <skos:definition xml:lang="nl"/>
      <skos:prefLabel xml:lang="no">Første desil</skos:prefLabel>
      <skos:definition xml:lang="no">Den første av ni verdier som separerer den totale frekvensen av en fordeling i ti like deler.</skos:definition>
      <skos:prefLabel xml:lang="pt">Primeiro decil</skos:prefLabel>
      <skos:definition xml:lang="pt">O primeiro dos nove valores que separam a frequência total de uma distribuição em dez partes iguais.</skos:definition>
      <skos:prefLabel xml:lang="sl">Prvi decil</skos:prefLabel>
      <skos:definition xml:lang="sl">Prva od devetih vrednosti, ki razdelijo celotno frekvenčno porazdelitev na deset enakih delov.</skos:definition>
      <skos:prefLabel xml:lang="sr">Prvi decil</skos:prefLabel>
      <skos:definition xml:lang="sr">Prva od devet vrednosti koja razdvaja ukupnu frekvenciju distribucije na deset jednakih delova.</skos:definition>
      <skos:prefLabel xml:lang="sv">Första decilen</skos:prefLabel>
      <skos:definition xml:lang="sv">Det första av nio värden som separerar den totala frekvensen av en fördelning i tio lika delar.</skos:definition>
   </rdf:Description>
   <rdf:Description rdf:about="http://rdf-vocabulary.ddialliance.org/cv/SummaryStatisticType/2.1/d40e2170">
      <rdf:type rdf:resource="http://www.w3.org/2004/02/skos/core#Concept"/>
      <skos:inScheme rdf:resource="http://rdf-vocabulary.ddialliance.org/cv/SummaryStatisticType/2.1"/>
      <skos:notation>SecondDecile</skos:notation>
      <skos:prefLabel xml:lang="en">Second decile</skos:prefLabel>
      <skos:definition xml:lang="en">The second of nine values which separate the total frequency of a distribution into ten equal parts.</skos:definition>
      <skos:prefLabel xml:lang="da">Anden decil</skos:prefLabel>
      <skos:definition xml:lang="da">Den anden af ni værdier, der adskiller den samlede frekvensfordeling i ti lige dele.</skos:definition>
      <skos:prefLabel xml:lang="fi">Toinen desiili</skos:prefLabel>
      <skos:definition xml:lang="fi">Toinen yhdeksästä arvosta, jotka jakavat jakauman kymmeneen yhtä suureen osaan.</skos:definition>
      <skos:prefLabel xml:lang="it">Secondo decile</skos:prefLabel>
      <skos:definition xml:lang="it">Il secondo dei nove valori che suddividono la frequenza totale di una distribuzione in dieci parti uguali.</skos:definition>
      <skos:prefLabel xml:lang="nl">Tweede deciel</skos:prefLabel>
      <skos:definition xml:lang="nl"/>
      <skos:prefLabel xml:lang="no">Andre desil</skos:prefLabel>
      <skos:definition xml:lang="no">Den andre av ni verdier som separerer den totale frekvensen av en fordeling i ti like deler.</skos:definition>
      <skos:prefLabel xml:lang="pt">Segundo decil</skos:prefLabel>
      <skos:definition xml:lang="pt">O segundo dos nove valores que separam a frequência total de uma distribuição em dez partes iguais.</skos:definition>
      <skos:prefLabel xml:lang="sl">Drugi decil</skos:prefLabel>
      <skos:definition xml:lang="sl">Druga od devetih vrednosti, ki razdelijo celotno frekvenčno porazdelitev na deset enakih delov.</skos:definition>
      <skos:prefLabel xml:lang="sr">Drugi decil</skos:prefLabel>
      <skos:definition xml:lang="sr">Druga od devet vrednosti koja razdvaja ukupnu frekvenciju distribucije na deset jednakih delova.</skos:definition>
      <skos:prefLabel xml:lang="sv">Andra decilen</skos:prefLabel>
      <skos:definition xml:lang="sv">Det andra av nio värden som separerar den totala frekvensen av en fördelning i tio lika delar.</skos:definition>
   </rdf:Description>
   <rdf:Description rdf:about="http://rdf-vocabulary.ddialliance.org/cv/SummaryStatisticType/2.1/d40e2241">
      <rdf:type rdf:resource="http://www.w3.org/2004/02/skos/core#Concept"/>
      <skos:inScheme rdf:resource="http://rdf-vocabulary.ddialliance.org/cv/SummaryStatisticType/2.1"/>
      <skos:notation>ThirdDecile</skos:notation>
      <skos:prefLabel xml:lang="en">Third decile</skos:prefLabel>
      <skos:definition xml:lang="en">The third of nine values which separate the total frequency of a distribution into ten equal parts.</skos:definition>
      <skos:prefLabel xml:lang="da">Tredje decil</skos:prefLabel>
      <skos:definition xml:lang="da">Den tredje af ni værdier, der adskiller den samlede frekvensfordeling i ti lige dele.</skos:definition>
      <skos:prefLabel xml:lang="fi">Kolmas desiili</skos:prefLabel>
      <skos:definition xml:lang="fi">Kolmas yhdeksästä arvosta, jotka jakavat jakauman kymmeneen yhtä suureen osaan.</skos:definition>
      <skos:prefLabel xml:lang="it">Terzo decile</skos:prefLabel>
      <skos:definition xml:lang="it">Il terzo dei nove valori che suddividono la frequenza totale di una distribuzione in dieci parti uguali.</skos:definition>
      <skos:prefLabel xml:lang="nl">Derde deciel</skos:prefLabel>
      <skos:definition xml:lang="nl"/>
      <skos:prefLabel xml:lang="no">Tredje desil</skos:prefLabel>
      <skos:definition xml:lang="no">Den tredje av ni verdier som separerer den totale frekvensen av en fordeling i ti like deler.</skos:definition>
      <skos:prefLabel xml:lang="pt">Terceiro decil</skos:prefLabel>
      <skos:definition xml:lang="pt">O terceiro dos nove valores que separam a frequência total de uma distribuição em dez partes iguais.</skos:definition>
      <skos:prefLabel xml:lang="sl">Tretji decil</skos:prefLabel>
      <skos:definition xml:lang="sl">Tretja od devetih vrednosti, ki razdelijo celotno frekvenčno porazdelitev na deset enakih delov.</skos:definition>
      <skos:prefLabel xml:lang="sr">Treći decil</skos:prefLabel>
      <skos:definition xml:lang="sr">Treća od devet vrednosti koja razdvaja ukupnu frekvenciju distribucije na deset jednakih delova.</skos:definition>
      <skos:prefLabel xml:lang="sv">Tredje decilen</skos:prefLabel>
      <skos:definition xml:lang="sv">Det tredje av nio värden som separerar den totala frekvensen av en fördelning i tio lika delar.</skos:definition>
   </rdf:Description>
   <rdf:Description rdf:about="http://rdf-vocabulary.ddialliance.org/cv/SummaryStatisticType/2.1/d40e2312">
      <rdf:type rdf:resource="http://www.w3.org/2004/02/skos/core#Concept"/>
      <skos:inScheme rdf:resource="http://rdf-vocabulary.ddialliance.org/cv/SummaryStatisticType/2.1"/>
      <skos:notation>FourthDecile</skos:notation>
      <skos:prefLabel xml:lang="en">Fourth decile</skos:prefLabel>
      <skos:definition xml:lang="en">The fourth of nine values which separate the total frequency of a distribution into ten equal parts.</skos:definition>
      <skos:prefLabel xml:lang="da">Fjerde decil</skos:prefLabel>
      <skos:definition xml:lang="da">Den fjerde af ni værdier, der adskiller den samlede frekvensfordeling i ti lige dele.</skos:definition>
      <skos:prefLabel xml:lang="fi">Neljäs desiili</skos:prefLabel>
      <skos:definition xml:lang="fi">Neljäs yhdeksästä arvosta, jotka jakavat jakauman kymmeneen yhtä suureen osaan.</skos:definition>
      <skos:prefLabel xml:lang="it">Quarto decile</skos:prefLabel>
      <skos:definition xml:lang="it">Il quarto dei nove valori che suddividono la frequenza totale di una distribuzione in dieci parti uguali.</skos:definition>
      <skos:prefLabel xml:lang="nl">Vierde deciel</skos:prefLabel>
      <skos:definition xml:lang="nl"/>
      <skos:prefLabel xml:lang="no">Fjerde desil</skos:prefLabel>
      <skos:definition xml:lang="no">Den fjerde av ni verdier som separerer den totale frekvensen av en fordeling i ti like deler.</skos:definition>
      <skos:prefLabel xml:lang="pt">Quarto decil</skos:prefLabel>
      <skos:definition xml:lang="pt">O quarto dos nove valores que separam a frequência total de uma distribuição em dez partes iguais.</skos:definition>
      <skos:prefLabel xml:lang="sl">Četrti decil</skos:prefLabel>
      <skos:definition xml:lang="sl">Četrta od devetih vrednosti, ki razdelijo celotno frekvenčno porazdelitev na deset enakih delov.</skos:definition>
      <skos:prefLabel xml:lang="sr">Četvrti decil</skos:prefLabel>
      <skos:definition xml:lang="sr">Četvrta od devet vrednosti koja razdvaja ukupnu frekvenciju distribucije na deset jednakih delova.</skos:definition>
      <skos:prefLabel xml:lang="sv">Fjärde decilen</skos:prefLabel>
      <skos:definition xml:lang="sv">Det fjärde av nio värden som separerar den totala frekvensen av en fördelning i tio lika delar.</skos:definition>
   </rdf:Description>
   <rdf:Description rdf:about="http://rdf-vocabulary.ddialliance.org/cv/SummaryStatisticType/2.1/d40e2383">
      <rdf:type rdf:resource="http://www.w3.org/2004/02/skos/core#Concept"/>
      <skos:inScheme rdf:resource="http://rdf-vocabulary.ddialliance.org/cv/SummaryStatisticType/2.1"/>
      <skos:notation>FifthDecile</skos:notation>
      <skos:prefLabel xml:lang="en">Fifth decile</skos:prefLabel>
      <skos:definition xml:lang="en">The fifth of nine values which separate the total frequency of a distribution into ten equal parts (= median).</skos:definition>
      <skos:prefLabel xml:lang="da">Femte decil</skos:prefLabel>
      <skos:definition xml:lang="da">Den femte af ni værdier, der adskiller den samlede frekvensfordeling i ti lige dele (=median).</skos:definition>
      <skos:prefLabel xml:lang="fi">Viides desiili</skos:prefLabel>
      <skos:definition xml:lang="fi">Viides yhdeksästä arvosta, jotka jakavat jakauman kymmeneen yhtä suureen osaan.</skos:definition>
      <skos:prefLabel xml:lang="it">Quinto decile</skos:prefLabel>
      <skos:definition xml:lang="it">Il quinto dei nove valori che suddividono la frequenza totale di una distribuzione in dieci parti uguali (= mediana).</skos:definition>
      <skos:prefLabel xml:lang="nl">Vijfde deciel</skos:prefLabel>
      <skos:definition xml:lang="nl"/>
      <skos:prefLabel xml:lang="no">Femte desil</skos:prefLabel>
      <skos:definition xml:lang="no">Den femte av ni verdier som separerer den totale frekvensen av en fordeling i ti like deler.</skos:definition>
      <skos:prefLabel xml:lang="pt">Quinto decil</skos:prefLabel>
      <skos:definition xml:lang="pt">O quinto dos nove valores que separam a frequência total de uma distribuição em dez partes iguais. (= mediana).</skos:definition>
      <skos:prefLabel xml:lang="sl">Peti decil</skos:prefLabel>
      <skos:definition xml:lang="sl">Peta od devetih vrednosti, ki razdelijo celotno frekvenčno porazdelitev na deset enakih delov (= mediana).</skos:definition>
      <skos:prefLabel xml:lang="sr">Peti decil</skos:prefLabel>
      <skos:definition xml:lang="sr">Peta od devet vrednosti koja razdvaja ukupnu frekvenciju distribucije na deset jednakih delova.</skos:definition>
      <skos:prefLabel xml:lang="sv">Femte decilen</skos:prefLabel>
      <skos:definition xml:lang="sv">Det femte av nio värden som separerar den totala frekvensen av en fördelning i tio lika delar (= median).</skos:definition>
   </rdf:Description>
   <rdf:Description rdf:about="http://rdf-vocabulary.ddialliance.org/cv/SummaryStatisticType/2.1/d40e2454">
      <rdf:type rdf:resource="http://www.w3.org/2004/02/skos/core#Concept"/>
      <skos:inScheme rdf:resource="http://rdf-vocabulary.ddialliance.org/cv/SummaryStatisticType/2.1"/>
      <skos:notation>SixthDecile</skos:notation>
      <skos:prefLabel xml:lang="en">Sixth decile</skos:prefLabel>
      <skos:definition xml:lang="en">The sixth of nine values which separate the total frequency of a distribution into ten equal parts.</skos:definition>
      <skos:prefLabel xml:lang="da">Sjette decil</skos:prefLabel>
      <skos:definition xml:lang="da">Den sjette af ni værdier, der adskiller den samlede frekvensfordeling i ti lige dele.</skos:definition>
      <skos:prefLabel xml:lang="fi">Kuudes desiili</skos:prefLabel>
      <skos:definition xml:lang="fi">Kuudes yhdeksästä arvosta, jotka jakavat jakauman kymmeneen yhtä suureen osaan.</skos:definition>
      <skos:prefLabel xml:lang="it">Sesto decile</skos:prefLabel>
      <skos:definition xml:lang="it">Il sesto dei nove valori che suddividono la frequenza totale di una distribuzione in dieci parti uguali.</skos:definition>
      <skos:prefLabel xml:lang="nl">Zesde deciel</skos:prefLabel>
      <skos:definition xml:lang="nl"/>
      <skos:prefLabel xml:lang="no">Sjette desil</skos:prefLabel>
      <skos:definition xml:lang="no">Den sjette av ni verdier som separerer den totale frekvensen av en fordeling i ti like deler.</skos:definition>
      <skos:prefLabel xml:lang="pt">Sexto decil</skos:prefLabel>
      <skos:definition xml:lang="pt">O sexto dos nove valores que separam a frequência total de uma distribuição em dez partes iguais.</skos:definition>
      <skos:prefLabel xml:lang="sl">Šesti decil</skos:prefLabel>
      <skos:definition xml:lang="sl">Šesta od devetih vrednosti, ki razdelijo celotno frekvenčno porazdelitev na deset enakih delov.</skos:definition>
      <skos:prefLabel xml:lang="sr">Šesti decil</skos:prefLabel>
      <skos:definition xml:lang="sr">Šesta od devet vrednosti koja razdvaja ukupnu frekvenciju distribucije na deset jednakih delova.</skos:definition>
      <skos:prefLabel xml:lang="sv">Sjätte decilen</skos:prefLabel>
      <skos:definition xml:lang="sv">Det sjätte av nio värden som separerar den totala frekvensen av en fördelning i tio lika delar.</skos:definition>
   </rdf:Description>
   <rdf:Description rdf:about="http://rdf-vocabulary.ddialliance.org/cv/SummaryStatisticType/2.1/d40e2525">
      <rdf:type rdf:resource="http://www.w3.org/2004/02/skos/core#Concept"/>
      <skos:inScheme rdf:resource="http://rdf-vocabulary.ddialliance.org/cv/SummaryStatisticType/2.1"/>
      <skos:notation>SeventhDecile</skos:notation>
      <skos:prefLabel xml:lang="en">Seventh decile</skos:prefLabel>
      <skos:definition xml:lang="en">The seventh of nine values which separate the total frequency of a distribution into ten equal parts.</skos:definition>
      <skos:prefLabel xml:lang="da">Syvende decil</skos:prefLabel>
      <skos:definition xml:lang="da">Den syvende af ni værdier, der adskiller den samlede frekvensfordeling i ti lige dele.</skos:definition>
      <skos:prefLabel xml:lang="fi">Seitsemäs desiili</skos:prefLabel>
      <skos:definition xml:lang="fi">Seitsemäs yhdeksästä arvosta, jotka jakavat jakauman kymmeneen yhtä suureen osaan.</skos:definition>
      <skos:prefLabel xml:lang="it">Settimo decile</skos:prefLabel>
      <skos:definition xml:lang="it">Il settimo dei nove valori che suddividono la frequenza totale di una distribuzione in dieci parti uguali.</skos:definition>
      <skos:prefLabel xml:lang="nl">Zevende deciel</skos:prefLabel>
      <skos:definition xml:lang="nl"/>
      <skos:prefLabel xml:lang="no">Syvende desil</skos:prefLabel>
      <skos:definition xml:lang="no">Den syvende av ni verdier som separerer den totale frekvensen av en fordeling i ti like deler.</skos:definition>
      <skos:prefLabel xml:lang="pt">Sétimo decil</skos:prefLabel>
      <skos:definition xml:lang="pt">O sétimo dos nove valores que separam a frequência total de uma distribuição em dez partes iguais.</skos:definition>
      <skos:prefLabel xml:lang="sl">Sedmi decil</skos:prefLabel>
      <skos:definition xml:lang="sl">Sedma od devetih vrednosti, ki razdelijo celotno frekvenčno porazdelitev na deset enakih delov.</skos:definition>
      <skos:prefLabel xml:lang="sr">Sedmi decil</skos:prefLabel>
      <skos:definition xml:lang="sr">Sedma od devet vrednosti koja razdvaja ukupnu frekvenciju distribucije na deset jednakih delova.</skos:definition>
      <skos:prefLabel xml:lang="sv">Sjunde decilen</skos:prefLabel>
      <skos:definition xml:lang="sv">Det sjunde av nio värden som separerar den totala frekvensen av en fördelning i tio lika delar.</skos:definition>
   </rdf:Description>
   <rdf:Description rdf:about="http://rdf-vocabulary.ddialliance.org/cv/SummaryStatisticType/2.1/d40e2597">
      <rdf:type rdf:resource="http://www.w3.org/2004/02/skos/core#Concept"/>
      <skos:inScheme rdf:resource="http://rdf-vocabulary.ddialliance.org/cv/SummaryStatisticType/2.1"/>
      <skos:notation>EighthDecile</skos:notation>
      <skos:prefLabel xml:lang="en">Eighth decile</skos:prefLabel>
      <skos:definition xml:lang="en">The eighth of nine values which separate the total frequency of a distribution into ten equal parts.</skos:definition>
      <skos:prefLabel xml:lang="da">Ottende decil</skos:prefLabel>
      <skos:definition xml:lang="da">Den ottende af ni værdier, der adskiller den samlede frekvensfordeling i ti lige dele.</skos:definition>
      <skos:prefLabel xml:lang="fi">Kahdeksas desiili</skos:prefLabel>
      <skos:definition xml:lang="fi">Kahdeksas yhdeksästä arvosta, jotka jakavat jakauman kymmeneen yhtä suureen osaan.</skos:definition>
      <skos:prefLabel xml:lang="it">Ottavo decile</skos:prefLabel>
      <skos:definition xml:lang="it">L'ottavo dei nove valori che suddividono la frequenza totale di una distribuzione in dieci parti uguali.</skos:definition>
      <skos:prefLabel xml:lang="nl">Achste deciel</skos:prefLabel>
      <skos:definition xml:lang="nl"/>
      <skos:prefLabel xml:lang="no">Åttende desil</skos:prefLabel>
      <skos:definition xml:lang="no">Den åttende av ni verdier som separerer den totale frekvensen av en fordeling i ti like deler.</skos:definition>
      <skos:prefLabel xml:lang="pt">Oitavo decil</skos:prefLabel>
      <skos:definition xml:lang="pt">O oitavo dos nove valores que separam a frequência total de uma distribuição em dez partes iguais.</skos:definition>
      <skos:prefLabel xml:lang="sl">Osmi decil</skos:prefLabel>
      <skos:definition xml:lang="sl">Osma od devetih vrednosti, ki razdelijo celotno frekvenčno porazdelitev na deset enakih delov.</skos:definition>
      <skos:prefLabel xml:lang="sr">Osmi decil</skos:prefLabel>
      <skos:definition xml:lang="sr">Osma od devet vrednosti koja razdvaja ukupnu frekvenciju distribucije na deset jednakih delova.</skos:definition>
      <skos:prefLabel xml:lang="sv">Åttonde decilen</skos:prefLabel>
      <skos:definition xml:lang="sv">Det åttonde av nio värden som separerar den totala frekvensen av en fördelning i tio lika delar.</skos:definition>
   </rdf:Description>
   <rdf:Description rdf:about="http://rdf-vocabulary.ddialliance.org/cv/SummaryStatisticType/2.1/d40e2668">
      <rdf:type rdf:resource="http://www.w3.org/2004/02/skos/core#Concept"/>
      <skos:inScheme rdf:resource="http://rdf-vocabulary.ddialliance.org/cv/SummaryStatisticType/2.1"/>
      <skos:notation>NinthDecile</skos:notation>
      <skos:prefLabel xml:lang="en">Ninth decile</skos:prefLabel>
      <skos:definition xml:lang="en">The ninth of nine values which separate the total frequency of a distribution into ten equal parts.</skos:definition>
      <skos:prefLabel xml:lang="da">Niende decil</skos:prefLabel>
      <skos:definition xml:lang="da">Den niende af ni værdier, der adskiller den samlede frekvensfordeling i ti lige dele.</skos:definition>
      <skos:prefLabel xml:lang="fi">Yhdeksäs desiili</skos:prefLabel>
      <skos:definition xml:lang="fi">Yhdeksäs yhdeksästä arvosta, jotka jakavat jakauman kymmeneen yhtä suureen osaan.</skos:definition>
      <skos:prefLabel xml:lang="it">Nono decile</skos:prefLabel>
      <skos:definition xml:lang="it">Il nono dei nove valori che suddividono la frequenza totale di una distribuzione in dieci parti uguali.</skos:definition>
      <skos:prefLabel xml:lang="nl">Negende deciel</skos:prefLabel>
      <skos:definition xml:lang="nl"/>
      <skos:prefLabel xml:lang="no">Niende desil</skos:prefLabel>
      <skos:definition xml:lang="no">Den niende av ni verdier som separerer den totale frekvensen av en fordeling i ti like deler.</skos:definition>
      <skos:prefLabel xml:lang="pt">Nono decil</skos:prefLabel>
      <skos:definition xml:lang="pt">O nono dos nove valores que separam a frequência total de uma distribuição em dez partes iguais.</skos:definition>
      <skos:prefLabel xml:lang="sl">Deveti decil</skos:prefLabel>
      <skos:definition xml:lang="sl">Deveta od devetih vrednosti, ki razdelijo celotno frekvenčno porazdelitev na deset enakih delov.</skos:definition>
      <skos:prefLabel xml:lang="sr">Deveti decil</skos:prefLabel>
      <skos:definition xml:lang="sr">Deveta od devet vrednosti koja razdvaja ukupnu frekvenciju distribucije na deset jednakih delova.</skos:definition>
      <skos:prefLabel xml:lang="sv">Nionde decilen</skos:prefLabel>
      <skos:definition xml:lang="sv">Det nionde av nio värden som separerar den totala frekvensen av en fördelning i tio lika delar.</skos:definition>
   </rdf:Description>
   <rdf:Description rdf:about="http://rdf-vocabulary.ddialliance.org/cv/SummaryStatisticType/2.1/d40e2739">
      <rdf:type rdf:resource="http://www.w3.org/2004/02/skos/core#Concept"/>
      <skos:inScheme rdf:resource="http://rdf-vocabulary.ddialliance.org/cv/SummaryStatisticType/2.1"/>
      <skos:notation>InterdecileRange</skos:notation>
      <skos:prefLabel xml:lang="en">Interdecile range</skos:prefLabel>
      <skos:definition xml:lang="en">The range between the first and ninth decile values.</skos:definition>
      <skos:prefLabel xml:lang="da">Afstanden mellem 1. og 9. decil</skos:prefLabel>
      <skos:definition xml:lang="da">Afstanden mellem 1. og 9. decilers værdier.</skos:definition>
      <skos:prefLabel xml:lang="fi">Desiiliväli</skos:prefLabel>
      <skos:definition xml:lang="fi">Väli ensimmäisestä desiilistä yhdeksänteen desiiliin.</skos:definition>
      <skos:prefLabel xml:lang="it">Ampiezza interdecile</skos:prefLabel>
      <skos:definition xml:lang="it">L'intervallo tra il primo e il nono decile.</skos:definition>
      <skos:prefLabel xml:lang="nl">Interdicielafstand</skos:prefLabel>
      <skos:definition xml:lang="nl"/>
      <skos:prefLabel xml:lang="no">Desilbredde</skos:prefLabel>
      <skos:definition xml:lang="no">Intervallet mellom første og niende desilverdi.</skos:definition>
      <skos:prefLabel xml:lang="pt">Amplitude interdecil</skos:prefLabel>
      <skos:definition xml:lang="pt">O intervalo entre os valores do primeiro e do nono decil.</skos:definition>
      <skos:prefLabel xml:lang="sl">Decilni razmik</skos:prefLabel>
      <skos:definition xml:lang="sl">Razpon med vrednostima prvega in devetega decila.</skos:definition>
      <skos:prefLabel xml:lang="sr">Međudecilni raspon</skos:prefLabel>
      <skos:definition xml:lang="sr">Raspon između prvog i devetog decila.</skos:definition>
      <skos:prefLabel xml:lang="sv">Decilavstånd</skos:prefLabel>
      <skos:definition xml:lang="sv">Intervallet mellan första och nionde decilen.</skos:definition>
   </rdf:Description>
   <rdf:Description rdf:about="http://rdf-vocabulary.ddialliance.org/cv/SummaryStatisticType/2.1/d40e2810">
      <rdf:type rdf:resource="http://www.w3.org/2004/02/skos/core#Concept"/>
      <skos:inScheme rdf:resource="http://rdf-vocabulary.ddialliance.org/cv/SummaryStatisticType/2.1"/>
      <skos:notation>OtherPercentile</skos:notation>
      <skos:prefLabel xml:lang="en">Other percentile</skos:prefLabel>
      <skos:definition xml:lang="en">A percentile not covered by any of the other percentile terms.</skos:definition>
      <skos:prefLabel xml:lang="da">Andre typer af percentiler</skos:prefLabel>
      <skos:definition xml:lang="da">Et percentil, der ikke er dækket af nogen af de andre percentilbetingelser.</skos:definition>
      <skos:prefLabel xml:lang="fi">Muu persentiili</skos:prefLabel>
      <skos:definition xml:lang="fi">Persentiili, joka ei sovi muihin fraktiilitermeihin.</skos:definition>
      <skos:prefLabel xml:lang="it">Altri percentili</skos:prefLabel>
      <skos:definition xml:lang="it">Un percentile non coperto da nessuno degli altri percentili indicati.</skos:definition>
      <skos:prefLabel xml:lang="nl">Ander percentiel</skos:prefLabel>
      <skos:definition xml:lang="nl"/>
      <skos:prefLabel xml:lang="no">Annen persentil</skos:prefLabel>
      <skos:definition xml:lang="no">En persentil som ikke inngår i noen av de andre persentilbegrepene.</skos:definition>
      <skos:prefLabel xml:lang="pt">Outro percentil</skos:prefLabel>
      <skos:definition xml:lang="pt">Um percentil não abrangido por nenhum outro termo relacionado com os percentis.</skos:definition>
      <skos:prefLabel xml:lang="sl">Drugi percentili</skos:prefLabel>
      <skos:definition xml:lang="sl">Percentil, ki ni zajet v katerem drugem percentilnem izrazu.</skos:definition>
      <skos:prefLabel xml:lang="sr">Ostali percentili</skos:prefLabel>
      <skos:definition xml:lang="sr">Perceptil koji nije obuhvaćen nijednim procentnim izrazom.</skos:definition>
      <skos:prefLabel xml:lang="sv">Annan percentil</skos:prefLabel>
      <skos:definition xml:lang="sv">En percentil som inte omfattas av någon av de andra percentiltermerna.</skos:definition>
   </rdf:Description>
   <rdf:Description rdf:about="http://rdf-vocabulary.ddialliance.org/cv/SummaryStatisticType/2.1/d40e2881">
      <rdf:type rdf:resource="http://www.w3.org/2004/02/skos/core#Concept"/>
      <skos:inScheme rdf:resource="http://rdf-vocabulary.ddialliance.org/cv/SummaryStatisticType/2.1"/>
      <skos:notation>Beta1</skos:notation>
      <skos:prefLabel xml:lang="en">Skewness</skos:prefLabel>
      <skos:definition xml:lang="en">A measure for the asymmetry of a probability distribution of a variable.</skos:definition>
      <skos:prefLabel xml:lang="da">Skævhed</skos:prefLabel>
      <skos:definition xml:lang="da">Et mål for asymmetri af en variabels sandsynlighedsfordeling.</skos:definition>
      <skos:prefLabel xml:lang="fi">Vinous</skos:prefLabel>
      <skos:definition xml:lang="fi">Muuttujan todennäköisyysjakauman epäsymmetrisyyttä kuvaava käsite.</skos:definition>
      <skos:prefLabel xml:lang="it">Indice di asimmetria</skos:prefLabel>
      <skos:definition xml:lang="it">Una misura dell'asimmetria di una distribuzione di probabilità di una variabile.</skos:definition>
      <skos:prefLabel xml:lang="nl">Scheefheid</skos:prefLabel>
      <skos:definition xml:lang="nl"/>
      <skos:prefLabel xml:lang="no">Skjevhet</skos:prefLabel>
      <skos:definition xml:lang="no">Et mål for asymmetri av en sannsynlighetsfordeling til en variabel.</skos:definition>
      <skos:prefLabel xml:lang="pt">Obliquidade (ou assimetria)</skos:prefLabel>
      <skos:definition xml:lang="pt">Medida de assimetria da distribuição das frequências de uma variável.</skos:definition>
      <skos:prefLabel xml:lang="sl">Asimetrija</skos:prefLabel>
      <skos:definition xml:lang="sl">Mera asimetrije verjetnostne porazdelitve spremenljivke.</skos:definition>
      <skos:prefLabel xml:lang="sr">Simetrija / zakrivljenost</skos:prefLabel>
      <skos:definition xml:lang="sr">„Skewness“ je mera simetrije ili preciznije, nedostatak simetrije. Distribucija skupa podataka je simetrična ako izgleda isto levo i desno u odnosu na centralnu vrednost.&amp;nbsp;</skos:definition>
      <skos:prefLabel xml:lang="sv">Skevhet</skos:prefLabel>
      <skos:definition xml:lang="sv">Ett mått för asymmetrin av en variabels sannolikhetsfördelning.</skos:definition>
   </rdf:Description>
   <rdf:Description rdf:about="http://rdf-vocabulary.ddialliance.org/cv/SummaryStatisticType/2.1/d40e2952">
      <rdf:type rdf:resource="http://www.w3.org/2004/02/skos/core#Concept"/>
      <skos:inScheme rdf:resource="http://rdf-vocabulary.ddialliance.org/cv/SummaryStatisticType/2.1"/>
      <skos:notation>Beta2</skos:notation>
      <skos:prefLabel xml:lang="en">Kurtosis</skos:prefLabel>
      <skos:definition xml:lang="en">A measure for the "peakedness" of a probability distribution of a variable.</skos:definition>
      <skos:prefLabel xml:lang="da">Kurtosis</skos:prefLabel>
      <skos:definition xml:lang="da">Et mål for “spidsheden” af en variabels sandsynlighedsfordeling.</skos:definition>
      <skos:prefLabel xml:lang="fi">Huipukkuus</skos:prefLabel>
      <skos:definition xml:lang="fi">Muuttujan todennäköisyysjakauman huipukkuutta kuvaava käsite.</skos:definition>
      <skos:prefLabel xml:lang="it">Curtosi</skos:prefLabel>
      <skos:definition xml:lang="it">Una misura del "picco" di una distribuzione di probabilità di una variabile.</skos:definition>
      <skos:prefLabel xml:lang="nl">Kurtosis</skos:prefLabel>
      <skos:definition xml:lang="nl"/>
      <skos:prefLabel xml:lang="no">Kurtose</skos:prefLabel>
      <skos:definition xml:lang="no">Et mål for 'spissheten' av en sannsynlighetsfordeling til en variabel.</skos:definition>
      <skos:prefLabel xml:lang="pt">Curtose (ou achatamento)</skos:prefLabel>
      <skos:definition xml:lang="pt">Medida para o "pico" da distribuição das frequências de uma variável.</skos:definition>
      <skos:prefLabel xml:lang="sl">Sploščenost</skos:prefLabel>
      <skos:definition xml:lang="sl">Mera 'koničanosti' verjetnostne porazdelitve spremenljivke.</skos:definition>
      <skos:prefLabel xml:lang="sr">Spljoštenost / zašiljenost</skos:prefLabel>
      <skos:definition xml:lang="sr">"Kurtosis" meri da li su podaci oštrije ili spljoštenije raspoređeni u odnosu na normalnu raspodelu.</skos:definition>
      <skos:prefLabel xml:lang="sv">Kurtosis</skos:prefLabel>
      <skos:definition xml:lang="sv">Ett mått för "spetsigheten" på en variabels sannolikhetsfördelning.</skos:definition>
   </rdf:Description>
   <rdf:Description rdf:about="http://rdf-vocabulary.ddialliance.org/cv/SummaryStatisticType/2.1/d40e3024">
      <rdf:type rdf:resource="http://www.w3.org/2004/02/skos/core#Concept"/>
      <skos:inScheme rdf:resource="http://rdf-vocabulary.ddialliance.org/cv/SummaryStatisticType/2.1"/>
      <skos:notation>ShapiroWilk</skos:notation>
      <skos:prefLabel xml:lang="en">Shapiro-Wilk</skos:prefLabel>
      <skos:definition xml:lang="en">Normality test statistics.</skos:definition>
      <skos:prefLabel xml:lang="da">Shapiro-Wilk- test</skos:prefLabel>
      <skos:definition xml:lang="da">Statistisk normalitetstest.</skos:definition>
      <skos:prefLabel xml:lang="fi">Shapiron–Wilkin testi</skos:prefLabel>
      <skos:definition xml:lang="fi">Eräs jakauman normaaliuden testeistä.</skos:definition>
      <skos:prefLabel xml:lang="it">Test di Shapiro-Wilk</skos:prefLabel>
      <skos:definition xml:lang="it">Test di normalità statistica.</skos:definition>
      <skos:prefLabel xml:lang="nl">Shapiro-Wilk</skos:prefLabel>
      <skos:definition xml:lang="nl"/>
      <skos:prefLabel xml:lang="no">Shapiro-Wilk</skos:prefLabel>
      <skos:definition xml:lang="no">Statistisk normalitetstest.</skos:definition>
      <skos:prefLabel xml:lang="pt">Shapiro-Wilk</skos:prefLabel>
      <skos:definition xml:lang="pt">Teste de normalidade estatística.</skos:definition>
      <skos:prefLabel xml:lang="sl">Shapiro-Wilkov test normalnosti porazdelitve</skos:prefLabel>
      <skos:definition xml:lang="sl">Test normalnosti porazdelitve.</skos:definition>
      <skos:prefLabel xml:lang="sr">Šapiro-Vilk</skos:prefLabel>
      <skos:definition xml:lang="sr">Šapiro-Vilk je test normalnosti koji se preporučuje za uzorke čiji obim nije veći od 2000 elemenata.</skos:definition>
      <skos:prefLabel xml:lang="sv">Shapiro-Wilk</skos:prefLabel>
      <skos:definition xml:lang="sv">Test som visar i vilken mån datamaterialet inte är normalfördelat.</skos:definition>
   </rdf:Description>
   <rdf:Description rdf:about="http://rdf-vocabulary.ddialliance.org/cv/SummaryStatisticType/2.1/d40e3095">
      <rdf:type rdf:resource="http://www.w3.org/2004/02/skos/core#Concept"/>
      <skos:inScheme rdf:resource="http://rdf-vocabulary.ddialliance.org/cv/SummaryStatisticType/2.1"/>
      <skos:notation>PercentageOfValidCases</skos:notation>
      <skos:prefLabel xml:lang="en">Percentage of valid cases</skos:prefLabel>
      <skos:definition xml:lang="en">Indicates the percentage of valid cases of the total number of cases.</skos:definition>
      <skos:prefLabel xml:lang="da">Andelen af valide cases</skos:prefLabel>
      <skos:definition xml:lang="da">Indikerer procentdelen af gyldige cases i det samlede antal af cases.</skos:definition>
      <skos:prefLabel xml:lang="fi">Validien havaintoyksiköiden prosentuaalinen osuus</skos:prefLabel>
      <skos:definition xml:lang="fi">Ilmaisee validien havaintoyksiköiden prosenttiosuuden kaikista havaintoyksiköistä.</skos:definition>
      <skos:prefLabel xml:lang="it">Percentuale di casi validi</skos:prefLabel>
      <skos:definition xml:lang="it">Indica la percentuale di casi validi sul numero totale dei casi.</skos:definition>
      <skos:prefLabel xml:lang="nl">Percentage geldige gevallen</skos:prefLabel>
      <skos:definition xml:lang="nl"/>
      <skos:prefLabel xml:lang="no">Prosentdel gyldige tilfeller</skos:prefLabel>
      <skos:definition xml:lang="no">Indikerer prosentdelen av gyldige tilfeller til det totale antallet tilfeller.</skos:definition>
      <skos:prefLabel xml:lang="pt">Percentagem de casos válidos</skos:prefLabel>
      <skos:definition xml:lang="pt">Indica a percentagem de casos válidos do número total de casos.</skos:definition>
      <skos:prefLabel xml:lang="sl">Delež veljavnih enot</skos:prefLabel>
      <skos:definition xml:lang="sl">Označuje odstotek veljavnih primerov glede na skupno število primerov.</skos:definition>
      <skos:prefLabel xml:lang="sr">Procenat ispravnih slučajeva</skos:prefLabel>
      <skos:definition xml:lang="sr">Pokazuje procenat ispravnih (validnih) opservacija u odnosu na ukupan broj opservacija.</skos:definition>
      <skos:prefLabel xml:lang="sv">Andelen giltiga fall</skos:prefLabel>
      <skos:definition xml:lang="sv">Indikerar andelen giltiga fall i förhållande till det totala antalet fall.</skos:definition>
   </rdf:Description>
   <rdf:Description rdf:about="http://rdf-vocabulary.ddialliance.org/cv/SummaryStatisticType/2.1/d40e3166">
      <rdf:type rdf:resource="http://www.w3.org/2004/02/skos/core#Concept"/>
      <skos:inScheme rdf:resource="http://rdf-vocabulary.ddialliance.org/cv/SummaryStatisticType/2.1"/>
      <skos:notation>PercentageOfInvalidCases</skos:notation>
      <skos:prefLabel xml:lang="en">Percentage of invalid cases</skos:prefLabel>
      <skos:definition xml:lang="en">Indicates the percentage of invalid cases of the total number of cases.</skos:definition>
      <skos:prefLabel xml:lang="da">Andelen af ugyldige cases</skos:prefLabel>
      <skos:definition xml:lang="da">Indikerer procentdelen af ugyldige cases i det samlede antal af cases.</skos:definition>
      <skos:prefLabel xml:lang="fi">Puuttuvien havaintoyksiköiden prosentuaalinen osuus</skos:prefLabel>
      <skos:definition xml:lang="fi">Ilmaisee puuttuvien havaintoyksiköiden prosenttiosuuden kaikista havaintoyksiköistä.</skos:definition>
      <skos:prefLabel xml:lang="it">Percentuale di casi non validi</skos:prefLabel>
      <skos:definition xml:lang="it">Indica la percentuale di casi non validi sul numero totale dei casi.</skos:definition>
      <skos:prefLabel xml:lang="nl">Percentage ongeldige gevallen</skos:prefLabel>
      <skos:definition xml:lang="nl"/>
      <skos:prefLabel xml:lang="no">Prosentdel ugyldige tilfeller</skos:prefLabel>
      <skos:definition xml:lang="no">Indikerer prosentdelen av ugyldige tilfeller til det totale antallet tilfeller.</skos:definition>
      <skos:prefLabel xml:lang="pt">Percentagem de casos inválidos</skos:prefLabel>
      <skos:definition xml:lang="pt">Indica a percentagem de casos inválidos do número total de casos.</skos:definition>
      <skos:prefLabel xml:lang="sl">Delež neveljavnih enot</skos:prefLabel>
      <skos:definition xml:lang="sl">Označuje odstotek neveljavnih primerov glede na skupno število primerov.</skos:definition>
      <skos:prefLabel xml:lang="sr">Procenat neispravnih slučajeva</skos:prefLabel>
      <skos:definition xml:lang="sr">Pokazuje procenat neispravnih opservacija u odnosu na ukupan broj opservacija.</skos:definition>
      <skos:prefLabel xml:lang="sv">Andelen ogiltiga fall</skos:prefLabel>
      <skos:definition xml:lang="sv">Indikerar andelen ogiltiga fall i förhållande till det totala antalet fall.</skos:definition>
   </rdf:Description>
   <rdf:Description rdf:about="http://rdf-vocabulary.ddialliance.org/cv/SummaryStatisticType/2.1/d40e3237">
      <rdf:type rdf:resource="http://www.w3.org/2004/02/skos/core#Concept"/>
      <skos:inScheme rdf:resource="http://rdf-vocabulary.ddialliance.org/cv/SummaryStatisticType/2.1"/>
      <skos:notation>Other</skos:notation>
      <skos:prefLabel xml:lang="en">Other</skos:prefLabel>
      <skos:definition xml:lang="en">Use if the summary statistic type is known, but not found in the list.</skos:definition>
      <skos:prefLabel xml:lang="da">Andet</skos:prefLabel>
      <skos:definition xml:lang="da">Anvend, hvis den summariske statistiktype er kendt, men ikke findes på listen.</skos:definition>
      <skos:prefLabel xml:lang="fi">Muu tunnusluku</skos:prefLabel>
      <skos:definition xml:lang="fi">Käytä, mikäli tilastollisen tunnusluvun tyyppi on tiedossa, mutta ei listassa.</skos:definition>
      <skos:prefLabel xml:lang="it">Altro</skos:prefLabel>
      <skos:definition xml:lang="it">Utilizzare se il tipo di statistica riassuntiva è conosciuto, ma non è presente nell'elenco.</skos:definition>
      <skos:prefLabel xml:lang="nl">Anders</skos:prefLabel>
      <skos:definition xml:lang="nl"/>
      <skos:prefLabel xml:lang="no">Annet</skos:prefLabel>
      <skos:definition xml:lang="no">Bruk dersom typen summeringsstatistikk er kjent, men mangler i listen.</skos:definition>
      <skos:prefLabel xml:lang="pt">Outro</skos:prefLabel>
      <skos:definition xml:lang="pt">Usar se o tipo de estatística sumária for conhecido, mas não se encontrar na lista.</skos:definition>
      <skos:prefLabel xml:lang="sl">Drugo</skos:prefLabel>
      <skos:definition xml:lang="sl">Uporabite, če je zbirna statistika znana, a je ne najdete na seznamu.</skos:definition>
      <skos:prefLabel xml:lang="sr">Ostalo</skos:prefLabel>
      <skos:definition xml:lang="sr">Koristite ukoliko je statistički tip poznat, ali se ne nalazi na listi.</skos:definition>
      <skos:prefLabel xml:lang="sv">Övrigt</skos:prefLabel>
      <skos:definition xml:lang="sv">Använd om typ av sammanfattande statistik är känd men saknas i listan.</skos:definition>
   </rdf:Description>
</rdf:RDF>
